<?xml version="1.0" encoding="UTF-8"?>
<rdf:RDF
	xmlns:rdf="http://www.w3.org/1999/02/22-rdf-syntax-ns#"
	xmlns:owl="http://www.w3.org/2002/07/owl#"
	xmlns:xsd="http://www.w3.org/2001/XMLSchema#"
	xmlns:fn="http://www.w3.org/2005/xpath-functions#"
	xmlns:dcterms="http://purl.org/dc/terms/"
	xmlns:rdfs="http://www.w3.org/2000/01/rdf-schema#"
	xmlns:sesame="http://www.openrdf.org/schema/sesame#"
	xmlns:foaf="http://xmlns.com/foaf/0.1/"
	xmlns:cycAnnot="http://sw.cyc.com/CycAnnotations_v1#"
	xmlns:csw="http://semantic-web.at/ontologies/csw.owl#"
	xmlns:freebase="http://rdf.freebase.com/ns/"
	xmlns:skos="http://www.w3.org/2004/02/skos/core#"
	xmlns:dbpedia="http://dbpedia.org/resource/"
	xmlns:cyc="http://sw.cyc.com/concept/"
	xmlns:tags="http://www.holygoat.co.uk/owl/redwood/0.1/tags/"
	xmlns:opencyc="http://sw.opencyc.org/concept/"
	xmlns:ctag="http://commontag.org/ns#"
	xmlns:dc="http://purl.org/dc/elements/1.1/">

<rdf:Description rdf:about="http://www.w3.org/1999/02/22-rdf-syntax-ns#type">
	<rdf:type rdf:resource="http://www.w3.org/1999/02/22-rdf-syntax-ns#Property"/>
	<rdf:type rdf:resource="http://www.w3.org/2000/01/rdf-schema#Resource"/>
	<rdfs:domain rdf:resource="http://www.w3.org/2000/01/rdf-schema#Resource"/>
	<rdfs:range rdf:resource="http://www.w3.org/2000/01/rdf-schema#Class"/>
	<rdfs:subPropertyOf rdf:resource="http://www.w3.org/1999/02/22-rdf-syntax-ns#type"/>
</rdf:Description>

<rdf:Description rdf:about="http://www.w3.org/1999/02/22-rdf-syntax-ns#Property">
	<rdf:type rdf:resource="http://www.w3.org/2000/01/rdf-schema#Resource"/>
	<rdf:type rdf:resource="http://www.w3.org/2000/01/rdf-schema#Class"/>
	<rdfs:subClassOf rdf:resource="http://www.w3.org/1999/02/22-rdf-syntax-ns#Property"/>
	<rdfs:subClassOf rdf:resource="http://www.w3.org/2000/01/rdf-schema#Resource"/>
</rdf:Description>

<rdf:Description rdf:about="http://www.w3.org/1999/02/22-rdf-syntax-ns#subject">
	<rdf:type rdf:resource="http://www.w3.org/1999/02/22-rdf-syntax-ns#Property"/>
	<rdf:type rdf:resource="http://www.w3.org/2000/01/rdf-schema#Resource"/>
	<rdfs:domain rdf:resource="http://www.w3.org/1999/02/22-rdf-syntax-ns#Statement"/>
	<rdfs:range rdf:resource="http://www.w3.org/2000/01/rdf-schema#Resource"/>
	<rdfs:subPropertyOf rdf:resource="http://www.w3.org/1999/02/22-rdf-syntax-ns#subject"/>
</rdf:Description>

<rdf:Description rdf:about="http://www.w3.org/1999/02/22-rdf-syntax-ns#predicate">
	<rdf:type rdf:resource="http://www.w3.org/1999/02/22-rdf-syntax-ns#Property"/>
	<rdf:type rdf:resource="http://www.w3.org/2000/01/rdf-schema#Resource"/>
	<rdfs:domain rdf:resource="http://www.w3.org/1999/02/22-rdf-syntax-ns#Statement"/>
	<rdfs:range rdf:resource="http://www.w3.org/2000/01/rdf-schema#Resource"/>
	<rdfs:subPropertyOf rdf:resource="http://www.w3.org/1999/02/22-rdf-syntax-ns#predicate"/>
</rdf:Description>

<rdf:Description rdf:about="http://www.w3.org/1999/02/22-rdf-syntax-ns#object">
	<rdf:type rdf:resource="http://www.w3.org/1999/02/22-rdf-syntax-ns#Property"/>
	<rdf:type rdf:resource="http://www.w3.org/2000/01/rdf-schema#Resource"/>
	<rdfs:domain rdf:resource="http://www.w3.org/1999/02/22-rdf-syntax-ns#Statement"/>
	<rdfs:range rdf:resource="http://www.w3.org/2000/01/rdf-schema#Resource"/>
	<rdfs:subPropertyOf rdf:resource="http://www.w3.org/1999/02/22-rdf-syntax-ns#object"/>
</rdf:Description>

<rdf:Description rdf:about="http://www.w3.org/1999/02/22-rdf-syntax-ns#first">
	<rdf:type rdf:resource="http://www.w3.org/1999/02/22-rdf-syntax-ns#Property"/>
	<rdf:type rdf:resource="http://www.w3.org/2000/01/rdf-schema#Resource"/>
	<rdfs:domain rdf:resource="http://www.w3.org/1999/02/22-rdf-syntax-ns#List"/>
	<rdfs:range rdf:resource="http://www.w3.org/2000/01/rdf-schema#Resource"/>
	<rdfs:subPropertyOf rdf:resource="http://www.w3.org/1999/02/22-rdf-syntax-ns#first"/>
</rdf:Description>

<rdf:Description rdf:about="http://www.w3.org/1999/02/22-rdf-syntax-ns#rest">
	<rdf:type rdf:resource="http://www.w3.org/1999/02/22-rdf-syntax-ns#Property"/>
	<rdf:type rdf:resource="http://www.w3.org/2000/01/rdf-schema#Resource"/>
	<rdfs:domain rdf:resource="http://www.w3.org/1999/02/22-rdf-syntax-ns#List"/>
	<rdfs:range rdf:resource="http://www.w3.org/1999/02/22-rdf-syntax-ns#List"/>
	<rdfs:subPropertyOf rdf:resource="http://www.w3.org/1999/02/22-rdf-syntax-ns#rest"/>
</rdf:Description>

<rdf:Description rdf:about="http://www.w3.org/1999/02/22-rdf-syntax-ns#value">
	<rdf:type rdf:resource="http://www.w3.org/1999/02/22-rdf-syntax-ns#Property"/>
	<rdf:type rdf:resource="http://www.w3.org/2000/01/rdf-schema#Resource"/>
	<rdfs:domain rdf:resource="http://www.w3.org/2000/01/rdf-schema#Resource"/>
	<rdfs:range rdf:resource="http://www.w3.org/2000/01/rdf-schema#Resource"/>
	<rdfs:subPropertyOf rdf:resource="http://www.w3.org/1999/02/22-rdf-syntax-ns#value"/>
</rdf:Description>

<rdf:Description rdf:about="http://www.w3.org/1999/02/22-rdf-syntax-ns#nil">
	<rdf:type rdf:resource="http://www.w3.org/1999/02/22-rdf-syntax-ns#List"/>
	<rdf:type rdf:resource="http://www.w3.org/2000/01/rdf-schema#Resource"/>
</rdf:Description>

<rdf:Description rdf:about="http://www.w3.org/1999/02/22-rdf-syntax-ns#List">
	<rdf:type rdf:resource="http://www.w3.org/2000/01/rdf-schema#Resource"/>
	<rdf:type rdf:resource="http://www.w3.org/2000/01/rdf-schema#Class"/>
	<rdfs:subClassOf rdf:resource="http://www.w3.org/1999/02/22-rdf-syntax-ns#List"/>
	<rdfs:subClassOf rdf:resource="http://www.w3.org/2000/01/rdf-schema#Resource"/>
</rdf:Description>

<rdf:Description rdf:about="http://www.w3.org/2000/01/rdf-schema#domain">
	<rdf:type rdf:resource="http://www.w3.org/1999/02/22-rdf-syntax-ns#Property"/>
	<rdf:type rdf:resource="http://www.w3.org/2000/01/rdf-schema#Resource"/>
	<rdfs:domain rdf:resource="http://www.w3.org/1999/02/22-rdf-syntax-ns#Property"/>
	<rdfs:range rdf:resource="http://www.w3.org/2000/01/rdf-schema#Class"/>
	<rdfs:subPropertyOf rdf:resource="http://www.w3.org/2000/01/rdf-schema#domain"/>
</rdf:Description>

<rdf:Description rdf:about="http://www.w3.org/2000/01/rdf-schema#Resource">
	<rdf:type rdf:resource="http://www.w3.org/2000/01/rdf-schema#Resource"/>
	<rdf:type rdf:resource="http://www.w3.org/2000/01/rdf-schema#Class"/>
	<rdfs:subClassOf rdf:resource="http://www.w3.org/2000/01/rdf-schema#Resource"/>
</rdf:Description>

<rdf:Description rdf:about="http://www.w3.org/2000/01/rdf-schema#range">
	<rdf:type rdf:resource="http://www.w3.org/1999/02/22-rdf-syntax-ns#Property"/>
	<rdf:type rdf:resource="http://www.w3.org/2000/01/rdf-schema#Resource"/>
	<rdfs:domain rdf:resource="http://www.w3.org/1999/02/22-rdf-syntax-ns#Property"/>
	<rdfs:range rdf:resource="http://www.w3.org/2000/01/rdf-schema#Class"/>
	<rdfs:subPropertyOf rdf:resource="http://www.w3.org/2000/01/rdf-schema#range"/>
</rdf:Description>

<rdf:Description rdf:about="http://www.w3.org/2000/01/rdf-schema#subPropertyOf">
	<rdf:type rdf:resource="http://www.w3.org/1999/02/22-rdf-syntax-ns#Property"/>
	<rdf:type rdf:resource="http://www.w3.org/2000/01/rdf-schema#Resource"/>
	<rdfs:domain rdf:resource="http://www.w3.org/1999/02/22-rdf-syntax-ns#Property"/>
	<rdfs:range rdf:resource="http://www.w3.org/1999/02/22-rdf-syntax-ns#Property"/>
	<rdfs:subPropertyOf rdf:resource="http://www.w3.org/2000/01/rdf-schema#subPropertyOf"/>
</rdf:Description>

<rdf:Description rdf:about="http://www.w3.org/2000/01/rdf-schema#subClassOf">
	<rdf:type rdf:resource="http://www.w3.org/1999/02/22-rdf-syntax-ns#Property"/>
	<rdf:type rdf:resource="http://www.w3.org/2000/01/rdf-schema#Resource"/>
	<rdfs:domain rdf:resource="http://www.w3.org/2000/01/rdf-schema#Class"/>
	<rdfs:range rdf:resource="http://www.w3.org/2000/01/rdf-schema#Class"/>
	<rdfs:subPropertyOf rdf:resource="http://www.w3.org/2000/01/rdf-schema#subClassOf"/>
</rdf:Description>

<rdf:Description rdf:about="http://www.w3.org/2000/01/rdf-schema#Class">
	<rdf:type rdf:resource="http://www.w3.org/2000/01/rdf-schema#Resource"/>
	<rdf:type rdf:resource="http://www.w3.org/2000/01/rdf-schema#Class"/>
	<rdfs:subClassOf rdf:resource="http://www.w3.org/2000/01/rdf-schema#Resource"/>
	<rdfs:subClassOf rdf:resource="http://www.w3.org/2000/01/rdf-schema#Class"/>
</rdf:Description>

<rdf:Description rdf:about="http://www.w3.org/1999/02/22-rdf-syntax-ns#Statement">
	<rdf:type rdf:resource="http://www.w3.org/2000/01/rdf-schema#Resource"/>
	<rdf:type rdf:resource="http://www.w3.org/2000/01/rdf-schema#Class"/>
	<rdfs:subClassOf rdf:resource="http://www.w3.org/2000/01/rdf-schema#Resource"/>
	<rdfs:subClassOf rdf:resource="http://www.w3.org/1999/02/22-rdf-syntax-ns#Statement"/>
</rdf:Description>

<rdf:Description rdf:about="http://www.w3.org/2000/01/rdf-schema#member">
	<rdf:type rdf:resource="http://www.w3.org/1999/02/22-rdf-syntax-ns#Property"/>
	<rdf:type rdf:resource="http://www.w3.org/2000/01/rdf-schema#Resource"/>
	<rdfs:domain rdf:resource="http://www.w3.org/2000/01/rdf-schema#Resource"/>
	<rdfs:range rdf:resource="http://www.w3.org/2000/01/rdf-schema#Resource"/>
	<rdfs:subPropertyOf rdf:resource="http://www.w3.org/2000/01/rdf-schema#member"/>
</rdf:Description>

<rdf:Description rdf:about="http://www.w3.org/2000/01/rdf-schema#seeAlso">
	<rdf:type rdf:resource="http://www.w3.org/1999/02/22-rdf-syntax-ns#Property"/>
	<rdf:type rdf:resource="http://www.w3.org/2000/01/rdf-schema#Resource"/>
	<rdfs:domain rdf:resource="http://www.w3.org/2000/01/rdf-schema#Resource"/>
	<rdfs:range rdf:resource="http://www.w3.org/2000/01/rdf-schema#Resource"/>
	<rdfs:subPropertyOf rdf:resource="http://www.w3.org/2000/01/rdf-schema#seeAlso"/>
</rdf:Description>

<rdf:Description rdf:about="http://www.w3.org/2000/01/rdf-schema#isDefinedBy">
	<rdf:type rdf:resource="http://www.w3.org/1999/02/22-rdf-syntax-ns#Property"/>
	<rdf:type rdf:resource="http://www.w3.org/2000/01/rdf-schema#Resource"/>
	<rdfs:domain rdf:resource="http://www.w3.org/2000/01/rdf-schema#Resource"/>
	<rdfs:range rdf:resource="http://www.w3.org/2000/01/rdf-schema#Resource"/>
	<rdfs:subPropertyOf rdf:resource="http://www.w3.org/2000/01/rdf-schema#seeAlso"/>
	<rdfs:subPropertyOf rdf:resource="http://www.w3.org/2000/01/rdf-schema#isDefinedBy"/>
</rdf:Description>

<rdf:Description rdf:about="http://www.w3.org/2000/01/rdf-schema#comment">
	<rdf:type rdf:resource="http://www.w3.org/1999/02/22-rdf-syntax-ns#Property"/>
	<rdf:type rdf:resource="http://www.w3.org/2000/01/rdf-schema#Resource"/>
	<rdfs:domain rdf:resource="http://www.w3.org/2000/01/rdf-schema#Resource"/>
	<rdfs:range rdf:resource="http://www.w3.org/2000/01/rdf-schema#Literal"/>
	<rdfs:subPropertyOf rdf:resource="http://www.w3.org/2000/01/rdf-schema#comment"/>
</rdf:Description>

<rdf:Description rdf:about="http://www.w3.org/2000/01/rdf-schema#label">
	<rdf:type rdf:resource="http://www.w3.org/1999/02/22-rdf-syntax-ns#Property"/>
	<rdf:type rdf:resource="http://www.w3.org/2000/01/rdf-schema#Resource"/>
	<rdfs:domain rdf:resource="http://www.w3.org/2000/01/rdf-schema#Resource"/>
	<rdfs:range rdf:resource="http://www.w3.org/2000/01/rdf-schema#Literal"/>
	<rdfs:subPropertyOf rdf:resource="http://www.w3.org/2000/01/rdf-schema#label"/>
</rdf:Description>

<rdf:Description rdf:about="http://www.w3.org/2000/01/rdf-schema#Literal">
	<rdf:type rdf:resource="http://www.w3.org/2000/01/rdf-schema#Resource"/>
	<rdf:type rdf:resource="http://www.w3.org/2000/01/rdf-schema#Class"/>
	<rdfs:subClassOf rdf:resource="http://www.w3.org/2000/01/rdf-schema#Resource"/>
	<rdfs:subClassOf rdf:resource="http://www.w3.org/2000/01/rdf-schema#Literal"/>
</rdf:Description>

<rdf:Description rdf:about="http://www.w3.org/1999/02/22-rdf-syntax-ns#Alt">
	<rdf:type rdf:resource="http://www.w3.org/2000/01/rdf-schema#Resource"/>
	<rdf:type rdf:resource="http://www.w3.org/2000/01/rdf-schema#Class"/>
	<rdfs:subClassOf rdf:resource="http://www.w3.org/2000/01/rdf-schema#Resource"/>
	<rdfs:subClassOf rdf:resource="http://www.w3.org/1999/02/22-rdf-syntax-ns#Alt"/>
	<rdfs:subClassOf rdf:resource="http://www.w3.org/2000/01/rdf-schema#Container"/>
</rdf:Description>

<rdf:Description rdf:about="http://www.w3.org/2000/01/rdf-schema#Container">
	<rdf:type rdf:resource="http://www.w3.org/2000/01/rdf-schema#Resource"/>
	<rdf:type rdf:resource="http://www.w3.org/2000/01/rdf-schema#Class"/>
	<rdfs:subClassOf rdf:resource="http://www.w3.org/2000/01/rdf-schema#Resource"/>
	<rdfs:subClassOf rdf:resource="http://www.w3.org/2000/01/rdf-schema#Container"/>
</rdf:Description>

<rdf:Description rdf:about="http://www.w3.org/1999/02/22-rdf-syntax-ns#Bag">
	<rdf:type rdf:resource="http://www.w3.org/2000/01/rdf-schema#Resource"/>
	<rdf:type rdf:resource="http://www.w3.org/2000/01/rdf-schema#Class"/>
	<rdfs:subClassOf rdf:resource="http://www.w3.org/2000/01/rdf-schema#Resource"/>
	<rdfs:subClassOf rdf:resource="http://www.w3.org/2000/01/rdf-schema#Container"/>
	<rdfs:subClassOf rdf:resource="http://www.w3.org/1999/02/22-rdf-syntax-ns#Bag"/>
</rdf:Description>

<rdf:Description rdf:about="http://www.w3.org/1999/02/22-rdf-syntax-ns#Seq">
	<rdf:type rdf:resource="http://www.w3.org/2000/01/rdf-schema#Resource"/>
	<rdf:type rdf:resource="http://www.w3.org/2000/01/rdf-schema#Class"/>
	<rdfs:subClassOf rdf:resource="http://www.w3.org/2000/01/rdf-schema#Resource"/>
	<rdfs:subClassOf rdf:resource="http://www.w3.org/2000/01/rdf-schema#Container"/>
	<rdfs:subClassOf rdf:resource="http://www.w3.org/1999/02/22-rdf-syntax-ns#Seq"/>
</rdf:Description>

<rdf:Description rdf:about="http://www.w3.org/2000/01/rdf-schema#ContainerMembershipProperty">
	<rdf:type rdf:resource="http://www.w3.org/2000/01/rdf-schema#Resource"/>
	<rdf:type rdf:resource="http://www.w3.org/2000/01/rdf-schema#Class"/>
	<rdfs:subClassOf rdf:resource="http://www.w3.org/1999/02/22-rdf-syntax-ns#Property"/>
	<rdfs:subClassOf rdf:resource="http://www.w3.org/2000/01/rdf-schema#Resource"/>
	<rdfs:subClassOf rdf:resource="http://www.w3.org/2000/01/rdf-schema#ContainerMembershipProperty"/>
</rdf:Description>

<rdf:Description rdf:about="http://www.w3.org/1999/02/22-rdf-syntax-ns#XMLLiteral">
	<rdf:type rdf:resource="http://www.w3.org/2000/01/rdf-schema#Resource"/>
	<rdf:type rdf:resource="http://www.w3.org/2000/01/rdf-schema#Class"/>
	<rdf:type rdf:resource="http://www.w3.org/2000/01/rdf-schema#Datatype"/>
	<rdfs:subClassOf rdf:resource="http://www.w3.org/2000/01/rdf-schema#Resource"/>
	<rdfs:subClassOf rdf:resource="http://www.w3.org/2000/01/rdf-schema#Literal"/>
	<rdfs:subClassOf rdf:resource="http://www.w3.org/1999/02/22-rdf-syntax-ns#XMLLiteral"/>
</rdf:Description>

<rdf:Description rdf:about="http://www.w3.org/2000/01/rdf-schema#Datatype">
	<rdf:type rdf:resource="http://www.w3.org/2000/01/rdf-schema#Resource"/>
	<rdf:type rdf:resource="http://www.w3.org/2000/01/rdf-schema#Class"/>
	<rdfs:subClassOf rdf:resource="http://www.w3.org/2000/01/rdf-schema#Resource"/>
	<rdfs:subClassOf rdf:resource="http://www.w3.org/2000/01/rdf-schema#Class"/>
	<rdfs:subClassOf rdf:resource="http://www.w3.org/2000/01/rdf-schema#Datatype"/>
</rdf:Description>

<rdf:Description rdf:about="http://editor.vocabs.ands.org.au/user/Claire-Butler">
	<rdf:type rdf:resource="http://www.w3.org/2000/01/rdf-schema#Resource"/>
	<rdf:type rdf:resource="http://purl.org/dc/terms/Agent"/>
	<foaf:name rdf:datatype="http://www.w3.org/2001/XMLSchema#string">Claire-Butler</foaf:name>
</rdf:Description>

<rdf:Description rdf:about="http://purl.org/dc/terms/Agent">
	<rdf:type rdf:resource="http://www.w3.org/2000/01/rdf-schema#Resource"/>
	<rdf:type rdf:resource="http://www.w3.org/2000/01/rdf-schema#Class"/>
	<rdfs:subClassOf rdf:resource="http://www.w3.org/2000/01/rdf-schema#Resource"/>
	<rdfs:subClassOf rdf:resource="http://purl.org/dc/terms/Agent"/>
</rdf:Description>

<rdf:Description rdf:about="http://xmlns.com/foaf/0.1/name">
	<rdf:type rdf:resource="http://www.w3.org/1999/02/22-rdf-syntax-ns#Property"/>
	<rdf:type rdf:resource="http://www.w3.org/2000/01/rdf-schema#Resource"/>
	<rdfs:subPropertyOf rdf:resource="http://xmlns.com/foaf/0.1/name"/>
</rdf:Description>

<rdf:Description rdf:about="http://editor.vocabs.ands.org.au/user/Institute-for-Marine-and-Antarctic-Studies-University-of-Tasmania">
	<rdf:type rdf:resource="http://www.w3.org/2000/01/rdf-schema#Resource"/>
	<rdf:type rdf:resource="http://purl.org/dc/terms/Agent"/>
	<foaf:name rdf:datatype="http://www.w3.org/2001/XMLSchema#string">Institute-for-Marine-and-Antarctic-Studies-University-of-Tasmania</foaf:name>
</rdf:Description>

<rdf:Description rdf:about="http://editor.vocabs.ands.org.au/user/Kim-Finney">
	<rdf:type rdf:resource="http://www.w3.org/2000/01/rdf-schema#Resource"/>
	<rdf:type rdf:resource="http://purl.org/dc/terms/Agent"/>
	<foaf:name rdf:datatype="http://www.w3.org/2001/XMLSchema#string">Kim-Finney</foaf:name>
</rdf:Description>

<rdf:Description rdf:about="http://editor.vocabs.ands.org.au/user/eMII_Finney.Kim_Admin">
	<rdf:type rdf:resource="http://www.w3.org/2000/01/rdf-schema#Resource"/>
	<rdf:type rdf:resource="http://purl.org/dc/terms/Agent"/>
	<foaf:name rdf:datatype="http://www.w3.org/2001/XMLSchema#string">eMII_Finney.Kim_Admin</foaf:name>
</rdf:Description>

<rdf:Description rdf:about="http://seamapaustralia.org.au/def/benthichabitatclassification/class/2">
	<rdf:type rdf:resource="http://www.w3.org/2000/01/rdf-schema#Resource"/>
	<rdfs:label xml:lang="en">Unknown Substrate (Not Mapped)</rdfs:label>
	<owl:deprecated rdf:datatype="http://www.w3.org/2001/XMLSchema#boolean">true</owl:deprecated>
</rdf:Description>

<rdf:Description rdf:about="http://www.w3.org/2002/07/owl#deprecated">
	<rdf:type rdf:resource="http://www.w3.org/1999/02/22-rdf-syntax-ns#Property"/>
	<rdf:type rdf:resource="http://www.w3.org/2000/01/rdf-schema#Resource"/>
	<rdfs:subPropertyOf rdf:resource="http://www.w3.org/2002/07/owl#deprecated"/>
</rdf:Description>

<rdf:Description rdf:about="http://seamapaustralia.org.au/def/benthichabitatclassification/class/100">
	<rdf:type rdf:resource="http://www.w3.org/2000/01/rdf-schema#Resource"/>
	<rdfs:label xml:lang="en">MEOW Province</rdfs:label>
	<owl:deprecated rdf:datatype="http://www.w3.org/2001/XMLSchema#boolean">true</owl:deprecated>
</rdf:Description>

<rdf:Description rdf:about="http://seamapaustralia.org.au/def/benthichabitatclassification/class/102">
	<rdf:type rdf:resource="http://www.w3.org/2000/01/rdf-schema#Resource"/>
	<rdfs:label xml:lang="en">MEOW Province</rdfs:label>
	<owl:deprecated rdf:datatype="http://www.w3.org/2001/XMLSchema#boolean">true</owl:deprecated>
</rdf:Description>

<rdf:Description rdf:about="http://seamapaustralia.org.au/def/benthichabitatclassification/class/99">
	<rdf:type rdf:resource="http://www.w3.org/2000/01/rdf-schema#Resource"/>
	<rdfs:label xml:lang="en">MEOW Arctic Realm</rdfs:label>
	<owl:deprecated rdf:datatype="http://www.w3.org/2001/XMLSchema#boolean">true</owl:deprecated>
</rdf:Description>

<rdf:Description rdf:about="http://seamapaustralia.org.au/def/benthichabitatclassification/class/101">
	<rdf:type rdf:resource="http://www.w3.org/2000/01/rdf-schema#Resource"/>
	<rdfs:label xml:lang="en">MEOW Temperate Northern Atlantic Realm</rdfs:label>
	<owl:deprecated rdf:datatype="http://www.w3.org/2001/XMLSchema#boolean">true</owl:deprecated>
</rdf:Description>

<rdf:Description rdf:about="http://seamapaustralia.org.au/def/benthichabitatclassification/class/103">
	<rdf:type rdf:resource="http://www.w3.org/2000/01/rdf-schema#Resource"/>
	<rdfs:label xml:lang="en">MEOW Temperate Northern Pacific Realm</rdfs:label>
	<owl:deprecated rdf:datatype="http://www.w3.org/2001/XMLSchema#boolean">true</owl:deprecated>
</rdf:Description>

<rdf:Description rdf:about="http://seamapaustralia.org.au/def/benthichabitatclassification/class/109">
	<rdf:type rdf:resource="http://www.w3.org/2000/01/rdf-schema#Resource"/>
	<rdfs:label xml:lang="en">MEOW Temperate South America Realm</rdfs:label>
	<owl:deprecated rdf:datatype="http://www.w3.org/2001/XMLSchema#boolean">true</owl:deprecated>
</rdf:Description>

<rdf:Description rdf:about="http://seamapaustralia.org.au/def/benthichabitatclassification/class/110">
	<rdf:type rdf:resource="http://www.w3.org/2000/01/rdf-schema#Resource"/>
	<rdfs:label xml:lang="en">MEOW Temperate Southern Africa Realm</rdfs:label>
	<owl:deprecated rdf:datatype="http://www.w3.org/2001/XMLSchema#boolean">true</owl:deprecated>
</rdf:Description>

<rdf:Description rdf:about="http://seamapaustralia.org.au/def/benthichabitatclassification/class/104">
	<rdf:type rdf:resource="http://www.w3.org/2000/01/rdf-schema#Resource"/>
	<rdfs:label xml:lang="en">MEOW Tropical Atlantic Realm</rdfs:label>
	<owl:deprecated rdf:datatype="http://www.w3.org/2001/XMLSchema#boolean">true</owl:deprecated>
</rdf:Description>

<rdf:Description rdf:about="http://seamapaustralia.org.au/def/benthichabitatclassification/class/133">
	<rdf:type rdf:resource="http://www.w3.org/2000/01/rdf-schema#Resource"/>
	<rdfs:label xml:lang="en">Offshore Subtidal</rdfs:label>
	<owl:deprecated rdf:datatype="http://www.w3.org/2001/XMLSchema#boolean">true</owl:deprecated>
</rdf:Description>

<rdf:Description rdf:about="http://seamapaustralia.org.au/def/benthichabitatclassification/class/52">
	<rdf:type rdf:resource="http://www.w3.org/2000/01/rdf-schema#Resource"/>
	<rdfs:label xml:lang="en">Unknown Worm</rdfs:label>
	<owl:deprecated rdf:datatype="http://www.w3.org/2001/XMLSchema#boolean">true</owl:deprecated>
</rdf:Description>

<rdf:Description rdf:about="http://seamapaustralia.org.au/def/benthichabitatclassification/class/77">
	<rdf:type rdf:resource="http://www.w3.org/2000/01/rdf-schema#Resource"/>
	<rdfs:label xml:lang="en">Coral</rdfs:label>
	<owl:deprecated rdf:datatype="http://www.w3.org/2001/XMLSchema#boolean">true</owl:deprecated>
</rdf:Description>

<rdf:Description rdf:about="http://seamapaustralia.org.au/def/benthichabitatclassification/class/87">
	<rdf:type rdf:resource="http://www.w3.org/2000/01/rdf-schema#Resource"/>
	<rdfs:label xml:lang="en">Hard Coral</rdfs:label>
	<owl:deprecated rdf:datatype="http://www.w3.org/2001/XMLSchema#boolean">true</owl:deprecated>
</rdf:Description>

<rdf:Description rdf:about="http://seamapaustralia.org.au/def/benthichabitatclassification/class/88">
	<rdf:type rdf:resource="http://www.w3.org/2000/01/rdf-schema#Resource"/>
	<rdfs:label xml:lang="en">Soft Coral</rdfs:label>
	<owl:deprecated rdf:datatype="http://www.w3.org/2001/XMLSchema#boolean">true</owl:deprecated>
</rdf:Description>

<rdf:Description rdf:about="http://seamapaustralia.org.au/def/benthichabitatclassification/class/89">
	<rdf:type rdf:resource="http://www.w3.org/2000/01/rdf-schema#Resource"/>
	<rdfs:label xml:lang="en">Mixed Corals</rdfs:label>
	<owl:deprecated rdf:datatype="http://www.w3.org/2001/XMLSchema#boolean">true</owl:deprecated>
</rdf:Description>

<rdf:Description rdf:about="http://seamapaustralia.org.au/def/benthichabitatclassification/class/81">
	<rdf:type rdf:resource="http://www.w3.org/2000/01/rdf-schema#Resource"/>
	<rdfs:label xml:lang="en">Mixed Invertebrate Community</rdfs:label>
	<owl:deprecated rdf:datatype="http://www.w3.org/2001/XMLSchema#boolean">true</owl:deprecated>
</rdf:Description>

<rdf:Description rdf:about="http://seamapaustralia.org.au/def/benthichabitatclassification/class/129">
	<rdf:type rdf:resource="http://www.w3.org/2000/01/rdf-schema#Resource"/>
	<rdfs:label xml:lang="en">Nearshore Intertidal</rdfs:label>
	<owl:deprecated rdf:datatype="http://www.w3.org/2001/XMLSchema#boolean">true</owl:deprecated>
</rdf:Description>

<rdf:Description rdf:about="http://seamapaustralia.org.au/def/benthichabitatclassification/class/107">
	<rdf:type rdf:resource="http://www.w3.org/2000/01/rdf-schema#Resource"/>
	<rdfs:label xml:lang="en">MEOW Eastern Indo-Pacific Realm</rdfs:label>
	<owl:deprecated rdf:datatype="http://www.w3.org/2001/XMLSchema#boolean">true</owl:deprecated>
</rdf:Description>

<rdf:Description rdf:about="http://seamapaustralia.org.au/def/benthichabitatclassification/class/216">
	<rdf:type rdf:resource="http://www.w3.org/2000/01/rdf-schema#Resource"/>
	<rdfs:label xml:lang="en">MEOW Amundsen-Bellinghausen Sea Ecoregion</rdfs:label>
	<owl:deprecated rdf:datatype="http://www.w3.org/2001/XMLSchema#boolean">true</owl:deprecated>
</rdf:Description>

<rdf:Description rdf:about="http://seamapaustralia.org.au/def/benthichabitatclassification/class/113">
	<rdf:type rdf:resource="http://www.w3.org/2000/01/rdf-schema#Resource"/>
	<rdfs:label xml:lang="en">MEOW Northern New Zealand Province</rdfs:label>
	<owl:deprecated rdf:datatype="http://www.w3.org/2001/XMLSchema#boolean">true</owl:deprecated>
</rdf:Description>

<rdf:Description rdf:about="http://seamapaustralia.org.au/def/benthichabitatclassification/class/114">
	<rdf:type rdf:resource="http://www.w3.org/2000/01/rdf-schema#Resource"/>
	<rdfs:label xml:lang="en">MEOW Southern New Zealand Province</rdfs:label>
	<owl:deprecated rdf:datatype="http://www.w3.org/2001/XMLSchema#boolean">true</owl:deprecated>
</rdf:Description>

<rdf:Description rdf:about="http://seamapaustralia.org.au/def/benthichabitatclassification/class/108">
	<rdf:type rdf:resource="http://www.w3.org/2000/01/rdf-schema#Resource"/>
	<rdfs:label xml:lang="en">MEOW Tropical Eastern Pacific Realm</rdfs:label>
	<owl:deprecated rdf:datatype="http://www.w3.org/2001/XMLSchema#boolean">true</owl:deprecated>
</rdf:Description>

<rdf:Description rdf:about="http://seamapaustralia.org.au/def/benthichabitatclassification/class/105">
	<rdf:type rdf:resource="http://www.w3.org/2000/01/rdf-schema#Resource"/>
	<rdfs:label xml:lang="en">MEOW Western Indo-Pacific Realm</rdfs:label>
	<owl:deprecated rdf:datatype="http://www.w3.org/2001/XMLSchema#boolean">true</owl:deprecated>
</rdf:Description>

<rdf:Description rdf:about="http://seamapaustralia.org.au/def/benthichabitatclassification/class/165">
	<rdf:type rdf:resource="http://www.w3.org/2000/01/rdf-schema#Resource"/>
	<rdfs:label xml:lang="en">MEOW South China Sea Province</rdfs:label>
	<owl:deprecated rdf:datatype="http://www.w3.org/2001/XMLSchema#boolean">true</owl:deprecated>
</rdf:Description>

<rdf:Description rdf:about="http://seamapaustralia.org.au/def/benthichabitatclassification/class/166">
	<rdf:type rdf:resource="http://www.w3.org/2000/01/rdf-schema#Resource"/>
	<rdfs:label xml:lang="en">MEOW Gulf of Tonkin Ecoregion</rdfs:label>
	<owl:deprecated rdf:datatype="http://www.w3.org/2001/XMLSchema#boolean">true</owl:deprecated>
</rdf:Description>

<rdf:Description rdf:about="http://seamapaustralia.org.au/def/benthichabitatclassification/class/167">
	<rdf:type rdf:resource="http://www.w3.org/2000/01/rdf-schema#Resource"/>
	<rdfs:label xml:lang="en">MEOW Southern China Ecoregion</rdfs:label>
	<owl:deprecated rdf:datatype="http://www.w3.org/2001/XMLSchema#boolean">true</owl:deprecated>
</rdf:Description>

<rdf:Description rdf:about="http://seamapaustralia.org.au/def/benthichabitatclassification/class/168">
	<rdf:type rdf:resource="http://www.w3.org/2000/01/rdf-schema#Resource"/>
	<rdfs:label xml:lang="en">MEOW South China Sea Oceanic Islands Ecoregion</rdfs:label>
	<owl:deprecated rdf:datatype="http://www.w3.org/2001/XMLSchema#boolean">true</owl:deprecated>
</rdf:Description>

<rdf:Description rdf:about="http://seamapaustralia.org.au/def/benthichabitatclassification/class/169">
	<rdf:type rdf:resource="http://www.w3.org/2000/01/rdf-schema#Resource"/>
	<rdfs:label xml:lang="en">MEOW Sunda Shelf Province</rdfs:label>
	<owl:deprecated rdf:datatype="http://www.w3.org/2001/XMLSchema#boolean">true</owl:deprecated>
</rdf:Description>

<rdf:Description rdf:about="http://seamapaustralia.org.au/def/benthichabitatclassification/class/193">
	<rdf:type rdf:resource="http://www.w3.org/2000/01/rdf-schema#Resource"/>
	<rdfs:label xml:lang="en">MEOW Gulf of Thailand Ecoregion</rdfs:label>
	<owl:deprecated rdf:datatype="http://www.w3.org/2001/XMLSchema#boolean">true</owl:deprecated>
</rdf:Description>

<rdf:Description rdf:about="http://seamapaustralia.org.au/def/benthichabitatclassification/class/194">
	<rdf:type rdf:resource="http://www.w3.org/2000/01/rdf-schema#Resource"/>
	<rdfs:label xml:lang="en">MEOW Southern Vietnam Ecoregion</rdfs:label>
	<owl:deprecated rdf:datatype="http://www.w3.org/2001/XMLSchema#boolean">true</owl:deprecated>
</rdf:Description>

<rdf:Description rdf:about="http://seamapaustralia.org.au/def/benthichabitatclassification/class/195">
	<rdf:type rdf:resource="http://www.w3.org/2000/01/rdf-schema#Resource"/>
	<rdfs:label xml:lang="en">MEOW Sunda Shelf-Java Sea Ecoregion</rdfs:label>
	<owl:deprecated rdf:datatype="http://www.w3.org/2001/XMLSchema#boolean">true</owl:deprecated>
</rdf:Description>

<rdf:Description rdf:about="http://seamapaustralia.org.au/def/benthichabitatclassification/class/196">
	<rdf:type rdf:resource="http://www.w3.org/2000/01/rdf-schema#Resource"/>
	<rdfs:label xml:lang="en">MEOW Malacca Strait Ecoregion</rdfs:label>
	<owl:deprecated rdf:datatype="http://www.w3.org/2001/XMLSchema#boolean">true</owl:deprecated>
</rdf:Description>

<rdf:Description rdf:about="http://seamapaustralia.org.au/def/benthichabitatclassification/class/198">
	<rdf:type rdf:resource="http://www.w3.org/2000/01/rdf-schema#Resource"/>
	<rdfs:label xml:lang="en">MEOW Fiji Islands Ecoregion</rdfs:label>
	<owl:deprecated rdf:datatype="http://www.w3.org/2001/XMLSchema#boolean">true</owl:deprecated>
</rdf:Description>

<rdf:Description rdf:about="http://seamapaustralia.org.au/def/benthichabitatclassification/class/197">
	<rdf:type rdf:resource="http://www.w3.org/2000/01/rdf-schema#Resource"/>
	<rdfs:label xml:lang="en">MEOW Tonga Islands Ecoregion</rdfs:label>
	<owl:deprecated rdf:datatype="http://www.w3.org/2001/XMLSchema#boolean">true</owl:deprecated>
</rdf:Description>

<rdf:Description rdf:about="http://seamapaustralia.org.au/def/benthichabitatclassification/class/199">
	<rdf:type rdf:resource="http://www.w3.org/2000/01/rdf-schema#Resource"/>
	<rdfs:label xml:lang="en">MEOW Vanuatu Ecoregion</rdfs:label>
	<owl:deprecated rdf:datatype="http://www.w3.org/2001/XMLSchema#boolean">true</owl:deprecated>
</rdf:Description>

<rdf:Description rdf:about="http://seamapaustralia.org.au/def/benthichabitatclassification/class/209">
	<rdf:type rdf:resource="http://www.w3.org/2000/01/rdf-schema#Resource"/>
	<rdfs:label xml:lang="en">MEOW Northeast Sulawesi Ecoregion</rdfs:label>
	<owl:deprecated rdf:datatype="http://www.w3.org/2001/XMLSchema#boolean">true</owl:deprecated>
</rdf:Description>

<rdf:Description rdf:about="http://seamapaustralia.org.au/def/benthichabitatclassification/class/202">
	<rdf:type rdf:resource="http://www.w3.org/2000/01/rdf-schema#Resource"/>
	<rdfs:label xml:lang="en">MEOW Palawan-North Borneo Ecoregion</rdfs:label>
	<owl:deprecated rdf:datatype="http://www.w3.org/2001/XMLSchema#boolean">true</owl:deprecated>
</rdf:Description>

<rdf:Description rdf:about="http://seamapaustralia.org.au/def/benthichabitatclassification/class/204">
	<rdf:type rdf:resource="http://www.w3.org/2000/01/rdf-schema#Resource"/>
	<rdfs:label xml:lang="en">MEOW Sulawesi Sea-Makassar Strait Ecoregion</rdfs:label>
	<owl:deprecated rdf:datatype="http://www.w3.org/2001/XMLSchema#boolean">true</owl:deprecated>
</rdf:Description>

<rdf:Description rdf:about="http://seamapaustralia.org.au/def/benthichabitatclassification/class/225">
	<rdf:type rdf:resource="http://www.w3.org/2000/01/rdf-schema#Resource"/>
	<rdfs:label xml:lang="en">MEOW Peter the First Island Ecoregion</rdfs:label>
	<owl:deprecated rdf:datatype="http://www.w3.org/2001/XMLSchema#boolean">true</owl:deprecated>
</rdf:Description>

<rdf:Description rdf:about="http://seamapaustralia.org.au/def/benthichabitatclassification/class/86">
	<rdf:type rdf:resource="http://www.w3.org/2000/01/rdf-schema#Resource"/>
	<rdfs:label xml:lang="en">Mixed Submerged Vegetation</rdfs:label>
	<owl:deprecated rdf:datatype="http://www.w3.org/2001/XMLSchema#boolean">true</owl:deprecated>
</rdf:Description>

<rdf:Description rdf:about="http://seamapaustralia.org.au/def/benthichabitatclassification/class/51">
	<rdf:type rdf:resource="http://www.w3.org/2000/01/rdf-schema#Resource"/>
	<rdfs:label xml:lang="en">Trash Origin</rdfs:label>
	<owl:deprecated rdf:datatype="http://www.w3.org/2001/XMLSchema#boolean">true</owl:deprecated>
</rdf:Description>

<rdf:Description rdf:about="http://seamapaustralia.org.au/def/benthichabitatclassification/class/247">
	<rdf:type rdf:resource="http://www.w3.org/2000/01/rdf-schema#Resource"/>
	<rdfs:label xml:lang="en">IMCRA 4 Provincial Bioregions</rdfs:label>
	<owl:deprecated rdf:datatype="http://www.w3.org/2001/XMLSchema#boolean">true</owl:deprecated>
</rdf:Description>

<rdf:Description rdf:about="http://seamapaustralia.org.au/def/benthichabitatclassification/class/248">
	<rdf:type rdf:resource="http://www.w3.org/2000/01/rdf-schema#Resource"/>
	<rdfs:label xml:lang="en">IMCRA 4 Provincial Bioregions</rdfs:label>
	<owl:deprecated rdf:datatype="http://www.w3.org/2001/XMLSchema#boolean">true</owl:deprecated>
</rdf:Description>

<rdf:Description rdf:about="http://seamapaustralia.org.au/def/benthichabitatclassification/class/249">
	<rdf:type rdf:resource="http://www.w3.org/2000/01/rdf-schema#Resource"/>
	<rdfs:label xml:lang="en">IMCRA 4 Mesoscale Regions</rdfs:label>
	<owl:deprecated rdf:datatype="http://www.w3.org/2001/XMLSchema#boolean">true</owl:deprecated>
</rdf:Description>

<rdf:Description rdf:about="http://seamapaustralia.org.au/def/benthichabitatclassification/class/260">
	<rdf:type rdf:resource="http://www.w3.org/2000/01/rdf-schema#Resource"/>
	<rdfs:label xml:lang="en">IMCRA Cape Howe Province</rdfs:label>
	<owl:deprecated rdf:datatype="http://www.w3.org/2001/XMLSchema#boolean">true</owl:deprecated>
</rdf:Description>

<rdf:Description rdf:about="http://seamapaustralia.org.au/def/benthichabitatclassification/class/317">
	<rdf:type rdf:resource="http://www.w3.org/2000/01/rdf-schema#Resource"/>
	<rdfs:label xml:lang="en">IMCRA Exmouth to Broome Bioregion</rdfs:label>
	<owl:deprecated rdf:datatype="http://www.w3.org/2001/XMLSchema#boolean">true</owl:deprecated>
</rdf:Description>

<rdf:Description rdf:about="http://seamapaustralia.org.au/def/benthichabitatclassification/class/160">
	<rdf:type rdf:resource="http://www.w3.org/2000/01/rdf-schema#Resource"/>
	<rdfs:label xml:lang="en">Urchin Barren</rdfs:label>
	<owl:deprecated rdf:datatype="http://www.w3.org/2001/XMLSchema#boolean">true</owl:deprecated>
</rdf:Description>

<rdf:Description rdf:about="http://seamapaustralia.org.au/def/benthichabitatclassification/class/156">
	<rdf:type rdf:resource="http://www.w3.org/2000/01/rdf-schema#Resource"/>
	<rdfs:label xml:lang="en">Bare Substratum</rdfs:label>
	<owl:deprecated rdf:datatype="http://www.w3.org/2001/XMLSchema#boolean">true</owl:deprecated>
</rdf:Description>

<rdf:Description rdf:about="http://seamapaustralia.org.au/def/benthichabitatclassification/class/234">
	<rdf:type rdf:resource="http://www.w3.org/2000/01/rdf-schema#Resource"/>
	<rdfs:label xml:lang="en">Clam</rdfs:label>
	<owl:deprecated rdf:datatype="http://www.w3.org/2001/XMLSchema#boolean">true</owl:deprecated>
</rdf:Description>

<rdf:Description rdf:about="http://seamapaustralia.org.au/def/benthichabitatclassification/class/40">
	<rdf:type rdf:resource="http://www.w3.org/2000/01/rdf-schema#Resource"/>
	<rdfs:label xml:lang="en">Shell</rdfs:label>
	<owl:deprecated rdf:datatype="http://www.w3.org/2001/XMLSchema#boolean">true</owl:deprecated>
</rdf:Description>

<rdf:Description rdf:about="http://seamapaustralia.org.au/def/benthichabitatclassification/class/57">
	<rdf:type rdf:resource="http://www.w3.org/2000/01/rdf-schema#Resource"/>
	<rdfs:label xml:lang="en">Other Shells</rdfs:label>
	<owl:deprecated rdf:datatype="http://www.w3.org/2001/XMLSchema#boolean">true</owl:deprecated>
</rdf:Description>

<rdf:Description rdf:about="http://seamapaustralia.org.au/def/benthichabitatclassification/class/58">
	<rdf:type rdf:resource="http://www.w3.org/2000/01/rdf-schema#Resource"/>
	<rdfs:label xml:lang="en">Screw Shell</rdfs:label>
	<owl:deprecated rdf:datatype="http://www.w3.org/2001/XMLSchema#boolean">true</owl:deprecated>
</rdf:Description>

<rdf:Description rdf:about="http://seamapaustralia.org.au/def/benthichabitatclassification/class/59">
	<rdf:type rdf:resource="http://www.w3.org/2000/01/rdf-schema#Resource"/>
	<rdfs:label xml:lang="en">Oyster Shell</rdfs:label>
	<owl:deprecated rdf:datatype="http://www.w3.org/2001/XMLSchema#boolean">true</owl:deprecated>
</rdf:Description>

<rdf:Description rdf:about="http://seamapaustralia.org.au/def/benthichabitatclassification/class/60">
	<rdf:type rdf:resource="http://www.w3.org/2000/01/rdf-schema#Resource"/>
	<rdfs:label xml:lang="en">Mussel Shell</rdfs:label>
	<owl:deprecated rdf:datatype="http://www.w3.org/2001/XMLSchema#boolean">true</owl:deprecated>
</rdf:Description>

<rdf:Description rdf:about="http://seamapaustralia.org.au/def/benthichabitatclassification/class/61">
	<rdf:type rdf:resource="http://www.w3.org/2000/01/rdf-schema#Resource"/>
	<rdfs:label xml:lang="en">Clam Shell</rdfs:label>
	<owl:deprecated rdf:datatype="http://www.w3.org/2001/XMLSchema#boolean">true</owl:deprecated>
</rdf:Description>

<rdf:Description rdf:about="http://seamapaustralia.org.au/def/benthichabitatclassification/class/41">
	<rdf:type rdf:resource="http://www.w3.org/2000/01/rdf-schema#Resource"/>
	<rdfs:label xml:lang="en">Coral</rdfs:label>
	<owl:deprecated rdf:datatype="http://www.w3.org/2001/XMLSchema#boolean">true</owl:deprecated>
</rdf:Description>

<rdf:Description rdf:about="http://seamapaustralia.org.au/def/benthichabitatclassification/class/330">
	<rdf:type rdf:resource="http://www.w3.org/2000/01/rdf-schema#Resource"/>
	<rdfs:label xml:lang="en">Screw Shell</rdfs:label>
	<owl:deprecated rdf:datatype="http://www.w3.org/2001/XMLSchema#boolean">true</owl:deprecated>
</rdf:Description>

<rdf:Description rdf:about="http://seamapaustralia.org.au/def/benthichabitatclassification/class/153">
	<rdf:type rdf:resource="http://www.w3.org/2000/01/rdf-schema#Resource"/>
	<rdfs:label xml:lang="en">Carbonate</rdfs:label>
	<owl:deprecated rdf:datatype="http://www.w3.org/2001/XMLSchema#boolean">true</owl:deprecated>
</rdf:Description>

<rdf:Description rdf:about="http://seamapaustralia.org.au/def/benthichabitatclassification/class/96">
	<rdf:type rdf:resource="http://www.w3.org/2000/01/rdf-schema#Resource"/>
	<rdf:type rdf:resource="http://www.w3.org/2004/02/skos/core#Concept"/>
	<skos:broader rdf:resource="http://seamapaustralia.org.au/def/benthichabitatclassification/class/80"/>
	<skos:prefLabel xml:lang="en">Other Shelled Biota</skos:prefLabel>
	<dcterms:contributor rdf:resource="http://editor.vocabs.ands.org.au/user/eMII_Finney.Kim_Admin"/>
	<dcterms:created rdf:datatype="http://www.w3.org/2001/XMLSchema#dateTime">2016-11-16T01:39:12Z</dcterms:created>
	<dcterms:creator rdf:resource="http://editor.vocabs.ands.org.au/user/eMII_Finney.Kim_Admin"/>
	<dcterms:modified rdf:datatype="http://www.w3.org/2001/XMLSchema#dateTime">2017-06-27T04:16:04Z</dcterms:modified>
	<dc:publisher rdf:datatype="http://www.w3.org/2001/XMLSchema#string">Institute for Marine and Antarctic Studies (IMAS) - UTAS</dc:publisher>
	<skos:definition xml:lang="en">An areas dominated by accumulations of living shells other that oysters, mussels, clams of screwshells, that are attached or closely associated with the substratum.</skos:definition>
	<dc:source rdf:datatype="http://www.w3.org/2001/XMLSchema#string">SeaMap Australia National Benthic Habitat Classification Scheme (2017)</dc:source>
</rdf:Description>

<rdf:Description rdf:about="http://www.w3.org/2004/02/skos/core#broader">
	<rdf:type rdf:resource="http://www.w3.org/1999/02/22-rdf-syntax-ns#Property"/>
	<rdf:type rdf:resource="http://www.w3.org/2000/01/rdf-schema#Resource"/>
	<rdfs:subPropertyOf rdf:resource="http://www.w3.org/2004/02/skos/core#broader"/>
</rdf:Description>

<rdf:Description rdf:about="http://seamapaustralia.org.au/def/benthichabitatclassification/class/80">
	<rdf:type rdf:resource="http://www.w3.org/2000/01/rdf-schema#Resource"/>
	<rdf:type rdf:resource="http://www.w3.org/2004/02/skos/core#Concept"/>
	<skos:broader rdf:resource="http://seamapaustralia.org.au/def/benthichabitatclassification/class/73"/>
	<skos:prefLabel xml:lang="en">Shelled Biota</skos:prefLabel>
	<dcterms:contributor rdf:resource="http://editor.vocabs.ands.org.au/user/eMII_Finney.Kim_Admin"/>
	<dcterms:created rdf:datatype="http://www.w3.org/2001/XMLSchema#dateTime">2016-11-16T01:19:31Z</dcterms:created>
	<dcterms:creator rdf:resource="http://editor.vocabs.ands.org.au/user/eMII_Finney.Kim_Admin"/>
	<dcterms:modified rdf:datatype="http://www.w3.org/2001/XMLSchema#dateTime">2017-06-27T04:15:47Z</dcterms:modified>
	<dc:publisher rdf:datatype="http://www.w3.org/2001/XMLSchema#string">Institute for Marine and Antarctic Studies (IMAS) - UTAS</dc:publisher>
	<skos:definition xml:lang="en">Biota with a shell.</skos:definition>
	<dc:source rdf:datatype="http://www.w3.org/2001/XMLSchema#string">SeaMap Australia National Benthic Habitat Classification Scheme (2017)</dc:source>
	<skos:narrower rdf:resource="http://seamapaustralia.org.au/def/benthichabitatclassification/class/96"/>
	<skos:narrower rdf:resource="http://seamapaustralia.org.au/def/benthichabitatclassification/class/326"/>
	<skos:narrower rdf:resource="http://seamapaustralia.org.au/def/benthichabitatclassification/class/94"/>
	<skos:narrower rdf:resource="http://seamapaustralia.org.au/def/benthichabitatclassification/class/95"/>
	<skos:narrower rdf:resource="http://seamapaustralia.org.au/def/benthichabitatclassification/class/157"/>
</rdf:Description>

<rdf:Description rdf:about="http://www.w3.org/2004/02/skos/core#prefLabel">
	<rdf:type rdf:resource="http://www.w3.org/1999/02/22-rdf-syntax-ns#Property"/>
	<rdf:type rdf:resource="http://www.w3.org/2000/01/rdf-schema#Resource"/>
	<rdfs:subPropertyOf rdf:resource="http://www.w3.org/2004/02/skos/core#prefLabel"/>
</rdf:Description>

<rdf:Description rdf:about="http://seamapaustralia.org.au/def/benthichabitatclassification/1">
	<rdf:type rdf:resource="http://www.w3.org/2000/01/rdf-schema#Resource"/>
	<rdf:type rdf:resource="http://www.w3.org/2004/02/skos/core#ConceptScheme"/>
	<rdfs:label xml:lang="en">Seamap Australia National Benthic Habitat Classification Scheme</rdfs:label>
	<dcterms:contributor rdf:resource="http://editor.vocabs.ands.org.au/user/eMII_Finney.Kim_Admin"/>
	<dcterms:created rdf:datatype="http://www.w3.org/2001/XMLSchema#dateTime">2016-11-15T04:32:34Z</dcterms:created>
	<dcterms:creator rdf:resource="http://editor.vocabs.ands.org.au/user/eMII_Finney.Kim_Admin"/>
	<dcterms:description xml:lang="en">A national in scope classification scheme for Australian benthic habitats</dcterms:description>
	<dcterms:modified rdf:datatype="http://www.w3.org/2001/XMLSchema#dateTime">2017-02-14T22:31:33Z</dcterms:modified>
	<dcterms:publisher rdf:resource="http://editor.vocabs.ands.org.au/user/Institute-for-Marine-and-Antarctic-Studies-University-of-Tasmania"/>
	<dcterms:subject xml:lang="en">Benthic Habitat Classification</dcterms:subject>
	<dcterms:title xml:lang="en">Seamap Australia National Benthic Habitat Classification Scheme</dcterms:title>
	<identifier xmlns="http://schema.semantic-web.at/ppt/" rdf:datatype="http://www.w3.org/2001/XMLSchema#string">class</identifier>
	<skos:hasTopConcept rdf:resource="http://seamapaustralia.org.au/def/benthichabitatclassification/class/3"/>
	<skos:hasTopConcept rdf:resource="http://seamapaustralia.org.au/def/benthichabitatclassification/class/34"/>
	<skos:hasTopConcept rdf:resource="http://seamapaustralia.org.au/def/benthichabitatclassification/class/69"/>
	<skos:hasTopConcept rdf:resource="http://seamapaustralia.org.au/def/benthichabitatclassification/class/97"/>
	<skos:hasTopConcept rdf:resource="http://seamapaustralia.org.au/def/benthichabitatclassification/class/98"/>
	<dcterms:identifier xml:lang="en">class</dcterms:identifier>
	<dcterms:issued rdf:datatype="http://www.w3.org/2001/XMLSchema#string">2017-06-28</dcterms:issued>
	<owl:versionInfo rdf:datatype="http://www.w3.org/2001/XMLSchema#string">Beta 0.1</owl:versionInfo>
</rdf:Description>

<rdf:Description rdf:about="http://purl.org/dc/terms/contributor">
	<rdf:type rdf:resource="http://www.w3.org/1999/02/22-rdf-syntax-ns#Property"/>
	<rdf:type rdf:resource="http://www.w3.org/2000/01/rdf-schema#Resource"/>
	<rdfs:subPropertyOf rdf:resource="http://purl.org/dc/terms/contributor"/>
</rdf:Description>

<rdf:Description rdf:about="http://purl.org/dc/terms/created">
	<rdf:type rdf:resource="http://www.w3.org/1999/02/22-rdf-syntax-ns#Property"/>
	<rdf:type rdf:resource="http://www.w3.org/2000/01/rdf-schema#Resource"/>
	<rdfs:subPropertyOf rdf:resource="http://purl.org/dc/terms/created"/>
</rdf:Description>

<rdf:Description rdf:about="http://purl.org/dc/terms/creator">
	<rdf:type rdf:resource="http://www.w3.org/1999/02/22-rdf-syntax-ns#Property"/>
	<rdf:type rdf:resource="http://www.w3.org/2000/01/rdf-schema#Resource"/>
	<rdfs:subPropertyOf rdf:resource="http://purl.org/dc/terms/creator"/>
</rdf:Description>

<rdf:Description rdf:about="http://purl.org/dc/terms/description">
	<rdf:type rdf:resource="http://www.w3.org/1999/02/22-rdf-syntax-ns#Property"/>
	<rdf:type rdf:resource="http://www.w3.org/2000/01/rdf-schema#Resource"/>
	<rdfs:subPropertyOf rdf:resource="http://purl.org/dc/terms/description"/>
</rdf:Description>

<rdf:Description rdf:about="http://purl.org/dc/terms/modified">
	<rdf:type rdf:resource="http://www.w3.org/1999/02/22-rdf-syntax-ns#Property"/>
	<rdf:type rdf:resource="http://www.w3.org/2000/01/rdf-schema#Resource"/>
	<rdfs:subPropertyOf rdf:resource="http://purl.org/dc/terms/modified"/>
</rdf:Description>

<rdf:Description rdf:about="http://purl.org/dc/terms/publisher">
	<rdf:type rdf:resource="http://www.w3.org/1999/02/22-rdf-syntax-ns#Property"/>
	<rdf:type rdf:resource="http://www.w3.org/2000/01/rdf-schema#Resource"/>
	<rdfs:subPropertyOf rdf:resource="http://purl.org/dc/terms/publisher"/>
</rdf:Description>

<rdf:Description rdf:about="http://purl.org/dc/terms/subject">
	<rdf:type rdf:resource="http://www.w3.org/1999/02/22-rdf-syntax-ns#Property"/>
	<rdf:type rdf:resource="http://www.w3.org/2000/01/rdf-schema#Resource"/>
	<rdfs:subPropertyOf rdf:resource="http://purl.org/dc/terms/subject"/>
</rdf:Description>

<rdf:Description rdf:about="http://purl.org/dc/terms/title">
	<rdf:type rdf:resource="http://www.w3.org/1999/02/22-rdf-syntax-ns#Property"/>
	<rdf:type rdf:resource="http://www.w3.org/2000/01/rdf-schema#Resource"/>
	<rdfs:subPropertyOf rdf:resource="http://purl.org/dc/terms/title"/>
</rdf:Description>

<rdf:Description rdf:about="http://schema.semantic-web.at/ppt/identifier">
	<rdf:type rdf:resource="http://www.w3.org/1999/02/22-rdf-syntax-ns#Property"/>
	<rdf:type rdf:resource="http://www.w3.org/2000/01/rdf-schema#Resource"/>
	<rdfs:subPropertyOf rdf:resource="http://schema.semantic-web.at/ppt/identifier"/>
</rdf:Description>

<rdf:Description rdf:about="http://www.w3.org/2004/02/skos/core#ConceptScheme">
	<rdf:type rdf:resource="http://www.w3.org/2000/01/rdf-schema#Resource"/>
	<rdf:type rdf:resource="http://www.w3.org/2000/01/rdf-schema#Class"/>
	<rdfs:subClassOf rdf:resource="http://www.w3.org/2000/01/rdf-schema#Resource"/>
	<rdfs:subClassOf rdf:resource="http://www.w3.org/2004/02/skos/core#ConceptScheme"/>
</rdf:Description>

<rdf:Description rdf:about="http://www.w3.org/2004/02/skos/core#hasTopConcept">
	<rdf:type rdf:resource="http://www.w3.org/1999/02/22-rdf-syntax-ns#Property"/>
	<rdf:type rdf:resource="http://www.w3.org/2000/01/rdf-schema#Resource"/>
	<rdfs:subPropertyOf rdf:resource="http://www.w3.org/2004/02/skos/core#hasTopConcept"/>
</rdf:Description>

<rdf:Description rdf:about="http://seamapaustralia.org.au/def/benthichabitatclassification/class/3">
	<rdf:type rdf:resource="http://www.w3.org/2000/01/rdf-schema#Resource"/>
	<rdf:type rdf:resource="http://www.w3.org/2004/02/skos/core#Concept"/>
	<skos:prefLabel xml:lang="en">Substratum Component</skos:prefLabel>
	<dcterms:contributor rdf:resource="http://editor.vocabs.ands.org.au/user/eMII_Finney.Kim_Admin"/>
	<dcterms:created rdf:datatype="http://www.w3.org/2001/XMLSchema#dateTime">2016-11-15T04:37:50Z</dcterms:created>
	<dcterms:creator rdf:resource="http://editor.vocabs.ands.org.au/user/eMII_Finney.Kim_Admin"/>
	<dcterms:modified rdf:datatype="http://www.w3.org/2001/XMLSchema#dateTime">2017-06-27T04:18:00Z</dcterms:modified>
	<dc:publisher rdf:datatype="http://www.w3.org/2001/XMLSchema#string">Institute for Marine and Antarctic Studies (IMAS) - UTAS</dc:publisher>
	<skos:definition xml:lang="en">The Seamap classification for substrate is based on the CMECS (FGDC, 2012) Substratum component, but with the modification of introducing a level describing the hardness of the substratum, which replaces the CMECS 'Origin' classifier. This modification is the same as is described in Edmunds and Flynn (2015). The Substratum Component of the CMECS is useful because it defines unique classes based on specific grainsizes or compositions, and the lower levels can be collapsed into higher level groups as required by the resolution of mapping. However, using standard CMECS, it is not possible to collapse the lower levels into hard and soft categories, and this represented a disadvantage of the scheme. The distinction between hard and soft substrata is one of the simplest and most common distinctions made when mapping the seafloor, and can be determined in all methods used for habitat mapping, including the use of satellite imagery, aerial photography, acoustic surveys and underwater video/photography. In terms of ecology, this characteristic also represents an important division between substratum types that are able to support reef ecosystems (hard), and those that cannot (soft). For these reasons a node describing the hardness of the substratum was included as indicated earlier. This modification is the same as that proposed in Edmunds and Flynn (2015). Hardness refers to the physical properties of the substratum, and can be determined through knowledge of acoustic or optical reflectivity, as well as by the stability of the substratum. This means that habitats such as worm or shell reefs and rhodolith beds are all classified as hard substratum, despite not being hard in the literal sense, whilst pebble habitats are not considered hard because they are not sufficiently stable to support a reef ecosystem. </skos:definition>
	<dc:source rdf:datatype="http://www.w3.org/2001/XMLSchema#string">SeaMap Australia National Benthic Habitat Classification Scheme (2017)</dc:source>
	<skos:narrower rdf:resource="http://seamapaustralia.org.au/def/benthichabitatclassification/class/5"/>
	<skos:narrower rdf:resource="http://seamapaustralia.org.au/def/benthichabitatclassification/class/6"/>
	<skos:narrower rdf:resource="http://seamapaustralia.org.au/def/benthichabitatclassification/class/4"/>
	<skos:narrower rdf:resource="http://seamapaustralia.org.au/def/benthichabitatclassification/class/7"/>
	<skos:closeMatch rdf:resource="https://www.cmecscatalog.org/cmecs/classification/dComponent/3.html"/>
	<skos:topConceptOf rdf:resource="http://seamapaustralia.org.au/def/benthichabitatclassification/1"/>
</rdf:Description>

<rdf:Description rdf:about="http://seamapaustralia.org.au/def/benthichabitatclassification/class/34">
	<rdf:type rdf:resource="http://www.w3.org/2000/01/rdf-schema#Resource"/>
	<rdf:type rdf:resource="http://www.w3.org/2004/02/skos/core#Concept"/>
	<skos:prefLabel xml:lang="en">Substratum Origin</skos:prefLabel>
	<dcterms:contributor rdf:resource="http://editor.vocabs.ands.org.au/user/eMII_Finney.Kim_Admin"/>
	<dcterms:created rdf:datatype="http://www.w3.org/2001/XMLSchema#dateTime">2016-11-16T00:40:53Z</dcterms:created>
	<dcterms:creator rdf:resource="http://editor.vocabs.ands.org.au/user/eMII_Finney.Kim_Admin"/>
	<dcterms:modified rdf:datatype="http://www.w3.org/2001/XMLSchema#dateTime">2017-06-27T04:24:39Z</dcterms:modified>
	<dc:publisher rdf:datatype="http://www.w3.org/2001/XMLSchema#string">Institute for Marine and Antarctic Studies (IMAS) - UTAS</dc:publisher>
	<skos:definition xml:lang="en">The CMECS (FGDC, 2012) 'origin' classifier provides valuable information on the source of substrate (geologic, biogenic and anthropogenic); however, it can also be one of the more difficult characteristics to classify as identified by Edmunds and Flynn (2015). The resolution required to clearly identify the origin of a substratum depends on the substratum in question. For example, rhodolith beds can be identified from acoustic surveys with simple in situ observation e.g. camera drop, whereas determining whether a sand is dominated by a mineral composition or Halimeda sp. may require analysis of sediment samples. CMECS includes 'origin' at the highest level of the substratum component hierarchy, which makes subsequent classification of substrata difficult if the 'origin' is unknown. Generally, 'origin' might be something identified at finer (lower) levels in a substrate because one would need to be at this level of resolution to obtain the information. Seamap has therefore included the origin classifier in the Seamap scheme, but has included it as a 'floating' category (rather than anchoring it within the substratum category).  </skos:definition>
	<dc:source rdf:datatype="http://www.w3.org/2001/XMLSchema#string">SeaMap Australia National Benthic Habitat Classification Scheme (2017)</dc:source>
	<skos:narrower rdf:resource="http://seamapaustralia.org.au/def/benthichabitatclassification/class/35"/>
	<skos:narrower rdf:resource="http://seamapaustralia.org.au/def/benthichabitatclassification/class/36"/>
	<skos:narrower rdf:resource="http://seamapaustralia.org.au/def/benthichabitatclassification/class/37"/>
	<skos:narrower rdf:resource="http://seamapaustralia.org.au/def/benthichabitatclassification/class/152"/>
	<skos:closeMatch rdf:resource="https://www.cmecscatalog.org/cmecs/classification/dComponent/3.html"/>
	<skos:topConceptOf rdf:resource="http://seamapaustralia.org.au/def/benthichabitatclassification/1"/>
</rdf:Description>

<rdf:Description rdf:about="http://seamapaustralia.org.au/def/benthichabitatclassification/class/69">
	<rdf:type rdf:resource="http://www.w3.org/2000/01/rdf-schema#Resource"/>
	<rdf:type rdf:resource="http://www.w3.org/2004/02/skos/core#Concept"/>
	<skos:prefLabel xml:lang="en">Biota Component</skos:prefLabel>
	<dcterms:contributor rdf:resource="http://editor.vocabs.ands.org.au/user/eMII_Finney.Kim_Admin"/>
	<dcterms:created rdf:datatype="http://www.w3.org/2001/XMLSchema#dateTime">2016-11-16T01:08:47Z</dcterms:created>
	<dcterms:creator rdf:resource="http://editor.vocabs.ands.org.au/user/eMII_Finney.Kim_Admin"/>
	<dcterms:modified rdf:datatype="http://www.w3.org/2001/XMLSchema#dateTime">2017-06-27T04:14:30Z</dcterms:modified>
	<dc:publisher rdf:datatype="http://www.w3.org/2001/XMLSchema#string">Institute for Marine and Antarctic Studies (IMAS) - UTAS
</dc:publisher>
	<skos:definition xml:lang="en">The Seamap classification of biota is a modification of the CMECS (FGCD, 2012) Biotic Component classification. The CMECS partitions have been redefined into broad biotic groups and taxonomic classes, which more accurately reflect the spatial resolution at which information in the Australian context is available. These hierarchical Seamap divisions encompass 'presence', 'class', 'subclass', 'group', 'CATAMI morphospecies' and 'species'.  The new divisions are based loosely on phylogenetic groups, with the broadest grouping in the higher levels. By using broad phylogenetic groups any dependency on substratum type (as is the case in CMECS) is removed and a true hierarchical structure is enforced. Seamap also introduces concepts for bare and unmapped areas, both of which can have important ecological ramifications. The CATAMI classification  (CATAMI Technical Working Group, 2013) is the 5th level of the Seamap scheme. Once biota have been identified to the finest level of the CATAMI scheme, species identifications are added where available. </skos:definition>
	<dc:source rdf:datatype="http://www.w3.org/2001/XMLSchema#string">SeaMap Australia National Benthic Habitat Classification Scheme (2017)
</dc:source>
	<skos:narrower rdf:resource="http://seamapaustralia.org.au/def/benthichabitatclassification/class/70"/>
	<skos:narrower rdf:resource="http://seamapaustralia.org.au/def/benthichabitatclassification/class/71"/>
	<skos:narrower rdf:resource="http://seamapaustralia.org.au/def/benthichabitatclassification/class/155"/>
	<skos:closeMatch rdf:resource="https://www.cmecscatalog.org/cmecs/classification/dComponent/2.html"/>
	<skos:topConceptOf rdf:resource="http://seamapaustralia.org.au/def/benthichabitatclassification/1"/>
	<skos:scopeNote xml:lang="en">See also http://www.catami.org</skos:scopeNote>
</rdf:Description>

<rdf:Description rdf:about="http://seamapaustralia.org.au/def/benthichabitatclassification/class/10">
	<rdf:type rdf:resource="http://www.w3.org/2000/01/rdf-schema#Resource"/>
	<rdf:type rdf:resource="http://www.w3.org/2004/02/skos/core#Concept"/>
	<skos:broader rdf:resource="http://seamapaustralia.org.au/def/benthichabitatclassification/class/5"/>
	<skos:prefLabel xml:lang="en">Mixed Hard Substrata</skos:prefLabel>
	<dcterms:contributor rdf:resource="http://editor.vocabs.ands.org.au/user/eMII_Finney.Kim_Admin"/>
	<dcterms:created rdf:datatype="http://www.w3.org/2001/XMLSchema#dateTime">2016-11-15T21:53:46Z</dcterms:created>
	<dcterms:creator rdf:resource="http://editor.vocabs.ands.org.au/user/eMII_Finney.Kim_Admin"/>
	<dcterms:modified rdf:datatype="http://www.w3.org/2001/XMLSchema#dateTime">2017-06-27T04:19:40Z</dcterms:modified>
	<dc:publisher rdf:datatype="http://www.w3.org/2001/XMLSchema#string">Institute for Marine and Antarctic Studies (IMAS) - UTAS</dc:publisher>
	<skos:definition xml:lang="en">A hard substratum composed of a mix of Consolidated Hard Substrata and Unconsolidated Hard Substrata where neither class is dominant (i.e. does not exceed ≥ 80 %) of the substratum surface/composition.</skos:definition>
	<dc:source rdf:datatype="http://www.w3.org/2001/XMLSchema#string">SeaMap Australia National Benthic Habitat Classification Scheme (2017)</dc:source>
</rdf:Description>

<rdf:Description rdf:about="http://purl.org/dc/elements/1.1/publisher">
	<rdf:type rdf:resource="http://www.w3.org/1999/02/22-rdf-syntax-ns#Property"/>
	<rdf:type rdf:resource="http://www.w3.org/2000/01/rdf-schema#Resource"/>
	<rdfs:subPropertyOf rdf:resource="http://purl.org/dc/elements/1.1/publisher"/>
</rdf:Description>

<rdf:Description rdf:about="http://www.w3.org/2004/02/skos/core#definition">
	<rdf:type rdf:resource="http://www.w3.org/1999/02/22-rdf-syntax-ns#Property"/>
	<rdf:type rdf:resource="http://www.w3.org/2000/01/rdf-schema#Resource"/>
	<rdfs:subPropertyOf rdf:resource="http://www.w3.org/2004/02/skos/core#definition"/>
</rdf:Description>

<rdf:Description rdf:about="http://www.w3.org/2004/02/skos/core#Concept">
	<rdf:type rdf:resource="http://www.w3.org/2000/01/rdf-schema#Resource"/>
	<rdf:type rdf:resource="http://www.w3.org/2000/01/rdf-schema#Class"/>
	<rdfs:subClassOf rdf:resource="http://www.w3.org/2000/01/rdf-schema#Resource"/>
	<rdfs:subClassOf rdf:resource="http://www.w3.org/2004/02/skos/core#Concept"/>
</rdf:Description>

<rdf:Description rdf:about="http://seamapaustralia.org.au/def/benthichabitatclassification/class/326">
	<rdf:type rdf:resource="http://www.w3.org/2000/01/rdf-schema#Resource"/>
	<rdf:type rdf:resource="http://www.w3.org/2004/02/skos/core#Concept"/>
	<skos:broader rdf:resource="http://seamapaustralia.org.au/def/benthichabitatclassification/class/80"/>
	<skos:prefLabel xml:lang="en">Mixed Shelled Biota</skos:prefLabel>
	<dcterms:contributor rdf:resource="http://editor.vocabs.ands.org.au/user/eMII_Finney.Kim_Admin"/>
	<dcterms:created rdf:datatype="http://www.w3.org/2001/XMLSchema#dateTime">2017-06-27T01:05:01Z</dcterms:created>
	<dcterms:creator rdf:resource="http://editor.vocabs.ands.org.au/user/eMII_Finney.Kim_Admin"/>
	<dcterms:modified rdf:datatype="http://www.w3.org/2001/XMLSchema#dateTime">2017-06-27T03:17:41Z</dcterms:modified>
	<skos:definition xml:lang="en">A habitat where the dominance of a single Shelled Biota group (Oyster, Mussel, Screwshell, Other) cannot be identified, or where the composition/biomass/surface coverage of the second-most dominant group lies within 30 % margin of the most-dominant group.</skos:definition>
</rdf:Description>

<rdf:Description rdf:about="http://seamapaustralia.org.au/def/benthichabitatclassification/class/5">
	<rdf:type rdf:resource="http://www.w3.org/2000/01/rdf-schema#Resource"/>
	<rdf:type rdf:resource="http://www.w3.org/2004/02/skos/core#Concept"/>
	<skos:broader rdf:resource="http://seamapaustralia.org.au/def/benthichabitatclassification/class/3"/>
	<skos:prefLabel xml:lang="en">Hard Substrata</skos:prefLabel>
	<dcterms:contributor rdf:resource="http://editor.vocabs.ands.org.au/user/eMII_Finney.Kim_Admin"/>
	<dcterms:created rdf:datatype="http://www.w3.org/2001/XMLSchema#dateTime">2016-11-15T04:42:42Z</dcterms:created>
	<dcterms:creator rdf:resource="http://editor.vocabs.ands.org.au/user/eMII_Finney.Kim_Admin"/>
	<dcterms:modified rdf:datatype="http://www.w3.org/2001/XMLSchema#dateTime">2017-06-27T04:18:33Z</dcterms:modified>
	<dc:publisher rdf:datatype="http://www.w3.org/2001/XMLSchema#string">Institute for Marine and Antarctic Studies (IMAS) - UTAS</dc:publisher>
	<skos:definition xml:lang="en">Substrata of any origin where ≥ 80% of the substratum surface is hard (i.e. acoustically or optically hard and/or stable enough through time to be able to maintain a reef ecosystem of some form). </skos:definition>
	<dc:source rdf:datatype="http://www.w3.org/2001/XMLSchema#string">SeaMap Australia National Benthic Habitat Classification Scheme (2017)</dc:source>
	<skos:narrower rdf:resource="http://seamapaustralia.org.au/def/benthichabitatclassification/class/10"/>
	<skos:narrower rdf:resource="http://seamapaustralia.org.au/def/benthichabitatclassification/class/8"/>
	<skos:narrower rdf:resource="http://seamapaustralia.org.au/def/benthichabitatclassification/class/9"/>
</rdf:Description>

<rdf:Description rdf:about="http://seamapaustralia.org.au/def/benthichabitatclassification/class/11">
	<rdf:type rdf:resource="http://www.w3.org/2000/01/rdf-schema#Resource"/>
	<rdf:type rdf:resource="http://www.w3.org/2004/02/skos/core#Concept"/>
	<skos:broader rdf:resource="http://seamapaustralia.org.au/def/benthichabitatclassification/class/8"/>
	<skos:prefLabel xml:lang="en">Pavement</skos:prefLabel>
	<dcterms:contributor rdf:resource="http://editor.vocabs.ands.org.au/user/eMII_Finney.Kim_Admin"/>
	<dcterms:created rdf:datatype="http://www.w3.org/2001/XMLSchema#dateTime">2016-11-15T21:57:59Z</dcterms:created>
	<dcterms:creator rdf:resource="http://editor.vocabs.ands.org.au/user/eMII_Finney.Kim_Admin"/>
	<dcterms:modified rdf:datatype="http://www.w3.org/2001/XMLSchema#dateTime">2017-06-27T04:19:34Z</dcterms:modified>
	<dc:publisher rdf:datatype="http://www.w3.org/2001/XMLSchema#string">Institute for Marine and Antarctic Studies (IMAS) - UTAS</dc:publisher>
	<skos:definition xml:lang="en">Consolidated substratum where ≥ 80 % of the consolidated surface comprises of more or less continuous rock formations where individual clasts are &gt; 1049 m in any dimension. This is equivalent to the monolith and megalith categories of Blair and McPherson (1999) grain size classes.</skos:definition>
	<dc:source rdf:datatype="http://www.w3.org/2001/XMLSchema#string">SeaMap Australia National Benthic Habitat Classification Scheme (2017)</dc:source>
</rdf:Description>

<rdf:Description rdf:about="http://purl.org/dc/elements/1.1/source">
	<rdf:type rdf:resource="http://www.w3.org/1999/02/22-rdf-syntax-ns#Property"/>
	<rdf:type rdf:resource="http://www.w3.org/2000/01/rdf-schema#Resource"/>
	<rdfs:subPropertyOf rdf:resource="http://purl.org/dc/elements/1.1/source"/>
</rdf:Description>

<rdf:Description rdf:about="http://seamapaustralia.org.au/def/benthichabitatclassification/class/8">
	<rdf:type rdf:resource="http://www.w3.org/2000/01/rdf-schema#Resource"/>
	<rdf:type rdf:resource="http://www.w3.org/2004/02/skos/core#Concept"/>
	<skos:broader rdf:resource="http://seamapaustralia.org.au/def/benthichabitatclassification/class/5"/>
	<skos:prefLabel xml:lang="en">Consolidated Hard Substrata</skos:prefLabel>
	<dcterms:contributor rdf:resource="http://editor.vocabs.ands.org.au/user/eMII_Finney.Kim_Admin"/>
	<dcterms:created rdf:datatype="http://www.w3.org/2001/XMLSchema#dateTime">2016-11-15T21:51:58Z</dcterms:created>
	<dcterms:creator rdf:resource="http://editor.vocabs.ands.org.au/user/eMII_Finney.Kim_Admin"/>
	<dcterms:modified rdf:datatype="http://www.w3.org/2001/XMLSchema#dateTime">2017-06-27T04:18:39Z</dcterms:modified>
	<dc:publisher rdf:datatype="http://www.w3.org/2001/XMLSchema#string">Institute for Marine and Antarctic Studies (IMAS) - UTAS</dc:publisher>
	<skos:definition xml:lang="en">A hard substratum where the dominant grainsize is ≥ 256 mm in any dimension.</skos:definition>
	<dc:source rdf:datatype="http://www.w3.org/2001/XMLSchema#string">SeaMap Australia National Benthic Habitat Classification Scheme (2017)</dc:source>
	<skos:narrower rdf:resource="http://seamapaustralia.org.au/def/benthichabitatclassification/class/11"/>
	<skos:narrower rdf:resource="http://seamapaustralia.org.au/def/benthichabitatclassification/class/12"/>
	<skos:narrower rdf:resource="http://seamapaustralia.org.au/def/benthichabitatclassification/class/13"/>
	<skos:narrower rdf:resource="http://seamapaustralia.org.au/def/benthichabitatclassification/class/14"/>
</rdf:Description>

<rdf:Description rdf:about="http://seamapaustralia.org.au/def/benthichabitatclassification/class/12">
	<rdf:type rdf:resource="http://www.w3.org/2000/01/rdf-schema#Resource"/>
	<rdf:type rdf:resource="http://www.w3.org/2004/02/skos/core#Concept"/>
	<skos:broader rdf:resource="http://seamapaustralia.org.au/def/benthichabitatclassification/class/8"/>
	<skos:prefLabel xml:lang="en">Megaclast</skos:prefLabel>
	<dcterms:contributor rdf:resource="http://editor.vocabs.ands.org.au/user/eMII_Finney.Kim_Admin"/>
	<dcterms:created rdf:datatype="http://www.w3.org/2001/XMLSchema#dateTime">2016-11-15T22:02:32Z</dcterms:created>
	<dcterms:creator rdf:resource="http://editor.vocabs.ands.org.au/user/eMII_Finney.Kim_Admin"/>
	<dcterms:modified rdf:datatype="http://www.w3.org/2001/XMLSchema#dateTime">2017-06-27T04:19:08Z</dcterms:modified>
	<dc:publisher rdf:datatype="http://www.w3.org/2001/XMLSchema#string">Institute for Marine and Antarctic Studies (IMAS) - UTAS</dc:publisher>
	<skos:definition xml:lang="en">Consolidated substrata where individual particles are between 4.096 -1049 m in any dimension and account ≥ 80 % of the consolidated surface/composition.</skos:definition>
	<dc:source rdf:datatype="http://www.w3.org/2001/XMLSchema#string">SeaMap Australia National Benthic Habitat Classification Scheme (2017)</dc:source>
	<skos:narrower rdf:resource="http://seamapaustralia.org.au/def/benthichabitatclassification/class/235"/>
	<skos:narrower rdf:resource="http://seamapaustralia.org.au/def/benthichabitatclassification/class/236"/>
</rdf:Description>

<rdf:Description rdf:about="http://seamapaustralia.org.au/def/benthichabitatclassification/class/337">
	<rdf:type rdf:resource="http://www.w3.org/2000/01/rdf-schema#Resource"/>
	<rdf:type rdf:resource="http://www.w3.org/2004/02/skos/core#Concept"/>
	<skos:broader rdf:resource="http://seamapaustralia.org.au/def/benthichabitatclassification/class/186"/>
	<skos:prefLabel xml:lang="en">IMCRA Northeast Province</skos:prefLabel>
	<dcterms:contributor rdf:resource="http://editor.vocabs.ands.org.au/user/eMII_Finney.Kim_Admin"/>
	<dcterms:created rdf:datatype="http://www.w3.org/2001/XMLSchema#dateTime">2017-06-27T03:28:13Z</dcterms:created>
	<dcterms:creator rdf:resource="http://editor.vocabs.ands.org.au/user/eMII_Finney.Kim_Admin"/>
	<dcterms:modified rdf:datatype="http://www.w3.org/2001/XMLSchema#dateTime">2017-06-27T03:57:49Z</dcterms:modified>
	<dc:publisher rdf:datatype="http://www.w3.org/2001/XMLSchema#string">Institute for Marine and Antarctic Studies (IMAS) - UTAS</dc:publisher>
	<skos:definition xml:lang="en">An IMCRA provincial bioregion reflects biogeographic patterns in distributions of bottom-dwelling fish. Provincial bioregions were defined for the continental shelf for IMCRA v3.3, and for the continental slope for the National Marine Bioregionalisation using similar analytical techniques. In both cases the distributions of demersal (bottom-dwelling) fish were plotted onto a line divided into equally spaced sections. The number of species in each section and the similarity between sections were calculated using a statistical tool called the Jaccard Index. Where the Jaccard Index changed greatly between sections a boundary was defined indicating differences in species assemblages between regions. Two types of provincial bioregions are defined in the IMCRA benthic bioregionalisation: provinces, which represent regions of biotic endemism; and transitions, which generally occur between the provinces, and are less well-defined mixing areas that capture the overlap of demersal fish species ranges between the provinces.</skos:definition>
	<dc:source rdf:datatype="http://www.w3.org/2001/XMLSchema#string">Commonwealth of Australia (2006). A Guide to the Integrated Marine and Coastal Regionalisation of Australia Version 4.0. Department of the Environment and Heritage, Canberra, Australia.</dc:source>
	<skos:narrower rdf:resource="http://seamapaustralia.org.au/def/benthichabitatclassification/class/338"/>
	<skos:narrower rdf:resource="http://seamapaustralia.org.au/def/benthichabitatclassification/class/343"/>
	<skos:narrower rdf:resource="http://seamapaustralia.org.au/def/benthichabitatclassification/class/339"/>
	<skos:narrower rdf:resource="http://seamapaustralia.org.au/def/benthichabitatclassification/class/340"/>
	<skos:narrower rdf:resource="http://seamapaustralia.org.au/def/benthichabitatclassification/class/342"/>
	<skos:narrower rdf:resource="http://seamapaustralia.org.au/def/benthichabitatclassification/class/341"/>
	<skos:exactMatch rdf:resource="http://www.environment.gov.au/mapping/rest/services/ogc_services/IMCRA_Provincial/MapServer/0/12"/>
</rdf:Description>

<rdf:Description rdf:about="http://seamapaustralia.org.au/def/benthichabitatclassification/class/13">
	<rdf:type rdf:resource="http://www.w3.org/2000/01/rdf-schema#Resource"/>
	<rdf:type rdf:resource="http://www.w3.org/2004/02/skos/core#Concept"/>
	<skos:broader rdf:resource="http://seamapaustralia.org.au/def/benthichabitatclassification/class/8"/>
	<skos:prefLabel xml:lang="en">Boulder</skos:prefLabel>
	<dcterms:contributor rdf:resource="http://editor.vocabs.ands.org.au/user/eMII_Finney.Kim_Admin"/>
	<dcterms:created rdf:datatype="http://www.w3.org/2001/XMLSchema#dateTime">2016-11-15T22:03:14Z</dcterms:created>
	<dcterms:creator rdf:resource="http://editor.vocabs.ands.org.au/user/eMII_Finney.Kim_Admin"/>
	<dcterms:modified rdf:datatype="http://www.w3.org/2001/XMLSchema#dateTime">2017-06-27T04:18:44Z</dcterms:modified>
	<dc:publisher rdf:datatype="http://www.w3.org/2001/XMLSchema#string">Institute for Marine and Antarctic Studies (IMAS) - UTAS</dc:publisher>
	<skos:definition xml:lang="en">Consolidated substrata where individual particles are between 256-4096 mm in any dimension and comprise ≥ 80 % of the surface</skos:definition>
	<dc:source rdf:datatype="http://www.w3.org/2001/XMLSchema#string">SeaMap Australia National Benthic Habitat Classification Scheme (2017)</dc:source>
	<skos:narrower rdf:resource="http://seamapaustralia.org.au/def/benthichabitatclassification/class/237"/>
	<skos:narrower rdf:resource="http://seamapaustralia.org.au/def/benthichabitatclassification/class/238"/>
	<skos:narrower rdf:resource="http://seamapaustralia.org.au/def/benthichabitatclassification/class/239"/>
	<skos:narrower rdf:resource="http://seamapaustralia.org.au/def/benthichabitatclassification/class/240"/>
</rdf:Description>

<rdf:Description rdf:about="http://seamapaustralia.org.au/def/benthichabitatclassification/class/338">
	<rdf:type rdf:resource="http://www.w3.org/2000/01/rdf-schema#Resource"/>
	<rdf:type rdf:resource="http://www.w3.org/2004/02/skos/core#Concept"/>
	<skos:broader rdf:resource="http://seamapaustralia.org.au/def/benthichabitatclassification/class/337"/>
	<skos:prefLabel xml:lang="en">IMCRA Wet Tropic Coast Bioregion</skos:prefLabel>
	<dcterms:contributor rdf:resource="http://editor.vocabs.ands.org.au/user/eMII_Finney.Kim_Admin"/>
	<dcterms:created rdf:datatype="http://www.w3.org/2001/XMLSchema#dateTime">2017-06-27T03:28:45Z</dcterms:created>
	<dcterms:creator rdf:resource="http://editor.vocabs.ands.org.au/user/eMII_Finney.Kim_Admin"/>
	<dcterms:modified rdf:datatype="http://www.w3.org/2001/XMLSchema#dateTime">2017-06-27T03:59:13Z</dcterms:modified>
	<dc:publisher rdf:datatype="http://www.w3.org/2001/XMLSchema#string">Institute for Marine and Antarctic Studies (IMAS) - UTAS</dc:publisher>
	<skos:definition xml:lang="en">An inshore regionalisation of Australian waters derived from biological and physical data, including the distribution of demersal fishes, marine plants and invertebrates, sea floor geomorphology and sediments, and oceanographic data. The meso-scale regionalisation was compiled from information supplied to the Australian Government Department of the Environment and Heritage by the relevant State, Northern Territory and Commonwealth marine research and management agencies. The seaward extent for the meso-scale IMCRA coverage is defined by the 200m isobath except where this boundary extends beyond the Australian Exclusive Economic Zone (AEEZ).</skos:definition>
	<dc:source rdf:datatype="http://www.w3.org/2001/XMLSchema#string">Commonwealth of Australia (2006). A Guide to the Integrated Marine and Coastal Regionalisation of Australia Version 4.0. Department of the Environment and Heritage, Canberra, Australia.</dc:source>
	<skos:exactMatch rdf:resource="http://www.environment.gov.au/mapping/rest/services/ogc_services/IMCRA_Mesoscale/MapServer/0/20"/>
</rdf:Description>

<rdf:Description rdf:about="http://seamapaustralia.org.au/def/benthichabitatclassification/class/14">
	<rdf:type rdf:resource="http://www.w3.org/2000/01/rdf-schema#Resource"/>
	<rdf:type rdf:resource="http://www.w3.org/2004/02/skos/core#Concept"/>
	<skos:broader rdf:resource="http://seamapaustralia.org.au/def/benthichabitatclassification/class/8"/>
	<skos:prefLabel xml:lang="en">Mixed Consolidated Substrata</skos:prefLabel>
	<dcterms:contributor rdf:resource="http://editor.vocabs.ands.org.au/user/eMII_Finney.Kim_Admin"/>
	<dcterms:created rdf:datatype="http://www.w3.org/2001/XMLSchema#dateTime">2016-11-15T22:03:54Z</dcterms:created>
	<dcterms:creator rdf:resource="http://editor.vocabs.ands.org.au/user/eMII_Finney.Kim_Admin"/>
	<dcterms:modified rdf:datatype="http://www.w3.org/2001/XMLSchema#dateTime">2017-06-27T04:19:28Z</dcterms:modified>
	<dc:publisher rdf:datatype="http://www.w3.org/2001/XMLSchema#string">Institute for Marine and Antarctic Studies (IMAS) - UTAS</dc:publisher>
	<skos:definition xml:lang="en">A Consolidated Hard Substratum composed of a mixture two or more of Pavement, Megaclasts and Boulders, but where no individual component exceeds ≥ 80 % of the substratum surface/composition.</skos:definition>
	<dc:source rdf:datatype="http://www.w3.org/2001/XMLSchema#string">SeaMap Australia National Benthic Habitat Classification Scheme (2017)</dc:source>
</rdf:Description>

<rdf:Description rdf:about="http://seamapaustralia.org.au/def/benthichabitatclassification/class/186">
	<rdf:type rdf:resource="http://www.w3.org/2000/01/rdf-schema#Resource"/>
	<rdf:type rdf:resource="http://www.w3.org/2004/02/skos/core#Concept"/>
	<skos:broader rdf:resource="http://seamapaustralia.org.au/def/benthichabitatclassification/class/174"/>
	<skos:prefLabel xml:lang="en">MEOW Central and Southern Great Barrier Reef Ecoregion</skos:prefLabel>
	<dcterms:contributor rdf:resource="http://editor.vocabs.ands.org.au/user/eMII_Finney.Kim_Admin"/>
	<dcterms:created rdf:datatype="http://www.w3.org/2001/XMLSchema#dateTime">2017-05-31T02:02:28Z</dcterms:created>
	<dcterms:creator rdf:resource="http://editor.vocabs.ands.org.au/user/eMII_Finney.Kim_Admin"/>
	<dcterms:modified rdf:datatype="http://www.w3.org/2001/XMLSchema#dateTime">2017-06-27T04:08:10Z</dcterms:modified>
	<dc:publisher rdf:datatype="http://www.w3.org/2001/XMLSchema#string">Institute for Marine and Antarctic Studies (IMAS) - UTAS</dc:publisher>
	<skos:definition xml:lang="en">An area of relatively homogenous species composition, clearly distinct from adjacent systems. The species composition is likely to be determined by the predominance of a small number of ecosystems and/or a distinct suite of oceanographic or topographic features. The dominant biogeographic forcing agents defining the ecoregions vary from location to location but may include isolation, upwelling, nutrient inputs, freshwater influx, temperature regimes, ice regimes, exposure, sediments, currents and bathymetric or coastal complexity.</skos:definition>
	<dc:source rdf:datatype="http://www.w3.org/2001/XMLSchema#string">Marine Ecoregions of the World (MEOW). Spalding et.al. (2007)</dc:source>
	<skos:narrower rdf:resource="http://seamapaustralia.org.au/def/benthichabitatclassification/class/337"/>
	<skos:exactMatch rdf:resource="http://www.marineregions.org/gazetteer.php?p=details&amp;id=21904"/>
</rdf:Description>

<rdf:Description rdf:about="http://www.w3.org/2004/02/skos/core#narrower">
	<rdf:type rdf:resource="http://www.w3.org/1999/02/22-rdf-syntax-ns#Property"/>
	<rdf:type rdf:resource="http://www.w3.org/2000/01/rdf-schema#Resource"/>
	<rdfs:subPropertyOf rdf:resource="http://www.w3.org/2004/02/skos/core#narrower"/>
</rdf:Description>

<rdf:Description rdf:about="http://seamapaustralia.org.au/def/benthichabitatclassification/class/15">
	<rdf:type rdf:resource="http://www.w3.org/2000/01/rdf-schema#Resource"/>
	<rdf:type rdf:resource="http://www.w3.org/2004/02/skos/core#Concept"/>
	<skos:broader rdf:resource="http://seamapaustralia.org.au/def/benthichabitatclassification/class/9"/>
	<skos:prefLabel xml:lang="en">Cobble</skos:prefLabel>
	<dcterms:contributor rdf:resource="http://editor.vocabs.ands.org.au/user/eMII_Finney.Kim_Admin"/>
	<dcterms:created rdf:datatype="http://www.w3.org/2001/XMLSchema#dateTime">2016-11-15T22:06:39Z</dcterms:created>
	<dcterms:creator rdf:resource="http://editor.vocabs.ands.org.au/user/eMII_Finney.Kim_Admin"/>
	<dcterms:modified rdf:datatype="http://www.w3.org/2001/XMLSchema#dateTime">2017-06-27T04:19:50Z</dcterms:modified>
	<dc:publisher rdf:datatype="http://www.w3.org/2001/XMLSchema#string">Institute for Marine and Antarctic Studies (IMAS) - UTAS</dc:publisher>
	<skos:definition xml:lang="en">Unconsolidated substrata from 64-256 mm in any dimension that cover ≥ 80 % of the unconsolidated component of the substratum.</skos:definition>
	<dc:source rdf:datatype="http://www.w3.org/2001/XMLSchema#string">  SeaMap Australia National Benthic Habitat Classification Scheme (2017)</dc:source>
	<skos:narrower rdf:resource="http://seamapaustralia.org.au/def/benthichabitatclassification/class/241"/>
	<skos:narrower rdf:resource="http://seamapaustralia.org.au/def/benthichabitatclassification/class/242"/>
</rdf:Description>

<rdf:Description rdf:about="http://seamapaustralia.org.au/def/benthichabitatclassification/class/325">
	<rdf:type rdf:resource="http://www.w3.org/2000/01/rdf-schema#Resource"/>
	<rdf:type rdf:resource="http://www.w3.org/2004/02/skos/core#Concept"/>
	<skos:broader rdf:resource="http://seamapaustralia.org.au/def/benthichabitatclassification/class/78"/>
	<skos:prefLabel xml:lang="en">Mixed Filter Feeder Community</skos:prefLabel>
	<dcterms:contributor rdf:resource="http://editor.vocabs.ands.org.au/user/eMII_Finney.Kim_Admin"/>
	<dcterms:created rdf:datatype="http://www.w3.org/2001/XMLSchema#dateTime">2017-06-27T01:03:54Z</dcterms:created>
	<dcterms:creator rdf:resource="http://editor.vocabs.ands.org.au/user/eMII_Finney.Kim_Admin"/>
	<dcterms:modified rdf:datatype="http://www.w3.org/2001/XMLSchema#dateTime">2017-06-27T03:17:13Z</dcterms:modified>
	<skos:definition xml:lang="en">A habitat where the dominance of a single Non-molluscan Filter Feeder group (Non-coral Cnidaria, Corals, Worms, Bryozoans, Sponges, Ascidians) cannot be identified, or where the composition/biomass/surface coverage of the second-most dominant group lies within 30 % margin of the most-dominant group.</skos:definition>
</rdf:Description>

<rdf:Description rdf:about="http://seamapaustralia.org.au/def/benthichabitatclassification/class/9">
	<rdf:type rdf:resource="http://www.w3.org/2000/01/rdf-schema#Resource"/>
	<rdf:type rdf:resource="http://www.w3.org/2004/02/skos/core#Concept"/>
	<skos:broader rdf:resource="http://seamapaustralia.org.au/def/benthichabitatclassification/class/5"/>
	<skos:prefLabel xml:lang="en">Unconsolidated Hard Susbtrata</skos:prefLabel>
	<dcterms:contributor rdf:resource="http://editor.vocabs.ands.org.au/user/eMII_Finney.Kim_Admin"/>
	<dcterms:created rdf:datatype="http://www.w3.org/2001/XMLSchema#dateTime">2016-11-15T21:53:13Z</dcterms:created>
	<dcterms:creator rdf:resource="http://editor.vocabs.ands.org.au/user/eMII_Finney.Kim_Admin"/>
	<dcterms:modified rdf:datatype="http://www.w3.org/2001/XMLSchema#dateTime">2017-06-27T04:19:45Z</dcterms:modified>
	<dc:publisher rdf:datatype="http://www.w3.org/2001/XMLSchema#string">Institute for Marine and Antarctic Studies (IMAS) - UTAS</dc:publisher>
	<skos:definition xml:lang="en">A hard substratum where grain sizes of &lt; 256 mm in any dimension are dominant (i.e ≥ 80 % of the hard substratum surface)</skos:definition>
	<dc:source rdf:datatype="http://www.w3.org/2001/XMLSchema#string">SeaMap Australia National Benthic Habitat Classification Scheme (2017)</dc:source>
	<skos:narrower rdf:resource="http://seamapaustralia.org.au/def/benthichabitatclassification/class/15"/>
</rdf:Description>

<rdf:Description rdf:about="http://seamapaustralia.org.au/def/benthichabitatclassification/class/16">
	<rdf:type rdf:resource="http://www.w3.org/2000/01/rdf-schema#Resource"/>
	<rdf:type rdf:resource="http://www.w3.org/2004/02/skos/core#Concept"/>
	<skos:broader rdf:resource="http://seamapaustralia.org.au/def/benthichabitatclassification/class/6"/>
	<skos:prefLabel xml:lang="en">Coarse Sediments</skos:prefLabel>
	<dcterms:contributor rdf:resource="http://editor.vocabs.ands.org.au/user/eMII_Finney.Kim_Admin"/>
	<dcterms:created rdf:datatype="http://www.w3.org/2001/XMLSchema#dateTime">2016-11-15T22:43:45Z</dcterms:created>
	<dcterms:creator rdf:resource="http://editor.vocabs.ands.org.au/user/eMII_Finney.Kim_Admin"/>
	<dcterms:modified rdf:datatype="http://www.w3.org/2001/XMLSchema#dateTime">2017-06-27T04:39:39Z</dcterms:modified>
	<dc:publisher rdf:datatype="http://www.w3.org/2001/XMLSchema#string">Institute for Marine and Antarctic Studies (IMAS) - UTAS</dc:publisher>
	<skos:definition xml:lang="en">A soft substratum where grainsizes of 0.0625 – 64 mm in any dimension are dominant (i.e. account for ≥ 80 % of the soft substratum composition). </skos:definition>
	<dc:source rdf:datatype="http://www.w3.org/2001/XMLSchema#string">SeaMap Australia National Benthic Habitat Classification Scheme (2017)</dc:source>
	<skos:narrower rdf:resource="http://seamapaustralia.org.au/def/benthichabitatclassification/class/19"/>
	<skos:narrower rdf:resource="http://seamapaustralia.org.au/def/benthichabitatclassification/class/20"/>
	<skos:narrower rdf:resource="http://seamapaustralia.org.au/def/benthichabitatclassification/class/21"/>
	<skos:narrower rdf:resource="http://seamapaustralia.org.au/def/benthichabitatclassification/class/29"/>
</rdf:Description>

<rdf:Description rdf:about="http://seamapaustralia.org.au/def/benthichabitatclassification/class/332">
	<rdf:type rdf:resource="http://www.w3.org/2000/01/rdf-schema#Resource"/>
	<rdf:type rdf:resource="http://www.w3.org/2004/02/skos/core#Concept"/>
	<skos:broader rdf:resource="http://seamapaustralia.org.au/def/benthichabitatclassification/class/331"/>
	<skos:prefLabel xml:lang="en">Screw Shell</skos:prefLabel>
	<dcterms:contributor rdf:resource="http://editor.vocabs.ands.org.au/user/eMII_Finney.Kim_Admin"/>
	<dcterms:created rdf:datatype="http://www.w3.org/2001/XMLSchema#dateTime">2017-06-27T01:47:18Z</dcterms:created>
	<dcterms:creator rdf:resource="http://editor.vocabs.ands.org.au/user/eMII_Finney.Kim_Admin"/>
	<dcterms:modified rdf:datatype="http://www.w3.org/2001/XMLSchema#dateTime">2017-06-27T01:53:05Z</dcterms:modified>
	<skos:definition xml:lang="en">Biogenic substrata dominated by screw shells.</skos:definition>
</rdf:Description>

<rdf:Description rdf:about="http://seamapaustralia.org.au/def/benthichabitatclassification/class/6">
	<rdf:type rdf:resource="http://www.w3.org/2000/01/rdf-schema#Resource"/>
	<rdf:type rdf:resource="http://www.w3.org/2004/02/skos/core#Concept"/>
	<skos:broader rdf:resource="http://seamapaustralia.org.au/def/benthichabitatclassification/class/3"/>
	<skos:prefLabel xml:lang="en">Soft Substrata</skos:prefLabel>
	<dcterms:contributor rdf:resource="http://editor.vocabs.ands.org.au/user/eMII_Finney.Kim_Admin"/>
	<dcterms:created rdf:datatype="http://www.w3.org/2001/XMLSchema#dateTime">2016-11-15T04:43:24Z</dcterms:created>
	<dcterms:creator rdf:resource="http://editor.vocabs.ands.org.au/user/eMII_Finney.Kim_Admin"/>
	<dcterms:modified rdf:datatype="http://www.w3.org/2001/XMLSchema#dateTime">2017-06-27T04:20:12Z</dcterms:modified>
	<dc:publisher rdf:datatype="http://www.w3.org/2001/XMLSchema#string">Institute for Marine and Antarctic Studies (IMAS) - UTAS</dc:publisher>
	<skos:definition xml:lang="en">Substrata of any origin where ≥ 80% of the substratum surface is soft (i.e. acoustically or optically soft and/or not stable enough through time to be able to maintain a reef ecosystem of some form). This is equivalent to a substratum where &lt; 20 %  of the substratum surface is hard. </skos:definition>
	<dc:source rdf:datatype="http://www.w3.org/2001/XMLSchema#string">SeaMap Australia National Benthic Habitat Classification Scheme (2017)</dc:source>
	<skos:narrower rdf:resource="http://seamapaustralia.org.au/def/benthichabitatclassification/class/16"/>
	<skos:narrower rdf:resource="http://seamapaustralia.org.au/def/benthichabitatclassification/class/17"/>
	<skos:narrower rdf:resource="http://seamapaustralia.org.au/def/benthichabitatclassification/class/18"/>
</rdf:Description>

<rdf:Description rdf:about="http://seamapaustralia.org.au/def/benthichabitatclassification/class/19">
	<rdf:type rdf:resource="http://www.w3.org/2000/01/rdf-schema#Resource"/>
	<rdf:type rdf:resource="http://www.w3.org/2004/02/skos/core#Concept"/>
	<skos:broader rdf:resource="http://seamapaustralia.org.au/def/benthichabitatclassification/class/16"/>
	<skos:prefLabel xml:lang="en">Pebble</skos:prefLabel>
	<dcterms:contributor rdf:resource="http://editor.vocabs.ands.org.au/user/eMII_Finney.Kim_Admin"/>
	<dcterms:created rdf:datatype="http://www.w3.org/2001/XMLSchema#dateTime">2016-11-15T22:49:35Z</dcterms:created>
	<dcterms:creator rdf:resource="http://editor.vocabs.ands.org.au/user/eMII_Finney.Kim_Admin"/>
	<dcterms:modified rdf:datatype="http://www.w3.org/2001/XMLSchema#dateTime">2017-06-27T04:20:44Z</dcterms:modified>
	<dc:publisher rdf:datatype="http://www.w3.org/2001/XMLSchema#string">Institute for Marine and Antarctic Studies (IMAS) - UTAS</dc:publisher>
	<skos:definition xml:lang="en">A Coarse Soft sediment where particles between 4-64 mm in any dimension are dominant (constitute ≥ 80 % of the coarse sediment).</skos:definition>
	<dc:source rdf:datatype="http://www.w3.org/2001/XMLSchema#string">SeaMap Australia National Benthic Habitat Classification Scheme (2017)</dc:source>
	<skos:narrower rdf:resource="http://seamapaustralia.org.au/def/benthichabitatclassification/class/243"/>
	<skos:narrower rdf:resource="http://seamapaustralia.org.au/def/benthichabitatclassification/class/244"/>
	<skos:narrower rdf:resource="http://seamapaustralia.org.au/def/benthichabitatclassification/class/245"/>
	<skos:narrower rdf:resource="http://seamapaustralia.org.au/def/benthichabitatclassification/class/246"/>
</rdf:Description>

<rdf:Description rdf:about="http://seamapaustralia.org.au/def/benthichabitatclassification/class/20">
	<rdf:type rdf:resource="http://www.w3.org/2000/01/rdf-schema#Resource"/>
	<rdf:type rdf:resource="http://www.w3.org/2004/02/skos/core#Concept"/>
	<skos:broader rdf:resource="http://seamapaustralia.org.au/def/benthichabitatclassification/class/16"/>
	<skos:prefLabel xml:lang="en">Granule</skos:prefLabel>
	<dcterms:contributor rdf:resource="http://editor.vocabs.ands.org.au/user/eMII_Finney.Kim_Admin"/>
	<dcterms:created rdf:datatype="http://www.w3.org/2001/XMLSchema#dateTime">2016-11-15T22:49:55Z</dcterms:created>
	<dcterms:creator rdf:resource="http://editor.vocabs.ands.org.au/user/eMII_Finney.Kim_Admin"/>
	<dcterms:modified rdf:datatype="http://www.w3.org/2001/XMLSchema#dateTime">2017-06-27T04:20:21Z</dcterms:modified>
	<dc:publisher rdf:datatype="http://www.w3.org/2001/XMLSchema#string">Institute for Marine and Antarctic Studies (IMAS) - UTAS</dc:publisher>
	<skos:definition xml:lang="en">A Coarse Soft Sediment where particles between 2-4 mm in any dimension are dominant (constitute ≥ 80 % of the coarse sediment).</skos:definition>
	<dc:source rdf:datatype="http://www.w3.org/2001/XMLSchema#string">SeaMap Australia National Benthic Habitat Classification Scheme (2017)</dc:source>
</rdf:Description>

<rdf:Description rdf:about="http://seamapaustralia.org.au/def/benthichabitatclassification/class/21">
	<rdf:type rdf:resource="http://www.w3.org/2000/01/rdf-schema#Resource"/>
	<rdf:type rdf:resource="http://www.w3.org/2004/02/skos/core#Concept"/>
	<skos:broader rdf:resource="http://seamapaustralia.org.au/def/benthichabitatclassification/class/16"/>
	<skos:prefLabel xml:lang="en">Sand</skos:prefLabel>
	<dcterms:contributor rdf:resource="http://editor.vocabs.ands.org.au/user/eMII_Finney.Kim_Admin"/>
	<dcterms:created rdf:datatype="http://www.w3.org/2001/XMLSchema#dateTime">2016-11-15T22:50:12Z</dcterms:created>
	<dcterms:creator rdf:resource="http://editor.vocabs.ands.org.au/user/eMII_Finney.Kim_Admin"/>
	<dcterms:modified rdf:datatype="http://www.w3.org/2001/XMLSchema#dateTime">2017-06-27T04:21:11Z</dcterms:modified>
	<dc:publisher rdf:datatype="http://www.w3.org/2001/XMLSchema#string">Institute for Marine and Antarctic Studies (IMAS) - UTAS</dc:publisher>
	<skos:definition xml:lang="en">A coarse substratum constituting a dominance (≥ 80 %) of particles with grainsizes 0.0625-2 mm in any dimension.</skos:definition>
	<dc:source rdf:datatype="http://www.w3.org/2001/XMLSchema#string">SeaMap Australia National Benthic Habitat Classification Scheme (2017)</dc:source>
	<skos:narrower rdf:resource="http://seamapaustralia.org.au/def/benthichabitatclassification/class/24"/>
	<skos:narrower rdf:resource="http://seamapaustralia.org.au/def/benthichabitatclassification/class/25"/>
	<skos:narrower rdf:resource="http://seamapaustralia.org.au/def/benthichabitatclassification/class/26"/>
	<skos:narrower rdf:resource="http://seamapaustralia.org.au/def/benthichabitatclassification/class/27"/>
	<skos:narrower rdf:resource="http://seamapaustralia.org.au/def/benthichabitatclassification/class/28"/>
</rdf:Description>

<rdf:Description rdf:about="http://seamapaustralia.org.au/def/benthichabitatclassification/class/29">
	<rdf:type rdf:resource="http://www.w3.org/2000/01/rdf-schema#Resource"/>
	<rdf:type rdf:resource="http://www.w3.org/2004/02/skos/core#Concept"/>
	<skos:broader rdf:resource="http://seamapaustralia.org.au/def/benthichabitatclassification/class/16"/>
	<skos:prefLabel xml:lang="en">Mixed Coarse Sediments</skos:prefLabel>
	<dcterms:contributor rdf:resource="http://editor.vocabs.ands.org.au/user/eMII_Finney.Kim_Admin"/>
	<dcterms:created rdf:datatype="http://www.w3.org/2001/XMLSchema#dateTime">2016-11-15T22:58:13Z</dcterms:created>
	<dcterms:creator rdf:resource="http://editor.vocabs.ands.org.au/user/eMII_Finney.Kim_Admin"/>
	<dcterms:modified rdf:datatype="http://www.w3.org/2001/XMLSchema#dateTime">2017-06-27T04:20:32Z</dcterms:modified>
	<dc:publisher rdf:datatype="http://www.w3.org/2001/XMLSchema#string">Institute for Marine and Antarctic Studies (IMAS) - UTAS</dc:publisher>
	<skos:definition xml:lang="en">A Coarse Sediment composed of a mixture of any combination of Pebble, Granule and Sand, but where no individual component exceeds ≥ 80 % of the substratum surface/composition. </skos:definition>
	<dc:source rdf:datatype="http://www.w3.org/2001/XMLSchema#string">SeaMap Australia National Benthic Habitat Classification Scheme (2017)</dc:source>
</rdf:Description>

<rdf:Description rdf:about="http://seamapaustralia.org.au/def/benthichabitatclassification/class/17">
	<rdf:type rdf:resource="http://www.w3.org/2000/01/rdf-schema#Resource"/>
	<rdf:type rdf:resource="http://www.w3.org/2004/02/skos/core#Concept"/>
	<skos:broader rdf:resource="http://seamapaustralia.org.au/def/benthichabitatclassification/class/6"/>
	<skos:prefLabel xml:lang="en">Fine Sediments</skos:prefLabel>
	<dcterms:contributor rdf:resource="http://editor.vocabs.ands.org.au/user/eMII_Finney.Kim_Admin"/>
	<dcterms:created rdf:datatype="http://www.w3.org/2001/XMLSchema#dateTime">2016-11-15T22:44:08Z</dcterms:created>
	<dcterms:creator rdf:resource="http://editor.vocabs.ands.org.au/user/eMII_Finney.Kim_Admin"/>
	<dcterms:modified rdf:datatype="http://www.w3.org/2001/XMLSchema#dateTime">2017-06-27T04:21:43Z</dcterms:modified>
	<dc:publisher rdf:datatype="http://www.w3.org/2001/XMLSchema#string">Institute for Marine and Antarctic Studies (IMAS) - UTAS</dc:publisher>
	<skos:definition xml:lang="en">A soft substratum where grainsizes of 0.0039 - 0.0625 mm in any dimension are dominant (i.e. account for ≥ 80 % of the soft substratum composition).</skos:definition>
	<dc:source rdf:datatype="http://www.w3.org/2001/XMLSchema#string">SeaMap Australia National Benthic Habitat Classification Scheme (2017)</dc:source>
	<skos:narrower rdf:resource="http://seamapaustralia.org.au/def/benthichabitatclassification/class/22"/>
	<skos:narrower rdf:resource="http://seamapaustralia.org.au/def/benthichabitatclassification/class/23"/>
	<skos:narrower rdf:resource="http://seamapaustralia.org.au/def/benthichabitatclassification/class/151"/>
</rdf:Description>

<rdf:Description rdf:about="http://seamapaustralia.org.au/def/benthichabitatclassification/class/318">
	<rdf:type rdf:resource="http://www.w3.org/2000/01/rdf-schema#Resource"/>
	<rdf:type rdf:resource="http://www.w3.org/2004/02/skos/core#Concept"/>
	<skos:broader rdf:resource="http://seamapaustralia.org.au/def/benthichabitatclassification/class/71"/>
	<skos:prefLabel xml:lang="en">Mixed Biota</skos:prefLabel>
	<dcterms:contributor rdf:resource="http://editor.vocabs.ands.org.au/user/eMII_Finney.Kim_Admin"/>
	<dcterms:created rdf:datatype="http://www.w3.org/2001/XMLSchema#dateTime">2017-06-27T00:49:51Z</dcterms:created>
	<dcterms:creator rdf:resource="http://editor.vocabs.ands.org.au/user/eMII_Finney.Kim_Admin"/>
	<dcterms:modified rdf:datatype="http://www.w3.org/2001/XMLSchema#dateTime">2017-06-27T03:14:22Z</dcterms:modified>
	<skos:definition xml:lang="en">A habitat where the dominance of a single biotic class (Vegetation, Microbes, Invertebrates or Urchin Barrens) is unclear, or where the composition/biomass/surface coverage of the second-most dominant class lies within 30 % margin of the most-dominant biotic class.</skos:definition>
</rdf:Description>

<rdf:Description rdf:about="http://seamapaustralia.org.au/def/benthichabitatclassification/class/22">
	<rdf:type rdf:resource="http://www.w3.org/2000/01/rdf-schema#Resource"/>
	<rdf:type rdf:resource="http://www.w3.org/2004/02/skos/core#Concept"/>
	<skos:broader rdf:resource="http://seamapaustralia.org.au/def/benthichabitatclassification/class/17"/>
	<skos:prefLabel xml:lang="en">Silt</skos:prefLabel>
	<dcterms:contributor rdf:resource="http://editor.vocabs.ands.org.au/user/eMII_Finney.Kim_Admin"/>
	<dcterms:created rdf:datatype="http://www.w3.org/2001/XMLSchema#dateTime">2016-11-15T22:50:43Z</dcterms:created>
	<dcterms:creator rdf:resource="http://editor.vocabs.ands.org.au/user/eMII_Finney.Kim_Admin"/>
	<dcterms:modified rdf:datatype="http://www.w3.org/2001/XMLSchema#dateTime">2017-06-27T04:22:03Z</dcterms:modified>
	<dc:publisher rdf:datatype="http://www.w3.org/2001/XMLSchema#string">Institute for Marine and Antarctic Studies (IMAS) - UTAS</dc:publisher>
	<skos:definition xml:lang="en">Fine substrata where ≥ 80 % of the grains are between 0.0039-0.0625 mm in any dimension.</skos:definition>
	<dc:source rdf:datatype="http://www.w3.org/2001/XMLSchema#string">SeaMap Australia National Benthic Habitat Classification Scheme (2017)</dc:source>
	<skos:narrower rdf:resource="http://seamapaustralia.org.au/def/benthichabitatclassification/class/30"/>
	<skos:narrower rdf:resource="http://seamapaustralia.org.au/def/benthichabitatclassification/class/31"/>
	<skos:narrower rdf:resource="http://seamapaustralia.org.au/def/benthichabitatclassification/class/32"/>
	<skos:narrower rdf:resource="http://seamapaustralia.org.au/def/benthichabitatclassification/class/33"/>
</rdf:Description>

<rdf:Description rdf:about="http://seamapaustralia.org.au/def/benthichabitatclassification/class/23">
	<rdf:type rdf:resource="http://www.w3.org/2000/01/rdf-schema#Resource"/>
	<rdf:type rdf:resource="http://www.w3.org/2004/02/skos/core#Concept"/>
	<skos:broader rdf:resource="http://seamapaustralia.org.au/def/benthichabitatclassification/class/17"/>
	<skos:prefLabel xml:lang="en">Clay</skos:prefLabel>
	<dcterms:contributor rdf:resource="http://editor.vocabs.ands.org.au/user/eMII_Finney.Kim_Admin"/>
	<dcterms:created rdf:datatype="http://www.w3.org/2001/XMLSchema#dateTime">2016-11-15T22:50:59Z</dcterms:created>
	<dcterms:creator rdf:resource="http://editor.vocabs.ands.org.au/user/eMII_Finney.Kim_Admin"/>
	<dcterms:modified rdf:datatype="http://www.w3.org/2001/XMLSchema#dateTime">2017-06-27T04:21:48Z</dcterms:modified>
	<dc:publisher rdf:datatype="http://www.w3.org/2001/XMLSchema#string">Institute for Marine and Antarctic Studies (IMAS) - UTAS</dc:publisher>
	<skos:definition xml:lang="en">Fine substrata where ≥ 80 % of the grains are between 0.00006-0.0039 mm in any dimension.</skos:definition>
	<dc:source rdf:datatype="http://www.w3.org/2001/XMLSchema#string">SeaMap Australia National Benthic Habitat Classification Scheme (2017)</dc:source>
</rdf:Description>

<rdf:Description rdf:about="http://seamapaustralia.org.au/def/benthichabitatclassification/class/18">
	<rdf:type rdf:resource="http://www.w3.org/2000/01/rdf-schema#Resource"/>
	<rdf:type rdf:resource="http://www.w3.org/2004/02/skos/core#Concept"/>
	<skos:broader rdf:resource="http://seamapaustralia.org.au/def/benthichabitatclassification/class/6"/>
	<skos:prefLabel xml:lang="en">Mixed Soft Substrata</skos:prefLabel>
	<dcterms:contributor rdf:resource="http://editor.vocabs.ands.org.au/user/eMII_Finney.Kim_Admin"/>
	<dcterms:created rdf:datatype="http://www.w3.org/2001/XMLSchema#dateTime">2016-11-15T22:44:30Z</dcterms:created>
	<dcterms:creator rdf:resource="http://editor.vocabs.ands.org.au/user/eMII_Finney.Kim_Admin"/>
	<dcterms:modified rdf:datatype="http://www.w3.org/2001/XMLSchema#dateTime">2017-06-27T04:22:29Z</dcterms:modified>
	<dc:publisher rdf:datatype="http://www.w3.org/2001/XMLSchema#string">Institute for Marine and Antarctic Studies (IMAS) - UTAS</dc:publisher>
	<skos:definition xml:lang="en">A substratum composed of a mix of hard and soft substrata such that the percentage cover of neither class is dominant (i.e. percentage cover of neither class is ≥ 80 %).</skos:definition>
	<dc:source rdf:datatype="http://www.w3.org/2001/XMLSchema#string">SeaMap Australia National Benthic Habitat Classification Scheme (2017)</dc:source>
</rdf:Description>

<rdf:Description rdf:about="http://seamapaustralia.org.au/def/benthichabitatclassification/class/323">
	<rdf:type rdf:resource="http://www.w3.org/2000/01/rdf-schema#Resource"/>
	<rdf:type rdf:resource="http://www.w3.org/2004/02/skos/core#Concept"/>
	<skos:broader rdf:resource="http://seamapaustralia.org.au/def/benthichabitatclassification/class/74"/>
	<skos:prefLabel xml:lang="en">Mixed Microbes</skos:prefLabel>
	<dcterms:contributor rdf:resource="http://editor.vocabs.ands.org.au/user/eMII_Finney.Kim_Admin"/>
	<dcterms:created rdf:datatype="http://www.w3.org/2001/XMLSchema#dateTime">2017-06-27T01:02:03Z</dcterms:created>
	<dcterms:creator rdf:resource="http://editor.vocabs.ands.org.au/user/eMII_Finney.Kim_Admin"/>
	<dcterms:modified rdf:datatype="http://www.w3.org/2001/XMLSchema#dateTime">2017-06-27T03:16:23Z</dcterms:modified>
	<skos:definition xml:lang="en">A habitat where the dominance of a single microbial subclass (Stromatolites, Bacterial Mat, Microphytobenthos) cannot be identified, or where the composition/biomass/surface coverage of the second-most dominant subclass lies within 30 % margin of the most-dominant subclass.</skos:definition>
</rdf:Description>

<rdf:Description rdf:about="http://seamapaustralia.org.au/def/benthichabitatclassification/class/324">
	<rdf:type rdf:resource="http://www.w3.org/2000/01/rdf-schema#Resource"/>
	<rdf:type rdf:resource="http://www.w3.org/2004/02/skos/core#Concept"/>
	<skos:broader rdf:resource="http://seamapaustralia.org.au/def/benthichabitatclassification/class/73"/>
	<skos:prefLabel xml:lang="en">Mixed Invertebrate Community</skos:prefLabel>
	<dcterms:contributor rdf:resource="http://editor.vocabs.ands.org.au/user/eMII_Finney.Kim_Admin"/>
	<dcterms:created rdf:datatype="http://www.w3.org/2001/XMLSchema#dateTime">2017-06-27T01:02:55Z</dcterms:created>
	<dcterms:creator rdf:resource="http://editor.vocabs.ands.org.au/user/eMII_Finney.Kim_Admin"/>
	<dcterms:modified rdf:datatype="http://www.w3.org/2001/XMLSchema#dateTime">2017-06-27T03:16:52Z</dcterms:modified>
	<skos:definition xml:lang="en">A habitat where the dominance of a single Invertebrate subclass (Non-molluscan Filter Feeders, Bioturbators, Shelled Biota) cannot be identified, or where the composition/biomass/surface coverage of the second-most dominant subclass lies within 30 % margin of the most-dominant subclass.</skos:definition>
</rdf:Description>

<rdf:Description rdf:about="http://seamapaustralia.org.au/def/benthichabitatclassification/class/321">
	<rdf:type rdf:resource="http://www.w3.org/2000/01/rdf-schema#Resource"/>
	<rdf:type rdf:resource="http://www.w3.org/2004/02/skos/core#Concept"/>
	<skos:broader rdf:resource="http://seamapaustralia.org.au/def/benthichabitatclassification/class/75"/>
	<skos:prefLabel xml:lang="en">Mixed Wetland Vegetation</skos:prefLabel>
	<dcterms:contributor rdf:resource="http://editor.vocabs.ands.org.au/user/eMII_Finney.Kim_Admin"/>
	<dcterms:created rdf:datatype="http://www.w3.org/2001/XMLSchema#dateTime">2017-06-27T01:00:49Z</dcterms:created>
	<dcterms:creator rdf:resource="http://editor.vocabs.ands.org.au/user/eMII_Finney.Kim_Admin"/>
	<dcterms:modified rdf:datatype="http://www.w3.org/2001/XMLSchema#dateTime">2017-06-27T03:15:23Z</dcterms:modified>
	<skos:definition xml:lang="en">A habitat where the dominance of a single Wetland Vegetation group (Mangroves, Saltmarsh) cannot be identified, or where the composition/biomass/surface coverage of the second-most dominant group lies within 30 % margin of the most-dominant group.</skos:definition>
</rdf:Description>

<rdf:Description rdf:about="http://seamapaustralia.org.au/def/benthichabitatclassification/class/24">
	<rdf:type rdf:resource="http://www.w3.org/2000/01/rdf-schema#Resource"/>
	<rdf:type rdf:resource="http://www.w3.org/2004/02/skos/core#Concept"/>
	<skos:broader rdf:resource="http://seamapaustralia.org.au/def/benthichabitatclassification/class/21"/>
	<skos:prefLabel xml:lang="en">Very Coarse Sand</skos:prefLabel>
	<dcterms:contributor rdf:resource="http://editor.vocabs.ands.org.au/user/eMII_Finney.Kim_Admin"/>
	<dcterms:created rdf:datatype="http://www.w3.org/2001/XMLSchema#dateTime">2016-11-15T22:53:49Z</dcterms:created>
	<dcterms:creator rdf:resource="http://editor.vocabs.ands.org.au/user/eMII_Finney.Kim_Admin"/>
	<dcterms:modified rdf:datatype="http://www.w3.org/2001/XMLSchema#dateTime">2017-06-27T04:21:30Z</dcterms:modified>
	<dc:publisher rdf:datatype="http://www.w3.org/2001/XMLSchema#string">Institute for Marine and Antarctic Studies (IMAS) - UTAS</dc:publisher>
	<skos:definition xml:lang="en">A sand where particles between 1-2 mm in any dimension are dominant (constitute ≥ 60 % of the sand).</skos:definition>
	<dc:source rdf:datatype="http://www.w3.org/2001/XMLSchema#string">SeaMap Australia National Benthic Habitat Classification Scheme (2017)</dc:source>
</rdf:Description>

<rdf:Description rdf:about="http://seamapaustralia.org.au/def/benthichabitatclassification/class/25">
	<rdf:type rdf:resource="http://www.w3.org/2000/01/rdf-schema#Resource"/>
	<rdf:type rdf:resource="http://www.w3.org/2004/02/skos/core#Concept"/>
	<skos:broader rdf:resource="http://seamapaustralia.org.au/def/benthichabitatclassification/class/21"/>
	<skos:prefLabel xml:lang="en">Coarse Sand</skos:prefLabel>
	<dcterms:contributor rdf:resource="http://editor.vocabs.ands.org.au/user/eMII_Finney.Kim_Admin"/>
	<dcterms:created rdf:datatype="http://www.w3.org/2001/XMLSchema#dateTime">2016-11-15T22:54:36Z</dcterms:created>
	<dcterms:creator rdf:resource="http://editor.vocabs.ands.org.au/user/eMII_Finney.Kim_Admin"/>
	<dcterms:modified rdf:datatype="http://www.w3.org/2001/XMLSchema#dateTime">2017-06-27T04:21:16Z</dcterms:modified>
	<dc:publisher rdf:datatype="http://www.w3.org/2001/XMLSchema#string">Institute for Marine and Antarctic Studies (IMAS) - UTAS</dc:publisher>
	<skos:definition xml:lang="en">A sand where particles between 0.5-1 mm in any dimension are dominant (constitute ≥ 80 % of the sand).</skos:definition>
	<dc:source rdf:datatype="http://www.w3.org/2001/XMLSchema#string">SeaMap Australia National Benthic Habitat Classification Scheme (2017)</dc:source>
</rdf:Description>

<rdf:Description rdf:about="http://seamapaustralia.org.au/def/benthichabitatclassification/class/26">
	<rdf:type rdf:resource="http://www.w3.org/2000/01/rdf-schema#Resource"/>
	<rdf:type rdf:resource="http://www.w3.org/2004/02/skos/core#Concept"/>
	<skos:broader rdf:resource="http://seamapaustralia.org.au/def/benthichabitatclassification/class/21"/>
	<skos:prefLabel xml:lang="en">Medium Sand</skos:prefLabel>
	<dcterms:contributor rdf:resource="http://editor.vocabs.ands.org.au/user/eMII_Finney.Kim_Admin"/>
	<dcterms:created rdf:datatype="http://www.w3.org/2001/XMLSchema#dateTime">2016-11-15T22:55:17Z</dcterms:created>
	<dcterms:creator rdf:resource="http://editor.vocabs.ands.org.au/user/eMII_Finney.Kim_Admin"/>
	<dcterms:modified rdf:datatype="http://www.w3.org/2001/XMLSchema#dateTime">2017-06-27T04:21:26Z</dcterms:modified>
	<dc:publisher rdf:datatype="http://www.w3.org/2001/XMLSchema#string">Institute for Marine and Antarctic Studies (IMAS) - UTAS</dc:publisher>
	<skos:definition xml:lang="en">A sand where particles between 0.25-0.5 mm in any dimension are dominant (constitute ≥ 80 % of the sand).</skos:definition>
	<dc:source rdf:datatype="http://www.w3.org/2001/XMLSchema#string">SeaMap Australia National Benthic Habitat Classification Scheme (2017)</dc:source>
</rdf:Description>

<rdf:Description rdf:about="http://seamapaustralia.org.au/def/benthichabitatclassification/class/27">
	<rdf:type rdf:resource="http://www.w3.org/2000/01/rdf-schema#Resource"/>
	<rdf:type rdf:resource="http://www.w3.org/2004/02/skos/core#Concept"/>
	<skos:broader rdf:resource="http://seamapaustralia.org.au/def/benthichabitatclassification/class/21"/>
	<skos:prefLabel xml:lang="en">Fine Sand</skos:prefLabel>
	<dcterms:contributor rdf:resource="http://editor.vocabs.ands.org.au/user/eMII_Finney.Kim_Admin"/>
	<dcterms:created rdf:datatype="http://www.w3.org/2001/XMLSchema#dateTime">2016-11-15T22:55:50Z</dcterms:created>
	<dcterms:creator rdf:resource="http://editor.vocabs.ands.org.au/user/eMII_Finney.Kim_Admin"/>
	<dcterms:modified rdf:datatype="http://www.w3.org/2001/XMLSchema#dateTime">2017-06-27T04:21:21Z</dcterms:modified>
	<dc:publisher rdf:datatype="http://www.w3.org/2001/XMLSchema#string">Institute for Marine and Antarctic Studies (IMAS) - UTAS</dc:publisher>
	<skos:definition xml:lang="en">A sand where particles between 0.125-0.250 mm in any dimension are dominant (constitute ≥ 80 % of the sand).</skos:definition>
	<dc:source rdf:datatype="http://www.w3.org/2001/XMLSchema#string">SeaMap Australia National Benthic Habitat Classification Scheme (2017)</dc:source>
</rdf:Description>

<rdf:Description rdf:about="http://seamapaustralia.org.au/def/benthichabitatclassification/class/28">
	<rdf:type rdf:resource="http://www.w3.org/2000/01/rdf-schema#Resource"/>
	<rdf:type rdf:resource="http://www.w3.org/2004/02/skos/core#Concept"/>
	<skos:broader rdf:resource="http://seamapaustralia.org.au/def/benthichabitatclassification/class/21"/>
	<skos:prefLabel xml:lang="en">Very Fine Sand</skos:prefLabel>
	<dcterms:contributor rdf:resource="http://editor.vocabs.ands.org.au/user/eMII_Finney.Kim_Admin"/>
	<dcterms:created rdf:datatype="http://www.w3.org/2001/XMLSchema#dateTime">2016-11-15T22:56:36Z</dcterms:created>
	<dcterms:creator rdf:resource="http://editor.vocabs.ands.org.au/user/eMII_Finney.Kim_Admin"/>
	<dcterms:modified rdf:datatype="http://www.w3.org/2001/XMLSchema#dateTime">2017-06-27T04:21:35Z</dcterms:modified>
	<dc:publisher rdf:datatype="http://www.w3.org/2001/XMLSchema#string">Institute for Marine and Antarctic Studies (IMAS) - UTAS</dc:publisher>
	<skos:definition xml:lang="en">A sand where particles between 0.0625-0.125 mm in any dimension are dominant (constitute ≥ 80 % of the sand).</skos:definition>
	<dc:source rdf:datatype="http://www.w3.org/2001/XMLSchema#string">SeaMap Australia National Benthic Habitat Classification Scheme (2017)</dc:source>
</rdf:Description>

<rdf:Description rdf:about="http://seamapaustralia.org.au/def/benthichabitatclassification/class/329">
	<rdf:type rdf:resource="http://www.w3.org/2000/01/rdf-schema#Resource"/>
	<rdf:type rdf:resource="http://www.w3.org/2004/02/skos/core#Concept"/>
	<skos:broader rdf:resource="http://seamapaustralia.org.au/def/benthichabitatclassification/class/327"/>
	<skos:prefLabel xml:lang="en">Limestone</skos:prefLabel>
	<dcterms:contributor rdf:resource="http://editor.vocabs.ands.org.au/user/eMII_Finney.Kim_Admin"/>
	<dcterms:created rdf:datatype="http://www.w3.org/2001/XMLSchema#dateTime">2017-06-27T01:32:02Z</dcterms:created>
	<dcterms:creator rdf:resource="http://editor.vocabs.ands.org.au/user/eMII_Finney.Kim_Admin"/>
	<dcterms:modified rdf:datatype="http://www.w3.org/2001/XMLSchema#dateTime">2017-06-27T03:13:22Z</dcterms:modified>
	<skos:definition xml:lang="en">A consolidated hard substratum formed by the accumulation of organic remains, predominantly calcium carbonate (e.g. shells, corals).</skos:definition>
</rdf:Description>

<rdf:Description rdf:about="http://seamapaustralia.org.au/def/benthichabitatclassification/class/30">
	<rdf:type rdf:resource="http://www.w3.org/2000/01/rdf-schema#Resource"/>
	<rdf:type rdf:resource="http://www.w3.org/2004/02/skos/core#Concept"/>
	<skos:broader rdf:resource="http://seamapaustralia.org.au/def/benthichabitatclassification/class/22"/>
	<skos:prefLabel xml:lang="en">Coarse Silt</skos:prefLabel>
	<dcterms:contributor rdf:resource="http://editor.vocabs.ands.org.au/user/eMII_Finney.Kim_Admin"/>
	<dcterms:created rdf:datatype="http://www.w3.org/2001/XMLSchema#dateTime">2016-11-15T23:04:36Z</dcterms:created>
	<dcterms:creator rdf:resource="http://editor.vocabs.ands.org.au/user/eMII_Finney.Kim_Admin"/>
	<dcterms:modified rdf:datatype="http://www.w3.org/2001/XMLSchema#dateTime">2017-06-27T04:22:08Z</dcterms:modified>
	<dc:publisher rdf:datatype="http://www.w3.org/2001/XMLSchema#string">Institute for Marine and Antarctic Studies (IMAS) - UTAS</dc:publisher>
	<skos:definition xml:lang="en">A silt where particles between 0.0310-0.0625 mm in any dimension are dominant (i.e. constitute ≥ 80% of the silt).</skos:definition>
	<dc:source rdf:datatype="http://www.w3.org/2001/XMLSchema#string">SeaMap Australia National Benthic Habitat Classification Scheme (2017)</dc:source>
</rdf:Description>

<rdf:Description rdf:about="http://seamapaustralia.org.au/def/benthichabitatclassification/class/31">
	<rdf:type rdf:resource="http://www.w3.org/2000/01/rdf-schema#Resource"/>
	<rdf:type rdf:resource="http://www.w3.org/2004/02/skos/core#Concept"/>
	<skos:broader rdf:resource="http://seamapaustralia.org.au/def/benthichabitatclassification/class/22"/>
	<skos:prefLabel xml:lang="en">Medium Silt</skos:prefLabel>
	<dcterms:contributor rdf:resource="http://editor.vocabs.ands.org.au/user/eMII_Finney.Kim_Admin"/>
	<dcterms:created rdf:datatype="http://www.w3.org/2001/XMLSchema#dateTime">2016-11-15T23:05:04Z</dcterms:created>
	<dcterms:creator rdf:resource="http://editor.vocabs.ands.org.au/user/eMII_Finney.Kim_Admin"/>
	<dcterms:modified rdf:datatype="http://www.w3.org/2001/XMLSchema#dateTime">2017-06-27T04:22:18Z</dcterms:modified>
	<dc:publisher rdf:datatype="http://www.w3.org/2001/XMLSchema#string">Institute for Marine and Antarctic Studies (IMAS) - UTAS</dc:publisher>
	<skos:definition xml:lang="en">A silt where particles between 0.0156-0.0310 mm in any dimension are dominant (i.e. constitute ≥ 80% of the silt).</skos:definition>
	<dc:source rdf:datatype="http://www.w3.org/2001/XMLSchema#string">SeaMap Australia National Benthic Habitat Classification Scheme (2017)</dc:source>
</rdf:Description>

<rdf:Description rdf:about="http://seamapaustralia.org.au/def/benthichabitatclassification/class/32">
	<rdf:type rdf:resource="http://www.w3.org/2000/01/rdf-schema#Resource"/>
	<rdf:type rdf:resource="http://www.w3.org/2004/02/skos/core#Concept"/>
	<skos:broader rdf:resource="http://seamapaustralia.org.au/def/benthichabitatclassification/class/22"/>
	<skos:prefLabel xml:lang="en">Fine Silt</skos:prefLabel>
	<dcterms:contributor rdf:resource="http://editor.vocabs.ands.org.au/user/eMII_Finney.Kim_Admin"/>
	<dcterms:created rdf:datatype="http://www.w3.org/2001/XMLSchema#dateTime">2016-11-15T23:05:40Z</dcterms:created>
	<dcterms:creator rdf:resource="http://editor.vocabs.ands.org.au/user/eMII_Finney.Kim_Admin"/>
	<dcterms:modified rdf:datatype="http://www.w3.org/2001/XMLSchema#dateTime">2017-06-27T04:22:13Z</dcterms:modified>
	<dc:publisher rdf:datatype="http://www.w3.org/2001/XMLSchema#string">Institute for Marine and Antarctic Studies (IMAS) - UTAS</dc:publisher>
	<skos:definition xml:lang="en">A silt where particles between 0.0078-0.0156 mm in any dimension are dominant (i.e. constitute ≥ 80% of the silt).</skos:definition>
	<dc:source rdf:datatype="http://www.w3.org/2001/XMLSchema#string">SeaMap Australia National Benthic Habitat Classification Scheme (2017)</dc:source>
</rdf:Description>

<rdf:Description rdf:about="http://seamapaustralia.org.au/def/benthichabitatclassification/class/33">
	<rdf:type rdf:resource="http://www.w3.org/2000/01/rdf-schema#Resource"/>
	<rdf:type rdf:resource="http://www.w3.org/2004/02/skos/core#Concept"/>
	<skos:broader rdf:resource="http://seamapaustralia.org.au/def/benthichabitatclassification/class/22"/>
	<skos:prefLabel xml:lang="en">Very Fine Silt</skos:prefLabel>
	<dcterms:contributor rdf:resource="http://editor.vocabs.ands.org.au/user/eMII_Finney.Kim_Admin"/>
	<dcterms:created rdf:datatype="http://www.w3.org/2001/XMLSchema#dateTime">2016-11-15T23:06:18Z</dcterms:created>
	<dcterms:creator rdf:resource="http://editor.vocabs.ands.org.au/user/eMII_Finney.Kim_Admin"/>
	<dcterms:modified rdf:datatype="http://www.w3.org/2001/XMLSchema#dateTime">2017-06-27T04:22:23Z</dcterms:modified>
	<dc:publisher rdf:datatype="http://www.w3.org/2001/XMLSchema#string">Institute for Marine and Antarctic Studies (IMAS) - UTAS</dc:publisher>
	<skos:definition xml:lang="en">A silt where particles between 0.0039-0.0078 mm in any dimension are dominant (i.e. constitute ≥ 80% of the silt).</skos:definition>
	<dc:source rdf:datatype="http://www.w3.org/2001/XMLSchema#string">SeaMap Australia National Benthic Habitat Classification Scheme (2017)</dc:source>
</rdf:Description>

<rdf:Description rdf:about="http://seamapaustralia.org.au/def/benthichabitatclassification/class/320">
	<rdf:type rdf:resource="http://www.w3.org/2000/01/rdf-schema#Resource"/>
	<rdf:type rdf:resource="http://www.w3.org/2004/02/skos/core#Concept"/>
	<skos:broader rdf:resource="http://seamapaustralia.org.au/def/benthichabitatclassification/class/72"/>
	<skos:prefLabel xml:lang="en">Mixed Vegetation</skos:prefLabel>
	<dcterms:contributor rdf:resource="http://editor.vocabs.ands.org.au/user/eMII_Finney.Kim_Admin"/>
	<dcterms:created rdf:datatype="http://www.w3.org/2001/XMLSchema#dateTime">2017-06-27T01:00:00Z</dcterms:created>
	<dcterms:creator rdf:resource="http://editor.vocabs.ands.org.au/user/eMII_Finney.Kim_Admin"/>
	<dcterms:modified rdf:datatype="http://www.w3.org/2001/XMLSchema#dateTime">2017-06-27T03:14:52Z</dcterms:modified>
	<skos:definition xml:lang="en">A habitat where the dominance of a single Vegetation subclass (Wetland Vegetation, Macrophytes) cannot be identified, or where the composition/biomass/surface coverage of the second-most dominant subclass lies within 30 % margin of the most-dominant subclass.</skos:definition>
</rdf:Description>

<rdf:Description rdf:about="http://www.w3.org/2004/02/skos/core#closeMatch">
	<rdf:type rdf:resource="http://www.w3.org/1999/02/22-rdf-syntax-ns#Property"/>
	<rdf:type rdf:resource="http://www.w3.org/2000/01/rdf-schema#Resource"/>
	<rdfs:subPropertyOf rdf:resource="http://www.w3.org/2004/02/skos/core#closeMatch"/>
</rdf:Description>

<rdf:Description rdf:about="https://www.cmecscatalog.org/cmecs/classification/dComponent/3.html">
	<rdf:type rdf:resource="http://www.w3.org/2000/01/rdf-schema#Resource"/>
</rdf:Description>

<rdf:Description rdf:about="http://seamapaustralia.org.au/def/benthichabitatclassification/class/343">
	<rdf:type rdf:resource="http://www.w3.org/2000/01/rdf-schema#Resource"/>
	<rdf:type rdf:resource="http://www.w3.org/2004/02/skos/core#Concept"/>
	<skos:broader rdf:resource="http://seamapaustralia.org.au/def/benthichabitatclassification/class/337"/>
	<skos:prefLabel xml:lang="en">IMCRA Pompey-Swains Bioregion</skos:prefLabel>
	<dcterms:contributor rdf:resource="http://editor.vocabs.ands.org.au/user/eMII_Finney.Kim_Admin"/>
	<dcterms:created rdf:datatype="http://www.w3.org/2001/XMLSchema#dateTime">2017-06-27T03:31:46Z</dcterms:created>
	<dcterms:creator rdf:resource="http://editor.vocabs.ands.org.au/user/eMII_Finney.Kim_Admin"/>
	<dcterms:modified rdf:datatype="http://www.w3.org/2001/XMLSchema#dateTime">2017-06-27T03:58:45Z</dcterms:modified>
	<dc:publisher rdf:datatype="http://www.w3.org/2001/XMLSchema#string">Institute for Marine and Antarctic Studies (IMAS) - UTAS</dc:publisher>
	<skos:definition xml:lang="en">An inshore regionalisation of Australian waters derived from biological and physical data, including the distribution of demersal fishes, marine plants and invertebrates, sea floor geomorphology and sediments, and oceanographic data. The meso-scale regionalisation was compiled from information supplied to the Australian Government Department of the Environment and Heritage by the relevant State, Northern Territory and Commonwealth marine research and management agencies. The seaward extent for the meso-scale IMCRA coverage is defined by the 200m isobath except where this boundary extends beyond the Australian Exclusive Economic Zone (AEEZ).</skos:definition>
	<dc:source rdf:datatype="http://www.w3.org/2001/XMLSchema#string">Commonwealth of Australia (2006). A Guide to the Integrated Marine and Coastal Regionalisation of Australia Version 4.0. Department of the Environment and Heritage, Canberra, Australia.</dc:source>
	<skos:exactMatch rdf:resource="http://www.environment.gov.au/mapping/rest/services/ogc_services/IMCRA_Mesoscale/MapServer/0/27"/>
</rdf:Description>

<rdf:Description rdf:about="http://seamapaustralia.org.au/def/benthichabitatclassification/class/4">
	<rdf:type rdf:resource="http://www.w3.org/2000/01/rdf-schema#Resource"/>
	<rdf:type rdf:resource="http://www.w3.org/2004/02/skos/core#Concept"/>
	<skos:broader rdf:resource="http://seamapaustralia.org.au/def/benthichabitatclassification/class/3"/>
	<skos:prefLabel xml:lang="en">Substratum Not Assessed (NA)</skos:prefLabel>
	<dcterms:contributor rdf:resource="http://editor.vocabs.ands.org.au/user/eMII_Finney.Kim_Admin"/>
	<dcterms:created rdf:datatype="http://www.w3.org/2001/XMLSchema#dateTime">2016-11-15T04:40:42Z</dcterms:created>
	<dcterms:creator rdf:resource="http://editor.vocabs.ands.org.au/user/eMII_Finney.Kim_Admin"/>
	<dcterms:modified rdf:datatype="http://www.w3.org/2001/XMLSchema#dateTime">2017-06-27T04:22:34Z</dcterms:modified>
	<dc:publisher rdf:datatype="http://www.w3.org/2001/XMLSchema#string">Institute for Marine and Antarctic Studies (IMAS) - UTAS</dc:publisher>
	<skos:definition xml:lang="en">An area where mapping has occurred, but where substratum characteristics were not assessed. An NA classification is distinct from an Unknown classification in that an Unknown implies an assessment was made however a classification was not possible (e.g. due to inadequate resolution, or poor quality data).</skos:definition>
	<dc:source rdf:datatype="http://www.w3.org/2001/XMLSchema#string">SeaMap Australia National Benthic Habitat Classification Scheme (2017)</dc:source>
</rdf:Description>

<rdf:Description rdf:about="http://seamapaustralia.org.au/def/benthichabitatclassification/class/7">
	<rdf:type rdf:resource="http://www.w3.org/2000/01/rdf-schema#Resource"/>
	<rdf:type rdf:resource="http://www.w3.org/2004/02/skos/core#Concept"/>
	<skos:broader rdf:resource="http://seamapaustralia.org.au/def/benthichabitatclassification/class/3"/>
	<skos:prefLabel xml:lang="en">Mixed Hard/Soft Substrata</skos:prefLabel>
	<dcterms:contributor rdf:resource="http://editor.vocabs.ands.org.au/user/eMII_Finney.Kim_Admin"/>
	<dcterms:created rdf:datatype="http://www.w3.org/2001/XMLSchema#dateTime">2016-11-15T04:44:09Z</dcterms:created>
	<dcterms:creator rdf:resource="http://editor.vocabs.ands.org.au/user/eMII_Finney.Kim_Admin"/>
	<dcterms:modified rdf:datatype="http://www.w3.org/2001/XMLSchema#dateTime">2017-06-27T04:20:06Z</dcterms:modified>
	<dc:publisher rdf:datatype="http://www.w3.org/2001/XMLSchema#string">Institute for Marine and Antarctic Studies (IMAS) - UTAS</dc:publisher>
	<skos:definition xml:lang="en">A hard substratum composed of a mix of Consolidated Hard Substrata and Unconsolidated Hard Substrata where neither class is dominant (i.e. does not exceed ≥ 80 %) of the substratum surface/composition.</skos:definition>
	<dc:source rdf:datatype="http://www.w3.org/2001/XMLSchema#string">SeaMap Australia National Benthic Habitat Classification Scheme (2017)</dc:source>
</rdf:Description>

<rdf:Description rdf:about="http://www.w3.org/2004/02/skos/core#topConceptOf">
	<rdf:type rdf:resource="http://www.w3.org/1999/02/22-rdf-syntax-ns#Property"/>
	<rdf:type rdf:resource="http://www.w3.org/2000/01/rdf-schema#Resource"/>
	<rdfs:subPropertyOf rdf:resource="http://www.w3.org/2004/02/skos/core#topConceptOf"/>
</rdf:Description>

<rdf:Description rdf:about="http://seamapaustralia.org.au/def/benthichabitatclassification/class/336">
	<rdf:type rdf:resource="http://www.w3.org/2000/01/rdf-schema#Resource"/>
	<rdf:type rdf:resource="http://www.w3.org/2004/02/skos/core#Concept"/>
	<skos:broader rdf:resource="http://seamapaustralia.org.au/def/benthichabitatclassification/class/331"/>
	<skos:prefLabel xml:lang="en">Other Shell</skos:prefLabel>
	<dcterms:contributor rdf:resource="http://editor.vocabs.ands.org.au/user/eMII_Finney.Kim_Admin"/>
	<dcterms:created rdf:datatype="http://www.w3.org/2001/XMLSchema#dateTime">2017-06-27T01:48:30Z</dcterms:created>
	<dcterms:creator rdf:resource="http://editor.vocabs.ands.org.au/user/eMII_Finney.Kim_Admin"/>
	<dcterms:modified rdf:datatype="http://www.w3.org/2001/XMLSchema#dateTime">2017-06-27T01:53:19Z</dcterms:modified>
	<skos:definition xml:lang="en">Biogenic substrata dominated by other shells.</skos:definition>
</rdf:Description>

<rdf:Description rdf:about="http://seamapaustralia.org.au/def/benthichabitatclassification/class/331">
	<rdf:type rdf:resource="http://www.w3.org/2000/01/rdf-schema#Resource"/>
	<rdf:type rdf:resource="http://www.w3.org/2004/02/skos/core#Concept"/>
	<skos:broader rdf:resource="http://seamapaustralia.org.au/def/benthichabitatclassification/class/327"/>
	<skos:prefLabel xml:lang="en">Shell</skos:prefLabel>
	<dcterms:contributor rdf:resource="http://editor.vocabs.ands.org.au/user/eMII_Finney.Kim_Admin"/>
	<dcterms:created rdf:datatype="http://www.w3.org/2001/XMLSchema#dateTime">2017-06-27T01:46:14Z</dcterms:created>
	<dcterms:creator rdf:resource="http://editor.vocabs.ands.org.au/user/eMII_Finney.Kim_Admin"/>
	<dcterms:modified rdf:datatype="http://www.w3.org/2001/XMLSchema#dateTime">2017-06-27T01:51:42Z</dcterms:modified>
	<skos:definition xml:lang="en">Biogenic substrata that is constructed from cemented/self-adhered non-living shells and shell fragments. These are typically (but not exclusively) molluscs. Living shells fauna may be present but these are described under the Biota Component.</skos:definition>
	<skos:narrower rdf:resource="http://seamapaustralia.org.au/def/benthichabitatclassification/class/332"/>
	<skos:narrower rdf:resource="http://seamapaustralia.org.au/def/benthichabitatclassification/class/336"/>
	<skos:narrower rdf:resource="http://seamapaustralia.org.au/def/benthichabitatclassification/class/335"/>
	<skos:narrower rdf:resource="http://seamapaustralia.org.au/def/benthichabitatclassification/class/334"/>
	<skos:narrower rdf:resource="http://seamapaustralia.org.au/def/benthichabitatclassification/class/333"/>
</rdf:Description>

<rdf:Description rdf:about="http://seamapaustralia.org.au/def/benthichabitatclassification/class/35">
	<rdf:type rdf:resource="http://www.w3.org/2000/01/rdf-schema#Resource"/>
	<rdf:type rdf:resource="http://www.w3.org/2004/02/skos/core#Concept"/>
	<skos:broader rdf:resource="http://seamapaustralia.org.au/def/benthichabitatclassification/class/34"/>
	<skos:prefLabel xml:lang="en">Biogenic Origin</skos:prefLabel>
	<dcterms:contributor rdf:resource="http://editor.vocabs.ands.org.au/user/eMII_Finney.Kim_Admin"/>
	<dcterms:created rdf:datatype="http://www.w3.org/2001/XMLSchema#dateTime">2016-11-16T00:41:34Z</dcterms:created>
	<dcterms:creator rdf:resource="http://editor.vocabs.ands.org.au/user/eMII_Finney.Kim_Admin"/>
	<dcterms:modified rdf:datatype="http://www.w3.org/2001/XMLSchema#dateTime">2017-06-27T04:25:19Z</dcterms:modified>
	<dc:publisher rdf:datatype="http://www.w3.org/2001/XMLSchema#string">Institute for Marine and Antarctic Studies (IMAS) - UTAS</dc:publisher>
	<dc:source rdf:datatype="http://www.w3.org/2001/XMLSchema#string">SeaMap Australia National Benthic Habitat Classification Scheme (2017)</dc:source>
	<skos:narrower rdf:resource="http://seamapaustralia.org.au/def/benthichabitatclassification/class/327"/>
	<skos:narrower rdf:resource="http://seamapaustralia.org.au/def/benthichabitatclassification/class/38"/>
	<skos:narrower rdf:resource="http://seamapaustralia.org.au/def/benthichabitatclassification/class/39"/>
	<skos:narrower rdf:resource="http://seamapaustralia.org.au/def/benthichabitatclassification/class/42"/>
	<skos:narrower rdf:resource="http://seamapaustralia.org.au/def/benthichabitatclassification/class/43"/>
</rdf:Description>

<rdf:Description rdf:about="http://seamapaustralia.org.au/def/benthichabitatclassification/class/36">
	<rdf:type rdf:resource="http://www.w3.org/2000/01/rdf-schema#Resource"/>
	<rdf:type rdf:resource="http://www.w3.org/2004/02/skos/core#Concept"/>
	<skos:broader rdf:resource="http://seamapaustralia.org.au/def/benthichabitatclassification/class/34"/>
	<skos:prefLabel xml:lang="en">Geologic Origin</skos:prefLabel>
	<dcterms:contributor rdf:resource="http://editor.vocabs.ands.org.au/user/eMII_Finney.Kim_Admin"/>
	<dcterms:created rdf:datatype="http://www.w3.org/2001/XMLSchema#dateTime">2016-11-16T00:42:11Z</dcterms:created>
	<dcterms:creator rdf:resource="http://editor.vocabs.ands.org.au/user/eMII_Finney.Kim_Admin"/>
	<dcterms:modified rdf:datatype="http://www.w3.org/2001/XMLSchema#dateTime">2017-06-27T04:27:17Z</dcterms:modified>
	<dc:publisher rdf:datatype="http://www.w3.org/2001/XMLSchema#string">Institute for Marine and Antarctic Studies (IMAS) - UTAS</dc:publisher>
	<skos:definition xml:lang="en">Where the substratum is composed of a greater percentage of geologic materials than either biogenic or anthropogenic. Geologic substrata can be igneous, metamorphic or sedimentary particles of any grain size class. </skos:definition>
	<dc:source rdf:datatype="http://www.w3.org/2001/XMLSchema#string">SeaMap Australia National Benthic Habitat Classification Scheme (2017)</dc:source>
	<skos:narrower rdf:resource="http://seamapaustralia.org.au/def/benthichabitatclassification/class/44"/>
	<skos:narrower rdf:resource="http://seamapaustralia.org.au/def/benthichabitatclassification/class/45"/>
	<skos:narrower rdf:resource="http://seamapaustralia.org.au/def/benthichabitatclassification/class/46"/>
</rdf:Description>

<rdf:Description rdf:about="http://seamapaustralia.org.au/def/benthichabitatclassification/class/37">
	<rdf:type rdf:resource="http://www.w3.org/2000/01/rdf-schema#Resource"/>
	<rdf:type rdf:resource="http://www.w3.org/2004/02/skos/core#Concept"/>
	<skos:broader rdf:resource="http://seamapaustralia.org.au/def/benthichabitatclassification/class/34"/>
	<skos:prefLabel xml:lang="en">Anthropogenic Origin</skos:prefLabel>
	<dcterms:contributor rdf:resource="http://editor.vocabs.ands.org.au/user/eMII_Finney.Kim_Admin"/>
	<dcterms:created rdf:datatype="http://www.w3.org/2001/XMLSchema#dateTime">2016-11-16T00:42:46Z</dcterms:created>
	<dcterms:creator rdf:resource="http://editor.vocabs.ands.org.au/user/eMII_Finney.Kim_Admin"/>
	<dcterms:modified rdf:datatype="http://www.w3.org/2001/XMLSchema#dateTime">2017-06-27T04:24:47Z</dcterms:modified>
	<dc:publisher rdf:datatype="http://www.w3.org/2001/XMLSchema#string">Institute for Marine and Antarctic Studies (IMAS) - UTAS</dc:publisher>
	<skos:definition xml:lang="en">Substratum that has a greater percentage cover, weight or composition of anthropogenic material than of either geologic or biogenic material. Anthropogenic material can be anything that is man-made, or which has been intentionally or accidentally placed by humans. </skos:definition>
	<dc:source rdf:datatype="http://www.w3.org/2001/XMLSchema#string">SeaMap Australia National Benthic Habitat Classification Scheme (2017)</dc:source>
	<skos:narrower rdf:resource="http://seamapaustralia.org.au/def/benthichabitatclassification/class/47"/>
	<skos:narrower rdf:resource="http://seamapaustralia.org.au/def/benthichabitatclassification/class/48"/>
	<skos:narrower rdf:resource="http://seamapaustralia.org.au/def/benthichabitatclassification/class/49"/>
	<skos:narrower rdf:resource="http://seamapaustralia.org.au/def/benthichabitatclassification/class/50"/>
	<skos:narrower rdf:resource="http://seamapaustralia.org.au/def/benthichabitatclassification/class/154"/>
	<skos:closeMatch rdf:resource="https://www.cmecscatalog.org/cmecs/classification/unit/217.html"/>
</rdf:Description>

<rdf:Description rdf:about="http://seamapaustralia.org.au/def/benthichabitatclassification/class/335">
	<rdf:type rdf:resource="http://www.w3.org/2000/01/rdf-schema#Resource"/>
	<rdf:type rdf:resource="http://www.w3.org/2004/02/skos/core#Concept"/>
	<skos:broader rdf:resource="http://seamapaustralia.org.au/def/benthichabitatclassification/class/331"/>
	<skos:prefLabel xml:lang="en">Clam Shell</skos:prefLabel>
	<dcterms:contributor rdf:resource="http://editor.vocabs.ands.org.au/user/eMII_Finney.Kim_Admin"/>
	<dcterms:created rdf:datatype="http://www.w3.org/2001/XMLSchema#dateTime">2017-06-27T01:48:16Z</dcterms:created>
	<dcterms:creator rdf:resource="http://editor.vocabs.ands.org.au/user/eMII_Finney.Kim_Admin"/>
	<dcterms:modified rdf:datatype="http://www.w3.org/2001/XMLSchema#dateTime">2017-06-27T01:52:17Z</dcterms:modified>
	<skos:definition xml:lang="en">Biogenic substrata dominated by clams.</skos:definition>
</rdf:Description>

<rdf:Description rdf:about="http://seamapaustralia.org.au/def/benthichabitatclassification/class/327">
	<rdf:type rdf:resource="http://www.w3.org/2000/01/rdf-schema#Resource"/>
	<rdf:type rdf:resource="http://www.w3.org/2004/02/skos/core#Concept"/>
	<skos:broader rdf:resource="http://seamapaustralia.org.au/def/benthichabitatclassification/class/35"/>
	<skos:prefLabel xml:lang="en">Carbonate</skos:prefLabel>
	<dcterms:contributor rdf:resource="http://editor.vocabs.ands.org.au/user/eMII_Finney.Kim_Admin"/>
	<dcterms:created rdf:datatype="http://www.w3.org/2001/XMLSchema#dateTime">2017-06-27T01:08:54Z</dcterms:created>
	<dcterms:creator rdf:resource="http://editor.vocabs.ands.org.au/user/eMII_Finney.Kim_Admin"/>
	<dcterms:modified rdf:datatype="http://www.w3.org/2001/XMLSchema#dateTime">2017-06-27T01:44:22Z</dcterms:modified>
	<skos:narrower rdf:resource="http://seamapaustralia.org.au/def/benthichabitatclassification/class/329"/>
	<skos:narrower rdf:resource="http://seamapaustralia.org.au/def/benthichabitatclassification/class/331"/>
	<skos:narrower rdf:resource="http://seamapaustralia.org.au/def/benthichabitatclassification/class/328"/>
</rdf:Description>

<rdf:Description rdf:about="http://seamapaustralia.org.au/def/benthichabitatclassification/class/38">
	<rdf:type rdf:resource="http://www.w3.org/2000/01/rdf-schema#Resource"/>
	<rdf:type rdf:resource="http://www.w3.org/2004/02/skos/core#Concept"/>
	<skos:broader rdf:resource="http://seamapaustralia.org.au/def/benthichabitatclassification/class/35"/>
	<skos:prefLabel xml:lang="en">Worm</skos:prefLabel>
	<dcterms:contributor rdf:resource="http://editor.vocabs.ands.org.au/user/eMII_Finney.Kim_Admin"/>
	<dcterms:created rdf:datatype="http://www.w3.org/2001/XMLSchema#dateTime">2016-11-16T00:43:31Z</dcterms:created>
	<dcterms:creator rdf:resource="http://editor.vocabs.ands.org.au/user/eMII_Finney.Kim_Admin"/>
	<dcterms:modified rdf:datatype="http://www.w3.org/2001/XMLSchema#dateTime">2017-06-27T04:27:00Z</dcterms:modified>
	<dc:publisher rdf:datatype="http://www.w3.org/2001/XMLSchema#string">Institute for Marine and Antarctic Studies (IMAS) - UTAS</dc:publisher>
	<skos:definition xml:lang="en">Biogenic substrata that are dominated by partially or fully cemented calcareous or muddy/sandy tubes of polychaetes or other worm-like fauna.</skos:definition>
	<dc:source rdf:datatype="http://www.w3.org/2001/XMLSchema#string">  SeaMap Australia National Benthic Habitat Classification Scheme (2017)</dc:source>
	<skos:narrower rdf:resource="http://seamapaustralia.org.au/def/benthichabitatclassification/class/53"/>
	<skos:narrower rdf:resource="http://seamapaustralia.org.au/def/benthichabitatclassification/class/54"/>
</rdf:Description>

<rdf:Description rdf:about="http://seamapaustralia.org.au/def/benthichabitatclassification/class/39">
	<rdf:type rdf:resource="http://www.w3.org/2000/01/rdf-schema#Resource"/>
	<rdf:type rdf:resource="http://www.w3.org/2004/02/skos/core#Concept"/>
	<skos:broader rdf:resource="http://seamapaustralia.org.au/def/benthichabitatclassification/class/35"/>
	<skos:prefLabel xml:lang="en">Algae</skos:prefLabel>
	<dcterms:contributor rdf:resource="http://editor.vocabs.ands.org.au/user/eMII_Finney.Kim_Admin"/>
	<dcterms:created rdf:datatype="http://www.w3.org/2001/XMLSchema#dateTime">2016-11-16T00:44:01Z</dcterms:created>
	<dcterms:creator rdf:resource="http://editor.vocabs.ands.org.au/user/eMII_Finney.Kim_Admin"/>
	<dcterms:modified rdf:datatype="http://www.w3.org/2001/XMLSchema#dateTime">2017-06-27T04:25:24Z</dcterms:modified>
	<dc:publisher rdf:datatype="http://www.w3.org/2001/XMLSchema#string">Institute for Marine and Antarctic Studies (IMAS) - UTAS</dc:publisher>
	<skos:definition xml:lang="en">A biogenic substratum that is dominated by non-living crustose and calcareous algae. Living algae may be present, but these are described under the Biotic Component.</skos:definition>
	<dc:source rdf:datatype="http://www.w3.org/2001/XMLSchema#string">  SeaMap Australia National Benthic Habitat Classification Scheme (2017)</dc:source>
	<skos:narrower rdf:resource="http://seamapaustralia.org.au/def/benthichabitatclassification/class/55"/>
	<skos:narrower rdf:resource="http://seamapaustralia.org.au/def/benthichabitatclassification/class/56"/>
</rdf:Description>

<rdf:Description rdf:about="http://seamapaustralia.org.au/def/benthichabitatclassification/class/303">
	<rdf:type rdf:resource="http://www.w3.org/2000/01/rdf-schema#Resource"/>
	<rdf:type rdf:resource="http://www.w3.org/2004/02/skos/core#Concept"/>
	<skos:broader rdf:resource="http://seamapaustralia.org.au/def/benthichabitatclassification/class/298"/>
	<skos:prefLabel xml:lang="en">IMCRA Groote Bioregion</skos:prefLabel>
	<dcterms:contributor rdf:resource="http://editor.vocabs.ands.org.au/user/eMII_Finney.Kim_Admin"/>
	<dcterms:created rdf:datatype="http://www.w3.org/2001/XMLSchema#dateTime">2017-06-14T05:27:22Z</dcterms:created>
	<dcterms:creator rdf:resource="http://editor.vocabs.ands.org.au/user/eMII_Finney.Kim_Admin"/>
	<dcterms:modified rdf:datatype="http://www.w3.org/2001/XMLSchema#dateTime">2017-06-26T23:27:45Z</dcterms:modified>
	<dc:publisher rdf:datatype="http://www.w3.org/2001/XMLSchema#string">Institute for Marine and Antarctic Studies (IMAS) - UTAS</dc:publisher>
	<skos:definition xml:lang="en">An inshore regionalisation of Australian waters derived from biological and physical data, including the distribution of demersal fishes, marine plants and invertebrates, sea floor geomorphology and sediments, and oceanographic data. The meso-scale regionalisation was compiled from information supplied to the Australian Government Department of the Environment and Heritage by the relevant State, Northern Territory and Commonwealth marine research and management agencies. The seaward extent for the meso-scale IMCRA coverage is defined by the 200m isobath except where this boundary extends beyond the Australian Exclusive Economic Zone (AEEZ).</skos:definition>
	<dc:source rdf:datatype="http://www.w3.org/2001/XMLSchema#string">Commonwealth of Australia (2006). A Guide to the Integrated Marine and Coastal Regionalisation of Australia Version 4.0. Department of the Environment and Heritage, Canberra, Australia.</dc:source>
	<skos:exactMatch rdf:resource="http://www.environment.gov.au/mapping/rest/services/ogc_services/IMCRA_Mesoscale/MapServer/0/14"/>
</rdf:Description>

<rdf:Description rdf:about="http://seamapaustralia.org.au/def/benthichabitatclassification/class/307">
	<rdf:type rdf:resource="http://www.w3.org/2000/01/rdf-schema#Resource"/>
	<rdf:type rdf:resource="http://www.w3.org/2004/02/skos/core#Concept"/>
	<skos:broader rdf:resource="http://seamapaustralia.org.au/def/benthichabitatclassification/class/298"/>
	<skos:prefLabel xml:lang="en">IMCRA Carpentaria Bioregion</skos:prefLabel>
	<dcterms:contributor rdf:resource="http://editor.vocabs.ands.org.au/user/eMII_Finney.Kim_Admin"/>
	<dcterms:created rdf:datatype="http://www.w3.org/2001/XMLSchema#dateTime">2017-06-14T05:28:37Z</dcterms:created>
	<dcterms:creator rdf:resource="http://editor.vocabs.ands.org.au/user/eMII_Finney.Kim_Admin"/>
	<dcterms:modified rdf:datatype="http://www.w3.org/2001/XMLSchema#dateTime">2017-06-26T23:26:15Z</dcterms:modified>
	<dc:publisher rdf:datatype="http://www.w3.org/2001/XMLSchema#string">Institute for Marine and Antarctic Studies (IMAS) - UTAS</dc:publisher>
	<skos:definition xml:lang="en">An inshore regionalisation of Australian waters derived from biological and physical data, including the distribution of demersal fishes, marine plants and invertebrates, sea floor geomorphology and sediments, and oceanographic data. The meso-scale regionalisation was compiled from information supplied to the Australian Government Department of the Environment and Heritage by the relevant State, Northern Territory and Commonwealth marine research and management agencies. The seaward extent for the meso-scale IMCRA coverage is defined by the 200m isobath except where this boundary extends beyond the Australian Exclusive Economic Zone (AEEZ).</skos:definition>
	<dc:source rdf:datatype="http://www.w3.org/2001/XMLSchema#string">Commonwealth of Australia (2006). A Guide to the Integrated Marine and Coastal Regionalisation of Australia Version 4.0. Department of the Environment and Heritage, Canberra, Australia.</dc:source>
	<skos:exactMatch rdf:resource="http://www.environment.gov.au/mapping/rest/services/ogc_services/IMCRA_Mesoscale/MapServer/0/7"/>
</rdf:Description>

<rdf:Description rdf:about="http://seamapaustralia.org.au/def/benthichabitatclassification/class/42">
	<rdf:type rdf:resource="http://www.w3.org/2000/01/rdf-schema#Resource"/>
	<rdf:type rdf:resource="http://www.w3.org/2004/02/skos/core#Concept"/>
	<skos:broader rdf:resource="http://seamapaustralia.org.au/def/benthichabitatclassification/class/35"/>
	<skos:prefLabel xml:lang="en">Terrigenous</skos:prefLabel>
	<dcterms:contributor rdf:resource="http://editor.vocabs.ands.org.au/user/eMII_Finney.Kim_Admin"/>
	<dcterms:created rdf:datatype="http://www.w3.org/2001/XMLSchema#dateTime">2016-11-16T00:45:49Z</dcterms:created>
	<dcterms:creator rdf:resource="http://editor.vocabs.ands.org.au/user/eMII_Finney.Kim_Admin"/>
	<dcterms:modified rdf:datatype="http://www.w3.org/2001/XMLSchema#dateTime">2017-06-27T04:26:53Z</dcterms:modified>
	<dc:publisher rdf:datatype="http://www.w3.org/2001/XMLSchema#string">Institute for Marine and Antarctic Studies (IMAS) - UTAS</dc:publisher>
	<skos:definition xml:lang="en">A biogenic substratum that is composed of sediments from a terrigenous origin, e.g. soils and other organic materials eroded from the land.</skos:definition>
	<dc:source rdf:datatype="http://www.w3.org/2001/XMLSchema#string">  SeaMap Australia National Benthic Habitat Classification Scheme (2017)</dc:source>
</rdf:Description>

<rdf:Description rdf:about="http://seamapaustralia.org.au/def/benthichabitatclassification/class/43">
	<rdf:type rdf:resource="http://www.w3.org/2000/01/rdf-schema#Resource"/>
	<rdf:type rdf:resource="http://www.w3.org/2004/02/skos/core#Concept"/>
	<skos:broader rdf:resource="http://seamapaustralia.org.au/def/benthichabitatclassification/class/35"/>
	<skos:prefLabel xml:lang="en">Ooze</skos:prefLabel>
	<dcterms:contributor rdf:resource="http://editor.vocabs.ands.org.au/user/eMII_Finney.Kim_Admin"/>
	<dcterms:created rdf:datatype="http://www.w3.org/2001/XMLSchema#dateTime">2016-11-16T00:46:22Z</dcterms:created>
	<dcterms:creator rdf:resource="http://editor.vocabs.ands.org.au/user/eMII_Finney.Kim_Admin"/>
	<dcterms:modified rdf:datatype="http://www.w3.org/2001/XMLSchema#dateTime">2017-06-27T04:26:04Z</dcterms:modified>
	<dc:publisher rdf:datatype="http://www.w3.org/2001/XMLSchema#string">Institute for Marine and Antarctic Studies (IMAS) - UTAS</dc:publisher>
	<skos:definition xml:lang="en">A deep-sea substratum that is composed of &gt; 30 % tests, shells or frustules of small plankton.</skos:definition>
	<dc:source rdf:datatype="http://www.w3.org/2001/XMLSchema#string">  SeaMap Australia National Benthic Habitat Classification Scheme (2017)</dc:source>
	<skos:narrower rdf:resource="http://seamapaustralia.org.au/def/benthichabitatclassification/class/62"/>
	<skos:narrower rdf:resource="http://seamapaustralia.org.au/def/benthichabitatclassification/class/63"/>
</rdf:Description>

<rdf:Description rdf:about="http://seamapaustralia.org.au/def/benthichabitatclassification/class/334">
	<rdf:type rdf:resource="http://www.w3.org/2000/01/rdf-schema#Resource"/>
	<rdf:type rdf:resource="http://www.w3.org/2004/02/skos/core#Concept"/>
	<skos:broader rdf:resource="http://seamapaustralia.org.au/def/benthichabitatclassification/class/331"/>
	<skos:prefLabel xml:lang="en">Oyster Shell</skos:prefLabel>
	<dcterms:contributor rdf:resource="http://editor.vocabs.ands.org.au/user/eMII_Finney.Kim_Admin"/>
	<dcterms:created rdf:datatype="http://www.w3.org/2001/XMLSchema#dateTime">2017-06-27T01:48:03Z</dcterms:created>
	<dcterms:creator rdf:resource="http://editor.vocabs.ands.org.au/user/eMII_Finney.Kim_Admin"/>
	<dcterms:modified rdf:datatype="http://www.w3.org/2001/XMLSchema#dateTime">2017-06-27T01:52:51Z</dcterms:modified>
	<skos:definition xml:lang="en">Biogenic substrata dominated by oysters.</skos:definition>
</rdf:Description>

<rdf:Description rdf:about="http://seamapaustralia.org.au/def/benthichabitatclassification/class/44">
	<rdf:type rdf:resource="http://www.w3.org/2000/01/rdf-schema#Resource"/>
	<rdf:type rdf:resource="http://www.w3.org/2004/02/skos/core#Concept"/>
	<skos:broader rdf:resource="http://seamapaustralia.org.au/def/benthichabitatclassification/class/36"/>
	<skos:prefLabel xml:lang="en">Metamorphic</skos:prefLabel>
	<dcterms:contributor rdf:resource="http://editor.vocabs.ands.org.au/user/eMII_Finney.Kim_Admin"/>
	<dcterms:created rdf:datatype="http://www.w3.org/2001/XMLSchema#dateTime">2016-11-16T00:48:56Z</dcterms:created>
	<dcterms:creator rdf:resource="http://editor.vocabs.ands.org.au/user/eMII_Finney.Kim_Admin"/>
	<dcterms:modified rdf:datatype="http://www.w3.org/2001/XMLSchema#dateTime">2017-06-27T04:27:30Z</dcterms:modified>
	<dc:publisher rdf:datatype="http://www.w3.org/2001/XMLSchema#string">Institute for Marine and Antarctic Studies (IMAS) - UTAS</dc:publisher>
	<skos:definition xml:lang="en">A geologic substratum that is composed of  ≥ 60 % metamorphic rock.</skos:definition>
	<dc:source rdf:datatype="http://www.w3.org/2001/XMLSchema#string">SeaMap Australia National Benthic Habitat Classification Scheme (2017)</dc:source>
</rdf:Description>

<rdf:Description rdf:about="http://seamapaustralia.org.au/def/benthichabitatclassification/class/45">
	<rdf:type rdf:resource="http://www.w3.org/2000/01/rdf-schema#Resource"/>
	<rdf:type rdf:resource="http://www.w3.org/2004/02/skos/core#Concept"/>
	<skos:broader rdf:resource="http://seamapaustralia.org.au/def/benthichabitatclassification/class/36"/>
	<skos:prefLabel xml:lang="en">Igneous</skos:prefLabel>
	<dcterms:contributor rdf:resource="http://editor.vocabs.ands.org.au/user/eMII_Finney.Kim_Admin"/>
	<dcterms:created rdf:datatype="http://www.w3.org/2001/XMLSchema#dateTime">2016-11-16T00:49:32Z</dcterms:created>
	<dcterms:creator rdf:resource="http://editor.vocabs.ands.org.au/user/eMII_Finney.Kim_Admin"/>
	<dcterms:modified rdf:datatype="http://www.w3.org/2001/XMLSchema#dateTime">2017-06-27T04:27:24Z</dcterms:modified>
	<dc:publisher rdf:datatype="http://www.w3.org/2001/XMLSchema#string">Institute for Marine and Antarctic Studies (IMAS) - UTAS</dc:publisher>
	<skos:definition xml:lang="en">A geologic substratum that is composed of  ≥ 60 % igneous rock.</skos:definition>
	<dc:source rdf:datatype="http://www.w3.org/2001/XMLSchema#string">SeaMap Australia National Benthic Habitat Classification Scheme (2017)</dc:source>
</rdf:Description>

<rdf:Description rdf:about="http://seamapaustralia.org.au/def/benthichabitatclassification/class/46">
	<rdf:type rdf:resource="http://www.w3.org/2000/01/rdf-schema#Resource"/>
	<rdf:type rdf:resource="http://www.w3.org/2004/02/skos/core#Concept"/>
	<skos:broader rdf:resource="http://seamapaustralia.org.au/def/benthichabitatclassification/class/36"/>
	<skos:prefLabel xml:lang="en">Sedimentary</skos:prefLabel>
	<dcterms:contributor rdf:resource="http://editor.vocabs.ands.org.au/user/eMII_Finney.Kim_Admin"/>
	<dcterms:created rdf:datatype="http://www.w3.org/2001/XMLSchema#dateTime">2016-11-16T00:50:11Z</dcterms:created>
	<dcterms:creator rdf:resource="http://editor.vocabs.ands.org.au/user/eMII_Finney.Kim_Admin"/>
	<dcterms:modified rdf:datatype="http://www.w3.org/2001/XMLSchema#dateTime">2017-06-27T04:27:36Z</dcterms:modified>
	<dc:publisher rdf:datatype="http://www.w3.org/2001/XMLSchema#string">Institute for Marine and Antarctic Studies (IMAS) - UTAS</dc:publisher>
	<skos:definition xml:lang="en">A geologic substratum that is composed of  ≥ 60 % sedimentary rock.</skos:definition>
	<dc:source rdf:datatype="http://www.w3.org/2001/XMLSchema#string">SeaMap Australia National Benthic Habitat Classification Scheme (2017)</dc:source>
</rdf:Description>

<rdf:Description rdf:about="http://seamapaustralia.org.au/def/benthichabitatclassification/class/47">
	<rdf:type rdf:resource="http://www.w3.org/2000/01/rdf-schema#Resource"/>
	<rdf:type rdf:resource="http://www.w3.org/2004/02/skos/core#Concept"/>
	<skos:broader rdf:resource="http://seamapaustralia.org.au/def/benthichabitatclassification/class/37"/>
	<skos:prefLabel xml:lang="en">Rock</skos:prefLabel>
	<dcterms:contributor rdf:resource="http://editor.vocabs.ands.org.au/user/eMII_Finney.Kim_Admin"/>
	<dcterms:created rdf:datatype="http://www.w3.org/2001/XMLSchema#dateTime">2016-11-16T00:50:43Z</dcterms:created>
	<dcterms:creator rdf:resource="http://editor.vocabs.ands.org.au/user/eMII_Finney.Kim_Admin"/>
	<dcterms:modified rdf:datatype="http://www.w3.org/2001/XMLSchema#dateTime">2017-06-27T04:25:07Z</dcterms:modified>
	<dc:publisher rdf:datatype="http://www.w3.org/2001/XMLSchema#string">Institute for Marine and Antarctic Studies (IMAS) - UTAS</dc:publisher>
	<skos:definition xml:lang="en">An anthropogenic substratum that is dominated (≥ 60 %) by natural mineral materials. This includes breakwaters and artificial reefs made of natural stone. If the origin cannot be identified, it is assumed to be natural and classed under Geologic Origin.  </skos:definition>
	<dc:source rdf:datatype="http://www.w3.org/2001/XMLSchema#string">SeaMap Australia National Benthic Habitat Classification Scheme (2017)</dc:source>
</rdf:Description>

<rdf:Description rdf:about="http://seamapaustralia.org.au/def/benthichabitatclassification/class/48">
	<rdf:type rdf:resource="http://www.w3.org/2000/01/rdf-schema#Resource"/>
	<rdf:type rdf:resource="http://www.w3.org/2004/02/skos/core#Concept"/>
	<skos:broader rdf:resource="http://seamapaustralia.org.au/def/benthichabitatclassification/class/37"/>
	<skos:prefLabel xml:lang="en">Wood</skos:prefLabel>
	<dcterms:contributor rdf:resource="http://editor.vocabs.ands.org.au/user/eMII_Finney.Kim_Admin"/>
	<dcterms:created rdf:datatype="http://www.w3.org/2001/XMLSchema#dateTime">2016-11-16T00:51:09Z</dcterms:created>
	<dcterms:creator rdf:resource="http://editor.vocabs.ands.org.au/user/eMII_Finney.Kim_Admin"/>
	<dcterms:modified rdf:datatype="http://www.w3.org/2001/XMLSchema#dateTime">2017-06-27T04:25:13Z</dcterms:modified>
	<dc:publisher rdf:datatype="http://www.w3.org/2001/XMLSchema#string">Institute for Marine and Antarctic Studies (IMAS) - UTAS</dc:publisher>
	<skos:definition xml:lang="en">An anthropogenic substratum that is dominated by wood and woody materials that were constructed and deposited in the marine environment by humans. </skos:definition>
	<dc:source rdf:datatype="http://www.w3.org/2001/XMLSchema#string">SeaMap Australia National Benthic Habitat Classification Scheme (2017)</dc:source>
</rdf:Description>

<rdf:Description rdf:about="http://seamapaustralia.org.au/def/benthichabitatclassification/class/49">
	<rdf:type rdf:resource="http://www.w3.org/2000/01/rdf-schema#Resource"/>
	<rdf:type rdf:resource="http://www.w3.org/2004/02/skos/core#Concept"/>
	<skos:broader rdf:resource="http://seamapaustralia.org.au/def/benthichabitatclassification/class/37"/>
	<skos:prefLabel xml:lang="en">Construction</skos:prefLabel>
	<dcterms:contributor rdf:resource="http://editor.vocabs.ands.org.au/user/eMII_Finney.Kim_Admin"/>
	<dcterms:created rdf:datatype="http://www.w3.org/2001/XMLSchema#dateTime">2016-11-16T00:51:39Z</dcterms:created>
	<dcterms:creator rdf:resource="http://editor.vocabs.ands.org.au/user/eMII_Finney.Kim_Admin"/>
	<dcterms:modified rdf:datatype="http://www.w3.org/2001/XMLSchema#dateTime">2017-06-27T04:24:52Z</dcterms:modified>
	<dc:publisher rdf:datatype="http://www.w3.org/2001/XMLSchema#string">Institute for Marine and Antarctic Studies (IMAS) - UTAS</dc:publisher>
	<skos:definition xml:lang="en">An anthropogenic substratum that is composed of unnatural mineral materials used in construction that have been assembled and deposited by humans, e.g. concrete, plastic, fibreglass, porcelain, rubber.</skos:definition>
	<dc:source rdf:datatype="http://www.w3.org/2001/XMLSchema#string">SeaMap Australia National Benthic Habitat Classification Scheme (2017)</dc:source>
</rdf:Description>

<rdf:Description rdf:about="http://seamapaustralia.org.au/def/benthichabitatclassification/class/50">
	<rdf:type rdf:resource="http://www.w3.org/2000/01/rdf-schema#Resource"/>
	<rdf:type rdf:resource="http://www.w3.org/2004/02/skos/core#Concept"/>
	<skos:broader rdf:resource="http://seamapaustralia.org.au/def/benthichabitatclassification/class/37"/>
	<skos:prefLabel xml:lang="en">Metal</skos:prefLabel>
	<dcterms:contributor rdf:resource="http://editor.vocabs.ands.org.au/user/eMII_Finney.Kim_Admin"/>
	<dcterms:created rdf:datatype="http://www.w3.org/2001/XMLSchema#dateTime">2016-11-16T00:52:04Z</dcterms:created>
	<dcterms:creator rdf:resource="http://editor.vocabs.ands.org.au/user/eMII_Finney.Kim_Admin"/>
	<dcterms:modified rdf:datatype="http://www.w3.org/2001/XMLSchema#dateTime">2017-06-27T04:25:02Z</dcterms:modified>
	<dc:publisher rdf:datatype="http://www.w3.org/2001/XMLSchema#string">Institute for Marine and Antarctic Studies (IMAS) - UTAS</dc:publisher>
	<skos:definition xml:lang="en">An anthropogenic substratum that constitutes ≥ 60 % metal that was manufactured by humans.  </skos:definition>
	<dc:source rdf:datatype="http://www.w3.org/2001/XMLSchema#string">SeaMap Australia National Benthic Habitat Classification Scheme (2017)</dc:source>
</rdf:Description>

<rdf:Description rdf:about="http://seamapaustralia.org.au/def/benthichabitatclassification/class/154">
	<rdf:type rdf:resource="http://www.w3.org/2000/01/rdf-schema#Resource"/>
	<rdf:type rdf:resource="http://www.w3.org/2004/02/skos/core#Concept"/>
	<skos:broader rdf:resource="http://seamapaustralia.org.au/def/benthichabitatclassification/class/37"/>
	<skos:prefLabel xml:lang="en">Garbage</skos:prefLabel>
	<dcterms:contributor rdf:resource="http://editor.vocabs.ands.org.au/user/eMII_Finney.Kim_Admin"/>
	<dcterms:created rdf:datatype="http://www.w3.org/2001/XMLSchema#dateTime">2017-05-23T05:34:13Z</dcterms:created>
	<dcterms:creator rdf:resource="http://editor.vocabs.ands.org.au/user/eMII_Finney.Kim_Admin"/>
	<dcterms:modified rdf:datatype="http://www.w3.org/2001/XMLSchema#dateTime">2017-06-27T04:24:57Z</dcterms:modified>
	<dc:publisher rdf:datatype="http://www.w3.org/2001/XMLSchema#string">Institute for Marine and Antarctic Studies (IMAS) - UTAS</dc:publisher>
	<skos:definition xml:lang="en">An anthropogenic substratum that is typically composed of plastic, but can include any amounts of rubber, glass, wax, metal and other rubbish materials, that has been manufactured and deposited by humans. </skos:definition>
	<dc:source rdf:datatype="http://www.w3.org/2001/XMLSchema#string">SeaMap Australia National Benthic Habitat Classification Scheme (2017)</dc:source>
	<skos:closeMatch rdf:resource="https://www.cmecscatalog.org/cmecs/classification/unit/259.html"/>
</rdf:Description>

<rdf:Description rdf:about="http://seamapaustralia.org.au/def/benthichabitatclassification/class/333">
	<rdf:type rdf:resource="http://www.w3.org/2000/01/rdf-schema#Resource"/>
	<rdf:type rdf:resource="http://www.w3.org/2004/02/skos/core#Concept"/>
	<skos:broader rdf:resource="http://seamapaustralia.org.au/def/benthichabitatclassification/class/331"/>
	<skos:prefLabel xml:lang="en">Mussel Shell</skos:prefLabel>
	<dcterms:contributor rdf:resource="http://editor.vocabs.ands.org.au/user/eMII_Finney.Kim_Admin"/>
	<dcterms:created rdf:datatype="http://www.w3.org/2001/XMLSchema#dateTime">2017-06-27T01:47:50Z</dcterms:created>
	<dcterms:creator rdf:resource="http://editor.vocabs.ands.org.au/user/eMII_Finney.Kim_Admin"/>
	<dcterms:modified rdf:datatype="http://www.w3.org/2001/XMLSchema#dateTime">2017-06-27T01:52:38Z</dcterms:modified>
	<skos:definition xml:lang="en">Biogenic substrata dominated by mussels.</skos:definition>
</rdf:Description>

<rdf:Description rdf:about="http://seamapaustralia.org.au/def/benthichabitatclassification/class/53">
	<rdf:type rdf:resource="http://www.w3.org/2000/01/rdf-schema#Resource"/>
	<rdf:type rdf:resource="http://www.w3.org/2004/02/skos/core#Concept"/>
	<skos:broader rdf:resource="http://seamapaustralia.org.au/def/benthichabitatclassification/class/38"/>
	<skos:prefLabel xml:lang="en">Serpulid</skos:prefLabel>
	<dcterms:contributor rdf:resource="http://editor.vocabs.ands.org.au/user/eMII_Finney.Kim_Admin"/>
	<dcterms:created rdf:datatype="http://www.w3.org/2001/XMLSchema#dateTime">2016-11-16T00:54:40Z</dcterms:created>
	<dcterms:creator rdf:resource="http://editor.vocabs.ands.org.au/user/eMII_Finney.Kim_Admin"/>
	<dcterms:modified rdf:datatype="http://www.w3.org/2001/XMLSchema#dateTime">2017-06-27T04:27:10Z</dcterms:modified>
	<dc:publisher rdf:datatype="http://www.w3.org/2001/XMLSchema#string">Institute for Marine and Antarctic Studies (IMAS) - UTAS</dc:publisher>
	<skos:definition xml:lang="en">Worm substrata that comprise tubes composed of calcium carbonate that have been constructed by serpulid worms (e.g. Serpulid sp., Galeolaria caespitose).</skos:definition>
	<dc:source rdf:datatype="http://www.w3.org/2001/XMLSchema#string">SeaMap Australia National Benthic Habitat Classification Scheme (2017)</dc:source>
</rdf:Description>

<rdf:Description rdf:about="http://seamapaustralia.org.au/def/benthichabitatclassification/class/54">
	<rdf:type rdf:resource="http://www.w3.org/2000/01/rdf-schema#Resource"/>
	<rdf:type rdf:resource="http://www.w3.org/2004/02/skos/core#Concept"/>
	<skos:broader rdf:resource="http://seamapaustralia.org.au/def/benthichabitatclassification/class/38"/>
	<skos:prefLabel xml:lang="en">Sabellarid</skos:prefLabel>
	<dcterms:contributor rdf:resource="http://editor.vocabs.ands.org.au/user/eMII_Finney.Kim_Admin"/>
	<dcterms:created rdf:datatype="http://www.w3.org/2001/XMLSchema#dateTime">2016-11-16T00:55:17Z</dcterms:created>
	<dcterms:creator rdf:resource="http://editor.vocabs.ands.org.au/user/eMII_Finney.Kim_Admin"/>
	<dcterms:modified rdf:datatype="http://www.w3.org/2001/XMLSchema#dateTime">2017-06-27T04:27:05Z</dcterms:modified>
	<dc:publisher rdf:datatype="http://www.w3.org/2001/XMLSchema#string">Institute for Marine and Antarctic Studies (IMAS) - UTAS</dc:publisher>
	<skos:definition xml:lang="en">Worm substrata that comprise tubes composed of shell and sand fragments that have been constructed by sabellariid worms (e.g. Idanthyrsus pennatus)</skos:definition>
	<dc:source rdf:datatype="http://www.w3.org/2001/XMLSchema#string">SeaMap Australia National Benthic Habitat Classification Scheme (2017)</dc:source>
</rdf:Description>

<rdf:Description rdf:about="http://seamapaustralia.org.au/def/benthichabitatclassification/class/55">
	<rdf:type rdf:resource="http://www.w3.org/2000/01/rdf-schema#Resource"/>
	<rdf:type rdf:resource="http://www.w3.org/2004/02/skos/core#Concept"/>
	<skos:broader rdf:resource="http://seamapaustralia.org.au/def/benthichabitatclassification/class/39"/>
	<skos:prefLabel xml:lang="en">Rhodolith</skos:prefLabel>
	<dcterms:contributor rdf:resource="http://editor.vocabs.ands.org.au/user/eMII_Finney.Kim_Admin"/>
	<dcterms:created rdf:datatype="http://www.w3.org/2001/XMLSchema#dateTime">2016-11-16T00:55:55Z</dcterms:created>
	<dcterms:creator rdf:resource="http://editor.vocabs.ands.org.au/user/eMII_Finney.Kim_Admin"/>
	<dcterms:modified rdf:datatype="http://www.w3.org/2001/XMLSchema#dateTime">2017-06-27T04:25:34Z</dcterms:modified>
	<dc:publisher rdf:datatype="http://www.w3.org/2001/XMLSchema#string">Institute for Marine and Antarctic Studies (IMAS) - UTAS</dc:publisher>
	<skos:definition xml:lang="en">Biogenic substrata that are primarily composed of rhodoliths, a crustose algae that forms rounded calcareous nodules.</skos:definition>
	<dc:source rdf:datatype="http://www.w3.org/2001/XMLSchema#string">SeaMap Australia National Benthic Habitat Classification Scheme (2017)</dc:source>
</rdf:Description>

<rdf:Description rdf:about="http://seamapaustralia.org.au/def/benthichabitatclassification/class/56">
	<rdf:type rdf:resource="http://www.w3.org/2000/01/rdf-schema#Resource"/>
	<rdf:type rdf:resource="http://www.w3.org/2004/02/skos/core#Concept"/>
	<skos:broader rdf:resource="http://seamapaustralia.org.au/def/benthichabitatclassification/class/39"/>
	<skos:prefLabel xml:lang="en">Halimeda</skos:prefLabel>
	<dcterms:contributor rdf:resource="http://editor.vocabs.ands.org.au/user/eMII_Finney.Kim_Admin"/>
	<dcterms:created rdf:datatype="http://www.w3.org/2001/XMLSchema#dateTime">2016-11-16T00:56:44Z</dcterms:created>
	<dcterms:creator rdf:resource="http://editor.vocabs.ands.org.au/user/eMII_Finney.Kim_Admin"/>
	<dcterms:modified rdf:datatype="http://www.w3.org/2001/XMLSchema#dateTime">2017-06-27T04:25:29Z</dcterms:modified>
	<dc:publisher rdf:datatype="http://www.w3.org/2001/XMLSchema#string">Institute for Marine and Antarctic Studies (IMAS) - UTAS</dc:publisher>
	<skos:definition xml:lang="en">Biogenic substrata that are primarily composed of Halimeda sp., a calcareous marine alga that can form extensive algal sands once it has died. </skos:definition>
	<dc:source rdf:datatype="http://www.w3.org/2001/XMLSchema#string">SeaMap Australia National Benthic Habitat Classification Scheme (2017)</dc:source>
</rdf:Description>

<rdf:Description rdf:about="http://seamapaustralia.org.au/def/benthichabitatclassification/class/306">
	<rdf:type rdf:resource="http://www.w3.org/2000/01/rdf-schema#Resource"/>
	<rdf:type rdf:resource="http://www.w3.org/2004/02/skos/core#Concept"/>
	<skos:broader rdf:resource="http://seamapaustralia.org.au/def/benthichabitatclassification/class/298"/>
	<skos:prefLabel xml:lang="en">IMCRA Karumba-Nassau Bioregion</skos:prefLabel>
	<dcterms:contributor rdf:resource="http://editor.vocabs.ands.org.au/user/eMII_Finney.Kim_Admin"/>
	<dcterms:created rdf:datatype="http://www.w3.org/2001/XMLSchema#dateTime">2017-06-14T05:28:20Z</dcterms:created>
	<dcterms:creator rdf:resource="http://editor.vocabs.ands.org.au/user/eMII_Finney.Kim_Admin"/>
	<dcterms:modified rdf:datatype="http://www.w3.org/2001/XMLSchema#dateTime">2017-06-26T23:28:18Z</dcterms:modified>
	<dc:publisher rdf:datatype="http://www.w3.org/2001/XMLSchema#string">Institute for Marine and Antarctic Studies (IMAS) - UTAS</dc:publisher>
	<skos:definition xml:lang="en">An inshore regionalisation of Australian waters derived from biological and physical data, including the distribution of demersal fishes, marine plants and invertebrates, sea floor geomorphology and sediments, and oceanographic data. The meso-scale regionalisation was compiled from information supplied to the Australian Government Department of the Environment and Heritage by the relevant State, Northern Territory and Commonwealth marine research and management agencies. The seaward extent for the meso-scale IMCRA coverage is defined by the 200m isobath except where this boundary extends beyond the Australian Exclusive Economic Zone (AEEZ).</skos:definition>
	<dc:source rdf:datatype="http://www.w3.org/2001/XMLSchema#string">Commonwealth of Australia (2006). A Guide to the Integrated Marine and Coastal Regionalisation of Australia Version 4.0. Department of the Environment and Heritage, Canberra, Australia.</dc:source>
	<skos:exactMatch rdf:resource="http://www.environment.gov.au/mapping/rest/services/ogc_services/IMCRA_Mesoscale/MapServer/0/16"/>
</rdf:Description>

<rdf:Description rdf:about="http://seamapaustralia.org.au/def/benthichabitatclassification/class/304">
	<rdf:type rdf:resource="http://www.w3.org/2000/01/rdf-schema#Resource"/>
	<rdf:type rdf:resource="http://www.w3.org/2004/02/skos/core#Concept"/>
	<skos:broader rdf:resource="http://seamapaustralia.org.au/def/benthichabitatclassification/class/298"/>
	<skos:prefLabel xml:lang="en">IMCRA Pellew Bioregion</skos:prefLabel>
	<dcterms:contributor rdf:resource="http://editor.vocabs.ands.org.au/user/eMII_Finney.Kim_Admin"/>
	<dcterms:created rdf:datatype="http://www.w3.org/2001/XMLSchema#dateTime">2017-06-14T05:27:40Z</dcterms:created>
	<dcterms:creator rdf:resource="http://editor.vocabs.ands.org.au/user/eMII_Finney.Kim_Admin"/>
	<dcterms:modified rdf:datatype="http://www.w3.org/2001/XMLSchema#dateTime">2017-06-26T23:28:52Z</dcterms:modified>
	<dc:publisher rdf:datatype="http://www.w3.org/2001/XMLSchema#string">Institute for Marine and Antarctic Studies (IMAS) - UTAS</dc:publisher>
	<skos:definition xml:lang="en">An inshore regionalisation of Australian waters derived from biological and physical data, including the distribution of demersal fishes, marine plants and invertebrates, sea floor geomorphology and sediments, and oceanographic data. The meso-scale regionalisation was compiled from information supplied to the Australian Government Department of the Environment and Heritage by the relevant State, Northern Territory and Commonwealth marine research and management agencies. The seaward extent for the meso-scale IMCRA coverage is defined by the 200m isobath except where this boundary extends beyond the Australian Exclusive Economic Zone (AEEZ).</skos:definition>
	<dc:source rdf:datatype="http://www.w3.org/2001/XMLSchema#string">Commonwealth of Australia (2006). A Guide to the Integrated Marine and Coastal Regionalisation of Australia Version 4.0. Department of the Environment and Heritage, Canberra, Australia.</dc:source>
	<skos:exactMatch rdf:resource="http://www.environment.gov.au/mapping/rest/services/ogc_services/IMCRA_Mesoscale/MapServer/0/19"/>
</rdf:Description>

<rdf:Description rdf:about="http://seamapaustralia.org.au/def/benthichabitatclassification/class/301">
	<rdf:type rdf:resource="http://www.w3.org/2000/01/rdf-schema#Resource"/>
	<rdf:type rdf:resource="http://www.w3.org/2004/02/skos/core#Concept"/>
	<skos:broader rdf:resource="http://seamapaustralia.org.au/def/benthichabitatclassification/class/298"/>
	<skos:prefLabel xml:lang="en">IMCRA Van Diemens Gulf Bioregion</skos:prefLabel>
	<dcterms:contributor rdf:resource="http://editor.vocabs.ands.org.au/user/eMII_Finney.Kim_Admin"/>
	<dcterms:created rdf:datatype="http://www.w3.org/2001/XMLSchema#dateTime">2017-06-14T05:26:41Z</dcterms:created>
	<dcterms:creator rdf:resource="http://editor.vocabs.ands.org.au/user/eMII_Finney.Kim_Admin"/>
	<dcterms:modified rdf:datatype="http://www.w3.org/2001/XMLSchema#dateTime">2017-06-26T23:30:20Z</dcterms:modified>
	<dc:publisher rdf:datatype="http://www.w3.org/2001/XMLSchema#string">Institute for Marine and Antarctic Studies (IMAS) - UTAS</dc:publisher>
	<skos:definition xml:lang="en">An inshore regionalisation of Australian waters derived from biological and physical data, including the distribution of demersal fishes, marine plants and invertebrates, sea floor geomorphology and sediments, and oceanographic data. The meso-scale regionalisation was compiled from information supplied to the Australian Government Department of the Environment and Heritage by the relevant State, Northern Territory and Commonwealth marine research and management agencies. The seaward extent for the meso-scale IMCRA coverage is defined by the 200m isobath except where this boundary extends beyond the Australian Exclusive Economic Zone (AEEZ).</skos:definition>
	<dc:source rdf:datatype="http://www.w3.org/2001/XMLSchema#string">Commonwealth of Australia (2006). A Guide to the Integrated Marine and Coastal Regionalisation of Australia Version 4.0. Department of the Environment and Heritage, Canberra, Australia.</dc:source>
	<skos:exactMatch rdf:resource="http://www.environment.gov.au/mapping/rest/services/ogc_services/IMCRA_Mesoscale/MapServer/0/12"/>
</rdf:Description>

<rdf:Description rdf:about="http://seamapaustralia.org.au/def/benthichabitatclassification/class/305">
	<rdf:type rdf:resource="http://www.w3.org/2000/01/rdf-schema#Resource"/>
	<rdf:type rdf:resource="http://www.w3.org/2004/02/skos/core#Concept"/>
	<skos:broader rdf:resource="http://seamapaustralia.org.au/def/benthichabitatclassification/class/298"/>
	<skos:prefLabel xml:lang="en">IMCRA Wellesley Bioregion</skos:prefLabel>
	<dcterms:contributor rdf:resource="http://editor.vocabs.ands.org.au/user/eMII_Finney.Kim_Admin"/>
	<dcterms:created rdf:datatype="http://www.w3.org/2001/XMLSchema#dateTime">2017-06-14T05:27:58Z</dcterms:created>
	<dcterms:creator rdf:resource="http://editor.vocabs.ands.org.au/user/eMII_Finney.Kim_Admin"/>
	<dcterms:modified rdf:datatype="http://www.w3.org/2001/XMLSchema#dateTime">2017-06-26T23:30:51Z</dcterms:modified>
	<dc:publisher rdf:datatype="http://www.w3.org/2001/XMLSchema#string">Institute for Marine and Antarctic Studies (IMAS) - UTAS</dc:publisher>
	<skos:definition xml:lang="en">An inshore regionalisation of Australian waters derived from biological and physical data, including the distribution of demersal fishes, marine plants and invertebrates, sea floor geomorphology and sediments, and oceanographic data. The meso-scale regionalisation was compiled from information supplied to the Australian Government Department of the Environment and Heritage by the relevant State, Northern Territory and Commonwealth marine research and management agencies. The seaward extent for the meso-scale IMCRA coverage is defined by the 200m isobath except where this boundary extends beyond the Australian Exclusive Economic Zone (AEEZ).</skos:definition>
	<dc:source rdf:datatype="http://www.w3.org/2001/XMLSchema#string">Commonwealth of Australia (2006). A Guide to the Integrated Marine and Coastal Regionalisation of Australia Version 4.0. Department of the Environment and Heritage, Canberra, Australia.</dc:source>
	<skos:exactMatch rdf:resource="http://www.environment.gov.au/mapping/rest/services/ogc_services/IMCRA_Mesoscale/MapServer/0/21"/>
</rdf:Description>

<rdf:Description rdf:about="http://seamapaustralia.org.au/def/benthichabitatclassification/class/308">
	<rdf:type rdf:resource="http://www.w3.org/2000/01/rdf-schema#Resource"/>
	<rdf:type rdf:resource="http://www.w3.org/2004/02/skos/core#Concept"/>
	<skos:broader rdf:resource="http://seamapaustralia.org.au/def/benthichabitatclassification/class/298"/>
	<skos:prefLabel xml:lang="en">IMCRA West Cape York Bioregion</skos:prefLabel>
	<dcterms:contributor rdf:resource="http://editor.vocabs.ands.org.au/user/eMII_Finney.Kim_Admin"/>
	<dcterms:created rdf:datatype="http://www.w3.org/2001/XMLSchema#dateTime">2017-06-14T05:28:53Z</dcterms:created>
	<dcterms:creator rdf:resource="http://editor.vocabs.ands.org.au/user/eMII_Finney.Kim_Admin"/>
	<dcterms:modified rdf:datatype="http://www.w3.org/2001/XMLSchema#dateTime">2017-06-26T23:31:24Z</dcterms:modified>
	<dc:publisher rdf:datatype="http://www.w3.org/2001/XMLSchema#string">Institute for Marine and Antarctic Studies (IMAS) - UTAS</dc:publisher>
	<skos:definition xml:lang="en">An inshore regionalisation of Australian waters derived from biological and physical data, including the distribution of demersal fishes, marine plants and invertebrates, sea floor geomorphology and sediments, and oceanographic data. The meso-scale regionalisation was compiled from information supplied to the Australian Government Department of the Environment and Heritage by the relevant State, Northern Territory and Commonwealth marine research and management agencies. The seaward extent for the meso-scale IMCRA coverage is defined by the 200m isobath except where this boundary extends beyond the Australian Exclusive Economic Zone (AEEZ).</skos:definition>
	<dc:source rdf:datatype="http://www.w3.org/2001/XMLSchema#string">Commonwealth of Australia (2006). A Guide to the Integrated Marine and Coastal Regionalisation of Australia Version 4.0. Department of the Environment and Heritage, Canberra, Australia.</dc:source>
	<skos:exactMatch rdf:resource="http://www.environment.gov.au/mapping/rest/services/ogc_services/IMCRA_Mesoscale/MapServer/0/6"/>
</rdf:Description>

<rdf:Description rdf:about="http://seamapaustralia.org.au/def/benthichabitatclassification/class/309">
	<rdf:type rdf:resource="http://www.w3.org/2000/01/rdf-schema#Resource"/>
	<rdf:type rdf:resource="http://www.w3.org/2004/02/skos/core#Concept"/>
	<skos:broader rdf:resource="http://seamapaustralia.org.au/def/benthichabitatclassification/class/192"/>
	<skos:prefLabel xml:lang="en">IMCRA Northwest Transition</skos:prefLabel>
	<dcterms:contributor rdf:resource="http://editor.vocabs.ands.org.au/user/eMII_Finney.Kim_Admin"/>
	<dcterms:created rdf:datatype="http://www.w3.org/2001/XMLSchema#dateTime">2017-06-14T05:29:16Z</dcterms:created>
	<dcterms:creator rdf:resource="http://editor.vocabs.ands.org.au/user/eMII_Finney.Kim_Admin"/>
	<dcterms:modified rdf:datatype="http://www.w3.org/2001/XMLSchema#dateTime">2017-06-26T23:36:23Z</dcterms:modified>
	<dc:publisher rdf:datatype="http://www.w3.org/2001/XMLSchema#string">Institute for Marine and Antarctic Studies (IMAS) - UTAS</dc:publisher>
	<skos:definition xml:lang="en">An IMCRA provincial bioregion reflects biogeographic patterns in distributions of bottom-dwelling fish. Provincial bioregions were defined for the continental shelf for IMCRA v3.3, and for the continental slope for the National Marine Bioregionalisation using similar analytical techniques. In both cases the distributions of demersal (bottom-dwelling) fish were plotted onto a line divided into equally spaced sections. The number of species in each section and the similarity between sections were calculated using a statistical tool called the Jaccard Index. Where the Jaccard Index changed greatly between sections a boundary was defined indicating differences in species assemblages between regions. Two types of provincial bioregions are defined in the IMCRA benthic bioregionalisation: provinces, which represent regions of biotic endemism; and transitions, which generally occur between the provinces, and are less well-defined mixing areas that capture the overlap of demersal fish species ranges between the provinces.</skos:definition>
	<dc:source rdf:datatype="http://www.w3.org/2001/XMLSchema#string">Commonwealth of Australia (2006). A Guide to the Integrated Marine and Coastal Regionalisation of Australia Version 4.0. Department of the Environment and Heritage, Canberra, Australia.</dc:source>
	<skos:narrower rdf:resource="http://seamapaustralia.org.au/def/benthichabitatclassification/class/314"/>
	<skos:narrower rdf:resource="http://seamapaustralia.org.au/def/benthichabitatclassification/class/312"/>
	<skos:narrower rdf:resource="http://seamapaustralia.org.au/def/benthichabitatclassification/class/313"/>
	<skos:narrower rdf:resource="http://seamapaustralia.org.au/def/benthichabitatclassification/class/311"/>
	<skos:narrower rdf:resource="http://seamapaustralia.org.au/def/benthichabitatclassification/class/310"/>
	<skos:narrower rdf:resource="http://seamapaustralia.org.au/def/benthichabitatclassification/class/316"/>
	<skos:narrower rdf:resource="http://seamapaustralia.org.au/def/benthichabitatclassification/class/315"/>
	<skos:exactMatch rdf:resource="http://www.environment.gov.au/mapping/rest/services/ogc_services/IMCRA_Provincial/MapServer/0/13"/>
</rdf:Description>

<rdf:Description rdf:about="http://seamapaustralia.org.au/def/benthichabitatclassification/class/300">
	<rdf:type rdf:resource="http://www.w3.org/2000/01/rdf-schema#Resource"/>
	<rdf:type rdf:resource="http://www.w3.org/2004/02/skos/core#Concept"/>
	<skos:broader rdf:resource="http://seamapaustralia.org.au/def/benthichabitatclassification/class/298"/>
	<skos:prefLabel xml:lang="en">IMCRA Cobourg Bioregion</skos:prefLabel>
	<dcterms:contributor rdf:resource="http://editor.vocabs.ands.org.au/user/eMII_Finney.Kim_Admin"/>
	<dcterms:created rdf:datatype="http://www.w3.org/2001/XMLSchema#dateTime">2017-06-14T05:26:17Z</dcterms:created>
	<dcterms:creator rdf:resource="http://editor.vocabs.ands.org.au/user/eMII_Finney.Kim_Admin"/>
	<dcterms:modified rdf:datatype="http://www.w3.org/2001/XMLSchema#dateTime">2017-06-26T23:27:16Z</dcterms:modified>
	<dc:publisher rdf:datatype="http://www.w3.org/2001/XMLSchema#string">Institute for Marine and Antarctic Studies (IMAS) - UTAS</dc:publisher>
	<skos:definition xml:lang="en">An inshore regionalisation of Australian waters derived from biological and physical data, including the distribution of demersal fishes, marine plants and invertebrates, sea floor geomorphology and sediments, and oceanographic data. The meso-scale regionalisation was compiled from information supplied to the Australian Government Department of the Environment and Heritage by the relevant State, Northern Territory and Commonwealth marine research and management agencies. The seaward extent for the meso-scale IMCRA coverage is defined by the 200m isobath except where this boundary extends beyond the Australian Exclusive Economic Zone (AEEZ).</skos:definition>
	<dc:source rdf:datatype="http://www.w3.org/2001/XMLSchema#string">Commonwealth of Australia (2006). A Guide to the Integrated Marine and Coastal Regionalisation of Australia Version 4.0. Department of the Environment and Heritage, Canberra, Australia.</dc:source>
	<skos:exactMatch rdf:resource="http://www.environment.gov.au/mapping/rest/services/ogc_services/IMCRA_Mesoscale/MapServer/0/8"/>
</rdf:Description>

<rdf:Description rdf:about="http://seamapaustralia.org.au/def/benthichabitatclassification/class/314">
	<rdf:type rdf:resource="http://www.w3.org/2000/01/rdf-schema#Resource"/>
	<rdf:type rdf:resource="http://www.w3.org/2004/02/skos/core#Concept"/>
	<skos:broader rdf:resource="http://seamapaustralia.org.au/def/benthichabitatclassification/class/309"/>
	<skos:prefLabel xml:lang="en">IMCRA Anson Beagle Bioregion</skos:prefLabel>
	<dcterms:contributor rdf:resource="http://editor.vocabs.ands.org.au/user/eMII_Finney.Kim_Admin"/>
	<dcterms:created rdf:datatype="http://www.w3.org/2001/XMLSchema#dateTime">2017-06-14T05:30:53Z</dcterms:created>
	<dcterms:creator rdf:resource="http://editor.vocabs.ands.org.au/user/eMII_Finney.Kim_Admin"/>
	<dcterms:modified rdf:datatype="http://www.w3.org/2001/XMLSchema#dateTime">2017-06-26T23:33:24Z</dcterms:modified>
	<dc:publisher rdf:datatype="http://www.w3.org/2001/XMLSchema#string">Institute for Marine and Antarctic Studies (IMAS) - UTAS</dc:publisher>
	<skos:definition xml:lang="en">An inshore regionalisation of Australian waters derived from biological and physical data, including the distribution of demersal fishes, marine plants and invertebrates, sea floor geomorphology and sediments, and oceanographic data. The meso-scale regionalisation was compiled from information supplied to the Australian Government Department of the Environment and Heritage by the relevant State, Northern Territory and Commonwealth marine research and management agencies. The seaward extent for the meso-scale IMCRA coverage is defined by the 200m isobath except where this boundary extends beyond the Australian Exclusive Economic Zone (AEEZ).</skos:definition>
	<dc:source rdf:datatype="http://www.w3.org/2001/XMLSchema#string">Commonwealth of Australia (2006). A Guide to the Integrated Marine and Coastal Regionalisation of Australia Version 4.0. Department of the Environment and Heritage, Canberra, Australia.</dc:source>
	<skos:exactMatch rdf:resource="http://www.environment.gov.au/mapping/rest/services/ogc_services/IMCRA_Mesoscale/MapServer/0/13"/>
</rdf:Description>

<rdf:Description rdf:about="http://seamapaustralia.org.au/def/benthichabitatclassification/class/312">
	<rdf:type rdf:resource="http://www.w3.org/2000/01/rdf-schema#Resource"/>
	<rdf:type rdf:resource="http://www.w3.org/2004/02/skos/core#Concept"/>
	<skos:broader rdf:resource="http://seamapaustralia.org.au/def/benthichabitatclassification/class/309"/>
	<skos:prefLabel xml:lang="en">IMCRA Bonaparte Gulf Bioregion</skos:prefLabel>
	<dcterms:contributor rdf:resource="http://editor.vocabs.ands.org.au/user/eMII_Finney.Kim_Admin"/>
	<dcterms:created rdf:datatype="http://www.w3.org/2001/XMLSchema#dateTime">2017-06-14T05:30:08Z</dcterms:created>
	<dcterms:creator rdf:resource="http://editor.vocabs.ands.org.au/user/eMII_Finney.Kim_Admin"/>
	<dcterms:modified rdf:datatype="http://www.w3.org/2001/XMLSchema#dateTime">2017-06-26T23:33:55Z</dcterms:modified>
	<dc:publisher rdf:datatype="http://www.w3.org/2001/XMLSchema#string">Institute for Marine and Antarctic Studies (IMAS) - UTAS</dc:publisher>
	<skos:definition xml:lang="en">An inshore regionalisation of Australian waters derived from biological and physical data, including the distribution of demersal fishes, marine plants and invertebrates, sea floor geomorphology and sediments, and oceanographic data. The meso-scale regionalisation was compiled from information supplied to the Australian Government Department of the Environment and Heritage by the relevant State, Northern Territory and Commonwealth marine research and management agencies. The seaward extent for the meso-scale IMCRA coverage is defined by the 200m isobath except where this boundary extends beyond the Australian Exclusive Economic Zone (AEEZ).</skos:definition>
	<dc:source rdf:datatype="http://www.w3.org/2001/XMLSchema#string">Commonwealth of Australia (2006). A Guide to the Integrated Marine and Coastal Regionalisation of Australia Version 4.0. Department of the Environment and Heritage, Canberra, Australia.</dc:source>
	<skos:exactMatch rdf:resource="http://www.environment.gov.au/mapping/rest/services/ogc_services/IMCRA_Mesoscale/MapServer/0/11"/>
</rdf:Description>

<rdf:Description rdf:about="http://seamapaustralia.org.au/def/benthichabitatclassification/class/313">
	<rdf:type rdf:resource="http://www.w3.org/2000/01/rdf-schema#Resource"/>
	<rdf:type rdf:resource="http://www.w3.org/2004/02/skos/core#Concept"/>
	<skos:broader rdf:resource="http://seamapaustralia.org.au/def/benthichabitatclassification/class/309"/>
	<skos:prefLabel xml:lang="en">IMCRA Cambridge-Bonaparte Bioregion</skos:prefLabel>
	<dcterms:contributor rdf:resource="http://editor.vocabs.ands.org.au/user/eMII_Finney.Kim_Admin"/>
	<dcterms:created rdf:datatype="http://www.w3.org/2001/XMLSchema#dateTime">2017-06-14T05:30:37Z</dcterms:created>
	<dcterms:creator rdf:resource="http://editor.vocabs.ands.org.au/user/eMII_Finney.Kim_Admin"/>
	<dcterms:modified rdf:datatype="http://www.w3.org/2001/XMLSchema#dateTime">2017-06-26T23:34:24Z</dcterms:modified>
	<dc:publisher rdf:datatype="http://www.w3.org/2001/XMLSchema#string">Institute for Marine and Antarctic Studies (IMAS) - UTAS</dc:publisher>
	<skos:definition xml:lang="en">An inshore regionalisation of Australian waters derived from biological and physical data, including the distribution of demersal fishes, marine plants and invertebrates, sea floor geomorphology and sediments, and oceanographic data. The meso-scale regionalisation was compiled from information supplied to the Australian Government Department of the Environment and Heritage by the relevant State, Northern Territory and Commonwealth marine research and management agencies. The seaward extent for the meso-scale IMCRA coverage is defined by the 200m isobath except where this boundary extends beyond the Australian Exclusive Economic Zone (AEEZ).</skos:definition>
	<dc:source rdf:datatype="http://www.w3.org/2001/XMLSchema#string">Commonwealth of Australia (2006). A Guide to the Integrated Marine and Coastal Regionalisation of Australia Version 4.0. Department of the Environment and Heritage, Canberra, Australia.</dc:source>
	<skos:exactMatch rdf:resource="http://www.environment.gov.au/mapping/rest/services/ogc_services/IMCRA_Mesoscale/MapServer/0/18"/>
</rdf:Description>

<rdf:Description rdf:about="http://seamapaustralia.org.au/def/benthichabitatclassification/class/311">
	<rdf:type rdf:resource="http://www.w3.org/2000/01/rdf-schema#Resource"/>
	<rdf:type rdf:resource="http://www.w3.org/2004/02/skos/core#Concept"/>
	<skos:broader rdf:resource="http://seamapaustralia.org.au/def/benthichabitatclassification/class/309"/>
	<skos:prefLabel xml:lang="en">IMCRA Kimberley Bioregion</skos:prefLabel>
	<dcterms:contributor rdf:resource="http://editor.vocabs.ands.org.au/user/eMII_Finney.Kim_Admin"/>
	<dcterms:created rdf:datatype="http://www.w3.org/2001/XMLSchema#dateTime">2017-06-14T05:29:52Z</dcterms:created>
	<dcterms:creator rdf:resource="http://editor.vocabs.ands.org.au/user/eMII_Finney.Kim_Admin"/>
	<dcterms:modified rdf:datatype="http://www.w3.org/2001/XMLSchema#dateTime">2017-06-27T00:31:05Z</dcterms:modified>
	<dc:publisher rdf:datatype="http://www.w3.org/2001/XMLSchema#string">Institute for Marine and Antarctic Studies (IMAS) - UTAS</dc:publisher>
	<skos:definition xml:lang="en">An inshore regionalisation of Australian waters derived from biological and physical data, including the distribution of demersal fishes, marine plants and invertebrates, sea floor geomorphology and sediments, and oceanographic data. The meso-scale regionalisation was compiled from information supplied to the Australian Government Department of the Environment and Heritage by the relevant State, Northern Territory and Commonwealth marine research and management agencies. The seaward extent for the meso-scale IMCRA coverage is defined by the 200m isobath except where this boundary extends beyond the Australian Exclusive Economic Zone (AEEZ).</skos:definition>
	<dc:source rdf:datatype="http://www.w3.org/2001/XMLSchema#string">Commonwealth of Australia (2006). A Guide to the Integrated Marine and Coastal Regionalisation of Australia Version 4.0. Department of the Environment and Heritage, Canberra, Australia.</dc:source>
	<skos:exactMatch rdf:resource="http://www.environment.gov.au/mapping/rest/services/ogc_services/IMCRA_Mesoscale/MapServer/0/15"/>
</rdf:Description>

<rdf:Description rdf:about="http://seamapaustralia.org.au/def/benthichabitatclassification/class/310">
	<rdf:type rdf:resource="http://www.w3.org/2000/01/rdf-schema#Resource"/>
	<rdf:type rdf:resource="http://www.w3.org/2004/02/skos/core#Concept"/>
	<skos:broader rdf:resource="http://seamapaustralia.org.au/def/benthichabitatclassification/class/309"/>
	<skos:prefLabel xml:lang="en">IMCRA King Sound Bioregion</skos:prefLabel>
	<dcterms:contributor rdf:resource="http://editor.vocabs.ands.org.au/user/eMII_Finney.Kim_Admin"/>
	<dcterms:created rdf:datatype="http://www.w3.org/2001/XMLSchema#dateTime">2017-06-14T05:29:34Z</dcterms:created>
	<dcterms:creator rdf:resource="http://editor.vocabs.ands.org.au/user/eMII_Finney.Kim_Admin"/>
	<dcterms:modified rdf:datatype="http://www.w3.org/2001/XMLSchema#dateTime">2017-06-27T00:31:38Z</dcterms:modified>
	<dc:publisher rdf:datatype="http://www.w3.org/2001/XMLSchema#string">Institute for Marine and Antarctic Studies (IMAS) - UTAS</dc:publisher>
	<skos:definition xml:lang="en">An inshore regionalisation of Australian waters derived from biological and physical data, including the distribution of demersal fishes, marine plants and invertebrates, sea floor geomorphology and sediments, and oceanographic data. The meso-scale regionalisation was compiled from information supplied to the Australian Government Department of the Environment and Heritage by the relevant State, Northern Territory and Commonwealth marine research and management agencies. The seaward extent for the meso-scale IMCRA coverage is defined by the 200m isobath except where this boundary extends beyond the Australian Exclusive Economic Zone (AEEZ).</skos:definition>
	<dc:source rdf:datatype="http://www.w3.org/2001/XMLSchema#string">Commonwealth of Australia (2006). A Guide to the Integrated Marine and Coastal Regionalisation of Australia Version 4.0. Department of the Environment and Heritage, Canberra, Australia.</dc:source>
	<skos:exactMatch rdf:resource="http://www.environment.gov.au/mapping/rest/services/ogc_services/IMCRA_Mesoscale/MapServer/0/24"/>
</rdf:Description>

<rdf:Description rdf:about="http://seamapaustralia.org.au/def/benthichabitatclassification/class/316">
	<rdf:type rdf:resource="http://www.w3.org/2000/01/rdf-schema#Resource"/>
	<rdf:type rdf:resource="http://www.w3.org/2004/02/skos/core#Concept"/>
	<skos:broader rdf:resource="http://seamapaustralia.org.au/def/benthichabitatclassification/class/309"/>
	<skos:prefLabel xml:lang="en">IMCRA Oceanic Shoals Bioregion</skos:prefLabel>
	<dcterms:contributor rdf:resource="http://editor.vocabs.ands.org.au/user/eMII_Finney.Kim_Admin"/>
	<dcterms:created rdf:datatype="http://www.w3.org/2001/XMLSchema#dateTime">2017-06-14T05:31:34Z</dcterms:created>
	<dcterms:creator rdf:resource="http://editor.vocabs.ands.org.au/user/eMII_Finney.Kim_Admin"/>
	<dcterms:modified rdf:datatype="http://www.w3.org/2001/XMLSchema#dateTime">2017-06-27T00:32:34Z</dcterms:modified>
	<dc:publisher rdf:datatype="http://www.w3.org/2001/XMLSchema#string">Institute for Marine and Antarctic Studies (IMAS) - UTAS</dc:publisher>
	<skos:definition xml:lang="en">An inshore regionalisation of Australian waters derived from biological and physical data, including the distribution of demersal fishes, marine plants and invertebrates, sea floor geomorphology and sediments, and oceanographic data. The meso-scale regionalisation was compiled from information supplied to the Australian Government Department of the Environment and Heritage by the relevant State, Northern Territory and Commonwealth marine research and management agencies. The seaward extent for the meso-scale IMCRA coverage is defined by the 200m isobath except where this boundary extends beyond the Australian Exclusive Economic Zone (AEEZ).</skos:definition>
	<dc:source rdf:datatype="http://www.w3.org/2001/XMLSchema#string">Commonwealth of Australia (2006). A Guide to the Integrated Marine and Coastal Regionalisation of Australia Version 4.0. Department of the Environment and Heritage, Canberra, Australia.</dc:source>
	<skos:exactMatch rdf:resource="http://www.environment.gov.au/mapping/rest/services/ogc_services/IMCRA_Mesoscale/MapServer/0/3"/>
</rdf:Description>

<rdf:Description rdf:about="http://seamapaustralia.org.au/def/benthichabitatclassification/class/315">
	<rdf:type rdf:resource="http://www.w3.org/2000/01/rdf-schema#Resource"/>
	<rdf:type rdf:resource="http://www.w3.org/2004/02/skos/core#Concept"/>
	<skos:broader rdf:resource="http://seamapaustralia.org.au/def/benthichabitatclassification/class/309"/>
	<skos:prefLabel xml:lang="en">IMCRA Tiwi Bioregion</skos:prefLabel>
	<dcterms:contributor rdf:resource="http://editor.vocabs.ands.org.au/user/eMII_Finney.Kim_Admin"/>
	<dcterms:created rdf:datatype="http://www.w3.org/2001/XMLSchema#dateTime">2017-06-14T05:31:10Z</dcterms:created>
	<dcterms:creator rdf:resource="http://editor.vocabs.ands.org.au/user/eMII_Finney.Kim_Admin"/>
	<dcterms:modified rdf:datatype="http://www.w3.org/2001/XMLSchema#dateTime">2017-06-27T00:33:01Z</dcterms:modified>
	<dc:publisher rdf:datatype="http://www.w3.org/2001/XMLSchema#string">Institute for Marine and Antarctic Studies (IMAS) - UTAS</dc:publisher>
	<skos:definition xml:lang="en">An inshore regionalisation of Australian waters derived from biological and physical data, including the distribution of demersal fishes, marine plants and invertebrates, sea floor geomorphology and sediments, and oceanographic data. The meso-scale regionalisation was compiled from information supplied to the Australian Government Department of the Environment and Heritage by the relevant State, Northern Territory and Commonwealth marine research and management agencies. The seaward extent for the meso-scale IMCRA coverage is defined by the 200m isobath except where this boundary extends beyond the Australian Exclusive Economic Zone (AEEZ).</skos:definition>
	<dc:source rdf:datatype="http://www.w3.org/2001/XMLSchema#string">Commonwealth of Australia (2006). A Guide to the Integrated Marine and Coastal Regionalisation of Australia Version 4.0. Department of the Environment and Heritage, Canberra, Australia.</dc:source>
	<skos:exactMatch rdf:resource="http://www.environment.gov.au/mapping/rest/services/ogc_services/IMCRA_Mesoscale/MapServer/0/10"/>
</rdf:Description>

<rdf:Description rdf:about="http://seamapaustralia.org.au/def/benthichabitatclassification/class/298">
	<rdf:type rdf:resource="http://www.w3.org/2000/01/rdf-schema#Resource"/>
	<rdf:type rdf:resource="http://www.w3.org/2004/02/skos/core#Concept"/>
	<skos:broader rdf:resource="http://seamapaustralia.org.au/def/benthichabitatclassification/class/191"/>
	<skos:prefLabel xml:lang="en">IMCRA Northern Province</skos:prefLabel>
	<dcterms:contributor rdf:resource="http://editor.vocabs.ands.org.au/user/eMII_Finney.Kim_Admin"/>
	<dcterms:created rdf:datatype="http://www.w3.org/2001/XMLSchema#dateTime">2017-06-14T05:25:36Z</dcterms:created>
	<dcterms:creator rdf:resource="http://editor.vocabs.ands.org.au/user/eMII_Finney.Kim_Admin"/>
	<dcterms:modified rdf:datatype="http://www.w3.org/2001/XMLSchema#dateTime">2017-06-26T23:21:00Z</dcterms:modified>
	<dc:publisher rdf:datatype="http://www.w3.org/2001/XMLSchema#string">Institute for Marine and Antarctic Studies (IMAS) - UTAS</dc:publisher>
	<skos:definition xml:lang="en">An IMCRA provincial bioregion reflects biogeographic patterns in distributions of bottom-dwelling fish. Provincial bioregions were defined for the continental shelf for IMCRA v3.3, and for the continental slope for the National Marine Bioregionalisation using similar analytical techniques. In both cases the distributions of demersal (bottom-dwelling) fish were plotted onto a line divided into equally spaced sections. The number of species in each section and the similarity between sections were calculated using a statistical tool called the Jaccard Index. Where the Jaccard Index changed greatly between sections a boundary was defined indicating differences in species assemblages between regions. Two types of provincial bioregions are defined in the IMCRA benthic bioregionalisation: provinces, which represent regions of biotic endemism; and transitions, which generally occur between the provinces, and are less well-defined mixing areas that capture the overlap of demersal fish species ranges between the provinces.</skos:definition>
	<dc:source rdf:datatype="http://www.w3.org/2001/XMLSchema#string">Commonwealth of Australia (2006). A Guide to the Integrated Marine and Coastal Regionalisation of Australia Version 4.0. Department of the Environment and Heritage, Canberra, Australia.</dc:source>
	<skos:narrower rdf:resource="http://seamapaustralia.org.au/def/benthichabitatclassification/class/303"/>
	<skos:narrower rdf:resource="http://seamapaustralia.org.au/def/benthichabitatclassification/class/307"/>
	<skos:narrower rdf:resource="http://seamapaustralia.org.au/def/benthichabitatclassification/class/306"/>
	<skos:narrower rdf:resource="http://seamapaustralia.org.au/def/benthichabitatclassification/class/304"/>
	<skos:narrower rdf:resource="http://seamapaustralia.org.au/def/benthichabitatclassification/class/301"/>
	<skos:narrower rdf:resource="http://seamapaustralia.org.au/def/benthichabitatclassification/class/305"/>
	<skos:narrower rdf:resource="http://seamapaustralia.org.au/def/benthichabitatclassification/class/308"/>
	<skos:narrower rdf:resource="http://seamapaustralia.org.au/def/benthichabitatclassification/class/300"/>
	<skos:narrower rdf:resource="http://seamapaustralia.org.au/def/benthichabitatclassification/class/299"/>
	<skos:narrower rdf:resource="http://seamapaustralia.org.au/def/benthichabitatclassification/class/302"/>
	<skos:exactMatch rdf:resource="http://www.environment.gov.au/mapping/rest/services/ogc_services/IMCRA_Provincial/MapServer/0/4"/>
</rdf:Description>

<rdf:Description rdf:about="http://seamapaustralia.org.au/def/benthichabitatclassification/class/62">
	<rdf:type rdf:resource="http://www.w3.org/2000/01/rdf-schema#Resource"/>
	<rdf:type rdf:resource="http://www.w3.org/2004/02/skos/core#Concept"/>
	<skos:broader rdf:resource="http://seamapaustralia.org.au/def/benthichabitatclassification/class/43"/>
	<skos:prefLabel xml:lang="en">Siliceous Ooze</skos:prefLabel>
	<dcterms:contributor rdf:resource="http://editor.vocabs.ands.org.au/user/eMII_Finney.Kim_Admin"/>
	<dcterms:created rdf:datatype="http://www.w3.org/2001/XMLSchema#dateTime">2016-11-16T01:00:11Z</dcterms:created>
	<dcterms:creator rdf:resource="http://editor.vocabs.ands.org.au/user/eMII_Finney.Kim_Admin"/>
	<dcterms:modified rdf:datatype="http://www.w3.org/2001/XMLSchema#dateTime">2017-06-27T04:26:33Z</dcterms:modified>
	<dc:publisher rdf:datatype="http://www.w3.org/2001/XMLSchema#string">Institute for Marine and Antarctic Studies (IMAS) - UTAS</dc:publisher>
	<skos:definition xml:lang="en">Oozes that are formed primarily from the siliceous tests, shells or frustules of diatoms, radiolarian or other siliceous plankton. These are typically most abundant at depths deeper than the Carbon Compensation Depth ( ~ 4000 m), because unlike carbonate oozes, silica-based oozes will not dissolve in the cooler and slightly more acidic waters at these depths. </skos:definition>
	<dc:source rdf:datatype="http://www.w3.org/2001/XMLSchema#string">SeaMap Australia National Benthic Habitat Classification Scheme (2017)</dc:source>
	<skos:narrower rdf:resource="http://seamapaustralia.org.au/def/benthichabitatclassification/class/64"/>
	<skos:narrower rdf:resource="http://seamapaustralia.org.au/def/benthichabitatclassification/class/65"/>
</rdf:Description>

<rdf:Description rdf:about="http://seamapaustralia.org.au/def/benthichabitatclassification/class/63">
	<rdf:type rdf:resource="http://www.w3.org/2000/01/rdf-schema#Resource"/>
	<rdf:type rdf:resource="http://www.w3.org/2004/02/skos/core#Concept"/>
	<skos:broader rdf:resource="http://seamapaustralia.org.au/def/benthichabitatclassification/class/43"/>
	<skos:prefLabel xml:lang="en">Carbonate Ooze</skos:prefLabel>
	<dcterms:contributor rdf:resource="http://editor.vocabs.ands.org.au/user/eMII_Finney.Kim_Admin"/>
	<dcterms:created rdf:datatype="http://www.w3.org/2001/XMLSchema#dateTime">2016-11-16T01:00:47Z</dcterms:created>
	<dcterms:creator rdf:resource="http://editor.vocabs.ands.org.au/user/eMII_Finney.Kim_Admin"/>
	<dcterms:modified rdf:datatype="http://www.w3.org/2001/XMLSchema#dateTime">2017-06-27T04:26:09Z</dcterms:modified>
	<dc:publisher rdf:datatype="http://www.w3.org/2001/XMLSchema#string">Institute for Marine and Antarctic Studies (IMAS) - UTAS</dc:publisher>
	<skos:definition xml:lang="en">Oozes that are formed primarily from the calcareous tests, shells or frustules of foraminifera, cocolithophores, pteropods and other calcareous plankton. These are most abundant in water at depths shallower than the Carbon Compensation Depth (~ 4000 m), because below this depth carbonate is usually dissolved given the colder and slightly more acidic waters.</skos:definition>
	<dc:source rdf:datatype="http://www.w3.org/2001/XMLSchema#string">SeaMap Australia National Benthic Habitat Classification Scheme (2017)</dc:source>
	<skos:narrower rdf:resource="http://seamapaustralia.org.au/def/benthichabitatclassification/class/66"/>
	<skos:narrower rdf:resource="http://seamapaustralia.org.au/def/benthichabitatclassification/class/67"/>
	<skos:narrower rdf:resource="http://seamapaustralia.org.au/def/benthichabitatclassification/class/68"/>
</rdf:Description>

<rdf:Description rdf:about="http://seamapaustralia.org.au/def/benthichabitatclassification/class/152">
	<rdf:type rdf:resource="http://www.w3.org/2000/01/rdf-schema#Resource"/>
	<rdf:type rdf:resource="http://www.w3.org/2004/02/skos/core#Concept"/>
	<skos:broader rdf:resource="http://seamapaustralia.org.au/def/benthichabitatclassification/class/34"/>
	<skos:prefLabel xml:lang="en">Unknown Origin</skos:prefLabel>
	<dcterms:contributor rdf:resource="http://editor.vocabs.ands.org.au/user/eMII_Finney.Kim_Admin"/>
	<dcterms:created rdf:datatype="http://www.w3.org/2001/XMLSchema#dateTime">2017-05-23T05:25:09Z</dcterms:created>
	<dcterms:creator rdf:resource="http://editor.vocabs.ands.org.au/user/eMII_Finney.Kim_Admin"/>
	<dcterms:modified rdf:datatype="http://www.w3.org/2001/XMLSchema#dateTime">2017-06-27T04:27:43Z</dcterms:modified>
	<dc:publisher rdf:datatype="http://www.w3.org/2001/XMLSchema#string">  Institute for Marine and Antarctic Studies (IMAS) - UTAS</dc:publisher>
	<dc:source rdf:datatype="http://www.w3.org/2001/XMLSchema#string">SeaMap Australia National Benthic Habitat Classification Scheme (2017)</dc:source>
</rdf:Description>

<rdf:Description rdf:about="https://www.cmecscatalog.org/cmecs/classification/unit/217.html">
	<rdf:type rdf:resource="http://www.w3.org/2000/01/rdf-schema#Resource"/>
</rdf:Description>

<rdf:Description rdf:about="http://seamapaustralia.org.au/def/benthichabitatclassification/class/299">
	<rdf:type rdf:resource="http://www.w3.org/2000/01/rdf-schema#Resource"/>
	<rdf:type rdf:resource="http://www.w3.org/2004/02/skos/core#Concept"/>
	<skos:broader rdf:resource="http://seamapaustralia.org.au/def/benthichabitatclassification/class/298"/>
	<skos:prefLabel xml:lang="en">IMCRA Arafura Bioregion</skos:prefLabel>
	<dcterms:contributor rdf:resource="http://editor.vocabs.ands.org.au/user/eMII_Finney.Kim_Admin"/>
	<dcterms:created rdf:datatype="http://www.w3.org/2001/XMLSchema#dateTime">2017-06-14T05:25:57Z</dcterms:created>
	<dcterms:creator rdf:resource="http://editor.vocabs.ands.org.au/user/eMII_Finney.Kim_Admin"/>
	<dcterms:modified rdf:datatype="http://www.w3.org/2001/XMLSchema#dateTime">2017-06-26T23:24:26Z</dcterms:modified>
	<dc:publisher rdf:datatype="http://www.w3.org/2001/XMLSchema#string">Institute for Marine and Antarctic Studies (IMAS) - UTAS</dc:publisher>
	<skos:definition xml:lang="en">An inshore regionalisation of Australian waters derived from biological and physical data, including the distribution of demersal fishes, marine plants and invertebrates, sea floor geomorphology and sediments, and oceanographic data. The meso-scale regionalisation was compiled from information supplied to the Australian Government Department of the Environment and Heritage by the relevant State, Northern Territory and Commonwealth marine research and management agencies. The seaward extent for the meso-scale IMCRA coverage is defined by the 200m isobath except where this boundary extends beyond the Australian Exclusive Economic Zone (AEEZ).</skos:definition>
	<dc:source rdf:datatype="http://www.w3.org/2001/XMLSchema#string">Commonwealth of Australia (2006). A Guide to the Integrated Marine and Coastal Regionalisation of Australia Version 4.0. Department of the Environment and Heritage, Canberra, Australia.</dc:source>
	<skos:exactMatch rdf:resource="http://www.environment.gov.au/mapping/rest/services/ogc_services/IMCRA_Mesoscale/MapServer/0/1"/>
</rdf:Description>

<rdf:Description rdf:about="http://www.w3.org/2004/02/skos/core#exactMatch">
	<rdf:type rdf:resource="http://www.w3.org/1999/02/22-rdf-syntax-ns#Property"/>
	<rdf:type rdf:resource="http://www.w3.org/2000/01/rdf-schema#Resource"/>
	<rdfs:subPropertyOf rdf:resource="http://www.w3.org/2004/02/skos/core#exactMatch"/>
</rdf:Description>

<rdf:Description rdf:about="http://www.environment.gov.au/mapping/rest/services/ogc_services/IMCRA_Mesoscale/MapServer/0/1">
	<rdf:type rdf:resource="http://www.w3.org/2000/01/rdf-schema#Resource"/>
</rdf:Description>

<rdf:Description rdf:about="http://seamapaustralia.org.au/def/benthichabitatclassification/class/302">
	<rdf:type rdf:resource="http://www.w3.org/2000/01/rdf-schema#Resource"/>
	<rdf:type rdf:resource="http://www.w3.org/2004/02/skos/core#Concept"/>
	<skos:broader rdf:resource="http://seamapaustralia.org.au/def/benthichabitatclassification/class/298"/>
	<skos:prefLabel xml:lang="en">IMCRA Arnhem Wessel Bioregion</skos:prefLabel>
	<dcterms:contributor rdf:resource="http://editor.vocabs.ands.org.au/user/eMII_Finney.Kim_Admin"/>
	<dcterms:created rdf:datatype="http://www.w3.org/2001/XMLSchema#dateTime">2017-06-14T05:27:06Z</dcterms:created>
	<dcterms:creator rdf:resource="http://editor.vocabs.ands.org.au/user/eMII_Finney.Kim_Admin"/>
	<dcterms:modified rdf:datatype="http://www.w3.org/2001/XMLSchema#dateTime">2017-06-26T23:25:29Z</dcterms:modified>
	<dc:publisher rdf:datatype="http://www.w3.org/2001/XMLSchema#string">Institute for Marine and Antarctic Studies (IMAS) - UTAS</dc:publisher>
	<skos:definition xml:lang="en">An inshore regionalisation of Australian waters derived from biological and physical data, including the distribution of demersal fishes, marine plants and invertebrates, sea floor geomorphology and sediments, and oceanographic data. The meso-scale regionalisation was compiled from information supplied to the Australian Government Department of the Environment and Heritage by the relevant State, Northern Territory and Commonwealth marine research and management agencies. The seaward extent for the meso-scale IMCRA coverage is defined by the 200m isobath except where this boundary extends beyond the Australian Exclusive Economic Zone (AEEZ).</skos:definition>
	<dc:source rdf:datatype="http://www.w3.org/2001/XMLSchema#string">Commonwealth of Australia (2006). A Guide to the Integrated Marine and Coastal Regionalisation of Australia Version 4.0. Department of the Environment and Heritage, Canberra, Australia.</dc:source>
	<skos:exactMatch rdf:resource="http://www.environment.gov.au/mapping/rest/services/ogc_services/IMCRA_Mesoscale/MapServer/0/9"/>
</rdf:Description>

<rdf:Description rdf:about="http://www.environment.gov.au/mapping/rest/services/ogc_services/IMCRA_Mesoscale/MapServer/0/9">
	<rdf:type rdf:resource="http://www.w3.org/2000/01/rdf-schema#Resource"/>
</rdf:Description>

<rdf:Description rdf:about="http://www.environment.gov.au/mapping/rest/services/ogc_services/IMCRA_Mesoscale/MapServer/0/7">
	<rdf:type rdf:resource="http://www.w3.org/2000/01/rdf-schema#Resource"/>
</rdf:Description>

<rdf:Description rdf:about="http://www.environment.gov.au/mapping/rest/services/ogc_services/IMCRA_Mesoscale/MapServer/0/8">
	<rdf:type rdf:resource="http://www.w3.org/2000/01/rdf-schema#Resource"/>
</rdf:Description>

<rdf:Description rdf:about="http://www.environment.gov.au/mapping/rest/services/ogc_services/IMCRA_Mesoscale/MapServer/0/14">
	<rdf:type rdf:resource="http://www.w3.org/2000/01/rdf-schema#Resource"/>
</rdf:Description>

<rdf:Description rdf:about="http://www.environment.gov.au/mapping/rest/services/ogc_services/IMCRA_Mesoscale/MapServer/0/16">
	<rdf:type rdf:resource="http://www.w3.org/2000/01/rdf-schema#Resource"/>
</rdf:Description>

<rdf:Description rdf:about="http://www.environment.gov.au/mapping/rest/services/ogc_services/IMCRA_Mesoscale/MapServer/0/19">
	<rdf:type rdf:resource="http://www.w3.org/2000/01/rdf-schema#Resource"/>
</rdf:Description>

<rdf:Description rdf:about="http://www.environment.gov.au/mapping/rest/services/ogc_services/IMCRA_Mesoscale/MapServer/0/12">
	<rdf:type rdf:resource="http://www.w3.org/2000/01/rdf-schema#Resource"/>
</rdf:Description>

<rdf:Description rdf:about="http://www.environment.gov.au/mapping/rest/services/ogc_services/IMCRA_Mesoscale/MapServer/0/21">
	<rdf:type rdf:resource="http://www.w3.org/2000/01/rdf-schema#Resource"/>
</rdf:Description>

<rdf:Description rdf:about="http://www.environment.gov.au/mapping/rest/services/ogc_services/IMCRA_Mesoscale/MapServer/0/6">
	<rdf:type rdf:resource="http://www.w3.org/2000/01/rdf-schema#Resource"/>
</rdf:Description>

<rdf:Description rdf:about="http://www.environment.gov.au/mapping/rest/services/ogc_services/IMCRA_Mesoscale/MapServer/0/13">
	<rdf:type rdf:resource="http://www.w3.org/2000/01/rdf-schema#Resource"/>
</rdf:Description>

<rdf:Description rdf:about="http://www.environment.gov.au/mapping/rest/services/ogc_services/IMCRA_Mesoscale/MapServer/0/11">
	<rdf:type rdf:resource="http://www.w3.org/2000/01/rdf-schema#Resource"/>
</rdf:Description>

<rdf:Description rdf:about="http://www.environment.gov.au/mapping/rest/services/ogc_services/IMCRA_Mesoscale/MapServer/0/18">
	<rdf:type rdf:resource="http://www.w3.org/2000/01/rdf-schema#Resource"/>
</rdf:Description>

<rdf:Description rdf:about="http://www.environment.gov.au/mapping/rest/services/ogc_services/IMCRA_Mesoscale/MapServer/0/24">
	<rdf:type rdf:resource="http://www.w3.org/2000/01/rdf-schema#Resource"/>
</rdf:Description>

<rdf:Description rdf:about="http://www.environment.gov.au/mapping/rest/services/ogc_services/IMCRA_Mesoscale/MapServer/0/3">
	<rdf:type rdf:resource="http://www.w3.org/2000/01/rdf-schema#Resource"/>
</rdf:Description>

<rdf:Description rdf:about="http://www.environment.gov.au/mapping/rest/services/ogc_services/IMCRA_Mesoscale/MapServer/0/10">
	<rdf:type rdf:resource="http://www.w3.org/2000/01/rdf-schema#Resource"/>
</rdf:Description>

<rdf:Description rdf:about="http://www.environment.gov.au/mapping/rest/services/ogc_services/IMCRA_Provincial/MapServer/0/4">
	<rdf:type rdf:resource="http://www.w3.org/2000/01/rdf-schema#Resource"/>
</rdf:Description>

<rdf:Description rdf:about="http://www.environment.gov.au/mapping/rest/services/ogc_services/IMCRA_Provincial/MapServer/0/13">
	<rdf:type rdf:resource="http://www.w3.org/2000/01/rdf-schema#Resource"/>
</rdf:Description>

<rdf:Description rdf:about="http://seamapaustralia.org.au/def/benthichabitatclassification/class/72">
	<rdf:type rdf:resource="http://www.w3.org/2000/01/rdf-schema#Resource"/>
	<rdf:type rdf:resource="http://www.w3.org/2004/02/skos/core#Concept"/>
	<skos:broader rdf:resource="http://seamapaustralia.org.au/def/benthichabitatclassification/class/71"/>
	<skos:prefLabel xml:lang="en">Vegetation</skos:prefLabel>
	<dcterms:contributor rdf:resource="http://editor.vocabs.ands.org.au/user/eMII_Finney.Kim_Admin"/>
	<dcterms:created rdf:datatype="http://www.w3.org/2001/XMLSchema#dateTime">2016-11-16T01:12:04Z</dcterms:created>
	<dcterms:creator rdf:resource="http://editor.vocabs.ands.org.au/user/eMII_Finney.Kim_Admin"/>
	<dcterms:modified rdf:datatype="http://www.w3.org/2001/XMLSchema#dateTime">2017-06-27T04:16:54Z</dcterms:modified>
	<dc:publisher rdf:datatype="http://www.w3.org/2001/XMLSchema#string">Institute for Marine and Antarctic Studies (IMAS) - UTAS</dc:publisher>
	<skos:definition xml:lang="en">A habitat where the dominant biota are plants or algae. </skos:definition>
	<dc:source rdf:datatype="http://www.w3.org/2001/XMLSchema#string"> SeaMap Australia National Benthic Habitat Classification Scheme (2017)</dc:source>
	<skos:narrower rdf:resource="http://seamapaustralia.org.au/def/benthichabitatclassification/class/320"/>
	<skos:narrower rdf:resource="http://seamapaustralia.org.au/def/benthichabitatclassification/class/75"/>
	<skos:narrower rdf:resource="http://seamapaustralia.org.au/def/benthichabitatclassification/class/76"/>
</rdf:Description>

<rdf:Description rdf:about="http://seamapaustralia.org.au/def/benthichabitatclassification/class/75">
	<rdf:type rdf:resource="http://www.w3.org/2000/01/rdf-schema#Resource"/>
	<rdf:type rdf:resource="http://www.w3.org/2004/02/skos/core#Concept"/>
	<skos:broader rdf:resource="http://seamapaustralia.org.au/def/benthichabitatclassification/class/72"/>
	<skos:prefLabel xml:lang="en">Wetland Vegetation</skos:prefLabel>
	<dcterms:contributor rdf:resource="http://editor.vocabs.ands.org.au/user/eMII_Finney.Kim_Admin"/>
	<dcterms:created rdf:datatype="http://www.w3.org/2001/XMLSchema#dateTime">2016-11-16T01:15:56Z</dcterms:created>
	<dcterms:creator rdf:resource="http://editor.vocabs.ands.org.au/user/eMII_Finney.Kim_Admin"/>
	<dcterms:modified rdf:datatype="http://www.w3.org/2001/XMLSchema#dateTime">2017-06-27T04:17:23Z</dcterms:modified>
	<dc:publisher rdf:datatype="http://www.w3.org/2001/XMLSchema#string">Institute for Marine and Antarctic Studies (IMAS) - UTAS</dc:publisher>
	<skos:definition xml:lang="en">This term describes vegetation that exists exclusively in areas that are permanently water logged, but may only be inundated with saline or brackish water periodically or occasionally. This includes areas such as marshes, tidal flats and river estuaries, but excludes oceans.  At the Highest Astronomical Tide (HAT) mark, vegetation in this class is never fully submerged and typically only the roots are immersed.</skos:definition>
	<dc:source rdf:datatype="http://www.w3.org/2001/XMLSchema#string">SeaMap Australia National Benthic Habitat Classification Scheme (2017)</dc:source>
	<skos:narrower rdf:resource="http://seamapaustralia.org.au/def/benthichabitatclassification/class/321"/>
	<skos:narrower rdf:resource="http://seamapaustralia.org.au/def/benthichabitatclassification/class/82"/>
	<skos:narrower rdf:resource="http://seamapaustralia.org.au/def/benthichabitatclassification/class/83"/>
</rdf:Description>

<rdf:Description rdf:about="http://seamapaustralia.org.au/def/benthichabitatclassification/class/322">
	<rdf:type rdf:resource="http://www.w3.org/2000/01/rdf-schema#Resource"/>
	<rdf:type rdf:resource="http://www.w3.org/2004/02/skos/core#Concept"/>
	<skos:broader rdf:resource="http://seamapaustralia.org.au/def/benthichabitatclassification/class/76"/>
	<skos:prefLabel xml:lang="en">Mixed Macrophytes</skos:prefLabel>
	<dcterms:contributor rdf:resource="http://editor.vocabs.ands.org.au/user/eMII_Finney.Kim_Admin"/>
	<dcterms:created rdf:datatype="http://www.w3.org/2001/XMLSchema#dateTime">2017-06-27T01:01:25Z</dcterms:created>
	<dcterms:creator rdf:resource="http://editor.vocabs.ands.org.au/user/eMII_Finney.Kim_Admin"/>
	<dcterms:modified rdf:datatype="http://www.w3.org/2001/XMLSchema#dateTime">2017-06-27T03:15:54Z</dcterms:modified>
	<skos:definition xml:lang="en">A habitat where the dominance of a Macrophyte group (Macroalgae, Seagrass) cannot be identified, or where the composition/biomass/surface coverage of the second-most dominant group lies within 30 % margin of the most-dominant group.</skos:definition>
</rdf:Description>

<rdf:Description rdf:about="http://seamapaustralia.org.au/def/benthichabitatclassification/class/76">
	<rdf:type rdf:resource="http://www.w3.org/2000/01/rdf-schema#Resource"/>
	<rdf:type rdf:resource="http://www.w3.org/2004/02/skos/core#Concept"/>
	<skos:broader rdf:resource="http://seamapaustralia.org.au/def/benthichabitatclassification/class/72"/>
	<skos:prefLabel xml:lang="en">Macrophytes (Non Wetland)</skos:prefLabel>
	<dcterms:contributor rdf:resource="http://editor.vocabs.ands.org.au/user/eMII_Finney.Kim_Admin"/>
	<dcterms:created rdf:datatype="http://www.w3.org/2001/XMLSchema#dateTime">2016-11-16T01:16:26Z</dcterms:created>
	<dcterms:creator rdf:resource="http://editor.vocabs.ands.org.au/user/eMII_Finney.Kim_Admin"/>
	<dcterms:modified rdf:datatype="http://www.w3.org/2001/XMLSchema#dateTime">2017-06-27T04:17:01Z</dcterms:modified>
	<dc:publisher rdf:datatype="http://www.w3.org/2001/XMLSchema#string">Institute for Marine and Antarctic Studies (IMAS) - UTAS</dc:publisher>
	<skos:definition xml:lang="en">This term describes vegetation that exists in areas that are inundated either permanently or with regular tidal flow. At the Highest Astronomical Tide (HAT) mark, this vegetation is fully submerged. </skos:definition>
	<dc:source rdf:datatype="http://www.w3.org/2001/XMLSchema#string">SeaMap Australia National Benthic Habitat Classification Scheme (2017)</dc:source>
	<skos:narrower rdf:resource="http://seamapaustralia.org.au/def/benthichabitatclassification/class/322"/>
	<skos:narrower rdf:resource="http://seamapaustralia.org.au/def/benthichabitatclassification/class/84"/>
	<skos:narrower rdf:resource="http://seamapaustralia.org.au/def/benthichabitatclassification/class/85"/>
</rdf:Description>

<rdf:Description rdf:about="http://seamapaustralia.org.au/def/benthichabitatclassification/class/74">
	<rdf:type rdf:resource="http://www.w3.org/2000/01/rdf-schema#Resource"/>
	<rdf:type rdf:resource="http://www.w3.org/2004/02/skos/core#Concept"/>
	<skos:broader rdf:resource="http://seamapaustralia.org.au/def/benthichabitatclassification/class/71"/>
	<skos:prefLabel xml:lang="en">Microbes</skos:prefLabel>
	<dcterms:contributor rdf:resource="http://editor.vocabs.ands.org.au/user/eMII_Finney.Kim_Admin"/>
	<dcterms:created rdf:datatype="http://www.w3.org/2001/XMLSchema#dateTime">2016-11-16T01:13:29Z</dcterms:created>
	<dcterms:creator rdf:resource="http://editor.vocabs.ands.org.au/user/eMII_Finney.Kim_Admin"/>
	<dcterms:modified rdf:datatype="http://www.w3.org/2001/XMLSchema#dateTime">2017-06-27T04:16:23Z</dcterms:modified>
	<dc:publisher rdf:datatype="http://www.w3.org/2001/XMLSchema#string">Institute for Marine and Antarctic Studies (IMAS) - UTAS</dc:publisher>
	<skos:definition xml:lang="en">Areas dominated by microbes that form a soft or hard structure visible to the eye. Soft structures are usually formed through accumulations of conspecifics and other microbes into a matrix that appears as strands, a thin film, or a thicker mat. Hard structures generally form through secretions and entrapment of minerals and sediments.</skos:definition>
	<dc:source rdf:datatype="http://www.w3.org/2001/XMLSchema#string"> SeaMap Australia National Benthic Habitat Classification Scheme (2017)</dc:source>
	<skos:narrower rdf:resource="http://seamapaustralia.org.au/def/benthichabitatclassification/class/323"/>
	<skos:narrower rdf:resource="http://seamapaustralia.org.au/def/benthichabitatclassification/class/161"/>
	<skos:narrower rdf:resource="http://seamapaustralia.org.au/def/benthichabitatclassification/class/162"/>
	<skos:narrower rdf:resource="http://seamapaustralia.org.au/def/benthichabitatclassification/class/163"/>
</rdf:Description>

<rdf:Description rdf:about="http://seamapaustralia.org.au/def/benthichabitatclassification/class/64">
	<rdf:type rdf:resource="http://www.w3.org/2000/01/rdf-schema#Resource"/>
	<rdf:type rdf:resource="http://www.w3.org/2004/02/skos/core#Concept"/>
	<skos:broader rdf:resource="http://seamapaustralia.org.au/def/benthichabitatclassification/class/62"/>
	<skos:prefLabel xml:lang="en">Radiolaria</skos:prefLabel>
	<dcterms:contributor rdf:resource="http://editor.vocabs.ands.org.au/user/eMII_Finney.Kim_Admin"/>
	<dcterms:created rdf:datatype="http://www.w3.org/2001/XMLSchema#dateTime">2016-11-16T01:01:27Z</dcterms:created>
	<dcterms:creator rdf:resource="http://editor.vocabs.ands.org.au/user/eMII_Finney.Kim_Admin"/>
	<dcterms:modified rdf:datatype="http://www.w3.org/2001/XMLSchema#dateTime">2017-06-27T04:26:46Z</dcterms:modified>
	<dc:publisher rdf:datatype="http://www.w3.org/2001/XMLSchema#string">Institute for Marine and Antarctic Studies (IMAS) - UTAS</dc:publisher>
	<skos:definition xml:lang="en">Siliceous oozes where the composition is dominated by the test and shells of radiolarian.</skos:definition>
	<dc:source rdf:datatype="http://www.w3.org/2001/XMLSchema#string">SeaMap Australia National Benthic Habitat Classification Scheme (2017)</dc:source>
</rdf:Description>

<rdf:Description rdf:about="http://seamapaustralia.org.au/def/benthichabitatclassification/class/65">
	<rdf:type rdf:resource="http://www.w3.org/2000/01/rdf-schema#Resource"/>
	<rdf:type rdf:resource="http://www.w3.org/2004/02/skos/core#Concept"/>
	<skos:broader rdf:resource="http://seamapaustralia.org.au/def/benthichabitatclassification/class/62"/>
	<skos:prefLabel xml:lang="en">Diatoms</skos:prefLabel>
	<dcterms:contributor rdf:resource="http://editor.vocabs.ands.org.au/user/eMII_Finney.Kim_Admin"/>
	<dcterms:created rdf:datatype="http://www.w3.org/2001/XMLSchema#dateTime">2016-11-16T01:02:00Z</dcterms:created>
	<dcterms:creator rdf:resource="http://editor.vocabs.ands.org.au/user/eMII_Finney.Kim_Admin"/>
	<dcterms:modified rdf:datatype="http://www.w3.org/2001/XMLSchema#dateTime">2017-06-27T04:26:40Z</dcterms:modified>
	<dc:publisher rdf:datatype="http://www.w3.org/2001/XMLSchema#string">Institute for Marine and Antarctic Studies (IMAS) - UTAS</dc:publisher>
	<skos:definition xml:lang="en">Siliceous oozes where the composition is dominated by the test and shells of diatoms.</skos:definition>
	<dc:source rdf:datatype="http://www.w3.org/2001/XMLSchema#string">SeaMap Australia National Benthic Habitat Classification Scheme (2017)</dc:source>
</rdf:Description>

<rdf:Description rdf:about="http://seamapaustralia.org.au/def/benthichabitatclassification/class/66">
	<rdf:type rdf:resource="http://www.w3.org/2000/01/rdf-schema#Resource"/>
	<rdf:type rdf:resource="http://www.w3.org/2004/02/skos/core#Concept"/>
	<skos:broader rdf:resource="http://seamapaustralia.org.au/def/benthichabitatclassification/class/63"/>
	<skos:prefLabel xml:lang="en">Foraminifera</skos:prefLabel>
	<dcterms:contributor rdf:resource="http://editor.vocabs.ands.org.au/user/eMII_Finney.Kim_Admin"/>
	<dcterms:created rdf:datatype="http://www.w3.org/2001/XMLSchema#dateTime">2016-11-16T01:03:04Z</dcterms:created>
	<dcterms:creator rdf:resource="http://editor.vocabs.ands.org.au/user/eMII_Finney.Kim_Admin"/>
	<dcterms:modified rdf:datatype="http://www.w3.org/2001/XMLSchema#dateTime">2017-06-27T04:26:18Z</dcterms:modified>
	<dc:publisher rdf:datatype="http://www.w3.org/2001/XMLSchema#string">Institute for Marine and Antarctic Studies (IMAS) - UTAS</dc:publisher>
	<skos:definition xml:lang="en">Carbonate oozes dominated by the tests and shells of foraminifera.</skos:definition>
	<dc:source rdf:datatype="http://www.w3.org/2001/XMLSchema#string">SeaMap Australia National Benthic Habitat Classification Scheme (2017)</dc:source>
</rdf:Description>

<rdf:Description rdf:about="http://seamapaustralia.org.au/def/benthichabitatclassification/class/67">
	<rdf:type rdf:resource="http://www.w3.org/2000/01/rdf-schema#Resource"/>
	<rdf:type rdf:resource="http://www.w3.org/2004/02/skos/core#Concept"/>
	<skos:broader rdf:resource="http://seamapaustralia.org.au/def/benthichabitatclassification/class/63"/>
	<skos:prefLabel xml:lang="en">Coccolithophore</skos:prefLabel>
	<dcterms:contributor rdf:resource="http://editor.vocabs.ands.org.au/user/eMII_Finney.Kim_Admin"/>
	<dcterms:created rdf:datatype="http://www.w3.org/2001/XMLSchema#dateTime">2016-11-16T01:04:02Z</dcterms:created>
	<dcterms:creator rdf:resource="http://editor.vocabs.ands.org.au/user/eMII_Finney.Kim_Admin"/>
	<dcterms:modified rdf:datatype="http://www.w3.org/2001/XMLSchema#dateTime">2017-06-27T04:26:14Z</dcterms:modified>
	<dc:publisher rdf:datatype="http://www.w3.org/2001/XMLSchema#string">Institute for Marine and Antarctic Studies (IMAS) - UTAS</dc:publisher>
	<skos:definition xml:lang="en">Carbonate oozes dominated by the tests and shells of cocolithophores.</skos:definition>
	<dc:source rdf:datatype="http://www.w3.org/2001/XMLSchema#string">SeaMap Australia National Benthic Habitat Classification Scheme (2017)</dc:source>
</rdf:Description>

<rdf:Description rdf:about="http://seamapaustralia.org.au/def/benthichabitatclassification/class/68">
	<rdf:type rdf:resource="http://www.w3.org/2000/01/rdf-schema#Resource"/>
	<rdf:type rdf:resource="http://www.w3.org/2004/02/skos/core#Concept"/>
	<skos:broader rdf:resource="http://seamapaustralia.org.au/def/benthichabitatclassification/class/63"/>
	<skos:prefLabel xml:lang="en">Pteropod</skos:prefLabel>
	<dcterms:contributor rdf:resource="http://editor.vocabs.ands.org.au/user/eMII_Finney.Kim_Admin"/>
	<dcterms:created rdf:datatype="http://www.w3.org/2001/XMLSchema#dateTime">2016-11-16T01:04:45Z</dcterms:created>
	<dcterms:creator rdf:resource="http://editor.vocabs.ands.org.au/user/eMII_Finney.Kim_Admin"/>
	<dcterms:modified rdf:datatype="http://www.w3.org/2001/XMLSchema#dateTime">2017-06-27T04:26:27Z</dcterms:modified>
	<dc:publisher rdf:datatype="http://www.w3.org/2001/XMLSchema#string">Institute for Marine and Antarctic Studies (IMAS) - UTAS</dc:publisher>
	<skos:definition xml:lang="en">Carbonate oozes dominated by the tests and shells of pteropods.</skos:definition>
	<dc:source rdf:datatype="http://www.w3.org/2001/XMLSchema#string">SeaMap Australia National Benthic Habitat Classification Scheme (2017)</dc:source>
</rdf:Description>

<rdf:Description rdf:about="https://www.cmecscatalog.org/cmecs/classification/dComponent/2.html">
	<rdf:type rdf:resource="http://www.w3.org/2000/01/rdf-schema#Resource"/>
</rdf:Description>

<rdf:Description rdf:about="http://seamapaustralia.org.au/def/benthichabitatclassification/class/70">
	<rdf:type rdf:resource="http://www.w3.org/2000/01/rdf-schema#Resource"/>
	<rdf:type rdf:resource="http://www.w3.org/2004/02/skos/core#Concept"/>
	<skos:broader rdf:resource="http://seamapaustralia.org.au/def/benthichabitatclassification/class/69"/>
	<skos:prefLabel xml:lang="en">Biota Not Assessed (NA)</skos:prefLabel>
	<dcterms:contributor rdf:resource="http://editor.vocabs.ands.org.au/user/eMII_Finney.Kim_Admin"/>
	<dcterms:created rdf:datatype="http://www.w3.org/2001/XMLSchema#dateTime">2016-11-16T01:10:25Z</dcterms:created>
	<dcterms:creator rdf:resource="http://editor.vocabs.ands.org.au/user/eMII_Finney.Kim_Admin"/>
	<dcterms:modified rdf:datatype="http://www.w3.org/2001/XMLSchema#dateTime">2017-06-27T04:17:46Z</dcterms:modified>
	<dc:publisher rdf:datatype="http://www.w3.org/2001/XMLSchema#string">Institute for Marine and Antarctic Studies (IMAS) - UTAS</dc:publisher>
	<skos:definition xml:lang="en">An area where mapping has occurred, however the presence or absence of biota was not assessed. An NA classification is distinct from an Unknown classification in that an Unknown implies an assessment was made however a classification was not possible for any reason (e.g. inadequate resolution).</skos:definition>
	<dc:source rdf:datatype="http://www.w3.org/2001/XMLSchema#string">SeaMap Australia National Benthic Habitat Classification Scheme (2017)</dc:source>
</rdf:Description>

<rdf:Description rdf:about="http://seamapaustralia.org.au/def/benthichabitatclassification/class/71">
	<rdf:type rdf:resource="http://www.w3.org/2000/01/rdf-schema#Resource"/>
	<rdf:type rdf:resource="http://www.w3.org/2004/02/skos/core#Concept"/>
	<skos:broader rdf:resource="http://seamapaustralia.org.au/def/benthichabitatclassification/class/69"/>
	<skos:prefLabel xml:lang="en">Biota Present</skos:prefLabel>
	<dcterms:contributor rdf:resource="http://editor.vocabs.ands.org.au/user/eMII_Finney.Kim_Admin"/>
	<dcterms:created rdf:datatype="http://www.w3.org/2001/XMLSchema#dateTime">2016-11-16T01:11:29Z</dcterms:created>
	<dcterms:creator rdf:resource="http://editor.vocabs.ands.org.au/user/eMII_Finney.Kim_Admin"/>
	<dcterms:modified rdf:datatype="http://www.w3.org/2001/XMLSchema#dateTime">2017-06-27T04:14:41Z</dcterms:modified>
	<dc:publisher rdf:datatype="http://www.w3.org/2001/XMLSchema#string">Institute for Marine and Antarctic Studies (IMAS) - UTAS</dc:publisher>
	<skos:definition xml:lang="en">Areas where benthic biota are present in the observational unit and account for a total ≥ 5 % of the substratum surface/composition/biomass.</skos:definition>
	<dc:source rdf:datatype="http://www.w3.org/2001/XMLSchema#string">SeaMap Australia National Benthic Habitat Classification Scheme (2017)</dc:source>
	<skos:narrower rdf:resource="http://seamapaustralia.org.au/def/benthichabitatclassification/class/318"/>
	<skos:narrower rdf:resource="http://seamapaustralia.org.au/def/benthichabitatclassification/class/72"/>
	<skos:narrower rdf:resource="http://seamapaustralia.org.au/def/benthichabitatclassification/class/74"/>
	<skos:narrower rdf:resource="http://seamapaustralia.org.au/def/benthichabitatclassification/class/73"/>
	<skos:narrower rdf:resource="http://seamapaustralia.org.au/def/benthichabitatclassification/class/319"/>
</rdf:Description>

<rdf:Description rdf:about="http://seamapaustralia.org.au/def/benthichabitatclassification/class/73">
	<rdf:type rdf:resource="http://www.w3.org/2000/01/rdf-schema#Resource"/>
	<rdf:type rdf:resource="http://www.w3.org/2004/02/skos/core#Concept"/>
	<skos:broader rdf:resource="http://seamapaustralia.org.au/def/benthichabitatclassification/class/71"/>
	<skos:prefLabel xml:lang="en">Invertebrates</skos:prefLabel>
	<dcterms:contributor rdf:resource="http://editor.vocabs.ands.org.au/user/eMII_Finney.Kim_Admin"/>
	<dcterms:created rdf:datatype="http://www.w3.org/2001/XMLSchema#dateTime">2016-11-16T01:12:49Z</dcterms:created>
	<dcterms:creator rdf:resource="http://editor.vocabs.ands.org.au/user/eMII_Finney.Kim_Admin"/>
	<dcterms:modified rdf:datatype="http://www.w3.org/2001/XMLSchema#dateTime">2017-06-27T04:14:46Z</dcterms:modified>
	<dc:publisher rdf:datatype="http://www.w3.org/2001/XMLSchema#string">Institute for Marine and Antarctic Studies (IMAS) - UTAS</dc:publisher>
	<skos:definition xml:lang="en">A habitat dominated by benthic macrofauna that do not have a backbone, i.e. are not vertebrates.</skos:definition>
	<dc:source rdf:datatype="http://www.w3.org/2001/XMLSchema#string"> SeaMap Australia National Benthic Habitat Classification Scheme (2017)</dc:source>
	<skos:narrower rdf:resource="http://seamapaustralia.org.au/def/benthichabitatclassification/class/80"/>
	<skos:narrower rdf:resource="http://seamapaustralia.org.au/def/benthichabitatclassification/class/324"/>
	<skos:narrower rdf:resource="http://seamapaustralia.org.au/def/benthichabitatclassification/class/78"/>
	<skos:narrower rdf:resource="http://seamapaustralia.org.au/def/benthichabitatclassification/class/79"/>
</rdf:Description>

<rdf:Description rdf:about="http://seamapaustralia.org.au/def/benthichabitatclassification/class/339">
	<rdf:type rdf:resource="http://www.w3.org/2000/01/rdf-schema#Resource"/>
	<rdf:type rdf:resource="http://www.w3.org/2004/02/skos/core#Concept"/>
	<skos:broader rdf:resource="http://seamapaustralia.org.au/def/benthichabitatclassification/class/337"/>
	<skos:prefLabel xml:lang="en">IMCRA Central Reef</skos:prefLabel>
	<dcterms:contributor rdf:resource="http://editor.vocabs.ands.org.au/user/eMII_Finney.Kim_Admin"/>
	<dcterms:created rdf:datatype="http://www.w3.org/2001/XMLSchema#dateTime">2017-06-27T03:29:39Z</dcterms:created>
	<dcterms:creator rdf:resource="http://editor.vocabs.ands.org.au/user/eMII_Finney.Kim_Admin"/>
	<dcterms:modified rdf:datatype="http://www.w3.org/2001/XMLSchema#dateTime">2017-06-27T03:58:00Z</dcterms:modified>
	<dc:publisher rdf:datatype="http://www.w3.org/2001/XMLSchema#string">Institute for Marine and Antarctic Studies (IMAS) - UTAS</dc:publisher>
	<skos:definition xml:lang="en">An inshore regionalisation of Australian waters derived from biological and physical data, including the distribution of demersal fishes, marine plants and invertebrates, sea floor geomorphology and sediments, and oceanographic data. The meso-scale regionalisation was compiled from information supplied to the Australian Government Department of the Environment and Heritage by the relevant State, Northern Territory and Commonwealth marine research and management agencies. The seaward extent for the meso-scale IMCRA coverage is defined by the 200m isobath except where this boundary extends beyond the Australian Exclusive Economic Zone (AEEZ).</skos:definition>
	<dc:source rdf:datatype="http://www.w3.org/2001/XMLSchema#string">Commonwealth of Australia (2006). A Guide to the Integrated Marine and Coastal Regionalisation of Australia Version 4.0. Department of the Environment and Heritage, Canberra, Australia.</dc:source>
	<skos:exactMatch rdf:resource="http://www.environment.gov.au/mapping/rest/services/ogc_services/IMCRA_Mesoscale/MapServer/0/23"/>
</rdf:Description>

<rdf:Description rdf:about="http://seamapaustralia.org.au/def/benthichabitatclassification/class/158">
	<rdf:type rdf:resource="http://www.w3.org/2000/01/rdf-schema#Resource"/>
	<rdf:type rdf:resource="http://www.w3.org/2004/02/skos/core#Concept"/>
	<skos:broader rdf:resource="http://seamapaustralia.org.au/def/benthichabitatclassification/class/78"/>
	<skos:prefLabel xml:lang="en">Worm Biota</skos:prefLabel>
	<dcterms:contributor rdf:resource="http://editor.vocabs.ands.org.au/user/eMII_Finney.Kim_Admin"/>
	<dcterms:created rdf:datatype="http://www.w3.org/2001/XMLSchema#dateTime">2017-05-23T05:49:42Z</dcterms:created>
	<dcterms:creator rdf:resource="http://editor.vocabs.ands.org.au/user/eMII_Finney.Kim_Admin"/>
	<dcterms:modified rdf:datatype="http://www.w3.org/2001/XMLSchema#dateTime">2017-06-27T04:15:42Z</dcterms:modified>
	<dc:publisher rdf:datatype="http://www.w3.org/2001/XMLSchema#string">Institute for Marine and Antarctic Studies (IMAS) - UTAS</dc:publisher>
	<skos:definition xml:lang="en">An area dominated by sessile marine worms, in particular tube dwelling polychaetes. These sedentary polychaetes have highly differentiated bodies and most live in secreted tubes attached to the seafloor. </skos:definition>
	<dc:source rdf:datatype="http://www.w3.org/2001/XMLSchema#string">SeaMap Australia National Benthic Habitat Classification Scheme (2017)</dc:source>
</rdf:Description>

<rdf:Description rdf:about="http://seamapaustralia.org.au/def/benthichabitatclassification/class/78">
	<rdf:type rdf:resource="http://www.w3.org/2000/01/rdf-schema#Resource"/>
	<rdf:type rdf:resource="http://www.w3.org/2004/02/skos/core#Concept"/>
	<skos:broader rdf:resource="http://seamapaustralia.org.au/def/benthichabitatclassification/class/73"/>
	<skos:prefLabel xml:lang="en">Non-Molluscan Filter Feeders</skos:prefLabel>
	<dcterms:contributor rdf:resource="http://editor.vocabs.ands.org.au/user/eMII_Finney.Kim_Admin"/>
	<dcterms:created rdf:datatype="http://www.w3.org/2001/XMLSchema#dateTime">2016-11-16T01:18:13Z</dcterms:created>
	<dcterms:creator rdf:resource="http://editor.vocabs.ands.org.au/user/eMII_Finney.Kim_Admin"/>
	<dcterms:modified rdf:datatype="http://www.w3.org/2001/XMLSchema#dateTime">2017-06-27T04:15:00Z</dcterms:modified>
	<dc:publisher rdf:datatype="http://www.w3.org/2001/XMLSchema#string">Institute for Marine and Antarctic Studies (IMAS) - UTAS</dc:publisher>
	<skos:definition xml:lang="en">A filter feeder habitat is characterised by biota dominated by organisms that feed by drawing water through a specialised structure and filtering out small particles and organisms in the water column.  </skos:definition>
	<dc:source rdf:datatype="http://www.w3.org/2001/XMLSchema#string">SeaMap Australia National Benthic Habitat Classification Scheme (2017)</dc:source>
	<skos:narrower rdf:resource="http://seamapaustralia.org.au/def/benthichabitatclassification/class/325"/>
	<skos:narrower rdf:resource="http://seamapaustralia.org.au/def/benthichabitatclassification/class/158"/>
	<skos:narrower rdf:resource="http://seamapaustralia.org.au/def/benthichabitatclassification/class/90"/>
	<skos:narrower rdf:resource="http://seamapaustralia.org.au/def/benthichabitatclassification/class/91"/>
	<skos:narrower rdf:resource="http://seamapaustralia.org.au/def/benthichabitatclassification/class/92"/>
	<skos:narrower rdf:resource="http://seamapaustralia.org.au/def/benthichabitatclassification/class/93"/>
	<skos:narrower rdf:resource="http://seamapaustralia.org.au/def/benthichabitatclassification/class/159"/>
</rdf:Description>

<rdf:Description rdf:about="http://seamapaustralia.org.au/def/benthichabitatclassification/class/79">
	<rdf:type rdf:resource="http://www.w3.org/2000/01/rdf-schema#Resource"/>
	<rdf:type rdf:resource="http://www.w3.org/2004/02/skos/core#Concept"/>
	<skos:broader rdf:resource="http://seamapaustralia.org.au/def/benthichabitatclassification/class/73"/>
	<skos:prefLabel xml:lang="en">Bioturbators</skos:prefLabel>
	<dcterms:contributor rdf:resource="http://editor.vocabs.ands.org.au/user/eMII_Finney.Kim_Admin"/>
	<dcterms:created rdf:datatype="http://www.w3.org/2001/XMLSchema#dateTime">2016-11-16T01:18:55Z</dcterms:created>
	<dcterms:creator rdf:resource="http://editor.vocabs.ands.org.au/user/eMII_Finney.Kim_Admin"/>
	<dcterms:modified rdf:datatype="http://www.w3.org/2001/XMLSchema#dateTime">2017-06-27T04:14:51Z</dcterms:modified>
	<dc:publisher rdf:datatype="http://www.w3.org/2001/XMLSchema#string">Institute for Marine and Antarctic Studies (IMAS) - UTAS</dc:publisher>
	<skos:definition xml:lang="en">Bioturbation refers to the signs and traces formed by the activity of macrofauna living in soft sediment habitats. This can include evidence of burrows, feeding or crawling traces and mounds from a hugely diverse group of organisms. While direct observations of the fauna may not be common, the existence of these traces and the type of trace can help inform which types of bioturbators might be present in an area.  </skos:definition>
	<dc:source rdf:datatype="http://www.w3.org/2001/XMLSchema#string">SeaMap Australia National Benthic Habitat Classification Scheme (2017)</dc:source>
	<skos:relatedMatch rdf:resource="https://www.cmecscatalog.org/cmecs/classification/unit/186.html"/>
</rdf:Description>

<rdf:Description rdf:about="http://seamapaustralia.org.au/def/benthichabitatclassification/class/340">
	<rdf:type rdf:resource="http://www.w3.org/2000/01/rdf-schema#Resource"/>
	<rdf:type rdf:resource="http://www.w3.org/2004/02/skos/core#Concept"/>
	<skos:broader rdf:resource="http://seamapaustralia.org.au/def/benthichabitatclassification/class/337"/>
	<skos:prefLabel xml:lang="en">IMCRA Lucinda-Mackay Coast</skos:prefLabel>
	<dcterms:contributor rdf:resource="http://editor.vocabs.ands.org.au/user/eMII_Finney.Kim_Admin"/>
	<dcterms:created rdf:datatype="http://www.w3.org/2001/XMLSchema#dateTime">2017-06-27T03:30:01Z</dcterms:created>
	<dcterms:creator rdf:resource="http://editor.vocabs.ands.org.au/user/eMII_Finney.Kim_Admin"/>
	<dcterms:modified rdf:datatype="http://www.w3.org/2001/XMLSchema#dateTime">2017-06-27T03:58:19Z</dcterms:modified>
	<dc:publisher rdf:datatype="http://www.w3.org/2001/XMLSchema#string">Institute for Marine and Antarctic Studies (IMAS) - UTAS</dc:publisher>
	<skos:definition xml:lang="en">An inshore regionalisation of Australian waters derived from biological and physical data, including the distribution of demersal fishes, marine plants and invertebrates, sea floor geomorphology and sediments, and oceanographic data. The meso-scale regionalisation was compiled from information supplied to the Australian Government Department of the Environment and Heritage by the relevant State, Northern Territory and Commonwealth marine research and management agencies. The seaward extent for the meso-scale IMCRA coverage is defined by the 200m isobath except where this boundary extends beyond the Australian Exclusive Economic Zone (AEEZ).</skos:definition>
	<dc:source rdf:datatype="http://www.w3.org/2001/XMLSchema#string">Commonwealth of Australia (2006). A Guide to the Integrated Marine and Coastal Regionalisation of Australia Version 4.0. Department of the Environment and Heritage, Canberra, Australia.</dc:source>
	<skos:exactMatch rdf:resource="http://www.environment.gov.au/mapping/rest/services/ogc_services/IMCRA_Mesoscale/MapServer/0/25"/>
</rdf:Description>

<rdf:Description rdf:about="http://seamapaustralia.org.au/def/benthichabitatclassification/class/82">
	<rdf:type rdf:resource="http://www.w3.org/2000/01/rdf-schema#Resource"/>
	<rdf:type rdf:resource="http://www.w3.org/2004/02/skos/core#Concept"/>
	<skos:broader rdf:resource="http://seamapaustralia.org.au/def/benthichabitatclassification/class/75"/>
	<skos:prefLabel xml:lang="en">Mangroves</skos:prefLabel>
	<dcterms:contributor rdf:resource="http://editor.vocabs.ands.org.au/user/eMII_Finney.Kim_Admin"/>
	<dcterms:created rdf:datatype="http://www.w3.org/2001/XMLSchema#dateTime">2016-11-16T01:28:44Z</dcterms:created>
	<dcterms:creator rdf:resource="http://editor.vocabs.ands.org.au/user/eMII_Finney.Kim_Admin"/>
	<dcterms:modified rdf:datatype="http://www.w3.org/2001/XMLSchema#dateTime">2017-06-27T04:17:30Z</dcterms:modified>
	<dc:publisher rdf:datatype="http://www.w3.org/2001/XMLSchema#string">Institute for Marine and Antarctic Studies (IMAS) - UTAS</dc:publisher>
	<skos:definition xml:lang="en">An area dominated by mangroves, a tree or shrub that occurs in saline and brackish water in coastal and estuarine environments between low and high tide levels on sheltered shores. Mangroves are typically considered a tropical species, however in Australia some species occur in temperate regions as well. They typically have a tangled, above ground root system, and can form extensive swampy forests (as in Edgar 2008).</skos:definition>
	<dc:source rdf:datatype="http://www.w3.org/2001/XMLSchema#string">SeaMap Australia National Benthic Habitat Classification Scheme (2017)</dc:source>
	<skos:closeMatch rdf:resource="https://www.cmecscatalog.org/cmecs/classification/unit/577.html"/>
	<skos:closeMatch rdf:resource="https://www.cmecscatalog.org/cmecs/classification/unit/581.html"/>
</rdf:Description>

<rdf:Description rdf:about="http://seamapaustralia.org.au/def/benthichabitatclassification/class/83">
	<rdf:type rdf:resource="http://www.w3.org/2000/01/rdf-schema#Resource"/>
	<rdf:type rdf:resource="http://www.w3.org/2004/02/skos/core#Concept"/>
	<skos:broader rdf:resource="http://seamapaustralia.org.au/def/benthichabitatclassification/class/75"/>
	<skos:prefLabel xml:lang="en">Saltmarsh</skos:prefLabel>
	<dcterms:contributor rdf:resource="http://editor.vocabs.ands.org.au/user/eMII_Finney.Kim_Admin"/>
	<dcterms:created rdf:datatype="http://www.w3.org/2001/XMLSchema#dateTime">2016-11-16T01:29:42Z</dcterms:created>
	<dcterms:creator rdf:resource="http://editor.vocabs.ands.org.au/user/eMII_Finney.Kim_Admin"/>
	<dcterms:modified rdf:datatype="http://www.w3.org/2001/XMLSchema#dateTime">2017-06-27T04:17:40Z</dcterms:modified>
	<dc:publisher rdf:datatype="http://www.w3.org/2001/XMLSchema#string">Institute for Marine and Antarctic Studies (IMAS) - UTAS</dc:publisher>
	<skos:definition xml:lang="en">An area dominated by saltmarsh plants (halophytes). These typically occur on sheltered intertidal mud and sand flats. They are easily distinguished from other plants in that their roots are (semi-) regularly inundated by saltwater, and from mangroves based on their smaller size (as in Edgar, 2008).</skos:definition>
	<dc:source rdf:datatype="http://www.w3.org/2001/XMLSchema#string">SeaMap Australia National Benthic Habitat Classification Scheme (2017)</dc:source>
	<skos:closeMatch rdf:resource="https://www.cmecscatalog.org/cmecs/classification/unit/570.html"/>
	<skos:closeMatch rdf:resource="https://www.cmecscatalog.org/cmecs/classification/unit/571.html"/>
</rdf:Description>

<rdf:Description rdf:about="http://seamapaustralia.org.au/def/benthichabitatclassification/class/344">
	<rdf:type rdf:resource="http://www.w3.org/2000/01/rdf-schema#Resource"/>
	<rdf:type rdf:resource="http://www.w3.org/2004/02/skos/core#Concept"/>
	<skos:broader rdf:resource="http://seamapaustralia.org.au/def/benthichabitatclassification/class/185"/>
	<skos:prefLabel xml:lang="en">IMCRA Northeast Transition</skos:prefLabel>
	<dcterms:contributor rdf:resource="http://editor.vocabs.ands.org.au/user/eMII_Finney.Kim_Admin"/>
	<dcterms:created rdf:datatype="http://www.w3.org/2001/XMLSchema#dateTime">2017-06-27T03:32:16Z</dcterms:created>
	<dcterms:creator rdf:resource="http://editor.vocabs.ands.org.au/user/eMII_Finney.Kim_Admin"/>
	<dcterms:modified rdf:datatype="http://www.w3.org/2001/XMLSchema#dateTime">2017-06-27T03:59:25Z</dcterms:modified>
	<dc:publisher rdf:datatype="http://www.w3.org/2001/XMLSchema#string">Institute for Marine and Antarctic Studies (IMAS) - UTAS</dc:publisher>
	<skos:definition xml:lang="en">An IMCRA provincial bioregion reflects biogeographic patterns in distributions of bottom-dwelling fish. Provincial bioregions were defined for the continental shelf for IMCRA v3.3, and for the continental slope for the National Marine Bioregionalisation using similar analytical techniques. In both cases the distributions of demersal (bottom-dwelling) fish were plotted onto a line divided into equally spaced sections. The number of species in each section and the similarity between sections were calculated using a statistical tool called the Jaccard Index. Where the Jaccard Index changed greatly between sections a boundary was defined indicating differences in species assemblages between regions. Two types of provincial bioregions are defined in the IMCRA benthic bioregionalisation: provinces, which represent regions of biotic endemism; and transitions, which generally occur between the provinces, and are less well-defined mixing areas that capture the overlap of demersal fish species ranges between the provinces.</skos:definition>
	<dc:source rdf:datatype="http://www.w3.org/2001/XMLSchema#string">Commonwealth of Australia (2006). A Guide to the Integrated Marine and Coastal Regionalisation of Australia Version 4.0. Department of the Environment and Heritage, Canberra, Australia.</dc:source>
	<skos:narrower rdf:resource="http://seamapaustralia.org.au/def/benthichabitatclassification/class/347"/>
	<skos:narrower rdf:resource="http://seamapaustralia.org.au/def/benthichabitatclassification/class/345"/>
	<skos:narrower rdf:resource="http://seamapaustralia.org.au/def/benthichabitatclassification/class/346"/>
	<skos:exactMatch rdf:resource="http://www.environment.gov.au/mapping/rest/services/ogc_services/IMCRA_Provincial/MapServer/0/9"/>
</rdf:Description>

<rdf:Description rdf:about="http://seamapaustralia.org.au/def/benthichabitatclassification/class/84">
	<rdf:type rdf:resource="http://www.w3.org/2000/01/rdf-schema#Resource"/>
	<rdf:type rdf:resource="http://www.w3.org/2004/02/skos/core#Concept"/>
	<skos:broader rdf:resource="http://seamapaustralia.org.au/def/benthichabitatclassification/class/76"/>
	<skos:prefLabel xml:lang="en">Macroalgae</skos:prefLabel>
	<dcterms:contributor rdf:resource="http://editor.vocabs.ands.org.au/user/eMII_Finney.Kim_Admin"/>
	<dcterms:created rdf:datatype="http://www.w3.org/2001/XMLSchema#dateTime">2016-11-16T01:30:35Z</dcterms:created>
	<dcterms:creator rdf:resource="http://editor.vocabs.ands.org.au/user/eMII_Finney.Kim_Admin"/>
	<dcterms:modified rdf:datatype="http://www.w3.org/2001/XMLSchema#dateTime">2017-06-27T04:17:07Z</dcterms:modified>
	<dc:publisher rdf:datatype="http://www.w3.org/2001/XMLSchema#string">Institute for Marine and Antarctic Studies (IMAS) - UTAS</dc:publisher>
	<skos:definition xml:lang="en">An area dominated by macroalgae, i.e. multicellular algae that are capable of attaching to the seafloor (CATAMI 2014). Macroalgae are commonly referred to as seaweeds, and consist of the phyla Chlorophyta and Rhodophyta, and class Phaeophyceae.</skos:definition>
	<dc:source rdf:datatype="http://www.w3.org/2001/XMLSchema#string"> SeaMap Australia National Benthic Habitat Classification Scheme (2017)</dc:source>
	<skos:closeMatch rdf:resource="https://www.cmecscatalog.org/cmecs/classification/unit/433.html"/>
</rdf:Description>

<rdf:Description rdf:about="http://seamapaustralia.org.au/def/benthichabitatclassification/class/85">
	<rdf:type rdf:resource="http://www.w3.org/2000/01/rdf-schema#Resource"/>
	<rdf:type rdf:resource="http://www.w3.org/2004/02/skos/core#Concept"/>
	<skos:broader rdf:resource="http://seamapaustralia.org.au/def/benthichabitatclassification/class/76"/>
	<skos:prefLabel xml:lang="en">Seagrass</skos:prefLabel>
	<dcterms:contributor rdf:resource="http://editor.vocabs.ands.org.au/user/eMII_Finney.Kim_Admin"/>
	<dcterms:created rdf:datatype="http://www.w3.org/2001/XMLSchema#dateTime">2016-11-16T01:31:12Z</dcterms:created>
	<dcterms:creator rdf:resource="http://editor.vocabs.ands.org.au/user/eMII_Finney.Kim_Admin"/>
	<dcterms:modified rdf:datatype="http://www.w3.org/2001/XMLSchema#dateTime">2017-06-27T04:17:15Z</dcterms:modified>
	<dc:publisher rdf:datatype="http://www.w3.org/2001/XMLSchema#string">Institute for Marine and Antarctic Studies (IMAS) - UTAS</dc:publisher>
	<skos:definition xml:lang="en">Areas dominated by seagrass, a flowering plant (angiosperm; Phylum Magnoliophyta) that typically occurs in sheltered intertidal or subtidal environments, and has elongated green and grass-like leaves. </skos:definition>
	<dc:source rdf:datatype="http://www.w3.org/2001/XMLSchema#string"> SeaMap Australia National Benthic Habitat Classification Scheme (2017)</dc:source>
	<skos:closeMatch rdf:resource="https://www.cmecscatalog.org/cmecs/classification/unit/567.html"/>
</rdf:Description>

<rdf:Description rdf:about="http://seamapaustralia.org.au/def/benthichabitatclassification/class/185">
	<rdf:type rdf:resource="http://www.w3.org/2000/01/rdf-schema#Resource"/>
	<rdf:type rdf:resource="http://www.w3.org/2004/02/skos/core#Concept"/>
	<skos:broader rdf:resource="http://seamapaustralia.org.au/def/benthichabitatclassification/class/174"/>
	<skos:prefLabel xml:lang="en">MEOW Torres Strait Northern Great Barrier Reef Ecoregion</skos:prefLabel>
	<dcterms:contributor rdf:resource="http://editor.vocabs.ands.org.au/user/eMII_Finney.Kim_Admin"/>
	<dcterms:created rdf:datatype="http://www.w3.org/2001/XMLSchema#dateTime">2017-05-31T02:01:48Z</dcterms:created>
	<dcterms:creator rdf:resource="http://editor.vocabs.ands.org.au/user/eMII_Finney.Kim_Admin"/>
	<dcterms:modified rdf:datatype="http://www.w3.org/2001/XMLSchema#dateTime">2017-06-27T04:34:02Z</dcterms:modified>
	<dc:publisher rdf:datatype="http://www.w3.org/2001/XMLSchema#string">Institute for Marine and Antarctic Studies (IMAS) - UTAS</dc:publisher>
	<skos:definition xml:lang="en">An area of relatively homogenous species composition, clearly distinct from adjacent systems. The species composition is likely to be determined by the predominance of a small number of ecosystems and/or a distinct suite of oceanographic or topographic features. The dominant biogeographic forcing agents defining the ecoregions vary from location to location but may include isolation, upwelling, nutrient inputs, freshwater influx, temperature regimes, ice regimes, exposure, sediments, currents and bathymetric or coastal complexity.</skos:definition>
	<dc:source rdf:datatype="http://www.w3.org/2001/XMLSchema#string">Marine Ecoregions of the World (MEOW). Spalding et.al. (2007)</dc:source>
	<skos:narrower rdf:resource="http://seamapaustralia.org.au/def/benthichabitatclassification/class/344"/>
	<skos:exactMatch rdf:resource="http://www.marineregions.org/gazetteer.php?p=details&amp;id=21905"/>
</rdf:Description>

<rdf:Description rdf:about="http://seamapaustralia.org.au/def/benthichabitatclassification/class/151">
	<rdf:type rdf:resource="http://www.w3.org/2000/01/rdf-schema#Resource"/>
	<rdf:type rdf:resource="http://www.w3.org/2004/02/skos/core#Concept"/>
	<skos:broader rdf:resource="http://seamapaustralia.org.au/def/benthichabitatclassification/class/17"/>
	<skos:prefLabel xml:lang="en">Mixed Fine Sediments</skos:prefLabel>
	<dcterms:contributor rdf:resource="http://editor.vocabs.ands.org.au/user/eMII_Finney.Kim_Admin"/>
	<dcterms:created rdf:datatype="http://www.w3.org/2001/XMLSchema#dateTime">2017-05-23T05:20:29Z</dcterms:created>
	<dcterms:creator rdf:resource="http://editor.vocabs.ands.org.au/user/eMII_Finney.Kim_Admin"/>
	<dcterms:modified rdf:datatype="http://www.w3.org/2001/XMLSchema#dateTime">2017-06-27T04:21:58Z</dcterms:modified>
	<dc:publisher rdf:datatype="http://www.w3.org/2001/XMLSchema#string">  Institute for Marine and Antarctic Studies (IMAS) - UTAS</dc:publisher>
	<skos:definition xml:lang="en">A Fine Sediment that comprises a mixture of Silt and Clay, but where neither component exceeds ≥ 80% of the substratum surface/composition.</skos:definition>
	<dc:source rdf:datatype="http://www.w3.org/2001/XMLSchema#string">SeaMap Australia National Benthic Habitat Classification Scheme (2017)</dc:source>
</rdf:Description>

<rdf:Description rdf:about="http://seamapaustralia.org.au/def/benthichabitatclassification/class/342">
	<rdf:type rdf:resource="http://www.w3.org/2000/01/rdf-schema#Resource"/>
	<rdf:type rdf:resource="http://www.w3.org/2004/02/skos/core#Concept"/>
	<skos:broader rdf:resource="http://seamapaustralia.org.au/def/benthichabitatclassification/class/337"/>
	<skos:prefLabel xml:lang="en">IMCRA Shoalwater Coast Bioregion</skos:prefLabel>
	<dcterms:contributor rdf:resource="http://editor.vocabs.ands.org.au/user/eMII_Finney.Kim_Admin"/>
	<dcterms:created rdf:datatype="http://www.w3.org/2001/XMLSchema#dateTime">2017-06-27T03:31:23Z</dcterms:created>
	<dcterms:creator rdf:resource="http://editor.vocabs.ands.org.au/user/eMII_Finney.Kim_Admin"/>
	<dcterms:modified rdf:datatype="http://www.w3.org/2001/XMLSchema#dateTime">2017-06-27T03:59:01Z</dcterms:modified>
	<dc:publisher rdf:datatype="http://www.w3.org/2001/XMLSchema#string">Institute for Marine and Antarctic Studies (IMAS) - UTAS</dc:publisher>
	<skos:definition xml:lang="en">An inshore regionalisation of Australian waters derived from biological and physical data, including the distribution of demersal fishes, marine plants and invertebrates, sea floor geomorphology and sediments, and oceanographic data. The meso-scale regionalisation was compiled from information supplied to the Australian Government Department of the Environment and Heritage by the relevant State, Northern Territory and Commonwealth marine research and management agencies. The seaward extent for the meso-scale IMCRA coverage is defined by the 200m isobath except where this boundary extends beyond the Australian Exclusive Economic Zone (AEEZ).</skos:definition>
	<dc:source rdf:datatype="http://www.w3.org/2001/XMLSchema#string">Commonwealth of Australia (2006). A Guide to the Integrated Marine and Coastal Regionalisation of Australia Version 4.0. Department of the Environment and Heritage, Canberra, Australia.</dc:source>
	<skos:exactMatch rdf:resource="http://www.environment.gov.au/mapping/rest/services/ogc_services/IMCRA_Mesoscale/MapServer/0/31"/>
</rdf:Description>

<rdf:Description rdf:about="http://seamapaustralia.org.au/def/benthichabitatclassification/class/90">
	<rdf:type rdf:resource="http://www.w3.org/2000/01/rdf-schema#Resource"/>
	<rdf:type rdf:resource="http://www.w3.org/2004/02/skos/core#Concept"/>
	<skos:broader rdf:resource="http://seamapaustralia.org.au/def/benthichabitatclassification/class/78"/>
	<skos:prefLabel xml:lang="en">Bryozoans</skos:prefLabel>
	<dcterms:contributor rdf:resource="http://editor.vocabs.ands.org.au/user/eMII_Finney.Kim_Admin"/>
	<dcterms:created rdf:datatype="http://www.w3.org/2001/XMLSchema#dateTime">2016-11-16T01:34:23Z</dcterms:created>
	<dcterms:creator rdf:resource="http://editor.vocabs.ands.org.au/user/eMII_Finney.Kim_Admin"/>
	<dcterms:modified rdf:datatype="http://www.w3.org/2001/XMLSchema#dateTime">2017-06-27T04:15:09Z</dcterms:modified>
	<dc:publisher rdf:datatype="http://www.w3.org/2001/XMLSchema#string">Institute for Marine and Antarctic Studies (IMAS) - UTAS</dc:publisher>
	<skos:definition xml:lang="en">A colonial animal of the Phylum Bryozoa that consist of numerous zooids, small box-like units about 1 mm long. They generally have a chitinous or calcareous covering that adds structural support, and feed by extending tentacles from an orifice in the upper sidewall. They may occur in many growth forms, including as flat encrusting, branched, fenestrate, soft dendroid and fouling communities (as in Edgar 2008, FGDC 2012).</skos:definition>
	<dc:source rdf:datatype="http://www.w3.org/2001/XMLSchema#string">SeaMap Australia National Benthic Habitat Classification Scheme (2017)</dc:source>
	<skos:closeMatch rdf:resource="https://www.cmecscatalog.org/cmecs/classification/unit/509.html"/>
	<skos:closeMatch rdf:resource="https://www.cmecscatalog.org/cmecs/classification/unit/523.html"/>
	<skos:closeMatch rdf:resource="https://www.cmecscatalog.org/cmecs/classification/unit/876.html"/>
</rdf:Description>

<rdf:Description rdf:about="http://seamapaustralia.org.au/def/benthichabitatclassification/class/91">
	<rdf:type rdf:resource="http://www.w3.org/2000/01/rdf-schema#Resource"/>
	<rdf:type rdf:resource="http://www.w3.org/2004/02/skos/core#Concept"/>
	<skos:broader rdf:resource="http://seamapaustralia.org.au/def/benthichabitatclassification/class/78"/>
	<skos:prefLabel xml:lang="en">Sponges</skos:prefLabel>
	<dcterms:contributor rdf:resource="http://editor.vocabs.ands.org.au/user/eMII_Finney.Kim_Admin"/>
	<dcterms:created rdf:datatype="http://www.w3.org/2001/XMLSchema#dateTime">2016-11-16T01:34:51Z</dcterms:created>
	<dcterms:creator rdf:resource="http://editor.vocabs.ands.org.au/user/eMII_Finney.Kim_Admin"/>
	<dcterms:modified rdf:datatype="http://www.w3.org/2001/XMLSchema#dateTime">2017-06-27T04:15:36Z</dcterms:modified>
	<dc:publisher rdf:datatype="http://www.w3.org/2001/XMLSchema#string">Institute for Marine and Antarctic Studies (IMAS) - UTAS</dc:publisher>
	<skos:definition xml:lang="en">An area dominated by sponges, simple multicellular animals of the Phylum Porifera that live attached to the seafloor. Their soft and porus body structure is supported by a framework of fibrous proteins, and spicules of calcium carbonate or silica. Sponges are morphologically diverse, but all draw in a current of water using specialised flagella and extract nutrients and oxygen from the flow. </skos:definition>
	<dc:source rdf:datatype="http://www.w3.org/2001/XMLSchema#string">SeaMap Australia National Benthic Habitat Classification Scheme (2017)</dc:source>
</rdf:Description>

<rdf:Description rdf:about="http://seamapaustralia.org.au/def/benthichabitatclassification/class/92">
	<rdf:type rdf:resource="http://www.w3.org/2000/01/rdf-schema#Resource"/>
	<rdf:type rdf:resource="http://www.w3.org/2004/02/skos/core#Concept"/>
	<skos:broader rdf:resource="http://seamapaustralia.org.au/def/benthichabitatclassification/class/78"/>
	<skos:prefLabel xml:lang="en">Ascidians</skos:prefLabel>
	<dcterms:contributor rdf:resource="http://editor.vocabs.ands.org.au/user/eMII_Finney.Kim_Admin"/>
	<dcterms:created rdf:datatype="http://www.w3.org/2001/XMLSchema#dateTime">2016-11-16T01:36:38Z</dcterms:created>
	<dcterms:creator rdf:resource="http://editor.vocabs.ands.org.au/user/eMII_Finney.Kim_Admin"/>
	<dcterms:modified rdf:datatype="http://www.w3.org/2001/XMLSchema#dateTime">2017-06-27T04:15:04Z</dcterms:modified>
	<dc:publisher rdf:datatype="http://www.w3.org/2001/XMLSchema#string">Institute for Marine and Antarctic Studies (IMAS) - UTAS</dc:publisher>
	<skos:definition xml:lang="en">An area dominated by ascidians (also known as seasquirts or tunicates; Class Ascidiacea), a diverse group of solitary or colonial animals, the adults of which are sessile. Ascidians are bag-like filter feeders, drawing water in and out through separate inhalant and exhalent siphons.  They occur from intertidal to deep ( &gt; 2000 m) subtidal waters, and can reach high abundances. </skos:definition>
	<dc:source rdf:datatype="http://www.w3.org/2001/XMLSchema#string">SeaMap Australia National Benthic Habitat Classification Scheme (2017)</dc:source>
</rdf:Description>

<rdf:Description rdf:about="http://seamapaustralia.org.au/def/benthichabitatclassification/class/93">
	<rdf:type rdf:resource="http://www.w3.org/2000/01/rdf-schema#Resource"/>
	<rdf:type rdf:resource="http://www.w3.org/2004/02/skos/core#Concept"/>
	<skos:broader rdf:resource="http://seamapaustralia.org.au/def/benthichabitatclassification/class/78"/>
	<skos:prefLabel xml:lang="en">Non-Coral Cnidaria</skos:prefLabel>
	<dcterms:contributor rdf:resource="http://editor.vocabs.ands.org.au/user/eMII_Finney.Kim_Admin"/>
	<dcterms:created rdf:datatype="http://www.w3.org/2001/XMLSchema#dateTime">2016-11-16T01:37:25Z</dcterms:created>
	<dcterms:creator rdf:resource="http://editor.vocabs.ands.org.au/user/eMII_Finney.Kim_Admin"/>
	<dcterms:modified rdf:datatype="http://www.w3.org/2001/XMLSchema#dateTime">2017-06-27T04:15:31Z</dcterms:modified>
	<dc:publisher rdf:datatype="http://www.w3.org/2001/XMLSchema#string">Institute for Marine and Antarctic Studies (IMAS) - UTAS</dc:publisher>
	<skos:definition xml:lang="en">Areas dominated by anemones, hydroids, hydrocorals or other benthic Cnidaria that are not corals. </skos:definition>
	<dc:source rdf:datatype="http://www.w3.org/2001/XMLSchema#string">SeaMap Australia National Benthic Habitat Classification Scheme (2017)</dc:source>
</rdf:Description>

<rdf:Description rdf:about="http://seamapaustralia.org.au/def/benthichabitatclassification/class/94">
	<rdf:type rdf:resource="http://www.w3.org/2000/01/rdf-schema#Resource"/>
	<rdf:type rdf:resource="http://www.w3.org/2004/02/skos/core#Concept"/>
	<skos:broader rdf:resource="http://seamapaustralia.org.au/def/benthichabitatclassification/class/80"/>
	<skos:prefLabel xml:lang="en">Oyster</skos:prefLabel>
	<dcterms:contributor rdf:resource="http://editor.vocabs.ands.org.au/user/eMII_Finney.Kim_Admin"/>
	<dcterms:created rdf:datatype="http://www.w3.org/2001/XMLSchema#dateTime">2016-11-16T01:38:05Z</dcterms:created>
	<dcterms:creator rdf:resource="http://editor.vocabs.ands.org.au/user/eMII_Finney.Kim_Admin"/>
	<dcterms:modified rdf:datatype="http://www.w3.org/2001/XMLSchema#dateTime">2017-06-27T04:16:10Z</dcterms:modified>
	<dc:publisher rdf:datatype="http://www.w3.org/2001/XMLSchema#string">Institute for Marine and Antarctic Studies (IMAS) - UTAS</dc:publisher>
	<skos:definition xml:lang="en">An area dominated by accumulations of living oysters attached to a substratum. </skos:definition>
	<dc:source rdf:datatype="http://www.w3.org/2001/XMLSchema#string">SeaMap Australia National Benthic Habitat Classification Scheme (2017)</dc:source>
	<skos:closeMatch rdf:resource="https://www.cmecscatalog.org/cmecs/classification/unit/505.html"/>
	<skos:closeMatch rdf:resource="https://www.cmecscatalog.org/cmecs/classification/unit/516.html"/>
	<skos:closeMatch rdf:resource="https://www.cmecscatalog.org/cmecs/classification/unit/534.html"/>
</rdf:Description>

<rdf:Description rdf:about="http://seamapaustralia.org.au/def/benthichabitatclassification/class/95">
	<rdf:type rdf:resource="http://www.w3.org/2000/01/rdf-schema#Resource"/>
	<rdf:type rdf:resource="http://www.w3.org/2004/02/skos/core#Concept"/>
	<skos:broader rdf:resource="http://seamapaustralia.org.au/def/benthichabitatclassification/class/80"/>
	<skos:prefLabel xml:lang="en">Mussel</skos:prefLabel>
	<dcterms:contributor rdf:resource="http://editor.vocabs.ands.org.au/user/eMII_Finney.Kim_Admin"/>
	<dcterms:created rdf:datatype="http://www.w3.org/2001/XMLSchema#dateTime">2016-11-16T01:38:36Z</dcterms:created>
	<dcterms:creator rdf:resource="http://editor.vocabs.ands.org.au/user/eMII_Finney.Kim_Admin"/>
	<dcterms:modified rdf:datatype="http://www.w3.org/2001/XMLSchema#dateTime">2017-06-27T04:15:55Z</dcterms:modified>
	<dc:publisher rdf:datatype="http://www.w3.org/2001/XMLSchema#string">Institute for Marine and Antarctic Studies (IMAS) - UTAS</dc:publisher>
	<skos:definition xml:lang="en">An area dominated by accumulations of living mussels attached to a substratum.</skos:definition>
	<dc:source rdf:datatype="http://www.w3.org/2001/XMLSchema#string">SeaMap Australia National Benthic Habitat Classification Scheme (2017)</dc:source>
	<skos:closeMatch rdf:resource="https://www.cmecscatalog.org/cmecs/classification/unit/504.html"/>
	<skos:closeMatch rdf:resource="https://www.cmecscatalog.org/cmecs/classification/unit/515.html"/>
	<skos:closeMatch rdf:resource="https://www.cmecscatalog.org/cmecs/classification/unit/532.html"/>
</rdf:Description>

<rdf:Description rdf:about="http://seamapaustralia.org.au/def/benthichabitatclassification/class/159">
	<rdf:type rdf:resource="http://www.w3.org/2000/01/rdf-schema#Resource"/>
	<rdf:type rdf:resource="http://www.w3.org/2004/02/skos/core#Concept"/>
	<skos:broader rdf:resource="http://seamapaustralia.org.au/def/benthichabitatclassification/class/78"/>
	<skos:prefLabel xml:lang="en">Coral Biota</skos:prefLabel>
	<dcterms:contributor rdf:resource="http://editor.vocabs.ands.org.au/user/eMII_Finney.Kim_Admin"/>
	<dcterms:created rdf:datatype="http://www.w3.org/2001/XMLSchema#dateTime">2017-05-23T05:50:34Z</dcterms:created>
	<dcterms:creator rdf:resource="http://editor.vocabs.ands.org.au/user/eMII_Finney.Kim_Admin"/>
	<dcterms:modified rdf:datatype="http://www.w3.org/2001/XMLSchema#dateTime">2017-06-27T04:15:22Z</dcterms:modified>
	<dc:publisher rdf:datatype="http://www.w3.org/2001/XMLSchema#string">Institute for Marine and Antarctic Studies (IMAS) - UTAS</dc:publisher>
	<skos:definition xml:lang="en">An area dominated by coral, a colonial marine Cnidarian from the Order Scleractinia, Antipatharia, Alcyonacea or Pennatulacea, where colonies are composed of individual polyps that are connected by living tissue. In some, corals polyps excrete an exoskeleton and are embedded within this structure, while others possess large amounts of gelatinous tissue and are much softer.  </skos:definition>
	<dc:source rdf:datatype="http://www.w3.org/2001/XMLSchema#string">SeaMap Australia National Benthic Habitat Classification Scheme (2017)</dc:source>
</rdf:Description>

<rdf:Description rdf:about="http://seamapaustralia.org.au/def/benthichabitatclassification/class/341">
	<rdf:type rdf:resource="http://www.w3.org/2000/01/rdf-schema#Resource"/>
	<rdf:type rdf:resource="http://www.w3.org/2004/02/skos/core#Concept"/>
	<skos:broader rdf:resource="http://seamapaustralia.org.au/def/benthichabitatclassification/class/337"/>
	<skos:prefLabel xml:lang="en">IMCRA Mackay-Capricorn Bioregion</skos:prefLabel>
	<dcterms:contributor rdf:resource="http://editor.vocabs.ands.org.au/user/eMII_Finney.Kim_Admin"/>
	<dcterms:created rdf:datatype="http://www.w3.org/2001/XMLSchema#dateTime">2017-06-27T03:30:31Z</dcterms:created>
	<dcterms:creator rdf:resource="http://editor.vocabs.ands.org.au/user/eMII_Finney.Kim_Admin"/>
	<dcterms:modified rdf:datatype="http://www.w3.org/2001/XMLSchema#dateTime">2017-06-27T03:58:32Z</dcterms:modified>
	<dc:publisher rdf:datatype="http://www.w3.org/2001/XMLSchema#string">Institute for Marine and Antarctic Studies (IMAS) - UTAS</dc:publisher>
	<skos:definition xml:lang="en">An inshore regionalisation of Australian waters derived from biological and physical data, including the distribution of demersal fishes, marine plants and invertebrates, sea floor geomorphology and sediments, and oceanographic data. The meso-scale regionalisation was compiled from information supplied to the Australian Government Department of the Environment and Heritage by the relevant State, Northern Territory and Commonwealth marine research and management agencies. The seaward extent for the meso-scale IMCRA coverage is defined by the 200m isobath except where this boundary extends beyond the Australian Exclusive Economic Zone (AEEZ).</skos:definition>
	<dc:source rdf:datatype="http://www.w3.org/2001/XMLSchema#string">Commonwealth of Australia (2006). A Guide to the Integrated Marine and Coastal Regionalisation of Australia Version 4.0. Department of the Environment and Heritage, Canberra, Australia.</dc:source>
	<skos:exactMatch rdf:resource="http://www.environment.gov.au/mapping/rest/services/ogc_services/IMCRA_Mesoscale/MapServer/0/29"/>
</rdf:Description>

<rdf:Description rdf:about="http://www.environment.gov.au/mapping/rest/services/ogc_services/IMCRA_Provincial/MapServer/0/12">
	<rdf:type rdf:resource="http://www.w3.org/2000/01/rdf-schema#Resource"/>
</rdf:Description>

<rdf:Description rdf:about="http://seamapaustralia.org.au/def/benthichabitatclassification/class/347">
	<rdf:type rdf:resource="http://www.w3.org/2000/01/rdf-schema#Resource"/>
	<rdf:type rdf:resource="http://www.w3.org/2004/02/skos/core#Concept"/>
	<skos:broader rdf:resource="http://seamapaustralia.org.au/def/benthichabitatclassification/class/344"/>
	<skos:prefLabel xml:lang="en">IMCRA Ribbons Bioregion</skos:prefLabel>
	<dcterms:contributor rdf:resource="http://editor.vocabs.ands.org.au/user/eMII_Finney.Kim_Admin"/>
	<dcterms:created rdf:datatype="http://www.w3.org/2001/XMLSchema#dateTime">2017-06-27T03:33:34Z</dcterms:created>
	<dcterms:creator rdf:resource="http://editor.vocabs.ands.org.au/user/eMII_Finney.Kim_Admin"/>
	<dcterms:modified rdf:datatype="http://www.w3.org/2001/XMLSchema#dateTime">2017-06-27T03:59:46Z</dcterms:modified>
	<dc:publisher rdf:datatype="http://www.w3.org/2001/XMLSchema#string">Institute for Marine and Antarctic Studies (IMAS) - UTAS</dc:publisher>
	<skos:definition xml:lang="en">An inshore regionalisation of Australian waters derived from biological and physical data, including the distribution of demersal fishes, marine plants and invertebrates, sea floor geomorphology and sediments, and oceanographic data. The meso-scale regionalisation was compiled from information supplied to the Australian Government Department of the Environment and Heritage by the relevant State, Northern Territory and Commonwealth marine research and management agencies. The seaward extent for the meso-scale IMCRA coverage is defined by the 200m isobath except where this boundary extends beyond the Australian Exclusive Economic Zone (AEEZ).</skos:definition>
	<dc:source rdf:datatype="http://www.w3.org/2001/XMLSchema#string">Commonwealth of Australia (2006). A Guide to the Integrated Marine and Coastal Regionalisation of Australia Version 4.0. Department of the Environment and Heritage, Canberra, Australia.</dc:source>
	<skos:exactMatch rdf:resource="http://www.environment.gov.au/mapping/rest/services/ogc_services/IMCRA_Mesoscale/MapServer/0/4"/>
</rdf:Description>

<rdf:Description rdf:about="http://seamapaustralia.org.au/def/benthichabitatclassification/class/345">
	<rdf:type rdf:resource="http://www.w3.org/2000/01/rdf-schema#Resource"/>
	<rdf:type rdf:resource="http://www.w3.org/2004/02/skos/core#Concept"/>
	<skos:broader rdf:resource="http://seamapaustralia.org.au/def/benthichabitatclassification/class/344"/>
	<skos:prefLabel xml:lang="en">IMCRA Torres Strait Bioregion</skos:prefLabel>
	<dcterms:contributor rdf:resource="http://editor.vocabs.ands.org.au/user/eMII_Finney.Kim_Admin"/>
	<dcterms:created rdf:datatype="http://www.w3.org/2001/XMLSchema#dateTime">2017-06-27T03:32:48Z</dcterms:created>
	<dcterms:creator rdf:resource="http://editor.vocabs.ands.org.au/user/eMII_Finney.Kim_Admin"/>
	<dcterms:modified rdf:datatype="http://www.w3.org/2001/XMLSchema#dateTime">2017-06-27T03:59:57Z</dcterms:modified>
	<dc:publisher rdf:datatype="http://www.w3.org/2001/XMLSchema#string">Institute for Marine and Antarctic Studies (IMAS) - UTAS</dc:publisher>
	<skos:definition xml:lang="en">An inshore regionalisation of Australian waters derived from biological and physical data, including the distribution of demersal fishes, marine plants and invertebrates, sea floor geomorphology and sediments, and oceanographic data. The meso-scale regionalisation was compiled from information supplied to the Australian Government Department of the Environment and Heritage by the relevant State, Northern Territory and Commonwealth marine research and management agencies. The seaward extent for the meso-scale IMCRA coverage is defined by the 200m isobath except where this boundary extends beyond the Australian Exclusive Economic Zone (AEEZ).</skos:definition>
	<dc:source rdf:datatype="http://www.w3.org/2001/XMLSchema#string">Commonwealth of Australia (2006). A Guide to the Integrated Marine and Coastal Regionalisation of Australia Version 4.0. Department of the Environment and Heritage, Canberra, Australia.</dc:source>
	<skos:exactMatch rdf:resource="http://www.environment.gov.au/mapping/rest/services/ogc_services/IMCRA_Mesoscale/MapServer/0/2"/>
</rdf:Description>

<rdf:Description rdf:about="http://seamapaustralia.org.au/def/benthichabitatclassification/class/155">
	<rdf:type rdf:resource="http://www.w3.org/2000/01/rdf-schema#Resource"/>
	<rdf:type rdf:resource="http://www.w3.org/2004/02/skos/core#Concept"/>
	<skos:broader rdf:resource="http://seamapaustralia.org.au/def/benthichabitatclassification/class/69"/>
	<skos:prefLabel xml:lang="en">Biota Absent</skos:prefLabel>
	<dcterms:contributor rdf:resource="http://editor.vocabs.ands.org.au/user/eMII_Finney.Kim_Admin"/>
	<dcterms:created rdf:datatype="http://www.w3.org/2001/XMLSchema#dateTime">2017-05-23T05:38:46Z</dcterms:created>
	<dcterms:creator rdf:resource="http://editor.vocabs.ands.org.au/user/eMII_Finney.Kim_Admin"/>
	<dcterms:modified rdf:datatype="http://www.w3.org/2001/XMLSchema#dateTime">2017-06-27T04:14:36Z</dcterms:modified>
	<dc:publisher rdf:datatype="http://www.w3.org/2001/XMLSchema#string">Institute for Marine and Antarctic Studies (IMAS) - UTAS</dc:publisher>
	<skos:definition xml:lang="en">An area where there is no evidence of living biota within the observational unit, either attached or closely associated with the seafloor, or where living biota account for a total of &lt; 5 % of the substratum surface/composition/biomass of the observational unit. </skos:definition>
	<dc:source rdf:datatype="http://www.w3.org/2001/XMLSchema#string">SeaMap Australia National Benthic Habitat Classification Scheme (2017)</dc:source>
</rdf:Description>

<rdf:Description rdf:about="http://seamapaustralia.org.au/def/benthichabitatclassification/class/319">
	<rdf:type rdf:resource="http://www.w3.org/2000/01/rdf-schema#Resource"/>
	<rdf:type rdf:resource="http://www.w3.org/2004/02/skos/core#Concept"/>
	<skos:broader rdf:resource="http://seamapaustralia.org.au/def/benthichabitatclassification/class/71"/>
	<skos:prefLabel xml:lang="en">Urchin Barren</skos:prefLabel>
	<dcterms:contributor rdf:resource="http://editor.vocabs.ands.org.au/user/eMII_Finney.Kim_Admin"/>
	<dcterms:created rdf:datatype="http://www.w3.org/2001/XMLSchema#dateTime">2017-06-27T00:54:45Z</dcterms:created>
	<dcterms:creator rdf:resource="http://editor.vocabs.ands.org.au/user/eMII_Finney.Kim_Admin"/>
	<dcterms:modified rdf:datatype="http://www.w3.org/2001/XMLSchema#dateTime">2017-06-27T00:54:55Z</dcterms:modified>
	<skos:definition xml:lang="en">An area where the absence of fleshy seaweeds on hard substratum is attributed to over-grazing from sea urchins. These areas are largely devoid of fleshy macroalgal cover where seaweeds would otherwise be expected to occur, and sea urchins are typically present at high densities, although once formed an urchin barren can be maintained by relatively low densities of urchins.</skos:definition>
</rdf:Description>

<rdf:Description rdf:about="http://seamapaustralia.org.au/def/benthichabitatclassification/class/297">
	<rdf:type rdf:resource="http://www.w3.org/2000/01/rdf-schema#Resource"/>
	<rdf:type rdf:resource="http://www.w3.org/2004/02/skos/core#Concept"/>
	<skos:broader rdf:resource="http://seamapaustralia.org.au/def/benthichabitatclassification/class/296"/>
	<skos:prefLabel xml:lang="en">IMCRA Ningaloo Bioregion</skos:prefLabel>
	<dcterms:contributor rdf:resource="http://editor.vocabs.ands.org.au/user/eMII_Finney.Kim_Admin"/>
	<dcterms:created rdf:datatype="http://www.w3.org/2001/XMLSchema#dateTime">2017-06-14T01:08:37Z</dcterms:created>
	<dcterms:creator rdf:resource="http://editor.vocabs.ands.org.au/user/eMII_Finney.Kim_Admin"/>
	<dcterms:modified rdf:datatype="http://www.w3.org/2001/XMLSchema#dateTime">2017-06-14T05:53:39Z</dcterms:modified>
	<dc:publisher rdf:datatype="http://www.w3.org/2001/XMLSchema#string">  Institute for Marine and Antarctic Studies (IMAS) - UTAS</dc:publisher>
	<skos:definition xml:lang="en">An inshore regionalisation of Australian waters derived from biological and physical data, including the distribution of demersal fishes, marine plants and invertebrates, sea floor geomorphology and sediments, and oceanographic data. The meso-scale regionalisation was compiled from information supplied to the Australian Government Department of the Environment and Heritage by the relevant State, Northern Territory and Commonwealth marine research and management agencies. The seaward extent for the meso-scale IMCRA coverage is defined by the 200m isobath except where this boundary extends beyond the Australian Exclusive Economic Zone (AEEZ).</skos:definition>
	<dc:source rdf:datatype="http://www.w3.org/2001/XMLSchema#string">Commonwealth of Australia (2006). A Guide to the Integrated Marine and Coastal Regionalisation of Australia Version 4.0. Department of the Environment and Heritage, Canberra, Australia.</dc:source>
	<skos:exactMatch rdf:resource="http://www.environment.gov.au/mapping/rest/services/ogc_services/IMCRA_Mesoscale/MapServer/0/32"/>
	<skos:scopeNote xml:lang="en">A small section of this bioregion falls within the MEOW Shark Bay Ecoregion.</skos:scopeNote>
</rdf:Description>

<rdf:Description rdf:about="http://seamapaustralia.org.au/def/benthichabitatclassification/class/157">
	<rdf:type rdf:resource="http://www.w3.org/2000/01/rdf-schema#Resource"/>
	<rdf:type rdf:resource="http://www.w3.org/2004/02/skos/core#Concept"/>
	<skos:broader rdf:resource="http://seamapaustralia.org.au/def/benthichabitatclassification/class/80"/>
	<skos:prefLabel xml:lang="en">Screw Shell Biota</skos:prefLabel>
	<dcterms:contributor rdf:resource="http://editor.vocabs.ands.org.au/user/eMII_Finney.Kim_Admin"/>
	<dcterms:created rdf:datatype="http://www.w3.org/2001/XMLSchema#dateTime">2017-05-23T05:44:26Z</dcterms:created>
	<dcterms:creator rdf:resource="http://editor.vocabs.ands.org.au/user/eMII_Finney.Kim_Admin"/>
	<dcterms:modified rdf:datatype="http://www.w3.org/2001/XMLSchema#dateTime">2017-06-27T04:16:15Z</dcterms:modified>
	<dc:publisher rdf:datatype="http://www.w3.org/2001/XMLSchema#string">Institute for Marine and Antarctic Studies (IMAS) - UTAS</dc:publisher>
	<skos:definition xml:lang="en">Areas dominated by accumulations of living screw shells.</skos:definition>
	<dc:source rdf:datatype="http://www.w3.org/2001/XMLSchema#string">SeaMap Australia National Benthic Habitat Classification Scheme (2017)</dc:source>
</rdf:Description>

<rdf:Description rdf:about="https://www.cmecscatalog.org/cmecs/classification/unit/509.html">
	<rdf:type rdf:resource="http://www.w3.org/2000/01/rdf-schema#Resource"/>
</rdf:Description>

<rdf:Description rdf:about="https://www.cmecscatalog.org/cmecs/classification/unit/505.html">
	<rdf:type rdf:resource="http://www.w3.org/2000/01/rdf-schema#Resource"/>
</rdf:Description>

<rdf:Description rdf:about="http://purl.org/dc/terms/identifier">
	<rdf:type rdf:resource="http://www.w3.org/1999/02/22-rdf-syntax-ns#Property"/>
	<rdf:type rdf:resource="http://www.w3.org/2000/01/rdf-schema#Resource"/>
	<rdfs:subPropertyOf rdf:resource="http://purl.org/dc/terms/identifier"/>
</rdf:Description>

<rdf:Description rdf:about="http://seamapaustralia.org.au/def/benthichabitatclassification/class/97">
	<rdf:type rdf:resource="http://www.w3.org/2000/01/rdf-schema#Resource"/>
	<rdf:type rdf:resource="http://www.w3.org/2004/02/skos/core#Concept"/>
	<skos:prefLabel xml:lang="en">Biogeographic Setting</skos:prefLabel>
	<dcterms:contributor rdf:resource="http://editor.vocabs.ands.org.au/user/eMII_Finney.Kim_Admin"/>
	<dcterms:created rdf:datatype="http://www.w3.org/2001/XMLSchema#dateTime">2017-05-23T02:35:35Z</dcterms:created>
	<dcterms:creator rdf:resource="http://editor.vocabs.ands.org.au/user/eMII_Finney.Kim_Admin"/>
	<dcterms:modified rdf:datatype="http://www.w3.org/2001/XMLSchema#dateTime">2017-06-27T04:06:47Z</dcterms:modified>
	<dc:publisher rdf:datatype="http://www.w3.org/2001/XMLSchema#string">Institute for Marine and Antarctic Studies (IMAS) - UTAS</dc:publisher>
	<skos:definition xml:lang="en">The Biogeographic Setting consists of a three tiered hierarchy that partitions the environment into Realms, Provinces and Ecoregions - based on the Marine Ecoregions of the World (MEOW; Spalding et al. , 2007) and additionally uses the Integrated Marine and Coastal Regionalisation of Australia (IMCRA, 2006). IMCRA (2006) consists of two levels, provinces which align approximately with MEOW Ecoregion boundaries and bioregions which nest under IMCRA provinces.These bioregions have been widely adopted for marine conservation and management purposes across Australia and as such are a useful addition to the biogeographic hierarchy.</skos:definition>
	<dc:source rdf:datatype="http://www.w3.org/2001/XMLSchema#string">SeaMap Australia National Benthic Habitat Classification Scheme (2017)</dc:source>
	<skos:narrower rdf:resource="http://seamapaustralia.org.au/def/benthichabitatclassification/class/106"/>
	<skos:narrower rdf:resource="http://seamapaustralia.org.au/def/benthichabitatclassification/class/111"/>
	<skos:narrower rdf:resource="http://seamapaustralia.org.au/def/benthichabitatclassification/class/112"/>
	<skos:closeMatch rdf:resource="http://marineregions.org/rest/getGazetteerRecordsBySource.xml/Spalding%20et%20al.%3B%202007/"/>
	<skos:closeMatch rdf:resource="http://spatial.ala.org.au/?layers=imcra4_pb"/>
	<skos:topConceptOf rdf:resource="http://seamapaustralia.org.au/def/benthichabitatclassification/1"/>
</rdf:Description>

<rdf:Description rdf:about="http://seamapaustralia.org.au/def/benthichabitatclassification/class/98">
	<rdf:type rdf:resource="http://www.w3.org/2000/01/rdf-schema#Resource"/>
	<rdf:type rdf:resource="http://www.w3.org/2004/02/skos/core#Concept"/>
	<skos:prefLabel xml:lang="en">Aquatic Setting</skos:prefLabel>
	<dcterms:contributor rdf:resource="http://editor.vocabs.ands.org.au/user/eMII_Finney.Kim_Admin"/>
	<dcterms:created rdf:datatype="http://www.w3.org/2001/XMLSchema#dateTime">2017-05-23T02:36:03Z</dcterms:created>
	<dcterms:creator rdf:resource="http://editor.vocabs.ands.org.au/user/eMII_Finney.Kim_Admin"/>
	<dcterms:modified rdf:datatype="http://www.w3.org/2001/XMLSchema#dateTime">2017-06-27T04:01:56Z</dcterms:modified>
	<dc:publisher rdf:datatype="http://www.w3.org/2001/XMLSchema#string">  Institute for Marine and Antarctic Studies (IMAS) - UTAS</dc:publisher>
	<skos:definition xml:lang="en">The Aquatic Setting in the CMECS (FGDC, 2012) Standard comprises three hierarchical levels (System, Subsystem and Tidal Zone) separating ocean, estuarine and lacustrine environments, deep and shallow waters, and submerged and intertidal environments. The 'system' is based on salinity and geomorphological characteristics, the 'subsystem' separates classes according to depth and position relative to the shoreline, and 'tidal zone' is determined by tidal influence. This Seamap classification setting has, however, been modified from CMECS in that the boundary between Open Water and Coastal Estuarine subsystems from 4m to 6m now align with the RAMSAR Wetlands of International Importance (UNESCO 1971) as suggested by Edmunds and Flynn (2015). Additionally the CMEC Standard Aquatic Setting uses Mean Lower Low Water (MLLW) and Mean Higher High Water (MHHW), to define tidal zones and estuarine subsystems, but Seamap considers the Lowest Astronomical Tide (LAT) and Highest Astronomical Tide (HAT) to be a better representation of these zones. The Seamap Aquatic Settings classification only applies to benthic substrates on the continental shelf between the HAT and 200m depth contour and Aquatic Setting concept definitions are modified to reflect this where necessary. CMECS Aquatic Setting classes outside of this zone (Marine oceanic, supra tidal zones) are excluded.</skos:definition>
	<dc:source rdf:datatype="http://www.w3.org/2001/XMLSchema#string">SeaMap Australia National Benthic Habitat Classification Scheme (2017)</dc:source>
	<skos:narrower rdf:resource="http://seamapaustralia.org.au/def/benthichabitatclassification/class/121"/>
	<skos:narrower rdf:resource="http://seamapaustralia.org.au/def/benthichabitatclassification/class/122"/>
	<skos:closeMatch rdf:resource="https://www.cmecscatalog.org/cmecs/classification/aquaticSettings.html"/>
	<skos:topConceptOf rdf:resource="http://seamapaustralia.org.au/def/benthichabitatclassification/1"/>
</rdf:Description>

<rdf:Description rdf:about="http://seamapaustralia.org.au/def/benthichabitatclassification/class/227">
	<rdf:type rdf:resource="http://www.w3.org/2000/01/rdf-schema#Resource"/>
	<rdf:type rdf:resource="http://www.w3.org/2004/02/skos/core#Concept"/>
	<skos:broader rdf:resource="http://seamapaustralia.org.au/def/benthichabitatclassification/class/115"/>
	<skos:prefLabel xml:lang="en">MEOW Manning-Hawkesbury Ecoregion</skos:prefLabel>
	<dcterms:contributor rdf:resource="http://editor.vocabs.ands.org.au/user/eMII_Finney.Kim_Admin"/>
	<dcterms:created rdf:datatype="http://www.w3.org/2001/XMLSchema#dateTime">2017-05-31T02:47:20Z</dcterms:created>
	<dcterms:creator rdf:resource="http://editor.vocabs.ands.org.au/user/eMII_Finney.Kim_Admin"/>
	<dcterms:modified rdf:datatype="http://www.w3.org/2001/XMLSchema#dateTime">2017-06-27T04:12:21Z</dcterms:modified>
	<dc:publisher rdf:datatype="http://www.w3.org/2001/XMLSchema#string">Institute for Marine and Antarctic Studies (IMAS) - UTAS</dc:publisher>
	<skos:definition xml:lang="en">An area of relatively homogenous species composition, clearly distinct from adjacent systems. The species composition is likely to be determined by the predominance of a small number of ecosystems and/or a distinct suite of oceanographic or topographic features. The dominant biogeographic forcing agents defining the ecoregions vary from location to location but may include isolation, upwelling, nutrient inputs, freshwater influx, temperature regimes, ice regimes, exposure, sediments, currents and bathymetric or coastal complexity.</skos:definition>
	<dc:source rdf:datatype="http://www.w3.org/2001/XMLSchema#string">Marine Ecoregions of the World (MEOW). Spalding et.al. (2007)</dc:source>
	<skos:narrower rdf:resource="http://seamapaustralia.org.au/def/benthichabitatclassification/class/285"/>
	<skos:exactMatch rdf:resource="http://www.marineregions.org/gazetteer.php?p=details&amp;id=21864"/>
</rdf:Description>

<rdf:Description rdf:about="http://seamapaustralia.org.au/def/benthichabitatclassification/class/115">
	<rdf:type rdf:resource="http://www.w3.org/2000/01/rdf-schema#Resource"/>
	<rdf:type rdf:resource="http://www.w3.org/2004/02/skos/core#Concept"/>
	<skos:broader rdf:resource="http://seamapaustralia.org.au/def/benthichabitatclassification/class/111"/>
	<skos:prefLabel xml:lang="en">MEOW East Central Australian Shelf Province</skos:prefLabel>
	<dcterms:contributor rdf:resource="http://editor.vocabs.ands.org.au/user/eMII_Finney.Kim_Admin"/>
	<dcterms:created rdf:datatype="http://www.w3.org/2001/XMLSchema#dateTime">2017-05-23T03:57:12Z</dcterms:created>
	<dcterms:creator rdf:resource="http://editor.vocabs.ands.org.au/user/eMII_Finney.Kim_Admin"/>
	<dcterms:modified rdf:datatype="http://www.w3.org/2001/XMLSchema#dateTime">2017-06-27T04:12:16Z</dcterms:modified>
	<dc:publisher rdf:datatype="http://www.w3.org/2001/XMLSchema#string">Institute for Marine and Antarctic Studies (IMAS) - UTAS</dc:publisher>
	<skos:definition xml:lang="en">A large area defined by the presence of distinct biotas that has at least some cohesion over evolutionary time frames. Provinces will hold some level of endemism, principally at the level of species. Although historical isolation will play a role, many of these distinct biotas have arisen as a result of distinctive abiotic features that circumscribe their boundaries. These may include geomorphological features (isoloated island and shelf systems, semienclosed seas); hydrographic features (currents, upwellings, ice dynamics); or geochemical influences (broadest-scale elements of nutrient supply and salinity).</skos:definition>
	<dc:source rdf:datatype="http://www.w3.org/2001/XMLSchema#string">Marine Ecoregions of the World (MEOW). Spalding et.al. (2007)</dc:source>
	<skos:narrower rdf:resource="http://seamapaustralia.org.au/def/benthichabitatclassification/class/227"/>
	<skos:narrower rdf:resource="http://seamapaustralia.org.au/def/benthichabitatclassification/class/226"/>
	<skos:exactMatch rdf:resource="http://www.marineregions.org/gazetteer.php?p=details&amp;id=21747"/>
</rdf:Description>

<rdf:Description rdf:about="http://seamapaustralia.org.au/def/benthichabitatclassification/class/106">
	<rdf:type rdf:resource="http://www.w3.org/2000/01/rdf-schema#Resource"/>
	<rdf:type rdf:resource="http://www.w3.org/2004/02/skos/core#Concept"/>
	<skos:broader rdf:resource="http://seamapaustralia.org.au/def/benthichabitatclassification/class/97"/>
	<skos:prefLabel xml:lang="en">MEOW Central Indo-Pacific Realm</skos:prefLabel>
	<dcterms:contributor rdf:resource="http://editor.vocabs.ands.org.au/user/eMII_Finney.Kim_Admin"/>
	<dcterms:created rdf:datatype="http://www.w3.org/2001/XMLSchema#dateTime">2017-05-23T03:47:48Z</dcterms:created>
	<dcterms:creator rdf:resource="http://editor.vocabs.ands.org.au/user/eMII_Finney.Kim_Admin"/>
	<dcterms:modified rdf:datatype="http://www.w3.org/2001/XMLSchema#dateTime">2017-06-27T04:06:54Z</dcterms:modified>
	<dc:publisher rdf:datatype="http://www.w3.org/2001/XMLSchema#string">Institute for Marine and Antarctic Studies (IMAS) - UTAS</dc:publisher>
	<skos:definition xml:lang="en">A very large region of coastal, benthic, or pelagic ocean across which biotas are internally coherent at higher taxonomic levels as a result of a shared and unique evolutionary history. Realms have high levels of endemism, including unique taxa at generic and family levels in some groups. Driving factors behind the development of such unique biota include water temperature, historical and broad scale isolation, and the proximity of the benthos.</skos:definition>
	<dc:source rdf:datatype="http://www.w3.org/2001/XMLSchema#string">Marine Ecoregions of the World (MEOW). Spalding et.al. (2007)</dc:source>
	<skos:narrower rdf:resource="http://seamapaustralia.org.au/def/benthichabitatclassification/class/176"/>
	<skos:narrower rdf:resource="http://seamapaustralia.org.au/def/benthichabitatclassification/class/173"/>
	<skos:narrower rdf:resource="http://seamapaustralia.org.au/def/benthichabitatclassification/class/171"/>
	<skos:narrower rdf:resource="http://seamapaustralia.org.au/def/benthichabitatclassification/class/170"/>
	<skos:narrower rdf:resource="http://seamapaustralia.org.au/def/benthichabitatclassification/class/172"/>
	<skos:narrower rdf:resource="http://seamapaustralia.org.au/def/benthichabitatclassification/class/174"/>
	<skos:narrower rdf:resource="http://seamapaustralia.org.au/def/benthichabitatclassification/class/175"/>
	<skos:narrower rdf:resource="http://seamapaustralia.org.au/def/benthichabitatclassification/class/177"/>
	<skos:exactMatch rdf:resource="http://www.marineregions.org/gazetteer.php?p=details&amp;id=21718"/>
</rdf:Description>

<rdf:Description rdf:about="http://seamapaustralia.org.au/def/benthichabitatclassification/class/111">
	<rdf:type rdf:resource="http://www.w3.org/2000/01/rdf-schema#Resource"/>
	<rdf:type rdf:resource="http://www.w3.org/2004/02/skos/core#Concept"/>
	<skos:broader rdf:resource="http://seamapaustralia.org.au/def/benthichabitatclassification/class/97"/>
	<skos:prefLabel xml:lang="en">MEOW Temperate Australasia Realm</skos:prefLabel>
	<dcterms:contributor rdf:resource="http://editor.vocabs.ands.org.au/user/eMII_Finney.Kim_Admin"/>
	<dcterms:created rdf:datatype="http://www.w3.org/2001/XMLSchema#dateTime">2017-05-23T03:50:09Z</dcterms:created>
	<dcterms:creator rdf:resource="http://editor.vocabs.ands.org.au/user/eMII_Finney.Kim_Admin"/>
	<dcterms:modified rdf:datatype="http://www.w3.org/2001/XMLSchema#dateTime">2017-06-27T04:11:56Z</dcterms:modified>
	<dc:publisher rdf:datatype="http://www.w3.org/2001/XMLSchema#string">Institute for Marine and Antarctic Studies (IMAS) - UTAS</dc:publisher>
	<skos:definition xml:lang="en">A very large region of coastal, benthic, or pelagic ocean across which biotas are internally coherent at higher taxonomic levels as a result of a shared and unique evolutionary history. Realms have high levels of endemism, including unique taxa at generic and family levels in some groups. Driving factors behind the development of such unique biota include water temperature, historical and broad scale isolation, and the proximity of the benthos.</skos:definition>
	<dc:source rdf:datatype="http://www.w3.org/2001/XMLSchema#string">Marine Ecoregions of the World (MEOW). Spalding et.al. (2007)</dc:source>
	<skos:narrower rdf:resource="http://seamapaustralia.org.au/def/benthichabitatclassification/class/115"/>
	<skos:narrower rdf:resource="http://seamapaustralia.org.au/def/benthichabitatclassification/class/117"/>
	<skos:narrower rdf:resource="http://seamapaustralia.org.au/def/benthichabitatclassification/class/116"/>
	<skos:narrower rdf:resource="http://seamapaustralia.org.au/def/benthichabitatclassification/class/118"/>
	<skos:exactMatch rdf:resource="http://www.marineregions.org/gazetteer.php?p=details&amp;id=21724"/>
</rdf:Description>

<rdf:Description rdf:about="http://seamapaustralia.org.au/def/benthichabitatclassification/class/191">
	<rdf:type rdf:resource="http://www.w3.org/2000/01/rdf-schema#Resource"/>
	<rdf:type rdf:resource="http://www.w3.org/2004/02/skos/core#Concept"/>
	<skos:broader rdf:resource="http://seamapaustralia.org.au/def/benthichabitatclassification/class/173"/>
	<skos:prefLabel xml:lang="en">MEOW Arnhem Coast to Gulf of Carpentaria Ecoregion</skos:prefLabel>
	<dcterms:contributor rdf:resource="http://editor.vocabs.ands.org.au/user/eMII_Finney.Kim_Admin"/>
	<dcterms:created rdf:datatype="http://www.w3.org/2001/XMLSchema#dateTime">2017-05-31T02:04:58Z</dcterms:created>
	<dcterms:creator rdf:resource="http://editor.vocabs.ands.org.au/user/eMII_Finney.Kim_Admin"/>
	<dcterms:modified rdf:datatype="http://www.w3.org/2001/XMLSchema#dateTime">2017-06-27T04:09:19Z</dcterms:modified>
	<dc:publisher rdf:datatype="http://www.w3.org/2001/XMLSchema#string">Institute for Marine and Antarctic Studies (IMAS) - UTAS</dc:publisher>
	<skos:definition xml:lang="en">An area of relatively homogenous species composition, clearly distinct from adjacent systems. The species composition is likely to be determined by the predominance of a small number of ecosystems and/or a distinct suite of oceanographic or topographic features. The dominant biogeographic forcing agents defining the ecoregions vary from location to location but may include isolation, upwelling, nutrient inputs, freshwater influx, temperature regimes, ice regimes, exposure, sediments, currents and bathymetric or coastal complexity.</skos:definition>
	<dc:source rdf:datatype="http://www.w3.org/2001/XMLSchema#string">Marine Ecoregions of the World (MEOW). Spalding et.al. (2007)</dc:source>
	<skos:narrower rdf:resource="http://seamapaustralia.org.au/def/benthichabitatclassification/class/298"/>
	<skos:exactMatch rdf:resource="http://www.marineregions.org/gazetteer.php?p=details&amp;id=21922"/>
</rdf:Description>

<rdf:Description rdf:about="http://seamapaustralia.org.au/def/benthichabitatclassification/class/189">
	<rdf:type rdf:resource="http://www.w3.org/2000/01/rdf-schema#Resource"/>
	<rdf:type rdf:resource="http://www.w3.org/2004/02/skos/core#Concept"/>
	<skos:broader rdf:resource="http://seamapaustralia.org.au/def/benthichabitatclassification/class/173"/>
	<skos:prefLabel xml:lang="en">MEOW Gulf of Papua Ecoregion</skos:prefLabel>
	<dcterms:contributor rdf:resource="http://editor.vocabs.ands.org.au/user/eMII_Finney.Kim_Admin"/>
	<dcterms:created rdf:datatype="http://www.w3.org/2001/XMLSchema#dateTime">2017-05-31T02:04:05Z</dcterms:created>
	<dcterms:creator rdf:resource="http://editor.vocabs.ands.org.au/user/eMII_Finney.Kim_Admin"/>
	<dcterms:modified rdf:datatype="http://www.w3.org/2001/XMLSchema#dateTime">2017-06-27T04:09:35Z</dcterms:modified>
	<dc:publisher rdf:datatype="http://www.w3.org/2001/XMLSchema#string">Institute for Marine and Antarctic Studies (IMAS) - UTAS</dc:publisher>
	<skos:definition xml:lang="en">An area of relatively homogenous species composition, clearly distinct from adjacent systems. The species composition is likely to be determined by the predominance of a small number of ecosystems and/or a distinct suite of oceanographic or topographic features. The dominant biogeographic forcing agents defining the ecoregions vary from location to location but may include isolation, upwelling, nutrient inputs, freshwater influx, temperature regimes, ice regimes, exposure, sediments, currents and bathymetric or coastal complexity.</skos:definition>
	<dc:source rdf:datatype="http://www.w3.org/2001/XMLSchema#string">Marine Ecoregions of the World (MEOW). Spalding et.al. (2007)</dc:source>
	<skos:exactMatch rdf:resource="http://www.marineregions.org/gazetteer.php?p=details&amp;id=21921"/>
</rdf:Description>

<rdf:Description rdf:about="http://www.marineregions.org/gazetteer.php?p=details&amp;id=21921">
	<rdf:type rdf:resource="http://www.w3.org/2000/01/rdf-schema#Resource"/>
</rdf:Description>

<rdf:Description rdf:about="http://seamapaustralia.org.au/def/benthichabitatclassification/class/232">
	<rdf:type rdf:resource="http://www.w3.org/2000/01/rdf-schema#Resource"/>
	<rdf:type rdf:resource="http://www.w3.org/2004/02/skos/core#Concept"/>
	<skos:broader rdf:resource="http://seamapaustralia.org.au/def/benthichabitatclassification/class/117"/>
	<skos:prefLabel xml:lang="en">MEOW Great Australian Bight Ecoregion</skos:prefLabel>
	<dcterms:contributor rdf:resource="http://editor.vocabs.ands.org.au/user/eMII_Finney.Kim_Admin"/>
	<dcterms:created rdf:datatype="http://www.w3.org/2001/XMLSchema#dateTime">2017-05-31T02:50:39Z</dcterms:created>
	<dcterms:creator rdf:resource="http://editor.vocabs.ands.org.au/user/eMII_Finney.Kim_Admin"/>
	<dcterms:modified rdf:datatype="http://www.w3.org/2001/XMLSchema#dateTime">2017-06-27T04:13:18Z</dcterms:modified>
	<dc:publisher rdf:datatype="http://www.w3.org/2001/XMLSchema#string">Institute for Marine and Antarctic Studies (IMAS) - UTAS</dc:publisher>
	<skos:definition xml:lang="en">An area of relatively homogenous species composition, clearly distinct from adjacent systems. The species composition is likely to be determined by the predominance of a small number of ecosystems and/or a distinct suite of oceanographic or topographic features. The dominant biogeographic forcing agents defining the ecoregions vary from location to location but may include isolation, upwelling, nutrient inputs, freshwater influx, temperature regimes, ice regimes, exposure, sediments, currents and bathymetric or coastal complexity.</skos:definition>
	<dc:source rdf:datatype="http://www.w3.org/2001/XMLSchema#string">Marine Ecoregions of the World (MEOW). Spalding et.al. (2007)</dc:source>
	<skos:narrower rdf:resource="http://seamapaustralia.org.au/def/benthichabitatclassification/class/267"/>
	<skos:exactMatch rdf:resource="http://www.marineregions.org/gazetteer.php?p=details&amp;id=21949"/>
</rdf:Description>

<rdf:Description rdf:about="http://seamapaustralia.org.au/def/benthichabitatclassification/class/117">
	<rdf:type rdf:resource="http://www.w3.org/2000/01/rdf-schema#Resource"/>
	<rdf:type rdf:resource="http://www.w3.org/2004/02/skos/core#Concept"/>
	<skos:broader rdf:resource="http://seamapaustralia.org.au/def/benthichabitatclassification/class/111"/>
	<skos:prefLabel xml:lang="en">MEOW Southwest Australian Shelf Province</skos:prefLabel>
	<dcterms:contributor rdf:resource="http://editor.vocabs.ands.org.au/user/eMII_Finney.Kim_Admin"/>
	<dcterms:created rdf:datatype="http://www.w3.org/2001/XMLSchema#dateTime">2017-05-23T03:58:03Z</dcterms:created>
	<dcterms:creator rdf:resource="http://editor.vocabs.ands.org.au/user/eMII_Finney.Kim_Admin"/>
	<dcterms:modified rdf:datatype="http://www.w3.org/2001/XMLSchema#dateTime">2017-06-27T04:13:13Z</dcterms:modified>
	<dc:publisher rdf:datatype="http://www.w3.org/2001/XMLSchema#string">Institute for Marine and Antarctic Studies (IMAS) - UTAS</dc:publisher>
	<skos:definition xml:lang="en">A large area defined by the presence of distinct biotas that has at least some cohesion over evolutionary time frames. Provinces will hold some level of endemism, principally at the level of species. Although historical isolation will play a role, many of these distinct biotas have arisen as a result of distinctive abiotic features that circumscribe their boundaries. These may include geomorphological features (isoloated island and shelf systems, semienclosed seas); hydrographic features (currents, upwellings, ice dynamics); or geochemical influences (broadest-scale elements of nutrient supply and salinity).</skos:definition>
	<dc:source rdf:datatype="http://www.w3.org/2001/XMLSchema#string">Marine Ecoregions of the World (MEOW). Spalding et.al. (2007)</dc:source>
	<skos:narrower rdf:resource="http://seamapaustralia.org.au/def/benthichabitatclassification/class/232"/>
	<skos:narrower rdf:resource="http://seamapaustralia.org.au/def/benthichabitatclassification/class/233"/>
	<skos:narrower rdf:resource="http://seamapaustralia.org.au/def/benthichabitatclassification/class/231"/>
	<skos:exactMatch rdf:resource="http://www.marineregions.org/gazetteer.php?p=details&amp;id=21745"/>
</rdf:Description>

<rdf:Description rdf:about="http://seamapaustralia.org.au/def/benthichabitatclassification/class/233">
	<rdf:type rdf:resource="http://www.w3.org/2000/01/rdf-schema#Resource"/>
	<rdf:type rdf:resource="http://www.w3.org/2004/02/skos/core#Concept"/>
	<skos:broader rdf:resource="http://seamapaustralia.org.au/def/benthichabitatclassification/class/117"/>
	<skos:prefLabel xml:lang="en">MEOW Leeuwin Ecoregion</skos:prefLabel>
	<dcterms:contributor rdf:resource="http://editor.vocabs.ands.org.au/user/eMII_Finney.Kim_Admin"/>
	<dcterms:created rdf:datatype="http://www.w3.org/2001/XMLSchema#dateTime">2017-05-31T02:51:05Z</dcterms:created>
	<dcterms:creator rdf:resource="http://editor.vocabs.ands.org.au/user/eMII_Finney.Kim_Admin"/>
	<dcterms:modified rdf:datatype="http://www.w3.org/2001/XMLSchema#dateTime">2017-06-27T04:13:25Z</dcterms:modified>
	<dc:publisher rdf:datatype="http://www.w3.org/2001/XMLSchema#string">Institute for Marine and Antarctic Studies (IMAS) - UTAS</dc:publisher>
	<skos:definition xml:lang="en">An area of relatively homogenous species composition, clearly distinct from adjacent systems. The species composition is likely to be determined by the predominance of a small number of ecosystems and/or a distinct suite of oceanographic or topographic features. The dominant biogeographic forcing agents defining the ecoregions vary from location to location but may include isolation, upwelling, nutrient inputs, freshwater influx, temperature regimes, ice regimes, exposure, sediments, currents and bathymetric or coastal complexity.</skos:definition>
	<dc:source rdf:datatype="http://www.w3.org/2001/XMLSchema#string">Marine Ecoregions of the World (MEOW). Spalding et.al. (2007)</dc:source>
	<skos:narrower rdf:resource="http://seamapaustralia.org.au/def/benthichabitatclassification/class/270"/>
	<skos:exactMatch rdf:resource="http://www.marineregions.org/gazetteer.php?p=details&amp;id=21950"/>
</rdf:Description>

<rdf:Description rdf:about="http://seamapaustralia.org.au/def/benthichabitatclassification/class/231">
	<rdf:type rdf:resource="http://www.w3.org/2000/01/rdf-schema#Resource"/>
	<rdf:type rdf:resource="http://www.w3.org/2004/02/skos/core#Concept"/>
	<skos:broader rdf:resource="http://seamapaustralia.org.au/def/benthichabitatclassification/class/117"/>
	<skos:prefLabel xml:lang="en">MEOW South Australian Gulfs Ecoregion</skos:prefLabel>
	<dcterms:contributor rdf:resource="http://editor.vocabs.ands.org.au/user/eMII_Finney.Kim_Admin"/>
	<dcterms:created rdf:datatype="http://www.w3.org/2001/XMLSchema#dateTime">2017-05-31T02:50:06Z</dcterms:created>
	<dcterms:creator rdf:resource="http://editor.vocabs.ands.org.au/user/eMII_Finney.Kim_Admin"/>
	<dcterms:modified rdf:datatype="http://www.w3.org/2001/XMLSchema#dateTime">2017-06-27T04:13:39Z</dcterms:modified>
	<dc:publisher rdf:datatype="http://www.w3.org/2001/XMLSchema#string">Institute for Marine and Antarctic Studies (IMAS) - UTAS</dc:publisher>
	<skos:definition xml:lang="en">An area of relatively homogenous species composition, clearly distinct from adjacent systems. The species composition is likely to be determined by the predominance of a small number of ecosystems and/or a distinct suite of oceanographic or topographic features. The dominant biogeographic forcing agents defining the ecoregions vary from location to location but may include isolation, upwelling, nutrient inputs, freshwater influx, temperature regimes, ice regimes, exposure, sediments, currents and bathymetric or coastal complexity.</skos:definition>
	<dc:source rdf:datatype="http://www.w3.org/2001/XMLSchema#string">Marine Ecoregions of the World (MEOW). Spalding et.al. (2007)</dc:source>
	<skos:narrower rdf:resource="http://seamapaustralia.org.au/def/benthichabitatclassification/class/273"/>
	<skos:exactMatch rdf:resource="http://www.marineregions.org/gazetteer.php?p=details&amp;id=21951"/>
</rdf:Description>

<rdf:Description rdf:about="http://marineregions.org/rest/getGazetteerRecordsBySource.xml/Spalding%20et%20al.%3B%202007/">
	<rdf:type rdf:resource="http://www.w3.org/2000/01/rdf-schema#Resource"/>
</rdf:Description>

<rdf:Description rdf:about="http://seamapaustralia.org.au/def/benthichabitatclassification/class/112">
	<rdf:type rdf:resource="http://www.w3.org/2000/01/rdf-schema#Resource"/>
	<rdf:type rdf:resource="http://www.w3.org/2004/02/skos/core#Concept"/>
	<skos:broader rdf:resource="http://seamapaustralia.org.au/def/benthichabitatclassification/class/97"/>
	<skos:prefLabel xml:lang="en">MEOW Southern Ocean Realm</skos:prefLabel>
	<dcterms:contributor rdf:resource="http://editor.vocabs.ands.org.au/user/eMII_Finney.Kim_Admin"/>
	<dcterms:created rdf:datatype="http://www.w3.org/2001/XMLSchema#dateTime">2017-05-23T03:54:13Z</dcterms:created>
	<dcterms:creator rdf:resource="http://editor.vocabs.ands.org.au/user/eMII_Finney.Kim_Admin"/>
	<dcterms:modified rdf:datatype="http://www.w3.org/2001/XMLSchema#dateTime">2017-06-27T04:10:31Z</dcterms:modified>
	<dc:publisher rdf:datatype="http://www.w3.org/2001/XMLSchema#string">Institute for Marine and Antarctic Studies (IMAS) - UTAS</dc:publisher>
	<skos:definition xml:lang="en">A very large region of coastal, benthic, or pelagic ocean across which biotas are internally coherent at higher taxonomic levels as a result of a shared and unique evolutionary history. Realms have high levels of endemism, including unique taxa at generic and family levels in some groups. Driving factors behind the development of such unique biota include water temperature, historical and broad scale isolation, and the proximity of the benthos.</skos:definition>
	<dc:source rdf:datatype="http://www.w3.org/2001/XMLSchema#string">Marine Ecoregions of the World (MEOW). Spalding et.al. (2007)</dc:source>
	<skos:narrower rdf:resource="http://seamapaustralia.org.au/def/benthichabitatclassification/class/211"/>
	<skos:narrower rdf:resource="http://seamapaustralia.org.au/def/benthichabitatclassification/class/210"/>
	<skos:exactMatch rdf:resource="http://www.marineregions.org/gazetteer.php?p=details&amp;id=21723"/>
</rdf:Description>

<rdf:Description rdf:about="http://seamapaustralia.org.au/def/benthichabitatclassification/class/226">
	<rdf:type rdf:resource="http://www.w3.org/2000/01/rdf-schema#Resource"/>
	<rdf:type rdf:resource="http://www.w3.org/2004/02/skos/core#Concept"/>
	<skos:broader rdf:resource="http://seamapaustralia.org.au/def/benthichabitatclassification/class/115"/>
	<skos:prefLabel xml:lang="en">MEOW Tweed-Moreton Ecoregion</skos:prefLabel>
	<dcterms:contributor rdf:resource="http://editor.vocabs.ands.org.au/user/eMII_Finney.Kim_Admin"/>
	<dcterms:created rdf:datatype="http://www.w3.org/2001/XMLSchema#dateTime">2017-05-31T02:46:39Z</dcterms:created>
	<dcterms:creator rdf:resource="http://editor.vocabs.ands.org.au/user/eMII_Finney.Kim_Admin"/>
	<dcterms:modified rdf:datatype="http://www.w3.org/2001/XMLSchema#dateTime">2017-06-27T04:12:32Z</dcterms:modified>
	<dc:publisher rdf:datatype="http://www.w3.org/2001/XMLSchema#string">Institute for Marine and Antarctic Studies (IMAS) - UTAS</dc:publisher>
	<skos:definition xml:lang="en">An area of relatively homogenous species composition, clearly distinct from adjacent systems. The species composition is likely to be determined by the predominance of a small number of ecosystems and/or a distinct suite of oceanographic or topographic features. The dominant biogeographic forcing agents defining the ecoregions vary from location to location but may include isolation, upwelling, nutrient inputs, freshwater influx, temperature regimes, ice regimes, exposure, sediments, currents and bathymetric or coastal complexity.</skos:definition>
	<dc:source rdf:datatype="http://www.w3.org/2001/XMLSchema#string">Marine Ecoregions of the World (MEOW). Spalding et.al. (2007)</dc:source>
	<skos:narrower rdf:resource="http://seamapaustralia.org.au/def/benthichabitatclassification/class/288"/>
	<skos:exactMatch rdf:resource="http://www.marineregions.org/gazetteer.php?p=details&amp;id=21863"/>
</rdf:Description>

<rdf:Description rdf:about="http://seamapaustralia.org.au/def/benthichabitatclassification/class/230">
	<rdf:type rdf:resource="http://www.w3.org/2000/01/rdf-schema#Resource"/>
	<rdf:type rdf:resource="http://www.w3.org/2004/02/skos/core#Concept"/>
	<skos:broader rdf:resource="http://seamapaustralia.org.au/def/benthichabitatclassification/class/116"/>
	<skos:prefLabel xml:lang="en">MEOW Western Bassian Ecoregion</skos:prefLabel>
	<dcterms:contributor rdf:resource="http://editor.vocabs.ands.org.au/user/eMII_Finney.Kim_Admin"/>
	<dcterms:created rdf:datatype="http://www.w3.org/2001/XMLSchema#dateTime">2017-05-31T02:49:05Z</dcterms:created>
	<dcterms:creator rdf:resource="http://editor.vocabs.ands.org.au/user/eMII_Finney.Kim_Admin"/>
	<dcterms:modified rdf:datatype="http://www.w3.org/2001/XMLSchema#dateTime">2017-06-27T04:13:04Z</dcterms:modified>
	<dc:publisher rdf:datatype="http://www.w3.org/2001/XMLSchema#string">Institute for Marine and Antarctic Studies (IMAS) - UTAS</dc:publisher>
	<skos:definition xml:lang="en">An area of relatively homogenous species composition, clearly distinct from adjacent systems. The species composition is likely to be determined by the predominance of a small number of ecosystems and/or a distinct suite of oceanographic or topographic features. The dominant biogeographic forcing agents defining the ecoregions vary from location to location but may include isolation, upwelling, nutrient inputs, freshwater influx, temperature regimes, ice regimes, exposure, sediments, currents and bathymetric or coastal complexity.</skos:definition>
	<dc:source rdf:datatype="http://www.w3.org/2001/XMLSchema#string">Marine Ecoregions of the World (MEOW). Spalding et.al. (2007)</dc:source>
	<skos:narrower rdf:resource="http://seamapaustralia.org.au/def/benthichabitatclassification/class/262"/>
	<skos:exactMatch rdf:resource="http://www.marineregions.org/gazetteer.php?p=details&amp;id=21939"/>
</rdf:Description>

<rdf:Description rdf:about="http://seamapaustralia.org.au/def/benthichabitatclassification/class/116">
	<rdf:type rdf:resource="http://www.w3.org/2000/01/rdf-schema#Resource"/>
	<rdf:type rdf:resource="http://www.w3.org/2004/02/skos/core#Concept"/>
	<skos:broader rdf:resource="http://seamapaustralia.org.au/def/benthichabitatclassification/class/111"/>
	<skos:prefLabel xml:lang="en">MEOW Southeast Australian Shelf Province</skos:prefLabel>
	<dcterms:contributor rdf:resource="http://editor.vocabs.ands.org.au/user/eMII_Finney.Kim_Admin"/>
	<dcterms:created rdf:datatype="http://www.w3.org/2001/XMLSchema#dateTime">2017-05-23T03:57:32Z</dcterms:created>
	<dcterms:creator rdf:resource="http://editor.vocabs.ands.org.au/user/eMII_Finney.Kim_Admin"/>
	<dcterms:modified rdf:datatype="http://www.w3.org/2001/XMLSchema#dateTime">2017-06-27T04:12:44Z</dcterms:modified>
	<dc:publisher rdf:datatype="http://www.w3.org/2001/XMLSchema#string">Institute for Marine and Antarctic Studies (IMAS) - UTAS</dc:publisher>
	<skos:definition xml:lang="en">A large area defined by the presence of distinct biotas that has at least some cohesion over evolutionary time frames. Provinces will hold some level of endemism, principally at the level of species. Although historical isolation will play a role, many of these distinct biotas have arisen as a result of distinctive abiotic features that circumscribe their boundaries. These may include geomorphological features (isoloated island and shelf systems, semienclosed seas); hydrographic features (currents, upwellings, ice dynamics); or geochemical influences (broadest-scale elements of nutrient supply and salinity).</skos:definition>
	<dc:source rdf:datatype="http://www.w3.org/2001/XMLSchema#string">Marine Ecoregions of the World (MEOW). Spalding et.al. (2007)</dc:source>
	<skos:narrower rdf:resource="http://seamapaustralia.org.au/def/benthichabitatclassification/class/230"/>
	<skos:narrower rdf:resource="http://seamapaustralia.org.au/def/benthichabitatclassification/class/229"/>
	<skos:narrower rdf:resource="http://seamapaustralia.org.au/def/benthichabitatclassification/class/228"/>
	<skos:exactMatch rdf:resource="http://www.marineregions.org/gazetteer.php?p=details&amp;id=21744"/>
</rdf:Description>

<rdf:Description rdf:about="http://seamapaustralia.org.au/def/benthichabitatclassification/class/229">
	<rdf:type rdf:resource="http://www.w3.org/2000/01/rdf-schema#Resource"/>
	<rdf:type rdf:resource="http://www.w3.org/2004/02/skos/core#Concept"/>
	<skos:broader rdf:resource="http://seamapaustralia.org.au/def/benthichabitatclassification/class/116"/>
	<skos:prefLabel xml:lang="en">MEOW Bassian Ecoregion</skos:prefLabel>
	<dcterms:contributor rdf:resource="http://editor.vocabs.ands.org.au/user/eMII_Finney.Kim_Admin"/>
	<dcterms:created rdf:datatype="http://www.w3.org/2001/XMLSchema#dateTime">2017-05-31T02:48:43Z</dcterms:created>
	<dcterms:creator rdf:resource="http://editor.vocabs.ands.org.au/user/eMII_Finney.Kim_Admin"/>
	<dcterms:modified rdf:datatype="http://www.w3.org/2001/XMLSchema#dateTime">2017-06-27T04:12:50Z</dcterms:modified>
	<dc:publisher rdf:datatype="http://www.w3.org/2001/XMLSchema#string">Institute for Marine and Antarctic Studies (IMAS) - UTAS</dc:publisher>
	<skos:definition xml:lang="en">An area of relatively homogenous species composition, clearly distinct from adjacent systems. The species composition is likely to be determined by the predominance of a small number of ecosystems and/or a distinct suite of oceanographic or topographic features. The dominant biogeographic forcing agents defining the ecoregions vary from location to location but may include isolation, upwelling, nutrient inputs, freshwater influx, temperature regimes, ice regimes, exposure, sediments, currents and bathymetric or coastal complexity.</skos:definition>
	<dc:source rdf:datatype="http://www.w3.org/2001/XMLSchema#string">Marine Ecoregions of the World (MEOW). Spalding et.al. (2007)</dc:source>
	<skos:narrower rdf:resource="http://seamapaustralia.org.au/def/benthichabitatclassification/class/250"/>
	<skos:narrower rdf:resource="http://seamapaustralia.org.au/def/benthichabitatclassification/class/251"/>
	<skos:exactMatch rdf:resource="http://www.marineregions.org/gazetteer.php?p=details&amp;id=21938"/>
</rdf:Description>

<rdf:Description rdf:about="http://seamapaustralia.org.au/def/benthichabitatclassification/class/118">
	<rdf:type rdf:resource="http://www.w3.org/2000/01/rdf-schema#Resource"/>
	<rdf:type rdf:resource="http://www.w3.org/2004/02/skos/core#Concept"/>
	<skos:broader rdf:resource="http://seamapaustralia.org.au/def/benthichabitatclassification/class/111"/>
	<skos:prefLabel xml:lang="en">MEOW West Central Australian Shelf Province</skos:prefLabel>
	<dcterms:contributor rdf:resource="http://editor.vocabs.ands.org.au/user/eMII_Finney.Kim_Admin"/>
	<dcterms:created rdf:datatype="http://www.w3.org/2001/XMLSchema#dateTime">2017-05-23T03:58:33Z</dcterms:created>
	<dcterms:creator rdf:resource="http://editor.vocabs.ands.org.au/user/eMII_Finney.Kim_Admin"/>
	<dcterms:modified rdf:datatype="http://www.w3.org/2001/XMLSchema#dateTime">2017-06-27T04:13:46Z</dcterms:modified>
	<dc:publisher rdf:datatype="http://www.w3.org/2001/XMLSchema#string">Institute for Marine and Antarctic Studies (IMAS) - UTAS</dc:publisher>
	<skos:definition xml:lang="en">A large area defined by the presence of distinct biotas that has at least some cohesion over evolutionary time frames. Provinces will hold some level of endemism, principally at the level of species. Although historical isolation will play a role, many of these distinct biotas have arisen as a result of distinctive abiotic features that circumscribe their boundaries. These may include geomorphological features (isoloated island and shelf systems, semienclosed seas); hydrographic features (currents, upwellings, ice dynamics); or geochemical influences (broadest-scale elements of nutrient supply and salinity).</skos:definition>
	<dc:source rdf:datatype="http://www.w3.org/2001/XMLSchema#string">Marine Ecoregions of the World (MEOW). Spalding et.al. (2007)</dc:source>
	<skos:narrower rdf:resource="http://seamapaustralia.org.au/def/benthichabitatclassification/class/119"/>
	<skos:narrower rdf:resource="http://seamapaustralia.org.au/def/benthichabitatclassification/class/120"/>
	<skos:exactMatch rdf:resource="http://www.marineregions.org/gazetteer.php?p=details&amp;id=21746"/>
</rdf:Description>

<rdf:Description rdf:about="http://seamapaustralia.org.au/def/benthichabitatclassification/class/119">
	<rdf:type rdf:resource="http://www.w3.org/2000/01/rdf-schema#Resource"/>
	<rdf:type rdf:resource="http://www.w3.org/2004/02/skos/core#Concept"/>
	<skos:broader rdf:resource="http://seamapaustralia.org.au/def/benthichabitatclassification/class/118"/>
	<skos:prefLabel xml:lang="en">MEOW Shark Bay Ecoregion</skos:prefLabel>
	<dcterms:contributor rdf:resource="http://editor.vocabs.ands.org.au/user/eMII_Finney.Kim_Admin"/>
	<dcterms:created rdf:datatype="http://www.w3.org/2001/XMLSchema#dateTime">2017-05-23T03:58:57Z</dcterms:created>
	<dcterms:creator rdf:resource="http://editor.vocabs.ands.org.au/user/eMII_Finney.Kim_Admin"/>
	<dcterms:modified rdf:datatype="http://www.w3.org/2001/XMLSchema#dateTime">2017-06-27T04:13:58Z</dcterms:modified>
	<dc:publisher rdf:datatype="http://www.w3.org/2001/XMLSchema#string">Institute for Marine and Antarctic Studies (IMAS) - UTAS</dc:publisher>
	<skos:definition xml:lang="en">An area of relatively homogenous species composition, clearly distinct from adjacent systems. The species composition is likely to be determined by the predominance of a small number of ecosystems and/or a distinct suite of oceanographic or topographic features. The dominant biogeographic forcing agents defining an ecoregion vary from location to location but may include isolation, upwelling, nutrient inputs, freshwater influx, temperature regimes, ice regimes, exposure, sediments, currents and bathymetric or coastal complexity.</skos:definition>
	<dc:source rdf:datatype="http://www.w3.org/2001/XMLSchema#string">Marine Ecoregions of the World (MEOW). Spalding et.al. (2007)</dc:source>
	<skos:exactMatch rdf:resource="http://www.marineregions.org/gazetteer.php?p=details&amp;id=22018"/>
</rdf:Description>

<rdf:Description rdf:about="http://seamapaustralia.org.au/def/benthichabitatclassification/class/120">
	<rdf:type rdf:resource="http://www.w3.org/2000/01/rdf-schema#Resource"/>
	<rdf:type rdf:resource="http://www.w3.org/2004/02/skos/core#Concept"/>
	<skos:broader rdf:resource="http://seamapaustralia.org.au/def/benthichabitatclassification/class/118"/>
	<skos:prefLabel xml:lang="en">MEOW Houtman Ecoregion</skos:prefLabel>
	<dcterms:contributor rdf:resource="http://editor.vocabs.ands.org.au/user/eMII_Finney.Kim_Admin"/>
	<dcterms:created rdf:datatype="http://www.w3.org/2001/XMLSchema#dateTime">2017-05-23T03:59:14Z</dcterms:created>
	<dcterms:creator rdf:resource="http://editor.vocabs.ands.org.au/user/eMII_Finney.Kim_Admin"/>
	<dcterms:modified rdf:datatype="http://www.w3.org/2001/XMLSchema#dateTime">2017-06-27T04:13:51Z</dcterms:modified>
	<dc:publisher rdf:datatype="http://www.w3.org/2001/XMLSchema#string">Institute for Marine and Antarctic Studies (IMAS) - UTAS</dc:publisher>
	<skos:definition xml:lang="en">An area of relatively homogenous species composition, clearly distinct from adjacent systems. The species composition is likely to be determined by the predominance of a small number of ecosystems and/or a distinct suite of oceanographic or topographic features. The dominant biogeographic forcing agents defining an ecoregion vary from location to location but may include isolation, upwelling, nutrient inputs, freshwater influx, temperature regimes, ice regimes, exposure, sediments, currents and bathymetric or coastal complexity.</skos:definition>
	<dc:source rdf:datatype="http://www.w3.org/2001/XMLSchema#string">  Marine Ecoregions of the World (MEOW). Spalding et.al. (2007)</dc:source>
	<skos:narrower rdf:resource="http://seamapaustralia.org.au/def/benthichabitatclassification/class/279"/>
	<skos:narrower rdf:resource="http://seamapaustralia.org.au/def/benthichabitatclassification/class/282"/>
	<skos:exactMatch rdf:resource="http://www.marineregions.org/gazetteer.php?p=details&amp;id=22019"/>
</rdf:Description>

<rdf:Description rdf:about="http://www.marineregions.org/gazetteer.php?p=details&amp;id=22019">
	<rdf:type rdf:resource="http://www.w3.org/2000/01/rdf-schema#Resource"/>
</rdf:Description>

<rdf:Description rdf:about="http://www.marineregions.org/gazetteer.php?p=details&amp;id=22018">
	<rdf:type rdf:resource="http://www.w3.org/2000/01/rdf-schema#Resource"/>
</rdf:Description>

<rdf:Description rdf:about="http://www.marineregions.org/gazetteer.php?p=details&amp;id=21746">
	<rdf:type rdf:resource="http://www.w3.org/2000/01/rdf-schema#Resource"/>
</rdf:Description>

<rdf:Description rdf:about="http://seamapaustralia.org.au/def/benthichabitatclassification/class/121">
	<rdf:type rdf:resource="http://www.w3.org/2000/01/rdf-schema#Resource"/>
	<rdf:type rdf:resource="http://www.w3.org/2004/02/skos/core#Concept"/>
	<skos:broader rdf:resource="http://seamapaustralia.org.au/def/benthichabitatclassification/class/98"/>
	<skos:prefLabel xml:lang="en">Estuarine System</skos:prefLabel>
	<dcterms:contributor rdf:resource="http://editor.vocabs.ands.org.au/user/eMII_Finney.Kim_Admin"/>
	<dcterms:created rdf:datatype="http://www.w3.org/2001/XMLSchema#dateTime">2017-05-23T04:37:46Z</dcterms:created>
	<dcterms:creator rdf:resource="http://editor.vocabs.ands.org.au/user/eMII_Finney.Kim_Admin"/>
	<dcterms:modified rdf:datatype="http://www.w3.org/2001/XMLSchema#dateTime">2017-06-27T04:02:04Z</dcterms:modified>
	<dc:publisher rdf:datatype="http://www.w3.org/2001/XMLSchema#string">Institute for Marine and Antarctic Studies (IMAS) - UTAS</dc:publisher>
	<skos:definition xml:lang="en">This system is defined by salinity and geomorphology. It includes tidally influenced waters that (a) have an open-surface connection to the sea, (b) are regularly diluted by freshwater runoff from land, and (c) exhibit some degree of land enclosure. The Estuarine System extends upstream to the Highest Astronomical Tide (HAT) mark and seaward to the mouth of the estuary. The HAT is defined as the highest level of water which can be predicted to occur under any combination of astronomical conditions (PCTMSL 2014). The mouth of the estuary is defined by an imaginary line connecting the seaward-most points of land that enclose the estuarine water mass at Mean Lower Low Water (MLLW). Islands are included as headlands if they contribute significantly to the enclosure.</skos:definition>
	<dc:source rdf:datatype="http://www.w3.org/2001/XMLSchema#string">SeaMap Australia National Benthic Habitat Classification Scheme (2017)</dc:source>
	<skos:narrower rdf:resource="http://seamapaustralia.org.au/def/benthichabitatclassification/class/123"/>
	<skos:narrower rdf:resource="http://seamapaustralia.org.au/def/benthichabitatclassification/class/124"/>
	<skos:narrower rdf:resource="http://seamapaustralia.org.au/def/benthichabitatclassification/class/125"/>
	<skos:narrower rdf:resource="http://seamapaustralia.org.au/def/benthichabitatclassification/class/126"/>
	<skos:closeMatch rdf:resource="https://www.cmecscatalog.org/cmecs/classification/aquaticSetting/2.html"/>
</rdf:Description>

<rdf:Description rdf:about="http://seamapaustralia.org.au/def/benthichabitatclassification/class/122">
	<rdf:type rdf:resource="http://www.w3.org/2000/01/rdf-schema#Resource"/>
	<rdf:type rdf:resource="http://www.w3.org/2004/02/skos/core#Concept"/>
	<skos:broader rdf:resource="http://seamapaustralia.org.au/def/benthichabitatclassification/class/98"/>
	<skos:prefLabel xml:lang="en">Marine System</skos:prefLabel>
	<dcterms:contributor rdf:resource="http://editor.vocabs.ands.org.au/user/eMII_Finney.Kim_Admin"/>
	<dcterms:created rdf:datatype="http://www.w3.org/2001/XMLSchema#dateTime">2017-05-23T04:37:56Z</dcterms:created>
	<dcterms:creator rdf:resource="http://editor.vocabs.ands.org.au/user/eMII_Finney.Kim_Admin"/>
	<dcterms:modified rdf:datatype="http://www.w3.org/2001/XMLSchema#dateTime">2017-06-27T04:04:11Z</dcterms:modified>
	<dc:publisher rdf:datatype="http://www.w3.org/2001/XMLSchema#string">Institute for Marine and Antarctic Studies (IMAS) - UTAS</dc:publisher>
	<skos:definition xml:lang="en">The Marine System is defined by salinity, which is typically 35 ‰, although can measure as low as 0.5 ‰ during the period of average annual low flow near freshwater outflows. This system has little or no significant dilution from fresh water except near the mouths of estuaries and rivers. The Marine System includes all non-estuarine waters from the coastline to central oceans. The landward boundary of this system is either the linear boundary across the mouth of an estuary or the limit of the intertidal zone.</skos:definition>
	<dc:source rdf:datatype="http://www.w3.org/2001/XMLSchema#string"> SeaMap Australia National Benthic Habitat Classification Scheme (2017)</dc:source>
	<skos:narrower rdf:resource="http://seamapaustralia.org.au/def/benthichabitatclassification/class/127"/>
	<skos:narrower rdf:resource="http://seamapaustralia.org.au/def/benthichabitatclassification/class/128"/>
	<skos:closeMatch rdf:resource="https://www.cmecscatalog.org/cmecs/classification/aquaticSetting/1.html"/>
</rdf:Description>

<rdf:Description rdf:about="http://seamapaustralia.org.au/def/benthichabitatclassification/class/123">
	<rdf:type rdf:resource="http://www.w3.org/2000/01/rdf-schema#Resource"/>
	<rdf:type rdf:resource="http://www.w3.org/2004/02/skos/core#Concept"/>
	<skos:broader rdf:resource="http://seamapaustralia.org.au/def/benthichabitatclassification/class/121"/>
	<skos:prefLabel xml:lang="en">Coastal</skos:prefLabel>
	<dcterms:contributor rdf:resource="http://editor.vocabs.ands.org.au/user/eMII_Finney.Kim_Admin"/>
	<dcterms:created rdf:datatype="http://www.w3.org/2001/XMLSchema#dateTime">2017-05-23T04:38:20Z</dcterms:created>
	<dcterms:creator rdf:resource="http://editor.vocabs.ands.org.au/user/eMII_Finney.Kim_Admin"/>
	<dcterms:modified rdf:datatype="http://www.w3.org/2001/XMLSchema#dateTime">2017-06-27T04:02:11Z</dcterms:modified>
	<dc:publisher rdf:datatype="http://www.w3.org/2001/XMLSchema#string">Institute for Marine and Antarctic Studies (IMAS) - UTAS</dc:publisher>
	<skos:definition xml:lang="en">In estuarine waters, the coastal subsystem extends from the upper limit of the intertidal zone down to the 6 m depth contour in waters that have salinity &gt; 0.5 ‰ (during the period of average annual low flow).</skos:definition>
	<dc:source rdf:datatype="http://www.w3.org/2001/XMLSchema#string">SeaMap Australia National Benthic Habitat Classification Scheme (2017)</dc:source>
	<skos:narrower rdf:resource="http://seamapaustralia.org.au/def/benthichabitatclassification/class/137"/>
	<skos:narrower rdf:resource="http://seamapaustralia.org.au/def/benthichabitatclassification/class/138"/>
	<skos:closeMatch rdf:resource="https://www.cmecscatalog.org/cmecs/classification/aquaticSetting/7.html"/>
</rdf:Description>

<rdf:Description rdf:about="http://seamapaustralia.org.au/def/benthichabitatclassification/class/124">
	<rdf:type rdf:resource="http://www.w3.org/2000/01/rdf-schema#Resource"/>
	<rdf:type rdf:resource="http://www.w3.org/2004/02/skos/core#Concept"/>
	<skos:broader rdf:resource="http://seamapaustralia.org.au/def/benthichabitatclassification/class/121"/>
	<skos:prefLabel xml:lang="en">Open Water</skos:prefLabel>
	<dcterms:contributor rdf:resource="http://editor.vocabs.ands.org.au/user/eMII_Finney.Kim_Admin"/>
	<dcterms:created rdf:datatype="http://www.w3.org/2001/XMLSchema#dateTime">2017-05-23T04:38:31Z</dcterms:created>
	<dcterms:creator rdf:resource="http://editor.vocabs.ands.org.au/user/eMII_Finney.Kim_Admin"/>
	<dcterms:modified rdf:datatype="http://www.w3.org/2001/XMLSchema#dateTime">2017-06-27T04:02:45Z</dcterms:modified>
	<dc:publisher rdf:datatype="http://www.w3.org/2001/XMLSchema#string">Institute for Marine and Antarctic Studies (IMAS) - UTAS</dc:publisher>
	<skos:definition xml:lang="en">Estuarine waters with a total depth &gt; 6 m below chart datum and in waters that have salinity &gt; 0.5 ‰ (during the period of average annual low flow).</skos:definition>
	<dc:source rdf:datatype="http://www.w3.org/2001/XMLSchema#string"> SeaMap Australia National Benthic Habitat Classification Scheme (2017)</dc:source>
	<skos:narrower rdf:resource="http://seamapaustralia.org.au/def/benthichabitatclassification/class/141"/>
	<skos:closeMatch rdf:resource="https://www.cmecscatalog.org/cmecs/classification/aquaticSetting/8.html"/>
</rdf:Description>

<rdf:Description rdf:about="http://seamapaustralia.org.au/def/benthichabitatclassification/class/125">
	<rdf:type rdf:resource="http://www.w3.org/2000/01/rdf-schema#Resource"/>
	<rdf:type rdf:resource="http://www.w3.org/2004/02/skos/core#Concept"/>
	<skos:broader rdf:resource="http://seamapaustralia.org.au/def/benthichabitatclassification/class/121"/>
	<skos:prefLabel xml:lang="en">Tidal Riverine Coastal</skos:prefLabel>
	<dcterms:contributor rdf:resource="http://editor.vocabs.ands.org.au/user/eMII_Finney.Kim_Admin"/>
	<dcterms:created rdf:datatype="http://www.w3.org/2001/XMLSchema#dateTime">2017-05-23T04:38:49Z</dcterms:created>
	<dcterms:creator rdf:resource="http://editor.vocabs.ands.org.au/user/eMII_Finney.Kim_Admin"/>
	<dcterms:modified rdf:datatype="http://www.w3.org/2001/XMLSchema#dateTime">2017-06-27T04:03:08Z</dcterms:modified>
	<dc:publisher rdf:datatype="http://www.w3.org/2001/XMLSchema#string">Institute for Marine and Antarctic Studies (IMAS) - UTAS</dc:publisher>
	<skos:definition xml:lang="en">This is the most upstream region of an estuary, in areas between Highest Astronomical Tide - HAT and the 6 m depth contour (below Lowest Astronomical Tide - LAT) in water that (a) can regularly be influenced by tides and (b) where salinity is &lt; 0.5 ‰ during the period of annual low flow.</skos:definition>
	<dc:source rdf:datatype="http://www.w3.org/2001/XMLSchema#string">  SeaMap Australia National Benthic Habitat Classification Scheme (2017)</dc:source>
	<skos:narrower rdf:resource="http://seamapaustralia.org.au/def/benthichabitatclassification/class/144"/>
	<skos:narrower rdf:resource="http://seamapaustralia.org.au/def/benthichabitatclassification/class/145"/>
	<skos:closeMatch rdf:resource="https://www.cmecscatalog.org/cmecs/classification/aquaticSetting/9.html"/>
</rdf:Description>

<rdf:Description rdf:about="http://seamapaustralia.org.au/def/benthichabitatclassification/class/126">
	<rdf:type rdf:resource="http://www.w3.org/2000/01/rdf-schema#Resource"/>
	<rdf:type rdf:resource="http://www.w3.org/2004/02/skos/core#Concept"/>
	<skos:broader rdf:resource="http://seamapaustralia.org.au/def/benthichabitatclassification/class/121"/>
	<skos:prefLabel xml:lang="en">Tidal Riverine Open Water</skos:prefLabel>
	<dcterms:contributor rdf:resource="http://editor.vocabs.ands.org.au/user/eMII_Finney.Kim_Admin"/>
	<dcterms:created rdf:datatype="http://www.w3.org/2001/XMLSchema#dateTime">2017-05-23T04:39:08Z</dcterms:created>
	<dcterms:creator rdf:resource="http://editor.vocabs.ands.org.au/user/eMII_Finney.Kim_Admin"/>
	<dcterms:modified rdf:datatype="http://www.w3.org/2001/XMLSchema#dateTime">2017-06-27T04:03:41Z</dcterms:modified>
	<dc:publisher rdf:datatype="http://www.w3.org/2001/XMLSchema#string">  Institute for Marine and Antarctic Studies (IMAS) - UTAS</dc:publisher>
	<skos:definition xml:lang="en">Tidal estuarine areas with a salinity of &lt; 0.5 ‰ and a depth &gt; 6 m below Lowest Astronomical Tide (LAT).</skos:definition>
	<dc:source rdf:datatype="http://www.w3.org/2001/XMLSchema#string">SeaMap Australia National Benthic Habitat Classification Scheme (2017)</dc:source>
	<skos:narrower rdf:resource="http://seamapaustralia.org.au/def/benthichabitatclassification/class/148"/>
	<skos:closeMatch rdf:resource="https://www.cmecscatalog.org/cmecs/classification/aquaticSetting/10.html"/>
</rdf:Description>

<rdf:Description rdf:about="http://seamapaustralia.org.au/def/benthichabitatclassification/class/127">
	<rdf:type rdf:resource="http://www.w3.org/2000/01/rdf-schema#Resource"/>
	<rdf:type rdf:resource="http://www.w3.org/2004/02/skos/core#Concept"/>
	<skos:broader rdf:resource="http://seamapaustralia.org.au/def/benthichabitatclassification/class/122"/>
	<skos:prefLabel xml:lang="en">Nearshore</skos:prefLabel>
	<dcterms:contributor rdf:resource="http://editor.vocabs.ands.org.au/user/eMII_Finney.Kim_Admin"/>
	<dcterms:created rdf:datatype="http://www.w3.org/2001/XMLSchema#dateTime">2017-05-23T04:39:27Z</dcterms:created>
	<dcterms:creator rdf:resource="http://editor.vocabs.ands.org.au/user/eMII_Finney.Kim_Admin"/>
	<dcterms:modified rdf:datatype="http://www.w3.org/2001/XMLSchema#dateTime">2017-06-27T04:04:17Z</dcterms:modified>
	<dc:publisher rdf:datatype="http://www.w3.org/2001/XMLSchema#string">Institute for Marine and Antarctic Studies (IMAS) - UTAS</dc:publisher>
	<skos:definition xml:lang="en">The Nearshore System extends from the upper limit of the intertidal zone (Highest Astronomical Tide - HAT) to the 30 m depth contour (as chart datum). As stated in the CMEC Standard (FGDC 2012), the 30 m depth contour was selected as a useful cut-off between shallower nearshore and deeper offshore waters. It is intended to represent an ecologically significant depth to which water column and benthic processes are strongly coupled. Surface currents and waves impinge the bottom at the storm wave base (Keen and Holland 2010) and vertical circulation generally distributes nutrients and sediments throughout the water column. The photic zone extends through the entire water column except in extreme cases (Kleypas et al. 1999). The presence of nutrients and light support the growth of vegetation on the seafloor including seagrass and macroalgal beds, and 30 meters generally represents the depth to which most living coral is found.  </skos:definition>
	<dc:source rdf:datatype="http://www.w3.org/2001/XMLSchema#string">SeaMap Australia National Benthic Habitat Classification Scheme (2017)</dc:source>
	<skos:narrower rdf:resource="http://seamapaustralia.org.au/def/benthichabitatclassification/class/130"/>
	<skos:narrower rdf:resource="http://seamapaustralia.org.au/def/benthichabitatclassification/class/164"/>
	<skos:closeMatch rdf:resource="https://www.cmecscatalog.org/cmecs/classification/aquaticSetting/4.html"/>
</rdf:Description>

<rdf:Description rdf:about="http://seamapaustralia.org.au/def/benthichabitatclassification/class/128">
	<rdf:type rdf:resource="http://www.w3.org/2000/01/rdf-schema#Resource"/>
	<rdf:type rdf:resource="http://www.w3.org/2004/02/skos/core#Concept"/>
	<skos:broader rdf:resource="http://seamapaustralia.org.au/def/benthichabitatclassification/class/122"/>
	<skos:prefLabel xml:lang="en">Offshore</skos:prefLabel>
	<dcterms:contributor rdf:resource="http://editor.vocabs.ands.org.au/user/eMII_Finney.Kim_Admin"/>
	<dcterms:created rdf:datatype="http://www.w3.org/2001/XMLSchema#dateTime">2017-05-23T04:39:38Z</dcterms:created>
	<dcterms:creator rdf:resource="http://editor.vocabs.ands.org.au/user/eMII_Finney.Kim_Admin"/>
	<dcterms:modified rdf:datatype="http://www.w3.org/2001/XMLSchema#dateTime">2017-06-27T04:04:49Z</dcterms:modified>
	<dc:publisher rdf:datatype="http://www.w3.org/2001/XMLSchema#string">Institute for Marine and Antarctic Studies (IMAS) - UTAS</dc:publisher>
	<skos:definition xml:lang="en">The Offshore system extends from the 30 m depth contour (chart datum) to the continental shelf break (200 m depth). </skos:definition>
	<dc:source rdf:datatype="http://www.w3.org/2001/XMLSchema#string">SeaMap Australia National Benthic Habitat Classification Scheme (2017)</dc:source>
	<skos:narrower rdf:resource="http://seamapaustralia.org.au/def/benthichabitatclassification/class/134"/>
	<skos:closeMatch rdf:resource="https://www.cmecscatalog.org/cmecs/classification/aquaticSetting/5.html"/>
</rdf:Description>

<rdf:Description rdf:about="https://www.cmecscatalog.org/cmecs/classification/aquaticSetting/4.html">
	<rdf:type rdf:resource="http://www.w3.org/2000/01/rdf-schema#Resource"/>
</rdf:Description>

<rdf:Description rdf:about="http://seamapaustralia.org.au/def/benthichabitatclassification/class/130">
	<rdf:type rdf:resource="http://www.w3.org/2000/01/rdf-schema#Resource"/>
	<rdf:type rdf:resource="http://www.w3.org/2004/02/skos/core#Concept"/>
	<skos:broader rdf:resource="http://seamapaustralia.org.au/def/benthichabitatclassification/class/127"/>
	<skos:prefLabel xml:lang="en">Nearshore Subtidal</skos:prefLabel>
	<dcterms:contributor rdf:resource="http://editor.vocabs.ands.org.au/user/eMII_Finney.Kim_Admin"/>
	<dcterms:created rdf:datatype="http://www.w3.org/2001/XMLSchema#dateTime">2017-05-23T04:40:55Z</dcterms:created>
	<dcterms:creator rdf:resource="http://editor.vocabs.ands.org.au/user/eMII_Finney.Kim_Admin"/>
	<dcterms:modified rdf:datatype="http://www.w3.org/2001/XMLSchema#dateTime">2017-06-27T04:04:30Z</dcterms:modified>
	<dc:publisher rdf:datatype="http://www.w3.org/2001/XMLSchema#string">Institute for Marine and Antarctic Studies (IMAS) - UTAS</dc:publisher>
	<skos:definition xml:lang="en">This zone cover areas below Lowest Astronomical Tide (LAT), i.e. areas where the substratum is continuously submerged. </skos:definition>
	<dc:source rdf:datatype="http://www.w3.org/2001/XMLSchema#string">SeaMap Australia National Benthic Habitat Classification Scheme (2017)</dc:source>
	<skos:narrower rdf:resource="http://seamapaustralia.org.au/def/benthichabitatclassification/class/131"/>
	<skos:narrower rdf:resource="http://seamapaustralia.org.au/def/benthichabitatclassification/class/132"/>
	<skos:closeMatch rdf:resource="https://www.cmecscatalog.org/cmecs/classification/aquaticSetting/13.html"/>
</rdf:Description>

<rdf:Description rdf:about="https://www.cmecscatalog.org/cmecs/classification/aquaticSetting/5.html">
	<rdf:type rdf:resource="http://www.w3.org/2000/01/rdf-schema#Resource"/>
</rdf:Description>

<rdf:Description rdf:about="http://seamapaustralia.org.au/def/benthichabitatclassification/class/131">
	<rdf:type rdf:resource="http://www.w3.org/2000/01/rdf-schema#Resource"/>
	<rdf:type rdf:resource="http://www.w3.org/2004/02/skos/core#Concept"/>
	<skos:broader rdf:resource="http://seamapaustralia.org.au/def/benthichabitatclassification/class/130"/>
	<skos:prefLabel xml:lang="en">Nearshore Infralittoral</skos:prefLabel>
	<dcterms:contributor rdf:resource="http://editor.vocabs.ands.org.au/user/eMII_Finney.Kim_Admin"/>
	<dcterms:created rdf:datatype="http://www.w3.org/2001/XMLSchema#dateTime">2017-05-23T04:42:22Z</dcterms:created>
	<dcterms:creator rdf:resource="http://editor.vocabs.ands.org.au/user/eMII_Finney.Kim_Admin"/>
	<dcterms:modified rdf:datatype="http://www.w3.org/2001/XMLSchema#dateTime">2017-06-27T04:04:42Z</dcterms:modified>
	<dc:publisher rdf:datatype="http://www.w3.org/2001/XMLSchema#string">Institute for Marine and Antarctic Studies (IMAS) - UTAS</dc:publisher>
	<skos:definition xml:lang="en">Subtidal areas where the benthos are algal dominated, wave-disturbed or within the euphotic zone </skos:definition>
	<dc:source rdf:datatype="http://www.w3.org/2001/XMLSchema#string">SeaMap Australia National Benthic Habitat Classification Scheme (2017)</dc:source>
</rdf:Description>

<rdf:Description rdf:about="http://seamapaustralia.org.au/def/benthichabitatclassification/class/132">
	<rdf:type rdf:resource="http://www.w3.org/2000/01/rdf-schema#Resource"/>
	<rdf:type rdf:resource="http://www.w3.org/2004/02/skos/core#Concept"/>
	<skos:broader rdf:resource="http://seamapaustralia.org.au/def/benthichabitatclassification/class/130"/>
	<skos:prefLabel xml:lang="en">Nearshore Circalittoral</skos:prefLabel>
	<dcterms:contributor rdf:resource="http://editor.vocabs.ands.org.au/user/eMII_Finney.Kim_Admin"/>
	<dcterms:created rdf:datatype="http://www.w3.org/2001/XMLSchema#dateTime">2017-05-23T04:43:14Z</dcterms:created>
	<dcterms:creator rdf:resource="http://editor.vocabs.ands.org.au/user/eMII_Finney.Kim_Admin"/>
	<dcterms:modified rdf:datatype="http://www.w3.org/2001/XMLSchema#dateTime">2017-06-27T04:04:37Z</dcterms:modified>
	<dc:publisher rdf:datatype="http://www.w3.org/2001/XMLSchema#string">Institute for Marine and Antarctic Studies (IMAS) - UTAS</dc:publisher>
	<skos:definition xml:lang="en">Subtidal areas where the benthos are below the euphotic zone and light penetration is thus insufficient to allow algae to dominate. May experience some wave action, and tidal currents may exert a strong influence. These zones are typically characterised by animal communities, although very sparse algae may be present. </skos:definition>
	<dc:source rdf:datatype="http://www.w3.org/2001/XMLSchema#string">SeaMap Australia National Benthic Habitat Classification Scheme (2017)</dc:source>
</rdf:Description>

<rdf:Description rdf:about="http://seamapaustralia.org.au/def/benthichabitatclassification/class/346">
	<rdf:type rdf:resource="http://www.w3.org/2000/01/rdf-schema#Resource"/>
	<rdf:type rdf:resource="http://www.w3.org/2004/02/skos/core#Concept"/>
	<skos:broader rdf:resource="http://seamapaustralia.org.au/def/benthichabitatclassification/class/344"/>
	<skos:prefLabel xml:lang="en">IMCRA East Cape York Bioregion</skos:prefLabel>
	<dcterms:contributor rdf:resource="http://editor.vocabs.ands.org.au/user/eMII_Finney.Kim_Admin"/>
	<dcterms:created rdf:datatype="http://www.w3.org/2001/XMLSchema#dateTime">2017-06-27T03:33:15Z</dcterms:created>
	<dcterms:creator rdf:resource="http://editor.vocabs.ands.org.au/user/eMII_Finney.Kim_Admin"/>
	<dcterms:modified rdf:datatype="http://www.w3.org/2001/XMLSchema#dateTime">2017-06-27T03:59:36Z</dcterms:modified>
	<dc:publisher rdf:datatype="http://www.w3.org/2001/XMLSchema#string">Institute for Marine and Antarctic Studies (IMAS) - UTAS</dc:publisher>
	<skos:definition xml:lang="en">An inshore regionalisation of Australian waters derived from biological and physical data, including the distribution of demersal fishes, marine plants and invertebrates, sea floor geomorphology and sediments, and oceanographic data. The meso-scale regionalisation was compiled from information supplied to the Australian Government Department of the Environment and Heritage by the relevant State, Northern Territory and Commonwealth marine research and management agencies. The seaward extent for the meso-scale IMCRA coverage is defined by the 200m isobath except where this boundary extends beyond the Australian Exclusive Economic Zone (AEEZ).</skos:definition>
	<dc:source rdf:datatype="http://www.w3.org/2001/XMLSchema#string">Commonwealth of Australia (2006). A Guide to the Integrated Marine and Coastal Regionalisation of Australia Version 4.0. Department of the Environment and Heritage, Canberra, Australia.</dc:source>
	<skos:exactMatch rdf:resource="http://www.environment.gov.au/mapping/rest/services/ogc_services/IMCRA_Mesoscale/MapServer/0/5"/>
</rdf:Description>

<rdf:Description rdf:about="http://seamapaustralia.org.au/def/benthichabitatclassification/class/134">
	<rdf:type rdf:resource="http://www.w3.org/2000/01/rdf-schema#Resource"/>
	<rdf:type rdf:resource="http://www.w3.org/2004/02/skos/core#Concept"/>
	<skos:broader rdf:resource="http://seamapaustralia.org.au/def/benthichabitatclassification/class/128"/>
	<skos:prefLabel xml:lang="en">Offshore Subtidal</skos:prefLabel>
	<dcterms:contributor rdf:resource="http://editor.vocabs.ands.org.au/user/eMII_Finney.Kim_Admin"/>
	<dcterms:created rdf:datatype="http://www.w3.org/2001/XMLSchema#dateTime">2017-05-23T04:45:16Z</dcterms:created>
	<dcterms:creator rdf:resource="http://editor.vocabs.ands.org.au/user/eMII_Finney.Kim_Admin"/>
	<dcterms:modified rdf:datatype="http://www.w3.org/2001/XMLSchema#dateTime">2017-06-27T04:04:56Z</dcterms:modified>
	<dc:publisher rdf:datatype="http://www.w3.org/2001/XMLSchema#string">Institute for Marine and Antarctic Studies (IMAS) - UTAS</dc:publisher>
	<skos:definition xml:lang="en">This zone cover areas below Lowest Astronomical Tide (LAT), i.e. areas where the substratum is continuously submerged. </skos:definition>
	<dc:source rdf:datatype="http://www.w3.org/2001/XMLSchema#string">SeaMap Australia National Benthic Habitat Classification Scheme (2017)</dc:source>
	<skos:narrower rdf:resource="http://seamapaustralia.org.au/def/benthichabitatclassification/class/135"/>
	<skos:narrower rdf:resource="http://seamapaustralia.org.au/def/benthichabitatclassification/class/136"/>
	<skos:closeMatch rdf:resource="https://www.cmecscatalog.org/cmecs/classification/aquaticSetting/5.html"/>
</rdf:Description>

<rdf:Description rdf:about="http://seamapaustralia.org.au/def/benthichabitatclassification/class/135">
	<rdf:type rdf:resource="http://www.w3.org/2000/01/rdf-schema#Resource"/>
	<rdf:type rdf:resource="http://www.w3.org/2004/02/skos/core#Concept"/>
	<skos:broader rdf:resource="http://seamapaustralia.org.au/def/benthichabitatclassification/class/134"/>
	<skos:prefLabel xml:lang="en">Offshore Infralittoral</skos:prefLabel>
	<dcterms:contributor rdf:resource="http://editor.vocabs.ands.org.au/user/eMII_Finney.Kim_Admin"/>
	<dcterms:created rdf:datatype="http://www.w3.org/2001/XMLSchema#dateTime">2017-05-23T04:45:55Z</dcterms:created>
	<dcterms:creator rdf:resource="http://editor.vocabs.ands.org.au/user/eMII_Finney.Kim_Admin"/>
	<dcterms:modified rdf:datatype="http://www.w3.org/2001/XMLSchema#dateTime">2017-06-27T04:05:08Z</dcterms:modified>
	<dc:publisher rdf:datatype="http://www.w3.org/2001/XMLSchema#string">Institute for Marine and Antarctic Studies (IMAS) - UTAS</dc:publisher>
	<skos:definition xml:lang="en">Subtidal areas where the benthos are algal dominated, wave-disturbed or within the euphotic zone </skos:definition>
	<dc:source rdf:datatype="http://www.w3.org/2001/XMLSchema#string">SeaMap Australia National Benthic Habitat Classification Scheme (2017)</dc:source>
</rdf:Description>

<rdf:Description rdf:about="http://seamapaustralia.org.au/def/benthichabitatclassification/class/136">
	<rdf:type rdf:resource="http://www.w3.org/2000/01/rdf-schema#Resource"/>
	<rdf:type rdf:resource="http://www.w3.org/2004/02/skos/core#Concept"/>
	<skos:broader rdf:resource="http://seamapaustralia.org.au/def/benthichabitatclassification/class/134"/>
	<skos:prefLabel xml:lang="en">Offshore Circalittoral</skos:prefLabel>
	<dcterms:contributor rdf:resource="http://editor.vocabs.ands.org.au/user/eMII_Finney.Kim_Admin"/>
	<dcterms:created rdf:datatype="http://www.w3.org/2001/XMLSchema#dateTime">2017-05-23T04:46:25Z</dcterms:created>
	<dcterms:creator rdf:resource="http://editor.vocabs.ands.org.au/user/eMII_Finney.Kim_Admin"/>
	<dcterms:modified rdf:datatype="http://www.w3.org/2001/XMLSchema#dateTime">2017-06-27T04:05:02Z</dcterms:modified>
	<dc:publisher rdf:datatype="http://www.w3.org/2001/XMLSchema#string">Institute for Marine and Antarctic Studies (IMAS) - UTAS</dc:publisher>
	<skos:definition xml:lang="en">Subtidal areas where the benthos are below the euphotic zone and light penetration is thus insufficient to allow algae to dominate. May experience some wave action, and tidal currents may exert a strong influence. These zones are typically characterised by animal communities, although very sparse algae may be present. </skos:definition>
	<dc:source rdf:datatype="http://www.w3.org/2001/XMLSchema#string">SeaMap Australia National Benthic Habitat Classification Scheme (2017)</dc:source>
</rdf:Description>

<rdf:Description rdf:about="http://seamapaustralia.org.au/def/benthichabitatclassification/class/137">
	<rdf:type rdf:resource="http://www.w3.org/2000/01/rdf-schema#Resource"/>
	<rdf:type rdf:resource="http://www.w3.org/2004/02/skos/core#Concept"/>
	<skos:broader rdf:resource="http://seamapaustralia.org.au/def/benthichabitatclassification/class/123"/>
	<skos:prefLabel xml:lang="en">Coastal Intertidal</skos:prefLabel>
	<dcterms:contributor rdf:resource="http://editor.vocabs.ands.org.au/user/eMII_Finney.Kim_Admin"/>
	<dcterms:created rdf:datatype="http://www.w3.org/2001/XMLSchema#dateTime">2017-05-23T04:47:17Z</dcterms:created>
	<dcterms:creator rdf:resource="http://editor.vocabs.ands.org.au/user/eMII_Finney.Kim_Admin"/>
	<dcterms:modified rdf:datatype="http://www.w3.org/2001/XMLSchema#dateTime">2017-06-27T04:02:21Z</dcterms:modified>
	<dc:publisher rdf:datatype="http://www.w3.org/2001/XMLSchema#string">  Institute for Marine and Antarctic Studies (IMAS) - UTAS</dc:publisher>
	<skos:definition xml:lang="en">This zone extends from Lowest Astronomical Tide to Highest Astronomical Tide, i.e. areas where the substratum is regularly or periodically exposed and flooded by tides. </skos:definition>
	<dc:source rdf:datatype="http://www.w3.org/2001/XMLSchema#string"> SeaMap Australia National Benthic Habitat Classification Scheme (2017)</dc:source>
	<skos:closeMatch rdf:resource="https://www.cmecscatalog.org/cmecs/classification/aquaticSetting/19.html"/>
</rdf:Description>

<rdf:Description rdf:about="http://seamapaustralia.org.au/def/benthichabitatclassification/class/138">
	<rdf:type rdf:resource="http://www.w3.org/2000/01/rdf-schema#Resource"/>
	<rdf:type rdf:resource="http://www.w3.org/2004/02/skos/core#Concept"/>
	<skos:broader rdf:resource="http://seamapaustralia.org.au/def/benthichabitatclassification/class/123"/>
	<skos:prefLabel xml:lang="en">Coastal Subtidal</skos:prefLabel>
	<dcterms:contributor rdf:resource="http://editor.vocabs.ands.org.au/user/eMII_Finney.Kim_Admin"/>
	<dcterms:created rdf:datatype="http://www.w3.org/2001/XMLSchema#dateTime">2017-05-23T04:47:34Z</dcterms:created>
	<dcterms:creator rdf:resource="http://editor.vocabs.ands.org.au/user/eMII_Finney.Kim_Admin"/>
	<dcterms:modified rdf:datatype="http://www.w3.org/2001/XMLSchema#dateTime">2017-06-27T04:02:28Z</dcterms:modified>
	<dc:publisher rdf:datatype="http://www.w3.org/2001/XMLSchema#string"> Institute for Marine and Antarctic Studies (IMAS) - UTAS</dc:publisher>
	<skos:definition xml:lang="en">This zone covers areas below LAT (Lowest Astronomical Tide), i.e. areas where the substratum is continuously submerged. </skos:definition>
	<dc:source rdf:datatype="http://www.w3.org/2001/XMLSchema#string">SeaMap Australia National Benthic Habitat Classification Scheme (2017)</dc:source>
	<skos:narrower rdf:resource="http://seamapaustralia.org.au/def/benthichabitatclassification/class/139"/>
	<skos:narrower rdf:resource="http://seamapaustralia.org.au/def/benthichabitatclassification/class/140"/>
	<skos:closeMatch rdf:resource="https://www.cmecscatalog.org/cmecs/classification/aquaticSetting/18.html"/>
</rdf:Description>

<rdf:Description rdf:about="http://seamapaustralia.org.au/def/benthichabitatclassification/class/139">
	<rdf:type rdf:resource="http://www.w3.org/2000/01/rdf-schema#Resource"/>
	<rdf:type rdf:resource="http://www.w3.org/2004/02/skos/core#Concept"/>
	<skos:broader rdf:resource="http://seamapaustralia.org.au/def/benthichabitatclassification/class/138"/>
	<skos:prefLabel xml:lang="en">Coastal Infralittoral</skos:prefLabel>
	<dcterms:contributor rdf:resource="http://editor.vocabs.ands.org.au/user/eMII_Finney.Kim_Admin"/>
	<dcterms:created rdf:datatype="http://www.w3.org/2001/XMLSchema#dateTime">2017-05-23T04:48:13Z</dcterms:created>
	<dcterms:creator rdf:resource="http://editor.vocabs.ands.org.au/user/eMII_Finney.Kim_Admin"/>
	<dcterms:modified rdf:datatype="http://www.w3.org/2001/XMLSchema#dateTime">2017-06-27T04:02:39Z</dcterms:modified>
	<dc:publisher rdf:datatype="http://www.w3.org/2001/XMLSchema#string">Institute for Marine and Antarctic Studies (IMAS) - UTAS</dc:publisher>
	<skos:definition xml:lang="en">Subtidal areas where the benthos are algal dominated, wave-disturbed or within the euphotic zone </skos:definition>
	<dc:source rdf:datatype="http://www.w3.org/2001/XMLSchema#string">SeaMap Australia National Benthic Habitat Classification Scheme (2017)</dc:source>
</rdf:Description>

<rdf:Description rdf:about="http://seamapaustralia.org.au/def/benthichabitatclassification/class/140">
	<rdf:type rdf:resource="http://www.w3.org/2000/01/rdf-schema#Resource"/>
	<rdf:type rdf:resource="http://www.w3.org/2004/02/skos/core#Concept"/>
	<skos:broader rdf:resource="http://seamapaustralia.org.au/def/benthichabitatclassification/class/138"/>
	<skos:prefLabel xml:lang="en">Coastal Circalittoral</skos:prefLabel>
	<dcterms:contributor rdf:resource="http://editor.vocabs.ands.org.au/user/eMII_Finney.Kim_Admin"/>
	<dcterms:created rdf:datatype="http://www.w3.org/2001/XMLSchema#dateTime">2017-05-23T04:48:36Z</dcterms:created>
	<dcterms:creator rdf:resource="http://editor.vocabs.ands.org.au/user/eMII_Finney.Kim_Admin"/>
	<dcterms:modified rdf:datatype="http://www.w3.org/2001/XMLSchema#dateTime">2017-06-27T04:02:33Z</dcterms:modified>
	<dc:publisher rdf:datatype="http://www.w3.org/2001/XMLSchema#string">Institute for Marine and Antarctic Studies (IMAS) - UTAS</dc:publisher>
	<skos:definition xml:lang="en">Subtidal areas where the benthos are below the euphotic zone and light penetration is thus insufficient to allow algae to dominate. May experience some wave action, and tidal currents may exert a strong influence. These zones are typically characterised by animal communities, although very sparse algae may be present. </skos:definition>
	<dc:source rdf:datatype="http://www.w3.org/2001/XMLSchema#string">SeaMap Australia National Benthic Habitat Classification Scheme (2017)</dc:source>
</rdf:Description>

<rdf:Description rdf:about="http://seamapaustralia.org.au/def/benthichabitatclassification/class/141">
	<rdf:type rdf:resource="http://www.w3.org/2000/01/rdf-schema#Resource"/>
	<rdf:type rdf:resource="http://www.w3.org/2004/02/skos/core#Concept"/>
	<skos:broader rdf:resource="http://seamapaustralia.org.au/def/benthichabitatclassification/class/124"/>
	<skos:prefLabel xml:lang="en">Open Water Subtidal</skos:prefLabel>
	<dcterms:contributor rdf:resource="http://editor.vocabs.ands.org.au/user/eMII_Finney.Kim_Admin"/>
	<dcterms:created rdf:datatype="http://www.w3.org/2001/XMLSchema#dateTime">2017-05-23T04:49:11Z</dcterms:created>
	<dcterms:creator rdf:resource="http://editor.vocabs.ands.org.au/user/eMII_Finney.Kim_Admin"/>
	<dcterms:modified rdf:datatype="http://www.w3.org/2001/XMLSchema#dateTime">2017-06-27T04:02:52Z</dcterms:modified>
	<dc:publisher rdf:datatype="http://www.w3.org/2001/XMLSchema#string">Institute for Marine and Antarctic Studies (IMAS) - UTAS</dc:publisher>
	<skos:definition xml:lang="en">This zone cover areas below LAT (Lowest Astronomical Tide), i.e. areas where the substratum is continuously submerged. </skos:definition>
	<dc:source rdf:datatype="http://www.w3.org/2001/XMLSchema#string">  SeaMap Australia National Benthic Habitat Classification Scheme (2017)</dc:source>
	<skos:narrower rdf:resource="http://seamapaustralia.org.au/def/benthichabitatclassification/class/142"/>
	<skos:narrower rdf:resource="http://seamapaustralia.org.au/def/benthichabitatclassification/class/143"/>
	<skos:closeMatch rdf:resource="https://www.cmecscatalog.org/cmecs/classification/aquaticSetting/21.html"/>
</rdf:Description>

<rdf:Description rdf:about="http://seamapaustralia.org.au/def/benthichabitatclassification/class/142">
	<rdf:type rdf:resource="http://www.w3.org/2000/01/rdf-schema#Resource"/>
	<rdf:type rdf:resource="http://www.w3.org/2004/02/skos/core#Concept"/>
	<skos:broader rdf:resource="http://seamapaustralia.org.au/def/benthichabitatclassification/class/141"/>
	<skos:prefLabel xml:lang="en">Open Water Infralittoral</skos:prefLabel>
	<dcterms:contributor rdf:resource="http://editor.vocabs.ands.org.au/user/eMII_Finney.Kim_Admin"/>
	<dcterms:created rdf:datatype="http://www.w3.org/2001/XMLSchema#dateTime">2017-05-23T04:49:43Z</dcterms:created>
	<dcterms:creator rdf:resource="http://editor.vocabs.ands.org.au/user/eMII_Finney.Kim_Admin"/>
	<dcterms:modified rdf:datatype="http://www.w3.org/2001/XMLSchema#dateTime">2017-06-27T04:03:02Z</dcterms:modified>
	<dc:publisher rdf:datatype="http://www.w3.org/2001/XMLSchema#string">  Institute for Marine and Antarctic Studies (IMAS) - UTAS</dc:publisher>
	<skos:definition xml:lang="en">Subtidal areas where the benthos are algal dominated, wave-disturbed or within the euphotic zone </skos:definition>
	<dc:source rdf:datatype="http://www.w3.org/2001/XMLSchema#string">SeaMap Australia National Benthic Habitat Classification Scheme (2017)</dc:source>
</rdf:Description>

<rdf:Description rdf:about="http://seamapaustralia.org.au/def/benthichabitatclassification/class/143">
	<rdf:type rdf:resource="http://www.w3.org/2000/01/rdf-schema#Resource"/>
	<rdf:type rdf:resource="http://www.w3.org/2004/02/skos/core#Concept"/>
	<skos:broader rdf:resource="http://seamapaustralia.org.au/def/benthichabitatclassification/class/141"/>
	<skos:prefLabel xml:lang="en">Open Water Circalittoral</skos:prefLabel>
	<dcterms:contributor rdf:resource="http://editor.vocabs.ands.org.au/user/eMII_Finney.Kim_Admin"/>
	<dcterms:created rdf:datatype="http://www.w3.org/2001/XMLSchema#dateTime">2017-05-23T04:50:08Z</dcterms:created>
	<dcterms:creator rdf:resource="http://editor.vocabs.ands.org.au/user/eMII_Finney.Kim_Admin"/>
	<dcterms:modified rdf:datatype="http://www.w3.org/2001/XMLSchema#dateTime">2017-06-27T04:02:57Z</dcterms:modified>
	<dc:publisher rdf:datatype="http://www.w3.org/2001/XMLSchema#string">Institute for Marine and Antarctic Studies (IMAS) - UTAS</dc:publisher>
	<skos:definition xml:lang="en">Subtidal areas where the benthos are below the euphotic zone and light penetration is thus insufficient to allow algae to dominate. May experience some wave action, and tidal currents may exert a strong influence. These zones are typically characterised by animal communities, although very sparse algae may be present. </skos:definition>
	<dc:source rdf:datatype="http://www.w3.org/2001/XMLSchema#string">SeaMap Australia National Benthic Habitat Classification Scheme (2017)</dc:source>
</rdf:Description>

<rdf:Description rdf:about="http://seamapaustralia.org.au/def/benthichabitatclassification/class/144">
	<rdf:type rdf:resource="http://www.w3.org/2000/01/rdf-schema#Resource"/>
	<rdf:type rdf:resource="http://www.w3.org/2004/02/skos/core#Concept"/>
	<skos:broader rdf:resource="http://seamapaustralia.org.au/def/benthichabitatclassification/class/125"/>
	<skos:prefLabel xml:lang="en">Tidal Riverine Coastal Intertidal</skos:prefLabel>
	<dcterms:contributor rdf:resource="http://editor.vocabs.ands.org.au/user/eMII_Finney.Kim_Admin"/>
	<dcterms:created rdf:datatype="http://www.w3.org/2001/XMLSchema#dateTime">2017-05-23T04:50:44Z</dcterms:created>
	<dcterms:creator rdf:resource="http://editor.vocabs.ands.org.au/user/eMII_Finney.Kim_Admin"/>
	<dcterms:modified rdf:datatype="http://www.w3.org/2001/XMLSchema#dateTime">2017-06-27T04:03:14Z</dcterms:modified>
	<dc:publisher rdf:datatype="http://www.w3.org/2001/XMLSchema#string">Institute for Marine and Antarctic Studies (IMAS) - UTAS</dc:publisher>
	<skos:definition xml:lang="en">This zone extends from LAT (Lowest Astronomical Tide) to Highest Astronomical Tide ( HAT), i.e. areas where the substratum is regularly or periodically exposed and flooded by tides. </skos:definition>
	<dc:source rdf:datatype="http://www.w3.org/2001/XMLSchema#string">SeaMap Australia National Benthic Habitat Classification Scheme (2017)</dc:source>
	<skos:closeMatch rdf:resource="https://www.cmecscatalog.org/cmecs/classification/aquaticSetting/24.html"/>
</rdf:Description>

<rdf:Description rdf:about="http://seamapaustralia.org.au/def/benthichabitatclassification/class/145">
	<rdf:type rdf:resource="http://www.w3.org/2000/01/rdf-schema#Resource"/>
	<rdf:type rdf:resource="http://www.w3.org/2004/02/skos/core#Concept"/>
	<skos:broader rdf:resource="http://seamapaustralia.org.au/def/benthichabitatclassification/class/125"/>
	<skos:prefLabel xml:lang="en">Tidal Riverine Coastal Subtidal</skos:prefLabel>
	<dcterms:contributor rdf:resource="http://editor.vocabs.ands.org.au/user/eMII_Finney.Kim_Admin"/>
	<dcterms:created rdf:datatype="http://www.w3.org/2001/XMLSchema#dateTime">2017-05-23T04:51:01Z</dcterms:created>
	<dcterms:creator rdf:resource="http://editor.vocabs.ands.org.au/user/eMII_Finney.Kim_Admin"/>
	<dcterms:modified rdf:datatype="http://www.w3.org/2001/XMLSchema#dateTime">2017-06-27T04:03:20Z</dcterms:modified>
	<dc:publisher rdf:datatype="http://www.w3.org/2001/XMLSchema#string">Institute for Marine and Antarctic Studies (IMAS) - UTAS</dc:publisher>
	<skos:definition xml:lang="en">This zone cover areas below Lowest Astronomical Tide -LAT, i.e. areas where the substratum is continuously submerged. </skos:definition>
	<dc:source rdf:datatype="http://www.w3.org/2001/XMLSchema#string"> SeaMap Australia National Benthic Habitat Classification Scheme (2017)</dc:source>
	<skos:narrower rdf:resource="http://seamapaustralia.org.au/def/benthichabitatclassification/class/146"/>
	<skos:narrower rdf:resource="http://seamapaustralia.org.au/def/benthichabitatclassification/class/147"/>
	<skos:closeMatch rdf:resource="https://www.cmecscatalog.org/cmecs/classification/aquaticSetting/23.html"/>
</rdf:Description>

<rdf:Description rdf:about="http://seamapaustralia.org.au/def/benthichabitatclassification/class/146">
	<rdf:type rdf:resource="http://www.w3.org/2000/01/rdf-schema#Resource"/>
	<rdf:type rdf:resource="http://www.w3.org/2004/02/skos/core#Concept"/>
	<skos:broader rdf:resource="http://seamapaustralia.org.au/def/benthichabitatclassification/class/145"/>
	<skos:prefLabel xml:lang="en">Tidal Riverine Coastal Infralittoral</skos:prefLabel>
	<dcterms:contributor rdf:resource="http://editor.vocabs.ands.org.au/user/eMII_Finney.Kim_Admin"/>
	<dcterms:created rdf:datatype="http://www.w3.org/2001/XMLSchema#dateTime">2017-05-23T04:51:33Z</dcterms:created>
	<dcterms:creator rdf:resource="http://editor.vocabs.ands.org.au/user/eMII_Finney.Kim_Admin"/>
	<dcterms:modified rdf:datatype="http://www.w3.org/2001/XMLSchema#dateTime">2017-06-27T04:03:33Z</dcterms:modified>
	<dc:publisher rdf:datatype="http://www.w3.org/2001/XMLSchema#string">Institute for Marine and Antarctic Studies (IMAS) - UTAS</dc:publisher>
	<skos:definition xml:lang="en">Subtidal areas where the benthos are algal dominated, wave-disturbed or within the euphoric zone. </skos:definition>
	<dc:source rdf:datatype="http://www.w3.org/2001/XMLSchema#string">SeaMap Australia National Benthic Habitat Classification Scheme (2017)</dc:source>
</rdf:Description>

<rdf:Description rdf:about="http://seamapaustralia.org.au/def/benthichabitatclassification/class/147">
	<rdf:type rdf:resource="http://www.w3.org/2000/01/rdf-schema#Resource"/>
	<rdf:type rdf:resource="http://www.w3.org/2004/02/skos/core#Concept"/>
	<skos:broader rdf:resource="http://seamapaustralia.org.au/def/benthichabitatclassification/class/145"/>
	<skos:prefLabel xml:lang="en">Tidal Riverine Coastal Circalittoral</skos:prefLabel>
	<dcterms:contributor rdf:resource="http://editor.vocabs.ands.org.au/user/eMII_Finney.Kim_Admin"/>
	<dcterms:created rdf:datatype="http://www.w3.org/2001/XMLSchema#dateTime">2017-05-23T04:51:56Z</dcterms:created>
	<dcterms:creator rdf:resource="http://editor.vocabs.ands.org.au/user/eMII_Finney.Kim_Admin"/>
	<dcterms:modified rdf:datatype="http://www.w3.org/2001/XMLSchema#dateTime">2017-06-27T04:03:27Z</dcterms:modified>
	<dc:publisher rdf:datatype="http://www.w3.org/2001/XMLSchema#string">Institute for Marine and Antarctic Studies (IMAS) - UTAS</dc:publisher>
	<skos:definition xml:lang="en">Subtidal areas where the benthos are below the euphotic zone and light penetration is thus insufficient to allow algae to dominate. May experience some wave action, and tidal currents may exert a strong influence. These zones are typically characterised by animal communities, although very sparse algae may be present.</skos:definition>
	<dc:source rdf:datatype="http://www.w3.org/2001/XMLSchema#string">SeaMap Australia National Benthic Habitat Classification Scheme (2017)</dc:source>
</rdf:Description>

<rdf:Description rdf:about="http://seamapaustralia.org.au/def/benthichabitatclassification/class/148">
	<rdf:type rdf:resource="http://www.w3.org/2000/01/rdf-schema#Resource"/>
	<rdf:type rdf:resource="http://www.w3.org/2004/02/skos/core#Concept"/>
	<skos:broader rdf:resource="http://seamapaustralia.org.au/def/benthichabitatclassification/class/126"/>
	<skos:prefLabel xml:lang="en">Tidal Riverine Open Water Subtidal</skos:prefLabel>
	<dcterms:contributor rdf:resource="http://editor.vocabs.ands.org.au/user/eMII_Finney.Kim_Admin"/>
	<dcterms:created rdf:datatype="http://www.w3.org/2001/XMLSchema#dateTime">2017-05-23T04:52:23Z</dcterms:created>
	<dcterms:creator rdf:resource="http://editor.vocabs.ands.org.au/user/eMII_Finney.Kim_Admin"/>
	<dcterms:modified rdf:datatype="http://www.w3.org/2001/XMLSchema#dateTime">2017-06-27T04:03:52Z</dcterms:modified>
	<dc:publisher rdf:datatype="http://www.w3.org/2001/XMLSchema#string">Institute for Marine and Antarctic Studies (IMAS) - UTAS</dc:publisher>
	<skos:definition xml:lang="en">This zone cover areas below Lowest Astronomical Tide (LAT), i.e. areas where the substratum is continuously submerged. </skos:definition>
	<dc:source rdf:datatype="http://www.w3.org/2001/XMLSchema#string">SeaMap Australia National Benthic Habitat Classification Scheme (2017)</dc:source>
	<skos:narrower rdf:resource="http://seamapaustralia.org.au/def/benthichabitatclassification/class/149"/>
	<skos:narrower rdf:resource="http://seamapaustralia.org.au/def/benthichabitatclassification/class/150"/>
	<skos:closeMatch rdf:resource="https://www.cmecscatalog.org/cmecs/classification/aquaticSetting/26.html"/>
</rdf:Description>

<rdf:Description rdf:about="http://seamapaustralia.org.au/def/benthichabitatclassification/class/149">
	<rdf:type rdf:resource="http://www.w3.org/2000/01/rdf-schema#Resource"/>
	<rdf:type rdf:resource="http://www.w3.org/2004/02/skos/core#Concept"/>
	<skos:broader rdf:resource="http://seamapaustralia.org.au/def/benthichabitatclassification/class/148"/>
	<skos:prefLabel xml:lang="en">Tidal Riverine Open Water Infralittoral</skos:prefLabel>
	<dcterms:contributor rdf:resource="http://editor.vocabs.ands.org.au/user/eMII_Finney.Kim_Admin"/>
	<dcterms:created rdf:datatype="http://www.w3.org/2001/XMLSchema#dateTime">2017-05-23T04:53:11Z</dcterms:created>
	<dcterms:creator rdf:resource="http://editor.vocabs.ands.org.au/user/eMII_Finney.Kim_Admin"/>
	<dcterms:modified rdf:datatype="http://www.w3.org/2001/XMLSchema#dateTime">2017-06-27T04:04:04Z</dcterms:modified>
	<dc:publisher rdf:datatype="http://www.w3.org/2001/XMLSchema#string">Institute for Marine and Antarctic Studies (IMAS) - UTAS</dc:publisher>
	<skos:definition xml:lang="en">Subtidal areas where the benthos are algal dominated, wave-disturbed or within the euphotic zone </skos:definition>
	<dc:source rdf:datatype="http://www.w3.org/2001/XMLSchema#string">SeaMap Australia National Benthic Habitat Classification Scheme (2017)</dc:source>
</rdf:Description>

<rdf:Description rdf:about="http://seamapaustralia.org.au/def/benthichabitatclassification/class/150">
	<rdf:type rdf:resource="http://www.w3.org/2000/01/rdf-schema#Resource"/>
	<rdf:type rdf:resource="http://www.w3.org/2004/02/skos/core#Concept"/>
	<skos:broader rdf:resource="http://seamapaustralia.org.au/def/benthichabitatclassification/class/148"/>
	<skos:prefLabel xml:lang="en">Tidal Riverine Open Water Circalittoral</skos:prefLabel>
	<dcterms:contributor rdf:resource="http://editor.vocabs.ands.org.au/user/eMII_Finney.Kim_Admin"/>
	<dcterms:created rdf:datatype="http://www.w3.org/2001/XMLSchema#dateTime">2017-05-23T04:53:42Z</dcterms:created>
	<dcterms:creator rdf:resource="http://editor.vocabs.ands.org.au/user/eMII_Finney.Kim_Admin"/>
	<dcterms:modified rdf:datatype="http://www.w3.org/2001/XMLSchema#dateTime">2017-06-27T04:03:58Z</dcterms:modified>
	<dc:publisher rdf:datatype="http://www.w3.org/2001/XMLSchema#string">Institute for Marine and Antarctic Studies (IMAS) - UTAS</dc:publisher>
	<skos:definition xml:lang="en">Subtidal areas where the benthos are below the euphotic zone and light penetration is thus insufficient to allow algae to dominate. May experience some wave action, and tidal currents may exert a strong influence. These zones are typically characterised by animal communities, although very sparse algae may be present. </skos:definition>
	<dc:source rdf:datatype="http://www.w3.org/2001/XMLSchema#string">SeaMap Australia National Benthic Habitat Classification Scheme (2017)</dc:source>
</rdf:Description>

<rdf:Description rdf:about="http://seamapaustralia.org.au/def/benthichabitatclassification/class/161">
	<rdf:type rdf:resource="http://www.w3.org/2000/01/rdf-schema#Resource"/>
	<rdf:type rdf:resource="http://www.w3.org/2004/02/skos/core#Concept"/>
	<skos:broader rdf:resource="http://seamapaustralia.org.au/def/benthichabitatclassification/class/74"/>
	<skos:prefLabel xml:lang="en">Stromatolite</skos:prefLabel>
	<dcterms:contributor rdf:resource="http://editor.vocabs.ands.org.au/user/eMII_Finney.Kim_Admin"/>
	<dcterms:created rdf:datatype="http://www.w3.org/2001/XMLSchema#dateTime">2017-05-23T05:53:40Z</dcterms:created>
	<dcterms:creator rdf:resource="http://editor.vocabs.ands.org.au/user/eMII_Finney.Kim_Admin"/>
	<dcterms:modified rdf:datatype="http://www.w3.org/2001/XMLSchema#dateTime">2017-06-27T04:16:42Z</dcterms:modified>
	<dc:publisher rdf:datatype="http://www.w3.org/2001/XMLSchema#string">Institute for Marine and Antarctic Studies (IMAS) - UTAS</dc:publisher>
	<skos:definition xml:lang="en">An area dominated by stromatolites, a microbial community forming a hard layered and mound-like structure, sometimes of considerable size. They occur only in specific areas in warm shallow water, and comprise of secretions of cyanobacteria.</skos:definition>
	<dc:source rdf:datatype="http://www.w3.org/2001/XMLSchema#string">  SeaMap Australia National Benthic Habitat Classification Scheme (2017)</dc:source>
	<skos:closeMatch rdf:resource="https://www.cmecscatalog.org/cmecs/classification/unit/547.html"/>
</rdf:Description>

<rdf:Description rdf:about="http://seamapaustralia.org.au/def/benthichabitatclassification/class/162">
	<rdf:type rdf:resource="http://www.w3.org/2000/01/rdf-schema#Resource"/>
	<rdf:type rdf:resource="http://www.w3.org/2004/02/skos/core#Concept"/>
	<skos:broader rdf:resource="http://seamapaustralia.org.au/def/benthichabitatclassification/class/74"/>
	<skos:prefLabel xml:lang="en">Bacterial Mat</skos:prefLabel>
	<dcterms:contributor rdf:resource="http://editor.vocabs.ands.org.au/user/eMII_Finney.Kim_Admin"/>
	<dcterms:created rdf:datatype="http://www.w3.org/2001/XMLSchema#dateTime">2017-05-23T05:54:17Z</dcterms:created>
	<dcterms:creator rdf:resource="http://editor.vocabs.ands.org.au/user/eMII_Finney.Kim_Admin"/>
	<dcterms:modified rdf:datatype="http://www.w3.org/2001/XMLSchema#dateTime">2017-06-27T04:16:28Z</dcterms:modified>
	<dc:publisher rdf:datatype="http://www.w3.org/2001/XMLSchema#string">Institute for Marine and Antarctic Studies (IMAS) - UTAS</dc:publisher>
	<skos:definition xml:lang="en">Areas dominated by colonies of bacterial decomposers and other decay organisms. These colonies can range in appearance from delicate and filamentous to a dense mass that may blanket the sediment surface.</skos:definition>
	<dc:source rdf:datatype="http://www.w3.org/2001/XMLSchema#string">  SeaMap Australia National Benthic Habitat Classification Scheme (2017)</dc:source>
	<skos:closeMatch rdf:resource="https://www.cmecscatalog.org/cmecs/classification/unit/549.html"/>
</rdf:Description>

<rdf:Description rdf:about="http://seamapaustralia.org.au/def/benthichabitatclassification/class/163">
	<rdf:type rdf:resource="http://www.w3.org/2000/01/rdf-schema#Resource"/>
	<rdf:type rdf:resource="http://www.w3.org/2004/02/skos/core#Concept"/>
	<skos:broader rdf:resource="http://seamapaustralia.org.au/def/benthichabitatclassification/class/74"/>
	<skos:prefLabel xml:lang="en">Microphytobenthos</skos:prefLabel>
	<dcterms:contributor rdf:resource="http://editor.vocabs.ands.org.au/user/eMII_Finney.Kim_Admin"/>
	<dcterms:created rdf:datatype="http://www.w3.org/2001/XMLSchema#dateTime">2017-05-23T05:54:40Z</dcterms:created>
	<dcterms:creator rdf:resource="http://editor.vocabs.ands.org.au/user/eMII_Finney.Kim_Admin"/>
	<dcterms:modified rdf:datatype="http://www.w3.org/2001/XMLSchema#dateTime">2017-06-27T04:16:34Z</dcterms:modified>
	<dc:publisher rdf:datatype="http://www.w3.org/2001/XMLSchema#string">Institute for Marine and Antarctic Studies (IMAS) - UTAS</dc:publisher>
	<skos:definition xml:lang="en">Unicellular eukaryotic algae and cyanobacteria that grow within the upper several mm of illuminated sediments, typically appearing as only a subtle brownish or greenish shading.</skos:definition>
	<dc:source rdf:datatype="http://www.w3.org/2001/XMLSchema#string">  SeaMap Australia National Benthic Habitat Classification Scheme (2017)</dc:source>
	<skos:closeMatch rdf:resource="https://www.cmecscatalog.org/cmecs/classification/unit/548.html"/>
</rdf:Description>

<rdf:Description rdf:about="https://www.cmecscatalog.org/cmecs/classification/aquaticSettings.html">
	<rdf:type rdf:resource="http://www.w3.org/2000/01/rdf-schema#Resource"/>
</rdf:Description>

<rdf:Description rdf:about="http://spatial.ala.org.au/?layers=imcra4_pb">
	<rdf:type rdf:resource="http://www.w3.org/2000/01/rdf-schema#Resource"/>
</rdf:Description>

<rdf:Description rdf:about="http://www.w3.org/2004/02/skos/core#scopeNote">
	<rdf:type rdf:resource="http://www.w3.org/1999/02/22-rdf-syntax-ns#Property"/>
	<rdf:type rdf:resource="http://www.w3.org/2000/01/rdf-schema#Resource"/>
	<rdfs:subPropertyOf rdf:resource="http://www.w3.org/2004/02/skos/core#scopeNote"/>
</rdf:Description>

<rdf:Description rdf:about="https://www.cmecscatalog.org/cmecs/classification/aquaticSetting/2.html">
	<rdf:type rdf:resource="http://www.w3.org/2000/01/rdf-schema#Resource"/>
</rdf:Description>

<rdf:Description rdf:about="https://www.cmecscatalog.org/cmecs/classification/aquaticSetting/7.html">
	<rdf:type rdf:resource="http://www.w3.org/2000/01/rdf-schema#Resource"/>
</rdf:Description>

<rdf:Description rdf:about="https://www.cmecscatalog.org/cmecs/classification/aquaticSetting/8.html">
	<rdf:type rdf:resource="http://www.w3.org/2000/01/rdf-schema#Resource"/>
</rdf:Description>

<rdf:Description rdf:about="https://www.cmecscatalog.org/cmecs/classification/aquaticSetting/9.html">
	<rdf:type rdf:resource="http://www.w3.org/2000/01/rdf-schema#Resource"/>
</rdf:Description>

<rdf:Description rdf:about="https://www.cmecscatalog.org/cmecs/classification/aquaticSetting/10.html">
	<rdf:type rdf:resource="http://www.w3.org/2000/01/rdf-schema#Resource"/>
</rdf:Description>

<rdf:Description rdf:about="https://www.cmecscatalog.org/cmecs/classification/aquaticSetting/1.html">
	<rdf:type rdf:resource="http://www.w3.org/2000/01/rdf-schema#Resource"/>
</rdf:Description>

<rdf:Description rdf:about="https://www.cmecscatalog.org/cmecs/classification/aquaticSetting/19.html">
	<rdf:type rdf:resource="http://www.w3.org/2000/01/rdf-schema#Resource"/>
</rdf:Description>

<rdf:Description rdf:about="https://www.cmecscatalog.org/cmecs/classification/aquaticSetting/18.html">
	<rdf:type rdf:resource="http://www.w3.org/2000/01/rdf-schema#Resource"/>
</rdf:Description>

<rdf:Description rdf:about="https://www.cmecscatalog.org/cmecs/classification/aquaticSetting/21.html">
	<rdf:type rdf:resource="http://www.w3.org/2000/01/rdf-schema#Resource"/>
</rdf:Description>

<rdf:Description rdf:about="https://www.cmecscatalog.org/cmecs/classification/aquaticSetting/24.html">
	<rdf:type rdf:resource="http://www.w3.org/2000/01/rdf-schema#Resource"/>
</rdf:Description>

<rdf:Description rdf:about="https://www.cmecscatalog.org/cmecs/classification/aquaticSetting/23.html">
	<rdf:type rdf:resource="http://www.w3.org/2000/01/rdf-schema#Resource"/>
</rdf:Description>

<rdf:Description rdf:about="https://www.cmecscatalog.org/cmecs/classification/aquaticSetting/26.html">
	<rdf:type rdf:resource="http://www.w3.org/2000/01/rdf-schema#Resource"/>
</rdf:Description>

<rdf:Description rdf:about="http://seamapaustralia.org.au/def/benthichabitatclassification/class/164">
	<rdf:type rdf:resource="http://www.w3.org/2000/01/rdf-schema#Resource"/>
	<rdf:type rdf:resource="http://www.w3.org/2004/02/skos/core#Concept"/>
	<skos:broader rdf:resource="http://seamapaustralia.org.au/def/benthichabitatclassification/class/127"/>
	<skos:prefLabel xml:lang="en">Nearshore Intertidal</skos:prefLabel>
	<dcterms:contributor rdf:resource="http://editor.vocabs.ands.org.au/user/eMII_Finney.Kim_Admin"/>
	<dcterms:created rdf:datatype="http://www.w3.org/2001/XMLSchema#dateTime">2017-05-31T00:11:45Z</dcterms:created>
	<dcterms:creator rdf:resource="http://editor.vocabs.ands.org.au/user/eMII_Finney.Kim_Admin"/>
	<dcterms:modified rdf:datatype="http://www.w3.org/2001/XMLSchema#dateTime">2017-06-27T04:04:23Z</dcterms:modified>
	<dc:publisher rdf:datatype="http://www.w3.org/2001/XMLSchema#string">Institute for Marine and Antarctic Studies (IMAS) - UTAS</dc:publisher>
	<skos:definition xml:lang="en">This zone extends from Lowest Astronomical Tide - (LAT) to Highest Astronomical Tide (HAT); areas where the substratum is regularly or periodically exposed and flooded by tides. </skos:definition>
	<dc:source rdf:datatype="http://www.w3.org/2001/XMLSchema#string">SeaMap Australia National Benthic Habitat Classification Scheme (2017)</dc:source>
	<skos:closeMatch rdf:resource="https://www.cmecscatalog.org/cmecs/classification/aquaticSetting/14.html"/>
</rdf:Description>

<rdf:Description rdf:about="https://www.cmecscatalog.org/cmecs/classification/aquaticSetting/14.html">
	<rdf:type rdf:resource="http://www.w3.org/2000/01/rdf-schema#Resource"/>
</rdf:Description>

<rdf:Description rdf:about="https://www.cmecscatalog.org/cmecs/classification/aquaticSetting/13.html">
	<rdf:type rdf:resource="http://www.w3.org/2000/01/rdf-schema#Resource"/>
</rdf:Description>

<rdf:Description rdf:about="http://seamapaustralia.org.au/def/benthichabitatclassification/class/178">
	<rdf:type rdf:resource="http://www.w3.org/2000/01/rdf-schema#Resource"/>
	<rdf:type rdf:resource="http://www.w3.org/2004/02/skos/core#Concept"/>
	<skos:broader rdf:resource="http://seamapaustralia.org.au/def/benthichabitatclassification/class/177"/>
	<skos:prefLabel xml:lang="en">MEOW Lord Howe and Norfolk Islands Ecoregion</skos:prefLabel>
	<dcterms:contributor rdf:resource="http://editor.vocabs.ands.org.au/user/eMII_Finney.Kim_Admin"/>
	<dcterms:created rdf:datatype="http://www.w3.org/2001/XMLSchema#dateTime">2017-05-31T01:57:05Z</dcterms:created>
	<dcterms:creator rdf:resource="http://editor.vocabs.ands.org.au/user/eMII_Finney.Kim_Admin"/>
	<dcterms:modified rdf:datatype="http://www.w3.org/2001/XMLSchema#dateTime">2017-06-27T04:07:58Z</dcterms:modified>
	<dc:publisher rdf:datatype="http://www.w3.org/2001/XMLSchema#string">Institute for Marine and Antarctic Studies (IMAS) - UTAS</dc:publisher>
	<skos:definition xml:lang="en">An area of relatively homogenous species composition, clearly distinct from adjacent systems. The species composition is likely to be determined by the predominance of a small number of ecosystems and/or a distinct suite of oceanographic or topographic features. The dominant biogeographic forcing agents defining the ecoregions vary from location to location but may include isolation, upwelling, nutrient inputs, freshwater influx, temperature regimes, ice regimes, exposure, sediments, currents and bathymetric or coastal complexity.</skos:definition>
	<dc:source rdf:datatype="http://www.w3.org/2001/XMLSchema#string">Marine Ecoregions of the World (MEOW). Spalding et.al. (2007)</dc:source>
	<skos:exactMatch rdf:resource="http://www.marineregions.org/gazetteer.php?p=details&amp;id=21883"/>
</rdf:Description>

<rdf:Description rdf:about="http://www.marineregions.org/gazetteer.php?p=details&amp;id=21883">
	<rdf:type rdf:resource="http://www.w3.org/2000/01/rdf-schema#Resource"/>
</rdf:Description>

<rdf:Description rdf:about="http://seamapaustralia.org.au/def/benthichabitatclassification/class/176">
	<rdf:type rdf:resource="http://www.w3.org/2000/01/rdf-schema#Resource"/>
	<rdf:type rdf:resource="http://www.w3.org/2004/02/skos/core#Concept"/>
	<skos:broader rdf:resource="http://seamapaustralia.org.au/def/benthichabitatclassification/class/106"/>
	<skos:prefLabel xml:lang="en">MEOW Tropical Southwestern Pacific Province</skos:prefLabel>
	<dcterms:contributor rdf:resource="http://editor.vocabs.ands.org.au/user/eMII_Finney.Kim_Admin"/>
	<dcterms:created rdf:datatype="http://www.w3.org/2001/XMLSchema#dateTime">2017-05-31T01:55:23Z</dcterms:created>
	<dcterms:creator rdf:resource="http://editor.vocabs.ands.org.au/user/eMII_Finney.Kim_Admin"/>
	<dcterms:modified rdf:datatype="http://www.w3.org/2001/XMLSchema#dateTime">2017-06-27T04:09:40Z</dcterms:modified>
	<dc:publisher rdf:datatype="http://www.w3.org/2001/XMLSchema#string">Institute for Marine and Antarctic Studies (IMAS) - UTAS</dc:publisher>
	<skos:definition xml:lang="en">A large area defined by the presence of distinct biotas that has at least some cohesion over evolutionary time frames. Provinces will hold some level of endemism, principally at the level of species. Although historical isolation will play a role, many of these distinct biotas have arisen as a result of distinctive abiotic features that circumscribe their boundaries. These may include geomorphological features (isoloated island and shelf systems, semienclosed seas); hydrographic features (currents, upwellings, ice dynamics); or geochemical influences (broadest-scale elements of nutrient supply and salinity).</skos:definition>
	<dc:source rdf:datatype="http://www.w3.org/2001/XMLSchema#string">Marine Ecoregions of the World (MEOW). Spalding et.al. (2007)</dc:source>
	<skos:narrower rdf:resource="http://seamapaustralia.org.au/def/benthichabitatclassification/class/201"/>
	<skos:narrower rdf:resource="http://seamapaustralia.org.au/def/benthichabitatclassification/class/200"/>
	<skos:exactMatch rdf:resource="http://www.marineregions.org/gazetteer.php?p=details&amp;id=21782"/>
</rdf:Description>

<rdf:Description rdf:about="http://www.marineregions.org/gazetteer.php?p=details&amp;id=21904">
	<rdf:type rdf:resource="http://www.w3.org/2000/01/rdf-schema#Resource"/>
</rdf:Description>

<rdf:Description rdf:about="http://www.marineregions.org/gazetteer.php?p=details&amp;id=21905">
	<rdf:type rdf:resource="http://www.w3.org/2000/01/rdf-schema#Resource"/>
</rdf:Description>

<rdf:Description rdf:about="http://seamapaustralia.org.au/def/benthichabitatclassification/class/187">
	<rdf:type rdf:resource="http://www.w3.org/2000/01/rdf-schema#Resource"/>
	<rdf:type rdf:resource="http://www.w3.org/2004/02/skos/core#Concept"/>
	<skos:broader rdf:resource="http://seamapaustralia.org.au/def/benthichabitatclassification/class/175"/>
	<skos:prefLabel xml:lang="en">MEOW Exmouth to Broome Ecoregion</skos:prefLabel>
	<dcterms:contributor rdf:resource="http://editor.vocabs.ands.org.au/user/eMII_Finney.Kim_Admin"/>
	<dcterms:created rdf:datatype="http://www.w3.org/2001/XMLSchema#dateTime">2017-05-31T02:03:07Z</dcterms:created>
	<dcterms:creator rdf:resource="http://editor.vocabs.ands.org.au/user/eMII_Finney.Kim_Admin"/>
	<dcterms:modified rdf:datatype="http://www.w3.org/2001/XMLSchema#dateTime">2017-06-27T04:08:51Z</dcterms:modified>
	<dc:publisher rdf:datatype="http://www.w3.org/2001/XMLSchema#string">Institute for Marine and Antarctic Studies (IMAS) - UTAS</dc:publisher>
	<skos:definition xml:lang="en">An area of relatively homogenous species composition, clearly distinct from adjacent systems. The species composition is likely to be determined by the predominance of a small number of ecosystems and/or a distinct suite of oceanographic or topographic features. The dominant biogeographic forcing agents defining the ecoregions vary from location to location but may include isolation, upwelling, nutrient inputs, freshwater influx, temperature regimes, ice regimes, exposure, sediments, currents and bathymetric or coastal complexity.</skos:definition>
	<dc:source rdf:datatype="http://www.w3.org/2001/XMLSchema#string">Marine Ecoregions of the World (MEOW). Spalding et.al. (2007)</dc:source>
	<skos:narrower rdf:resource="http://seamapaustralia.org.au/def/benthichabitatclassification/class/290"/>
	<skos:exactMatch rdf:resource="http://www.marineregions.org/gazetteer.php?p=details&amp;id=21916"/>
</rdf:Description>

<rdf:Description rdf:about="http://www.marineregions.org/gazetteer.php?p=details&amp;id=21916">
	<rdf:type rdf:resource="http://www.w3.org/2000/01/rdf-schema#Resource"/>
</rdf:Description>

<rdf:Description rdf:about="http://seamapaustralia.org.au/def/benthichabitatclassification/class/188">
	<rdf:type rdf:resource="http://www.w3.org/2000/01/rdf-schema#Resource"/>
	<rdf:type rdf:resource="http://www.w3.org/2004/02/skos/core#Concept"/>
	<skos:broader rdf:resource="http://seamapaustralia.org.au/def/benthichabitatclassification/class/175"/>
	<skos:prefLabel xml:lang="en">MEOW Ningaloo Ecoregion</skos:prefLabel>
	<dcterms:contributor rdf:resource="http://editor.vocabs.ands.org.au/user/eMII_Finney.Kim_Admin"/>
	<dcterms:created rdf:datatype="http://www.w3.org/2001/XMLSchema#dateTime">2017-05-31T02:03:30Z</dcterms:created>
	<dcterms:creator rdf:resource="http://editor.vocabs.ands.org.au/user/eMII_Finney.Kim_Admin"/>
	<dcterms:modified rdf:datatype="http://www.w3.org/2001/XMLSchema#dateTime">2017-06-27T04:09:01Z</dcterms:modified>
	<dc:publisher rdf:datatype="http://www.w3.org/2001/XMLSchema#string">Institute for Marine and Antarctic Studies (IMAS) - UTAS</dc:publisher>
	<skos:definition xml:lang="en">An area of relatively homogenous species composition, clearly distinct from adjacent systems. The species composition is likely to be determined by the predominance of a small number of ecosystems and/or a distinct suite of oceanographic or topographic features. The dominant biogeographic forcing agents defining the ecoregions vary from location to location but may include isolation, upwelling, nutrient inputs, freshwater influx, temperature regimes, ice regimes, exposure, sediments, currents and bathymetric or coastal complexity.</skos:definition>
	<dc:source rdf:datatype="http://www.w3.org/2001/XMLSchema#string">Marine Ecoregions of the World (MEOW). Spalding et.al. (2007)</dc:source>
	<skos:narrower rdf:resource="http://seamapaustralia.org.au/def/benthichabitatclassification/class/296"/>
	<skos:exactMatch rdf:resource="http://www.marineregions.org/gazetteer.php?p=details&amp;id=21917"/>
</rdf:Description>

<rdf:Description rdf:about="http://www.marineregions.org/gazetteer.php?p=details&amp;id=21917">
	<rdf:type rdf:resource="http://www.w3.org/2000/01/rdf-schema#Resource"/>
</rdf:Description>

<rdf:Description rdf:about="http://www.marineregions.org/gazetteer.php?p=details&amp;id=21922">
	<rdf:type rdf:resource="http://www.w3.org/2000/01/rdf-schema#Resource"/>
</rdf:Description>

<rdf:Description rdf:about="http://seamapaustralia.org.au/def/benthichabitatclassification/class/190">
	<rdf:type rdf:resource="http://www.w3.org/2000/01/rdf-schema#Resource"/>
	<rdf:type rdf:resource="http://www.w3.org/2004/02/skos/core#Concept"/>
	<skos:broader rdf:resource="http://seamapaustralia.org.au/def/benthichabitatclassification/class/173"/>
	<skos:prefLabel xml:lang="en">MEOW Arafura Sea Ecoregion</skos:prefLabel>
	<dcterms:contributor rdf:resource="http://editor.vocabs.ands.org.au/user/eMII_Finney.Kim_Admin"/>
	<dcterms:created rdf:datatype="http://www.w3.org/2001/XMLSchema#dateTime">2017-05-31T02:04:23Z</dcterms:created>
	<dcterms:creator rdf:resource="http://editor.vocabs.ands.org.au/user/eMII_Finney.Kim_Admin"/>
	<dcterms:modified rdf:datatype="http://www.w3.org/2001/XMLSchema#dateTime">2017-06-27T04:09:14Z</dcterms:modified>
	<dc:publisher rdf:datatype="http://www.w3.org/2001/XMLSchema#string">Institute for Marine and Antarctic Studies (IMAS) - UTAS</dc:publisher>
	<skos:definition xml:lang="en">An area of relatively homogenous species composition, clearly distinct from adjacent systems. The species composition is likely to be determined by the predominance of a small number of ecosystems and/or a distinct suite of oceanographic or topographic features. The dominant biogeographic forcing agents defining the ecoregions vary from location to location but may include isolation, upwelling, nutrient inputs, freshwater influx, temperature regimes, ice regimes, exposure, sediments, currents and bathymetric or coastal complexity.</skos:definition>
	<dc:source rdf:datatype="http://www.w3.org/2001/XMLSchema#string">Marine Ecoregions of the World (MEOW). Spalding et.al. (2007)</dc:source>
	<skos:exactMatch rdf:resource="http://www.marineregions.org/gazetteer.php?p=details&amp;id=21924"/>
</rdf:Description>

<rdf:Description rdf:about="http://www.marineregions.org/gazetteer.php?p=details&amp;id=21924">
	<rdf:type rdf:resource="http://www.w3.org/2000/01/rdf-schema#Resource"/>
</rdf:Description>

<rdf:Description rdf:about="http://seamapaustralia.org.au/def/benthichabitatclassification/class/192">
	<rdf:type rdf:resource="http://www.w3.org/2000/01/rdf-schema#Resource"/>
	<rdf:type rdf:resource="http://www.w3.org/2004/02/skos/core#Concept"/>
	<skos:broader rdf:resource="http://seamapaustralia.org.au/def/benthichabitatclassification/class/173"/>
	<skos:prefLabel xml:lang="en">MEOW Bonaparte Coast Ecoregion</skos:prefLabel>
	<dcterms:contributor rdf:resource="http://editor.vocabs.ands.org.au/user/eMII_Finney.Kim_Admin"/>
	<dcterms:created rdf:datatype="http://www.w3.org/2001/XMLSchema#dateTime">2017-05-31T02:05:22Z</dcterms:created>
	<dcterms:creator rdf:resource="http://editor.vocabs.ands.org.au/user/eMII_Finney.Kim_Admin"/>
	<dcterms:modified rdf:datatype="http://www.w3.org/2001/XMLSchema#dateTime">2017-06-27T04:09:27Z</dcterms:modified>
	<dc:publisher rdf:datatype="http://www.w3.org/2001/XMLSchema#string">Institute for Marine and Antarctic Studies (IMAS) - UTAS</dc:publisher>
	<skos:definition xml:lang="en">An area of relatively homogenous species composition, clearly distinct from adjacent systems. The species composition is likely to be determined by the predominance of a small number of ecosystems and/or a distinct suite of oceanographic or topographic features. The dominant biogeographic forcing agents defining the ecoregions vary from location to location but may include isolation, upwelling, nutrient inputs, freshwater influx, temperature regimes, ice regimes, exposure, sediments, currents and bathymetric or coastal complexity.</skos:definition>
	<dc:source rdf:datatype="http://www.w3.org/2001/XMLSchema#string">Marine Ecoregions of the World (MEOW). Spalding et.al. (2007)</dc:source>
	<skos:narrower rdf:resource="http://seamapaustralia.org.au/def/benthichabitatclassification/class/309"/>
	<skos:exactMatch rdf:resource="http://www.marineregions.org/gazetteer.php?p=details&amp;id=21923"/>
</rdf:Description>

<rdf:Description rdf:about="http://seamapaustralia.org.au/def/benthichabitatclassification/class/173">
	<rdf:type rdf:resource="http://www.w3.org/2000/01/rdf-schema#Resource"/>
	<rdf:type rdf:resource="http://www.w3.org/2004/02/skos/core#Concept"/>
	<skos:broader rdf:resource="http://seamapaustralia.org.au/def/benthichabitatclassification/class/106"/>
	<skos:prefLabel xml:lang="en">MEOW Sahul Shelf Province</skos:prefLabel>
	<dcterms:contributor rdf:resource="http://editor.vocabs.ands.org.au/user/eMII_Finney.Kim_Admin"/>
	<dcterms:created rdf:datatype="http://www.w3.org/2001/XMLSchema#dateTime">2017-05-31T01:53:26Z</dcterms:created>
	<dcterms:creator rdf:resource="http://editor.vocabs.ands.org.au/user/eMII_Finney.Kim_Admin"/>
	<dcterms:modified rdf:datatype="http://www.w3.org/2001/XMLSchema#dateTime">2017-06-27T04:09:08Z</dcterms:modified>
	<dc:publisher rdf:datatype="http://www.w3.org/2001/XMLSchema#string">Institute for Marine and Antarctic Studies (IMAS) - UTAS</dc:publisher>
	<skos:definition xml:lang="en">A large area defined by the presence of distinct biotas that has at least some cohesion over evolutionary time frames. Provinces will hold some level of endemism, principally at the level of species. Although historical isolation will play a role, many of these distinct biotas have arisen as a result of distinctive abiotic features that circumscribe their boundaries. These may include geomorphological features (isoloated island and shelf systems, semienclosed seas); hydrographic features (currents, upwellings, ice dynamics); or geochemical influences (broadest-scale elements of nutrient supply and salinity).</skos:definition>
	<dc:source rdf:datatype="http://www.w3.org/2001/XMLSchema#string">Marine Ecoregions of the World (MEOW). Spalding et.al. (2007)</dc:source>
	<skos:narrower rdf:resource="http://seamapaustralia.org.au/def/benthichabitatclassification/class/191"/>
	<skos:narrower rdf:resource="http://seamapaustralia.org.au/def/benthichabitatclassification/class/189"/>
	<skos:narrower rdf:resource="http://seamapaustralia.org.au/def/benthichabitatclassification/class/190"/>
	<skos:narrower rdf:resource="http://seamapaustralia.org.au/def/benthichabitatclassification/class/192"/>
	<skos:exactMatch rdf:resource="http://www.marineregions.org/gazetteer.php?p=details&amp;id=21727"/>
</rdf:Description>

<rdf:Description rdf:about="http://seamapaustralia.org.au/def/benthichabitatclassification/class/171">
	<rdf:type rdf:resource="http://www.w3.org/2000/01/rdf-schema#Resource"/>
	<rdf:type rdf:resource="http://www.w3.org/2004/02/skos/core#Concept"/>
	<skos:broader rdf:resource="http://seamapaustralia.org.au/def/benthichabitatclassification/class/106"/>
	<skos:prefLabel xml:lang="en">MEOW Western Coral Triangle Province</skos:prefLabel>
	<dcterms:contributor rdf:resource="http://editor.vocabs.ands.org.au/user/eMII_Finney.Kim_Admin"/>
	<dcterms:created rdf:datatype="http://www.w3.org/2001/XMLSchema#dateTime">2017-05-31T01:38:54Z</dcterms:created>
	<dcterms:creator rdf:resource="http://editor.vocabs.ands.org.au/user/eMII_Finney.Kim_Admin"/>
	<dcterms:modified rdf:datatype="http://www.w3.org/2001/XMLSchema#dateTime">2017-06-27T04:09:58Z</dcterms:modified>
	<dc:publisher rdf:datatype="http://www.w3.org/2001/XMLSchema#string">Institute for Marine and Antarctic Studies (IMAS) - UTAS</dc:publisher>
	<skos:definition xml:lang="en">A large area defined by the presence of distinct biotas that has at least some cohesion over evolutionary time frames. Provinces will hold some level of endemism, principally at the level of species. Although historical isolation will play a role, many of these distinct biotas have arisen as a result of distinctive abiotic features that circumscribe their boundaries. These may include geomorphological features (isoloated island and shelf systems, semienclosed seas); hydrographic features (currents, upwellings, ice dynamics); or geochemical influences (broadest-scale elements of nutrient supply and salinity).</skos:definition>
	<dc:source rdf:datatype="http://www.w3.org/2001/XMLSchema#string">Marine Ecoregions of the World (MEOW). Spalding et.al. (2007)</dc:source>
	<skos:narrower rdf:resource="http://seamapaustralia.org.au/def/benthichabitatclassification/class/203"/>
	<skos:narrower rdf:resource="http://seamapaustralia.org.au/def/benthichabitatclassification/class/205"/>
	<skos:narrower rdf:resource="http://seamapaustralia.org.au/def/benthichabitatclassification/class/206"/>
	<skos:narrower rdf:resource="http://seamapaustralia.org.au/def/benthichabitatclassification/class/207"/>
	<skos:narrower rdf:resource="http://seamapaustralia.org.au/def/benthichabitatclassification/class/208"/>
	<skos:exactMatch rdf:resource="http://www.marineregions.org/gazetteer.php?p=details&amp;id=21728"/>
</rdf:Description>

<rdf:Description rdf:about="http://www.marineregions.org/gazetteer.php?p=details&amp;id=21728">
	<rdf:type rdf:resource="http://www.w3.org/2000/01/rdf-schema#Resource"/>
</rdf:Description>

<rdf:Description rdf:about="http://www.marineregions.org/gazetteer.php?p=details&amp;id=21718">
	<rdf:type rdf:resource="http://www.w3.org/2000/01/rdf-schema#Resource"/>
</rdf:Description>

<rdf:Description rdf:about="http://www.marineregions.org/gazetteer.php?p=details&amp;id=21923">
	<rdf:type rdf:resource="http://www.w3.org/2000/01/rdf-schema#Resource"/>
</rdf:Description>

<rdf:Description rdf:about="http://seamapaustralia.org.au/def/benthichabitatclassification/class/170">
	<rdf:type rdf:resource="http://www.w3.org/2000/01/rdf-schema#Resource"/>
	<rdf:type rdf:resource="http://www.w3.org/2004/02/skos/core#Concept"/>
	<skos:broader rdf:resource="http://seamapaustralia.org.au/def/benthichabitatclassification/class/106"/>
	<skos:prefLabel xml:lang="en">MEOW Java Transitional Province</skos:prefLabel>
	<dcterms:contributor rdf:resource="http://editor.vocabs.ands.org.au/user/eMII_Finney.Kim_Admin"/>
	<dcterms:created rdf:datatype="http://www.w3.org/2001/XMLSchema#dateTime">2017-05-31T01:27:48Z</dcterms:created>
	<dcterms:creator rdf:resource="http://editor.vocabs.ands.org.au/user/eMII_Finney.Kim_Admin"/>
	<dcterms:modified rdf:datatype="http://www.w3.org/2001/XMLSchema#dateTime">2017-06-27T04:07:36Z</dcterms:modified>
	<dc:publisher rdf:datatype="http://www.w3.org/2001/XMLSchema#string">Institute for Marine and Antarctic Studies (IMAS) - UTAS</dc:publisher>
	<skos:definition xml:lang="en">A large area defined by the presence of distinct biotas that has at least some cohesion over evolutionary time frames. Provinces will hold some level of endemism, principally at the level of species. Although historical isolation will play a role, many of these distinct biotas have arisen as a result of distinctive abiotic features that circumscribe their boundaries. These may include geomorphological features (isoloated island and shelf systems, semienclosed seas); hydrographic features (currents, upwellings, ice dynamics); or geochemical influences (broadest-scale elements of nutrient supply and salinity).</skos:definition>
	<dc:source rdf:datatype="http://www.w3.org/2001/XMLSchema#string">Marine Ecoregions of the World (MEOW). Spalding et.al. (2007)</dc:source>
	<skos:narrower rdf:resource="http://seamapaustralia.org.au/def/benthichabitatclassification/class/183"/>
	<skos:narrower rdf:resource="http://seamapaustralia.org.au/def/benthichabitatclassification/class/184"/>
	<skos:exactMatch rdf:resource="http://www.marineregions.org/gazetteer.php?p=details&amp;id=21730"/>
</rdf:Description>

<rdf:Description rdf:about="http://seamapaustralia.org.au/def/benthichabitatclassification/class/172">
	<rdf:type rdf:resource="http://www.w3.org/2000/01/rdf-schema#Resource"/>
	<rdf:type rdf:resource="http://www.w3.org/2004/02/skos/core#Concept"/>
	<skos:broader rdf:resource="http://seamapaustralia.org.au/def/benthichabitatclassification/class/106"/>
	<skos:prefLabel xml:lang="en">MEOW Eastern Coral Triangle Province</skos:prefLabel>
	<dcterms:contributor rdf:resource="http://editor.vocabs.ands.org.au/user/eMII_Finney.Kim_Admin"/>
	<dcterms:created rdf:datatype="http://www.w3.org/2001/XMLSchema#dateTime">2017-05-31T01:39:30Z</dcterms:created>
	<dcterms:creator rdf:resource="http://editor.vocabs.ands.org.au/user/eMII_Finney.Kim_Admin"/>
	<dcterms:modified rdf:datatype="http://www.w3.org/2001/XMLSchema#dateTime">2017-06-27T04:07:02Z</dcterms:modified>
	<dc:publisher rdf:datatype="http://www.w3.org/2001/XMLSchema#string">Institute for Marine and Antarctic Studies (IMAS) - UTAS</dc:publisher>
	<skos:definition xml:lang="en">A large area defined by the presence of distinct biotas that has at least some cohesion over evolutionary time frames. Provinces will hold some level of endemism, principally at the level of species. Although historical isolation will play a role, many of these distinct biotas have arisen as a result of distinctive abiotic features that circumscribe their boundaries. These may include geomorphological features (isoloated island and shelf systems, semienclosed seas); hydrographic features (currents, upwellings, ice dynamics); or geochemical influences (broadest-scale elements of nutrient supply and salinity).</skos:definition>
	<dc:source rdf:datatype="http://www.w3.org/2001/XMLSchema#string">Marine Ecoregions of the World (MEOW). Spalding et.al. (2007)</dc:source>
	<skos:narrower rdf:resource="http://seamapaustralia.org.au/def/benthichabitatclassification/class/179"/>
	<skos:narrower rdf:resource="http://seamapaustralia.org.au/def/benthichabitatclassification/class/180"/>
	<skos:narrower rdf:resource="http://seamapaustralia.org.au/def/benthichabitatclassification/class/181"/>
	<skos:narrower rdf:resource="http://seamapaustralia.org.au/def/benthichabitatclassification/class/182"/>
	<skos:exactMatch rdf:resource="http://www.marineregions.org/gazetteer.php?p=details&amp;id=21729"/>
</rdf:Description>

<rdf:Description rdf:about="http://seamapaustralia.org.au/def/benthichabitatclassification/class/174">
	<rdf:type rdf:resource="http://www.w3.org/2000/01/rdf-schema#Resource"/>
	<rdf:type rdf:resource="http://www.w3.org/2004/02/skos/core#Concept"/>
	<skos:broader rdf:resource="http://seamapaustralia.org.au/def/benthichabitatclassification/class/106"/>
	<skos:prefLabel xml:lang="en">MEOW Northeast Australian Shelf Province</skos:prefLabel>
	<dcterms:contributor rdf:resource="http://editor.vocabs.ands.org.au/user/eMII_Finney.Kim_Admin"/>
	<dcterms:created rdf:datatype="http://www.w3.org/2001/XMLSchema#dateTime">2017-05-31T01:53:55Z</dcterms:created>
	<dcterms:creator rdf:resource="http://editor.vocabs.ands.org.au/user/eMII_Finney.Kim_Admin"/>
	<dcterms:modified rdf:datatype="http://www.w3.org/2001/XMLSchema#dateTime">2017-06-27T04:08:04Z</dcterms:modified>
	<dc:publisher rdf:datatype="http://www.w3.org/2001/XMLSchema#string">Institute for Marine and Antarctic Studies (IMAS) - UTAS</dc:publisher>
	<skos:definition xml:lang="en">A large area defined by the presence of distinct biotas that has at least some cohesion over evolutionary time frames. Provinces will hold some level of endemism, principally at the level of species. Although historical isolation will play a role, many of these distinct biotas have arisen as a result of distinctive abiotic features that circumscribe their boundaries. These may include geomorphological features (isoloated island and shelf systems, semienclosed seas); hydrographic features (currents, upwellings, ice dynamics); or geochemical influences (broadest-scale elements of nutrient supply and salinity).</skos:definition>
	<dc:source rdf:datatype="http://www.w3.org/2001/XMLSchema#string">Marine Ecoregions of the World (MEOW). Spalding et.al. (2007)</dc:source>
	<skos:narrower rdf:resource="http://seamapaustralia.org.au/def/benthichabitatclassification/class/186"/>
	<skos:narrower rdf:resource="http://seamapaustralia.org.au/def/benthichabitatclassification/class/185"/>
	<skos:exactMatch rdf:resource="http://www.marineregions.org/gazetteer.php?p=details&amp;id=21737"/>
</rdf:Description>

<rdf:Description rdf:about="http://seamapaustralia.org.au/def/benthichabitatclassification/class/175">
	<rdf:type rdf:resource="http://www.w3.org/2000/01/rdf-schema#Resource"/>
	<rdf:type rdf:resource="http://www.w3.org/2004/02/skos/core#Concept"/>
	<skos:broader rdf:resource="http://seamapaustralia.org.au/def/benthichabitatclassification/class/106"/>
	<skos:prefLabel xml:lang="en">MEOW Northwest Australian Shelf Province</skos:prefLabel>
	<dcterms:contributor rdf:resource="http://editor.vocabs.ands.org.au/user/eMII_Finney.Kim_Admin"/>
	<dcterms:created rdf:datatype="http://www.w3.org/2001/XMLSchema#dateTime">2017-05-31T01:54:38Z</dcterms:created>
	<dcterms:creator rdf:resource="http://editor.vocabs.ands.org.au/user/eMII_Finney.Kim_Admin"/>
	<dcterms:modified rdf:datatype="http://www.w3.org/2001/XMLSchema#dateTime">2017-06-27T04:08:45Z</dcterms:modified>
	<dc:publisher rdf:datatype="http://www.w3.org/2001/XMLSchema#string">Institute for Marine and Antarctic Studies (IMAS) - UTAS</dc:publisher>
	<skos:definition xml:lang="en">A large area defined by the presence of distinct biotas that has at least some cohesion over evolutionary time frames. Provinces will hold some level of endemism, principally at the level of species. Although historical isolation will play a role, many of these distinct biotas have arisen as a result of distinctive abiotic features that circumscribe their boundaries. These may include geomorphological features (isoloated island and shelf systems, semienclosed seas); hydrographic features (currents, upwellings, ice dynamics); or geochemical influences (broadest-scale elements of nutrient supply and salinity).</skos:definition>
	<dc:source rdf:datatype="http://www.w3.org/2001/XMLSchema#string">Marine Ecoregions of the World (MEOW). Spalding et.al. (2007)</dc:source>
	<skos:narrower rdf:resource="http://seamapaustralia.org.au/def/benthichabitatclassification/class/187"/>
	<skos:narrower rdf:resource="http://seamapaustralia.org.au/def/benthichabitatclassification/class/188"/>
	<skos:exactMatch rdf:resource="http://www.marineregions.org/gazetteer.php?p=details&amp;id=21732"/>
</rdf:Description>

<rdf:Description rdf:about="http://seamapaustralia.org.au/def/benthichabitatclassification/class/177">
	<rdf:type rdf:resource="http://www.w3.org/2000/01/rdf-schema#Resource"/>
	<rdf:type rdf:resource="http://www.w3.org/2004/02/skos/core#Concept"/>
	<skos:broader rdf:resource="http://seamapaustralia.org.au/def/benthichabitatclassification/class/106"/>
	<skos:prefLabel xml:lang="en">MEOW Lord Howe and Norfolk Islands Province</skos:prefLabel>
	<dcterms:contributor rdf:resource="http://editor.vocabs.ands.org.au/user/eMII_Finney.Kim_Admin"/>
	<dcterms:created rdf:datatype="http://www.w3.org/2001/XMLSchema#dateTime">2017-05-31T01:56:11Z</dcterms:created>
	<dcterms:creator rdf:resource="http://editor.vocabs.ands.org.au/user/eMII_Finney.Kim_Admin"/>
	<dcterms:modified rdf:datatype="http://www.w3.org/2001/XMLSchema#dateTime">2017-06-27T04:07:53Z</dcterms:modified>
	<dc:publisher rdf:datatype="http://www.w3.org/2001/XMLSchema#string">Institute for Marine and Antarctic Studies (IMAS) - UTAS</dc:publisher>
	<skos:definition xml:lang="en">A large area defined by the presence of distinct biotas that has at least some cohesion over evolutionary time frames. Provinces will hold some level of endemism, principally at the level of species. Although historical isolation will play a role, many of these distinct biotas have arisen as a result of distinctive abiotic features that circumscribe their boundaries. These may include geomorphological features (isoloated island and shelf systems, semienclosed seas); hydrographic features (currents, upwellings, ice dynamics); or geochemical influences (broadest-scale elements of nutrient supply and salinity).</skos:definition>
	<dc:source rdf:datatype="http://www.w3.org/2001/XMLSchema#string">Marine Ecoregions of the World (MEOW). Spalding et.al. (2007)</dc:source>
	<skos:narrower rdf:resource="http://seamapaustralia.org.au/def/benthichabitatclassification/class/178"/>
	<skos:exactMatch rdf:resource="http://www.marineregions.org/gazetteer.php?p=details&amp;id=21735"/>
</rdf:Description>

<rdf:Description rdf:about="http://seamapaustralia.org.au/def/benthichabitatclassification/class/179">
	<rdf:type rdf:resource="http://www.w3.org/2000/01/rdf-schema#Resource"/>
	<rdf:type rdf:resource="http://www.w3.org/2004/02/skos/core#Concept"/>
	<skos:broader rdf:resource="http://seamapaustralia.org.au/def/benthichabitatclassification/class/172"/>
	<skos:prefLabel xml:lang="en">MEOW Bismarck Sea Ecoregion</skos:prefLabel>
	<dcterms:contributor rdf:resource="http://editor.vocabs.ands.org.au/user/eMII_Finney.Kim_Admin"/>
	<dcterms:created rdf:datatype="http://www.w3.org/2001/XMLSchema#dateTime">2017-05-31T01:57:54Z</dcterms:created>
	<dcterms:creator rdf:resource="http://editor.vocabs.ands.org.au/user/eMII_Finney.Kim_Admin"/>
	<dcterms:modified rdf:datatype="http://www.w3.org/2001/XMLSchema#dateTime">2017-06-27T04:07:10Z</dcterms:modified>
	<dc:publisher rdf:datatype="http://www.w3.org/2001/XMLSchema#string">Institute for Marine and Antarctic Studies (IMAS) - UTAS</dc:publisher>
	<skos:definition xml:lang="en">An area of relatively homogenous species composition, clearly distinct from adjacent systems. The species composition is likely to be determined by the predominance of a small number of ecosystems and/or a distinct suite of oceanographic or topographic features. The dominant biogeographic forcing agents defining the ecoregions vary from location to location but may include isolation, upwelling, nutrient inputs, freshwater influx, temperature regimes, ice regimes, exposure, sediments, currents and bathymetric or coastal complexity.</skos:definition>
	<dc:source rdf:datatype="http://www.w3.org/2001/XMLSchema#string">Marine Ecoregions of the World (MEOW). Spalding et.al. (2007)</dc:source>
	<skos:exactMatch rdf:resource="http://www.marineregions.org/gazetteer.php?p=details&amp;id=21869"/>
</rdf:Description>

<rdf:Description rdf:about="http://seamapaustralia.org.au/def/benthichabitatclassification/class/180">
	<rdf:type rdf:resource="http://www.w3.org/2000/01/rdf-schema#Resource"/>
	<rdf:type rdf:resource="http://www.w3.org/2004/02/skos/core#Concept"/>
	<skos:broader rdf:resource="http://seamapaustralia.org.au/def/benthichabitatclassification/class/172"/>
	<skos:prefLabel xml:lang="en">MEOW Soloman Archipelago Ecoregion</skos:prefLabel>
	<dcterms:contributor rdf:resource="http://editor.vocabs.ands.org.au/user/eMII_Finney.Kim_Admin"/>
	<dcterms:created rdf:datatype="http://www.w3.org/2001/XMLSchema#dateTime">2017-05-31T01:58:22Z</dcterms:created>
	<dcterms:creator rdf:resource="http://editor.vocabs.ands.org.au/user/eMII_Finney.Kim_Admin"/>
	<dcterms:modified rdf:datatype="http://www.w3.org/2001/XMLSchema#dateTime">2017-06-27T04:07:16Z</dcterms:modified>
	<dc:publisher rdf:datatype="http://www.w3.org/2001/XMLSchema#string">Institute for Marine and Antarctic Studies (IMAS) - UTAS</dc:publisher>
	<skos:definition xml:lang="en">An area of relatively homogenous species composition, clearly distinct from adjacent systems. The species composition is likely to be determined by the predominance of a small number of ecosystems and/or a distinct suite of oceanographic or topographic features. The dominant biogeographic forcing agents defining the ecoregions vary from location to location but may include isolation, upwelling, nutrient inputs, freshwater influx, temperature regimes, ice regimes, exposure, sediments, currents and bathymetric or coastal complexity.</skos:definition>
	<dc:source rdf:datatype="http://www.w3.org/2001/XMLSchema#string">Marine Ecoregions of the World (MEOW). Spalding et.al. (2007)</dc:source>
	<skos:exactMatch rdf:resource="http://www.marineregions.org/gazetteer.php?p=details&amp;id=21868"/>
</rdf:Description>

<rdf:Description rdf:about="http://seamapaustralia.org.au/def/benthichabitatclassification/class/181">
	<rdf:type rdf:resource="http://www.w3.org/2000/01/rdf-schema#Resource"/>
	<rdf:type rdf:resource="http://www.w3.org/2004/02/skos/core#Concept"/>
	<skos:broader rdf:resource="http://seamapaustralia.org.au/def/benthichabitatclassification/class/172"/>
	<skos:prefLabel xml:lang="en">MEOW Soloman Sea Ecoregion</skos:prefLabel>
	<dcterms:contributor rdf:resource="http://editor.vocabs.ands.org.au/user/eMII_Finney.Kim_Admin"/>
	<dcterms:created rdf:datatype="http://www.w3.org/2001/XMLSchema#dateTime">2017-05-31T01:58:45Z</dcterms:created>
	<dcterms:creator rdf:resource="http://editor.vocabs.ands.org.au/user/eMII_Finney.Kim_Admin"/>
	<dcterms:modified rdf:datatype="http://www.w3.org/2001/XMLSchema#dateTime">2017-06-27T04:07:24Z</dcterms:modified>
	<dc:publisher rdf:datatype="http://www.w3.org/2001/XMLSchema#string">Institute for Marine and Antarctic Studies (IMAS) - UTAS</dc:publisher>
	<skos:definition xml:lang="en">An area of relatively homogenous species composition, clearly distinct from adjacent systems. The species composition is likely to be determined by the predominance of a small number of ecosystems and/or a distinct suite of oceanographic or topographic features. The dominant biogeographic forcing agents defining the ecoregions vary from location to location but may include isolation, upwelling, nutrient inputs, freshwater influx, temperature regimes, ice regimes, exposure, sediments, currents and bathymetric or coastal complexity.</skos:definition>
	<dc:source rdf:datatype="http://www.w3.org/2001/XMLSchema#string">Marine Ecoregions of the World (MEOW). Spalding et.al. (2007)</dc:source>
	<skos:exactMatch rdf:resource="http://www.marineregions.org/gazetteer.php?p=details&amp;id=21867"/>
</rdf:Description>

<rdf:Description rdf:about="http://seamapaustralia.org.au/def/benthichabitatclassification/class/182">
	<rdf:type rdf:resource="http://www.w3.org/2000/01/rdf-schema#Resource"/>
	<rdf:type rdf:resource="http://www.w3.org/2004/02/skos/core#Concept"/>
	<skos:broader rdf:resource="http://seamapaustralia.org.au/def/benthichabitatclassification/class/172"/>
	<skos:prefLabel xml:lang="en">MEOW Southeast Papua New Guinea Ecoregion</skos:prefLabel>
	<dcterms:contributor rdf:resource="http://editor.vocabs.ands.org.au/user/eMII_Finney.Kim_Admin"/>
	<dcterms:created rdf:datatype="http://www.w3.org/2001/XMLSchema#dateTime">2017-05-31T01:59:27Z</dcterms:created>
	<dcterms:creator rdf:resource="http://editor.vocabs.ands.org.au/user/eMII_Finney.Kim_Admin"/>
	<dcterms:modified rdf:datatype="http://www.w3.org/2001/XMLSchema#dateTime">2017-06-27T04:07:30Z</dcterms:modified>
	<dc:publisher rdf:datatype="http://www.w3.org/2001/XMLSchema#string">Institute for Marine and Antarctic Studies (IMAS) - UTAS</dc:publisher>
	<skos:definition xml:lang="en">An area of relatively homogenous species composition, clearly distinct from adjacent systems. The species composition is likely to be determined by the predominance of a small number of ecosystems and/or a distinct suite of oceanographic or topographic features. The dominant biogeographic forcing agents defining the ecoregions vary from location to location but may include isolation, upwelling, nutrient inputs, freshwater influx, temperature regimes, ice regimes, exposure, sediments, currents and bathymetric or coastal complexity.</skos:definition>
	<dc:source rdf:datatype="http://www.w3.org/2001/XMLSchema#string">Marine Ecoregions of the World (MEOW). Spalding et.al. (2007)</dc:source>
	<skos:exactMatch rdf:resource="http://www.marineregions.org/gazetteer.php?p=details&amp;id=21866"/>
</rdf:Description>

<rdf:Description rdf:about="http://seamapaustralia.org.au/def/benthichabitatclassification/class/183">
	<rdf:type rdf:resource="http://www.w3.org/2000/01/rdf-schema#Resource"/>
	<rdf:type rdf:resource="http://www.w3.org/2004/02/skos/core#Concept"/>
	<skos:broader rdf:resource="http://seamapaustralia.org.au/def/benthichabitatclassification/class/170"/>
	<skos:prefLabel xml:lang="en">MEOW Souther Java Ecoregion</skos:prefLabel>
	<dcterms:contributor rdf:resource="http://editor.vocabs.ands.org.au/user/eMII_Finney.Kim_Admin"/>
	<dcterms:created rdf:datatype="http://www.w3.org/2001/XMLSchema#dateTime">2017-05-31T02:00:24Z</dcterms:created>
	<dcterms:creator rdf:resource="http://editor.vocabs.ands.org.au/user/eMII_Finney.Kim_Admin"/>
	<dcterms:modified rdf:datatype="http://www.w3.org/2001/XMLSchema#dateTime">2017-06-27T04:07:47Z</dcterms:modified>
	<dc:publisher rdf:datatype="http://www.w3.org/2001/XMLSchema#string">Institute for Marine and Antarctic Studies (IMAS) - UTAS</dc:publisher>
	<skos:definition xml:lang="en">An area of relatively homogenous species composition, clearly distinct from adjacent systems. The species composition is likely to be determined by the predominance of a small number of ecosystems and/or a distinct suite of oceanographic or topographic features. The dominant biogeographic forcing agents defining the ecoregions vary from location to location but may include isolation, upwelling, nutrient inputs, freshwater influx, temperature regimes, ice regimes, exposure, sediments, currents and bathymetric or coastal complexity.</skos:definition>
	<dc:source rdf:datatype="http://www.w3.org/2001/XMLSchema#string">Marine Ecoregions of the World (MEOW). Spalding et.al. (2007)</dc:source>
	<skos:exactMatch rdf:resource="http://www.marineregions.org/gazetteer.php?p=details&amp;id=21880"/>
</rdf:Description>

<rdf:Description rdf:about="http://seamapaustralia.org.au/def/benthichabitatclassification/class/184">
	<rdf:type rdf:resource="http://www.w3.org/2000/01/rdf-schema#Resource"/>
	<rdf:type rdf:resource="http://www.w3.org/2004/02/skos/core#Concept"/>
	<skos:broader rdf:resource="http://seamapaustralia.org.au/def/benthichabitatclassification/class/170"/>
	<skos:prefLabel xml:lang="en">MEOW Cocos-Keeling-Christmas Island Ecoregion</skos:prefLabel>
	<dcterms:contributor rdf:resource="http://editor.vocabs.ands.org.au/user/eMII_Finney.Kim_Admin"/>
	<dcterms:created rdf:datatype="http://www.w3.org/2001/XMLSchema#dateTime">2017-05-31T02:01:03Z</dcterms:created>
	<dcterms:creator rdf:resource="http://editor.vocabs.ands.org.au/user/eMII_Finney.Kim_Admin"/>
	<dcterms:modified rdf:datatype="http://www.w3.org/2001/XMLSchema#dateTime">2017-06-27T04:07:42Z</dcterms:modified>
	<dc:publisher rdf:datatype="http://www.w3.org/2001/XMLSchema#string">Institute for Marine and Antarctic Studies (IMAS) - UTAS</dc:publisher>
	<skos:definition xml:lang="en">An area of relatively homogenous species composition, clearly distinct from adjacent systems. The species composition is likely to be determined by the predominance of a small number of ecosystems and/or a distinct suite of oceanographic or topographic features. The dominant biogeographic forcing agents defining the ecoregions vary from location to location but may include isolation, upwelling, nutrient inputs, freshwater influx, temperature regimes, ice regimes, exposure, sediments, currents and bathymetric or coastal complexity.</skos:definition>
	<dc:source rdf:datatype="http://www.w3.org/2001/XMLSchema#string">Marine Ecoregions of the World (MEOW). Spalding et.al. (2007)</dc:source>
	<skos:exactMatch rdf:resource="http://www.marineregions.org/gazetteer.php?p=details&amp;id=21881"/>
</rdf:Description>

<rdf:Description rdf:about="http://seamapaustralia.org.au/def/benthichabitatclassification/class/211">
	<rdf:type rdf:resource="http://www.w3.org/2000/01/rdf-schema#Resource"/>
	<rdf:type rdf:resource="http://www.w3.org/2004/02/skos/core#Concept"/>
	<skos:broader rdf:resource="http://seamapaustralia.org.au/def/benthichabitatclassification/class/112"/>
	<skos:prefLabel xml:lang="en">MEOW Continental High Antarctic Province</skos:prefLabel>
	<dcterms:contributor rdf:resource="http://editor.vocabs.ands.org.au/user/eMII_Finney.Kim_Admin"/>
	<dcterms:created rdf:datatype="http://www.w3.org/2001/XMLSchema#dateTime">2017-05-31T02:35:17Z</dcterms:created>
	<dcterms:creator rdf:resource="http://editor.vocabs.ands.org.au/user/eMII_Finney.Kim_Admin"/>
	<dcterms:modified rdf:datatype="http://www.w3.org/2001/XMLSchema#dateTime">2017-06-27T04:10:37Z</dcterms:modified>
	<dc:publisher rdf:datatype="http://www.w3.org/2001/XMLSchema#string">Institute for Marine and Antarctic Studies (IMAS) - UTAS</dc:publisher>
	<skos:definition xml:lang="en">A large area defined by the presence of distinct biotas that has at least some cohesion over evolutionary time frames. Provinces will hold some level of endemism, principally at the level of species. Although historical isolation will play a role, many of these distinct biotas have arisen as a result of distinctive abiotic features that circumscribe their boundaries. These may include geomorphological features (isoloated island and shelf systems, semienclosed seas); hydrographic features (currents, upwellings, ice dynamics); or geochemical influences (broadest-scale elements of nutrient supply and salinity).</skos:definition>
	<dc:source rdf:datatype="http://www.w3.org/2001/XMLSchema#string">Marine Ecoregions of the World (MEOW). Spalding et.al. (2007)</dc:source>
	<skos:narrower rdf:resource="http://seamapaustralia.org.au/def/benthichabitatclassification/class/212"/>
	<skos:narrower rdf:resource="http://seamapaustralia.org.au/def/benthichabitatclassification/class/213"/>
	<skos:narrower rdf:resource="http://seamapaustralia.org.au/def/benthichabitatclassification/class/214"/>
	<skos:narrower rdf:resource="http://seamapaustralia.org.au/def/benthichabitatclassification/class/215"/>
	<skos:narrower rdf:resource="http://seamapaustralia.org.au/def/benthichabitatclassification/class/217"/>
	<skos:narrower rdf:resource="http://seamapaustralia.org.au/def/benthichabitatclassification/class/218"/>
	<skos:exactMatch rdf:resource="http://www.marineregions.org/gazetteer.php?p=details&amp;id=21778"/>
</rdf:Description>

<rdf:Description rdf:about="http://www.marineregions.org/gazetteer.php?p=details&amp;id=21778">
	<rdf:type rdf:resource="http://www.w3.org/2000/01/rdf-schema#Resource"/>
</rdf:Description>

<rdf:Description rdf:about="http://seamapaustralia.org.au/def/benthichabitatclassification/class/210">
	<rdf:type rdf:resource="http://www.w3.org/2000/01/rdf-schema#Resource"/>
	<rdf:type rdf:resource="http://www.w3.org/2004/02/skos/core#Concept"/>
	<skos:broader rdf:resource="http://seamapaustralia.org.au/def/benthichabitatclassification/class/112"/>
	<skos:prefLabel xml:lang="en">MEOW Subantarctic Islands Province</skos:prefLabel>
	<dcterms:contributor rdf:resource="http://editor.vocabs.ands.org.au/user/eMII_Finney.Kim_Admin"/>
	<dcterms:created rdf:datatype="http://www.w3.org/2001/XMLSchema#dateTime">2017-05-31T02:34:32Z</dcterms:created>
	<dcterms:creator rdf:resource="http://editor.vocabs.ands.org.au/user/eMII_Finney.Kim_Admin"/>
	<dcterms:modified rdf:datatype="http://www.w3.org/2001/XMLSchema#dateTime">2017-06-27T04:11:15Z</dcterms:modified>
	<dc:publisher rdf:datatype="http://www.w3.org/2001/XMLSchema#string">Institute for Marine and Antarctic Studies (IMAS) - UTAS</dc:publisher>
	<skos:definition xml:lang="en">A large area defined by the presence of distinct biotas that has at least some cohesion over evolutionary time frames. Provinces will hold some level of endemism, principally at the level of species. Although historical isolation will play a role, many of these distinct biotas have arisen as a result of distinctive abiotic features that circumscribe their boundaries. These may include geomorphological features (isoloated island and shelf systems, semienclosed seas); hydrographic features (currents, upwellings, ice dynamics); or geochemical influences (broadest-scale elements of nutrient supply and salinity).</skos:definition>
	<dc:source rdf:datatype="http://www.w3.org/2001/XMLSchema#string">Marine Ecoregions of the World (MEOW). Spalding et.al. (2007)</dc:source>
	<skos:narrower rdf:resource="http://seamapaustralia.org.au/def/benthichabitatclassification/class/219"/>
	<skos:narrower rdf:resource="http://seamapaustralia.org.au/def/benthichabitatclassification/class/220"/>
	<skos:narrower rdf:resource="http://seamapaustralia.org.au/def/benthichabitatclassification/class/221"/>
	<skos:narrower rdf:resource="http://seamapaustralia.org.au/def/benthichabitatclassification/class/222"/>
	<skos:narrower rdf:resource="http://seamapaustralia.org.au/def/benthichabitatclassification/class/223"/>
	<skos:narrower rdf:resource="http://seamapaustralia.org.au/def/benthichabitatclassification/class/224"/>
	<skos:exactMatch rdf:resource="http://www.marineregions.org/gazetteer.php?p=details&amp;id=21743"/>
</rdf:Description>

<rdf:Description rdf:about="http://www.marineregions.org/gazetteer.php?p=details&amp;id=21743">
	<rdf:type rdf:resource="http://www.w3.org/2000/01/rdf-schema#Resource"/>
</rdf:Description>

<rdf:Description rdf:about="http://www.marineregions.org/gazetteer.php?p=details&amp;id=21747">
	<rdf:type rdf:resource="http://www.w3.org/2000/01/rdf-schema#Resource"/>
</rdf:Description>

<rdf:Description rdf:about="http://www.marineregions.org/gazetteer.php?p=details&amp;id=21744">
	<rdf:type rdf:resource="http://www.w3.org/2000/01/rdf-schema#Resource"/>
</rdf:Description>

<rdf:Description rdf:about="http://www.marineregions.org/gazetteer.php?p=details&amp;id=21745">
	<rdf:type rdf:resource="http://www.w3.org/2000/01/rdf-schema#Resource"/>
</rdf:Description>

<rdf:Description rdf:about="http://www.marineregions.org/gazetteer.php?p=details&amp;id=21869">
	<rdf:type rdf:resource="http://www.w3.org/2000/01/rdf-schema#Resource"/>
</rdf:Description>

<rdf:Description rdf:about="http://www.marineregions.org/gazetteer.php?p=details&amp;id=21868">
	<rdf:type rdf:resource="http://www.w3.org/2000/01/rdf-schema#Resource"/>
</rdf:Description>

<rdf:Description rdf:about="http://www.marineregions.org/gazetteer.php?p=details&amp;id=21867">
	<rdf:type rdf:resource="http://www.w3.org/2000/01/rdf-schema#Resource"/>
</rdf:Description>

<rdf:Description rdf:about="http://www.marineregions.org/gazetteer.php?p=details&amp;id=21866">
	<rdf:type rdf:resource="http://www.w3.org/2000/01/rdf-schema#Resource"/>
</rdf:Description>

<rdf:Description rdf:about="http://www.marineregions.org/gazetteer.php?p=details&amp;id=21881">
	<rdf:type rdf:resource="http://www.w3.org/2000/01/rdf-schema#Resource"/>
</rdf:Description>

<rdf:Description rdf:about="http://www.marineregions.org/gazetteer.php?p=details&amp;id=21880">
	<rdf:type rdf:resource="http://www.w3.org/2000/01/rdf-schema#Resource"/>
</rdf:Description>

<rdf:Description rdf:about="http://seamapaustralia.org.au/def/benthichabitatclassification/class/201">
	<rdf:type rdf:resource="http://www.w3.org/2000/01/rdf-schema#Resource"/>
	<rdf:type rdf:resource="http://www.w3.org/2004/02/skos/core#Concept"/>
	<skos:broader rdf:resource="http://seamapaustralia.org.au/def/benthichabitatclassification/class/176"/>
	<skos:prefLabel xml:lang="en">MEOW Coral Sea Ecoregion</skos:prefLabel>
	<dcterms:contributor rdf:resource="http://editor.vocabs.ands.org.au/user/eMII_Finney.Kim_Admin"/>
	<dcterms:created rdf:datatype="http://www.w3.org/2001/XMLSchema#dateTime">2017-05-31T02:09:25Z</dcterms:created>
	<dcterms:creator rdf:resource="http://editor.vocabs.ands.org.au/user/eMII_Finney.Kim_Admin"/>
	<dcterms:modified rdf:datatype="http://www.w3.org/2001/XMLSchema#dateTime">2017-06-27T04:09:46Z</dcterms:modified>
	<dc:publisher rdf:datatype="http://www.w3.org/2001/XMLSchema#string">Institute for Marine and Antarctic Studies (IMAS) - UTAS</dc:publisher>
	<skos:definition xml:lang="en">An area of relatively homogenous species composition, clearly distinct from adjacent systems. The species composition is likely to be determined by the predominance of a small number of ecosystems and/or a distinct suite of oceanographic or topographic features. The dominant biogeographic forcing agents defining the ecoregions vary from location to location but may include isolation, upwelling, nutrient inputs, freshwater influx, temperature regimes, ice regimes, exposure, sediments, currents and bathymetric or coastal complexity.</skos:definition>
	<dc:source rdf:datatype="http://www.w3.org/2001/XMLSchema#string">Marine Ecoregions of the World (MEOW). Spalding et.al. (2007)</dc:source>
	<skos:exactMatch rdf:resource="http://www.marineregions.org/gazetteer.php?p=details&amp;id=21995"/>
</rdf:Description>

<rdf:Description rdf:about="http://www.marineregions.org/gazetteer.php?p=details&amp;id=21737">
	<rdf:type rdf:resource="http://www.w3.org/2000/01/rdf-schema#Resource"/>
</rdf:Description>

<rdf:Description rdf:about="http://www.marineregions.org/gazetteer.php?p=details&amp;id=21995">
	<rdf:type rdf:resource="http://www.w3.org/2000/01/rdf-schema#Resource"/>
</rdf:Description>

<rdf:Description rdf:about="http://seamapaustralia.org.au/def/benthichabitatclassification/class/200">
	<rdf:type rdf:resource="http://www.w3.org/2000/01/rdf-schema#Resource"/>
	<rdf:type rdf:resource="http://www.w3.org/2004/02/skos/core#Concept"/>
	<skos:broader rdf:resource="http://seamapaustralia.org.au/def/benthichabitatclassification/class/176"/>
	<skos:prefLabel xml:lang="en">MEOW New Caledonia Ecoregion</skos:prefLabel>
	<dcterms:contributor rdf:resource="http://editor.vocabs.ands.org.au/user/eMII_Finney.Kim_Admin"/>
	<dcterms:created rdf:datatype="http://www.w3.org/2001/XMLSchema#dateTime">2017-05-31T02:09:00Z</dcterms:created>
	<dcterms:creator rdf:resource="http://editor.vocabs.ands.org.au/user/eMII_Finney.Kim_Admin"/>
	<dcterms:modified rdf:datatype="http://www.w3.org/2001/XMLSchema#dateTime">2017-06-27T04:09:52Z</dcterms:modified>
	<dc:publisher rdf:datatype="http://www.w3.org/2001/XMLSchema#string">Institute for Marine and Antarctic Studies (IMAS) - UTAS</dc:publisher>
	<skos:definition xml:lang="en">An area of relatively homogenous species composition, clearly distinct from adjacent systems. The species composition is likely to be determined by the predominance of a small number of ecosystems and/or a distinct suite of oceanographic or topographic features. The dominant biogeographic forcing agents defining the ecoregions vary from location to location but may include isolation, upwelling, nutrient inputs, freshwater influx, temperature regimes, ice regimes, exposure, sediments, currents and bathymetric or coastal complexity.</skos:definition>
	<dc:source rdf:datatype="http://www.w3.org/2001/XMLSchema#string">Marine Ecoregions of the World (MEOW). Spalding et.al. (2007)</dc:source>
	<skos:exactMatch rdf:resource="http://www.marineregions.org/gazetteer.php?p=details&amp;id=21997"/>
</rdf:Description>

<rdf:Description rdf:about="http://www.marineregions.org/gazetteer.php?p=details&amp;id=21997">
	<rdf:type rdf:resource="http://www.w3.org/2000/01/rdf-schema#Resource"/>
</rdf:Description>

<rdf:Description rdf:about="http://www.marineregions.org/gazetteer.php?p=details&amp;id=21782">
	<rdf:type rdf:resource="http://www.w3.org/2000/01/rdf-schema#Resource"/>
</rdf:Description>

<rdf:Description rdf:about="http://www.marineregions.org/gazetteer.php?p=details&amp;id=21732">
	<rdf:type rdf:resource="http://www.w3.org/2000/01/rdf-schema#Resource"/>
</rdf:Description>

<rdf:Description rdf:about="http://www.marineregions.org/gazetteer.php?p=details&amp;id=21727">
	<rdf:type rdf:resource="http://www.w3.org/2000/01/rdf-schema#Resource"/>
</rdf:Description>

<rdf:Description rdf:about="http://www.environment.gov.au/mapping/rest/services/ogc_services/IMCRA_Provincial/MapServer/0/9">
	<rdf:type rdf:resource="http://www.w3.org/2000/01/rdf-schema#Resource"/>
</rdf:Description>

<rdf:Description rdf:about="http://www.environment.gov.au/mapping/rest/services/ogc_services/IMCRA_Mesoscale/MapServer/0/2">
	<rdf:type rdf:resource="http://www.w3.org/2000/01/rdf-schema#Resource"/>
</rdf:Description>

<rdf:Description rdf:about="http://www.environment.gov.au/mapping/rest/services/ogc_services/IMCRA_Mesoscale/MapServer/0/31">
	<rdf:type rdf:resource="http://www.w3.org/2000/01/rdf-schema#Resource"/>
</rdf:Description>

<rdf:Description rdf:about="http://seamapaustralia.org.au/def/benthichabitatclassification/class/203">
	<rdf:type rdf:resource="http://www.w3.org/2000/01/rdf-schema#Resource"/>
	<rdf:type rdf:resource="http://www.w3.org/2004/02/skos/core#Concept"/>
	<skos:broader rdf:resource="http://seamapaustralia.org.au/def/benthichabitatclassification/class/171"/>
	<skos:prefLabel xml:lang="en">MEOW Eastern Philippines Ecoregion</skos:prefLabel>
	<dcterms:contributor rdf:resource="http://editor.vocabs.ands.org.au/user/eMII_Finney.Kim_Admin"/>
	<dcterms:created rdf:datatype="http://www.w3.org/2001/XMLSchema#dateTime">2017-05-31T02:11:06Z</dcterms:created>
	<dcterms:creator rdf:resource="http://editor.vocabs.ands.org.au/user/eMII_Finney.Kim_Admin"/>
	<dcterms:modified rdf:datatype="http://www.w3.org/2001/XMLSchema#dateTime">2017-06-27T04:10:07Z</dcterms:modified>
	<dc:publisher rdf:datatype="http://www.w3.org/2001/XMLSchema#string">Institute for Marine and Antarctic Studies (IMAS) - UTAS</dc:publisher>
	<skos:definition xml:lang="en">An area of relatively homogenous species composition, clearly distinct from adjacent systems. The species composition is likely to be determined by the predominance of a small number of ecosystems and/or a distinct suite of oceanographic or topographic features. The dominant biogeographic forcing agents defining the ecoregions vary from location to location but may include isolation, upwelling, nutrient inputs, freshwater influx, temperature regimes, ice regimes, exposure, sediments, currents and bathymetric or coastal complexity.</skos:definition>
	<dc:source rdf:datatype="http://www.w3.org/2001/XMLSchema#string">Marine Ecoregions of the World (MEOW). Spalding et.al. (2007)</dc:source>
	<skos:exactMatch rdf:resource="http://www.marineregions.org/gazetteer.php?p=details&amp;id=22020"/>
</rdf:Description>

<rdf:Description rdf:about="http://www.environment.gov.au/mapping/rest/services/ogc_services/IMCRA_Mesoscale/MapServer/0/20">
	<rdf:type rdf:resource="http://www.w3.org/2000/01/rdf-schema#Resource"/>
</rdf:Description>

<rdf:Description rdf:about="http://seamapaustralia.org.au/def/benthichabitatclassification/class/205">
	<rdf:type rdf:resource="http://www.w3.org/2000/01/rdf-schema#Resource"/>
	<rdf:type rdf:resource="http://www.w3.org/2004/02/skos/core#Concept"/>
	<skos:broader rdf:resource="http://seamapaustralia.org.au/def/benthichabitatclassification/class/171"/>
	<skos:prefLabel xml:lang="en">MEOW Halmahera Ecoregion</skos:prefLabel>
	<dcterms:contributor rdf:resource="http://editor.vocabs.ands.org.au/user/eMII_Finney.Kim_Admin"/>
	<dcterms:created rdf:datatype="http://www.w3.org/2001/XMLSchema#dateTime">2017-05-31T02:12:01Z</dcterms:created>
	<dcterms:creator rdf:resource="http://editor.vocabs.ands.org.au/user/eMII_Finney.Kim_Admin"/>
	<dcterms:modified rdf:datatype="http://www.w3.org/2001/XMLSchema#dateTime">2017-06-27T04:10:11Z</dcterms:modified>
	<dc:publisher rdf:datatype="http://www.w3.org/2001/XMLSchema#string">Institute for Marine and Antarctic Studies (IMAS) - UTAS</dc:publisher>
	<skos:definition xml:lang="en">An area of relatively homogenous species composition, clearly distinct from adjacent systems. The species composition is likely to be determined by the predominance of a small number of ecosystems and/or a distinct suite of oceanographic or topographic features. The dominant biogeographic forcing agents defining the ecoregions vary from location to location but may include isolation, upwelling, nutrient inputs, freshwater influx, temperature regimes, ice regimes, exposure, sediments, currents and bathymetric or coastal complexity.</skos:definition>
	<dc:source rdf:datatype="http://www.w3.org/2001/XMLSchema#string">Marine Ecoregions of the World (MEOW). Spalding et.al. (2007)</dc:source>
	<skos:exactMatch rdf:resource="http://www.marineregions.org/gazetteer.php?p=details&amp;id=22025"/>
</rdf:Description>

<rdf:Description rdf:about="http://seamapaustralia.org.au/def/benthichabitatclassification/class/206">
	<rdf:type rdf:resource="http://www.w3.org/2000/01/rdf-schema#Resource"/>
	<rdf:type rdf:resource="http://www.w3.org/2004/02/skos/core#Concept"/>
	<skos:broader rdf:resource="http://seamapaustralia.org.au/def/benthichabitatclassification/class/171"/>
	<skos:prefLabel xml:lang="en">MEOW Papua Ecoregion</skos:prefLabel>
	<dcterms:contributor rdf:resource="http://editor.vocabs.ands.org.au/user/eMII_Finney.Kim_Admin"/>
	<dcterms:created rdf:datatype="http://www.w3.org/2001/XMLSchema#dateTime">2017-05-31T02:12:23Z</dcterms:created>
	<dcterms:creator rdf:resource="http://editor.vocabs.ands.org.au/user/eMII_Finney.Kim_Admin"/>
	<dcterms:modified rdf:datatype="http://www.w3.org/2001/XMLSchema#dateTime">2017-06-27T04:10:22Z</dcterms:modified>
	<dc:publisher rdf:datatype="http://www.w3.org/2001/XMLSchema#string">Institute for Marine and Antarctic Studies (IMAS) - UTAS</dc:publisher>
	<skos:definition xml:lang="en">An area of relatively homogenous species composition, clearly distinct from adjacent systems. The species composition is likely to be determined by the predominance of a small number of ecosystems and/or a distinct suite of oceanographic or topographic features. The dominant biogeographic forcing agents defining the ecoregions vary from location to location but may include isolation, upwelling, nutrient inputs, freshwater influx, temperature regimes, ice regimes, exposure, sediments, currents and bathymetric or coastal complexity.</skos:definition>
	<dc:source rdf:datatype="http://www.w3.org/2001/XMLSchema#string">Marine Ecoregions of the World (MEOW). Spalding et.al. (2007)</dc:source>
	<skos:exactMatch rdf:resource="http://www.marineregions.org/gazetteer.php?p=details&amp;id=22024"/>
</rdf:Description>

<rdf:Description rdf:about="http://seamapaustralia.org.au/def/benthichabitatclassification/class/207">
	<rdf:type rdf:resource="http://www.w3.org/2000/01/rdf-schema#Resource"/>
	<rdf:type rdf:resource="http://www.w3.org/2004/02/skos/core#Concept"/>
	<skos:broader rdf:resource="http://seamapaustralia.org.au/def/benthichabitatclassification/class/171"/>
	<skos:prefLabel xml:lang="en">MEOW Banda Sea Ecoregion</skos:prefLabel>
	<dcterms:contributor rdf:resource="http://editor.vocabs.ands.org.au/user/eMII_Finney.Kim_Admin"/>
	<dcterms:created rdf:datatype="http://www.w3.org/2001/XMLSchema#dateTime">2017-05-31T02:12:43Z</dcterms:created>
	<dcterms:creator rdf:resource="http://editor.vocabs.ands.org.au/user/eMII_Finney.Kim_Admin"/>
	<dcterms:modified rdf:datatype="http://www.w3.org/2001/XMLSchema#dateTime">2017-06-27T04:10:02Z</dcterms:modified>
	<dc:publisher rdf:datatype="http://www.w3.org/2001/XMLSchema#string">Institute for Marine and Antarctic Studies (IMAS) - UTAS</dc:publisher>
	<skos:definition xml:lang="en">An area of relatively homogenous species composition, clearly distinct from adjacent systems. The species composition is likely to be determined by the predominance of a small number of ecosystems and/or a distinct suite of oceanographic or topographic features. The dominant biogeographic forcing agents defining the ecoregions vary from location to location but may include isolation, upwelling, nutrient inputs, freshwater influx, temperature regimes, ice regimes, exposure, sediments, currents and bathymetric or coastal complexity.</skos:definition>
	<dc:source rdf:datatype="http://www.w3.org/2001/XMLSchema#string">Marine Ecoregions of the World (MEOW). Spalding et.al. (2007)</dc:source>
	<skos:exactMatch rdf:resource="http://www.marineregions.org/gazetteer.php?p=details&amp;id=22021"/>
</rdf:Description>

<rdf:Description rdf:about="http://seamapaustralia.org.au/def/benthichabitatclassification/class/208">
	<rdf:type rdf:resource="http://www.w3.org/2000/01/rdf-schema#Resource"/>
	<rdf:type rdf:resource="http://www.w3.org/2004/02/skos/core#Concept"/>
	<skos:broader rdf:resource="http://seamapaustralia.org.au/def/benthichabitatclassification/class/171"/>
	<skos:prefLabel xml:lang="en">MEOW Lesser Sunda Ecoregion</skos:prefLabel>
	<dcterms:contributor rdf:resource="http://editor.vocabs.ands.org.au/user/eMII_Finney.Kim_Admin"/>
	<dcterms:created rdf:datatype="http://www.w3.org/2001/XMLSchema#dateTime">2017-05-31T02:13:05Z</dcterms:created>
	<dcterms:creator rdf:resource="http://editor.vocabs.ands.org.au/user/eMII_Finney.Kim_Admin"/>
	<dcterms:modified rdf:datatype="http://www.w3.org/2001/XMLSchema#dateTime">2017-06-27T04:10:15Z</dcterms:modified>
	<dc:publisher rdf:datatype="http://www.w3.org/2001/XMLSchema#string">Institute for Marine and Antarctic Studies (IMAS) - UTAS</dc:publisher>
	<skos:definition xml:lang="en">An area of relatively homogenous species composition, clearly distinct from adjacent systems. The species composition is likely to be determined by the predominance of a small number of ecosystems and/or a distinct suite of oceanographic or topographic features. The dominant biogeographic forcing agents defining the ecoregions vary from location to location but may include isolation, upwelling, nutrient inputs, freshwater influx, temperature regimes, ice regimes, exposure, sediments, currents and bathymetric or coastal complexity.</skos:definition>
	<dc:source rdf:datatype="http://www.w3.org/2001/XMLSchema#string">Marine Ecoregions of the World (MEOW). Spalding et.al. (2007)</dc:source>
	<skos:exactMatch rdf:resource="http://www.marineregions.org/gazetteer.php?p=details&amp;id=22026"/>
</rdf:Description>

<rdf:Description rdf:about="http://www.environment.gov.au/mapping/rest/services/ogc_services/IMCRA_Mesoscale/MapServer/0/27">
	<rdf:type rdf:resource="http://www.w3.org/2000/01/rdf-schema#Resource"/>
</rdf:Description>

<rdf:Description rdf:about="http://seamapaustralia.org.au/def/benthichabitatclassification/class/212">
	<rdf:type rdf:resource="http://www.w3.org/2000/01/rdf-schema#Resource"/>
	<rdf:type rdf:resource="http://www.w3.org/2004/02/skos/core#Concept"/>
	<skos:broader rdf:resource="http://seamapaustralia.org.au/def/benthichabitatclassification/class/211"/>
	<skos:prefLabel xml:lang="en">MEOW East Antarctic Wilkes Land Ecoregion</skos:prefLabel>
	<dcterms:contributor rdf:resource="http://editor.vocabs.ands.org.au/user/eMII_Finney.Kim_Admin"/>
	<dcterms:created rdf:datatype="http://www.w3.org/2001/XMLSchema#dateTime">2017-05-31T02:36:10Z</dcterms:created>
	<dcterms:creator rdf:resource="http://editor.vocabs.ands.org.au/user/eMII_Finney.Kim_Admin"/>
	<dcterms:modified rdf:datatype="http://www.w3.org/2001/XMLSchema#dateTime">2017-06-27T04:10:59Z</dcterms:modified>
	<dc:publisher rdf:datatype="http://www.w3.org/2001/XMLSchema#string">Institute for Marine and Antarctic Studies (IMAS) - UTAS</dc:publisher>
	<skos:definition xml:lang="en">An area of relatively homogenous species composition, clearly distinct from adjacent systems. The species composition is likely to be determined by the predominance of a small number of ecosystems and/or a distinct suite of oceanographic or topographic features. The dominant biogeographic forcing agents defining the ecoregions vary from location to location but may include isolation, upwelling, nutrient inputs, freshwater influx, temperature regimes, ice regimes, exposure, sediments, currents and bathymetric or coastal complexity.</skos:definition>
	<dc:source rdf:datatype="http://www.w3.org/2001/XMLSchema#string">Marine Ecoregions of the World (MEOW). Spalding et.al. (2007)</dc:source>
	<skos:exactMatch rdf:resource="http://www.marineregions.org/gazetteer.php?p=details&amp;id=21858"/>
</rdf:Description>

<rdf:Description rdf:about="http://seamapaustralia.org.au/def/benthichabitatclassification/class/213">
	<rdf:type rdf:resource="http://www.w3.org/2000/01/rdf-schema#Resource"/>
	<rdf:type rdf:resource="http://www.w3.org/2004/02/skos/core#Concept"/>
	<skos:broader rdf:resource="http://seamapaustralia.org.au/def/benthichabitatclassification/class/211"/>
	<skos:prefLabel xml:lang="en">MEOW East Antarctic Enderby Land Ecoregion</skos:prefLabel>
	<dcterms:contributor rdf:resource="http://editor.vocabs.ands.org.au/user/eMII_Finney.Kim_Admin"/>
	<dcterms:created rdf:datatype="http://www.w3.org/2001/XMLSchema#dateTime">2017-05-31T02:36:37Z</dcterms:created>
	<dcterms:creator rdf:resource="http://editor.vocabs.ands.org.au/user/eMII_Finney.Kim_Admin"/>
	<dcterms:modified rdf:datatype="http://www.w3.org/2001/XMLSchema#dateTime">2017-06-27T04:10:54Z</dcterms:modified>
	<dc:publisher rdf:datatype="http://www.w3.org/2001/XMLSchema#string">Institute for Marine and Antarctic Studies (IMAS) - UTAS</dc:publisher>
	<skos:definition xml:lang="en">An area of relatively homogenous species composition, clearly distinct from adjacent systems. The species composition is likely to be determined by the predominance of a small number of ecosystems and/or a distinct suite of oceanographic or topographic features. The dominant biogeographic forcing agents defining the ecoregions vary from location to location but may include isolation, upwelling, nutrient inputs, freshwater influx, temperature regimes, ice regimes, exposure, sediments, currents and bathymetric or coastal complexity.</skos:definition>
	<dc:source rdf:datatype="http://www.w3.org/2001/XMLSchema#string">Marine Ecoregions of the World (MEOW). Spalding et.al. (2007)</dc:source>
	<skos:exactMatch rdf:resource="http://www.marineregions.org/gazetteer.php?p=details&amp;id=21862"/>
</rdf:Description>

<rdf:Description rdf:about="http://seamapaustralia.org.au/def/benthichabitatclassification/class/214">
	<rdf:type rdf:resource="http://www.w3.org/2000/01/rdf-schema#Resource"/>
	<rdf:type rdf:resource="http://www.w3.org/2004/02/skos/core#Concept"/>
	<skos:broader rdf:resource="http://seamapaustralia.org.au/def/benthichabitatclassification/class/211"/>
	<skos:prefLabel xml:lang="en">MEOW East Antarctic Droning Maud Land Ecoregion</skos:prefLabel>
	<dcterms:contributor rdf:resource="http://editor.vocabs.ands.org.au/user/eMII_Finney.Kim_Admin"/>
	<dcterms:created rdf:datatype="http://www.w3.org/2001/XMLSchema#dateTime">2017-05-31T02:37:04Z</dcterms:created>
	<dcterms:creator rdf:resource="http://editor.vocabs.ands.org.au/user/eMII_Finney.Kim_Admin"/>
	<dcterms:modified rdf:datatype="http://www.w3.org/2001/XMLSchema#dateTime">2017-06-27T04:10:49Z</dcterms:modified>
	<dc:publisher rdf:datatype="http://www.w3.org/2001/XMLSchema#string">Institute for Marine and Antarctic Studies (IMAS) - UTAS</dc:publisher>
	<skos:definition xml:lang="en">An area of relatively homogenous species composition, clearly distinct from adjacent systems. The species composition is likely to be determined by the predominance of a small number of ecosystems and/or a distinct suite of oceanographic or topographic features. The dominant biogeographic forcing agents defining the ecoregions vary from location to location but may include isolation, upwelling, nutrient inputs, freshwater influx, temperature regimes, ice regimes, exposure, sediments, currents and bathymetric or coastal complexity.</skos:definition>
	<dc:source rdf:datatype="http://www.w3.org/2001/XMLSchema#string">Marine Ecoregions of the World (MEOW). Spalding et.al. (2007)</dc:source>
	<skos:exactMatch rdf:resource="http://www.marineregions.org/gazetteer.php?p=details&amp;id=21861"/>
</rdf:Description>

<rdf:Description rdf:about="http://seamapaustralia.org.au/def/benthichabitatclassification/class/215">
	<rdf:type rdf:resource="http://www.w3.org/2000/01/rdf-schema#Resource"/>
	<rdf:type rdf:resource="http://www.w3.org/2004/02/skos/core#Concept"/>
	<skos:broader rdf:resource="http://seamapaustralia.org.au/def/benthichabitatclassification/class/211"/>
	<skos:prefLabel xml:lang="en">MEOW Weddell Sea Ecoregion</skos:prefLabel>
	<dcterms:contributor rdf:resource="http://editor.vocabs.ands.org.au/user/eMII_Finney.Kim_Admin"/>
	<dcterms:created rdf:datatype="http://www.w3.org/2001/XMLSchema#dateTime">2017-05-31T02:37:36Z</dcterms:created>
	<dcterms:creator rdf:resource="http://editor.vocabs.ands.org.au/user/eMII_Finney.Kim_Admin"/>
	<dcterms:modified rdf:datatype="http://www.w3.org/2001/XMLSchema#dateTime">2017-06-27T04:11:09Z</dcterms:modified>
	<dc:publisher rdf:datatype="http://www.w3.org/2001/XMLSchema#string">Institute for Marine and Antarctic Studies (IMAS) - UTAS</dc:publisher>
	<skos:definition xml:lang="en">An area of relatively homogenous species composition, clearly distinct from adjacent systems. The species composition is likely to be determined by the predominance of a small number of ecosystems and/or a distinct suite of oceanographic or topographic features. The dominant biogeographic forcing agents defining the ecoregions vary from location to location but may include isolation, upwelling, nutrient inputs, freshwater influx, temperature regimes, ice regimes, exposure, sediments, currents and bathymetric or coastal complexity.</skos:definition>
	<dc:source rdf:datatype="http://www.w3.org/2001/XMLSchema#string">Marine Ecoregions of the World (MEOW). Spalding et.al. (2007)</dc:source>
	<skos:exactMatch rdf:resource="http://www.marineregions.org/gazetteer.php?p=details&amp;id=21860"/>
</rdf:Description>

<rdf:Description rdf:about="http://seamapaustralia.org.au/def/benthichabitatclassification/class/217">
	<rdf:type rdf:resource="http://www.w3.org/2000/01/rdf-schema#Resource"/>
	<rdf:type rdf:resource="http://www.w3.org/2004/02/skos/core#Concept"/>
	<skos:broader rdf:resource="http://seamapaustralia.org.au/def/benthichabitatclassification/class/211"/>
	<skos:prefLabel xml:lang="en">MEOW Amundsen-Bellingshauseb Sea Ecoregion</skos:prefLabel>
	<dcterms:contributor rdf:resource="http://editor.vocabs.ands.org.au/user/eMII_Finney.Kim_Admin"/>
	<dcterms:created rdf:datatype="http://www.w3.org/2001/XMLSchema#dateTime">2017-05-31T02:39:23Z</dcterms:created>
	<dcterms:creator rdf:resource="http://editor.vocabs.ands.org.au/user/eMII_Finney.Kim_Admin"/>
	<dcterms:modified rdf:datatype="http://www.w3.org/2001/XMLSchema#dateTime">2017-06-27T04:10:42Z</dcterms:modified>
	<dc:publisher rdf:datatype="http://www.w3.org/2001/XMLSchema#string">Institute for Marine and Antarctic Studies (IMAS) - UTAS</dc:publisher>
	<skos:definition xml:lang="en">An area of relatively homogenous species composition, clearly distinct from adjacent systems. The species composition is likely to be determined by the predominance of a small number of ecosystems and/or a distinct suite of oceanographic or topographic features. The dominant biogeographic forcing agents defining the ecoregions vary from location to location but may include isolation, upwelling, nutrient inputs, freshwater influx, temperature regimes, ice regimes, exposure, sediments, currents and bathymetric or coastal complexity.</skos:definition>
	<dc:source rdf:datatype="http://www.w3.org/2001/XMLSchema#string">Marine Ecoregions of the World (MEOW). Spalding et.al. (2007)</dc:source>
	<skos:exactMatch rdf:resource="http://www.marineregions.org/gazetteer.php?p=details&amp;id=21857"/>
</rdf:Description>

<rdf:Description rdf:about="http://seamapaustralia.org.au/def/benthichabitatclassification/class/218">
	<rdf:type rdf:resource="http://www.w3.org/2000/01/rdf-schema#Resource"/>
	<rdf:type rdf:resource="http://www.w3.org/2004/02/skos/core#Concept"/>
	<skos:broader rdf:resource="http://seamapaustralia.org.au/def/benthichabitatclassification/class/211"/>
	<skos:prefLabel xml:lang="en">MEOW Ross Sea Ecoregion</skos:prefLabel>
	<dcterms:contributor rdf:resource="http://editor.vocabs.ands.org.au/user/eMII_Finney.Kim_Admin"/>
	<dcterms:created rdf:datatype="http://www.w3.org/2001/XMLSchema#dateTime">2017-05-31T02:39:57Z</dcterms:created>
	<dcterms:creator rdf:resource="http://editor.vocabs.ands.org.au/user/eMII_Finney.Kim_Admin"/>
	<dcterms:modified rdf:datatype="http://www.w3.org/2001/XMLSchema#dateTime">2017-06-27T04:11:04Z</dcterms:modified>
	<dc:publisher rdf:datatype="http://www.w3.org/2001/XMLSchema#string">Institute for Marine and Antarctic Studies (IMAS) - UTAS</dc:publisher>
	<skos:definition xml:lang="en">An area of relatively homogenous species composition, clearly distinct from adjacent systems. The species composition is likely to be determined by the predominance of a small number of ecosystems and/or a distinct suite of oceanographic or topographic features. The dominant biogeographic forcing agents defining the ecoregions vary from location to location but may include isolation, upwelling, nutrient inputs, freshwater influx, temperature regimes, ice regimes, exposure, sediments, currents and bathymetric or coastal complexity.</skos:definition>
	<dc:source rdf:datatype="http://www.w3.org/2001/XMLSchema#string">Marine Ecoregions of the World (MEOW). Spalding et.al. (2007)</dc:source>
	<skos:exactMatch rdf:resource="http://www.marineregions.org/gazetteer.php?p=details&amp;id=21859"/>
</rdf:Description>

<rdf:Description rdf:about="http://seamapaustralia.org.au/def/benthichabitatclassification/class/219">
	<rdf:type rdf:resource="http://www.w3.org/2000/01/rdf-schema#Resource"/>
	<rdf:type rdf:resource="http://www.w3.org/2004/02/skos/core#Concept"/>
	<skos:broader rdf:resource="http://seamapaustralia.org.au/def/benthichabitatclassification/class/210"/>
	<skos:prefLabel xml:lang="en">MEOW Macquarie Island Ecoregion</skos:prefLabel>
	<dcterms:contributor rdf:resource="http://editor.vocabs.ands.org.au/user/eMII_Finney.Kim_Admin"/>
	<dcterms:created rdf:datatype="http://www.w3.org/2001/XMLSchema#dateTime">2017-05-31T02:41:29Z</dcterms:created>
	<dcterms:creator rdf:resource="http://editor.vocabs.ands.org.au/user/eMII_Finney.Kim_Admin"/>
	<dcterms:modified rdf:datatype="http://www.w3.org/2001/XMLSchema#dateTime">2017-06-27T04:11:39Z</dcterms:modified>
	<dc:publisher rdf:datatype="http://www.w3.org/2001/XMLSchema#string">Institute for Marine and Antarctic Studies (IMAS) - UTAS</dc:publisher>
	<skos:definition xml:lang="en">An area of relatively homogenous species composition, clearly distinct from adjacent systems. The species composition is likely to be determined by the predominance of a small number of ecosystems and/or a distinct suite of oceanographic or topographic features. The dominant biogeographic forcing agents defining the ecoregions vary from location to location but may include isolation, upwelling, nutrient inputs, freshwater influx, temperature regimes, ice regimes, exposure, sediments, currents and bathymetric or coastal complexity.</skos:definition>
	<dc:source rdf:datatype="http://www.w3.org/2001/XMLSchema#string">Marine Ecoregions of the World (MEOW). Spalding et.al. (2007)</dc:source>
	<skos:exactMatch rdf:resource="http://www.marineregions.org/gazetteer.php?p=details&amp;id=21957"/>
</rdf:Description>

<rdf:Description rdf:about="http://seamapaustralia.org.au/def/benthichabitatclassification/class/220">
	<rdf:type rdf:resource="http://www.w3.org/2000/01/rdf-schema#Resource"/>
	<rdf:type rdf:resource="http://www.w3.org/2004/02/skos/core#Concept"/>
	<skos:broader rdf:resource="http://seamapaustralia.org.au/def/benthichabitatclassification/class/210"/>
	<skos:prefLabel xml:lang="en">MEOW Heard and McDonald Islands Ecoregion</skos:prefLabel>
	<dcterms:contributor rdf:resource="http://editor.vocabs.ands.org.au/user/eMII_Finney.Kim_Admin"/>
	<dcterms:created rdf:datatype="http://www.w3.org/2001/XMLSchema#dateTime">2017-05-31T02:42:32Z</dcterms:created>
	<dcterms:creator rdf:resource="http://editor.vocabs.ands.org.au/user/eMII_Finney.Kim_Admin"/>
	<dcterms:modified rdf:datatype="http://www.w3.org/2001/XMLSchema#dateTime">2017-06-27T04:11:29Z</dcterms:modified>
	<dc:publisher rdf:datatype="http://www.w3.org/2001/XMLSchema#string">Institute for Marine and Antarctic Studies (IMAS) - UTAS</dc:publisher>
	<skos:definition xml:lang="en">An area of relatively homogenous species composition, clearly distinct from adjacent systems. The species composition is likely to be determined by the predominance of a small number of ecosystems and/or a distinct suite of oceanographic or topographic features. The dominant biogeographic forcing agents defining the ecoregions vary from location to location but may include isolation, upwelling, nutrient inputs, freshwater influx, temperature regimes, ice regimes, exposure, sediments, currents and bathymetric or coastal complexity.</skos:definition>
	<dc:source rdf:datatype="http://www.w3.org/2001/XMLSchema#string">Marine Ecoregions of the World (MEOW). Spalding et.al. (2007)</dc:source>
	<skos:exactMatch rdf:resource="http://www.marineregions.org/gazetteer.php?p=details&amp;id=21955"/>
</rdf:Description>

<rdf:Description rdf:about="http://seamapaustralia.org.au/def/benthichabitatclassification/class/221">
	<rdf:type rdf:resource="http://www.w3.org/2000/01/rdf-schema#Resource"/>
	<rdf:type rdf:resource="http://www.w3.org/2004/02/skos/core#Concept"/>
	<skos:broader rdf:resource="http://seamapaustralia.org.au/def/benthichabitatclassification/class/210"/>
	<skos:prefLabel xml:lang="en">MEOW Kerguelen Islands Ecoregion</skos:prefLabel>
	<dcterms:contributor rdf:resource="http://editor.vocabs.ands.org.au/user/eMII_Finney.Kim_Admin"/>
	<dcterms:created rdf:datatype="http://www.w3.org/2001/XMLSchema#dateTime">2017-05-31T02:43:17Z</dcterms:created>
	<dcterms:creator rdf:resource="http://editor.vocabs.ands.org.au/user/eMII_Finney.Kim_Admin"/>
	<dcterms:modified rdf:datatype="http://www.w3.org/2001/XMLSchema#dateTime">2017-06-27T04:11:34Z</dcterms:modified>
	<dc:publisher rdf:datatype="http://www.w3.org/2001/XMLSchema#string">Institute for Marine and Antarctic Studies (IMAS) - UTAS</dc:publisher>
	<skos:definition xml:lang="en">An area of relatively homogenous species composition, clearly distinct from adjacent systems. The species composition is likely to be determined by the predominance of a small number of ecosystems and/or a distinct suite of oceanographic or topographic features. The dominant biogeographic forcing agents defining the ecoregions vary from location to location but may include isolation, upwelling, nutrient inputs, freshwater influx, temperature regimes, ice regimes, exposure, sediments, currents and bathymetric or coastal complexity.</skos:definition>
	<dc:source rdf:datatype="http://www.w3.org/2001/XMLSchema#string">Marine Ecoregions of the World (MEOW). Spalding et.al. (2007)</dc:source>
	<skos:exactMatch rdf:resource="http://www.marineregions.org/gazetteer.php?p=details&amp;id=21956"/>
</rdf:Description>

<rdf:Description rdf:about="http://seamapaustralia.org.au/def/benthichabitatclassification/class/222">
	<rdf:type rdf:resource="http://www.w3.org/2000/01/rdf-schema#Resource"/>
	<rdf:type rdf:resource="http://www.w3.org/2004/02/skos/core#Concept"/>
	<skos:broader rdf:resource="http://seamapaustralia.org.au/def/benthichabitatclassification/class/210"/>
	<skos:prefLabel xml:lang="en">MEOW Crozet Islands Ecoregion</skos:prefLabel>
	<dcterms:contributor rdf:resource="http://editor.vocabs.ands.org.au/user/eMII_Finney.Kim_Admin"/>
	<dcterms:created rdf:datatype="http://www.w3.org/2001/XMLSchema#dateTime">2017-05-31T02:43:53Z</dcterms:created>
	<dcterms:creator rdf:resource="http://editor.vocabs.ands.org.au/user/eMII_Finney.Kim_Admin"/>
	<dcterms:modified rdf:datatype="http://www.w3.org/2001/XMLSchema#dateTime">2017-06-27T04:11:25Z</dcterms:modified>
	<dc:publisher rdf:datatype="http://www.w3.org/2001/XMLSchema#string">Institute for Marine and Antarctic Studies (IMAS) - UTAS</dc:publisher>
	<skos:definition xml:lang="en">An area of relatively homogenous species composition, clearly distinct from adjacent systems. The species composition is likely to be determined by the predominance of a small number of ecosystems and/or a distinct suite of oceanographic or topographic features. The dominant biogeographic forcing agents defining the ecoregions vary from location to location but may include isolation, upwelling, nutrient inputs, freshwater influx, temperature regimes, ice regimes, exposure, sediments, currents and bathymetric or coastal complexity.</skos:definition>
	<dc:source rdf:datatype="http://www.w3.org/2001/XMLSchema#string">Marine Ecoregions of the World (MEOW). Spalding et.al. (2007)</dc:source>
	<skos:exactMatch rdf:resource="http://www.marineregions.org/gazetteer.php?p=details&amp;id=21954"/>
</rdf:Description>

<rdf:Description rdf:about="http://seamapaustralia.org.au/def/benthichabitatclassification/class/223">
	<rdf:type rdf:resource="http://www.w3.org/2000/01/rdf-schema#Resource"/>
	<rdf:type rdf:resource="http://www.w3.org/2004/02/skos/core#Concept"/>
	<skos:broader rdf:resource="http://seamapaustralia.org.au/def/benthichabitatclassification/class/210"/>
	<skos:prefLabel xml:lang="en">MEOW Prince Edwards Islands Ecoregion</skos:prefLabel>
	<dcterms:contributor rdf:resource="http://editor.vocabs.ands.org.au/user/eMII_Finney.Kim_Admin"/>
	<dcterms:created rdf:datatype="http://www.w3.org/2001/XMLSchema#dateTime">2017-05-31T02:44:29Z</dcterms:created>
	<dcterms:creator rdf:resource="http://editor.vocabs.ands.org.au/user/eMII_Finney.Kim_Admin"/>
	<dcterms:modified rdf:datatype="http://www.w3.org/2001/XMLSchema#dateTime">2017-06-27T04:11:47Z</dcterms:modified>
	<dc:publisher rdf:datatype="http://www.w3.org/2001/XMLSchema#string">Institute for Marine and Antarctic Studies (IMAS) - UTAS</dc:publisher>
	<skos:definition xml:lang="en">An area of relatively homogenous species composition, clearly distinct from adjacent systems. The species composition is likely to be determined by the predominance of a small number of ecosystems and/or a distinct suite of oceanographic or topographic features. The dominant biogeographic forcing agents defining the ecoregions vary from location to location but may include isolation, upwelling, nutrient inputs, freshwater influx, temperature regimes, ice regimes, exposure, sediments, currents and bathymetric or coastal complexity.</skos:definition>
	<dc:source rdf:datatype="http://www.w3.org/2001/XMLSchema#string">Marine Ecoregions of the World (MEOW). Spalding et.al. (2007)</dc:source>
	<skos:exactMatch rdf:resource="http://www.marineregions.org/gazetteer.php?p=details&amp;id=21959"/>
</rdf:Description>

<rdf:Description rdf:about="http://seamapaustralia.org.au/def/benthichabitatclassification/class/224">
	<rdf:type rdf:resource="http://www.w3.org/2000/01/rdf-schema#Resource"/>
	<rdf:type rdf:resource="http://www.w3.org/2004/02/skos/core#Concept"/>
	<skos:broader rdf:resource="http://seamapaustralia.org.au/def/benthichabitatclassification/class/210"/>
	<skos:prefLabel xml:lang="en">MEOW Bouvet Island Ecoregion</skos:prefLabel>
	<dcterms:contributor rdf:resource="http://editor.vocabs.ands.org.au/user/eMII_Finney.Kim_Admin"/>
	<dcterms:created rdf:datatype="http://www.w3.org/2001/XMLSchema#dateTime">2017-05-31T02:45:02Z</dcterms:created>
	<dcterms:creator rdf:resource="http://editor.vocabs.ands.org.au/user/eMII_Finney.Kim_Admin"/>
	<dcterms:modified rdf:datatype="http://www.w3.org/2001/XMLSchema#dateTime">2017-06-27T04:11:20Z</dcterms:modified>
	<dc:publisher rdf:datatype="http://www.w3.org/2001/XMLSchema#string">Institute for Marine and Antarctic Studies (IMAS) - UTAS</dc:publisher>
	<skos:definition xml:lang="en">An area of relatively homogenous species composition, clearly distinct from adjacent systems. The species composition is likely to be determined by the predominance of a small number of ecosystems and/or a distinct suite of oceanographic or topographic features. The dominant biogeographic forcing agents defining the ecoregions vary from location to location but may include isolation, upwelling, nutrient inputs, freshwater influx, temperature regimes, ice regimes, exposure, sediments, currents and bathymetric or coastal complexity.</skos:definition>
	<dc:source rdf:datatype="http://www.w3.org/2001/XMLSchema#string">Marine Ecoregions of the World (MEOW). Spalding et.al. (2007)</dc:source>
	<skos:exactMatch rdf:resource="http://www.marineregions.org/gazetteer.php?p=details&amp;id=21953"/>
</rdf:Description>

<rdf:Description rdf:about="http://seamapaustralia.org.au/def/benthichabitatclassification/class/228">
	<rdf:type rdf:resource="http://www.w3.org/2000/01/rdf-schema#Resource"/>
	<rdf:type rdf:resource="http://www.w3.org/2004/02/skos/core#Concept"/>
	<skos:broader rdf:resource="http://seamapaustralia.org.au/def/benthichabitatclassification/class/116"/>
	<skos:prefLabel xml:lang="en">MEOW Cape Howe Ecoregion</skos:prefLabel>
	<dcterms:contributor rdf:resource="http://editor.vocabs.ands.org.au/user/eMII_Finney.Kim_Admin"/>
	<dcterms:created rdf:datatype="http://www.w3.org/2001/XMLSchema#dateTime">2017-05-31T02:48:24Z</dcterms:created>
	<dcterms:creator rdf:resource="http://editor.vocabs.ands.org.au/user/eMII_Finney.Kim_Admin"/>
	<dcterms:modified rdf:datatype="http://www.w3.org/2001/XMLSchema#dateTime">2017-06-27T04:12:56Z</dcterms:modified>
	<dc:publisher rdf:datatype="http://www.w3.org/2001/XMLSchema#string">Institute for Marine and Antarctic Studies (IMAS) - UTAS</dc:publisher>
	<skos:definition xml:lang="en">An area of relatively homogenous species composition, clearly distinct from adjacent systems. The species composition is likely to be determined by the predominance of a small number of ecosystems and/or a distinct suite of oceanographic or topographic features. The dominant biogeographic forcing agents defining the ecoregions vary from location to location but may include isolation, upwelling, nutrient inputs, freshwater influx, temperature regimes, ice regimes, exposure, sediments, currents and bathymetric or coastal complexity.</skos:definition>
	<dc:source rdf:datatype="http://www.w3.org/2001/XMLSchema#string">Marine Ecoregions of the World (MEOW). Spalding et.al. (2007)</dc:source>
	<skos:narrower rdf:resource="http://seamapaustralia.org.au/def/benthichabitatclassification/class/261"/>
	<skos:exactMatch rdf:resource="http://www.marineregions.org/gazetteer.php?p=details&amp;id=21940"/>
</rdf:Description>

<rdf:Description rdf:about="http://www.marineregions.org/gazetteer.php?p=details&amp;id=21723">
	<rdf:type rdf:resource="http://www.w3.org/2000/01/rdf-schema#Resource"/>
</rdf:Description>

<rdf:Description rdf:about="http://www.marineregions.org/gazetteer.php?p=details&amp;id=21724">
	<rdf:type rdf:resource="http://www.w3.org/2000/01/rdf-schema#Resource"/>
</rdf:Description>

<rdf:Description rdf:about="http://www.marineregions.org/gazetteer.php?p=details&amp;id=21729">
	<rdf:type rdf:resource="http://www.w3.org/2000/01/rdf-schema#Resource"/>
</rdf:Description>

<rdf:Description rdf:about="http://www.marineregions.org/gazetteer.php?p=details&amp;id=21730">
	<rdf:type rdf:resource="http://www.w3.org/2000/01/rdf-schema#Resource"/>
</rdf:Description>

<rdf:Description rdf:about="http://www.marineregions.org/gazetteer.php?p=details&amp;id=21735">
	<rdf:type rdf:resource="http://www.w3.org/2000/01/rdf-schema#Resource"/>
</rdf:Description>

<rdf:Description rdf:about="http://www.marineregions.org/gazetteer.php?p=details&amp;id=22021">
	<rdf:type rdf:resource="http://www.w3.org/2000/01/rdf-schema#Resource"/>
</rdf:Description>

<rdf:Description rdf:about="http://www.marineregions.org/gazetteer.php?p=details&amp;id=22020">
	<rdf:type rdf:resource="http://www.w3.org/2000/01/rdf-schema#Resource"/>
</rdf:Description>

<rdf:Description rdf:about="http://www.marineregions.org/gazetteer.php?p=details&amp;id=22025">
	<rdf:type rdf:resource="http://www.w3.org/2000/01/rdf-schema#Resource"/>
</rdf:Description>

<rdf:Description rdf:about="http://www.marineregions.org/gazetteer.php?p=details&amp;id=22026">
	<rdf:type rdf:resource="http://www.w3.org/2000/01/rdf-schema#Resource"/>
</rdf:Description>

<rdf:Description rdf:about="http://www.environment.gov.au/mapping/rest/services/ogc_services/IMCRA_Mesoscale/MapServer/0/29">
	<rdf:type rdf:resource="http://www.w3.org/2000/01/rdf-schema#Resource"/>
</rdf:Description>

<rdf:Description rdf:about="http://www.environment.gov.au/mapping/rest/services/ogc_services/IMCRA_Mesoscale/MapServer/0/4">
	<rdf:type rdf:resource="http://www.w3.org/2000/01/rdf-schema#Resource"/>
</rdf:Description>

<rdf:Description rdf:about="http://www.marineregions.org/gazetteer.php?p=details&amp;id=22024">
	<rdf:type rdf:resource="http://www.w3.org/2000/01/rdf-schema#Resource"/>
</rdf:Description>

<rdf:Description rdf:about="http://www.environment.gov.au/mapping/rest/services/ogc_services/IMCRA_Mesoscale/MapServer/0/25">
	<rdf:type rdf:resource="http://www.w3.org/2000/01/rdf-schema#Resource"/>
</rdf:Description>

<rdf:Description rdf:about="http://www.marineregions.org/gazetteer.php?p=details&amp;id=21861">
	<rdf:type rdf:resource="http://www.w3.org/2000/01/rdf-schema#Resource"/>
</rdf:Description>

<rdf:Description rdf:about="http://www.marineregions.org/gazetteer.php?p=details&amp;id=21862">
	<rdf:type rdf:resource="http://www.w3.org/2000/01/rdf-schema#Resource"/>
</rdf:Description>

<rdf:Description rdf:about="http://www.marineregions.org/gazetteer.php?p=details&amp;id=21857">
	<rdf:type rdf:resource="http://www.w3.org/2000/01/rdf-schema#Resource"/>
</rdf:Description>

<rdf:Description rdf:about="http://www.marineregions.org/gazetteer.php?p=details&amp;id=21858">
	<rdf:type rdf:resource="http://www.w3.org/2000/01/rdf-schema#Resource"/>
</rdf:Description>

<rdf:Description rdf:about="http://www.marineregions.org/gazetteer.php?p=details&amp;id=21859">
	<rdf:type rdf:resource="http://www.w3.org/2000/01/rdf-schema#Resource"/>
</rdf:Description>

<rdf:Description rdf:about="http://www.marineregions.org/gazetteer.php?p=details&amp;id=21860">
	<rdf:type rdf:resource="http://www.w3.org/2000/01/rdf-schema#Resource"/>
</rdf:Description>

<rdf:Description rdf:about="http://www.marineregions.org/gazetteer.php?p=details&amp;id=21953">
	<rdf:type rdf:resource="http://www.w3.org/2000/01/rdf-schema#Resource"/>
</rdf:Description>

<rdf:Description rdf:about="http://www.marineregions.org/gazetteer.php?p=details&amp;id=21954">
	<rdf:type rdf:resource="http://www.w3.org/2000/01/rdf-schema#Resource"/>
</rdf:Description>

<rdf:Description rdf:about="http://www.marineregions.org/gazetteer.php?p=details&amp;id=21955">
	<rdf:type rdf:resource="http://www.w3.org/2000/01/rdf-schema#Resource"/>
</rdf:Description>

<rdf:Description rdf:about="http://www.marineregions.org/gazetteer.php?p=details&amp;id=21956">
	<rdf:type rdf:resource="http://www.w3.org/2000/01/rdf-schema#Resource"/>
</rdf:Description>

<rdf:Description rdf:about="http://www.marineregions.org/gazetteer.php?p=details&amp;id=21957">
	<rdf:type rdf:resource="http://www.w3.org/2000/01/rdf-schema#Resource"/>
</rdf:Description>

<rdf:Description rdf:about="http://www.marineregions.org/gazetteer.php?p=details&amp;id=21959">
	<rdf:type rdf:resource="http://www.w3.org/2000/01/rdf-schema#Resource"/>
</rdf:Description>

<rdf:Description rdf:about="http://www.marineregions.org/gazetteer.php?p=details&amp;id=21864">
	<rdf:type rdf:resource="http://www.w3.org/2000/01/rdf-schema#Resource"/>
</rdf:Description>

<rdf:Description rdf:about="http://www.marineregions.org/gazetteer.php?p=details&amp;id=21863">
	<rdf:type rdf:resource="http://www.w3.org/2000/01/rdf-schema#Resource"/>
</rdf:Description>

<rdf:Description rdf:about="http://www.marineregions.org/gazetteer.php?p=details&amp;id=21938">
	<rdf:type rdf:resource="http://www.w3.org/2000/01/rdf-schema#Resource"/>
</rdf:Description>

<rdf:Description rdf:about="http://www.marineregions.org/gazetteer.php?p=details&amp;id=21940">
	<rdf:type rdf:resource="http://www.w3.org/2000/01/rdf-schema#Resource"/>
</rdf:Description>

<rdf:Description rdf:about="http://www.marineregions.org/gazetteer.php?p=details&amp;id=21939">
	<rdf:type rdf:resource="http://www.w3.org/2000/01/rdf-schema#Resource"/>
</rdf:Description>

<rdf:Description rdf:about="http://www.marineregions.org/gazetteer.php?p=details&amp;id=21949">
	<rdf:type rdf:resource="http://www.w3.org/2000/01/rdf-schema#Resource"/>
</rdf:Description>

<rdf:Description rdf:about="http://www.marineregions.org/gazetteer.php?p=details&amp;id=21950">
	<rdf:type rdf:resource="http://www.w3.org/2000/01/rdf-schema#Resource"/>
</rdf:Description>

<rdf:Description rdf:about="http://www.marineregions.org/gazetteer.php?p=details&amp;id=21951">
	<rdf:type rdf:resource="http://www.w3.org/2000/01/rdf-schema#Resource"/>
</rdf:Description>

<rdf:Description rdf:about="http://www.environment.gov.au/mapping/rest/services/ogc_services/IMCRA_Mesoscale/MapServer/0/23">
	<rdf:type rdf:resource="http://www.w3.org/2000/01/rdf-schema#Resource"/>
</rdf:Description>

<rdf:Description rdf:about="http://www.environment.gov.au/mapping/rest/services/ogc_services/IMCRA_Mesoscale/MapServer/0/5">
	<rdf:type rdf:resource="http://www.w3.org/2000/01/rdf-schema#Resource"/>
</rdf:Description>

<rdf:Description rdf:about="https://www.cmecscatalog.org/cmecs/classification/unit/549.html">
	<rdf:type rdf:resource="http://www.w3.org/2000/01/rdf-schema#Resource"/>
</rdf:Description>

<rdf:Description rdf:about="https://www.cmecscatalog.org/cmecs/classification/unit/548.html">
	<rdf:type rdf:resource="http://www.w3.org/2000/01/rdf-schema#Resource"/>
</rdf:Description>

<rdf:Description rdf:about="https://www.cmecscatalog.org/cmecs/classification/unit/547.html">
	<rdf:type rdf:resource="http://www.w3.org/2000/01/rdf-schema#Resource"/>
</rdf:Description>

<rdf:Description rdf:about="https://www.cmecscatalog.org/cmecs/classification/unit/577.html">
	<rdf:type rdf:resource="http://www.w3.org/2000/01/rdf-schema#Resource"/>
</rdf:Description>

<rdf:Description rdf:about="https://www.cmecscatalog.org/cmecs/classification/unit/570.html">
	<rdf:type rdf:resource="http://www.w3.org/2000/01/rdf-schema#Resource"/>
</rdf:Description>

<rdf:Description rdf:about="https://www.cmecscatalog.org/cmecs/classification/unit/581.html">
	<rdf:type rdf:resource="http://www.w3.org/2000/01/rdf-schema#Resource"/>
</rdf:Description>

<rdf:Description rdf:about="https://www.cmecscatalog.org/cmecs/classification/unit/571.html">
	<rdf:type rdf:resource="http://www.w3.org/2000/01/rdf-schema#Resource"/>
</rdf:Description>

<rdf:Description rdf:about="https://www.cmecscatalog.org/cmecs/classification/unit/433.html">
	<rdf:type rdf:resource="http://www.w3.org/2000/01/rdf-schema#Resource"/>
</rdf:Description>

<rdf:Description rdf:about="https://www.cmecscatalog.org/cmecs/classification/unit/567.html">
	<rdf:type rdf:resource="http://www.w3.org/2000/01/rdf-schema#Resource"/>
</rdf:Description>

<rdf:Description rdf:about="http://www.w3.org/2004/02/skos/core#relatedMatch">
	<rdf:type rdf:resource="http://www.w3.org/1999/02/22-rdf-syntax-ns#Property"/>
	<rdf:type rdf:resource="http://www.w3.org/2000/01/rdf-schema#Resource"/>
	<rdfs:subPropertyOf rdf:resource="http://www.w3.org/2004/02/skos/core#relatedMatch"/>
</rdf:Description>

<rdf:Description rdf:about="https://www.cmecscatalog.org/cmecs/classification/unit/186.html">
	<rdf:type rdf:resource="http://www.w3.org/2000/01/rdf-schema#Resource"/>
</rdf:Description>

<rdf:Description rdf:about="https://www.cmecscatalog.org/cmecs/classification/unit/523.html">
	<rdf:type rdf:resource="http://www.w3.org/2000/01/rdf-schema#Resource"/>
</rdf:Description>

<rdf:Description rdf:about="https://www.cmecscatalog.org/cmecs/classification/unit/876.html">
	<rdf:type rdf:resource="http://www.w3.org/2000/01/rdf-schema#Resource"/>
</rdf:Description>

<rdf:Description rdf:about="https://www.cmecscatalog.org/cmecs/classification/unit/504.html">
	<rdf:type rdf:resource="http://www.w3.org/2000/01/rdf-schema#Resource"/>
</rdf:Description>

<rdf:Description rdf:about="https://www.cmecscatalog.org/cmecs/classification/unit/515.html">
	<rdf:type rdf:resource="http://www.w3.org/2000/01/rdf-schema#Resource"/>
</rdf:Description>

<rdf:Description rdf:about="https://www.cmecscatalog.org/cmecs/classification/unit/532.html">
	<rdf:type rdf:resource="http://www.w3.org/2000/01/rdf-schema#Resource"/>
</rdf:Description>

<rdf:Description rdf:about="https://www.cmecscatalog.org/cmecs/classification/unit/516.html">
	<rdf:type rdf:resource="http://www.w3.org/2000/01/rdf-schema#Resource"/>
</rdf:Description>

<rdf:Description rdf:about="https://www.cmecscatalog.org/cmecs/classification/unit/534.html">
	<rdf:type rdf:resource="http://www.w3.org/2000/01/rdf-schema#Resource"/>
</rdf:Description>

<rdf:Description rdf:about="http://seamapaustralia.org.au/def/benthichabitatclassification/class/235">
	<rdf:type rdf:resource="http://www.w3.org/2000/01/rdf-schema#Resource"/>
	<rdf:type rdf:resource="http://www.w3.org/2004/02/skos/core#Concept"/>
	<skos:broader rdf:resource="http://seamapaustralia.org.au/def/benthichabitatclassification/class/12"/>
	<skos:prefLabel xml:lang="en">Slab</skos:prefLabel>
	<dcterms:contributor rdf:resource="http://editor.vocabs.ands.org.au/user/eMII_Finney.Kim_Admin"/>
	<dcterms:created rdf:datatype="http://www.w3.org/2001/XMLSchema#dateTime">2017-06-05T23:25:31Z</dcterms:created>
	<dcterms:creator rdf:resource="http://editor.vocabs.ands.org.au/user/eMII_Finney.Kim_Admin"/>
	<dcterms:modified rdf:datatype="http://www.w3.org/2001/XMLSchema#dateTime">2017-06-27T04:19:18Z</dcterms:modified>
	<dc:publisher rdf:datatype="http://www.w3.org/2001/XMLSchema#string">Institute for Marine and Antarctic Studies (IMAS) - UTAS</dc:publisher>
	<skos:definition xml:lang="en">A megaclast-dominated substratum where ≥ 80 % of the megaclasts are between 65.5 – 1049 m in any dimension.</skos:definition>
	<dc:source rdf:datatype="http://www.w3.org/2001/XMLSchema#string">SeaMap Australia National Benthic Habitat Classification Scheme (2017)</dc:source>
</rdf:Description>

<rdf:Description rdf:about="http://seamapaustralia.org.au/def/benthichabitatclassification/class/236">
	<rdf:type rdf:resource="http://www.w3.org/2000/01/rdf-schema#Resource"/>
	<rdf:type rdf:resource="http://www.w3.org/2004/02/skos/core#Concept"/>
	<skos:broader rdf:resource="http://seamapaustralia.org.au/def/benthichabitatclassification/class/12"/>
	<skos:prefLabel xml:lang="en">Block</skos:prefLabel>
	<dcterms:contributor rdf:resource="http://editor.vocabs.ands.org.au/user/eMII_Finney.Kim_Admin"/>
	<dcterms:created rdf:datatype="http://www.w3.org/2001/XMLSchema#dateTime">2017-06-05T23:25:45Z</dcterms:created>
	<dcterms:creator rdf:resource="http://editor.vocabs.ands.org.au/user/eMII_Finney.Kim_Admin"/>
	<dcterms:modified rdf:datatype="http://www.w3.org/2001/XMLSchema#dateTime">2017-06-27T04:19:14Z</dcterms:modified>
	<dc:publisher rdf:datatype="http://www.w3.org/2001/XMLSchema#string">Institute for Marine and Antarctic Studies (IMAS) - UTAS</dc:publisher>
	<skos:definition xml:lang="en">A megaclast-dominated substratum where ≥ 80 % of the clasts are between 4.1 – 65.5 m in any dimension.</skos:definition>
	<dc:source rdf:datatype="http://www.w3.org/2001/XMLSchema#string">SeaMap Australia National Benthic Habitat Classification Scheme (2017)</dc:source>
</rdf:Description>

<rdf:Description rdf:about="http://seamapaustralia.org.au/def/benthichabitatclassification/class/237">
	<rdf:type rdf:resource="http://www.w3.org/2000/01/rdf-schema#Resource"/>
	<rdf:type rdf:resource="http://www.w3.org/2004/02/skos/core#Concept"/>
	<skos:broader rdf:resource="http://seamapaustralia.org.au/def/benthichabitatclassification/class/13"/>
	<skos:prefLabel xml:lang="en">Very Coarse Boulder</skos:prefLabel>
	<dcterms:contributor rdf:resource="http://editor.vocabs.ands.org.au/user/eMII_Finney.Kim_Admin"/>
	<dcterms:created rdf:datatype="http://www.w3.org/2001/XMLSchema#dateTime">2017-06-05T23:26:11Z</dcterms:created>
	<dcterms:creator rdf:resource="http://editor.vocabs.ands.org.au/user/eMII_Finney.Kim_Admin"/>
	<dcterms:modified rdf:datatype="http://www.w3.org/2001/XMLSchema#dateTime">2017-06-27T04:19:04Z</dcterms:modified>
	<dc:publisher rdf:datatype="http://www.w3.org/2001/XMLSchema#string">Institute for Marine and Antarctic Studies (IMAS) - UTAS</dc:publisher>
	<skos:definition xml:lang="en">A boulder-dominated substratum where ≥ 80 % of the boulders are between 2048-4096 mm in any dimension.</skos:definition>
	<dc:source rdf:datatype="http://www.w3.org/2001/XMLSchema#string">SeaMap Australia National Benthic Habitat Classification Scheme (2017)</dc:source>
</rdf:Description>

<rdf:Description rdf:about="http://seamapaustralia.org.au/def/benthichabitatclassification/class/238">
	<rdf:type rdf:resource="http://www.w3.org/2000/01/rdf-schema#Resource"/>
	<rdf:type rdf:resource="http://www.w3.org/2004/02/skos/core#Concept"/>
	<skos:broader rdf:resource="http://seamapaustralia.org.au/def/benthichabitatclassification/class/13"/>
	<skos:prefLabel xml:lang="en">Coarse Boulder</skos:prefLabel>
	<dcterms:contributor rdf:resource="http://editor.vocabs.ands.org.au/user/eMII_Finney.Kim_Admin"/>
	<dcterms:created rdf:datatype="http://www.w3.org/2001/XMLSchema#dateTime">2017-06-05T23:26:25Z</dcterms:created>
	<dcterms:creator rdf:resource="http://editor.vocabs.ands.org.au/user/eMII_Finney.Kim_Admin"/>
	<dcterms:modified rdf:datatype="http://www.w3.org/2001/XMLSchema#dateTime">2017-06-27T04:18:50Z</dcterms:modified>
	<dc:publisher rdf:datatype="http://www.w3.org/2001/XMLSchema#string">Institute for Marine and Antarctic Studies (IMAS) - UTAS</dc:publisher>
	<skos:definition xml:lang="en">A boulder-dominated substratum where ≥ 80 % of the boulders are between 1024-2048 mm in any dimension.</skos:definition>
	<dc:source rdf:datatype="http://www.w3.org/2001/XMLSchema#string">SeaMap Australia National Benthic Habitat Classification Scheme (2017)</dc:source>
</rdf:Description>

<rdf:Description rdf:about="http://seamapaustralia.org.au/def/benthichabitatclassification/class/239">
	<rdf:type rdf:resource="http://www.w3.org/2000/01/rdf-schema#Resource"/>
	<rdf:type rdf:resource="http://www.w3.org/2004/02/skos/core#Concept"/>
	<skos:broader rdf:resource="http://seamapaustralia.org.au/def/benthichabitatclassification/class/13"/>
	<skos:prefLabel xml:lang="en">Medium Boulder</skos:prefLabel>
	<dcterms:contributor rdf:resource="http://editor.vocabs.ands.org.au/user/eMII_Finney.Kim_Admin"/>
	<dcterms:created rdf:datatype="http://www.w3.org/2001/XMLSchema#dateTime">2017-06-05T23:26:40Z</dcterms:created>
	<dcterms:creator rdf:resource="http://editor.vocabs.ands.org.au/user/eMII_Finney.Kim_Admin"/>
	<dcterms:modified rdf:datatype="http://www.w3.org/2001/XMLSchema#dateTime">2017-06-27T04:19:00Z</dcterms:modified>
	<dc:publisher rdf:datatype="http://www.w3.org/2001/XMLSchema#string">Institute for Marine and Antarctic Studies (IMAS) - UTAS</dc:publisher>
	<skos:definition xml:lang="en">A boulder-dominated substratum where ≥ 80 % of the boulders are between 512-1024 mm in any dimension.</skos:definition>
	<dc:source rdf:datatype="http://www.w3.org/2001/XMLSchema#string">SeaMap Australia National Benthic Habitat Classification Scheme (2017)</dc:source>
</rdf:Description>

<rdf:Description rdf:about="http://seamapaustralia.org.au/def/benthichabitatclassification/class/240">
	<rdf:type rdf:resource="http://www.w3.org/2000/01/rdf-schema#Resource"/>
	<rdf:type rdf:resource="http://www.w3.org/2004/02/skos/core#Concept"/>
	<skos:broader rdf:resource="http://seamapaustralia.org.au/def/benthichabitatclassification/class/13"/>
	<skos:prefLabel xml:lang="en">Fine Boulder</skos:prefLabel>
	<dcterms:contributor rdf:resource="http://editor.vocabs.ands.org.au/user/eMII_Finney.Kim_Admin"/>
	<dcterms:created rdf:datatype="http://www.w3.org/2001/XMLSchema#dateTime">2017-06-05T23:26:59Z</dcterms:created>
	<dcterms:creator rdf:resource="http://editor.vocabs.ands.org.au/user/eMII_Finney.Kim_Admin"/>
	<dcterms:modified rdf:datatype="http://www.w3.org/2001/XMLSchema#dateTime">2017-06-27T04:18:55Z</dcterms:modified>
	<dc:publisher rdf:datatype="http://www.w3.org/2001/XMLSchema#string">Institute for Marine and Antarctic Studies (IMAS) - UTAS</dc:publisher>
	<skos:definition xml:lang="en">A boulder-dominated substratum where ≥ 80 % of the boulders are between 256-512 mm in any dimension.</skos:definition>
	<dc:source rdf:datatype="http://www.w3.org/2001/XMLSchema#string">SeaMap Australia National Benthic Habitat Classification Scheme (2017)</dc:source>
</rdf:Description>

<rdf:Description rdf:about="http://seamapaustralia.org.au/def/benthichabitatclassification/class/241">
	<rdf:type rdf:resource="http://www.w3.org/2000/01/rdf-schema#Resource"/>
	<rdf:type rdf:resource="http://www.w3.org/2004/02/skos/core#Concept"/>
	<skos:broader rdf:resource="http://seamapaustralia.org.au/def/benthichabitatclassification/class/15"/>
	<skos:prefLabel xml:lang="en">Coarse Cobble</skos:prefLabel>
	<dcterms:contributor rdf:resource="http://editor.vocabs.ands.org.au/user/eMII_Finney.Kim_Admin"/>
	<dcterms:created rdf:datatype="http://www.w3.org/2001/XMLSchema#dateTime">2017-06-05T23:34:59Z</dcterms:created>
	<dcterms:creator rdf:resource="http://editor.vocabs.ands.org.au/user/eMII_Finney.Kim_Admin"/>
	<dcterms:modified rdf:datatype="http://www.w3.org/2001/XMLSchema#dateTime">2017-06-27T04:19:55Z</dcterms:modified>
	<dc:publisher rdf:datatype="http://www.w3.org/2001/XMLSchema#string">Institute for Marine and Antarctic Studies (IMAS) - UTAS</dc:publisher>
	<skos:definition xml:lang="en">A cobble-dominated substratum where ≥ 80 % of the cobbles are between 128-256 mm in any dimension.</skos:definition>
	<dc:source rdf:datatype="http://www.w3.org/2001/XMLSchema#string">SeaMap Australia National Benthic Habitat Classification Scheme (2017)</dc:source>
</rdf:Description>

<rdf:Description rdf:about="http://seamapaustralia.org.au/def/benthichabitatclassification/class/242">
	<rdf:type rdf:resource="http://www.w3.org/2000/01/rdf-schema#Resource"/>
	<rdf:type rdf:resource="http://www.w3.org/2004/02/skos/core#Concept"/>
	<skos:broader rdf:resource="http://seamapaustralia.org.au/def/benthichabitatclassification/class/15"/>
	<skos:prefLabel xml:lang="en">Fine Cobble</skos:prefLabel>
	<dcterms:contributor rdf:resource="http://editor.vocabs.ands.org.au/user/eMII_Finney.Kim_Admin"/>
	<dcterms:created rdf:datatype="http://www.w3.org/2001/XMLSchema#dateTime">2017-06-05T23:35:09Z</dcterms:created>
	<dcterms:creator rdf:resource="http://editor.vocabs.ands.org.au/user/eMII_Finney.Kim_Admin"/>
	<dcterms:modified rdf:datatype="http://www.w3.org/2001/XMLSchema#dateTime">2017-06-27T04:20:01Z</dcterms:modified>
	<dc:publisher rdf:datatype="http://www.w3.org/2001/XMLSchema#string">Institute for Marine and Antarctic Studies (IMAS) - UTAS</dc:publisher>
	<skos:definition xml:lang="en">A cobble-dominated substratum where ≥ 80 % of the cobbles are between 64-128 mm in any dimension.</skos:definition>
	<dc:source rdf:datatype="http://www.w3.org/2001/XMLSchema#string">SeaMap Australia National Benthic Habitat Classification Scheme (2017)</dc:source>
</rdf:Description>

<rdf:Description rdf:about="http://seamapaustralia.org.au/def/benthichabitatclassification/class/243">
	<rdf:type rdf:resource="http://www.w3.org/2000/01/rdf-schema#Resource"/>
	<rdf:type rdf:resource="http://www.w3.org/2004/02/skos/core#Concept"/>
	<skos:broader rdf:resource="http://seamapaustralia.org.au/def/benthichabitatclassification/class/19"/>
	<skos:prefLabel xml:lang="en">Very Coarse Pebble</skos:prefLabel>
	<dcterms:contributor rdf:resource="http://editor.vocabs.ands.org.au/user/eMII_Finney.Kim_Admin"/>
	<dcterms:created rdf:datatype="http://www.w3.org/2001/XMLSchema#dateTime">2017-06-05T23:46:40Z</dcterms:created>
	<dcterms:creator rdf:resource="http://editor.vocabs.ands.org.au/user/eMII_Finney.Kim_Admin"/>
	<dcterms:modified rdf:datatype="http://www.w3.org/2001/XMLSchema#dateTime">2017-06-27T04:21:07Z</dcterms:modified>
	<dc:publisher rdf:datatype="http://www.w3.org/2001/XMLSchema#string">  Institute for Marine and Antarctic Studies (IMAS) - UTAS</dc:publisher>
	<skos:definition xml:lang="en">A pebble-dominated substratum where ≥ 80 % of the pebbles are between 32-64 mm in any dimension.</skos:definition>
	<dc:source rdf:datatype="http://www.w3.org/2001/XMLSchema#string">SeaMap Australia National Benthic Habitat Classification Scheme (2017)</dc:source>
</rdf:Description>

<rdf:Description rdf:about="http://seamapaustralia.org.au/def/benthichabitatclassification/class/244">
	<rdf:type rdf:resource="http://www.w3.org/2000/01/rdf-schema#Resource"/>
	<rdf:type rdf:resource="http://www.w3.org/2004/02/skos/core#Concept"/>
	<skos:broader rdf:resource="http://seamapaustralia.org.au/def/benthichabitatclassification/class/19"/>
	<skos:prefLabel xml:lang="en">Coarse Pebble</skos:prefLabel>
	<dcterms:contributor rdf:resource="http://editor.vocabs.ands.org.au/user/eMII_Finney.Kim_Admin"/>
	<dcterms:created rdf:datatype="http://www.w3.org/2001/XMLSchema#dateTime">2017-06-05T23:46:55Z</dcterms:created>
	<dcterms:creator rdf:resource="http://editor.vocabs.ands.org.au/user/eMII_Finney.Kim_Admin"/>
	<dcterms:modified rdf:datatype="http://www.w3.org/2001/XMLSchema#dateTime">2017-06-27T04:20:52Z</dcterms:modified>
	<dc:publisher rdf:datatype="http://www.w3.org/2001/XMLSchema#string">  Institute for Marine and Antarctic Studies (IMAS) - UTAS</dc:publisher>
	<skos:definition xml:lang="en">A pebble-dominated substratum where ≥ 80 % of the pebbles are between 16-32 mm in any dimension.</skos:definition>
	<dc:source rdf:datatype="http://www.w3.org/2001/XMLSchema#string">SeaMap Australia National Benthic Habitat Classification Scheme (2017)</dc:source>
</rdf:Description>

<rdf:Description rdf:about="http://seamapaustralia.org.au/def/benthichabitatclassification/class/245">
	<rdf:type rdf:resource="http://www.w3.org/2000/01/rdf-schema#Resource"/>
	<rdf:type rdf:resource="http://www.w3.org/2004/02/skos/core#Concept"/>
	<skos:broader rdf:resource="http://seamapaustralia.org.au/def/benthichabitatclassification/class/19"/>
	<skos:prefLabel xml:lang="en">Medium Pebble</skos:prefLabel>
	<dcterms:contributor rdf:resource="http://editor.vocabs.ands.org.au/user/eMII_Finney.Kim_Admin"/>
	<dcterms:created rdf:datatype="http://www.w3.org/2001/XMLSchema#dateTime">2017-06-05T23:47:09Z</dcterms:created>
	<dcterms:creator rdf:resource="http://editor.vocabs.ands.org.au/user/eMII_Finney.Kim_Admin"/>
	<dcterms:modified rdf:datatype="http://www.w3.org/2001/XMLSchema#dateTime">2017-06-27T04:21:02Z</dcterms:modified>
	<dc:publisher rdf:datatype="http://www.w3.org/2001/XMLSchema#string">  Institute for Marine and Antarctic Studies (IMAS) - UTAS</dc:publisher>
	<skos:definition xml:lang="en">A pebble-dominated substratum where ≥ 80 % of the pebbles are between 8-16 mm in any dimension.</skos:definition>
	<dc:source rdf:datatype="http://www.w3.org/2001/XMLSchema#string">SeaMap Australia National Benthic Habitat Classification Scheme (2017)</dc:source>
</rdf:Description>

<rdf:Description rdf:about="http://seamapaustralia.org.au/def/benthichabitatclassification/class/246">
	<rdf:type rdf:resource="http://www.w3.org/2000/01/rdf-schema#Resource"/>
	<rdf:type rdf:resource="http://www.w3.org/2004/02/skos/core#Concept"/>
	<skos:broader rdf:resource="http://seamapaustralia.org.au/def/benthichabitatclassification/class/19"/>
	<skos:prefLabel xml:lang="en">Fine Pebble</skos:prefLabel>
	<dcterms:contributor rdf:resource="http://editor.vocabs.ands.org.au/user/eMII_Finney.Kim_Admin"/>
	<dcterms:created rdf:datatype="http://www.w3.org/2001/XMLSchema#dateTime">2017-06-05T23:47:24Z</dcterms:created>
	<dcterms:creator rdf:resource="http://editor.vocabs.ands.org.au/user/eMII_Finney.Kim_Admin"/>
	<dcterms:modified rdf:datatype="http://www.w3.org/2001/XMLSchema#dateTime">2017-06-27T04:20:58Z</dcterms:modified>
	<dc:publisher rdf:datatype="http://www.w3.org/2001/XMLSchema#string">  Institute for Marine and Antarctic Studies (IMAS) - UTAS</dc:publisher>
	<skos:definition xml:lang="en">A pebble-dominated substratum where ≥ 80 % of the pebbles are between 4-8 mm in any dimension.</skos:definition>
	<dc:source rdf:datatype="http://www.w3.org/2001/XMLSchema#string">SeaMap Australia National Benthic Habitat Classification Scheme (2017)</dc:source>
</rdf:Description>

<rdf:Description rdf:about="https://www.cmecscatalog.org/cmecs/classification/unit/259.html">
	<rdf:type rdf:resource="http://www.w3.org/2000/01/rdf-schema#Resource"/>
</rdf:Description>

<rdf:Description rdf:about="http://seamapaustralia.org.au/def/benthichabitatclassification/class/250">
	<rdf:type rdf:resource="http://www.w3.org/2000/01/rdf-schema#Resource"/>
	<rdf:type rdf:resource="http://www.w3.org/2004/02/skos/core#Concept"/>
	<skos:broader rdf:resource="http://seamapaustralia.org.au/def/benthichabitatclassification/class/229"/>
	<skos:prefLabel xml:lang="en">IMCRA Bass Strait Province</skos:prefLabel>
	<dcterms:contributor rdf:resource="http://editor.vocabs.ands.org.au/user/eMII_Finney.Kim_Admin"/>
	<dcterms:created rdf:datatype="http://www.w3.org/2001/XMLSchema#dateTime">2017-06-13T04:21:42Z</dcterms:created>
	<dcterms:creator rdf:resource="http://editor.vocabs.ands.org.au/user/eMII_Finney.Kim_Admin"/>
	<dcterms:modified rdf:datatype="http://www.w3.org/2001/XMLSchema#dateTime">2017-06-13T23:12:12Z</dcterms:modified>
	<dc:publisher rdf:datatype="http://www.w3.org/2001/XMLSchema#string">Institute for Marine and Antarctic Studies (IMAS) - UTAS</dc:publisher>
	<skos:definition xml:lang="en">An IMCRA provincial bioregion reflects biogeographic patterns in distributions of bottom-dwelling fish. Provincial bioregions were defined for the continental shelf for IMCRA v3.3, and for the continental slope for the National Marine Bioregionalisation using similar analytical techniques. In both cases the distributions of demersal (bottom-dwelling) fish were plotted onto a line divided into equally spaced sections. The number of species in each section and the similarity between sections were calculated using a statistical tool called the Jaccard Index. Where the Jaccard Index changed greatly between sections a boundary was defined indicating differences in species assemblages between regions. Two types of provincial bioregions are defined in the IMCRA benthic bioregionalisation: provinces, which represent regions of biotic endemism; and transitions, which generally occur between the provinces, and are less well-defined mixing areas that capture the overlap of demersal fish species ranges between the provinces.</skos:definition>
	<dc:source rdf:datatype="http://www.w3.org/2001/XMLSchema#string">Commonwealth of Australia (2006). A Guide to the Integrated Marine and Coastal Regionalisation of Australia Version 4.0. Department of the Environment and Heritage, Canberra, Australia.</dc:source>
	<skos:narrower rdf:resource="http://seamapaustralia.org.au/def/benthichabitatclassification/class/252"/>
	<skos:narrower rdf:resource="http://seamapaustralia.org.au/def/benthichabitatclassification/class/253"/>
	<skos:narrower rdf:resource="http://seamapaustralia.org.au/def/benthichabitatclassification/class/254"/>
	<skos:narrower rdf:resource="http://seamapaustralia.org.au/def/benthichabitatclassification/class/255"/>
	<skos:exactMatch rdf:resource="http://www.environment.gov.au/mapping/rest/services/ogc_services/IMCRA_Provincial/MapServer/0/38"/>
</rdf:Description>

<rdf:Description rdf:about="http://seamapaustralia.org.au/def/benthichabitatclassification/class/277">
	<rdf:type rdf:resource="http://www.w3.org/2000/01/rdf-schema#Resource"/>
	<rdf:type rdf:resource="http://www.w3.org/2004/02/skos/core#Concept"/>
	<skos:broader rdf:resource="http://seamapaustralia.org.au/def/benthichabitatclassification/class/273"/>
	<skos:prefLabel xml:lang="en">IMCRA St Vincent Gulf Bioregion</skos:prefLabel>
	<dcterms:contributor rdf:resource="http://editor.vocabs.ands.org.au/user/eMII_Finney.Kim_Admin"/>
	<dcterms:created rdf:datatype="http://www.w3.org/2001/XMLSchema#dateTime">2017-06-13T22:05:31Z</dcterms:created>
	<dcterms:creator rdf:resource="http://editor.vocabs.ands.org.au/user/eMII_Finney.Kim_Admin"/>
	<dcterms:modified rdf:datatype="http://www.w3.org/2001/XMLSchema#dateTime">2017-06-13T23:09:27Z</dcterms:modified>
	<dc:publisher rdf:datatype="http://www.w3.org/2001/XMLSchema#string">Institute for Marine and Antarctic Studies (IMAS) - UTAS</dc:publisher>
	<skos:definition xml:lang="en">An inshore regionalisation of Australian waters derived from biological and physical data, including the distribution of demersal fishes, marine plants and invertebrates, sea floor geomorphology and sediments, and oceanographic data. The meso-scale regionalisation was compiled from information supplied to the Australian Government Department of the Environment and Heritage by the relevant State, Northern Territory and Commonwealth marine research and management agencies. The seaward extent for the meso-scale IMCRA coverage is defined by the 200m isobath except where this boundary extends beyond the Australian Exclusive Economic Zone (AEEZ).</skos:definition>
	<dc:source rdf:datatype="http://www.w3.org/2001/XMLSchema#string">Commonwealth of Australia (2006). A Guide to the Integrated Marine and Coastal Regionalisation of Australia Version 4.0. Department of the Environment and Heritage, Canberra, Australia.</dc:source>
	<skos:exactMatch rdf:resource="http://www.environment.gov.au/mapping/rest/services/ogc_services/IMCRA_Mesoscale/MapServer/0/47"/>
</rdf:Description>

<rdf:Description rdf:about="http://seamapaustralia.org.au/def/benthichabitatclassification/class/251">
	<rdf:type rdf:resource="http://www.w3.org/2000/01/rdf-schema#Resource"/>
	<rdf:type rdf:resource="http://www.w3.org/2004/02/skos/core#Concept"/>
	<skos:broader rdf:resource="http://seamapaustralia.org.au/def/benthichabitatclassification/class/229"/>
	<skos:prefLabel xml:lang="en">IMCRA Tasmanian Province</skos:prefLabel>
	<dcterms:contributor rdf:resource="http://editor.vocabs.ands.org.au/user/eMII_Finney.Kim_Admin"/>
	<dcterms:created rdf:datatype="http://www.w3.org/2001/XMLSchema#dateTime">2017-06-13T04:34:13Z</dcterms:created>
	<dcterms:creator rdf:resource="http://editor.vocabs.ands.org.au/user/eMII_Finney.Kim_Admin"/>
	<dcterms:modified rdf:datatype="http://www.w3.org/2001/XMLSchema#dateTime">2017-06-13T23:12:54Z</dcterms:modified>
	<dc:publisher rdf:datatype="http://www.w3.org/2001/XMLSchema#string">Institute for Marine and Antarctic Studies (IMAS) - UTAS</dc:publisher>
	<skos:definition xml:lang="en">An IMCRA provincial bioregion reflects biogeographic patterns in distributions of bottom-dwelling fish. Provincial bioregions were defined for the continental shelf for IMCRA v3.3, and for the continental slope for the National Marine Bioregionalisation using similar analytical techniques. In both cases the distributions of demersal (bottom-dwelling) fish were plotted onto a line divided into equally spaced sections. The number of species in each section and the similarity between sections were calculated using a statistical tool called the Jaccard Index. Where the Jaccard Index changed greatly between sections a boundary was defined indicating differences in species assemblages between regions. Two types of provincial bioregions are defined in the IMCRA benthic bioregionalisation: provinces, which represent regions of biotic endemism; and transitions, which generally occur between the provinces, and are less well-defined mixing areas that capture the overlap of demersal fish species ranges between the provinces.</skos:definition>
	<dc:source rdf:datatype="http://www.w3.org/2001/XMLSchema#string">Commonwealth of Australia (2006). A Guide to the Integrated Marine and Coastal Regionalisation of Australia Version 4.0. Department of the Environment and Heritage, Canberra, Australia.</dc:source>
	<skos:narrower rdf:resource="http://seamapaustralia.org.au/def/benthichabitatclassification/class/257"/>
	<skos:narrower rdf:resource="http://seamapaustralia.org.au/def/benthichabitatclassification/class/256"/>
	<skos:narrower rdf:resource="http://seamapaustralia.org.au/def/benthichabitatclassification/class/258"/>
	<skos:narrower rdf:resource="http://seamapaustralia.org.au/def/benthichabitatclassification/class/259"/>
	<skos:exactMatch rdf:resource="http://www.environment.gov.au/mapping/rest/services/ogc_services/IMCRA_Provincial/MapServer/0/39"/>
</rdf:Description>

<rdf:Description rdf:about="http://seamapaustralia.org.au/def/benthichabitatclassification/class/252">
	<rdf:type rdf:resource="http://www.w3.org/2000/01/rdf-schema#Resource"/>
	<rdf:type rdf:resource="http://www.w3.org/2004/02/skos/core#Concept"/>
	<skos:broader rdf:resource="http://seamapaustralia.org.au/def/benthichabitatclassification/class/250"/>
	<skos:prefLabel xml:lang="en">IMCRA Victorian Embayments Bioregion</skos:prefLabel>
	<dcterms:contributor rdf:resource="http://editor.vocabs.ands.org.au/user/eMII_Finney.Kim_Admin"/>
	<dcterms:created rdf:datatype="http://www.w3.org/2001/XMLSchema#dateTime">2017-06-13T04:36:50Z</dcterms:created>
	<dcterms:creator rdf:resource="http://editor.vocabs.ands.org.au/user/eMII_Finney.Kim_Admin"/>
	<dcterms:modified rdf:datatype="http://www.w3.org/2001/XMLSchema#dateTime">2017-06-13T23:20:33Z</dcterms:modified>
	<dc:publisher rdf:datatype="http://www.w3.org/2001/XMLSchema#string">Institute for Marine and Antarctic Studies (IMAS) - UTAS</dc:publisher>
	<skos:definition xml:lang="en">An inshore regionalisation of Australian waters derived from biological and physical data, including the distribution of demersal fishes, marine plants and invertebrates, sea floor geomorphology and sediments, and oceanographic data. The meso-scale regionalisation was compiled from information supplied to the Australian Government Department of the Environment and Heritage by the relevant State, Northern Territory and Commonwealth marine research and management agencies. The seaward extent for the meso-scale IMCRA coverage is defined by the 200m isobath except where this boundary extends beyond the Australian Exclusive Economic Zone (AEEZ).</skos:definition>
	<dc:source rdf:datatype="http://www.w3.org/2001/XMLSchema#string">Commonwealth of Australia (2006). A Guide to the Integrated Marine and Coastal Regionalisation of Australia Version 4.0. Department of the Environment and Heritage, Canberra, Australia.</dc:source>
	<skos:exactMatch rdf:resource="http://www.environment.gov.au/mapping/rest/services/ogc_services/IMCRA_Mesoscale/MapServer/0/52"/>
	<skos:scopeNote xml:lang="en">Note. A section of this bioregion also nests within the MEOW Cape Howe Ecoregion.</skos:scopeNote>
</rdf:Description>

<rdf:Description rdf:about="http://seamapaustralia.org.au/def/benthichabitatclassification/class/253">
	<rdf:type rdf:resource="http://www.w3.org/2000/01/rdf-schema#Resource"/>
	<rdf:type rdf:resource="http://www.w3.org/2004/02/skos/core#Concept"/>
	<skos:broader rdf:resource="http://seamapaustralia.org.au/def/benthichabitatclassification/class/250"/>
	<skos:prefLabel xml:lang="en">IMCRA Central Victoria Bioregion</skos:prefLabel>
	<dcterms:contributor rdf:resource="http://editor.vocabs.ands.org.au/user/eMII_Finney.Kim_Admin"/>
	<dcterms:created rdf:datatype="http://www.w3.org/2001/XMLSchema#dateTime">2017-06-13T04:37:20Z</dcterms:created>
	<dcterms:creator rdf:resource="http://editor.vocabs.ands.org.au/user/eMII_Finney.Kim_Admin"/>
	<dcterms:modified rdf:datatype="http://www.w3.org/2001/XMLSchema#dateTime">2017-06-13T23:20:47Z</dcterms:modified>
	<dc:publisher rdf:datatype="http://www.w3.org/2001/XMLSchema#string">Institute for Marine and Antarctic Studies (IMAS) - UTAS</dc:publisher>
	<skos:definition xml:lang="en">An inshore regionalisation of Australian waters derived from biological and physical data, including the distribution of demersal fishes, marine plants and invertebrates, sea floor geomorphology and sediments, and oceanographic data. The meso-scale regionalisation was compiled from information supplied to the Australian Government Department of the Environment and Heritage by the relevant State, Northern Territory and Commonwealth marine research and management agencies. The seaward extent for the meso-scale IMCRA coverage is defined by the 200m isobath except where this boundary extends beyond the Australian Exclusive Economic Zone (AEEZ).</skos:definition>
	<dc:source rdf:datatype="http://www.w3.org/2001/XMLSchema#string">Commonwealth of Australia (2006). A Guide to the Integrated Marine and Coastal Regionalisation of Australia Version 4.0. Department of the Environment and Heritage, Canberra, Australia.</dc:source>
	<skos:exactMatch rdf:resource="http://www.environment.gov.au/mapping/rest/services/ogc_services/IMCRA_Mesoscale/MapServer/0/54"/>
</rdf:Description>

<rdf:Description rdf:about="http://seamapaustralia.org.au/def/benthichabitatclassification/class/254">
	<rdf:type rdf:resource="http://www.w3.org/2000/01/rdf-schema#Resource"/>
	<rdf:type rdf:resource="http://www.w3.org/2004/02/skos/core#Concept"/>
	<skos:broader rdf:resource="http://seamapaustralia.org.au/def/benthichabitatclassification/class/250"/>
	<skos:prefLabel xml:lang="en">IMCRA Central Bass Strait Bioregion</skos:prefLabel>
	<dcterms:contributor rdf:resource="http://editor.vocabs.ands.org.au/user/eMII_Finney.Kim_Admin"/>
	<dcterms:created rdf:datatype="http://www.w3.org/2001/XMLSchema#dateTime">2017-06-13T04:38:02Z</dcterms:created>
	<dcterms:creator rdf:resource="http://editor.vocabs.ands.org.au/user/eMII_Finney.Kim_Admin"/>
	<dcterms:modified rdf:datatype="http://www.w3.org/2001/XMLSchema#dateTime">2017-06-13T23:21:00Z</dcterms:modified>
	<dc:publisher rdf:datatype="http://www.w3.org/2001/XMLSchema#string">Institute for Marine and Antarctic Studies (IMAS) - UTAS</dc:publisher>
	<skos:definition xml:lang="en">An inshore regionalisation of Australian waters derived from biological and physical data, including the distribution of demersal fishes, marine plants and invertebrates, sea floor geomorphology and sediments, and oceanographic data. The meso-scale regionalisation was compiled from information supplied to the Australian Government Department of the Environment and Heritage by the relevant State, Northern Territory and Commonwealth marine research and management agencies. The seaward extent for the meso-scale IMCRA coverage is defined by the 200m isobath except where this boundary extends beyond the Australian Exclusive Economic Zone (AEEZ).</skos:definition>
	<dc:source rdf:datatype="http://www.w3.org/2001/XMLSchema#string">Commonwealth of Australia (2006). A Guide to the Integrated Marine and Coastal Regionalisation of Australia Version 4.0. Department of the Environment and Heritage, Canberra, Australia.</dc:source>
	<skos:exactMatch rdf:resource="http://www.environment.gov.au/mapping/rest/services/ogc_services/IMCRA_Mesoscale/MapServer/0/55"/>
</rdf:Description>

<rdf:Description rdf:about="http://seamapaustralia.org.au/def/benthichabitatclassification/class/255">
	<rdf:type rdf:resource="http://www.w3.org/2000/01/rdf-schema#Resource"/>
	<rdf:type rdf:resource="http://www.w3.org/2004/02/skos/core#Concept"/>
	<skos:broader rdf:resource="http://seamapaustralia.org.au/def/benthichabitatclassification/class/250"/>
	<skos:prefLabel xml:lang="en">IMCRA Boags Bioregion</skos:prefLabel>
	<dcterms:contributor rdf:resource="http://editor.vocabs.ands.org.au/user/eMII_Finney.Kim_Admin"/>
	<dcterms:created rdf:datatype="http://www.w3.org/2001/XMLSchema#dateTime">2017-06-13T04:38:24Z</dcterms:created>
	<dcterms:creator rdf:resource="http://editor.vocabs.ands.org.au/user/eMII_Finney.Kim_Admin"/>
	<dcterms:modified rdf:datatype="http://www.w3.org/2001/XMLSchema#dateTime">2017-06-13T23:21:14Z</dcterms:modified>
	<dc:publisher rdf:datatype="http://www.w3.org/2001/XMLSchema#string">Institute for Marine and Antarctic Studies (IMAS) - UTAS</dc:publisher>
	<skos:definition xml:lang="en">An inshore regionalisation of Australian waters derived from biological and physical data, including the distribution of demersal fishes, marine plants and invertebrates, sea floor geomorphology and sediments, and oceanographic data. The meso-scale regionalisation was compiled from information supplied to the Australian Government Department of the Environment and Heritage by the relevant State, Northern Territory and Commonwealth marine research and management agencies. The seaward extent for the meso-scale IMCRA coverage is defined by the 200m isobath except where this boundary extends beyond the Australian Exclusive Economic Zone (AEEZ).</skos:definition>
	<dc:source rdf:datatype="http://www.w3.org/2001/XMLSchema#string">Commonwealth of Australia (2006). A Guide to the Integrated Marine and Coastal Regionalisation of Australia Version 4.0. Department of the Environment and Heritage, Canberra, Australia.</dc:source>
	<skos:exactMatch rdf:resource="http://www.environment.gov.au/mapping/rest/services/ogc_services/IMCRA_Mesoscale/MapServer/0/58"/>
</rdf:Description>

<rdf:Description rdf:about="http://seamapaustralia.org.au/def/benthichabitatclassification/class/257">
	<rdf:type rdf:resource="http://www.w3.org/2000/01/rdf-schema#Resource"/>
	<rdf:type rdf:resource="http://www.w3.org/2004/02/skos/core#Concept"/>
	<skos:broader rdf:resource="http://seamapaustralia.org.au/def/benthichabitatclassification/class/251"/>
	<skos:prefLabel xml:lang="en">IMCRA Bruny Bioregion</skos:prefLabel>
	<dcterms:contributor rdf:resource="http://editor.vocabs.ands.org.au/user/eMII_Finney.Kim_Admin"/>
	<dcterms:created rdf:datatype="http://www.w3.org/2001/XMLSchema#dateTime">2017-06-13T04:48:13Z</dcterms:created>
	<dcterms:creator rdf:resource="http://editor.vocabs.ands.org.au/user/eMII_Finney.Kim_Admin"/>
	<dcterms:modified rdf:datatype="http://www.w3.org/2001/XMLSchema#dateTime">2017-06-13T23:20:19Z</dcterms:modified>
	<dc:publisher rdf:datatype="http://www.w3.org/2001/XMLSchema#string">Institute for Marine and Antarctic Studies (IMAS) - UTAS</dc:publisher>
	<skos:definition xml:lang="en">An inshore regionalisation of Australian waters derived from biological and physical data, including the distribution of demersal fishes, marine plants and invertebrates, sea floor geomorphology and sediments, and oceanographic data. The meso-scale regionalisation was compiled from information supplied to the Australian Government Department of the Environment and Heritage by the relevant State, Northern Territory and Commonwealth marine research and management agencies. The seaward extent for the meso-scale IMCRA coverage is defined by the 200m isobath except where this boundary extends beyond the Australian Exclusive Economic Zone (AEEZ).</skos:definition>
	<dc:source rdf:datatype="http://www.w3.org/2001/XMLSchema#string"> Commonwealth of Australia (2006). A Guide to the Integrated Marine and Coastal Regionalisation of Australia Version 4.0. Department of the Environment and Heritage, Canberra, Australia.</dc:source>
	<skos:exactMatch rdf:resource="http://www.environment.gov.au/mapping/rest/services/ogc_services/IMCRA_Mesoscale/MapServer/0/61"/>
</rdf:Description>

<rdf:Description rdf:about="http://seamapaustralia.org.au/def/benthichabitatclassification/class/256">
	<rdf:type rdf:resource="http://www.w3.org/2000/01/rdf-schema#Resource"/>
	<rdf:type rdf:resource="http://www.w3.org/2004/02/skos/core#Concept"/>
	<skos:broader rdf:resource="http://seamapaustralia.org.au/def/benthichabitatclassification/class/251"/>
	<skos:prefLabel xml:lang="en">IMCRA Freycinet Bioregion</skos:prefLabel>
	<dcterms:contributor rdf:resource="http://editor.vocabs.ands.org.au/user/eMII_Finney.Kim_Admin"/>
	<dcterms:created rdf:datatype="http://www.w3.org/2001/XMLSchema#dateTime">2017-06-13T04:47:56Z</dcterms:created>
	<dcterms:creator rdf:resource="http://editor.vocabs.ands.org.au/user/eMII_Finney.Kim_Admin"/>
	<dcterms:modified rdf:datatype="http://www.w3.org/2001/XMLSchema#dateTime">2017-06-13T23:19:36Z</dcterms:modified>
	<dc:publisher rdf:datatype="http://www.w3.org/2001/XMLSchema#string">Institute for Marine and Antarctic Studies (IMAS) - UTAS</dc:publisher>
	<skos:definition xml:lang="en">An inshore regionalisation of Australian waters derived from biological and physical data, including the distribution of demersal fishes, marine plants and invertebrates, sea floor geomorphology and sediments, and oceanographic data. The meso-scale regionalisation was compiled from information supplied to the Australian Government Department of the Environment and Heritage by the relevant State, Northern Territory and Commonwealth marine research and management agencies. The seaward extent for the meso-scale IMCRA coverage is defined by the 200m isobath except where this boundary extends beyond the Australian Exclusive Economic Zone (AEEZ).</skos:definition>
	<dc:source rdf:datatype="http://www.w3.org/2001/XMLSchema#string"> Commonwealth of Australia (2006). A Guide to the Integrated Marine and Coastal Regionalisation of Australia Version 4.0. Department of the Environment and Heritage, Canberra, Australia.</dc:source>
	<skos:exactMatch rdf:resource="http://www.environment.gov.au/mapping/rest/services/ogc_services/IMCRA_Mesoscale/MapServer/0/59"/>
</rdf:Description>

<rdf:Description rdf:about="http://seamapaustralia.org.au/def/benthichabitatclassification/class/258">
	<rdf:type rdf:resource="http://www.w3.org/2000/01/rdf-schema#Resource"/>
	<rdf:type rdf:resource="http://www.w3.org/2004/02/skos/core#Concept"/>
	<skos:broader rdf:resource="http://seamapaustralia.org.au/def/benthichabitatclassification/class/251"/>
	<skos:prefLabel xml:lang="en">IMCRA Davey Bioregion</skos:prefLabel>
	<dcterms:contributor rdf:resource="http://editor.vocabs.ands.org.au/user/eMII_Finney.Kim_Admin"/>
	<dcterms:created rdf:datatype="http://www.w3.org/2001/XMLSchema#dateTime">2017-06-13T04:48:39Z</dcterms:created>
	<dcterms:creator rdf:resource="http://editor.vocabs.ands.org.au/user/eMII_Finney.Kim_Admin"/>
	<dcterms:modified rdf:datatype="http://www.w3.org/2001/XMLSchema#dateTime">2017-06-13T23:20:04Z</dcterms:modified>
	<dc:publisher rdf:datatype="http://www.w3.org/2001/XMLSchema#string">Institute for Marine and Antarctic Studies (IMAS) - UTAS</dc:publisher>
	<skos:definition xml:lang="en">An inshore regionalisation of Australian waters derived from biological and physical data, including the distribution of demersal fishes, marine plants and invertebrates, sea floor geomorphology and sediments, and oceanographic data. The meso-scale regionalisation was compiled from information supplied to the Australian Government Department of the Environment and Heritage by the relevant State, Northern Territory and Commonwealth marine research and management agencies. The seaward extent for the meso-scale IMCRA coverage is defined by the 200m isobath except where this boundary extends beyond the Australian Exclusive Economic Zone (AEEZ).</skos:definition>
	<dc:source rdf:datatype="http://www.w3.org/2001/XMLSchema#string"> Commonwealth of Australia (2006). A Guide to the Integrated Marine and Coastal Regionalisation of Australia Version 4.0. Department of the Environment and Heritage, Canberra, Australia.</dc:source>
	<skos:exactMatch rdf:resource="http://www.environment.gov.au/mapping/rest/services/ogc_services/IMCRA_Mesoscale/MapServer/0/62"/>
</rdf:Description>

<rdf:Description rdf:about="http://seamapaustralia.org.au/def/benthichabitatclassification/class/259">
	<rdf:type rdf:resource="http://www.w3.org/2000/01/rdf-schema#Resource"/>
	<rdf:type rdf:resource="http://www.w3.org/2004/02/skos/core#Concept"/>
	<skos:broader rdf:resource="http://seamapaustralia.org.au/def/benthichabitatclassification/class/251"/>
	<skos:prefLabel xml:lang="en">IMCRA Franklin Bioregion</skos:prefLabel>
	<dcterms:contributor rdf:resource="http://editor.vocabs.ands.org.au/user/eMII_Finney.Kim_Admin"/>
	<dcterms:created rdf:datatype="http://www.w3.org/2001/XMLSchema#dateTime">2017-06-13T04:49:02Z</dcterms:created>
	<dcterms:creator rdf:resource="http://editor.vocabs.ands.org.au/user/eMII_Finney.Kim_Admin"/>
	<dcterms:modified rdf:datatype="http://www.w3.org/2001/XMLSchema#dateTime">2017-06-13T23:19:50Z</dcterms:modified>
	<dc:publisher rdf:datatype="http://www.w3.org/2001/XMLSchema#string">Institute for Marine and Antarctic Studies (IMAS) - UTAS</dc:publisher>
	<skos:definition xml:lang="en">An inshore regionalisation of Australian waters derived from biological and physical data, including the distribution of demersal fishes, marine plants and invertebrates, sea floor geomorphology and sediments, and oceanographic data. The meso-scale regionalisation was compiled from information supplied to the Australian Government Department of the Environment and Heritage by the relevant State, Northern Territory and Commonwealth marine research and management agencies. The seaward extent for the meso-scale IMCRA coverage is defined by the 200m isobath except where this boundary extends beyond the Australian Exclusive Economic Zone (AEEZ).</skos:definition>
	<dc:source rdf:datatype="http://www.w3.org/2001/XMLSchema#string"> Commonwealth of Australia (2006). A Guide to the Integrated Marine and Coastal Regionalisation of Australia Version 4.0. Department of the Environment and Heritage, Canberra, Australia.</dc:source>
	<skos:exactMatch rdf:resource="http://www.environment.gov.au/mapping/rest/services/ogc_services/IMCRA_Mesoscale/MapServer/0/60"/>
</rdf:Description>

<rdf:Description rdf:about="http://seamapaustralia.org.au/def/benthichabitatclassification/class/264">
	<rdf:type rdf:resource="http://www.w3.org/2000/01/rdf-schema#Resource"/>
	<rdf:type rdf:resource="http://www.w3.org/2004/02/skos/core#Concept"/>
	<skos:broader rdf:resource="http://seamapaustralia.org.au/def/benthichabitatclassification/class/261"/>
	<skos:prefLabel xml:lang="en">IMCRA Batemans Shelf Bioregion</skos:prefLabel>
	<dcterms:contributor rdf:resource="http://editor.vocabs.ands.org.au/user/eMII_Finney.Kim_Admin"/>
	<dcterms:created rdf:datatype="http://www.w3.org/2001/XMLSchema#dateTime">2017-06-13T04:57:44Z</dcterms:created>
	<dcterms:creator rdf:resource="http://editor.vocabs.ands.org.au/user/eMII_Finney.Kim_Admin"/>
	<dcterms:modified rdf:datatype="http://www.w3.org/2001/XMLSchema#dateTime">2017-06-13T23:19:22Z</dcterms:modified>
	<dc:publisher rdf:datatype="http://www.w3.org/2001/XMLSchema#string">Institute for Marine and Antarctic Studies (IMAS) - UTAS</dc:publisher>
	<skos:definition xml:lang="en">An inshore regionalisation of Australian waters derived from biological and physical data, including the distribution of demersal fishes, marine plants and invertebrates, sea floor geomorphology and sediments, and oceanographic data. The meso-scale regionalisation was compiled from information supplied to the Australian Government Department of the Environment and Heritage by the relevant State, Northern Territory and Commonwealth marine research and management agencies. The seaward extent for the meso-scale IMCRA coverage is defined by the 200m isobath except where this boundary extends beyond the Australian Exclusive Economic Zone (AEEZ).</skos:definition>
	<dc:source rdf:datatype="http://www.w3.org/2001/XMLSchema#string"> Commonwealth of Australia (2006). A Guide to the Integrated Marine and Coastal Regionalisation of Australia Version 4.0. Department of the Environment and Heritage, Canberra, Australia.</dc:source>
	<skos:exactMatch rdf:resource="http://www.environment.gov.au/mapping/rest/services/ogc_services/IMCRA_Mesoscale/MapServer/0/48"/>
</rdf:Description>

<rdf:Description rdf:about="http://seamapaustralia.org.au/def/benthichabitatclassification/class/261">
	<rdf:type rdf:resource="http://www.w3.org/2000/01/rdf-schema#Resource"/>
	<rdf:type rdf:resource="http://www.w3.org/2004/02/skos/core#Concept"/>
	<skos:broader rdf:resource="http://seamapaustralia.org.au/def/benthichabitatclassification/class/228"/>
	<skos:prefLabel xml:lang="en">IMCRA Southeast Transition</skos:prefLabel>
	<dcterms:contributor rdf:resource="http://editor.vocabs.ands.org.au/user/eMII_Finney.Kim_Admin"/>
	<dcterms:created rdf:datatype="http://www.w3.org/2001/XMLSchema#dateTime">2017-06-13T04:56:02Z</dcterms:created>
	<dcterms:creator rdf:resource="http://editor.vocabs.ands.org.au/user/eMII_Finney.Kim_Admin"/>
	<dcterms:modified rdf:datatype="http://www.w3.org/2001/XMLSchema#dateTime">2017-06-13T23:13:24Z</dcterms:modified>
	<dc:publisher rdf:datatype="http://www.w3.org/2001/XMLSchema#string">Institute for Marine and Antarctic Studies (IMAS) - UTAS</dc:publisher>
	<skos:definition xml:lang="en">An IMCRA provincial bioregion reflects biogeographic patterns in distributions of bottom-dwelling fish. Provincial bioregions were defined for the continental shelf for IMCRA v3.3, and for the continental slope for the National Marine Bioregionalisation using similar analytical techniques. In both cases the distributions of demersal (bottom-dwelling) fish were plotted onto a line divided into equally spaced sections. The number of species in each section and the similarity between sections were calculated using a statistical tool called the Jaccard Index. Where the Jaccard Index changed greatly between sections a boundary was defined indicating differences in species assemblages between regions. Two types of provincial bioregions are defined in the IMCRA benthic bioregionalisation: provinces, which represent regions of biotic endemism; and transitions, which generally occur between the provinces, and are less well-defined mixing areas that capture the overlap of demersal fish species ranges between the provinces.</skos:definition>
	<dc:source rdf:datatype="http://www.w3.org/2001/XMLSchema#string"> Commonwealth of Australia (2006). A Guide to the Integrated Marine and Coastal Regionalisation of Australia Version 4.0. Department of the Environment and Heritage, Canberra, Australia.</dc:source>
	<skos:narrower rdf:resource="http://seamapaustralia.org.au/def/benthichabitatclassification/class/264"/>
	<skos:narrower rdf:resource="http://seamapaustralia.org.au/def/benthichabitatclassification/class/265"/>
	<skos:narrower rdf:resource="http://seamapaustralia.org.au/def/benthichabitatclassification/class/266"/>
	<skos:exactMatch rdf:resource="http://www.environment.gov.au/mapping/rest/services/ogc_services/IMCRA_Provincial/MapServer/0/35"/>
</rdf:Description>

<rdf:Description rdf:about="http://seamapaustralia.org.au/def/benthichabitatclassification/class/262">
	<rdf:type rdf:resource="http://www.w3.org/2000/01/rdf-schema#Resource"/>
	<rdf:type rdf:resource="http://www.w3.org/2004/02/skos/core#Concept"/>
	<skos:broader rdf:resource="http://seamapaustralia.org.au/def/benthichabitatclassification/class/230"/>
	<skos:prefLabel xml:lang="en">IMCRA Western Bassian Transition</skos:prefLabel>
	<dcterms:contributor rdf:resource="http://editor.vocabs.ands.org.au/user/eMII_Finney.Kim_Admin"/>
	<dcterms:created rdf:datatype="http://www.w3.org/2001/XMLSchema#dateTime">2017-06-13T04:56:55Z</dcterms:created>
	<dcterms:creator rdf:resource="http://editor.vocabs.ands.org.au/user/eMII_Finney.Kim_Admin"/>
	<dcterms:modified rdf:datatype="http://www.w3.org/2001/XMLSchema#dateTime">2017-06-13T23:14:12Z</dcterms:modified>
	<dc:publisher rdf:datatype="http://www.w3.org/2001/XMLSchema#string">Institute for Marine and Antarctic Studies (IMAS) - UTAS</dc:publisher>
	<skos:definition xml:lang="en">An IMCRA provincial bioregion reflects biogeographic patterns in distributions of bottom-dwelling fish. Provincial bioregions were defined for the continental shelf for IMCRA v3.3, and for the continental slope for the National Marine Bioregionalisation using similar analytical techniques. In both cases the distributions of demersal (bottom-dwelling) fish were plotted onto a line divided into equally spaced sections. The number of species in each section and the similarity between sections were calculated using a statistical tool called the Jaccard Index. Where the Jaccard Index changed greatly between sections a boundary was defined indicating differences in species assemblages between regions. Two types of provincial bioregions are defined in the IMCRA benthic bioregionalisation: provinces, which represent regions of biotic endemism; and transitions, which generally occur between the provinces, and are less well-defined mixing areas that capture the overlap of demersal fish species ranges between the provinces.</skos:definition>
	<dc:source rdf:datatype="http://www.w3.org/2001/XMLSchema#string"> Commonwealth of Australia (2006). A Guide to the Integrated Marine and Coastal Regionalisation of Australia Version 4.0. Department of the Environment and Heritage, Canberra, Australia.</dc:source>
	<skos:narrower rdf:resource="http://seamapaustralia.org.au/def/benthichabitatclassification/class/263"/>
	<skos:exactMatch rdf:resource="http://www.environment.gov.au/mapping/rest/services/ogc_services/IMCRA_Provincial/MapServer/0/36"/>
</rdf:Description>

<rdf:Description rdf:about="http://seamapaustralia.org.au/def/benthichabitatclassification/class/263">
	<rdf:type rdf:resource="http://www.w3.org/2000/01/rdf-schema#Resource"/>
	<rdf:type rdf:resource="http://www.w3.org/2004/02/skos/core#Concept"/>
	<skos:broader rdf:resource="http://seamapaustralia.org.au/def/benthichabitatclassification/class/262"/>
	<skos:prefLabel xml:lang="en">IMCRA Ottway Bioregion</skos:prefLabel>
	<dcterms:contributor rdf:resource="http://editor.vocabs.ands.org.au/user/eMII_Finney.Kim_Admin"/>
	<dcterms:created rdf:datatype="http://www.w3.org/2001/XMLSchema#dateTime">2017-06-13T04:57:15Z</dcterms:created>
	<dcterms:creator rdf:resource="http://editor.vocabs.ands.org.au/user/eMII_Finney.Kim_Admin"/>
	<dcterms:modified rdf:datatype="http://www.w3.org/2001/XMLSchema#dateTime">2017-06-13T23:17:45Z</dcterms:modified>
	<dc:publisher rdf:datatype="http://www.w3.org/2001/XMLSchema#string">Institute for Marine and Antarctic Studies (IMAS) - UTAS</dc:publisher>
	<skos:definition xml:lang="en">An inshore regionalisation of Australian waters derived from biological and physical data, including the distribution of demersal fishes, marine plants and invertebrates, sea floor geomorphology and sediments, and oceanographic data. The meso-scale regionalisation was compiled from information supplied to the Australian Government Department of the Environment and Heritage by the relevant State, Northern Territory and Commonwealth marine research and management agencies. The seaward extent for the meso-scale IMCRA coverage is defined by the 200m isobath except where this boundary extends beyond the Australian Exclusive Economic Zone (AEEZ).</skos:definition>
	<dc:source rdf:datatype="http://www.w3.org/2001/XMLSchema#string"> Commonwealth of Australia (2006). A Guide to the Integrated Marine and Coastal Regionalisation of Australia Version 4.0. Department of the Environment and Heritage, Canberra, Australia.</dc:source>
	<skos:exactMatch rdf:resource="http://www.environment.gov.au/mapping/rest/services/ogc_services/IMCRA_Mesoscale/MapServer/0/51"/>
</rdf:Description>

<rdf:Description rdf:about="http://seamapaustralia.org.au/def/benthichabitatclassification/class/265">
	<rdf:type rdf:resource="http://www.w3.org/2000/01/rdf-schema#Resource"/>
	<rdf:type rdf:resource="http://www.w3.org/2004/02/skos/core#Concept"/>
	<skos:broader rdf:resource="http://seamapaustralia.org.au/def/benthichabitatclassification/class/261"/>
	<skos:prefLabel xml:lang="en">IMCRA Twofold Shelf Bioregion</skos:prefLabel>
	<dcterms:contributor rdf:resource="http://editor.vocabs.ands.org.au/user/eMII_Finney.Kim_Admin"/>
	<dcterms:created rdf:datatype="http://www.w3.org/2001/XMLSchema#dateTime">2017-06-13T04:58:05Z</dcterms:created>
	<dcterms:creator rdf:resource="http://editor.vocabs.ands.org.au/user/eMII_Finney.Kim_Admin"/>
	<dcterms:modified rdf:datatype="http://www.w3.org/2001/XMLSchema#dateTime">2017-06-13T23:18:50Z</dcterms:modified>
	<dc:publisher rdf:datatype="http://www.w3.org/2001/XMLSchema#string">Institute for Marine and Antarctic Studies (IMAS) - UTAS</dc:publisher>
	<skos:definition xml:lang="en">An inshore regionalisation of Australian waters derived from biological and physical data, including the distribution of demersal fishes, marine plants and invertebrates, sea floor geomorphology and sediments, and oceanographic data. The meso-scale regionalisation was compiled from information supplied to the Australian Government Department of the Environment and Heritage by the relevant State, Northern Territory and Commonwealth marine research and management agencies. The seaward extent for the meso-scale IMCRA coverage is defined by the 200m isobath except where this boundary extends beyond the Australian Exclusive Economic Zone (AEEZ).</skos:definition>
	<dc:source rdf:datatype="http://www.w3.org/2001/XMLSchema#string"> Commonwealth of Australia (2006). A Guide to the Integrated Marine and Coastal Regionalisation of Australia Version 4.0. Department of the Environment and Heritage, Canberra, Australia.</dc:source>
	<skos:exactMatch rdf:resource="http://www.environment.gov.au/mapping/rest/services/ogc_services/IMCRA_Mesoscale/MapServer/0/50"/>
</rdf:Description>

<rdf:Description rdf:about="http://seamapaustralia.org.au/def/benthichabitatclassification/class/266">
	<rdf:type rdf:resource="http://www.w3.org/2000/01/rdf-schema#Resource"/>
	<rdf:type rdf:resource="http://www.w3.org/2004/02/skos/core#Concept"/>
	<skos:broader rdf:resource="http://seamapaustralia.org.au/def/benthichabitatclassification/class/261"/>
	<skos:prefLabel xml:lang="en">IMCRA Flinders Bioregion</skos:prefLabel>
	<dcterms:contributor rdf:resource="http://editor.vocabs.ands.org.au/user/eMII_Finney.Kim_Admin"/>
	<dcterms:created rdf:datatype="http://www.w3.org/2001/XMLSchema#dateTime">2017-06-13T04:58:23Z</dcterms:created>
	<dcterms:creator rdf:resource="http://editor.vocabs.ands.org.au/user/eMII_Finney.Kim_Admin"/>
	<dcterms:modified rdf:datatype="http://www.w3.org/2001/XMLSchema#dateTime">2017-06-13T23:19:07Z</dcterms:modified>
	<dc:publisher rdf:datatype="http://www.w3.org/2001/XMLSchema#string">Institute for Marine and Antarctic Studies (IMAS) - UTAS</dc:publisher>
	<skos:definition xml:lang="en">An inshore regionalisation of Australian waters derived from biological and physical data, including the distribution of demersal fishes, marine plants and invertebrates, sea floor geomorphology and sediments, and oceanographic data. The meso-scale regionalisation was compiled from information supplied to the Australian Government Department of the Environment and Heritage by the relevant State, Northern Territory and Commonwealth marine research and management agencies. The seaward extent for the meso-scale IMCRA coverage is defined by the 200m isobath except where this boundary extends beyond the Australian Exclusive Economic Zone (AEEZ).</skos:definition>
	<dc:source rdf:datatype="http://www.w3.org/2001/XMLSchema#string"> Commonwealth of Australia (2006). A Guide to the Integrated Marine and Coastal Regionalisation of Australia Version 4.0. Department of the Environment and Heritage, Canberra, Australia.</dc:source>
	<skos:exactMatch rdf:resource="http://www.environment.gov.au/mapping/rest/services/ogc_services/IMCRA_Mesoscale/MapServer/0/57"/>
</rdf:Description>

<rdf:Description rdf:about="http://www.environment.gov.au/mapping/rest/services/ogc_services/IMCRA_Mesoscale/MapServer/0/52">
	<rdf:type rdf:resource="http://www.w3.org/2000/01/rdf-schema#Resource"/>
</rdf:Description>

<rdf:Description rdf:about="http://www.environment.gov.au/mapping/rest/services/ogc_services/IMCRA_Mesoscale/MapServer/0/54">
	<rdf:type rdf:resource="http://www.w3.org/2000/01/rdf-schema#Resource"/>
</rdf:Description>

<rdf:Description rdf:about="http://www.environment.gov.au/mapping/rest/services/ogc_services/IMCRA_Mesoscale/MapServer/0/55">
	<rdf:type rdf:resource="http://www.w3.org/2000/01/rdf-schema#Resource"/>
</rdf:Description>

<rdf:Description rdf:about="http://www.environment.gov.au/mapping/rest/services/ogc_services/IMCRA_Mesoscale/MapServer/0/58">
	<rdf:type rdf:resource="http://www.w3.org/2000/01/rdf-schema#Resource"/>
</rdf:Description>

<rdf:Description rdf:about="http://www.environment.gov.au/mapping/rest/services/ogc_services/IMCRA_Mesoscale/MapServer/0/61">
	<rdf:type rdf:resource="http://www.w3.org/2000/01/rdf-schema#Resource"/>
</rdf:Description>

<rdf:Description rdf:about="http://www.environment.gov.au/mapping/rest/services/ogc_services/IMCRA_Mesoscale/MapServer/0/60">
	<rdf:type rdf:resource="http://www.w3.org/2000/01/rdf-schema#Resource"/>
</rdf:Description>

<rdf:Description rdf:about="http://www.environment.gov.au/mapping/rest/services/ogc_services/IMCRA_Mesoscale/MapServer/0/62">
	<rdf:type rdf:resource="http://www.w3.org/2000/01/rdf-schema#Resource"/>
</rdf:Description>

<rdf:Description rdf:about="http://www.environment.gov.au/mapping/rest/services/ogc_services/IMCRA_Mesoscale/MapServer/0/59">
	<rdf:type rdf:resource="http://www.w3.org/2000/01/rdf-schema#Resource"/>
</rdf:Description>

<rdf:Description rdf:about="http://www.environment.gov.au/mapping/rest/services/ogc_services/IMCRA_Mesoscale/MapServer/0/48">
	<rdf:type rdf:resource="http://www.w3.org/2000/01/rdf-schema#Resource"/>
</rdf:Description>

<rdf:Description rdf:about="http://www.environment.gov.au/mapping/rest/services/ogc_services/IMCRA_Mesoscale/MapServer/0/57">
	<rdf:type rdf:resource="http://www.w3.org/2000/01/rdf-schema#Resource"/>
</rdf:Description>

<rdf:Description rdf:about="http://www.environment.gov.au/mapping/rest/services/ogc_services/IMCRA_Mesoscale/MapServer/0/50">
	<rdf:type rdf:resource="http://www.w3.org/2000/01/rdf-schema#Resource"/>
</rdf:Description>

<rdf:Description rdf:about="http://www.environment.gov.au/mapping/rest/services/ogc_services/IMCRA_Mesoscale/MapServer/0/51">
	<rdf:type rdf:resource="http://www.w3.org/2000/01/rdf-schema#Resource"/>
</rdf:Description>

<rdf:Description rdf:about="http://www.environment.gov.au/mapping/rest/services/ogc_services/IMCRA_Provincial/MapServer/0/38">
	<rdf:type rdf:resource="http://www.w3.org/2000/01/rdf-schema#Resource"/>
</rdf:Description>

<rdf:Description rdf:about="http://www.environment.gov.au/mapping/rest/services/ogc_services/IMCRA_Provincial/MapServer/0/39">
	<rdf:type rdf:resource="http://www.w3.org/2000/01/rdf-schema#Resource"/>
</rdf:Description>

<rdf:Description rdf:about="http://www.environment.gov.au/mapping/rest/services/ogc_services/IMCRA_Provincial/MapServer/0/35">
	<rdf:type rdf:resource="http://www.w3.org/2000/01/rdf-schema#Resource"/>
</rdf:Description>

<rdf:Description rdf:about="http://www.environment.gov.au/mapping/rest/services/ogc_services/IMCRA_Provincial/MapServer/0/36">
	<rdf:type rdf:resource="http://www.w3.org/2000/01/rdf-schema#Resource"/>
</rdf:Description>

<rdf:Description rdf:about="http://seamapaustralia.org.au/def/benthichabitatclassification/class/267">
	<rdf:type rdf:resource="http://www.w3.org/2000/01/rdf-schema#Resource"/>
	<rdf:type rdf:resource="http://www.w3.org/2004/02/skos/core#Concept"/>
	<skos:broader rdf:resource="http://seamapaustralia.org.au/def/benthichabitatclassification/class/232"/>
	<skos:prefLabel xml:lang="en">IMCRA Great Australian Bight Transition</skos:prefLabel>
	<dcterms:contributor rdf:resource="http://editor.vocabs.ands.org.au/user/eMII_Finney.Kim_Admin"/>
	<dcterms:created rdf:datatype="http://www.w3.org/2001/XMLSchema#dateTime">2017-06-13T22:00:59Z</dcterms:created>
	<dcterms:creator rdf:resource="http://editor.vocabs.ands.org.au/user/eMII_Finney.Kim_Admin"/>
	<dcterms:modified rdf:datatype="http://www.w3.org/2001/XMLSchema#dateTime">2017-06-13T22:57:10Z</dcterms:modified>
	<dc:publisher rdf:datatype="http://www.w3.org/2001/XMLSchema#string">Institute for Marine and Antarctic Studies (IMAS) - UTAS</dc:publisher>
	<skos:definition xml:lang="en">An IMCRA provincial bioregion reflects biogeographic patterns in distributions of bottom-dwelling fish. Provincial bioregions were defined for the continental shelf for IMCRA v3.3, and for the continental slope for the National Marine Bioregionalisation using similar analytical techniques. In both cases the distributions of demersal (bottom-dwelling) fish were plotted onto a line divided into equally spaced sections. The number of species in each section and the similarity between sections were calculated using a statistical tool called the Jaccard Index. Where the Jaccard Index changed greatly between sections a boundary was defined indicating differences in species assemblages between regions. Two types of provincial bioregions are defined in the IMCRA benthic bioregionalisation: provinces, which represent regions of biotic endemism; and transitions, which generally occur between the provinces, and are less well-defined mixing areas that capture the overlap of demersal fish species ranges between the provinces.</skos:definition>
	<dc:source rdf:datatype="http://www.w3.org/2001/XMLSchema#string">Commonwealth of Australia (2006). A Guide to the Integrated Marine and Coastal Regionalisation of Australia Version 4.0. Department of the Environment and Heritage, Canberra, Australia.</dc:source>
	<skos:narrower rdf:resource="http://seamapaustralia.org.au/def/benthichabitatclassification/class/268"/>
	<skos:narrower rdf:resource="http://seamapaustralia.org.au/def/benthichabitatclassification/class/269"/>
	<skos:exactMatch rdf:resource="http://www.environment.gov.au/mapping/rest/services/ogc_services/IMCRA_Provincial/MapServer/0/29"/>
</rdf:Description>

<rdf:Description rdf:about="http://seamapaustralia.org.au/def/benthichabitatclassification/class/268">
	<rdf:type rdf:resource="http://www.w3.org/2000/01/rdf-schema#Resource"/>
	<rdf:type rdf:resource="http://www.w3.org/2004/02/skos/core#Concept"/>
	<skos:broader rdf:resource="http://seamapaustralia.org.au/def/benthichabitatclassification/class/267"/>
	<skos:prefLabel xml:lang="en">IMCRA Murat Bioregion</skos:prefLabel>
	<dcterms:contributor rdf:resource="http://editor.vocabs.ands.org.au/user/eMII_Finney.Kim_Admin"/>
	<dcterms:created rdf:datatype="http://www.w3.org/2001/XMLSchema#dateTime">2017-06-13T22:01:31Z</dcterms:created>
	<dcterms:creator rdf:resource="http://editor.vocabs.ands.org.au/user/eMII_Finney.Kim_Admin"/>
	<dcterms:modified rdf:datatype="http://www.w3.org/2001/XMLSchema#dateTime">2017-06-13T23:03:11Z</dcterms:modified>
	<dc:publisher rdf:datatype="http://www.w3.org/2001/XMLSchema#string">Institute for Marine and Antarctic Studies (IMAS) - UTAS</dc:publisher>
	<skos:definition xml:lang="en">An inshore regionalisation of Australian waters derived from biological and physical data, including the distribution of demersal fishes, marine plants and invertebrates, sea floor geomorphology and sediments, and oceanographic data. The meso-scale regionalisation was compiled from information supplied to the Australian Government Department of the Environment and Heritage by the relevant State, Northern Territory and Commonwealth marine research and management agencies. The seaward extent for the meso-scale IMCRA coverage is defined by the 200m isobath except where this boundary extends beyond the Australian Exclusive Economic Zone (AEEZ).</skos:definition>
	<dc:source rdf:datatype="http://www.w3.org/2001/XMLSchema#string">Commonwealth of Australia (2006). A Guide to the Integrated Marine and Coastal Regionalisation of Australia Version 4.0. Department of the Environment and Heritage, Canberra, Australia.</dc:source>
	<skos:exactMatch rdf:resource="http://www.environment.gov.au/mapping/rest/services/ogc_services/IMCRA_Mesoscale/MapServer/0/40"/>
</rdf:Description>

<rdf:Description rdf:about="http://seamapaustralia.org.au/def/benthichabitatclassification/class/269">
	<rdf:type rdf:resource="http://www.w3.org/2000/01/rdf-schema#Resource"/>
	<rdf:type rdf:resource="http://www.w3.org/2004/02/skos/core#Concept"/>
	<skos:broader rdf:resource="http://seamapaustralia.org.au/def/benthichabitatclassification/class/267"/>
	<skos:prefLabel xml:lang="en">IMCRA Eucla Bioregion</skos:prefLabel>
	<dcterms:contributor rdf:resource="http://editor.vocabs.ands.org.au/user/eMII_Finney.Kim_Admin"/>
	<dcterms:created rdf:datatype="http://www.w3.org/2001/XMLSchema#dateTime">2017-06-13T22:01:52Z</dcterms:created>
	<dcterms:creator rdf:resource="http://editor.vocabs.ands.org.au/user/eMII_Finney.Kim_Admin"/>
	<dcterms:modified rdf:datatype="http://www.w3.org/2001/XMLSchema#dateTime">2017-06-13T23:01:47Z</dcterms:modified>
	<dc:publisher rdf:datatype="http://www.w3.org/2001/XMLSchema#string">Institute for Marine and Antarctic Studies (IMAS) - UTAS</dc:publisher>
	<skos:definition xml:lang="en">An inshore regionalisation of Australian waters derived from biological and physical data, including the distribution of demersal fishes, marine plants and invertebrates, sea floor geomorphology and sediments, and oceanographic data. The meso-scale regionalisation was compiled from information supplied to the Australian Government Department of the Environment and Heritage by the relevant State, Northern Territory and Commonwealth marine research and management agencies. The seaward extent for the meso-scale IMCRA coverage is defined by the 200m isobath except where this boundary extends beyond the Australian Exclusive Economic Zone (AEEZ).</skos:definition>
	<dc:source rdf:datatype="http://www.w3.org/2001/XMLSchema#string">Commonwealth of Australia (2006). A Guide to the Integrated Marine and Coastal Regionalisation of Australia Version 4.0. Department of the Environment and Heritage, Canberra, Australia.</dc:source>
	<skos:exactMatch rdf:resource="http://www.environment.gov.au/mapping/rest/services/ogc_services/IMCRA_Mesoscale/MapServer/0/39"/>
</rdf:Description>

<rdf:Description rdf:about="http://seamapaustralia.org.au/def/benthichabitatclassification/class/270">
	<rdf:type rdf:resource="http://www.w3.org/2000/01/rdf-schema#Resource"/>
	<rdf:type rdf:resource="http://www.w3.org/2004/02/skos/core#Concept"/>
	<skos:broader rdf:resource="http://seamapaustralia.org.au/def/benthichabitatclassification/class/233"/>
	<skos:prefLabel xml:lang="en">IMCRA Southwest Province</skos:prefLabel>
	<dcterms:contributor rdf:resource="http://editor.vocabs.ands.org.au/user/eMII_Finney.Kim_Admin"/>
	<dcterms:created rdf:datatype="http://www.w3.org/2001/XMLSchema#dateTime">2017-06-13T22:02:26Z</dcterms:created>
	<dcterms:creator rdf:resource="http://editor.vocabs.ands.org.au/user/eMII_Finney.Kim_Admin"/>
	<dcterms:modified rdf:datatype="http://www.w3.org/2001/XMLSchema#dateTime">2017-06-13T22:56:06Z</dcterms:modified>
	<dc:publisher rdf:datatype="http://www.w3.org/2001/XMLSchema#string">Institute for Marine and Antarctic Studies (IMAS) - UTAS</dc:publisher>
	<skos:definition xml:lang="en">An IMCRA provincial bioregion reflects biogeographic patterns in distributions of bottom-dwelling fish. Provincial bioregions were defined for the continental shelf for IMCRA v3.3, and for the continental slope for the National Marine Bioregionalisation using similar analytical techniques. In both cases the distributions of demersal (bottom-dwelling) fish were plotted onto a line divided into equally spaced sections. The number of species in each section and the similarity between sections were calculated using a statistical tool called the Jaccard Index. Where the Jaccard Index changed greatly between sections a boundary was defined indicating differences in species assemblages between regions. Two types of provincial bioregions are defined in the IMCRA benthic bioregionalisation: provinces, which represent regions of biotic endemism; and transitions, which generally occur between the provinces, and are less well-defined mixing areas that capture the overlap of demersal fish species ranges between the provinces.</skos:definition>
	<dc:source rdf:datatype="http://www.w3.org/2001/XMLSchema#string">Commonwealth of Australia (2006). A Guide to the Integrated Marine and Coastal Regionalisation of Australia Version 4.0. Department of the Environment and Heritage, Canberra, Australia.</dc:source>
	<skos:narrower rdf:resource="http://seamapaustralia.org.au/def/benthichabitatclassification/class/271"/>
	<skos:narrower rdf:resource="http://seamapaustralia.org.au/def/benthichabitatclassification/class/272"/>
	<skos:exactMatch rdf:resource="http://www.environment.gov.au/mapping/rest/services/ogc_services/IMCRA_Provincial/MapServer/0/31"/>
</rdf:Description>

<rdf:Description rdf:about="http://seamapaustralia.org.au/def/benthichabitatclassification/class/271">
	<rdf:type rdf:resource="http://www.w3.org/2000/01/rdf-schema#Resource"/>
	<rdf:type rdf:resource="http://www.w3.org/2004/02/skos/core#Concept"/>
	<skos:broader rdf:resource="http://seamapaustralia.org.au/def/benthichabitatclassification/class/270"/>
	<skos:prefLabel xml:lang="en">IMCRA Leeuwin-Naturaliste Bioregion</skos:prefLabel>
	<dcterms:contributor rdf:resource="http://editor.vocabs.ands.org.au/user/eMII_Finney.Kim_Admin"/>
	<dcterms:created rdf:datatype="http://www.w3.org/2001/XMLSchema#dateTime">2017-06-13T22:02:55Z</dcterms:created>
	<dcterms:creator rdf:resource="http://editor.vocabs.ands.org.au/user/eMII_Finney.Kim_Admin"/>
	<dcterms:modified rdf:datatype="http://www.w3.org/2001/XMLSchema#dateTime">2017-06-13T23:04:15Z</dcterms:modified>
	<dc:publisher rdf:datatype="http://www.w3.org/2001/XMLSchema#string">Institute for Marine and Antarctic Studies (IMAS) - UTAS</dc:publisher>
	<skos:definition xml:lang="en">An inshore regionalisation of Australian waters derived from biological and physical data, including the distribution of demersal fishes, marine plants and invertebrates, sea floor geomorphology and sediments, and oceanographic data. The meso-scale regionalisation was compiled from information supplied to the Australian Government Department of the Environment and Heritage by the relevant State, Northern Territory and Commonwealth marine research and management agencies. The seaward extent for the meso-scale IMCRA coverage is defined by the 200m isobath except where this boundary extends beyond the Australian Exclusive Economic Zone (AEEZ).</skos:definition>
	<dc:source rdf:datatype="http://www.w3.org/2001/XMLSchema#string">Commonwealth of Australia (2006). A Guide to the Integrated Marine and Coastal Regionalisation of Australia Version 4.0. Department of the Environment and Heritage, Canberra, Australia.</dc:source>
	<skos:exactMatch rdf:resource="http://www.environment.gov.au/mapping/rest/services/ogc_services/IMCRA_Mesoscale/MapServer/0/41"/>
</rdf:Description>

<rdf:Description rdf:about="http://seamapaustralia.org.au/def/benthichabitatclassification/class/272">
	<rdf:type rdf:resource="http://www.w3.org/2000/01/rdf-schema#Resource"/>
	<rdf:type rdf:resource="http://www.w3.org/2004/02/skos/core#Concept"/>
	<skos:broader rdf:resource="http://seamapaustralia.org.au/def/benthichabitatclassification/class/270"/>
	<skos:prefLabel xml:lang="en">IMCRA WA South Coast Bioregion</skos:prefLabel>
	<dcterms:contributor rdf:resource="http://editor.vocabs.ands.org.au/user/eMII_Finney.Kim_Admin"/>
	<dcterms:created rdf:datatype="http://www.w3.org/2001/XMLSchema#dateTime">2017-06-13T22:03:17Z</dcterms:created>
	<dcterms:creator rdf:resource="http://editor.vocabs.ands.org.au/user/eMII_Finney.Kim_Admin"/>
	<dcterms:modified rdf:datatype="http://www.w3.org/2001/XMLSchema#dateTime">2017-06-13T23:04:59Z</dcterms:modified>
	<dc:publisher rdf:datatype="http://www.w3.org/2001/XMLSchema#string">Institute for Marine and Antarctic Studies (IMAS) - UTAS</dc:publisher>
	<skos:definition xml:lang="en">An inshore regionalisation of Australian waters derived from biological and physical data, including the distribution of demersal fishes, marine plants and invertebrates, sea floor geomorphology and sediments, and oceanographic data. The meso-scale regionalisation was compiled from information supplied to the Australian Government Department of the Environment and Heritage by the relevant State, Northern Territory and Commonwealth marine research and management agencies. The seaward extent for the meso-scale IMCRA coverage is defined by the 200m isobath except where this boundary extends beyond the Australian Exclusive Economic Zone (AEEZ).</skos:definition>
	<dc:source rdf:datatype="http://www.w3.org/2001/XMLSchema#string">Commonwealth of Australia (2006). A Guide to the Integrated Marine and Coastal Regionalisation of Australia Version 4.0. Department of the Environment and Heritage, Canberra, Australia.</dc:source>
	<skos:exactMatch rdf:resource="http://www.environment.gov.au/mapping/rest/services/ogc_services/IMCRA_Mesoscale/MapServer/0/45"/>
</rdf:Description>

<rdf:Description rdf:about="http://seamapaustralia.org.au/def/benthichabitatclassification/class/273">
	<rdf:type rdf:resource="http://www.w3.org/2000/01/rdf-schema#Resource"/>
	<rdf:type rdf:resource="http://www.w3.org/2004/02/skos/core#Concept"/>
	<skos:broader rdf:resource="http://seamapaustralia.org.au/def/benthichabitatclassification/class/231"/>
	<skos:prefLabel xml:lang="en">IMCRA Spencer Gulf Province</skos:prefLabel>
	<dcterms:contributor rdf:resource="http://editor.vocabs.ands.org.au/user/eMII_Finney.Kim_Admin"/>
	<dcterms:created rdf:datatype="http://www.w3.org/2001/XMLSchema#dateTime">2017-06-13T22:03:51Z</dcterms:created>
	<dcterms:creator rdf:resource="http://editor.vocabs.ands.org.au/user/eMII_Finney.Kim_Admin"/>
	<dcterms:modified rdf:datatype="http://www.w3.org/2001/XMLSchema#dateTime">2017-06-13T22:55:25Z</dcterms:modified>
	<dc:publisher rdf:datatype="http://www.w3.org/2001/XMLSchema#string">Institute for Marine and Antarctic Studies (IMAS) - UTAS</dc:publisher>
	<skos:definition xml:lang="en">An IMCRA provincial bioregion reflects biogeographic patterns in distributions of bottom-dwelling fish. Provincial bioregions were defined for the continental shelf for IMCRA v3.3, and for the continental slope for the National Marine Bioregionalisation using similar analytical techniques. In both cases the distributions of demersal (bottom-dwelling) fish were plotted onto a line divided into equally spaced sections. The number of species in each section and the similarity between sections were calculated using a statistical tool called the Jaccard Index. Where the Jaccard Index changed greatly between sections a boundary was defined indicating differences in species assemblages between regions. Two types of provincial bioregions are defined in the IMCRA benthic bioregionalisation: provinces, which represent regions of biotic endemism; and transitions, which generally occur between the provinces, and are less well-defined mixing areas that capture the overlap of demersal fish species ranges between the provinces.</skos:definition>
	<dc:source rdf:datatype="http://www.w3.org/2001/XMLSchema#string">Commonwealth of Australia (2006). A Guide to the Integrated Marine and Coastal Regionalisation of Australia Version 4.0. Department of the Environment and Heritage, Canberra, Australia.</dc:source>
	<skos:narrower rdf:resource="http://seamapaustralia.org.au/def/benthichabitatclassification/class/277"/>
	<skos:narrower rdf:resource="http://seamapaustralia.org.au/def/benthichabitatclassification/class/274"/>
	<skos:narrower rdf:resource="http://seamapaustralia.org.au/def/benthichabitatclassification/class/275"/>
	<skos:narrower rdf:resource="http://seamapaustralia.org.au/def/benthichabitatclassification/class/276"/>
	<skos:narrower rdf:resource="http://seamapaustralia.org.au/def/benthichabitatclassification/class/278"/>
	<skos:exactMatch rdf:resource="http://www.environment.gov.au/mapping/rest/services/ogc_services/IMCRA_Provincial/MapServer/0/32"/>
</rdf:Description>

<rdf:Description rdf:about="http://seamapaustralia.org.au/def/benthichabitatclassification/class/274">
	<rdf:type rdf:resource="http://www.w3.org/2000/01/rdf-schema#Resource"/>
	<rdf:type rdf:resource="http://www.w3.org/2004/02/skos/core#Concept"/>
	<skos:broader rdf:resource="http://seamapaustralia.org.au/def/benthichabitatclassification/class/273"/>
	<skos:prefLabel xml:lang="en">IMCRA Spencer Gulf Bioregion</skos:prefLabel>
	<dcterms:contributor rdf:resource="http://editor.vocabs.ands.org.au/user/eMII_Finney.Kim_Admin"/>
	<dcterms:created rdf:datatype="http://www.w3.org/2001/XMLSchema#dateTime">2017-06-13T22:04:15Z</dcterms:created>
	<dcterms:creator rdf:resource="http://editor.vocabs.ands.org.au/user/eMII_Finney.Kim_Admin"/>
	<dcterms:modified rdf:datatype="http://www.w3.org/2001/XMLSchema#dateTime">2017-06-13T23:08:29Z</dcterms:modified>
	<dc:publisher rdf:datatype="http://www.w3.org/2001/XMLSchema#string">Institute for Marine and Antarctic Studies (IMAS) - UTAS</dc:publisher>
	<skos:definition xml:lang="en">An inshore regionalisation of Australian waters derived from biological and physical data, including the distribution of demersal fishes, marine plants and invertebrates, sea floor geomorphology and sediments, and oceanographic data. The meso-scale regionalisation was compiled from information supplied to the Australian Government Department of the Environment and Heritage by the relevant State, Northern Territory and Commonwealth marine research and management agencies. The seaward extent for the meso-scale IMCRA coverage is defined by the 200m isobath except where this boundary extends beyond the Australian Exclusive Economic Zone (AEEZ).</skos:definition>
	<dc:source rdf:datatype="http://www.w3.org/2001/XMLSchema#string">Commonwealth of Australia (2006). A Guide to the Integrated Marine and Coastal Regionalisation of Australia Version 4.0. Department of the Environment and Heritage, Canberra, Australia.</dc:source>
	<skos:exactMatch rdf:resource="http://www.environment.gov.au/mapping/rest/services/ogc_services/IMCRA_Mesoscale/MapServer/0/46"/>
</rdf:Description>

<rdf:Description rdf:about="http://seamapaustralia.org.au/def/benthichabitatclassification/class/275">
	<rdf:type rdf:resource="http://www.w3.org/2000/01/rdf-schema#Resource"/>
	<rdf:type rdf:resource="http://www.w3.org/2004/02/skos/core#Concept"/>
	<skos:broader rdf:resource="http://seamapaustralia.org.au/def/benthichabitatclassification/class/273"/>
	<skos:prefLabel xml:lang="en">IMCRA North Spencer Gulf Bioregion</skos:prefLabel>
	<dcterms:contributor rdf:resource="http://editor.vocabs.ands.org.au/user/eMII_Finney.Kim_Admin"/>
	<dcterms:created rdf:datatype="http://www.w3.org/2001/XMLSchema#dateTime">2017-06-13T22:04:38Z</dcterms:created>
	<dcterms:creator rdf:resource="http://editor.vocabs.ands.org.au/user/eMII_Finney.Kim_Admin"/>
	<dcterms:modified rdf:datatype="http://www.w3.org/2001/XMLSchema#dateTime">2017-06-13T23:07:51Z</dcterms:modified>
	<dc:publisher rdf:datatype="http://www.w3.org/2001/XMLSchema#string">Institute for Marine and Antarctic Studies (IMAS) - UTAS</dc:publisher>
	<skos:definition xml:lang="en">An inshore regionalisation of Australian waters derived from biological and physical data, including the distribution of demersal fishes, marine plants and invertebrates, sea floor geomorphology and sediments, and oceanographic data. The meso-scale regionalisation was compiled from information supplied to the Australian Government Department of the Environment and Heritage by the relevant State, Northern Territory and Commonwealth marine research and management agencies. The seaward extent for the meso-scale IMCRA coverage is defined by the 200m isobath except where this boundary extends beyond the Australian Exclusive Economic Zone (AEEZ).</skos:definition>
	<dc:source rdf:datatype="http://www.w3.org/2001/XMLSchema#string">Commonwealth of Australia (2006). A Guide to the Integrated Marine and Coastal Regionalisation of Australia Version 4.0. Department of the Environment and Heritage, Canberra, Australia.</dc:source>
	<skos:exactMatch rdf:resource="http://www.environment.gov.au/mapping/rest/services/ogc_services/IMCRA_Mesoscale/MapServer/0/43"/>
</rdf:Description>

<rdf:Description rdf:about="http://seamapaustralia.org.au/def/benthichabitatclassification/class/276">
	<rdf:type rdf:resource="http://www.w3.org/2000/01/rdf-schema#Resource"/>
	<rdf:type rdf:resource="http://www.w3.org/2004/02/skos/core#Concept"/>
	<skos:broader rdf:resource="http://seamapaustralia.org.au/def/benthichabitatclassification/class/273"/>
	<skos:prefLabel xml:lang="en">IMCRA Eyre Bioregion</skos:prefLabel>
	<dcterms:contributor rdf:resource="http://editor.vocabs.ands.org.au/user/eMII_Finney.Kim_Admin"/>
	<dcterms:created rdf:datatype="http://www.w3.org/2001/XMLSchema#dateTime">2017-06-13T22:04:56Z</dcterms:created>
	<dcterms:creator rdf:resource="http://editor.vocabs.ands.org.au/user/eMII_Finney.Kim_Admin"/>
	<dcterms:modified rdf:datatype="http://www.w3.org/2001/XMLSchema#dateTime">2017-06-13T23:07:10Z</dcterms:modified>
	<dc:publisher rdf:datatype="http://www.w3.org/2001/XMLSchema#string">Institute for Marine and Antarctic Studies (IMAS) - UTAS</dc:publisher>
	<skos:definition xml:lang="en">An inshore regionalisation of Australian waters derived from biological and physical data, including the distribution of demersal fishes, marine plants and invertebrates, sea floor geomorphology and sediments, and oceanographic data. The meso-scale regionalisation was compiled from information supplied to the Australian Government Department of the Environment and Heritage by the relevant State, Northern Territory and Commonwealth marine research and management agencies. The seaward extent for the meso-scale IMCRA coverage is defined by the 200m isobath except where this boundary extends beyond the Australian Exclusive Economic Zone (AEEZ).</skos:definition>
	<dc:source rdf:datatype="http://www.w3.org/2001/XMLSchema#string">Commonwealth of Australia (2006). A Guide to the Integrated Marine and Coastal Regionalisation of Australia Version 4.0. Department of the Environment and Heritage, Canberra, Australia.</dc:source>
	<skos:exactMatch rdf:resource="http://www.environment.gov.au/mapping/rest/services/ogc_services/IMCRA_Mesoscale/MapServer/0/42"/>
</rdf:Description>

<rdf:Description rdf:about="http://seamapaustralia.org.au/def/benthichabitatclassification/class/278">
	<rdf:type rdf:resource="http://www.w3.org/2000/01/rdf-schema#Resource"/>
	<rdf:type rdf:resource="http://www.w3.org/2004/02/skos/core#Concept"/>
	<skos:broader rdf:resource="http://seamapaustralia.org.au/def/benthichabitatclassification/class/273"/>
	<skos:prefLabel xml:lang="en">IMCRA Coorong Bioregion</skos:prefLabel>
	<dcterms:contributor rdf:resource="http://editor.vocabs.ands.org.au/user/eMII_Finney.Kim_Admin"/>
	<dcterms:created rdf:datatype="http://www.w3.org/2001/XMLSchema#dateTime">2017-06-13T22:05:54Z</dcterms:created>
	<dcterms:creator rdf:resource="http://editor.vocabs.ands.org.au/user/eMII_Finney.Kim_Admin"/>
	<dcterms:modified rdf:datatype="http://www.w3.org/2001/XMLSchema#dateTime">2017-06-13T23:06:36Z</dcterms:modified>
	<dc:publisher rdf:datatype="http://www.w3.org/2001/XMLSchema#string">Institute for Marine and Antarctic Studies (IMAS) - UTAS</dc:publisher>
	<skos:definition xml:lang="en">An inshore regionalisation of Australian waters derived from biological and physical data, including the distribution of demersal fishes, marine plants and invertebrates, sea floor geomorphology and sediments, and oceanographic data. The meso-scale regionalisation was compiled from information supplied to the Australian Government Department of the Environment and Heritage by the relevant State, Northern Territory and Commonwealth marine research and management agencies. The seaward extent for the meso-scale IMCRA coverage is defined by the 200m isobath except where this boundary extends beyond the Australian Exclusive Economic Zone (AEEZ).</skos:definition>
	<dc:source rdf:datatype="http://www.w3.org/2001/XMLSchema#string">Commonwealth of Australia (2006). A Guide to the Integrated Marine and Coastal Regionalisation of Australia Version 4.0. Department of the Environment and Heritage, Canberra, Australia.</dc:source>
	<skos:exactMatch rdf:resource="http://www.environment.gov.au/mapping/rest/services/ogc_services/IMCRA_Mesoscale/MapServer/0/49"/>
	<skos:scopeNote xml:lang="en">This bioregion also partially sits within the MEOW Western Bassian Ecoregion.</skos:scopeNote>
</rdf:Description>

<rdf:Description rdf:about="http://www.environment.gov.au/mapping/rest/services/ogc_services/IMCRA_Provincial/MapServer/0/32">
	<rdf:type rdf:resource="http://www.w3.org/2000/01/rdf-schema#Resource"/>
</rdf:Description>

<rdf:Description rdf:about="http://www.environment.gov.au/mapping/rest/services/ogc_services/IMCRA_Mesoscale/MapServer/0/40">
	<rdf:type rdf:resource="http://www.w3.org/2000/01/rdf-schema#Resource"/>
</rdf:Description>

<rdf:Description rdf:about="http://www.environment.gov.au/mapping/rest/services/ogc_services/IMCRA_Mesoscale/MapServer/0/41">
	<rdf:type rdf:resource="http://www.w3.org/2000/01/rdf-schema#Resource"/>
</rdf:Description>

<rdf:Description rdf:about="http://www.environment.gov.au/mapping/rest/services/ogc_services/IMCRA_Mesoscale/MapServer/0/45">
	<rdf:type rdf:resource="http://www.w3.org/2000/01/rdf-schema#Resource"/>
</rdf:Description>

<rdf:Description rdf:about="http://www.environment.gov.au/mapping/rest/services/ogc_services/IMCRA_Mesoscale/MapServer/0/42">
	<rdf:type rdf:resource="http://www.w3.org/2000/01/rdf-schema#Resource"/>
</rdf:Description>

<rdf:Description rdf:about="http://www.environment.gov.au/mapping/rest/services/ogc_services/IMCRA_Mesoscale/MapServer/0/43">
	<rdf:type rdf:resource="http://www.w3.org/2000/01/rdf-schema#Resource"/>
</rdf:Description>

<rdf:Description rdf:about="http://www.environment.gov.au/mapping/rest/services/ogc_services/IMCRA_Mesoscale/MapServer/0/46">
	<rdf:type rdf:resource="http://www.w3.org/2000/01/rdf-schema#Resource"/>
</rdf:Description>

<rdf:Description rdf:about="http://www.environment.gov.au/mapping/rest/services/ogc_services/IMCRA_Mesoscale/MapServer/0/47">
	<rdf:type rdf:resource="http://www.w3.org/2000/01/rdf-schema#Resource"/>
</rdf:Description>

<rdf:Description rdf:about="http://www.environment.gov.au/mapping/rest/services/ogc_services/IMCRA_Mesoscale/MapServer/0/49">
	<rdf:type rdf:resource="http://www.w3.org/2000/01/rdf-schema#Resource"/>
</rdf:Description>

<rdf:Description rdf:about="http://www.environment.gov.au/mapping/rest/services/ogc_services/IMCRA_Mesoscale/MapServer/0/39">
	<rdf:type rdf:resource="http://www.w3.org/2000/01/rdf-schema#Resource"/>
</rdf:Description>

<rdf:Description rdf:about="http://www.environment.gov.au/mapping/rest/services/ogc_services/IMCRA_Provincial/MapServer/0/29">
	<rdf:type rdf:resource="http://www.w3.org/2000/01/rdf-schema#Resource"/>
</rdf:Description>

<rdf:Description rdf:about="http://www.environment.gov.au/mapping/rest/services/ogc_services/IMCRA_Provincial/MapServer/0/31">
	<rdf:type rdf:resource="http://www.w3.org/2000/01/rdf-schema#Resource"/>
</rdf:Description>

<rdf:Description rdf:about="http://seamapaustralia.org.au/def/benthichabitatclassification/class/279">
	<rdf:type rdf:resource="http://www.w3.org/2000/01/rdf-schema#Resource"/>
	<rdf:type rdf:resource="http://www.w3.org/2004/02/skos/core#Concept"/>
	<skos:broader rdf:resource="http://seamapaustralia.org.au/def/benthichabitatclassification/class/120"/>
	<skos:prefLabel xml:lang="en">IMCRA Southwest Transition</skos:prefLabel>
	<dcterms:contributor rdf:resource="http://editor.vocabs.ands.org.au/user/eMII_Finney.Kim_Admin"/>
	<dcterms:created rdf:datatype="http://www.w3.org/2001/XMLSchema#dateTime">2017-06-13T23:26:38Z</dcterms:created>
	<dcterms:creator rdf:resource="http://editor.vocabs.ands.org.au/user/eMII_Finney.Kim_Admin"/>
	<dcterms:modified rdf:datatype="http://www.w3.org/2001/XMLSchema#dateTime">2017-06-13T23:55:14Z</dcterms:modified>
	<dc:publisher rdf:datatype="http://www.w3.org/2001/XMLSchema#string">Institute for Marine and Antarctic Studies (IMAS) - UTAS</dc:publisher>
	<skos:definition xml:lang="en">An IMCRA provincial bioregion reflects biogeographic patterns in distributions of bottom-dwelling fish. Provincial bioregions were defined for the continental shelf for IMCRA v3.3, and for the continental slope for the National Marine Bioregionalisation using similar analytical techniques. In both cases the distributions of demersal (bottom-dwelling) fish were plotted onto a line divided into equally spaced sections. The number of species in each section and the similarity between sections were calculated using a statistical tool called the Jaccard Index. Where the Jaccard Index changed greatly between sections a boundary was defined indicating differences in species assemblages between regions. Two types of provincial bioregions are defined in the IMCRA benthic bioregionalisation: provinces, which represent regions of biotic endemism; and transitions, which generally occur between the provinces, and are less well-defined mixing areas that capture the overlap of demersal fish species ranges between the provinces.</skos:definition>
	<dc:source rdf:datatype="http://www.w3.org/2001/XMLSchema#string">Commonwealth of Australia (2006). A Guide to the Integrated Marine and Coastal Regionalisation of Australia Version 4.0. Department of the Environment and Heritage, Canberra, Australia.</dc:source>
	<skos:narrower rdf:resource="http://seamapaustralia.org.au/def/benthichabitatclassification/class/280"/>
	<skos:narrower rdf:resource="http://seamapaustralia.org.au/def/benthichabitatclassification/class/281"/>
	<skos:exactMatch rdf:resource="http://www.environment.gov.au/mapping/rest/services/ogc_services/IMCRA_Provincial/MapServer/0/30"/>
</rdf:Description>

<rdf:Description rdf:about="http://seamapaustralia.org.au/def/benthichabitatclassification/class/280">
	<rdf:type rdf:resource="http://www.w3.org/2000/01/rdf-schema#Resource"/>
	<rdf:type rdf:resource="http://www.w3.org/2004/02/skos/core#Concept"/>
	<skos:broader rdf:resource="http://seamapaustralia.org.au/def/benthichabitatclassification/class/279"/>
	<skos:prefLabel xml:lang="en">IMCRA Abrolhos Islands Bioregion</skos:prefLabel>
	<dcterms:contributor rdf:resource="http://editor.vocabs.ands.org.au/user/eMII_Finney.Kim_Admin"/>
	<dcterms:created rdf:datatype="http://www.w3.org/2001/XMLSchema#dateTime">2017-06-13T23:27:06Z</dcterms:created>
	<dcterms:creator rdf:resource="http://editor.vocabs.ands.org.au/user/eMII_Finney.Kim_Admin"/>
	<dcterms:modified rdf:datatype="http://www.w3.org/2001/XMLSchema#dateTime">2017-06-13T23:56:51Z</dcterms:modified>
	<dc:publisher rdf:datatype="http://www.w3.org/2001/XMLSchema#string">Institute for Marine and Antarctic Studies (IMAS) - UTAS</dc:publisher>
	<skos:definition xml:lang="en">An inshore regionalisation of Australian waters derived from biological and physical data, including the distribution of demersal fishes, marine plants and invertebrates, sea floor geomorphology and sediments, and oceanographic data. The meso-scale regionalisation was compiled from information supplied to the Australian Government Department of the Environment and Heritage by the relevant State, Northern Territory and Commonwealth marine research and management agencies. The seaward extent for the meso-scale IMCRA coverage is defined by the 200m isobath except where this boundary extends beyond the Australian Exclusive Economic Zone (AEEZ).</skos:definition>
	<dc:source rdf:datatype="http://www.w3.org/2001/XMLSchema#string">Commonwealth of Australia (2006). A Guide to the Integrated Marine and Coastal Regionalisation of Australia Version 4.0. Department of the Environment and Heritage, Canberra, Australia.</dc:source>
	<skos:exactMatch rdf:resource="http://www.environment.gov.au/mapping/rest/services/ogc_services/IMCRA_Mesoscale/MapServer/0/37"/>
</rdf:Description>

<rdf:Description rdf:about="http://seamapaustralia.org.au/def/benthichabitatclassification/class/281">
	<rdf:type rdf:resource="http://www.w3.org/2000/01/rdf-schema#Resource"/>
	<rdf:type rdf:resource="http://www.w3.org/2004/02/skos/core#Concept"/>
	<skos:broader rdf:resource="http://seamapaustralia.org.au/def/benthichabitatclassification/class/279"/>
	<skos:prefLabel xml:lang="en">IMCRA Central West Coast Bioregion</skos:prefLabel>
	<dcterms:contributor rdf:resource="http://editor.vocabs.ands.org.au/user/eMII_Finney.Kim_Admin"/>
	<dcterms:created rdf:datatype="http://www.w3.org/2001/XMLSchema#dateTime">2017-06-13T23:28:41Z</dcterms:created>
	<dcterms:creator rdf:resource="http://editor.vocabs.ands.org.au/user/eMII_Finney.Kim_Admin"/>
	<dcterms:modified rdf:datatype="http://www.w3.org/2001/XMLSchema#dateTime">2017-06-13T23:57:37Z</dcterms:modified>
	<dc:publisher rdf:datatype="http://www.w3.org/2001/XMLSchema#string">Institute for Marine and Antarctic Studies (IMAS) - UTAS</dc:publisher>
	<skos:definition xml:lang="en">An inshore regionalisation of Australian waters derived from biological and physical data, including the distribution of demersal fishes, marine plants and invertebrates, sea floor geomorphology and sediments, and oceanographic data. The meso-scale regionalisation was compiled from information supplied to the Australian Government Department of the Environment and Heritage by the relevant State, Northern Territory and Commonwealth marine research and management agencies. The seaward extent for the meso-scale IMCRA coverage is defined by the 200m isobath except where this boundary extends beyond the Australian Exclusive Economic Zone (AEEZ).</skos:definition>
	<dc:source rdf:datatype="http://www.w3.org/2001/XMLSchema#string">Commonwealth of Australia (2006). A Guide to the Integrated Marine and Coastal Regionalisation of Australia Version 4.0. Department of the Environment and Heritage, Canberra, Australia.</dc:source>
	<skos:exactMatch rdf:resource="http://www.environment.gov.au/mapping/rest/services/ogc_services/IMCRA_Mesoscale/MapServer/0/36"/>
</rdf:Description>

<rdf:Description rdf:about="http://seamapaustralia.org.au/def/benthichabitatclassification/class/282">
	<rdf:type rdf:resource="http://www.w3.org/2000/01/rdf-schema#Resource"/>
	<rdf:type rdf:resource="http://www.w3.org/2004/02/skos/core#Concept"/>
	<skos:broader rdf:resource="http://seamapaustralia.org.au/def/benthichabitatclassification/class/120"/>
	<skos:prefLabel xml:lang="en">IMCRA Central Western Province</skos:prefLabel>
	<dcterms:contributor rdf:resource="http://editor.vocabs.ands.org.au/user/eMII_Finney.Kim_Admin"/>
	<dcterms:created rdf:datatype="http://www.w3.org/2001/XMLSchema#dateTime">2017-06-13T23:43:47Z</dcterms:created>
	<dcterms:creator rdf:resource="http://editor.vocabs.ands.org.au/user/eMII_Finney.Kim_Admin"/>
	<dcterms:modified rdf:datatype="http://www.w3.org/2001/XMLSchema#dateTime">2017-06-13T23:52:54Z</dcterms:modified>
	<dc:publisher rdf:datatype="http://www.w3.org/2001/XMLSchema#string">Institute for Marine and Antarctic Studies (IMAS) - UTAS</dc:publisher>
	<skos:definition xml:lang="en">An IMCRA provincial bioregion reflects biogeographic patterns in distributions of bottom-dwelling fish. Provincial bioregions were defined for the continental shelf for IMCRA v3.3, and for the continental slope for the National Marine Bioregionalisation using similar analytical techniques. In both cases the distributions of demersal (bottom-dwelling) fish were plotted onto a line divided into equally spaced sections. The number of species in each section and the similarity between sections were calculated using a statistical tool called the Jaccard Index. Where the Jaccard Index changed greatly between sections a boundary was defined indicating differences in species assemblages between regions. Two types of provincial bioregions are defined in the IMCRA benthic bioregionalisation: provinces, which represent regions of biotic endemism; and transitions, which generally occur between the provinces, and are less well-defined mixing areas that capture the overlap of demersal fish species ranges between the provinces.</skos:definition>
	<dc:source rdf:datatype="http://www.w3.org/2001/XMLSchema#string">Commonwealth of Australia (2006). A Guide to the Integrated Marine and Coastal Regionalisation of Australia Version 4.0. Department of the Environment and Heritage, Canberra, Australia.</dc:source>
	<skos:narrower rdf:resource="http://seamapaustralia.org.au/def/benthichabitatclassification/class/283"/>
	<skos:narrower rdf:resource="http://seamapaustralia.org.au/def/benthichabitatclassification/class/284"/>
	<skos:exactMatch rdf:resource="http://www.environment.gov.au/mapping/rest/services/ogc_services/IMCRA_Provincial/MapServer/0/20"/>
</rdf:Description>

<rdf:Description rdf:about="http://seamapaustralia.org.au/def/benthichabitatclassification/class/283">
	<rdf:type rdf:resource="http://www.w3.org/2000/01/rdf-schema#Resource"/>
	<rdf:type rdf:resource="http://www.w3.org/2004/02/skos/core#Concept"/>
	<skos:broader rdf:resource="http://seamapaustralia.org.au/def/benthichabitatclassification/class/282"/>
	<skos:prefLabel xml:lang="en">IMCRA Shark Bay Bioregion</skos:prefLabel>
	<dcterms:contributor rdf:resource="http://editor.vocabs.ands.org.au/user/eMII_Finney.Kim_Admin"/>
	<dcterms:created rdf:datatype="http://www.w3.org/2001/XMLSchema#dateTime">2017-06-13T23:44:17Z</dcterms:created>
	<dcterms:creator rdf:resource="http://editor.vocabs.ands.org.au/user/eMII_Finney.Kim_Admin"/>
	<dcterms:modified rdf:datatype="http://www.w3.org/2001/XMLSchema#dateTime">2017-06-13T23:53:29Z</dcterms:modified>
	<dc:publisher rdf:datatype="http://www.w3.org/2001/XMLSchema#string">Institute for Marine and Antarctic Studies (IMAS) - UTAS</dc:publisher>
	<skos:definition xml:lang="en">An inshore regionalisation of Australian waters derived from biological and physical data, including the distribution of demersal fishes, marine plants and invertebrates, sea floor geomorphology and sediments, and oceanographic data. The meso-scale regionalisation was compiled from information supplied to the Australian Government Department of the Environment and Heritage by the relevant State, Northern Territory and Commonwealth marine research and management agencies. The seaward extent for the meso-scale IMCRA coverage is defined by the 200m isobath except where this boundary extends beyond the Australian Exclusive Economic Zone (AEEZ).</skos:definition>
	<dc:source rdf:datatype="http://www.w3.org/2001/XMLSchema#string">Commonwealth of Australia (2006). A Guide to the Integrated Marine and Coastal Regionalisation of Australia Version 4.0. Department of the Environment and Heritage, Canberra, Australia.</dc:source>
	<skos:exactMatch rdf:resource="http://www.environment.gov.au/mapping/rest/services/ogc_services/IMCRA_Mesoscale/MapServer/0/35"/>
</rdf:Description>

<rdf:Description rdf:about="http://seamapaustralia.org.au/def/benthichabitatclassification/class/284">
	<rdf:type rdf:resource="http://www.w3.org/2000/01/rdf-schema#Resource"/>
	<rdf:type rdf:resource="http://www.w3.org/2004/02/skos/core#Concept"/>
	<skos:broader rdf:resource="http://seamapaustralia.org.au/def/benthichabitatclassification/class/282"/>
	<skos:prefLabel xml:lang="en">IMCRA Zuytdorp Bioregion</skos:prefLabel>
	<dcterms:contributor rdf:resource="http://editor.vocabs.ands.org.au/user/eMII_Finney.Kim_Admin"/>
	<dcterms:created rdf:datatype="http://www.w3.org/2001/XMLSchema#dateTime">2017-06-13T23:44:43Z</dcterms:created>
	<dcterms:creator rdf:resource="http://editor.vocabs.ands.org.au/user/eMII_Finney.Kim_Admin"/>
	<dcterms:modified rdf:datatype="http://www.w3.org/2001/XMLSchema#dateTime">2017-06-13T23:54:29Z</dcterms:modified>
	<dc:publisher rdf:datatype="http://www.w3.org/2001/XMLSchema#string">Institute for Marine and Antarctic Studies (IMAS) - UTAS</dc:publisher>
	<skos:definition xml:lang="en">An inshore regionalisation of Australian waters derived from biological and physical data, including the distribution of demersal fishes, marine plants and invertebrates, sea floor geomorphology and sediments, and oceanographic data. The meso-scale regionalisation was compiled from information supplied to the Australian Government Department of the Environment and Heritage by the relevant State, Northern Territory and Commonwealth marine research and management agencies. The seaward extent for the meso-scale IMCRA coverage is defined by the 200m isobath except where this boundary extends beyond the Australian Exclusive Economic Zone (AEEZ).</skos:definition>
	<dc:source rdf:datatype="http://www.w3.org/2001/XMLSchema#string">Commonwealth of Australia (2006). A Guide to the Integrated Marine and Coastal Regionalisation of Australia Version 4.0. Department of the Environment and Heritage, Canberra, Australia.</dc:source>
	<skos:exactMatch rdf:resource="http://www.environment.gov.au/mapping/rest/services/ogc_services/IMCRA_Mesoscale/MapServer/0/33"/>
</rdf:Description>

<rdf:Description rdf:about="http://www.environment.gov.au/mapping/rest/services/ogc_services/IMCRA_Provincial/MapServer/0/20">
	<rdf:type rdf:resource="http://www.w3.org/2000/01/rdf-schema#Resource"/>
</rdf:Description>

<rdf:Description rdf:about="http://www.environment.gov.au/mapping/rest/services/ogc_services/IMCRA_Provincial/MapServer/0/30">
	<rdf:type rdf:resource="http://www.w3.org/2000/01/rdf-schema#Resource"/>
</rdf:Description>

<rdf:Description rdf:about="http://www.environment.gov.au/mapping/rest/services/ogc_services/IMCRA_Mesoscale/MapServer/0/35">
	<rdf:type rdf:resource="http://www.w3.org/2000/01/rdf-schema#Resource"/>
</rdf:Description>

<rdf:Description rdf:about="http://www.environment.gov.au/mapping/rest/services/ogc_services/IMCRA_Mesoscale/MapServer/0/33">
	<rdf:type rdf:resource="http://www.w3.org/2000/01/rdf-schema#Resource"/>
</rdf:Description>

<rdf:Description rdf:about="http://www.environment.gov.au/mapping/rest/services/ogc_services/IMCRA_Mesoscale/MapServer/0/37">
	<rdf:type rdf:resource="http://www.w3.org/2000/01/rdf-schema#Resource"/>
</rdf:Description>

<rdf:Description rdf:about="http://www.environment.gov.au/mapping/rest/services/ogc_services/IMCRA_Mesoscale/MapServer/0/36">
	<rdf:type rdf:resource="http://www.w3.org/2000/01/rdf-schema#Resource"/>
</rdf:Description>

<rdf:Description rdf:about="http://seamapaustralia.org.au/def/benthichabitatclassification/class/285">
	<rdf:type rdf:resource="http://www.w3.org/2000/01/rdf-schema#Resource"/>
	<rdf:type rdf:resource="http://www.w3.org/2004/02/skos/core#Concept"/>
	<skos:broader rdf:resource="http://seamapaustralia.org.au/def/benthichabitatclassification/class/227"/>
	<skos:prefLabel xml:lang="en">IMCRA Central Eastern Province</skos:prefLabel>
	<dcterms:contributor rdf:resource="http://editor.vocabs.ands.org.au/user/eMII_Finney.Kim_Admin"/>
	<dcterms:created rdf:datatype="http://www.w3.org/2001/XMLSchema#dateTime">2017-06-13T23:59:07Z</dcterms:created>
	<dcterms:creator rdf:resource="http://editor.vocabs.ands.org.au/user/eMII_Finney.Kim_Admin"/>
	<dcterms:modified rdf:datatype="http://www.w3.org/2001/XMLSchema#dateTime">2017-06-14T00:10:30Z</dcterms:modified>
	<dc:publisher rdf:datatype="http://www.w3.org/2001/XMLSchema#string">Institute for Marine and Antarctic Studies (IMAS) - UTAS</dc:publisher>
	<skos:definition xml:lang="en">An IMCRA provincial bioregion reflects biogeographic patterns in distributions of bottom-dwelling fish. Provincial bioregions were defined for the continental shelf for IMCRA v3.3, and for the continental slope for the National Marine Bioregionalisation using similar analytical techniques. In both cases the distributions of demersal (bottom-dwelling) fish were plotted onto a line divided into equally spaced sections. The number of species in each section and the similarity between sections were calculated using a statistical tool called the Jaccard Index. Where the Jaccard Index changed greatly between sections a boundary was defined indicating differences in species assemblages between regions. Two types of provincial bioregions are defined in the IMCRA benthic bioregionalisation: provinces, which represent regions of biotic endemism; and transitions, which generally occur between the provinces, and are less well-defined mixing areas that capture the overlap of demersal fish species ranges between the provinces.</skos:definition>
	<dc:source rdf:datatype="http://www.w3.org/2001/XMLSchema#string">Commonwealth of Australia (2006). A Guide to the Integrated Marine and Coastal Regionalisation of Australia Version 4.0. Department of the Environment and Heritage, Canberra, Australia.</dc:source>
	<skos:narrower rdf:resource="http://seamapaustralia.org.au/def/benthichabitatclassification/class/286"/>
	<skos:narrower rdf:resource="http://seamapaustralia.org.au/def/benthichabitatclassification/class/287"/>
	<skos:exactMatch rdf:resource="http://www.environment.gov.au/mapping/rest/services/ogc_services/IMCRA_Provincial/MapServer/0/28"/>
</rdf:Description>

<rdf:Description rdf:about="http://seamapaustralia.org.au/def/benthichabitatclassification/class/286">
	<rdf:type rdf:resource="http://www.w3.org/2000/01/rdf-schema#Resource"/>
	<rdf:type rdf:resource="http://www.w3.org/2004/02/skos/core#Concept"/>
	<skos:broader rdf:resource="http://seamapaustralia.org.au/def/benthichabitatclassification/class/285"/>
	<skos:prefLabel xml:lang="en">IMCRA Manning Shelf Bioregion</skos:prefLabel>
	<dcterms:contributor rdf:resource="http://editor.vocabs.ands.org.au/user/eMII_Finney.Kim_Admin"/>
	<dcterms:created rdf:datatype="http://www.w3.org/2001/XMLSchema#dateTime">2017-06-13T23:59:26Z</dcterms:created>
	<dcterms:creator rdf:resource="http://editor.vocabs.ands.org.au/user/eMII_Finney.Kim_Admin"/>
	<dcterms:modified rdf:datatype="http://www.w3.org/2001/XMLSchema#dateTime">2017-06-14T00:11:36Z</dcterms:modified>
	<dc:publisher rdf:datatype="http://www.w3.org/2001/XMLSchema#string">Institute for Marine and Antarctic Studies (IMAS) - UTAS</dc:publisher>
	<skos:definition xml:lang="en">An inshore regionalisation of Australian waters derived from biological and physical data, including the distribution of demersal fishes, marine plants and invertebrates, sea floor geomorphology and sediments, and oceanographic data. The meso-scale regionalisation was compiled from information supplied to the Australian Government Department of the Environment and Heritage by the relevant State, Northern Territory and Commonwealth marine research and management agencies. The seaward extent for the meso-scale IMCRA coverage is defined by the 200m isobath except where this boundary extends beyond the Australian Exclusive Economic Zone (AEEZ).</skos:definition>
	<dc:source rdf:datatype="http://www.w3.org/2001/XMLSchema#string">Commonwealth of Australia (2006). A Guide to the Integrated Marine and Coastal Regionalisation of Australia Version 4.0. Department of the Environment and Heritage, Canberra, Australia.</dc:source>
	<skos:exactMatch rdf:resource="http://www.environment.gov.au/mapping/rest/services/ogc_services/IMCRA_Mesoscale/MapServer/0/38"/>
</rdf:Description>

<rdf:Description rdf:about="http://seamapaustralia.org.au/def/benthichabitatclassification/class/287">
	<rdf:type rdf:resource="http://www.w3.org/2000/01/rdf-schema#Resource"/>
	<rdf:type rdf:resource="http://www.w3.org/2004/02/skos/core#Concept"/>
	<skos:broader rdf:resource="http://seamapaustralia.org.au/def/benthichabitatclassification/class/285"/>
	<skos:prefLabel xml:lang="en">IMCRA Hawkesbury Shelf Bioregion</skos:prefLabel>
	<dcterms:contributor rdf:resource="http://editor.vocabs.ands.org.au/user/eMII_Finney.Kim_Admin"/>
	<dcterms:created rdf:datatype="http://www.w3.org/2001/XMLSchema#dateTime">2017-06-14T00:00:01Z</dcterms:created>
	<dcterms:creator rdf:resource="http://editor.vocabs.ands.org.au/user/eMII_Finney.Kim_Admin"/>
	<dcterms:modified rdf:datatype="http://www.w3.org/2001/XMLSchema#dateTime">2017-06-14T00:11:07Z</dcterms:modified>
	<dc:publisher rdf:datatype="http://www.w3.org/2001/XMLSchema#string">Institute for Marine and Antarctic Studies (IMAS) - UTAS</dc:publisher>
	<skos:definition xml:lang="en">An inshore regionalisation of Australian waters derived from biological and physical data, including the distribution of demersal fishes, marine plants and invertebrates, sea floor geomorphology and sediments, and oceanographic data. The meso-scale regionalisation was compiled from information supplied to the Australian Government Department of the Environment and Heritage by the relevant State, Northern Territory and Commonwealth marine research and management agencies. The seaward extent for the meso-scale IMCRA coverage is defined by the 200m isobath except where this boundary extends beyond the Australian Exclusive Economic Zone (AEEZ).</skos:definition>
	<dc:source rdf:datatype="http://www.w3.org/2001/XMLSchema#string">Commonwealth of Australia (2006). A Guide to the Integrated Marine and Coastal Regionalisation of Australia Version 4.0. Department of the Environment and Heritage, Canberra, Australia.</dc:source>
	<skos:exactMatch rdf:resource="http://www.environment.gov.au/mapping/rest/services/ogc_services/IMCRA_Mesoscale/MapServer/0/44"/>
</rdf:Description>

<rdf:Description rdf:about="http://seamapaustralia.org.au/def/benthichabitatclassification/class/288">
	<rdf:type rdf:resource="http://www.w3.org/2000/01/rdf-schema#Resource"/>
	<rdf:type rdf:resource="http://www.w3.org/2004/02/skos/core#Concept"/>
	<skos:broader rdf:resource="http://seamapaustralia.org.au/def/benthichabitatclassification/class/226"/>
	<skos:prefLabel xml:lang="en">IMCRA Central Eastern Transition</skos:prefLabel>
	<dcterms:contributor rdf:resource="http://editor.vocabs.ands.org.au/user/eMII_Finney.Kim_Admin"/>
	<dcterms:created rdf:datatype="http://www.w3.org/2001/XMLSchema#dateTime">2017-06-14T00:00:38Z</dcterms:created>
	<dcterms:creator rdf:resource="http://editor.vocabs.ands.org.au/user/eMII_Finney.Kim_Admin"/>
	<dcterms:modified rdf:datatype="http://www.w3.org/2001/XMLSchema#dateTime">2017-06-14T00:12:13Z</dcterms:modified>
	<dc:publisher rdf:datatype="http://www.w3.org/2001/XMLSchema#string">Institute for Marine and Antarctic Studies (IMAS) - UTAS</dc:publisher>
	<skos:definition xml:lang="en">An IMCRA provincial bioregion reflects biogeographic patterns in distributions of bottom-dwelling fish. Provincial bioregions were defined for the continental shelf for IMCRA v3.3, and for the continental slope for the National Marine Bioregionalisation using similar analytical techniques. In both cases the distributions of demersal (bottom-dwelling) fish were plotted onto a line divided into equally spaced sections. The number of species in each section and the similarity between sections were calculated using a statistical tool called the Jaccard Index. Where the Jaccard Index changed greatly between sections a boundary was defined indicating differences in species assemblages between regions. Two types of provincial bioregions are defined in the IMCRA benthic bioregionalisation: provinces, which represent regions of biotic endemism; and transitions, which generally occur between the provinces, and are less well-defined mixing areas that capture the overlap of demersal fish species ranges between the provinces.</skos:definition>
	<dc:source rdf:datatype="http://www.w3.org/2001/XMLSchema#string">Commonwealth of Australia (2006). A Guide to the Integrated Marine and Coastal Regionalisation of Australia Version 4.0. Department of the Environment and Heritage, Canberra, Australia.</dc:source>
	<skos:narrower rdf:resource="http://seamapaustralia.org.au/def/benthichabitatclassification/class/289"/>
	<skos:exactMatch rdf:resource="http://www.environment.gov.au/mapping/rest/services/ogc_services/IMCRA_Provincial/MapServer/0/19"/>
</rdf:Description>

<rdf:Description rdf:about="http://seamapaustralia.org.au/def/benthichabitatclassification/class/289">
	<rdf:type rdf:resource="http://www.w3.org/2000/01/rdf-schema#Resource"/>
	<rdf:type rdf:resource="http://www.w3.org/2004/02/skos/core#Concept"/>
	<skos:broader rdf:resource="http://seamapaustralia.org.au/def/benthichabitatclassification/class/288"/>
	<skos:prefLabel xml:lang="en">IMCRA Tweed-Moreton Bioregion</skos:prefLabel>
	<dcterms:contributor rdf:resource="http://editor.vocabs.ands.org.au/user/eMII_Finney.Kim_Admin"/>
	<dcterms:created rdf:datatype="http://www.w3.org/2001/XMLSchema#dateTime">2017-06-14T00:01:02Z</dcterms:created>
	<dcterms:creator rdf:resource="http://editor.vocabs.ands.org.au/user/eMII_Finney.Kim_Admin"/>
	<dcterms:modified rdf:datatype="http://www.w3.org/2001/XMLSchema#dateTime">2017-06-14T00:12:49Z</dcterms:modified>
	<dc:publisher rdf:datatype="http://www.w3.org/2001/XMLSchema#string">Institute for Marine and Antarctic Studies (IMAS) - UTAS</dc:publisher>
	<skos:definition xml:lang="en">An inshore regionalisation of Australian waters derived from biological and physical data, including the distribution of demersal fishes, marine plants and invertebrates, sea floor geomorphology and sediments, and oceanographic data. The meso-scale regionalisation was compiled from information supplied to the Australian Government Department of the Environment and Heritage by the relevant State, Northern Territory and Commonwealth marine research and management agencies. The seaward extent for the meso-scale IMCRA coverage is defined by the 200m isobath except where this boundary extends beyond the Australian Exclusive Economic Zone (AEEZ).</skos:definition>
	<dc:source rdf:datatype="http://www.w3.org/2001/XMLSchema#string">Commonwealth of Australia (2006). A Guide to the Integrated Marine and Coastal Regionalisation of Australia Version 4.0. Department of the Environment and Heritage, Canberra, Australia.</dc:source>
	<skos:exactMatch rdf:resource="http://www.environment.gov.au/mapping/rest/services/ogc_services/IMCRA_Mesoscale/MapServer/0/34"/>
	<skos:scopeNote xml:lang="en">A very small section of this bioregion falls within the MEOW Manning-Hawkesbury Ecoregion.</skos:scopeNote>
</rdf:Description>

<rdf:Description rdf:about="http://www.environment.gov.au/mapping/rest/services/ogc_services/IMCRA_Provincial/MapServer/0/28">
	<rdf:type rdf:resource="http://www.w3.org/2000/01/rdf-schema#Resource"/>
</rdf:Description>

<rdf:Description rdf:about="http://www.environment.gov.au/mapping/rest/services/ogc_services/IMCRA_Provincial/MapServer/0/19">
	<rdf:type rdf:resource="http://www.w3.org/2000/01/rdf-schema#Resource"/>
</rdf:Description>

<rdf:Description rdf:about="http://www.environment.gov.au/mapping/rest/services/ogc_services/IMCRA_Mesoscale/MapServer/0/44">
	<rdf:type rdf:resource="http://www.w3.org/2000/01/rdf-schema#Resource"/>
</rdf:Description>

<rdf:Description rdf:about="http://www.environment.gov.au/mapping/rest/services/ogc_services/IMCRA_Mesoscale/MapServer/0/38">
	<rdf:type rdf:resource="http://www.w3.org/2000/01/rdf-schema#Resource"/>
</rdf:Description>

<rdf:Description rdf:about="http://www.environment.gov.au/mapping/rest/services/ogc_services/IMCRA_Mesoscale/MapServer/0/34">
	<rdf:type rdf:resource="http://www.w3.org/2000/01/rdf-schema#Resource"/>
</rdf:Description>

<rdf:Description rdf:about="http://seamapaustralia.org.au/def/benthichabitatclassification/class/290">
	<rdf:type rdf:resource="http://www.w3.org/2000/01/rdf-schema#Resource"/>
	<rdf:type rdf:resource="http://www.w3.org/2004/02/skos/core#Concept"/>
	<skos:broader rdf:resource="http://seamapaustralia.org.au/def/benthichabitatclassification/class/187"/>
	<skos:prefLabel xml:lang="en">IMCRA Northwest Province</skos:prefLabel>
	<dcterms:contributor rdf:resource="http://editor.vocabs.ands.org.au/user/eMII_Finney.Kim_Admin"/>
	<dcterms:created rdf:datatype="http://www.w3.org/2001/XMLSchema#dateTime">2017-06-14T01:06:00Z</dcterms:created>
	<dcterms:creator rdf:resource="http://editor.vocabs.ands.org.au/user/eMII_Finney.Kim_Admin"/>
	<dcterms:modified rdf:datatype="http://www.w3.org/2001/XMLSchema#dateTime">2017-06-14T05:17:29Z</dcterms:modified>
	<dc:publisher rdf:datatype="http://www.w3.org/2001/XMLSchema#string">  Institute for Marine and Antarctic Studies (IMAS) - UTAS</dc:publisher>
	<skos:definition xml:lang="en">An IMCRA provincial bioregion reflects biogeographic patterns in distributions of bottom-dwelling fish. Provincial bioregions were defined for the continental shelf for IMCRA v3.3, and for the continental slope for the National Marine Bioregionalisation using similar analytical techniques. In both cases the distributions of demersal (bottom-dwelling) fish were plotted onto a line divided into equally spaced sections. The number of species in each section and the similarity between sections were calculated using a statistical tool called the Jaccard Index. Where the Jaccard Index changed greatly between sections a boundary was defined indicating differences in species assemblages between regions. Two types of provincial bioregions are defined in the IMCRA benthic bioregionalisation: provinces, which represent regions of biotic endemism; and transitions, which generally occur between the provinces, and are less well-defined mixing areas that capture the overlap of demersal fish species ranges between the provinces.</skos:definition>
	<dc:source rdf:datatype="http://www.w3.org/2001/XMLSchema#string">Commonwealth of Australia (2006). A Guide to the Integrated Marine and Coastal Regionalisation of Australia Version 4.0. Department of the Environment and Heritage, Canberra, Australia.</dc:source>
	<skos:narrower rdf:resource="http://seamapaustralia.org.au/def/benthichabitatclassification/class/291"/>
	<skos:narrower rdf:resource="http://seamapaustralia.org.au/def/benthichabitatclassification/class/292"/>
	<skos:narrower rdf:resource="http://seamapaustralia.org.au/def/benthichabitatclassification/class/293"/>
	<skos:narrower rdf:resource="http://seamapaustralia.org.au/def/benthichabitatclassification/class/294"/>
	<skos:narrower rdf:resource="http://seamapaustralia.org.au/def/benthichabitatclassification/class/295"/>
	<skos:exactMatch rdf:resource="http://www.environment.gov.au/mapping/rest/services/ogc_services/IMCRA_Provincial/MapServer/0/15"/>
</rdf:Description>

<rdf:Description rdf:about="http://seamapaustralia.org.au/def/benthichabitatclassification/class/291">
	<rdf:type rdf:resource="http://www.w3.org/2000/01/rdf-schema#Resource"/>
	<rdf:type rdf:resource="http://www.w3.org/2004/02/skos/core#Concept"/>
	<skos:broader rdf:resource="http://seamapaustralia.org.au/def/benthichabitatclassification/class/290"/>
	<skos:prefLabel xml:lang="en">IMCRA Pilbarra (near-shore) Bioregion</skos:prefLabel>
	<dcterms:contributor rdf:resource="http://editor.vocabs.ands.org.au/user/eMII_Finney.Kim_Admin"/>
	<dcterms:created rdf:datatype="http://www.w3.org/2001/XMLSchema#dateTime">2017-06-14T01:06:25Z</dcterms:created>
	<dcterms:creator rdf:resource="http://editor.vocabs.ands.org.au/user/eMII_Finney.Kim_Admin"/>
	<dcterms:modified rdf:datatype="http://www.w3.org/2001/XMLSchema#dateTime">2017-06-14T05:22:56Z</dcterms:modified>
	<dc:publisher rdf:datatype="http://www.w3.org/2001/XMLSchema#string">  Institute for Marine and Antarctic Studies (IMAS) - UTAS</dc:publisher>
	<skos:definition xml:lang="en">An inshore regionalisation of Australian waters derived from biological and physical data, including the distribution of demersal fishes, marine plants and invertebrates, sea floor geomorphology and sediments, and oceanographic data. The meso-scale regionalisation was compiled from information supplied to the Australian Government Department of the Environment and Heritage by the relevant State, Northern Territory and Commonwealth marine research and management agencies. The seaward extent for the meso-scale IMCRA coverage is defined by the 200m isobath except where this boundary extends beyond the Australian Exclusive Economic Zone (AEEZ).</skos:definition>
	<dc:source rdf:datatype="http://www.w3.org/2001/XMLSchema#string">Commonwealth of Australia (2006). A Guide to the Integrated Marine and Coastal Regionalisation of Australia Version 4.0. Department of the Environment and Heritage, Canberra, Australia.</dc:source>
	<skos:exactMatch rdf:resource="http://www.environment.gov.au/mapping/rest/services/ogc_services/IMCRA_Mesoscale/MapServer/0/30"/>
</rdf:Description>

<rdf:Description rdf:about="http://seamapaustralia.org.au/def/benthichabitatclassification/class/292">
	<rdf:type rdf:resource="http://www.w3.org/2000/01/rdf-schema#Resource"/>
	<rdf:type rdf:resource="http://www.w3.org/2004/02/skos/core#Concept"/>
	<skos:broader rdf:resource="http://seamapaustralia.org.au/def/benthichabitatclassification/class/290"/>
	<skos:prefLabel xml:lang="en">IMCRA Pilbarra (off-shore) Bioregion</skos:prefLabel>
	<dcterms:contributor rdf:resource="http://editor.vocabs.ands.org.au/user/eMII_Finney.Kim_Admin"/>
	<dcterms:created rdf:datatype="http://www.w3.org/2001/XMLSchema#dateTime">2017-06-14T01:06:47Z</dcterms:created>
	<dcterms:creator rdf:resource="http://editor.vocabs.ands.org.au/user/eMII_Finney.Kim_Admin"/>
	<dcterms:modified rdf:datatype="http://www.w3.org/2001/XMLSchema#dateTime">2017-06-14T05:23:48Z</dcterms:modified>
	<dc:publisher rdf:datatype="http://www.w3.org/2001/XMLSchema#string">  Institute for Marine and Antarctic Studies (IMAS) - UTAS</dc:publisher>
	<skos:definition xml:lang="en">An inshore regionalisation of Australian waters derived from biological and physical data, including the distribution of demersal fishes, marine plants and invertebrates, sea floor geomorphology and sediments, and oceanographic data. The meso-scale regionalisation was compiled from information supplied to the Australian Government Department of the Environment and Heritage by the relevant State, Northern Territory and Commonwealth marine research and management agencies. The seaward extent for the meso-scale IMCRA coverage is defined by the 200m isobath except where this boundary extends beyond the Australian Exclusive Economic Zone (AEEZ).</skos:definition>
	<dc:source rdf:datatype="http://www.w3.org/2001/XMLSchema#string">Commonwealth of Australia (2006). A Guide to the Integrated Marine and Coastal Regionalisation of Australia Version 4.0. Department of the Environment and Heritage, Canberra, Australia.</dc:source>
	<skos:exactMatch rdf:resource="http://www.environment.gov.au/mapping/rest/services/ogc_services/IMCRA_Mesoscale/MapServer/0/28"/>
</rdf:Description>

<rdf:Description rdf:about="http://www.environment.gov.au/mapping/rest/services/ogc_services/IMCRA_Mesoscale/MapServer/0/28">
	<rdf:type rdf:resource="http://www.w3.org/2000/01/rdf-schema#Resource"/>
</rdf:Description>

<rdf:Description rdf:about="http://seamapaustralia.org.au/def/benthichabitatclassification/class/293">
	<rdf:type rdf:resource="http://www.w3.org/2000/01/rdf-schema#Resource"/>
	<rdf:type rdf:resource="http://www.w3.org/2004/02/skos/core#Concept"/>
	<skos:broader rdf:resource="http://seamapaustralia.org.au/def/benthichabitatclassification/class/290"/>
	<skos:prefLabel xml:lang="en">IMCRA Eighty Mile Beach Bioregion</skos:prefLabel>
	<dcterms:contributor rdf:resource="http://editor.vocabs.ands.org.au/user/eMII_Finney.Kim_Admin"/>
	<dcterms:created rdf:datatype="http://www.w3.org/2001/XMLSchema#dateTime">2017-06-14T01:07:11Z</dcterms:created>
	<dcterms:creator rdf:resource="http://editor.vocabs.ands.org.au/user/eMII_Finney.Kim_Admin"/>
	<dcterms:modified rdf:datatype="http://www.w3.org/2001/XMLSchema#dateTime">2017-06-14T05:20:05Z</dcterms:modified>
	<dc:publisher rdf:datatype="http://www.w3.org/2001/XMLSchema#string">  Institute for Marine and Antarctic Studies (IMAS) - UTAS</dc:publisher>
	<skos:definition xml:lang="en">An inshore regionalisation of Australian waters derived from biological and physical data, including the distribution of demersal fishes, marine plants and invertebrates, sea floor geomorphology and sediments, and oceanographic data. The meso-scale regionalisation was compiled from information supplied to the Australian Government Department of the Environment and Heritage by the relevant State, Northern Territory and Commonwealth marine research and management agencies. The seaward extent for the meso-scale IMCRA coverage is defined by the 200m isobath except where this boundary extends beyond the Australian Exclusive Economic Zone (AEEZ).</skos:definition>
	<dc:source rdf:datatype="http://www.w3.org/2001/XMLSchema#string">Commonwealth of Australia (2006). A Guide to the Integrated Marine and Coastal Regionalisation of Australia Version 4.0. Department of the Environment and Heritage, Canberra, Australia.</dc:source>
	<skos:exactMatch rdf:resource="http://www.environment.gov.au/mapping/rest/services/ogc_services/IMCRA_Mesoscale/MapServer/0/26"/>
</rdf:Description>

<rdf:Description rdf:about="http://seamapaustralia.org.au/def/benthichabitatclassification/class/294">
	<rdf:type rdf:resource="http://www.w3.org/2000/01/rdf-schema#Resource"/>
	<rdf:type rdf:resource="http://www.w3.org/2004/02/skos/core#Concept"/>
	<skos:broader rdf:resource="http://seamapaustralia.org.au/def/benthichabitatclassification/class/290"/>
	<skos:prefLabel xml:lang="en">IMCRA Canning Bioregion</skos:prefLabel>
	<dcterms:contributor rdf:resource="http://editor.vocabs.ands.org.au/user/eMII_Finney.Kim_Admin"/>
	<dcterms:created rdf:datatype="http://www.w3.org/2001/XMLSchema#dateTime">2017-06-14T01:07:27Z</dcterms:created>
	<dcterms:creator rdf:resource="http://editor.vocabs.ands.org.au/user/eMII_Finney.Kim_Admin"/>
	<dcterms:modified rdf:datatype="http://www.w3.org/2001/XMLSchema#dateTime">2017-06-14T05:19:31Z</dcterms:modified>
	<dc:publisher rdf:datatype="http://www.w3.org/2001/XMLSchema#string">  Institute for Marine and Antarctic Studies (IMAS) - UTAS</dc:publisher>
	<skos:definition xml:lang="en">An inshore regionalisation of Australian waters derived from biological and physical data, including the distribution of demersal fishes, marine plants and invertebrates, sea floor geomorphology and sediments, and oceanographic data. The meso-scale regionalisation was compiled from information supplied to the Australian Government Department of the Environment and Heritage by the relevant State, Northern Territory and Commonwealth marine research and management agencies. The seaward extent for the meso-scale IMCRA coverage is defined by the 200m isobath except where this boundary extends beyond the Australian Exclusive Economic Zone (AEEZ).</skos:definition>
	<dc:source rdf:datatype="http://www.w3.org/2001/XMLSchema#string">Commonwealth of Australia (2006). A Guide to the Integrated Marine and Coastal Regionalisation of Australia Version 4.0. Department of the Environment and Heritage, Canberra, Australia.</dc:source>
	<skos:exactMatch rdf:resource="http://www.environment.gov.au/mapping/rest/services/ogc_services/IMCRA_Mesoscale/MapServer/0/22"/>
</rdf:Description>

<rdf:Description rdf:about="http://seamapaustralia.org.au/def/benthichabitatclassification/class/295">
	<rdf:type rdf:resource="http://www.w3.org/2000/01/rdf-schema#Resource"/>
	<rdf:type rdf:resource="http://www.w3.org/2004/02/skos/core#Concept"/>
	<skos:broader rdf:resource="http://seamapaustralia.org.au/def/benthichabitatclassification/class/290"/>
	<skos:prefLabel xml:lang="en">IMCRA Northwest Shelf Bioregion</skos:prefLabel>
	<dcterms:contributor rdf:resource="http://editor.vocabs.ands.org.au/user/eMII_Finney.Kim_Admin"/>
	<dcterms:created rdf:datatype="http://www.w3.org/2001/XMLSchema#dateTime">2017-06-14T01:07:46Z</dcterms:created>
	<dcterms:creator rdf:resource="http://editor.vocabs.ands.org.au/user/eMII_Finney.Kim_Admin"/>
	<dcterms:modified rdf:datatype="http://www.w3.org/2001/XMLSchema#dateTime">2017-06-14T05:20:41Z</dcterms:modified>
	<dc:publisher rdf:datatype="http://www.w3.org/2001/XMLSchema#string">  Institute for Marine and Antarctic Studies (IMAS) - UTAS</dc:publisher>
	<skos:definition xml:lang="en">An inshore regionalisation of Australian waters derived from biological and physical data, including the distribution of demersal fishes, marine plants and invertebrates, sea floor geomorphology and sediments, and oceanographic data. The meso-scale regionalisation was compiled from information supplied to the Australian Government Department of the Environment and Heritage by the relevant State, Northern Territory and Commonwealth marine research and management agencies. The seaward extent for the meso-scale IMCRA coverage is defined by the 200m isobath except where this boundary extends beyond the Australian Exclusive Economic Zone (AEEZ).</skos:definition>
	<dc:source rdf:datatype="http://www.w3.org/2001/XMLSchema#string">Commonwealth of Australia (2006). A Guide to the Integrated Marine and Coastal Regionalisation of Australia Version 4.0. Department of the Environment and Heritage, Canberra, Australia.</dc:source>
	<skos:exactMatch rdf:resource="http://www.environment.gov.au/mapping/rest/services/ogc_services/IMCRA_Mesoscale/MapServer/0/17"/>
</rdf:Description>

<rdf:Description rdf:about="http://seamapaustralia.org.au/def/benthichabitatclassification/class/296">
	<rdf:type rdf:resource="http://www.w3.org/2000/01/rdf-schema#Resource"/>
	<rdf:type rdf:resource="http://www.w3.org/2004/02/skos/core#Concept"/>
	<skos:broader rdf:resource="http://seamapaustralia.org.au/def/benthichabitatclassification/class/188"/>
	<skos:prefLabel xml:lang="en">IMCRA Central Western Transition</skos:prefLabel>
	<dcterms:contributor rdf:resource="http://editor.vocabs.ands.org.au/user/eMII_Finney.Kim_Admin"/>
	<dcterms:created rdf:datatype="http://www.w3.org/2001/XMLSchema#dateTime">2017-06-14T01:08:17Z</dcterms:created>
	<dcterms:creator rdf:resource="http://editor.vocabs.ands.org.au/user/eMII_Finney.Kim_Admin"/>
	<dcterms:modified rdf:datatype="http://www.w3.org/2001/XMLSchema#dateTime">2017-06-14T05:18:26Z</dcterms:modified>
	<dc:publisher rdf:datatype="http://www.w3.org/2001/XMLSchema#string">  Institute for Marine and Antarctic Studies (IMAS) - UTAS</dc:publisher>
	<skos:definition xml:lang="en">An IMCRA provincial bioregion reflects biogeographic patterns in distributions of bottom-dwelling fish. Provincial bioregions were defined for the continental shelf for IMCRA v3.3, and for the continental slope for the National Marine Bioregionalisation using similar analytical techniques. In both cases the distributions of demersal (bottom-dwelling) fish were plotted onto a line divided into equally spaced sections. The number of species in each section and the similarity between sections were calculated using a statistical tool called the Jaccard Index. Where the Jaccard Index changed greatly between sections a boundary was defined indicating differences in species assemblages between regions. Two types of provincial bioregions are defined in the IMCRA benthic bioregionalisation: provinces, which represent regions of biotic endemism; and transitions, which generally occur between the provinces, and are less well-defined mixing areas that capture the overlap of demersal fish species ranges between the provinces.</skos:definition>
	<dc:source rdf:datatype="http://www.w3.org/2001/XMLSchema#string">Commonwealth of Australia (2006). A Guide to the Integrated Marine and Coastal Regionalisation of Australia Version 4.0. Department of the Environment and Heritage, Canberra, Australia.</dc:source>
	<skos:narrower rdf:resource="http://seamapaustralia.org.au/def/benthichabitatclassification/class/297"/>
	<skos:exactMatch rdf:resource="http://www.environment.gov.au/mapping/rest/services/ogc_services/IMCRA_Provincial/MapServer/0/17"/>
</rdf:Description>

<rdf:Description rdf:about="http://www.environment.gov.au/mapping/rest/services/ogc_services/IMCRA_Provincial/MapServer/0/15">
	<rdf:type rdf:resource="http://www.w3.org/2000/01/rdf-schema#Resource"/>
</rdf:Description>

<rdf:Description rdf:about="http://www.environment.gov.au/mapping/rest/services/ogc_services/IMCRA_Provincial/MapServer/0/17">
	<rdf:type rdf:resource="http://www.w3.org/2000/01/rdf-schema#Resource"/>
</rdf:Description>

<rdf:Description rdf:about="http://www.environment.gov.au/mapping/rest/services/ogc_services/IMCRA_Mesoscale/MapServer/0/22">
	<rdf:type rdf:resource="http://www.w3.org/2000/01/rdf-schema#Resource"/>
</rdf:Description>

<rdf:Description rdf:about="http://www.environment.gov.au/mapping/rest/services/ogc_services/IMCRA_Mesoscale/MapServer/0/26">
	<rdf:type rdf:resource="http://www.w3.org/2000/01/rdf-schema#Resource"/>
</rdf:Description>

<rdf:Description rdf:about="http://www.environment.gov.au/mapping/rest/services/ogc_services/IMCRA_Mesoscale/MapServer/0/17">
	<rdf:type rdf:resource="http://www.w3.org/2000/01/rdf-schema#Resource"/>
</rdf:Description>

<rdf:Description rdf:about="http://www.environment.gov.au/mapping/rest/services/ogc_services/IMCRA_Mesoscale/MapServer/0/30">
	<rdf:type rdf:resource="http://www.w3.org/2000/01/rdf-schema#Resource"/>
</rdf:Description>

<rdf:Description rdf:about="http://www.environment.gov.au/mapping/rest/services/ogc_services/IMCRA_Mesoscale/MapServer/0/32">
	<rdf:type rdf:resource="http://www.w3.org/2000/01/rdf-schema#Resource"/>
</rdf:Description>

<rdf:Description rdf:about="http://www.environment.gov.au/mapping/rest/services/ogc_services/IMCRA_Mesoscale/MapServer/0/15">
	<rdf:type rdf:resource="http://www.w3.org/2000/01/rdf-schema#Resource"/>
</rdf:Description>

<rdf:Description rdf:about="http://seamapaustralia.org.au/def/benthichabitatclassification/class/328">
	<rdf:type rdf:resource="http://www.w3.org/2000/01/rdf-schema#Resource"/>
	<rdf:type rdf:resource="http://www.w3.org/2004/02/skos/core#Concept"/>
	<skos:broader rdf:resource="http://seamapaustralia.org.au/def/benthichabitatclassification/class/327"/>
	<skos:prefLabel xml:lang="en">Coral</skos:prefLabel>
	<dcterms:contributor rdf:resource="http://editor.vocabs.ands.org.au/user/eMII_Finney.Kim_Admin"/>
	<dcterms:created rdf:datatype="http://www.w3.org/2001/XMLSchema#dateTime">2017-06-27T01:31:33Z</dcterms:created>
	<dcterms:creator rdf:resource="http://editor.vocabs.ands.org.au/user/eMII_Finney.Kim_Admin"/>
	<dcterms:modified rdf:datatype="http://www.w3.org/2001/XMLSchema#dateTime">2017-06-27T01:31:42Z</dcterms:modified>
	<skos:definition xml:lang="en">A biogenic substratum that is dominated by non-living scleractinian coral. Living coral may be present, but these are described under the Biotic Component.</skos:definition>
</rdf:Description>

<rdf:Description rdf:about="http://purl.org/dc/terms/issued">
	<rdf:type rdf:resource="http://www.w3.org/1999/02/22-rdf-syntax-ns#Property"/>
	<rdf:type rdf:resource="http://www.w3.org/2000/01/rdf-schema#Resource"/>
	<rdfs:subPropertyOf rdf:resource="http://purl.org/dc/terms/issued"/>
</rdf:Description>

<rdf:Description rdf:about="http://www.w3.org/2002/07/owl#versionInfo">
	<rdf:type rdf:resource="http://www.w3.org/1999/02/22-rdf-syntax-ns#Property"/>
	<rdf:type rdf:resource="http://www.w3.org/2000/01/rdf-schema#Resource"/>
	<rdfs:subPropertyOf rdf:resource="http://www.w3.org/2002/07/owl#versionInfo"/>
</rdf:Description>

</rdf:RDF>