<?xml version="1.0" encoding="UTF-8"?>
<rdf:RDF
	xmlns="http://schema.semantic-web.at/ppt/"
	xmlns:tags="http://www.holygoat.co.uk/owl/redwood/0.1/tags/"
	xmlns:dc="http://purl.org/dc/elements/1.1/"
	xmlns:foaf="http://xmlns.com/foaf/0.1/"
	xmlns:dcterms="http://purl.org/dc/terms/"
	xmlns:rdfs="http://www.w3.org/2000/01/rdf-schema#"
	xmlns:cycAnnot="http://sw.cyc.com/CycAnnotations_v1#"
	xmlns:ctag="http://commontag.org/ns#"
	xmlns:owl="http://www.w3.org/2002/07/owl#"
	xmlns:dbpedia="http://dbpedia.org/resource/"
	xmlns:xsd="http://www.w3.org/2001/XMLSchema#"
	xmlns:rdf="http://www.w3.org/1999/02/22-rdf-syntax-ns#"
	xmlns:freebase="http://rdf.freebase.com/ns/"
	xmlns:csw="http://semantic-web.at/ontologies/csw.owl#"
	xmlns:cyc="http://sw.cyc.com/concept/"
	xmlns:sesame="http://www.openrdf.org/schema/sesame#"
	xmlns:fn="http://www.w3.org/2005/xpath-functions#"
	xmlns:skos="http://www.w3.org/2004/02/skos/core#"
	xmlns:opencyc="http://sw.opencyc.org/concept/">

<rdf:Description rdf:about="http://www.w3.org/1999/02/22-rdf-syntax-ns#type">
	<rdf:type rdf:resource="http://www.w3.org/1999/02/22-rdf-syntax-ns#Property"/>
	<rdf:type rdf:resource="http://www.w3.org/2000/01/rdf-schema#Resource"/>
	<rdfs:domain rdf:resource="http://www.w3.org/2000/01/rdf-schema#Resource"/>
	<rdfs:range rdf:resource="http://www.w3.org/2000/01/rdf-schema#Class"/>
	<rdfs:subPropertyOf rdf:resource="http://www.w3.org/1999/02/22-rdf-syntax-ns#type"/>
</rdf:Description>

<rdf:Description rdf:about="http://www.w3.org/1999/02/22-rdf-syntax-ns#Property">
	<rdf:type rdf:resource="http://www.w3.org/2000/01/rdf-schema#Resource"/>
	<rdf:type rdf:resource="http://www.w3.org/2000/01/rdf-schema#Class"/>
	<rdfs:subClassOf rdf:resource="http://www.w3.org/1999/02/22-rdf-syntax-ns#Property"/>
	<rdfs:subClassOf rdf:resource="http://www.w3.org/2000/01/rdf-schema#Resource"/>
</rdf:Description>

<rdf:Description rdf:about="http://www.w3.org/1999/02/22-rdf-syntax-ns#subject">
	<rdf:type rdf:resource="http://www.w3.org/1999/02/22-rdf-syntax-ns#Property"/>
	<rdf:type rdf:resource="http://www.w3.org/2000/01/rdf-schema#Resource"/>
	<rdfs:domain rdf:resource="http://www.w3.org/1999/02/22-rdf-syntax-ns#Statement"/>
	<rdfs:range rdf:resource="http://www.w3.org/2000/01/rdf-schema#Resource"/>
	<rdfs:subPropertyOf rdf:resource="http://www.w3.org/1999/02/22-rdf-syntax-ns#subject"/>
</rdf:Description>

<rdf:Description rdf:about="http://www.w3.org/1999/02/22-rdf-syntax-ns#predicate">
	<rdf:type rdf:resource="http://www.w3.org/1999/02/22-rdf-syntax-ns#Property"/>
	<rdf:type rdf:resource="http://www.w3.org/2000/01/rdf-schema#Resource"/>
	<rdfs:domain rdf:resource="http://www.w3.org/1999/02/22-rdf-syntax-ns#Statement"/>
	<rdfs:range rdf:resource="http://www.w3.org/2000/01/rdf-schema#Resource"/>
	<rdfs:subPropertyOf rdf:resource="http://www.w3.org/1999/02/22-rdf-syntax-ns#predicate"/>
</rdf:Description>

<rdf:Description rdf:about="http://www.w3.org/1999/02/22-rdf-syntax-ns#object">
	<rdf:type rdf:resource="http://www.w3.org/1999/02/22-rdf-syntax-ns#Property"/>
	<rdf:type rdf:resource="http://www.w3.org/2000/01/rdf-schema#Resource"/>
	<rdfs:domain rdf:resource="http://www.w3.org/1999/02/22-rdf-syntax-ns#Statement"/>
	<rdfs:range rdf:resource="http://www.w3.org/2000/01/rdf-schema#Resource"/>
	<rdfs:subPropertyOf rdf:resource="http://www.w3.org/1999/02/22-rdf-syntax-ns#object"/>
</rdf:Description>

<rdf:Description rdf:about="http://www.w3.org/1999/02/22-rdf-syntax-ns#first">
	<rdf:type rdf:resource="http://www.w3.org/1999/02/22-rdf-syntax-ns#Property"/>
	<rdf:type rdf:resource="http://www.w3.org/2000/01/rdf-schema#Resource"/>
	<rdfs:domain rdf:resource="http://www.w3.org/1999/02/22-rdf-syntax-ns#List"/>
	<rdfs:range rdf:resource="http://www.w3.org/2000/01/rdf-schema#Resource"/>
	<rdfs:subPropertyOf rdf:resource="http://www.w3.org/1999/02/22-rdf-syntax-ns#first"/>
</rdf:Description>

<rdf:Description rdf:about="http://www.w3.org/1999/02/22-rdf-syntax-ns#rest">
	<rdf:type rdf:resource="http://www.w3.org/1999/02/22-rdf-syntax-ns#Property"/>
	<rdf:type rdf:resource="http://www.w3.org/2000/01/rdf-schema#Resource"/>
	<rdfs:domain rdf:resource="http://www.w3.org/1999/02/22-rdf-syntax-ns#List"/>
	<rdfs:range rdf:resource="http://www.w3.org/1999/02/22-rdf-syntax-ns#List"/>
	<rdfs:subPropertyOf rdf:resource="http://www.w3.org/1999/02/22-rdf-syntax-ns#rest"/>
</rdf:Description>

<rdf:Description rdf:about="http://www.w3.org/1999/02/22-rdf-syntax-ns#value">
	<rdf:type rdf:resource="http://www.w3.org/1999/02/22-rdf-syntax-ns#Property"/>
	<rdf:type rdf:resource="http://www.w3.org/2000/01/rdf-schema#Resource"/>
	<rdfs:domain rdf:resource="http://www.w3.org/2000/01/rdf-schema#Resource"/>
	<rdfs:range rdf:resource="http://www.w3.org/2000/01/rdf-schema#Resource"/>
	<rdfs:subPropertyOf rdf:resource="http://www.w3.org/1999/02/22-rdf-syntax-ns#value"/>
</rdf:Description>

<rdf:Description rdf:about="http://www.w3.org/1999/02/22-rdf-syntax-ns#nil">
	<rdf:type rdf:resource="http://www.w3.org/1999/02/22-rdf-syntax-ns#List"/>
	<rdf:type rdf:resource="http://www.w3.org/2000/01/rdf-schema#Resource"/>
</rdf:Description>

<rdf:Description rdf:about="http://www.w3.org/1999/02/22-rdf-syntax-ns#List">
	<rdf:type rdf:resource="http://www.w3.org/2000/01/rdf-schema#Resource"/>
	<rdf:type rdf:resource="http://www.w3.org/2000/01/rdf-schema#Class"/>
	<rdfs:subClassOf rdf:resource="http://www.w3.org/1999/02/22-rdf-syntax-ns#List"/>
	<rdfs:subClassOf rdf:resource="http://www.w3.org/2000/01/rdf-schema#Resource"/>
</rdf:Description>

<rdf:Description rdf:about="http://www.w3.org/2000/01/rdf-schema#domain">
	<rdf:type rdf:resource="http://www.w3.org/1999/02/22-rdf-syntax-ns#Property"/>
	<rdf:type rdf:resource="http://www.w3.org/2000/01/rdf-schema#Resource"/>
	<rdfs:domain rdf:resource="http://www.w3.org/1999/02/22-rdf-syntax-ns#Property"/>
	<rdfs:range rdf:resource="http://www.w3.org/2000/01/rdf-schema#Class"/>
	<rdfs:subPropertyOf rdf:resource="http://www.w3.org/2000/01/rdf-schema#domain"/>
</rdf:Description>

<rdf:Description rdf:about="http://www.w3.org/2000/01/rdf-schema#Resource">
	<rdf:type rdf:resource="http://www.w3.org/2000/01/rdf-schema#Resource"/>
	<rdf:type rdf:resource="http://www.w3.org/2000/01/rdf-schema#Class"/>
	<rdfs:subClassOf rdf:resource="http://www.w3.org/2000/01/rdf-schema#Resource"/>
</rdf:Description>

<rdf:Description rdf:about="http://www.w3.org/2000/01/rdf-schema#range">
	<rdf:type rdf:resource="http://www.w3.org/1999/02/22-rdf-syntax-ns#Property"/>
	<rdf:type rdf:resource="http://www.w3.org/2000/01/rdf-schema#Resource"/>
	<rdfs:domain rdf:resource="http://www.w3.org/1999/02/22-rdf-syntax-ns#Property"/>
	<rdfs:range rdf:resource="http://www.w3.org/2000/01/rdf-schema#Class"/>
	<rdfs:subPropertyOf rdf:resource="http://www.w3.org/2000/01/rdf-schema#range"/>
</rdf:Description>

<rdf:Description rdf:about="http://www.w3.org/2000/01/rdf-schema#subPropertyOf">
	<rdf:type rdf:resource="http://www.w3.org/1999/02/22-rdf-syntax-ns#Property"/>
	<rdf:type rdf:resource="http://www.w3.org/2000/01/rdf-schema#Resource"/>
	<rdfs:domain rdf:resource="http://www.w3.org/1999/02/22-rdf-syntax-ns#Property"/>
	<rdfs:range rdf:resource="http://www.w3.org/1999/02/22-rdf-syntax-ns#Property"/>
	<rdfs:subPropertyOf rdf:resource="http://www.w3.org/2000/01/rdf-schema#subPropertyOf"/>
</rdf:Description>

<rdf:Description rdf:about="http://www.w3.org/2000/01/rdf-schema#subClassOf">
	<rdf:type rdf:resource="http://www.w3.org/1999/02/22-rdf-syntax-ns#Property"/>
	<rdf:type rdf:resource="http://www.w3.org/2000/01/rdf-schema#Resource"/>
	<rdfs:domain rdf:resource="http://www.w3.org/2000/01/rdf-schema#Class"/>
	<rdfs:range rdf:resource="http://www.w3.org/2000/01/rdf-schema#Class"/>
	<rdfs:subPropertyOf rdf:resource="http://www.w3.org/2000/01/rdf-schema#subClassOf"/>
</rdf:Description>

<rdf:Description rdf:about="http://www.w3.org/2000/01/rdf-schema#Class">
	<rdf:type rdf:resource="http://www.w3.org/2000/01/rdf-schema#Resource"/>
	<rdf:type rdf:resource="http://www.w3.org/2000/01/rdf-schema#Class"/>
	<rdfs:subClassOf rdf:resource="http://www.w3.org/2000/01/rdf-schema#Resource"/>
	<rdfs:subClassOf rdf:resource="http://www.w3.org/2000/01/rdf-schema#Class"/>
</rdf:Description>

<rdf:Description rdf:about="http://www.w3.org/1999/02/22-rdf-syntax-ns#Statement">
	<rdf:type rdf:resource="http://www.w3.org/2000/01/rdf-schema#Resource"/>
	<rdf:type rdf:resource="http://www.w3.org/2000/01/rdf-schema#Class"/>
	<rdfs:subClassOf rdf:resource="http://www.w3.org/2000/01/rdf-schema#Resource"/>
	<rdfs:subClassOf rdf:resource="http://www.w3.org/1999/02/22-rdf-syntax-ns#Statement"/>
</rdf:Description>

<rdf:Description rdf:about="http://www.w3.org/2000/01/rdf-schema#member">
	<rdf:type rdf:resource="http://www.w3.org/1999/02/22-rdf-syntax-ns#Property"/>
	<rdf:type rdf:resource="http://www.w3.org/2000/01/rdf-schema#Resource"/>
	<rdfs:domain rdf:resource="http://www.w3.org/2000/01/rdf-schema#Resource"/>
	<rdfs:range rdf:resource="http://www.w3.org/2000/01/rdf-schema#Resource"/>
	<rdfs:subPropertyOf rdf:resource="http://www.w3.org/2000/01/rdf-schema#member"/>
</rdf:Description>

<rdf:Description rdf:about="http://www.w3.org/2000/01/rdf-schema#seeAlso">
	<rdf:type rdf:resource="http://www.w3.org/1999/02/22-rdf-syntax-ns#Property"/>
	<rdf:type rdf:resource="http://www.w3.org/2000/01/rdf-schema#Resource"/>
	<rdfs:domain rdf:resource="http://www.w3.org/2000/01/rdf-schema#Resource"/>
	<rdfs:range rdf:resource="http://www.w3.org/2000/01/rdf-schema#Resource"/>
	<rdfs:subPropertyOf rdf:resource="http://www.w3.org/2000/01/rdf-schema#seeAlso"/>
</rdf:Description>

<rdf:Description rdf:about="http://www.w3.org/2000/01/rdf-schema#isDefinedBy">
	<rdf:type rdf:resource="http://www.w3.org/1999/02/22-rdf-syntax-ns#Property"/>
	<rdf:type rdf:resource="http://www.w3.org/2000/01/rdf-schema#Resource"/>
	<rdfs:domain rdf:resource="http://www.w3.org/2000/01/rdf-schema#Resource"/>
	<rdfs:range rdf:resource="http://www.w3.org/2000/01/rdf-schema#Resource"/>
	<rdfs:subPropertyOf rdf:resource="http://www.w3.org/2000/01/rdf-schema#seeAlso"/>
	<rdfs:subPropertyOf rdf:resource="http://www.w3.org/2000/01/rdf-schema#isDefinedBy"/>
</rdf:Description>

<rdf:Description rdf:about="http://www.w3.org/2000/01/rdf-schema#comment">
	<rdf:type rdf:resource="http://www.w3.org/1999/02/22-rdf-syntax-ns#Property"/>
	<rdf:type rdf:resource="http://www.w3.org/2000/01/rdf-schema#Resource"/>
	<rdfs:domain rdf:resource="http://www.w3.org/2000/01/rdf-schema#Resource"/>
	<rdfs:range rdf:resource="http://www.w3.org/2000/01/rdf-schema#Literal"/>
	<rdfs:subPropertyOf rdf:resource="http://www.w3.org/2000/01/rdf-schema#comment"/>
</rdf:Description>

<rdf:Description rdf:about="http://www.w3.org/2000/01/rdf-schema#label">
	<rdf:type rdf:resource="http://www.w3.org/1999/02/22-rdf-syntax-ns#Property"/>
	<rdf:type rdf:resource="http://www.w3.org/2000/01/rdf-schema#Resource"/>
	<rdfs:domain rdf:resource="http://www.w3.org/2000/01/rdf-schema#Resource"/>
	<rdfs:range rdf:resource="http://www.w3.org/2000/01/rdf-schema#Literal"/>
	<rdfs:subPropertyOf rdf:resource="http://www.w3.org/2000/01/rdf-schema#label"/>
</rdf:Description>

<rdf:Description rdf:about="http://www.w3.org/2000/01/rdf-schema#Literal">
	<rdf:type rdf:resource="http://www.w3.org/2000/01/rdf-schema#Resource"/>
	<rdf:type rdf:resource="http://www.w3.org/2000/01/rdf-schema#Class"/>
	<rdfs:subClassOf rdf:resource="http://www.w3.org/2000/01/rdf-schema#Resource"/>
	<rdfs:subClassOf rdf:resource="http://www.w3.org/2000/01/rdf-schema#Literal"/>
</rdf:Description>

<rdf:Description rdf:about="http://www.w3.org/1999/02/22-rdf-syntax-ns#Alt">
	<rdf:type rdf:resource="http://www.w3.org/2000/01/rdf-schema#Resource"/>
	<rdf:type rdf:resource="http://www.w3.org/2000/01/rdf-schema#Class"/>
	<rdfs:subClassOf rdf:resource="http://www.w3.org/2000/01/rdf-schema#Resource"/>
	<rdfs:subClassOf rdf:resource="http://www.w3.org/1999/02/22-rdf-syntax-ns#Alt"/>
	<rdfs:subClassOf rdf:resource="http://www.w3.org/2000/01/rdf-schema#Container"/>
</rdf:Description>

<rdf:Description rdf:about="http://www.w3.org/2000/01/rdf-schema#Container">
	<rdf:type rdf:resource="http://www.w3.org/2000/01/rdf-schema#Resource"/>
	<rdf:type rdf:resource="http://www.w3.org/2000/01/rdf-schema#Class"/>
	<rdfs:subClassOf rdf:resource="http://www.w3.org/2000/01/rdf-schema#Resource"/>
	<rdfs:subClassOf rdf:resource="http://www.w3.org/2000/01/rdf-schema#Container"/>
</rdf:Description>

<rdf:Description rdf:about="http://www.w3.org/1999/02/22-rdf-syntax-ns#Bag">
	<rdf:type rdf:resource="http://www.w3.org/2000/01/rdf-schema#Resource"/>
	<rdf:type rdf:resource="http://www.w3.org/2000/01/rdf-schema#Class"/>
	<rdfs:subClassOf rdf:resource="http://www.w3.org/2000/01/rdf-schema#Resource"/>
	<rdfs:subClassOf rdf:resource="http://www.w3.org/2000/01/rdf-schema#Container"/>
	<rdfs:subClassOf rdf:resource="http://www.w3.org/1999/02/22-rdf-syntax-ns#Bag"/>
</rdf:Description>

<rdf:Description rdf:about="http://www.w3.org/1999/02/22-rdf-syntax-ns#Seq">
	<rdf:type rdf:resource="http://www.w3.org/2000/01/rdf-schema#Resource"/>
	<rdf:type rdf:resource="http://www.w3.org/2000/01/rdf-schema#Class"/>
	<rdfs:subClassOf rdf:resource="http://www.w3.org/2000/01/rdf-schema#Resource"/>
	<rdfs:subClassOf rdf:resource="http://www.w3.org/2000/01/rdf-schema#Container"/>
	<rdfs:subClassOf rdf:resource="http://www.w3.org/1999/02/22-rdf-syntax-ns#Seq"/>
</rdf:Description>

<rdf:Description rdf:about="http://www.w3.org/2000/01/rdf-schema#ContainerMembershipProperty">
	<rdf:type rdf:resource="http://www.w3.org/2000/01/rdf-schema#Resource"/>
	<rdf:type rdf:resource="http://www.w3.org/2000/01/rdf-schema#Class"/>
	<rdfs:subClassOf rdf:resource="http://www.w3.org/1999/02/22-rdf-syntax-ns#Property"/>
	<rdfs:subClassOf rdf:resource="http://www.w3.org/2000/01/rdf-schema#Resource"/>
	<rdfs:subClassOf rdf:resource="http://www.w3.org/2000/01/rdf-schema#ContainerMembershipProperty"/>
</rdf:Description>

<rdf:Description rdf:about="http://www.w3.org/1999/02/22-rdf-syntax-ns#XMLLiteral">
	<rdf:type rdf:resource="http://www.w3.org/2000/01/rdf-schema#Resource"/>
	<rdf:type rdf:resource="http://www.w3.org/2000/01/rdf-schema#Class"/>
	<rdf:type rdf:resource="http://www.w3.org/2000/01/rdf-schema#Datatype"/>
	<rdfs:subClassOf rdf:resource="http://www.w3.org/2000/01/rdf-schema#Resource"/>
	<rdfs:subClassOf rdf:resource="http://www.w3.org/2000/01/rdf-schema#Literal"/>
	<rdfs:subClassOf rdf:resource="http://www.w3.org/1999/02/22-rdf-syntax-ns#XMLLiteral"/>
</rdf:Description>

<rdf:Description rdf:about="http://www.w3.org/2000/01/rdf-schema#Datatype">
	<rdf:type rdf:resource="http://www.w3.org/2000/01/rdf-schema#Resource"/>
	<rdf:type rdf:resource="http://www.w3.org/2000/01/rdf-schema#Class"/>
	<rdfs:subClassOf rdf:resource="http://www.w3.org/2000/01/rdf-schema#Resource"/>
	<rdfs:subClassOf rdf:resource="http://www.w3.org/2000/01/rdf-schema#Class"/>
	<rdfs:subClassOf rdf:resource="http://www.w3.org/2000/01/rdf-schema#Datatype"/>
</rdf:Description>

<rdf:Description rdf:about="http://vocab.aodn.org.au/def/organisation/1">
	<rdf:type rdf:resource="http://www.w3.org/2000/01/rdf-schema#Resource"/>
	<rdf:type rdf:resource="http://www.w3.org/2004/02/skos/core#ConceptScheme"/>
	<csw:hierarchyRoot rdf:datatype="http://www.w3.org/2001/XMLSchema#boolean">true</csw:hierarchyRoot>
	<csw:hierarchyRootType rdf:resource="http://www.w3.org/2004/02/skos/core#ConceptScheme"/>
	<dcterms:title xml:lang="en">AODN Organisation Vocabulary</dcterms:title>
	<dcterms:description xml:lang="en">An AODN controlled vocabulary describing organisational entities.</dcterms:description>
	<dcterms:modified rdf:datatype="http://www.w3.org/2001/XMLSchema#dateTime">2015-09-29T03:14:43Z</dcterms:modified>
	<dcterms:modified rdf:datatype="http://www.w3.org/2001/XMLSchema#dateTime">2016-01-07T03:24:43Z</dcterms:modified>
	<dcterms:subject xml:lang="en">organisation</dcterms:subject>
	<dcterms:publisher xml:lang="en">eMarine Information Infrastructure (eMII)</dcterms:publisher>
	<dcterms:creator xml:lang="en">Natalia Atkins</dcterms:creator>
	<dcterms:created rdf:datatype="http://www.w3.org/2001/XMLSchema#dateTime">2015-04-27T10:38:15Z</dcterms:created>
	<dc:rights rdf:datatype="http://www.w3.org/2001/XMLSchema#string">Freely Available For Reuse</dc:rights>
	<identifier rdf:datatype="http://www.w3.org/2001/XMLSchema#string">entity</identifier>
	<skos:hasTopConcept rdf:resource="http://vocab.aodn.org.au/def/organisation/entity/1"/>
	<skos:hasTopConcept rdf:resource="http://vocab.aodn.org.au/def/organisation/entity/8"/>
	<skos:hasTopConcept rdf:resource="http://vocab.aodn.org.au/def/organisation/entity/13"/>
	<skos:hasTopConcept rdf:resource="http://vocab.aodn.org.au/def/organisation/entity/23"/>
	<skos:hasTopConcept rdf:resource="http://vocab.aodn.org.au/def/organisation/entity/24"/>
	<skos:hasTopConcept rdf:resource="http://vocab.aodn.org.au/def/organisation/entity/26"/>
	<skos:hasTopConcept rdf:resource="http://vocab.aodn.org.au/def/organisation/entity/27"/>
	<skos:hasTopConcept rdf:resource="http://vocab.aodn.org.au/def/organisation/entity/28"/>
	<skos:hasTopConcept rdf:resource="http://vocab.aodn.org.au/def/organisation/entity/30"/>
	<skos:hasTopConcept rdf:resource="http://vocab.aodn.org.au/def/organisation/entity/31"/>
	<skos:hasTopConcept rdf:resource="http://vocab.aodn.org.au/def/organisation/entity/32"/>
	<skos:hasTopConcept rdf:resource="http://vocab.aodn.org.au/def/organisation/entity/33"/>
	<skos:hasTopConcept rdf:resource="http://vocab.aodn.org.au/def/organisation/entity/34"/>
	<skos:hasTopConcept rdf:resource="http://vocab.aodn.org.au/def/organisation/entity/35"/>
	<skos:hasTopConcept rdf:resource="http://vocab.aodn.org.au/def/organisation/entity/36"/>
	<skos:hasTopConcept rdf:resource="http://vocab.aodn.org.au/def/organisation/entity/37"/>
	<skos:hasTopConcept rdf:resource="http://vocab.aodn.org.au/def/organisation/entity/38"/>
	<skos:hasTopConcept rdf:resource="http://vocab.aodn.org.au/def/organisation/entity/39"/>
	<skos:hasTopConcept rdf:resource="http://vocab.aodn.org.au/def/organisation/entity/40"/>
	<skos:hasTopConcept rdf:resource="http://vocab.aodn.org.au/def/organisation/entity/41"/>
	<skos:hasTopConcept rdf:resource="http://vocab.aodn.org.au/def/organisation/entity/42"/>
	<skos:hasTopConcept rdf:resource="http://vocab.aodn.org.au/def/organisation/entity/43"/>
	<skos:hasTopConcept rdf:resource="http://vocab.aodn.org.au/def/organisation/entity/44"/>
	<skos:hasTopConcept rdf:resource="http://vocab.aodn.org.au/def/organisation/entity/45"/>
	<skos:hasTopConcept rdf:resource="http://vocab.aodn.org.au/def/organisation/entity/46"/>
	<skos:hasTopConcept rdf:resource="http://vocab.aodn.org.au/def/organisation/entity/47"/>
	<skos:hasTopConcept rdf:resource="http://vocab.aodn.org.au/def/organisation/entity/48"/>
	<skos:hasTopConcept rdf:resource="http://vocab.aodn.org.au/def/organisation/entity/49"/>
	<skos:hasTopConcept rdf:resource="http://vocab.aodn.org.au/def/organisation/entity/50"/>
	<skos:hasTopConcept rdf:resource="http://vocab.aodn.org.au/def/organisation/entity/51"/>
	<skos:hasTopConcept rdf:resource="http://vocab.aodn.org.au/def/organisation/entity/52"/>
	<skos:hasTopConcept rdf:resource="http://vocab.aodn.org.au/def/organisation/entity/53"/>
	<skos:hasTopConcept rdf:resource="http://vocab.aodn.org.au/def/organisation/entity/54"/>
	<skos:hasTopConcept rdf:resource="http://vocab.aodn.org.au/def/organisation/entity/55"/>
	<skos:hasTopConcept rdf:resource="http://vocab.aodn.org.au/def/organisation/entity/56"/>
	<skos:hasTopConcept rdf:resource="http://vocab.aodn.org.au/def/organisation/entity/57"/>
	<skos:hasTopConcept rdf:resource="http://vocab.aodn.org.au/def/organisation/entity/58"/>
	<skos:hasTopConcept rdf:resource="http://vocab.aodn.org.au/def/organisation/entity/59"/>
	<skos:hasTopConcept rdf:resource="http://vocab.aodn.org.au/def/organisation/entity/60"/>
	<skos:hasTopConcept rdf:resource="http://vocab.aodn.org.au/def/organisation/entity/61"/>
	<skos:hasTopConcept rdf:resource="http://vocab.aodn.org.au/def/organisation/entity/62"/>
	<skos:hasTopConcept rdf:resource="http://vocab.aodn.org.au/def/organisation/entity/63"/>
	<skos:hasTopConcept rdf:resource="http://vocab.aodn.org.au/def/organisation/entity/64"/>
	<skos:hasTopConcept rdf:resource="http://vocab.aodn.org.au/def/organisation/entity/65"/>
	<skos:hasTopConcept rdf:resource="http://vocab.aodn.org.au/def/organisation/entity/66"/>
	<skos:hasTopConcept rdf:resource="http://vocab.aodn.org.au/def/organisation/entity/67"/>
	<skos:hasTopConcept rdf:resource="http://vocab.aodn.org.au/def/organisation/entity/69"/>
	<skos:hasTopConcept rdf:resource="http://vocab.aodn.org.au/def/organisation/entity/70"/>
	<skos:hasTopConcept rdf:resource="http://vocab.aodn.org.au/def/organisation/entity/71"/>
	<skos:hasTopConcept rdf:resource="http://vocab.aodn.org.au/def/organisation/entity/72"/>
	<skos:hasTopConcept rdf:resource="http://vocab.aodn.org.au/def/organisation/entity/73"/>
	<skos:hasTopConcept rdf:resource="http://vocab.aodn.org.au/def/organisation/entity/74"/>
	<skos:hasTopConcept rdf:resource="http://vocab.aodn.org.au/def/organisation/entity/75"/>
	<skos:hasTopConcept rdf:resource="http://vocab.aodn.org.au/def/organisation/entity/76"/>
	<skos:hasTopConcept rdf:resource="http://vocab.aodn.org.au/def/organisation/entity/77"/>
	<skos:hasTopConcept rdf:resource="http://vocab.aodn.org.au/def/organisation/entity/78"/>
	<skos:hasTopConcept rdf:resource="http://vocab.aodn.org.au/def/organisation/entity/79"/>
	<skos:hasTopConcept rdf:resource="http://vocab.aodn.org.au/def/organisation/entity/80"/>
	<skos:hasTopConcept rdf:resource="http://vocab.aodn.org.au/def/organisation/entity/81"/>
	<skos:hasTopConcept rdf:resource="http://vocab.aodn.org.au/def/organisation/entity/82"/>
	<skos:hasTopConcept rdf:resource="http://vocab.aodn.org.au/def/organisation/entity/83"/>
	<skos:hasTopConcept rdf:resource="http://vocab.aodn.org.au/def/organisation/entity/84"/>
	<skos:hasTopConcept rdf:resource="http://vocab.aodn.org.au/def/organisation/entity/85"/>
	<skos:hasTopConcept rdf:resource="http://vocab.aodn.org.au/def/organisation/entity/86"/>
	<skos:hasTopConcept rdf:resource="http://vocab.aodn.org.au/def/organisation/entity/87"/>
	<skos:hasTopConcept rdf:resource="http://vocab.aodn.org.au/def/organisation/entity/88"/>
	<skos:hasTopConcept rdf:resource="http://vocab.aodn.org.au/def/organisation/entity/89"/>
	<skos:hasTopConcept rdf:resource="http://vocab.aodn.org.au/def/organisation/entity/90"/>
	<skos:hasTopConcept rdf:resource="http://vocab.aodn.org.au/def/organisation/entity/92"/>
	<skos:hasTopConcept rdf:resource="http://vocab.aodn.org.au/def/organisation/entity/93"/>
	<skos:hasTopConcept rdf:resource="http://vocab.aodn.org.au/def/organisation/entity/94"/>
	<skos:hasTopConcept rdf:resource="http://vocab.aodn.org.au/def/organisation/entity/95"/>
	<skos:hasTopConcept rdf:resource="http://vocab.aodn.org.au/def/organisation/entity/96"/>
	<skos:hasTopConcept rdf:resource="http://vocab.aodn.org.au/def/organisation/entity/97"/>
	<skos:hasTopConcept rdf:resource="http://vocab.aodn.org.au/def/organisation/entity/98"/>
	<skos:hasTopConcept rdf:resource="http://vocab.aodn.org.au/def/organisation/entity/99"/>
	<skos:hasTopConcept rdf:resource="http://vocab.aodn.org.au/def/organisation/entity/100"/>
	<skos:hasTopConcept rdf:resource="http://vocab.aodn.org.au/def/organisation/entity/101"/>
	<skos:hasTopConcept rdf:resource="http://vocab.aodn.org.au/def/organisation/entity/102"/>
	<skos:hasTopConcept rdf:resource="http://vocab.aodn.org.au/def/organisation/entity/103"/>
	<skos:hasTopConcept rdf:resource="http://vocab.aodn.org.au/def/organisation/entity/104"/>
	<skos:hasTopConcept rdf:resource="http://vocab.aodn.org.au/def/organisation/entity/105"/>
	<skos:hasTopConcept rdf:resource="http://vocab.aodn.org.au/def/organisation/entity/106"/>
	<skos:hasTopConcept rdf:resource="http://vocab.aodn.org.au/def/organisation/entity/107"/>
	<skos:hasTopConcept rdf:resource="http://vocab.aodn.org.au/def/organisation/entity/108"/>
	<skos:hasTopConcept rdf:resource="http://vocab.aodn.org.au/def/organisation/entity/109"/>
	<skos:hasTopConcept rdf:resource="http://vocab.aodn.org.au/def/organisation/entity/110"/>
	<skos:hasTopConcept rdf:resource="http://vocab.aodn.org.au/def/organisation/entity/111"/>
	<skos:hasTopConcept rdf:resource="http://vocab.aodn.org.au/def/organisation/entity/112"/>
	<skos:hasTopConcept rdf:resource="http://vocab.aodn.org.au/def/organisation/entity/113"/>
	<skos:hasTopConcept rdf:resource="http://vocab.aodn.org.au/def/organisation/entity/114"/>
	<skos:hasTopConcept rdf:resource="http://vocab.aodn.org.au/def/organisation/entity/115"/>
	<skos:hasTopConcept rdf:resource="http://vocab.aodn.org.au/def/organisation/entity/116"/>
	<skos:hasTopConcept rdf:resource="http://vocab.aodn.org.au/def/organisation/entity/117"/>
	<skos:hasTopConcept rdf:resource="http://vocab.aodn.org.au/def/organisation/entity/118"/>
	<skos:hasTopConcept rdf:resource="http://vocab.aodn.org.au/def/organisation/entity/119"/>
	<skos:hasTopConcept rdf:resource="http://vocab.aodn.org.au/def/organisation/entity/120"/>
	<skos:hasTopConcept rdf:resource="http://vocab.aodn.org.au/def/organisation/entity/121"/>
	<skos:hasTopConcept rdf:resource="http://vocab.aodn.org.au/def/organisation/entity/122"/>
	<skos:hasTopConcept rdf:resource="http://vocab.aodn.org.au/def/organisation/entity/124"/>
	<skos:hasTopConcept rdf:resource="http://vocab.aodn.org.au/def/organisation/entity/125"/>
	<skos:hasTopConcept rdf:resource="http://vocab.aodn.org.au/def/organisation/entity/126"/>
	<skos:hasTopConcept rdf:resource="http://vocab.aodn.org.au/def/organisation/entity/127"/>
	<skos:hasTopConcept rdf:resource="http://vocab.aodn.org.au/def/organisation/entity/128"/>
	<skos:hasTopConcept rdf:resource="http://vocab.aodn.org.au/def/organisation/entity/129"/>
	<skos:hasTopConcept rdf:resource="http://vocab.aodn.org.au/def/organisation/entity/130"/>
	<skos:hasTopConcept rdf:resource="http://vocab.aodn.org.au/def/organisation/entity/131"/>
	<skos:hasTopConcept rdf:resource="http://vocab.aodn.org.au/def/organisation/entity/132"/>
	<skos:hasTopConcept rdf:resource="http://vocab.aodn.org.au/def/organisation/entity/133"/>
	<skos:hasTopConcept rdf:resource="http://vocab.aodn.org.au/def/organisation/entity/168"/>
	<skos:hasTopConcept rdf:resource="http://vocab.aodn.org.au/def/organisation/entity/171"/>
	<skos:hasTopConcept rdf:resource="http://vocab.aodn.org.au/def/organisation/entity/173"/>
	<skos:hasTopConcept rdf:resource="http://vocab.aodn.org.au/def/organisation/entity/174"/>
	<skos:hasTopConcept rdf:resource="http://vocab.aodn.org.au/def/organisation/entity/175"/>
	<skos:hasTopConcept rdf:resource="http://vocab.aodn.org.au/def/organisation/entity/176"/>
	<skos:hasTopConcept rdf:resource="http://vocab.aodn.org.au/def/organisation/entity/177"/>
	<skos:hasTopConcept rdf:resource="http://vocab.aodn.org.au/def/organisation/entity/172"/>
	<skos:hasTopConcept rdf:resource="http://vocab.aodn.org.au/def/organisation/entity/178"/>
	<skos:hasTopConcept rdf:resource="http://vocab.aodn.org.au/def/organisation/entity/189"/>
	<skos:hasTopConcept rdf:resource="http://vocab.aodn.org.au/def/organisation/entity/194"/>
	<skos:hasTopConcept rdf:resource="http://vocab.aodn.org.au/def/organisation/entity/210"/>
	<skos:hasTopConcept rdf:resource="http://vocab.aodn.org.au/def/organisation/entity/215"/>
	<skos:hasTopConcept rdf:resource="http://vocab.aodn.org.au/def/organisation/entity/217"/>
	<skos:hasTopConcept rdf:resource="http://vocab.aodn.org.au/def/organisation/entity/224"/>
	<skos:hasTopConcept rdf:resource="http://vocab.aodn.org.au/def/organisation/entity/235"/>
	<skos:hasTopConcept rdf:resource="http://vocab.aodn.org.au/def/organisation/entity/252"/>
	<skos:hasTopConcept rdf:resource="http://vocab.aodn.org.au/def/organisation/entity/262"/>
	<skos:hasTopConcept rdf:resource="http://vocab.aodn.org.au/def/organisation/entity/263"/>
	<skos:hasTopConcept rdf:resource="http://vocab.aodn.org.au/def/organisation/entity/268"/>
	<skos:hasTopConcept rdf:resource="http://vocab.aodn.org.au/def/organisation/entity/270"/>
	<skos:hasTopConcept rdf:resource="http://vocab.aodn.org.au/def/organisation/entity/274"/>
	<skos:hasTopConcept rdf:resource="http://vocab.aodn.org.au/def/organisation/entity/278"/>
	<skos:hasTopConcept rdf:resource="http://vocab.aodn.org.au/def/organisation/entity/287"/>
	<skos:hasTopConcept rdf:resource="http://vocab.aodn.org.au/def/organisation/entity/398"/>
	<skos:hasTopConcept rdf:resource="http://vocab.aodn.org.au/def/organisation/entity/303"/>
	<skos:hasTopConcept rdf:resource="http://vocab.aodn.org.au/def/organisation/entity/305"/>
	<skos:hasTopConcept rdf:resource="http://vocab.aodn.org.au/def/organisation/entity/307"/>
	<skos:hasTopConcept rdf:resource="http://vocab.aodn.org.au/def/organisation/entity/309"/>
	<skos:hasTopConcept rdf:resource="http://vocab.aodn.org.au/def/organisation/entity/279"/>
	<skos:hasTopConcept rdf:resource="http://vocab.aodn.org.au/def/organisation/entity/289"/>
	<skos:hasTopConcept rdf:resource="http://vocab.aodn.org.au/def/organisation/entity/294"/>
	<skos:hasTopConcept rdf:resource="http://vocab.aodn.org.au/def/organisation/entity/316"/>
	<skos:hasTopConcept rdf:resource="http://vocab.aodn.org.au/def/organisation/entity/318"/>
	<skos:hasTopConcept rdf:resource="http://vocab.aodn.org.au/def/organisation/entity/319"/>
	<skos:hasTopConcept rdf:resource="http://vocab.aodn.org.au/def/organisation/entity/320"/>
	<skos:hasTopConcept rdf:resource="http://vocab.aodn.org.au/def/organisation/entity/321"/>
	<skos:hasTopConcept rdf:resource="http://vocab.aodn.org.au/def/organisation/entity/322"/>
	<skos:hasTopConcept rdf:resource="http://vocab.aodn.org.au/def/organisation/entity/323"/>
	<skos:hasTopConcept rdf:resource="http://vocab.aodn.org.au/def/organisation/entity/324"/>
	<skos:hasTopConcept rdf:resource="http://vocab.aodn.org.au/def/organisation/entity/325"/>
	<skos:hasTopConcept rdf:resource="http://vocab.aodn.org.au/def/organisation/entity/326"/>
	<skos:hasTopConcept rdf:resource="http://vocab.aodn.org.au/def/organisation/entity/327"/>
	<skos:hasTopConcept rdf:resource="http://vocab.aodn.org.au/def/organisation/entity/328"/>
	<skos:hasTopConcept rdf:resource="http://vocab.aodn.org.au/def/organisation/entity/329"/>
	<skos:hasTopConcept rdf:resource="http://vocab.aodn.org.au/def/organisation/entity/330"/>
	<skos:hasTopConcept rdf:resource="http://vocab.aodn.org.au/def/organisation/entity/331"/>
	<skos:hasTopConcept rdf:resource="http://vocab.aodn.org.au/def/organisation/entity/332"/>
	<skos:hasTopConcept rdf:resource="http://vocab.aodn.org.au/def/organisation/entity/333"/>
	<skos:hasTopConcept rdf:resource="http://vocab.aodn.org.au/def/organisation/entity/334"/>
	<skos:hasTopConcept rdf:resource="http://vocab.aodn.org.au/def/organisation/entity/335"/>
	<skos:hasTopConcept rdf:resource="http://vocab.aodn.org.au/def/organisation/entity/337"/>
	<skos:hasTopConcept rdf:resource="http://vocab.aodn.org.au/def/organisation/entity/339"/>
	<skos:hasTopConcept rdf:resource="http://vocab.aodn.org.au/def/organisation/entity/341"/>
	<skos:hasTopConcept rdf:resource="http://vocab.aodn.org.au/def/organisation/entity/343"/>
	<skos:hasTopConcept rdf:resource="http://vocab.aodn.org.au/def/organisation/entity/344"/>
	<skos:hasTopConcept rdf:resource="http://vocab.aodn.org.au/def/organisation/entity/345"/>
	<skos:hasTopConcept rdf:resource="http://vocab.aodn.org.au/def/organisation/entity/346"/>
	<skos:hasTopConcept rdf:resource="http://vocab.aodn.org.au/def/organisation/entity/347"/>
	<skos:hasTopConcept rdf:resource="http://vocab.aodn.org.au/def/organisation/entity/348"/>
	<skos:hasTopConcept rdf:resource="http://vocab.aodn.org.au/def/organisation/entity/349"/>
	<skos:hasTopConcept rdf:resource="http://vocab.aodn.org.au/def/organisation/entity/350"/>
	<skos:hasTopConcept rdf:resource="http://vocab.aodn.org.au/def/organisation/entity/351"/>
	<skos:hasTopConcept rdf:resource="http://vocab.aodn.org.au/def/organisation/entity/352"/>
	<skos:hasTopConcept rdf:resource="http://vocab.aodn.org.au/def/organisation/entity/354"/>
	<skos:hasTopConcept rdf:resource="http://vocab.aodn.org.au/def/organisation/entity/353"/>
	<skos:hasTopConcept rdf:resource="http://vocab.aodn.org.au/def/organisation/entity/360"/>
	<skos:hasTopConcept rdf:resource="http://vocab.aodn.org.au/def/organisation/entity/358"/>
	<skos:hasTopConcept rdf:resource="http://vocab.aodn.org.au/def/organisation/entity/369"/>
	<skos:hasTopConcept rdf:resource="http://vocab.aodn.org.au/def/organisation/entity/366"/>
	<skos:hasTopConcept rdf:resource="http://vocab.aodn.org.au/def/organisation/entity/364"/>
	<skos:hasTopConcept rdf:resource="http://vocab.aodn.org.au/def/organisation/entity/367"/>
	<skos:hasTopConcept rdf:resource="http://vocab.aodn.org.au/def/organisation/entity/355"/>
	<skos:hasTopConcept rdf:resource="http://vocab.aodn.org.au/def/organisation/entity/397"/>
	<skos:hasTopConcept rdf:resource="http://vocab.aodn.org.au/def/organisation/entity/396"/>
	<skos:hasTopConcept rdf:resource="http://vocab.aodn.org.au/def/organisation/entity/395"/>
	<skos:hasTopConcept rdf:resource="http://vocab.aodn.org.au/def/organisation/entity/400"/>
	<skos:hasTopConcept rdf:resource="http://vocab.aodn.org.au/def/organisation/entity/401"/>
	<skos:hasTopConcept rdf:resource="http://vocab.aodn.org.au/def/organisation/entity/402"/>
	<skos:hasTopConcept rdf:resource="http://vocab.aodn.org.au/def/organisation/entity/403"/>
	<skos:hasTopConcept rdf:resource="http://vocab.aodn.org.au/def/organisation/entity/371"/>
	<skos:hasTopConcept rdf:resource="http://vocab.aodn.org.au/def/organisation/entity/372"/>
	<skos:hasTopConcept rdf:resource="http://vocab.aodn.org.au/def/organisation/entity/373"/>
	<skos:hasTopConcept rdf:resource="http://vocab.aodn.org.au/def/organisation/entity/374"/>
	<skos:hasTopConcept rdf:resource="http://vocab.aodn.org.au/def/organisation/entity/375"/>
	<skos:hasTopConcept rdf:resource="http://vocab.aodn.org.au/def/organisation/entity/376"/>
	<skos:hasTopConcept rdf:resource="http://vocab.aodn.org.au/def/organisation/entity/377"/>
	<skos:hasTopConcept rdf:resource="http://vocab.aodn.org.au/def/organisation/entity/378"/>
	<skos:hasTopConcept rdf:resource="http://vocab.aodn.org.au/def/organisation/entity/379"/>
	<skos:hasTopConcept rdf:resource="http://vocab.aodn.org.au/def/organisation/entity/380"/>
	<skos:hasTopConcept rdf:resource="http://vocab.aodn.org.au/def/organisation/entity/381"/>
	<skos:hasTopConcept rdf:resource="http://vocab.aodn.org.au/def/organisation/entity/382"/>
	<skos:hasTopConcept rdf:resource="http://vocab.aodn.org.au/def/organisation/entity/383"/>
	<skos:hasTopConcept rdf:resource="http://vocab.aodn.org.au/def/organisation/entity/384"/>
	<skos:hasTopConcept rdf:resource="http://vocab.aodn.org.au/def/organisation/entity/385"/>
	<skos:hasTopConcept rdf:resource="http://vocab.aodn.org.au/def/organisation/entity/386"/>
	<skos:hasTopConcept rdf:resource="http://vocab.aodn.org.au/def/organisation/entity/387"/>
	<skos:hasTopConcept rdf:resource="http://vocab.aodn.org.au/def/organisation/entity/388"/>
	<skos:hasTopConcept rdf:resource="http://vocab.aodn.org.au/def/organisation/entity/389"/>
	<skos:hasTopConcept rdf:resource="http://vocab.aodn.org.au/def/organisation/entity/390"/>
	<skos:hasTopConcept rdf:resource="http://vocab.aodn.org.au/def/organisation/entity/391"/>
	<skos:hasTopConcept rdf:resource="http://vocab.aodn.org.au/def/organisation/entity/393"/>
	<skos:hasTopConcept rdf:resource="http://vocab.aodn.org.au/def/organisation/entity/394"/>
	<skos:hasTopConcept rdf:resource="http://vocab.aodn.org.au/def/organisation/entity/404"/>
	<skos:hasTopConcept rdf:resource="http://vocab.aodn.org.au/def/organisation/entity/408"/>
	<skos:hasTopConcept rdf:resource="http://vocab.aodn.org.au/def/organisation/entity/409"/>
	<skos:hasTopConcept rdf:resource="http://vocab.aodn.org.au/def/organisation/entity/412"/>
	<skos:hasTopConcept rdf:resource="http://vocab.aodn.org.au/def/organisation/entity/413"/>
	<skos:hasTopConcept rdf:resource="http://vocab.aodn.org.au/def/organisation/entity/414"/>
	<skos:hasTopConcept rdf:resource="http://vocab.aodn.org.au/def/organisation/entity/415"/>
	<skos:hasTopConcept rdf:resource="http://vocab.aodn.org.au/def/organisation/entity/416"/>
	<skos:hasTopConcept rdf:resource="http://vocab.aodn.org.au/def/organisation/entity/417"/>
	<skos:hasTopConcept rdf:resource="http://vocab.aodn.org.au/def/organisation/entity/418"/>
	<skos:hasTopConcept rdf:resource="http://vocab.aodn.org.au/def/organisation/entity/420"/>
	<skos:hasTopConcept rdf:resource="http://vocab.aodn.org.au/def/organisation/entity/424"/>
	<skos:hasTopConcept rdf:resource="http://vocab.aodn.org.au/def/organisation/entity/431"/>
	<skos:hasTopConcept rdf:resource="http://vocab.aodn.org.au/def/organisation/entity/436"/>
	<skos:hasTopConcept rdf:resource="http://vocab.aodn.org.au/def/organisation/entity/440"/>
	<skos:hasTopConcept rdf:resource="http://vocab.aodn.org.au/def/organisation/entity/443"/>
	<skos:hasTopConcept rdf:resource="http://vocab.aodn.org.au/def/organisation/entity/444"/>
	<skos:hasTopConcept rdf:resource="http://vocab.aodn.org.au/def/organisation/entity/445"/>
	<skos:hasTopConcept rdf:resource="http://vocab.aodn.org.au/def/organisation/entity/446"/>
	<skos:hasTopConcept rdf:resource="http://vocab.aodn.org.au/def/organisation/entity/449"/>
	<skos:hasTopConcept rdf:resource="http://vocab.aodn.org.au/def/organisation/entity/447"/>
	<skos:hasTopConcept rdf:resource="http://vocab.aodn.org.au/def/organisation/entity/451"/>
	<skos:hasTopConcept rdf:resource="http://vocab.aodn.org.au/def/organisation/entity/452"/>
	<skos:hasTopConcept rdf:resource="http://vocab.aodn.org.au/def/organisation/entity/453"/>
	<dcterms:contributor rdf:datatype="http://www.w3.org/2001/XMLSchema#string">eMII_Atkins.Natalia</dcterms:contributor>
	<dcterms:issued rdf:datatype="http://www.w3.org/2001/XMLSchema#string">2015-11-08</dcterms:issued>
	<owl:versionInfo rdf:datatype="http://www.w3.org/2001/XMLSchema#string">Version 1.2</owl:versionInfo>
</rdf:Description>

<rdf:Description rdf:about="http://www.w3.org/2004/02/skos/core#ConceptScheme">
	<rdf:type rdf:resource="http://www.w3.org/2000/01/rdf-schema#Resource"/>
	<rdf:type rdf:resource="http://www.w3.org/2000/01/rdf-schema#Class"/>
	<rdfs:subClassOf rdf:resource="http://www.w3.org/2000/01/rdf-schema#Resource"/>
	<rdfs:subClassOf rdf:resource="http://www.w3.org/2004/02/skos/core#ConceptScheme"/>
</rdf:Description>

<rdf:Description rdf:about="http://semantic-web.at/ontologies/csw.owl#hierarchyRoot">
	<rdf:type rdf:resource="http://www.w3.org/1999/02/22-rdf-syntax-ns#Property"/>
	<rdf:type rdf:resource="http://www.w3.org/2000/01/rdf-schema#Resource"/>
	<rdfs:subPropertyOf rdf:resource="http://semantic-web.at/ontologies/csw.owl#hierarchyRoot"/>
</rdf:Description>

<rdf:Description rdf:about="http://semantic-web.at/ontologies/csw.owl#hierarchyRootType">
	<rdf:type rdf:resource="http://www.w3.org/1999/02/22-rdf-syntax-ns#Property"/>
	<rdf:type rdf:resource="http://www.w3.org/2000/01/rdf-schema#Resource"/>
	<rdfs:subPropertyOf rdf:resource="http://semantic-web.at/ontologies/csw.owl#hierarchyRootType"/>
</rdf:Description>

<rdf:Description rdf:about="http://purl.org/dc/terms/title">
	<rdf:type rdf:resource="http://www.w3.org/1999/02/22-rdf-syntax-ns#Property"/>
	<rdf:type rdf:resource="http://www.w3.org/2000/01/rdf-schema#Resource"/>
	<rdfs:subPropertyOf rdf:resource="http://purl.org/dc/terms/title"/>
</rdf:Description>

<rdf:Description rdf:about="http://purl.org/dc/terms/description">
	<rdf:type rdf:resource="http://www.w3.org/1999/02/22-rdf-syntax-ns#Property"/>
	<rdf:type rdf:resource="http://www.w3.org/2000/01/rdf-schema#Resource"/>
	<rdfs:subPropertyOf rdf:resource="http://purl.org/dc/terms/description"/>
</rdf:Description>

<rdf:Description rdf:about="http://purl.org/dc/terms/modified">
	<rdf:type rdf:resource="http://www.w3.org/1999/02/22-rdf-syntax-ns#Property"/>
	<rdf:type rdf:resource="http://www.w3.org/2000/01/rdf-schema#Resource"/>
	<rdfs:subPropertyOf rdf:resource="http://purl.org/dc/terms/modified"/>
</rdf:Description>

<rdf:Description rdf:about="http://purl.org/dc/terms/subject">
	<rdf:type rdf:resource="http://www.w3.org/1999/02/22-rdf-syntax-ns#Property"/>
	<rdf:type rdf:resource="http://www.w3.org/2000/01/rdf-schema#Resource"/>
	<rdfs:subPropertyOf rdf:resource="http://purl.org/dc/terms/subject"/>
</rdf:Description>

<rdf:Description rdf:about="http://purl.org/dc/terms/publisher">
	<rdf:type rdf:resource="http://www.w3.org/1999/02/22-rdf-syntax-ns#Property"/>
	<rdf:type rdf:resource="http://www.w3.org/2000/01/rdf-schema#Resource"/>
	<rdfs:subPropertyOf rdf:resource="http://purl.org/dc/terms/publisher"/>
</rdf:Description>

<rdf:Description rdf:about="http://purl.org/dc/terms/creator">
	<rdf:type rdf:resource="http://www.w3.org/1999/02/22-rdf-syntax-ns#Property"/>
	<rdf:type rdf:resource="http://www.w3.org/2000/01/rdf-schema#Resource"/>
	<rdfs:subPropertyOf rdf:resource="http://purl.org/dc/terms/creator"/>
</rdf:Description>

<rdf:Description rdf:about="http://purl.org/dc/terms/created">
	<rdf:type rdf:resource="http://www.w3.org/1999/02/22-rdf-syntax-ns#Property"/>
	<rdf:type rdf:resource="http://www.w3.org/2000/01/rdf-schema#Resource"/>
	<rdfs:subPropertyOf rdf:resource="http://purl.org/dc/terms/created"/>
</rdf:Description>

<rdf:Description rdf:about="http://purl.org/dc/elements/1.1/rights">
	<rdf:type rdf:resource="http://www.w3.org/1999/02/22-rdf-syntax-ns#Property"/>
	<rdf:type rdf:resource="http://www.w3.org/2000/01/rdf-schema#Resource"/>
	<rdfs:subPropertyOf rdf:resource="http://purl.org/dc/elements/1.1/rights"/>
</rdf:Description>

<rdf:Description rdf:about="http://schema.semantic-web.at/ppt/identifier">
	<rdf:type rdf:resource="http://www.w3.org/1999/02/22-rdf-syntax-ns#Property"/>
	<rdf:type rdf:resource="http://www.w3.org/2000/01/rdf-schema#Resource"/>
	<rdfs:subPropertyOf rdf:resource="http://schema.semantic-web.at/ppt/identifier"/>
</rdf:Description>

<rdf:Description rdf:about="http://www.w3.org/2004/02/skos/core#hasTopConcept">
	<rdf:type rdf:resource="http://www.w3.org/1999/02/22-rdf-syntax-ns#Property"/>
	<rdf:type rdf:resource="http://www.w3.org/2000/01/rdf-schema#Resource"/>
	<rdfs:subPropertyOf rdf:resource="http://www.w3.org/2004/02/skos/core#hasTopConcept"/>
</rdf:Description>

<rdf:Description rdf:about="http://vocab.aodn.org.au/def/organisation/entity/1">
	<rdf:type rdf:resource="http://www.w3.org/2000/01/rdf-schema#Resource"/>
	<rdf:type rdf:resource="http://www.w3.org/2004/02/skos/core#Concept"/>
	<dcterms:modified rdf:datatype="http://www.w3.org/2001/XMLSchema#dateTime">2015-05-12T01:14:57Z</dcterms:modified>
	<dcterms:modified rdf:datatype="http://www.w3.org/2001/XMLSchema#dateTime">2016-01-27T05:56:02Z</dcterms:modified>
	<dcterms:creator rdf:datatype="http://www.w3.org/2001/XMLSchema#string">Natalia Atkins</dcterms:creator>
	<dcterms:created rdf:datatype="http://www.w3.org/2001/XMLSchema#dateTime">2015-04-27T10:38:15Z</dcterms:created>
	<dcterms:contributor rdf:datatype="http://www.w3.org/2001/XMLSchema#string">eMII_Atkins.Natalia</dcterms:contributor>
	<skos:broadMatch rdf:resource="http://vocab.aodn.org.au/def/organisation_classes/category/1"/>
	<skos:prefLabel xml:lang="en">Department of Defence (DoD), Australian Government</skos:prefLabel>
	<skos:altLabel xml:lang="en">Department of Defence (DoD)</skos:altLabel>
	<skos:hiddenLabel xml:lang="en">DoD</skos:hiddenLabel>
	<skos:definition xml:lang="en">The primary role of Defence is to defend Australia against armed attack. Australia's defence policy is founded on the principle of self-reliance in the direct defence of Australia, but with a capacity to do more where there are shared interests with partners and allies.</skos:definition>
	<dc:source rdf:datatype="http://www.w3.org/2001/XMLSchema#string">Australian Ocean Data Network Organisation Register</dc:source>
	<dc:publisher rdf:datatype="http://www.w3.org/2001/XMLSchema#string">eMarine Information Infrastructure (eMII)</dc:publisher>
	<skos:exactMatch rdf:resource="http://seadatanet.maris2.nl/v_edmo/print.asp?n_code=3932"/>
	<skos:narrower rdf:resource="http://vocab.aodn.org.au/def/organisation/entity/2"/>
	<skos:narrower rdf:resource="http://vocab.aodn.org.au/def/organisation/entity/4"/>
	<skos:narrower rdf:resource="http://vocab.aodn.org.au/def/organisation/entity/5"/>
	<skos:narrower rdf:resource="http://vocab.aodn.org.au/def/organisation/entity/406"/>
	<skos:topConceptOf rdf:resource="http://vocab.aodn.org.au/def/organisation/1"/>
	<skos:inScheme rdf:resource="http://vocab.aodn.org.au/def/organisation/1"/>
</rdf:Description>

<rdf:Description rdf:about="http://vocab.aodn.org.au/def/organisation/entity/8">
	<rdf:type rdf:resource="http://www.w3.org/2000/01/rdf-schema#Resource"/>
	<rdf:type rdf:resource="http://www.w3.org/2004/02/skos/core#Concept"/>
	<dcterms:modified rdf:datatype="http://www.w3.org/2001/XMLSchema#dateTime">2015-05-12T01:18:32Z</dcterms:modified>
	<dcterms:creator rdf:datatype="http://www.w3.org/2001/XMLSchema#string">Natalia Atkins</dcterms:creator>
	<dcterms:created rdf:datatype="http://www.w3.org/2001/XMLSchema#dateTime">2015-04-27T10:38:15Z</dcterms:created>
	<skos:broadMatch rdf:resource="http://vocab.aodn.org.au/def/organisation_classes/category/1"/>
	<skos:prefLabel xml:lang="en">Department of the Environment (DoE), Australian Government</skos:prefLabel>
	<skos:altLabel xml:lang="en">Department of the Environment (DoE)</skos:altLabel>
	<skos:hiddenLabel xml:lang="en">DoE</skos:hiddenLabel>
	<skos:definition xml:lang="en">The Department of the Environment designs and implements the Australian Government’s policies and programmes to protect and conserve the environment, water and heritage and promote climate action. The environmental framework is being delivered under four pillars: Clean air, Clean water, Clean land, and National heritage.</skos:definition>
	<dc:source rdf:datatype="http://www.w3.org/2001/XMLSchema#string">Australian Ocean Data Network Organisation Register</dc:source>
	<dc:publisher rdf:datatype="http://www.w3.org/2001/XMLSchema#string">eMarine Information Infrastructure (eMII)</dc:publisher>
	<skos:exactMatch rdf:resource="http://seadatanet.maris2.nl/v_edmo/print.asp?n_code=3956"/>
	<skos:narrower rdf:resource="http://vocab.aodn.org.au/def/organisation/entity/9"/>
	<skos:narrower rdf:resource="http://vocab.aodn.org.au/def/organisation/entity/11"/>
	<skos:topConceptOf rdf:resource="http://vocab.aodn.org.au/def/organisation/1"/>
	<skos:inScheme rdf:resource="http://vocab.aodn.org.au/def/organisation/1"/>
	<skos:scopeNote xml:lang="en">Replaces http://vocab.aodn.org.au/def/organisation/entity/23</skos:scopeNote>
	<dcterms:replaces rdf:resource="http://vocab.aodn.org.au/def/organisation/entity/23"/>
	<dcterms:replaces xml:lang="en">Department of the Environment, Water, Heritage and the Arts (DEWHA), Australian Government</dcterms:replaces>
</rdf:Description>

<rdf:Description rdf:about="http://vocab.aodn.org.au/def/organisation/entity/13">
	<rdf:type rdf:resource="http://www.w3.org/2000/01/rdf-schema#Resource"/>
	<rdf:type rdf:resource="http://www.w3.org/2004/02/skos/core#Concept"/>
	<dcterms:modified rdf:datatype="http://www.w3.org/2001/XMLSchema#dateTime">2015-05-12T01:16:08Z</dcterms:modified>
	<dcterms:creator rdf:datatype="http://www.w3.org/2001/XMLSchema#string">Natalia Atkins</dcterms:creator>
	<dcterms:created rdf:datatype="http://www.w3.org/2001/XMLSchema#dateTime">2015-04-27T10:38:15Z</dcterms:created>
	<skos:broadMatch rdf:resource="http://vocab.aodn.org.au/def/organisation_classes/category/1"/>
	<skos:prefLabel xml:lang="en">Department of Industry and Science, Australian Government</skos:prefLabel>
	<skos:altLabel xml:lang="en">Department of Industry and Science</skos:altLabel>
	<skos:definition xml:lang="en">The department consolidates the Australian Government’s efforts to drive economic growth, productivity and competitiveness by bringing together industry, energy, resources, science and skills.</skos:definition>
	<dc:source rdf:datatype="http://www.w3.org/2001/XMLSchema#string">Australian Ocean Data Network Organisation Register</dc:source>
	<dc:publisher rdf:datatype="http://www.w3.org/2001/XMLSchema#string">eMarine Information Infrastructure (eMII)</dc:publisher>
	<skos:exactMatch rdf:resource="http://seadatanet.maris2.nl/v_edmo/print.asp?n_code=3943"/>
	<skos:narrower rdf:resource="http://vocab.aodn.org.au/def/organisation/entity/14"/>
	<skos:narrower rdf:resource="http://vocab.aodn.org.au/def/organisation/entity/15"/>
	<skos:narrower rdf:resource="http://vocab.aodn.org.au/def/organisation/entity/20"/>
	<skos:narrower rdf:resource="http://vocab.aodn.org.au/def/organisation/entity/21"/>
	<skos:narrower rdf:resource="http://vocab.aodn.org.au/def/organisation/entity/22"/>
	<skos:topConceptOf rdf:resource="http://vocab.aodn.org.au/def/organisation/1"/>
	<skos:inScheme rdf:resource="http://vocab.aodn.org.au/def/organisation/1"/>
</rdf:Description>

<rdf:Description rdf:about="http://vocab.aodn.org.au/def/organisation/entity/23">
	<rdf:type rdf:resource="http://www.w3.org/2000/01/rdf-schema#Resource"/>
	<rdf:type rdf:resource="http://www.w3.org/2004/02/skos/core#Concept"/>
	<dcterms:modified rdf:datatype="http://www.w3.org/2001/XMLSchema#dateTime">2015-05-12T01:18:43Z</dcterms:modified>
	<dcterms:creator rdf:datatype="http://www.w3.org/2001/XMLSchema#string">Natalia Atkins</dcterms:creator>
	<dcterms:created rdf:datatype="http://www.w3.org/2001/XMLSchema#dateTime">2015-04-27T10:38:15Z</dcterms:created>
	<skos:broadMatch rdf:resource="http://vocab.aodn.org.au/def/organisation_classes/category/1"/>
	<skos:prefLabel xml:lang="en">Department of the Environment, Water, Heritage and the Arts (DEWHA), Australian Government</skos:prefLabel>
	<skos:altLabel xml:lang="en">Department of the Environment, Water, Heritage and the Arts (DEWHA)</skos:altLabel>
	<skos:hiddenLabel xml:lang="en">DEWHA</skos:hiddenLabel>
	<skos:definition xml:lang="en">The Department of the Environment, Water, Heritage and the Arts was an Australian Government department that existed between December 2007 and September 2010. (Courtesy of Wikipedia)</skos:definition>
	<dc:source rdf:datatype="http://www.w3.org/2001/XMLSchema#string">Australian Ocean Data Network Organisation Register</dc:source>
	<dc:publisher rdf:datatype="http://www.w3.org/2001/XMLSchema#string">eMarine Information Infrastructure (eMII)</dc:publisher>
	<skos:topConceptOf rdf:resource="http://vocab.aodn.org.au/def/organisation/1"/>
	<skos:inScheme rdf:resource="http://vocab.aodn.org.au/def/organisation/1"/>
	<skos:scopeNote xml:lang="en">Organisation no longer exists</skos:scopeNote>
	<skos:scopeNote xml:lang="en">Organisation no longer exists. Replaced by http://vocab.aodn.org.au/def/organisation/entity/8</skos:scopeNote>
	<dcterms:isReplacedBy rdf:resource="http://vocab.aodn.org.au/def/organisation/entity/8"/>
	<dcterms:isReplacedBy xml:lang="en">Department of the Environment (DoE), Australian Government</dcterms:isReplacedBy>
</rdf:Description>

<rdf:Description rdf:about="http://vocab.aodn.org.au/def/organisation/entity/24">
	<rdf:type rdf:resource="http://www.w3.org/2000/01/rdf-schema#Resource"/>
	<rdf:type rdf:resource="http://www.w3.org/2004/02/skos/core#Concept"/>
	<dcterms:modified rdf:datatype="http://www.w3.org/2001/XMLSchema#dateTime">2015-05-12T01:14:23Z</dcterms:modified>
	<dcterms:creator rdf:datatype="http://www.w3.org/2001/XMLSchema#string">Natalia Atkins</dcterms:creator>
	<dcterms:created rdf:datatype="http://www.w3.org/2001/XMLSchema#dateTime">2015-04-27T10:38:15Z</dcterms:created>
	<skos:broadMatch rdf:resource="http://vocab.aodn.org.au/def/organisation_classes/category/1"/>
	<skos:prefLabel xml:lang="en">Department of Agriculture, Australian Government</skos:prefLabel>
	<skos:altLabel xml:lang="en">Department of Agriculture</skos:altLabel>
	<skos:definition xml:lang="en">The Australian Department of Agriculture's role is to develop and implement policies and programs that ensure Australia's agricultural, fisheries, food and forestry industries remain competitive, profitable and sustainable.</skos:definition>
	<dc:source rdf:datatype="http://www.w3.org/2001/XMLSchema#string">Australian Ocean Data Network Organisation Register</dc:source>
	<dc:publisher rdf:datatype="http://www.w3.org/2001/XMLSchema#string">eMarine Information Infrastructure (eMII)</dc:publisher>
	<skos:exactMatch rdf:resource="http://seadatanet.maris2.nl/v_edmo/print.asp?n_code=4060"/>
	<skos:narrower rdf:resource="http://vocab.aodn.org.au/def/organisation/entity/25"/>
	<skos:topConceptOf rdf:resource="http://vocab.aodn.org.au/def/organisation/1"/>
	<skos:inScheme rdf:resource="http://vocab.aodn.org.au/def/organisation/1"/>
</rdf:Description>

<rdf:Description rdf:about="http://vocab.aodn.org.au/def/organisation/entity/26">
	<rdf:type rdf:resource="http://www.w3.org/2000/01/rdf-schema#Resource"/>
	<rdf:type rdf:resource="http://www.w3.org/2004/02/skos/core#Concept"/>
	<dcterms:modified rdf:datatype="http://www.w3.org/2001/XMLSchema#dateTime">2015-05-12T00:51:31Z</dcterms:modified>
	<dcterms:creator rdf:datatype="http://www.w3.org/2001/XMLSchema#string">Natalia Atkins</dcterms:creator>
	<dcterms:created rdf:datatype="http://www.w3.org/2001/XMLSchema#dateTime">2015-04-27T10:38:15Z</dcterms:created>
	<skos:broadMatch rdf:resource="http://vocab.aodn.org.au/def/organisation_classes/category/1"/>
	<skos:prefLabel xml:lang="en">Australian Fisheries Management Authority (AFMA), Australian Government</skos:prefLabel>
	<skos:altLabel xml:lang="en">Australian Fisheries Management Authority (AFMA)</skos:altLabel>
	<skos:hiddenLabel xml:lang="en">AFMA</skos:hiddenLabel>
	<skos:definition xml:lang="en">The Australian Fisheries Management Authority (AFMA) is the Australian Government agency responsible for the efficient management and sustainable use of Commonwealth fish resources on behalf of the Australian community.</skos:definition>
	<dc:source rdf:datatype="http://www.w3.org/2001/XMLSchema#string">Australian Ocean Data Network Organisation Register</dc:source>
	<dc:publisher rdf:datatype="http://www.w3.org/2001/XMLSchema#string">eMarine Information Infrastructure (eMII)</dc:publisher>
	<skos:exactMatch rdf:resource="http://seadatanet.maris2.nl/v_edmo/print.asp?n_code=4063"/>
	<skos:topConceptOf rdf:resource="http://vocab.aodn.org.au/def/organisation/1"/>
	<skos:inScheme rdf:resource="http://vocab.aodn.org.au/def/organisation/1"/>
</rdf:Description>

<rdf:Description rdf:about="http://vocab.aodn.org.au/def/organisation/entity/27">
	<rdf:type rdf:resource="http://www.w3.org/2000/01/rdf-schema#Resource"/>
	<rdf:type rdf:resource="http://www.w3.org/2004/02/skos/core#Concept"/>
	<dcterms:modified rdf:datatype="http://www.w3.org/2001/XMLSchema#dateTime">2015-05-12T00:51:48Z</dcterms:modified>
	<dcterms:creator rdf:datatype="http://www.w3.org/2001/XMLSchema#string">Natalia Atkins</dcterms:creator>
	<dcterms:created rdf:datatype="http://www.w3.org/2001/XMLSchema#dateTime">2015-04-27T10:38:15Z</dcterms:created>
	<skos:broadMatch rdf:resource="http://vocab.aodn.org.au/def/organisation_classes/category/1"/>
	<skos:prefLabel xml:lang="en">Australian Maritime Safety Authority (AMSA), Australian Government</skos:prefLabel>
	<skos:altLabel xml:lang="en">Australian Maritime Safety Authority (AMSA)</skos:altLabel>
	<skos:hiddenLabel xml:lang="en">AMSA</skos:hiddenLabel>
	<skos:definition xml:lang="en">The Australian Maritime Safety Authority (AMSA) is a statutory authority established under the Australian Maritime Safety Authority Act 1990 (the AMSA Act). AMSA’s principal functions are: promoting maritime safety and protection of the marine environment, preventing and combating ship-sourced pollution in the marine environment, providing infrastructure to support safety of navigation in Australian waters, and providing a national search and rescue service to the maritime and aviation sectors.</skos:definition>
	<dc:source rdf:datatype="http://www.w3.org/2001/XMLSchema#string">Australian Ocean Data Network Organisation Register</dc:source>
	<dc:publisher rdf:datatype="http://www.w3.org/2001/XMLSchema#string">eMarine Information Infrastructure (eMII)</dc:publisher>
	<skos:exactMatch rdf:resource="http://seadatanet.maris2.nl/v_edmo/print.asp?n_code=4064"/>
	<skos:topConceptOf rdf:resource="http://vocab.aodn.org.au/def/organisation/1"/>
	<skos:inScheme rdf:resource="http://vocab.aodn.org.au/def/organisation/1"/>
</rdf:Description>

<rdf:Description rdf:about="http://vocab.aodn.org.au/def/organisation/entity/28">
	<rdf:type rdf:resource="http://www.w3.org/2000/01/rdf-schema#Resource"/>
	<rdf:type rdf:resource="http://www.w3.org/2004/02/skos/core#Concept"/>
	<dcterms:modified rdf:datatype="http://www.w3.org/2001/XMLSchema#dateTime">2015-05-11T22:53:27Z</dcterms:modified>
	<dcterms:creator rdf:datatype="http://www.w3.org/2001/XMLSchema#string">Natalia Atkins</dcterms:creator>
	<dcterms:created rdf:datatype="http://www.w3.org/2001/XMLSchema#dateTime">2015-04-27T10:38:15Z</dcterms:created>
	<skos:broadMatch rdf:resource="http://vocab.aodn.org.au/def/organisation_classes/category/5"/>
	<skos:prefLabel xml:lang="en">Alex Wyllie and Associates Pty Ltd</skos:prefLabel>
	<skos:definition xml:lang="en">Provide clients with products derived from remotely sensed data. Consulting on remote sensing systems and other geospatial matters. This organisation ceased in 2003.</skos:definition>
	<dc:source rdf:datatype="http://www.w3.org/2001/XMLSchema#string">Australian Ocean Data Network Organisation Register</dc:source>
	<dc:publisher rdf:datatype="http://www.w3.org/2001/XMLSchema#string">eMarine Information Infrastructure (eMII)</dc:publisher>
	<skos:topConceptOf rdf:resource="http://vocab.aodn.org.au/def/organisation/1"/>
	<skos:inScheme rdf:resource="http://vocab.aodn.org.au/def/organisation/1"/>
	<skos:scopeNote xml:lang="en">Organisation no longer exists</skos:scopeNote>
</rdf:Description>

<rdf:Description rdf:about="http://vocab.aodn.org.au/def/organisation/entity/30">
	<rdf:type rdf:resource="http://www.w3.org/2000/01/rdf-schema#Resource"/>
	<rdf:type rdf:resource="http://www.w3.org/2004/02/skos/core#Concept"/>
	<dcterms:modified rdf:datatype="http://www.w3.org/2001/XMLSchema#dateTime">2015-05-12T00:50:54Z</dcterms:modified>
	<dcterms:creator rdf:datatype="http://www.w3.org/2001/XMLSchema#string">Natalia Atkins</dcterms:creator>
	<dcterms:created rdf:datatype="http://www.w3.org/2001/XMLSchema#dateTime">2015-04-27T10:38:15Z</dcterms:created>
	<skos:broadMatch rdf:resource="http://vocab.aodn.org.au/def/organisation_classes/category/5"/>
	<skos:prefLabel xml:lang="en">Apache Energy Limited</skos:prefLabel>
	<skos:definition xml:lang="en">Apache’s holdings in Australia are focused offshore Western Australia in the Carnarvon, Exmouth and Browse basins, with production operations in the Carnarvon and Exmouth basins.</skos:definition>
	<dc:source rdf:datatype="http://www.w3.org/2001/XMLSchema#string">Australian Ocean Data Network Organisation Register</dc:source>
	<dc:publisher rdf:datatype="http://www.w3.org/2001/XMLSchema#string">eMarine Information Infrastructure (eMII)</dc:publisher>
	<skos:exactMatch rdf:resource="http://seadatanet.maris2.nl/v_edmo/print.asp?n_code=4065"/>
	<skos:topConceptOf rdf:resource="http://vocab.aodn.org.au/def/organisation/1"/>
	<skos:inScheme rdf:resource="http://vocab.aodn.org.au/def/organisation/1"/>
</rdf:Description>

<rdf:Description rdf:about="http://vocab.aodn.org.au/def/organisation/entity/31">
	<rdf:type rdf:resource="http://www.w3.org/2000/01/rdf-schema#Resource"/>
	<rdf:type rdf:resource="http://www.w3.org/2004/02/skos/core#Concept"/>
	<dcterms:modified rdf:datatype="http://www.w3.org/2001/XMLSchema#dateTime">2015-05-12T01:30:06Z</dcterms:modified>
	<dcterms:creator rdf:datatype="http://www.w3.org/2001/XMLSchema#string">Natalia Atkins</dcterms:creator>
	<dcterms:created rdf:datatype="http://www.w3.org/2001/XMLSchema#dateTime">2015-04-27T10:38:15Z</dcterms:created>
	<skos:broadMatch rdf:resource="http://vocab.aodn.org.au/def/organisation_classes/category/5"/>
	<skos:prefLabel xml:lang="en">RPS APASA Pty Ltd</skos:prefLabel>
	<skos:hiddenLabel xml:lang="en">RSP APASA</skos:hiddenLabel>
	<skos:definition xml:lang="en">RPS APASA specializes in the development and application of sophisticated numerical tools for application to environmental, engineering and safety issues.</skos:definition>
	<dc:source rdf:datatype="http://www.w3.org/2001/XMLSchema#string">Australian Ocean Data Network Organisation Register</dc:source>
	<dc:publisher rdf:datatype="http://www.w3.org/2001/XMLSchema#string">eMarine Information Infrastructure (eMII)</dc:publisher>
	<skos:exactMatch rdf:resource="http://seadatanet.maris2.nl/v_edmo/print.asp?n_code=4066"/>
	<skos:topConceptOf rdf:resource="http://vocab.aodn.org.au/def/organisation/1"/>
	<skos:inScheme rdf:resource="http://vocab.aodn.org.au/def/organisation/1"/>
</rdf:Description>

<rdf:Description rdf:about="http://vocab.aodn.org.au/def/organisation/entity/32">
	<rdf:type rdf:resource="http://www.w3.org/2000/01/rdf-schema#Resource"/>
	<rdf:type rdf:resource="http://www.w3.org/2004/02/skos/core#Concept"/>
	<dcterms:modified rdf:datatype="http://www.w3.org/2001/XMLSchema#dateTime">2015-05-12T00:51:16Z</dcterms:modified>
	<dcterms:creator rdf:datatype="http://www.w3.org/2001/XMLSchema#string">Natalia Atkins</dcterms:creator>
	<dcterms:created rdf:datatype="http://www.w3.org/2001/XMLSchema#dateTime">2015-04-27T10:38:15Z</dcterms:created>
	<skos:broadMatch rdf:resource="http://vocab.aodn.org.au/def/organisation_classes/category/5"/>
	<skos:prefLabel xml:lang="en">Astron Environmental Services</skos:prefLabel>
	<skos:definition xml:lang="en">Astron is one of Australia’s longest established environmental consultancies with over 30 years continuous experience in Western Australia. They provide a range of environmental services to clients whose businesses are in mining, energy, infrastructure, land development and utilities. They have offices in Perth, Karratha and Margaret River.</skos:definition>
	<dc:source rdf:datatype="http://www.w3.org/2001/XMLSchema#string">Australian Ocean Data Network Organisation Register</dc:source>
	<dc:publisher rdf:datatype="http://www.w3.org/2001/XMLSchema#string">eMarine Information Infrastructure (eMII)</dc:publisher>
	<skos:exactMatch rdf:resource="http://seadatanet.maris2.nl/v_edmo/print.asp?n_code=4067"/>
	<skos:topConceptOf rdf:resource="http://vocab.aodn.org.au/def/organisation/1"/>
	<skos:inScheme rdf:resource="http://vocab.aodn.org.au/def/organisation/1"/>
</rdf:Description>

<rdf:Description rdf:about="http://vocab.aodn.org.au/def/organisation/entity/33">
	<rdf:type rdf:resource="http://www.w3.org/2000/01/rdf-schema#Resource"/>
	<rdf:type rdf:resource="http://www.w3.org/2004/02/skos/core#Concept"/>
	<dcterms:creator rdf:datatype="http://www.w3.org/2001/XMLSchema#string">Natalia Atkins</dcterms:creator>
	<dcterms:created rdf:datatype="http://www.w3.org/2001/XMLSchema#dateTime">2015-04-27T10:38:15Z</dcterms:created>
	<skos:broadMatch rdf:resource="http://vocab.aodn.org.au/def/organisation_classes/category/2"/>
	<skos:prefLabel xml:lang="en">Australian Museum</skos:prefLabel>
	<skos:definition xml:lang="en">This is Australia's first museum, and is based in Sydney.</skos:definition>
	<dc:source rdf:datatype="http://www.w3.org/2001/XMLSchema#string">Australian Ocean Data Network Organisation Register</dc:source>
	<dc:publisher rdf:datatype="http://www.w3.org/2001/XMLSchema#string">eMarine Information Infrastructure (eMII)</dc:publisher>
	<skos:exactMatch rdf:resource="http://seadatanet.maris2.nl/v_edmo/print.asp?n_code=4026"/>
	<skos:topConceptOf rdf:resource="http://vocab.aodn.org.au/def/organisation/1"/>
	<skos:inScheme rdf:resource="http://vocab.aodn.org.au/def/organisation/1"/>
</rdf:Description>

<rdf:Description rdf:about="http://vocab.aodn.org.au/def/organisation/entity/34">
	<rdf:type rdf:resource="http://www.w3.org/2000/01/rdf-schema#Resource"/>
	<rdf:type rdf:resource="http://www.w3.org/2004/02/skos/core#Concept"/>
	<dcterms:modified rdf:datatype="http://www.w3.org/2001/XMLSchema#dateTime">2015-05-12T00:52:08Z</dcterms:modified>
	<dcterms:creator rdf:datatype="http://www.w3.org/2001/XMLSchema#string">Natalia Atkins</dcterms:creator>
	<dcterms:created rdf:datatype="http://www.w3.org/2001/XMLSchema#dateTime">2015-04-27T10:38:15Z</dcterms:created>
	<skos:broadMatch rdf:resource="http://vocab.aodn.org.au/def/organisation_classes/category/1"/>
	<skos:prefLabel xml:lang="en">Australian Ocean Data Network (AODN)</skos:prefLabel>
	<skos:hiddenLabel xml:lang="en">AODN</skos:hiddenLabel>
	<skos:definition xml:lang="en">The vision of the Australian Ocean Data Network (AODN) was articulated in 2005 by the Australian Ocean Data Centre Joint Facility (AODCJF), a joint venture between the six Commonwealth Agencies[1] with primary responsibility for marine data.</skos:definition>
	<dc:source rdf:datatype="http://www.w3.org/2001/XMLSchema#string">Australian Ocean Data Network Organisation Register</dc:source>
	<dc:publisher rdf:datatype="http://www.w3.org/2001/XMLSchema#string">eMarine Information Infrastructure (eMII)</dc:publisher>
	<skos:exactMatch rdf:resource="http://seadatanet.maris2.nl/v_edmo/print.asp?n_code=4068"/>
	<skos:topConceptOf rdf:resource="http://vocab.aodn.org.au/def/organisation/1"/>
	<skos:inScheme rdf:resource="http://vocab.aodn.org.au/def/organisation/1"/>
</rdf:Description>

<rdf:Description rdf:about="http://vocab.aodn.org.au/def/organisation/entity/35">
	<rdf:type rdf:resource="http://www.w3.org/2000/01/rdf-schema#Resource"/>
	<rdf:type rdf:resource="http://www.w3.org/2004/02/skos/core#Concept"/>
	<dcterms:modified rdf:datatype="http://www.w3.org/2001/XMLSchema#dateTime">2015-05-12T00:52:59Z</dcterms:modified>
	<dcterms:creator rdf:datatype="http://www.w3.org/2001/XMLSchema#string">Natalia Atkins</dcterms:creator>
	<dcterms:created rdf:datatype="http://www.w3.org/2001/XMLSchema#dateTime">2015-04-27T10:38:15Z</dcterms:created>
	<skos:broadMatch rdf:resource="http://vocab.aodn.org.au/def/organisation_classes/category/5"/>
	<skos:prefLabel xml:lang="en">Bamford Consulting Ecologists (BCE)</skos:prefLabel>
	<skos:hiddenLabel xml:lang="en">BCE</skos:hiddenLabel>
	<skos:definition xml:lang="en">Bamford Consulting Ecologists (BCE) is a partnership specialising in fauna investigations for environmental impact assessment, and long-term ecological monitoring of fauna populations, particularly in relation to disturbance, mining and rehabilitation.</skos:definition>
	<dc:source rdf:datatype="http://www.w3.org/2001/XMLSchema#string">Australian Ocean Data Network Organisation Register</dc:source>
	<dc:publisher rdf:datatype="http://www.w3.org/2001/XMLSchema#string">eMarine Information Infrastructure (eMII)</dc:publisher>
	<skos:exactMatch rdf:resource="http://seadatanet.maris2.nl/v_edmo/print.asp?n_code=4069"/>
	<skos:topConceptOf rdf:resource="http://vocab.aodn.org.au/def/organisation/1"/>
	<skos:inScheme rdf:resource="http://vocab.aodn.org.au/def/organisation/1"/>
</rdf:Description>

<rdf:Description rdf:about="http://vocab.aodn.org.au/def/organisation/entity/36">
	<rdf:type rdf:resource="http://www.w3.org/2000/01/rdf-schema#Resource"/>
	<rdf:type rdf:resource="http://www.w3.org/2004/02/skos/core#Concept"/>
	<dcterms:modified rdf:datatype="http://www.w3.org/2001/XMLSchema#dateTime">2015-05-12T01:00:05Z</dcterms:modified>
	<dcterms:creator rdf:datatype="http://www.w3.org/2001/XMLSchema#string">Natalia Atkins</dcterms:creator>
	<dcterms:created rdf:datatype="http://www.w3.org/2001/XMLSchema#dateTime">2015-04-27T10:38:15Z</dcterms:created>
	<skos:broadMatch rdf:resource="http://vocab.aodn.org.au/def/organisation_classes/category/6"/>
	<skos:prefLabel xml:lang="en">Birdlife Australia</skos:prefLabel>
	<skos:definition xml:lang="en">The Royal Australasian Ornithologists Union, now known as Birdlife Australia, was founded in 1901 to promote the study and conservation of the native bird species of Australia and adjacent regions. This makes it Australia's oldest national birding association. It was also Australia's largest non-government, non-profit, bird conservation organisation. In 1996 it adopted the trading name of Birds Australia for most public purposes, while retaining its original name for legal purposes and as the publisher of its journal the Emu. In 2012 it merged with Bird Observation and Conservation Australia to form BirdLife Australia.</skos:definition>
	<dc:source rdf:datatype="http://www.w3.org/2001/XMLSchema#string">Australian Ocean Data Network Organisation Register</dc:source>
	<dc:publisher rdf:datatype="http://www.w3.org/2001/XMLSchema#string">eMarine Information Infrastructure (eMII)</dc:publisher>
	<skos:exactMatch rdf:resource="http://seadatanet.maris2.nl/v_edmo/print.asp?n_code=4070"/>
	<skos:topConceptOf rdf:resource="http://vocab.aodn.org.au/def/organisation/1"/>
	<skos:inScheme rdf:resource="http://vocab.aodn.org.au/def/organisation/1"/>
</rdf:Description>

<rdf:Description rdf:about="http://vocab.aodn.org.au/def/organisation/entity/37">
	<rdf:type rdf:resource="http://www.w3.org/2000/01/rdf-schema#Resource"/>
	<rdf:type rdf:resource="http://www.w3.org/2004/02/skos/core#Concept"/>
	<dcterms:modified rdf:datatype="http://www.w3.org/2001/XMLSchema#dateTime">2015-05-12T01:01:15Z</dcterms:modified>
	<dcterms:creator rdf:datatype="http://www.w3.org/2001/XMLSchema#string">Natalia Atkins</dcterms:creator>
	<dcterms:created rdf:datatype="http://www.w3.org/2001/XMLSchema#dateTime">2015-04-27T10:38:15Z</dcterms:created>
	<skos:broadMatch rdf:resource="http://vocab.aodn.org.au/def/organisation_classes/category/5"/>
	<skos:prefLabel xml:lang="en">Broome International Airport Holdings Pty Ltd (BIAH)</skos:prefLabel>
	<skos:hiddenLabel xml:lang="en">BIAH</skos:hiddenLabel>
	<dc:source rdf:datatype="http://www.w3.org/2001/XMLSchema#string">Australian Ocean Data Network Organisation Register</dc:source>
	<dc:publisher rdf:datatype="http://www.w3.org/2001/XMLSchema#string">eMarine Information Infrastructure (eMII)</dc:publisher>
	<skos:exactMatch rdf:resource="http://seadatanet.maris2.nl/v_edmo/print.asp?n_code=4071"/>
	<skos:topConceptOf rdf:resource="http://vocab.aodn.org.au/def/organisation/1"/>
	<skos:inScheme rdf:resource="http://vocab.aodn.org.au/def/organisation/1"/>
</rdf:Description>

<rdf:Description rdf:about="http://vocab.aodn.org.au/def/organisation/entity/38">
	<rdf:type rdf:resource="http://www.w3.org/2000/01/rdf-schema#Resource"/>
	<rdf:type rdf:resource="http://www.w3.org/2004/02/skos/core#Concept"/>
	<dcterms:modified rdf:datatype="http://www.w3.org/2001/XMLSchema#dateTime">2015-05-12T01:02:55Z</dcterms:modified>
	<dcterms:creator rdf:datatype="http://www.w3.org/2001/XMLSchema#string">Natalia Atkins</dcterms:creator>
	<dcterms:created rdf:datatype="http://www.w3.org/2001/XMLSchema#dateTime">2015-04-27T10:38:15Z</dcterms:created>
	<skos:broadMatch rdf:resource="http://vocab.aodn.org.au/def/organisation_classes/category/5"/>
	<skos:prefLabel xml:lang="en">Busselton Underwater Observatory</skos:prefLabel>
	<skos:definition xml:lang="en">Located 1.7 kilometres from shore at the end of the Busselton Jetty, the Underwater Observatory has been designed to accommodate up to 40 people at one time. Descending 8 metres beneath the waters’ surface, visitors can view the amazing corals and fish life through eleven viewing windows, at various levels within a 9.5 metre diameter observation chamber.</skos:definition>
	<dc:source rdf:datatype="http://www.w3.org/2001/XMLSchema#string">Australian Ocean Data Network Organisation Register</dc:source>
	<dc:publisher rdf:datatype="http://www.w3.org/2001/XMLSchema#string">eMarine Information Infrastructure (eMII)</dc:publisher>
	<skos:exactMatch rdf:resource="http://seadatanet.maris2.nl/v_edmo/print.asp?n_code=4072"/>
	<skos:topConceptOf rdf:resource="http://vocab.aodn.org.au/def/organisation/1"/>
	<skos:inScheme rdf:resource="http://vocab.aodn.org.au/def/organisation/1"/>
</rdf:Description>

<rdf:Description rdf:about="http://vocab.aodn.org.au/def/organisation/entity/39">
	<rdf:type rdf:resource="http://www.w3.org/2000/01/rdf-schema#Resource"/>
	<rdf:type rdf:resource="http://www.w3.org/2004/02/skos/core#Concept"/>
	<dcterms:modified rdf:datatype="http://www.w3.org/2001/XMLSchema#dateTime">2015-05-12T00:52:32Z</dcterms:modified>
	<dcterms:creator rdf:datatype="http://www.w3.org/2001/XMLSchema#string">Natalia Atkins</dcterms:creator>
	<dcterms:created rdf:datatype="http://www.w3.org/2001/XMLSchema#dateTime">2015-04-27T10:38:15Z</dcterms:created>
	<skos:broadMatch rdf:resource="http://vocab.aodn.org.au/def/organisation_classes/category/5"/>
	<skos:prefLabel xml:lang="en">BHP Billiton Petroleum Australia</skos:prefLabel>
	<skos:definition xml:lang="en">BHP Billiton Petroleum has exploration, development, production and marketing activities in more than a dozen countries around the globe, with a significant position in the deep water Gulf of Mexico, Onshore US and Australia.  Petroleum also operates assets in the United States, Australia, United Kingdom, Trinidad and Tobago and Pakistan.</skos:definition>
	<dc:source rdf:datatype="http://www.w3.org/2001/XMLSchema#string">Australian Ocean Data Network Organisation Register</dc:source>
	<dc:publisher rdf:datatype="http://www.w3.org/2001/XMLSchema#string">eMarine Information Infrastructure (eMII)</dc:publisher>
	<skos:exactMatch rdf:resource="http://seadatanet.maris2.nl/v_edmo/print.asp?n_code=4073"/>
	<skos:topConceptOf rdf:resource="http://vocab.aodn.org.au/def/organisation/1"/>
	<skos:inScheme rdf:resource="http://vocab.aodn.org.au/def/organisation/1"/>
</rdf:Description>

<rdf:Description rdf:about="http://vocab.aodn.org.au/def/organisation/entity/40">
	<rdf:type rdf:resource="http://www.w3.org/2000/01/rdf-schema#Resource"/>
	<rdf:type rdf:resource="http://www.w3.org/2004/02/skos/core#Concept"/>
	<dcterms:modified rdf:datatype="http://www.w3.org/2001/XMLSchema#dateTime">2015-05-19T03:11:31Z</dcterms:modified>
	<dcterms:creator rdf:datatype="http://www.w3.org/2001/XMLSchema#string">Natalia Atkins</dcterms:creator>
	<dcterms:created rdf:datatype="http://www.w3.org/2001/XMLSchema#dateTime">2015-04-27T10:38:15Z</dcterms:created>
	<skos:broadMatch rdf:resource="http://vocab.aodn.org.au/def/organisation_classes/category/5"/>
	<skos:prefLabel xml:lang="en">BHP Billiton Iron Ore</skos:prefLabel>
	<skos:definition xml:lang="en">BHP Billiton Iron Ore is one of the world’s leading iron ore producers with operations in Australia and Brazil. We sell lump and fine product from Australia and iron ore pellets from our Samarco operation in Brazil.</skos:definition>
	<dc:source rdf:datatype="http://www.w3.org/2001/XMLSchema#string">Australian Ocean Data Network Organisation Register</dc:source>
	<dc:publisher rdf:datatype="http://www.w3.org/2001/XMLSchema#string">eMarine Information Infrastructure (eMII)</dc:publisher>
	<skos:exactMatch rdf:resource="http://seadatanet.maris2.nl/v_edmo/print.asp?n_code=4074"/>
	<skos:topConceptOf rdf:resource="http://vocab.aodn.org.au/def/organisation/1"/>
	<skos:inScheme rdf:resource="http://vocab.aodn.org.au/def/organisation/1"/>
</rdf:Description>

<rdf:Description rdf:about="http://vocab.aodn.org.au/def/organisation/entity/41">
	<rdf:type rdf:resource="http://www.w3.org/2000/01/rdf-schema#Resource"/>
	<rdf:type rdf:resource="http://www.w3.org/2004/02/skos/core#Concept"/>
	<dcterms:modified rdf:datatype="http://www.w3.org/2001/XMLSchema#dateTime">2015-05-12T00:52:22Z</dcterms:modified>
	<dcterms:creator rdf:datatype="http://www.w3.org/2001/XMLSchema#string">Natalia Atkins</dcterms:creator>
	<dcterms:created rdf:datatype="http://www.w3.org/2001/XMLSchema#dateTime">2015-04-27T10:38:15Z</dcterms:created>
	<skos:broadMatch rdf:resource="http://vocab.aodn.org.au/def/organisation_classes/category/5"/>
	<skos:prefLabel xml:lang="en">BHP Billiton Limited</skos:prefLabel>
	<skos:definition xml:lang="en">BHP Billiton is an Anglo-Australian multinational mining, metals and petroleum company headquartered in Melbourne, Australia. It is the world's largest mining company measured by 2013 revenues. BHP Billiton was created in 2001 through the merger of the Australian Broken Hill Proprietary Company Limited (BHP) and the Anglo–Dutch Billiton plc. (Courtesy of Wikipedia)</skos:definition>
	<dc:source rdf:datatype="http://www.w3.org/2001/XMLSchema#string">Australian Ocean Data Network Organisation Register</dc:source>
	<dc:publisher rdf:datatype="http://www.w3.org/2001/XMLSchema#string">eMarine Information Infrastructure (eMII)</dc:publisher>
	<skos:exactMatch rdf:resource="http://seadatanet.maris2.nl/v_edmo/print.asp?n_code=4075"/>
	<skos:topConceptOf rdf:resource="http://vocab.aodn.org.au/def/organisation/1"/>
	<skos:inScheme rdf:resource="http://vocab.aodn.org.au/def/organisation/1"/>
</rdf:Description>

<rdf:Description rdf:about="http://vocab.aodn.org.au/def/organisation/entity/42">
	<rdf:type rdf:resource="http://www.w3.org/2000/01/rdf-schema#Resource"/>
	<rdf:type rdf:resource="http://www.w3.org/2004/02/skos/core#Concept"/>
	<dcterms:modified rdf:datatype="http://www.w3.org/2001/XMLSchema#dateTime">2015-05-12T01:00:57Z</dcterms:modified>
	<dcterms:creator rdf:datatype="http://www.w3.org/2001/XMLSchema#string">Natalia Atkins</dcterms:creator>
	<dcterms:created rdf:datatype="http://www.w3.org/2001/XMLSchema#dateTime">2015-04-27T10:38:15Z</dcterms:created>
	<skos:broadMatch rdf:resource="http://vocab.aodn.org.au/def/organisation_classes/category/1"/>
	<skos:prefLabel xml:lang="en">BlueNet</skos:prefLabel>
	<skos:definition xml:lang="en">The BlueNet project was established by a grant from the Australian Government to provide a virtual data centre to support long term curation and management of data for Australia's marine science researchers. BlueNet linked vast data repositories and marine resources that currently reside in academic and government institutions both in Australia and overseas. Funding for the project concluded in 2009, and management of the project is now undertaken by staff from the Australian Ocean Data Network (AODN).</skos:definition>
	<dc:source rdf:datatype="http://www.w3.org/2001/XMLSchema#string">Australian Ocean Data Network Organisation Register</dc:source>
	<dc:publisher rdf:datatype="http://www.w3.org/2001/XMLSchema#string">eMarine Information Infrastructure (eMII)</dc:publisher>
	<skos:topConceptOf rdf:resource="http://vocab.aodn.org.au/def/organisation/1"/>
	<skos:inScheme rdf:resource="http://vocab.aodn.org.au/def/organisation/1"/>
	<skos:scopeNote xml:lang="en">Organisation no longer exists</skos:scopeNote>
</rdf:Description>

<rdf:Description rdf:about="http://vocab.aodn.org.au/def/organisation/entity/43">
	<rdf:type rdf:resource="http://www.w3.org/2000/01/rdf-schema#Resource"/>
	<rdf:type rdf:resource="http://www.w3.org/2004/02/skos/core#Concept"/>
	<dcterms:modified rdf:datatype="http://www.w3.org/2001/XMLSchema#dateTime">2015-05-12T01:01:05Z</dcterms:modified>
	<dcterms:creator rdf:datatype="http://www.w3.org/2001/XMLSchema#string">Natalia Atkins</dcterms:creator>
	<dcterms:created rdf:datatype="http://www.w3.org/2001/XMLSchema#dateTime">2015-04-27T10:38:15Z</dcterms:created>
	<skos:broadMatch rdf:resource="http://vocab.aodn.org.au/def/organisation_classes/category/5"/>
	<skos:prefLabel xml:lang="en">Boggabri Coal Pty Ltd</skos:prefLabel>
	<skos:definition xml:lang="en">Boggabri Coal Pty Limited is an entity of Idemitsu Australia Resources Pty Ltd.</skos:definition>
	<dc:source rdf:datatype="http://www.w3.org/2001/XMLSchema#string">Australian Ocean Data Network Organisation Register</dc:source>
	<dc:publisher rdf:datatype="http://www.w3.org/2001/XMLSchema#string">eMarine Information Infrastructure (eMII)</dc:publisher>
	<skos:exactMatch rdf:resource="http://seadatanet.maris2.nl/v_edmo/print.asp?n_code=3939"/>
	<skos:topConceptOf rdf:resource="http://vocab.aodn.org.au/def/organisation/1"/>
	<skos:inScheme rdf:resource="http://vocab.aodn.org.au/def/organisation/1"/>
</rdf:Description>

<rdf:Description rdf:about="http://vocab.aodn.org.au/def/organisation/entity/44">
	<rdf:type rdf:resource="http://www.w3.org/2000/01/rdf-schema#Resource"/>
	<rdf:type rdf:resource="http://www.w3.org/2004/02/skos/core#Concept"/>
	<dcterms:modified rdf:datatype="http://www.w3.org/2001/XMLSchema#dateTime">2015-05-12T01:03:03Z</dcterms:modified>
	<dcterms:creator rdf:datatype="http://www.w3.org/2001/XMLSchema#string">Natalia Atkins</dcterms:creator>
	<dcterms:created rdf:datatype="http://www.w3.org/2001/XMLSchema#dateTime">2015-04-27T10:38:15Z</dcterms:created>
	<skos:broadMatch rdf:resource="http://vocab.aodn.org.au/def/organisation_classes/category/5"/>
	<skos:prefLabel xml:lang="en">C-AID Consultants</skos:prefLabel>
	<skos:definition xml:lang="en">C-AID Consultants specialises in providing professional advice on: the sustainable use of aquatic resources, natural resource management, seafood safety and fishery and environmental legislation.</skos:definition>
	<dc:source rdf:datatype="http://www.w3.org/2001/XMLSchema#string">Australian Ocean Data Network Organisation Register</dc:source>
	<dc:publisher rdf:datatype="http://www.w3.org/2001/XMLSchema#string">eMarine Information Infrastructure (eMII)</dc:publisher>
	<skos:exactMatch rdf:resource="http://seadatanet.maris2.nl/v_edmo/print.asp?n_code=4076"/>
	<skos:topConceptOf rdf:resource="http://vocab.aodn.org.au/def/organisation/1"/>
	<skos:inScheme rdf:resource="http://vocab.aodn.org.au/def/organisation/1"/>
</rdf:Description>

<rdf:Description rdf:about="http://vocab.aodn.org.au/def/organisation/entity/45">
	<rdf:type rdf:resource="http://www.w3.org/2000/01/rdf-schema#Resource"/>
	<rdf:type rdf:resource="http://www.w3.org/2004/02/skos/core#Concept"/>
	<dcterms:modified rdf:datatype="http://www.w3.org/2001/XMLSchema#dateTime">2015-05-12T01:03:49Z</dcterms:modified>
	<dcterms:creator rdf:datatype="http://www.w3.org/2001/XMLSchema#string">Natalia Atkins</dcterms:creator>
	<dcterms:created rdf:datatype="http://www.w3.org/2001/XMLSchema#dateTime">2015-04-27T10:38:15Z</dcterms:created>
	<skos:broadMatch rdf:resource="http://vocab.aodn.org.au/def/organisation_classes/category/6"/>
	<skos:prefLabel xml:lang="en">Centre for Whale Research (CWR)</skos:prefLabel>
	<skos:hiddenLabel xml:lang="en">CWR</skos:hiddenLabel>
	<skos:definition xml:lang="en">Not for profit registered research institute. Centre for Whale Research (CWR)'s scientists conduct research all around Australia and the Southern Ocean.</skos:definition>
	<dc:source rdf:datatype="http://www.w3.org/2001/XMLSchema#string">Australian Ocean Data Network Organisation Register</dc:source>
	<dc:publisher rdf:datatype="http://www.w3.org/2001/XMLSchema#string">eMarine Information Infrastructure (eMII)</dc:publisher>
	<skos:exactMatch rdf:resource="http://seadatanet.maris2.nl/v_edmo/print.asp?n_code=4077"/>
	<skos:topConceptOf rdf:resource="http://vocab.aodn.org.au/def/organisation/1"/>
	<skos:inScheme rdf:resource="http://vocab.aodn.org.au/def/organisation/1"/>
</rdf:Description>

<rdf:Description rdf:about="http://vocab.aodn.org.au/def/organisation/entity/46">
	<rdf:type rdf:resource="http://www.w3.org/2000/01/rdf-schema#Resource"/>
	<rdf:type rdf:resource="http://www.w3.org/2004/02/skos/core#Concept"/>
	<dcterms:modified rdf:datatype="http://www.w3.org/2001/XMLSchema#dateTime">2015-05-12T01:03:56Z</dcterms:modified>
	<dcterms:creator rdf:datatype="http://www.w3.org/2001/XMLSchema#string">Natalia Atkins</dcterms:creator>
	<dcterms:created rdf:datatype="http://www.w3.org/2001/XMLSchema#dateTime">2015-04-27T10:38:15Z</dcterms:created>
	<skos:broadMatch rdf:resource="http://vocab.aodn.org.au/def/organisation_classes/category/5"/>
	<skos:prefLabel xml:lang="en">Chevron Australia Pty Ltd</skos:prefLabel>
	<skos:definition xml:lang="en">Chevron Austalia is a subsidiary of Chevron an international energy corporation.</skos:definition>
	<dc:source rdf:datatype="http://www.w3.org/2001/XMLSchema#string">Australian Ocean Data Network Organisation Register</dc:source>
	<dc:publisher rdf:datatype="http://www.w3.org/2001/XMLSchema#string">eMarine Information Infrastructure (eMII)</dc:publisher>
	<skos:exactMatch rdf:resource="http://seadatanet.maris2.nl/v_edmo/print.asp?n_code=4078"/>
	<skos:topConceptOf rdf:resource="http://vocab.aodn.org.au/def/organisation/1"/>
	<skos:inScheme rdf:resource="http://vocab.aodn.org.au/def/organisation/1"/>
</rdf:Description>

<rdf:Description rdf:about="http://vocab.aodn.org.au/def/organisation/entity/47">
	<rdf:type rdf:resource="http://www.w3.org/2000/01/rdf-schema#Resource"/>
	<rdf:type rdf:resource="http://www.w3.org/2004/02/skos/core#Concept"/>
	<dcterms:modified rdf:datatype="http://www.w3.org/2001/XMLSchema#dateTime">2015-05-12T01:04:45Z</dcterms:modified>
	<dcterms:creator rdf:datatype="http://www.w3.org/2001/XMLSchema#string">Natalia Atkins</dcterms:creator>
	<dcterms:created rdf:datatype="http://www.w3.org/2001/XMLSchema#dateTime">2015-04-27T10:38:15Z</dcterms:created>
	<skos:broadMatch rdf:resource="http://vocab.aodn.org.au/def/organisation_classes/category/6"/>
	<skos:prefLabel xml:lang="en">Coastalwatch</skos:prefLabel>
	<skos:definition xml:lang="en">Since 1998, Coastalwatch has provided live camera vision, daily surf reports and forecasts and news and features from around the country’s coast. It provides Australia’s most comprehensive coastal reference site.</skos:definition>
	<dc:source rdf:datatype="http://www.w3.org/2001/XMLSchema#string">Australian Ocean Data Network Organisation Register</dc:source>
	<dc:publisher rdf:datatype="http://www.w3.org/2001/XMLSchema#string">eMarine Information Infrastructure (eMII)</dc:publisher>
	<skos:exactMatch rdf:resource="http://seadatanet.maris2.nl/v_edmo/print.asp?n_code=3937"/>
	<skos:topConceptOf rdf:resource="http://vocab.aodn.org.au/def/organisation/1"/>
	<skos:inScheme rdf:resource="http://vocab.aodn.org.au/def/organisation/1"/>
</rdf:Description>

<rdf:Description rdf:about="http://vocab.aodn.org.au/def/organisation/entity/48">
	<rdf:type rdf:resource="http://www.w3.org/2000/01/rdf-schema#Resource"/>
	<rdf:type rdf:resource="http://www.w3.org/2004/02/skos/core#Concept"/>
	<dcterms:modified rdf:datatype="http://www.w3.org/2001/XMLSchema#dateTime">2015-05-12T01:04:56Z</dcterms:modified>
	<dcterms:creator rdf:datatype="http://www.w3.org/2001/XMLSchema#string">Natalia Atkins</dcterms:creator>
	<dcterms:created rdf:datatype="http://www.w3.org/2001/XMLSchema#dateTime">2015-04-27T10:38:15Z</dcterms:created>
	<skos:broadMatch rdf:resource="http://vocab.aodn.org.au/def/organisation_classes/category/5"/>
	<skos:prefLabel xml:lang="en">ConocoPhillips Australia Pty Ltd</skos:prefLabel>
	<skos:definition xml:lang="en">This is the Australian operation of one of the world's largest independent oil and gas exploration and production company, which is headquartered in Houston, USA. ConocoPhillips established operations in Australia almost two decades ago.</skos:definition>
	<dc:source rdf:datatype="http://www.w3.org/2001/XMLSchema#string">Australian Ocean Data Network Organisation Register</dc:source>
	<dc:publisher rdf:datatype="http://www.w3.org/2001/XMLSchema#string">eMarine Information Infrastructure (eMII)</dc:publisher>
	<skos:exactMatch rdf:resource="http://seadatanet.maris2.nl/v_edmo/print.asp?n_code=4079"/>
	<skos:topConceptOf rdf:resource="http://vocab.aodn.org.au/def/organisation/1"/>
	<skos:inScheme rdf:resource="http://vocab.aodn.org.au/def/organisation/1"/>
</rdf:Description>

<rdf:Description rdf:about="http://vocab.aodn.org.au/def/organisation/entity/49">
	<rdf:type rdf:resource="http://www.w3.org/2000/01/rdf-schema#Resource"/>
	<rdf:type rdf:resource="http://www.w3.org/2004/02/skos/core#Concept"/>
	<dcterms:modified rdf:datatype="http://www.w3.org/2001/XMLSchema#dateTime">2015-05-12T01:05:42Z</dcterms:modified>
	<dcterms:creator rdf:datatype="http://www.w3.org/2001/XMLSchema#string">Natalia Atkins</dcterms:creator>
	<dcterms:created rdf:datatype="http://www.w3.org/2001/XMLSchema#dateTime">2015-04-27T10:38:15Z</dcterms:created>
	<skos:broadMatch rdf:resource="http://vocab.aodn.org.au/def/organisation_classes/category/6"/>
	<skos:prefLabel xml:lang="en">Conservation Council of Western Australia (CCWA)</skos:prefLabel>
	<skos:hiddenLabel xml:lang="en">CCWA</skos:hiddenLabel>
	<skos:definition xml:lang="en">The Conservation Council of Western Australia (CCWA) is a non-profit, non-government conservation organisation.</skos:definition>
	<dc:source rdf:datatype="http://www.w3.org/2001/XMLSchema#string">Australian Ocean Data Network Organisation Register</dc:source>
	<dc:publisher rdf:datatype="http://www.w3.org/2001/XMLSchema#string">eMarine Information Infrastructure (eMII)</dc:publisher>
	<skos:exactMatch rdf:resource="http://seadatanet.maris2.nl/v_edmo/print.asp?n_code=4080"/>
	<skos:topConceptOf rdf:resource="http://vocab.aodn.org.au/def/organisation/1"/>
	<skos:inScheme rdf:resource="http://vocab.aodn.org.au/def/organisation/1"/>
</rdf:Description>

<rdf:Description rdf:about="http://vocab.aodn.org.au/def/organisation/entity/50">
	<rdf:type rdf:resource="http://www.w3.org/2000/01/rdf-schema#Resource"/>
	<rdf:type rdf:resource="http://www.w3.org/2004/02/skos/core#Concept"/>
	<dcterms:creator rdf:datatype="http://www.w3.org/2001/XMLSchema#string">Natalia Atkins</dcterms:creator>
	<dcterms:created rdf:datatype="http://www.w3.org/2001/XMLSchema#dateTime">2015-04-27T10:38:15Z</dcterms:created>
	<skos:broadMatch rdf:resource="http://vocab.aodn.org.au/def/organisation_classes/category/6"/>
	<skos:prefLabel xml:lang="en">Coral Reef Research</skos:prefLabel>
	<skos:definition xml:lang="en">Coral Reef Research built and published the three volume book Corals of the World in 2000 followed by Coral ID in 2002 and in 2015 will be releasing a website: Corals of the World.</skos:definition>
	<dc:source rdf:datatype="http://www.w3.org/2001/XMLSchema#string">Australian Ocean Data Network Organisation Register</dc:source>
	<dc:publisher rdf:datatype="http://www.w3.org/2001/XMLSchema#string">eMarine Information Infrastructure (eMII)</dc:publisher>
	<skos:exactMatch rdf:resource="http://seadatanet.maris2.nl/v_edmo/print.asp?n_code=4081"/>
	<skos:topConceptOf rdf:resource="http://vocab.aodn.org.au/def/organisation/1"/>
	<skos:inScheme rdf:resource="http://vocab.aodn.org.au/def/organisation/1"/>
</rdf:Description>

<rdf:Description rdf:about="http://vocab.aodn.org.au/def/organisation/entity/51">
	<rdf:type rdf:resource="http://www.w3.org/2000/01/rdf-schema#Resource"/>
	<rdf:type rdf:resource="http://www.w3.org/2004/02/skos/core#Concept"/>
	<dcterms:modified rdf:datatype="http://www.w3.org/2001/XMLSchema#dateTime">2015-05-12T01:12:36Z</dcterms:modified>
	<dcterms:creator rdf:datatype="http://www.w3.org/2001/XMLSchema#string">Natalia Atkins</dcterms:creator>
	<dcterms:created rdf:datatype="http://www.w3.org/2001/XMLSchema#dateTime">2015-04-27T10:38:15Z</dcterms:created>
	<skos:broadMatch rdf:resource="http://vocab.aodn.org.au/def/organisation_classes/category/7"/>
	<skos:prefLabel xml:lang="en">Council of Heads of Australian Faunal Collections (CHAFC)</skos:prefLabel>
	<skos:hiddenLabel xml:lang="en">CHAFC</skos:hiddenLabel>
	<skos:definition xml:lang="en">Council of Heads of Australian Faunal Collections Incorporated (ACT) is the peak body representing Australia’s publicly accessible zoological and palaeontological collections, primarily within the jurisdiction of regional, state and territory, and commonwealth governments.</skos:definition>
	<dc:source rdf:datatype="http://www.w3.org/2001/XMLSchema#string">Australian Ocean Data Network Organisation Register</dc:source>
	<dc:publisher rdf:datatype="http://www.w3.org/2001/XMLSchema#string">eMarine Information Infrastructure (eMII)</dc:publisher>
	<skos:exactMatch rdf:resource="http://seadatanet.maris2.nl/v_edmo/print.asp?n_code=4082"/>
	<skos:topConceptOf rdf:resource="http://vocab.aodn.org.au/def/organisation/1"/>
	<skos:inScheme rdf:resource="http://vocab.aodn.org.au/def/organisation/1"/>
</rdf:Description>

<rdf:Description rdf:about="http://vocab.aodn.org.au/def/organisation/entity/52">
	<rdf:type rdf:resource="http://www.w3.org/2000/01/rdf-schema#Resource"/>
	<rdf:type rdf:resource="http://www.w3.org/2004/02/skos/core#Concept"/>
	<dcterms:modified rdf:datatype="http://www.w3.org/2001/XMLSchema#dateTime">2015-05-12T01:12:44Z</dcterms:modified>
	<dcterms:creator rdf:datatype="http://www.w3.org/2001/XMLSchema#string">Natalia Atkins</dcterms:creator>
	<dcterms:created rdf:datatype="http://www.w3.org/2001/XMLSchema#dateTime">2015-04-27T10:38:15Z</dcterms:created>
	<skos:broadMatch rdf:resource="http://vocab.aodn.org.au/def/organisation_classes/category/5"/>
	<skos:prefLabel xml:lang="en">D.A. Lord and Associates Pty Ltd (DAL)</skos:prefLabel>
	<skos:hiddenLabel xml:lang="en">DAL</skos:hiddenLabel>
	<skos:definition xml:lang="en">D.A Lord and Associates provided marine and coastal environmental consulting services. This company became known as DAL Science and Engineering (DALSE), then Oceanica, and is now part of BMT Oceanica.</skos:definition>
	<dc:source rdf:datatype="http://www.w3.org/2001/XMLSchema#string">Australian Ocean Data Network Organisation Register</dc:source>
	<dc:publisher rdf:datatype="http://www.w3.org/2001/XMLSchema#string">eMarine Information Infrastructure (eMII)</dc:publisher>
	<skos:topConceptOf rdf:resource="http://vocab.aodn.org.au/def/organisation/1"/>
	<skos:inScheme rdf:resource="http://vocab.aodn.org.au/def/organisation/1"/>
	<skos:scopeNote xml:lang="en">Organisation no longer exists</skos:scopeNote>
</rdf:Description>

<rdf:Description rdf:about="http://vocab.aodn.org.au/def/organisation/entity/53">
	<rdf:type rdf:resource="http://www.w3.org/2000/01/rdf-schema#Resource"/>
	<rdf:type rdf:resource="http://www.w3.org/2004/02/skos/core#Concept"/>
	<dcterms:modified rdf:datatype="http://www.w3.org/2001/XMLSchema#dateTime">2015-05-12T01:13:24Z</dcterms:modified>
	<dcterms:creator rdf:datatype="http://www.w3.org/2001/XMLSchema#string">Natalia Atkins</dcterms:creator>
	<dcterms:created rdf:datatype="http://www.w3.org/2001/XMLSchema#dateTime">2015-04-27T10:38:15Z</dcterms:created>
	<skos:broadMatch rdf:resource="http://vocab.aodn.org.au/def/organisation_classes/category/5"/>
	<skos:prefLabel xml:lang="en">Dcafe</skos:prefLabel>
	<skos:definition xml:lang="en">DCafe is an economics consultancy company.</skos:definition>
	<dc:source rdf:datatype="http://www.w3.org/2001/XMLSchema#string">Australian Ocean Data Network Organisation Register</dc:source>
	<dc:publisher rdf:datatype="http://www.w3.org/2001/XMLSchema#string">eMarine Information Infrastructure (eMII)</dc:publisher>
	<skos:exactMatch rdf:resource="http://seadatanet.maris2.nl/v_edmo/print.asp?n_code=4083"/>
	<skos:topConceptOf rdf:resource="http://vocab.aodn.org.au/def/organisation/1"/>
	<skos:inScheme rdf:resource="http://vocab.aodn.org.au/def/organisation/1"/>
</rdf:Description>

<rdf:Description rdf:about="http://vocab.aodn.org.au/def/organisation/entity/54">
	<rdf:type rdf:resource="http://www.w3.org/2000/01/rdf-schema#Resource"/>
	<rdf:type rdf:resource="http://www.w3.org/2004/02/skos/core#Concept"/>
	<dcterms:modified rdf:datatype="http://www.w3.org/2001/XMLSchema#dateTime">2015-05-12T01:15:42Z</dcterms:modified>
	<dcterms:modified rdf:datatype="http://www.w3.org/2001/XMLSchema#dateTime">2016-01-28T04:30:57Z</dcterms:modified>
	<dcterms:creator rdf:datatype="http://www.w3.org/2001/XMLSchema#string">Natalia Atkins</dcterms:creator>
	<dcterms:created rdf:datatype="http://www.w3.org/2001/XMLSchema#dateTime">2015-04-27T10:38:15Z</dcterms:created>
	<dcterms:contributor rdf:datatype="http://www.w3.org/2001/XMLSchema#string">eMII_Atkins.Natalia</dcterms:contributor>
	<skos:broadMatch rdf:resource="http://vocab.aodn.org.au/def/organisation_classes/category/2"/>
	<skos:prefLabel xml:lang="en">Department of Environment, Land, Water and Planning (DELWP), Victorian Government</skos:prefLabel>
	<skos:altLabel xml:lang="en">Department of Environment, Land, Water and Planning (DELWP)</skos:altLabel>
	<skos:hiddenLabel xml:lang="en">DELWP</skos:hiddenLabel>
	<skos:definition xml:lang="en">The Department of Environment, Land, Water and Planning replaced the former government's Department of Environment and Primary Industries, in 2014. The department is tasked with creating liveable, inclusive and sustainable communities, with a focus on caring for and protecting the environment, and helping to respond to climate change through risk mitigation and adaptation strategies.</skos:definition>
	<dc:source rdf:datatype="http://www.w3.org/2001/XMLSchema#string">Australian Ocean Data Network Organisation Register</dc:source>
	<dc:publisher rdf:datatype="http://www.w3.org/2001/XMLSchema#string">eMarine Information Infrastructure (eMII)</dc:publisher>
	<skos:exactMatch rdf:resource="http://seadatanet.maris2.nl/v_edmo/print.asp?n_code=4030"/>
	<skos:topConceptOf rdf:resource="http://vocab.aodn.org.au/def/organisation/1"/>
	<skos:inScheme rdf:resource="http://vocab.aodn.org.au/def/organisation/1"/>
	<skos:scopeNote xml:lang="en">Replaces http://vocab.aodn.org.au/def/organisation/entity/57 and http://vocab.aodn.org.au/def/organisation/entity/127</skos:scopeNote>
	<dcterms:replaces rdf:resource="http://vocab.aodn.org.au/def/organisation/entity/57"/>
	<dcterms:replaces xml:lang="en">Department of Primary Industries (DPI), Victorian Government</dcterms:replaces>
	<dcterms:replaces xml:lang="en">Victorian Institute of Marine Sciences (VIMS)</dcterms:replaces>
</rdf:Description>

<rdf:Description rdf:about="http://vocab.aodn.org.au/def/organisation/entity/55">
	<rdf:type rdf:resource="http://www.w3.org/2000/01/rdf-schema#Resource"/>
	<rdf:type rdf:resource="http://www.w3.org/2004/02/skos/core#Concept"/>
	<dcterms:modified rdf:datatype="http://www.w3.org/2001/XMLSchema#dateTime">2015-05-12T01:21:08Z</dcterms:modified>
	<dcterms:creator rdf:datatype="http://www.w3.org/2001/XMLSchema#string">Natalia Atkins</dcterms:creator>
	<dcterms:created rdf:datatype="http://www.w3.org/2001/XMLSchema#dateTime">2015-04-27T10:38:15Z</dcterms:created>
	<skos:broadMatch rdf:resource="http://vocab.aodn.org.au/def/organisation_classes/category/2"/>
	<skos:prefLabel xml:lang="en">Environment Protection Authority Victoria (EPA), Victorian Government</skos:prefLabel>
	<skos:altLabel xml:lang="en">Environment Protection Authority Victoria (EPA)</skos:altLabel>
	<skos:hiddenLabel xml:lang="en">EPA Vic</skos:hiddenLabel>
	<skos:definition xml:lang="en">Environment Protection Authority (EPA) Victoria was established in 1971 under the auspices of the Environment Protection Act 1970. It's role is to be an effective environmental regulator and an influential authority on environmental impacts, with a vision for a healthy environment that supports a liveable and prosperous Victoria.</skos:definition>
	<dc:source rdf:datatype="http://www.w3.org/2001/XMLSchema#string">Australian Ocean Data Network Organisation Register</dc:source>
	<dc:publisher rdf:datatype="http://www.w3.org/2001/XMLSchema#string">eMarine Information Infrastructure (eMII)</dc:publisher>
	<skos:exactMatch rdf:resource="http://seadatanet.maris2.nl/v_edmo/print.asp?n_code=3944"/>
	<skos:topConceptOf rdf:resource="http://vocab.aodn.org.au/def/organisation/1"/>
	<skos:inScheme rdf:resource="http://vocab.aodn.org.au/def/organisation/1"/>
</rdf:Description>

<rdf:Description rdf:about="http://vocab.aodn.org.au/def/organisation/entity/56">
	<rdf:type rdf:resource="http://www.w3.org/2000/01/rdf-schema#Resource"/>
	<rdf:type rdf:resource="http://www.w3.org/2004/02/skos/core#Concept"/>
	<dcterms:modified rdf:datatype="http://www.w3.org/2001/XMLSchema#dateTime">2015-06-24T02:11:16Z</dcterms:modified>
	<dcterms:creator rdf:datatype="http://www.w3.org/2001/XMLSchema#string">Natalia Atkins</dcterms:creator>
	<dcterms:created rdf:datatype="http://www.w3.org/2001/XMLSchema#dateTime">2015-04-27T10:38:15Z</dcterms:created>
	<dcterms:contributor rdf:datatype="http://www.w3.org/2001/XMLSchema#string">eMII_Finney.Kim</dcterms:contributor>
	<skos:broadMatch rdf:resource="http://vocab.aodn.org.au/def/organisation_classes/category/2"/>
	<skos:prefLabel xml:lang="en">Department of Primary Industries, Parks, Water and Environment (DPIPWE), Tasmanian Government</skos:prefLabel>
	<skos:altLabel xml:lang="en">Department of Primary Industries, Parks, Water and Environment (DPIPWE)</skos:altLabel>
	<skos:hiddenLabel xml:lang="en">DPIPWE</skos:hiddenLabel>
	<skos:definition xml:lang="en">The Department of Primary Industries, Parks, Water and Environment (DPIPWE) is responsible for the sustainable management and protection of Tasmania's natural and cultural assets for the benefit of Tasmanian communities and the economy.</skos:definition>
	<dc:source rdf:datatype="http://www.w3.org/2001/XMLSchema#string">Australian Ocean Data Network Organisation Register</dc:source>
	<dc:publisher rdf:datatype="http://www.w3.org/2001/XMLSchema#string">eMarine Information Infrastructure (eMII)</dc:publisher>
	<skos:exactMatch rdf:resource="http://seadatanet.maris2.nl/v_edmo/print.asp?n_code=3946"/>
	<skos:topConceptOf rdf:resource="http://vocab.aodn.org.au/def/organisation/1"/>
	<skos:inScheme rdf:resource="http://vocab.aodn.org.au/def/organisation/1"/>
	<skos:scopeNote xml:lang="en">Replaces http://vocab.aodn.org.au/def/organisation/entity/171</skos:scopeNote>
	<dcterms:replaces xml:lang="en">http://vocab.aodn.org.au/def/organisation/entity/171</dcterms:replaces>
	<dcterms:replaces xml:lang="en">Department of Primary Industries and Fisheries, Tasmanian Government</dcterms:replaces>
</rdf:Description>

<rdf:Description rdf:about="http://vocab.aodn.org.au/def/organisation/entity/57">
	<rdf:type rdf:resource="http://www.w3.org/2000/01/rdf-schema#Resource"/>
	<rdf:type rdf:resource="http://www.w3.org/2004/02/skos/core#Concept"/>
	<dcterms:modified rdf:datatype="http://www.w3.org/2001/XMLSchema#dateTime">2015-05-12T01:17:14Z</dcterms:modified>
	<dcterms:modified rdf:datatype="http://www.w3.org/2001/XMLSchema#dateTime">2016-01-28T04:30:34Z</dcterms:modified>
	<dcterms:creator rdf:datatype="http://www.w3.org/2001/XMLSchema#string">Natalia Atkins</dcterms:creator>
	<dcterms:created rdf:datatype="http://www.w3.org/2001/XMLSchema#dateTime">2015-04-27T10:38:15Z</dcterms:created>
	<dcterms:contributor rdf:datatype="http://www.w3.org/2001/XMLSchema#string">eMII_Atkins.Natalia</dcterms:contributor>
	<skos:broadMatch rdf:resource="http://vocab.aodn.org.au/def/organisation_classes/category/2"/>
	<skos:prefLabel xml:lang="en">Department of Primary Industries (DPI), Victorian Government</skos:prefLabel>
	<skos:altLabel xml:lang="en">Department of Primary Industries (DPI)</skos:altLabel>
	<skos:hiddenLabel xml:lang="en">DPI</skos:hiddenLabel>
	<skos:definition xml:lang="en">The Department of Primary Industries was a government agency responsible for agriculture, biosecurity, fisheries, earth resources, energy and forestry policy and programs in the State of Victoria, Australia. The Department of Primary Industries (DPI) was established in 2002. It was formed from the split of the Department of Natural Resources and Environment (1996–2002) which was divided into two separate entities: The Department of Sustainability and Environment and The Department of Primary Industries. The Department of Primary Industries was merged with the Department of Sustainability and Environment to form the Department of Environment and Primary Industries (Victoria) in April 2013. (Courtesy of Wikipedia)</skos:definition>
	<dc:source rdf:datatype="http://www.w3.org/2001/XMLSchema#string">Australian Ocean Data Network Organisation Register</dc:source>
	<dc:publisher rdf:datatype="http://www.w3.org/2001/XMLSchema#string">eMarine Information Infrastructure (eMII)</dc:publisher>
	<skos:topConceptOf rdf:resource="http://vocab.aodn.org.au/def/organisation/1"/>
	<skos:inScheme rdf:resource="http://vocab.aodn.org.au/def/organisation/1"/>
	<skos:scopeNote xml:lang="en">Organisation no longer exists</skos:scopeNote>
	<skos:scopeNote xml:lang="en">Organisation no longer exists. Replaced by http://vocab.aodn.org.au/def/organisation/entity/54. Replaces http://vocab.aodn.org.au/def/organisation/entity/127</skos:scopeNote>
	<dcterms:replaces xml:lang="en">Victorian Institute of Marine Sciences (VIMS)</dcterms:replaces>
	<dcterms:isReplacedBy rdf:resource="http://vocab.aodn.org.au/def/organisation/entity/54"/>
	<dcterms:isReplacedBy xml:lang="en">Department of Environment, Land, Water and Planning (DELWP), Victorian Government</dcterms:isReplacedBy>
</rdf:Description>

<rdf:Description rdf:about="http://vocab.aodn.org.au/def/organisation/entity/58">
	<rdf:type rdf:resource="http://www.w3.org/2000/01/rdf-schema#Resource"/>
	<rdf:type rdf:resource="http://www.w3.org/2004/02/skos/core#Concept"/>
	<dcterms:modified rdf:datatype="http://www.w3.org/2001/XMLSchema#dateTime">2015-05-12T01:15:36Z</dcterms:modified>
	<dcterms:creator rdf:datatype="http://www.w3.org/2001/XMLSchema#string">Natalia Atkins</dcterms:creator>
	<dcterms:created rdf:datatype="http://www.w3.org/2001/XMLSchema#dateTime">2015-04-27T10:38:15Z</dcterms:created>
	<skos:broadMatch rdf:resource="http://vocab.aodn.org.au/def/organisation_classes/category/2"/>
	<skos:prefLabel xml:lang="en">Department of Environment and Heritage Protection, Queensland Government</skos:prefLabel>
	<skos:altLabel xml:lang="en">Department of Environment and Heritage Protection</skos:altLabel>
	<skos:definition xml:lang="en">This department is responsible for managing the health of the environment to protect Queensland’s unique ecosystems, including its landscapes and waterways, as well as its native plants and animals and biodiversity.</skos:definition>
	<dc:source rdf:datatype="http://www.w3.org/2001/XMLSchema#string">Australian Ocean Data Network Organisation Register</dc:source>
	<dc:publisher rdf:datatype="http://www.w3.org/2001/XMLSchema#string">eMarine Information Infrastructure (eMII)</dc:publisher>
	<skos:exactMatch rdf:resource="http://seadatanet.maris2.nl/v_edmo/print.asp?n_code=4084"/>
	<skos:topConceptOf rdf:resource="http://vocab.aodn.org.au/def/organisation/1"/>
	<skos:inScheme rdf:resource="http://vocab.aodn.org.au/def/organisation/1"/>
</rdf:Description>

<rdf:Description rdf:about="http://vocab.aodn.org.au/def/organisation/entity/59">
	<rdf:type rdf:resource="http://www.w3.org/2000/01/rdf-schema#Resource"/>
	<rdf:type rdf:resource="http://www.w3.org/2004/02/skos/core#Concept"/>
	<dcterms:modified rdf:datatype="http://www.w3.org/2001/XMLSchema#dateTime">2015-05-12T01:13:50Z</dcterms:modified>
	<dcterms:creator rdf:datatype="http://www.w3.org/2001/XMLSchema#string">Natalia Atkins</dcterms:creator>
	<dcterms:created rdf:datatype="http://www.w3.org/2001/XMLSchema#dateTime">2015-04-27T10:38:15Z</dcterms:created>
	<skos:broadMatch rdf:resource="http://vocab.aodn.org.au/def/organisation_classes/category/2"/>
	<skos:prefLabel xml:lang="en">Department of Agriculture and Fisheries, Queensland Government</skos:prefLabel>
	<skos:altLabel xml:lang="en">Department of Agriculture and Fisheries</skos:altLabel>
	<skos:definition xml:lang="en">The Department's work spans across the agriculture, fisheries and forestry industries and includes provision of agricultural research, development and extension for the management of biological, animal welfare and product integrity risks.</skos:definition>
	<dc:source rdf:datatype="http://www.w3.org/2001/XMLSchema#string">Australian Ocean Data Network Organisation Register</dc:source>
	<dc:publisher rdf:datatype="http://www.w3.org/2001/XMLSchema#string">eMarine Information Infrastructure (eMII)</dc:publisher>
	<skos:exactMatch rdf:resource="http://seadatanet.maris2.nl/v_edmo/print.asp?n_code=4085"/>
	<skos:topConceptOf rdf:resource="http://vocab.aodn.org.au/def/organisation/1"/>
	<skos:inScheme rdf:resource="http://vocab.aodn.org.au/def/organisation/1"/>
</rdf:Description>

<rdf:Description rdf:about="http://vocab.aodn.org.au/def/organisation/entity/60">
	<rdf:type rdf:resource="http://www.w3.org/2000/01/rdf-schema#Resource"/>
	<rdf:type rdf:resource="http://www.w3.org/2004/02/skos/core#Concept"/>
	<dcterms:modified rdf:datatype="http://www.w3.org/2001/XMLSchema#dateTime">2015-05-12T01:29:00Z</dcterms:modified>
	<dcterms:creator rdf:datatype="http://www.w3.org/2001/XMLSchema#string">Natalia Atkins</dcterms:creator>
	<dcterms:created rdf:datatype="http://www.w3.org/2001/XMLSchema#dateTime">2015-04-27T10:38:15Z</dcterms:created>
	<skos:broadMatch rdf:resource="http://vocab.aodn.org.au/def/organisation_classes/category/2"/>
	<skos:prefLabel xml:lang="en">NSW Water Information, New South Wales Government</skos:prefLabel>
	<skos:altLabel xml:lang="en">NSW Water Information</skos:altLabel>
	<skos:definition xml:lang="en">The NSW Government WaterInfo website contains a range of provisional data from a range of State Government agencies concerning NSW rivers and water bodies. This data is generally used for the management of our rivers, storages and the surrounding environment.</skos:definition>
	<dc:source rdf:datatype="http://www.w3.org/2001/XMLSchema#string">Australian Ocean Data Network Organisation Register</dc:source>
	<dc:publisher rdf:datatype="http://www.w3.org/2001/XMLSchema#string">eMarine Information Infrastructure (eMII)</dc:publisher>
	<skos:exactMatch rdf:resource="http://seadatanet.maris2.nl/v_edmo/print.asp?n_code=4086"/>
	<skos:topConceptOf rdf:resource="http://vocab.aodn.org.au/def/organisation/1"/>
	<skos:inScheme rdf:resource="http://vocab.aodn.org.au/def/organisation/1"/>
</rdf:Description>

<rdf:Description rdf:about="http://vocab.aodn.org.au/def/organisation/entity/61">
	<rdf:type rdf:resource="http://www.w3.org/2000/01/rdf-schema#Resource"/>
	<rdf:type rdf:resource="http://www.w3.org/2004/02/skos/core#Concept"/>
	<dcterms:modified rdf:datatype="http://www.w3.org/2001/XMLSchema#dateTime">2015-05-12T01:26:49Z</dcterms:modified>
	<dcterms:creator rdf:datatype="http://www.w3.org/2001/XMLSchema#string">Natalia Atkins</dcterms:creator>
	<dcterms:created rdf:datatype="http://www.w3.org/2001/XMLSchema#dateTime">2015-04-27T10:38:15Z</dcterms:created>
	<skos:broadMatch rdf:resource="http://vocab.aodn.org.au/def/organisation_classes/category/2"/>
	<skos:prefLabel xml:lang="en">Land and Property Information, New South Wales Government</skos:prefLabel>
	<skos:altLabel xml:lang="en">Land and Property Information</skos:altLabel>
	<skos:definition xml:lang="en">Land and Property Information (LPI), a division of the Office of Finance and Services, is the key provider of land information services in New South Wales.</skos:definition>
	<dc:source rdf:datatype="http://www.w3.org/2001/XMLSchema#string">Australian Ocean Data Network Organisation Register</dc:source>
	<dc:publisher rdf:datatype="http://www.w3.org/2001/XMLSchema#string">eMarine Information Infrastructure (eMII)</dc:publisher>
	<skos:exactMatch rdf:resource="http://seadatanet.maris2.nl/v_edmo/print.asp?n_code=4087"/>
	<skos:topConceptOf rdf:resource="http://vocab.aodn.org.au/def/organisation/1"/>
	<skos:inScheme rdf:resource="http://vocab.aodn.org.au/def/organisation/1"/>
</rdf:Description>

<rdf:Description rdf:about="http://vocab.aodn.org.au/def/organisation/entity/62">
	<rdf:type rdf:resource="http://www.w3.org/2000/01/rdf-schema#Resource"/>
	<rdf:type rdf:resource="http://www.w3.org/2004/02/skos/core#Concept"/>
	<dcterms:modified rdf:datatype="http://www.w3.org/2001/XMLSchema#dateTime">2015-05-12T01:17:08Z</dcterms:modified>
	<dcterms:creator rdf:datatype="http://www.w3.org/2001/XMLSchema#string">Natalia Atkins</dcterms:creator>
	<dcterms:created rdf:datatype="http://www.w3.org/2001/XMLSchema#dateTime">2015-04-27T10:38:15Z</dcterms:created>
	<skos:broadMatch rdf:resource="http://vocab.aodn.org.au/def/organisation_classes/category/2"/>
	<skos:prefLabel xml:lang="en">Department of Primary Industries (DPI), New South Wales Government</skos:prefLabel>
	<skos:altLabel xml:lang="en">Department of Primary Industries (DPI)</skos:altLabel>
	<skos:hiddenLabel xml:lang="en">DPI</skos:hiddenLabel>
	<skos:definition xml:lang="en">The Department of Primary Industries is a division within NSW Trade and Investment and works to develop and sustain diverse, profitable food and fibre industries, and ensures best practice management of our natural resources.</skos:definition>
	<dc:source rdf:datatype="http://www.w3.org/2001/XMLSchema#string">Australian Ocean Data Network Organisation Register</dc:source>
	<dc:publisher rdf:datatype="http://www.w3.org/2001/XMLSchema#string">eMarine Information Infrastructure (eMII)</dc:publisher>
	<skos:exactMatch rdf:resource="http://seadatanet.maris2.nl/v_edmo/print.asp?n_code=4088"/>
	<skos:topConceptOf rdf:resource="http://vocab.aodn.org.au/def/organisation/1"/>
	<skos:inScheme rdf:resource="http://vocab.aodn.org.au/def/organisation/1"/>
</rdf:Description>

<rdf:Description rdf:about="http://vocab.aodn.org.au/def/organisation/entity/63">
	<rdf:type rdf:resource="http://www.w3.org/2000/01/rdf-schema#Resource"/>
	<rdf:type rdf:resource="http://www.w3.org/2004/02/skos/core#Concept"/>
	<dcterms:modified rdf:datatype="http://www.w3.org/2001/XMLSchema#dateTime">2015-05-12T01:15:51Z</dcterms:modified>
	<dcterms:creator rdf:datatype="http://www.w3.org/2001/XMLSchema#string">Natalia Atkins</dcterms:creator>
	<dcterms:created rdf:datatype="http://www.w3.org/2001/XMLSchema#dateTime">2015-04-27T10:38:15Z</dcterms:created>
	<skos:broadMatch rdf:resource="http://vocab.aodn.org.au/def/organisation_classes/category/2"/>
	<skos:prefLabel xml:lang="en">Department of Fisheries (DoF), Western Australian Government</skos:prefLabel>
	<skos:altLabel xml:lang="en">Department of Fisheries (DoF)</skos:altLabel>
	<skos:hiddenLabel xml:lang="en">DoF</skos:hiddenLabel>
	<skos:definition xml:lang="en">The Department of Fisheries’ primary responsibility is to conserve, develop and manage the fish and aquatic resources of Western Australia to ensure there are ‘fish for the future’.</skos:definition>
	<dc:source rdf:datatype="http://www.w3.org/2001/XMLSchema#string">Australian Ocean Data Network Organisation Register</dc:source>
	<dc:publisher rdf:datatype="http://www.w3.org/2001/XMLSchema#string">eMarine Information Infrastructure (eMII)</dc:publisher>
	<skos:exactMatch rdf:resource="http://seadatanet.maris2.nl/v_edmo/print.asp?n_code=3958"/>
	<skos:topConceptOf rdf:resource="http://vocab.aodn.org.au/def/organisation/1"/>
	<skos:inScheme rdf:resource="http://vocab.aodn.org.au/def/organisation/1"/>
</rdf:Description>

<rdf:Description rdf:about="http://vocab.aodn.org.au/def/organisation/entity/64">
	<rdf:type rdf:resource="http://www.w3.org/2000/01/rdf-schema#Resource"/>
	<rdf:type rdf:resource="http://www.w3.org/2004/02/skos/core#Concept"/>
	<dcterms:modified rdf:datatype="http://www.w3.org/2001/XMLSchema#dateTime">2015-05-12T01:18:12Z</dcterms:modified>
	<dcterms:creator rdf:datatype="http://www.w3.org/2001/XMLSchema#string">Natalia Atkins</dcterms:creator>
	<dcterms:created rdf:datatype="http://www.w3.org/2001/XMLSchema#dateTime">2015-04-27T10:38:15Z</dcterms:created>
	<skos:broadMatch rdf:resource="http://vocab.aodn.org.au/def/organisation_classes/category/2"/>
	<skos:prefLabel xml:lang="en">Department of Water (DoW), Western Australian Government</skos:prefLabel>
	<skos:altLabel xml:lang="en">Department of Water (DoW)</skos:altLabel>
	<skos:hiddenLabel xml:lang="en">DOW</skos:hiddenLabel>
	<skos:definition xml:lang="en">The Department of Water is the department of the Government of Western Australia that is responsible for management of Western Australia's water resources. The department provides information to industry, technical support and professional guidance to government on the status of water and the viability of new water source developments. It also issues licences for artesian groundwater wells throughout the State. (Courtesy of Wikipedia)</skos:definition>
	<dc:source rdf:datatype="http://www.w3.org/2001/XMLSchema#string">Australian Ocean Data Network Organisation Register</dc:source>
	<dc:publisher rdf:datatype="http://www.w3.org/2001/XMLSchema#string">eMarine Information Infrastructure (eMII)</dc:publisher>
	<skos:exactMatch rdf:resource="http://seadatanet.maris2.nl/v_edmo/print.asp?n_code=3959"/>
	<skos:topConceptOf rdf:resource="http://vocab.aodn.org.au/def/organisation/1"/>
	<skos:inScheme rdf:resource="http://vocab.aodn.org.au/def/organisation/1"/>
</rdf:Description>

<rdf:Description rdf:about="http://vocab.aodn.org.au/def/organisation/entity/65">
	<rdf:type rdf:resource="http://www.w3.org/2000/01/rdf-schema#Resource"/>
	<rdf:type rdf:resource="http://www.w3.org/2004/02/skos/core#Concept"/>
	<dcterms:modified rdf:datatype="http://www.w3.org/2001/XMLSchema#dateTime">2015-05-12T01:15:14Z</dcterms:modified>
	<dcterms:creator rdf:datatype="http://www.w3.org/2001/XMLSchema#string">Natalia Atkins</dcterms:creator>
	<dcterms:created rdf:datatype="http://www.w3.org/2001/XMLSchema#dateTime">2015-04-27T10:38:15Z</dcterms:created>
	<skos:broadMatch rdf:resource="http://vocab.aodn.org.au/def/organisation_classes/category/2"/>
	<skos:prefLabel xml:lang="en">Department of Environment and Conservation (DEC) , Western Australian Government</skos:prefLabel>
	<skos:altLabel xml:lang="en">Department of Environment and Conservation (DEC)</skos:altLabel>
	<skos:hiddenLabel xml:lang="en">DEC</skos:hiddenLabel>
	<skos:definition xml:lang="en">The Department of Environment and Conservation (DEC) was a department of the Government of Western Australia that was responsible for implementing the state's conservation and environment legislation and regulations. It was formed on 1 July 2006 by the amalgamation of the Department of Environment (DoE) and the Department of Conservation and Land Management (CALM). The DEC was separated on 30 June 2013 forming the Department of Parks and Wildlife (DPaW) and the Department of Environment Regulation (DER) which both commenced operations on 1 July 2013. (Courtesy of Wikipedia)</skos:definition>
	<dc:source rdf:datatype="http://www.w3.org/2001/XMLSchema#string">Australian Ocean Data Network Organisation Register</dc:source>
	<dc:publisher rdf:datatype="http://www.w3.org/2001/XMLSchema#string">eMarine Information Infrastructure (eMII)</dc:publisher>
	<skos:exactMatch rdf:resource="http://seadatanet.maris2.nl/v_edmo/print.asp?n_code=3948"/>
	<skos:topConceptOf rdf:resource="http://vocab.aodn.org.au/def/organisation/1"/>
	<skos:inScheme rdf:resource="http://vocab.aodn.org.au/def/organisation/1"/>
	<skos:scopeNote xml:lang="en">Organisation no longer exists</skos:scopeNote>
	<skos:scopeNote xml:lang="en">Organisation no longer exists. Replaced by http://vocab.aodn.org.au/def/organisation/entity/66 and http://vocab.aodn.org.au/def/organisation/entity/67</skos:scopeNote>
	<dcterms:isReplacedBy rdf:resource="http://vocab.aodn.org.au/def/organisation/entity/66"/>
	<dcterms:isReplacedBy rdf:resource="http://vocab.aodn.org.au/def/organisation/entity/67"/>
	<dcterms:isReplacedBy xml:lang="en">Department of Parks and Wildlife (DPaW), Western Australian Government</dcterms:isReplacedBy>
	<dcterms:isReplacedBy xml:lang="en">Department of Environment Regulation (DER), Western Australian Government</dcterms:isReplacedBy>
</rdf:Description>

<rdf:Description rdf:about="http://vocab.aodn.org.au/def/organisation/entity/66">
	<rdf:type rdf:resource="http://www.w3.org/2000/01/rdf-schema#Resource"/>
	<rdf:type rdf:resource="http://www.w3.org/2004/02/skos/core#Concept"/>
	<dcterms:modified rdf:datatype="http://www.w3.org/2001/XMLSchema#dateTime">2015-05-12T01:16:30Z</dcterms:modified>
	<dcterms:creator rdf:datatype="http://www.w3.org/2001/XMLSchema#string">Natalia Atkins</dcterms:creator>
	<dcterms:created rdf:datatype="http://www.w3.org/2001/XMLSchema#dateTime">2015-04-27T10:38:15Z</dcterms:created>
	<skos:broadMatch rdf:resource="http://vocab.aodn.org.au/def/organisation_classes/category/2"/>
	<skos:prefLabel xml:lang="en">Department of Parks and Wildlife (DPaW), Western Australian Government</skos:prefLabel>
	<skos:altLabel xml:lang="en">Department of Parks and Wildlife (DPaW)</skos:altLabel>
	<skos:hiddenLabel xml:lang="en">DPaW</skos:hiddenLabel>
	<skos:definition xml:lang="en">The Department of Parks and Wildlife protects and conserves the State’s natural environment on behalf of the people of Western Australia. Its key responsibilities include conserving biodiversity and managing the State’s national parks, marine parks and other reserves, which cover a total area of more than 27 million hectares. The department was established on 1 July 2013, when the former Department of Environment and Conservation was split into the Department of Parks and Wildlife and the Department of Enviroment Regulation, and is in the portfolio of the Minister for Environment.</skos:definition>
	<dc:source rdf:datatype="http://www.w3.org/2001/XMLSchema#string">Australian Ocean Data Network Organisation Register</dc:source>
	<dc:publisher rdf:datatype="http://www.w3.org/2001/XMLSchema#string">eMarine Information Infrastructure (eMII)</dc:publisher>
	<skos:exactMatch rdf:resource="http://seadatanet.maris2.nl/v_edmo/print.asp?n_code=3949"/>
	<skos:topConceptOf rdf:resource="http://vocab.aodn.org.au/def/organisation/1"/>
	<skos:inScheme rdf:resource="http://vocab.aodn.org.au/def/organisation/1"/>
	<skos:scopeNote xml:lang="en">Organisation no longer exists</skos:scopeNote>
	<skos:scopeNote xml:lang="en">Organisation no longer exists. Replaces http://vocab.aodn.org.au/def/organisation/entity/65</skos:scopeNote>
	<dcterms:replaces rdf:resource="http://vocab.aodn.org.au/def/organisation/entity/65"/>
	<dcterms:replaces xml:lang="en">Department of Environment and Conservation (DEC) , Western Australian Government</dcterms:replaces>
</rdf:Description>

<rdf:Description rdf:about="http://vocab.aodn.org.au/def/organisation/entity/67">
	<rdf:type rdf:resource="http://www.w3.org/2000/01/rdf-schema#Resource"/>
	<rdf:type rdf:resource="http://www.w3.org/2004/02/skos/core#Concept"/>
	<dcterms:modified rdf:datatype="http://www.w3.org/2001/XMLSchema#dateTime">2015-05-12T01:15:06Z</dcterms:modified>
	<dcterms:creator rdf:datatype="http://www.w3.org/2001/XMLSchema#string">Natalia Atkins</dcterms:creator>
	<dcterms:created rdf:datatype="http://www.w3.org/2001/XMLSchema#dateTime">2015-04-27T10:38:15Z</dcterms:created>
	<skos:broadMatch rdf:resource="http://vocab.aodn.org.au/def/organisation_classes/category/2"/>
	<skos:prefLabel xml:lang="en">Department of Environment Regulation (DER), Western Australian Government</skos:prefLabel>
	<skos:altLabel xml:lang="en">Department of Environment Regulation (DER)</skos:altLabel>
	<skos:hiddenLabel xml:lang="en">DER</skos:hiddenLabel>
	<skos:definition xml:lang="en">The Department focuses on environmental regulation, approvals and appeals processes, and pollution prevention. The department was established on 1 July 2013, when the former Department of Environment and Conservation was split into the Department of Parks and Wildlife and the Department of Enviroment Regulation. (Courtesy of Wikipedia)</skos:definition>
	<dc:source rdf:datatype="http://www.w3.org/2001/XMLSchema#string">Australian Ocean Data Network Organisation Register</dc:source>
	<dc:publisher rdf:datatype="http://www.w3.org/2001/XMLSchema#string">eMarine Information Infrastructure (eMII)</dc:publisher>
	<skos:exactMatch rdf:resource="http://seadatanet.maris2.nl/v_edmo/print.asp?n_code=3957"/>
	<skos:narrower rdf:resource="http://vocab.aodn.org.au/def/organisation/entity/68"/>
	<skos:topConceptOf rdf:resource="http://vocab.aodn.org.au/def/organisation/1"/>
	<skos:inScheme rdf:resource="http://vocab.aodn.org.au/def/organisation/1"/>
	<skos:scopeNote xml:lang="en">Replaces http://vocab.aodn.org.au/def/organisation/entity/65</skos:scopeNote>
	<dcterms:replaces rdf:resource="http://vocab.aodn.org.au/def/organisation/entity/65"/>
	<dcterms:replaces xml:lang="en">Department of Environment and Conservation (DEC) , Western Australian Government</dcterms:replaces>
</rdf:Description>

<rdf:Description rdf:about="http://vocab.aodn.org.au/def/organisation/entity/69">
	<rdf:type rdf:resource="http://www.w3.org/2000/01/rdf-schema#Resource"/>
	<rdf:type rdf:resource="http://www.w3.org/2004/02/skos/core#Concept"/>
	<dcterms:modified rdf:datatype="http://www.w3.org/2001/XMLSchema#dateTime">2015-05-12T01:17:01Z</dcterms:modified>
	<dcterms:creator rdf:datatype="http://www.w3.org/2001/XMLSchema#string">Natalia Atkins</dcterms:creator>
	<dcterms:created rdf:datatype="http://www.w3.org/2001/XMLSchema#dateTime">2015-04-27T10:38:15Z</dcterms:created>
	<skos:broadMatch rdf:resource="http://vocab.aodn.org.au/def/organisation_classes/category/2"/>
	<skos:prefLabel xml:lang="en">Department of Planning and Infrastructure, Western Australian Government</skos:prefLabel>
	<skos:altLabel xml:lang="en">Department of Planning and Infrastructure</skos:altLabel>
	<skos:definition xml:lang="en">The Department for Planning and Infrastructure was a department of the Government of Western Australia that was responsible for implementing the state's planning, infrastructure and transport policies. It was formed on 1 July 2001 by the amalgamation of the Ministry for Planning and the Department of Transport. On 1 July 2009, the department was reformed into the Department of Transport and Department of Planning, with State Land Services and Pastoral Leases being transferred to the newly formed Department of Regional Development and Lands. (Courtesy of Wikipedia)</skos:definition>
	<dc:source rdf:datatype="http://www.w3.org/2001/XMLSchema#string">Australian Ocean Data Network Organisation Register</dc:source>
	<dc:publisher rdf:datatype="http://www.w3.org/2001/XMLSchema#string">eMarine Information Infrastructure (eMII)</dc:publisher>
	<skos:exactMatch rdf:resource="http://seadatanet.maris2.nl/v_edmo/print.asp?n_code=3960"/>
	<skos:topConceptOf rdf:resource="http://vocab.aodn.org.au/def/organisation/1"/>
	<skos:inScheme rdf:resource="http://vocab.aodn.org.au/def/organisation/1"/>
	<skos:scopeNote xml:lang="en">Organisation no longer exists</skos:scopeNote>
	<skos:scopeNote xml:lang="en">Organisation no longer exists. Replaced by http://vocab.aodn.org.au/def/organisation/entity/70 and http://vocab.aodn.org.au/def/organisation/entity/71</skos:scopeNote>
	<dcterms:isReplacedBy rdf:resource="http://vocab.aodn.org.au/def/organisation/entity/70"/>
	<dcterms:isReplacedBy rdf:resource="http://vocab.aodn.org.au/def/organisation/entity/71"/>
	<dcterms:isReplacedBy xml:lang="en">Department of Planning (DoP), Western Australian Government</dcterms:isReplacedBy>
	<dcterms:isReplacedBy xml:lang="en">Department of Transport (DoT), Western Australian Government</dcterms:isReplacedBy>
</rdf:Description>

<rdf:Description rdf:about="http://vocab.aodn.org.au/def/organisation/entity/70">
	<rdf:type rdf:resource="http://www.w3.org/2000/01/rdf-schema#Resource"/>
	<rdf:type rdf:resource="http://www.w3.org/2004/02/skos/core#Concept"/>
	<dcterms:modified rdf:datatype="http://www.w3.org/2001/XMLSchema#dateTime">2015-05-12T01:16:46Z</dcterms:modified>
	<dcterms:creator rdf:datatype="http://www.w3.org/2001/XMLSchema#string">Natalia Atkins</dcterms:creator>
	<dcterms:created rdf:datatype="http://www.w3.org/2001/XMLSchema#dateTime">2015-04-27T10:38:15Z</dcterms:created>
	<skos:broadMatch rdf:resource="http://vocab.aodn.org.au/def/organisation_classes/category/2"/>
	<skos:prefLabel xml:lang="en">Department of Planning (DoP), Western Australian Government</skos:prefLabel>
	<skos:altLabel xml:lang="en">Department of Planning (DoP)</skos:altLabel>
	<skos:hiddenLabel xml:lang="en">DoP</skos:hiddenLabel>
	<skos:definition xml:lang="en">The Department of Planning has statewide responsibility for the planning for future communities. The department plays a vital role in improving the quality of life of all Western Australians.</skos:definition>
	<dc:source rdf:datatype="http://www.w3.org/2001/XMLSchema#string">Australian Ocean Data Network Organisation Register</dc:source>
	<dc:publisher rdf:datatype="http://www.w3.org/2001/XMLSchema#string">eMarine Information Infrastructure (eMII)</dc:publisher>
	<skos:exactMatch rdf:resource="http://seadatanet.maris2.nl/v_edmo/print.asp?n_code=3961"/>
	<skos:topConceptOf rdf:resource="http://vocab.aodn.org.au/def/organisation/1"/>
	<skos:inScheme rdf:resource="http://vocab.aodn.org.au/def/organisation/1"/>
	<skos:scopeNote xml:lang="en">Replaces http://vocab.aodn.org.au/def/organisation/entity/69</skos:scopeNote>
	<dcterms:replaces rdf:resource="http://vocab.aodn.org.au/def/organisation/entity/69"/>
	<dcterms:replaces xml:lang="en">Department of Planning and Infrastructure, Western Australian Government</dcterms:replaces>
</rdf:Description>

<rdf:Description rdf:about="http://vocab.aodn.org.au/def/organisation/entity/71">
	<rdf:type rdf:resource="http://www.w3.org/2000/01/rdf-schema#Resource"/>
	<rdf:type rdf:resource="http://www.w3.org/2004/02/skos/core#Concept"/>
	<dcterms:modified rdf:datatype="http://www.w3.org/2001/XMLSchema#dateTime">2015-05-12T01:18:02Z</dcterms:modified>
	<dcterms:creator rdf:datatype="http://www.w3.org/2001/XMLSchema#string">Natalia Atkins</dcterms:creator>
	<dcterms:created rdf:datatype="http://www.w3.org/2001/XMLSchema#dateTime">2015-04-27T10:38:15Z</dcterms:created>
	<skos:broadMatch rdf:resource="http://vocab.aodn.org.au/def/organisation_classes/category/2"/>
	<skos:prefLabel xml:lang="en">Department of Transport (DoT), Western Australian Government</skos:prefLabel>
	<skos:altLabel xml:lang="en">Department of Transport (DoT)</skos:altLabel>
	<skos:hiddenLabel xml:lang="en">DoT</skos:hiddenLabel>
	<skos:definition xml:lang="en">The Department of Transport began operations on 1 July 2009, after the former Department for Planning and Infrastructure was split into 3 new agencies. The transport function is integral to business and commerce and important for social interaction and connecting communities. It's key focus is on operational transport functions and strategic transport planning and policy across the range of public and commercial transport systems that service Western Australia.</skos:definition>
	<dc:source rdf:datatype="http://www.w3.org/2001/XMLSchema#string">Australian Ocean Data Network Organisation Register</dc:source>
	<dc:publisher rdf:datatype="http://www.w3.org/2001/XMLSchema#string">eMarine Information Infrastructure (eMII)</dc:publisher>
	<skos:exactMatch rdf:resource="http://seadatanet.maris2.nl/v_edmo/print.asp?n_code=3935"/>
	<skos:topConceptOf rdf:resource="http://vocab.aodn.org.au/def/organisation/1"/>
	<skos:inScheme rdf:resource="http://vocab.aodn.org.au/def/organisation/1"/>
	<skos:scopeNote xml:lang="en">Organisation no longer exists</skos:scopeNote>
	<skos:scopeNote xml:lang="en">Organisation no longer exists. Replaces http://vocab.aodn.org.au/def/organisation/entity/69</skos:scopeNote>
	<dcterms:replaces rdf:resource="http://vocab.aodn.org.au/def/organisation/entity/69"/>
	<dcterms:replaces xml:lang="en">Department of Planning and Infrastructure, Western Australian Government</dcterms:replaces>
</rdf:Description>

<rdf:Description rdf:about="http://vocab.aodn.org.au/def/organisation/entity/72">
	<rdf:type rdf:resource="http://www.w3.org/2000/01/rdf-schema#Resource"/>
	<rdf:type rdf:resource="http://www.w3.org/2004/02/skos/core#Concept"/>
	<dcterms:modified rdf:datatype="http://www.w3.org/2001/XMLSchema#dateTime">2015-05-12T01:44:01Z</dcterms:modified>
	<dcterms:creator rdf:datatype="http://www.w3.org/2001/XMLSchema#string">Natalia Atkins</dcterms:creator>
	<dcterms:created rdf:datatype="http://www.w3.org/2001/XMLSchema#dateTime">2015-04-27T10:38:15Z</dcterms:created>
	<skos:broadMatch rdf:resource="http://vocab.aodn.org.au/def/organisation_classes/category/2"/>
	<skos:prefLabel xml:lang="en">W.A. Water Corporation</skos:prefLabel>
	<skos:definition xml:lang="en">The Water Corporation is a business enterprise, owned by the WA Government and accountable to its sole shareholder, the Minister for Water. They are the principal supplier of water, wastewater and drainage services in WA.</skos:definition>
	<dc:source rdf:datatype="http://www.w3.org/2001/XMLSchema#string">Australian Ocean Data Network Organisation Register</dc:source>
	<dc:publisher rdf:datatype="http://www.w3.org/2001/XMLSchema#string">eMarine Information Infrastructure (eMII)</dc:publisher>
	<skos:exactMatch rdf:resource="http://seadatanet.maris2.nl/v_edmo/print.asp?n_code=4089"/>
	<skos:topConceptOf rdf:resource="http://vocab.aodn.org.au/def/organisation/1"/>
	<skos:inScheme rdf:resource="http://vocab.aodn.org.au/def/organisation/1"/>
</rdf:Description>

<rdf:Description rdf:about="http://vocab.aodn.org.au/def/organisation/entity/73">
	<rdf:type rdf:resource="http://www.w3.org/2000/01/rdf-schema#Resource"/>
	<rdf:type rdf:resource="http://www.w3.org/2004/02/skos/core#Concept"/>
	<dcterms:modified rdf:datatype="http://www.w3.org/2001/XMLSchema#dateTime">2015-05-12T01:14:47Z</dcterms:modified>
	<dcterms:creator rdf:datatype="http://www.w3.org/2001/XMLSchema#string">Natalia Atkins</dcterms:creator>
	<dcterms:created rdf:datatype="http://www.w3.org/2001/XMLSchema#dateTime">2015-04-27T10:38:15Z</dcterms:created>
	<skos:broadMatch rdf:resource="http://vocab.aodn.org.au/def/organisation_classes/category/2"/>
	<skos:prefLabel xml:lang="en">Department of Conservation and Environment, West Australian Government</skos:prefLabel>
	<skos:altLabel xml:lang="en">Department of Conservation and Environment</skos:altLabel>
	<skos:definition xml:lang="en">A former West Australian State Government department.</skos:definition>
	<dc:source rdf:datatype="http://www.w3.org/2001/XMLSchema#string">Australian Ocean Data Network Organisation Register</dc:source>
	<dc:publisher rdf:datatype="http://www.w3.org/2001/XMLSchema#string">eMarine Information Infrastructure (eMII)</dc:publisher>
	<skos:topConceptOf rdf:resource="http://vocab.aodn.org.au/def/organisation/1"/>
	<skos:inScheme rdf:resource="http://vocab.aodn.org.au/def/organisation/1"/>
	<skos:scopeNote xml:lang="en">Organisation no longer exists</skos:scopeNote>
</rdf:Description>

<rdf:Description rdf:about="http://vocab.aodn.org.au/def/organisation/entity/74">
	<rdf:type rdf:resource="http://www.w3.org/2000/01/rdf-schema#Resource"/>
	<rdf:type rdf:resource="http://www.w3.org/2004/02/skos/core#Concept"/>
	<dcterms:modified rdf:datatype="http://www.w3.org/2001/XMLSchema#dateTime">2015-05-12T01:15:58Z</dcterms:modified>
	<dcterms:creator rdf:datatype="http://www.w3.org/2001/XMLSchema#string">Natalia Atkins</dcterms:creator>
	<dcterms:created rdf:datatype="http://www.w3.org/2001/XMLSchema#dateTime">2015-04-27T10:38:15Z</dcterms:created>
	<skos:broadMatch rdf:resource="http://vocab.aodn.org.au/def/organisation_classes/category/2"/>
	<skos:prefLabel xml:lang="en">Department of Industry and Resources (DOIR), Western Australian Government</skos:prefLabel>
	<skos:altLabel xml:lang="en">Department of Industry and Resources (DOIR)</skos:altLabel>
	<skos:hiddenLabel xml:lang="en">DOIR</skos:hiddenLabel>
	<skos:definition xml:lang="en">On the 1st of January 2009, this department was combined with the Department of Consumer and Employment Protection, which were then split into three new departments, the Department of Mines and Petroleum, the Department of State Development and the Department of Commerce. (Courtesy of Wikipedia)</skos:definition>
	<dc:source rdf:datatype="http://www.w3.org/2001/XMLSchema#string">Australian Ocean Data Network Organisation Register</dc:source>
	<dc:publisher rdf:datatype="http://www.w3.org/2001/XMLSchema#string">eMarine Information Infrastructure (eMII)</dc:publisher>
	<skos:topConceptOf rdf:resource="http://vocab.aodn.org.au/def/organisation/1"/>
	<skos:inScheme rdf:resource="http://vocab.aodn.org.au/def/organisation/1"/>
	<skos:scopeNote xml:lang="en">Organisation no longer exists</skos:scopeNote>
	<skos:scopeNote xml:lang="en">Organisation no longer exists. Replaced by http://vocab.aodn.org.au/def/organisation/entity/75</skos:scopeNote>
	<dcterms:isReplacedBy rdf:resource="http://vocab.aodn.org.au/def/organisation/entity/75"/>
	<dcterms:isReplacedBy xml:lang="en">Department of Mines and Petroleum (DMP), Western Australian Government</dcterms:isReplacedBy>
</rdf:Description>

<rdf:Description rdf:about="http://vocab.aodn.org.au/def/organisation/entity/75">
	<rdf:type rdf:resource="http://www.w3.org/2000/01/rdf-schema#Resource"/>
	<rdf:type rdf:resource="http://www.w3.org/2004/02/skos/core#Concept"/>
	<dcterms:modified rdf:datatype="http://www.w3.org/2001/XMLSchema#dateTime">2015-05-12T01:16:23Z</dcterms:modified>
	<dcterms:creator rdf:datatype="http://www.w3.org/2001/XMLSchema#string">Natalia Atkins</dcterms:creator>
	<dcterms:created rdf:datatype="http://www.w3.org/2001/XMLSchema#dateTime">2015-04-27T10:38:15Z</dcterms:created>
	<skos:broadMatch rdf:resource="http://vocab.aodn.org.au/def/organisation_classes/category/2"/>
	<skos:prefLabel xml:lang="en">Department of Mines and Petroleum (DMP), Western Australian Government</skos:prefLabel>
	<skos:altLabel xml:lang="en">Department of Mines and Petroleum (DMP)</skos:altLabel>
	<skos:hiddenLabel xml:lang="en">DMP</skos:hiddenLabel>
	<skos:definition xml:lang="en">The Department of Mines and Petroleum (DMP) is the State’s lead agency in attracting private investment in resources exploration and development through the provision of geoscientific information on minerals and energy resources, and management of an equitable and secure titles systems for the mining, petroleum and geothermal industries.</skos:definition>
	<dc:source rdf:datatype="http://www.w3.org/2001/XMLSchema#string">Australian Ocean Data Network Organisation Register</dc:source>
	<dc:publisher rdf:datatype="http://www.w3.org/2001/XMLSchema#string">eMarine Information Infrastructure (eMII)</dc:publisher>
	<skos:exactMatch rdf:resource="http://seadatanet.maris2.nl/v_edmo/print.asp?n_code=4090"/>
	<skos:topConceptOf rdf:resource="http://vocab.aodn.org.au/def/organisation/1"/>
	<skos:inScheme rdf:resource="http://vocab.aodn.org.au/def/organisation/1"/>
	<skos:scopeNote xml:lang="en">Replaces http://vocab.aodn.org.au/def/organisation/entity/74</skos:scopeNote>
	<dcterms:replaces rdf:resource="http://vocab.aodn.org.au/def/organisation/entity/74"/>
	<dcterms:replaces xml:lang="en">Department of Industry and Resources (DOIR), Western Australian Government</dcterms:replaces>
</rdf:Description>

<rdf:Description rdf:about="http://vocab.aodn.org.au/def/organisation/entity/76">
	<rdf:type rdf:resource="http://www.w3.org/2000/01/rdf-schema#Resource"/>
	<rdf:type rdf:resource="http://www.w3.org/2004/02/skos/core#Concept"/>
	<dcterms:modified rdf:datatype="http://www.w3.org/2001/XMLSchema#dateTime">2015-05-12T01:21:14Z</dcterms:modified>
	<dcterms:creator rdf:datatype="http://www.w3.org/2001/XMLSchema#string">Natalia Atkins</dcterms:creator>
	<dcterms:created rdf:datatype="http://www.w3.org/2001/XMLSchema#dateTime">2015-04-27T10:38:15Z</dcterms:created>
	<skos:broadMatch rdf:resource="http://vocab.aodn.org.au/def/organisation_classes/category/2"/>
	<skos:prefLabel xml:lang="en">Environmental Protection Authority (EPA), Western Australian Government</skos:prefLabel>
	<skos:altLabel xml:lang="en">Environmental Protection Authority (EPA)</skos:altLabel>
	<skos:hiddenLabel xml:lang="en">EPA</skos:hiddenLabel>
	<skos:definition xml:lang="en">The Environmental Protection Authority (EPA) was originally established in 1971. The Authority comprises five members appointed by the Governor on the recommendation of the Minister for Environment. The EPA is independent, in that it is not subject to direction by the Minister, and its advice to Government is public. EPA members are not public servants. Its operations are governed by the Environmental Protection Act 1986 which stipulates that the objective of the EPA is to: 'use its best endeavours – a) to protect the environment; and b) to prevent, control and abate pollution and environmental harm.'</skos:definition>
	<dc:source rdf:datatype="http://www.w3.org/2001/XMLSchema#string">Australian Ocean Data Network Organisation Register</dc:source>
	<dc:publisher rdf:datatype="http://www.w3.org/2001/XMLSchema#string">eMarine Information Infrastructure (eMII)</dc:publisher>
	<skos:exactMatch rdf:resource="http://seadatanet.maris2.nl/v_edmo/print.asp?n_code=4091"/>
	<skos:topConceptOf rdf:resource="http://vocab.aodn.org.au/def/organisation/1"/>
	<skos:inScheme rdf:resource="http://vocab.aodn.org.au/def/organisation/1"/>
</rdf:Description>

<rdf:Description rdf:about="http://vocab.aodn.org.au/def/organisation/entity/77">
	<rdf:type rdf:resource="http://www.w3.org/2000/01/rdf-schema#Resource"/>
	<rdf:type rdf:resource="http://www.w3.org/2004/02/skos/core#Concept"/>
	<dcterms:modified rdf:datatype="http://www.w3.org/2001/XMLSchema#dateTime">2015-05-12T01:29:31Z</dcterms:modified>
	<dcterms:creator rdf:datatype="http://www.w3.org/2001/XMLSchema#string">Natalia Atkins</dcterms:creator>
	<dcterms:created rdf:datatype="http://www.w3.org/2001/XMLSchema#dateTime">2015-04-27T10:38:15Z</dcterms:created>
	<skos:broadMatch rdf:resource="http://vocab.aodn.org.au/def/organisation_classes/category/2"/>
	<skos:prefLabel xml:lang="en">Office of Environmental Protection Authority (OEPA), Western Australian Government</skos:prefLabel>
	<skos:altLabel xml:lang="en">Office of Environmental Protection Authority (OEPA)</skos:altLabel>
	<skos:hiddenLabel xml:lang="en">OEPA</skos:hiddenLabel>
	<skos:definition xml:lang="en">The Office of the Environmental Protection Authority was established on 27 November 2009 to support the EPA in conducting environmental impact assessments and developing policies to protect the environment. The OEPA also monitors compliance with Ministerial conditions related to approvals.</skos:definition>
	<dc:source rdf:datatype="http://www.w3.org/2001/XMLSchema#string">Australian Ocean Data Network Organisation Register</dc:source>
	<dc:publisher rdf:datatype="http://www.w3.org/2001/XMLSchema#string">eMarine Information Infrastructure (eMII)</dc:publisher>
	<skos:exactMatch rdf:resource="http://seadatanet.maris2.nl/v_edmo/print.asp?n_code=4092"/>
	<skos:topConceptOf rdf:resource="http://vocab.aodn.org.au/def/organisation/1"/>
	<skos:inScheme rdf:resource="http://vocab.aodn.org.au/def/organisation/1"/>
</rdf:Description>

<rdf:Description rdf:about="http://vocab.aodn.org.au/def/organisation/entity/78">
	<rdf:type rdf:resource="http://www.w3.org/2000/01/rdf-schema#Resource"/>
	<rdf:type rdf:resource="http://www.w3.org/2004/02/skos/core#Concept"/>
	<dcterms:modified rdf:datatype="http://www.w3.org/2001/XMLSchema#dateTime">2015-05-12T01:13:58Z</dcterms:modified>
	<dcterms:creator rdf:datatype="http://www.w3.org/2001/XMLSchema#string">Natalia Atkins</dcterms:creator>
	<dcterms:created rdf:datatype="http://www.w3.org/2001/XMLSchema#dateTime">2015-04-27T10:38:15Z</dcterms:created>
	<skos:broadMatch rdf:resource="http://vocab.aodn.org.au/def/organisation_classes/category/2"/>
	<skos:prefLabel xml:lang="en">Department of Agriculture and Food (DAFWA), Western Australian Government</skos:prefLabel>
	<skos:altLabel xml:lang="en">Department of Agriculture and Food (DAFWA)</skos:altLabel>
	<skos:hiddenLabel xml:lang="en">DAFWA</skos:hiddenLabel>
	<skos:definition xml:lang="en">The Department of Agriculture and Food, Western Australia drives the economic development of the agriculture and food sector in Western Australia (WA), with a focus on export-led growth.</skos:definition>
	<dc:source rdf:datatype="http://www.w3.org/2001/XMLSchema#string">Australian Ocean Data Network Organisation Register</dc:source>
	<dc:publisher rdf:datatype="http://www.w3.org/2001/XMLSchema#string">eMarine Information Infrastructure (eMII)</dc:publisher>
	<skos:exactMatch rdf:resource="http://seadatanet.maris2.nl/v_edmo/print.asp?n_code=4093"/>
	<skos:topConceptOf rdf:resource="http://vocab.aodn.org.au/def/organisation/1"/>
	<skos:inScheme rdf:resource="http://vocab.aodn.org.au/def/organisation/1"/>
</rdf:Description>

<rdf:Description rdf:about="http://vocab.aodn.org.au/def/organisation/entity/79">
	<rdf:type rdf:resource="http://www.w3.org/2000/01/rdf-schema#Resource"/>
	<rdf:type rdf:resource="http://www.w3.org/2004/02/skos/core#Concept"/>
	<dcterms:modified rdf:datatype="http://www.w3.org/2001/XMLSchema#dateTime">2015-05-12T01:13:39Z</dcterms:modified>
	<dcterms:creator rdf:datatype="http://www.w3.org/2001/XMLSchema#string">Natalia Atkins</dcterms:creator>
	<dcterms:created rdf:datatype="http://www.w3.org/2001/XMLSchema#dateTime">2015-04-27T10:38:15Z</dcterms:created>
	<skos:broadMatch rdf:resource="http://vocab.aodn.org.au/def/organisation_classes/category/2"/>
	<skos:prefLabel xml:lang="en">Department of Aboriginal Affairs (DAA), Western Australian Government</skos:prefLabel>
	<skos:altLabel xml:lang="en">Department of Aboriginal Affairs (DAA)</skos:altLabel>
	<skos:hiddenLabel xml:lang="en">DAA</skos:hiddenLabel>
	<skos:definition xml:lang="en">The Department engages with Aboriginal Western Australians and all levels of Government to improve the delivery of services, to facilitate the development of policy and programs which deliver sustainable economic, environmental and social benefits to Aboriginal communities.</skos:definition>
	<dc:source rdf:datatype="http://www.w3.org/2001/XMLSchema#string">Australian Ocean Data Network Organisation Register</dc:source>
	<dc:publisher rdf:datatype="http://www.w3.org/2001/XMLSchema#string">eMarine Information Infrastructure (eMII)</dc:publisher>
	<skos:exactMatch rdf:resource="http://seadatanet.maris2.nl/v_edmo/print.asp?n_code=4094"/>
	<skos:topConceptOf rdf:resource="http://vocab.aodn.org.au/def/organisation/1"/>
	<skos:inScheme rdf:resource="http://vocab.aodn.org.au/def/organisation/1"/>
</rdf:Description>

<rdf:Description rdf:about="http://vocab.aodn.org.au/def/organisation/entity/80">
	<rdf:type rdf:resource="http://www.w3.org/2000/01/rdf-schema#Resource"/>
	<rdf:type rdf:resource="http://www.w3.org/2004/02/skos/core#Concept"/>
	<dcterms:modified rdf:datatype="http://www.w3.org/2001/XMLSchema#dateTime">2015-05-12T01:16:15Z</dcterms:modified>
	<dcterms:creator rdf:datatype="http://www.w3.org/2001/XMLSchema#string">Natalia Atkins</dcterms:creator>
	<dcterms:created rdf:datatype="http://www.w3.org/2001/XMLSchema#dateTime">2015-04-27T10:38:15Z</dcterms:created>
	<skos:broadMatch rdf:resource="http://vocab.aodn.org.au/def/organisation_classes/category/2"/>
	<skos:prefLabel xml:lang="en">Department of Local Government and Communities (DLGC), Western Australian Government</skos:prefLabel>
	<skos:altLabel xml:lang="en">Department of Local Government and Communities (DLGC)</skos:altLabel>
	<skos:hiddenLabel xml:lang="en">DLGC</skos:hiddenLabel>
	<skos:definition xml:lang="en">The Department of Local Government and Communities is the State Government agency responsible for strengthening and supporting the local government and community sectors in Western Australia. It was established on 1 July 2013.</skos:definition>
	<dc:source rdf:datatype="http://www.w3.org/2001/XMLSchema#string">Australian Ocean Data Network Organisation Register</dc:source>
	<dc:publisher rdf:datatype="http://www.w3.org/2001/XMLSchema#string">eMarine Information Infrastructure (eMII)</dc:publisher>
	<skos:exactMatch rdf:resource="http://seadatanet.maris2.nl/v_edmo/print.asp?n_code=4095"/>
	<skos:topConceptOf rdf:resource="http://vocab.aodn.org.au/def/organisation/1"/>
	<skos:inScheme rdf:resource="http://vocab.aodn.org.au/def/organisation/1"/>
</rdf:Description>

<rdf:Description rdf:about="http://vocab.aodn.org.au/def/organisation/entity/81">
	<rdf:type rdf:resource="http://www.w3.org/2000/01/rdf-schema#Resource"/>
	<rdf:type rdf:resource="http://www.w3.org/2004/02/skos/core#Concept"/>
	<dcterms:modified rdf:datatype="http://www.w3.org/2001/XMLSchema#dateTime">2015-05-12T01:19:53Z</dcterms:modified>
	<dcterms:creator rdf:datatype="http://www.w3.org/2001/XMLSchema#string">Natalia Atkins</dcterms:creator>
	<dcterms:created rdf:datatype="http://www.w3.org/2001/XMLSchema#dateTime">2015-04-27T10:38:15Z</dcterms:created>
	<skos:broadMatch rdf:resource="http://vocab.aodn.org.au/def/organisation_classes/category/2"/>
	<skos:prefLabel xml:lang="en">Derwent Estuary Program (DEP)</skos:prefLabel>
	<skos:hiddenLabel xml:lang="en">DEP</skos:hiddenLabel>
	<skos:definition xml:lang="en">The Derwent Estuary Program (DEP) is a regional partnership between local governments, the Tasmanian state government, commercial and industrial enterprises, and community-based groups to restore and promote our estuary. The DEP was established in 1999.</skos:definition>
	<dc:source rdf:datatype="http://www.w3.org/2001/XMLSchema#string">Australian Ocean Data Network Organisation Register</dc:source>
	<dc:publisher rdf:datatype="http://www.w3.org/2001/XMLSchema#string">eMarine Information Infrastructure (eMII)</dc:publisher>
	<skos:exactMatch rdf:resource="http://seadatanet.maris2.nl/v_edmo/print.asp?n_code=3947"/>
	<skos:topConceptOf rdf:resource="http://vocab.aodn.org.au/def/organisation/1"/>
	<skos:inScheme rdf:resource="http://vocab.aodn.org.au/def/organisation/1"/>
</rdf:Description>

<rdf:Description rdf:about="http://vocab.aodn.org.au/def/organisation/entity/82">
	<rdf:type rdf:resource="http://www.w3.org/2000/01/rdf-schema#Resource"/>
	<rdf:type rdf:resource="http://www.w3.org/2004/02/skos/core#Concept"/>
	<dcterms:modified rdf:datatype="http://www.w3.org/2001/XMLSchema#dateTime">2015-05-12T01:20:58Z</dcterms:modified>
	<dcterms:creator rdf:datatype="http://www.w3.org/2001/XMLSchema#string">Natalia Atkins</dcterms:creator>
	<dcterms:created rdf:datatype="http://www.w3.org/2001/XMLSchema#dateTime">2015-04-27T10:38:15Z</dcterms:created>
	<skos:broadMatch rdf:resource="http://vocab.aodn.org.au/def/organisation_classes/category/5"/>
	<skos:prefLabel xml:lang="en">Earth Ocean and Space</skos:prefLabel>
	<skos:definition xml:lang="en">Earth Ocean and Space is a climate change and environmental engineering consultancy.</skos:definition>
	<dc:source rdf:datatype="http://www.w3.org/2001/XMLSchema#string">Australian Ocean Data Network Organisation Register</dc:source>
	<dc:publisher rdf:datatype="http://www.w3.org/2001/XMLSchema#string">eMarine Information Infrastructure (eMII)</dc:publisher>
	<skos:exactMatch rdf:resource="http://seadatanet.maris2.nl/v_edmo/print.asp?n_code=4096"/>
	<skos:topConceptOf rdf:resource="http://vocab.aodn.org.au/def/organisation/1"/>
	<skos:inScheme rdf:resource="http://vocab.aodn.org.au/def/organisation/1"/>
</rdf:Description>

<rdf:Description rdf:about="http://vocab.aodn.org.au/def/organisation/entity/83">
	<rdf:type rdf:resource="http://www.w3.org/2000/01/rdf-schema#Resource"/>
	<rdf:type rdf:resource="http://www.w3.org/2004/02/skos/core#Concept"/>
	<dcterms:modified rdf:datatype="http://www.w3.org/2001/XMLSchema#dateTime">2015-05-12T01:22:31Z</dcterms:modified>
	<dcterms:creator rdf:datatype="http://www.w3.org/2001/XMLSchema#string">Natalia Atkins</dcterms:creator>
	<dcterms:created rdf:datatype="http://www.w3.org/2001/XMLSchema#dateTime">2015-04-27T10:38:15Z</dcterms:created>
	<skos:broadMatch rdf:resource="http://vocab.aodn.org.au/def/organisation_classes/category/6"/>
	<skos:prefLabel xml:lang="en">Environs Kimberley (EK)</skos:prefLabel>
	<skos:hiddenLabel xml:lang="en">EK</skos:hiddenLabel>
	<skos:definition xml:lang="en"> Environs Kimberley or EK is the peak conservation organisation for the Kimberley region.</skos:definition>
	<dc:source rdf:datatype="http://www.w3.org/2001/XMLSchema#string">Australian Ocean Data Network Organisation Register</dc:source>
	<dc:publisher rdf:datatype="http://www.w3.org/2001/XMLSchema#string">eMarine Information Infrastructure (eMII)</dc:publisher>
	<skos:exactMatch rdf:resource="http://seadatanet.maris2.nl/v_edmo/print.asp?n_code=4097"/>
	<skos:topConceptOf rdf:resource="http://vocab.aodn.org.au/def/organisation/1"/>
	<skos:inScheme rdf:resource="http://vocab.aodn.org.au/def/organisation/1"/>
</rdf:Description>

<rdf:Description rdf:about="http://vocab.aodn.org.au/def/organisation/entity/84">
	<rdf:type rdf:resource="http://www.w3.org/2000/01/rdf-schema#Resource"/>
	<rdf:type rdf:resource="http://www.w3.org/2004/02/skos/core#Concept"/>
	<dcterms:modified rdf:datatype="http://www.w3.org/2001/XMLSchema#dateTime">2015-05-12T01:20:52Z</dcterms:modified>
	<dcterms:creator rdf:datatype="http://www.w3.org/2001/XMLSchema#string">Natalia Atkins</dcterms:creator>
	<dcterms:created rdf:datatype="http://www.w3.org/2001/XMLSchema#dateTime">2015-04-27T10:38:15Z</dcterms:created>
	<skos:broadMatch rdf:resource="http://vocab.aodn.org.au/def/organisation_classes/category/6"/>
	<skos:prefLabel xml:lang="en">ECOCEAN</skos:prefLabel>
	<skos:definition xml:lang="en">ECOCEAN (Australia) is a non-government, not-for-profit organization based in Western Australia working towards scientific research,  education  and conservation  of the marine environment. ECOCEAN (Australia) was founded by marine and conservation biologist Brad Norman who also helped establish the partner organisation ECOCEAN (USA). ECOCEAN’s flagship species is the iconic yet threatened whale shark (Rhincodon typus).</skos:definition>
	<dc:source rdf:datatype="http://www.w3.org/2001/XMLSchema#string">Australian Ocean Data Network Organisation Register</dc:source>
	<dc:publisher rdf:datatype="http://www.w3.org/2001/XMLSchema#string">eMarine Information Infrastructure (eMII)</dc:publisher>
	<skos:exactMatch rdf:resource="http://seadatanet.maris2.nl/v_edmo/print.asp?n_code=4098"/>
	<skos:topConceptOf rdf:resource="http://vocab.aodn.org.au/def/organisation/1"/>
	<skos:inScheme rdf:resource="http://vocab.aodn.org.au/def/organisation/1"/>
</rdf:Description>

<rdf:Description rdf:about="http://vocab.aodn.org.au/def/organisation/entity/85">
	<rdf:type rdf:resource="http://www.w3.org/2000/01/rdf-schema#Resource"/>
	<rdf:type rdf:resource="http://www.w3.org/2004/02/skos/core#Concept"/>
	<dcterms:modified rdf:datatype="http://www.w3.org/2001/XMLSchema#dateTime">2015-05-12T01:22:44Z</dcterms:modified>
	<dcterms:creator rdf:datatype="http://www.w3.org/2001/XMLSchema#string">Natalia Atkins</dcterms:creator>
	<dcterms:created rdf:datatype="http://www.w3.org/2001/XMLSchema#dateTime">2015-04-27T10:38:15Z</dcterms:created>
	<skos:broadMatch rdf:resource="http://vocab.aodn.org.au/def/organisation_classes/category/5"/>
	<skos:prefLabel xml:lang="en">Gaia Resources</skos:prefLabel>
	<skos:definition xml:lang="en">Gaia Resources is an environmental technology consultancy company, that have been operating since 2004.</skos:definition>
	<dc:source rdf:datatype="http://www.w3.org/2001/XMLSchema#string">Australian Ocean Data Network Organisation Register</dc:source>
	<dc:publisher rdf:datatype="http://www.w3.org/2001/XMLSchema#string">eMarine Information Infrastructure (eMII)</dc:publisher>
	<skos:exactMatch rdf:resource="http://seadatanet.maris2.nl/v_edmo/print.asp?n_code=4099"/>
	<skos:topConceptOf rdf:resource="http://vocab.aodn.org.au/def/organisation/1"/>
	<skos:inScheme rdf:resource="http://vocab.aodn.org.au/def/organisation/1"/>
</rdf:Description>

<rdf:Description rdf:about="http://vocab.aodn.org.au/def/organisation/entity/86">
	<rdf:type rdf:resource="http://www.w3.org/2000/01/rdf-schema#Resource"/>
	<rdf:type rdf:resource="http://www.w3.org/2004/02/skos/core#Concept"/>
	<dcterms:modified rdf:datatype="http://www.w3.org/2001/XMLSchema#dateTime">2015-05-12T01:22:49Z</dcterms:modified>
	<dcterms:creator rdf:datatype="http://www.w3.org/2001/XMLSchema#string">Natalia Atkins</dcterms:creator>
	<dcterms:created rdf:datatype="http://www.w3.org/2001/XMLSchema#dateTime">2015-04-27T10:38:15Z</dcterms:created>
	<skos:broadMatch rdf:resource="http://vocab.aodn.org.au/def/organisation_classes/category/2"/>
	<skos:prefLabel xml:lang="en">Gippsland Water</skos:prefLabel>
	<skos:definition xml:lang="en">Gippsland Water look after water and wastewater (sewage) services in Central Gippsland, Victoria,</skos:definition>
	<dc:source rdf:datatype="http://www.w3.org/2001/XMLSchema#string">Australian Ocean Data Network Organisation Register</dc:source>
	<dc:publisher rdf:datatype="http://www.w3.org/2001/XMLSchema#string">eMarine Information Infrastructure (eMII)</dc:publisher>
	<skos:exactMatch rdf:resource="http://seadatanet.maris2.nl/v_edmo/print.asp?n_code=4100"/>
	<skos:topConceptOf rdf:resource="http://vocab.aodn.org.au/def/organisation/1"/>
	<skos:inScheme rdf:resource="http://vocab.aodn.org.au/def/organisation/1"/>
</rdf:Description>

<rdf:Description rdf:about="http://vocab.aodn.org.au/def/organisation/entity/87">
	<rdf:type rdf:resource="http://www.w3.org/2000/01/rdf-schema#Resource"/>
	<rdf:type rdf:resource="http://www.w3.org/2004/02/skos/core#Concept"/>
	<dcterms:modified rdf:datatype="http://www.w3.org/2001/XMLSchema#dateTime">2015-05-12T01:23:46Z</dcterms:modified>
	<dcterms:creator rdf:datatype="http://www.w3.org/2001/XMLSchema#string">Natalia Atkins</dcterms:creator>
	<dcterms:created rdf:datatype="http://www.w3.org/2001/XMLSchema#dateTime">2015-04-27T10:38:15Z</dcterms:created>
	<skos:broadMatch rdf:resource="http://vocab.aodn.org.au/def/organisation_classes/category/5"/>
	<skos:prefLabel xml:lang="en">Halfmoon Biosciences</skos:prefLabel>
	<skos:definition xml:lang="en">Halfmoon Biosciences is an environmental consultancy specialising in seabird ecology, scientific research, designing field monitoring programs, environmental planning and mitigation, offshore environmental project supervision (audits and compliance) and Marine Mammal Observations for the Offshore Oil and Gas, Fishing and Tourism Industries.</skos:definition>
	<dc:source rdf:datatype="http://www.w3.org/2001/XMLSchema#string">Australian Ocean Data Network Organisation Register</dc:source>
	<dc:publisher rdf:datatype="http://www.w3.org/2001/XMLSchema#string">eMarine Information Infrastructure (eMII)</dc:publisher>
	<skos:exactMatch rdf:resource="http://seadatanet.maris2.nl/v_edmo/print.asp?n_code=3955"/>
	<skos:topConceptOf rdf:resource="http://vocab.aodn.org.au/def/organisation/1"/>
	<skos:inScheme rdf:resource="http://vocab.aodn.org.au/def/organisation/1"/>
</rdf:Description>

<rdf:Description rdf:about="http://vocab.aodn.org.au/def/organisation/entity/88">
	<rdf:type rdf:resource="http://www.w3.org/2000/01/rdf-schema#Resource"/>
	<rdf:type rdf:resource="http://www.w3.org/2004/02/skos/core#Concept"/>
	<dcterms:modified rdf:datatype="http://www.w3.org/2001/XMLSchema#dateTime">2015-05-12T01:23:53Z</dcterms:modified>
	<dcterms:creator rdf:datatype="http://www.w3.org/2001/XMLSchema#string">Natalia Atkins</dcterms:creator>
	<dcterms:created rdf:datatype="http://www.w3.org/2001/XMLSchema#dateTime">2015-04-27T10:38:15Z</dcterms:created>
	<skos:broadMatch rdf:resource="http://vocab.aodn.org.au/def/organisation_classes/category/5"/>
	<skos:prefLabel xml:lang="en">Horizon Oil Ltd</skos:prefLabel>
	<skos:definition xml:lang="en">Horizon Oil Limited (‘Horizon Oil’) is an oil and gas exploration, development and production company, incorporated and domiciled in Australia. </skos:definition>
	<dc:source rdf:datatype="http://www.w3.org/2001/XMLSchema#string">Australian Ocean Data Network Organisation Register</dc:source>
	<dc:publisher rdf:datatype="http://www.w3.org/2001/XMLSchema#string">eMarine Information Infrastructure (eMII)</dc:publisher>
	<skos:exactMatch rdf:resource="http://seadatanet.maris2.nl/v_edmo/print.asp?n_code=3972"/>
	<skos:topConceptOf rdf:resource="http://vocab.aodn.org.au/def/organisation/1"/>
	<skos:inScheme rdf:resource="http://vocab.aodn.org.au/def/organisation/1"/>
</rdf:Description>

<rdf:Description rdf:about="http://vocab.aodn.org.au/def/organisation/entity/89">
	<rdf:type rdf:resource="http://www.w3.org/2000/01/rdf-schema#Resource"/>
	<rdf:type rdf:resource="http://www.w3.org/2004/02/skos/core#Concept"/>
	<dcterms:modified rdf:datatype="http://www.w3.org/2001/XMLSchema#dateTime">2015-05-12T01:23:59Z</dcterms:modified>
	<dcterms:creator rdf:datatype="http://www.w3.org/2001/XMLSchema#string">Natalia Atkins</dcterms:creator>
	<dcterms:created rdf:datatype="http://www.w3.org/2001/XMLSchema#dateTime">2015-04-27T10:38:15Z</dcterms:created>
	<skos:broadMatch rdf:resource="http://vocab.aodn.org.au/def/organisation_classes/category/5"/>
	<skos:prefLabel xml:lang="en">HydroNumerics Pty Ltd</skos:prefLabel>
	<skos:definition xml:lang="en">HydroNumerics Pty Ltd was founded in 2010 to deliver innovative engineering services to deliver products and services to water utilities, government, consultants and industry.</skos:definition>
	<dc:source rdf:datatype="http://www.w3.org/2001/XMLSchema#string">Australian Ocean Data Network Organisation Register</dc:source>
	<dc:publisher rdf:datatype="http://www.w3.org/2001/XMLSchema#string">eMarine Information Infrastructure (eMII)</dc:publisher>
	<skos:exactMatch rdf:resource="http://seadatanet.maris2.nl/v_edmo/print.asp?n_code=4101"/>
	<skos:topConceptOf rdf:resource="http://vocab.aodn.org.au/def/organisation/1"/>
	<skos:inScheme rdf:resource="http://vocab.aodn.org.au/def/organisation/1"/>
</rdf:Description>

<rdf:Description rdf:about="http://vocab.aodn.org.au/def/organisation/entity/90">
	<rdf:type rdf:resource="http://www.w3.org/2000/01/rdf-schema#Resource"/>
	<rdf:type rdf:resource="http://www.w3.org/2004/02/skos/core#Concept"/>
	<dcterms:modified rdf:datatype="http://www.w3.org/2001/XMLSchema#dateTime">2015-05-12T01:25:29Z</dcterms:modified>
	<dcterms:creator rdf:datatype="http://www.w3.org/2001/XMLSchema#string">Natalia Atkins</dcterms:creator>
	<dcterms:created rdf:datatype="http://www.w3.org/2001/XMLSchema#dateTime">2015-04-27T10:38:15Z</dcterms:created>
	<skos:broadMatch rdf:resource="http://vocab.aodn.org.au/def/organisation_classes/category/5"/>
	<skos:prefLabel xml:lang="en">INPEX</skos:prefLabel>
	<dc:source rdf:datatype="http://www.w3.org/2001/XMLSchema#string">Australian Ocean Data Network Organisation Register</dc:source>
	<dc:publisher rdf:datatype="http://www.w3.org/2001/XMLSchema#string">eMarine Information Infrastructure (eMII)</dc:publisher>
	<skos:exactMatch rdf:resource="http://seadatanet.maris2.nl/v_edmo/print.asp?n_code=4102"/>
	<skos:narrower rdf:resource="http://vocab.aodn.org.au/def/organisation/entity/91"/>
	<skos:topConceptOf rdf:resource="http://vocab.aodn.org.au/def/organisation/1"/>
	<skos:inScheme rdf:resource="http://vocab.aodn.org.au/def/organisation/1"/>
</rdf:Description>

<rdf:Description rdf:about="http://vocab.aodn.org.au/def/organisation/entity/92">
	<rdf:type rdf:resource="http://www.w3.org/2000/01/rdf-schema#Resource"/>
	<rdf:type rdf:resource="http://www.w3.org/2004/02/skos/core#Concept"/>
	<dcterms:modified rdf:datatype="http://www.w3.org/2001/XMLSchema#dateTime">2015-05-12T01:26:41Z</dcterms:modified>
	<dcterms:creator rdf:datatype="http://www.w3.org/2001/XMLSchema#string">Natalia Atkins</dcterms:creator>
	<dcterms:created rdf:datatype="http://www.w3.org/2001/XMLSchema#dateTime">2015-04-27T10:38:15Z</dcterms:created>
	<skos:broadMatch rdf:resource="http://vocab.aodn.org.au/def/organisation_classes/category/5"/>
	<skos:prefLabel xml:lang="en">Kimberley Quest</skos:prefLabel>
	<skos:definition xml:lang="en">The company was first launched in Broome in 1994, under the name Pearl Sea Coastal Cruises. Originally Pearl Sea Coastal Cruises operated the pilot boat for Broome Port, commercial and research vessels as well as full day fishing charters out of Broome with three vessels: Kimberley Quest, Vantage and Sentosa. In 2013 Pearl Sea Coastal Cruises' trading name was changed to Kimberley Quest and a new brand was launched. Kimberley Quest II is the only vessel operated by Kimberley Quest.</skos:definition>
	<dc:source rdf:datatype="http://www.w3.org/2001/XMLSchema#string">Australian Ocean Data Network Organisation Register</dc:source>
	<dc:publisher rdf:datatype="http://www.w3.org/2001/XMLSchema#string">eMarine Information Infrastructure (eMII)</dc:publisher>
	<skos:exactMatch rdf:resource="http://seadatanet.maris2.nl/v_edmo/print.asp?n_code=4103"/>
	<skos:topConceptOf rdf:resource="http://vocab.aodn.org.au/def/organisation/1"/>
	<skos:inScheme rdf:resource="http://vocab.aodn.org.au/def/organisation/1"/>
</rdf:Description>

<rdf:Description rdf:about="http://vocab.aodn.org.au/def/organisation/entity/93">
	<rdf:type rdf:resource="http://www.w3.org/2000/01/rdf-schema#Resource"/>
	<rdf:type rdf:resource="http://www.w3.org/2004/02/skos/core#Concept"/>
	<dcterms:modified rdf:datatype="http://www.w3.org/2001/XMLSchema#dateTime">2015-05-12T01:26:53Z</dcterms:modified>
	<dcterms:creator rdf:datatype="http://www.w3.org/2001/XMLSchema#string">Natalia Atkins</dcterms:creator>
	<dcterms:created rdf:datatype="http://www.w3.org/2001/XMLSchema#dateTime">2015-04-27T10:38:15Z</dcterms:created>
	<skos:broadMatch rdf:resource="http://vocab.aodn.org.au/def/organisation_classes/category/5"/>
	<skos:prefLabel xml:lang="en">Lawson and Treloar Pty Ltd</skos:prefLabel>
	<skos:definition xml:lang="en">This environment/engineering consultant company became Cardno Lawson Treloar in 2004, and is now part of the larger Cardno group.</skos:definition>
	<dc:source rdf:datatype="http://www.w3.org/2001/XMLSchema#string">Australian Ocean Data Network Organisation Register</dc:source>
	<dc:publisher rdf:datatype="http://www.w3.org/2001/XMLSchema#string">eMarine Information Infrastructure (eMII)</dc:publisher>
	<skos:topConceptOf rdf:resource="http://vocab.aodn.org.au/def/organisation/1"/>
	<skos:inScheme rdf:resource="http://vocab.aodn.org.au/def/organisation/1"/>
	<skos:scopeNote xml:lang="en">Organisation no longer exists</skos:scopeNote>
</rdf:Description>

<rdf:Description rdf:about="http://vocab.aodn.org.au/def/organisation/entity/94">
	<rdf:type rdf:resource="http://www.w3.org/2000/01/rdf-schema#Resource"/>
	<rdf:type rdf:resource="http://www.w3.org/2004/02/skos/core#Concept"/>
	<dcterms:modified rdf:datatype="http://www.w3.org/2001/XMLSchema#dateTime">2015-05-12T01:26:59Z</dcterms:modified>
	<dcterms:creator rdf:datatype="http://www.w3.org/2001/XMLSchema#string">Natalia Atkins</dcterms:creator>
	<dcterms:created rdf:datatype="http://www.w3.org/2001/XMLSchema#dateTime">2015-04-27T10:38:15Z</dcterms:created>
	<skos:broadMatch rdf:resource="http://vocab.aodn.org.au/def/organisation_classes/category/5"/>
	<skos:prefLabel xml:lang="en">LeProvost Dames and Moore (LDM)</skos:prefLabel>
	<skos:hiddenLabel xml:lang="en">LDM</skos:hiddenLabel>
	<skos:definition xml:lang="en">An environmental consultancy company.</skos:definition>
	<dc:source rdf:datatype="http://www.w3.org/2001/XMLSchema#string">Australian Ocean Data Network Organisation Register</dc:source>
	<dc:publisher rdf:datatype="http://www.w3.org/2001/XMLSchema#string">eMarine Information Infrastructure (eMII)</dc:publisher>
	<skos:exactMatch rdf:resource="http://seadatanet.maris2.nl/v_edmo/print.asp?n_code=4104"/>
	<skos:topConceptOf rdf:resource="http://vocab.aodn.org.au/def/organisation/1"/>
	<skos:inScheme rdf:resource="http://vocab.aodn.org.au/def/organisation/1"/>
</rdf:Description>

<rdf:Description rdf:about="http://vocab.aodn.org.au/def/organisation/entity/95">
	<rdf:type rdf:resource="http://www.w3.org/2000/01/rdf-schema#Resource"/>
	<rdf:type rdf:resource="http://www.w3.org/2004/02/skos/core#Concept"/>
	<dcterms:modified rdf:datatype="http://www.w3.org/2001/XMLSchema#dateTime">2015-05-12T01:25:53Z</dcterms:modified>
	<dcterms:creator rdf:datatype="http://www.w3.org/2001/XMLSchema#string">Natalia Atkins</dcterms:creator>
	<dcterms:created rdf:datatype="http://www.w3.org/2001/XMLSchema#dateTime">2015-04-27T10:38:15Z</dcterms:created>
	<skos:broadMatch rdf:resource="http://vocab.aodn.org.au/def/organisation_classes/category/5"/>
	<skos:prefLabel xml:lang="en">Kevron Aerial Surveys Pty Ltd</skos:prefLabel>
	<skos:definition xml:lang="en">Commercial photography company.</skos:definition>
	<dc:source rdf:datatype="http://www.w3.org/2001/XMLSchema#string">Australian Ocean Data Network Organisation Register</dc:source>
	<dc:publisher rdf:datatype="http://www.w3.org/2001/XMLSchema#string">eMarine Information Infrastructure (eMII)</dc:publisher>
	<skos:topConceptOf rdf:resource="http://vocab.aodn.org.au/def/organisation/1"/>
	<skos:inScheme rdf:resource="http://vocab.aodn.org.au/def/organisation/1"/>
	<skos:scopeNote xml:lang="en">Organisation no longer exists</skos:scopeNote>
</rdf:Description>

<rdf:Description rdf:about="http://vocab.aodn.org.au/def/organisation/entity/96">
	<rdf:type rdf:resource="http://www.w3.org/2000/01/rdf-schema#Resource"/>
	<rdf:type rdf:resource="http://www.w3.org/2004/02/skos/core#Concept"/>
	<dcterms:modified rdf:datatype="http://www.w3.org/2001/XMLSchema#dateTime">2015-05-12T01:27:11Z</dcterms:modified>
	<dcterms:creator rdf:datatype="http://www.w3.org/2001/XMLSchema#string">Natalia Atkins</dcterms:creator>
	<dcterms:created rdf:datatype="http://www.w3.org/2001/XMLSchema#dateTime">2015-04-27T10:38:15Z</dcterms:created>
	<skos:broadMatch rdf:resource="http://vocab.aodn.org.au/def/organisation_classes/category/2"/>
	<skos:prefLabel xml:lang="en">Manly Hydraulics Laboratory (MHL)</skos:prefLabel>
	<skos:hiddenLabel xml:lang="en">MHL</skos:hiddenLabel>
	<skos:definition xml:lang="en">Manly Hydraulics Laboratory (MHL) provides specialist services in the areas of water, sewer, stormwater, irrigation, coastal and environmental solutions including physical and numerical modelling investigations and delivery of extensive data collection programs. MHL is a business unit within NSW Public Works, a Division of the NSW Office of Finance and Services.</skos:definition>
	<dc:source rdf:datatype="http://www.w3.org/2001/XMLSchema#string">Australian Ocean Data Network Organisation Register</dc:source>
	<dc:publisher rdf:datatype="http://www.w3.org/2001/XMLSchema#string">eMarine Information Infrastructure (eMII)</dc:publisher>
	<skos:exactMatch rdf:resource="http://seadatanet.maris2.nl/v_edmo/print.asp?n_code=3967"/>
	<skos:topConceptOf rdf:resource="http://vocab.aodn.org.au/def/organisation/1"/>
	<skos:inScheme rdf:resource="http://vocab.aodn.org.au/def/organisation/1"/>
</rdf:Description>

<rdf:Description rdf:about="http://vocab.aodn.org.au/def/organisation/entity/97">
	<rdf:type rdf:resource="http://www.w3.org/2000/01/rdf-schema#Resource"/>
	<rdf:type rdf:resource="http://www.w3.org/2004/02/skos/core#Concept"/>
	<dcterms:modified rdf:datatype="http://www.w3.org/2001/XMLSchema#dateTime">2015-05-12T01:27:04Z</dcterms:modified>
	<dcterms:creator rdf:datatype="http://www.w3.org/2001/XMLSchema#string">Natalia Atkins</dcterms:creator>
	<dcterms:created rdf:datatype="http://www.w3.org/2001/XMLSchema#dateTime">2015-04-27T10:38:15Z</dcterms:created>
	<skos:broadMatch rdf:resource="http://vocab.aodn.org.au/def/organisation_classes/category/5"/>
	<skos:prefLabel xml:lang="en">M.E. Trudgen and Associates</skos:prefLabel>
	<skos:definition xml:lang="en">Environment Consultancy company.</skos:definition>
	<dc:source rdf:datatype="http://www.w3.org/2001/XMLSchema#string">Australian Ocean Data Network Organisation Register</dc:source>
	<dc:publisher rdf:datatype="http://www.w3.org/2001/XMLSchema#string">eMarine Information Infrastructure (eMII)</dc:publisher>
	<skos:exactMatch rdf:resource="http://seadatanet.maris2.nl/v_edmo/print.asp?n_code=4105"/>
	<skos:topConceptOf rdf:resource="http://vocab.aodn.org.au/def/organisation/1"/>
	<skos:inScheme rdf:resource="http://vocab.aodn.org.au/def/organisation/1"/>
</rdf:Description>

<rdf:Description rdf:about="http://vocab.aodn.org.au/def/organisation/entity/98">
	<rdf:type rdf:resource="http://www.w3.org/2000/01/rdf-schema#Resource"/>
	<rdf:type rdf:resource="http://www.w3.org/2004/02/skos/core#Concept"/>
	<dcterms:modified rdf:datatype="http://www.w3.org/2001/XMLSchema#dateTime">2015-05-12T01:27:52Z</dcterms:modified>
	<dcterms:creator rdf:datatype="http://www.w3.org/2001/XMLSchema#string">Natalia Atkins</dcterms:creator>
	<dcterms:created rdf:datatype="http://www.w3.org/2001/XMLSchema#dateTime">2015-04-27T10:38:15Z</dcterms:created>
	<skos:broadMatch rdf:resource="http://vocab.aodn.org.au/def/organisation_classes/category/5"/>
	<skos:prefLabel xml:lang="en">Marine Environmental Systems</skos:prefLabel>
	<dc:source rdf:datatype="http://www.w3.org/2001/XMLSchema#string">Australian Ocean Data Network Organisation Register</dc:source>
	<dc:publisher rdf:datatype="http://www.w3.org/2001/XMLSchema#string">eMarine Information Infrastructure (eMII)</dc:publisher>
	<skos:topConceptOf rdf:resource="http://vocab.aodn.org.au/def/organisation/1"/>
	<skos:inScheme rdf:resource="http://vocab.aodn.org.au/def/organisation/1"/>
	<skos:scopeNote xml:lang="en">Organisation no longer exists</skos:scopeNote>
</rdf:Description>

<rdf:Description rdf:about="http://vocab.aodn.org.au/def/organisation/entity/99">
	<rdf:type rdf:resource="http://www.w3.org/2000/01/rdf-schema#Resource"/>
	<rdf:type rdf:resource="http://www.w3.org/2004/02/skos/core#Concept"/>
	<dcterms:modified rdf:datatype="http://www.w3.org/2001/XMLSchema#dateTime">2015-05-12T01:27:56Z</dcterms:modified>
	<dcterms:creator rdf:datatype="http://www.w3.org/2001/XMLSchema#string">Natalia Atkins</dcterms:creator>
	<dcterms:created rdf:datatype="http://www.w3.org/2001/XMLSchema#dateTime">2015-04-27T10:38:15Z</dcterms:created>
	<skos:broadMatch rdf:resource="http://vocab.aodn.org.au/def/organisation_classes/category/5"/>
	<skos:prefLabel xml:lang="en">Mscience Pty Ltd</skos:prefLabel>
	<skos:definition xml:lang="en">MScience Pty Ltd commenced operations in 2003 on the campus of the University of Western Australia. The company was established to provide a link between marine scientists and the resource industries requiring the commercial application of their expertise.</skos:definition>
	<dc:source rdf:datatype="http://www.w3.org/2001/XMLSchema#string">Australian Ocean Data Network Organisation Register</dc:source>
	<dc:publisher rdf:datatype="http://www.w3.org/2001/XMLSchema#string">eMarine Information Infrastructure (eMII)</dc:publisher>
	<skos:exactMatch rdf:resource="http://seadatanet.maris2.nl/v_edmo/print.asp?n_code=4106"/>
	<skos:topConceptOf rdf:resource="http://vocab.aodn.org.au/def/organisation/1"/>
	<skos:inScheme rdf:resource="http://vocab.aodn.org.au/def/organisation/1"/>
</rdf:Description>

<rdf:Description rdf:about="http://vocab.aodn.org.au/def/organisation/entity/100">
	<rdf:type rdf:resource="http://www.w3.org/2000/01/rdf-schema#Resource"/>
	<rdf:type rdf:resource="http://www.w3.org/2004/02/skos/core#Concept"/>
	<dcterms:modified rdf:datatype="http://www.w3.org/2001/XMLSchema#dateTime">2015-05-12T01:28:01Z</dcterms:modified>
	<dcterms:creator rdf:datatype="http://www.w3.org/2001/XMLSchema#string">Natalia Atkins</dcterms:creator>
	<dcterms:created rdf:datatype="http://www.w3.org/2001/XMLSchema#dateTime">2015-04-27T10:38:15Z</dcterms:created>
	<skos:broadMatch rdf:resource="http://vocab.aodn.org.au/def/organisation_classes/category/5"/>
	<skos:prefLabel xml:lang="en">Murphy Australia Oil Pty Ltd</skos:prefLabel>
	<skos:definition xml:lang="en">Murphy Oil Corporation is an independent exploration and production company with a strong portfolio of global offshore and onshore assets delivering oil-weighted growth. Murphy produces oil and /or natural gas in the United States, Canada, and Malaysia and conducts exploration activities worldwide.</skos:definition>
	<dc:source rdf:datatype="http://www.w3.org/2001/XMLSchema#string">Australian Ocean Data Network Organisation Register</dc:source>
	<dc:publisher rdf:datatype="http://www.w3.org/2001/XMLSchema#string">eMarine Information Infrastructure (eMII)</dc:publisher>
	<skos:exactMatch rdf:resource="http://seadatanet.maris2.nl/v_edmo/print.asp?n_code=4107"/>
	<skos:topConceptOf rdf:resource="http://vocab.aodn.org.au/def/organisation/1"/>
	<skos:inScheme rdf:resource="http://vocab.aodn.org.au/def/organisation/1"/>
</rdf:Description>

<rdf:Description rdf:about="http://vocab.aodn.org.au/def/organisation/entity/101">
	<rdf:type rdf:resource="http://www.w3.org/2000/01/rdf-schema#Resource"/>
	<rdf:type rdf:resource="http://www.w3.org/2004/02/skos/core#Concept"/>
	<dcterms:modified rdf:datatype="http://www.w3.org/2001/XMLSchema#dateTime">2015-05-12T01:28:11Z</dcterms:modified>
	<dcterms:creator rdf:datatype="http://www.w3.org/2001/XMLSchema#string">Natalia Atkins</dcterms:creator>
	<dcterms:created rdf:datatype="http://www.w3.org/2001/XMLSchema#dateTime">2015-04-27T10:38:15Z</dcterms:created>
	<skos:broadMatch rdf:resource="http://vocab.aodn.org.au/def/organisation_classes/category/5"/>
	<skos:prefLabel xml:lang="en">Myriax</skos:prefLabel>
	<skos:definition xml:lang="en">Myriax Software specializes in the design, development and sales of Echoview, an advanced water column data processing software solution.</skos:definition>
	<dc:source rdf:datatype="http://www.w3.org/2001/XMLSchema#string">Australian Ocean Data Network Organisation Register</dc:source>
	<dc:publisher rdf:datatype="http://www.w3.org/2001/XMLSchema#string">eMarine Information Infrastructure (eMII)</dc:publisher>
	<skos:exactMatch rdf:resource="http://seadatanet.maris2.nl/v_edmo/print.asp?n_code=3938"/>
	<skos:topConceptOf rdf:resource="http://vocab.aodn.org.au/def/organisation/1"/>
	<skos:inScheme rdf:resource="http://vocab.aodn.org.au/def/organisation/1"/>
</rdf:Description>

<rdf:Description rdf:about="http://vocab.aodn.org.au/def/organisation/entity/102">
	<rdf:type rdf:resource="http://www.w3.org/2000/01/rdf-schema#Resource"/>
	<rdf:type rdf:resource="http://www.w3.org/2004/02/skos/core#Concept"/>
	<dcterms:modified rdf:datatype="http://www.w3.org/2001/XMLSchema#dateTime">2015-05-12T01:28:06Z</dcterms:modified>
	<dcterms:creator rdf:datatype="http://www.w3.org/2001/XMLSchema#string">Natalia Atkins</dcterms:creator>
	<dcterms:created rdf:datatype="http://www.w3.org/2001/XMLSchema#dateTime">2015-04-27T10:38:15Z</dcterms:created>
	<skos:broadMatch rdf:resource="http://vocab.aodn.org.au/def/organisation_classes/category/2"/>
	<skos:prefLabel xml:lang="en">Museum Victoria</skos:prefLabel>
	<skos:definition xml:lang="en">Museum Victoria is the state museum for the state of Victoria. It is Australia's largest public museum organisation. Museum Victoria’s origins date back to 1854, with the founding of the National Museum of Victoria and the establishment, in 1870, of the Industrial and Technological Museum of Victoria (later known as the Science Museum of Victoria). By proclamation of the Museums Act 1983 (Vic.), these two institutions were amalgamated to form what is known today as Museum Victoria, governed by the Museums Board of Victoria. In 1996, Museum Victoria took over custodianship of the World Heritage listed Royal Exhibition Building.</skos:definition>
	<dc:source rdf:datatype="http://www.w3.org/2001/XMLSchema#string">Australian Ocean Data Network Organisation Register</dc:source>
	<dc:publisher rdf:datatype="http://www.w3.org/2001/XMLSchema#string">eMarine Information Infrastructure (eMII)</dc:publisher>
	<skos:exactMatch rdf:resource="http://seadatanet.maris2.nl/v_edmo/print.asp?n_code=4025"/>
	<skos:topConceptOf rdf:resource="http://vocab.aodn.org.au/def/organisation/1"/>
	<skos:inScheme rdf:resource="http://vocab.aodn.org.au/def/organisation/1"/>
</rdf:Description>

<rdf:Description rdf:about="http://vocab.aodn.org.au/def/organisation/entity/103">
	<rdf:type rdf:resource="http://www.w3.org/2000/01/rdf-schema#Resource"/>
	<rdf:type rdf:resource="http://www.w3.org/2004/02/skos/core#Concept"/>
	<dcterms:modified rdf:datatype="http://www.w3.org/2001/XMLSchema#dateTime">2015-05-12T01:28:54Z</dcterms:modified>
	<dcterms:creator rdf:datatype="http://www.w3.org/2001/XMLSchema#string">Natalia Atkins</dcterms:creator>
	<dcterms:created rdf:datatype="http://www.w3.org/2001/XMLSchema#dateTime">2015-04-27T10:38:15Z</dcterms:created>
	<skos:broadMatch rdf:resource="http://vocab.aodn.org.au/def/organisation_classes/category/5"/>
	<skos:prefLabel xml:lang="en">NGIS Australia</skos:prefLabel>
	<skos:definition xml:lang="en">NGIS Australia commenced operations in 1993 from Perth, Western Australia. It is a provider of location-based technology solutions.</skos:definition>
	<dc:source rdf:datatype="http://www.w3.org/2001/XMLSchema#string">Australian Ocean Data Network Organisation Register</dc:source>
	<dc:publisher rdf:datatype="http://www.w3.org/2001/XMLSchema#string">eMarine Information Infrastructure (eMII)</dc:publisher>
	<skos:exactMatch rdf:resource="http://seadatanet.maris2.nl/v_edmo/print.asp?n_code=4108"/>
	<skos:topConceptOf rdf:resource="http://vocab.aodn.org.au/def/organisation/1"/>
	<skos:inScheme rdf:resource="http://vocab.aodn.org.au/def/organisation/1"/>
</rdf:Description>

<rdf:Description rdf:about="http://vocab.aodn.org.au/def/organisation/entity/104">
	<rdf:type rdf:resource="http://www.w3.org/2000/01/rdf-schema#Resource"/>
	<rdf:type rdf:resource="http://www.w3.org/2004/02/skos/core#Concept"/>
	<dcterms:modified rdf:datatype="http://www.w3.org/2001/XMLSchema#dateTime">2015-05-12T01:29:11Z</dcterms:modified>
	<dcterms:creator rdf:datatype="http://www.w3.org/2001/XMLSchema#string">Natalia Atkins</dcterms:creator>
	<dcterms:created rdf:datatype="http://www.w3.org/2001/XMLSchema#dateTime">2015-04-27T10:38:15Z</dcterms:created>
	<skos:broadMatch rdf:resource="http://vocab.aodn.org.au/def/organisation_classes/category/5"/>
	<skos:prefLabel xml:lang="en">Ocean Vision Environmental Research Pty Ltd</skos:prefLabel>
	<skos:definition xml:lang="en">Ocean Vision Environmental Research is a specialised marine consultancy that provides products and services for the monitoring of marine and estuarine environments.</skos:definition>
	<dc:source rdf:datatype="http://www.w3.org/2001/XMLSchema#string">Australian Ocean Data Network Organisation Register</dc:source>
	<dc:publisher rdf:datatype="http://www.w3.org/2001/XMLSchema#string">eMarine Information Infrastructure (eMII)</dc:publisher>
	<skos:exactMatch rdf:resource="http://seadatanet.maris2.nl/v_edmo/print.asp?n_code=4109"/>
	<skos:topConceptOf rdf:resource="http://vocab.aodn.org.au/def/organisation/1"/>
	<skos:inScheme rdf:resource="http://vocab.aodn.org.au/def/organisation/1"/>
</rdf:Description>

<rdf:Description rdf:about="http://vocab.aodn.org.au/def/organisation/entity/105">
	<rdf:type rdf:resource="http://www.w3.org/2000/01/rdf-schema#Resource"/>
	<rdf:type rdf:resource="http://www.w3.org/2004/02/skos/core#Concept"/>
	<dcterms:modified rdf:datatype="http://www.w3.org/2001/XMLSchema#dateTime">2015-05-12T01:29:21Z</dcterms:modified>
	<dcterms:creator rdf:datatype="http://www.w3.org/2001/XMLSchema#string">Natalia Atkins</dcterms:creator>
	<dcterms:created rdf:datatype="http://www.w3.org/2001/XMLSchema#dateTime">2015-04-27T10:38:15Z</dcterms:created>
	<skos:broadMatch rdf:resource="http://vocab.aodn.org.au/def/organisation_classes/category/5"/>
	<skos:prefLabel xml:lang="en">Oceanwise Expeditions</skos:prefLabel>
	<skos:definition xml:lang="en">Oceanwise was first initiated in 1998 by a group of dedicated young scientists to promote awareness of the Ningaloo environment. To achieve this goal, the group aimed to conduct original research and management initiatives in conjunction with the Department of Conservation and Environment, WA Universities and other public and private bodies.</skos:definition>
	<dc:source rdf:datatype="http://www.w3.org/2001/XMLSchema#string">Australian Ocean Data Network Organisation Register</dc:source>
	<dc:publisher rdf:datatype="http://www.w3.org/2001/XMLSchema#string">eMarine Information Infrastructure (eMII)</dc:publisher>
	<skos:exactMatch rdf:resource="http://seadatanet.maris2.nl/v_edmo/print.asp?n_code=4110"/>
	<skos:topConceptOf rdf:resource="http://vocab.aodn.org.au/def/organisation/1"/>
	<skos:inScheme rdf:resource="http://vocab.aodn.org.au/def/organisation/1"/>
</rdf:Description>

<rdf:Description rdf:about="http://vocab.aodn.org.au/def/organisation/entity/106">
	<rdf:type rdf:resource="http://www.w3.org/2000/01/rdf-schema#Resource"/>
	<rdf:type rdf:resource="http://www.w3.org/2004/02/skos/core#Concept"/>
	<dcterms:modified rdf:datatype="http://www.w3.org/2001/XMLSchema#dateTime">2015-05-12T00:52:42Z</dcterms:modified>
	<dcterms:creator rdf:datatype="http://www.w3.org/2001/XMLSchema#string">Natalia Atkins</dcterms:creator>
	<dcterms:created rdf:datatype="http://www.w3.org/2001/XMLSchema#dateTime">2015-04-27T10:38:15Z</dcterms:created>
	<skos:broadMatch rdf:resource="http://vocab.aodn.org.au/def/organisation_classes/category/5"/>
	<skos:prefLabel xml:lang="en">BMT Oceanica</skos:prefLabel>
	<skos:definition xml:lang="en">BMT Oceanica provides marine and coastal environmental consulting services.</skos:definition>
	<dc:source rdf:datatype="http://www.w3.org/2001/XMLSchema#string">Australian Ocean Data Network Organisation Register</dc:source>
	<dc:publisher rdf:datatype="http://www.w3.org/2001/XMLSchema#string">eMarine Information Infrastructure (eMII)</dc:publisher>
	<skos:exactMatch rdf:resource="http://seadatanet.maris2.nl/v_edmo/print.asp?n_code=3970"/>
	<skos:topConceptOf rdf:resource="http://vocab.aodn.org.au/def/organisation/1"/>
	<skos:inScheme rdf:resource="http://vocab.aodn.org.au/def/organisation/1"/>
</rdf:Description>

<rdf:Description rdf:about="http://vocab.aodn.org.au/def/organisation/entity/107">
	<rdf:type rdf:resource="http://www.w3.org/2000/01/rdf-schema#Resource"/>
	<rdf:type rdf:resource="http://www.w3.org/2004/02/skos/core#Concept"/>
	<dcterms:modified rdf:datatype="http://www.w3.org/2001/XMLSchema#dateTime">2015-05-12T01:29:16Z</dcterms:modified>
	<dcterms:creator rdf:datatype="http://www.w3.org/2001/XMLSchema#string">Natalia Atkins</dcterms:creator>
	<dcterms:created rdf:datatype="http://www.w3.org/2001/XMLSchema#dateTime">2015-04-27T10:38:15Z</dcterms:created>
	<skos:broadMatch rdf:resource="http://vocab.aodn.org.au/def/organisation_classes/category/5"/>
	<skos:prefLabel xml:lang="en">Oceanographic Field Services Pty Ltd</skos:prefLabel>
	<dc:source rdf:datatype="http://www.w3.org/2001/XMLSchema#string">Australian Ocean Data Network Organisation Register</dc:source>
	<dc:publisher rdf:datatype="http://www.w3.org/2001/XMLSchema#string">eMarine Information Infrastructure (eMII)</dc:publisher>
	<skos:exactMatch rdf:resource="http://seadatanet.maris2.nl/v_edmo/print.asp?n_code=3952"/>
	<skos:topConceptOf rdf:resource="http://vocab.aodn.org.au/def/organisation/1"/>
	<skos:inScheme rdf:resource="http://vocab.aodn.org.au/def/organisation/1"/>
</rdf:Description>

<rdf:Description rdf:about="http://vocab.aodn.org.au/def/organisation/entity/108">
	<rdf:type rdf:resource="http://www.w3.org/2000/01/rdf-schema#Resource"/>
	<rdf:type rdf:resource="http://www.w3.org/2004/02/skos/core#Concept"/>
	<dcterms:modified rdf:datatype="http://www.w3.org/2001/XMLSchema#dateTime">2015-05-12T01:29:06Z</dcterms:modified>
	<dcterms:creator rdf:datatype="http://www.w3.org/2001/XMLSchema#string">Natalia Atkins</dcterms:creator>
	<dcterms:created rdf:datatype="http://www.w3.org/2001/XMLSchema#dateTime">2015-04-27T10:38:15Z</dcterms:created>
	<skos:broadMatch rdf:resource="http://vocab.aodn.org.au/def/organisation_classes/category/5"/>
	<skos:prefLabel xml:lang="en">OMC International Pty Ltd</skos:prefLabel>
	<skos:hiddenLabel xml:lang="en"></skos:hiddenLabel>
	<skos:definition xml:lang="en">OMC International, an Australian maritime engineering company, was established in 1987.</skos:definition>
	<dc:source rdf:datatype="http://www.w3.org/2001/XMLSchema#string">Australian Ocean Data Network Organisation Register</dc:source>
	<dc:publisher rdf:datatype="http://www.w3.org/2001/XMLSchema#string">eMarine Information Infrastructure (eMII)</dc:publisher>
	<skos:exactMatch rdf:resource="http://seadatanet.maris2.nl/v_edmo/print.asp?n_code=4111"/>
	<skos:topConceptOf rdf:resource="http://vocab.aodn.org.au/def/organisation/1"/>
	<skos:inScheme rdf:resource="http://vocab.aodn.org.au/def/organisation/1"/>
</rdf:Description>

<rdf:Description rdf:about="http://vocab.aodn.org.au/def/organisation/entity/109">
	<rdf:type rdf:resource="http://www.w3.org/2000/01/rdf-schema#Resource"/>
	<rdf:type rdf:resource="http://www.w3.org/2004/02/skos/core#Concept"/>
	<dcterms:modified rdf:datatype="http://www.w3.org/2001/XMLSchema#dateTime">2015-05-12T01:29:42Z</dcterms:modified>
	<dcterms:creator rdf:datatype="http://www.w3.org/2001/XMLSchema#string">Natalia Atkins</dcterms:creator>
	<dcterms:created rdf:datatype="http://www.w3.org/2001/XMLSchema#dateTime">2015-04-27T10:38:15Z</dcterms:created>
	<skos:broadMatch rdf:resource="http://vocab.aodn.org.au/def/organisation_classes/category/2"/>
	<skos:prefLabel xml:lang="en">Pawsey Supercomputing Centre</skos:prefLabel>
	<skos:definition xml:lang="en">The centre comprises a purpose-built building, housing supercomputers and associated works at Kensington, Western Australia. The primary aim of the centre is to host new supercomputing facilities and expertise to support SKA (Square Kilometre Array) pathfinder research, geosciences and other high-end science.</skos:definition>
	<dc:source rdf:datatype="http://www.w3.org/2001/XMLSchema#string">Australian Ocean Data Network Organisation Register</dc:source>
	<dc:publisher rdf:datatype="http://www.w3.org/2001/XMLSchema#string">eMarine Information Infrastructure (eMII)</dc:publisher>
	<skos:exactMatch rdf:resource="http://seadatanet.maris2.nl/v_edmo/print.asp?n_code=3954"/>
	<skos:topConceptOf rdf:resource="http://vocab.aodn.org.au/def/organisation/1"/>
	<skos:inScheme rdf:resource="http://vocab.aodn.org.au/def/organisation/1"/>
</rdf:Description>

<rdf:Description rdf:about="http://vocab.aodn.org.au/def/organisation/entity/110">
	<rdf:type rdf:resource="http://www.w3.org/2000/01/rdf-schema#Resource"/>
	<rdf:type rdf:resource="http://www.w3.org/2004/02/skos/core#Concept"/>
	<dcterms:modified rdf:datatype="http://www.w3.org/2001/XMLSchema#dateTime">2015-05-12T01:29:46Z</dcterms:modified>
	<dcterms:creator rdf:datatype="http://www.w3.org/2001/XMLSchema#string">Natalia Atkins</dcterms:creator>
	<dcterms:created rdf:datatype="http://www.w3.org/2001/XMLSchema#dateTime">2015-04-27T10:38:15Z</dcterms:created>
	<skos:broadMatch rdf:resource="http://vocab.aodn.org.au/def/organisation_classes/category/5"/>
	<skos:prefLabel xml:lang="en">Pearl Producers Association Inc (PPA)</skos:prefLabel>
	<skos:hiddenLabel xml:lang="en">PPA</skos:hiddenLabel>
	<dc:source rdf:datatype="http://www.w3.org/2001/XMLSchema#string">Australian Ocean Data Network Organisation Register</dc:source>
	<dc:publisher rdf:datatype="http://www.w3.org/2001/XMLSchema#string">eMarine Information Infrastructure (eMII)</dc:publisher>
	<skos:exactMatch rdf:resource="http://seadatanet.maris2.nl/v_edmo/print.asp?n_code=4112"/>
	<skos:topConceptOf rdf:resource="http://vocab.aodn.org.au/def/organisation/1"/>
	<skos:inScheme rdf:resource="http://vocab.aodn.org.au/def/organisation/1"/>
</rdf:Description>

<rdf:Description rdf:about="http://vocab.aodn.org.au/def/organisation/entity/111">
	<rdf:type rdf:resource="http://www.w3.org/2000/01/rdf-schema#Resource"/>
	<rdf:type rdf:resource="http://www.w3.org/2004/02/skos/core#Concept"/>
	<dcterms:modified rdf:datatype="http://www.w3.org/2001/XMLSchema#dateTime">2015-05-12T01:29:51Z</dcterms:modified>
	<dcterms:creator rdf:datatype="http://www.w3.org/2001/XMLSchema#string">Natalia Atkins</dcterms:creator>
	<dcterms:created rdf:datatype="http://www.w3.org/2001/XMLSchema#dateTime">2015-04-27T10:38:15Z</dcterms:created>
	<skos:broadMatch rdf:resource="http://vocab.aodn.org.au/def/organisation_classes/category/5"/>
	<skos:prefLabel xml:lang="en">Pendoley Environmental Pty Ltd</skos:prefLabel>
	<skos:definition xml:lang="en">Pendoley Environmental is a Western Australian based marine conservation biology consultancy service.</skos:definition>
	<dc:source rdf:datatype="http://www.w3.org/2001/XMLSchema#string">Australian Ocean Data Network Organisation Register</dc:source>
	<dc:publisher rdf:datatype="http://www.w3.org/2001/XMLSchema#string">eMarine Information Infrastructure (eMII)</dc:publisher>
	<skos:exactMatch rdf:resource="http://seadatanet.maris2.nl/v_edmo/print.asp?n_code=3940"/>
	<skos:topConceptOf rdf:resource="http://vocab.aodn.org.au/def/organisation/1"/>
	<skos:inScheme rdf:resource="http://vocab.aodn.org.au/def/organisation/1"/>
</rdf:Description>

<rdf:Description rdf:about="http://vocab.aodn.org.au/def/organisation/entity/112">
	<rdf:type rdf:resource="http://www.w3.org/2000/01/rdf-schema#Resource"/>
	<rdf:type rdf:resource="http://www.w3.org/2004/02/skos/core#Concept"/>
	<dcterms:modified rdf:datatype="http://www.w3.org/2001/XMLSchema#dateTime">2015-05-12T01:29:36Z</dcterms:modified>
	<dcterms:creator rdf:datatype="http://www.w3.org/2001/XMLSchema#string">Natalia Atkins</dcterms:creator>
	<dcterms:created rdf:datatype="http://www.w3.org/2001/XMLSchema#dateTime">2015-04-27T10:38:15Z</dcterms:created>
	<skos:broadMatch rdf:resource="http://vocab.aodn.org.au/def/organisation_classes/category/5"/>
	<skos:prefLabel xml:lang="en">PPK Environment and Infrastructure Pty Ltd</skos:prefLabel>
	<dc:source rdf:datatype="http://www.w3.org/2001/XMLSchema#string">Australian Ocean Data Network Organisation Register</dc:source>
	<dc:publisher rdf:datatype="http://www.w3.org/2001/XMLSchema#string">eMarine Information Infrastructure (eMII)</dc:publisher>
	<skos:exactMatch rdf:resource="http://seadatanet.maris2.nl/v_edmo/print.asp?n_code=4113"/>
	<skos:topConceptOf rdf:resource="http://vocab.aodn.org.au/def/organisation/1"/>
	<skos:inScheme rdf:resource="http://vocab.aodn.org.au/def/organisation/1"/>
</rdf:Description>

<rdf:Description rdf:about="http://vocab.aodn.org.au/def/organisation/entity/113">
	<rdf:type rdf:resource="http://www.w3.org/2000/01/rdf-schema#Resource"/>
	<rdf:type rdf:resource="http://www.w3.org/2004/02/skos/core#Concept"/>
	<dcterms:modified rdf:datatype="http://www.w3.org/2001/XMLSchema#dateTime">2015-05-12T01:29:56Z</dcterms:modified>
	<dcterms:creator rdf:datatype="http://www.w3.org/2001/XMLSchema#string">Natalia Atkins</dcterms:creator>
	<dcterms:created rdf:datatype="http://www.w3.org/2001/XMLSchema#dateTime">2015-04-27T10:38:15Z</dcterms:created>
	<skos:broadMatch rdf:resource="http://vocab.aodn.org.au/def/organisation_classes/category/2"/>
	<skos:prefLabel xml:lang="en">Primary Industries and Regions SA (PIRSA)</skos:prefLabel>
	<skos:hiddenLabel xml:lang="en">PIRSA</skos:hiddenLabel>
	<skos:definition xml:lang="en">Primary Industries and Regions SA (PIRSA) is a Government of South Australia agency with the vision of growing sustainable and competitive regions. PIRSA is committed to the sustainable use of the state's agriculture, wine, seafood, forestry, and food industries along with the provision of associated research, regulation, policy development and biosecurity imperatives. PIRSA leads and drives the State Government’s strategic priority of Premium Food and Wine from our Clean Environment.</skos:definition>
	<dc:source rdf:datatype="http://www.w3.org/2001/XMLSchema#string">Australian Ocean Data Network Organisation Register</dc:source>
	<dc:publisher rdf:datatype="http://www.w3.org/2001/XMLSchema#string">eMarine Information Infrastructure (eMII)</dc:publisher>
	<skos:exactMatch rdf:resource="http://seadatanet.maris2.nl/v_edmo/print.asp?n_code=4114"/>
	<skos:topConceptOf rdf:resource="http://vocab.aodn.org.au/def/organisation/1"/>
	<skos:inScheme rdf:resource="http://vocab.aodn.org.au/def/organisation/1"/>
</rdf:Description>

<rdf:Description rdf:about="http://vocab.aodn.org.au/def/organisation/entity/114">
	<rdf:type rdf:resource="http://www.w3.org/2000/01/rdf-schema#Resource"/>
	<rdf:type rdf:resource="http://www.w3.org/2004/02/skos/core#Concept"/>
	<dcterms:modified rdf:datatype="http://www.w3.org/2001/XMLSchema#dateTime">2015-05-12T01:30:00Z</dcterms:modified>
	<dcterms:creator rdf:datatype="http://www.w3.org/2001/XMLSchema#string">Natalia Atkins</dcterms:creator>
	<dcterms:created rdf:datatype="http://www.w3.org/2001/XMLSchema#dateTime">2015-04-27T10:38:15Z</dcterms:created>
	<skos:broadMatch rdf:resource="http://vocab.aodn.org.au/def/organisation_classes/category/2"/>
	<skos:prefLabel xml:lang="en">Queensland Museum</skos:prefLabel>
	<skos:definition xml:lang="en">Queensland Museum is a museum of natural history, cultural heritage, science and human achievement that tells the changing story of Queensland.</skos:definition>
	<dc:source rdf:datatype="http://www.w3.org/2001/XMLSchema#string">Australian Ocean Data Network Organisation Register</dc:source>
	<dc:publisher rdf:datatype="http://www.w3.org/2001/XMLSchema#string">eMarine Information Infrastructure (eMII)</dc:publisher>
	<skos:exactMatch rdf:resource="http://seadatanet.maris2.nl/v_edmo/print.asp?n_code=4115"/>
	<skos:topConceptOf rdf:resource="http://vocab.aodn.org.au/def/organisation/1"/>
	<skos:inScheme rdf:resource="http://vocab.aodn.org.au/def/organisation/1"/>
</rdf:Description>

<rdf:Description rdf:about="http://vocab.aodn.org.au/def/organisation/entity/115">
	<rdf:type rdf:resource="http://www.w3.org/2000/01/rdf-schema#Resource"/>
	<rdf:type rdf:resource="http://www.w3.org/2004/02/skos/core#Concept"/>
	<dcterms:modified rdf:datatype="http://www.w3.org/2001/XMLSchema#dateTime">2015-05-12T01:30:21Z</dcterms:modified>
	<dcterms:creator rdf:datatype="http://www.w3.org/2001/XMLSchema#string">Natalia Atkins</dcterms:creator>
	<dcterms:created rdf:datatype="http://www.w3.org/2001/XMLSchema#dateTime">2015-04-27T10:38:15Z</dcterms:created>
	<skos:broadMatch rdf:resource="http://vocab.aodn.org.au/def/organisation_classes/category/5"/>
	<skos:prefLabel xml:lang="en">Rick Scoones and Associates</skos:prefLabel>
	<dc:source rdf:datatype="http://www.w3.org/2001/XMLSchema#string">Australian Ocean Data Network Organisation Register</dc:source>
	<dc:publisher rdf:datatype="http://www.w3.org/2001/XMLSchema#string">eMarine Information Infrastructure (eMII)</dc:publisher>
	<skos:topConceptOf rdf:resource="http://vocab.aodn.org.au/def/organisation/1"/>
	<skos:inScheme rdf:resource="http://vocab.aodn.org.au/def/organisation/1"/>
</rdf:Description>

<rdf:Description rdf:about="http://vocab.aodn.org.au/def/organisation/entity/116">
	<rdf:type rdf:resource="http://www.w3.org/2000/01/rdf-schema#Resource"/>
	<rdf:type rdf:resource="http://www.w3.org/2004/02/skos/core#Concept"/>
	<dcterms:modified rdf:datatype="http://www.w3.org/2001/XMLSchema#dateTime">2015-05-12T01:30:10Z</dcterms:modified>
	<dcterms:creator rdf:datatype="http://www.w3.org/2001/XMLSchema#string">Natalia Atkins</dcterms:creator>
	<dcterms:created rdf:datatype="http://www.w3.org/2001/XMLSchema#dateTime">2015-04-27T10:38:15Z</dcterms:created>
	<skos:broadMatch rdf:resource="http://vocab.aodn.org.au/def/organisation_classes/category/5"/>
	<skos:prefLabel xml:lang="en">RPS MetOcean Pty Ltd</skos:prefLabel>
	<skos:definition xml:lang="en">"RPS MetOcean designs and implements sophisticated meteorological and oceanographic measurement programs to obtain reliable information on winds, waves, tides, currents and seawater properties.  
RPS MetOcean's experienced staff are skilled in ocean and environmental engineering, electronics, computing and mathematics, numerical modelling, data analysis, technical reporting and project management."</skos:definition>
	<dc:source rdf:datatype="http://www.w3.org/2001/XMLSchema#string">Australian Ocean Data Network Organisation Register</dc:source>
	<dc:publisher rdf:datatype="http://www.w3.org/2001/XMLSchema#string">eMarine Information Infrastructure (eMII)</dc:publisher>
	<skos:exactMatch rdf:resource="http://seadatanet.maris2.nl/v_edmo/print.asp?n_code=4116"/>
	<skos:topConceptOf rdf:resource="http://vocab.aodn.org.au/def/organisation/1"/>
	<skos:inScheme rdf:resource="http://vocab.aodn.org.au/def/organisation/1"/>
</rdf:Description>

<rdf:Description rdf:about="http://vocab.aodn.org.au/def/organisation/entity/117">
	<rdf:type rdf:resource="http://www.w3.org/2000/01/rdf-schema#Resource"/>
	<rdf:type rdf:resource="http://www.w3.org/2004/02/skos/core#Concept"/>
	<dcterms:modified rdf:datatype="http://www.w3.org/2001/XMLSchema#dateTime">2015-05-12T01:30:35Z</dcterms:modified>
	<dcterms:creator rdf:datatype="http://www.w3.org/2001/XMLSchema#string">Natalia Atkins</dcterms:creator>
	<dcterms:created rdf:datatype="http://www.w3.org/2001/XMLSchema#dateTime">2015-04-27T10:38:15Z</dcterms:created>
	<skos:broadMatch rdf:resource="http://vocab.aodn.org.au/def/organisation_classes/category/2"/>
	<skos:prefLabel xml:lang="en">SA Water</skos:prefLabel>
	<skos:definition xml:lang="en">SA Water is a government enterprise, wholly owned by the Government of South Australia and was established by the proclamation of the South Australian Water Corporation Act 1994 on 1 July 1995. It provides water and wastewater services to approximately 1.5 million people in South Australia.</skos:definition>
	<dc:source rdf:datatype="http://www.w3.org/2001/XMLSchema#string">Australian Ocean Data Network Organisation Register</dc:source>
	<dc:publisher rdf:datatype="http://www.w3.org/2001/XMLSchema#string">eMarine Information Infrastructure (eMII)</dc:publisher>
	<skos:exactMatch rdf:resource="http://seadatanet.maris2.nl/v_edmo/print.asp?n_code=4117"/>
	<skos:topConceptOf rdf:resource="http://vocab.aodn.org.au/def/organisation/1"/>
	<skos:inScheme rdf:resource="http://vocab.aodn.org.au/def/organisation/1"/>
</rdf:Description>

<rdf:Description rdf:about="http://vocab.aodn.org.au/def/organisation/entity/118">
	<rdf:type rdf:resource="http://www.w3.org/2000/01/rdf-schema#Resource"/>
	<rdf:type rdf:resource="http://www.w3.org/2004/02/skos/core#Concept"/>
	<dcterms:modified rdf:datatype="http://www.w3.org/2001/XMLSchema#dateTime">2015-05-12T01:30:40Z</dcterms:modified>
	<dcterms:creator rdf:datatype="http://www.w3.org/2001/XMLSchema#string">Natalia Atkins</dcterms:creator>
	<dcterms:created rdf:datatype="http://www.w3.org/2001/XMLSchema#dateTime">2015-04-27T10:38:15Z</dcterms:created>
	<skos:broadMatch rdf:resource="http://vocab.aodn.org.au/def/organisation_classes/category/5"/>
	<skos:prefLabel xml:lang="en">Santos Ltd</skos:prefLabel>
	<skos:definition xml:lang="en">An Australian energy pioneer since 1954, Santos is a leading oil and gas producer, supplying Australian and Asian customers. With its origins in the Cooper Basin, Santos is one of Australia’s largest producers of gas to the domestic market and has the largest exploration and production acreage position in Australia of any company.</skos:definition>
	<dc:source rdf:datatype="http://www.w3.org/2001/XMLSchema#string">Australian Ocean Data Network Organisation Register</dc:source>
	<dc:publisher rdf:datatype="http://www.w3.org/2001/XMLSchema#string">eMarine Information Infrastructure (eMII)</dc:publisher>
	<skos:exactMatch rdf:resource="http://seadatanet.maris2.nl/v_edmo/print.asp?n_code=4118"/>
	<skos:topConceptOf rdf:resource="http://vocab.aodn.org.au/def/organisation/1"/>
	<skos:inScheme rdf:resource="http://vocab.aodn.org.au/def/organisation/1"/>
</rdf:Description>

<rdf:Description rdf:about="http://vocab.aodn.org.au/def/organisation/entity/119">
	<rdf:type rdf:resource="http://www.w3.org/2000/01/rdf-schema#Resource"/>
	<rdf:type rdf:resource="http://www.w3.org/2004/02/skos/core#Concept"/>
	<dcterms:modified rdf:datatype="http://www.w3.org/2001/XMLSchema#dateTime">2015-05-12T01:30:29Z</dcterms:modified>
	<dcterms:creator rdf:datatype="http://www.w3.org/2001/XMLSchema#string">Natalia Atkins</dcterms:creator>
	<dcterms:created rdf:datatype="http://www.w3.org/2001/XMLSchema#dateTime">2015-04-27T10:38:15Z</dcterms:created>
	<skos:broadMatch rdf:resource="http://vocab.aodn.org.au/def/organisation_classes/category/5"/>
	<skos:prefLabel xml:lang="en">S2V Consulting Pty Ltd</skos:prefLabel>
	<skos:definition xml:lang="en">S2V Consulting provides technical and strategic advice to the oil and gas industry.</skos:definition>
	<dc:source rdf:datatype="http://www.w3.org/2001/XMLSchema#string">Australian Ocean Data Network Organisation Register</dc:source>
	<dc:publisher rdf:datatype="http://www.w3.org/2001/XMLSchema#string">eMarine Information Infrastructure (eMII)</dc:publisher>
	<skos:exactMatch rdf:resource="http://seadatanet.maris2.nl/v_edmo/print.asp?n_code=4119"/>
	<skos:topConceptOf rdf:resource="http://vocab.aodn.org.au/def/organisation/1"/>
	<skos:inScheme rdf:resource="http://vocab.aodn.org.au/def/organisation/1"/>
</rdf:Description>

<rdf:Description rdf:about="http://vocab.aodn.org.au/def/organisation/entity/120">
	<rdf:type rdf:resource="http://www.w3.org/2000/01/rdf-schema#Resource"/>
	<rdf:type rdf:resource="http://www.w3.org/2004/02/skos/core#Concept"/>
	<dcterms:modified rdf:datatype="http://www.w3.org/2001/XMLSchema#dateTime">2015-05-12T01:31:20Z</dcterms:modified>
	<dcterms:creator rdf:datatype="http://www.w3.org/2001/XMLSchema#string">Natalia Atkins</dcterms:creator>
	<dcterms:created rdf:datatype="http://www.w3.org/2001/XMLSchema#dateTime">2015-04-27T10:38:15Z</dcterms:created>
	<skos:broadMatch rdf:resource="http://vocab.aodn.org.au/def/organisation_classes/category/6"/>
	<skos:prefLabel xml:lang="en">SeaCare Inc</skos:prefLabel>
	<skos:definition xml:lang="en">SeaCare was formed in 1998 as a nonprofit organisation supported by the National Heritage Trust of Australia Fisheries Action Program. It is a community based group formed to facilitate projects aimed at benefiting the marine environment in Tasmania.</skos:definition>
	<dc:source rdf:datatype="http://www.w3.org/2001/XMLSchema#string">Australian Ocean Data Network Organisation Register</dc:source>
	<dc:publisher rdf:datatype="http://www.w3.org/2001/XMLSchema#string">eMarine Information Infrastructure (eMII)</dc:publisher>
	<skos:exactMatch rdf:resource="http://seadatanet.maris2.nl/v_edmo/print.asp?n_code=4120"/>
	<skos:topConceptOf rdf:resource="http://vocab.aodn.org.au/def/organisation/1"/>
	<skos:inScheme rdf:resource="http://vocab.aodn.org.au/def/organisation/1"/>
</rdf:Description>

<rdf:Description rdf:about="http://vocab.aodn.org.au/def/organisation/entity/121">
	<rdf:type rdf:resource="http://www.w3.org/2000/01/rdf-schema#Resource"/>
	<rdf:type rdf:resource="http://www.w3.org/2004/02/skos/core#Concept"/>
	<dcterms:modified rdf:datatype="http://www.w3.org/2001/XMLSchema#dateTime">2015-05-12T01:31:35Z</dcterms:modified>
	<dcterms:creator rdf:datatype="http://www.w3.org/2001/XMLSchema#string">Natalia Atkins</dcterms:creator>
	<dcterms:created rdf:datatype="http://www.w3.org/2001/XMLSchema#dateTime">2015-04-27T10:38:15Z</dcterms:created>
	<skos:broadMatch rdf:resource="http://vocab.aodn.org.au/def/organisation_classes/category/2"/>
	<skos:prefLabel xml:lang="en">Sydney Institute of Marine Science (SIMS)</skos:prefLabel>
	<skos:hiddenLabel xml:lang="en">SIMS</skos:hiddenLabel>
	<skos:definition xml:lang="en">The Sydney Institute of Marine Science (SIMS) conducts multidisciplinary marine research across five core research themes  - Urbanisation, Biodiversity, Climate Change, Ocean Resources, and Marine Management. SIMS is also the operator of the NSW node of the Australian Government’s Integrated Marine Observing System – IMOS.</skos:definition>
	<dc:source rdf:datatype="http://www.w3.org/2001/XMLSchema#string">Australian Ocean Data Network Organisation Register</dc:source>
	<dc:publisher rdf:datatype="http://www.w3.org/2001/XMLSchema#string">eMarine Information Infrastructure (eMII)</dc:publisher>
	<skos:exactMatch rdf:resource="http://seadatanet.maris2.nl/v_edmo/print.asp?n_code=3953"/>
	<skos:topConceptOf rdf:resource="http://vocab.aodn.org.au/def/organisation/1"/>
	<skos:inScheme rdf:resource="http://vocab.aodn.org.au/def/organisation/1"/>
</rdf:Description>

<rdf:Description rdf:about="http://vocab.aodn.org.au/def/organisation/entity/122">
	<rdf:type rdf:resource="http://www.w3.org/2000/01/rdf-schema#Resource"/>
	<rdf:type rdf:resource="http://www.w3.org/2004/02/skos/core#Concept"/>
	<dcterms:modified rdf:datatype="http://www.w3.org/2001/XMLSchema#dateTime">2015-05-12T01:31:30Z</dcterms:modified>
	<dcterms:creator rdf:datatype="http://www.w3.org/2001/XMLSchema#string">Natalia Atkins</dcterms:creator>
	<dcterms:created rdf:datatype="http://www.w3.org/2001/XMLSchema#dateTime">2015-04-27T10:38:15Z</dcterms:created>
	<skos:broadMatch rdf:resource="http://vocab.aodn.org.au/def/organisation_classes/category/2"/>
	<skos:prefLabel xml:lang="en">South Australian Research and Development Institute (SARDI)</skos:prefLabel>
	<skos:hiddenLabel xml:lang="en">SARDI</skos:hiddenLabel>
	<skos:definition xml:lang="en">SARDI is a world-class research and development institute delivering innovation to enhance the food, fibre and bioscience industries and living environmental systems in southern Australia. As the SA Government's principal research and development capability, science programs embrace industry and community needs aligned to South Australia's strategic plan and 10-year vision for Science, Technology and Innovation. SARDI pursues excellence through highly skilled scientists, post-graduates students and technicians supported by state-of-the-art advanced research facilities at 16 locations throughout the State. Regional sites provide significant regional employment, community capacity, technology transfer and industry development. Programs focus on innovative, cost-effective technologies to meet emerging market needs that underpin internationally competitive and ecologically sustainable industries.</skos:definition>
	<dc:source rdf:datatype="http://www.w3.org/2001/XMLSchema#string">Australian Ocean Data Network Organisation Register</dc:source>
	<dc:publisher rdf:datatype="http://www.w3.org/2001/XMLSchema#string">eMarine Information Infrastructure (eMII)</dc:publisher>
	<skos:exactMatch rdf:resource="http://seadatanet.maris2.nl/v_edmo/print.asp?n_code=1486"/>
	<skos:narrower rdf:resource="http://vocab.aodn.org.au/def/organisation/entity/123"/>
	<skos:topConceptOf rdf:resource="http://vocab.aodn.org.au/def/organisation/1"/>
	<skos:inScheme rdf:resource="http://vocab.aodn.org.au/def/organisation/1"/>
</rdf:Description>

<rdf:Description rdf:about="http://vocab.aodn.org.au/def/organisation/entity/124">
	<rdf:type rdf:resource="http://www.w3.org/2000/01/rdf-schema#Resource"/>
	<rdf:type rdf:resource="http://www.w3.org/2004/02/skos/core#Concept"/>
	<dcterms:modified rdf:datatype="http://www.w3.org/2001/XMLSchema#dateTime">2015-05-12T01:31:41Z</dcterms:modified>
	<dcterms:creator rdf:datatype="http://www.w3.org/2001/XMLSchema#string">Natalia Atkins</dcterms:creator>
	<dcterms:created rdf:datatype="http://www.w3.org/2001/XMLSchema#dateTime">2015-04-27T10:38:15Z</dcterms:created>
	<skos:broadMatch rdf:resource="http://vocab.aodn.org.au/def/organisation_classes/category/5"/>
	<skos:prefLabel xml:lang="en">Synnot and Wilkinson Strategic Environmental Consulting</skos:prefLabel>
	<skos:definition xml:lang="en">Synnot Wilkinson are a specialist strategic environmental consulting firm based in Victoria, Australia.</skos:definition>
	<dc:source rdf:datatype="http://www.w3.org/2001/XMLSchema#string">Australian Ocean Data Network Organisation Register</dc:source>
	<dc:publisher rdf:datatype="http://www.w3.org/2001/XMLSchema#string">eMarine Information Infrastructure (eMII)</dc:publisher>
	<skos:exactMatch rdf:resource="http://seadatanet.maris2.nl/v_edmo/print.asp?n_code=3966"/>
	<skos:topConceptOf rdf:resource="http://vocab.aodn.org.au/def/organisation/1"/>
	<skos:inScheme rdf:resource="http://vocab.aodn.org.au/def/organisation/1"/>
</rdf:Description>

<rdf:Description rdf:about="http://vocab.aodn.org.au/def/organisation/entity/125">
	<rdf:type rdf:resource="http://www.w3.org/2000/01/rdf-schema#Resource"/>
	<rdf:type rdf:resource="http://www.w3.org/2004/02/skos/core#Concept"/>
	<dcterms:modified rdf:datatype="http://www.w3.org/2001/XMLSchema#dateTime">2015-05-12T01:40:42Z</dcterms:modified>
	<dcterms:creator rdf:datatype="http://www.w3.org/2001/XMLSchema#string">Natalia Atkins</dcterms:creator>
	<dcterms:created rdf:datatype="http://www.w3.org/2001/XMLSchema#dateTime">2015-04-27T10:38:15Z</dcterms:created>
	<skos:broadMatch rdf:resource="http://vocab.aodn.org.au/def/organisation_classes/category/5"/>
	<skos:prefLabel xml:lang="en">Tasmanian Sea Urchin Developments</skos:prefLabel>
	<dc:source rdf:datatype="http://www.w3.org/2001/XMLSchema#string">Australian Ocean Data Network Organisation Register</dc:source>
	<dc:publisher rdf:datatype="http://www.w3.org/2001/XMLSchema#string">eMarine Information Infrastructure (eMII)</dc:publisher>
	<skos:topConceptOf rdf:resource="http://vocab.aodn.org.au/def/organisation/1"/>
	<skos:inScheme rdf:resource="http://vocab.aodn.org.au/def/organisation/1"/>
	<skos:scopeNote xml:lang="en">Organisation no longer exists</skos:scopeNote>
</rdf:Description>

<rdf:Description rdf:about="http://vocab.aodn.org.au/def/organisation/entity/126">
	<rdf:type rdf:resource="http://www.w3.org/2000/01/rdf-schema#Resource"/>
	<rdf:type rdf:resource="http://www.w3.org/2004/02/skos/core#Concept"/>
	<dcterms:modified rdf:datatype="http://www.w3.org/2001/XMLSchema#dateTime">2015-05-12T01:41:46Z</dcterms:modified>
	<dcterms:creator rdf:datatype="http://www.w3.org/2001/XMLSchema#string">Natalia Atkins</dcterms:creator>
	<dcterms:created rdf:datatype="http://www.w3.org/2001/XMLSchema#dateTime">2015-04-27T10:38:15Z</dcterms:created>
	<skos:broadMatch rdf:resource="http://vocab.aodn.org.au/def/organisation_classes/category/5"/>
	<skos:prefLabel xml:lang="en">URS Australia</skos:prefLabel>
	<skos:definition xml:lang="en">URS is a leading provider of engineering, construction, and technical services for public agencies and private sector companies around the world.</skos:definition>
	<dc:source rdf:datatype="http://www.w3.org/2001/XMLSchema#string">Australian Ocean Data Network Organisation Register</dc:source>
	<dc:publisher rdf:datatype="http://www.w3.org/2001/XMLSchema#string">eMarine Information Infrastructure (eMII)</dc:publisher>
	<skos:exactMatch rdf:resource="http://seadatanet.maris2.nl/v_edmo/print.asp?n_code=4121"/>
	<skos:topConceptOf rdf:resource="http://vocab.aodn.org.au/def/organisation/1"/>
	<skos:inScheme rdf:resource="http://vocab.aodn.org.au/def/organisation/1"/>
</rdf:Description>

<rdf:Description rdf:about="http://vocab.aodn.org.au/def/organisation/entity/127">
	<rdf:type rdf:resource="http://www.w3.org/2000/01/rdf-schema#Resource"/>
	<rdf:type rdf:resource="http://www.w3.org/2004/02/skos/core#Concept"/>
	<dcterms:modified rdf:datatype="http://www.w3.org/2001/XMLSchema#dateTime">2015-05-12T01:41:56Z</dcterms:modified>
	<dcterms:modified rdf:datatype="http://www.w3.org/2001/XMLSchema#dateTime">2016-01-28T04:25:01Z</dcterms:modified>
	<dcterms:creator rdf:datatype="http://www.w3.org/2001/XMLSchema#string">Natalia Atkins</dcterms:creator>
	<dcterms:created rdf:datatype="http://www.w3.org/2001/XMLSchema#dateTime">2015-04-27T10:38:15Z</dcterms:created>
	<dcterms:contributor rdf:datatype="http://www.w3.org/2001/XMLSchema#string">eMII_Atkins.Natalia</dcterms:contributor>
	<skos:broadMatch rdf:resource="http://vocab.aodn.org.au/def/organisation_classes/category/2"/>
	<skos:prefLabel xml:lang="en">Victorian Institute of Marine Sciences (VIMS)</skos:prefLabel>
	<skos:hiddenLabel xml:lang="en">VIMS</skos:hiddenLabel>
	<skos:definition xml:lang="en">The Victorian Institute of Marine Sciences (VIMS) was established by the Victorian Institute of Marine Sciences Act 1974 as a body corporate, its objects including: 'to provide facilities for and foster, carry on and support scientific research and technological development in all branches of learning concerning or touching upon marine sciences, including but without limiting the generality of that expression, the sea, the sea-bed, sea shores, and the resources and inhabitants thereof and mankind's relationship with the use of the sea'. VIMS began operations in 1978. In July 1996 the Victorian Institute of Marine Sciences, along with two other marine and freshwater groups, became a part of the Marine and Freshwater Resources Institute (MAFRI). In 1998 the decision was made to repeal the Victorian Institute of Marine Sciences Act 1974 and to include the Institute as part of the Fisheries Division of the Department of Natural Resources and Environment. In 2002 it was handed over to the newly formed Department of Primary Industries. This Department is now known as the Department of Environment, Land, Water and Planning (DELWP), as of 2014 .(Courtesy of Encyclopedia of Australian Science)</skos:definition>
	<dc:source rdf:datatype="http://www.w3.org/2001/XMLSchema#string">Australian Ocean Data Network Organisation Register</dc:source>
	<dc:publisher rdf:datatype="http://www.w3.org/2001/XMLSchema#string">eMarine Information Infrastructure (eMII)</dc:publisher>
	<skos:exactMatch rdf:resource="http://seadatanet.maris2.nl/v_edmo/print.asp?n_code=4029"/>
	<skos:topConceptOf rdf:resource="http://vocab.aodn.org.au/def/organisation/1"/>
	<skos:inScheme rdf:resource="http://vocab.aodn.org.au/def/organisation/1"/>
	<skos:scopeNote xml:lang="en">Organisation no longer exists</skos:scopeNote>
	<skos:scopeNote xml:lang="en">Organisation no longer exists. Replaced by http://vocab.aodn.org.au/def/organisation/entity/54 and http://vocab.aodn.org.au/def/organisation/entity/57</skos:scopeNote>
	<dcterms:isReplacedBy rdf:resource="http://vocab.aodn.org.au/def/organisation/entity/54"/>
	<dcterms:isReplacedBy xml:lang="en">Department of Environment, Land, Water and Planning (DELWP), Victorian Government</dcterms:isReplacedBy>
	<dcterms:isReplacedBy xml:lang="en">Department of Primary Industries (DPI), Victorian Government</dcterms:isReplacedBy>
</rdf:Description>

<rdf:Description rdf:about="http://vocab.aodn.org.au/def/organisation/entity/128">
	<rdf:type rdf:resource="http://www.w3.org/2000/01/rdf-schema#Resource"/>
	<rdf:type rdf:resource="http://www.w3.org/2004/02/skos/core#Concept"/>
	<dcterms:modified rdf:datatype="http://www.w3.org/2001/XMLSchema#dateTime">2015-05-12T01:42:54Z</dcterms:modified>
	<dcterms:creator rdf:datatype="http://www.w3.org/2001/XMLSchema#string">Natalia Atkins</dcterms:creator>
	<dcterms:created rdf:datatype="http://www.w3.org/2001/XMLSchema#dateTime">2015-04-27T10:38:15Z</dcterms:created>
	<skos:broadMatch rdf:resource="http://vocab.aodn.org.au/def/organisation_classes/category/2"/>
	<skos:prefLabel xml:lang="en">Western Australian Land Information System (WALIS)</skos:prefLabel>
	<skos:hiddenLabel xml:lang="en">WALIS</skos:hiddenLabel>
	<skos:definition xml:lang="en">Established by the WA Government in 1981, WALIS is responsible for coordinating across-government access and delivery of spatial information (marine, coastal and terrestrial). WALIS drives innovative partnerships and works with business, academia and the community to make it easier to find, use and improve location information for WA. WALIS provides a Data Discovery and Access service using the Shared Location Information Platform (SLIP).</skos:definition>
	<dc:source rdf:datatype="http://www.w3.org/2001/XMLSchema#string">Australian Ocean Data Network Organisation Register</dc:source>
	<dc:publisher rdf:datatype="http://www.w3.org/2001/XMLSchema#string">eMarine Information Infrastructure (eMII)</dc:publisher>
	<skos:exactMatch rdf:resource="http://seadatanet.maris2.nl/v_edmo/print.asp?n_code=4124"/>
	<skos:topConceptOf rdf:resource="http://vocab.aodn.org.au/def/organisation/1"/>
	<skos:inScheme rdf:resource="http://vocab.aodn.org.au/def/organisation/1"/>
</rdf:Description>

<rdf:Description rdf:about="http://vocab.aodn.org.au/def/organisation/entity/129">
	<rdf:type rdf:resource="http://www.w3.org/2000/01/rdf-schema#Resource"/>
	<rdf:type rdf:resource="http://www.w3.org/2004/02/skos/core#Concept"/>
	<dcterms:modified rdf:datatype="http://www.w3.org/2001/XMLSchema#dateTime">2015-05-12T01:43:02Z</dcterms:modified>
	<dcterms:creator rdf:datatype="http://www.w3.org/2001/XMLSchema#string">Natalia Atkins</dcterms:creator>
	<dcterms:created rdf:datatype="http://www.w3.org/2001/XMLSchema#dateTime">2015-04-27T10:38:15Z</dcterms:created>
	<skos:broadMatch rdf:resource="http://vocab.aodn.org.au/def/organisation_classes/category/2"/>
	<skos:prefLabel xml:lang="en">Western Australian Marine Science Institution (WAMSI)</skos:prefLabel>
	<skos:hiddenLabel xml:lang="en">WAMSI</skos:hiddenLabel>
	<skos:definition xml:lang="en">The Western Australian Marine Science Institution (WAMSI) is an Australian marine research organisation, and is a collaboration between State, Federal, industry and academic entities.</skos:definition>
	<dc:source rdf:datatype="http://www.w3.org/2001/XMLSchema#string">Australian Ocean Data Network Organisation Register</dc:source>
	<dc:publisher rdf:datatype="http://www.w3.org/2001/XMLSchema#string">eMarine Information Infrastructure (eMII)</dc:publisher>
	<skos:exactMatch rdf:resource="http://seadatanet.maris2.nl/v_edmo/print.asp?n_code=4122"/>
	<skos:topConceptOf rdf:resource="http://vocab.aodn.org.au/def/organisation/1"/>
	<skos:inScheme rdf:resource="http://vocab.aodn.org.au/def/organisation/1"/>
</rdf:Description>

<rdf:Description rdf:about="http://vocab.aodn.org.au/def/organisation/entity/130">
	<rdf:type rdf:resource="http://www.w3.org/2000/01/rdf-schema#Resource"/>
	<rdf:type rdf:resource="http://www.w3.org/2004/02/skos/core#Concept"/>
	<dcterms:modified rdf:datatype="http://www.w3.org/2001/XMLSchema#dateTime">2015-05-12T01:43:09Z</dcterms:modified>
	<dcterms:creator rdf:datatype="http://www.w3.org/2001/XMLSchema#string">Natalia Atkins</dcterms:creator>
	<dcterms:created rdf:datatype="http://www.w3.org/2001/XMLSchema#dateTime">2015-04-27T10:38:15Z</dcterms:created>
	<skos:broadMatch rdf:resource="http://vocab.aodn.org.au/def/organisation_classes/category/2"/>
	<skos:prefLabel xml:lang="en">Western Australian Museum (WAM)</skos:prefLabel>
	<skos:hiddenLabel xml:lang="en">WAM</skos:hiddenLabel>
	<skos:definition xml:lang="en">The Western Australian Museum is the state’s premier cultural organisation, housing WA’s scientific and cultural collection. It has six main sites: one in Perth, two in Fremantle (Maritime and Shipwreck Galleries), and one each in Albany, Geraldton, and Kalgoorlie-Boulder.</skos:definition>
	<dc:source rdf:datatype="http://www.w3.org/2001/XMLSchema#string">Australian Ocean Data Network Organisation Register</dc:source>
	<dc:publisher rdf:datatype="http://www.w3.org/2001/XMLSchema#string">eMarine Information Infrastructure (eMII)</dc:publisher>
	<skos:exactMatch rdf:resource="http://seadatanet.maris2.nl/v_edmo/print.asp?n_code=3969"/>
	<skos:topConceptOf rdf:resource="http://vocab.aodn.org.au/def/organisation/1"/>
	<skos:inScheme rdf:resource="http://vocab.aodn.org.au/def/organisation/1"/>
</rdf:Description>

<rdf:Description rdf:about="http://vocab.aodn.org.au/def/organisation/entity/131">
	<rdf:type rdf:resource="http://www.w3.org/2000/01/rdf-schema#Resource"/>
	<rdf:type rdf:resource="http://www.w3.org/2004/02/skos/core#Concept"/>
	<dcterms:modified rdf:datatype="http://www.w3.org/2001/XMLSchema#dateTime">2015-05-12T01:43:16Z</dcterms:modified>
	<dcterms:creator rdf:datatype="http://www.w3.org/2001/XMLSchema#string">Natalia Atkins</dcterms:creator>
	<dcterms:created rdf:datatype="http://www.w3.org/2001/XMLSchema#dateTime">2015-04-27T10:38:15Z</dcterms:created>
	<skos:broadMatch rdf:resource="http://vocab.aodn.org.au/def/organisation_classes/category/5"/>
	<skos:prefLabel xml:lang="en">Woodside Energy Ltd</skos:prefLabel>
	<skos:definition xml:lang="en">Woodside is Australia’s largest independent oil and gas company.</skos:definition>
	<dc:source rdf:datatype="http://www.w3.org/2001/XMLSchema#string">Australian Ocean Data Network Organisation Register</dc:source>
	<dc:publisher rdf:datatype="http://www.w3.org/2001/XMLSchema#string">eMarine Information Infrastructure (eMII)</dc:publisher>
	<skos:exactMatch rdf:resource="http://seadatanet.maris2.nl/v_edmo/print.asp?n_code=3963"/>
	<skos:topConceptOf rdf:resource="http://vocab.aodn.org.au/def/organisation/1"/>
	<skos:inScheme rdf:resource="http://vocab.aodn.org.au/def/organisation/1"/>
</rdf:Description>

<rdf:Description rdf:about="http://vocab.aodn.org.au/def/organisation/entity/132">
	<rdf:type rdf:resource="http://www.w3.org/2000/01/rdf-schema#Resource"/>
	<rdf:type rdf:resource="http://www.w3.org/2004/02/skos/core#Concept"/>
	<dcterms:modified rdf:datatype="http://www.w3.org/2001/XMLSchema#dateTime">2015-05-12T01:43:22Z</dcterms:modified>
	<dcterms:creator rdf:datatype="http://www.w3.org/2001/XMLSchema#string">Natalia Atkins</dcterms:creator>
	<dcterms:created rdf:datatype="http://www.w3.org/2001/XMLSchema#dateTime">2015-04-27T10:38:15Z</dcterms:created>
	<skos:broadMatch rdf:resource="http://vocab.aodn.org.au/def/organisation_classes/category/5"/>
	<skos:prefLabel xml:lang="en">Yara Pilbara Holdings Ltd (YPHL)</skos:prefLabel>
	<skos:hiddenLabel xml:lang="en">YPHL</skos:hiddenLabel>
	<skos:definition xml:lang="en">Yara produces fertilisers and crop nutrition programs.</skos:definition>
	<dc:source rdf:datatype="http://www.w3.org/2001/XMLSchema#string">Australian Ocean Data Network Organisation Register</dc:source>
	<dc:publisher rdf:datatype="http://www.w3.org/2001/XMLSchema#string">eMarine Information Infrastructure (eMII)</dc:publisher>
	<skos:exactMatch rdf:resource="http://seadatanet.maris2.nl/v_edmo/print.asp?n_code=4123"/>
	<skos:topConceptOf rdf:resource="http://vocab.aodn.org.au/def/organisation/1"/>
	<skos:inScheme rdf:resource="http://vocab.aodn.org.au/def/organisation/1"/>
</rdf:Description>

<rdf:Description rdf:about="http://vocab.aodn.org.au/def/organisation/entity/133">
	<rdf:type rdf:resource="http://www.w3.org/2000/01/rdf-schema#Resource"/>
	<rdf:type rdf:resource="http://www.w3.org/2004/02/skos/core#Concept"/>
	<dcterms:modified rdf:datatype="http://www.w3.org/2001/XMLSchema#dateTime">2015-05-12T01:25:45Z</dcterms:modified>
	<dcterms:creator rdf:datatype="http://www.w3.org/2001/XMLSchema#string">Natalia Atkins</dcterms:creator>
	<dcterms:created rdf:datatype="http://www.w3.org/2001/XMLSchema#dateTime">2015-04-27T10:38:15Z</dcterms:created>
	<skos:broadMatch rdf:resource="http://vocab.aodn.org.au/def/organisation_classes/category/1"/>
	<skos:prefLabel xml:lang="en">Integrated Marine Observing System (IMOS)</skos:prefLabel>
	<skos:hiddenLabel xml:lang="en">IMOS</skos:hiddenLabel>
	<skos:definition xml:lang="en">IMOS routinely operates a wide range of observing equipment throughout Australia’s coastal and open oceans, making all of its data accessible to the marine and climate science community, other stakeholders and users, and international collaborators. IMOS is designed to be a fully-integrated, national system, observing at ocean-basin and regional scales, and covering physical, chemical and biological variables. IMOS is a national collaborative research infrastructure, supported by Australian Government. It is led by University of Tasmania in partnership with the Australian marine and climate science community.</skos:definition>
	<dc:source rdf:datatype="http://www.w3.org/2001/XMLSchema#string">Australian Ocean Data Network Organisation Register</dc:source>
	<dc:publisher rdf:datatype="http://www.w3.org/2001/XMLSchema#string">eMarine Information Infrastructure (eMII)</dc:publisher>
	<skos:exactMatch rdf:resource="http://seadatanet.maris2.nl/v_edmo/print.asp?n_code=3973"/>
	<skos:narrower rdf:resource="http://vocab.aodn.org.au/def/organisation/entity/134"/>
	<skos:narrower rdf:resource="http://vocab.aodn.org.au/def/organisation/entity/135"/>
	<skos:narrower rdf:resource="http://vocab.aodn.org.au/def/organisation/entity/136"/>
	<skos:narrower rdf:resource="http://vocab.aodn.org.au/def/organisation/entity/145"/>
	<skos:narrower rdf:resource="http://vocab.aodn.org.au/def/organisation/entity/149"/>
	<skos:narrower rdf:resource="http://vocab.aodn.org.au/def/organisation/entity/150"/>
	<skos:narrower rdf:resource="http://vocab.aodn.org.au/def/organisation/entity/151"/>
	<skos:narrower rdf:resource="http://vocab.aodn.org.au/def/organisation/entity/159"/>
	<skos:narrower rdf:resource="http://vocab.aodn.org.au/def/organisation/entity/160"/>
	<skos:narrower rdf:resource="http://vocab.aodn.org.au/def/organisation/entity/161"/>
	<skos:narrower rdf:resource="http://vocab.aodn.org.au/def/organisation/entity/162"/>
	<skos:topConceptOf rdf:resource="http://vocab.aodn.org.au/def/organisation/1"/>
	<skos:inScheme rdf:resource="http://vocab.aodn.org.au/def/organisation/1"/>
</rdf:Description>

<rdf:Description rdf:about="http://vocab.aodn.org.au/def/organisation/entity/168">
	<rdf:type rdf:resource="http://www.w3.org/2000/01/rdf-schema#Resource"/>
	<rdf:type rdf:resource="http://www.w3.org/2004/02/skos/core#Concept"/>
	<dcterms:modified rdf:datatype="http://www.w3.org/2001/XMLSchema#dateTime">2015-05-12T01:01:24Z</dcterms:modified>
	<dcterms:creator rdf:datatype="http://www.w3.org/2001/XMLSchema#string">Kim_Finney</dcterms:creator>
	<dcterms:created rdf:datatype="http://www.w3.org/2001/XMLSchema#dateTime">2015-05-12T00:34:15Z</dcterms:created>
	<skos:broadMatch rdf:resource="http://vocab.aodn.org.au/def/organisation_classes/category/1"/>
	<skos:prefLabel xml:lang="en">Bureau of Rural Sciences (BRS), Australian Government</skos:prefLabel>
	<skos:altLabel xml:lang="en">Bureau of Rural Sciences (BRS)</skos:altLabel>
	<skos:hiddenLabel xml:lang="en">BRS</skos:hiddenLabel>
	<skos:definition xml:lang="en">The Bureau of Rural Sciences, was a scientific agency within the Department of Agriculture, Fisheries and Forestry, which existed between 1986 and 2010. It is now part of the Australian Bureau of Agricultural and Resource Economics and Sciences.</skos:definition>
	<dc:source rdf:datatype="http://www.w3.org/2001/XMLSchema#string">Australian Ocean Data Network Organisation Register</dc:source>
	<dc:publisher rdf:datatype="http://www.w3.org/2001/XMLSchema#string">eMarine Information Infrastructure (eMII)</dc:publisher>
	<skos:topConceptOf rdf:resource="http://vocab.aodn.org.au/def/organisation/1"/>
	<skos:inScheme rdf:resource="http://vocab.aodn.org.au/def/organisation/1"/>
	<skos:scopeNote xml:lang="en">This organisation no longer exists.</skos:scopeNote>
	<skos:scopeNote xml:lang="en">This organisation no longer exists. Replaced by ttp://vocab.aodn.org.au/def/organisation/entity/25</skos:scopeNote>
	<dcterms:isReplacedBy xml:lang="en">Australian Bureau of Agriculture and Resource Economics and Sciences (ABARES), Department of Agriculture, Australian Government</dcterms:isReplacedBy>
	<dcterms:isReplacedBy xml:lang="en">http://vocab.aodn.org.au/def/organisation/entity/25</dcterms:isReplacedBy>
</rdf:Description>

<rdf:Description rdf:about="http://vocab.aodn.org.au/def/organisation/entity/171">
	<rdf:type rdf:resource="http://www.w3.org/2000/01/rdf-schema#Resource"/>
	<rdf:type rdf:resource="http://www.w3.org/2004/02/skos/core#Concept"/>
	<dcterms:modified rdf:datatype="http://www.w3.org/2001/XMLSchema#dateTime">2015-06-24T03:15:46Z</dcterms:modified>
	<dcterms:creator rdf:datatype="http://www.w3.org/2001/XMLSchema#string">eMII_Finney.Kim</dcterms:creator>
	<dcterms:created rdf:datatype="http://www.w3.org/2001/XMLSchema#dateTime">2015-06-24T02:05:15Z</dcterms:created>
	<dcterms:contributor rdf:datatype="http://www.w3.org/2001/XMLSchema#string">eMII_Finney.Kim</dcterms:contributor>
	<skos:broadMatch rdf:resource="http://vocab.aodn.org.au/def/organisation_classes/category/2"/>
	<skos:prefLabel xml:lang="en">Department of Primary Industries and Fisheries, Tasmanian Government</skos:prefLabel>
	<skos:altLabel xml:lang="en">Department of Primary Industries and Fisheries</skos:altLabel>
	<skos:definition xml:lang="en">This former state department was merged with the Tasmanian Parks and Wildlife service, and the Government Analytical and Forensic Laboratories (GAFL) to create the Department of Primary Industries, Water and Environment (DPIPWE), in 1998. (Courtesy of Wikipedia)</skos:definition>
	<dc:source rdf:datatype="http://www.w3.org/2001/XMLSchema#string">Australian Ocean Data Network Organisation Register</dc:source>
	<dc:publisher rdf:datatype="http://www.w3.org/2001/XMLSchema#string">eMarine Information Infrastructure (eMII)</dc:publisher>
	<skos:topConceptOf rdf:resource="http://vocab.aodn.org.au/def/organisation/1"/>
	<skos:inScheme rdf:resource="http://vocab.aodn.org.au/def/organisation/1"/>
	<skos:scopeNote xml:lang="en">organisation no longer exists</skos:scopeNote>
	<skos:scopeNote xml:lang="en">organisation no longer exists. Replaced by http://vocab.aodn.org.au/def/organisation/entity/56</skos:scopeNote>
	<dcterms:isReplacedBy xml:lang="en">Department of Primary Industries, Parks, Water and Environment (DPIPWE), Tasmanian Government</dcterms:isReplacedBy>
	<dcterms:isReplacedBy xml:lang="en">http://vocab.aodn.org.au/def/organisation/entity/56</dcterms:isReplacedBy>
</rdf:Description>

<rdf:Description rdf:about="http://vocab.aodn.org.au/def/organisation/entity/173">
	<rdf:type rdf:resource="http://www.w3.org/2000/01/rdf-schema#Resource"/>
	<rdf:type rdf:resource="http://www.w3.org/2004/02/skos/core#Concept"/>
	<dcterms:modified rdf:datatype="http://www.w3.org/2001/XMLSchema#dateTime">2015-06-24T03:11:06Z</dcterms:modified>
	<dcterms:creator rdf:datatype="http://www.w3.org/2001/XMLSchema#string">Natalia Atkins</dcterms:creator>
	<dcterms:created rdf:datatype="http://www.w3.org/2001/XMLSchema#dateTime">2015-06-24T10:38:15Z</dcterms:created>
	<dcterms:contributor rdf:datatype="http://www.w3.org/2001/XMLSchema#string">eMII_Finney.Kim</dcterms:contributor>
	<skos:broadMatch rdf:resource="http://vocab.aodn.org.au/def/organisation_classes/category/5"/>
	<skos:prefLabel xml:lang="en">Des Mills Marine Environmental Reviews</skos:prefLabel>
	<skos:altLabel xml:lang="en"></skos:altLabel>
	<skos:hiddenLabel xml:lang="en"></skos:hiddenLabel>
	<skos:definition xml:lang="en">Des Mills Marine Environmental Reviews is a private consultancy company.</skos:definition>
	<dc:source rdf:datatype="http://www.w3.org/2001/XMLSchema#string">Australian Ocean Data Network Organisation Register</dc:source>
	<dc:publisher rdf:datatype="http://www.w3.org/2001/XMLSchema#string">eMarine Information Infrastructure (eMMI)</dc:publisher>
	<skos:exactMatch rdf:resource="http://seadatanet.maris2.nl/v_edmo/print.asp?n_code=4187"/>
	<skos:topConceptOf rdf:resource="http://vocab.aodn.org.au/def/organisation/1"/>
	<skos:inScheme rdf:resource="http://vocab.aodn.org.au/def/organisation/1"/>
</rdf:Description>

<rdf:Description rdf:about="http://vocab.aodn.org.au/def/organisation/entity/174">
	<rdf:type rdf:resource="http://www.w3.org/2000/01/rdf-schema#Resource"/>
	<rdf:type rdf:resource="http://www.w3.org/2004/02/skos/core#Concept"/>
	<dcterms:modified rdf:datatype="http://www.w3.org/2001/XMLSchema#dateTime">2015-06-24T03:11:24Z</dcterms:modified>
	<dcterms:creator rdf:datatype="http://www.w3.org/2001/XMLSchema#string">Natalia Atkins</dcterms:creator>
	<dcterms:created rdf:datatype="http://www.w3.org/2001/XMLSchema#dateTime">2015-06-24T10:38:15Z</dcterms:created>
	<dcterms:contributor rdf:datatype="http://www.w3.org/2001/XMLSchema#string">eMII_Finney.Kim</dcterms:contributor>
	<skos:broadMatch rdf:resource="http://vocab.aodn.org.au/def/organisation_classes/category/5"/>
	<skos:prefLabel xml:lang="en">Seashore Engineering Pty Ltd</skos:prefLabel>
	<skos:altLabel xml:lang="en"></skos:altLabel>
	<skos:hiddenLabel xml:lang="en"></skos:hiddenLabel>
	<skos:definition xml:lang="en">Seashore Engineering Pty Ltd delivers high quality coastal and maritime engineering services.</skos:definition>
	<dc:source rdf:datatype="http://www.w3.org/2001/XMLSchema#string">Australian Ocean Data Network Organisation Register</dc:source>
	<dc:publisher rdf:datatype="http://www.w3.org/2001/XMLSchema#string">eMarine Information Infrastructure (eMMI)</dc:publisher>
	<skos:exactMatch rdf:resource="http://seadatanet.maris2.nl/v_edmo/print.asp?n_code=4188"/>
	<skos:topConceptOf rdf:resource="http://vocab.aodn.org.au/def/organisation/1"/>
	<skos:inScheme rdf:resource="http://vocab.aodn.org.au/def/organisation/1"/>
</rdf:Description>

<rdf:Description rdf:about="http://vocab.aodn.org.au/def/organisation/entity/175">
	<rdf:type rdf:resource="http://www.w3.org/2000/01/rdf-schema#Resource"/>
	<rdf:type rdf:resource="http://www.w3.org/2004/02/skos/core#Concept"/>
	<dcterms:modified rdf:datatype="http://www.w3.org/2001/XMLSchema#dateTime">2015-06-24T03:11:49Z</dcterms:modified>
	<dcterms:creator rdf:datatype="http://www.w3.org/2001/XMLSchema#string">Natalia Atkins</dcterms:creator>
	<dcterms:created rdf:datatype="http://www.w3.org/2001/XMLSchema#dateTime">2015-06-24T10:38:15Z</dcterms:created>
	<dcterms:contributor rdf:datatype="http://www.w3.org/2001/XMLSchema#string">eMII_Finney.Kim</dcterms:contributor>
	<skos:broadMatch rdf:resource="http://vocab.aodn.org.au/def/organisation_classes/category/5"/>
	<skos:prefLabel xml:lang="en">Eni Australia Ltd</skos:prefLabel>
	<skos:altLabel xml:lang="en"></skos:altLabel>
	<skos:hiddenLabel xml:lang="en"></skos:hiddenLabel>
	<skos:definition xml:lang="en">Eni is an integrated energy company, which is headquartered in Rome.</skos:definition>
	<dc:source rdf:datatype="http://www.w3.org/2001/XMLSchema#string">Australian Ocean Data Network Organisation Register</dc:source>
	<dc:publisher rdf:datatype="http://www.w3.org/2001/XMLSchema#string">eMarine Information Infrastructure (eMMI)</dc:publisher>
	<skos:exactMatch rdf:resource="http://seadatanet.maris2.nl/v_edmo/print.asp?n_code=4189"/>
	<skos:topConceptOf rdf:resource="http://vocab.aodn.org.au/def/organisation/1"/>
	<skos:inScheme rdf:resource="http://vocab.aodn.org.au/def/organisation/1"/>
</rdf:Description>

<rdf:Description rdf:about="http://vocab.aodn.org.au/def/organisation/entity/176">
	<rdf:type rdf:resource="http://www.w3.org/2000/01/rdf-schema#Resource"/>
	<rdf:type rdf:resource="http://www.w3.org/2004/02/skos/core#Concept"/>
	<dcterms:modified rdf:datatype="http://www.w3.org/2001/XMLSchema#dateTime">2015-06-24T03:12:15Z</dcterms:modified>
	<dcterms:creator rdf:datatype="http://www.w3.org/2001/XMLSchema#string">Natalia Atkins</dcterms:creator>
	<dcterms:created rdf:datatype="http://www.w3.org/2001/XMLSchema#dateTime">2015-06-24T10:38:15Z</dcterms:created>
	<dcterms:contributor rdf:datatype="http://www.w3.org/2001/XMLSchema#string">eMII_Finney.Kim</dcterms:contributor>
	<skos:broadMatch rdf:resource="http://vocab.aodn.org.au/def/organisation_classes/category/5"/>
	<skos:prefLabel xml:lang="en">Ningaloo Marine Interactions</skos:prefLabel>
	<skos:altLabel xml:lang="en"></skos:altLabel>
	<skos:hiddenLabel xml:lang="en"></skos:hiddenLabel>
	<skos:definition xml:lang="en">Ningaloo Marine Interactions have been operating tours out of Coral Bay since 2011.</skos:definition>
	<dc:source rdf:datatype="http://www.w3.org/2001/XMLSchema#string">Australian Ocean Data Network Organisation Register</dc:source>
	<dc:publisher rdf:datatype="http://www.w3.org/2001/XMLSchema#string">eMarine Information Infrastructure (eMMI)</dc:publisher>
	<skos:exactMatch rdf:resource="http://seadatanet.maris2.nl/v_edmo/print.asp?n_code=4190"/>
	<skos:topConceptOf rdf:resource="http://vocab.aodn.org.au/def/organisation/1"/>
	<skos:inScheme rdf:resource="http://vocab.aodn.org.au/def/organisation/1"/>
</rdf:Description>

<rdf:Description rdf:about="http://vocab.aodn.org.au/def/organisation/entity/177">
	<rdf:type rdf:resource="http://www.w3.org/2000/01/rdf-schema#Resource"/>
	<rdf:type rdf:resource="http://www.w3.org/2004/02/skos/core#Concept"/>
	<dcterms:modified rdf:datatype="http://www.w3.org/2001/XMLSchema#dateTime">2015-06-24T03:12:32Z</dcterms:modified>
	<dcterms:creator rdf:datatype="http://www.w3.org/2001/XMLSchema#string">Natalia Atkins</dcterms:creator>
	<dcterms:created rdf:datatype="http://www.w3.org/2001/XMLSchema#dateTime">2015-06-24T10:38:15Z</dcterms:created>
	<dcterms:contributor rdf:datatype="http://www.w3.org/2001/XMLSchema#string">eMII_Finney.Kim</dcterms:contributor>
	<skos:broadMatch rdf:resource="http://vocab.aodn.org.au/def/organisation_classes/category/2"/>
	<skos:prefLabel xml:lang="en">Landgate's Satellite Remote Sensing Services (SRSS), Western Australian Government</skos:prefLabel>
	<skos:altLabel xml:lang="en">Landgate's Satellite Remote Sensing Services (SRSS)</skos:altLabel>
	<skos:hiddenLabel xml:lang="en">SRSS</skos:hiddenLabel>
	<skos:definition xml:lang="en">Landgate's Satellite Remote Sensing Services (SRSS) is a dedicated remote sensing facility. They provide a full range of remote sensing services – from direct acquisition of satellite data, to processing of data and then delivering that data to government and business via our products and services.</skos:definition>
	<dc:source rdf:datatype="http://www.w3.org/2001/XMLSchema#string">Australian Ocean Data Network Organisation Register</dc:source>
	<dc:publisher rdf:datatype="http://www.w3.org/2001/XMLSchema#string">eMarine Information Infrastructure (eMMI)</dc:publisher>
	<skos:exactMatch rdf:resource="http://seadatanet.maris2.nl/v_edmo/print.asp?n_code=4191"/>
	<skos:topConceptOf rdf:resource="http://vocab.aodn.org.au/def/organisation/1"/>
	<skos:inScheme rdf:resource="http://vocab.aodn.org.au/def/organisation/1"/>
</rdf:Description>

<rdf:Description rdf:about="http://vocab.aodn.org.au/def/organisation/entity/172">
	<rdf:type rdf:resource="http://www.w3.org/2000/01/rdf-schema#Resource"/>
	<rdf:type rdf:resource="http://www.w3.org/2004/02/skos/core#Concept"/>
	<dcterms:modified rdf:datatype="http://www.w3.org/2001/XMLSchema#dateTime">2015-06-24T03:10:10Z</dcterms:modified>
	<dcterms:creator rdf:datatype="http://www.w3.org/2001/XMLSchema#string">Natalia Atkins</dcterms:creator>
	<dcterms:created rdf:datatype="http://www.w3.org/2001/XMLSchema#dateTime">2015-06-24T10:38:15Z</dcterms:created>
	<dcterms:contributor rdf:datatype="http://www.w3.org/2001/XMLSchema#string">eMII_Finney.Kim</dcterms:contributor>
	<skos:broadMatch rdf:resource="http://vocab.aodn.org.au/def/organisation_classes/category/5"/>
	<skos:prefLabel xml:lang="en">Hydroweb Pty Ltd</skos:prefLabel>
	<skos:altLabel xml:lang="en"></skos:altLabel>
	<skos:hiddenLabel xml:lang="en"></skos:hiddenLabel>
	<skos:definition xml:lang="en">Hydroweb Pty Ltd is a private consultancy company</skos:definition>
	<dc:source rdf:datatype="http://www.w3.org/2001/XMLSchema#string">Australian Ocean Data Network Organisation Register</dc:source>
	<dc:publisher rdf:datatype="http://www.w3.org/2001/XMLSchema#string">eMarine Information Infrastructure (eMMI)</dc:publisher>
	<skos:exactMatch rdf:resource="http://seadatanet.maris2.nl/v_edmo/print.asp?n_code=4186"/>
	<skos:topConceptOf rdf:resource="http://vocab.aodn.org.au/def/organisation/1"/>
	<skos:inScheme rdf:resource="http://vocab.aodn.org.au/def/organisation/1"/>
</rdf:Description>

<rdf:Description rdf:about="http://vocab.aodn.org.au/def/organisation/entity/178">
	<rdf:type rdf:resource="http://www.w3.org/2000/01/rdf-schema#Resource"/>
	<rdf:type rdf:resource="http://www.w3.org/2004/02/skos/core#Concept"/>
	<dcterms:creator rdf:datatype="http://www.w3.org/2001/XMLSchema#string">Natalia Atkins</dcterms:creator>
	<dcterms:created rdf:datatype="http://www.w3.org/2001/XMLSchema#dateTime">2015-07-08T10:38:15Z</dcterms:created>
	<skos:broadMatch rdf:resource="http://vocab.aodn.org.au/def/organisation_classes/category/3"/>
	<skos:prefLabel xml:lang="en">Curtin University</skos:prefLabel>
	<skos:altLabel xml:lang="en"></skos:altLabel>
	<skos:hiddenLabel xml:lang="en"></skos:hiddenLabel>
	<skos:definition xml:lang="en">Curtin University is based in Bentley, Perth, Western Australia. It was previously known as the Curtin University of Technology from 1987 until 2010. It also has campuses in Sydney, Malaysia and Singapore.</skos:definition>
	<dc:source rdf:datatype="http://www.w3.org/2001/XMLSchema#string">Australian Ocean Data Network Organisation Register</dc:source>
	<dc:publisher rdf:datatype="http://www.w3.org/2001/XMLSchema#string">eMarine Information Infrastructure (eMII)</dc:publisher>
	<skos:exactMatch rdf:resource="http://seadatanet.maris2.nl/v_edmo/print.asp?n_code=4027"/>
	<skos:narrower rdf:resource="http://vocab.aodn.org.au/def/organisation/entity/180"/>
	<skos:narrower rdf:resource="http://vocab.aodn.org.au/def/organisation/entity/181"/>
	<skos:narrower rdf:resource="http://vocab.aodn.org.au/def/organisation/entity/182"/>
	<skos:narrower rdf:resource="http://vocab.aodn.org.au/def/organisation/entity/183"/>
	<skos:narrower rdf:resource="http://vocab.aodn.org.au/def/organisation/entity/184"/>
	<skos:narrower rdf:resource="http://vocab.aodn.org.au/def/organisation/entity/185"/>
	<skos:narrower rdf:resource="http://vocab.aodn.org.au/def/organisation/entity/186"/>
	<skos:narrower rdf:resource="http://vocab.aodn.org.au/def/organisation/entity/187"/>
	<skos:narrower rdf:resource="http://vocab.aodn.org.au/def/organisation/entity/188"/>
	<skos:narrower rdf:resource="http://vocab.aodn.org.au/def/organisation/entity/179"/>
	<skos:topConceptOf rdf:resource="http://vocab.aodn.org.au/def/organisation/1"/>
	<skos:inScheme rdf:resource="http://vocab.aodn.org.au/def/organisation/1"/>
</rdf:Description>

<rdf:Description rdf:about="http://vocab.aodn.org.au/def/organisation/entity/189">
	<rdf:type rdf:resource="http://www.w3.org/2000/01/rdf-schema#Resource"/>
	<rdf:type rdf:resource="http://www.w3.org/2004/02/skos/core#Concept"/>
	<dcterms:creator rdf:datatype="http://www.w3.org/2001/XMLSchema#string">Natalia Atkins</dcterms:creator>
	<dcterms:created rdf:datatype="http://www.w3.org/2001/XMLSchema#dateTime">2015-07-08T10:38:15Z</dcterms:created>
	<skos:broadMatch rdf:resource="http://vocab.aodn.org.au/def/organisation_classes/category/3"/>
	<skos:prefLabel xml:lang="en">Flinders University</skos:prefLabel>
	<skos:altLabel xml:lang="en"></skos:altLabel>
	<skos:hiddenLabel xml:lang="en"></skos:hiddenLabel>
	<skos:definition xml:lang="en">Flinders University is in Adelaide, South Australia, and was founded in 1966. The University's main campus is in the Adelaide suburb of Bedford Par. It is also located in Victoria Square in the centre of the Adelaide, and is situated at numerous other locations in regional South Australia, south-west Victoria and the Northern Territory.</skos:definition>
	<dc:source rdf:datatype="http://www.w3.org/2001/XMLSchema#string">Australian Ocean Data Network Organisation Register</dc:source>
	<dc:publisher rdf:datatype="http://www.w3.org/2001/XMLSchema#string">eMarine Information Infrastructure (eMII)</dc:publisher>
	<skos:exactMatch rdf:resource="http://seadatanet.maris2.nl/v_edmo/print.asp?n_code=4266"/>
	<skos:narrower rdf:resource="http://vocab.aodn.org.au/def/organisation/entity/190"/>
	<skos:narrower rdf:resource="http://vocab.aodn.org.au/def/organisation/entity/191"/>
	<skos:narrower rdf:resource="http://vocab.aodn.org.au/def/organisation/entity/192"/>
	<skos:narrower rdf:resource="http://vocab.aodn.org.au/def/organisation/entity/193"/>
	<skos:narrower rdf:resource="http://vocab.aodn.org.au/def/organisation/entity/410"/>
	<skos:topConceptOf rdf:resource="http://vocab.aodn.org.au/def/organisation/1"/>
	<skos:inScheme rdf:resource="http://vocab.aodn.org.au/def/organisation/1"/>
</rdf:Description>

<rdf:Description rdf:about="http://vocab.aodn.org.au/def/organisation/entity/194">
	<rdf:type rdf:resource="http://www.w3.org/2000/01/rdf-schema#Resource"/>
	<rdf:type rdf:resource="http://www.w3.org/2004/02/skos/core#Concept"/>
	<dcterms:modified rdf:datatype="http://www.w3.org/2001/XMLSchema#dateTime">2015-07-14T00:13:54Z</dcterms:modified>
	<dcterms:creator rdf:datatype="http://www.w3.org/2001/XMLSchema#string">Natalia Atkins</dcterms:creator>
	<dcterms:created rdf:datatype="http://www.w3.org/2001/XMLSchema#dateTime">2015-07-09T10:38:15Z</dcterms:created>
	<dcterms:contributor rdf:datatype="http://www.w3.org/2001/XMLSchema#string">Natalia_Atkins</dcterms:contributor>
	<skos:broadMatch rdf:resource="http://vocab.aodn.org.au/def/organisation_classes/category/3"/>
	<skos:prefLabel xml:lang="en">The Australian National University (ANU)</skos:prefLabel>
	<skos:altLabel xml:lang="en"></skos:altLabel>
	<skos:hiddenLabel xml:lang="en">ANU</skos:hiddenLabel>
	<skos:definition xml:lang="en">The Australian National University (ANU) is a university in Canberra, Australian Capital Territory, which is located in the suburb of Acton. ANU occupies additional locations including Mount Stromlo Observatory on the outskirts of Canberra, Siding Spring Observatory near Coonabarabran, a campus at Kioloa on the South Coast of New South Wales and a research unit in Darwin.</skos:definition>
	<dc:source rdf:datatype="http://www.w3.org/2001/XMLSchema#string">Australian Ocean Data Network Organisation Register</dc:source>
	<dc:publisher rdf:datatype="http://www.w3.org/2001/XMLSchema#string">eMarine Information Infrastructure (eMII)</dc:publisher>
	<skos:exactMatch rdf:resource="http://seadatanet.maris2.nl/v_edmo/print.asp?n_code=4287"/>
	<skos:narrower rdf:resource="http://vocab.aodn.org.au/def/organisation/entity/195"/>
	<skos:narrower rdf:resource="http://vocab.aodn.org.au/def/organisation/entity/196"/>
	<skos:narrower rdf:resource="http://vocab.aodn.org.au/def/organisation/entity/197"/>
	<skos:narrower rdf:resource="http://vocab.aodn.org.au/def/organisation/entity/198"/>
	<skos:narrower rdf:resource="http://vocab.aodn.org.au/def/organisation/entity/199"/>
	<skos:narrower rdf:resource="http://vocab.aodn.org.au/def/organisation/entity/200"/>
	<skos:narrower rdf:resource="http://vocab.aodn.org.au/def/organisation/entity/201"/>
	<skos:narrower rdf:resource="http://vocab.aodn.org.au/def/organisation/entity/202"/>
	<skos:narrower rdf:resource="http://vocab.aodn.org.au/def/organisation/entity/203"/>
	<skos:narrower rdf:resource="http://vocab.aodn.org.au/def/organisation/entity/204"/>
	<skos:narrower rdf:resource="http://vocab.aodn.org.au/def/organisation/entity/205"/>
	<skos:narrower rdf:resource="http://vocab.aodn.org.au/def/organisation/entity/206"/>
	<skos:narrower rdf:resource="http://vocab.aodn.org.au/def/organisation/entity/207"/>
	<skos:narrower rdf:resource="http://vocab.aodn.org.au/def/organisation/entity/209"/>
	<skos:topConceptOf rdf:resource="http://vocab.aodn.org.au/def/organisation/1"/>
	<skos:inScheme rdf:resource="http://vocab.aodn.org.au/def/organisation/1"/>
</rdf:Description>

<rdf:Description rdf:about="http://vocab.aodn.org.au/def/organisation/entity/210">
	<rdf:type rdf:resource="http://www.w3.org/2000/01/rdf-schema#Resource"/>
	<rdf:type rdf:resource="http://www.w3.org/2004/02/skos/core#Concept"/>
	<dcterms:creator rdf:datatype="http://www.w3.org/2001/XMLSchema#string">Natalia Atkins</dcterms:creator>
	<dcterms:created rdf:datatype="http://www.w3.org/2001/XMLSchema#dateTime">2015-07-09T10:38:15Z</dcterms:created>
	<skos:broadMatch rdf:resource="http://vocab.aodn.org.au/def/organisation_classes/category/3"/>
	<skos:prefLabel xml:lang="en">The University of New South Wales (UNSW)</skos:prefLabel>
	<skos:altLabel xml:lang="en"></skos:altLabel>
	<skos:hiddenLabel xml:lang="en">UNSW</skos:hiddenLabel>
	<skos:definition xml:lang="en">The University of New South Wales (UNSW) is an Australian university that was established in 1949. The main UNSW campus is located at Kensington, Sydney. Other campuses are the College of Fine Arts in Paddington; UNSW@ADFA, the University College at the Australian Defence Force Academy in Canberra; and sub-campuses at Randwick and Coogee in Sydney, as well as research institutes around New South Wales.</skos:definition>
	<dc:source rdf:datatype="http://www.w3.org/2001/XMLSchema#string">Australian Ocean Data Network Organisation Register</dc:source>
	<dc:publisher rdf:datatype="http://www.w3.org/2001/XMLSchema#string">eMarine Information Infrastructure (eMII)</dc:publisher>
	<skos:exactMatch rdf:resource="http://seadatanet.maris2.nl/v_edmo/print.asp?n_code=4294"/>
	<skos:narrower rdf:resource="http://vocab.aodn.org.au/def/organisation/entity/211"/>
	<skos:narrower rdf:resource="http://vocab.aodn.org.au/def/organisation/entity/212"/>
	<skos:narrower rdf:resource="http://vocab.aodn.org.au/def/organisation/entity/213"/>
	<skos:narrower rdf:resource="http://vocab.aodn.org.au/def/organisation/entity/214"/>
	<skos:topConceptOf rdf:resource="http://vocab.aodn.org.au/def/organisation/1"/>
	<skos:inScheme rdf:resource="http://vocab.aodn.org.au/def/organisation/1"/>
</rdf:Description>

<rdf:Description rdf:about="http://vocab.aodn.org.au/def/organisation/entity/215">
	<rdf:type rdf:resource="http://www.w3.org/2000/01/rdf-schema#Resource"/>
	<rdf:type rdf:resource="http://www.w3.org/2004/02/skos/core#Concept"/>
	<dcterms:creator rdf:datatype="http://www.w3.org/2001/XMLSchema#string">Natalia Atkins</dcterms:creator>
	<dcterms:created rdf:datatype="http://www.w3.org/2001/XMLSchema#dateTime">2015-07-09T10:38:15Z</dcterms:created>
	<skos:broadMatch rdf:resource="http://vocab.aodn.org.au/def/organisation_classes/category/3"/>
	<skos:prefLabel xml:lang="en">The University of Newcastle (UON)</skos:prefLabel>
	<skos:altLabel xml:lang="en"></skos:altLabel>
	<skos:hiddenLabel xml:lang="en">UON</skos:hiddenLabel>
	<skos:definition xml:lang="en">The University of Newcastle has three main campuses and a key prescence in Singapore, Sydney and in five regional centres in Australia.</skos:definition>
	<dc:source rdf:datatype="http://www.w3.org/2001/XMLSchema#string">Australian Ocean Data Network Organisation Register</dc:source>
	<dc:publisher rdf:datatype="http://www.w3.org/2001/XMLSchema#string">eMarine Information Infrastructure (eMII)</dc:publisher>
	<skos:exactMatch rdf:resource="http://seadatanet.maris2.nl/v_edmo/print.asp?n_code=4297"/>
	<skos:narrower rdf:resource="http://vocab.aodn.org.au/def/organisation/entity/216"/>
	<skos:topConceptOf rdf:resource="http://vocab.aodn.org.au/def/organisation/1"/>
	<skos:inScheme rdf:resource="http://vocab.aodn.org.au/def/organisation/1"/>
</rdf:Description>

<rdf:Description rdf:about="http://vocab.aodn.org.au/def/organisation/entity/217">
	<rdf:type rdf:resource="http://www.w3.org/2000/01/rdf-schema#Resource"/>
	<rdf:type rdf:resource="http://www.w3.org/2004/02/skos/core#Concept"/>
	<dcterms:modified rdf:datatype="http://www.w3.org/2001/XMLSchema#dateTime">2015-07-28T06:07:34Z</dcterms:modified>
	<dcterms:creator rdf:datatype="http://www.w3.org/2001/XMLSchema#string">Natalia Atkins</dcterms:creator>
	<dcterms:created rdf:datatype="http://www.w3.org/2001/XMLSchema#dateTime">2015-07-10T10:38:15Z</dcterms:created>
	<dcterms:contributor rdf:datatype="http://www.w3.org/2001/XMLSchema#string">Natalia_Atkins</dcterms:contributor>
	<skos:broadMatch rdf:resource="http://vocab.aodn.org.au/def/organisation_classes/category/3"/>
	<skos:prefLabel xml:lang="en">The University of Queensland (UQ)</skos:prefLabel>
	<skos:altLabel xml:lang="en"></skos:altLabel>
	<skos:hiddenLabel xml:lang="en">UQ</skos:hiddenLabel>
	<skos:definition xml:lang="en"></skos:definition>
	<skos:definition xml:lang="en">The University of Queensland is an Australian university primarily located in Brisbane, Queensland, which was founded in 1909. The main campus is located in the suburb of St Lucia, southwest of the Brisbane City Central Business District, with other major UQ campuses in Gatton, and Herston.</skos:definition>
	<dc:source rdf:datatype="http://www.w3.org/2001/XMLSchema#string">Australian Ocean Data Network Organisation Register</dc:source>
	<dc:publisher rdf:datatype="http://www.w3.org/2001/XMLSchema#string">eMarine Information Infrastructure (eMII)</dc:publisher>
	<skos:exactMatch rdf:resource="http://seadatanet.maris2.nl/v_edmo/print.asp?n_code=3025"/>
	<skos:narrower rdf:resource="http://vocab.aodn.org.au/def/organisation/entity/218"/>
	<skos:narrower rdf:resource="http://vocab.aodn.org.au/def/organisation/entity/219"/>
	<skos:narrower rdf:resource="http://vocab.aodn.org.au/def/organisation/entity/220"/>
	<skos:narrower rdf:resource="http://vocab.aodn.org.au/def/organisation/entity/221"/>
	<skos:narrower rdf:resource="http://vocab.aodn.org.au/def/organisation/entity/222"/>
	<skos:narrower rdf:resource="http://vocab.aodn.org.au/def/organisation/entity/223"/>
	<skos:topConceptOf rdf:resource="http://vocab.aodn.org.au/def/organisation/1"/>
	<skos:inScheme rdf:resource="http://vocab.aodn.org.au/def/organisation/1"/>
</rdf:Description>

<rdf:Description rdf:about="http://vocab.aodn.org.au/def/organisation/entity/224">
	<rdf:type rdf:resource="http://www.w3.org/2000/01/rdf-schema#Resource"/>
	<rdf:type rdf:resource="http://www.w3.org/2004/02/skos/core#Concept"/>
	<dcterms:modified rdf:datatype="http://www.w3.org/2001/XMLSchema#dateTime">2015-07-14T01:56:51Z</dcterms:modified>
	<dcterms:creator rdf:datatype="http://www.w3.org/2001/XMLSchema#string">Natalia Atkins</dcterms:creator>
	<dcterms:created rdf:datatype="http://www.w3.org/2001/XMLSchema#dateTime">2015-07-10T10:38:15Z</dcterms:created>
	<dcterms:contributor rdf:datatype="http://www.w3.org/2001/XMLSchema#string">Natalia_Atkins</dcterms:contributor>
	<skos:broadMatch rdf:resource="http://vocab.aodn.org.au/def/organisation_classes/category/3"/>
	<skos:prefLabel xml:lang="en">The University of Sydney (USYD)</skos:prefLabel>
	<skos:altLabel xml:lang="en"></skos:altLabel>
	<skos:hiddenLabel xml:lang="en">USYD</skos:hiddenLabel>
	<skos:definition xml:lang="en">The University of Sydney, was founded in 1850. The University of Sydney has a network of teaching campuses spread throughout the Sydney area.</skos:definition>
	<dc:source rdf:datatype="http://www.w3.org/2001/XMLSchema#string">Australian Ocean Data Network Organisation Register</dc:source>
	<dc:publisher rdf:datatype="http://www.w3.org/2001/XMLSchema#string">eMarine Information Infrastructure (eMII)</dc:publisher>
	<skos:exactMatch rdf:resource="http://seadatanet.maris2.nl/v_edmo/print.asp?n_code=4303"/>
	<skos:narrower rdf:resource="http://vocab.aodn.org.au/def/organisation/entity/225"/>
	<skos:narrower rdf:resource="http://vocab.aodn.org.au/def/organisation/entity/226"/>
	<skos:narrower rdf:resource="http://vocab.aodn.org.au/def/organisation/entity/227"/>
	<skos:narrower rdf:resource="http://vocab.aodn.org.au/def/organisation/entity/228"/>
	<skos:narrower rdf:resource="http://vocab.aodn.org.au/def/organisation/entity/229"/>
	<skos:narrower rdf:resource="http://vocab.aodn.org.au/def/organisation/entity/231"/>
	<skos:narrower rdf:resource="http://vocab.aodn.org.au/def/organisation/entity/232"/>
	<skos:narrower rdf:resource="http://vocab.aodn.org.au/def/organisation/entity/233"/>
	<skos:narrower rdf:resource="http://vocab.aodn.org.au/def/organisation/entity/234"/>
	<skos:topConceptOf rdf:resource="http://vocab.aodn.org.au/def/organisation/1"/>
	<skos:inScheme rdf:resource="http://vocab.aodn.org.au/def/organisation/1"/>
</rdf:Description>

<rdf:Description rdf:about="http://vocab.aodn.org.au/def/organisation/entity/235">
	<rdf:type rdf:resource="http://www.w3.org/2000/01/rdf-schema#Resource"/>
	<rdf:type rdf:resource="http://www.w3.org/2004/02/skos/core#Concept"/>
	<dcterms:creator rdf:datatype="http://www.w3.org/2001/XMLSchema#string">Natalia Atkins</dcterms:creator>
	<dcterms:created rdf:datatype="http://www.w3.org/2001/XMLSchema#dateTime">2015-07-09T10:38:15Z</dcterms:created>
	<skos:broadMatch rdf:resource="http://vocab.aodn.org.au/def/organisation_classes/category/3"/>
	<skos:prefLabel xml:lang="en">The University of Western Australia (UWA)</skos:prefLabel>
	<skos:altLabel xml:lang="en"></skos:altLabel>
	<skos:hiddenLabel xml:lang="en">UWA</skos:hiddenLabel>
	<skos:definition xml:lang="en">The University of Western Australia (UWA) has its main campus in Perth, Australia, and was established in 1911. The university has smaller centres at Claremont and Albany.</skos:definition>
	<dc:source rdf:datatype="http://www.w3.org/2001/XMLSchema#string">Australian Ocean Data Network Organisation Register</dc:source>
	<dc:publisher rdf:datatype="http://www.w3.org/2001/XMLSchema#string">eMarine Information Infrastructure (eMII)</dc:publisher>
	<skos:exactMatch rdf:resource="http://seadatanet.maris2.nl/v_edmo/print.asp?n_code=4308"/>
	<skos:narrower rdf:resource="http://vocab.aodn.org.au/def/organisation/entity/236"/>
	<skos:narrower rdf:resource="http://vocab.aodn.org.au/def/organisation/entity/237"/>
	<skos:narrower rdf:resource="http://vocab.aodn.org.au/def/organisation/entity/238"/>
	<skos:narrower rdf:resource="http://vocab.aodn.org.au/def/organisation/entity/239"/>
	<skos:narrower rdf:resource="http://vocab.aodn.org.au/def/organisation/entity/240"/>
	<skos:narrower rdf:resource="http://vocab.aodn.org.au/def/organisation/entity/241"/>
	<skos:narrower rdf:resource="http://vocab.aodn.org.au/def/organisation/entity/242"/>
	<skos:narrower rdf:resource="http://vocab.aodn.org.au/def/organisation/entity/243"/>
	<skos:narrower rdf:resource="http://vocab.aodn.org.au/def/organisation/entity/244"/>
	<skos:narrower rdf:resource="http://vocab.aodn.org.au/def/organisation/entity/245"/>
	<skos:narrower rdf:resource="http://vocab.aodn.org.au/def/organisation/entity/246"/>
	<skos:narrower rdf:resource="http://vocab.aodn.org.au/def/organisation/entity/247"/>
	<skos:narrower rdf:resource="http://vocab.aodn.org.au/def/organisation/entity/248"/>
	<skos:narrower rdf:resource="http://vocab.aodn.org.au/def/organisation/entity/249"/>
	<skos:narrower rdf:resource="http://vocab.aodn.org.au/def/organisation/entity/250"/>
	<skos:narrower rdf:resource="http://vocab.aodn.org.au/def/organisation/entity/251"/>
	<skos:topConceptOf rdf:resource="http://vocab.aodn.org.au/def/organisation/1"/>
	<skos:inScheme rdf:resource="http://vocab.aodn.org.au/def/organisation/1"/>
</rdf:Description>

<rdf:Description rdf:about="http://vocab.aodn.org.au/def/organisation/entity/252">
	<rdf:type rdf:resource="http://www.w3.org/2000/01/rdf-schema#Resource"/>
	<rdf:type rdf:resource="http://www.w3.org/2004/02/skos/core#Concept"/>
	<dcterms:modified rdf:datatype="http://www.w3.org/2001/XMLSchema#dateTime">2015-07-15T02:46:01Z</dcterms:modified>
	<dcterms:creator rdf:datatype="http://www.w3.org/2001/XMLSchema#string">Natalia Atkins</dcterms:creator>
	<dcterms:created rdf:datatype="http://www.w3.org/2001/XMLSchema#dateTime">2015-07-13T10:38:15Z</dcterms:created>
	<dcterms:contributor rdf:datatype="http://www.w3.org/2001/XMLSchema#string">Natalia_Atkins</dcterms:contributor>
	<skos:broadMatch rdf:resource="http://vocab.aodn.org.au/def/organisation_classes/category/3"/>
	<skos:prefLabel xml:lang="en">University of Tasmania (UTAS)</skos:prefLabel>
	<skos:altLabel xml:lang="en"></skos:altLabel>
	<skos:hiddenLabel xml:lang="en">UTAS</skos:hiddenLabel>
	<skos:definition xml:lang="en">The University of Tasmania is an Australian university, which was founded in 1890. The University has three main campuses around Tasmania: Sandy Bay, Newnham and the Cradle Coast campuses, and numerous smaller campuses - mostly scattered around Hobart, but also including sites at Darlinghurst and Rozelle in Sydney.</skos:definition>
	<dc:source rdf:datatype="http://www.w3.org/2001/XMLSchema#string">Australian Ocean Data Network Organisation Register</dc:source>
	<dc:publisher rdf:datatype="http://www.w3.org/2001/XMLSchema#string">eMarine Information Infrastructure (eMII)</dc:publisher>
	<skos:exactMatch rdf:resource="http://seadatanet.maris2.nl/v_edmo/print.asp?n_code=4324"/>
	<skos:narrower rdf:resource="http://vocab.aodn.org.au/def/organisation/entity/253"/>
	<skos:narrower rdf:resource="http://vocab.aodn.org.au/def/organisation/entity/254"/>
	<skos:narrower rdf:resource="http://vocab.aodn.org.au/def/organisation/entity/255"/>
	<skos:narrower rdf:resource="http://vocab.aodn.org.au/def/organisation/entity/256"/>
	<skos:narrower rdf:resource="http://vocab.aodn.org.au/def/organisation/entity/257"/>
	<skos:narrower rdf:resource="http://vocab.aodn.org.au/def/organisation/entity/258"/>
	<skos:narrower rdf:resource="http://vocab.aodn.org.au/def/organisation/entity/259"/>
	<skos:narrower rdf:resource="http://vocab.aodn.org.au/def/organisation/entity/260"/>
	<skos:narrower rdf:resource="http://vocab.aodn.org.au/def/organisation/entity/261"/>
	<skos:narrower rdf:resource="http://vocab.aodn.org.au/def/organisation/entity/29"/>
	<skos:narrower rdf:resource="http://vocab.aodn.org.au/def/organisation/entity/405"/>
	<skos:topConceptOf rdf:resource="http://vocab.aodn.org.au/def/organisation/1"/>
	<skos:inScheme rdf:resource="http://vocab.aodn.org.au/def/organisation/1"/>
</rdf:Description>

<rdf:Description rdf:about="http://vocab.aodn.org.au/def/organisation/entity/262">
	<rdf:type rdf:resource="http://www.w3.org/2000/01/rdf-schema#Resource"/>
	<rdf:type rdf:resource="http://www.w3.org/2004/02/skos/core#Concept"/>
	<dcterms:modified rdf:datatype="http://www.w3.org/2001/XMLSchema#dateTime">2016-01-27T01:25:28Z</dcterms:modified>
	<dcterms:creator rdf:datatype="http://www.w3.org/2001/XMLSchema#string">Natalia Atkins</dcterms:creator>
	<dcterms:created rdf:datatype="http://www.w3.org/2001/XMLSchema#dateTime">2015-07-13T10:38:15Z</dcterms:created>
	<dcterms:contributor rdf:datatype="http://www.w3.org/2001/XMLSchema#string">eMII_Finney.Kim_Admin</dcterms:contributor>
	<skos:broadMatch rdf:resource="http://vocab.aodn.org.au/def/organisation_classes/category/3"/>
	<skos:prefLabel xml:lang="en">Central Queensland University (CQU)</skos:prefLabel>
	<skos:altLabel xml:lang="en"></skos:altLabel>
	<skos:hiddenLabel xml:lang="en">CQU</skos:hiddenLabel>
	<skos:definition xml:lang="en">The University was originally founded in Rockhampton in 1967 and was known as the Queensland Institute of Technology (Capricornia), achieving full university status in 1992. Its main campus is in North Rockhampton, Queensland. Along with locations in regional Queensland (Bundaberg, Emerald, Gladstone, and Mackay), CQUniversity has also expanded its presence throughout Australia with campuses in Adelaide, Brisbane, Melbourne, Noosa and Sydney, Study Centres in Biloela and Yeppoon, a Cairns Distance Education Study Centre, a delivery site in Edithvale, Victoria, and Partner Study Hubs in Cannonvale, Queensland and Geraldton, Western Australia.</skos:definition>
	<dc:source rdf:datatype="http://www.w3.org/2001/XMLSchema#string">Australian Ocean Data Network Organisation Register</dc:source>
	<dc:publisher rdf:datatype="http://www.w3.org/2001/XMLSchema#string">eMarine Information Infrastructure (eMII)</dc:publisher>
	<skos:exactMatch rdf:resource="http://seadatanet.maris2.nl/v_edmo/print.asp?n_code=4249"/>
	<skos:topConceptOf rdf:resource="http://vocab.aodn.org.au/def/organisation/1"/>
	<skos:inScheme rdf:resource="http://vocab.aodn.org.au/def/organisation/1"/>
</rdf:Description>

<rdf:Description rdf:about="http://vocab.aodn.org.au/def/organisation/entity/263">
	<rdf:type rdf:resource="http://www.w3.org/2000/01/rdf-schema#Resource"/>
	<rdf:type rdf:resource="http://www.w3.org/2004/02/skos/core#Concept"/>
	<dcterms:modified rdf:datatype="http://www.w3.org/2001/XMLSchema#dateTime">2016-01-28T03:37:32Z</dcterms:modified>
	<dcterms:creator rdf:datatype="http://www.w3.org/2001/XMLSchema#string">Natalia Atkins</dcterms:creator>
	<dcterms:created rdf:datatype="http://www.w3.org/2001/XMLSchema#dateTime">2015-07-13T10:38:15Z</dcterms:created>
	<dcterms:contributor rdf:datatype="http://www.w3.org/2001/XMLSchema#string">eMII_Atkins.Natalia</dcterms:contributor>
	<skos:broadMatch rdf:resource="http://vocab.aodn.org.au/def/organisation_classes/category/3"/>
	<skos:prefLabel xml:lang="en">Charles Darwin University (CDU)</skos:prefLabel>
	<skos:altLabel xml:lang="en"></skos:altLabel>
	<skos:hiddenLabel xml:lang="en">CDU</skos:hiddenLabel>
	<skos:definition xml:lang="en">Charles Darwin University was 'created' in 2003, from the merger of the Northern Territory University and the Alice Spring's Centralian College. CDU teaches students at four campuses and four training centres across Australia.</skos:definition>
	<dc:source rdf:datatype="http://www.w3.org/2001/XMLSchema#string">Australian Ocean Data Network Organisation Register</dc:source>
	<dc:publisher rdf:datatype="http://www.w3.org/2001/XMLSchema#string">eMarine Information Infrastructure (eMII)</dc:publisher>
	<skos:exactMatch rdf:resource="http://seadatanet.maris2.nl/v_edmo/print.asp?n_code=4250"/>
	<skos:narrower rdf:resource="http://vocab.aodn.org.au/def/organisation/entity/264"/>
	<skos:narrower rdf:resource="http://vocab.aodn.org.au/def/organisation/entity/265"/>
	<skos:narrower rdf:resource="http://vocab.aodn.org.au/def/organisation/entity/266"/>
	<skos:narrower rdf:resource="http://vocab.aodn.org.au/def/organisation/entity/267"/>
	<skos:topConceptOf rdf:resource="http://vocab.aodn.org.au/def/organisation/1"/>
	<skos:inScheme rdf:resource="http://vocab.aodn.org.au/def/organisation/1"/>
	<skos:scopeNote xml:lang="en">Replaces http://vocab.aodn.org.au/def/organisation/entity/303</skos:scopeNote>
	<dcterms:replaces xml:lang="en">Northern Territory University (NTU)</dcterms:replaces>
</rdf:Description>

<rdf:Description rdf:about="http://vocab.aodn.org.au/def/organisation/entity/268">
	<rdf:type rdf:resource="http://www.w3.org/2000/01/rdf-schema#Resource"/>
	<rdf:type rdf:resource="http://www.w3.org/2004/02/skos/core#Concept"/>
	<dcterms:creator rdf:datatype="http://www.w3.org/2001/XMLSchema#string">Natalia Atkins</dcterms:creator>
	<dcterms:created rdf:datatype="http://www.w3.org/2001/XMLSchema#dateTime">2015-07-08T10:38:15Z</dcterms:created>
	<skos:broadMatch rdf:resource="http://vocab.aodn.org.au/def/organisation_classes/category/3"/>
	<skos:prefLabel xml:lang="en">Charles Sturt University (CSU)</skos:prefLabel>
	<skos:altLabel xml:lang="en"></skos:altLabel>
	<skos:hiddenLabel xml:lang="en">CSU</skos:hiddenLabel>
	<skos:definition xml:lang="en">Charles Sturt University has campuses at Bathurst, Canberra, Albury-Wodonga, Dubbo, Goulburn, Orange, Port Macquarie, Wagga Wagga and Burlington, Ontario (Canada). It has specialist centres in North Parramatta, Manly (Sydney), Melbourne, Sydney and Wangaratta.</skos:definition>
	<dc:source rdf:datatype="http://www.w3.org/2001/XMLSchema#string">Australian Ocean Data Network Organisation Register</dc:source>
	<dc:publisher rdf:datatype="http://www.w3.org/2001/XMLSchema#string">eMarine Information Infrastructure (eMII)</dc:publisher>
	<skos:exactMatch rdf:resource="http://seadatanet.maris2.nl/v_edmo/print.asp?n_code=4253"/>
	<skos:narrower rdf:resource="http://vocab.aodn.org.au/def/organisation/entity/269"/>
	<skos:topConceptOf rdf:resource="http://vocab.aodn.org.au/def/organisation/1"/>
	<skos:inScheme rdf:resource="http://vocab.aodn.org.au/def/organisation/1"/>
</rdf:Description>

<rdf:Description rdf:about="http://vocab.aodn.org.au/def/organisation/entity/270">
	<rdf:type rdf:resource="http://www.w3.org/2000/01/rdf-schema#Resource"/>
	<rdf:type rdf:resource="http://www.w3.org/2004/02/skos/core#Concept"/>
	<dcterms:creator rdf:datatype="http://www.w3.org/2001/XMLSchema#string">Natalia Atkins</dcterms:creator>
	<dcterms:created rdf:datatype="http://www.w3.org/2001/XMLSchema#dateTime">2015-07-16T10:38:15Z</dcterms:created>
	<skos:broadMatch rdf:resource="http://vocab.aodn.org.au/def/organisation_classes/category/3"/>
	<skos:prefLabel xml:lang="en">Deakin University</skos:prefLabel>
	<skos:altLabel xml:lang="en"></skos:altLabel>
	<skos:hiddenLabel xml:lang="en"></skos:hiddenLabel>
	<skos:definition xml:lang="en">Established in 1974, Deakin University has four campuses: Melbourne Burwood, Geelong Waterfront, Geelong Waurn Ponds and Warrnambool.</skos:definition>
	<dc:source rdf:datatype="http://www.w3.org/2001/XMLSchema#string">Australian Ocean Data Network Organisation Register</dc:source>
	<dc:publisher rdf:datatype="http://www.w3.org/2001/XMLSchema#string">eMarine Information Infrastructure (eMII)</dc:publisher>
	<skos:exactMatch rdf:resource="http://seadatanet.maris2.nl/v_edmo/print.asp?n_code=4260"/>
	<skos:narrower rdf:resource="http://vocab.aodn.org.au/def/organisation/entity/271"/>
	<skos:narrower rdf:resource="http://vocab.aodn.org.au/def/organisation/entity/272"/>
	<skos:narrower rdf:resource="http://vocab.aodn.org.au/def/organisation/entity/273"/>
	<skos:topConceptOf rdf:resource="http://vocab.aodn.org.au/def/organisation/1"/>
	<skos:inScheme rdf:resource="http://vocab.aodn.org.au/def/organisation/1"/>
</rdf:Description>

<rdf:Description rdf:about="http://vocab.aodn.org.au/def/organisation/entity/274">
	<rdf:type rdf:resource="http://www.w3.org/2000/01/rdf-schema#Resource"/>
	<rdf:type rdf:resource="http://www.w3.org/2004/02/skos/core#Concept"/>
	<dcterms:modified rdf:datatype="http://www.w3.org/2001/XMLSchema#dateTime">2015-07-16T06:06:13Z</dcterms:modified>
	<dcterms:creator rdf:datatype="http://www.w3.org/2001/XMLSchema#string">Natalia Atkins</dcterms:creator>
	<dcterms:created rdf:datatype="http://www.w3.org/2001/XMLSchema#dateTime">2015-07-16T10:38:15Z</dcterms:created>
	<dcterms:contributor rdf:datatype="http://www.w3.org/2001/XMLSchema#string">Natalia_Atkins</dcterms:contributor>
	<skos:broadMatch rdf:resource="http://vocab.aodn.org.au/def/organisation_classes/category/3"/>
	<skos:prefLabel xml:lang="en">Edith Cowan University (ECU)</skos:prefLabel>
	<skos:altLabel xml:lang="en"></skos:altLabel>
	<skos:hiddenLabel xml:lang="en">ECU</skos:hiddenLabel>
	<skos:definition xml:lang="en">Edith Cowan University (ECU) is located in Perth, Western Australia, and was established in 1991. The university offers courses across two city campuses, in Mount Lawley and Joondalup, and has a regional campus: South West, which is in Bunbury.</skos:definition>
	<dc:source rdf:datatype="http://www.w3.org/2001/XMLSchema#string">Australian Ocean Data Network Organisation Register</dc:source>
	<dc:publisher rdf:datatype="http://www.w3.org/2001/XMLSchema#string">eMarine Information Infrastructure (eMII)</dc:publisher>
	<skos:exactMatch rdf:resource="http://seadatanet.maris2.nl/v_edmo/print.asp?n_code=4262"/>
	<skos:narrower rdf:resource="http://vocab.aodn.org.au/def/organisation/entity/275"/>
	<skos:topConceptOf rdf:resource="http://vocab.aodn.org.au/def/organisation/1"/>
	<skos:inScheme rdf:resource="http://vocab.aodn.org.au/def/organisation/1"/>
</rdf:Description>

<rdf:Description rdf:about="http://vocab.aodn.org.au/def/organisation/entity/278">
	<rdf:type rdf:resource="http://www.w3.org/2000/01/rdf-schema#Resource"/>
	<rdf:type rdf:resource="http://www.w3.org/2004/02/skos/core#Concept"/>
	<dcterms:modified rdf:datatype="http://www.w3.org/2001/XMLSchema#dateTime">2015-11-04T23:01:03Z</dcterms:modified>
	<dcterms:creator rdf:datatype="http://www.w3.org/2001/XMLSchema#string">Natalia Atkins</dcterms:creator>
	<dcterms:created rdf:datatype="http://www.w3.org/2001/XMLSchema#dateTime">2015-07-16T10:38:15Z</dcterms:created>
	<dcterms:contributor rdf:datatype="http://www.w3.org/2001/XMLSchema#string">eMII_Atkins.Natalia</dcterms:contributor>
	<skos:broadMatch rdf:resource="http://vocab.aodn.org.au/def/organisation_classes/category/3"/>
	<skos:prefLabel xml:lang="en">Griffith University (GU)</skos:prefLabel>
	<skos:altLabel xml:lang="en"></skos:altLabel>
	<skos:hiddenLabel xml:lang="en">GU</skos:hiddenLabel>
	<skos:definition xml:lang="en">Founded in 1971, Griffith University has five campuses spanning three cities in South East Queensland: Nathan, Mount Gravatt and South Bank in Brisbane and campuses at Logan and the Gold Coast.</skos:definition>
	<dc:source rdf:datatype="http://www.w3.org/2001/XMLSchema#string">Australian Ocean Data Network Organisation Register</dc:source>
	<dc:publisher rdf:datatype="http://www.w3.org/2001/XMLSchema#string">eMarine Information Infrastructure (eMII)</dc:publisher>
	<skos:exactMatch rdf:resource="http://seadatanet.maris2.nl/v_edmo/print.asp?n_code=4269"/>
	<skos:narrower rdf:resource="http://vocab.aodn.org.au/def/organisation/entity/342"/>
	<skos:narrower rdf:resource="http://vocab.aodn.org.au/def/organisation/entity/411"/>
	<skos:topConceptOf rdf:resource="http://vocab.aodn.org.au/def/organisation/1"/>
	<skos:inScheme rdf:resource="http://vocab.aodn.org.au/def/organisation/1"/>
</rdf:Description>

<rdf:Description rdf:about="http://vocab.aodn.org.au/def/organisation/entity/287">
	<rdf:type rdf:resource="http://www.w3.org/2000/01/rdf-schema#Resource"/>
	<rdf:type rdf:resource="http://www.w3.org/2004/02/skos/core#Concept"/>
	<dcterms:creator rdf:datatype="http://www.w3.org/2001/XMLSchema#string">Natalia Atkins</dcterms:creator>
	<dcterms:created rdf:datatype="http://www.w3.org/2001/XMLSchema#dateTime">2015-07-17T10:38:15Z</dcterms:created>
	<skos:broadMatch rdf:resource="http://vocab.aodn.org.au/def/organisation_classes/category/3"/>
	<skos:prefLabel xml:lang="en">Macquarie University</skos:prefLabel>
	<skos:altLabel xml:lang="en"></skos:altLabel>
	<skos:hiddenLabel xml:lang="en"></skos:hiddenLabel>
	<skos:definition xml:lang="en">Founded in 1964, Macquarie University is based in Sydney, Australia, and has two campuses: North Ryde and City.</skos:definition>
	<dc:source rdf:datatype="http://www.w3.org/2001/XMLSchema#string">Australian Ocean Data Network Organisation Register</dc:source>
	<dc:publisher rdf:datatype="http://www.w3.org/2001/XMLSchema#string">eMarine Information Infrastructure (eMII)</dc:publisher>
	<skos:exactMatch rdf:resource="http://seadatanet.maris2.nl/v_edmo/print.asp?n_code=4276"/>
	<skos:narrower rdf:resource="http://vocab.aodn.org.au/def/organisation/entity/288"/>
	<skos:topConceptOf rdf:resource="http://vocab.aodn.org.au/def/organisation/1"/>
	<skos:inScheme rdf:resource="http://vocab.aodn.org.au/def/organisation/1"/>
</rdf:Description>

<rdf:Description rdf:about="http://vocab.aodn.org.au/def/organisation/entity/398">
	<rdf:type rdf:resource="http://www.w3.org/2000/01/rdf-schema#Resource"/>
	<rdf:type rdf:resource="http://www.w3.org/2004/02/skos/core#Concept"/>
	<dcterms:modified rdf:datatype="http://www.w3.org/2001/XMLSchema#dateTime">2015-09-22T23:38:58Z</dcterms:modified>
	<dcterms:creator rdf:datatype="http://www.w3.org/2001/XMLSchema#string">Natalia Atkins</dcterms:creator>
	<dcterms:created rdf:datatype="http://www.w3.org/2001/XMLSchema#dateTime">2015-09-23T10:38:15Z</dcterms:created>
	<dcterms:contributor rdf:datatype="http://www.w3.org/2001/XMLSchema#string">eMII_Atkins.Natalia</dcterms:contributor>
	<skos:broadMatch rdf:resource="http://vocab.aodn.org.au/def/organisation_classes/category/4"/>
	<skos:prefLabel xml:lang="en">Antarctic Biodiversity Information Facility (ANTABIF)</skos:prefLabel>
	<skos:altLabel xml:lang="en"></skos:altLabel>
	<skos:hiddenLabel xml:lang="en">ANTABIF</skos:hiddenLabel>
	<skos:definition xml:lang="en">Funded by the Belgian Science Policy Office, biodiversity.aq is building an innovative Antarctic biodiversity information system, giving access to a distributed network of contributing database, according to the principles of the Global Biodiversity Information Facility. It is building a new data discovery tool using two complementary networks and will expand these by using an advanced technical architecture, capable of linking with many potential data resources. Biodiversity.aq is recognised as an official SCAR Product and integrates SCAR-MarBIN (Scientific Committee on Antarctic Research - Marine Biodiversity Information Network), with the biodiversity databases managed by the Australian Antarctic Division, bringing together data from marine and terrestrial realms. biodiversity.aq is the data management tool and repository for the biodiversity-related research conducted at the Princess Elisabeth Station. Biodiversity.aq will use the best available technology to integrate, share and disseminate all available information on Antarctic Biodiversity. Its implementation by the Belgian Biodiversity Platform ascertains that biodiversity.aq can take advantage of the relevant experience of the Belgian GBIF node. biodiversity.aq is steered by an International Steering Committee composed of selected experts in the field of Polar biodiversity.</skos:definition>
	<dc:source rdf:datatype="http://www.w3.org/2001/XMLSchema#string">Australian Ocean Data Network Organisation Register</dc:source>
	<dc:publisher rdf:datatype="http://www.w3.org/2001/XMLSchema#string">eMarine Information Infrastructure (eMMI)</dc:publisher>
	<skos:exactMatch rdf:resource="http://seadatanet.maris2.nl/v_edmerp/print.asp?n_code=12142"/>
	<skos:topConceptOf rdf:resource="http://vocab.aodn.org.au/def/organisation/1"/>
	<skos:inScheme rdf:resource="http://vocab.aodn.org.au/def/organisation/1"/>
</rdf:Description>

<rdf:Description rdf:about="http://vocab.aodn.org.au/def/organisation/entity/303">
	<rdf:type rdf:resource="http://www.w3.org/2000/01/rdf-schema#Resource"/>
	<rdf:type rdf:resource="http://www.w3.org/2004/02/skos/core#Concept"/>
	<dcterms:creator rdf:datatype="http://www.w3.org/2001/XMLSchema#string">Natalia Atkins</dcterms:creator>
	<dcterms:created rdf:datatype="http://www.w3.org/2001/XMLSchema#dateTime">2015-07-22T10:38:15Z</dcterms:created>
	<skos:broadMatch rdf:resource="http://vocab.aodn.org.au/def/organisation_classes/category/3"/>
	<skos:prefLabel xml:lang="en">Northern Territory University (NTU)</skos:prefLabel>
	<skos:altLabel xml:lang="en"></skos:altLabel>
	<skos:hiddenLabel xml:lang="en">NTU</skos:hiddenLabel>
	<skos:definition xml:lang="en">The Northern Territory University was established in January 1989, after an amalgamation took place between the Darwin Institute of Technology and the University College of the Northern Territory. In 2004 the Northern Territory University merged with the Alice Springs' Centralian College to form the Charles Darwin University. (Courtesy of Encyclopedia of Australian Science)</skos:definition>
	<dc:source rdf:datatype="http://www.w3.org/2001/XMLSchema#string">Australian Ocean Data Network Organisation Register</dc:source>
	<dc:publisher rdf:datatype="http://www.w3.org/2001/XMLSchema#string">eMarine Information Infrastructure (eMII)</dc:publisher>
	<skos:narrower rdf:resource="http://vocab.aodn.org.au/def/organisation/entity/304"/>
	<skos:topConceptOf rdf:resource="http://vocab.aodn.org.au/def/organisation/1"/>
	<skos:inScheme rdf:resource="http://vocab.aodn.org.au/def/organisation/1"/>
	<skos:scopeNote xml:lang="en">Organisation no longer exists</skos:scopeNote>
	<skos:scopeNote xml:lang="en">Organisation no longer exists. Replaced by http://vocab.aodn.org.au/def/organisation/entity/263</skos:scopeNote>
	<dcterms:isReplacedBy rdf:resource="http://vocab.aodn.org.au/def/organisation/entity/263"/>
	<dcterms:isReplacedBy xml:lang="en">Charles Darwin University (CDU)</dcterms:isReplacedBy>
</rdf:Description>

<rdf:Description rdf:about="http://vocab.aodn.org.au/def/organisation/entity/305">
	<rdf:type rdf:resource="http://www.w3.org/2000/01/rdf-schema#Resource"/>
	<rdf:type rdf:resource="http://www.w3.org/2004/02/skos/core#Concept"/>
	<dcterms:creator rdf:datatype="http://www.w3.org/2001/XMLSchema#string">Natalia Atkins</dcterms:creator>
	<dcterms:created rdf:datatype="http://www.w3.org/2001/XMLSchema#dateTime">2015-07-22T10:38:15Z</dcterms:created>
	<skos:broadMatch rdf:resource="http://vocab.aodn.org.au/def/organisation_classes/category/3"/>
	<skos:prefLabel xml:lang="en">The University of Adelaide</skos:prefLabel>
	<skos:altLabel xml:lang="en"></skos:altLabel>
	<skos:hiddenLabel xml:lang="en"></skos:hiddenLabel>
	<skos:definition xml:lang="en">The University of Adelaide is a university in Adelaide, South Australia, which was established in 1874. Its main campus is on North Terrace in the Adelaide city centre. The university has three other campuses throughout the state: Roseworthy; Waite; and Thebarton; and the Ngee Ann–Adelaide Education Centre (NAAEC), in Singapore.</skos:definition>
	<dc:source rdf:datatype="http://www.w3.org/2001/XMLSchema#string">Australian Ocean Data Network Organisation Register</dc:source>
	<dc:publisher rdf:datatype="http://www.w3.org/2001/XMLSchema#string">eMarine Information Infrastructure (eMII)</dc:publisher>
	<skos:exactMatch rdf:resource="http://seadatanet.maris2.nl/v_edmo/print.asp?n_code=4028"/>
	<skos:narrower rdf:resource="http://vocab.aodn.org.au/def/organisation/entity/306"/>
	<skos:topConceptOf rdf:resource="http://vocab.aodn.org.au/def/organisation/1"/>
	<skos:inScheme rdf:resource="http://vocab.aodn.org.au/def/organisation/1"/>
</rdf:Description>

<rdf:Description rdf:about="http://vocab.aodn.org.au/def/organisation/entity/307">
	<rdf:type rdf:resource="http://www.w3.org/2000/01/rdf-schema#Resource"/>
	<rdf:type rdf:resource="http://www.w3.org/2004/02/skos/core#Concept"/>
	<dcterms:creator rdf:datatype="http://www.w3.org/2001/XMLSchema#string">Natalia Atkins</dcterms:creator>
	<dcterms:created rdf:datatype="http://www.w3.org/2001/XMLSchema#dateTime">2015-07-22T10:38:15Z</dcterms:created>
	<skos:broadMatch rdf:resource="http://vocab.aodn.org.au/def/organisation_classes/category/3"/>
	<skos:prefLabel xml:lang="en">University of Canberra (UC)</skos:prefLabel>
	<skos:altLabel xml:lang="en"></skos:altLabel>
	<skos:hiddenLabel xml:lang="en">UC</skos:hiddenLabel>
	<skos:definition xml:lang="en">The University of Canberra was first established in 1967 as the Canberra College of Advanced Education. The Canberra CAE became the University of Canberra under sponsorship of Monash University in 1990. The University is located in Bruce, Canberra. (Courtesy of wikipedia)</skos:definition>
	<dc:source rdf:datatype="http://www.w3.org/2001/XMLSchema#string">Australian Ocean Data Network Organisation Register</dc:source>
	<dc:publisher rdf:datatype="http://www.w3.org/2001/XMLSchema#string">eMarine Information Infrastructure (eMII)</dc:publisher>
	<skos:exactMatch rdf:resource="http://seadatanet.maris2.nl/v_edmo/print.asp?n_code=4318"/>
	<skos:narrower rdf:resource="http://vocab.aodn.org.au/def/organisation/entity/308"/>
	<skos:topConceptOf rdf:resource="http://vocab.aodn.org.au/def/organisation/1"/>
	<skos:inScheme rdf:resource="http://vocab.aodn.org.au/def/organisation/1"/>
</rdf:Description>

<rdf:Description rdf:about="http://vocab.aodn.org.au/def/organisation/entity/309">
	<rdf:type rdf:resource="http://www.w3.org/2000/01/rdf-schema#Resource"/>
	<rdf:type rdf:resource="http://www.w3.org/2004/02/skos/core#Concept"/>
	<dcterms:creator rdf:datatype="http://www.w3.org/2001/XMLSchema#string">Natalia Atkins</dcterms:creator>
	<dcterms:created rdf:datatype="http://www.w3.org/2001/XMLSchema#dateTime">2015-07-22T10:38:15Z</dcterms:created>
	<skos:broadMatch rdf:resource="http://vocab.aodn.org.au/def/organisation_classes/category/3"/>
	<skos:prefLabel xml:lang="en">The University of Melbourne</skos:prefLabel>
	<skos:altLabel xml:lang="en"></skos:altLabel>
	<skos:hiddenLabel xml:lang="en"></skos:hiddenLabel>
	<skos:definition xml:lang="en">The University of Melbourne is an Australian university located in Melbourne, Victoria, which was founded in 1853. There are seven campus locations across Melbourne and rural Victoria, including the main Parkville campus.</skos:definition>
	<dc:source rdf:datatype="http://www.w3.org/2001/XMLSchema#string">Australian Ocean Data Network Organisation Register</dc:source>
	<dc:publisher rdf:datatype="http://www.w3.org/2001/XMLSchema#string">eMarine Information Infrastructure (eMII)</dc:publisher>
	<skos:exactMatch rdf:resource="http://seadatanet.maris2.nl/v_edmo/print.asp?n_code=4320"/>
	<skos:narrower rdf:resource="http://vocab.aodn.org.au/def/organisation/entity/310"/>
	<skos:narrower rdf:resource="http://vocab.aodn.org.au/def/organisation/entity/311"/>
	<skos:narrower rdf:resource="http://vocab.aodn.org.au/def/organisation/entity/312"/>
	<skos:narrower rdf:resource="http://vocab.aodn.org.au/def/organisation/entity/313"/>
	<skos:narrower rdf:resource="http://vocab.aodn.org.au/def/organisation/entity/314"/>
	<skos:narrower rdf:resource="http://vocab.aodn.org.au/def/organisation/entity/315"/>
	<skos:topConceptOf rdf:resource="http://vocab.aodn.org.au/def/organisation/1"/>
	<skos:inScheme rdf:resource="http://vocab.aodn.org.au/def/organisation/1"/>
</rdf:Description>

<rdf:Description rdf:about="http://vocab.aodn.org.au/def/organisation/entity/279">
	<rdf:type rdf:resource="http://www.w3.org/2000/01/rdf-schema#Resource"/>
	<rdf:type rdf:resource="http://www.w3.org/2004/02/skos/core#Concept"/>
	<dcterms:modified rdf:datatype="http://www.w3.org/2001/XMLSchema#dateTime">2016-01-27T05:55:50Z</dcterms:modified>
	<dcterms:creator rdf:datatype="http://www.w3.org/2001/XMLSchema#string">Natalia Atkins</dcterms:creator>
	<dcterms:created rdf:datatype="http://www.w3.org/2001/XMLSchema#dateTime">2015-07-16T10:38:15Z</dcterms:created>
	<dcterms:contributor rdf:datatype="http://www.w3.org/2001/XMLSchema#string">eMII_Atkins.Natalia</dcterms:contributor>
	<skos:broadMatch rdf:resource="http://vocab.aodn.org.au/def/organisation_classes/category/3"/>
	<skos:prefLabel xml:lang="en">James Cook University (JCU)</skos:prefLabel>
	<skos:altLabel xml:lang="en"></skos:altLabel>
	<skos:hiddenLabel xml:lang="en">JCU</skos:hiddenLabel>
	<skos:definition xml:lang="en">Established in 1970, James Cook University (JCU) is a multi-campus institution with it's main campuses in the cities of Cairns, Singapore and Townsville, with smaller centres in Mount Isa, Thursday Island and Mackay. It also has a campus in Brisbane, operated by Russo Higher Education.</skos:definition>
	<dc:source rdf:datatype="http://www.w3.org/2001/XMLSchema#string">Australian Ocean Data Network Organisation Register</dc:source>
	<dc:publisher rdf:datatype="http://www.w3.org/2001/XMLSchema#string">eMarine Information Infrastructure (eMII)</dc:publisher>
	<skos:exactMatch rdf:resource="http://seadatanet.maris2.nl/v_edmo/print.asp?n_code=4270"/>
	<skos:narrower rdf:resource="http://vocab.aodn.org.au/def/organisation/entity/280"/>
	<skos:narrower rdf:resource="http://vocab.aodn.org.au/def/organisation/entity/281"/>
	<skos:narrower rdf:resource="http://vocab.aodn.org.au/def/organisation/entity/282"/>
	<skos:narrower rdf:resource="http://vocab.aodn.org.au/def/organisation/entity/283"/>
	<skos:narrower rdf:resource="http://vocab.aodn.org.au/def/organisation/entity/284"/>
	<skos:narrower rdf:resource="http://vocab.aodn.org.au/def/organisation/entity/285"/>
	<skos:narrower rdf:resource="http://vocab.aodn.org.au/def/organisation/entity/286"/>
	<skos:topConceptOf rdf:resource="http://vocab.aodn.org.au/def/organisation/1"/>
	<skos:inScheme rdf:resource="http://vocab.aodn.org.au/def/organisation/1"/>
</rdf:Description>

<rdf:Description rdf:about="http://vocab.aodn.org.au/def/organisation/entity/289">
	<rdf:type rdf:resource="http://www.w3.org/2000/01/rdf-schema#Resource"/>
	<rdf:type rdf:resource="http://www.w3.org/2004/02/skos/core#Concept"/>
	<dcterms:creator rdf:datatype="http://www.w3.org/2001/XMLSchema#string">Natalia Atkins</dcterms:creator>
	<dcterms:created rdf:datatype="http://www.w3.org/2001/XMLSchema#dateTime">2015-07-17T10:38:15Z</dcterms:created>
	<skos:broadMatch rdf:resource="http://vocab.aodn.org.au/def/organisation_classes/category/3"/>
	<skos:prefLabel xml:lang="en">Monash University</skos:prefLabel>
	<skos:altLabel xml:lang="en"></skos:altLabel>
	<skos:hiddenLabel xml:lang="en"></skos:hiddenLabel>
	<skos:definition xml:lang="en">Monash University, based in Melbourne, was founded in 1958. It also has five Australian campuses (Clayton, Caulfield, Berwick, Peninsula and Parkville), a campus in Malaysia, a joint graduate school in China, a learning centre in Italy, and a research centre in India. Monash University courses are also delivered at other locations, including at Monash South Africa.</skos:definition>
	<dc:source rdf:datatype="http://www.w3.org/2001/XMLSchema#string">Australian Ocean Data Network Organisation Register</dc:source>
	<dc:publisher rdf:datatype="http://www.w3.org/2001/XMLSchema#string">eMarine Information Infrastructure (eMII)</dc:publisher>
	<skos:exactMatch rdf:resource="http://seadatanet.maris2.nl/v_edmo/print.asp?n_code=4278"/>
	<skos:narrower rdf:resource="http://vocab.aodn.org.au/def/organisation/entity/290"/>
	<skos:narrower rdf:resource="http://vocab.aodn.org.au/def/organisation/entity/291"/>
	<skos:narrower rdf:resource="http://vocab.aodn.org.au/def/organisation/entity/292"/>
	<skos:narrower rdf:resource="http://vocab.aodn.org.au/def/organisation/entity/293"/>
	<skos:topConceptOf rdf:resource="http://vocab.aodn.org.au/def/organisation/1"/>
	<skos:inScheme rdf:resource="http://vocab.aodn.org.au/def/organisation/1"/>
</rdf:Description>

<rdf:Description rdf:about="http://vocab.aodn.org.au/def/organisation/entity/294">
	<rdf:type rdf:resource="http://www.w3.org/2000/01/rdf-schema#Resource"/>
	<rdf:type rdf:resource="http://www.w3.org/2004/02/skos/core#Concept"/>
	<dcterms:creator rdf:datatype="http://www.w3.org/2001/XMLSchema#string">Natalia Atkins</dcterms:creator>
	<dcterms:created rdf:datatype="http://www.w3.org/2001/XMLSchema#dateTime">2015-07-17T10:38:15Z</dcterms:created>
	<skos:broadMatch rdf:resource="http://vocab.aodn.org.au/def/organisation_classes/category/3"/>
	<skos:prefLabel xml:lang="en">Murdoch University</skos:prefLabel>
	<skos:altLabel xml:lang="en"></skos:altLabel>
	<skos:hiddenLabel xml:lang="en"></skos:hiddenLabel>
	<skos:definition xml:lang="en">Founded in 1973, Murdoch University is a university based in Perth, Western Australia with campuses also in Rockingham and Mandurah, Western Australia; Singapore; Malaysia; and Dubai.</skos:definition>
	<dc:source rdf:datatype="http://www.w3.org/2001/XMLSchema#string">Australian Ocean Data Network Organisation Register</dc:source>
	<dc:publisher rdf:datatype="http://www.w3.org/2001/XMLSchema#string">eMarine Information Infrastructure (eMII)</dc:publisher>
	<skos:exactMatch rdf:resource="http://seadatanet.maris2.nl/v_edmo/print.asp?n_code=4282"/>
	<skos:narrower rdf:resource="http://vocab.aodn.org.au/def/organisation/entity/295"/>
	<skos:narrower rdf:resource="http://vocab.aodn.org.au/def/organisation/entity/296"/>
	<skos:narrower rdf:resource="http://vocab.aodn.org.au/def/organisation/entity/297"/>
	<skos:narrower rdf:resource="http://vocab.aodn.org.au/def/organisation/entity/298"/>
	<skos:narrower rdf:resource="http://vocab.aodn.org.au/def/organisation/entity/299"/>
	<skos:narrower rdf:resource="http://vocab.aodn.org.au/def/organisation/entity/300"/>
	<skos:narrower rdf:resource="http://vocab.aodn.org.au/def/organisation/entity/301"/>
	<skos:narrower rdf:resource="http://vocab.aodn.org.au/def/organisation/entity/302"/>
	<skos:topConceptOf rdf:resource="http://vocab.aodn.org.au/def/organisation/1"/>
	<skos:inScheme rdf:resource="http://vocab.aodn.org.au/def/organisation/1"/>
</rdf:Description>

<rdf:Description rdf:about="http://vocab.aodn.org.au/def/organisation/entity/316">
	<rdf:type rdf:resource="http://www.w3.org/2000/01/rdf-schema#Resource"/>
	<rdf:type rdf:resource="http://www.w3.org/2004/02/skos/core#Concept"/>
	<dcterms:creator rdf:datatype="http://www.w3.org/2001/XMLSchema#string">Natalia Atkins</dcterms:creator>
	<dcterms:created rdf:datatype="http://www.w3.org/2001/XMLSchema#dateTime">2015-07-22T10:38:15Z</dcterms:created>
	<skos:broadMatch rdf:resource="http://vocab.aodn.org.au/def/organisation_classes/category/3"/>
	<skos:prefLabel xml:lang="en">University of the Sunshine Coast (USC)</skos:prefLabel>
	<skos:altLabel xml:lang="en"></skos:altLabel>
	<skos:hiddenLabel xml:lang="en">USC</skos:hiddenLabel>
	<skos:definition xml:lang="en">The University of the Sunshine Coast's main campus is located in Sippy Downs, with five other study locations at: Gympie, South Bank in Brisbane, Noosa, Caboolture and North Lakes. In addition there is a Research and Learning Centre on Fraser Island.</skos:definition>
	<dc:source rdf:datatype="http://www.w3.org/2001/XMLSchema#string">Australian Ocean Data Network Organisation Register</dc:source>
	<dc:publisher rdf:datatype="http://www.w3.org/2001/XMLSchema#string">eMarine Information Infrastructure (eMII)</dc:publisher>
	<skos:exactMatch rdf:resource="http://seadatanet.maris2.nl/v_edmo/print.asp?n_code=4323"/>
	<skos:narrower rdf:resource="http://vocab.aodn.org.au/def/organisation/entity/317"/>
	<skos:topConceptOf rdf:resource="http://vocab.aodn.org.au/def/organisation/1"/>
	<skos:inScheme rdf:resource="http://vocab.aodn.org.au/def/organisation/1"/>
</rdf:Description>

<rdf:Description rdf:about="http://vocab.aodn.org.au/def/organisation/entity/318">
	<rdf:type rdf:resource="http://www.w3.org/2000/01/rdf-schema#Resource"/>
	<rdf:type rdf:resource="http://www.w3.org/2004/02/skos/core#Concept"/>
	<dcterms:creator rdf:datatype="http://www.w3.org/2001/XMLSchema#string">Natalia Atkins</dcterms:creator>
	<dcterms:created rdf:datatype="http://www.w3.org/2001/XMLSchema#dateTime">2015-07-22T10:38:15Z</dcterms:created>
	<skos:broadMatch rdf:resource="http://vocab.aodn.org.au/def/organisation_classes/category/3"/>
	<skos:prefLabel xml:lang="en">University of Technology, Sydney (UTS)</skos:prefLabel>
	<skos:altLabel xml:lang="en"></skos:altLabel>
	<skos:hiddenLabel xml:lang="en">UTS</skos:hiddenLabel>
	<skos:definition xml:lang="en">This university was established in 1988. It has two campuses: Sydney city, and Kuring-gai campus in Lindfield, Sydney.</skos:definition>
	<dc:source rdf:datatype="http://www.w3.org/2001/XMLSchema#string">Australian Ocean Data Network Organisation Register</dc:source>
	<dc:publisher rdf:datatype="http://www.w3.org/2001/XMLSchema#string">eMarine Information Infrastructure (eMII)</dc:publisher>
	<skos:exactMatch rdf:resource="http://seadatanet.maris2.nl/v_edmo/print.asp?n_code=4328"/>
	<skos:topConceptOf rdf:resource="http://vocab.aodn.org.au/def/organisation/1"/>
	<skos:inScheme rdf:resource="http://vocab.aodn.org.au/def/organisation/1"/>
</rdf:Description>

<rdf:Description rdf:about="http://vocab.aodn.org.au/def/organisation/entity/319">
	<rdf:type rdf:resource="http://www.w3.org/2000/01/rdf-schema#Resource"/>
	<rdf:type rdf:resource="http://www.w3.org/2004/02/skos/core#Concept"/>
	<dcterms:modified rdf:datatype="http://www.w3.org/2001/XMLSchema#dateTime">2015-09-18T03:22:08Z</dcterms:modified>
	<dcterms:creator rdf:datatype="http://www.w3.org/2001/XMLSchema#string">Natalia Atkins</dcterms:creator>
	<dcterms:created rdf:datatype="http://www.w3.org/2001/XMLSchema#dateTime">2015-07-28T10:38:15Z</dcterms:created>
	<dcterms:contributor rdf:datatype="http://www.w3.org/2001/XMLSchema#string">eMII_Atkins.Natalia</dcterms:contributor>
	<skos:broadMatch rdf:resource="http://vocab.aodn.org.au/def/organisation_classes/category/4"/>
	<skos:prefLabel xml:lang="en">Leibniz Institute of Marine Sciences (IFM-GEOMAR), University of Kiel</skos:prefLabel>
	<skos:altLabel xml:lang="en">Leibniz Institute of Marine Sciences</skos:altLabel>
	<skos:hiddenLabel xml:lang="en">IFM-GEOMAR</skos:hiddenLabel>
	<skos:definition xml:lang="en">The Leibniz Institute of Marine Sciences at the University of Kiel (IFM-GEOMAR) was founded January 1st, 2004 through the merger of the Institute for Marine Science (IfM) and the Research Center for Marine Geosciences (GEOMAR).The goal of the institute is the investigation of all areas relevant for actual research in marine sciences, ranging from Geology of the Ocean Floor to Marine Meteorology. The institute operates world-wide in all ocean basins. The main research topics are grouped in four areas: Ocean Circulation and Climate Dynamics, Marine Biogeochemistry, Marine Ecology, and Dynamics of the Ocean Floor.</skos:definition>
	<dc:source rdf:datatype="http://www.w3.org/2001/XMLSchema#string">Australian Ocean Data Network Organisation Register</dc:source>
	<dc:publisher rdf:datatype="http://www.w3.org/2001/XMLSchema#string">eMarine Information Infrastructure (eMII)</dc:publisher>
	<skos:exactMatch rdf:resource="http://seadatanet.maris2.nl/v_edmo/print.asp?n_code=992"/>
	<skos:topConceptOf rdf:resource="http://vocab.aodn.org.au/def/organisation/1"/>
	<skos:inScheme rdf:resource="http://vocab.aodn.org.au/def/organisation/1"/>
	<skos:scopeNote xml:lang="en">Organisation no longer exists</skos:scopeNote>
	<skos:scopeNote xml:lang="en">Organisation no longer exists. Replaced by http://vocab.aodn.org.au/def/organisation/entity/382</skos:scopeNote>
	<dcterms:isReplacedBy xml:lang="en">http://vocab.aodn.org.au/def/organisation/entity/382</dcterms:isReplacedBy>
	<dcterms:isReplacedBy xml:lang="en">GEOMAR Helmholtz Centre for Ocean Research Kiel</dcterms:isReplacedBy>
</rdf:Description>

<rdf:Description rdf:about="http://vocab.aodn.org.au/def/organisation/entity/320">
	<rdf:type rdf:resource="http://www.w3.org/2000/01/rdf-schema#Resource"/>
	<rdf:type rdf:resource="http://www.w3.org/2004/02/skos/core#Concept"/>
	<dcterms:creator rdf:datatype="http://www.w3.org/2001/XMLSchema#string">Natalia Atkins</dcterms:creator>
	<dcterms:created rdf:datatype="http://www.w3.org/2001/XMLSchema#dateTime">2015-07-28T10:38:15Z</dcterms:created>
	<skos:broadMatch rdf:resource="http://vocab.aodn.org.au/def/organisation_classes/category/4"/>
	<skos:prefLabel xml:lang="en">Oregon State University (OSU)</skos:prefLabel>
	<skos:altLabel xml:lang="en"></skos:altLabel>
	<skos:hiddenLabel xml:lang="en">OSU</skos:hiddenLabel>
	<skos:definition xml:lang="en">Oregon State University (OSU) is a flagship university of the Oregon University System. A coeducational, public research university located in Corvallis, Oregon. The university offers undergraduate, graduate, doctoral degrees and a multitude of research opportunities.</skos:definition>
	<dc:source rdf:datatype="http://www.w3.org/2001/XMLSchema#string">Australian Ocean Data Network Organisation Register</dc:source>
	<dc:publisher rdf:datatype="http://www.w3.org/2001/XMLSchema#string">eMarine Information Infrastructure (eMII)</dc:publisher>
	<skos:exactMatch rdf:resource="http://seadatanet.maris2.nl/v_edmo/print.asp?n_code=3807"/>
	<skos:topConceptOf rdf:resource="http://vocab.aodn.org.au/def/organisation/1"/>
	<skos:inScheme rdf:resource="http://vocab.aodn.org.au/def/organisation/1"/>
</rdf:Description>

<rdf:Description rdf:about="http://vocab.aodn.org.au/def/organisation/entity/321">
	<rdf:type rdf:resource="http://www.w3.org/2000/01/rdf-schema#Resource"/>
	<rdf:type rdf:resource="http://www.w3.org/2004/02/skos/core#Concept"/>
	<dcterms:creator rdf:datatype="http://www.w3.org/2001/XMLSchema#string">Natalia Atkins</dcterms:creator>
	<dcterms:created rdf:datatype="http://www.w3.org/2001/XMLSchema#dateTime">2015-07-28T10:38:15Z</dcterms:created>
	<skos:broadMatch rdf:resource="http://vocab.aodn.org.au/def/organisation_classes/category/4"/>
	<skos:prefLabel xml:lang="en">University of California, San Diego (UCSD)</skos:prefLabel>
	<skos:altLabel xml:lang="en"></skos:altLabel>
	<skos:hiddenLabel xml:lang="en">UCSD</skos:hiddenLabel>
	<skos:definition xml:lang="en">The University of California, San Diego (UCSD) is a public research university located in the La Jolla area of San Diego, California. UC San Diego is the seventh oldest of the 10 University of California campuses and offers over 200 undergraduate and graduate degree programs, enrolling about 22,700 undergraduate and 6,300 graduate students. UC San Diego is one of America's Public Ivy universities, which recognizes top public research universities in the United States.</skos:definition>
	<dc:source rdf:datatype="http://www.w3.org/2001/XMLSchema#string">Australian Ocean Data Network Organisation Register</dc:source>
	<dc:publisher rdf:datatype="http://www.w3.org/2001/XMLSchema#string">eMarine Information Infrastructure (eMII)</dc:publisher>
	<skos:exactMatch rdf:resource="http://seadatanet.maris2.nl/v_edmo/print.asp?n_code=3790"/>
	<skos:topConceptOf rdf:resource="http://vocab.aodn.org.au/def/organisation/1"/>
	<skos:inScheme rdf:resource="http://vocab.aodn.org.au/def/organisation/1"/>
</rdf:Description>

<rdf:Description rdf:about="http://vocab.aodn.org.au/def/organisation/entity/322">
	<rdf:type rdf:resource="http://www.w3.org/2000/01/rdf-schema#Resource"/>
	<rdf:type rdf:resource="http://www.w3.org/2004/02/skos/core#Concept"/>
	<dcterms:creator rdf:datatype="http://www.w3.org/2001/XMLSchema#string">Natalia Atkins</dcterms:creator>
	<dcterms:created rdf:datatype="http://www.w3.org/2001/XMLSchema#dateTime">2015-07-28T10:38:15Z</dcterms:created>
	<skos:broadMatch rdf:resource="http://vocab.aodn.org.au/def/organisation_classes/category/4"/>
	<skos:prefLabel xml:lang="en">University of Miami</skos:prefLabel>
	<skos:altLabel xml:lang="en"></skos:altLabel>
	<skos:hiddenLabel xml:lang="en"></skos:hiddenLabel>
	<skos:definition xml:lang="en">The University of Miami is a private, nonsectarian university located in Coral Gables, Florida offering approximately 115 undergraduate, 114 master's, 51 doctoral, and two professional areas of study.</skos:definition>
	<dc:source rdf:datatype="http://www.w3.org/2001/XMLSchema#string">Australian Ocean Data Network Organisation Register</dc:source>
	<dc:publisher rdf:datatype="http://www.w3.org/2001/XMLSchema#string">eMarine Information Infrastructure (eMII)</dc:publisher>
	<skos:exactMatch rdf:resource="http://seadatanet.maris2.nl/v_edmo/print.asp?n_code=3829"/>
	<skos:narrower rdf:resource="http://vocab.aodn.org.au/def/organisation/entity/426"/>
	<skos:topConceptOf rdf:resource="http://vocab.aodn.org.au/def/organisation/1"/>
	<skos:inScheme rdf:resource="http://vocab.aodn.org.au/def/organisation/1"/>
</rdf:Description>

<rdf:Description rdf:about="http://vocab.aodn.org.au/def/organisation/entity/323">
	<rdf:type rdf:resource="http://www.w3.org/2000/01/rdf-schema#Resource"/>
	<rdf:type rdf:resource="http://www.w3.org/2004/02/skos/core#Concept"/>
	<dcterms:creator rdf:datatype="http://www.w3.org/2001/XMLSchema#string">Natalia Atkins</dcterms:creator>
	<dcterms:created rdf:datatype="http://www.w3.org/2001/XMLSchema#dateTime">2015-07-28T10:38:15Z</dcterms:created>
	<skos:broadMatch rdf:resource="http://vocab.aodn.org.au/def/organisation_classes/category/4"/>
	<skos:prefLabel xml:lang="en">University of Wisconsin-Madison (UW-Madison)</skos:prefLabel>
	<skos:altLabel xml:lang="en"></skos:altLabel>
	<skos:hiddenLabel xml:lang="en">UW-Madison</skos:hiddenLabel>
	<skos:definition xml:lang="en">The University of Wisconsin–Madison is a public research university located in Wisconsin. Founded when Wisconsin achieved statehood in 1848, UW–Madison is the official state university of Wisconsin, and the flagship campus of the University of Wisconsin System. It was the first public university established in Wisconsin and remains the oldest and largest public university in the state. It became a land-grant institution in 1866.</skos:definition>
	<dc:source rdf:datatype="http://www.w3.org/2001/XMLSchema#string">Australian Ocean Data Network Organisation Register</dc:source>
	<dc:publisher rdf:datatype="http://www.w3.org/2001/XMLSchema#string">eMarine Information Infrastructure (eMII)</dc:publisher>
	<skos:exactMatch rdf:resource="http://seadatanet.maris2.nl/v_edmo/print.asp?n_code=3840"/>
	<skos:narrower rdf:resource="http://vocab.aodn.org.au/def/organisation/entity/427"/>
	<skos:topConceptOf rdf:resource="http://vocab.aodn.org.au/def/organisation/1"/>
	<skos:inScheme rdf:resource="http://vocab.aodn.org.au/def/organisation/1"/>
</rdf:Description>

<rdf:Description rdf:about="http://vocab.aodn.org.au/def/organisation/entity/324">
	<rdf:type rdf:resource="http://www.w3.org/2000/01/rdf-schema#Resource"/>
	<rdf:type rdf:resource="http://www.w3.org/2004/02/skos/core#Concept"/>
	<dcterms:creator rdf:datatype="http://www.w3.org/2001/XMLSchema#string">Natalia Atkins</dcterms:creator>
	<dcterms:created rdf:datatype="http://www.w3.org/2001/XMLSchema#dateTime">2015-07-28T10:38:15Z</dcterms:created>
	<skos:broadMatch rdf:resource="http://vocab.aodn.org.au/def/organisation_classes/category/4"/>
	<skos:prefLabel xml:lang="en">Columbia University</skos:prefLabel>
	<skos:altLabel xml:lang="en"></skos:altLabel>
	<skos:hiddenLabel xml:lang="en"></skos:hiddenLabel>
	<skos:definition xml:lang="en">Columbia University was founded in 1754 as King's College by royal charter of King George II of England. It is the oldest institution of higher learning in the state of New York and the fifth oldest in the United States.</skos:definition>
	<dc:source rdf:datatype="http://www.w3.org/2001/XMLSchema#string">Australian Ocean Data Network Organisation Register</dc:source>
	<dc:publisher rdf:datatype="http://www.w3.org/2001/XMLSchema#string">eMarine Information Infrastructure (eMII)</dc:publisher>
	<skos:exactMatch rdf:resource="http://seadatanet.maris2.nl/v_edmo/print.asp?n_code=3533"/>
	<skos:narrower rdf:resource="http://vocab.aodn.org.au/def/organisation/entity/433"/>
	<skos:narrower rdf:resource="http://vocab.aodn.org.au/def/organisation/entity/434"/>
	<skos:topConceptOf rdf:resource="http://vocab.aodn.org.au/def/organisation/1"/>
	<skos:inScheme rdf:resource="http://vocab.aodn.org.au/def/organisation/1"/>
</rdf:Description>

<rdf:Description rdf:about="http://vocab.aodn.org.au/def/organisation/entity/325">
	<rdf:type rdf:resource="http://www.w3.org/2000/01/rdf-schema#Resource"/>
	<rdf:type rdf:resource="http://www.w3.org/2004/02/skos/core#Concept"/>
	<dcterms:creator rdf:datatype="http://www.w3.org/2001/XMLSchema#string">Natalia Atkins</dcterms:creator>
	<dcterms:created rdf:datatype="http://www.w3.org/2001/XMLSchema#dateTime">2015-07-28T10:38:15Z</dcterms:created>
	<skos:broadMatch rdf:resource="http://vocab.aodn.org.au/def/organisation_classes/category/4"/>
	<skos:prefLabel xml:lang="en">University of Washington (UW)</skos:prefLabel>
	<skos:altLabel xml:lang="en"></skos:altLabel>
	<skos:hiddenLabel xml:lang="en">UW</skos:hiddenLabel>
	<skos:definition xml:lang="en">The University of Washington (UW) is a public research university in Seattle, Washington. Founded in 1861, UW is one of the oldest universities on the West Coast. </skos:definition>
	<dc:source rdf:datatype="http://www.w3.org/2001/XMLSchema#string">Australian Ocean Data Network Organisation Register</dc:source>
	<dc:publisher rdf:datatype="http://www.w3.org/2001/XMLSchema#string">eMarine Information Infrastructure (eMII)</dc:publisher>
	<skos:exactMatch rdf:resource="http://seadatanet.maris2.nl/v_edmo/print.asp?n_code=3839"/>
	<skos:narrower rdf:resource="http://vocab.aodn.org.au/def/organisation/entity/428"/>
	<skos:narrower rdf:resource="http://vocab.aodn.org.au/def/organisation/entity/429"/>
	<skos:topConceptOf rdf:resource="http://vocab.aodn.org.au/def/organisation/1"/>
	<skos:inScheme rdf:resource="http://vocab.aodn.org.au/def/organisation/1"/>
</rdf:Description>

<rdf:Description rdf:about="http://vocab.aodn.org.au/def/organisation/entity/326">
	<rdf:type rdf:resource="http://www.w3.org/2000/01/rdf-schema#Resource"/>
	<rdf:type rdf:resource="http://www.w3.org/2004/02/skos/core#Concept"/>
	<dcterms:creator rdf:datatype="http://www.w3.org/2001/XMLSchema#string">Natalia Atkins</dcterms:creator>
	<dcterms:created rdf:datatype="http://www.w3.org/2001/XMLSchema#dateTime">2015-07-28T10:38:15Z</dcterms:created>
	<skos:broadMatch rdf:resource="http://vocab.aodn.org.au/def/organisation_classes/category/4"/>
	<skos:prefLabel xml:lang="en">The College of William and Mary</skos:prefLabel>
	<skos:altLabel xml:lang="en"></skos:altLabel>
	<skos:hiddenLabel xml:lang="en"></skos:hiddenLabel>
	<skos:definition xml:lang="en">The College of William and Mary in Virginia is a public research university located in Williamsburg, Virginia, United States.</skos:definition>
	<dc:source rdf:datatype="http://www.w3.org/2001/XMLSchema#string">Australian Ocean Data Network Organisation Register</dc:source>
	<dc:publisher rdf:datatype="http://www.w3.org/2001/XMLSchema#string">eMarine Information Infrastructure (eMII)</dc:publisher>
	<skos:exactMatch rdf:resource="http://seadatanet.maris2.nl/v_edmo/print.asp?n_code=3633"/>
	<skos:narrower rdf:resource="http://vocab.aodn.org.au/def/organisation/entity/430"/>
	<skos:topConceptOf rdf:resource="http://vocab.aodn.org.au/def/organisation/1"/>
	<skos:inScheme rdf:resource="http://vocab.aodn.org.au/def/organisation/1"/>
</rdf:Description>

<rdf:Description rdf:about="http://vocab.aodn.org.au/def/organisation/entity/327">
	<rdf:type rdf:resource="http://www.w3.org/2000/01/rdf-schema#Resource"/>
	<rdf:type rdf:resource="http://www.w3.org/2004/02/skos/core#Concept"/>
	<dcterms:creator rdf:datatype="http://www.w3.org/2001/XMLSchema#string">Natalia Atkins</dcterms:creator>
	<dcterms:created rdf:datatype="http://www.w3.org/2001/XMLSchema#dateTime">2015-07-28T10:38:15Z</dcterms:created>
	<skos:broadMatch rdf:resource="http://vocab.aodn.org.au/def/organisation_classes/category/4"/>
	<skos:prefLabel xml:lang="en">University of Ottawa</skos:prefLabel>
	<skos:altLabel xml:lang="en"></skos:altLabel>
	<skos:hiddenLabel xml:lang="en"></skos:hiddenLabel>
	<skos:definition xml:lang="en">The University of Ottawa (uOttawa or U of O ) (French: Université d'Ottawa) is a bilingual public research university in Ottawa, Ontario, Canada.</skos:definition>
	<dc:source rdf:datatype="http://www.w3.org/2001/XMLSchema#string">Australian Ocean Data Network Organisation Register</dc:source>
	<dc:publisher rdf:datatype="http://www.w3.org/2001/XMLSchema#string">eMarine Information Infrastructure (eMII)</dc:publisher>
	<skos:exactMatch rdf:resource="http://seadatanet.maris2.nl/v_edmo/print.asp?n_code=3721"/>
	<skos:narrower rdf:resource="http://vocab.aodn.org.au/def/organisation/entity/363"/>
	<skos:topConceptOf rdf:resource="http://vocab.aodn.org.au/def/organisation/1"/>
	<skos:inScheme rdf:resource="http://vocab.aodn.org.au/def/organisation/1"/>
</rdf:Description>

<rdf:Description rdf:about="http://vocab.aodn.org.au/def/organisation/entity/328">
	<rdf:type rdf:resource="http://www.w3.org/2000/01/rdf-schema#Resource"/>
	<rdf:type rdf:resource="http://www.w3.org/2004/02/skos/core#Concept"/>
	<dcterms:creator rdf:datatype="http://www.w3.org/2001/XMLSchema#string">Natalia Atkins</dcterms:creator>
	<dcterms:created rdf:datatype="http://www.w3.org/2001/XMLSchema#dateTime">2015-07-28T10:38:15Z</dcterms:created>
	<skos:broadMatch rdf:resource="http://vocab.aodn.org.au/def/organisation_classes/category/4"/>
	<skos:prefLabel xml:lang="en">University of California, Los Angeles (UCLA)</skos:prefLabel>
	<skos:altLabel xml:lang="en"></skos:altLabel>
	<skos:hiddenLabel xml:lang="en">UCLA</skos:hiddenLabel>
	<skos:definition xml:lang="en">The University of California, Los Angeles, is a public research university located in the Westwood neighborhood of Los Angeles, California, United States. Founded in 1919, it is the second-oldest campus of the University of California system.</skos:definition>
	<dc:source rdf:datatype="http://www.w3.org/2001/XMLSchema#string">Australian Ocean Data Network Organisation Register</dc:source>
	<dc:publisher rdf:datatype="http://www.w3.org/2001/XMLSchema#string">eMarine Information Infrastructure (eMII)</dc:publisher>
	<skos:exactMatch rdf:resource="http://seadatanet.maris2.nl/v_edmo/print.asp?n_code=3646"/>
	<skos:narrower rdf:resource="http://vocab.aodn.org.au/def/organisation/entity/435"/>
	<skos:topConceptOf rdf:resource="http://vocab.aodn.org.au/def/organisation/1"/>
	<skos:inScheme rdf:resource="http://vocab.aodn.org.au/def/organisation/1"/>
</rdf:Description>

<rdf:Description rdf:about="http://vocab.aodn.org.au/def/organisation/entity/329">
	<rdf:type rdf:resource="http://www.w3.org/2000/01/rdf-schema#Resource"/>
	<rdf:type rdf:resource="http://www.w3.org/2004/02/skos/core#Concept"/>
	<dcterms:creator rdf:datatype="http://www.w3.org/2001/XMLSchema#string">Natalia Atkins</dcterms:creator>
	<dcterms:created rdf:datatype="http://www.w3.org/2001/XMLSchema#dateTime">2015-07-28T10:38:15Z</dcterms:created>
	<skos:broadMatch rdf:resource="http://vocab.aodn.org.au/def/organisation_classes/category/4"/>
	<skos:prefLabel xml:lang="en">San Francisco State University (SFSU)</skos:prefLabel>
	<skos:altLabel xml:lang="en"></skos:altLabel>
	<skos:hiddenLabel xml:lang="en">SFSU</skos:hiddenLabel>
	<skos:definition xml:lang="en">San Francisco State University (SFSU) is a public comprehensive university located in San Francisco, California. As part of the 23-campus California State University system, the university offers 118 different Bachelor's degrees, 94 Master's degrees, and 5 Doctoral degrees.</skos:definition>
	<dc:source rdf:datatype="http://www.w3.org/2001/XMLSchema#string">Australian Ocean Data Network Organisation Register</dc:source>
	<dc:publisher rdf:datatype="http://www.w3.org/2001/XMLSchema#string">eMarine Information Infrastructure (eMII)</dc:publisher>
	<skos:exactMatch rdf:resource="http://seadatanet.maris2.nl/v_edmo/print.asp?n_code=3810"/>
	<skos:narrower rdf:resource="http://vocab.aodn.org.au/def/organisation/entity/439"/>
	<skos:topConceptOf rdf:resource="http://vocab.aodn.org.au/def/organisation/1"/>
	<skos:inScheme rdf:resource="http://vocab.aodn.org.au/def/organisation/1"/>
</rdf:Description>

<rdf:Description rdf:about="http://vocab.aodn.org.au/def/organisation/entity/330">
	<rdf:type rdf:resource="http://www.w3.org/2000/01/rdf-schema#Resource"/>
	<rdf:type rdf:resource="http://www.w3.org/2004/02/skos/core#Concept"/>
	<dcterms:creator rdf:datatype="http://www.w3.org/2001/XMLSchema#string">Natalia Atkins</dcterms:creator>
	<dcterms:created rdf:datatype="http://www.w3.org/2001/XMLSchema#dateTime">2015-07-28T10:38:15Z</dcterms:created>
	<skos:broadMatch rdf:resource="http://vocab.aodn.org.au/def/organisation_classes/category/4"/>
	<skos:prefLabel xml:lang="en">University of Illinois at Chicago (UIC)</skos:prefLabel>
	<skos:altLabel xml:lang="en"></skos:altLabel>
	<skos:hiddenLabel xml:lang="en">UIC</skos:hiddenLabel>
	<skos:definition xml:lang="en">The University of Illinois at Chicago, or UIC, is a state-funded public research university located in Chicago, Illinois, United States.</skos:definition>
	<dc:source rdf:datatype="http://www.w3.org/2001/XMLSchema#string">Australian Ocean Data Network Organisation Register</dc:source>
	<dc:publisher rdf:datatype="http://www.w3.org/2001/XMLSchema#string">eMarine Information Infrastructure (eMII)</dc:publisher>
	<skos:exactMatch rdf:resource="http://seadatanet.maris2.nl/v_edmo/print.asp?n_code=3649"/>
	<skos:narrower rdf:resource="http://vocab.aodn.org.au/def/organisation/entity/441"/>
	<skos:topConceptOf rdf:resource="http://vocab.aodn.org.au/def/organisation/1"/>
	<skos:inScheme rdf:resource="http://vocab.aodn.org.au/def/organisation/1"/>
</rdf:Description>

<rdf:Description rdf:about="http://vocab.aodn.org.au/def/organisation/entity/331">
	<rdf:type rdf:resource="http://www.w3.org/2000/01/rdf-schema#Resource"/>
	<rdf:type rdf:resource="http://www.w3.org/2004/02/skos/core#Concept"/>
	<dcterms:creator rdf:datatype="http://www.w3.org/2001/XMLSchema#string">Natalia Atkins</dcterms:creator>
	<dcterms:created rdf:datatype="http://www.w3.org/2001/XMLSchema#dateTime">2015-07-28T10:38:15Z</dcterms:created>
	<skos:broadMatch rdf:resource="http://vocab.aodn.org.au/def/organisation_classes/category/4"/>
	<skos:prefLabel xml:lang="en">Nova Southeastern University (NSU)</skos:prefLabel>
	<skos:altLabel xml:lang="en"></skos:altLabel>
	<skos:hiddenLabel xml:lang="en">NSU</skos:hiddenLabel>
	<skos:definition xml:lang="en">Nova Southeastern University, formerly referred to as Nova and now commonly called NSU,is a private, coeducational, nonsectarian, research university located in Broward County, Florida, United States.</skos:definition>
	<dc:source rdf:datatype="http://www.w3.org/2001/XMLSchema#string">Australian Ocean Data Network Organisation Register</dc:source>
	<dc:publisher rdf:datatype="http://www.w3.org/2001/XMLSchema#string">eMarine Information Infrastructure (eMII)</dc:publisher>
	<skos:exactMatch rdf:resource="http://seadatanet.maris2.nl/v_edmo/print.asp?n_code=3597"/>
	<skos:narrower rdf:resource="http://vocab.aodn.org.au/def/organisation/entity/442"/>
	<skos:topConceptOf rdf:resource="http://vocab.aodn.org.au/def/organisation/1"/>
	<skos:inScheme rdf:resource="http://vocab.aodn.org.au/def/organisation/1"/>
</rdf:Description>

<rdf:Description rdf:about="http://vocab.aodn.org.au/def/organisation/entity/332">
	<rdf:type rdf:resource="http://www.w3.org/2000/01/rdf-schema#Resource"/>
	<rdf:type rdf:resource="http://www.w3.org/2004/02/skos/core#Concept"/>
	<dcterms:creator rdf:datatype="http://www.w3.org/2001/XMLSchema#string">Natalia Atkins</dcterms:creator>
	<dcterms:created rdf:datatype="http://www.w3.org/2001/XMLSchema#dateTime">2015-07-28T10:38:15Z</dcterms:created>
	<dcterms:created rdf:datatype="http://www.w3.org/2001/XMLSchema#dateTime">2016-01-07T10:38:15Z</dcterms:created>
	<skos:broadMatch rdf:resource="http://vocab.aodn.org.au/def/organisation_classes/category/4"/>
	<skos:prefLabel xml:lang="en">School of Ocean and Earth Science, University of Southampton</skos:prefLabel>
	<skos:altLabel xml:lang="en">School of Ocean and Earth Science</skos:altLabel>
	<skos:hiddenLabel xml:lang="en"></skos:hiddenLabel>
	<skos:definition xml:lang="en"></skos:definition>
	<dc:source rdf:datatype="http://www.w3.org/2001/XMLSchema#string">Australian Ocean Data Network Organisation Register</dc:source>
	<dc:publisher rdf:datatype="http://www.w3.org/2001/XMLSchema#string">eMarine Information Infrastructure (eMII)</dc:publisher>
	<dc:publisher rdf:datatype="http://www.w3.org/2001/XMLSchema#string">eMarine Information Infrastructure (eMMI)</dc:publisher>
	<skos:exactMatch rdf:resource="http://seadatanet.maris2.nl/v_edmo/print.asp?n_code=1801"/>
	<skos:topConceptOf rdf:resource="http://vocab.aodn.org.au/def/organisation/1"/>
	<skos:inScheme rdf:resource="http://vocab.aodn.org.au/def/organisation/1"/>
	<skos:broader rdf:resource="http://vocab.aodn.org.au/def/organisation/entity/449"/>
</rdf:Description>

<rdf:Description rdf:about="http://vocab.aodn.org.au/def/organisation/entity/333">
	<rdf:type rdf:resource="http://www.w3.org/2000/01/rdf-schema#Resource"/>
	<rdf:type rdf:resource="http://www.w3.org/2004/02/skos/core#Concept"/>
	<dcterms:modified rdf:datatype="http://www.w3.org/2001/XMLSchema#dateTime">2015-08-06T00:03:14Z</dcterms:modified>
	<dcterms:creator rdf:datatype="http://www.w3.org/2001/XMLSchema#string">Natalia Atkins</dcterms:creator>
	<dcterms:created rdf:datatype="http://www.w3.org/2001/XMLSchema#dateTime">2015-07-28T10:38:15Z</dcterms:created>
	<dcterms:contributor rdf:datatype="http://www.w3.org/2001/XMLSchema#string">Natalia_Atkins</dcterms:contributor>
	<skos:broadMatch rdf:resource="http://vocab.aodn.org.au/def/organisation_classes/category/4"/>
	<skos:prefLabel xml:lang="en">University of Groningen</skos:prefLabel>
	<skos:altLabel xml:lang="en"></skos:altLabel>
	<skos:hiddenLabel xml:lang="en">RUG</skos:hiddenLabel>
	<skos:definition xml:lang="en">The University of Groningen has a long academic tradition extending back to 1614, which makes Groningen the oldest university in the Netherlands after Leiden. Many very talented people in a variety of disciplines have studied or worked at the university during the 390 years of its existence, including a Nobel Prize winner, the first female University student in the Netherlands and the first female lecturer, the first Dutch astronaut and the first president of the European Bank. They share their academic roots with more than 200,000 other people who have attended the University of Groningen as students, lecturers or research workers. The young University of Groningen was already an outstanding example of an international community in the seventeenth century. Almost half of the students and lecturers came from outside the Netherlands – the first Rector Magnificus, Ubbo Emmius, was German, for instance – but at the same time there was already a close relationship between the university and the city and the surrounding region. The founding of the university – at that time still a college of higher education – was an initiative taken by the Regional Assembly of the city of Groningen and the Ommelanden, or surrounding region. There were four faculties – Theology, Law, Medicine and Philosophy. The first 75 years of its existence were very fruitful for the university with about 100 students enrolling every year. The development of the university came to a standstill at the end of the seventeenth and during the eighteenth century because of theological differences of opinion, a difficult relationship with the Regional Assembly and political problems that included the siege of the city by ‘Bommen Berend’ in 1672. On average two to three hundred students were registered with the university at any one time during this period. Petrus Camper, though, was a shining academic example during the second half of the eighteenth century and was famous far beyond the city limits as an anatomist, a fighter against rinderpest and the founder of the first outpatient’s clinic for surgical medicine. Opportunities and threats followed on each other’s heels during the nineteenth century. In 1815, at the same time as Leiden and Utrecht, the university gained recognition as a national college of higher education, but this was followed by discussions about closure. The situation improved markedly when a new main university building, the Academiegebouw, was constructed in 1850, a building that was largely financed by the people of Groningen. This made the fire that completely destroyed this building in 1906 even more poignant. In the meantime, the Higher Education Act of 1876 had radically improved the position of the university, which was renamed the Rijksuniversiteit Groningen (RUG). Teaching now took place in Dutch as well as in Latin and the University was given a research as well as an educational duty. This laid the foundations for the present research university. The University of Groningen developed apace during the first decades of the twentieth century. The number of faculties and courses grew steadily while the number of students showed an explosive growth. When the university celebrated its first 300 years in 1914 there were 611 registered students; this had already grown to 1000 by 1924. After a drop back during the Depression, and in particular during the Second World War, the number of students grew rapidly from 1945 to reach 20,000 in 1994. At the present time there are about 21,000 students registered at the University of Groningen with the number of foreign students again growing steadily, and following the tradition set by the first Rector Magnificus, the number of German students and researchers has grown strongly in recent years.</skos:definition>
	<dc:source rdf:datatype="http://www.w3.org/2001/XMLSchema#string">Australian Ocean Data Network Organisation Register</dc:source>
	<dc:publisher rdf:datatype="http://www.w3.org/2001/XMLSchema#string">eMarine Information Infrastructure (eMII)</dc:publisher>
	<skos:exactMatch rdf:resource="http://seadatanet.maris2.nl/v_edmo/print.asp?n_code=1596"/>
	<skos:narrower rdf:resource="http://vocab.aodn.org.au/def/organisation/entity/357"/>
	<skos:topConceptOf rdf:resource="http://vocab.aodn.org.au/def/organisation/1"/>
	<skos:inScheme rdf:resource="http://vocab.aodn.org.au/def/organisation/1"/>
</rdf:Description>

<rdf:Description rdf:about="http://vocab.aodn.org.au/def/organisation/entity/334">
	<rdf:type rdf:resource="http://www.w3.org/2000/01/rdf-schema#Resource"/>
	<rdf:type rdf:resource="http://www.w3.org/2004/02/skos/core#Concept"/>
	<dcterms:creator rdf:datatype="http://www.w3.org/2001/XMLSchema#string">Natalia Atkins</dcterms:creator>
	<dcterms:created rdf:datatype="http://www.w3.org/2001/XMLSchema#dateTime">2015-07-28T10:38:15Z</dcterms:created>
	<skos:broadMatch rdf:resource="http://vocab.aodn.org.au/def/organisation_classes/category/4"/>
	<skos:prefLabel xml:lang="en">University of Bordeaux I</skos:prefLabel>
	<skos:altLabel xml:lang="en"></skos:altLabel>
	<skos:hiddenLabel xml:lang="en"></skos:hiddenLabel>
	<skos:definition xml:lang="en">Sciences and Technologies at the service of Mankind and Environment.</skos:definition>
	<dc:source rdf:datatype="http://www.w3.org/2001/XMLSchema#string">Australian Ocean Data Network Organisation Register</dc:source>
	<dc:publisher rdf:datatype="http://www.w3.org/2001/XMLSchema#string">eMarine Information Infrastructure (eMII)</dc:publisher>
	<skos:exactMatch rdf:resource="http://seadatanet.maris2.nl/v_edmo/print.asp?n_code=2884"/>
	<skos:topConceptOf rdf:resource="http://vocab.aodn.org.au/def/organisation/1"/>
	<skos:inScheme rdf:resource="http://vocab.aodn.org.au/def/organisation/1"/>
</rdf:Description>

<rdf:Description rdf:about="http://vocab.aodn.org.au/def/organisation/entity/335">
	<rdf:type rdf:resource="http://www.w3.org/2000/01/rdf-schema#Resource"/>
	<rdf:type rdf:resource="http://www.w3.org/2004/02/skos/core#Concept"/>
	<dcterms:creator rdf:datatype="http://www.w3.org/2001/XMLSchema#string">Natalia Atkins</dcterms:creator>
	<dcterms:created rdf:datatype="http://www.w3.org/2001/XMLSchema#dateTime">2015-07-29T10:38:15Z</dcterms:created>
	<skos:broadMatch rdf:resource="http://vocab.aodn.org.au/def/organisation_classes/category/4"/>
	<skos:prefLabel xml:lang="en">University of Colorado at Boulder</skos:prefLabel>
	<skos:altLabel xml:lang="en"></skos:altLabel>
	<skos:hiddenLabel xml:lang="en"></skos:hiddenLabel>
	<skos:definition xml:lang="en">The University of Colorado Boulder is a public research university, and the flagship university of the University of Colorado system. The organization was founded five months before Colorado was admitted to the union in 1876.</skos:definition>
	<dc:source rdf:datatype="http://www.w3.org/2001/XMLSchema#string">Australian Ocean Data Network Organisation Register</dc:source>
	<dc:publisher rdf:datatype="http://www.w3.org/2001/XMLSchema#string">eMarine Information Infrastructure (eMII)</dc:publisher>
	<skos:exactMatch rdf:resource="http://seadatanet.maris2.nl/v_edmo/print.asp?n_code=3823"/>
	<skos:narrower rdf:resource="http://vocab.aodn.org.au/def/organisation/entity/336"/>
	<skos:topConceptOf rdf:resource="http://vocab.aodn.org.au/def/organisation/1"/>
	<skos:inScheme rdf:resource="http://vocab.aodn.org.au/def/organisation/1"/>
</rdf:Description>

<rdf:Description rdf:about="http://vocab.aodn.org.au/def/organisation/entity/337">
	<rdf:type rdf:resource="http://www.w3.org/2000/01/rdf-schema#Resource"/>
	<rdf:type rdf:resource="http://www.w3.org/2004/02/skos/core#Concept"/>
	<dcterms:creator rdf:datatype="http://www.w3.org/2001/XMLSchema#string">Natalia Atkins</dcterms:creator>
	<dcterms:created rdf:datatype="http://www.w3.org/2001/XMLSchema#dateTime">2015-07-29T10:38:15Z</dcterms:created>
	<skos:broadMatch rdf:resource="http://vocab.aodn.org.au/def/organisation_classes/category/4"/>
	<skos:prefLabel xml:lang="en">Stanford University</skos:prefLabel>
	<skos:altLabel xml:lang="en"></skos:altLabel>
	<skos:hiddenLabel xml:lang="en"></skos:hiddenLabel>
	<skos:definition xml:lang="en">Stanford University is a private research university in Stanford, California, and one of the world's most prestigious institutions with the highest undergraduate selectivity and fundraising performance in the United States. Stanford was founded in 1885 by Leland Stanford, former governor of and U.S. senator from California and leading railroad tycoon, and his wife, Jane Lathrop Stanford.</skos:definition>
	<dc:source rdf:datatype="http://www.w3.org/2001/XMLSchema#string">Australian Ocean Data Network Organisation Register</dc:source>
	<dc:publisher rdf:datatype="http://www.w3.org/2001/XMLSchema#string">eMarine Information Infrastructure (eMII)</dc:publisher>
	<skos:exactMatch rdf:resource="http://seadatanet.maris2.nl/v_edmo/print.asp?n_code=3812"/>
	<skos:narrower rdf:resource="http://vocab.aodn.org.au/def/organisation/entity/338"/>
	<skos:topConceptOf rdf:resource="http://vocab.aodn.org.au/def/organisation/1"/>
	<skos:inScheme rdf:resource="http://vocab.aodn.org.au/def/organisation/1"/>
</rdf:Description>

<rdf:Description rdf:about="http://vocab.aodn.org.au/def/organisation/entity/339">
	<rdf:type rdf:resource="http://www.w3.org/2000/01/rdf-schema#Resource"/>
	<rdf:type rdf:resource="http://www.w3.org/2004/02/skos/core#Concept"/>
	<dcterms:creator rdf:datatype="http://www.w3.org/2001/XMLSchema#string">Natalia Atkins</dcterms:creator>
	<dcterms:created rdf:datatype="http://www.w3.org/2001/XMLSchema#dateTime">2015-07-29T10:38:15Z</dcterms:created>
	<skos:broadMatch rdf:resource="http://vocab.aodn.org.au/def/organisation_classes/category/4"/>
	<skos:prefLabel xml:lang="en">University of Portsmouth</skos:prefLabel>
	<skos:altLabel xml:lang="en"></skos:altLabel>
	<skos:hiddenLabel xml:lang="en"></skos:hiddenLabel>
	<skos:definition xml:lang="en">The University of Portsmouth is a leading modern university with a strong reputation for teaching and research. Many of our academics are international leaders in their fields and our students learn from experts who are pushing forward the boundaries of knowledge. Our 19,000 students, including 3,000 from over 100 countries, are supported by over 3,000 staff. We offer superb facilities in a vibrant waterfront location – a university by the sea but in the heart of one of Britain's most historic cities. The main Guildhall campus, dotted around the city centre, has undergone extensive redevelopment with the establishment of a University Quarter. The University of Portsmouth is a research-active university with wide range of activities across many subjects. Areas of international excellence include the Institute of Biomedical and Biomolecular Sciences, the Centre for European and International Research and the Institute of Cosmology and Gravitation. We also have well-developed strengths in applied research with business, industry, and the public and voluntary sectors. We are proud of our teaching record, receiving the highest possible rating in the most recent Quality Assurance Agency audit.  The 2011 National Students Survey places Portsmouth within the top 30 mainstream English universities for overall satisfaction with 85 per cent of full-time students reporting being satisfied or very satisfied with their course, higher than the national average of 83 per cent. Applications to the University of Portsmouth increased by 20 per cent (28,448) in 2010 and by 26 per cent (23,632) in 2009 and we received a 13 per cent increase in research funding following success in the 2008 Research Assessment Exercise (RAE). The average increase across the sector was 8 per cent. The University has excellent links with industry and a strong record of student employability. The University recruitment agency, Purple Door Careers and Recruitment, offers a wide range of careers resources, skills workshops, careers guidance, and employer events to support students and graduates in gaining graduate employment. Our experienced recruitment consultants work in collaboration with local and national businesses, charities, and organisations to source graduate opportunities and assist graduates at every step of the recruitment process. We have a clear focus on Enterprise, and our Centre for Enterprise, established in 2000, aims to inspire Portsmouth students to learn and succeed in entrepreneurship, offering free training and mentoring to both former and current students. Arts and Humanities are additional areas of strength; the Faculty of Creative and Cultural Industries meets the need for talented graduates of the fast-growing creative and cultural sector of the regional and national economy.</skos:definition>
	<dc:source rdf:datatype="http://www.w3.org/2001/XMLSchema#string">Australian Ocean Data Network Organisation Register</dc:source>
	<dc:publisher rdf:datatype="http://www.w3.org/2001/XMLSchema#string">eMarine Information Infrastructure (eMII)</dc:publisher>
	<skos:exactMatch rdf:resource="http://seadatanet.maris2.nl/v_edmo/print.asp?n_code=2924"/>
	<skos:narrower rdf:resource="http://vocab.aodn.org.au/def/organisation/entity/340"/>
	<skos:topConceptOf rdf:resource="http://vocab.aodn.org.au/def/organisation/1"/>
	<skos:inScheme rdf:resource="http://vocab.aodn.org.au/def/organisation/1"/>
</rdf:Description>

<rdf:Description rdf:about="http://vocab.aodn.org.au/def/organisation/entity/341">
	<rdf:type rdf:resource="http://www.w3.org/2000/01/rdf-schema#Resource"/>
	<rdf:type rdf:resource="http://www.w3.org/2004/02/skos/core#Concept"/>
	<dcterms:creator rdf:datatype="http://www.w3.org/2001/XMLSchema#string">Natalia Atkins</dcterms:creator>
	<dcterms:created rdf:datatype="http://www.w3.org/2001/XMLSchema#dateTime">2015-07-29T10:38:15Z</dcterms:created>
	<skos:broadMatch rdf:resource="http://vocab.aodn.org.au/def/organisation_classes/category/4"/>
	<skos:prefLabel xml:lang="en">Institute F.-A. Forel, University of Geneva</skos:prefLabel>
	<skos:altLabel xml:lang="en">Institute F.-A. Forel</skos:altLabel>
	<skos:hiddenLabel xml:lang="en"></skos:hiddenLabel>
	<skos:definition xml:lang="en">The Institute F.-A. Forel , in its new configuration meets academically Faculty of teachers and researchers of Sciences responsible for the development of natural environmental sciences within the University. areas:  Limnology and environmental geology, Environmental Geochemistry - Ecotoxicology, Ecology and Aquatic Biology,  Energy,  Environmental Physical Chemistry,  Climatology, Spatial analysis and modeling, and Botany and floristic.</skos:definition>
	<dc:source rdf:datatype="http://www.w3.org/2001/XMLSchema#string">Australian Ocean Data Network Organisation Register</dc:source>
	<dc:publisher rdf:datatype="http://www.w3.org/2001/XMLSchema#string">eMarine Information Infrastructure (eMII)</dc:publisher>
	<skos:exactMatch rdf:resource="http://seadatanet.maris2.nl/v_edmo/print.asp?n_code=1987"/>
	<skos:topConceptOf rdf:resource="http://vocab.aodn.org.au/def/organisation/1"/>
	<skos:inScheme rdf:resource="http://vocab.aodn.org.au/def/organisation/1"/>
</rdf:Description>

<rdf:Description rdf:about="http://vocab.aodn.org.au/def/organisation/entity/343">
	<rdf:type rdf:resource="http://www.w3.org/2000/01/rdf-schema#Resource"/>
	<rdf:type rdf:resource="http://www.w3.org/2004/02/skos/core#Concept"/>
	<dcterms:creator rdf:datatype="http://www.w3.org/2001/XMLSchema#string">Natalia Atkins</dcterms:creator>
	<dcterms:created rdf:datatype="http://www.w3.org/2001/XMLSchema#dateTime">2015-08-04T10:38:15Z</dcterms:created>
	<skos:broadMatch rdf:resource="http://vocab.aodn.org.au/def/organisation_classes/category/5"/>
	<skos:prefLabel xml:lang="en">Microalgal Services</skos:prefLabel>
	<skos:altLabel xml:lang="en"></skos:altLabel>
	<skos:hiddenLabel xml:lang="en"></skos:hiddenLabel>
	<skos:definition xml:lang="en">Microalgal Services is a specialist Melbourne based laboratory whose core business is the routine monitoring and identification of marine and estuarine phytoplankton species.</skos:definition>
	<dc:source rdf:datatype="http://www.w3.org/2001/XMLSchema#string">Australian Ocean Data Network Organisation Register</dc:source>
	<dc:publisher rdf:datatype="http://www.w3.org/2001/XMLSchema#string">eMarine Information Infrastructure (eMII)</dc:publisher>
	<skos:exactMatch rdf:resource="http://seadatanet.maris2.nl/v_edmo/print.asp?n_code=4366"/>
	<skos:topConceptOf rdf:resource="http://vocab.aodn.org.au/def/organisation/1"/>
	<skos:inScheme rdf:resource="http://vocab.aodn.org.au/def/organisation/1"/>
</rdf:Description>

<rdf:Description rdf:about="http://vocab.aodn.org.au/def/organisation/entity/344">
	<rdf:type rdf:resource="http://www.w3.org/2000/01/rdf-schema#Resource"/>
	<rdf:type rdf:resource="http://www.w3.org/2004/02/skos/core#Concept"/>
	<dcterms:creator rdf:datatype="http://www.w3.org/2001/XMLSchema#string">Natalia Atkins</dcterms:creator>
	<dcterms:created rdf:datatype="http://www.w3.org/2001/XMLSchema#dateTime">2015-08-04T10:38:15Z</dcterms:created>
	<skos:broadMatch rdf:resource="http://vocab.aodn.org.au/def/organisation_classes/category/2"/>
	<skos:prefLabel xml:lang="en">Department of Environment and Climate Change (DECC), New South Wales Government</skos:prefLabel>
	<skos:altLabel xml:lang="en">Department of Environment and Climate Change (DECC)</skos:altLabel>
	<skos:hiddenLabel xml:lang="en">DECC</skos:hiddenLabel>
	<skos:definition xml:lang="en">This department became part of the former Department of Environment, Climate Change and Water (DECCW). After 2011, DECCW was broken up with its responsibilities split between the new Office of Environment and Heritage and the residual functions managed by the Industry, Innovation and Investment Division of the Department of Trade and Investment, Regional Infrastructure and Services. (Courtesy of Wikipedia)</skos:definition>
	<dc:source rdf:datatype="http://www.w3.org/2001/XMLSchema#string">Australian Ocean Data Network Organisation Register</dc:source>
	<dc:publisher rdf:datatype="http://www.w3.org/2001/XMLSchema#string">eMarine Information Infrastructure (eMMI)</dc:publisher>
	<skos:topConceptOf rdf:resource="http://vocab.aodn.org.au/def/organisation/1"/>
	<skos:inScheme rdf:resource="http://vocab.aodn.org.au/def/organisation/1"/>
	<skos:scopeNote xml:lang="en">Organisation no longer exists</skos:scopeNote>
	<skos:scopeNote xml:lang="en">Organisation no longer exists. Replaced by http://vocab.aodn.org.au/def/organisation/entity/345</skos:scopeNote>
	<dcterms:isReplacedBy rdf:resource="http://vocab.aodn.org.au/def/organisation/entity/345"/>
	<dcterms:isReplacedBy xml:lang="en">Office of Environment and Heritage (OEH), New South Wales Government</dcterms:isReplacedBy>
</rdf:Description>

<rdf:Description rdf:about="http://vocab.aodn.org.au/def/organisation/entity/345">
	<rdf:type rdf:resource="http://www.w3.org/2000/01/rdf-schema#Resource"/>
	<rdf:type rdf:resource="http://www.w3.org/2004/02/skos/core#Concept"/>
	<dcterms:creator rdf:datatype="http://www.w3.org/2001/XMLSchema#string">Natalia Atkins</dcterms:creator>
	<dcterms:created rdf:datatype="http://www.w3.org/2001/XMLSchema#dateTime">2015-08-04T10:38:15Z</dcterms:created>
	<skos:broadMatch rdf:resource="http://vocab.aodn.org.au/def/organisation_classes/category/2"/>
	<skos:prefLabel xml:lang="en">Office of Environment and Heritage (OEH), New South Wales Government</skos:prefLabel>
	<skos:altLabel xml:lang="en">Office of Environment and Heritage (OEH)</skos:altLabel>
	<skos:hiddenLabel xml:lang="en">OEH</skos:hiddenLabel>
	<skos:definition xml:lang="en">The Office of Environment and Heritage (OEH) is a separate agency within the Planning and Environment cluster. OEH was formed on 4 April 2011 and works to protect and conserve the NSW environment, including the natural environment, Aboriginal country, culture and heritage and our built heritage, and manages NSW national parks and reserves.</skos:definition>
	<dc:source rdf:datatype="http://www.w3.org/2001/XMLSchema#string">Australian Ocean Data Network Organisation Register</dc:source>
	<dc:publisher rdf:datatype="http://www.w3.org/2001/XMLSchema#string">eMarine Information Infrastructure (eMMI)</dc:publisher>
	<skos:exactMatch rdf:resource="http://seadatanet.maris2.nl/v_edmo/print.asp?n_code=4364"/>
	<skos:topConceptOf rdf:resource="http://vocab.aodn.org.au/def/organisation/1"/>
	<skos:inScheme rdf:resource="http://vocab.aodn.org.au/def/organisation/1"/>
	<skos:scopeNote xml:lang="en">Replaces http://vocab.aodn.org.au/def/organisation/entity/344</skos:scopeNote>
	<dcterms:replaces rdf:resource="http://vocab.aodn.org.au/def/organisation/entity/344"/>
	<dcterms:replaces xml:lang="en">Department of Environment and Climate Change (DECC), New South Wales Government</dcterms:replaces>
</rdf:Description>

<rdf:Description rdf:about="http://vocab.aodn.org.au/def/organisation/entity/346">
	<rdf:type rdf:resource="http://www.w3.org/2000/01/rdf-schema#Resource"/>
	<rdf:type rdf:resource="http://www.w3.org/2004/02/skos/core#Concept"/>
	<dcterms:creator rdf:datatype="http://www.w3.org/2001/XMLSchema#string">Natalia Atkins</dcterms:creator>
	<dcterms:created rdf:datatype="http://www.w3.org/2001/XMLSchema#dateTime">2015-08-04T10:38:15Z</dcterms:created>
	<skos:broadMatch rdf:resource="http://vocab.aodn.org.au/def/organisation_classes/category/2"/>
	<skos:prefLabel xml:lang="en">Food Authority, New South Wales Government</skos:prefLabel>
	<skos:altLabel xml:lang="en">Food Authority</skos:altLabel>
	<skos:hiddenLabel xml:lang="en"></skos:hiddenLabel>
	<skos:definition xml:lang="en">The NSW Food Authority is the government organisation that helps ensure food in NSW is safe and correctly labelled.</skos:definition>
	<dc:source rdf:datatype="http://www.w3.org/2001/XMLSchema#string">Australian Ocean Data Network Organisation Register</dc:source>
	<dc:publisher rdf:datatype="http://www.w3.org/2001/XMLSchema#string">eMarine Information Infrastructure (eMMI)</dc:publisher>
	<skos:exactMatch rdf:resource="http://seadatanet.maris2.nl/v_edmo/print.asp?n_code=4365"/>
	<skos:topConceptOf rdf:resource="http://vocab.aodn.org.au/def/organisation/1"/>
	<skos:inScheme rdf:resource="http://vocab.aodn.org.au/def/organisation/1"/>
</rdf:Description>

<rdf:Description rdf:about="http://vocab.aodn.org.au/def/organisation/entity/347">
	<rdf:type rdf:resource="http://www.w3.org/2000/01/rdf-schema#Resource"/>
	<rdf:type rdf:resource="http://www.w3.org/2004/02/skos/core#Concept"/>
	<dcterms:creator rdf:datatype="http://www.w3.org/2001/XMLSchema#string">Natalia Atkins</dcterms:creator>
	<dcterms:created rdf:datatype="http://www.w3.org/2001/XMLSchema#dateTime">2015-08-05T10:38:15Z</dcterms:created>
	<skos:broadMatch rdf:resource="http://vocab.aodn.org.au/def/organisation_classes/category/5"/>
	<skos:prefLabel xml:lang="en">GHD</skos:prefLabel>
	<skos:altLabel xml:lang="en"></skos:altLabel>
	<skos:hiddenLabel xml:lang="en"></skos:hiddenLabel>
	<skos:definition xml:lang="en">GHD is one of the world’s leading professional services companies operating in the global markets of water, energy and resources, environment, property and buildings, and transportation. They provide engineering, architecture, environmental and construction services to private and public sector clients. Established in 1928 and privately owned by its people, GHD operates across five continents – Asia, Australia, Europe, North and South America.</skos:definition>
	<dc:source rdf:datatype="http://www.w3.org/2001/XMLSchema#string">Australian Ocean Data Network Organisation Register</dc:source>
	<dc:publisher rdf:datatype="http://www.w3.org/2001/XMLSchema#string">eMarine Information Infrastructure (eMMI)</dc:publisher>
	<skos:exactMatch rdf:resource="http://seadatanet.maris2.nl/v_edmo/print.asp?n_code=4354"/>
	<skos:topConceptOf rdf:resource="http://vocab.aodn.org.au/def/organisation/1"/>
	<skos:inScheme rdf:resource="http://vocab.aodn.org.au/def/organisation/1"/>
</rdf:Description>

<rdf:Description rdf:about="http://vocab.aodn.org.au/def/organisation/entity/348">
	<rdf:type rdf:resource="http://www.w3.org/2000/01/rdf-schema#Resource"/>
	<rdf:type rdf:resource="http://www.w3.org/2004/02/skos/core#Concept"/>
	<dcterms:creator rdf:datatype="http://www.w3.org/2001/XMLSchema#string">Natalia Atkins</dcterms:creator>
	<dcterms:created rdf:datatype="http://www.w3.org/2001/XMLSchema#dateTime">2015-08-05T10:38:15Z</dcterms:created>
	<skos:broadMatch rdf:resource="http://vocab.aodn.org.au/def/organisation_classes/category/4"/>
	<skos:prefLabel xml:lang="en">FishBase</skos:prefLabel>
	<skos:altLabel xml:lang="en"></skos:altLabel>
	<skos:hiddenLabel xml:lang="en"></skos:hiddenLabel>
	<skos:definition xml:lang="en">FishBase is a relational database with information to cater to different professionals such as research scientists, fisheries managers, zoologists and many more. FishBase was developed at the WorldFish Center in collaboration with the Food and Agriculture Organization of the United Nations ( FAO) and many other partners, and with support from the European Commission ( EC). Since 2001 FishBase is supported by a consortium of nine research institutions.</skos:definition>
	<dc:source rdf:datatype="http://www.w3.org/2001/XMLSchema#string">Australian Ocean Data Network Organisation Register</dc:source>
	<dc:publisher rdf:datatype="http://www.w3.org/2001/XMLSchema#string">eMarine Information Infrastructure (eMMI)</dc:publisher>
	<skos:exactMatch rdf:resource="http://seadatanet.maris2.nl/v_edmo/print.asp?n_code=4352"/>
	<skos:topConceptOf rdf:resource="http://vocab.aodn.org.au/def/organisation/1"/>
	<skos:inScheme rdf:resource="http://vocab.aodn.org.au/def/organisation/1"/>
</rdf:Description>

<rdf:Description rdf:about="http://vocab.aodn.org.au/def/organisation/entity/349">
	<rdf:type rdf:resource="http://www.w3.org/2000/01/rdf-schema#Resource"/>
	<rdf:type rdf:resource="http://www.w3.org/2004/02/skos/core#Concept"/>
	<dcterms:creator rdf:datatype="http://www.w3.org/2001/XMLSchema#string">Natalia Atkins</dcterms:creator>
	<dcterms:created rdf:datatype="http://www.w3.org/2001/XMLSchema#dateTime">2015-08-05T10:38:15Z</dcterms:created>
	<skos:broadMatch rdf:resource="http://vocab.aodn.org.au/def/organisation_classes/category/4"/>
	<skos:prefLabel xml:lang="en">International Council for Science (ICSU)</skos:prefLabel>
	<skos:altLabel xml:lang="en"></skos:altLabel>
	<skos:hiddenLabel xml:lang="en">ICSU</skos:hiddenLabel>
	<skos:definition xml:lang="en">The International Council for Science (ICSU) is a non-governmental organisation with a global membership of national scientific bodies (122 Members, representing 142 countries) and International Scientific Unions (31 Members). ICSU’s mission is to strengthen international science for the benefit of society. The main ICSU Secretariat (20 staff in 2012) is based in Paris and ensures the day-to-day planning and operations under the guidance of an elected Executive Board. A small number of Policy Committees assist the Executive Board in its work and a General Assembly of all Members is convened every three years. ICSU has three Regional Offices – Africa, Asia and the Pacific and Latin America and the Caribbean.</skos:definition>
	<dc:source rdf:datatype="http://www.w3.org/2001/XMLSchema#string">Australian Ocean Data Network Organisation Register</dc:source>
	<dc:publisher rdf:datatype="http://www.w3.org/2001/XMLSchema#string">eMarine Information Infrastructure (eMMI)</dc:publisher>
	<skos:exactMatch rdf:resource="http://seadatanet.maris2.nl/v_edmo/print.asp?n_code=4353"/>
	<skos:topConceptOf rdf:resource="http://vocab.aodn.org.au/def/organisation/1"/>
	<skos:inScheme rdf:resource="http://vocab.aodn.org.au/def/organisation/1"/>
</rdf:Description>

<rdf:Description rdf:about="http://vocab.aodn.org.au/def/organisation/entity/350">
	<rdf:type rdf:resource="http://www.w3.org/2000/01/rdf-schema#Resource"/>
	<rdf:type rdf:resource="http://www.w3.org/2004/02/skos/core#Concept"/>
	<dcterms:creator rdf:datatype="http://www.w3.org/2001/XMLSchema#string">Natalia Atkins</dcterms:creator>
	<dcterms:created rdf:datatype="http://www.w3.org/2001/XMLSchema#dateTime">2015-08-05T10:38:15Z</dcterms:created>
	<skos:broadMatch rdf:resource="http://vocab.aodn.org.au/def/organisation_classes/category/4"/>
	<skos:prefLabel xml:lang="en">Ocean Biogeographic Information System (OBIS)</skos:prefLabel>
	<skos:altLabel xml:lang="en"></skos:altLabel>
	<skos:hiddenLabel xml:lang="en">OBIS</skos:hiddenLabel>
	<skos:definition xml:lang="en">The Ocean Biogeographic information System (OBIS) seeks to absorb, integrate, and assess isolated datasets into a larger, more comprehensive pictures of life in our oceans. The system hopes to stimulate research about our oceans to generate new hypotheses concerning evolutionary processes, species distributions, and roles of organisms in marine systems on a global scale. The abstract maps that OBIS generates are maps that contribute to the ‘big picture’ of our oceans: a comprehensive, collaborative, world-wide view of our oceans.</skos:definition>
	<dc:source rdf:datatype="http://www.w3.org/2001/XMLSchema#string">Australian Ocean Data Network Organisation Register</dc:source>
	<dc:publisher rdf:datatype="http://www.w3.org/2001/XMLSchema#string">eMarine Information Infrastructure (eMMI)</dc:publisher>
	<skos:exactMatch rdf:resource="http://seadatanet.maris2.nl/v_edmo/print.asp?n_code=4362"/>
	<skos:narrower rdf:resource="http://vocab.aodn.org.au/def/organisation/entity/419"/>
	<skos:topConceptOf rdf:resource="http://vocab.aodn.org.au/def/organisation/1"/>
	<skos:inScheme rdf:resource="http://vocab.aodn.org.au/def/organisation/1"/>
</rdf:Description>

<rdf:Description rdf:about="http://vocab.aodn.org.au/def/organisation/entity/351">
	<rdf:type rdf:resource="http://www.w3.org/2000/01/rdf-schema#Resource"/>
	<rdf:type rdf:resource="http://www.w3.org/2004/02/skos/core#Concept"/>
	<dcterms:modified rdf:datatype="http://www.w3.org/2001/XMLSchema#dateTime">2015-09-23T01:22:29Z</dcterms:modified>
	<dcterms:creator rdf:datatype="http://www.w3.org/2001/XMLSchema#string">Natalia Atkins</dcterms:creator>
	<dcterms:created rdf:datatype="http://www.w3.org/2001/XMLSchema#dateTime">2015-08-05T10:38:15Z</dcterms:created>
	<dcterms:contributor rdf:datatype="http://www.w3.org/2001/XMLSchema#string">eMII_Atkins.Natalia</dcterms:contributor>
	<skos:broadMatch rdf:resource="http://vocab.aodn.org.au/def/organisation_classes/category/4"/>
	<skos:prefLabel xml:lang="en">Scientific Committee on Antarctic Research (SCAR)</skos:prefLabel>
	<skos:altLabel xml:lang="en"></skos:altLabel>
	<skos:hiddenLabel xml:lang="en">SCAR</skos:hiddenLabel>
	<skos:definition xml:lang="en">The Scientific Committee on Antarctic Research (SCAR) is an inter-disciplinary committee of the International Council for Science (ICSU). SCAR is charged with initiating, developing and coordinating high quality international scientific research in the Antarctic region (including the Southern Ocean), and on the role of the Antarctic region in the Earth system. The scientific business of SCAR is conducted by its Standing Scientific Groups which represent the scientific disciplines active in Antarctic research and report to SCAR. In addition to carrying out its primary scientific role, SCAR also provides objective and independent scientific advice to the Antarctic Treaty Consultative Meetings and other organizations such as the UNFCCC and IPCC on issues of science and conservation affecting the management of Antarctica and the Southern Ocean and on the role of the Antarctic region in the Earth system. SCAR has made numerous recommendations on a variety of matters, many of which have been incorporated into Antarctic Treaty instruments. Foremost amongst these have been the advice provided for the many international agreements which provide protection for the ecology and environment of the Antarctic. SCAR meets every two years to conduct its administrative business at the SCAR Delegates' Meeting. At these meetings the members of SCAR, through their appointed Delegates, are responsible for formulating SCAR policy and strategy. They also elect an Executive Committee from among themselves which is responsible for the day-to-day administration of SCAR through its Secretariat at the Scott Polar Research Institute in Cambridge, England. The Executive Committee comprises the President, Past-President, four Vice-Presidents and the SCAR Executive Director. The SCAR Secretariat is staffed by the Executive Director, Executive Officer and a part-time Administrative Assistant. SCAR also holds, prior to the Delegates Meeting, a major Open Science Conference to draw attention to Antarctic issues, along with meetings of the Standing Scientific Groups that are designed to finalise the Science Programmes for eventual approval by the Delegates.</skos:definition>
	<dc:source rdf:datatype="http://www.w3.org/2001/XMLSchema#string">Australian Ocean Data Network Organisation Register</dc:source>
	<dc:publisher rdf:datatype="http://www.w3.org/2001/XMLSchema#string">eMarine Information Infrastructure (eMMI)</dc:publisher>
	<skos:exactMatch rdf:resource="http://seadatanet.maris2.nl/v_edmo/print.asp?n_code=4357"/>
	<skos:narrower rdf:resource="http://vocab.aodn.org.au/def/organisation/entity/399"/>
	<skos:topConceptOf rdf:resource="http://vocab.aodn.org.au/def/organisation/1"/>
	<skos:inScheme rdf:resource="http://vocab.aodn.org.au/def/organisation/1"/>
</rdf:Description>

<rdf:Description rdf:about="http://vocab.aodn.org.au/def/organisation/entity/352">
	<rdf:type rdf:resource="http://www.w3.org/2000/01/rdf-schema#Resource"/>
	<rdf:type rdf:resource="http://www.w3.org/2004/02/skos/core#Concept"/>
	<dcterms:creator rdf:datatype="http://www.w3.org/2001/XMLSchema#string">Natalia Atkins</dcterms:creator>
	<dcterms:created rdf:datatype="http://www.w3.org/2001/XMLSchema#dateTime">2015-08-05T10:38:15Z</dcterms:created>
	<skos:broadMatch rdf:resource="http://vocab.aodn.org.au/def/organisation_classes/category/4"/>
	<skos:prefLabel xml:lang="en">United Nations Economic and Social Commission for Asia and the Pacific (ESCAP)</skos:prefLabel>
	<skos:altLabel xml:lang="en"></skos:altLabel>
	<skos:hiddenLabel xml:lang="en">ESCAP</skos:hiddenLabel>
	<skos:definition xml:lang="en">The United Nations Economic and Social Commission for Asia and the Pacific (ESCAP) is the regional development arm of the United Nations for the Asia-Pacific region. Made up of 53 Member States and 9 Associate Members, with a geographical scope that stretches from Turkey in the west to the Pacific island nation of Kiribati in the east, and from the Russian Federation in the north to New Zealand in the south, the region is home to 4.1 billion people, or two thirds of the world’s population. This makes ESCAP the most comprehensive of the United Nations five regional commissions, and the largest United Nations body serving the Asia-Pacific region with over 600 staff. Established in 1947 with its headquarters in Bangkok, Thailand, ESCAP works to overcome some of the region’s greatest challenges by providing results oriented projects, technical assistance and capacity building to member States.</skos:definition>
	<dc:source rdf:datatype="http://www.w3.org/2001/XMLSchema#string">Australian Ocean Data Network Organisation Register</dc:source>
	<dc:publisher rdf:datatype="http://www.w3.org/2001/XMLSchema#string">eMarine Information Infrastructure (eMMI)</dc:publisher>
	<skos:exactMatch rdf:resource="http://seadatanet.maris2.nl/v_edmo/print.asp?n_code=4355"/>
	<skos:topConceptOf rdf:resource="http://vocab.aodn.org.au/def/organisation/1"/>
	<skos:inScheme rdf:resource="http://vocab.aodn.org.au/def/organisation/1"/>
</rdf:Description>

<rdf:Description rdf:about="http://vocab.aodn.org.au/def/organisation/entity/354">
	<rdf:type rdf:resource="http://www.w3.org/2000/01/rdf-schema#Resource"/>
	<rdf:type rdf:resource="http://www.w3.org/2004/02/skos/core#Concept"/>
	<dcterms:creator rdf:datatype="http://www.w3.org/2001/XMLSchema#string">Natalia Atkins</dcterms:creator>
	<dcterms:created rdf:datatype="http://www.w3.org/2001/XMLSchema#dateTime">2015-08-05T10:38:15Z</dcterms:created>
	<skos:broadMatch rdf:resource="http://vocab.aodn.org.au/def/organisation_classes/category/4"/>
	<skos:prefLabel xml:lang="en">WorldFish Center</skos:prefLabel>
	<skos:altLabel xml:lang="en"></skos:altLabel>
	<skos:hiddenLabel xml:lang="en"></skos:hiddenLabel>
	<skos:definition xml:lang="en">Their mission is to reduce poverty and hunger by improving fisheries and aquaculture. They strive to achieve large scale, environmentally sustainable, increases in supply and access to fish at affordable prices for poor consumers in developing countries. With more than 400 staff, there are seven offices across Asia, Africa and the Pacific, with their headquarters in Malaysia.</skos:definition>
	<dc:source rdf:datatype="http://www.w3.org/2001/XMLSchema#string">Australian Ocean Data Network Organisation Register</dc:source>
	<dc:publisher rdf:datatype="http://www.w3.org/2001/XMLSchema#string">eMarine Information Infrastructure (eMMI)</dc:publisher>
	<skos:exactMatch rdf:resource="http://seadatanet.maris2.nl/v_edmo/print.asp?n_code=4351"/>
	<skos:topConceptOf rdf:resource="http://vocab.aodn.org.au/def/organisation/1"/>
	<skos:inScheme rdf:resource="http://vocab.aodn.org.au/def/organisation/1"/>
</rdf:Description>

<rdf:Description rdf:about="http://vocab.aodn.org.au/def/organisation/entity/353">
	<rdf:type rdf:resource="http://www.w3.org/2000/01/rdf-schema#Resource"/>
	<rdf:type rdf:resource="http://www.w3.org/2004/02/skos/core#Concept"/>
	<dcterms:creator rdf:datatype="http://www.w3.org/2001/XMLSchema#string">Natalia Atkins</dcterms:creator>
	<dcterms:created rdf:datatype="http://www.w3.org/2001/XMLSchema#dateTime">2015-08-05T10:38:15Z</dcterms:created>
	<skos:broadMatch rdf:resource="http://vocab.aodn.org.au/def/organisation_classes/category/4"/>
	<skos:prefLabel xml:lang="en">World Ocean Observatory</skos:prefLabel>
	<skos:altLabel xml:lang="en"></skos:altLabel>
	<skos:hiddenLabel xml:lang="en"></skos:hiddenLabel>
	<skos:definition xml:lang="en">World Ocean Observatory is the leading organization advocating for the health and sustainability of the ocean through an accessible worldwide network of communication. Through education, partnership, information exchange, public connection, and relentless communications, W2O is committed to building an expansive global community of Citizens of the Ocean to promote and conserve marine resources for the future of all mankind. It's headquarters are in Maine, USA.</skos:definition>
	<dc:source rdf:datatype="http://www.w3.org/2001/XMLSchema#string">Australian Ocean Data Network Organisation Register</dc:source>
	<dc:publisher rdf:datatype="http://www.w3.org/2001/XMLSchema#string">eMarine Information Infrastructure (eMMI)</dc:publisher>
	<skos:exactMatch rdf:resource="http://seadatanet.maris2.nl/v_edmo/print.asp?n_code=4356"/>
	<skos:topConceptOf rdf:resource="http://vocab.aodn.org.au/def/organisation/1"/>
	<skos:inScheme rdf:resource="http://vocab.aodn.org.au/def/organisation/1"/>
</rdf:Description>

<rdf:Description rdf:about="http://vocab.aodn.org.au/def/organisation/entity/360">
	<rdf:type rdf:resource="http://www.w3.org/2000/01/rdf-schema#Resource"/>
	<rdf:type rdf:resource="http://www.w3.org/2004/02/skos/core#Concept"/>
	<dcterms:creator rdf:datatype="http://www.w3.org/2001/XMLSchema#string">Natalia Atkins</dcterms:creator>
	<dcterms:created rdf:datatype="http://www.w3.org/2001/XMLSchema#dateTime">2015-08-05T10:38:15Z</dcterms:created>
	<skos:broadMatch rdf:resource="http://vocab.aodn.org.au/def/organisation_classes/category/4"/>
	<skos:prefLabel xml:lang="en">The University of the South Pacific (USP)</skos:prefLabel>
	<skos:altLabel xml:lang="en"></skos:altLabel>
	<skos:hiddenLabel xml:lang="en">USP</skos:hiddenLabel>
	<skos:definition xml:lang="en">Established in 1968, USP is one of only two universities of its type in the world. It is jointly owned by the governments of 12 member countries: Cook Islands, Fiji, Kiribati, Marshall Islands, Nauru, Niue, Solomon Islands, Tokelau, Tonga, Tuvalu, Vanuatu and Samoa. The University has campuses in all member countries. The main campus, Laucala, is in Fiji. The Alafua Campus in Samoa is where the School of Agriculture and Food Technology is situated, and the Emalus Campus in Vanuatu is the location for the School of Law.</skos:definition>
	<dc:source rdf:datatype="http://www.w3.org/2001/XMLSchema#string">Australian Ocean Data Network Organisation Register</dc:source>
	<dc:publisher rdf:datatype="http://www.w3.org/2001/XMLSchema#string">eMarine Information Infrastructure (eMII)</dc:publisher>
	<skos:exactMatch rdf:resource="http://seadatanet.maris2.nl/v_edmo/print.asp?n_code=4358"/>
	<skos:narrower rdf:resource="http://vocab.aodn.org.au/def/organisation/entity/361"/>
	<skos:topConceptOf rdf:resource="http://vocab.aodn.org.au/def/organisation/1"/>
	<skos:inScheme rdf:resource="http://vocab.aodn.org.au/def/organisation/1"/>
</rdf:Description>

<rdf:Description rdf:about="http://vocab.aodn.org.au/def/organisation/entity/358">
	<rdf:type rdf:resource="http://www.w3.org/2000/01/rdf-schema#Resource"/>
	<rdf:type rdf:resource="http://www.w3.org/2004/02/skos/core#Concept"/>
	<dcterms:creator rdf:datatype="http://www.w3.org/2001/XMLSchema#string">Natalia Atkins</dcterms:creator>
	<dcterms:created rdf:datatype="http://www.w3.org/2001/XMLSchema#dateTime">2015-08-05T10:38:15Z</dcterms:created>
	<skos:broadMatch rdf:resource="http://vocab.aodn.org.au/def/organisation_classes/category/4"/>
	<skos:prefLabel xml:lang="en">University of Waikato</skos:prefLabel>
	<skos:altLabel xml:lang="en"></skos:altLabel>
	<skos:hiddenLabel xml:lang="en"></skos:hiddenLabel>
	<skos:definition xml:lang="en">The University of Waikato, established in 1965, is based in Hamilton, New Zealand with a satellite campus located in Tauranga.</skos:definition>
	<dc:source rdf:datatype="http://www.w3.org/2001/XMLSchema#string">Australian Ocean Data Network Organisation Register</dc:source>
	<dc:publisher rdf:datatype="http://www.w3.org/2001/XMLSchema#string">eMarine Information Infrastructure (eMII)</dc:publisher>
	<skos:exactMatch rdf:resource="http://seadatanet.maris2.nl/v_edmo/print.asp?n_code=4360"/>
	<skos:narrower rdf:resource="http://vocab.aodn.org.au/def/organisation/entity/359"/>
	<skos:topConceptOf rdf:resource="http://vocab.aodn.org.au/def/organisation/1"/>
	<skos:inScheme rdf:resource="http://vocab.aodn.org.au/def/organisation/1"/>
</rdf:Description>

<rdf:Description rdf:about="http://vocab.aodn.org.au/def/organisation/entity/369">
	<rdf:type rdf:resource="http://www.w3.org/2000/01/rdf-schema#Resource"/>
	<rdf:type rdf:resource="http://www.w3.org/2004/02/skos/core#Concept"/>
	<dcterms:creator rdf:datatype="http://www.w3.org/2001/XMLSchema#string">Natalia Atkins</dcterms:creator>
	<dcterms:created rdf:datatype="http://www.w3.org/2001/XMLSchema#dateTime">2015-08-05T10:38:15Z</dcterms:created>
	<skos:broadMatch rdf:resource="http://vocab.aodn.org.au/def/organisation_classes/category/4"/>
	<skos:prefLabel xml:lang="en">Universiti Pertanian Malaysia</skos:prefLabel>
	<skos:altLabel xml:lang="en"></skos:altLabel>
	<skos:hiddenLabel xml:lang="en"></skos:hiddenLabel>
	<skos:definition xml:lang="en">This university is now known as Universiti Putra Malaysia</skos:definition>
	<dc:source rdf:datatype="http://www.w3.org/2001/XMLSchema#string">Australian Ocean Data Network Organisation Register</dc:source>
	<dc:publisher rdf:datatype="http://www.w3.org/2001/XMLSchema#string">eMarine Information Infrastructure (eMMI)</dc:publisher>
	<skos:topConceptOf rdf:resource="http://vocab.aodn.org.au/def/organisation/1"/>
	<skos:inScheme rdf:resource="http://vocab.aodn.org.au/def/organisation/1"/>
	<skos:scopeNote xml:lang="en">Organisation no longer exists</skos:scopeNote>
</rdf:Description>

<rdf:Description rdf:about="http://vocab.aodn.org.au/def/organisation/entity/366">
	<rdf:type rdf:resource="http://www.w3.org/2000/01/rdf-schema#Resource"/>
	<rdf:type rdf:resource="http://www.w3.org/2004/02/skos/core#Concept"/>
	<dcterms:creator rdf:datatype="http://www.w3.org/2001/XMLSchema#string">Natalia Atkins</dcterms:creator>
	<dcterms:created rdf:datatype="http://www.w3.org/2001/XMLSchema#dateTime">2015-08-05T10:38:15Z</dcterms:created>
	<skos:broadMatch rdf:resource="http://vocab.aodn.org.au/def/organisation_classes/category/4"/>
	<skos:prefLabel xml:lang="en">Norwegian School of Economics and Business Administration</skos:prefLabel>
	<skos:altLabel xml:lang="en"></skos:altLabel>
	<skos:hiddenLabel xml:lang="en"></skos:hiddenLabel>
	<skos:definition xml:lang="en"></skos:definition>
	<dc:source rdf:datatype="http://www.w3.org/2001/XMLSchema#string">Australian Ocean Data Network Organisation Register</dc:source>
	<dc:publisher rdf:datatype="http://www.w3.org/2001/XMLSchema#string">eMarine Information Infrastructure (eMMI)</dc:publisher>
	<skos:topConceptOf rdf:resource="http://vocab.aodn.org.au/def/organisation/1"/>
	<skos:inScheme rdf:resource="http://vocab.aodn.org.au/def/organisation/1"/>
	<skos:scopeNote xml:lang="en">Organisation no longer exists</skos:scopeNote>
</rdf:Description>

<rdf:Description rdf:about="http://vocab.aodn.org.au/def/organisation/entity/364">
	<rdf:type rdf:resource="http://www.w3.org/2000/01/rdf-schema#Resource"/>
	<rdf:type rdf:resource="http://www.w3.org/2004/02/skos/core#Concept"/>
	<dcterms:modified rdf:datatype="http://www.w3.org/2001/XMLSchema#dateTime">2015-08-05T05:57:51Z</dcterms:modified>
	<dcterms:creator rdf:datatype="http://www.w3.org/2001/XMLSchema#string">Natalia Atkins</dcterms:creator>
	<dcterms:created rdf:datatype="http://www.w3.org/2001/XMLSchema#dateTime">2015-08-05T10:38:15Z</dcterms:created>
	<dcterms:contributor rdf:datatype="http://www.w3.org/2001/XMLSchema#string">Natalia_Atkins</dcterms:contributor>
	<skos:broadMatch rdf:resource="http://vocab.aodn.org.au/def/organisation_classes/category/4"/>
	<skos:prefLabel xml:lang="en">Centre for Ecology and Energy Physiology, University of Strasbourg</skos:prefLabel>
	<skos:altLabel xml:lang="en">Centre for Ecology and Energy Physiology</skos:altLabel>
	<skos:hiddenLabel xml:lang="en"></skos:hiddenLabel>
	<skos:definition xml:lang="en">This former centre is now known as the Département d'Écologie, de Physiologie et d'Éthologie, Institut pluridisciplinaire Hubert Curien.</skos:definition>
	<dc:source rdf:datatype="http://www.w3.org/2001/XMLSchema#string">Australian Ocean Data Network Organisation Register</dc:source>
	<dc:publisher rdf:datatype="http://www.w3.org/2001/XMLSchema#string">eMarine Information Infrastructure (eMMI)</dc:publisher>
	<skos:topConceptOf rdf:resource="http://vocab.aodn.org.au/def/organisation/1"/>
	<skos:inScheme rdf:resource="http://vocab.aodn.org.au/def/organisation/1"/>
	<skos:scopeNote xml:lang="en">Organisation no longer exists</skos:scopeNote>
</rdf:Description>

<rdf:Description rdf:about="http://vocab.aodn.org.au/def/organisation/entity/367">
	<rdf:type rdf:resource="http://www.w3.org/2000/01/rdf-schema#Resource"/>
	<rdf:type rdf:resource="http://www.w3.org/2004/02/skos/core#Concept"/>
	<dcterms:creator rdf:datatype="http://www.w3.org/2001/XMLSchema#string">Natalia Atkins</dcterms:creator>
	<dcterms:created rdf:datatype="http://www.w3.org/2001/XMLSchema#dateTime">2015-08-05T10:38:15Z</dcterms:created>
	<skos:broadMatch rdf:resource="http://vocab.aodn.org.au/def/organisation_classes/category/4"/>
	<skos:prefLabel xml:lang="en">University of Wales Swansea</skos:prefLabel>
	<skos:altLabel xml:lang="en"></skos:altLabel>
	<skos:hiddenLabel xml:lang="en"></skos:hiddenLabel>
	<skos:definition xml:lang="en">This university is now known as Swansea University (Courtesy of wikipedia)</skos:definition>
	<dc:source rdf:datatype="http://www.w3.org/2001/XMLSchema#string">Australian Ocean Data Network Organisation Register</dc:source>
	<dc:publisher rdf:datatype="http://www.w3.org/2001/XMLSchema#string">eMarine Information Infrastructure (eMII)</dc:publisher>
	<skos:narrower rdf:resource="http://vocab.aodn.org.au/def/organisation/entity/368"/>
	<skos:topConceptOf rdf:resource="http://vocab.aodn.org.au/def/organisation/1"/>
	<skos:inScheme rdf:resource="http://vocab.aodn.org.au/def/organisation/1"/>
	<skos:scopeNote xml:lang="en">Organisation no longer exists</skos:scopeNote>
</rdf:Description>

<rdf:Description rdf:about="http://vocab.aodn.org.au/def/organisation/entity/355">
	<rdf:type rdf:resource="http://www.w3.org/2000/01/rdf-schema#Resource"/>
	<rdf:type rdf:resource="http://www.w3.org/2004/02/skos/core#Concept"/>
	<dcterms:creator rdf:datatype="http://www.w3.org/2001/XMLSchema#string">Natalia Atkins</dcterms:creator>
	<dcterms:created rdf:datatype="http://www.w3.org/2001/XMLSchema#dateTime">2015-08-05T10:38:15Z</dcterms:created>
	<skos:broadMatch rdf:resource="http://vocab.aodn.org.au/def/organisation_classes/category/4"/>
	<skos:prefLabel xml:lang="en">University of Zurich</skos:prefLabel>
	<skos:altLabel xml:lang="en"></skos:altLabel>
	<skos:hiddenLabel xml:lang="en"></skos:hiddenLabel>
	<skos:definition xml:lang="en">The University of Zurich is found across four campuses across the city: City, Irchel, Oerlikon and Schlieren; and was founded in 1833.</skos:definition>
	<dc:source rdf:datatype="http://www.w3.org/2001/XMLSchema#string">Australian Ocean Data Network Organisation Register</dc:source>
	<dc:publisher rdf:datatype="http://www.w3.org/2001/XMLSchema#string">eMarine Information Infrastructure (eMII)</dc:publisher>
	<skos:exactMatch rdf:resource="http://seadatanet.maris2.nl/v_edmo/print.asp?n_code=4370"/>
	<skos:narrower rdf:resource="http://vocab.aodn.org.au/def/organisation/entity/356"/>
	<skos:topConceptOf rdf:resource="http://vocab.aodn.org.au/def/organisation/1"/>
	<skos:inScheme rdf:resource="http://vocab.aodn.org.au/def/organisation/1"/>
</rdf:Description>

<rdf:Description rdf:about="http://purl.org/dc/terms/contributor">
	<rdf:type rdf:resource="http://www.w3.org/1999/02/22-rdf-syntax-ns#Property"/>
	<rdf:type rdf:resource="http://www.w3.org/2000/01/rdf-schema#Resource"/>
	<rdfs:subPropertyOf rdf:resource="http://purl.org/dc/terms/contributor"/>
</rdf:Description>

<rdf:Description rdf:about="http://vocab.aodn.org.au/def/organisation/entity/397">
	<rdf:type rdf:resource="http://www.w3.org/2000/01/rdf-schema#Resource"/>
	<rdf:type rdf:resource="http://www.w3.org/2004/02/skos/core#Concept"/>
	<dcterms:modified rdf:datatype="http://www.w3.org/2001/XMLSchema#dateTime">2015-09-21T03:42:14Z</dcterms:modified>
	<dcterms:creator rdf:datatype="http://www.w3.org/2001/XMLSchema#string">Natalia Atkins</dcterms:creator>
	<dcterms:created rdf:datatype="http://www.w3.org/2001/XMLSchema#dateTime">2015-09-21T10:38:15Z</dcterms:created>
	<dcterms:contributor rdf:datatype="http://www.w3.org/2001/XMLSchema#string">eMII_Atkins.Natalia</dcterms:contributor>
	<skos:broadMatch rdf:resource="http://vocab.aodn.org.au/def/organisation_classes/category/4"/>
	<skos:prefLabel xml:lang="en">ReefQuest Centre for Shark Research</skos:prefLabel>
	<skos:altLabel xml:lang="en"></skos:altLabel>
	<skos:hiddenLabel xml:lang="en"></skos:hiddenLabel>
	<skos:definition xml:lang="en">Founded in 2001, the ReefQuest Centre for Shark Research is dedicated to shark and ray conservation through its scientific research and public education programs. The Centre maintains research equipment and facilities, reference collections of fossil and extant elasmobranch specimens, a scientific library, elasmobranch data bases, and public education materials. The centre's founder, Aidan Martin died in 2007, so the website is maintained in his honour.</skos:definition>
	<dc:source rdf:datatype="http://www.w3.org/2001/XMLSchema#string">Australian Ocean Data Network Organisation Register</dc:source>
	<dc:publisher rdf:datatype="http://www.w3.org/2001/XMLSchema#string">eMarine Information Infrastructure (eMMI)</dc:publisher>
	<skos:topConceptOf rdf:resource="http://vocab.aodn.org.au/def/organisation/1"/>
	<skos:inScheme rdf:resource="http://vocab.aodn.org.au/def/organisation/1"/>
</rdf:Description>

<rdf:Description rdf:about="http://vocab.aodn.org.au/def/organisation/entity/396">
	<rdf:type rdf:resource="http://www.w3.org/2000/01/rdf-schema#Resource"/>
	<rdf:type rdf:resource="http://www.w3.org/2004/02/skos/core#Concept"/>
	<dcterms:modified rdf:datatype="http://www.w3.org/2001/XMLSchema#dateTime">2015-09-21T03:42:09Z</dcterms:modified>
	<dcterms:creator rdf:datatype="http://www.w3.org/2001/XMLSchema#string">Natalia Atkins</dcterms:creator>
	<dcterms:created rdf:datatype="http://www.w3.org/2001/XMLSchema#dateTime">2015-09-21T10:38:15Z</dcterms:created>
	<dcterms:contributor rdf:datatype="http://www.w3.org/2001/XMLSchema#string">eMII_Atkins.Natalia</dcterms:contributor>
	<skos:broadMatch rdf:resource="http://vocab.aodn.org.au/def/organisation_classes/category/4"/>
	<skos:prefLabel xml:lang="en">Pacific Fisheries Management Inc</skos:prefLabel>
	<skos:altLabel xml:lang="en"></skos:altLabel>
	<skos:hiddenLabel xml:lang="en"></skos:hiddenLabel>
	<skos:definition xml:lang="en">Pacific Fisheries Management Inc. provides consulting, executive management, policy and strategic planning services for individuals, companies, NGOs and government agencies involved in commercial fisheries.  Focus on policy development, program analysis, and the negotiation, coordination and implementation of commercial fishery management programs.</skos:definition>
	<dc:source rdf:datatype="http://www.w3.org/2001/XMLSchema#string">Australian Ocean Data Network Organisation Register</dc:source>
	<dc:publisher rdf:datatype="http://www.w3.org/2001/XMLSchema#string">eMarine Information Infrastructure (eMMI)</dc:publisher>
	<skos:topConceptOf rdf:resource="http://vocab.aodn.org.au/def/organisation/1"/>
	<skos:inScheme rdf:resource="http://vocab.aodn.org.au/def/organisation/1"/>
</rdf:Description>

<rdf:Description rdf:about="http://vocab.aodn.org.au/def/organisation/entity/395">
	<rdf:type rdf:resource="http://www.w3.org/2000/01/rdf-schema#Resource"/>
	<rdf:type rdf:resource="http://www.w3.org/2004/02/skos/core#Concept"/>
	<dcterms:modified rdf:datatype="http://www.w3.org/2001/XMLSchema#dateTime">2015-09-29T03:27:00Z</dcterms:modified>
	<dcterms:creator rdf:datatype="http://www.w3.org/2001/XMLSchema#string">Natalia Atkins</dcterms:creator>
	<dcterms:created rdf:datatype="http://www.w3.org/2001/XMLSchema#dateTime">2015-09-21T10:38:15Z</dcterms:created>
	<dcterms:contributor rdf:datatype="http://www.w3.org/2001/XMLSchema#string">eMII_Atkins.Natalia</dcterms:contributor>
	<skos:broadMatch rdf:resource="http://vocab.aodn.org.au/def/organisation_classes/category/4"/>
	<skos:prefLabel xml:lang="en">Ministry of Fisheries, New Zealand Government</skos:prefLabel>
	<skos:altLabel xml:lang="en">Ministry of Fisheries</skos:altLabel>
	<skos:hiddenLabel xml:lang="en"></skos:hiddenLabel>
	<skos:definition xml:lang="en">The Ministry of Fisheries, was established in 1995, to ensure the sustainable utilisation of fisheries. In April 2012 it was merged into the newly formed Ministry for Primary Industries. (Courtesy of Wikipedia)</skos:definition>
	<dc:source rdf:datatype="http://www.w3.org/2001/XMLSchema#string">Australian Ocean Data Network Organisation Register</dc:source>
	<dc:publisher rdf:datatype="http://www.w3.org/2001/XMLSchema#string">eMarine Information Infrastructure (eMMI)</dc:publisher>
	<skos:topConceptOf rdf:resource="http://vocab.aodn.org.au/def/organisation/1"/>
	<skos:inScheme rdf:resource="http://vocab.aodn.org.au/def/organisation/1"/>
	<skos:scopeNote xml:lang="en">Organisation no longer exists</skos:scopeNote>
	<skos:scopeNote xml:lang="en">Organisation no longer exists. Replaced by http://vocab.aodn.org.au/def/organisation/entity/402</skos:scopeNote>
	<dcterms:isReplacedBy xml:lang="en">http://vocab.aodn.org.au/def/organisation/entity/402</dcterms:isReplacedBy>
	<dcterms:isReplacedBy xml:lang="en">Ministry for Primary Industries (MPI), New Zealand Government</dcterms:isReplacedBy>
</rdf:Description>

<rdf:Description rdf:about="http://vocab.aodn.org.au/def/organisation/entity/400">
	<rdf:type rdf:resource="http://www.w3.org/2000/01/rdf-schema#Resource"/>
	<rdf:type rdf:resource="http://www.w3.org/2004/02/skos/core#Concept"/>
	<dcterms:modified rdf:datatype="http://www.w3.org/2001/XMLSchema#dateTime">2015-09-29T03:24:53Z</dcterms:modified>
	<dcterms:creator rdf:datatype="http://www.w3.org/2001/XMLSchema#string">Natalia Atkins</dcterms:creator>
	<dcterms:created rdf:datatype="http://www.w3.org/2001/XMLSchema#dateTime">2015-09-25T10:38:15Z</dcterms:created>
	<dcterms:contributor rdf:datatype="http://www.w3.org/2001/XMLSchema#string">eMII_Atkins.Natalia</dcterms:contributor>
	<skos:broadMatch rdf:resource="http://vocab.aodn.org.au/def/organisation_classes/category/6"/>
	<skos:prefLabel xml:lang="en">Great Barrier Reef Foundation</skos:prefLabel>
	<skos:altLabel xml:lang="en"></skos:altLabel>
	<skos:hiddenLabel xml:lang="en"></skos:hiddenLabel>
	<skos:definition xml:lang="en">The Great Barrier Reef Foundation was established in 2000, in accordance with Article 17 of the World Heritage Convention. The Foundation is the only independent not-for-profit organisation in Australia dedicated solely to raising funds for scientific research into preserving the Great Barrier Reef.</skos:definition>
	<dc:source rdf:datatype="http://www.w3.org/2001/XMLSchema#string">Australian Ocean Data Network Organisation Register</dc:source>
	<dc:publisher rdf:datatype="http://www.w3.org/2001/XMLSchema#string">eMarine Information Infrastructure (eMMI)</dc:publisher>
	<skos:exactMatch rdf:resource="http://seadatanet.maris2.nl/v_edmo/print.asp?n_code=4380"/>
	<skos:topConceptOf rdf:resource="http://vocab.aodn.org.au/def/organisation/1"/>
	<skos:inScheme rdf:resource="http://vocab.aodn.org.au/def/organisation/1"/>
</rdf:Description>

<rdf:Description rdf:about="http://vocab.aodn.org.au/def/organisation/entity/401">
	<rdf:type rdf:resource="http://www.w3.org/2000/01/rdf-schema#Resource"/>
	<rdf:type rdf:resource="http://www.w3.org/2004/02/skos/core#Concept"/>
	<dcterms:modified rdf:datatype="http://www.w3.org/2001/XMLSchema#dateTime">2015-09-29T03:25:28Z</dcterms:modified>
	<dcterms:creator rdf:datatype="http://www.w3.org/2001/XMLSchema#string">Natalia Atkins</dcterms:creator>
	<dcterms:created rdf:datatype="http://www.w3.org/2001/XMLSchema#dateTime">2015-09-25T10:38:15Z</dcterms:created>
	<dcterms:contributor rdf:datatype="http://www.w3.org/2001/XMLSchema#string">eMII_Atkins.Natalia</dcterms:contributor>
	<skos:broadMatch rdf:resource="http://vocab.aodn.org.au/def/organisation_classes/category/5"/>
	<skos:prefLabel xml:lang="en">Rio Tinto Alcan</skos:prefLabel>
	<skos:altLabel xml:lang="en"></skos:altLabel>
	<skos:hiddenLabel xml:lang="en"></skos:hiddenLabel>
	<skos:definition xml:lang="en">Rio Tinto Alcan is the world's largest producer of bauxite, alumina and aluminium. They are one of five product groups operated by Rio Tinto, a leading international mining group. Rio Tinto's aluminium business started with Comalco in Australia in the mid 1950s. Rio Tinto bought Comalco in 2000, and the company was renamed Rio Tinto Aluminium in late 2006. In October 2007, leading mining organisation Rio Tinto acquired Alcan, which orginated in Canada in 1902. Alcan integrated with Rio Tinto's existing aluminium business, resulting in Rio Tinto Alcan. Operations in Australia can be found in: Tasmania, Queensland, Nothern Territory and New South Wales.</skos:definition>
	<dc:source rdf:datatype="http://www.w3.org/2001/XMLSchema#string">Australian Ocean Data Network Organisation Register</dc:source>
	<dc:publisher rdf:datatype="http://www.w3.org/2001/XMLSchema#string">eMarine Information Infrastructure (eMMI)</dc:publisher>
	<skos:exactMatch rdf:resource="http://seadatanet.maris2.nl/v_edmo/print.asp?n_code=4379"/>
	<skos:topConceptOf rdf:resource="http://vocab.aodn.org.au/def/organisation/1"/>
	<skos:inScheme rdf:resource="http://vocab.aodn.org.au/def/organisation/1"/>
</rdf:Description>

<rdf:Description rdf:about="http://vocab.aodn.org.au/def/organisation/entity/402">
	<rdf:type rdf:resource="http://www.w3.org/2000/01/rdf-schema#Resource"/>
	<rdf:type rdf:resource="http://www.w3.org/2004/02/skos/core#Concept"/>
	<dcterms:creator rdf:datatype="http://www.w3.org/2001/XMLSchema#string">Natalia Atkins</dcterms:creator>
	<dcterms:created rdf:datatype="http://www.w3.org/2001/XMLSchema#dateTime">2015-09-25T10:38:15Z</dcterms:created>
	<skos:prefLabel xml:lang="en">Ministry for Primary Industries (MPI), New Zealand Government</skos:prefLabel>
	<skos:altLabel xml:lang="en">Ministry for Primary Industries (MPI)</skos:altLabel>
	<skos:hiddenLabel xml:lang="en">MPI</skos:hiddenLabel>
	<skos:definition xml:lang="en"></skos:definition>
	<dc:source rdf:datatype="http://www.w3.org/2001/XMLSchema#string">Australian Ocean Data Network Organisation Register</dc:source>
	<dc:publisher rdf:datatype="http://www.w3.org/2001/XMLSchema#string">eMarine Information Infrastructure (eMMI)</dc:publisher>
	<skos:exactMatch rdf:resource="http://seadatanet.maris2.nl/v_edmo/print.asp?n_code=4381"/>
	<skos:topConceptOf rdf:resource="http://vocab.aodn.org.au/def/organisation/1"/>
	<skos:inScheme rdf:resource="http://vocab.aodn.org.au/def/organisation/1"/>
	<skos:scopeNote xml:lang="en">Replaces http://vocab.aodn.org.au/def/organisation/entity/395</skos:scopeNote>
	<dcterms:replaces xml:lang="en">Ministry of Fisheries, New Zealand Government</dcterms:replaces>
	<dcterms:replaces rdf:resource="http://vocab.aodn.org.au/organisation/entity/395"/>
</rdf:Description>

<rdf:Description rdf:about="http://vocab.aodn.org.au/def/organisation/entity/403">
	<rdf:type rdf:resource="http://www.w3.org/2000/01/rdf-schema#Resource"/>
	<rdf:type rdf:resource="http://www.w3.org/2004/02/skos/core#Concept"/>
	<dcterms:modified rdf:datatype="http://www.w3.org/2001/XMLSchema#dateTime">2015-09-29T03:25:58Z</dcterms:modified>
	<dcterms:creator rdf:datatype="http://www.w3.org/2001/XMLSchema#string">Natalia Atkins</dcterms:creator>
	<dcterms:created rdf:datatype="http://www.w3.org/2001/XMLSchema#dateTime">2015-09-28T10:38:15Z</dcterms:created>
	<dcterms:contributor rdf:datatype="http://www.w3.org/2001/XMLSchema#string">eMII_Atkins.Natalia</dcterms:contributor>
	<skos:broadMatch rdf:resource="http://vocab.aodn.org.au/def/organisation_classes/category/4"/>
	<skos:prefLabel xml:lang="en">National Institute of Polar Research (NIPR)</skos:prefLabel>
	<skos:altLabel xml:lang="en"></skos:altLabel>
	<skos:hiddenLabel xml:lang="en">NIPR</skos:hiddenLabel>
	<skos:definition xml:lang="en"></skos:definition>
	<dc:source rdf:datatype="http://www.w3.org/2001/XMLSchema#string">Australian Ocean Data Network Organisation Register</dc:source>
	<dc:publisher rdf:datatype="http://www.w3.org/2001/XMLSchema#string">eMarine Information Infrastructure (eMMI)</dc:publisher>
	<skos:exactMatch rdf:resource="http://seadatanet.maris2.nl/v_edmo/print.asp?n_code=4368"/>
	<skos:topConceptOf rdf:resource="http://vocab.aodn.org.au/def/organisation/1"/>
	<skos:inScheme rdf:resource="http://vocab.aodn.org.au/def/organisation/1"/>
</rdf:Description>

<rdf:Description rdf:about="http://vocab.aodn.org.au/def/organisation/entity/371">
	<rdf:type rdf:resource="http://www.w3.org/2000/01/rdf-schema#Resource"/>
	<rdf:type rdf:resource="http://www.w3.org/2004/02/skos/core#Concept"/>
	<dcterms:modified rdf:datatype="http://www.w3.org/2001/XMLSchema#dateTime">2015-09-29T03:29:17Z</dcterms:modified>
	<dcterms:modified rdf:datatype="http://www.w3.org/2001/XMLSchema#dateTime">2016-01-27T01:28:50Z</dcterms:modified>
	<dcterms:creator rdf:datatype="http://www.w3.org/2001/XMLSchema#string">Natalia Atkins</dcterms:creator>
	<dcterms:created rdf:datatype="http://www.w3.org/2001/XMLSchema#dateTime">2015-09-18T10:38:15Z</dcterms:created>
	<dcterms:contributor rdf:datatype="http://www.w3.org/2001/XMLSchema#string">eMII_Atkins.Natalia</dcterms:contributor>
	<dcterms:contributor rdf:datatype="http://www.w3.org/2001/XMLSchema#string">eMII_Finney.Kim_Admin</dcterms:contributor>
	<skos:broadMatch rdf:resource="http://vocab.aodn.org.au/def/organisation_classes/category/4"/>
	<skos:prefLabel xml:lang="en">British Oceanographic Data Centre (BODC)</skos:prefLabel>
	<skos:altLabel xml:lang="en"></skos:altLabel>
	<skos:hiddenLabel xml:lang="en">BODC</skos:hiddenLabel>
	<skos:definition xml:lang="en">BODC operates on behalf of the Marine Science and Technology Board of the UK's Natural Environment Research Council and acts as the UK's focal point for international oceanographic data exchange. It participates within the Intergovernmental Oceanographic Commission (IOC)'s network of national oceanographic data centres (NODCs) and was a founding partner of the European Sea-Search network. BODC maintains a national oceanographic database, and provides a data service to research scientists, industry, and local and central government, and to major oceanographic programmes. In particular, it provides active data management support to NERC's Thematic Projects, including the AUTOSUB, LOIS and PRIME projects and the UK components of JGOFS and WOCE. It is the WOCE Data Assembly Centre for sea level data and, on behalf of the IOC and IHO Joint Guiding Committee for the General Bathymetric Chart of the Oceans (GEBCO), is responsible for developing the GEBCO Digital Atlas. BODC also acts as the data centre for a number of EC/MAST projects including OMEX, INDIA and PROVESS. BODC exchanges data freely with other NODCs on a bilateral basis, but reserves the right to charge other users the marginal costs involved in making data available e.g. costs of copying, materials and postage. These charges may be waived for reasonable requests in support of bona-fide scientific research. Some data held by BODC are of restricted availability, awaiting final clearance by the scientists involved in their original collection.</skos:definition>
	<dc:source rdf:datatype="http://www.w3.org/2001/XMLSchema#string">Australian Ocean Data Network Organisation Register</dc:source>
	<dc:publisher rdf:datatype="http://www.w3.org/2001/XMLSchema#string">eMarine Information Infrastructure (eMMI)</dc:publisher>
	<skos:exactMatch rdf:resource="http://seadatanet.maris2.nl/v_edmo/print.asp?n_code=43"/>
	<skos:topConceptOf rdf:resource="http://vocab.aodn.org.au/def/organisation/1"/>
	<skos:inScheme rdf:resource="http://vocab.aodn.org.au/def/organisation/1"/>
</rdf:Description>

<rdf:Description rdf:about="http://vocab.aodn.org.au/def/organisation/entity/372">
	<rdf:type rdf:resource="http://www.w3.org/2000/01/rdf-schema#Resource"/>
	<rdf:type rdf:resource="http://www.w3.org/2004/02/skos/core#Concept"/>
	<dcterms:modified rdf:datatype="http://www.w3.org/2001/XMLSchema#dateTime">2015-09-29T03:29:53Z</dcterms:modified>
	<dcterms:creator rdf:datatype="http://www.w3.org/2001/XMLSchema#string">Natalia Atkins</dcterms:creator>
	<dcterms:created rdf:datatype="http://www.w3.org/2001/XMLSchema#dateTime">2015-09-18T10:38:15Z</dcterms:created>
	<dcterms:contributor rdf:datatype="http://www.w3.org/2001/XMLSchema#string">eMII_Atkins.Natalia</dcterms:contributor>
	<skos:broadMatch rdf:resource="http://vocab.aodn.org.au/def/organisation_classes/category/4"/>
	<skos:prefLabel xml:lang="en">Federal Maritime and Hydrographic Agency (BSH)</skos:prefLabel>
	<skos:altLabel xml:lang="en"></skos:altLabel>
	<skos:hiddenLabel xml:lang="en">BSH</skos:hiddenLabel>
	<skos:definition xml:lang="en">BSH is the maritime partner to industry, science, and environmental organisations. Over 900 dedicated employees, a budget of some 60 million Euro, and unique competence form a solid basis for our wide range of services:  * Services to maritime shipping, including tonnage measurement, law of the flag, International Shipping Register  * Promotion of the German commercial fleet  * Issue and registration of mariners' certificates  * Type-testing and approval of radiocommunications and navigation equipment * Surveys in the North and Baltic Seas performed by BSH vessels * Publication of nautical charts and small-craft charts * Approval of offshore activities, e.g. wind farms, pipelines, submarine cables * Prediction of tides, water levels, and storm surges  * Monitoring of the marine environment * Prosecution of environmental offences * Improvement of knowledge of the oceans. With its historical roots in the "Norddeutsche Seewarte" (North German Maritime Observatory) which issued detailed sailing directions based on nautical and meteorological observations as early as 1868, the BSH has long ceased to be only a provider of the traditional services to shipping but has focused on additional maritime target groups and applications - e.g. the offshore wind industry and marine environmental protection.</skos:definition>
	<dc:source rdf:datatype="http://www.w3.org/2001/XMLSchema#string">Australian Ocean Data Network Organisation Register</dc:source>
	<dc:publisher rdf:datatype="http://www.w3.org/2001/XMLSchema#string">eMarine Information Infrastructure (eMMI)</dc:publisher>
	<skos:exactMatch rdf:resource="http://seadatanet.maris2.nl/v_edmo/print.asp?n_code=1850"/>
	<skos:topConceptOf rdf:resource="http://vocab.aodn.org.au/def/organisation/1"/>
	<skos:inScheme rdf:resource="http://vocab.aodn.org.au/def/organisation/1"/>
</rdf:Description>

<rdf:Description rdf:about="http://vocab.aodn.org.au/def/organisation/entity/373">
	<rdf:type rdf:resource="http://www.w3.org/2000/01/rdf-schema#Resource"/>
	<rdf:type rdf:resource="http://www.w3.org/2004/02/skos/core#Concept"/>
	<dcterms:modified rdf:datatype="http://www.w3.org/2001/XMLSchema#dateTime">2015-09-29T03:30:13Z</dcterms:modified>
	<dcterms:creator rdf:datatype="http://www.w3.org/2001/XMLSchema#string">Natalia Atkins</dcterms:creator>
	<dcterms:created rdf:datatype="http://www.w3.org/2001/XMLSchema#dateTime">2015-09-18T10:38:15Z</dcterms:created>
	<dcterms:contributor rdf:datatype="http://www.w3.org/2001/XMLSchema#string">eMII_Atkins.Natalia</dcterms:contributor>
	<skos:broadMatch rdf:resource="http://vocab.aodn.org.au/def/organisation_classes/category/4"/>
	<skos:prefLabel xml:lang="en">China Second Institute of Oceanography (CSIO)</skos:prefLabel>
	<skos:altLabel xml:lang="en"></skos:altLabel>
	<skos:hiddenLabel xml:lang="en">CSIO</skos:hiddenLabel>
	<skos:definition xml:lang="en"></skos:definition>
	<dc:source rdf:datatype="http://www.w3.org/2001/XMLSchema#string">Australian Ocean Data Network Organisation Register</dc:source>
	<dc:publisher rdf:datatype="http://www.w3.org/2001/XMLSchema#string">eMarine Information Infrastructure (eMMI)</dc:publisher>
	<skos:exactMatch rdf:resource="http://seadatanet.maris2.nl/v_edmo/print.asp?n_code=3335"/>
	<skos:topConceptOf rdf:resource="http://vocab.aodn.org.au/def/organisation/1"/>
	<skos:inScheme rdf:resource="http://vocab.aodn.org.au/def/organisation/1"/>
</rdf:Description>

<rdf:Description rdf:about="http://vocab.aodn.org.au/def/organisation/entity/374">
	<rdf:type rdf:resource="http://www.w3.org/2000/01/rdf-schema#Resource"/>
	<rdf:type rdf:resource="http://www.w3.org/2004/02/skos/core#Concept"/>
	<dcterms:modified rdf:datatype="http://www.w3.org/2001/XMLSchema#dateTime">2015-09-29T03:30:29Z</dcterms:modified>
	<dcterms:creator rdf:datatype="http://www.w3.org/2001/XMLSchema#string">Natalia Atkins</dcterms:creator>
	<dcterms:created rdf:datatype="http://www.w3.org/2001/XMLSchema#dateTime">2015-09-18T10:38:15Z</dcterms:created>
	<dcterms:contributor rdf:datatype="http://www.w3.org/2001/XMLSchema#string">eMII_Atkins.Natalia</dcterms:contributor>
	<skos:broadMatch rdf:resource="http://vocab.aodn.org.au/def/organisation_classes/category/4"/>
	<skos:prefLabel xml:lang="en">Carbon Dioxide Information Analysis Center (CDIAC)</skos:prefLabel>
	<skos:altLabel xml:lang="en"></skos:altLabel>
	<skos:hiddenLabel xml:lang="en">CDIAC</skos:hiddenLabel>
	<skos:definition xml:lang="en">International data centre for carbonate system parameters such as pH, DIC and pCO2. Located in the Environmental Sciences Division of the Oak Ridge National Laboratory,</skos:definition>
	<dc:source rdf:datatype="http://www.w3.org/2001/XMLSchema#string">Australian Ocean Data Network Organisation Register</dc:source>
	<dc:publisher rdf:datatype="http://www.w3.org/2001/XMLSchema#string">eMarine Information Infrastructure (eMMI)</dc:publisher>
	<skos:exactMatch rdf:resource="http://seadatanet.maris2.nl/v_edmo/print.asp?n_code=2872"/>
	<skos:topConceptOf rdf:resource="http://vocab.aodn.org.au/def/organisation/1"/>
	<skos:inScheme rdf:resource="http://vocab.aodn.org.au/def/organisation/1"/>
</rdf:Description>

<rdf:Description rdf:about="http://vocab.aodn.org.au/def/organisation/entity/375">
	<rdf:type rdf:resource="http://www.w3.org/2000/01/rdf-schema#Resource"/>
	<rdf:type rdf:resource="http://www.w3.org/2004/02/skos/core#Concept"/>
	<dcterms:modified rdf:datatype="http://www.w3.org/2001/XMLSchema#dateTime">2015-09-29T03:30:44Z</dcterms:modified>
	<dcterms:creator rdf:datatype="http://www.w3.org/2001/XMLSchema#string">Natalia Atkins</dcterms:creator>
	<dcterms:created rdf:datatype="http://www.w3.org/2001/XMLSchema#dateTime">2015-09-18T10:38:15Z</dcterms:created>
	<dcterms:contributor rdf:datatype="http://www.w3.org/2001/XMLSchema#string">eMII_Atkins.Natalia</dcterms:contributor>
	<skos:broadMatch rdf:resource="http://vocab.aodn.org.au/def/organisation_classes/category/4"/>
	<skos:prefLabel xml:lang="en">IFREMER</skos:prefLabel>
	<skos:altLabel xml:lang="en"></skos:altLabel>
	<skos:hiddenLabel xml:lang="en"></skos:hiddenLabel>
	<skos:definition xml:lang="en">The Head Office of IFREMER is located in a suburb close to Paris.</skos:definition>
	<dc:source rdf:datatype="http://www.w3.org/2001/XMLSchema#string">Australian Ocean Data Network Organisation Register</dc:source>
	<dc:publisher rdf:datatype="http://www.w3.org/2001/XMLSchema#string">eMarine Information Infrastructure (eMMI)</dc:publisher>
	<skos:exactMatch rdf:resource="http://seadatanet.maris2.nl/v_edmo/print.asp?n_code=1054"/>
	<skos:topConceptOf rdf:resource="http://vocab.aodn.org.au/def/organisation/1"/>
	<skos:inScheme rdf:resource="http://vocab.aodn.org.au/def/organisation/1"/>
</rdf:Description>

<rdf:Description rdf:about="http://vocab.aodn.org.au/def/organisation/entity/376">
	<rdf:type rdf:resource="http://www.w3.org/2000/01/rdf-schema#Resource"/>
	<rdf:type rdf:resource="http://www.w3.org/2004/02/skos/core#Concept"/>
	<dcterms:modified rdf:datatype="http://www.w3.org/2001/XMLSchema#dateTime">2015-09-29T03:30:59Z</dcterms:modified>
	<dcterms:creator rdf:datatype="http://www.w3.org/2001/XMLSchema#string">Natalia Atkins</dcterms:creator>
	<dcterms:created rdf:datatype="http://www.w3.org/2001/XMLSchema#dateTime">2015-09-18T10:38:15Z</dcterms:created>
	<dcterms:contributor rdf:datatype="http://www.w3.org/2001/XMLSchema#string">eMII_Atkins.Natalia</dcterms:contributor>
	<skos:broadMatch rdf:resource="http://vocab.aodn.org.au/def/organisation_classes/category/4"/>
	<skos:prefLabel xml:lang="en">National Aeronautics and Space Administration Goddard Space Flight Center (NASA GSFC)</skos:prefLabel>
	<skos:altLabel xml:lang="en"></skos:altLabel>
	<skos:hiddenLabel xml:lang="en">NASA GSFC</skos:hiddenLabel>
	<skos:definition xml:lang="en">The Center, located in a Maryland suburb outside of Washington, DC, is home to the Nation's largest organization of combined scientists and engineers dedicated to learning and sharing their knowledge of the Earth, solar system, and Universe. The mission of the Goddard Space Flight Center is to expand knowledge of the Earth and its environment, the solar system and the universe through observations from space. It is committed to excellence in scientific investigation, in the development and operation of space systems, and in the advancement of essential technologies. In pursuit of this challenge, the Center will: 1) Conduct a preeminent program of research in the space and Earth science disciplines using measurements from space complemented by suborbital, ground-based and laboratory measurements and by theoretical investigations. 2) Develop and operate a broad spectrum of flight missions that are responsive to the needs of the science community. 3) Provide and operate spaceflight tracking and data acquisition networks. 4) Develop innovative technology and instruments critical to the success of our mission. 5) Develop and maintain advanced information systems for the display, analysis, archiving and distribution of space and Earth science data. 6) Develop National Oceanic and Atmospheric Administration (NOAA) satellite systems that provide environmental data for forecasting and research.</skos:definition>
	<dc:source rdf:datatype="http://www.w3.org/2001/XMLSchema#string">Australian Ocean Data Network Organisation Register</dc:source>
	<dc:publisher rdf:datatype="http://www.w3.org/2001/XMLSchema#string">eMarine Information Infrastructure (eMMI)</dc:publisher>
	<skos:exactMatch rdf:resource="http://seadatanet.maris2.nl/v_edmo/print.asp?n_code=1225"/>
	<skos:topConceptOf rdf:resource="http://vocab.aodn.org.au/def/organisation/1"/>
	<skos:inScheme rdf:resource="http://vocab.aodn.org.au/def/organisation/1"/>
</rdf:Description>

<rdf:Description rdf:about="http://vocab.aodn.org.au/def/organisation/entity/377">
	<rdf:type rdf:resource="http://www.w3.org/2000/01/rdf-schema#Resource"/>
	<rdf:type rdf:resource="http://www.w3.org/2004/02/skos/core#Concept"/>
	<dcterms:modified rdf:datatype="http://www.w3.org/2001/XMLSchema#dateTime">2015-09-29T03:32:28Z</dcterms:modified>
	<dcterms:creator rdf:datatype="http://www.w3.org/2001/XMLSchema#string">Natalia Atkins</dcterms:creator>
	<dcterms:created rdf:datatype="http://www.w3.org/2001/XMLSchema#dateTime">2015-09-18T10:38:15Z</dcterms:created>
	<dcterms:contributor rdf:datatype="http://www.w3.org/2001/XMLSchema#string">eMII_Atkins.Natalia</dcterms:contributor>
	<skos:broadMatch rdf:resource="http://vocab.aodn.org.au/def/organisation_classes/category/4"/>
	<skos:prefLabel xml:lang="en">Indian National Centre For Ocean Information Services (INCOIS)</skos:prefLabel>
	<skos:altLabel xml:lang="en"></skos:altLabel>
	<skos:hiddenLabel xml:lang="en">INCOIS</skos:hiddenLabel>
	<skos:definition xml:lang="en">To provide ocean information and advisory services to the society, industry, government and scientific community through sustained ocean observations and constant improvements through systematic and focused research.</skos:definition>
	<dc:source rdf:datatype="http://www.w3.org/2001/XMLSchema#string">Australian Ocean Data Network Organisation Register</dc:source>
	<dc:publisher rdf:datatype="http://www.w3.org/2001/XMLSchema#string">eMarine Information Infrastructure (eMMI)</dc:publisher>
	<skos:exactMatch rdf:resource="http://seadatanet.maris2.nl/v_edmo/print.asp?n_code=3334"/>
	<skos:topConceptOf rdf:resource="http://vocab.aodn.org.au/def/organisation/1"/>
	<skos:inScheme rdf:resource="http://vocab.aodn.org.au/def/organisation/1"/>
</rdf:Description>

<rdf:Description rdf:about="http://vocab.aodn.org.au/def/organisation/entity/378">
	<rdf:type rdf:resource="http://www.w3.org/2000/01/rdf-schema#Resource"/>
	<rdf:type rdf:resource="http://www.w3.org/2004/02/skos/core#Concept"/>
	<dcterms:modified rdf:datatype="http://www.w3.org/2001/XMLSchema#dateTime">2015-09-29T03:32:41Z</dcterms:modified>
	<dcterms:creator rdf:datatype="http://www.w3.org/2001/XMLSchema#string">Natalia Atkins</dcterms:creator>
	<dcterms:created rdf:datatype="http://www.w3.org/2001/XMLSchema#dateTime">2015-09-18T10:38:15Z</dcterms:created>
	<dcterms:contributor rdf:datatype="http://www.w3.org/2001/XMLSchema#string">eMII_Atkins.Natalia</dcterms:contributor>
	<skos:broadMatch rdf:resource="http://vocab.aodn.org.au/def/organisation_classes/category/4"/>
	<skos:prefLabel xml:lang="en">Japan Agency for Marine-Earth Science and Technology (JAMSTEC)</skos:prefLabel>
	<skos:altLabel xml:lang="en"></skos:altLabel>
	<skos:hiddenLabel xml:lang="en">JAMSTEC</skos:hiddenLabel>
	<skos:definition xml:lang="en">On April 1, 2004, Japan Agency for Marine-Earth Science and Technology (JAMSTEC) was inaugurated as one of the independent administrative institutions upon re-organized from its former organization, Japan Marine Science and Technology Center. JAMSTEC has the main objective to contribute to the advancement of academic research in addition to the improvement of marine science and technology by proceeding the fundamental research and development on marine, and the cooperative activities on the academic research related to the Ocean for the benefit of the peace and human welfare.</skos:definition>
	<dc:source rdf:datatype="http://www.w3.org/2001/XMLSchema#string">Australian Ocean Data Network Organisation Register</dc:source>
	<dc:publisher rdf:datatype="http://www.w3.org/2001/XMLSchema#string">eMarine Information Infrastructure (eMMI)</dc:publisher>
	<skos:exactMatch rdf:resource="http://seadatanet.maris2.nl/v_edmo/print.asp?n_code=1537"/>
	<skos:topConceptOf rdf:resource="http://vocab.aodn.org.au/def/organisation/1"/>
	<skos:inScheme rdf:resource="http://vocab.aodn.org.au/def/organisation/1"/>
</rdf:Description>

<rdf:Description rdf:about="http://vocab.aodn.org.au/def/organisation/entity/379">
	<rdf:type rdf:resource="http://www.w3.org/2000/01/rdf-schema#Resource"/>
	<rdf:type rdf:resource="http://www.w3.org/2004/02/skos/core#Concept"/>
	<dcterms:modified rdf:datatype="http://www.w3.org/2001/XMLSchema#dateTime">2015-09-29T03:32:58Z</dcterms:modified>
	<dcterms:creator rdf:datatype="http://www.w3.org/2001/XMLSchema#string">Natalia Atkins</dcterms:creator>
	<dcterms:created rdf:datatype="http://www.w3.org/2001/XMLSchema#dateTime">2015-09-18T10:38:15Z</dcterms:created>
	<dcterms:contributor rdf:datatype="http://www.w3.org/2001/XMLSchema#string">eMII_Atkins.Natalia</dcterms:contributor>
	<skos:broadMatch rdf:resource="http://vocab.aodn.org.au/def/organisation_classes/category/4"/>
	<skos:prefLabel xml:lang="en">Japan Meteorological Agency (JMA)</skos:prefLabel>
	<skos:altLabel xml:lang="en"></skos:altLabel>
	<skos:hiddenLabel xml:lang="en">JMA</skos:hiddenLabel>
	<skos:definition xml:lang="en"></skos:definition>
	<dc:source rdf:datatype="http://www.w3.org/2001/XMLSchema#string">Australian Ocean Data Network Organisation Register</dc:source>
	<dc:publisher rdf:datatype="http://www.w3.org/2001/XMLSchema#string">eMarine Information Infrastructure (eMMI)</dc:publisher>
	<skos:exactMatch rdf:resource="http://seadatanet.maris2.nl/v_edmo/print.asp?n_code=1778"/>
	<skos:topConceptOf rdf:resource="http://vocab.aodn.org.au/def/organisation/1"/>
	<skos:inScheme rdf:resource="http://vocab.aodn.org.au/def/organisation/1"/>
</rdf:Description>

<rdf:Description rdf:about="http://vocab.aodn.org.au/def/organisation/entity/380">
	<rdf:type rdf:resource="http://www.w3.org/2000/01/rdf-schema#Resource"/>
	<rdf:type rdf:resource="http://www.w3.org/2004/02/skos/core#Concept"/>
	<dcterms:modified rdf:datatype="http://www.w3.org/2001/XMLSchema#dateTime">2015-09-29T03:33:11Z</dcterms:modified>
	<dcterms:modified rdf:datatype="http://www.w3.org/2001/XMLSchema#dateTime">2015-09-29T03:33:10Z</dcterms:modified>
	<dcterms:creator rdf:datatype="http://www.w3.org/2001/XMLSchema#string">Natalia Atkins</dcterms:creator>
	<dcterms:created rdf:datatype="http://www.w3.org/2001/XMLSchema#dateTime">2015-09-18T10:38:15Z</dcterms:created>
	<dcterms:contributor rdf:datatype="http://www.w3.org/2001/XMLSchema#string">eMII_Atkins.Natalia</dcterms:contributor>
	<skos:broadMatch rdf:resource="http://vocab.aodn.org.au/def/organisation_classes/category/4"/>
	<skos:prefLabel xml:lang="en">Korea Meteorological Administration (KMA)</skos:prefLabel>
	<skos:altLabel xml:lang="en"></skos:altLabel>
	<skos:hiddenLabel xml:lang="en">KMA</skos:hiddenLabel>
	<skos:definition xml:lang="en"></skos:definition>
	<dc:source rdf:datatype="http://www.w3.org/2001/XMLSchema#string">Australian Ocean Data Network Organisation Register</dc:source>
	<dc:publisher rdf:datatype="http://www.w3.org/2001/XMLSchema#string">eMarine Information Infrastructure (eMMI)</dc:publisher>
	<skos:exactMatch rdf:resource="http://seadatanet.maris2.nl/v_edmo/print.asp?n_code=3333"/>
	<skos:topConceptOf rdf:resource="http://vocab.aodn.org.au/def/organisation/1"/>
	<skos:inScheme rdf:resource="http://vocab.aodn.org.au/def/organisation/1"/>
</rdf:Description>

<rdf:Description rdf:about="http://vocab.aodn.org.au/def/organisation/entity/381">
	<rdf:type rdf:resource="http://www.w3.org/2000/01/rdf-schema#Resource"/>
	<rdf:type rdf:resource="http://www.w3.org/2004/02/skos/core#Concept"/>
	<dcterms:modified rdf:datatype="http://www.w3.org/2001/XMLSchema#dateTime">2015-09-29T03:33:23Z</dcterms:modified>
	<dcterms:creator rdf:datatype="http://www.w3.org/2001/XMLSchema#string">Natalia Atkins</dcterms:creator>
	<dcterms:created rdf:datatype="http://www.w3.org/2001/XMLSchema#dateTime">2015-09-18T10:38:15Z</dcterms:created>
	<dcterms:contributor rdf:datatype="http://www.w3.org/2001/XMLSchema#string">eMII_Atkins.Natalia</dcterms:contributor>
	<skos:broadMatch rdf:resource="http://vocab.aodn.org.au/def/organisation_classes/category/4"/>
	<skos:prefLabel xml:lang="en">Korea Institute Of Ocean Science and Technology (KIOST)</skos:prefLabel>
	<skos:altLabel xml:lang="en"></skos:altLabel>
	<skos:hiddenLabel xml:lang="en">KIOST</skos:hiddenLabel>
	<skos:definition xml:lang="en"></skos:definition>
	<dc:source rdf:datatype="http://www.w3.org/2001/XMLSchema#string">Australian Ocean Data Network Organisation Register</dc:source>
	<dc:publisher rdf:datatype="http://www.w3.org/2001/XMLSchema#string">eMarine Information Infrastructure (eMMI)</dc:publisher>
	<skos:exactMatch rdf:resource="http://seadatanet.maris2.nl/v_edmo/print.asp?n_code=3332"/>
	<skos:topConceptOf rdf:resource="http://vocab.aodn.org.au/def/organisation/1"/>
	<skos:inScheme rdf:resource="http://vocab.aodn.org.au/def/organisation/1"/>
	<skos:scopeNote xml:lang="en">Replaces http://vocab.aodn.org.au/def/organisation/entity/394</skos:scopeNote>
	<dcterms:replaces rdf:resource="http://vocab.aodn.org.au/organisation/entity/394"/>
	<dcterms:replaces xml:lang="en">Korea Ocean Research and Development Institute (KORDI)</dcterms:replaces>
</rdf:Description>

<rdf:Description rdf:about="http://vocab.aodn.org.au/def/organisation/entity/382">
	<rdf:type rdf:resource="http://www.w3.org/2000/01/rdf-schema#Resource"/>
	<rdf:type rdf:resource="http://www.w3.org/2004/02/skos/core#Concept"/>
	<dcterms:modified rdf:datatype="http://www.w3.org/2001/XMLSchema#dateTime">2015-09-29T03:33:35Z</dcterms:modified>
	<dcterms:creator rdf:datatype="http://www.w3.org/2001/XMLSchema#string">Natalia Atkins</dcterms:creator>
	<dcterms:created rdf:datatype="http://www.w3.org/2001/XMLSchema#dateTime">2015-09-18T10:38:15Z</dcterms:created>
	<dcterms:contributor rdf:datatype="http://www.w3.org/2001/XMLSchema#string">eMII_Atkins.Natalia</dcterms:contributor>
	<skos:broadMatch rdf:resource="http://vocab.aodn.org.au/def/organisation_classes/category/4"/>
	<skos:prefLabel xml:lang="en">GEOMAR Helmholtz Centre for Ocean Research Kiel</skos:prefLabel>
	<skos:altLabel xml:lang="en"></skos:altLabel>
	<skos:hiddenLabel xml:lang="en"></skos:hiddenLabel>
	<skos:definition xml:lang="en">GEOMAR | Helmholtz Centre for Ocean Research is the successor of the Leibniz Institute of Marine Sciences (IFM-GEOMAR) which was founded in January 2004 through the merger of the Institut für Meereskunde (IfM) and the Research Center for Marine Geosciences (GEOMAR). The institute is a member of the Helmholtz Association and employs more than 750 scientific and technical staff. The institutes’ mandate is the interdisciplinary investigation of all relevant aspects of modern marine sciences, from sea floor geology to marine meteorology. Research is conducted worldwide in all oceans. The institute has four major research divisions: Ocean Circulation and Climate Dynamics, Marine Biogeochemistry, Marine Ecology, and Dynamics of the Ocean Floor.</skos:definition>
	<dc:source rdf:datatype="http://www.w3.org/2001/XMLSchema#string">Australian Ocean Data Network Organisation Register</dc:source>
	<dc:publisher rdf:datatype="http://www.w3.org/2001/XMLSchema#string">eMarine Information Infrastructure (eMMI)</dc:publisher>
	<skos:exactMatch rdf:resource="http://seadatanet.maris2.nl/v_edmo/print.asp?n_code=2947"/>
	<skos:topConceptOf rdf:resource="http://vocab.aodn.org.au/def/organisation/1"/>
	<skos:inScheme rdf:resource="http://vocab.aodn.org.au/def/organisation/1"/>
	<skos:scopeNote xml:lang="en">Replaces http://vocab.aodn.org.au/def/organisation/entity/319</skos:scopeNote>
	<dcterms:replaces xml:lang="en">Leibniz Institute of Marine Sciences (IFM-GEOMAR), University of Kiel</dcterms:replaces>
	<dcterms:replaces rdf:resource="http://vocab.aodn.org.au/organisation/entity/319"/>
</rdf:Description>

<rdf:Description rdf:about="http://vocab.aodn.org.au/def/organisation/entity/383">
	<rdf:type rdf:resource="http://www.w3.org/2000/01/rdf-schema#Resource"/>
	<rdf:type rdf:resource="http://www.w3.org/2004/02/skos/core#Concept"/>
	<dcterms:modified rdf:datatype="http://www.w3.org/2001/XMLSchema#dateTime">2015-09-29T03:33:57Z</dcterms:modified>
	<dcterms:creator rdf:datatype="http://www.w3.org/2001/XMLSchema#string">Natalia Atkins</dcterms:creator>
	<dcterms:created rdf:datatype="http://www.w3.org/2001/XMLSchema#dateTime">2015-09-18T10:38:15Z</dcterms:created>
	<dcterms:contributor rdf:datatype="http://www.w3.org/2001/XMLSchema#string">eMII_Atkins.Natalia</dcterms:contributor>
	<skos:broadMatch rdf:resource="http://vocab.aodn.org.au/def/organisation_classes/category/4"/>
	<skos:prefLabel xml:lang="en">National Institute of Water and Atmospheric Research (NIWA)</skos:prefLabel>
	<skos:altLabel xml:lang="en"></skos:altLabel>
	<skos:hiddenLabel xml:lang="en">NIWA</skos:hiddenLabel>
	<skos:definition xml:lang="en">NIWA conducts commercial and non-commercial research across a broad range of disciplines in the environmental sciences. It also maintains nationally and, in some cases, internationally important environmental monitoring networks, databases, and collections.</skos:definition>
	<dc:source rdf:datatype="http://www.w3.org/2001/XMLSchema#string">Australian Ocean Data Network Organisation Register</dc:source>
	<dc:publisher rdf:datatype="http://www.w3.org/2001/XMLSchema#string">eMarine Information Infrastructure (eMMI)</dc:publisher>
	<skos:exactMatch rdf:resource="http://seadatanet.maris2.nl/v_edmo/print.asp?n_code=3739"/>
	<skos:topConceptOf rdf:resource="http://vocab.aodn.org.au/def/organisation/1"/>
	<skos:inScheme rdf:resource="http://vocab.aodn.org.au/def/organisation/1"/>
</rdf:Description>

<rdf:Description rdf:about="http://vocab.aodn.org.au/def/organisation/entity/384">
	<rdf:type rdf:resource="http://www.w3.org/2000/01/rdf-schema#Resource"/>
	<rdf:type rdf:resource="http://www.w3.org/2004/02/skos/core#Concept"/>
	<dcterms:modified rdf:datatype="http://www.w3.org/2001/XMLSchema#dateTime">2015-09-29T03:34:05Z</dcterms:modified>
	<dcterms:creator rdf:datatype="http://www.w3.org/2001/XMLSchema#string">Natalia Atkins</dcterms:creator>
	<dcterms:created rdf:datatype="http://www.w3.org/2001/XMLSchema#dateTime">2015-09-18T10:38:15Z</dcterms:created>
	<dcterms:contributor rdf:datatype="http://www.w3.org/2001/XMLSchema#string">eMII_Atkins.Natalia</dcterms:contributor>
	<skos:broadMatch rdf:resource="http://vocab.aodn.org.au/def/organisation_classes/category/4"/>
	<skos:prefLabel xml:lang="en">National Oceanic and Atmospheric Administration (NOAA)</skos:prefLabel>
	<skos:altLabel xml:lang="en"></skos:altLabel>
	<skos:hiddenLabel xml:lang="en">NOAA</skos:hiddenLabel>
	<skos:definition xml:lang="en"></skos:definition>
	<dc:source rdf:datatype="http://www.w3.org/2001/XMLSchema#string">Australian Ocean Data Network Organisation Register</dc:source>
	<dc:publisher rdf:datatype="http://www.w3.org/2001/XMLSchema#string">eMarine Information Infrastructure (eMMI)</dc:publisher>
	<skos:exactMatch rdf:resource="http://seadatanet.maris2.nl/v_edmo/print.asp?n_code=1433"/>
	<skos:narrower rdf:resource="http://vocab.aodn.org.au/def/organisation/entity/370"/>
	<skos:narrower rdf:resource="http://vocab.aodn.org.au/def/organisation/entity/392"/>
	<skos:topConceptOf rdf:resource="http://vocab.aodn.org.au/def/organisation/1"/>
	<skos:inScheme rdf:resource="http://vocab.aodn.org.au/def/organisation/1"/>
</rdf:Description>

<rdf:Description rdf:about="http://vocab.aodn.org.au/def/organisation/entity/385">
	<rdf:type rdf:resource="http://www.w3.org/2000/01/rdf-schema#Resource"/>
	<rdf:type rdf:resource="http://www.w3.org/2004/02/skos/core#Concept"/>
	<dcterms:modified rdf:datatype="http://www.w3.org/2001/XMLSchema#dateTime">2015-09-29T03:34:16Z</dcterms:modified>
	<dcterms:creator rdf:datatype="http://www.w3.org/2001/XMLSchema#string">Natalia Atkins</dcterms:creator>
	<dcterms:created rdf:datatype="http://www.w3.org/2001/XMLSchema#dateTime">2015-09-18T10:38:15Z</dcterms:created>
	<dcterms:contributor rdf:datatype="http://www.w3.org/2001/XMLSchema#string">eMII_Atkins.Natalia</dcterms:contributor>
	<skos:broadMatch rdf:resource="http://vocab.aodn.org.au/def/organisation_classes/category/4"/>
	<skos:prefLabel xml:lang="en">National Aeronautics and Space Administration Jet Propulsion Laboratory (NASA JPL)</skos:prefLabel>
	<skos:altLabel xml:lang="en"></skos:altLabel>
	<skos:hiddenLabel xml:lang="en">NASA JPL</skos:hiddenLabel>
	<skos:definition xml:lang="en">The Jet Propulsion Laboratory is a federally funded research and development center and NASA field center located in La Cañada Flintridge, California</skos:definition>
	<dc:source rdf:datatype="http://www.w3.org/2001/XMLSchema#string">Australian Ocean Data Network Organisation Register</dc:source>
	<dc:publisher rdf:datatype="http://www.w3.org/2001/XMLSchema#string">eMarine Information Infrastructure (eMMI)</dc:publisher>
	<skos:exactMatch rdf:resource="http://seadatanet.maris2.nl/v_edmo/print.asp?n_code=1224"/>
	<skos:topConceptOf rdf:resource="http://vocab.aodn.org.au/def/organisation/1"/>
	<skos:inScheme rdf:resource="http://vocab.aodn.org.au/def/organisation/1"/>
</rdf:Description>

<rdf:Description rdf:about="http://vocab.aodn.org.au/def/organisation/entity/386">
	<rdf:type rdf:resource="http://www.w3.org/2000/01/rdf-schema#Resource"/>
	<rdf:type rdf:resource="http://www.w3.org/2004/02/skos/core#Concept"/>
	<dcterms:modified rdf:datatype="http://www.w3.org/2001/XMLSchema#dateTime">2015-09-29T03:34:28Z</dcterms:modified>
	<dcterms:creator rdf:datatype="http://www.w3.org/2001/XMLSchema#string">Natalia Atkins</dcterms:creator>
	<dcterms:created rdf:datatype="http://www.w3.org/2001/XMLSchema#dateTime">2015-09-18T10:38:15Z</dcterms:created>
	<dcterms:contributor rdf:datatype="http://www.w3.org/2001/XMLSchema#string">eMII_Atkins.Natalia</dcterms:contributor>
	<skos:broadMatch rdf:resource="http://vocab.aodn.org.au/def/organisation_classes/category/4"/>
	<skos:prefLabel xml:lang="en">Naval Oceanographic Office (NAVO)</skos:prefLabel>
	<skos:altLabel xml:lang="en"></skos:altLabel>
	<skos:hiddenLabel xml:lang="en">NAVO</skos:hiddenLabel>
	<skos:definition xml:lang="en">The Naval Oceanographic Office (NAVO) maximizes seapower by applying relevant oceanographic knowledge in support of U.S. National Security.</skos:definition>
	<dc:source rdf:datatype="http://www.w3.org/2001/XMLSchema#string">Australian Ocean Data Network Organisation Register</dc:source>
	<dc:publisher rdf:datatype="http://www.w3.org/2001/XMLSchema#string">eMarine Information Infrastructure (eMMI)</dc:publisher>
	<skos:exactMatch rdf:resource="http://seadatanet.maris2.nl/v_edmo/print.asp?n_code=3577"/>
	<skos:topConceptOf rdf:resource="http://vocab.aodn.org.au/def/organisation/1"/>
	<skos:inScheme rdf:resource="http://vocab.aodn.org.au/def/organisation/1"/>
</rdf:Description>

<rdf:Description rdf:about="http://vocab.aodn.org.au/def/organisation/entity/387">
	<rdf:type rdf:resource="http://www.w3.org/2000/01/rdf-schema#Resource"/>
	<rdf:type rdf:resource="http://www.w3.org/2004/02/skos/core#Concept"/>
	<dcterms:modified rdf:datatype="http://www.w3.org/2001/XMLSchema#dateTime">2015-09-29T03:34:38Z</dcterms:modified>
	<dcterms:creator rdf:datatype="http://www.w3.org/2001/XMLSchema#string">Natalia Atkins</dcterms:creator>
	<dcterms:created rdf:datatype="http://www.w3.org/2001/XMLSchema#dateTime">2015-09-18T10:38:15Z</dcterms:created>
	<dcterms:contributor rdf:datatype="http://www.w3.org/2001/XMLSchema#string">eMII_Atkins.Natalia</dcterms:contributor>
	<skos:broadMatch rdf:resource="http://vocab.aodn.org.au/def/organisation_classes/category/4"/>
	<skos:prefLabel xml:lang="en">National Oceanography Centre, Southampton (NOC)</skos:prefLabel>
	<skos:altLabel xml:lang="en"></skos:altLabel>
	<skos:hiddenLabel xml:lang="en">NOC</skos:hiddenLabel>
	<skos:definition xml:lang="en">The National Oceanography Centre, part of the Natural Environment Research Council (NERC) is one of the few world-class centres of excellence in ocean sciences, earth sciences and ocean technology. This unique combination of interdisciplinary research and teaching resources comprises the University of Southampton's School of Ocean and Earth Science together with 4 specialist NERC research divisions. The scientific mission of the National Oceanography Centre is: To deliver scientific excellence and understanding of the earth and its oceans as a dynamic interdisciplinary system; To provide the highest quality teaching and training in ocean and earth science within an active research environment;     To provide large scale national facilities for ocean and earth science.
This mission is achieved through integration between staff and facilities of the Natural Environment Research Council and the University of Southampton. Success in this mission will deliver our goal, to establish NOC as a major national and international centre of excellence for research, teaching and training in marine and earth science and in marine technology. Research work is conducted through a variety of organisations. Data are retained in a variety of forms and individual members of staff of the Department should be contacted for particular data. Details of the Department are available from the Departmental Secretary. Degrees of B.Sc., M.Sc. and Ph.D. are awarded in Oceanography.</skos:definition>
	<dc:source rdf:datatype="http://www.w3.org/2001/XMLSchema#string">Australian Ocean Data Network Organisation Register</dc:source>
	<dc:publisher rdf:datatype="http://www.w3.org/2001/XMLSchema#string">eMarine Information Infrastructure (eMMI)</dc:publisher>
	<skos:exactMatch rdf:resource="http://seadatanet.maris2.nl/v_edmo/print.asp?n_code=17"/>
	<skos:topConceptOf rdf:resource="http://vocab.aodn.org.au/def/organisation/1"/>
	<skos:inScheme rdf:resource="http://vocab.aodn.org.au/def/organisation/1"/>
</rdf:Description>

<rdf:Description rdf:about="http://vocab.aodn.org.au/def/organisation/entity/388">
	<rdf:type rdf:resource="http://www.w3.org/2000/01/rdf-schema#Resource"/>
	<rdf:type rdf:resource="http://www.w3.org/2004/02/skos/core#Concept"/>
	<dcterms:modified rdf:datatype="http://www.w3.org/2001/XMLSchema#dateTime">2015-09-29T03:34:52Z</dcterms:modified>
	<dcterms:creator rdf:datatype="http://www.w3.org/2001/XMLSchema#string">Natalia Atkins</dcterms:creator>
	<dcterms:created rdf:datatype="http://www.w3.org/2001/XMLSchema#dateTime">2015-09-18T10:38:15Z</dcterms:created>
	<dcterms:contributor rdf:datatype="http://www.w3.org/2001/XMLSchema#string">eMII_Atkins.Natalia</dcterms:contributor>
	<skos:broadMatch rdf:resource="http://vocab.aodn.org.au/def/organisation_classes/category/4"/>
	<skos:prefLabel xml:lang="en">PANGAEA - Data Publisher for Earth and Environmental Science</skos:prefLabel>
	<skos:altLabel xml:lang="en"></skos:altLabel>
	<skos:hiddenLabel xml:lang="en"></skos:hiddenLabel>
	<skos:definition xml:lang="en">The Centre for Marine Environmental Sciences (MARUM) at University Bremen (UniHB), in collaboration with the Alfred Wegener Institute for Polar and Marine Research (AWI), operates PANGAEA®, the Publishing Network for Geoscientific and Environmental Data (www.PANGAEA.de) as a permanent facility, partnering in over 50 research projects at national (Germany), European and international levels. PANGAEA® aims at collecting, scrutinising, and disseminating geo-referenced data about natural and anthropogenic components and functions in ecosystems at scales ranging from individual organisms, mesoscale features (e.g. upwelling, eddies, seamounts, coral reefs), and oceanic basin to global planetary scales. Core services supplied by PANGAEA® are scientific data management, long-term data archiving, data publication, and data dissemination via visualisation and analysis software and via interoperability with other European and international data dissemination systems. Data management includes quality control of metadata and the development of ontologies and vocabularies according to international protocols and standards. PANGAEA® has further defined work flows and technologies to allow automatic ingestion of data from marine observatories based on OGC standards ( (SWE - Sensor Web Enablement). Metadata are extensive and each dataset is citable and accessible by Digital Object Identifier (DOI). Datasets published by PANGAEA® are extremely diverse and include for example water column profiles, sediment core profiles, biogeographic distributions, meteorological and oceanographic time series, vital rate measurements on individual organisms or communities, sea bed photographs, audio and video records, and ROV surveys. PANGAEA® integrates biological data on plankton (including viruses, bacteria, autotrophic and heterotophic protists, crustaceans and jellyfish), fish, corals, micro-, meio- and macrobenthos, marine mammals and birds. In addition to contemporary observations we offer an extensive paleobiogeographic record from marine sediment cores. Biological data include key biodiversity parameters such as taxon-specific abundance and biomass, and also an extensive range of parameters describing the life history and vital rates of marine life. PANGAEA® is accredited as a World Data Centre by the International Council for Sciences (ICSU) World Data System (WDS) and accredited as World Radiation Monitoring Centre (WRMC) by the World Meteorological Organisation (WMO) as part of their WMO Information System. At present PANGAEA® holds metadata and data for more than 300.000 datasets comprising more than 6 billion data items for more than 80.000 different measurement types (parameters), more than 17.000 principal investigators (authors), and around 20.000 references to journal articles. The system is operated in the sense of the Berlin Declaration on Open Access to Knowledge in the Sciences and Humanities which is a follow up to the Budapest Open Access Initiative. Some ongoing projects are under moratorium so that access to data may be restricted, but metadata is always freely accessible.</skos:definition>
	<dc:source rdf:datatype="http://www.w3.org/2001/XMLSchema#string">Australian Ocean Data Network Organisation Register</dc:source>
	<dc:publisher rdf:datatype="http://www.w3.org/2001/XMLSchema#string">eMarine Information Infrastructure (eMMI)</dc:publisher>
	<skos:exactMatch rdf:resource="http://seadatanet.maris2.nl/v_edmo/print.asp?n_code=3234"/>
	<skos:topConceptOf rdf:resource="http://vocab.aodn.org.au/def/organisation/1"/>
	<skos:inScheme rdf:resource="http://vocab.aodn.org.au/def/organisation/1"/>
</rdf:Description>

<rdf:Description rdf:about="http://vocab.aodn.org.au/def/organisation/entity/389">
	<rdf:type rdf:resource="http://www.w3.org/2000/01/rdf-schema#Resource"/>
	<rdf:type rdf:resource="http://www.w3.org/2004/02/skos/core#Concept"/>
	<dcterms:modified rdf:datatype="http://www.w3.org/2001/XMLSchema#dateTime">2015-09-29T03:35:03Z</dcterms:modified>
	<dcterms:creator rdf:datatype="http://www.w3.org/2001/XMLSchema#string">Natalia Atkins</dcterms:creator>
	<dcterms:created rdf:datatype="http://www.w3.org/2001/XMLSchema#dateTime">2015-09-18T10:38:15Z</dcterms:created>
	<dcterms:contributor rdf:datatype="http://www.w3.org/2001/XMLSchema#string">eMII_Atkins.Natalia</dcterms:contributor>
	<skos:broadMatch rdf:resource="http://vocab.aodn.org.au/def/organisation_classes/category/4"/>
	<skos:prefLabel xml:lang="en">NIOZ Royal Netherlands Institute for Sea Research</skos:prefLabel>
	<skos:altLabel xml:lang="en"></skos:altLabel>
	<skos:hiddenLabel xml:lang="en"></skos:hiddenLabel>
	<skos:definition xml:lang="en">NIOZ Royal Netherlands Institute for Sea Research is the National Oceanographic Institute of the Netherlands. NIOZ is part of the Netherlands Organization for Scientific Research (NWO). The institute employs around 220 people and the annual budget is approximately €20 million. The mission of NIOZ is to gain and communicate scientific knowledge on seas and oceans for the understanding and sustainability of our planet. The institute also facilitates and supports marine research and education in the Netherlands and Europe. In order to fulfil its mission, the institute performs tasks in three specific fields: Research: The emphasis is on innovative and independent fundamental research in continental seas and open oceans. The institute also carries out research based on societal questions when this merges well with its fundamental work. The senior scientists at NIOZ all participate in international research projects. Education: The institute educates PhD and other students of universities and schools for professional education. Together universities NIOZ also organises courses for PhD students and master students in the marine sciences. A number of our senior scientists is also appointed as professor at Dutch and foreign universities. Facilitary services: NIOZ invites marine scientists from Dutch and foreign institutes and universities to write scientific proposals involving the institute’s research vessels, laboratories, and the large research equipment, which is often designed and built by the institute’s own technical department. The basic oceanographic disciplines at NIOZ are physics, chemistry, biology and geology. Multidisciplinary research is regarded as one of the main strengths of the institute. There are 5 scientific departments: Physical Oceanography, Marine Geology, Marine Organic Biogeochemistry, Biological Oceanography and Marine Ecology.</skos:definition>
	<dc:source rdf:datatype="http://www.w3.org/2001/XMLSchema#string">Australian Ocean Data Network Organisation Register</dc:source>
	<dc:publisher rdf:datatype="http://www.w3.org/2001/XMLSchema#string">eMarine Information Infrastructure (eMMI)</dc:publisher>
	<skos:exactMatch rdf:resource="http://seadatanet.maris2.nl/v_edmo/print.asp?n_code=630"/>
	<skos:topConceptOf rdf:resource="http://vocab.aodn.org.au/def/organisation/1"/>
	<skos:inScheme rdf:resource="http://vocab.aodn.org.au/def/organisation/1"/>
</rdf:Description>

<rdf:Description rdf:about="http://vocab.aodn.org.au/def/organisation/entity/390">
	<rdf:type rdf:resource="http://www.w3.org/2000/01/rdf-schema#Resource"/>
	<rdf:type rdf:resource="http://www.w3.org/2004/02/skos/core#Concept"/>
	<dcterms:modified rdf:datatype="http://www.w3.org/2001/XMLSchema#dateTime">2015-09-29T03:35:12Z</dcterms:modified>
	<dcterms:creator rdf:datatype="http://www.w3.org/2001/XMLSchema#string">Natalia Atkins</dcterms:creator>
	<dcterms:created rdf:datatype="http://www.w3.org/2001/XMLSchema#dateTime">2015-09-18T10:38:15Z</dcterms:created>
	<dcterms:contributor rdf:datatype="http://www.w3.org/2001/XMLSchema#string">eMII_Atkins.Natalia</dcterms:contributor>
	<skos:broadMatch rdf:resource="http://vocab.aodn.org.au/def/organisation_classes/category/4"/>
	<skos:prefLabel xml:lang="en">RPS Group</skos:prefLabel>
	<skos:altLabel xml:lang="en"></skos:altLabel>
	<skos:hiddenLabel xml:lang="en"></skos:hiddenLabel>
	<skos:definition xml:lang="en">RPS is an international consultancy providing advice upon: the exploration and production of energy and other natural resources, the development and management of the built and natural environment.</skos:definition>
	<dc:source rdf:datatype="http://www.w3.org/2001/XMLSchema#string">Australian Ocean Data Network Organisation Register</dc:source>
	<dc:publisher rdf:datatype="http://www.w3.org/2001/XMLSchema#string">eMarine Information Infrastructure (eMMI)</dc:publisher>
	<skos:exactMatch rdf:resource="http://seadatanet.maris2.nl/v_edmo/print.asp?n_code=3057"/>
	<skos:topConceptOf rdf:resource="http://vocab.aodn.org.au/def/organisation/1"/>
	<skos:inScheme rdf:resource="http://vocab.aodn.org.au/def/organisation/1"/>
</rdf:Description>

<rdf:Description rdf:about="http://vocab.aodn.org.au/def/organisation/entity/391">
	<rdf:type rdf:resource="http://www.w3.org/2000/01/rdf-schema#Resource"/>
	<rdf:type rdf:resource="http://www.w3.org/2004/02/skos/core#Concept"/>
	<dcterms:modified rdf:datatype="http://www.w3.org/2001/XMLSchema#dateTime">2015-09-29T03:35:24Z</dcterms:modified>
	<dcterms:creator rdf:datatype="http://www.w3.org/2001/XMLSchema#string">Natalia Atkins</dcterms:creator>
	<dcterms:created rdf:datatype="http://www.w3.org/2001/XMLSchema#dateTime">2015-09-18T10:38:15Z</dcterms:created>
	<dcterms:contributor rdf:datatype="http://www.w3.org/2001/XMLSchema#string">eMII_Atkins.Natalia</dcterms:contributor>
	<skos:broadMatch rdf:resource="http://vocab.aodn.org.au/def/organisation_classes/category/4"/>
	<skos:prefLabel xml:lang="en">U.S. Geological Survey (USGS)</skos:prefLabel>
	<skos:altLabel xml:lang="en"></skos:altLabel>
	<skos:hiddenLabel xml:lang="en">USGS</skos:hiddenLabel>
	<skos:definition xml:lang="en">Mission: The USGS serves the Nation by providing reliable scientific information to describe and understand the Earth; minimize loss of life and property from natural disasters; manage water, biological, energy, and mineral resources; and enhance and protect our quality of life. Vision: USGS has become a world leader in the natural sciences thanks to our scientific excellence and responsiveness to society's needs. As the Nation's largest water, earth, and biological science and civilian mapping agency, the U.S. Geological Survey (USGS) collects, monitors, analyzes, and provides scientific understanding about natural resource conditions, issues, and problems. The diversity of our scientific expertise enables us to carry out large-scale, multi-disciplinary investigations and provide impartial scientific information to resource managers, planners, and other customers.</skos:definition>
	<dc:source rdf:datatype="http://www.w3.org/2001/XMLSchema#string">Australian Ocean Data Network Organisation Register</dc:source>
	<dc:publisher rdf:datatype="http://www.w3.org/2001/XMLSchema#string">eMarine Information Infrastructure (eMMI)</dc:publisher>
	<skos:exactMatch rdf:resource="http://seadatanet.maris2.nl/v_edmo/print.asp?n_code=1566"/>
	<skos:topConceptOf rdf:resource="http://vocab.aodn.org.au/def/organisation/1"/>
	<skos:inScheme rdf:resource="http://vocab.aodn.org.au/def/organisation/1"/>
</rdf:Description>

<rdf:Description rdf:about="http://vocab.aodn.org.au/def/organisation/entity/393">
	<rdf:type rdf:resource="http://www.w3.org/2000/01/rdf-schema#Resource"/>
	<rdf:type rdf:resource="http://www.w3.org/2004/02/skos/core#Concept"/>
	<dcterms:modified rdf:datatype="http://www.w3.org/2001/XMLSchema#dateTime">2015-09-29T03:35:31Z</dcterms:modified>
	<dcterms:creator rdf:datatype="http://www.w3.org/2001/XMLSchema#string">Natalia Atkins</dcterms:creator>
	<dcterms:created rdf:datatype="http://www.w3.org/2001/XMLSchema#dateTime">2015-09-18T10:38:15Z</dcterms:created>
	<dcterms:contributor rdf:datatype="http://www.w3.org/2001/XMLSchema#string">eMII_Atkins.Natalia</dcterms:contributor>
	<skos:broadMatch rdf:resource="http://vocab.aodn.org.au/def/organisation_classes/category/4"/>
	<skos:prefLabel xml:lang="en">Woods Hole Oceanographic Institution (WHOI)</skos:prefLabel>
	<skos:altLabel xml:lang="en"></skos:altLabel>
	<skos:hiddenLabel xml:lang="en">WHOI</skos:hiddenLabel>
	<skos:definition xml:lang="en">Woods Hole Oceanographic Institution is the world's largest private, non-profit oceanographic research institution and a global leader in the study and exploration of the ocean.</skos:definition>
	<dc:source rdf:datatype="http://www.w3.org/2001/XMLSchema#string">Australian Ocean Data Network Organisation Register</dc:source>
	<dc:publisher rdf:datatype="http://www.w3.org/2001/XMLSchema#string">eMarine Information Infrastructure (eMMI)</dc:publisher>
	<skos:exactMatch rdf:resource="http://seadatanet.maris2.nl/v_edmo/print.asp?n_code=3844"/>
	<skos:topConceptOf rdf:resource="http://vocab.aodn.org.au/def/organisation/1"/>
	<skos:inScheme rdf:resource="http://vocab.aodn.org.au/def/organisation/1"/>
</rdf:Description>

<rdf:Description rdf:about="http://vocab.aodn.org.au/def/organisation/entity/394">
	<rdf:type rdf:resource="http://www.w3.org/2000/01/rdf-schema#Resource"/>
	<rdf:type rdf:resource="http://www.w3.org/2004/02/skos/core#Concept"/>
	<dcterms:modified rdf:datatype="http://www.w3.org/2001/XMLSchema#dateTime">2015-09-29T03:35:48Z</dcterms:modified>
	<dcterms:creator rdf:datatype="http://www.w3.org/2001/XMLSchema#string">Natalia Atkins</dcterms:creator>
	<dcterms:created rdf:datatype="http://www.w3.org/2001/XMLSchema#dateTime">2015-09-18T10:38:15Z</dcterms:created>
	<dcterms:contributor rdf:datatype="http://www.w3.org/2001/XMLSchema#string">eMII_Atkins.Natalia</dcterms:contributor>
	<skos:broadMatch rdf:resource="http://vocab.aodn.org.au/def/organisation_classes/category/4"/>
	<skos:prefLabel xml:lang="en">Korea Ocean Research and Development Institute (KORDI)</skos:prefLabel>
	<skos:altLabel xml:lang="en"></skos:altLabel>
	<skos:hiddenLabel xml:lang="en">KORDI</skos:hiddenLabel>
	<skos:definition xml:lang="en">The Korean Ocean Research and Development Institute (KORDI) with its headquarters in Ansan, Gyeonggi-do, South Korea, has driven development of the marine sciences and technology of Korea for over 40 years since its establishment in 1973. It started functioning with a new name of Korean Institute of Ocean Science and Technology (KIOST) from July 1, 2012. (Courtesy of wikipedia)</skos:definition>
	<dc:source rdf:datatype="http://www.w3.org/2001/XMLSchema#string">Australian Ocean Data Network Organisation Register</dc:source>
	<dc:publisher rdf:datatype="http://www.w3.org/2001/XMLSchema#string">eMarine Information Infrastructure (eMMI)</dc:publisher>
	<skos:topConceptOf rdf:resource="http://vocab.aodn.org.au/def/organisation/1"/>
	<skos:inScheme rdf:resource="http://vocab.aodn.org.au/def/organisation/1"/>
	<skos:scopeNote xml:lang="en">Organisation no longer exists</skos:scopeNote>
	<skos:scopeNote xml:lang="en">Organisation no longer exists. http://vocab.aodn.org.au/def/organisation/entity/381</skos:scopeNote>
	<dcterms:isReplacedBy xml:lang="en">Korea Institute Of Ocean Science and Technology (KIOST)</dcterms:isReplacedBy>
	<dcterms:isReplacedBy rdf:resource="http://vocab.aodn.org.au/organisation/entity/381"/>
</rdf:Description>

<rdf:Description rdf:about="http://vocab.aodn.org.au/def/organisation/entity/404">
	<rdf:type rdf:resource="http://www.w3.org/2000/01/rdf-schema#Resource"/>
	<rdf:type rdf:resource="http://www.w3.org/2004/02/skos/core#Concept"/>
	<dcterms:modified rdf:datatype="http://www.w3.org/2001/XMLSchema#dateTime">2015-10-15T02:01:42Z</dcterms:modified>
	<dcterms:creator rdf:datatype="http://www.w3.org/2001/XMLSchema#string">Natalia Atkins</dcterms:creator>
	<dcterms:created rdf:datatype="http://www.w3.org/2001/XMLSchema#dateTime">2015-10-15T10:38:15Z</dcterms:created>
	<dcterms:contributor rdf:datatype="http://www.w3.org/2001/XMLSchema#string">eMII_Atkins.Natalia</dcterms:contributor>
	<skos:broadMatch rdf:resource="http://vocab.aodn.org.au/def/organisation_classes/category/4"/>
	<skos:prefLabel xml:lang="en">World Wide Fund For Nature (WWF)</skos:prefLabel>
	<skos:altLabel xml:lang="en"></skos:altLabel>
	<skos:hiddenLabel xml:lang="en">WWF</skos:hiddenLabel>
	<skos:definition xml:lang="en"></skos:definition>
	<dc:source rdf:datatype="http://www.w3.org/2001/XMLSchema#string">Australian Ocean Data Network Organisation Register</dc:source>
	<dc:publisher rdf:datatype="http://www.w3.org/2001/XMLSchema#string">eMarine Information Infrastructure (eMMI)</dc:publisher>
	<skos:exactMatch rdf:resource="http://seadatanet.maris2.nl/v_edmo/print.asp?n_code=4388"/>
	<skos:topConceptOf rdf:resource="http://vocab.aodn.org.au/def/organisation/1"/>
	<skos:inScheme rdf:resource="http://vocab.aodn.org.au/def/organisation/1"/>
</rdf:Description>

<rdf:Description rdf:about="http://vocab.aodn.org.au/def/organisation/entity/408">
	<rdf:type rdf:resource="http://www.w3.org/2000/01/rdf-schema#Resource"/>
	<rdf:type rdf:resource="http://www.w3.org/2004/02/skos/core#Concept"/>
	<dcterms:modified rdf:datatype="http://www.w3.org/2001/XMLSchema#dateTime">2015-11-09T00:25:19Z</dcterms:modified>
	<dcterms:creator rdf:datatype="http://www.w3.org/2001/XMLSchema#string">Natalia Atkins</dcterms:creator>
	<dcterms:created rdf:datatype="http://www.w3.org/2001/XMLSchema#dateTime">2015-11-03T10:38:15Z</dcterms:created>
	<dcterms:contributor rdf:datatype="http://www.w3.org/2001/XMLSchema#string">eMII_Atkins.Natalia</dcterms:contributor>
	<skos:broadMatch rdf:resource="http://vocab.aodn.org.au/def/organisation_classes/category/1"/>
	<skos:prefLabel xml:lang="en">Hornsby Shire Council</skos:prefLabel>
	<skos:altLabel xml:lang="en"></skos:altLabel>
	<skos:hiddenLabel xml:lang="en"></skos:hiddenLabel>
	<skos:definition xml:lang="en">The Hornsby Shire Council presides over Hornsby Shire which covers approximately 510 square kilometres, including 6,000 hectares of public bushland for which Council is responsible. The Shire extends from Brooklyn in the north, to Wisemans Ferry and Glenorie/Dural in the west, Wahroonga in the east and Epping in the south, in New South Wales.</skos:definition>
	<dc:source rdf:datatype="http://www.w3.org/2001/XMLSchema#string">Australian Ocean Data Network Organisation Register</dc:source>
	<dc:publisher rdf:datatype="http://www.w3.org/2001/XMLSchema#string">eMarine Information Infrastructure (eMMI)</dc:publisher>
	<skos:topConceptOf rdf:resource="http://vocab.aodn.org.au/def/organisation/1"/>
	<skos:inScheme rdf:resource="http://vocab.aodn.org.au/def/organisation/1"/>
</rdf:Description>

<rdf:Description rdf:about="http://vocab.aodn.org.au/def/organisation/entity/409">
	<rdf:type rdf:resource="http://www.w3.org/2000/01/rdf-schema#Resource"/>
	<rdf:type rdf:resource="http://www.w3.org/2004/02/skos/core#Concept"/>
	<dcterms:modified rdf:datatype="http://www.w3.org/2001/XMLSchema#dateTime">2015-11-09T00:25:29Z</dcterms:modified>
	<dcterms:creator rdf:datatype="http://www.w3.org/2001/XMLSchema#string">Natalia Atkins</dcterms:creator>
	<dcterms:created rdf:datatype="http://www.w3.org/2001/XMLSchema#dateTime">2015-11-03T10:38:15Z</dcterms:created>
	<dcterms:contributor rdf:datatype="http://www.w3.org/2001/XMLSchema#string">eMII_Atkins.Natalia</dcterms:contributor>
	<skos:broadMatch rdf:resource="http://vocab.aodn.org.au/def/organisation_classes/category/1"/>
	<skos:prefLabel xml:lang="en">Warringah Council</skos:prefLabel>
	<skos:altLabel xml:lang="en"></skos:altLabel>
	<skos:hiddenLabel xml:lang="en"></skos:hiddenLabel>
	<skos:definition xml:lang="en">Warringah Council was established in 1906. It administers an area of 149 square km on Sydney’s northern beaches, extending from Manly in the south to Pittwater in the north and inland to the Ku-ring-gai Chase National Park, in New South Wales.</skos:definition>
	<dc:source rdf:datatype="http://www.w3.org/2001/XMLSchema#string">Australian Ocean Data Network Organisation Register</dc:source>
	<dc:publisher rdf:datatype="http://www.w3.org/2001/XMLSchema#string">eMarine Information Infrastructure (eMMI)</dc:publisher>
	<skos:topConceptOf rdf:resource="http://vocab.aodn.org.au/def/organisation/1"/>
	<skos:inScheme rdf:resource="http://vocab.aodn.org.au/def/organisation/1"/>
</rdf:Description>

<rdf:Description rdf:about="http://vocab.aodn.org.au/def/organisation/entity/412">
	<rdf:type rdf:resource="http://www.w3.org/2000/01/rdf-schema#Resource"/>
	<rdf:type rdf:resource="http://www.w3.org/2004/02/skos/core#Concept"/>
	<dcterms:modified rdf:datatype="http://www.w3.org/2001/XMLSchema#dateTime">2015-11-09T00:29:44Z</dcterms:modified>
	<dcterms:creator rdf:datatype="http://www.w3.org/2001/XMLSchema#string">Natalia Atkins</dcterms:creator>
	<dcterms:created rdf:datatype="http://www.w3.org/2001/XMLSchema#dateTime">2015-11-09T10:38:15Z</dcterms:created>
	<dcterms:contributor rdf:datatype="http://www.w3.org/2001/XMLSchema#string">eMII_Atkins.Natalia</dcterms:contributor>
	<skos:broadMatch rdf:resource="http://vocab.aodn.org.au/def/organisation_classes/category/4"/>
	<skos:prefLabel xml:lang="en">Center for Aquatic Sciences at Adventure Aquarium</skos:prefLabel>
	<skos:altLabel xml:lang="en"></skos:altLabel>
	<skos:hiddenLabel xml:lang="en"></skos:hiddenLabel>
	<skos:definition xml:lang="en">The Center for Aquatic Sciences was founded in 1989 and has since been advancing the understanding of and concern for aquatic animals and their habitats. The Center’s mission is: “education and youth development through promoting the understanding, appreciation and protection of aquatic life and habitats.” In performing this mission, the Center strives to be a responsible member of the community, assisting in its economic and social redevelopment by providing opportunities for education, enrichment and employment.</skos:definition>
	<dc:source rdf:datatype="http://www.w3.org/2001/XMLSchema#string">Australian Ocean Data Network Organisation Register</dc:source>
	<dc:publisher rdf:datatype="http://www.w3.org/2001/XMLSchema#string">eMarine Information Infrastructure (eMMI)</dc:publisher>
	<skos:exactMatch rdf:resource="http://seadatanet.maris2.nl/v_edmo/print.asp?n_code=4433"/>
	<skos:topConceptOf rdf:resource="http://vocab.aodn.org.au/def/organisation/1"/>
	<skos:inScheme rdf:resource="http://vocab.aodn.org.au/def/organisation/1"/>
</rdf:Description>

<rdf:Description rdf:about="http://vocab.aodn.org.au/def/organisation/entity/413">
	<rdf:type rdf:resource="http://www.w3.org/2000/01/rdf-schema#Resource"/>
	<rdf:type rdf:resource="http://www.w3.org/2004/02/skos/core#Concept"/>
	<dcterms:modified rdf:datatype="http://www.w3.org/2001/XMLSchema#dateTime">2015-11-09T00:29:55Z</dcterms:modified>
	<dcterms:creator rdf:datatype="http://www.w3.org/2001/XMLSchema#string">Natalia Atkins</dcterms:creator>
	<dcterms:created rdf:datatype="http://www.w3.org/2001/XMLSchema#dateTime">2015-11-09T10:38:15Z</dcterms:created>
	<dcterms:contributor rdf:datatype="http://www.w3.org/2001/XMLSchema#string">eMII_Atkins.Natalia</dcterms:contributor>
	<skos:broadMatch rdf:resource="http://vocab.aodn.org.au/def/organisation_classes/category/4"/>
	<skos:prefLabel xml:lang="en">Cliffs Natural Resources</skos:prefLabel>
	<skos:altLabel xml:lang="en"></skos:altLabel>
	<skos:hiddenLabel xml:lang="en">Cliffs</skos:hiddenLabel>
	<skos:definition xml:lang="en">Cliffs is a leading mining and natural resources company. We supply iron ore pellets to the North American steel industry from mines and plants located in Michigan and Minnesota. We also produce low-volatile metallurgical coal from mines located in West Virginia and Alabama. Additionally, we operate an iron ore mining complex in Western Australia.</skos:definition>
	<dc:source rdf:datatype="http://www.w3.org/2001/XMLSchema#string">Australian Ocean Data Network Organisation Register</dc:source>
	<dc:publisher rdf:datatype="http://www.w3.org/2001/XMLSchema#string">eMarine Information Infrastructure (eMMI)</dc:publisher>
	<skos:exactMatch rdf:resource="http://seadatanet.maris2.nl/v_edmo/print.asp?n_code=4434"/>
	<skos:topConceptOf rdf:resource="http://vocab.aodn.org.au/def/organisation/1"/>
	<skos:inScheme rdf:resource="http://vocab.aodn.org.au/def/organisation/1"/>
</rdf:Description>

<rdf:Description rdf:about="http://vocab.aodn.org.au/def/organisation/entity/414">
	<rdf:type rdf:resource="http://www.w3.org/2000/01/rdf-schema#Resource"/>
	<rdf:type rdf:resource="http://www.w3.org/2004/02/skos/core#Concept"/>
	<dcterms:modified rdf:datatype="http://www.w3.org/2001/XMLSchema#dateTime">2015-11-09T00:30:08Z</dcterms:modified>
	<dcterms:creator rdf:datatype="http://www.w3.org/2001/XMLSchema#string">Natalia Atkins</dcterms:creator>
	<dcterms:created rdf:datatype="http://www.w3.org/2001/XMLSchema#dateTime">2015-11-09T10:38:15Z</dcterms:created>
	<dcterms:contributor rdf:datatype="http://www.w3.org/2001/XMLSchema#string">eMII_Atkins.Natalia</dcterms:contributor>
	<skos:broadMatch rdf:resource="http://vocab.aodn.org.au/def/organisation_classes/category/4"/>
	<skos:prefLabel xml:lang="en">International Risk Consultants Inc (IRC)</skos:prefLabel>
	<skos:altLabel xml:lang="en"></skos:altLabel>
	<skos:hiddenLabel xml:lang="en">IRC</skos:hiddenLabel>
	<skos:definition xml:lang="en">RC specializes in trade credit insurance, political risk Insurance and related trade finance solutions.  Since our 1987 founding in Columbus, Ohio (USA), we have grown into the industry’s largest globally-integrated brokerage with partner-led offices in Hong Kong, China, Brazil, India and throughout the USA.   We offer thorough market explorations and bespoke placements with unmatched post-placement training, service and claims advocacy.</skos:definition>
	<dc:source rdf:datatype="http://www.w3.org/2001/XMLSchema#string">Australian Ocean Data Network Organisation Register</dc:source>
	<dc:publisher rdf:datatype="http://www.w3.org/2001/XMLSchema#string">eMarine Information Infrastructure (eMMI)</dc:publisher>
	<skos:exactMatch rdf:resource="http://seadatanet.maris2.nl/v_edmo/print.asp?n_code=4435"/>
	<skos:topConceptOf rdf:resource="http://vocab.aodn.org.au/def/organisation/1"/>
	<skos:inScheme rdf:resource="http://vocab.aodn.org.au/def/organisation/1"/>
</rdf:Description>

<rdf:Description rdf:about="http://vocab.aodn.org.au/def/organisation/entity/415">
	<rdf:type rdf:resource="http://www.w3.org/2000/01/rdf-schema#Resource"/>
	<rdf:type rdf:resource="http://www.w3.org/2004/02/skos/core#Concept"/>
	<dcterms:modified rdf:datatype="http://www.w3.org/2001/XMLSchema#dateTime">2015-11-09T00:30:15Z</dcterms:modified>
	<dcterms:creator rdf:datatype="http://www.w3.org/2001/XMLSchema#string">Natalia Atkins</dcterms:creator>
	<dcterms:created rdf:datatype="http://www.w3.org/2001/XMLSchema#dateTime">2015-11-09T10:38:15Z</dcterms:created>
	<dcterms:contributor rdf:datatype="http://www.w3.org/2001/XMLSchema#string">eMII_Atkins.Natalia</dcterms:contributor>
	<skos:broadMatch rdf:resource="http://vocab.aodn.org.au/def/organisation_classes/category/4"/>
	<skos:prefLabel xml:lang="en">Jacobs Engineering Group Inc.</skos:prefLabel>
	<skos:altLabel xml:lang="en"></skos:altLabel>
	<skos:hiddenLabel xml:lang="en">Jacobs</skos:hiddenLabel>
	<skos:definition xml:lang="en"></skos:definition>
	<dc:source rdf:datatype="http://www.w3.org/2001/XMLSchema#string">Australian Ocean Data Network Organisation Register</dc:source>
	<dc:publisher rdf:datatype="http://www.w3.org/2001/XMLSchema#string">eMarine Information Infrastructure (eMMI)</dc:publisher>
	<skos:exactMatch rdf:resource="http://seadatanet.maris2.nl/v_edmo/print.asp?n_code=4436"/>
	<skos:topConceptOf rdf:resource="http://vocab.aodn.org.au/def/organisation/1"/>
	<skos:inScheme rdf:resource="http://vocab.aodn.org.au/def/organisation/1"/>
</rdf:Description>

<rdf:Description rdf:about="http://vocab.aodn.org.au/def/organisation/entity/416">
	<rdf:type rdf:resource="http://www.w3.org/2000/01/rdf-schema#Resource"/>
	<rdf:type rdf:resource="http://www.w3.org/2004/02/skos/core#Concept"/>
	<dcterms:modified rdf:datatype="http://www.w3.org/2001/XMLSchema#dateTime">2015-11-09T00:30:25Z</dcterms:modified>
	<dcterms:creator rdf:datatype="http://www.w3.org/2001/XMLSchema#string">Natalia Atkins</dcterms:creator>
	<dcterms:created rdf:datatype="http://www.w3.org/2001/XMLSchema#dateTime">2015-11-09T10:38:15Z</dcterms:created>
	<dcterms:contributor rdf:datatype="http://www.w3.org/2001/XMLSchema#string">eMII_Atkins.Natalia</dcterms:contributor>
	<skos:broadMatch rdf:resource="http://vocab.aodn.org.au/def/organisation_classes/category/4"/>
	<skos:prefLabel xml:lang="en">Marine Conservation Science Institute (MCSI)</skos:prefLabel>
	<skos:altLabel xml:lang="en"></skos:altLabel>
	<skos:hiddenLabel xml:lang="en">MCSI</skos:hiddenLabel>
	<skos:definition xml:lang="en">The Marine Conservation Science Institute (MCSI) is a nonprofit 501(c)(3) organization founded on the belief that focused research can make a difference in how we view and manage our marine resources.  MCSI is committed to promoting important issues in marine biology and fisheries, and is currently involved in research projects around the globe dedicated to protecting and conserving marine resources.</skos:definition>
	<dc:source rdf:datatype="http://www.w3.org/2001/XMLSchema#string">Australian Ocean Data Network Organisation Register</dc:source>
	<dc:publisher rdf:datatype="http://www.w3.org/2001/XMLSchema#string">eMarine Information Infrastructure (eMMI)</dc:publisher>
	<skos:exactMatch rdf:resource="http://seadatanet.maris2.nl/v_edmo/print.asp?n_code=4437"/>
	<skos:topConceptOf rdf:resource="http://vocab.aodn.org.au/def/organisation/1"/>
	<skos:inScheme rdf:resource="http://vocab.aodn.org.au/def/organisation/1"/>
</rdf:Description>

<rdf:Description rdf:about="http://vocab.aodn.org.au/def/organisation/entity/417">
	<rdf:type rdf:resource="http://www.w3.org/2000/01/rdf-schema#Resource"/>
	<rdf:type rdf:resource="http://www.w3.org/2004/02/skos/core#Concept"/>
	<dcterms:modified rdf:datatype="http://www.w3.org/2001/XMLSchema#dateTime">2015-11-09T00:30:33Z</dcterms:modified>
	<dcterms:creator rdf:datatype="http://www.w3.org/2001/XMLSchema#string">Natalia Atkins</dcterms:creator>
	<dcterms:created rdf:datatype="http://www.w3.org/2001/XMLSchema#dateTime">2015-11-09T10:38:15Z</dcterms:created>
	<dcterms:contributor rdf:datatype="http://www.w3.org/2001/XMLSchema#string">eMII_Atkins.Natalia</dcterms:contributor>
	<skos:broadMatch rdf:resource="http://vocab.aodn.org.au/def/organisation_classes/category/4"/>
	<skos:prefLabel xml:lang="en">The Nature Conservancy (TNC)</skos:prefLabel>
	<skos:altLabel xml:lang="en"></skos:altLabel>
	<skos:hiddenLabel xml:lang="en">TNC</skos:hiddenLabel>
	<skos:definition xml:lang="en">The mission of The Nature Conservancy is to conserve the lands and waters on which all life depends. Our vision is a world where the diversity of life thrives, and people act to conserve nature for its own sake and its ability to fulfill our needs and enrich our lives.</skos:definition>
	<dc:source rdf:datatype="http://www.w3.org/2001/XMLSchema#string">Australian Ocean Data Network Organisation Register</dc:source>
	<dc:publisher rdf:datatype="http://www.w3.org/2001/XMLSchema#string">eMarine Information Infrastructure (eMMI)</dc:publisher>
	<skos:exactMatch rdf:resource="http://seadatanet.maris2.nl/v_edmo/print.asp?n_code=4438"/>
	<skos:topConceptOf rdf:resource="http://vocab.aodn.org.au/def/organisation/1"/>
	<skos:inScheme rdf:resource="http://vocab.aodn.org.au/def/organisation/1"/>
</rdf:Description>

<rdf:Description rdf:about="http://vocab.aodn.org.au/def/organisation/entity/418">
	<rdf:type rdf:resource="http://www.w3.org/2000/01/rdf-schema#Resource"/>
	<rdf:type rdf:resource="http://www.w3.org/2004/02/skos/core#Concept"/>
	<dcterms:modified rdf:datatype="http://www.w3.org/2001/XMLSchema#dateTime">2015-11-09T00:30:43Z</dcterms:modified>
	<dcterms:creator rdf:datatype="http://www.w3.org/2001/XMLSchema#string">Natalia Atkins</dcterms:creator>
	<dcterms:created rdf:datatype="http://www.w3.org/2001/XMLSchema#dateTime">2015-11-09T10:38:15Z</dcterms:created>
	<dcterms:contributor rdf:datatype="http://www.w3.org/2001/XMLSchema#string">eMII_Atkins.Natalia</dcterms:contributor>
	<skos:broadMatch rdf:resource="http://vocab.aodn.org.au/def/organisation_classes/category/4"/>
	<skos:prefLabel xml:lang="en">Oceanweather Inc.</skos:prefLabel>
	<skos:altLabel xml:lang="en"></skos:altLabel>
	<skos:hiddenLabel xml:lang="en"></skos:hiddenLabel>
	<skos:definition xml:lang="en">Since its formation in 1977, the company had been fully engaged with support divided between the private and public sector. In the public sector the company continues to perform basic and applied research in marine meteorology and ocean response numerical modeling, supported by both US and foreign government agencies. Our staff continues to gain international reputations through active participation in international scientific conferences and research programs, and in open publication.

Oceanweather functions as a specialized consulting firm serving the coastal and ocean engineering communities with its unique capacity to integrate several areas of expertise into specification of definitive design data on the physical environment. Oceanweather's approach is to consistently develop and apply its high-level technology to satisfy practical requirements in the areas of marine meteorology, ocean wave and current specification, ocean engineering, and statistics of environmental data. In the past quarter century Oceanweather has performed dedicated hindcast studies and Joint Industry Projects (JIPs) in virtually every ocean basin in the world. Since 1983, Oceanweather has operated a real time forecasting division following a unique approach which optimally combines the traditional approach to weather forecasting, which retains the contributions of individual forecasters, and Oceanweather's high-level technology developed and applied so successfully in its hindcasting and consulting divisions. The system includes a global wind and wave forecast system and various high resolution regional applications.</skos:definition>
	<dc:source rdf:datatype="http://www.w3.org/2001/XMLSchema#string">Australian Ocean Data Network Organisation Register</dc:source>
	<dc:publisher rdf:datatype="http://www.w3.org/2001/XMLSchema#string">eMarine Information Infrastructure (eMMI)</dc:publisher>
	<skos:exactMatch rdf:resource="http://seadatanet.maris2.nl/v_edmo/print.asp?n_code=4440"/>
	<skos:topConceptOf rdf:resource="http://vocab.aodn.org.au/def/organisation/1"/>
	<skos:inScheme rdf:resource="http://vocab.aodn.org.au/def/organisation/1"/>
</rdf:Description>

<rdf:Description rdf:about="http://www.w3.org/2004/02/skos/core#broadMatch">
	<rdf:type rdf:resource="http://www.w3.org/1999/02/22-rdf-syntax-ns#Property"/>
	<rdf:type rdf:resource="http://www.w3.org/2000/01/rdf-schema#Resource"/>
	<rdfs:subPropertyOf rdf:resource="http://www.w3.org/2004/02/skos/core#broadMatch"/>
</rdf:Description>

<rdf:Description rdf:about="http://vocab.aodn.org.au/def/organisation_classes/category/3">
	<rdf:type rdf:resource="http://www.w3.org/2000/01/rdf-schema#Resource"/>
</rdf:Description>

<rdf:Description rdf:about="http://www.w3.org/2004/02/skos/core#Concept">
	<rdf:type rdf:resource="http://www.w3.org/2000/01/rdf-schema#Resource"/>
	<rdf:type rdf:resource="http://www.w3.org/2000/01/rdf-schema#Class"/>
	<rdfs:subClassOf rdf:resource="http://www.w3.org/2000/01/rdf-schema#Resource"/>
	<rdfs:subClassOf rdf:resource="http://www.w3.org/2004/02/skos/core#Concept"/>
</rdf:Description>

<rdf:Description rdf:about="http://www.w3.org/2004/02/skos/core#prefLabel">
	<rdf:type rdf:resource="http://www.w3.org/1999/02/22-rdf-syntax-ns#Property"/>
	<rdf:type rdf:resource="http://www.w3.org/2000/01/rdf-schema#Resource"/>
	<rdfs:subPropertyOf rdf:resource="http://www.w3.org/2004/02/skos/core#prefLabel"/>
</rdf:Description>

<rdf:Description rdf:about="http://www.w3.org/2004/02/skos/core#altLabel">
	<rdf:type rdf:resource="http://www.w3.org/1999/02/22-rdf-syntax-ns#Property"/>
	<rdf:type rdf:resource="http://www.w3.org/2000/01/rdf-schema#Resource"/>
	<rdfs:subPropertyOf rdf:resource="http://www.w3.org/2004/02/skos/core#altLabel"/>
</rdf:Description>

<rdf:Description rdf:about="http://www.w3.org/2004/02/skos/core#hiddenLabel">
	<rdf:type rdf:resource="http://www.w3.org/1999/02/22-rdf-syntax-ns#Property"/>
	<rdf:type rdf:resource="http://www.w3.org/2000/01/rdf-schema#Resource"/>
	<rdfs:subPropertyOf rdf:resource="http://www.w3.org/2004/02/skos/core#hiddenLabel"/>
</rdf:Description>

<rdf:Description rdf:about="http://www.w3.org/2004/02/skos/core#definition">
	<rdf:type rdf:resource="http://www.w3.org/1999/02/22-rdf-syntax-ns#Property"/>
	<rdf:type rdf:resource="http://www.w3.org/2000/01/rdf-schema#Resource"/>
	<rdfs:subPropertyOf rdf:resource="http://www.w3.org/2004/02/skos/core#definition"/>
</rdf:Description>

<rdf:Description rdf:about="http://purl.org/dc/elements/1.1/source">
	<rdf:type rdf:resource="http://www.w3.org/1999/02/22-rdf-syntax-ns#Property"/>
	<rdf:type rdf:resource="http://www.w3.org/2000/01/rdf-schema#Resource"/>
	<rdfs:subPropertyOf rdf:resource="http://purl.org/dc/elements/1.1/source"/>
</rdf:Description>

<rdf:Description rdf:about="http://purl.org/dc/elements/1.1/publisher">
	<rdf:type rdf:resource="http://www.w3.org/1999/02/22-rdf-syntax-ns#Property"/>
	<rdf:type rdf:resource="http://www.w3.org/2000/01/rdf-schema#Resource"/>
	<rdfs:subPropertyOf rdf:resource="http://purl.org/dc/elements/1.1/publisher"/>
</rdf:Description>

<rdf:Description rdf:about="http://www.w3.org/2004/02/skos/core#exactMatch">
	<rdf:type rdf:resource="http://www.w3.org/1999/02/22-rdf-syntax-ns#Property"/>
	<rdf:type rdf:resource="http://www.w3.org/2000/01/rdf-schema#Resource"/>
	<rdfs:subPropertyOf rdf:resource="http://www.w3.org/2004/02/skos/core#exactMatch"/>
</rdf:Description>

<rdf:Description rdf:about="http://seadatanet.maris2.nl/v_edmo/print.asp?n_code=4297">
	<rdf:type rdf:resource="http://www.w3.org/2000/01/rdf-schema#Resource"/>
</rdf:Description>

<rdf:Description rdf:about="http://www.w3.org/2004/02/skos/core#narrower">
	<rdf:type rdf:resource="http://www.w3.org/1999/02/22-rdf-syntax-ns#Property"/>
	<rdf:type rdf:resource="http://www.w3.org/2000/01/rdf-schema#Resource"/>
	<rdfs:subPropertyOf rdf:resource="http://www.w3.org/2004/02/skos/core#narrower"/>
</rdf:Description>

<rdf:Description rdf:about="http://vocab.aodn.org.au/def/organisation/entity/216">
	<rdf:type rdf:resource="http://www.w3.org/2000/01/rdf-schema#Resource"/>
	<rdf:type rdf:resource="http://www.w3.org/2004/02/skos/core#Concept"/>
	<dcterms:modified rdf:datatype="http://www.w3.org/2001/XMLSchema#dateTime">2015-07-28T05:44:40Z</dcterms:modified>
	<dcterms:creator rdf:datatype="http://www.w3.org/2001/XMLSchema#string">Natalia Atkins</dcterms:creator>
	<dcterms:created rdf:datatype="http://www.w3.org/2001/XMLSchema#dateTime">2015-07-09T10:38:15Z</dcterms:created>
	<dcterms:contributor rdf:datatype="http://www.w3.org/2001/XMLSchema#string">Natalia_Atkins</dcterms:contributor>
	<skos:prefLabel xml:lang="en">School of Environmental and Life Sciences, The University of Newcastle (UON)</skos:prefLabel>
	<skos:altLabel xml:lang="en">School of Environmental and Life Sciences</skos:altLabel>
	<skos:hiddenLabel xml:lang="en"></skos:hiddenLabel>
	<skos:definition xml:lang="en"></skos:definition>
	<skos:definition xml:lang="en">The School is made up of six disciplines which includes applied sciences, biology, chemistry, earth sciences, geography and environmental studies and environmental science and management.</skos:definition>
	<dc:source rdf:datatype="http://www.w3.org/2001/XMLSchema#string">Australian Ocean Data Network Organisation Register</dc:source>
	<dc:publisher rdf:datatype="http://www.w3.org/2001/XMLSchema#string">eMarine Information Infrastructure (eMII)</dc:publisher>
	<skos:exactMatch rdf:resource="http://seadatanet.maris2.nl/v_edmo/print.asp?n_code=1488"/>
	<skos:inScheme rdf:resource="http://vocab.aodn.org.au/def/organisation/1"/>
	<skos:broader rdf:resource="http://vocab.aodn.org.au/def/organisation/entity/215"/>
</rdf:Description>

<rdf:Description rdf:about="http://www.w3.org/2004/02/skos/core#topConceptOf">
	<rdf:type rdf:resource="http://www.w3.org/1999/02/22-rdf-syntax-ns#Property"/>
	<rdf:type rdf:resource="http://www.w3.org/2000/01/rdf-schema#Resource"/>
	<rdfs:subPropertyOf rdf:resource="http://www.w3.org/2004/02/skos/core#topConceptOf"/>
</rdf:Description>

<rdf:Description rdf:about="http://www.w3.org/2004/02/skos/core#inScheme">
	<rdf:type rdf:resource="http://www.w3.org/1999/02/22-rdf-syntax-ns#Property"/>
	<rdf:type rdf:resource="http://www.w3.org/2000/01/rdf-schema#Resource"/>
	<rdfs:subPropertyOf rdf:resource="http://www.w3.org/2004/02/skos/core#inScheme"/>
</rdf:Description>

<rdf:Description rdf:about="http://seadatanet.maris2.nl/v_edmo/print.asp?n_code=1488">
	<rdf:type rdf:resource="http://www.w3.org/2000/01/rdf-schema#Resource"/>
</rdf:Description>

<rdf:Description rdf:about="http://www.w3.org/2004/02/skos/core#broader">
	<rdf:type rdf:resource="http://www.w3.org/1999/02/22-rdf-syntax-ns#Property"/>
	<rdf:type rdf:resource="http://www.w3.org/2000/01/rdf-schema#Resource"/>
	<rdfs:subPropertyOf rdf:resource="http://www.w3.org/2004/02/skos/core#broader"/>
</rdf:Description>

<rdf:Description rdf:about="http://seadatanet.maris2.nl/v_edmo/print.asp?n_code=3025">
	<rdf:type rdf:resource="http://www.w3.org/2000/01/rdf-schema#Resource"/>
</rdf:Description>

<rdf:Description rdf:about="http://vocab.aodn.org.au/def/organisation/entity/218">
	<rdf:type rdf:resource="http://www.w3.org/2000/01/rdf-schema#Resource"/>
	<rdf:type rdf:resource="http://www.w3.org/2004/02/skos/core#Concept"/>
	<dcterms:creator rdf:datatype="http://www.w3.org/2001/XMLSchema#string">Natalia Atkins</dcterms:creator>
	<dcterms:created rdf:datatype="http://www.w3.org/2001/XMLSchema#dateTime">2015-07-10T10:38:15Z</dcterms:created>
	<skos:prefLabel xml:lang="en">School of Biological Sciences (SBS), The University of Queensland (UQ)</skos:prefLabel>
	<skos:altLabel xml:lang="en">School of Biological Sciences (SBS)</skos:altLabel>
	<skos:hiddenLabel xml:lang="en">SBS</skos:hiddenLabel>
	<skos:definition xml:lang="en">The School of Biological Sciences at The University of Queensland is situated on the St Lucia campus in Brisbane and is part of the Faculty of Science. Research is conducted in evolution, global change biology, ecology, aquaculture, behaviour, physiology, entomology, zoology, botany, genomics, development and conservation biology.</skos:definition>
	<dc:source rdf:datatype="http://www.w3.org/2001/XMLSchema#string">Australian Ocean Data Network Organisation Register</dc:source>
	<dc:publisher rdf:datatype="http://www.w3.org/2001/XMLSchema#string">eMarine Information Infrastructure (eMII)</dc:publisher>
	<skos:exactMatch rdf:resource="http://seadatanet.maris2.nl/v_edmo/print.asp?n_code=4298"/>
	<skos:inScheme rdf:resource="http://vocab.aodn.org.au/def/organisation/1"/>
	<skos:broader rdf:resource="http://vocab.aodn.org.au/def/organisation/entity/217"/>
</rdf:Description>

<rdf:Description rdf:about="http://vocab.aodn.org.au/def/organisation/entity/219">
	<rdf:type rdf:resource="http://www.w3.org/2000/01/rdf-schema#Resource"/>
	<rdf:type rdf:resource="http://www.w3.org/2004/02/skos/core#Concept"/>
	<dcterms:creator rdf:datatype="http://www.w3.org/2001/XMLSchema#string">Natalia Atkins</dcterms:creator>
	<dcterms:created rdf:datatype="http://www.w3.org/2001/XMLSchema#dateTime">2015-07-10T10:38:15Z</dcterms:created>
	<skos:prefLabel xml:lang="en">School of Economics, The University of Queensland (UQ)</skos:prefLabel>
	<skos:altLabel xml:lang="en">School of Economics</skos:altLabel>
	<skos:hiddenLabel xml:lang="en"></skos:hiddenLabel>
	<skos:definition xml:lang="en">The School of Economics at the University of Queensland, is situated on the St Lucia campus, and is part of the Faculty of Business, Economics and Law.</skos:definition>
	<dc:publisher rdf:datatype="http://www.w3.org/2001/XMLSchema#string">eMarine Information Infrastructure (eMII)</dc:publisher>
	<skos:exactMatch rdf:resource="http://seadatanet.maris2.nl/v_edmo/print.asp?n_code=4299"/>
	<skos:inScheme rdf:resource="http://vocab.aodn.org.au/def/organisation/1"/>
	<skos:broader rdf:resource="http://vocab.aodn.org.au/def/organisation/entity/217"/>
</rdf:Description>

<rdf:Description rdf:about="http://vocab.aodn.org.au/def/organisation/entity/220">
	<rdf:type rdf:resource="http://www.w3.org/2000/01/rdf-schema#Resource"/>
	<rdf:type rdf:resource="http://www.w3.org/2004/02/skos/core#Concept"/>
	<dcterms:creator rdf:datatype="http://www.w3.org/2001/XMLSchema#string">Natalia Atkins</dcterms:creator>
	<dcterms:created rdf:datatype="http://www.w3.org/2001/XMLSchema#dateTime">2015-07-10T10:38:15Z</dcterms:created>
	<skos:prefLabel xml:lang="en">National Research Centre for Environmental Toxicology (entox), The University of Queensland (UQ)</skos:prefLabel>
	<skos:altLabel xml:lang="en">National Research Centre for Environmental Toxicology (entox)</skos:altLabel>
	<skos:hiddenLabel xml:lang="en">entox</skos:hiddenLabel>
	<skos:definition xml:lang="en">Entox is a joint venture of the University of Queensland and the Queensland Department of Health. The centre's aim is to provide leading-edge science to improve human health through a healthy environment.</skos:definition>
	<dc:source rdf:datatype="http://www.w3.org/2001/XMLSchema#string">Australian Ocean Data Network Organisation Register</dc:source>
	<dc:publisher rdf:datatype="http://www.w3.org/2001/XMLSchema#string">eMarine Information Infrastructure (eMII)</dc:publisher>
	<skos:exactMatch rdf:resource="http://seadatanet.maris2.nl/v_edmo/print.asp?n_code=4300"/>
	<skos:inScheme rdf:resource="http://vocab.aodn.org.au/def/organisation/1"/>
	<skos:broader rdf:resource="http://vocab.aodn.org.au/def/organisation/entity/217"/>
</rdf:Description>

<rdf:Description rdf:about="http://vocab.aodn.org.au/def/organisation/entity/221">
	<rdf:type rdf:resource="http://www.w3.org/2000/01/rdf-schema#Resource"/>
	<rdf:type rdf:resource="http://www.w3.org/2004/02/skos/core#Concept"/>
	<dcterms:creator rdf:datatype="http://www.w3.org/2001/XMLSchema#string">Natalia Atkins</dcterms:creator>
	<dcterms:created rdf:datatype="http://www.w3.org/2001/XMLSchema#dateTime">2015-07-10T10:38:15Z</dcterms:created>
	<skos:prefLabel xml:lang="en">Division of Civil Engineering, The University of Queensland (UQ)</skos:prefLabel>
	<skos:altLabel xml:lang="en">Division of Civil Engineering</skos:altLabel>
	<skos:hiddenLabel xml:lang="en"></skos:hiddenLabel>
	<skos:definition xml:lang="en">This Division of Civil Engineering is now known as the School of Civil Engineering.</skos:definition>
	<dc:source rdf:datatype="http://www.w3.org/2001/XMLSchema#string">Australian Ocean Data Network Organisation Register</dc:source>
	<dc:publisher rdf:datatype="http://www.w3.org/2001/XMLSchema#string">eMarine Information Infrastructure (eMII)</dc:publisher>
	<skos:inScheme rdf:resource="http://vocab.aodn.org.au/def/organisation/1"/>
	<skos:broader rdf:resource="http://vocab.aodn.org.au/def/organisation/entity/217"/>
	<skos:scopeNote xml:lang="en">Organisation no longer exists</skos:scopeNote>
</rdf:Description>

<rdf:Description rdf:about="http://vocab.aodn.org.au/def/organisation/entity/222">
	<rdf:type rdf:resource="http://www.w3.org/2000/01/rdf-schema#Resource"/>
	<rdf:type rdf:resource="http://www.w3.org/2004/02/skos/core#Concept"/>
	<dcterms:creator rdf:datatype="http://www.w3.org/2001/XMLSchema#string">Natalia Atkins</dcterms:creator>
	<dcterms:created rdf:datatype="http://www.w3.org/2001/XMLSchema#dateTime">2015-07-10T10:38:15Z</dcterms:created>
	<skos:prefLabel xml:lang="en">Global Change Institute (GCI), The University of Queensland (UQ)</skos:prefLabel>
	<skos:altLabel xml:lang="en">Global Change Institute (GCI)</skos:altLabel>
	<skos:hiddenLabel xml:lang="en">GCI</skos:hiddenLabel>
	<skos:definition xml:lang="en">Established in 2010, the Global Change Institute (CGI) at The University of Queensland, Australia, is an independent source of innovative research, ideas and advice for addressing the challenges of a changing world. GCI works to address the impacts of climate change, technological innovation and population growth through collaborative research across four key themes: Clean Energy, Food Systems, Healthy Oceans and Sustainable Water.</skos:definition>
	<dc:source rdf:datatype="http://www.w3.org/2001/XMLSchema#string">Australian Ocean Data Network Organisation Register</dc:source>
	<dc:publisher rdf:datatype="http://www.w3.org/2001/XMLSchema#string">eMarine Information Infrastructure (eMII)</dc:publisher>
	<skos:exactMatch rdf:resource="http://seadatanet.maris2.nl/v_edmo/print.asp?n_code=4301"/>
	<skos:inScheme rdf:resource="http://vocab.aodn.org.au/def/organisation/1"/>
	<skos:broader rdf:resource="http://vocab.aodn.org.au/def/organisation/entity/217"/>
</rdf:Description>

<rdf:Description rdf:about="http://vocab.aodn.org.au/def/organisation/entity/223">
	<rdf:type rdf:resource="http://www.w3.org/2000/01/rdf-schema#Resource"/>
	<rdf:type rdf:resource="http://www.w3.org/2004/02/skos/core#Concept"/>
	<dcterms:creator rdf:datatype="http://www.w3.org/2001/XMLSchema#string">Natalia Atkins</dcterms:creator>
	<dcterms:created rdf:datatype="http://www.w3.org/2001/XMLSchema#dateTime">2015-07-10T10:38:15Z</dcterms:created>
	<skos:prefLabel xml:lang="en">School of Veterinary Science (SVS), The University of Queensland (UQ)</skos:prefLabel>
	<skos:altLabel xml:lang="en">School of Veterinary Science (SVS)</skos:altLabel>
	<skos:hiddenLabel xml:lang="en">SVS</skos:hiddenLabel>
	<skos:definition xml:lang="en">The school was founded in 1936, and the large and diverse group of academic and clinical staff in the School has established an outstanding record of teaching and research to benefit farm and companion animals, their owners and industry sectors. Major contributions have been in tropical/sub-tropical animal health and medicine.</skos:definition>
	<dc:source rdf:datatype="http://www.w3.org/2001/XMLSchema#string">Australian Ocean Data Network Organisation Register</dc:source>
	<dc:publisher rdf:datatype="http://www.w3.org/2001/XMLSchema#string">eMarine Information Infrastructure (eMII)</dc:publisher>
	<skos:exactMatch rdf:resource="http://seadatanet.maris2.nl/v_edmo/print.asp?n_code=4302"/>
	<skos:inScheme rdf:resource="http://vocab.aodn.org.au/def/organisation/1"/>
	<skos:broader rdf:resource="http://vocab.aodn.org.au/def/organisation/entity/217"/>
</rdf:Description>

<rdf:Description rdf:about="http://seadatanet.maris2.nl/v_edmo/print.asp?n_code=4298">
	<rdf:type rdf:resource="http://www.w3.org/2000/01/rdf-schema#Resource"/>
</rdf:Description>

<rdf:Description rdf:about="http://seadatanet.maris2.nl/v_edmo/print.asp?n_code=4299">
	<rdf:type rdf:resource="http://www.w3.org/2000/01/rdf-schema#Resource"/>
</rdf:Description>

<rdf:Description rdf:about="http://seadatanet.maris2.nl/v_edmo/print.asp?n_code=4300">
	<rdf:type rdf:resource="http://www.w3.org/2000/01/rdf-schema#Resource"/>
</rdf:Description>

<rdf:Description rdf:about="http://www.w3.org/2004/02/skos/core#scopeNote">
	<rdf:type rdf:resource="http://www.w3.org/1999/02/22-rdf-syntax-ns#Property"/>
	<rdf:type rdf:resource="http://www.w3.org/2000/01/rdf-schema#Resource"/>
	<rdfs:subPropertyOf rdf:resource="http://www.w3.org/2004/02/skos/core#scopeNote"/>
</rdf:Description>

<rdf:Description rdf:about="http://seadatanet.maris2.nl/v_edmo/print.asp?n_code=4301">
	<rdf:type rdf:resource="http://www.w3.org/2000/01/rdf-schema#Resource"/>
</rdf:Description>

<rdf:Description rdf:about="http://seadatanet.maris2.nl/v_edmo/print.asp?n_code=4302">
	<rdf:type rdf:resource="http://www.w3.org/2000/01/rdf-schema#Resource"/>
</rdf:Description>

<rdf:Description rdf:about="http://seadatanet.maris2.nl/v_edmo/print.asp?n_code=4303">
	<rdf:type rdf:resource="http://www.w3.org/2000/01/rdf-schema#Resource"/>
</rdf:Description>

<rdf:Description rdf:about="http://vocab.aodn.org.au/def/organisation/entity/225">
	<rdf:type rdf:resource="http://www.w3.org/2000/01/rdf-schema#Resource"/>
	<rdf:type rdf:resource="http://www.w3.org/2004/02/skos/core#Concept"/>
	<dcterms:modified rdf:datatype="http://www.w3.org/2001/XMLSchema#dateTime">2015-07-28T06:16:35Z</dcterms:modified>
	<dcterms:creator rdf:datatype="http://www.w3.org/2001/XMLSchema#string">Natalia Atkins</dcterms:creator>
	<dcterms:created rdf:datatype="http://www.w3.org/2001/XMLSchema#dateTime">2015-07-10T10:38:15Z</dcterms:created>
	<dcterms:contributor rdf:datatype="http://www.w3.org/2001/XMLSchema#string">Natalia_Atkins</dcterms:contributor>
	<skos:prefLabel xml:lang="en">School of Geosciences, The University of Sydney (USYD)</skos:prefLabel>
	<skos:altLabel xml:lang="en">School of Geosciences</skos:altLabel>
	<skos:hiddenLabel xml:lang="en"></skos:hiddenLabel>
	<skos:definition xml:lang="en"></skos:definition>
	<skos:definition xml:lang="en">The school is made up of three geoscience disciplines: geography, geology and geophysics. Both marine science and environmental studies are co-taught with other schools at the University of Sydney.</skos:definition>
	<dc:source rdf:datatype="http://www.w3.org/2001/XMLSchema#string">Australian Ocean Data Network Organisation Register</dc:source>
	<dc:publisher rdf:datatype="http://www.w3.org/2001/XMLSchema#string">eMarine Information Infrastructure (eMII)</dc:publisher>
	<skos:exactMatch rdf:resource="http://seadatanet.maris2.nl/v_edmo/print.asp?n_code=3056"/>
	<skos:inScheme rdf:resource="http://vocab.aodn.org.au/def/organisation/1"/>
	<skos:broader rdf:resource="http://vocab.aodn.org.au/def/organisation/entity/224"/>
	<skos:scopeNote xml:lang="en">Replaces http://vocab.aodn.org.au/def/organisation/entity/233</skos:scopeNote>
	<dcterms:replaces rdf:resource="http://vocab.aodn.org.au/def/organisation/entity/233"/>
	<dcterms:replaces xml:lang="en">Department of Geography, The University of Sydney (USYD)</dcterms:replaces>
</rdf:Description>

<rdf:Description rdf:about="http://vocab.aodn.org.au/def/organisation/entity/226">
	<rdf:type rdf:resource="http://www.w3.org/2000/01/rdf-schema#Resource"/>
	<rdf:type rdf:resource="http://www.w3.org/2004/02/skos/core#Concept"/>
	<dcterms:modified rdf:datatype="http://www.w3.org/2001/XMLSchema#dateTime">2015-07-22T06:23:49Z</dcterms:modified>
	<dcterms:creator rdf:datatype="http://www.w3.org/2001/XMLSchema#string">Natalia Atkins</dcterms:creator>
	<dcterms:created rdf:datatype="http://www.w3.org/2001/XMLSchema#dateTime">2015-07-10T10:38:15Z</dcterms:created>
	<dcterms:contributor rdf:datatype="http://www.w3.org/2001/XMLSchema#string">Natalia_Atkins</dcterms:contributor>
	<skos:prefLabel xml:lang="en">Centre for Research on Ecological Impacts of Coastal Cities (EICC), The University of Sydney (USYD)</skos:prefLabel>
	<skos:altLabel xml:lang="en">Centre for Research on Ecological Impacts of Coastal Cities (EICC)</skos:altLabel>
	<skos:hiddenLabel xml:lang="en">EICC</skos:hiddenLabel>
	<skos:definition xml:lang="en"></skos:definition>
	<skos:definition xml:lang="en">The role of the Centre for Research on Ecological Impacts of Coastal Cities (EICC) is to do world-class research on ecological problems arising from urbanisation of coastal environments. We work with councils, regulatory agencies, Federal, State and Local Governments to identify problems and suggest valid solutions based on experimental evidence.</skos:definition>
	<dc:source rdf:datatype="http://www.w3.org/2001/XMLSchema#string">Australian Ocean Data Network Organisation Register</dc:source>
	<dc:publisher rdf:datatype="http://www.w3.org/2001/XMLSchema#string">eMarine Information Infrastructure (eMII)</dc:publisher>
	<skos:exactMatch rdf:resource="http://seadatanet.maris2.nl/v_edmo/print.asp?n_code=3208"/>
	<skos:inScheme rdf:resource="http://vocab.aodn.org.au/def/organisation/1"/>
	<skos:broader rdf:resource="http://vocab.aodn.org.au/def/organisation/entity/224"/>
</rdf:Description>

<rdf:Description rdf:about="http://vocab.aodn.org.au/def/organisation/entity/227">
	<rdf:type rdf:resource="http://www.w3.org/2000/01/rdf-schema#Resource"/>
	<rdf:type rdf:resource="http://www.w3.org/2004/02/skos/core#Concept"/>
	<dcterms:creator rdf:datatype="http://www.w3.org/2001/XMLSchema#string">Natalia Atkins</dcterms:creator>
	<dcterms:created rdf:datatype="http://www.w3.org/2001/XMLSchema#dateTime">2015-07-10T10:38:15Z</dcterms:created>
	<skos:prefLabel xml:lang="en">University of Sydney Institute of Marine Science (USIMS)</skos:prefLabel>
	<skos:altLabel xml:lang="en"></skos:altLabel>
	<skos:hiddenLabel xml:lang="en">USIMS</skos:hiddenLabel>
	<skos:definition xml:lang="en"></skos:definition>
	<dc:source rdf:datatype="http://www.w3.org/2001/XMLSchema#string">Australian Ocean Data Network Organisation Register</dc:source>
	<dc:publisher rdf:datatype="http://www.w3.org/2001/XMLSchema#string">eMarine Information Infrastructure (eMII)</dc:publisher>
	<skos:exactMatch rdf:resource="http://seadatanet.maris2.nl/v_edmo/print.asp?n_code=3856"/>
	<skos:inScheme rdf:resource="http://vocab.aodn.org.au/def/organisation/1"/>
	<skos:broader rdf:resource="http://vocab.aodn.org.au/def/organisation/entity/224"/>
	<skos:scopeNote xml:lang="en">Replaces http://vocab.aodn.org.au/def/organisation/entity/234</skos:scopeNote>
	<dcterms:replaces rdf:resource="http://vocab.aodn.org.au/def/organisation/entity/234"/>
	<dcterms:replaces xml:lang="en">Ocean Science Institute, The University of Sydney (USYD)</dcterms:replaces>
</rdf:Description>

<rdf:Description rdf:about="http://vocab.aodn.org.au/def/organisation/entity/228">
	<rdf:type rdf:resource="http://www.w3.org/2000/01/rdf-schema#Resource"/>
	<rdf:type rdf:resource="http://www.w3.org/2004/02/skos/core#Concept"/>
	<dcterms:creator rdf:datatype="http://www.w3.org/2001/XMLSchema#string">Natalia Atkins</dcterms:creator>
	<dcterms:created rdf:datatype="http://www.w3.org/2001/XMLSchema#dateTime">2015-07-10T10:38:15Z</dcterms:created>
	<skos:prefLabel xml:lang="en">Discipline of Anatomy and Histology, The University of Sydney (USYD)</skos:prefLabel>
	<skos:altLabel xml:lang="en">Discipline of Anatomy and Histology</skos:altLabel>
	<skos:hiddenLabel xml:lang="en"></skos:hiddenLabel>
	<skos:definition xml:lang="en">The Discipline of Anatomy and Histology is an education and research institution. Anatomy and Histology maintains a large catalogue of specimens for education and research. Research tools include a high-resolution transmission electron microscope and confocal microscope and excellent specimen preparation facilities.</skos:definition>
	<dc:source rdf:datatype="http://www.w3.org/2001/XMLSchema#string">Australian Ocean Data Network Organisation Register</dc:source>
	<dc:publisher rdf:datatype="http://www.w3.org/2001/XMLSchema#string">eMarine Information Infrastructure (eMII)</dc:publisher>
	<skos:inScheme rdf:resource="http://vocab.aodn.org.au/def/organisation/1"/>
	<skos:broader rdf:resource="http://vocab.aodn.org.au/def/organisation/entity/224"/>
</rdf:Description>

<rdf:Description rdf:about="http://vocab.aodn.org.au/def/organisation/entity/229">
	<rdf:type rdf:resource="http://www.w3.org/2000/01/rdf-schema#Resource"/>
	<rdf:type rdf:resource="http://www.w3.org/2004/02/skos/core#Concept"/>
	<dcterms:modified rdf:datatype="http://www.w3.org/2001/XMLSchema#dateTime">2015-07-14T01:56:43Z</dcterms:modified>
	<dcterms:creator rdf:datatype="http://www.w3.org/2001/XMLSchema#string">Natalia Atkins</dcterms:creator>
	<dcterms:created rdf:datatype="http://www.w3.org/2001/XMLSchema#dateTime">2015-07-10T10:38:15Z</dcterms:created>
	<dcterms:contributor rdf:datatype="http://www.w3.org/2001/XMLSchema#string">Natalia_Atkins</dcterms:contributor>
	<skos:prefLabel xml:lang="en">School of Aerospace, Mechanical and Mechatronic Engineering, The University of Sydney (USYD)</skos:prefLabel>
	<skos:altLabel xml:lang="en">School of Aerospace, Mechanical and Mechatronic Engineering</skos:altLabel>
	<skos:hiddenLabel xml:lang="en"></skos:hiddenLabel>
	<skos:definition xml:lang="en">The School of Aerospace, Mechanical and Mechatronic Engineering at the University of Sydney, has research areas including Biomaterials and Biomechanics, Combustion, Design Optimisation, Energy Production, Field Robotics, Fluid Dynamics, Materials and Manufacturing, Navigation and Control, Rheology, Smart Structures, Thermofluids and UAV Flight Systems.</skos:definition>
	<dc:source rdf:datatype="http://www.w3.org/2001/XMLSchema#string">Australian Ocean Data Network Organisation Register</dc:source>
	<dc:publisher rdf:datatype="http://www.w3.org/2001/XMLSchema#string">eMarine Information Infrastructure (eMII)</dc:publisher>
	<skos:exactMatch rdf:resource="http://seadatanet.maris2.nl/v_edmo/print.asp?n_code=4304"/>
	<skos:narrower rdf:resource="http://vocab.aodn.org.au/def/organisation/entity/230"/>
	<skos:inScheme rdf:resource="http://vocab.aodn.org.au/def/organisation/1"/>
	<skos:broader rdf:resource="http://vocab.aodn.org.au/def/organisation/entity/224"/>
</rdf:Description>

<rdf:Description rdf:about="http://vocab.aodn.org.au/def/organisation/entity/231">
	<rdf:type rdf:resource="http://www.w3.org/2000/01/rdf-schema#Resource"/>
	<rdf:type rdf:resource="http://www.w3.org/2004/02/skos/core#Concept"/>
	<dcterms:creator rdf:datatype="http://www.w3.org/2001/XMLSchema#string">Natalia Atkins</dcterms:creator>
	<dcterms:created rdf:datatype="http://www.w3.org/2001/XMLSchema#dateTime">2015-07-10T10:38:15Z</dcterms:created>
	<skos:prefLabel xml:lang="en">School of Biological Sciences, The University of Sydney (USYD)</skos:prefLabel>
	<skos:altLabel xml:lang="en">School of Biological Sciences</skos:altLabel>
	<skos:hiddenLabel xml:lang="en"></skos:hiddenLabel>
	<skos:definition xml:lang="en">The School of Biological Sciences study areas encompass: molecular biology; genetics; cell biology; physiology; behaviour; biodiversity; ecology and evolution of Australian plants and animals; and student-learning in biology.</skos:definition>
	<dc:source rdf:datatype="http://www.w3.org/2001/XMLSchema#string">Australian Ocean Data Network Organisation Register</dc:source>
	<dc:publisher rdf:datatype="http://www.w3.org/2001/XMLSchema#string">eMarine Information Infrastructure (eMII)</dc:publisher>
	<skos:exactMatch rdf:resource="http://seadatanet.maris2.nl/v_edmo/print.asp?n_code=4306"/>
	<skos:inScheme rdf:resource="http://vocab.aodn.org.au/def/organisation/1"/>
	<skos:broader rdf:resource="http://vocab.aodn.org.au/def/organisation/entity/224"/>
</rdf:Description>

<rdf:Description rdf:about="http://vocab.aodn.org.au/def/organisation/entity/232">
	<rdf:type rdf:resource="http://www.w3.org/2000/01/rdf-schema#Resource"/>
	<rdf:type rdf:resource="http://www.w3.org/2004/02/skos/core#Concept"/>
	<dcterms:creator rdf:datatype="http://www.w3.org/2001/XMLSchema#string">Natalia Atkins</dcterms:creator>
	<dcterms:created rdf:datatype="http://www.w3.org/2001/XMLSchema#dateTime">2015-07-10T10:38:15Z</dcterms:created>
	<skos:prefLabel xml:lang="en">Ocean Technology Group (OTG), The University of Sydney (USYD)</skos:prefLabel>
	<skos:altLabel xml:lang="en">Ocean Technology Group (OTG)</skos:altLabel>
	<skos:hiddenLabel xml:lang="en">OTG</skos:hiddenLabel>
	<skos:definition xml:lang="en">The Ocean Technology Group carries out research into aspects of ocean engineering, and is a member of The University of Sydney Institute of Marine Science.</skos:definition>
	<dc:source rdf:datatype="http://www.w3.org/2001/XMLSchema#string">Australian Ocean Data Network Organisation Register</dc:source>
	<dc:publisher rdf:datatype="http://www.w3.org/2001/XMLSchema#string">eMarine Information Infrastructure (eMII)</dc:publisher>
	<skos:exactMatch rdf:resource="http://seadatanet.maris2.nl/v_edmo/print.asp?n_code=4307"/>
	<skos:inScheme rdf:resource="http://vocab.aodn.org.au/def/organisation/1"/>
	<skos:broader rdf:resource="http://vocab.aodn.org.au/def/organisation/entity/224"/>
</rdf:Description>

<rdf:Description rdf:about="http://vocab.aodn.org.au/def/organisation/entity/233">
	<rdf:type rdf:resource="http://www.w3.org/2000/01/rdf-schema#Resource"/>
	<rdf:type rdf:resource="http://www.w3.org/2004/02/skos/core#Concept"/>
	<dcterms:creator rdf:datatype="http://www.w3.org/2001/XMLSchema#string">Natalia Atkins</dcterms:creator>
	<dcterms:created rdf:datatype="http://www.w3.org/2001/XMLSchema#dateTime">2015-07-10T10:38:15Z</dcterms:created>
	<skos:prefLabel xml:lang="en">Department of Geography, The University of Sydney (USYD)</skos:prefLabel>
	<skos:altLabel xml:lang="en">Department of Geography</skos:altLabel>
	<skos:hiddenLabel xml:lang="en"></skos:hiddenLabel>
	<skos:definition xml:lang="en">The Department of Geography merged with the Department of Geology and Geophysics in 1998, to form the current School of Geosciences.</skos:definition>
	<dc:source rdf:datatype="http://www.w3.org/2001/XMLSchema#string">Australian Ocean Data Network Organisation Register</dc:source>
	<dc:publisher rdf:datatype="http://www.w3.org/2001/XMLSchema#string">eMarine Information Infrastructure (eMII)</dc:publisher>
	<skos:inScheme rdf:resource="http://vocab.aodn.org.au/def/organisation/1"/>
	<skos:broader rdf:resource="http://vocab.aodn.org.au/def/organisation/entity/224"/>
	<skos:scopeNote xml:lang="en">Organisation no longer exists</skos:scopeNote>
	<skos:scopeNote xml:lang="en">Organisation no longer exists. Replaced by http://vocab.aodn.org.au/def/organisation/entity/225</skos:scopeNote>
	<dcterms:isReplacedBy rdf:resource="http://vocab.aodn.org.au/def/organisation/entity/225"/>
	<dcterms:isReplacedBy xml:lang="en">School of Geosciences, The University of Sydney (USYD)</dcterms:isReplacedBy>
</rdf:Description>

<rdf:Description rdf:about="http://vocab.aodn.org.au/def/organisation/entity/234">
	<rdf:type rdf:resource="http://www.w3.org/2000/01/rdf-schema#Resource"/>
	<rdf:type rdf:resource="http://www.w3.org/2004/02/skos/core#Concept"/>
	<dcterms:creator rdf:datatype="http://www.w3.org/2001/XMLSchema#string">Natalia Atkins</dcterms:creator>
	<dcterms:created rdf:datatype="http://www.w3.org/2001/XMLSchema#dateTime">2015-07-10T10:38:15Z</dcterms:created>
	<skos:prefLabel xml:lang="en">Ocean Science Institute, The University of Sydney (USYD)</skos:prefLabel>
	<skos:altLabel xml:lang="en">Ocean Science Institute</skos:altLabel>
	<skos:hiddenLabel xml:lang="en"></skos:hiddenLabel>
	<skos:definition xml:lang="en">Marine Science at the University of Sydney dates back to the 1880's. The Marine Studies Centre and the Ocean Science Institute were established in 1970, and these were replaced by the University of Sydney Institute of Marine Science (USIMS) in 2002.</skos:definition>
	<dc:source rdf:datatype="http://www.w3.org/2001/XMLSchema#string">Australian Ocean Data Network Organisation Register</dc:source>
	<dc:publisher rdf:datatype="http://www.w3.org/2001/XMLSchema#string">eMarine Information Infrastructure (eMII)</dc:publisher>
	<skos:inScheme rdf:resource="http://vocab.aodn.org.au/def/organisation/1"/>
	<skos:broader rdf:resource="http://vocab.aodn.org.au/def/organisation/entity/224"/>
	<skos:scopeNote xml:lang="en">Organisation no longer exists</skos:scopeNote>
	<skos:scopeNote xml:lang="en">Organisation no longer exists. Replaced by http://vocab.aodn.org.au/def/organisation/entity/227</skos:scopeNote>
	<dcterms:isReplacedBy rdf:resource="http://vocab.aodn.org.au/def/organisation/entity/227"/>
	<dcterms:isReplacedBy xml:lang="en">University of Sydney Institute of Marine Science (USIMS)</dcterms:isReplacedBy>
</rdf:Description>

<rdf:Description rdf:about="http://seadatanet.maris2.nl/v_edmo/print.asp?n_code=3056">
	<rdf:type rdf:resource="http://www.w3.org/2000/01/rdf-schema#Resource"/>
</rdf:Description>

<rdf:Description rdf:about="http://purl.org/dc/terms/replaces">
	<rdf:type rdf:resource="http://www.w3.org/1999/02/22-rdf-syntax-ns#Property"/>
	<rdf:type rdf:resource="http://www.w3.org/2000/01/rdf-schema#Resource"/>
	<rdfs:subPropertyOf rdf:resource="http://purl.org/dc/terms/replaces"/>
</rdf:Description>

<rdf:Description rdf:about="http://seadatanet.maris2.nl/v_edmo/print.asp?n_code=3208">
	<rdf:type rdf:resource="http://www.w3.org/2000/01/rdf-schema#Resource"/>
</rdf:Description>

<rdf:Description rdf:about="http://seadatanet.maris2.nl/v_edmo/print.asp?n_code=3856">
	<rdf:type rdf:resource="http://www.w3.org/2000/01/rdf-schema#Resource"/>
</rdf:Description>

<rdf:Description rdf:about="http://seadatanet.maris2.nl/v_edmo/print.asp?n_code=4304">
	<rdf:type rdf:resource="http://www.w3.org/2000/01/rdf-schema#Resource"/>
</rdf:Description>

<rdf:Description rdf:about="http://vocab.aodn.org.au/def/organisation/entity/230">
	<rdf:type rdf:resource="http://www.w3.org/2000/01/rdf-schema#Resource"/>
	<rdf:type rdf:resource="http://www.w3.org/2004/02/skos/core#Concept"/>
	<dcterms:modified rdf:datatype="http://www.w3.org/2001/XMLSchema#dateTime">2015-07-14T01:56:51Z</dcterms:modified>
	<dcterms:creator rdf:datatype="http://www.w3.org/2001/XMLSchema#string">Natalia Atkins</dcterms:creator>
	<dcterms:created rdf:datatype="http://www.w3.org/2001/XMLSchema#dateTime">2015-07-10T10:38:15Z</dcterms:created>
	<dcterms:contributor rdf:datatype="http://www.w3.org/2001/XMLSchema#string">Natalia_Atkins</dcterms:contributor>
	<skos:prefLabel xml:lang="en">Australian Centre for Field Robotics (ACFR), School of Aerospace, Mechanical and Mechatronic Engineering, The University of Sydney (USYD)</skos:prefLabel>
	<skos:altLabel xml:lang="en">Australian Centre for Field Robotics (ACFR)</skos:altLabel>
	<skos:hiddenLabel xml:lang="en">ACFR</skos:hiddenLabel>
	<skos:definition xml:lang="en">The Australian Centre for Field Robotics (ACFR) is based in the School of Aerospace, Mechanical and Mechatronic Engineering at The University of Sydney, and is dedicated to the research, development, application and dissemination of autonomous and intelligent robots and systems for operation in outdoor environments.</skos:definition>
	<dc:source rdf:datatype="http://www.w3.org/2001/XMLSchema#string">Australian Ocean Data Network Organisation Register</dc:source>
	<dc:publisher rdf:datatype="http://www.w3.org/2001/XMLSchema#string">eMarine Information Infrastructure (eMII)</dc:publisher>
	<skos:exactMatch rdf:resource="http://seadatanet.maris2.nl/v_edmo/print.asp?n_code=4305"/>
	<skos:inScheme rdf:resource="http://vocab.aodn.org.au/def/organisation/1"/>
	<skos:broader rdf:resource="http://vocab.aodn.org.au/def/organisation/entity/229"/>
</rdf:Description>

<rdf:Description rdf:about="http://seadatanet.maris2.nl/v_edmo/print.asp?n_code=4305">
	<rdf:type rdf:resource="http://www.w3.org/2000/01/rdf-schema#Resource"/>
</rdf:Description>

<rdf:Description rdf:about="http://seadatanet.maris2.nl/v_edmo/print.asp?n_code=4306">
	<rdf:type rdf:resource="http://www.w3.org/2000/01/rdf-schema#Resource"/>
</rdf:Description>

<rdf:Description rdf:about="http://seadatanet.maris2.nl/v_edmo/print.asp?n_code=4307">
	<rdf:type rdf:resource="http://www.w3.org/2000/01/rdf-schema#Resource"/>
</rdf:Description>

<rdf:Description rdf:about="http://purl.org/dc/terms/isReplacedBy">
	<rdf:type rdf:resource="http://www.w3.org/1999/02/22-rdf-syntax-ns#Property"/>
	<rdf:type rdf:resource="http://www.w3.org/2000/01/rdf-schema#Resource"/>
	<rdfs:subPropertyOf rdf:resource="http://purl.org/dc/terms/isReplacedBy"/>
</rdf:Description>

<rdf:Description rdf:about="http://seadatanet.maris2.nl/v_edmo/print.asp?n_code=4308">
	<rdf:type rdf:resource="http://www.w3.org/2000/01/rdf-schema#Resource"/>
</rdf:Description>

<rdf:Description rdf:about="http://vocab.aodn.org.au/def/organisation/entity/236">
	<rdf:type rdf:resource="http://www.w3.org/2000/01/rdf-schema#Resource"/>
	<rdf:type rdf:resource="http://www.w3.org/2004/02/skos/core#Concept"/>
	<dcterms:creator rdf:datatype="http://www.w3.org/2001/XMLSchema#string">Natalia Atkins</dcterms:creator>
	<dcterms:created rdf:datatype="http://www.w3.org/2001/XMLSchema#dateTime">2015-07-10T10:38:15Z</dcterms:created>
	<skos:prefLabel xml:lang="en">School of Environmental Systems Engineering, The University of Western Australia (UWA)</skos:prefLabel>
	<skos:altLabel xml:lang="en">School of Environmental Systems Engineering</skos:altLabel>
	<skos:hiddenLabel xml:lang="en"></skos:hiddenLabel>
	<skos:definition xml:lang="en"></skos:definition>
	<dc:source rdf:datatype="http://www.w3.org/2001/XMLSchema#string">Australian Ocean Data Network Organisation Register</dc:source>
	<dc:publisher rdf:datatype="http://www.w3.org/2001/XMLSchema#string">eMarine Information Infrastructure (eMII)</dc:publisher>
	<skos:exactMatch rdf:resource="http://seadatanet.maris2.nl/v_edmo/print.asp?n_code=2372"/>
	<skos:inScheme rdf:resource="http://vocab.aodn.org.au/def/organisation/1"/>
	<skos:broader rdf:resource="http://vocab.aodn.org.au/def/organisation/entity/235"/>
	<skos:scopeNote xml:lang="en">Organisation no longer exists</skos:scopeNote>
	<skos:scopeNote xml:lang="en">Organisation no longer exists. Replaced by http://vocab.aodn.org.au/def/organisation/entity/237</skos:scopeNote>
	<dcterms:isReplacedBy rdf:resource="http://vocab.aodn.org.au/def/organisation/entity/237"/>
	<dcterms:isReplacedBy xml:lang="en">School of Civil, Environmental and Mining Engineering (CEME), The University of Western Australia (UWA)</dcterms:isReplacedBy>
</rdf:Description>

<rdf:Description rdf:about="http://vocab.aodn.org.au/def/organisation/entity/237">
	<rdf:type rdf:resource="http://www.w3.org/2000/01/rdf-schema#Resource"/>
	<rdf:type rdf:resource="http://www.w3.org/2004/02/skos/core#Concept"/>
	<dcterms:creator rdf:datatype="http://www.w3.org/2001/XMLSchema#string">Natalia Atkins</dcterms:creator>
	<dcterms:created rdf:datatype="http://www.w3.org/2001/XMLSchema#dateTime">2015-07-10T10:38:15Z</dcterms:created>
	<skos:prefLabel xml:lang="en">School of Civil, Environmental and Mining Engineering (CEME), The University of Western Australia (UWA)</skos:prefLabel>
	<skos:altLabel xml:lang="en">School of Civil, Environmental and Mining Engineering (CEME)</skos:altLabel>
	<skos:hiddenLabel xml:lang="en">CEME</skos:hiddenLabel>
	<skos:definition xml:lang="en">The School offers  coursework and research opportunities in all major areas of Civil, Environmental and Mining Engineering, with a focus on research in Engineering for Remote Operations.</skos:definition>
	<dc:source rdf:datatype="http://www.w3.org/2001/XMLSchema#string">Australian Ocean Data Network Organisation Register</dc:source>
	<dc:publisher rdf:datatype="http://www.w3.org/2001/XMLSchema#string">eMarine Information Infrastructure (eMII)</dc:publisher>
	<skos:exactMatch rdf:resource="http://seadatanet.maris2.nl/v_edmo/print.asp?n_code=4309"/>
	<skos:inScheme rdf:resource="http://vocab.aodn.org.au/def/organisation/1"/>
	<skos:broader rdf:resource="http://vocab.aodn.org.au/def/organisation/entity/235"/>
	<skos:scopeNote xml:lang="en">Replaces http://vocab.aodn.org.au/def/organisation/entity/236</skos:scopeNote>
	<dcterms:replaces rdf:resource="http://vocab.aodn.org.au/def/organisation/entity/236"/>
	<dcterms:replaces xml:lang="en">School of Environmental Systems Engineering, The University of Western Australia (UWA)</dcterms:replaces>
</rdf:Description>

<rdf:Description rdf:about="http://vocab.aodn.org.au/def/organisation/entity/238">
	<rdf:type rdf:resource="http://www.w3.org/2000/01/rdf-schema#Resource"/>
	<rdf:type rdf:resource="http://www.w3.org/2004/02/skos/core#Concept"/>
	<dcterms:creator rdf:datatype="http://www.w3.org/2001/XMLSchema#string">Natalia Atkins</dcterms:creator>
	<dcterms:created rdf:datatype="http://www.w3.org/2001/XMLSchema#dateTime">2015-07-10T10:38:15Z</dcterms:created>
	<skos:prefLabel xml:lang="en">Centre for Water Research (CWR), The University of Western Australia (UWA)</skos:prefLabel>
	<skos:altLabel xml:lang="en">Centre for Water Research (CWR)</skos:altLabel>
	<skos:hiddenLabel xml:lang="en">CWR</skos:hiddenLabel>
	<skos:definition xml:lang="en">This centre was established in 1982 and contributed to the understanding of the transport and mixing processes in stratified lakes, estuaries and coastal seas. It  was shut in 2015.</skos:definition>
	<dc:source rdf:datatype="http://www.w3.org/2001/XMLSchema#string">Australian Ocean Data Network Organisation Register</dc:source>
	<dc:publisher rdf:datatype="http://www.w3.org/2001/XMLSchema#string">eMarine Information Infrastructure (eMII)</dc:publisher>
	<skos:inScheme rdf:resource="http://vocab.aodn.org.au/def/organisation/1"/>
	<skos:broader rdf:resource="http://vocab.aodn.org.au/def/organisation/entity/235"/>
	<skos:scopeNote xml:lang="en">Organisation no longer exists</skos:scopeNote>
</rdf:Description>

<rdf:Description rdf:about="http://vocab.aodn.org.au/def/organisation/entity/239">
	<rdf:type rdf:resource="http://www.w3.org/2000/01/rdf-schema#Resource"/>
	<rdf:type rdf:resource="http://www.w3.org/2004/02/skos/core#Concept"/>
	<dcterms:creator rdf:datatype="http://www.w3.org/2001/XMLSchema#string">Natalia Atkins</dcterms:creator>
	<dcterms:created rdf:datatype="http://www.w3.org/2001/XMLSchema#dateTime">2015-07-10T10:38:15Z</dcterms:created>
	<skos:prefLabel xml:lang="en">Department of Botany, The University of Western Australia (UWA)</skos:prefLabel>
	<skos:altLabel xml:lang="en">Department of Botany</skos:altLabel>
	<skos:hiddenLabel xml:lang="en"></skos:hiddenLabel>
	<skos:definition xml:lang="en">This former department is now known as the School of Plant Biology.</skos:definition>
	<dc:source rdf:datatype="http://www.w3.org/2001/XMLSchema#string">Australian Ocean Data Network Organisation Register</dc:source>
	<dc:publisher rdf:datatype="http://www.w3.org/2001/XMLSchema#string">eMarine Information Infrastructure (eMII)</dc:publisher>
	<skos:inScheme rdf:resource="http://vocab.aodn.org.au/def/organisation/1"/>
	<skos:broader rdf:resource="http://vocab.aodn.org.au/def/organisation/entity/235"/>
	<skos:scopeNote xml:lang="en">Organisation no longer exists</skos:scopeNote>
	<skos:scopeNote xml:lang="en">Organisation no longer exists. Replaced by http://vocab.aodn.org.au/def/organisation/entity/240</skos:scopeNote>
	<dcterms:isReplacedBy rdf:resource="http://vocab.aodn.org.au/def/organisation/entity/240"/>
	<dcterms:isReplacedBy xml:lang="en">School of Plant Biology (SPB), The University of Western Australia (UWA)</dcterms:isReplacedBy>
</rdf:Description>

<rdf:Description rdf:about="http://vocab.aodn.org.au/def/organisation/entity/240">
	<rdf:type rdf:resource="http://www.w3.org/2000/01/rdf-schema#Resource"/>
	<rdf:type rdf:resource="http://www.w3.org/2004/02/skos/core#Concept"/>
	<dcterms:creator rdf:datatype="http://www.w3.org/2001/XMLSchema#string">Natalia Atkins</dcterms:creator>
	<dcterms:created rdf:datatype="http://www.w3.org/2001/XMLSchema#dateTime">2015-07-10T10:38:15Z</dcterms:created>
	<skos:prefLabel xml:lang="en">School of Plant Biology (SPB), The University of Western Australia (UWA)</skos:prefLabel>
	<skos:altLabel xml:lang="en">School of Plant Biology (SPB)</skos:altLabel>
	<skos:hiddenLabel xml:lang="en">SPB</skos:hiddenLabel>
	<skos:definition xml:lang="en">The School of Plant Biology is a research intensive school focusing on cropping, marine and natural terrestrial systems.</skos:definition>
	<dc:source rdf:datatype="http://www.w3.org/2001/XMLSchema#string">Australian Ocean Data Network Organisation Register</dc:source>
	<dc:publisher rdf:datatype="http://www.w3.org/2001/XMLSchema#string">eMarine Information Infrastructure (eMII)</dc:publisher>
	<skos:exactMatch rdf:resource="http://seadatanet.maris2.nl/v_edmo/print.asp?n_code=4310"/>
	<skos:inScheme rdf:resource="http://vocab.aodn.org.au/def/organisation/1"/>
	<skos:broader rdf:resource="http://vocab.aodn.org.au/def/organisation/entity/235"/>
	<skos:scopeNote xml:lang="en">Replaces http://vocab.aodn.org.au/def/organisation/entity/239</skos:scopeNote>
	<dcterms:replaces rdf:resource="http://vocab.aodn.org.au/def/organisation/entity/239"/>
	<dcterms:replaces xml:lang="en">Department of Botany, The University of Western Australia (UWA)</dcterms:replaces>
</rdf:Description>

<rdf:Description rdf:about="http://vocab.aodn.org.au/def/organisation/entity/241">
	<rdf:type rdf:resource="http://www.w3.org/2000/01/rdf-schema#Resource"/>
	<rdf:type rdf:resource="http://www.w3.org/2004/02/skos/core#Concept"/>
	<dcterms:creator rdf:datatype="http://www.w3.org/2001/XMLSchema#string">Natalia Atkins</dcterms:creator>
	<dcterms:created rdf:datatype="http://www.w3.org/2001/XMLSchema#dateTime">2015-07-10T10:38:15Z</dcterms:created>
	<skos:prefLabel xml:lang="en">UWA Oceans Institute (OI), The University of Western Australia (UWA)</skos:prefLabel>
	<skos:altLabel xml:lang="en">UWA Oceans Institute (OI)</skos:altLabel>
	<skos:hiddenLabel xml:lang="en">OI</skos:hiddenLabel>
	<skos:definition xml:lang="en">The UWA Oceans Institute brings together UWA's researchers into a multidisciplinary, integrated research focus. It's goal is to capitalise on UWA's existing research strengths – in areas such as oceanography, ecology, engineering, resource management, and governance.</skos:definition>
	<dc:source rdf:datatype="http://www.w3.org/2001/XMLSchema#string">Australian Ocean Data Network Organisation Register</dc:source>
	<dc:publisher rdf:datatype="http://www.w3.org/2001/XMLSchema#string">eMarine Information Infrastructure (eMII)</dc:publisher>
	<skos:exactMatch rdf:resource="http://seadatanet.maris2.nl/v_edmo/print.asp?n_code=4311"/>
	<skos:inScheme rdf:resource="http://vocab.aodn.org.au/def/organisation/1"/>
	<skos:broader rdf:resource="http://vocab.aodn.org.au/def/organisation/entity/235"/>
</rdf:Description>

<rdf:Description rdf:about="http://vocab.aodn.org.au/def/organisation/entity/242">
	<rdf:type rdf:resource="http://www.w3.org/2000/01/rdf-schema#Resource"/>
	<rdf:type rdf:resource="http://www.w3.org/2004/02/skos/core#Concept"/>
	<dcterms:creator rdf:datatype="http://www.w3.org/2001/XMLSchema#string">Natalia Atkins</dcterms:creator>
	<dcterms:created rdf:datatype="http://www.w3.org/2001/XMLSchema#dateTime">2015-07-10T10:38:15Z</dcterms:created>
	<skos:prefLabel xml:lang="en">Department of Zoology, The University of Western Australia (UWA)</skos:prefLabel>
	<skos:altLabel xml:lang="en">Department of Zoology</skos:altLabel>
	<skos:hiddenLabel xml:lang="en"></skos:hiddenLabel>
	<skos:definition xml:lang="en">This former departments is now known as the School of Animal Biology.</skos:definition>
	<dc:source rdf:datatype="http://www.w3.org/2001/XMLSchema#string">Australian Ocean Data Network Organisation Register</dc:source>
	<dc:publisher rdf:datatype="http://www.w3.org/2001/XMLSchema#string">eMarine Information Infrastructure (eMII)</dc:publisher>
	<skos:inScheme rdf:resource="http://vocab.aodn.org.au/def/organisation/1"/>
	<skos:broader rdf:resource="http://vocab.aodn.org.au/def/organisation/entity/235"/>
	<skos:scopeNote xml:lang="en">Organisation no longer exists</skos:scopeNote>
	<skos:scopeNote xml:lang="en">Organisation no longer exists. Replaced by http://vocab.aodn.org.au/def/organisation/entity/243</skos:scopeNote>
	<dcterms:isReplacedBy rdf:resource="http://vocab.aodn.org.au/def/organisation/entity/243"/>
	<dcterms:isReplacedBy xml:lang="en">School of Animal Biology (SAB), The University of Western Australia (UWA)</dcterms:isReplacedBy>
</rdf:Description>

<rdf:Description rdf:about="http://vocab.aodn.org.au/def/organisation/entity/243">
	<rdf:type rdf:resource="http://www.w3.org/2000/01/rdf-schema#Resource"/>
	<rdf:type rdf:resource="http://www.w3.org/2004/02/skos/core#Concept"/>
	<dcterms:creator rdf:datatype="http://www.w3.org/2001/XMLSchema#string">Natalia Atkins</dcterms:creator>
	<dcterms:created rdf:datatype="http://www.w3.org/2001/XMLSchema#dateTime">2015-07-10T10:38:15Z</dcterms:created>
	<skos:prefLabel xml:lang="en">School of Animal Biology (SAB), The University of Western Australia (UWA)</skos:prefLabel>
	<skos:altLabel xml:lang="en">School of Animal Biology (SAB)</skos:altLabel>
	<skos:hiddenLabel xml:lang="en">SAB</skos:hiddenLabel>
	<skos:definition xml:lang="en">The School offers coursework and research opportunities in animals and industry, animal structure and function, ecology, evolutionary biology, experimental and regenerative neurosciences, marine biology, neuroecology, science communication and wildlife management.</skos:definition>
	<dc:source rdf:datatype="http://www.w3.org/2001/XMLSchema#string">Australian Ocean Data Network Organisation Register</dc:source>
	<dc:publisher rdf:datatype="http://www.w3.org/2001/XMLSchema#string">eMarine Information Infrastructure (eMII)</dc:publisher>
	<skos:exactMatch rdf:resource="http://seadatanet.maris2.nl/v_edmo/print.asp?n_code=4312"/>
	<skos:inScheme rdf:resource="http://vocab.aodn.org.au/def/organisation/1"/>
	<skos:broader rdf:resource="http://vocab.aodn.org.au/def/organisation/entity/235"/>
	<skos:scopeNote xml:lang="en">Replaces http://vocab.aodn.org.au/def/organisation/entity/242</skos:scopeNote>
	<dcterms:replaces rdf:resource="http://vocab.aodn.org.au/def/organisation/entity/242"/>
	<dcterms:replaces xml:lang="en">Department of Zoology, The University of Western Australia (UWA)</dcterms:replaces>
</rdf:Description>

<rdf:Description rdf:about="http://vocab.aodn.org.au/def/organisation/entity/244">
	<rdf:type rdf:resource="http://www.w3.org/2000/01/rdf-schema#Resource"/>
	<rdf:type rdf:resource="http://www.w3.org/2004/02/skos/core#Concept"/>
	<dcterms:creator rdf:datatype="http://www.w3.org/2001/XMLSchema#string">Natalia Atkins</dcterms:creator>
	<dcterms:created rdf:datatype="http://www.w3.org/2001/XMLSchema#dateTime">2015-07-10T10:38:15Z</dcterms:created>
	<skos:prefLabel xml:lang="en">School of Earth and Environment (SEE), The University of Western Australia (UWA)</skos:prefLabel>
	<skos:altLabel xml:lang="en">School of Earth and Environment (SEE)</skos:altLabel>
	<skos:hiddenLabel xml:lang="en">SEE</skos:hiddenLabel>
	<skos:definition xml:lang="en">The School offers coursework and research opportunities spanning geosciences, geography and planning, soil science, environmental science and more.</skos:definition>
	<dc:source rdf:datatype="http://www.w3.org/2001/XMLSchema#string">Australian Ocean Data Network Organisation Register</dc:source>
	<dc:publisher rdf:datatype="http://www.w3.org/2001/XMLSchema#string">eMarine Information Infrastructure (eMII)</dc:publisher>
	<skos:exactMatch rdf:resource="http://seadatanet.maris2.nl/v_edmo/print.asp?n_code=4313"/>
	<skos:inScheme rdf:resource="http://vocab.aodn.org.au/def/organisation/1"/>
	<skos:broader rdf:resource="http://vocab.aodn.org.au/def/organisation/entity/235"/>
	<skos:scopeNote xml:lang="en">Replaces http://vocab.aodn.org.au/def/organisation/entity/248</skos:scopeNote>
	<dcterms:replaces rdf:resource="http://vocab.aodn.org.au/def/organisation/entity/248"/>
	<dcterms:replaces xml:lang="en">Department of Geography, The University of Western Australia (UWA)</dcterms:replaces>
</rdf:Description>

<rdf:Description rdf:about="http://vocab.aodn.org.au/def/organisation/entity/245">
	<rdf:type rdf:resource="http://www.w3.org/2000/01/rdf-schema#Resource"/>
	<rdf:type rdf:resource="http://www.w3.org/2004/02/skos/core#Concept"/>
	<dcterms:creator rdf:datatype="http://www.w3.org/2001/XMLSchema#string">Natalia Atkins</dcterms:creator>
	<dcterms:created rdf:datatype="http://www.w3.org/2001/XMLSchema#dateTime">2015-07-10T10:38:15Z</dcterms:created>
	<skos:prefLabel xml:lang="en">Centre of Excellence in Natural Resource Management(CENRM) , The University of Western Australia (UWA)</skos:prefLabel>
	<skos:altLabel xml:lang="en">Centre of Excellence in Natural Resource Management(CENRM)</skos:altLabel>
	<skos:hiddenLabel xml:lang="en">CENRM</skos:hiddenLabel>
	<skos:definition xml:lang="en">The centre's research focuses on enhancing the environmental, economic, social and cultural well-being of south-western Australia and elsewhere. The Centre is located in Western Australia's Great Southern region, a global hotspot of biodiversity. The centre complements its research through applied consultancy, education and communication.</skos:definition>
	<dc:source rdf:datatype="http://www.w3.org/2001/XMLSchema#string">Australian Ocean Data Network Organisation Register</dc:source>
	<dc:publisher rdf:datatype="http://www.w3.org/2001/XMLSchema#string">eMarine Information Infrastructure (eMII)</dc:publisher>
	<skos:exactMatch rdf:resource="http://seadatanet.maris2.nl/v_edmo/print.asp?n_code=4314"/>
	<skos:inScheme rdf:resource="http://vocab.aodn.org.au/def/organisation/1"/>
	<skos:broader rdf:resource="http://vocab.aodn.org.au/def/organisation/entity/235"/>
</rdf:Description>

<rdf:Description rdf:about="http://vocab.aodn.org.au/def/organisation/entity/246">
	<rdf:type rdf:resource="http://www.w3.org/2000/01/rdf-schema#Resource"/>
	<rdf:type rdf:resource="http://www.w3.org/2004/02/skos/core#Concept"/>
	<dcterms:creator rdf:datatype="http://www.w3.org/2001/XMLSchema#string">Natalia Atkins</dcterms:creator>
	<dcterms:created rdf:datatype="http://www.w3.org/2001/XMLSchema#dateTime">2015-07-10T10:38:15Z</dcterms:created>
	<skos:prefLabel xml:lang="en">Harry Perkins Institute of Medical Research</skos:prefLabel>
	<skos:altLabel xml:lang="en"></skos:altLabel>
	<skos:hiddenLabel xml:lang="en"></skos:hiddenLabel>
	<skos:definition xml:lang="en">The Harry Perkins Institute of Medical Research was established in 1998 as the Western Australian Institute for Medical Research (WAIMR) with the vision of creating a multi-site Institute that would enhance collaboration between Western Australian medical researchers. The University of Western Australia, Royal Perth Hospital and Sir Charles Gairdner Hospital were our founding partners and in July 2003, Fremantle Hospital also became a partner. In October 2013, WAIMR changed its name to the Harry Perkins Institute of Medical Research to honour our inaugural Chairman, Harry Perkins AO.</skos:definition>
	<dc:source rdf:datatype="http://www.w3.org/2001/XMLSchema#string">Australian Ocean Data Network Organisation Register</dc:source>
	<dc:publisher rdf:datatype="http://www.w3.org/2001/XMLSchema#string">eMarine Information Infrastructure (eMII)</dc:publisher>
	<skos:inScheme rdf:resource="http://vocab.aodn.org.au/def/organisation/1"/>
	<skos:broader rdf:resource="http://vocab.aodn.org.au/def/organisation/entity/235"/>
</rdf:Description>

<rdf:Description rdf:about="http://vocab.aodn.org.au/def/organisation/entity/247">
	<rdf:type rdf:resource="http://www.w3.org/2000/01/rdf-schema#Resource"/>
	<rdf:type rdf:resource="http://www.w3.org/2004/02/skos/core#Concept"/>
	<dcterms:creator rdf:datatype="http://www.w3.org/2001/XMLSchema#string">Natalia Atkins</dcterms:creator>
	<dcterms:created rdf:datatype="http://www.w3.org/2001/XMLSchema#dateTime">2015-07-10T10:38:15Z</dcterms:created>
	<skos:prefLabel xml:lang="en">Centre for Marine Futures, The University of Western Australia (UWA)</skos:prefLabel>
	<skos:altLabel xml:lang="en">Centre for Marine Futures</skos:altLabel>
	<skos:hiddenLabel xml:lang="en"></skos:hiddenLabel>
	<skos:definition xml:lang="en">The Centre for Marine Futures applies innovative science to a wide range of marine environmental challenges.</skos:definition>
	<dc:source rdf:datatype="http://www.w3.org/2001/XMLSchema#string">Australian Ocean Data Network Organisation Register</dc:source>
	<dc:publisher rdf:datatype="http://www.w3.org/2001/XMLSchema#string">eMarine Information Infrastructure (eMII)</dc:publisher>
	<skos:exactMatch rdf:resource="http://seadatanet.maris2.nl/v_edmo/print.asp?n_code=4315"/>
	<skos:inScheme rdf:resource="http://vocab.aodn.org.au/def/organisation/1"/>
	<skos:broader rdf:resource="http://vocab.aodn.org.au/def/organisation/entity/235"/>
</rdf:Description>

<rdf:Description rdf:about="http://vocab.aodn.org.au/def/organisation/entity/248">
	<rdf:type rdf:resource="http://www.w3.org/2000/01/rdf-schema#Resource"/>
	<rdf:type rdf:resource="http://www.w3.org/2004/02/skos/core#Concept"/>
	<dcterms:creator rdf:datatype="http://www.w3.org/2001/XMLSchema#string">Natalia Atkins</dcterms:creator>
	<dcterms:created rdf:datatype="http://www.w3.org/2001/XMLSchema#dateTime">2015-07-10T10:38:15Z</dcterms:created>
	<skos:prefLabel xml:lang="en">Department of Geography, The University of Western Australia (UWA)</skos:prefLabel>
	<skos:altLabel xml:lang="en">Department of Geography</skos:altLabel>
	<skos:hiddenLabel xml:lang="en"></skos:hiddenLabel>
	<skos:definition xml:lang="en">This former departments is now part of the School of Earth and Environment.</skos:definition>
	<dc:source rdf:datatype="http://www.w3.org/2001/XMLSchema#string">Australian Ocean Data Network Organisation Register</dc:source>
	<dc:publisher rdf:datatype="http://www.w3.org/2001/XMLSchema#string">eMarine Information Infrastructure (eMII)</dc:publisher>
	<skos:inScheme rdf:resource="http://vocab.aodn.org.au/def/organisation/1"/>
	<skos:broader rdf:resource="http://vocab.aodn.org.au/def/organisation/entity/235"/>
	<skos:scopeNote xml:lang="en">Organisation no longer exists</skos:scopeNote>
	<skos:scopeNote xml:lang="en">Organisation no longer exists. Replaced by http://vocab.aodn.org.au/def/organisation/entity/244</skos:scopeNote>
	<dcterms:isReplacedBy rdf:resource="http://vocab.aodn.org.au/def/organisation/entity/244"/>
	<dcterms:isReplacedBy xml:lang="en">School of Earth and Environment (SEE), The University of Western Australia (UWA)</dcterms:isReplacedBy>
</rdf:Description>

<rdf:Description rdf:about="http://vocab.aodn.org.au/def/organisation/entity/249">
	<rdf:type rdf:resource="http://www.w3.org/2000/01/rdf-schema#Resource"/>
	<rdf:type rdf:resource="http://www.w3.org/2004/02/skos/core#Concept"/>
	<dcterms:creator rdf:datatype="http://www.w3.org/2001/XMLSchema#string">Natalia Atkins</dcterms:creator>
	<dcterms:created rdf:datatype="http://www.w3.org/2001/XMLSchema#dateTime">2015-07-10T10:38:15Z</dcterms:created>
	<skos:prefLabel xml:lang="en">School of Pathology and Laboratory Medicine, The University of Western Australia (UWA)</skos:prefLabel>
	<skos:altLabel xml:lang="en">School of Pathology and Laboratory Medicine</skos:altLabel>
	<skos:hiddenLabel xml:lang="en"></skos:hiddenLabel>
	<skos:definition xml:lang="en">This school was formed in January 2008, adding to the University's reputation for excellence in both medical teaching and research. Located at Queen Elizabeth II Medical Centre and Royal Perth Hospital, we give students hospital-based learning, while staff and postgraduates can access to major research facilities.</skos:definition>
	<dc:source rdf:datatype="http://www.w3.org/2001/XMLSchema#string">Australian Ocean Data Network Organisation Register</dc:source>
	<dc:publisher rdf:datatype="http://www.w3.org/2001/XMLSchema#string">eMarine Information Infrastructure (eMII)</dc:publisher>
	<skos:inScheme rdf:resource="http://vocab.aodn.org.au/def/organisation/1"/>
	<skos:broader rdf:resource="http://vocab.aodn.org.au/def/organisation/entity/235"/>
</rdf:Description>

<rdf:Description rdf:about="http://vocab.aodn.org.au/def/organisation/entity/250">
	<rdf:type rdf:resource="http://www.w3.org/2000/01/rdf-schema#Resource"/>
	<rdf:type rdf:resource="http://www.w3.org/2004/02/skos/core#Concept"/>
	<dcterms:creator rdf:datatype="http://www.w3.org/2001/XMLSchema#string">Natalia Atkins</dcterms:creator>
	<dcterms:created rdf:datatype="http://www.w3.org/2001/XMLSchema#dateTime">2015-07-10T10:38:15Z</dcterms:created>
	<skos:prefLabel xml:lang="en">School of Agricultural and Resource Economics, The University of Western Australia (UWA)</skos:prefLabel>
	<skos:altLabel xml:lang="en">School of Agricultural and Resource Economics</skos:altLabel>
	<skos:hiddenLabel xml:lang="en"></skos:hiddenLabel>
	<skos:definition xml:lang="en">The school focuses on the interaction of people with natural resources, with expertise in natural resource management, bioeconomic modelling, agricultural risk management and policy analysis.</skos:definition>
	<dc:source rdf:datatype="http://www.w3.org/2001/XMLSchema#string">Australian Ocean Data Network Organisation Register</dc:source>
	<dc:publisher rdf:datatype="http://www.w3.org/2001/XMLSchema#string">eMarine Information Infrastructure (eMII)</dc:publisher>
	<skos:exactMatch rdf:resource="http://seadatanet.maris2.nl/v_edmo/print.asp?n_code=4316"/>
	<skos:inScheme rdf:resource="http://vocab.aodn.org.au/def/organisation/1"/>
	<skos:broader rdf:resource="http://vocab.aodn.org.au/def/organisation/entity/235"/>
</rdf:Description>

<rdf:Description rdf:about="http://vocab.aodn.org.au/def/organisation/entity/251">
	<rdf:type rdf:resource="http://www.w3.org/2000/01/rdf-schema#Resource"/>
	<rdf:type rdf:resource="http://www.w3.org/2004/02/skos/core#Concept"/>
	<dcterms:creator rdf:datatype="http://www.w3.org/2001/XMLSchema#string">Natalia Atkins</dcterms:creator>
	<dcterms:created rdf:datatype="http://www.w3.org/2001/XMLSchema#dateTime">2015-07-10T10:38:15Z</dcterms:created>
	<skos:prefLabel xml:lang="en">School of Social Sciences, The University of Western Australia (UWA)</skos:prefLabel>
	<skos:altLabel xml:lang="en">School of Social Sciences</skos:altLabel>
	<skos:hiddenLabel xml:lang="en"></skos:hiddenLabel>
	<skos:definition xml:lang="en">The school offers a learning and research environment spanning social and cultural studies in Australia, Europe and Asia.</skos:definition>
	<dc:source rdf:datatype="http://www.w3.org/2001/XMLSchema#string">Australian Ocean Data Network Organisation Register</dc:source>
	<dc:publisher rdf:datatype="http://www.w3.org/2001/XMLSchema#string">eMarine Information Infrastructure (eMII)</dc:publisher>
	<skos:inScheme rdf:resource="http://vocab.aodn.org.au/def/organisation/1"/>
	<skos:broader rdf:resource="http://vocab.aodn.org.au/def/organisation/entity/235"/>
</rdf:Description>

<rdf:Description rdf:about="http://seadatanet.maris2.nl/v_edmo/print.asp?n_code=2372">
	<rdf:type rdf:resource="http://www.w3.org/2000/01/rdf-schema#Resource"/>
</rdf:Description>

<rdf:Description rdf:about="http://seadatanet.maris2.nl/v_edmo/print.asp?n_code=4309">
	<rdf:type rdf:resource="http://www.w3.org/2000/01/rdf-schema#Resource"/>
</rdf:Description>

<rdf:Description rdf:about="http://seadatanet.maris2.nl/v_edmo/print.asp?n_code=4310">
	<rdf:type rdf:resource="http://www.w3.org/2000/01/rdf-schema#Resource"/>
</rdf:Description>

<rdf:Description rdf:about="http://seadatanet.maris2.nl/v_edmo/print.asp?n_code=4311">
	<rdf:type rdf:resource="http://www.w3.org/2000/01/rdf-schema#Resource"/>
</rdf:Description>

<rdf:Description rdf:about="http://seadatanet.maris2.nl/v_edmo/print.asp?n_code=4312">
	<rdf:type rdf:resource="http://www.w3.org/2000/01/rdf-schema#Resource"/>
</rdf:Description>

<rdf:Description rdf:about="http://seadatanet.maris2.nl/v_edmo/print.asp?n_code=4313">
	<rdf:type rdf:resource="http://www.w3.org/2000/01/rdf-schema#Resource"/>
</rdf:Description>

<rdf:Description rdf:about="http://seadatanet.maris2.nl/v_edmo/print.asp?n_code=4314">
	<rdf:type rdf:resource="http://www.w3.org/2000/01/rdf-schema#Resource"/>
</rdf:Description>

<rdf:Description rdf:about="http://seadatanet.maris2.nl/v_edmo/print.asp?n_code=4315">
	<rdf:type rdf:resource="http://www.w3.org/2000/01/rdf-schema#Resource"/>
</rdf:Description>

<rdf:Description rdf:about="http://seadatanet.maris2.nl/v_edmo/print.asp?n_code=4316">
	<rdf:type rdf:resource="http://www.w3.org/2000/01/rdf-schema#Resource"/>
</rdf:Description>

<rdf:Description rdf:about="http://seadatanet.maris2.nl/v_edmo/print.asp?n_code=4324">
	<rdf:type rdf:resource="http://www.w3.org/2000/01/rdf-schema#Resource"/>
</rdf:Description>

<rdf:Description rdf:about="http://vocab.aodn.org.au/def/organisation/entity/253">
	<rdf:type rdf:resource="http://www.w3.org/2000/01/rdf-schema#Resource"/>
	<rdf:type rdf:resource="http://www.w3.org/2004/02/skos/core#Concept"/>
	<dcterms:creator rdf:datatype="http://www.w3.org/2001/XMLSchema#string">Natalia Atkins</dcterms:creator>
	<dcterms:created rdf:datatype="http://www.w3.org/2001/XMLSchema#dateTime">2015-07-13T10:38:15Z</dcterms:created>
	<skos:prefLabel xml:lang="en">School of Agricultural Science, University of Tasmania (UTAS)</skos:prefLabel>
	<skos:altLabel xml:lang="en">School of Agricultural Science</skos:altLabel>
	<skos:hiddenLabel xml:lang="en"></skos:hiddenLabel>
	<skos:definition xml:lang="en">This school became part of the School of Land and Food (SLAF), in 2014.</skos:definition>
	<dc:source rdf:datatype="http://www.w3.org/2001/XMLSchema#string">Australian Ocean Data Network Organisation Register</dc:source>
	<dc:publisher rdf:datatype="http://www.w3.org/2001/XMLSchema#string">eMarine Information Infrastructure (eMII)</dc:publisher>
	<skos:inScheme rdf:resource="http://vocab.aodn.org.au/def/organisation/1"/>
	<skos:broader rdf:resource="http://vocab.aodn.org.au/def/organisation/entity/252"/>
	<skos:scopeNote xml:lang="en">Organisation no longer exists</skos:scopeNote>
	<skos:scopeNote xml:lang="en">Organisation no longer exists. Replaced by http://vocab.aodn.org.au/def/organisation/entity/255</skos:scopeNote>
	<dcterms:isReplacedBy rdf:resource="http://vocab.aodn.org.au/def/organisation/entity/255"/>
	<dcterms:isReplacedBy xml:lang="en">School of Land and Food (SLAF), University of Tasmania (UTAS)</dcterms:isReplacedBy>
</rdf:Description>

<rdf:Description rdf:about="http://vocab.aodn.org.au/def/organisation/entity/254">
	<rdf:type rdf:resource="http://www.w3.org/2000/01/rdf-schema#Resource"/>
	<rdf:type rdf:resource="http://www.w3.org/2004/02/skos/core#Concept"/>
	<dcterms:creator rdf:datatype="http://www.w3.org/2001/XMLSchema#string">Natalia Atkins</dcterms:creator>
	<dcterms:created rdf:datatype="http://www.w3.org/2001/XMLSchema#dateTime">2015-07-13T10:38:15Z</dcterms:created>
	<skos:prefLabel xml:lang="en">School of Geography and Environmental Studies, University of Tasmania (UTAS)</skos:prefLabel>
	<skos:altLabel xml:lang="en">School of Geography and Environmental Studies</skos:altLabel>
	<skos:hiddenLabel xml:lang="en"></skos:hiddenLabel>
	<skos:definition xml:lang="en">This school became part of the School of Land and Food (SLAF), in 2014.</skos:definition>
	<dc:source rdf:datatype="http://www.w3.org/2001/XMLSchema#string">Australian Ocean Data Network Organisation Register</dc:source>
	<dc:publisher rdf:datatype="http://www.w3.org/2001/XMLSchema#string">eMarine Information Infrastructure (eMII)</dc:publisher>
	<skos:inScheme rdf:resource="http://vocab.aodn.org.au/def/organisation/1"/>
	<skos:broader rdf:resource="http://vocab.aodn.org.au/def/organisation/entity/252"/>
	<skos:scopeNote xml:lang="en">Organisation no longer exists</skos:scopeNote>
	<skos:scopeNote xml:lang="en">Organisation no longer exists. Replaced by http://vocab.aodn.org.au/def/organisation/entity/255</skos:scopeNote>
	<dcterms:isReplacedBy rdf:resource="http://vocab.aodn.org.au/def/organisation/entity/255"/>
	<dcterms:isReplacedBy xml:lang="en">School of Land and Food (SLAF), University of Tasmania (UTAS)</dcterms:isReplacedBy>
</rdf:Description>

<rdf:Description rdf:about="http://vocab.aodn.org.au/def/organisation/entity/255">
	<rdf:type rdf:resource="http://www.w3.org/2000/01/rdf-schema#Resource"/>
	<rdf:type rdf:resource="http://www.w3.org/2004/02/skos/core#Concept"/>
	<dcterms:creator rdf:datatype="http://www.w3.org/2001/XMLSchema#string">Natalia Atkins</dcterms:creator>
	<dcterms:created rdf:datatype="http://www.w3.org/2001/XMLSchema#dateTime">2015-07-13T10:38:15Z</dcterms:created>
	<skos:prefLabel xml:lang="en">School of Land and Food (SLAF), University of Tasmania (UTAS)</skos:prefLabel>
	<skos:altLabel xml:lang="en">School of Land and Food (SLAF)</skos:altLabel>
	<skos:hiddenLabel xml:lang="en">SLAF</skos:hiddenLabel>
	<skos:definition xml:lang="en">The School of Land and Food was formed in 2014. It brings together the disciplines of geography, spatial science, agricultural science and food systems.</skos:definition>
	<dc:source rdf:datatype="http://www.w3.org/2001/XMLSchema#string">Australian Ocean Data Network Organisation Register</dc:source>
	<dc:publisher rdf:datatype="http://www.w3.org/2001/XMLSchema#string">eMarine Information Infrastructure (eMII)</dc:publisher>
	<skos:exactMatch rdf:resource="http://seadatanet.maris2.nl/v_edmo/print.asp?n_code=4325"/>
	<skos:inScheme rdf:resource="http://vocab.aodn.org.au/def/organisation/1"/>
	<skos:broader rdf:resource="http://vocab.aodn.org.au/def/organisation/entity/252"/>
	<skos:scopeNote xml:lang="en">Replaces http://vocab.aodn.org.au/def/organisation/entity/253 and http://vocab.aodn.org.au/def/organisation/entity/254</skos:scopeNote>
	<dcterms:replaces rdf:resource="http://vocab.aodn.org.au/def/organisation/entity/253"/>
	<dcterms:replaces rdf:resource="http://vocab.aodn.org.au/def/organisation/entity/254"/>
	<dcterms:replaces xml:lang="en">School of Agricultural Science, University of Tasmania (UTAS)</dcterms:replaces>
	<dcterms:replaces xml:lang="en">School of Geography and Environmental Studies, University of Tasmania (UTAS)</dcterms:replaces>
</rdf:Description>

<rdf:Description rdf:about="http://vocab.aodn.org.au/def/organisation/entity/256">
	<rdf:type rdf:resource="http://www.w3.org/2000/01/rdf-schema#Resource"/>
	<rdf:type rdf:resource="http://www.w3.org/2004/02/skos/core#Concept"/>
	<dcterms:creator rdf:datatype="http://www.w3.org/2001/XMLSchema#string">Natalia Atkins</dcterms:creator>
	<dcterms:created rdf:datatype="http://www.w3.org/2001/XMLSchema#dateTime">2015-07-13T10:38:15Z</dcterms:created>
	<skos:prefLabel xml:lang="en">School of Zoology, University of Tasmania (UTAS)</skos:prefLabel>
	<skos:altLabel xml:lang="en">School of Zoology</skos:altLabel>
	<skos:hiddenLabel xml:lang="en"></skos:hiddenLabel>
	<skos:definition xml:lang="en">This school became part of the School of Biological Sciences (SBS), in 2014.</skos:definition>
	<dc:source rdf:datatype="http://www.w3.org/2001/XMLSchema#string">Australian Ocean Data Network Organisation Register</dc:source>
	<dc:publisher rdf:datatype="http://www.w3.org/2001/XMLSchema#string">eMarine Information Infrastructure (eMII)</dc:publisher>
	<skos:inScheme rdf:resource="http://vocab.aodn.org.au/def/organisation/1"/>
	<skos:broader rdf:resource="http://vocab.aodn.org.au/def/organisation/entity/252"/>
	<skos:scopeNote xml:lang="en">Organisation no longer exists</skos:scopeNote>
	<skos:scopeNote xml:lang="en">Organisation no longer exists. Replaced by http://vocab.aodn.org.au/def/organisation/entity/258</skos:scopeNote>
	<dcterms:isReplacedBy rdf:resource="http://vocab.aodn.org.au/def/organisation/entity/258"/>
	<dcterms:isReplacedBy xml:lang="en">School of Biological Sciences (SBS), University of Tasmania (UTAS)</dcterms:isReplacedBy>
</rdf:Description>

<rdf:Description rdf:about="http://vocab.aodn.org.au/def/organisation/entity/257">
	<rdf:type rdf:resource="http://www.w3.org/2000/01/rdf-schema#Resource"/>
	<rdf:type rdf:resource="http://www.w3.org/2004/02/skos/core#Concept"/>
	<dcterms:creator rdf:datatype="http://www.w3.org/2001/XMLSchema#string">Natalia Atkins</dcterms:creator>
	<dcterms:created rdf:datatype="http://www.w3.org/2001/XMLSchema#dateTime">2015-07-13T10:38:15Z</dcterms:created>
	<skos:prefLabel xml:lang="en">School of Plant Science, University of Tasmania (UTAS)</skos:prefLabel>
	<skos:altLabel xml:lang="en">School of Plant Science</skos:altLabel>
	<skos:hiddenLabel xml:lang="en"></skos:hiddenLabel>
	<skos:definition xml:lang="en">This school became part of the School of Biological Sciences (SBS), in 2014.</skos:definition>
	<dc:source rdf:datatype="http://www.w3.org/2001/XMLSchema#string">Australian Ocean Data Network Organisation Register</dc:source>
	<dc:publisher rdf:datatype="http://www.w3.org/2001/XMLSchema#string">eMarine Information Infrastructure (eMII)</dc:publisher>
	<skos:inScheme rdf:resource="http://vocab.aodn.org.au/def/organisation/1"/>
	<skos:broader rdf:resource="http://vocab.aodn.org.au/def/organisation/entity/252"/>
	<skos:scopeNote xml:lang="en">Organisation no longer exists</skos:scopeNote>
	<skos:scopeNote xml:lang="en">Organisation no longer exists. Replaced by http://vocab.aodn.org.au/def/organisation/entity/258</skos:scopeNote>
	<dcterms:isReplacedBy rdf:resource="http://vocab.aodn.org.au/def/organisation/entity/258"/>
	<dcterms:isReplacedBy xml:lang="en">School of Biological Sciences (SBS), University of Tasmania (UTAS)</dcterms:isReplacedBy>
</rdf:Description>

<rdf:Description rdf:about="http://vocab.aodn.org.au/def/organisation/entity/258">
	<rdf:type rdf:resource="http://www.w3.org/2000/01/rdf-schema#Resource"/>
	<rdf:type rdf:resource="http://www.w3.org/2004/02/skos/core#Concept"/>
	<dcterms:creator rdf:datatype="http://www.w3.org/2001/XMLSchema#string">Natalia Atkins</dcterms:creator>
	<dcterms:created rdf:datatype="http://www.w3.org/2001/XMLSchema#dateTime">2015-07-13T10:38:15Z</dcterms:created>
	<skos:prefLabel xml:lang="en">School of Biological Sciences (SBS), University of Tasmania (UTAS)</skos:prefLabel>
	<skos:altLabel xml:lang="en">School of Biological Sciences (SBS)</skos:altLabel>
	<skos:hiddenLabel xml:lang="en">SBS</skos:hiddenLabel>
	<skos:definition xml:lang="en">The school of Biological Sciences was formed in 2014, bringing together the former schools of Zoology and Plant Science.</skos:definition>
	<dc:source rdf:datatype="http://www.w3.org/2001/XMLSchema#string">Australian Ocean Data Network Organisation Register</dc:source>
	<dc:publisher rdf:datatype="http://www.w3.org/2001/XMLSchema#string">eMarine Information Infrastructure (eMII)</dc:publisher>
	<skos:exactMatch rdf:resource="http://seadatanet.maris2.nl/v_edmo/print.asp?n_code=4326"/>
	<skos:inScheme rdf:resource="http://vocab.aodn.org.au/def/organisation/1"/>
	<skos:broader rdf:resource="http://vocab.aodn.org.au/def/organisation/entity/252"/>
	<skos:scopeNote xml:lang="en">Replaces http://vocab.aodn.org.au/def/organisation/entity/256 and http://vocab.aodn.org.au/def/organisation/entity/257</skos:scopeNote>
	<dcterms:replaces rdf:resource="http://vocab.aodn.org.au/def/organisation/entity/256"/>
	<dcterms:replaces rdf:resource="http://vocab.aodn.org.au/def/organisation/entity/257"/>
	<dcterms:replaces xml:lang="en">School of Zoology, University of Tasmania (UTAS)</dcterms:replaces>
	<dcterms:replaces xml:lang="en">School of Plant Science, University of Tasmania (UTAS)</dcterms:replaces>
</rdf:Description>

<rdf:Description rdf:about="http://vocab.aodn.org.au/def/organisation/entity/259">
	<rdf:type rdf:resource="http://www.w3.org/2000/01/rdf-schema#Resource"/>
	<rdf:type rdf:resource="http://www.w3.org/2004/02/skos/core#Concept"/>
	<dcterms:creator rdf:datatype="http://www.w3.org/2001/XMLSchema#string">Natalia Atkins</dcterms:creator>
	<dcterms:created rdf:datatype="http://www.w3.org/2001/XMLSchema#dateTime">2015-07-13T10:38:15Z</dcterms:created>
	<skos:prefLabel xml:lang="en">Tasmanian Aquaculture and Fisheries Institute (TAFI)</skos:prefLabel>
	<skos:altLabel xml:lang="en"></skos:altLabel>
	<skos:hiddenLabel xml:lang="en">TAFI</skos:hiddenLabel>
	<skos:definition xml:lang="en">The institute was established, in 1998,  as a centre of excellence in applied marine research to support the development and sustainable management of Tasmania's living marine resources. It was a joint venture between the University of Tasmania and the Tasmanian Government, utilising the expertise and facilities of the Department of Primary Industries and Water. It became part of the Institute for Marine and Antarctic Studies in 2010.</skos:definition>
	<dc:source rdf:datatype="http://www.w3.org/2001/XMLSchema#string">Australian Ocean Data Network Organisation Register</dc:source>
	<dc:publisher rdf:datatype="http://www.w3.org/2001/XMLSchema#string">eMarine Information Infrastructure (eMII)</dc:publisher>
	<skos:inScheme rdf:resource="http://vocab.aodn.org.au/def/organisation/1"/>
	<skos:broader rdf:resource="http://vocab.aodn.org.au/def/organisation/entity/252"/>
	<skos:scopeNote xml:lang="en">Organisation no longer exists</skos:scopeNote>
	<skos:scopeNote xml:lang="en">Organisation no longer exists. Replaced by http://vocab.aodn.org.au/def/organisation/entity/260</skos:scopeNote>
	<dcterms:isReplacedBy rdf:resource="http://vocab.aodn.org.au/def/organisation/entity/260"/>
	<dcterms:isReplacedBy xml:lang="en">Institute for Marine and Antarctic Studies (IMAS), University of Tasmania (UTAS)</dcterms:isReplacedBy>
</rdf:Description>

<rdf:Description rdf:about="http://vocab.aodn.org.au/def/organisation/entity/260">
	<rdf:type rdf:resource="http://www.w3.org/2000/01/rdf-schema#Resource"/>
	<rdf:type rdf:resource="http://www.w3.org/2004/02/skos/core#Concept"/>
	<dcterms:creator rdf:datatype="http://www.w3.org/2001/XMLSchema#string">Natalia Atkins</dcterms:creator>
	<dcterms:created rdf:datatype="http://www.w3.org/2001/XMLSchema#dateTime">2015-07-13T10:38:15Z</dcterms:created>
	<skos:prefLabel xml:lang="en">Institute for Marine and Antarctic Studies (IMAS), University of Tasmania (UTAS)</skos:prefLabel>
	<skos:altLabel xml:lang="en">Institute for Marine and Antarctic Studies (IMAS)</skos:altLabel>
	<skos:hiddenLabel xml:lang="en">IMAS</skos:hiddenLabel>
	<skos:definition xml:lang="en">The Institute for Marine and Antarctic Studies (IMAS) was established in 2009. It was created by the University of Tasmania (UTAS) Council to bring together the many strands of marine and Antarctic research currently being pursued in and around Hobart, to encourage the development of strengthened research links and exploit new research opportunities. IMAS brought together staff and students from the Tasmanian Aquaculture and Fisheries Institute (TAFI) , the Institute for Antarctic and Southern Ocean Studies (IASOS), and marine and Antarctic scientists from the academic Schools of UTAS.</skos:definition>
	<dc:source rdf:datatype="http://www.w3.org/2001/XMLSchema#string">Australian Ocean Data Network Organisation Register</dc:source>
	<dc:publisher rdf:datatype="http://www.w3.org/2001/XMLSchema#string">eMarine Information Infrastructure (eMII)</dc:publisher>
	<skos:exactMatch rdf:resource="http://seadatanet.maris2.nl/v_edmo/print.asp?n_code=4327"/>
	<skos:inScheme rdf:resource="http://vocab.aodn.org.au/def/organisation/1"/>
	<skos:broader rdf:resource="http://vocab.aodn.org.au/def/organisation/entity/252"/>
	<skos:scopeNote xml:lang="en">Replaces http://vocab.aodn.org.au/def/organisation/entity/259 and http://vocab.aodn.org.au/def/organisation/entity/261</skos:scopeNote>
	<dcterms:replaces rdf:resource="http://vocab.aodn.org.au/def/organisation/entity/259"/>
	<dcterms:replaces rdf:resource="http://vocab.aodn.org.au/def/organisation/entity/261"/>
	<dcterms:replaces xml:lang="en">Tasmanian Aquaculture and Fisheries Institute (TAFI)</dcterms:replaces>
	<dcterms:replaces xml:lang="en">School of Aquaculture, University of Tasmania (UTAS)</dcterms:replaces>
</rdf:Description>

<rdf:Description rdf:about="http://vocab.aodn.org.au/def/organisation/entity/261">
	<rdf:type rdf:resource="http://www.w3.org/2000/01/rdf-schema#Resource"/>
	<rdf:type rdf:resource="http://www.w3.org/2004/02/skos/core#Concept"/>
	<dcterms:creator rdf:datatype="http://www.w3.org/2001/XMLSchema#string">Natalia Atkins</dcterms:creator>
	<dcterms:created rdf:datatype="http://www.w3.org/2001/XMLSchema#dateTime">2015-07-13T10:38:15Z</dcterms:created>
	<skos:prefLabel xml:lang="en">School of Aquaculture, University of Tasmania (UTAS)</skos:prefLabel>
	<skos:altLabel xml:lang="en">School of Aquaculture</skos:altLabel>
	<skos:hiddenLabel xml:lang="en"></skos:hiddenLabel>
	<skos:definition xml:lang="en">The School of Aquaculture was conducted within the Australian Maritime College at the University of Tasmania, and in 2014 was incorporated into Institute for Marine and Antarctic Studies (IMAS) Launceston.</skos:definition>
	<dc:source rdf:datatype="http://www.w3.org/2001/XMLSchema#string">Australian Ocean Data Network Organisation Register</dc:source>
	<dc:publisher rdf:datatype="http://www.w3.org/2001/XMLSchema#string">eMarine Information Infrastructure (eMII)</dc:publisher>
	<skos:inScheme rdf:resource="http://vocab.aodn.org.au/def/organisation/1"/>
	<skos:broader rdf:resource="http://vocab.aodn.org.au/def/organisation/entity/252"/>
	<skos:scopeNote xml:lang="en">Organisation no longer exists</skos:scopeNote>
	<skos:scopeNote xml:lang="en">Organisation no longer exists. Replaced by http://vocab.aodn.org.au/def/organisation/entity/260</skos:scopeNote>
	<dcterms:isReplacedBy rdf:resource="http://vocab.aodn.org.au/def/organisation/entity/260"/>
	<dcterms:isReplacedBy xml:lang="en">Institute for Marine and Antarctic Studies (IMAS), University of Tasmania (UTAS)</dcterms:isReplacedBy>
</rdf:Description>

<rdf:Description rdf:about="http://vocab.aodn.org.au/def/organisation/entity/29">
	<rdf:type rdf:resource="http://www.w3.org/2000/01/rdf-schema#Resource"/>
	<rdf:type rdf:resource="http://www.w3.org/2004/02/skos/core#Concept"/>
	<dcterms:creator rdf:datatype="http://www.w3.org/2001/XMLSchema#string">Natalia Atkins</dcterms:creator>
	<dcterms:created rdf:datatype="http://www.w3.org/2001/XMLSchema#dateTime">2015-06-24T10:38:15Z</dcterms:created>
	<skos:prefLabel xml:lang="en">Antarctic Climate and Ecosystems Cooperative Research Centre (ACE CRC)</skos:prefLabel>
	<skos:altLabel xml:lang="en"></skos:altLabel>
	<skos:hiddenLabel xml:lang="en">ACE CRC</skos:hiddenLabel>
	<skos:definition xml:lang="en">The Antarctic Climate and Ecosystems Cooperative Research Centre (ACE CRC) provides a focus for Australia's national effort to understand the variability of Antarctica and the Southern Ocean and their role in Australia's future. The ACE CRC is a partnership dedicated to sustainable management of Antarctic marine ecosystem resources and the study of atmospheric and oceanic processes of the Southern Ocean and their role in global and regional climate change. ACE CRC's Mission Statement: * Extend the existing research base in the Antarctic physical environment into the science of Southern Ocean and Antarctic ecosystem dynamics * Encourage sustainable management of Southern Ocean and Antarctic marine living resources * Connect physical variability and change in the Southern Ocean and Antarctica with their climate impacts on Australia and the surrounding region to permit efficient response and adaptation * Enhance Australian leadership in Antarctic affairs and advance Australia's objectives for its Antarctic Territory and Exclusive Economic Zones * Expand engagement of the international science community in Southern Ocean and Antarctic research relevant to Australia's interests to deliver the knowledge and information needed by our diverse research users * Encourage the realisation of policy and commercial opportunities in Antarctica and the Southern Ocean * Produce expertly-trained scientists with international experience, skills in research, its broad application and its role in enterprise and policy.</skos:definition>
	<dc:source rdf:datatype="http://www.w3.org/2001/XMLSchema#string">Australian Ocean Data Network Organisation Register</dc:source>
	<dc:publisher rdf:datatype="http://www.w3.org/2001/XMLSchema#string">eMarine Information Infrastructure (eMMI)</dc:publisher>
	<skos:exactMatch rdf:resource="http://seadatanet.maris2.nl/v_edmo/print.asp?n_code=1490"/>
	<skos:inScheme rdf:resource="http://vocab.aodn.org.au/def/organisation/1"/>
	<skos:broader rdf:resource="http://vocab.aodn.org.au/def/organisation/entity/252"/>
</rdf:Description>

<rdf:Description rdf:about="http://vocab.aodn.org.au/def/organisation/entity/405">
	<rdf:type rdf:resource="http://www.w3.org/2000/01/rdf-schema#Resource"/>
	<rdf:type rdf:resource="http://www.w3.org/2004/02/skos/core#Concept"/>
	<dcterms:creator rdf:datatype="http://www.w3.org/2001/XMLSchema#string">Natalia Atkins</dcterms:creator>
	<dcterms:created rdf:datatype="http://www.w3.org/2001/XMLSchema#dateTime">2015-10-15T10:38:15Z</dcterms:created>
	<skos:prefLabel xml:lang="en">Tasmanian Partnership for Advanced Computing (TPAC)</skos:prefLabel>
	<skos:altLabel xml:lang="en"></skos:altLabel>
	<skos:hiddenLabel xml:lang="en">TPAC</skos:hiddenLabel>
	<skos:definition xml:lang="en">TPAC is located at the University of Tasmania in Hobart, and its partners are the University of Tasmania, CSIRO Oceans and Atmosphere, the Australian Government Antarctic Division, Antarctic Climate and Ecosystems Cooperative Research Centre (ACE CRC), Bureau of Meteorology Research Centre, and the Australian Maritime College.TPAC provides expertise and high performance computing facilities to the Australian and International research community.</skos:definition>
	<dc:source rdf:datatype="http://www.w3.org/2001/XMLSchema#string">Australian Ocean Data Network Organisation Register</dc:source>
	<dc:publisher rdf:datatype="http://www.w3.org/2001/XMLSchema#string">eMarine Information Infrastructure (eMMI)</dc:publisher>
	<skos:exactMatch rdf:resource="http://seadatanet.maris2.nl/v_edmo/print.asp?n_code=4390"/>
	<skos:inScheme rdf:resource="http://vocab.aodn.org.au/def/organisation/1"/>
	<skos:broader rdf:resource="http://vocab.aodn.org.au/def/organisation/entity/252"/>
</rdf:Description>

<rdf:Description rdf:about="http://seadatanet.maris2.nl/v_edmo/print.asp?n_code=4325">
	<rdf:type rdf:resource="http://www.w3.org/2000/01/rdf-schema#Resource"/>
</rdf:Description>

<rdf:Description rdf:about="http://seadatanet.maris2.nl/v_edmo/print.asp?n_code=4326">
	<rdf:type rdf:resource="http://www.w3.org/2000/01/rdf-schema#Resource"/>
</rdf:Description>

<rdf:Description rdf:about="http://seadatanet.maris2.nl/v_edmo/print.asp?n_code=4327">
	<rdf:type rdf:resource="http://www.w3.org/2000/01/rdf-schema#Resource"/>
</rdf:Description>

<rdf:Description rdf:about="http://seadatanet.maris2.nl/v_edmo/print.asp?n_code=4249">
	<rdf:type rdf:resource="http://www.w3.org/2000/01/rdf-schema#Resource"/>
</rdf:Description>

<rdf:Description rdf:about="http://seadatanet.maris2.nl/v_edmo/print.asp?n_code=4250">
	<rdf:type rdf:resource="http://www.w3.org/2000/01/rdf-schema#Resource"/>
</rdf:Description>

<rdf:Description rdf:about="http://vocab.aodn.org.au/def/organisation/entity/264">
	<rdf:type rdf:resource="http://www.w3.org/2000/01/rdf-schema#Resource"/>
	<rdf:type rdf:resource="http://www.w3.org/2004/02/skos/core#Concept"/>
	<dcterms:creator rdf:datatype="http://www.w3.org/2001/XMLSchema#string">Natalia Atkins</dcterms:creator>
	<dcterms:created rdf:datatype="http://www.w3.org/2001/XMLSchema#dateTime">2015-07-13T10:38:15Z</dcterms:created>
	<skos:prefLabel xml:lang="en">School for Environmental Research, Institute of Advanced Studies, Charles Darwin University (CDU)</skos:prefLabel>
	<skos:altLabel xml:lang="en">School for Environmental Research</skos:altLabel>
	<skos:hiddenLabel xml:lang="en"></skos:hiddenLabel>
	<skos:definition xml:lang="en">This school became part of the Research Institute for the Environment and Livelihoods (RIEL).</skos:definition>
	<dc:source rdf:datatype="http://www.w3.org/2001/XMLSchema#string">Australian Ocean Data Network Organisation Register</dc:source>
	<dc:publisher rdf:datatype="http://www.w3.org/2001/XMLSchema#string">eMarine Information Infrastructure (eMII)</dc:publisher>
	<skos:inScheme rdf:resource="http://vocab.aodn.org.au/def/organisation/1"/>
	<skos:broader rdf:resource="http://vocab.aodn.org.au/def/organisation/entity/263"/>
	<skos:scopeNote xml:lang="en">Organisation no longer exists</skos:scopeNote>
	<skos:scopeNote xml:lang="en">Organisation no longer exists. Replaced by http://vocab.aodn.org.au/def/organisation/entity/265</skos:scopeNote>
	<dcterms:isReplacedBy rdf:resource="http://vocab.aodn.org.au/def/organisation/entity/265"/>
	<dcterms:isReplacedBy xml:lang="en">Research Institute for the Environment and Livelihoods (RIEL), Charles Darwin University (CDU)</dcterms:isReplacedBy>
</rdf:Description>

<rdf:Description rdf:about="http://vocab.aodn.org.au/def/organisation/entity/265">
	<rdf:type rdf:resource="http://www.w3.org/2000/01/rdf-schema#Resource"/>
	<rdf:type rdf:resource="http://www.w3.org/2004/02/skos/core#Concept"/>
	<dcterms:creator rdf:datatype="http://www.w3.org/2001/XMLSchema#string">Natalia Atkins</dcterms:creator>
	<dcterms:created rdf:datatype="http://www.w3.org/2001/XMLSchema#dateTime">2015-07-13T10:38:15Z</dcterms:created>
	<skos:prefLabel xml:lang="en">Research Institute for the Environment and Livelihoods (RIEL), Charles Darwin University (CDU)</skos:prefLabel>
	<skos:altLabel xml:lang="en">Research Institute for the Environment and Livelihoods (RIEL)</skos:altLabel>
	<skos:hiddenLabel xml:lang="en"></skos:hiddenLabel>
	<skos:definition xml:lang="en">The Research Institute for the Environment and Livelihoods (RIEL) is a Tier 1 institute that consolidates CDU's environmental and natural resource management research.</skos:definition>
	<dc:source rdf:datatype="http://www.w3.org/2001/XMLSchema#string">Australian Ocean Data Network Organisation Register</dc:source>
	<dc:publisher rdf:datatype="http://www.w3.org/2001/XMLSchema#string">eMarine Information Infrastructure (eMII)</dc:publisher>
	<skos:exactMatch rdf:resource="http://seadatanet.maris2.nl/v_edmo/print.asp?n_code=4251"/>
	<skos:inScheme rdf:resource="http://vocab.aodn.org.au/def/organisation/1"/>
	<skos:broader rdf:resource="http://vocab.aodn.org.au/def/organisation/entity/263"/>
	<skos:scopeNote xml:lang="en">Replaces http://vocab.aodn.org.au/def/organisation/entity/264</skos:scopeNote>
	<dcterms:replaces rdf:resource="http://vocab.aodn.org.au/def/organisation/entity/264"/>
	<dcterms:replaces xml:lang="en">School for Environmental Research, Institute of Advanced Studies, Charles Darwin University (CDU)</dcterms:replaces>
</rdf:Description>

<rdf:Description rdf:about="http://vocab.aodn.org.au/def/organisation/entity/266">
	<rdf:type rdf:resource="http://www.w3.org/2000/01/rdf-schema#Resource"/>
	<rdf:type rdf:resource="http://www.w3.org/2004/02/skos/core#Concept"/>
	<dcterms:creator rdf:datatype="http://www.w3.org/2001/XMLSchema#string">Natalia Atkins</dcterms:creator>
	<dcterms:created rdf:datatype="http://www.w3.org/2001/XMLSchema#dateTime">2015-07-13T10:38:15Z</dcterms:created>
	<skos:prefLabel xml:lang="en">School of Environmental and Life Sciences (SELS), Charles Darwin University (CDU)</skos:prefLabel>
	<skos:altLabel xml:lang="en">School of Environmental and Life Sciences (SELS)</skos:altLabel>
	<skos:hiddenLabel xml:lang="en">SELS</skos:hiddenLabel>
	<skos:definition xml:lang="en">This school became part of the School of Environment.</skos:definition>
	<dc:source rdf:datatype="http://www.w3.org/2001/XMLSchema#string">Australian Ocean Data Network Organisation Register</dc:source>
	<dc:publisher rdf:datatype="http://www.w3.org/2001/XMLSchema#string">eMarine Information Infrastructure (eMII)</dc:publisher>
	<skos:inScheme rdf:resource="http://vocab.aodn.org.au/def/organisation/1"/>
	<skos:broader rdf:resource="http://vocab.aodn.org.au/def/organisation/entity/263"/>
	<skos:scopeNote xml:lang="en">Organisation no longer exists</skos:scopeNote>
	<skos:scopeNote xml:lang="en">Organisation no longer exists. Replaced by http://vocab.aodn.org.au/def/organisation/entity/267</skos:scopeNote>
	<dcterms:isReplacedBy rdf:resource="http://vocab.aodn.org.au/def/organisation/entity/267"/>
	<dcterms:isReplacedBy xml:lang="en">School of Environment, Charles Darwin University (CDU)</dcterms:isReplacedBy>
</rdf:Description>

<rdf:Description rdf:about="http://vocab.aodn.org.au/def/organisation/entity/267">
	<rdf:type rdf:resource="http://www.w3.org/2000/01/rdf-schema#Resource"/>
	<rdf:type rdf:resource="http://www.w3.org/2004/02/skos/core#Concept"/>
	<dcterms:creator rdf:datatype="http://www.w3.org/2001/XMLSchema#string">Natalia Atkins</dcterms:creator>
	<dcterms:created rdf:datatype="http://www.w3.org/2001/XMLSchema#dateTime">2015-07-13T10:38:15Z</dcterms:created>
	<skos:prefLabel xml:lang="en">School of Environment, Charles Darwin University (CDU)</skos:prefLabel>
	<skos:altLabel xml:lang="en">School of Environment</skos:altLabel>
	<skos:hiddenLabel xml:lang="en"></skos:hiddenLabel>
	<skos:definition xml:lang="en">The School of Environment is responsible for teaching and research in the fields of: biological science, environmental science, environmental policy and management, chemistry and biochemistry, ecology, spatial science and remote sensing, marine and freshwater ecology, wildlife conservation, management of natural resources.</skos:definition>
	<dc:source rdf:datatype="http://www.w3.org/2001/XMLSchema#string">Australian Ocean Data Network Organisation Register</dc:source>
	<dc:publisher rdf:datatype="http://www.w3.org/2001/XMLSchema#string">eMarine Information Infrastructure (eMII)</dc:publisher>
	<skos:exactMatch rdf:resource="http://seadatanet.maris2.nl/v_edmo/print.asp?n_code=4252"/>
	<skos:inScheme rdf:resource="http://vocab.aodn.org.au/def/organisation/1"/>
	<skos:broader rdf:resource="http://vocab.aodn.org.au/def/organisation/entity/263"/>
	<skos:scopeNote xml:lang="en">Replaces http://vocab.aodn.org.au/def/organisation/entity/266</skos:scopeNote>
	<dcterms:replaces rdf:resource="http://vocab.aodn.org.au/def/organisation/entity/266"/>
	<dcterms:replaces xml:lang="en">School of Environmental and Life Sciences (SELS), Charles Darwin University (CDU)</dcterms:replaces>
</rdf:Description>

<rdf:Description rdf:about="http://seadatanet.maris2.nl/v_edmo/print.asp?n_code=4251">
	<rdf:type rdf:resource="http://www.w3.org/2000/01/rdf-schema#Resource"/>
</rdf:Description>

<rdf:Description rdf:about="http://seadatanet.maris2.nl/v_edmo/print.asp?n_code=4252">
	<rdf:type rdf:resource="http://www.w3.org/2000/01/rdf-schema#Resource"/>
</rdf:Description>

<rdf:Description rdf:about="http://vocab.aodn.org.au/def/organisation_classes/category/1">
	<rdf:type rdf:resource="http://www.w3.org/2000/01/rdf-schema#Resource"/>
</rdf:Description>

<rdf:Description rdf:about="http://seadatanet.maris2.nl/v_edmo/print.asp?n_code=3932">
	<rdf:type rdf:resource="http://www.w3.org/2000/01/rdf-schema#Resource"/>
</rdf:Description>

<rdf:Description rdf:about="http://vocab.aodn.org.au/def/organisation/entity/2">
	<rdf:type rdf:resource="http://www.w3.org/2000/01/rdf-schema#Resource"/>
	<rdf:type rdf:resource="http://www.w3.org/2004/02/skos/core#Concept"/>
	<dcterms:modified rdf:datatype="http://www.w3.org/2001/XMLSchema#dateTime">2015-10-30T06:15:48Z</dcterms:modified>
	<dcterms:creator rdf:datatype="http://www.w3.org/2001/XMLSchema#string">Natalia Atkins</dcterms:creator>
	<dcterms:created rdf:datatype="http://www.w3.org/2001/XMLSchema#dateTime">2015-04-27T10:38:15Z</dcterms:created>
	<dcterms:contributor rdf:datatype="http://www.w3.org/2001/XMLSchema#string">eMII_Atkins.Natalia</dcterms:contributor>
	<skos:prefLabel xml:lang="en">Defence Science and Technology Organisation (DSTO), Department of Defence (DoD), Australian Government</skos:prefLabel>
	<skos:altLabel xml:lang="en">Defence Science and Technology Organisation (DSTO)</skos:altLabel>
	<skos:hiddenLabel xml:lang="en">DSTO</skos:hiddenLabel>
	<skos:definition xml:lang="en">Defence Science and Technology Organisation (DSTO) is the Australian government's lead agency responsible for applying science and technology to safeguard Australia and its national interests. This organisation has changed its name to the Defence Science and Technology Group (DST Group) in 2015.</skos:definition>
	<dc:source rdf:datatype="http://www.w3.org/2001/XMLSchema#string">Australian Ocean Data Network Organisation Register</dc:source>
	<dc:publisher rdf:datatype="http://www.w3.org/2001/XMLSchema#string">eMarine Information Infrastructure (eMII)</dc:publisher>
	<skos:exactMatch rdf:resource="http://seadatanet.maris2.nl/v_edmo/print.asp?n_code=3933"/>
	<skos:narrower rdf:resource="http://vocab.aodn.org.au/def/organisation/entity/3"/>
	<skos:narrower rdf:resource="http://vocab.aodn.org.au/def/organisation/entity/169"/>
	<skos:inScheme rdf:resource="http://vocab.aodn.org.au/def/organisation/1"/>
	<skos:broader rdf:resource="http://vocab.aodn.org.au/def/organisation/entity/1"/>
	<skos:scopeNote xml:lang="en">Organisation no longer exists</skos:scopeNote>
	<skos:scopeNote xml:lang="en">Organisation no longer exists. Replaced by http://vocab.aodn.org.au/def/organisation/entity/406</skos:scopeNote>
	<dcterms:isReplacedBy xml:lang="en">http://vocab.aodn.org.au/def/organisation/entity/406</dcterms:isReplacedBy>
	<dcterms:isReplacedBy xml:lang="en">Defence Science and Technology Group (DST Group), Department of Defence (DoD), Australian Government</dcterms:isReplacedBy>
</rdf:Description>

<rdf:Description rdf:about="http://vocab.aodn.org.au/def/organisation/entity/4">
	<rdf:type rdf:resource="http://www.w3.org/2000/01/rdf-schema#Resource"/>
	<rdf:type rdf:resource="http://www.w3.org/2004/02/skos/core#Concept"/>
	<dcterms:creator rdf:datatype="http://www.w3.org/2001/XMLSchema#string">Natalia Atkins</dcterms:creator>
	<dcterms:created rdf:datatype="http://www.w3.org/2001/XMLSchema#dateTime">2015-04-27T10:38:15Z</dcterms:created>
	<skos:prefLabel xml:lang="en">Australian Defence Force Academy (ADFA), Department of Defence (DoD), Australian Government</skos:prefLabel>
	<skos:altLabel xml:lang="en">Australian Defence Force Academy (ADFA)</skos:altLabel>
	<skos:hiddenLabel xml:lang="en">ADFA</skos:hiddenLabel>
	<skos:definition xml:lang="en">The Australian Defence Force Academy (ADFA) is a unique military institution which combines military education and training with academic study for an undergraduate degree through the University of New South Wales.</skos:definition>
	<dc:source rdf:datatype="http://www.w3.org/2001/XMLSchema#string">Australian Ocean Data Network Organisation Register</dc:source>
	<dc:publisher rdf:datatype="http://www.w3.org/2001/XMLSchema#string">eMarine Information Infrastructure (eMII)</dc:publisher>
	<skos:exactMatch rdf:resource="http://seadatanet.maris2.nl/v_edmo/print.asp?n_code=3942"/>
	<skos:inScheme rdf:resource="http://vocab.aodn.org.au/def/organisation/1"/>
	<skos:broader rdf:resource="http://vocab.aodn.org.au/def/organisation/entity/1"/>
</rdf:Description>

<rdf:Description rdf:about="http://vocab.aodn.org.au/def/organisation/entity/5">
	<rdf:type rdf:resource="http://www.w3.org/2000/01/rdf-schema#Resource"/>
	<rdf:type rdf:resource="http://www.w3.org/2004/02/skos/core#Concept"/>
	<dcterms:creator rdf:datatype="http://www.w3.org/2001/XMLSchema#string">Natalia Atkins</dcterms:creator>
	<dcterms:created rdf:datatype="http://www.w3.org/2001/XMLSchema#dateTime">2015-04-27T10:38:15Z</dcterms:created>
	<skos:prefLabel xml:lang="en">Royal Australian Navy (RAN), Department of Defence (DoD), Australian Government</skos:prefLabel>
	<skos:altLabel xml:lang="en">Royal Australian Navy (RAN)</skos:altLabel>
	<skos:hiddenLabel xml:lang="en">RAN</skos:hiddenLabel>
	<skos:definition xml:lang="en">The Royal Australian Navy (RAN) is the naval branch of the Australian Defence Force (ADF).</skos:definition>
	<dc:source rdf:datatype="http://www.w3.org/2001/XMLSchema#string">Australian Ocean Data Network Organisation Register</dc:source>
	<dc:publisher rdf:datatype="http://www.w3.org/2001/XMLSchema#string">eMarine Information Infrastructure (eMII)</dc:publisher>
	<skos:exactMatch rdf:resource="http://seadatanet.maris2.nl/v_edmo/print.asp?n_code=3936"/>
	<skos:narrower rdf:resource="http://vocab.aodn.org.au/def/organisation/entity/6"/>
	<skos:narrower rdf:resource="http://vocab.aodn.org.au/def/organisation/entity/7"/>
	<skos:inScheme rdf:resource="http://vocab.aodn.org.au/def/organisation/1"/>
	<skos:broader rdf:resource="http://vocab.aodn.org.au/def/organisation/entity/1"/>
</rdf:Description>

<rdf:Description rdf:about="http://vocab.aodn.org.au/def/organisation/entity/406">
	<rdf:type rdf:resource="http://www.w3.org/2000/01/rdf-schema#Resource"/>
	<rdf:type rdf:resource="http://www.w3.org/2004/02/skos/core#Concept"/>
	<dcterms:creator rdf:datatype="http://www.w3.org/2001/XMLSchema#string">Natalia Atkins</dcterms:creator>
	<dcterms:created rdf:datatype="http://www.w3.org/2001/XMLSchema#dateTime">2015-10-30T10:38:15Z</dcterms:created>
	<skos:prefLabel xml:lang="en">Defence Science and Technology Group (DST Group), Department of Defence (DoD), Australian Government</skos:prefLabel>
	<skos:altLabel xml:lang="en">Defence Science and Technology Group (DST Group)</skos:altLabel>
	<skos:hiddenLabel xml:lang="en">DST Group</skos:hiddenLabel>
	<skos:definition xml:lang="en">Defence Science and Technology Group (DST Group) is the Australian government's lead agency responsible for applying science and technology to safeguard Australia and its national interests.</skos:definition>
	<dc:source rdf:datatype="http://www.w3.org/2001/XMLSchema#string">Australian Ocean Data Network Organisation Register</dc:source>
	<dc:publisher rdf:datatype="http://www.w3.org/2001/XMLSchema#string">eMarine Information Infrastructure (eMII)</dc:publisher>
	<skos:exactMatch rdf:resource="http://seadatanet.maris2.nl/v_edmo/print.asp?n_code=3933"/>
	<skos:narrower rdf:resource="http://vocab.aodn.org.au/def/organisation/entity/407"/>
	<skos:inScheme rdf:resource="http://vocab.aodn.org.au/def/organisation/1"/>
	<skos:broader rdf:resource="http://vocab.aodn.org.au/def/organisation/entity/1"/>
	<skos:scopeNote xml:lang="en">Replaces http://vocab.aodn.org.au/def/organisation/entity/2</skos:scopeNote>
	<dcterms:replaces rdf:resource="http://vocab.aodn.org.au/def/organisation/entity/2"/>
	<dcterms:replaces xml:lang="en">Defence Science and Technology Organisation (DSTO), Department of Defence (DoD), Australian Government</dcterms:replaces>
</rdf:Description>

<rdf:Description rdf:about="http://seadatanet.maris2.nl/v_edmo/print.asp?n_code=3933">
	<rdf:type rdf:resource="http://www.w3.org/2000/01/rdf-schema#Resource"/>
</rdf:Description>

<rdf:Description rdf:about="http://vocab.aodn.org.au/def/organisation/entity/3">
	<rdf:type rdf:resource="http://www.w3.org/2000/01/rdf-schema#Resource"/>
	<rdf:type rdf:resource="http://www.w3.org/2004/02/skos/core#Concept"/>
	<dcterms:modified rdf:datatype="http://www.w3.org/2001/XMLSchema#dateTime">2015-10-30T06:17:06Z</dcterms:modified>
	<dcterms:creator rdf:datatype="http://www.w3.org/2001/XMLSchema#string">Natalia Atkins</dcterms:creator>
	<dcterms:created rdf:datatype="http://www.w3.org/2001/XMLSchema#dateTime">2015-04-27T10:38:15Z</dcterms:created>
	<dcterms:contributor rdf:datatype="http://www.w3.org/2001/XMLSchema#string">eMII_Atkins.Natalia</dcterms:contributor>
	<skos:prefLabel xml:lang="en">Maritime Division, Defence Science and Technology Organisation (DSTO), Department of Defence (DoD), Australian Government</skos:prefLabel>
	<skos:altLabel xml:lang="en">Maritime Division, Defence Science and Technology Organisation (DSTO)</skos:altLabel>
	<skos:definition xml:lang="en">Defence Science and Technology Organisation's (DSTO) Maritime Division provides technologies and scientific and technical expertise to deliver the capability edge to the war fighter and enhance the operational performance and survivability of defence platforms in the maritime domain. In 2015, the DSTO changed its name to the Defence Science and Technology Group (DST Group).</skos:definition>
	<dc:source rdf:datatype="http://www.w3.org/2001/XMLSchema#string">Australian Ocean Data Network Organisation Register</dc:source>
	<dc:publisher rdf:datatype="http://www.w3.org/2001/XMLSchema#string">eMarine Information Infrastructure (eMII)</dc:publisher>
	<skos:exactMatch rdf:resource="http://seadatanet.maris2.nl/v_edmo/print.asp?n_code=3934"/>
	<skos:inScheme rdf:resource="http://vocab.aodn.org.au/def/organisation/1"/>
	<skos:broader rdf:resource="http://vocab.aodn.org.au/def/organisation/entity/2"/>
	<skos:scopeNote xml:lang="en">Organisation no longer exists</skos:scopeNote>
	<skos:scopeNote xml:lang="en">Organisation no longer exists. Replaced by http://vocab.aodn.org.au/def/organisation/entity/407</skos:scopeNote>
	<dcterms:isReplacedBy xml:lang="en">http://vocab.aodn.org.au/def/organisation/entity/407</dcterms:isReplacedBy>
	<dcterms:isReplacedBy xml:lang="en">Maritime Division, Defence Science and Technology Group (DST Group), Department of Defence (DoD), Australian Government</dcterms:isReplacedBy>
</rdf:Description>

<rdf:Description rdf:about="http://vocab.aodn.org.au/def/organisation/entity/169">
	<rdf:type rdf:resource="http://www.w3.org/2000/01/rdf-schema#Resource"/>
	<rdf:type rdf:resource="http://www.w3.org/2004/02/skos/core#Concept"/>
	<dcterms:modified rdf:datatype="http://www.w3.org/2001/XMLSchema#dateTime">2015-06-24T00:04:53Z</dcterms:modified>
	<dcterms:creator rdf:datatype="http://www.w3.org/2001/XMLSchema#string">eMII_Finney.Kim</dcterms:creator>
	<dcterms:created rdf:datatype="http://www.w3.org/2001/XMLSchema#dateTime">2015-06-24T00:01:21Z</dcterms:created>
	<dcterms:contributor rdf:datatype="http://www.w3.org/2001/XMLSchema#string">eMII_Finney.Kim</dcterms:contributor>
	<skos:prefLabel xml:lang="en">Aeronautical Maritime Research Labs (AMRL), Defence Science and Technology Organisation (DSTO), Department of Defence (DoD), Australian Government</skos:prefLabel>
	<skos:altLabel xml:lang="en">Aeronautical Maritime Research Labs (AMRL), Defence Science and Technology Organisation (DSTO)</skos:altLabel>
	<skos:hiddenLabel xml:lang="en">AMRL</skos:hiddenLabel>
	<skos:definition xml:lang="en">In July 1994 the Materials Research Laboratory and Aeronautical Research Laboratory merged to form the Aeronautical and Maritime Research Laboratory (AMRL). A restructure of the Defence Science and Technology Organisation in 2002 resulted in the closure of all existing research Laboratories for the creation of three new ones. (Courtesy of Encyclopedia of Australian Science)</skos:definition>
	<dc:source rdf:datatype="http://www.w3.org/2001/XMLSchema#string">Australian Ocean Data Network Organisation Register</dc:source>
	<dc:publisher rdf:datatype="http://www.w3.org/2001/XMLSchema#string">eMarine Information Infrastructure (eMII)</dc:publisher>
	<skos:inScheme rdf:resource="http://vocab.aodn.org.au/def/organisation/1"/>
	<skos:broader rdf:resource="http://vocab.aodn.org.au/def/organisation/entity/2"/>
	<skos:scopeNote xml:lang="en">Organisation no longer exists</skos:scopeNote>
</rdf:Description>

<rdf:Description rdf:about="http://seadatanet.maris2.nl/v_edmo/print.asp?n_code=3934">
	<rdf:type rdf:resource="http://www.w3.org/2000/01/rdf-schema#Resource"/>
</rdf:Description>

<rdf:Description rdf:about="http://seadatanet.maris2.nl/v_edmo/print.asp?n_code=3942">
	<rdf:type rdf:resource="http://www.w3.org/2000/01/rdf-schema#Resource"/>
</rdf:Description>

<rdf:Description rdf:about="http://seadatanet.maris2.nl/v_edmo/print.asp?n_code=3936">
	<rdf:type rdf:resource="http://www.w3.org/2000/01/rdf-schema#Resource"/>
</rdf:Description>

<rdf:Description rdf:about="http://vocab.aodn.org.au/def/organisation/entity/6">
	<rdf:type rdf:resource="http://www.w3.org/2000/01/rdf-schema#Resource"/>
	<rdf:type rdf:resource="http://www.w3.org/2004/02/skos/core#Concept"/>
	<dcterms:creator rdf:datatype="http://www.w3.org/2001/XMLSchema#string">Natalia Atkins</dcterms:creator>
	<dcterms:created rdf:datatype="http://www.w3.org/2001/XMLSchema#dateTime">2015-04-27T10:38:15Z</dcterms:created>
	<skos:prefLabel xml:lang="en">Royal Australian Navy Hydrography and METOC Branch, Royal Australian Navy (RAN), Department of Defence (DoD), Australian Government</skos:prefLabel>
	<skos:altLabel xml:lang="en">Royal Australian Navy Hydrography and METOC Branch</skos:altLabel>
	<skos:definition xml:lang="en">Navy METOC (Meteorology and Oceanography) is a component of the Royal Australian Navy´s Hydrography and METOC Branch, of which the Australian Hydrographic Service is the other component.</skos:definition>
	<dc:source rdf:datatype="http://www.w3.org/2001/XMLSchema#string">Australian Ocean Data Network Organisation Register</dc:source>
	<dc:publisher rdf:datatype="http://www.w3.org/2001/XMLSchema#string">eMarine Information Infrastructure (eMII)</dc:publisher>
	<skos:exactMatch rdf:resource="http://seadatanet.maris2.nl/v_edmo/print.asp?n_code=3964"/>
	<skos:inScheme rdf:resource="http://vocab.aodn.org.au/def/organisation/1"/>
	<skos:broader rdf:resource="http://vocab.aodn.org.au/def/organisation/entity/5"/>
</rdf:Description>

<rdf:Description rdf:about="http://vocab.aodn.org.au/def/organisation/entity/7">
	<rdf:type rdf:resource="http://www.w3.org/2000/01/rdf-schema#Resource"/>
	<rdf:type rdf:resource="http://www.w3.org/2004/02/skos/core#Concept"/>
	<dcterms:creator rdf:datatype="http://www.w3.org/2001/XMLSchema#string">Natalia Atkins</dcterms:creator>
	<dcterms:created rdf:datatype="http://www.w3.org/2001/XMLSchema#dateTime">2015-04-27T10:38:15Z</dcterms:created>
	<skos:prefLabel xml:lang="en">Australian Hydrographic Service (AHS), Royal Australian Navy (RAN), Department of Defence (DoD), Australian Government</skos:prefLabel>
	<skos:altLabel xml:lang="en">Australian Hydrographic Service (AHS)</skos:altLabel>
	<skos:hiddenLabel xml:lang="en">AHS</skos:hiddenLabel>
	<skos:definition xml:lang="en">The RAN Australian Hydrographic Service is the Commonwealth Government agency responsible for the publication and distribution of nautical charts and other information required for the safety of ships navigating in Australian waters. It is also the Australian Defence Force (ADF) agency responsible for the provision of operational surveying support and maritime Military Geographic Information (MGI) for ADF operations and exercises.</skos:definition>
	<dc:source rdf:datatype="http://www.w3.org/2001/XMLSchema#string">Australian Ocean Data Network Organisation Register</dc:source>
	<dc:publisher rdf:datatype="http://www.w3.org/2001/XMLSchema#string">eMarine Information Infrastructure (eMII)</dc:publisher>
	<skos:inScheme rdf:resource="http://vocab.aodn.org.au/def/organisation/1"/>
	<skos:broader rdf:resource="http://vocab.aodn.org.au/def/organisation/entity/5"/>
</rdf:Description>

<rdf:Description rdf:about="http://seadatanet.maris2.nl/v_edmo/print.asp?n_code=3964">
	<rdf:type rdf:resource="http://www.w3.org/2000/01/rdf-schema#Resource"/>
</rdf:Description>

<rdf:Description rdf:about="http://seadatanet.maris2.nl/v_edmo/print.asp?n_code=3956">
	<rdf:type rdf:resource="http://www.w3.org/2000/01/rdf-schema#Resource"/>
</rdf:Description>

<rdf:Description rdf:about="http://vocab.aodn.org.au/def/organisation/entity/9">
	<rdf:type rdf:resource="http://www.w3.org/2000/01/rdf-schema#Resource"/>
	<rdf:type rdf:resource="http://www.w3.org/2004/02/skos/core#Concept"/>
	<dcterms:creator rdf:datatype="http://www.w3.org/2001/XMLSchema#string">Natalia Atkins</dcterms:creator>
	<dcterms:created rdf:datatype="http://www.w3.org/2001/XMLSchema#dateTime">2015-04-27T10:38:15Z</dcterms:created>
	<skos:prefLabel xml:lang="en">Australian Antarctic Division (AAD), Department of the Environment (DoE), Australian Government</skos:prefLabel>
	<skos:altLabel xml:lang="en">Australian Antarctic Division (AAD)</skos:altLabel>
	<skos:hiddenLabel xml:lang="en">AAD</skos:hiddenLabel>
	<skos:definition xml:lang="en">"The Australian Antarctic Division (AAD) is a division of the Department of the Environment. The AAD is responsible for delivering Outcome 3 of the Department's Strategic Plan 2013–2017, “Advancement of Australia’s strategic, scientific, environmental and economic interests in the Antarctic by protecting administering and researching the region”. The Australian Antarctic Division is also responsible for delivering the Australian Antarctic program (AAp) in accordance with government priorities as articulated in the plan.
These are to:
    Lead and collaborate internationally to further Australia’s research and policy interests.
    Enhance Australia’s capability to deliver on Antarctic priorities, and derive optimum benefit from our assets in the region.
    Gain recognition as an international leader in Antarctic science and environmental management.
    Maintain and reinforce Australian sovereignty in the Australian Antarctic Territory.
"</skos:definition>
	<dc:source rdf:datatype="http://www.w3.org/2001/XMLSchema#string">Australian Ocean Data Network Organisation Register</dc:source>
	<dc:publisher rdf:datatype="http://www.w3.org/2001/XMLSchema#string">eMarine Information Infrastructure (eMII)</dc:publisher>
	<skos:exactMatch rdf:resource="http://seadatanet.maris2.nl/v_edmo/print.asp?n_code=3950"/>
	<skos:narrower rdf:resource="http://vocab.aodn.org.au/def/organisation/entity/10"/>
	<skos:inScheme rdf:resource="http://vocab.aodn.org.au/def/organisation/1"/>
	<skos:broader rdf:resource="http://vocab.aodn.org.au/def/organisation/entity/8"/>
</rdf:Description>

<rdf:Description rdf:about="http://vocab.aodn.org.au/def/organisation/entity/11">
	<rdf:type rdf:resource="http://www.w3.org/2000/01/rdf-schema#Resource"/>
	<rdf:type rdf:resource="http://www.w3.org/2004/02/skos/core#Concept"/>
	<dcterms:modified rdf:datatype="http://www.w3.org/2001/XMLSchema#dateTime">2015-07-22T06:21:48Z</dcterms:modified>
	<dcterms:creator rdf:datatype="http://www.w3.org/2001/XMLSchema#string">Natalia Atkins</dcterms:creator>
	<dcterms:created rdf:datatype="http://www.w3.org/2001/XMLSchema#dateTime">2015-04-27T10:38:15Z</dcterms:created>
	<dcterms:contributor rdf:datatype="http://www.w3.org/2001/XMLSchema#string">Natalia_Atkins</dcterms:contributor>
	<skos:prefLabel xml:lang="en">Bureau of Meteorology (BOM), Department of Environment (DoE), Australian Government</skos:prefLabel>
	<skos:altLabel xml:lang="en">Bureau of Meteorology (BOM)</skos:altLabel>
	<skos:hiddenLabel xml:lang="en">BOM</skos:hiddenLabel>
	<skos:definition xml:lang="en">The Bureau of Meteorology is Australia's national weather, climate and water agency. Its expertise and services assist Australians in dealing with the harsh realities of their natural environment, including drought, floods, fires, storms, tsunami and tropical cyclones. Through regular forecasts, warnings, monitoring and advice spanning the Australian region and Antarctic territory, the Bureau provides one of the most fundamental and widely used services of government. The Bureau contributes to national social, economic, cultural and environmental goals by providing observational, meteorological, hydrological and oceanographic services and by undertaking research into science and environment related issues in support of its operations and services.</skos:definition>
	<dc:source rdf:datatype="http://www.w3.org/2001/XMLSchema#string">Australian Ocean Data Network Organisation Register</dc:source>
	<dc:publisher rdf:datatype="http://www.w3.org/2001/XMLSchema#string">eMarine Information Infrastructure (eMII)</dc:publisher>
	<skos:exactMatch rdf:resource="http://seadatanet.maris2.nl/v_edmo/print.asp?n_code=1485"/>
	<skos:narrower rdf:resource="http://vocab.aodn.org.au/def/organisation/entity/12"/>
	<skos:inScheme rdf:resource="http://vocab.aodn.org.au/def/organisation/1"/>
	<skos:broader rdf:resource="http://vocab.aodn.org.au/def/organisation/entity/8"/>
</rdf:Description>

<rdf:Description rdf:about="http://seadatanet.maris2.nl/v_edmo/print.asp?n_code=3950">
	<rdf:type rdf:resource="http://www.w3.org/2000/01/rdf-schema#Resource"/>
</rdf:Description>

<rdf:Description rdf:about="http://vocab.aodn.org.au/def/organisation/entity/10">
	<rdf:type rdf:resource="http://www.w3.org/2000/01/rdf-schema#Resource"/>
	<rdf:type rdf:resource="http://www.w3.org/2004/02/skos/core#Concept"/>
	<dcterms:creator rdf:datatype="http://www.w3.org/2001/XMLSchema#string">Natalia Atkins</dcterms:creator>
	<dcterms:created rdf:datatype="http://www.w3.org/2001/XMLSchema#dateTime">2015-04-27T10:38:15Z</dcterms:created>
	<skos:prefLabel xml:lang="en">Australian Antarctic Data Centre (AADC), Australian Antarctic Division (AAD), Department of the Environment (DoE), Australian Government</skos:prefLabel>
	<skos:altLabel xml:lang="en">Australian Antarctic Data Centre (AADC), Australian Antarctic Division (AAD)</skos:altLabel>
	<skos:hiddenLabel xml:lang="en">AADC</skos:hiddenLabel>
	<skos:definition xml:lang="en">The Australian Antarctic Data Centre (AADC) was established in 1996 to provide long-term management of Australia's Antarctic data, thereby improving the value and impact of our scientific activities. The Data Centre is committed to the free and open exchange of scientific data, consistent with the Antarctic Treaty's position that "to the greatest extent feasible and practicable scientific observations and results from Antarctica shall be exchanged and made freely available". As Australia's Antarctic Mapping agency, the AADC supports the logistical operations of the Australian Antarctic Program. The AADC also incorporates a group of quantitative research scientists who value-add to the AADC's holdings and provide analytical research capability to the Antarctic Program.</skos:definition>
	<dc:source rdf:datatype="http://www.w3.org/2001/XMLSchema#string">Australian Ocean Data Network Organisation Register</dc:source>
	<dc:publisher rdf:datatype="http://www.w3.org/2001/XMLSchema#string">eMarine Information Infrastructure (eMII)</dc:publisher>
	<skos:exactMatch rdf:resource="http://seadatanet.maris2.nl/v_edmo/print.asp?n_code=3951"/>
	<skos:inScheme rdf:resource="http://vocab.aodn.org.au/def/organisation/1"/>
	<skos:broader rdf:resource="http://vocab.aodn.org.au/def/organisation/entity/9"/>
</rdf:Description>

<rdf:Description rdf:about="http://seadatanet.maris2.nl/v_edmo/print.asp?n_code=3951">
	<rdf:type rdf:resource="http://www.w3.org/2000/01/rdf-schema#Resource"/>
</rdf:Description>

<rdf:Description rdf:about="http://seadatanet.maris2.nl/v_edmo/print.asp?n_code=1485">
	<rdf:type rdf:resource="http://www.w3.org/2000/01/rdf-schema#Resource"/>
</rdf:Description>

<rdf:Description rdf:about="http://vocab.aodn.org.au/def/organisation/entity/12">
	<rdf:type rdf:resource="http://www.w3.org/2000/01/rdf-schema#Resource"/>
	<rdf:type rdf:resource="http://www.w3.org/2004/02/skos/core#Concept"/>
	<dcterms:modified rdf:datatype="http://www.w3.org/2001/XMLSchema#dateTime">2015-05-11T23:45:34Z</dcterms:modified>
	<dcterms:creator rdf:datatype="http://www.w3.org/2001/XMLSchema#string">Natalia Atkins</dcterms:creator>
	<dcterms:created rdf:datatype="http://www.w3.org/2001/XMLSchema#dateTime">2015-04-27T10:38:15Z</dcterms:created>
	<skos:prefLabel xml:lang="en">National Tidal Unit (NTU)</skos:prefLabel>
	<skos:hiddenLabel xml:lang="en">NTU</skos:hiddenLabel>
	<skos:definition xml:lang="en">Australian national facility operated since January 2004 by the Bureau of Meteorology. Until then it was known as the National Tidal Facility of Australia operated by Flinders University.</skos:definition>
	<dc:source rdf:datatype="http://www.w3.org/2001/XMLSchema#string">Australian Ocean Data Network Organisation Register</dc:source>
	<dc:publisher rdf:datatype="http://www.w3.org/2001/XMLSchema#string">eMarine Information Infrastructure (eMII)</dc:publisher>
	<skos:exactMatch rdf:resource="http://seadatanet.maris2.nl/v_edmo/print.asp?n_code=2094"/>
	<skos:inScheme rdf:resource="http://vocab.aodn.org.au/def/organisation/1"/>
	<skos:broader rdf:resource="http://vocab.aodn.org.au/def/organisation/entity/11"/>
</rdf:Description>

<rdf:Description rdf:about="http://seadatanet.maris2.nl/v_edmo/print.asp?n_code=2094">
	<rdf:type rdf:resource="http://www.w3.org/2000/01/rdf-schema#Resource"/>
</rdf:Description>

<rdf:Description rdf:about="http://seadatanet.maris2.nl/v_edmo/print.asp?n_code=3943">
	<rdf:type rdf:resource="http://www.w3.org/2000/01/rdf-schema#Resource"/>
</rdf:Description>

<rdf:Description rdf:about="http://vocab.aodn.org.au/def/organisation/entity/14">
	<rdf:type rdf:resource="http://www.w3.org/2000/01/rdf-schema#Resource"/>
	<rdf:type rdf:resource="http://www.w3.org/2004/02/skos/core#Concept"/>
	<dcterms:modified rdf:datatype="http://www.w3.org/2001/XMLSchema#dateTime">2015-07-22T05:52:55Z</dcterms:modified>
	<dcterms:creator rdf:datatype="http://www.w3.org/2001/XMLSchema#string">Natalia Atkins</dcterms:creator>
	<dcterms:created rdf:datatype="http://www.w3.org/2001/XMLSchema#dateTime">2015-04-27T10:38:15Z</dcterms:created>
	<dcterms:contributor rdf:datatype="http://www.w3.org/2001/XMLSchema#string">Natalia_Atkins</dcterms:contributor>
	<skos:prefLabel xml:lang="en">Australian Institute of Marine Science (AIMS), Department of Industry and Science, Australian Government</skos:prefLabel>
	<skos:altLabel xml:lang="en">Australian Institute of Marine Science (AIMS)</skos:altLabel>
	<skos:hiddenLabel xml:lang="en">AIMS</skos:hiddenLabel>
	<skos:definition xml:lang="en">The Australian Institute of Marine Science (AIMS) is Australia’s premiere tropical marine research agency. They play a pivotal role in providing large-scale, long-term and world-class research that helps governments, industry and the wider community to make informed decisions about the management of Australia’s marine estate.</skos:definition>
	<dc:source rdf:datatype="http://www.w3.org/2001/XMLSchema#string">Australian Ocean Data Network Organisation Register</dc:source>
	<dc:publisher rdf:datatype="http://www.w3.org/2001/XMLSchema#string">eMarine Information Infrastructure (eMII)</dc:publisher>
	<skos:exactMatch rdf:resource="http://seadatanet.maris2.nl/v_edmo/print.asp?n_code=2008"/>
	<skos:inScheme rdf:resource="http://vocab.aodn.org.au/def/organisation/1"/>
	<skos:broader rdf:resource="http://vocab.aodn.org.au/def/organisation/entity/13"/>
</rdf:Description>

<rdf:Description rdf:about="http://vocab.aodn.org.au/def/organisation/entity/15">
	<rdf:type rdf:resource="http://www.w3.org/2000/01/rdf-schema#Resource"/>
	<rdf:type rdf:resource="http://www.w3.org/2004/02/skos/core#Concept"/>
	<dcterms:creator rdf:datatype="http://www.w3.org/2001/XMLSchema#string">Natalia Atkins</dcterms:creator>
	<dcterms:created rdf:datatype="http://www.w3.org/2001/XMLSchema#dateTime">2015-04-27T10:38:15Z</dcterms:created>
	<skos:prefLabel xml:lang="en">Commonwealth Scientific and Industrial Research Organisation (CSIRO)</skos:prefLabel>
	<skos:hiddenLabel xml:lang="en">CSIRO</skos:hiddenLabel>
	<skos:definition xml:lang="en">CSIRO, the Commonwealth Scientific and Industrial Research Organisation, is Australia's national science agency and one of the largest and most diverse research agencies in the world.</skos:definition>
	<dc:source rdf:datatype="http://www.w3.org/2001/XMLSchema#string">Australian Ocean Data Network Organisation Register</dc:source>
	<dc:publisher rdf:datatype="http://www.w3.org/2001/XMLSchema#string">eMarine Information Infrastructure (eMII)</dc:publisher>
	<skos:exactMatch rdf:resource="http://seadatanet.maris2.nl/v_edmo/print.asp?n_code=3945"/>
	<skos:narrower rdf:resource="http://vocab.aodn.org.au/def/organisation/entity/16"/>
	<skos:narrower rdf:resource="http://vocab.aodn.org.au/def/organisation/entity/17"/>
	<skos:narrower rdf:resource="http://vocab.aodn.org.au/def/organisation/entity/18"/>
	<skos:inScheme rdf:resource="http://vocab.aodn.org.au/def/organisation/1"/>
	<skos:broader rdf:resource="http://vocab.aodn.org.au/def/organisation/entity/13"/>
</rdf:Description>

<rdf:Description rdf:about="http://vocab.aodn.org.au/def/organisation/entity/20">
	<rdf:type rdf:resource="http://www.w3.org/2000/01/rdf-schema#Resource"/>
	<rdf:type rdf:resource="http://www.w3.org/2004/02/skos/core#Concept"/>
	<dcterms:creator rdf:datatype="http://www.w3.org/2001/XMLSchema#string">Natalia Atkins</dcterms:creator>
	<dcterms:created rdf:datatype="http://www.w3.org/2001/XMLSchema#dateTime">2015-04-27T10:38:15Z</dcterms:created>
	<skos:prefLabel xml:lang="en">Geoscience Australia (GA), Department of Industry and Science, Australian Government</skos:prefLabel>
	<skos:altLabel xml:lang="en">Commonwealth of Australia (Geoscience Australia)</skos:altLabel>
	<skos:hiddenLabel xml:lang="en">GA</skos:hiddenLabel>
	<skos:definition xml:lang="en">Geoscience Australia is a prescribed Australian Government agency within the Industry and Science portfolio. Geoscience Australia applies geoscience to Australia's most important challenges by providing geoscience information, services and capability to the Australian Government, industry and stakeholders.</skos:definition>
	<dc:source rdf:datatype="http://www.w3.org/2001/XMLSchema#string">Australian Ocean Data Network Organisation Register</dc:source>
	<dc:publisher rdf:datatype="http://www.w3.org/2001/XMLSchema#string">eMarine Information Infrastructure (eMII)</dc:publisher>
	<skos:exactMatch rdf:resource="http://seadatanet.maris2.nl/v_edmo/print.asp?n_code=3968"/>
	<skos:inScheme rdf:resource="http://vocab.aodn.org.au/def/organisation/1"/>
	<skos:broader rdf:resource="http://vocab.aodn.org.au/def/organisation/entity/13"/>
	<skos:scopeNote xml:lang="en">Replaces http://vocab.aodn.org.au/def/organisation/entity/21 and http://vocab.aodn.org.au/def/organisation/entity/22</skos:scopeNote>
	<dcterms:replaces rdf:resource="http://vocab.aodn.org.au/def/organisation/entity/21"/>
	<dcterms:replaces rdf:resource="http://vocab.aodn.org.au/def/organisation/entity/22"/>
	<dcterms:replaces xml:lang="en">Bureau of Mineral Resources, Geology and Geophysics (BMR)</dcterms:replaces>
	<dcterms:replaces xml:lang="en">Australian Geological Survey Organisation (AGSO)</dcterms:replaces>
</rdf:Description>

<rdf:Description rdf:about="http://vocab.aodn.org.au/def/organisation/entity/21">
	<rdf:type rdf:resource="http://www.w3.org/2000/01/rdf-schema#Resource"/>
	<rdf:type rdf:resource="http://www.w3.org/2004/02/skos/core#Concept"/>
	<dcterms:creator rdf:datatype="http://www.w3.org/2001/XMLSchema#string">Natalia Atkins</dcterms:creator>
	<dcterms:created rdf:datatype="http://www.w3.org/2001/XMLSchema#dateTime">2015-04-27T10:38:15Z</dcterms:created>
	<skos:prefLabel xml:lang="en">Bureau of Mineral Resources, Geology and Geophysics (BMR)</skos:prefLabel>
	<skos:hiddenLabel xml:lang="en">BMR</skos:hiddenLabel>
	<skos:definition xml:lang="en">Australian Geological Survey Organisation (AGSO)’s predecessor organisation the Bureau of Mineral Resources, Geology and Geophysics (BMR) was established in 1946; with the name changing to AGSO in 1992. BMR’s main objective was the systematic geological and geophysical mapping of the continent as the basis for informed mineral exploration. (Courtesy of Wikipedia)</skos:definition>
	<dc:source rdf:datatype="http://www.w3.org/2001/XMLSchema#string">Australian Ocean Data Network Organisation Register</dc:source>
	<dc:publisher rdf:datatype="http://www.w3.org/2001/XMLSchema#string">eMarine Information Infrastructure (eMII)</dc:publisher>
	<skos:inScheme rdf:resource="http://vocab.aodn.org.au/def/organisation/1"/>
	<skos:broader rdf:resource="http://vocab.aodn.org.au/def/organisation/entity/13"/>
	<skos:scopeNote xml:lang="en">Organisation no longer exists</skos:scopeNote>
	<skos:scopeNote xml:lang="en">Organisation no longer exists. Replaced by http://vocab.aodn.org.au/def/organisation/entity/22</skos:scopeNote>
	<dcterms:isReplacedBy rdf:resource="http://vocab.aodn.org.au/def/organisation/entity/22"/>
	<dcterms:isReplacedBy xml:lang="en">Australian Geological Survey Organisation (AGSO)</dcterms:isReplacedBy>
</rdf:Description>

<rdf:Description rdf:about="http://vocab.aodn.org.au/def/organisation/entity/22">
	<rdf:type rdf:resource="http://www.w3.org/2000/01/rdf-schema#Resource"/>
	<rdf:type rdf:resource="http://www.w3.org/2004/02/skos/core#Concept"/>
	<dcterms:modified rdf:datatype="http://www.w3.org/2001/XMLSchema#dateTime">2016-01-28T03:34:58Z</dcterms:modified>
	<dcterms:creator rdf:datatype="http://www.w3.org/2001/XMLSchema#string">Natalia Atkins</dcterms:creator>
	<dcterms:created rdf:datatype="http://www.w3.org/2001/XMLSchema#dateTime">2015-04-27T10:38:15Z</dcterms:created>
	<dcterms:contributor rdf:datatype="http://www.w3.org/2001/XMLSchema#string">eMII_Atkins.Natalia</dcterms:contributor>
	<skos:prefLabel xml:lang="en">Australian Geological Survey Organisation (AGSO)</skos:prefLabel>
	<skos:hiddenLabel xml:lang="en">AGSO</skos:hiddenLabel>
	<skos:definition xml:lang="en">Geoscience Australia Australian Geological Survey Organisation (AGSO). The BMR (Bureau of Mineral Resources, Geology and Geophysics) became the Australian Geological Survey Organisation (AGSO) in 1992. AGSO provided much of the geoscience information that underpinned exploration and development work for petroleum and minerals in Australia. A review carried out in AGSO's infancy concluded that geoscience was relevant to society by providing information essential for economic prosperity and for the proper use of resources to protect the local and global economy. In November 2001, the combined agencies adopted the current name of Geoscience Australia, recognising vital geoscientific work in a wide range of contexts and across many disciplines. The National Mapping and Geohazards Divisions of Geoscience Australia merged in 2005 to reflect a global trend in dealing with an increasing range of real world phenomena. Under the new Geospatial and Earth Monitoring Division (GEMD), the maintenance of standard small scale national topographic mapping remains a major responsibility.</skos:definition>
	<dc:source rdf:datatype="http://www.w3.org/2001/XMLSchema#string">Australian Ocean Data Network Organisation Register</dc:source>
	<dc:publisher rdf:datatype="http://www.w3.org/2001/XMLSchema#string">eMarine Information Infrastructure (eMII)</dc:publisher>
	<skos:inScheme rdf:resource="http://vocab.aodn.org.au/def/organisation/1"/>
	<skos:broader rdf:resource="http://vocab.aodn.org.au/def/organisation/entity/13"/>
	<skos:scopeNote xml:lang="en">Organisation no longer exists</skos:scopeNote>
	<skos:scopeNote xml:lang="en">Organisation no longer exists. Replaced by http://vocab.aodn.org.au/def/organisation/entity/20. Replaces http://vocab.aodn.org.au/def/organisation/entity/21</skos:scopeNote>
	<dcterms:replaces xml:lang="en">Bureau of Mineral Resources, Geology and Geophysics (BMR)</dcterms:replaces>
	<dcterms:isReplacedBy rdf:resource="http://vocab.aodn.org.au/def/organisation/entity/20"/>
	<dcterms:isReplacedBy xml:lang="en">Geoscience Australia (GA), Department of Industry and Science, Australian Government</dcterms:isReplacedBy>
</rdf:Description>

<rdf:Description rdf:about="http://seadatanet.maris2.nl/v_edmo/print.asp?n_code=2008">
	<rdf:type rdf:resource="http://www.w3.org/2000/01/rdf-schema#Resource"/>
</rdf:Description>

<rdf:Description rdf:about="http://seadatanet.maris2.nl/v_edmo/print.asp?n_code=3945">
	<rdf:type rdf:resource="http://www.w3.org/2000/01/rdf-schema#Resource"/>
</rdf:Description>

<rdf:Description rdf:about="http://vocab.aodn.org.au/def/organisation/entity/16">
	<rdf:type rdf:resource="http://www.w3.org/2000/01/rdf-schema#Resource"/>
	<rdf:type rdf:resource="http://www.w3.org/2004/02/skos/core#Concept"/>
	<dcterms:modified rdf:datatype="http://www.w3.org/2001/XMLSchema#dateTime">2015-10-30T05:47:36Z</dcterms:modified>
	<dcterms:creator rdf:datatype="http://www.w3.org/2001/XMLSchema#string">Natalia Atkins</dcterms:creator>
	<dcterms:created rdf:datatype="http://www.w3.org/2001/XMLSchema#dateTime">2015-04-27T10:38:15Z</dcterms:created>
	<dcterms:contributor rdf:datatype="http://www.w3.org/2001/XMLSchema#string">eMII_Atkins.Natalia</dcterms:contributor>
	<skos:prefLabel xml:lang="en">CSIRO Land and Water</skos:prefLabel>
	<skos:definition xml:lang="en">A provider of innovative research solutions to the most significant land, water and ecosystem management challenges.</skos:definition>
	<dc:source rdf:datatype="http://www.w3.org/2001/XMLSchema#string">Australian Ocean Data Network Organisation Register</dc:source>
	<dc:publisher rdf:datatype="http://www.w3.org/2001/XMLSchema#string">eMarine Information Infrastructure (eMII)</dc:publisher>
	<skos:exactMatch rdf:resource="http://seadatanet.maris2.nl/v_edmo/print.asp?n_code=3941"/>
	<skos:inScheme rdf:resource="http://vocab.aodn.org.au/def/organisation/1"/>
	<skos:broader rdf:resource="http://vocab.aodn.org.au/def/organisation/entity/15"/>
</rdf:Description>

<rdf:Description rdf:about="http://vocab.aodn.org.au/def/organisation/entity/17">
	<rdf:type rdf:resource="http://www.w3.org/2000/01/rdf-schema#Resource"/>
	<rdf:type rdf:resource="http://www.w3.org/2004/02/skos/core#Concept"/>
	<dcterms:creator rdf:datatype="http://www.w3.org/2001/XMLSchema#string">Natalia Atkins</dcterms:creator>
	<dcterms:created rdf:datatype="http://www.w3.org/2001/XMLSchema#dateTime">2015-04-27T10:38:15Z</dcterms:created>
	<skos:prefLabel xml:lang="en">CSIRO Marine and Atmospheric Research (CMAR)</skos:prefLabel>
	<skos:hiddenLabel xml:lang="en">CMAR</skos:hiddenLabel>
	<skos:definition xml:lang="en">ConceptDescription</skos:definition>
	<dc:source rdf:datatype="http://www.w3.org/2001/XMLSchema#string">Australian Ocean Data Network Organisation Register</dc:source>
	<dc:publisher rdf:datatype="http://www.w3.org/2001/XMLSchema#string">eMarine Information Infrastructure (eMII)</dc:publisher>
	<skos:exactMatch rdf:resource="http://seadatanet.maris2.nl/v_edmo/print.asp?n_code=1484"/>
	<skos:inScheme rdf:resource="http://vocab.aodn.org.au/def/organisation/1"/>
	<skos:broader rdf:resource="http://vocab.aodn.org.au/def/organisation/entity/15"/>
	<skos:scopeNote xml:lang="en">Organisation no longer exists</skos:scopeNote>
	<skos:scopeNote xml:lang="en">Organisation no longer exists. Replaced by http://vocab.aodn.org.au/def/organisation/entity/18</skos:scopeNote>
	<dcterms:isReplacedBy rdf:resource="http://vocab.aodn.org.au/def/organisation/entity/18"/>
	<dcterms:isReplacedBy xml:lang="en">CSIRO Oceans and Atmosphere</dcterms:isReplacedBy>
</rdf:Description>

<rdf:Description rdf:about="http://vocab.aodn.org.au/def/organisation/entity/18">
	<rdf:type rdf:resource="http://www.w3.org/2000/01/rdf-schema#Resource"/>
	<rdf:type rdf:resource="http://www.w3.org/2004/02/skos/core#Concept"/>
	<dcterms:modified rdf:datatype="http://www.w3.org/2001/XMLSchema#dateTime">2015-10-30T05:49:06Z</dcterms:modified>
	<dcterms:creator rdf:datatype="http://www.w3.org/2001/XMLSchema#string">Natalia Atkins</dcterms:creator>
	<dcterms:created rdf:datatype="http://www.w3.org/2001/XMLSchema#dateTime">2015-04-27T10:38:15Z</dcterms:created>
	<dcterms:contributor rdf:datatype="http://www.w3.org/2001/XMLSchema#string">eMII_Atkins.Natalia</dcterms:contributor>
	<skos:prefLabel xml:lang="en">CSIRO Oceans and Atmosphere </skos:prefLabel>
	<skos:prefLabel xml:lang="en">CSIRO Oceans and Atmosphere</skos:prefLabel>
	<skos:altLabel xml:lang="en">CSIRO Oceans and Atmosphere - Aspendale</skos:altLabel>
	<skos:altLabel xml:lang="en">CSIRO Oceans and Atmosphere - Dutton Park</skos:altLabel>
	<skos:altLabel xml:lang="en">CSIRO Oceans and Atmosphere - Floreat</skos:altLabel>
	<skos:altLabel xml:lang="en">CSIRO Oceans and Atmosphere - Hobart</skos:altLabel>
	<skos:definition xml:lang="en">Oceans and Atmosphere provides research to help plan for and respond to weather and climate related natural hazards and ensure sustainable coastal development and growth of marine industries.</skos:definition>
	<dc:source rdf:datatype="http://www.w3.org/2001/XMLSchema#string">Australian Ocean Data Network Organisation Register</dc:source>
	<dc:publisher rdf:datatype="http://www.w3.org/2001/XMLSchema#string">eMarine Information Infrastructure (eMII)</dc:publisher>
	<skos:exactMatch rdf:resource="http://seadatanet.maris2.nl/v_edmo/print.asp?n_code=1484"/>
	<skos:narrower rdf:resource="http://vocab.aodn.org.au/def/organisation/entity/19"/>
	<skos:inScheme rdf:resource="http://vocab.aodn.org.au/def/organisation/1"/>
	<skos:broader rdf:resource="http://vocab.aodn.org.au/def/organisation/entity/15"/>
	<skos:scopeNote xml:lang="en">Replaces http://vocab.aodn.org.au/def/organisation/entity/17</skos:scopeNote>
	<dcterms:replaces rdf:resource="http://vocab.aodn.org.au/def/organisation/entity/17"/>
	<dcterms:replaces xml:lang="en">CSIRO Marine and Atmospheric Research (CMAR)</dcterms:replaces>
</rdf:Description>

<rdf:Description rdf:about="http://seadatanet.maris2.nl/v_edmo/print.asp?n_code=3941">
	<rdf:type rdf:resource="http://www.w3.org/2000/01/rdf-schema#Resource"/>
</rdf:Description>

<rdf:Description rdf:about="http://seadatanet.maris2.nl/v_edmo/print.asp?n_code=1484">
	<rdf:type rdf:resource="http://www.w3.org/2000/01/rdf-schema#Resource"/>
</rdf:Description>

<rdf:Description rdf:about="http://vocab.aodn.org.au/def/organisation/entity/19">
	<rdf:type rdf:resource="http://www.w3.org/2000/01/rdf-schema#Resource"/>
	<rdf:type rdf:resource="http://www.w3.org/2004/02/skos/core#Concept"/>
	<dcterms:modified rdf:datatype="http://www.w3.org/2001/XMLSchema#dateTime">2015-10-30T05:49:23Z</dcterms:modified>
	<dcterms:creator rdf:datatype="http://www.w3.org/2001/XMLSchema#string">Natalia Atkins</dcterms:creator>
	<dcterms:created rdf:datatype="http://www.w3.org/2001/XMLSchema#dateTime">2015-04-27T10:38:15Z</dcterms:created>
	<dcterms:contributor rdf:datatype="http://www.w3.org/2001/XMLSchema#string">eMII_Atkins.Natalia</dcterms:contributor>
	<skos:prefLabel xml:lang="en">Information and Data Centre, CSIRO Oceans and Atmosphere </skos:prefLabel>
	<skos:prefLabel xml:lang="en">Information and Data Centre, CSIRO Oceans and Atmosphere</skos:prefLabel>
	<skos:definition xml:lang="en">ConceptDescription</skos:definition>
	<dc:source rdf:datatype="http://www.w3.org/2001/XMLSchema#string">Australian Ocean Data Network Organisation Register</dc:source>
	<dc:publisher rdf:datatype="http://www.w3.org/2001/XMLSchema#string">eMarine Information Infrastructure (eMII)</dc:publisher>
	<skos:exactMatch rdf:resource="http://seadatanet.maris2.nl/v_edmo/print.asp?n_code=4062"/>
	<skos:inScheme rdf:resource="http://vocab.aodn.org.au/def/organisation/1"/>
	<skos:broader rdf:resource="http://vocab.aodn.org.au/def/organisation/entity/18"/>
</rdf:Description>

<rdf:Description rdf:about="http://seadatanet.maris2.nl/v_edmo/print.asp?n_code=4062">
	<rdf:type rdf:resource="http://www.w3.org/2000/01/rdf-schema#Resource"/>
</rdf:Description>

<rdf:Description rdf:about="http://seadatanet.maris2.nl/v_edmo/print.asp?n_code=3968">
	<rdf:type rdf:resource="http://www.w3.org/2000/01/rdf-schema#Resource"/>
</rdf:Description>

<rdf:Description rdf:about="http://seadatanet.maris2.nl/v_edmo/print.asp?n_code=4060">
	<rdf:type rdf:resource="http://www.w3.org/2000/01/rdf-schema#Resource"/>
</rdf:Description>

<rdf:Description rdf:about="http://vocab.aodn.org.au/def/organisation/entity/25">
	<rdf:type rdf:resource="http://www.w3.org/2000/01/rdf-schema#Resource"/>
	<rdf:type rdf:resource="http://www.w3.org/2004/02/skos/core#Concept"/>
	<dcterms:modified rdf:datatype="http://www.w3.org/2001/XMLSchema#dateTime">2015-05-12T00:42:42Z</dcterms:modified>
	<dcterms:creator rdf:datatype="http://www.w3.org/2001/XMLSchema#string">Natalia Atkins</dcterms:creator>
	<dcterms:created rdf:datatype="http://www.w3.org/2001/XMLSchema#dateTime">2015-04-27T10:38:15Z</dcterms:created>
	<skos:prefLabel xml:lang="en">Australian Bureau of Agriculture and Resource Economics and Sciences (ABARES), Department of Agriculture, Australian Government</skos:prefLabel>
	<skos:altLabel xml:lang="en">Australian Bureau of Agriculture and Resource Economics and Sciences (ABARES)</skos:altLabel>
	<skos:hiddenLabel xml:lang="en">ABARES</skos:hiddenLabel>
	<skos:definition xml:lang="en">The Australian Bureau of Agricultural and Resource Economics and Sciences is a research organisation within the Australian Government Department of Agriculture. ABARES was formed following the merger of the Australian Bureau of Agricultural and Resource Economics (ABARE) and the Bureau of Rural Sciences (RBS) in 2010.</skos:definition>
	<dc:source rdf:datatype="http://www.w3.org/2001/XMLSchema#string">Australian Ocean Data Network Organisation Register</dc:source>
	<dc:publisher rdf:datatype="http://www.w3.org/2001/XMLSchema#string">eMarine Information Infrastructure (eMII)</dc:publisher>
	<skos:exactMatch rdf:resource="http://seadatanet.maris2.nl/v_edmo/print.asp?n_code=4061"/>
	<skos:inScheme rdf:resource="http://vocab.aodn.org.au/def/organisation/1"/>
	<skos:broader rdf:resource="http://vocab.aodn.org.au/def/organisation/entity/24"/>
	<skos:scopeNote xml:lang="en">Replaces http://vocab.aodn.org.au/def/organisation/entity/168</skos:scopeNote>
	<dcterms:replaces xml:lang="en">http://vocab.aodn.org.au/def/organisation/entity/168</dcterms:replaces>
	<dcterms:replaces xml:lang="en">Bureau of Rural Sciences (BRS), Australian Government</dcterms:replaces>
</rdf:Description>

<rdf:Description rdf:about="http://seadatanet.maris2.nl/v_edmo/print.asp?n_code=4061">
	<rdf:type rdf:resource="http://www.w3.org/2000/01/rdf-schema#Resource"/>
</rdf:Description>

<rdf:Description rdf:about="http://seadatanet.maris2.nl/v_edmo/print.asp?n_code=4063">
	<rdf:type rdf:resource="http://www.w3.org/2000/01/rdf-schema#Resource"/>
</rdf:Description>

<rdf:Description rdf:about="http://seadatanet.maris2.nl/v_edmo/print.asp?n_code=4064">
	<rdf:type rdf:resource="http://www.w3.org/2000/01/rdf-schema#Resource"/>
</rdf:Description>

<rdf:Description rdf:about="http://vocab.aodn.org.au/def/organisation_classes/category/5">
	<rdf:type rdf:resource="http://www.w3.org/2000/01/rdf-schema#Resource"/>
</rdf:Description>

<rdf:Description rdf:about="http://seadatanet.maris2.nl/v_edmo/print.asp?n_code=4065">
	<rdf:type rdf:resource="http://www.w3.org/2000/01/rdf-schema#Resource"/>
</rdf:Description>

<rdf:Description rdf:about="http://seadatanet.maris2.nl/v_edmo/print.asp?n_code=4066">
	<rdf:type rdf:resource="http://www.w3.org/2000/01/rdf-schema#Resource"/>
</rdf:Description>

<rdf:Description rdf:about="http://seadatanet.maris2.nl/v_edmo/print.asp?n_code=4067">
	<rdf:type rdf:resource="http://www.w3.org/2000/01/rdf-schema#Resource"/>
</rdf:Description>

<rdf:Description rdf:about="http://vocab.aodn.org.au/def/organisation_classes/category/2">
	<rdf:type rdf:resource="http://www.w3.org/2000/01/rdf-schema#Resource"/>
</rdf:Description>

<rdf:Description rdf:about="http://seadatanet.maris2.nl/v_edmo/print.asp?n_code=4026">
	<rdf:type rdf:resource="http://www.w3.org/2000/01/rdf-schema#Resource"/>
</rdf:Description>

<rdf:Description rdf:about="http://seadatanet.maris2.nl/v_edmo/print.asp?n_code=4068">
	<rdf:type rdf:resource="http://www.w3.org/2000/01/rdf-schema#Resource"/>
</rdf:Description>

<rdf:Description rdf:about="http://seadatanet.maris2.nl/v_edmo/print.asp?n_code=4069">
	<rdf:type rdf:resource="http://www.w3.org/2000/01/rdf-schema#Resource"/>
</rdf:Description>

<rdf:Description rdf:about="http://vocab.aodn.org.au/def/organisation_classes/category/6">
	<rdf:type rdf:resource="http://www.w3.org/2000/01/rdf-schema#Resource"/>
</rdf:Description>

<rdf:Description rdf:about="http://seadatanet.maris2.nl/v_edmo/print.asp?n_code=4070">
	<rdf:type rdf:resource="http://www.w3.org/2000/01/rdf-schema#Resource"/>
</rdf:Description>

<rdf:Description rdf:about="http://seadatanet.maris2.nl/v_edmo/print.asp?n_code=4071">
	<rdf:type rdf:resource="http://www.w3.org/2000/01/rdf-schema#Resource"/>
</rdf:Description>

<rdf:Description rdf:about="http://seadatanet.maris2.nl/v_edmo/print.asp?n_code=4072">
	<rdf:type rdf:resource="http://www.w3.org/2000/01/rdf-schema#Resource"/>
</rdf:Description>

<rdf:Description rdf:about="http://seadatanet.maris2.nl/v_edmo/print.asp?n_code=4073">
	<rdf:type rdf:resource="http://www.w3.org/2000/01/rdf-schema#Resource"/>
</rdf:Description>

<rdf:Description rdf:about="http://seadatanet.maris2.nl/v_edmo/print.asp?n_code=4074">
	<rdf:type rdf:resource="http://www.w3.org/2000/01/rdf-schema#Resource"/>
</rdf:Description>

<rdf:Description rdf:about="http://seadatanet.maris2.nl/v_edmo/print.asp?n_code=4075">
	<rdf:type rdf:resource="http://www.w3.org/2000/01/rdf-schema#Resource"/>
</rdf:Description>

<rdf:Description rdf:about="http://seadatanet.maris2.nl/v_edmo/print.asp?n_code=3939">
	<rdf:type rdf:resource="http://www.w3.org/2000/01/rdf-schema#Resource"/>
</rdf:Description>

<rdf:Description rdf:about="http://seadatanet.maris2.nl/v_edmo/print.asp?n_code=4076">
	<rdf:type rdf:resource="http://www.w3.org/2000/01/rdf-schema#Resource"/>
</rdf:Description>

<rdf:Description rdf:about="http://seadatanet.maris2.nl/v_edmo/print.asp?n_code=4077">
	<rdf:type rdf:resource="http://www.w3.org/2000/01/rdf-schema#Resource"/>
</rdf:Description>

<rdf:Description rdf:about="http://seadatanet.maris2.nl/v_edmo/print.asp?n_code=4078">
	<rdf:type rdf:resource="http://www.w3.org/2000/01/rdf-schema#Resource"/>
</rdf:Description>

<rdf:Description rdf:about="http://seadatanet.maris2.nl/v_edmo/print.asp?n_code=3937">
	<rdf:type rdf:resource="http://www.w3.org/2000/01/rdf-schema#Resource"/>
</rdf:Description>

<rdf:Description rdf:about="http://seadatanet.maris2.nl/v_edmo/print.asp?n_code=4079">
	<rdf:type rdf:resource="http://www.w3.org/2000/01/rdf-schema#Resource"/>
</rdf:Description>

<rdf:Description rdf:about="http://seadatanet.maris2.nl/v_edmo/print.asp?n_code=4080">
	<rdf:type rdf:resource="http://www.w3.org/2000/01/rdf-schema#Resource"/>
</rdf:Description>

<rdf:Description rdf:about="http://seadatanet.maris2.nl/v_edmo/print.asp?n_code=4081">
	<rdf:type rdf:resource="http://www.w3.org/2000/01/rdf-schema#Resource"/>
</rdf:Description>

<rdf:Description rdf:about="http://vocab.aodn.org.au/def/organisation_classes/category/7">
	<rdf:type rdf:resource="http://www.w3.org/2000/01/rdf-schema#Resource"/>
</rdf:Description>

<rdf:Description rdf:about="http://seadatanet.maris2.nl/v_edmo/print.asp?n_code=4082">
	<rdf:type rdf:resource="http://www.w3.org/2000/01/rdf-schema#Resource"/>
</rdf:Description>

<rdf:Description rdf:about="http://seadatanet.maris2.nl/v_edmo/print.asp?n_code=4083">
	<rdf:type rdf:resource="http://www.w3.org/2000/01/rdf-schema#Resource"/>
</rdf:Description>

<rdf:Description rdf:about="http://seadatanet.maris2.nl/v_edmo/print.asp?n_code=4030">
	<rdf:type rdf:resource="http://www.w3.org/2000/01/rdf-schema#Resource"/>
</rdf:Description>

<rdf:Description rdf:about="http://seadatanet.maris2.nl/v_edmo/print.asp?n_code=3944">
	<rdf:type rdf:resource="http://www.w3.org/2000/01/rdf-schema#Resource"/>
</rdf:Description>

<rdf:Description rdf:about="http://seadatanet.maris2.nl/v_edmo/print.asp?n_code=3946">
	<rdf:type rdf:resource="http://www.w3.org/2000/01/rdf-schema#Resource"/>
</rdf:Description>

<rdf:Description rdf:about="http://seadatanet.maris2.nl/v_edmo/print.asp?n_code=4084">
	<rdf:type rdf:resource="http://www.w3.org/2000/01/rdf-schema#Resource"/>
</rdf:Description>

<rdf:Description rdf:about="http://seadatanet.maris2.nl/v_edmo/print.asp?n_code=4085">
	<rdf:type rdf:resource="http://www.w3.org/2000/01/rdf-schema#Resource"/>
</rdf:Description>

<rdf:Description rdf:about="http://seadatanet.maris2.nl/v_edmo/print.asp?n_code=4086">
	<rdf:type rdf:resource="http://www.w3.org/2000/01/rdf-schema#Resource"/>
</rdf:Description>

<rdf:Description rdf:about="http://seadatanet.maris2.nl/v_edmo/print.asp?n_code=4087">
	<rdf:type rdf:resource="http://www.w3.org/2000/01/rdf-schema#Resource"/>
</rdf:Description>

<rdf:Description rdf:about="http://seadatanet.maris2.nl/v_edmo/print.asp?n_code=4088">
	<rdf:type rdf:resource="http://www.w3.org/2000/01/rdf-schema#Resource"/>
</rdf:Description>

<rdf:Description rdf:about="http://seadatanet.maris2.nl/v_edmo/print.asp?n_code=3958">
	<rdf:type rdf:resource="http://www.w3.org/2000/01/rdf-schema#Resource"/>
</rdf:Description>

<rdf:Description rdf:about="http://seadatanet.maris2.nl/v_edmo/print.asp?n_code=3959">
	<rdf:type rdf:resource="http://www.w3.org/2000/01/rdf-schema#Resource"/>
</rdf:Description>

<rdf:Description rdf:about="http://seadatanet.maris2.nl/v_edmo/print.asp?n_code=3948">
	<rdf:type rdf:resource="http://www.w3.org/2000/01/rdf-schema#Resource"/>
</rdf:Description>

<rdf:Description rdf:about="http://seadatanet.maris2.nl/v_edmo/print.asp?n_code=3949">
	<rdf:type rdf:resource="http://www.w3.org/2000/01/rdf-schema#Resource"/>
</rdf:Description>

<rdf:Description rdf:about="http://seadatanet.maris2.nl/v_edmo/print.asp?n_code=3957">
	<rdf:type rdf:resource="http://www.w3.org/2000/01/rdf-schema#Resource"/>
</rdf:Description>

<rdf:Description rdf:about="http://vocab.aodn.org.au/def/organisation/entity/68">
	<rdf:type rdf:resource="http://www.w3.org/2000/01/rdf-schema#Resource"/>
	<rdf:type rdf:resource="http://www.w3.org/2004/02/skos/core#Concept"/>
	<dcterms:creator rdf:datatype="http://www.w3.org/2001/XMLSchema#string">Natalia Atkins</dcterms:creator>
	<dcterms:created rdf:datatype="http://www.w3.org/2001/XMLSchema#dateTime">2015-04-27T10:38:15Z</dcterms:created>
	<skos:prefLabel xml:lang="en">Cockburn Sound Management Council (CSMC), Department of Environment Regulation (DER), Western Australia Government</skos:prefLabel>
	<skos:altLabel xml:lang="en">Cockburn Sound Management Council (CSMC)</skos:altLabel>
	<skos:hiddenLabel xml:lang="en">CSMC</skos:hiddenLabel>
	<skos:definition xml:lang="en">The Cockburn Sound Management Council (CSMC) was established in August 2000 and works to implement sections 9, 10 and 11 of the State Environmental (Cockburn Sound) Policy 2005.</skos:definition>
	<dc:source rdf:datatype="http://www.w3.org/2001/XMLSchema#string">Australian Ocean Data Network Organisation Register</dc:source>
	<dc:publisher rdf:datatype="http://www.w3.org/2001/XMLSchema#string">eMarine Information Infrastructure (eMII)</dc:publisher>
	<skos:exactMatch rdf:resource="http://seadatanet.maris2.nl/v_edmo/print.asp?n_code=3965"/>
	<skos:inScheme rdf:resource="http://vocab.aodn.org.au/def/organisation/1"/>
	<skos:broader rdf:resource="http://vocab.aodn.org.au/def/organisation/entity/67"/>
</rdf:Description>

<rdf:Description rdf:about="http://seadatanet.maris2.nl/v_edmo/print.asp?n_code=3965">
	<rdf:type rdf:resource="http://www.w3.org/2000/01/rdf-schema#Resource"/>
</rdf:Description>

<rdf:Description rdf:about="http://seadatanet.maris2.nl/v_edmo/print.asp?n_code=3960">
	<rdf:type rdf:resource="http://www.w3.org/2000/01/rdf-schema#Resource"/>
</rdf:Description>

<rdf:Description rdf:about="http://seadatanet.maris2.nl/v_edmo/print.asp?n_code=3961">
	<rdf:type rdf:resource="http://www.w3.org/2000/01/rdf-schema#Resource"/>
</rdf:Description>

<rdf:Description rdf:about="http://seadatanet.maris2.nl/v_edmo/print.asp?n_code=3935">
	<rdf:type rdf:resource="http://www.w3.org/2000/01/rdf-schema#Resource"/>
</rdf:Description>

<rdf:Description rdf:about="http://seadatanet.maris2.nl/v_edmo/print.asp?n_code=4089">
	<rdf:type rdf:resource="http://www.w3.org/2000/01/rdf-schema#Resource"/>
</rdf:Description>

<rdf:Description rdf:about="http://seadatanet.maris2.nl/v_edmo/print.asp?n_code=4090">
	<rdf:type rdf:resource="http://www.w3.org/2000/01/rdf-schema#Resource"/>
</rdf:Description>

<rdf:Description rdf:about="http://seadatanet.maris2.nl/v_edmo/print.asp?n_code=4091">
	<rdf:type rdf:resource="http://www.w3.org/2000/01/rdf-schema#Resource"/>
</rdf:Description>

<rdf:Description rdf:about="http://seadatanet.maris2.nl/v_edmo/print.asp?n_code=4092">
	<rdf:type rdf:resource="http://www.w3.org/2000/01/rdf-schema#Resource"/>
</rdf:Description>

<rdf:Description rdf:about="http://seadatanet.maris2.nl/v_edmo/print.asp?n_code=4093">
	<rdf:type rdf:resource="http://www.w3.org/2000/01/rdf-schema#Resource"/>
</rdf:Description>

<rdf:Description rdf:about="http://seadatanet.maris2.nl/v_edmo/print.asp?n_code=4094">
	<rdf:type rdf:resource="http://www.w3.org/2000/01/rdf-schema#Resource"/>
</rdf:Description>

<rdf:Description rdf:about="http://seadatanet.maris2.nl/v_edmo/print.asp?n_code=4095">
	<rdf:type rdf:resource="http://www.w3.org/2000/01/rdf-schema#Resource"/>
</rdf:Description>

<rdf:Description rdf:about="http://seadatanet.maris2.nl/v_edmo/print.asp?n_code=3947">
	<rdf:type rdf:resource="http://www.w3.org/2000/01/rdf-schema#Resource"/>
</rdf:Description>

<rdf:Description rdf:about="http://seadatanet.maris2.nl/v_edmo/print.asp?n_code=4096">
	<rdf:type rdf:resource="http://www.w3.org/2000/01/rdf-schema#Resource"/>
</rdf:Description>

<rdf:Description rdf:about="http://seadatanet.maris2.nl/v_edmo/print.asp?n_code=4097">
	<rdf:type rdf:resource="http://www.w3.org/2000/01/rdf-schema#Resource"/>
</rdf:Description>

<rdf:Description rdf:about="http://seadatanet.maris2.nl/v_edmo/print.asp?n_code=4098">
	<rdf:type rdf:resource="http://www.w3.org/2000/01/rdf-schema#Resource"/>
</rdf:Description>

<rdf:Description rdf:about="http://seadatanet.maris2.nl/v_edmo/print.asp?n_code=4099">
	<rdf:type rdf:resource="http://www.w3.org/2000/01/rdf-schema#Resource"/>
</rdf:Description>

<rdf:Description rdf:about="http://seadatanet.maris2.nl/v_edmo/print.asp?n_code=4100">
	<rdf:type rdf:resource="http://www.w3.org/2000/01/rdf-schema#Resource"/>
</rdf:Description>

<rdf:Description rdf:about="http://seadatanet.maris2.nl/v_edmo/print.asp?n_code=3955">
	<rdf:type rdf:resource="http://www.w3.org/2000/01/rdf-schema#Resource"/>
</rdf:Description>

<rdf:Description rdf:about="http://seadatanet.maris2.nl/v_edmo/print.asp?n_code=3972">
	<rdf:type rdf:resource="http://www.w3.org/2000/01/rdf-schema#Resource"/>
</rdf:Description>

<rdf:Description rdf:about="http://seadatanet.maris2.nl/v_edmo/print.asp?n_code=4101">
	<rdf:type rdf:resource="http://www.w3.org/2000/01/rdf-schema#Resource"/>
</rdf:Description>

<rdf:Description rdf:about="http://seadatanet.maris2.nl/v_edmo/print.asp?n_code=4102">
	<rdf:type rdf:resource="http://www.w3.org/2000/01/rdf-schema#Resource"/>
</rdf:Description>

<rdf:Description rdf:about="http://vocab.aodn.org.au/def/organisation/entity/91">
	<rdf:type rdf:resource="http://www.w3.org/2000/01/rdf-schema#Resource"/>
	<rdf:type rdf:resource="http://www.w3.org/2004/02/skos/core#Concept"/>
	<dcterms:creator rdf:datatype="http://www.w3.org/2001/XMLSchema#string">Natalia Atkins</dcterms:creator>
	<dcterms:created rdf:datatype="http://www.w3.org/2001/XMLSchema#dateTime">2015-04-27T10:38:15Z</dcterms:created>
	<skos:broadMatch rdf:resource="http://vocab.aodn.org.au/def/organisation_classes/category/5"/>
	<skos:prefLabel xml:lang="en">INPEX Browse Ltd</skos:prefLabel>
	<skos:definition xml:lang="en">A venture company of INPEX that was created in 1998, for the Ichthys gas field development.  (Courtesy of Wikipedia)</skos:definition>
	<dc:source rdf:datatype="http://www.w3.org/2001/XMLSchema#string">Australian Ocean Data Network Organisation Register</dc:source>
	<dc:publisher rdf:datatype="http://www.w3.org/2001/XMLSchema#string">eMarine Information Infrastructure (eMII)</dc:publisher>
	<skos:exactMatch rdf:resource="http://seadatanet.maris2.nl/v_edmo/print.asp?n_code=3962"/>
	<skos:inScheme rdf:resource="http://vocab.aodn.org.au/def/organisation/1"/>
	<skos:broader rdf:resource="http://vocab.aodn.org.au/def/organisation/entity/90"/>
</rdf:Description>

<rdf:Description rdf:about="http://seadatanet.maris2.nl/v_edmo/print.asp?n_code=3962">
	<rdf:type rdf:resource="http://www.w3.org/2000/01/rdf-schema#Resource"/>
</rdf:Description>

<rdf:Description rdf:about="http://seadatanet.maris2.nl/v_edmo/print.asp?n_code=4103">
	<rdf:type rdf:resource="http://www.w3.org/2000/01/rdf-schema#Resource"/>
</rdf:Description>

<rdf:Description rdf:about="http://seadatanet.maris2.nl/v_edmo/print.asp?n_code=4104">
	<rdf:type rdf:resource="http://www.w3.org/2000/01/rdf-schema#Resource"/>
</rdf:Description>

<rdf:Description rdf:about="http://seadatanet.maris2.nl/v_edmo/print.asp?n_code=3967">
	<rdf:type rdf:resource="http://www.w3.org/2000/01/rdf-schema#Resource"/>
</rdf:Description>

<rdf:Description rdf:about="http://seadatanet.maris2.nl/v_edmo/print.asp?n_code=4105">
	<rdf:type rdf:resource="http://www.w3.org/2000/01/rdf-schema#Resource"/>
</rdf:Description>

<rdf:Description rdf:about="http://seadatanet.maris2.nl/v_edmo/print.asp?n_code=4106">
	<rdf:type rdf:resource="http://www.w3.org/2000/01/rdf-schema#Resource"/>
</rdf:Description>

<rdf:Description rdf:about="http://seadatanet.maris2.nl/v_edmo/print.asp?n_code=4107">
	<rdf:type rdf:resource="http://www.w3.org/2000/01/rdf-schema#Resource"/>
</rdf:Description>

<rdf:Description rdf:about="http://seadatanet.maris2.nl/v_edmo/print.asp?n_code=3938">
	<rdf:type rdf:resource="http://www.w3.org/2000/01/rdf-schema#Resource"/>
</rdf:Description>

<rdf:Description rdf:about="http://seadatanet.maris2.nl/v_edmo/print.asp?n_code=4025">
	<rdf:type rdf:resource="http://www.w3.org/2000/01/rdf-schema#Resource"/>
</rdf:Description>

<rdf:Description rdf:about="http://seadatanet.maris2.nl/v_edmo/print.asp?n_code=4108">
	<rdf:type rdf:resource="http://www.w3.org/2000/01/rdf-schema#Resource"/>
</rdf:Description>

<rdf:Description rdf:about="http://seadatanet.maris2.nl/v_edmo/print.asp?n_code=4109">
	<rdf:type rdf:resource="http://www.w3.org/2000/01/rdf-schema#Resource"/>
</rdf:Description>

<rdf:Description rdf:about="http://seadatanet.maris2.nl/v_edmo/print.asp?n_code=4110">
	<rdf:type rdf:resource="http://www.w3.org/2000/01/rdf-schema#Resource"/>
</rdf:Description>

<rdf:Description rdf:about="http://seadatanet.maris2.nl/v_edmo/print.asp?n_code=3970">
	<rdf:type rdf:resource="http://www.w3.org/2000/01/rdf-schema#Resource"/>
</rdf:Description>

<rdf:Description rdf:about="http://seadatanet.maris2.nl/v_edmo/print.asp?n_code=3952">
	<rdf:type rdf:resource="http://www.w3.org/2000/01/rdf-schema#Resource"/>
</rdf:Description>

<rdf:Description rdf:about="http://seadatanet.maris2.nl/v_edmo/print.asp?n_code=4111">
	<rdf:type rdf:resource="http://www.w3.org/2000/01/rdf-schema#Resource"/>
</rdf:Description>

<rdf:Description rdf:about="http://seadatanet.maris2.nl/v_edmo/print.asp?n_code=3954">
	<rdf:type rdf:resource="http://www.w3.org/2000/01/rdf-schema#Resource"/>
</rdf:Description>

<rdf:Description rdf:about="http://seadatanet.maris2.nl/v_edmo/print.asp?n_code=4112">
	<rdf:type rdf:resource="http://www.w3.org/2000/01/rdf-schema#Resource"/>
</rdf:Description>

<rdf:Description rdf:about="http://seadatanet.maris2.nl/v_edmo/print.asp?n_code=3940">
	<rdf:type rdf:resource="http://www.w3.org/2000/01/rdf-schema#Resource"/>
</rdf:Description>

<rdf:Description rdf:about="http://seadatanet.maris2.nl/v_edmo/print.asp?n_code=4113">
	<rdf:type rdf:resource="http://www.w3.org/2000/01/rdf-schema#Resource"/>
</rdf:Description>

<rdf:Description rdf:about="http://seadatanet.maris2.nl/v_edmo/print.asp?n_code=4114">
	<rdf:type rdf:resource="http://www.w3.org/2000/01/rdf-schema#Resource"/>
</rdf:Description>

<rdf:Description rdf:about="http://seadatanet.maris2.nl/v_edmo/print.asp?n_code=4115">
	<rdf:type rdf:resource="http://www.w3.org/2000/01/rdf-schema#Resource"/>
</rdf:Description>

<rdf:Description rdf:about="http://seadatanet.maris2.nl/v_edmo/print.asp?n_code=4116">
	<rdf:type rdf:resource="http://www.w3.org/2000/01/rdf-schema#Resource"/>
</rdf:Description>

<rdf:Description rdf:about="http://seadatanet.maris2.nl/v_edmo/print.asp?n_code=4117">
	<rdf:type rdf:resource="http://www.w3.org/2000/01/rdf-schema#Resource"/>
</rdf:Description>

<rdf:Description rdf:about="http://seadatanet.maris2.nl/v_edmo/print.asp?n_code=4118">
	<rdf:type rdf:resource="http://www.w3.org/2000/01/rdf-schema#Resource"/>
</rdf:Description>

<rdf:Description rdf:about="http://seadatanet.maris2.nl/v_edmo/print.asp?n_code=4119">
	<rdf:type rdf:resource="http://www.w3.org/2000/01/rdf-schema#Resource"/>
</rdf:Description>

<rdf:Description rdf:about="http://seadatanet.maris2.nl/v_edmo/print.asp?n_code=4120">
	<rdf:type rdf:resource="http://www.w3.org/2000/01/rdf-schema#Resource"/>
</rdf:Description>

<rdf:Description rdf:about="http://seadatanet.maris2.nl/v_edmo/print.asp?n_code=3953">
	<rdf:type rdf:resource="http://www.w3.org/2000/01/rdf-schema#Resource"/>
</rdf:Description>

<rdf:Description rdf:about="http://seadatanet.maris2.nl/v_edmo/print.asp?n_code=1486">
	<rdf:type rdf:resource="http://www.w3.org/2000/01/rdf-schema#Resource"/>
</rdf:Description>

<rdf:Description rdf:about="http://vocab.aodn.org.au/def/organisation/entity/123">
	<rdf:type rdf:resource="http://www.w3.org/2000/01/rdf-schema#Resource"/>
	<rdf:type rdf:resource="http://www.w3.org/2004/02/skos/core#Concept"/>
	<dcterms:creator rdf:datatype="http://www.w3.org/2001/XMLSchema#string">Natalia Atkins</dcterms:creator>
	<dcterms:created rdf:datatype="http://www.w3.org/2001/XMLSchema#dateTime">2015-04-27T10:38:15Z</dcterms:created>
	<skos:prefLabel xml:lang="en">SARDI Aquatic Sciences, South Australian Research and Development Institute (SARDI)</skos:prefLabel>
	<skos:altLabel xml:lang="en">SARDI Aquatic Sciences</skos:altLabel>
	<skos:hiddenLabel xml:lang="en"></skos:hiddenLabel>
	<skos:definition xml:lang="en">At SARDI Aquatic Sciences the major science programs covered are: Aquaculture, Fisheries, Inland Waters and Catchment Ecology, and Marine Ecosystems. Needs and opportunities for seafood value-adding, safety and market access are actively pursued through SARDI's Food Safety and Innovation science program dedicated to local food industries.</skos:definition>
	<dc:source rdf:datatype="http://www.w3.org/2001/XMLSchema#string">Australian Ocean Data Network Organisation Register</dc:source>
	<dc:publisher rdf:datatype="http://www.w3.org/2001/XMLSchema#string">eMarine Information Infrastructure (eMII)</dc:publisher>
	<skos:exactMatch rdf:resource="http://seadatanet.maris2.nl/v_edmo/print.asp?n_code=3971"/>
	<skos:inScheme rdf:resource="http://vocab.aodn.org.au/def/organisation/1"/>
	<skos:broader rdf:resource="http://vocab.aodn.org.au/def/organisation/entity/122"/>
</rdf:Description>

<rdf:Description rdf:about="http://seadatanet.maris2.nl/v_edmo/print.asp?n_code=3971">
	<rdf:type rdf:resource="http://www.w3.org/2000/01/rdf-schema#Resource"/>
</rdf:Description>

<rdf:Description rdf:about="http://seadatanet.maris2.nl/v_edmo/print.asp?n_code=3966">
	<rdf:type rdf:resource="http://www.w3.org/2000/01/rdf-schema#Resource"/>
</rdf:Description>

<rdf:Description rdf:about="http://seadatanet.maris2.nl/v_edmo/print.asp?n_code=4121">
	<rdf:type rdf:resource="http://www.w3.org/2000/01/rdf-schema#Resource"/>
</rdf:Description>

<rdf:Description rdf:about="http://seadatanet.maris2.nl/v_edmo/print.asp?n_code=4029">
	<rdf:type rdf:resource="http://www.w3.org/2000/01/rdf-schema#Resource"/>
</rdf:Description>

<rdf:Description rdf:about="http://seadatanet.maris2.nl/v_edmo/print.asp?n_code=4124">
	<rdf:type rdf:resource="http://www.w3.org/2000/01/rdf-schema#Resource"/>
</rdf:Description>

<rdf:Description rdf:about="http://seadatanet.maris2.nl/v_edmo/print.asp?n_code=4122">
	<rdf:type rdf:resource="http://www.w3.org/2000/01/rdf-schema#Resource"/>
</rdf:Description>

<rdf:Description rdf:about="http://seadatanet.maris2.nl/v_edmo/print.asp?n_code=3969">
	<rdf:type rdf:resource="http://www.w3.org/2000/01/rdf-schema#Resource"/>
</rdf:Description>

<rdf:Description rdf:about="http://seadatanet.maris2.nl/v_edmo/print.asp?n_code=3963">
	<rdf:type rdf:resource="http://www.w3.org/2000/01/rdf-schema#Resource"/>
</rdf:Description>

<rdf:Description rdf:about="http://seadatanet.maris2.nl/v_edmo/print.asp?n_code=4123">
	<rdf:type rdf:resource="http://www.w3.org/2000/01/rdf-schema#Resource"/>
</rdf:Description>

<rdf:Description rdf:about="http://seadatanet.maris2.nl/v_edmo/print.asp?n_code=3973">
	<rdf:type rdf:resource="http://www.w3.org/2000/01/rdf-schema#Resource"/>
</rdf:Description>

<rdf:Description rdf:about="http://vocab.aodn.org.au/def/organisation/entity/134">
	<rdf:type rdf:resource="http://www.w3.org/2000/01/rdf-schema#Resource"/>
	<rdf:type rdf:resource="http://www.w3.org/2004/02/skos/core#Concept"/>
	<dcterms:modified rdf:datatype="http://www.w3.org/2001/XMLSchema#dateTime">2015-07-28T05:33:33Z</dcterms:modified>
	<dcterms:creator rdf:datatype="http://www.w3.org/2001/XMLSchema#string">Natalia Atkins</dcterms:creator>
	<dcterms:created rdf:datatype="http://www.w3.org/2001/XMLSchema#dateTime">2015-04-27T10:38:15Z</dcterms:created>
	<dcterms:contributor rdf:datatype="http://www.w3.org/2001/XMLSchema#string">Natalia_Atkins</dcterms:contributor>
	<skos:prefLabel xml:lang="en">eMarine Information Infrastructure (eMII), Integrated Marine Observing Sytem (IMOS)</skos:prefLabel>
	<skos:altLabel xml:lang="en">Marine information</skos:altLabel>
	<skos:hiddenLabel xml:lang="en">eMII</skos:hiddenLabel>
	<skos:definition xml:lang="en">Marine data and information are the main products of IMOS, and data management is therefore a central element to the project's success. eMII provides a single integrative framework for data and information management that allows discovery and access of the data by scientists, managers and the public.</skos:definition>
	<dc:source rdf:datatype="http://www.w3.org/2001/XMLSchema#string">Australian Ocean Data Network Organisation Register</dc:source>
	<dc:publisher rdf:datatype="http://www.w3.org/2001/XMLSchema#string">eMarine Information Infrastructure (eMII)</dc:publisher>
	<skos:exactMatch rdf:resource="http://seadatanet.maris2.nl/v_edmo/print.asp?n_code=2454"/>
	<skos:inScheme rdf:resource="http://vocab.aodn.org.au/def/organisation/1"/>
	<skos:broader rdf:resource="http://vocab.aodn.org.au/def/organisation/entity/133"/>
</rdf:Description>

<rdf:Description rdf:about="http://vocab.aodn.org.au/def/organisation/entity/135">
	<rdf:type rdf:resource="http://www.w3.org/2000/01/rdf-schema#Resource"/>
	<rdf:type rdf:resource="http://www.w3.org/2004/02/skos/core#Concept"/>
	<dcterms:creator rdf:datatype="http://www.w3.org/2001/XMLSchema#string">Natalia Atkins</dcterms:creator>
	<dcterms:created rdf:datatype="http://www.w3.org/2001/XMLSchema#dateTime">2015-04-27T10:38:15Z</dcterms:created>
	<skos:prefLabel xml:lang="en">Argo Australia Facility, Integrated Marine Observing System (IMOS)</skos:prefLabel>
	<skos:altLabel xml:lang="en">Argo floats</skos:altLabel>
	<skos:hiddenLabel xml:lang="en">Argo</skos:hiddenLabel>
	<dc:source rdf:datatype="http://www.w3.org/2001/XMLSchema#string">Australian Ocean Data Network Organisation Register</dc:source>
	<dc:publisher rdf:datatype="http://www.w3.org/2001/XMLSchema#string">eMarine Information Infrastructure (eMII)</dc:publisher>
	<skos:inScheme rdf:resource="http://vocab.aodn.org.au/def/organisation/1"/>
	<skos:broader rdf:resource="http://vocab.aodn.org.au/def/organisation/entity/133"/>
</rdf:Description>

<rdf:Description rdf:about="http://vocab.aodn.org.au/def/organisation/entity/136">
	<rdf:type rdf:resource="http://www.w3.org/2000/01/rdf-schema#Resource"/>
	<rdf:type rdf:resource="http://www.w3.org/2004/02/skos/core#Concept"/>
	<dcterms:creator rdf:datatype="http://www.w3.org/2001/XMLSchema#string">Natalia Atkins</dcterms:creator>
	<dcterms:created rdf:datatype="http://www.w3.org/2001/XMLSchema#dateTime">2015-04-27T10:38:15Z</dcterms:created>
	<skos:prefLabel xml:lang="en">Ships of Opportunity (SOOP) Facility, Integrated Marine Observing System (IMOS)</skos:prefLabel>
	<skos:altLabel xml:lang="en">Ships of opportunity</skos:altLabel>
	<skos:hiddenLabel xml:lang="en">SOOP</skos:hiddenLabel>
	<dc:source rdf:datatype="http://www.w3.org/2001/XMLSchema#string">Australian Ocean Data Network Organisation Register</dc:source>
	<dc:publisher rdf:datatype="http://www.w3.org/2001/XMLSchema#string">eMarine Information Infrastructure (eMII)</dc:publisher>
	<skos:narrower rdf:resource="http://vocab.aodn.org.au/def/organisation/entity/137"/>
	<skos:narrower rdf:resource="http://vocab.aodn.org.au/def/organisation/entity/138"/>
	<skos:narrower rdf:resource="http://vocab.aodn.org.au/def/organisation/entity/139"/>
	<skos:narrower rdf:resource="http://vocab.aodn.org.au/def/organisation/entity/140"/>
	<skos:narrower rdf:resource="http://vocab.aodn.org.au/def/organisation/entity/141"/>
	<skos:narrower rdf:resource="http://vocab.aodn.org.au/def/organisation/entity/142"/>
	<skos:narrower rdf:resource="http://vocab.aodn.org.au/def/organisation/entity/143"/>
	<skos:narrower rdf:resource="http://vocab.aodn.org.au/def/organisation/entity/144"/>
	<skos:inScheme rdf:resource="http://vocab.aodn.org.au/def/organisation/1"/>
	<skos:broader rdf:resource="http://vocab.aodn.org.au/def/organisation/entity/133"/>
</rdf:Description>

<rdf:Description rdf:about="http://vocab.aodn.org.au/def/organisation/entity/145">
	<rdf:type rdf:resource="http://www.w3.org/2000/01/rdf-schema#Resource"/>
	<rdf:type rdf:resource="http://www.w3.org/2004/02/skos/core#Concept"/>
	<dcterms:creator rdf:datatype="http://www.w3.org/2001/XMLSchema#string">Natalia Atkins</dcterms:creator>
	<dcterms:created rdf:datatype="http://www.w3.org/2001/XMLSchema#dateTime">2015-04-27T10:38:15Z</dcterms:created>
	<skos:prefLabel xml:lang="en">Australian Bluewater Observing System (ABOS) Facility, Integrated Marine Observing System (IMOS)</skos:prefLabel>
	<skos:altLabel xml:lang="en">Deep water moorings</skos:altLabel>
	<skos:hiddenLabel xml:lang="en">ABOS</skos:hiddenLabel>
	<dc:source rdf:datatype="http://www.w3.org/2001/XMLSchema#string">Australian Ocean Data Network Organisation Register</dc:source>
	<dc:publisher rdf:datatype="http://www.w3.org/2001/XMLSchema#string">eMarine Information Infrastructure (eMII)</dc:publisher>
	<skos:narrower rdf:resource="http://vocab.aodn.org.au/def/organisation/entity/146"/>
	<skos:narrower rdf:resource="http://vocab.aodn.org.au/def/organisation/entity/147"/>
	<skos:narrower rdf:resource="http://vocab.aodn.org.au/def/organisation/entity/148"/>
	<skos:inScheme rdf:resource="http://vocab.aodn.org.au/def/organisation/1"/>
	<skos:broader rdf:resource="http://vocab.aodn.org.au/def/organisation/entity/133"/>
</rdf:Description>

<rdf:Description rdf:about="http://vocab.aodn.org.au/def/organisation/entity/149">
	<rdf:type rdf:resource="http://www.w3.org/2000/01/rdf-schema#Resource"/>
	<rdf:type rdf:resource="http://www.w3.org/2004/02/skos/core#Concept"/>
	<dcterms:creator rdf:datatype="http://www.w3.org/2001/XMLSchema#string">Natalia Atkins</dcterms:creator>
	<dcterms:created rdf:datatype="http://www.w3.org/2001/XMLSchema#dateTime">2015-04-27T10:38:15Z</dcterms:created>
	<skos:prefLabel xml:lang="en">Australian National Facility for Ocean Gliders (ANFOG), Integrated Marine Observing System (IMOS)</skos:prefLabel>
	<skos:altLabel xml:lang="en">Ocean gliders</skos:altLabel>
	<skos:hiddenLabel xml:lang="en">ANFOG</skos:hiddenLabel>
	<dc:source rdf:datatype="http://www.w3.org/2001/XMLSchema#string">Australian Ocean Data Network Organisation Register</dc:source>
	<dc:publisher rdf:datatype="http://www.w3.org/2001/XMLSchema#string">eMarine Information Infrastructure (eMII)</dc:publisher>
	<skos:inScheme rdf:resource="http://vocab.aodn.org.au/def/organisation/1"/>
	<skos:broader rdf:resource="http://vocab.aodn.org.au/def/organisation/entity/133"/>
</rdf:Description>

<rdf:Description rdf:about="http://vocab.aodn.org.au/def/organisation/entity/150">
	<rdf:type rdf:resource="http://www.w3.org/2000/01/rdf-schema#Resource"/>
	<rdf:type rdf:resource="http://www.w3.org/2004/02/skos/core#Concept"/>
	<dcterms:creator rdf:datatype="http://www.w3.org/2001/XMLSchema#string">Natalia Atkins</dcterms:creator>
	<dcterms:created rdf:datatype="http://www.w3.org/2001/XMLSchema#dateTime">2015-04-27T10:38:15Z</dcterms:created>
	<skos:prefLabel xml:lang="en">Autonomous Underwater Vehicle (AUV) Facility, Integrated Marine Observing System (IMOS)</skos:prefLabel>
	<skos:altLabel xml:lang="en">Autonomous underwater vehicle</skos:altLabel>
	<skos:hiddenLabel xml:lang="en">AUV</skos:hiddenLabel>
	<dc:source rdf:datatype="http://www.w3.org/2001/XMLSchema#string">Australian Ocean Data Network Organisation Register</dc:source>
	<dc:publisher rdf:datatype="http://www.w3.org/2001/XMLSchema#string">eMarine Information Infrastructure (eMII)</dc:publisher>
	<skos:inScheme rdf:resource="http://vocab.aodn.org.au/def/organisation/1"/>
	<skos:broader rdf:resource="http://vocab.aodn.org.au/def/organisation/entity/133"/>
</rdf:Description>

<rdf:Description rdf:about="http://vocab.aodn.org.au/def/organisation/entity/151">
	<rdf:type rdf:resource="http://www.w3.org/2000/01/rdf-schema#Resource"/>
	<rdf:type rdf:resource="http://www.w3.org/2004/02/skos/core#Concept"/>
	<dcterms:creator rdf:datatype="http://www.w3.org/2001/XMLSchema#string">Natalia Atkins</dcterms:creator>
	<dcterms:created rdf:datatype="http://www.w3.org/2001/XMLSchema#dateTime">2015-04-27T10:38:15Z</dcterms:created>
	<skos:prefLabel xml:lang="en">Australian National Mooring Network (ANMN) Facility, Integrated Marine Observing System (IMOS)</skos:prefLabel>
	<skos:altLabel xml:lang="en">National mooring network</skos:altLabel>
	<skos:hiddenLabel xml:lang="en">ANMN</skos:hiddenLabel>
	<dc:source rdf:datatype="http://www.w3.org/2001/XMLSchema#string">Australian Ocean Data Network Organisation Register</dc:source>
	<dc:publisher rdf:datatype="http://www.w3.org/2001/XMLSchema#string">eMarine Information Infrastructure (eMII)</dc:publisher>
	<skos:narrower rdf:resource="http://vocab.aodn.org.au/def/organisation/entity/152"/>
	<skos:narrower rdf:resource="http://vocab.aodn.org.au/def/organisation/entity/153"/>
	<skos:narrower rdf:resource="http://vocab.aodn.org.au/def/organisation/entity/154"/>
	<skos:narrower rdf:resource="http://vocab.aodn.org.au/def/organisation/entity/155"/>
	<skos:narrower rdf:resource="http://vocab.aodn.org.au/def/organisation/entity/156"/>
	<skos:narrower rdf:resource="http://vocab.aodn.org.au/def/organisation/entity/157"/>
	<skos:narrower rdf:resource="http://vocab.aodn.org.au/def/organisation/entity/158"/>
	<skos:inScheme rdf:resource="http://vocab.aodn.org.au/def/organisation/1"/>
	<skos:broader rdf:resource="http://vocab.aodn.org.au/def/organisation/entity/133"/>
</rdf:Description>

<rdf:Description rdf:about="http://vocab.aodn.org.au/def/organisation/entity/159">
	<rdf:type rdf:resource="http://www.w3.org/2000/01/rdf-schema#Resource"/>
	<rdf:type rdf:resource="http://www.w3.org/2004/02/skos/core#Concept"/>
	<dcterms:creator rdf:datatype="http://www.w3.org/2001/XMLSchema#string">Natalia Atkins</dcterms:creator>
	<dcterms:created rdf:datatype="http://www.w3.org/2001/XMLSchema#dateTime">2015-04-27T10:38:15Z</dcterms:created>
	<skos:prefLabel xml:lang="en">Australian Coastal Ocean Radar Network (ACORN) Facility, Integrated Marine Observing System (IMOS)</skos:prefLabel>
	<skos:altLabel xml:lang="en">Ocean radar</skos:altLabel>
	<skos:hiddenLabel xml:lang="en">ACORN</skos:hiddenLabel>
	<dc:source rdf:datatype="http://www.w3.org/2001/XMLSchema#string">Australian Ocean Data Network Organisation Register</dc:source>
	<dc:publisher rdf:datatype="http://www.w3.org/2001/XMLSchema#string">eMarine Information Infrastructure (eMII)</dc:publisher>
	<skos:inScheme rdf:resource="http://vocab.aodn.org.au/def/organisation/1"/>
	<skos:broader rdf:resource="http://vocab.aodn.org.au/def/organisation/entity/133"/>
</rdf:Description>

<rdf:Description rdf:about="http://vocab.aodn.org.au/def/organisation/entity/160">
	<rdf:type rdf:resource="http://www.w3.org/2000/01/rdf-schema#Resource"/>
	<rdf:type rdf:resource="http://www.w3.org/2004/02/skos/core#Concept"/>
	<dcterms:modified rdf:datatype="http://www.w3.org/2001/XMLSchema#dateTime">2015-09-08T00:01:54Z</dcterms:modified>
	<dcterms:creator rdf:datatype="http://www.w3.org/2001/XMLSchema#string">Natalia Atkins</dcterms:creator>
	<dcterms:created rdf:datatype="http://www.w3.org/2001/XMLSchema#dateTime">2015-04-27T10:38:15Z</dcterms:created>
	<dcterms:contributor rdf:datatype="http://www.w3.org/2001/XMLSchema#string">eMII_Atkins.Natalia</dcterms:contributor>
	<skos:prefLabel xml:lang="en">Australian Animal Tracking and Monitoring System (AATAMS) Facility, Integrated Marine Observing System (IMOS)</skos:prefLabel>
	<skos:altLabel xml:lang="en">Animal Tracking</skos:altLabel>
	<skos:hiddenLabel xml:lang="en">AATAMS</skos:hiddenLabel>
	<dc:source rdf:datatype="http://www.w3.org/2001/XMLSchema#string">Australian Ocean Data Network Organisation Register</dc:source>
	<dc:publisher rdf:datatype="http://www.w3.org/2001/XMLSchema#string">eMarine Information Infrastructure (eMII)</dc:publisher>
	<skos:inScheme rdf:resource="http://vocab.aodn.org.au/def/organisation/1"/>
	<skos:broader rdf:resource="http://vocab.aodn.org.au/def/organisation/entity/133"/>
</rdf:Description>

<rdf:Description rdf:about="http://vocab.aodn.org.au/def/organisation/entity/161">
	<rdf:type rdf:resource="http://www.w3.org/2000/01/rdf-schema#Resource"/>
	<rdf:type rdf:resource="http://www.w3.org/2004/02/skos/core#Concept"/>
	<dcterms:creator rdf:datatype="http://www.w3.org/2001/XMLSchema#string">Natalia Atkins</dcterms:creator>
	<dcterms:created rdf:datatype="http://www.w3.org/2001/XMLSchema#dateTime">2015-04-27T10:38:15Z</dcterms:created>
	<skos:prefLabel xml:lang="en">Facility for Automated Intelligent Monitoring of Marine Systems (FAIMMS), Integrated Marine Observing System (IMOS)</skos:prefLabel>
	<skos:altLabel xml:lang="en">Wireless sensor networks</skos:altLabel>
	<skos:hiddenLabel xml:lang="en">FAIMMS</skos:hiddenLabel>
	<dc:source rdf:datatype="http://www.w3.org/2001/XMLSchema#string">Australian Ocean Data Network Organisation Register</dc:source>
	<dc:publisher rdf:datatype="http://www.w3.org/2001/XMLSchema#string">eMarine Information Infrastructure (eMII)</dc:publisher>
	<skos:inScheme rdf:resource="http://vocab.aodn.org.au/def/organisation/1"/>
	<skos:broader rdf:resource="http://vocab.aodn.org.au/def/organisation/entity/133"/>
</rdf:Description>

<rdf:Description rdf:about="http://vocab.aodn.org.au/def/organisation/entity/162">
	<rdf:type rdf:resource="http://www.w3.org/2000/01/rdf-schema#Resource"/>
	<rdf:type rdf:resource="http://www.w3.org/2004/02/skos/core#Concept"/>
	<dcterms:creator rdf:datatype="http://www.w3.org/2001/XMLSchema#string">Natalia Atkins</dcterms:creator>
	<dcterms:created rdf:datatype="http://www.w3.org/2001/XMLSchema#dateTime">2015-04-27T10:38:15Z</dcterms:created>
	<skos:prefLabel xml:lang="en">Satellite Remote Sensing (SRS) Facility, Integrated Marine Observing System (IMOS)</skos:prefLabel>
	<skos:altLabel xml:lang="en">Satellite remote sensing</skos:altLabel>
	<skos:hiddenLabel xml:lang="en">SRS</skos:hiddenLabel>
	<dc:source rdf:datatype="http://www.w3.org/2001/XMLSchema#string">Australian Ocean Data Network Organisation Register</dc:source>
	<dc:publisher rdf:datatype="http://www.w3.org/2001/XMLSchema#string">eMarine Information Infrastructure (eMII)</dc:publisher>
	<skos:narrower rdf:resource="http://vocab.aodn.org.au/def/organisation/entity/163"/>
	<skos:narrower rdf:resource="http://vocab.aodn.org.au/def/organisation/entity/164"/>
	<skos:narrower rdf:resource="http://vocab.aodn.org.au/def/organisation/entity/165"/>
	<skos:narrower rdf:resource="http://vocab.aodn.org.au/def/organisation/entity/166"/>
	<skos:narrower rdf:resource="http://vocab.aodn.org.au/def/organisation/entity/167"/>
	<skos:inScheme rdf:resource="http://vocab.aodn.org.au/def/organisation/1"/>
	<skos:broader rdf:resource="http://vocab.aodn.org.au/def/organisation/entity/133"/>
</rdf:Description>

<rdf:Description rdf:about="http://seadatanet.maris2.nl/v_edmo/print.asp?n_code=2454">
	<rdf:type rdf:resource="http://www.w3.org/2000/01/rdf-schema#Resource"/>
</rdf:Description>

<rdf:Description rdf:about="http://vocab.aodn.org.au/def/organisation/entity/137">
	<rdf:type rdf:resource="http://www.w3.org/2000/01/rdf-schema#Resource"/>
	<rdf:type rdf:resource="http://www.w3.org/2004/02/skos/core#Concept"/>
	<dcterms:creator rdf:datatype="http://www.w3.org/2001/XMLSchema#string">Natalia Atkins</dcterms:creator>
	<dcterms:created rdf:datatype="http://www.w3.org/2001/XMLSchema#dateTime">2015-04-27T10:38:15Z</dcterms:created>
	<skos:prefLabel xml:lang="en">SOOP Expandable Bathythermographs (XBT) Sub-Facility, Integrated Marine Observing System (IMOS)</skos:prefLabel>
	<skos:altLabel xml:lang="en">Bathythermograph</skos:altLabel>
	<skos:hiddenLabel xml:lang="en">XBT</skos:hiddenLabel>
	<dc:source rdf:datatype="http://www.w3.org/2001/XMLSchema#string">Australian Ocean Data Network Organisation Register</dc:source>
	<dc:publisher rdf:datatype="http://www.w3.org/2001/XMLSchema#string">eMarine Information Infrastructure (eMII)</dc:publisher>
	<skos:inScheme rdf:resource="http://vocab.aodn.org.au/def/organisation/1"/>
	<skos:broader rdf:resource="http://vocab.aodn.org.au/def/organisation/entity/136"/>
</rdf:Description>

<rdf:Description rdf:about="http://vocab.aodn.org.au/def/organisation/entity/138">
	<rdf:type rdf:resource="http://www.w3.org/2000/01/rdf-schema#Resource"/>
	<rdf:type rdf:resource="http://www.w3.org/2004/02/skos/core#Concept"/>
	<dcterms:creator rdf:datatype="http://www.w3.org/2001/XMLSchema#string">Natalia Atkins</dcterms:creator>
	<dcterms:created rdf:datatype="http://www.w3.org/2001/XMLSchema#dateTime">2015-04-27T10:38:15Z</dcterms:created>
	<skos:prefLabel xml:lang="en">SOOP Biogeochemical Sensors (BGC) Sub-Facility, Integrated Marine Observing System (IMOS)</skos:prefLabel>
	<skos:altLabel xml:lang="en">Biogeochemical</skos:altLabel>
	<skos:hiddenLabel xml:lang="en">BGC</skos:hiddenLabel>
	<dc:source rdf:datatype="http://www.w3.org/2001/XMLSchema#string">Australian Ocean Data Network Organisation Register</dc:source>
	<dc:publisher rdf:datatype="http://www.w3.org/2001/XMLSchema#string">eMarine Information Infrastructure (eMII)</dc:publisher>
	<skos:inScheme rdf:resource="http://vocab.aodn.org.au/def/organisation/1"/>
	<skos:broader rdf:resource="http://vocab.aodn.org.au/def/organisation/entity/136"/>
</rdf:Description>

<rdf:Description rdf:about="http://vocab.aodn.org.au/def/organisation/entity/139">
	<rdf:type rdf:resource="http://www.w3.org/2000/01/rdf-schema#Resource"/>
	<rdf:type rdf:resource="http://www.w3.org/2004/02/skos/core#Concept"/>
	<dcterms:creator rdf:datatype="http://www.w3.org/2001/XMLSchema#string">Natalia Atkins</dcterms:creator>
	<dcterms:created rdf:datatype="http://www.w3.org/2001/XMLSchema#dateTime">2015-04-27T10:38:15Z</dcterms:created>
	<skos:prefLabel xml:lang="en">SOOP Australian Continuous Plankton Recorder (AusCPR) Sub-Facility, Integrated Marine Observing System (IMOS)</skos:prefLabel>
	<skos:altLabel xml:lang="en">Plankton recorder</skos:altLabel>
	<skos:hiddenLabel xml:lang="en">CPR</skos:hiddenLabel>
	<dc:source rdf:datatype="http://www.w3.org/2001/XMLSchema#string">Australian Ocean Data Network Organisation Register</dc:source>
	<dc:publisher rdf:datatype="http://www.w3.org/2001/XMLSchema#string">eMarine Information Infrastructure (eMII)</dc:publisher>
	<skos:inScheme rdf:resource="http://vocab.aodn.org.au/def/organisation/1"/>
	<skos:broader rdf:resource="http://vocab.aodn.org.au/def/organisation/entity/136"/>
</rdf:Description>

<rdf:Description rdf:about="http://vocab.aodn.org.au/def/organisation/entity/140">
	<rdf:type rdf:resource="http://www.w3.org/2000/01/rdf-schema#Resource"/>
	<rdf:type rdf:resource="http://www.w3.org/2004/02/skos/core#Concept"/>
	<dcterms:creator rdf:datatype="http://www.w3.org/2001/XMLSchema#string">Natalia Atkins</dcterms:creator>
	<dcterms:created rdf:datatype="http://www.w3.org/2001/XMLSchema#dateTime">2015-04-27T10:38:15Z</dcterms:created>
	<skos:prefLabel xml:lang="en">SOOP Sensors on Tropical Research Vessels (TRV) Sub-Facility, Integrated Marine Observing System (IMOS)</skos:prefLabel>
	<skos:altLabel xml:lang="en">Tropical research vessels</skos:altLabel>
	<skos:hiddenLabel xml:lang="en">Tropical</skos:hiddenLabel>
	<dc:source rdf:datatype="http://www.w3.org/2001/XMLSchema#string">Australian Ocean Data Network Organisation Register</dc:source>
	<dc:publisher rdf:datatype="http://www.w3.org/2001/XMLSchema#string">eMarine Information Infrastructure (eMII)</dc:publisher>
	<skos:inScheme rdf:resource="http://vocab.aodn.org.au/def/organisation/1"/>
	<skos:broader rdf:resource="http://vocab.aodn.org.au/def/organisation/entity/136"/>
</rdf:Description>

<rdf:Description rdf:about="http://vocab.aodn.org.au/def/organisation/entity/141">
	<rdf:type rdf:resource="http://www.w3.org/2000/01/rdf-schema#Resource"/>
	<rdf:type rdf:resource="http://www.w3.org/2004/02/skos/core#Concept"/>
	<dcterms:creator rdf:datatype="http://www.w3.org/2001/XMLSchema#string">Natalia Atkins</dcterms:creator>
	<dcterms:created rdf:datatype="http://www.w3.org/2001/XMLSchema#dateTime">2015-04-27T10:38:15Z</dcterms:created>
	<skos:prefLabel xml:lang="en">SOOP Temperate Merchant Vessel (TMV) Sub-Facility, Integrated Marine Observing System (IMOS)</skos:prefLabel>
	<skos:altLabel xml:lang="en">Temperate merchant vessels</skos:altLabel>
	<skos:hiddenLabel xml:lang="en">TMV</skos:hiddenLabel>
	<dc:source rdf:datatype="http://www.w3.org/2001/XMLSchema#string">Australian Ocean Data Network Organisation Register</dc:source>
	<dc:publisher rdf:datatype="http://www.w3.org/2001/XMLSchema#string">eMarine Information Infrastructure (eMII)</dc:publisher>
	<skos:inScheme rdf:resource="http://vocab.aodn.org.au/def/organisation/1"/>
	<skos:broader rdf:resource="http://vocab.aodn.org.au/def/organisation/entity/136"/>
</rdf:Description>

<rdf:Description rdf:about="http://vocab.aodn.org.au/def/organisation/entity/142">
	<rdf:type rdf:resource="http://www.w3.org/2000/01/rdf-schema#Resource"/>
	<rdf:type rdf:resource="http://www.w3.org/2004/02/skos/core#Concept"/>
	<dcterms:creator rdf:datatype="http://www.w3.org/2001/XMLSchema#string">Natalia Atkins</dcterms:creator>
	<dcterms:created rdf:datatype="http://www.w3.org/2001/XMLSchema#dateTime">2015-04-27T10:38:15Z</dcterms:created>
	<skos:prefLabel xml:lang="en">SOOP Sea Surface Temperature (SST) Sub-Facility, Integrated Marine Observing System (IMOS)</skos:prefLabel>
	<skos:altLabel xml:lang="en">SST vessels</skos:altLabel>
	<skos:hiddenLabel xml:lang="en">SST</skos:hiddenLabel>
	<dc:source rdf:datatype="http://www.w3.org/2001/XMLSchema#string">Australian Ocean Data Network Organisation Register</dc:source>
	<dc:publisher rdf:datatype="http://www.w3.org/2001/XMLSchema#string">eMarine Information Infrastructure (eMII)</dc:publisher>
	<skos:inScheme rdf:resource="http://vocab.aodn.org.au/def/organisation/1"/>
	<skos:broader rdf:resource="http://vocab.aodn.org.au/def/organisation/entity/136"/>
</rdf:Description>

<rdf:Description rdf:about="http://vocab.aodn.org.au/def/organisation/entity/143">
	<rdf:type rdf:resource="http://www.w3.org/2000/01/rdf-schema#Resource"/>
	<rdf:type rdf:resource="http://www.w3.org/2004/02/skos/core#Concept"/>
	<dcterms:creator rdf:datatype="http://www.w3.org/2001/XMLSchema#string">Natalia Atkins</dcterms:creator>
	<dcterms:created rdf:datatype="http://www.w3.org/2001/XMLSchema#dateTime">2015-04-27T10:38:15Z</dcterms:created>
	<skos:prefLabel xml:lang="en">SOOP Air-Sea Flux (ASF) Sub-Facility, Integrated Marine Observing System (IMOS)</skos:prefLabel>
	<skos:altLabel xml:lang="en">Air-sea flux vessels</skos:altLabel>
	<skos:hiddenLabel xml:lang="en">Flux</skos:hiddenLabel>
	<dc:source rdf:datatype="http://www.w3.org/2001/XMLSchema#string">Australian Ocean Data Network Organisation Register</dc:source>
	<dc:publisher rdf:datatype="http://www.w3.org/2001/XMLSchema#string">eMarine Information Infrastructure (eMII)</dc:publisher>
	<skos:inScheme rdf:resource="http://vocab.aodn.org.au/def/organisation/1"/>
	<skos:broader rdf:resource="http://vocab.aodn.org.au/def/organisation/entity/136"/>
</rdf:Description>

<rdf:Description rdf:about="http://vocab.aodn.org.au/def/organisation/entity/144">
	<rdf:type rdf:resource="http://www.w3.org/2000/01/rdf-schema#Resource"/>
	<rdf:type rdf:resource="http://www.w3.org/2004/02/skos/core#Concept"/>
	<dcterms:creator rdf:datatype="http://www.w3.org/2001/XMLSchema#string">Natalia Atkins</dcterms:creator>
	<dcterms:created rdf:datatype="http://www.w3.org/2001/XMLSchema#dateTime">2015-04-27T10:38:15Z</dcterms:created>
	<skos:prefLabel xml:lang="en">Bio-Acoustic Ships of Opportunity (BA SOOP) Sub-Facility,  Integrated Marine Observing System (IMOS)</skos:prefLabel>
	<skos:altLabel xml:lang="en">Bio-acoustic</skos:altLabel>
	<skos:hiddenLabel xml:lang="en">BioAcous</skos:hiddenLabel>
	<dc:source rdf:datatype="http://www.w3.org/2001/XMLSchema#string">Australian Ocean Data Network Organisation Register</dc:source>
	<dc:publisher rdf:datatype="http://www.w3.org/2001/XMLSchema#string">eMarine Information Infrastructure (eMII)</dc:publisher>
	<skos:inScheme rdf:resource="http://vocab.aodn.org.au/def/organisation/1"/>
	<skos:broader rdf:resource="http://vocab.aodn.org.au/def/organisation/entity/136"/>
</rdf:Description>

<rdf:Description rdf:about="http://vocab.aodn.org.au/def/organisation/entity/146">
	<rdf:type rdf:resource="http://www.w3.org/2000/01/rdf-schema#Resource"/>
	<rdf:type rdf:resource="http://www.w3.org/2004/02/skos/core#Concept"/>
	<dcterms:creator rdf:datatype="http://www.w3.org/2001/XMLSchema#string">Natalia Atkins</dcterms:creator>
	<dcterms:created rdf:datatype="http://www.w3.org/2001/XMLSchema#dateTime">2015-04-27T10:38:15Z</dcterms:created>
	<skos:prefLabel xml:lang="en">ABOS Air Sea Flux Station (ASFS) Sub-Facility, Integrated Marine Observing System (IMOS)</skos:prefLabel>
	<skos:altLabel xml:lang="en">Air-sea flux stations</skos:altLabel>
	<skos:hiddenLabel xml:lang="en">ASFS</skos:hiddenLabel>
	<dc:source rdf:datatype="http://www.w3.org/2001/XMLSchema#string">Australian Ocean Data Network Organisation Register</dc:source>
	<dc:publisher rdf:datatype="http://www.w3.org/2001/XMLSchema#string">eMarine Information Infrastructure (eMII)</dc:publisher>
	<skos:inScheme rdf:resource="http://vocab.aodn.org.au/def/organisation/1"/>
	<skos:broader rdf:resource="http://vocab.aodn.org.au/def/organisation/entity/145"/>
</rdf:Description>

<rdf:Description rdf:about="http://vocab.aodn.org.au/def/organisation/entity/147">
	<rdf:type rdf:resource="http://www.w3.org/2000/01/rdf-schema#Resource"/>
	<rdf:type rdf:resource="http://www.w3.org/2004/02/skos/core#Concept"/>
	<dcterms:creator rdf:datatype="http://www.w3.org/2001/XMLSchema#string">Natalia Atkins</dcterms:creator>
	<dcterms:created rdf:datatype="http://www.w3.org/2001/XMLSchema#dateTime">2015-04-27T10:38:15Z</dcterms:created>
	<skos:prefLabel xml:lang="en">ABOS Southern Ocean Time Series (SOTS) Sub-Facility, Integrated Marine Observing System (IMOS)</skos:prefLabel>
	<skos:altLabel xml:lang="en">Southern ocean time series</skos:altLabel>
	<skos:hiddenLabel xml:lang="en">SOTS</skos:hiddenLabel>
	<dc:source rdf:datatype="http://www.w3.org/2001/XMLSchema#string">Australian Ocean Data Network Organisation Register</dc:source>
	<dc:publisher rdf:datatype="http://www.w3.org/2001/XMLSchema#string">eMarine Information Infrastructure (eMII)</dc:publisher>
	<skos:inScheme rdf:resource="http://vocab.aodn.org.au/def/organisation/1"/>
	<skos:broader rdf:resource="http://vocab.aodn.org.au/def/organisation/entity/145"/>
</rdf:Description>

<rdf:Description rdf:about="http://vocab.aodn.org.au/def/organisation/entity/148">
	<rdf:type rdf:resource="http://www.w3.org/2000/01/rdf-schema#Resource"/>
	<rdf:type rdf:resource="http://www.w3.org/2004/02/skos/core#Concept"/>
	<dcterms:creator rdf:datatype="http://www.w3.org/2001/XMLSchema#string">Natalia Atkins</dcterms:creator>
	<dcterms:created rdf:datatype="http://www.w3.org/2001/XMLSchema#dateTime">2015-04-27T10:38:15Z</dcterms:created>
	<skos:prefLabel xml:lang="en">ABOS Deepwater Arrays (DA) Sub-Facility, Integrated Marine Observing System (IMOS)</skos:prefLabel>
	<skos:altLabel xml:lang="en">Deepwater arrays</skos:altLabel>
	<skos:hiddenLabel xml:lang="en">DA</skos:hiddenLabel>
	<dc:source rdf:datatype="http://www.w3.org/2001/XMLSchema#string">Australian Ocean Data Network Organisation Register</dc:source>
	<dc:publisher rdf:datatype="http://www.w3.org/2001/XMLSchema#string">eMarine Information Infrastructure (eMII)</dc:publisher>
	<skos:inScheme rdf:resource="http://vocab.aodn.org.au/def/organisation/1"/>
	<skos:broader rdf:resource="http://vocab.aodn.org.au/def/organisation/entity/145"/>
</rdf:Description>

<rdf:Description rdf:about="http://vocab.aodn.org.au/def/organisation/entity/152">
	<rdf:type rdf:resource="http://www.w3.org/2000/01/rdf-schema#Resource"/>
	<rdf:type rdf:resource="http://www.w3.org/2004/02/skos/core#Concept"/>
	<dcterms:creator rdf:datatype="http://www.w3.org/2001/XMLSchema#string">Natalia Atkins</dcterms:creator>
	<dcterms:created rdf:datatype="http://www.w3.org/2001/XMLSchema#dateTime">2015-04-27T10:38:15Z</dcterms:created>
	<skos:prefLabel xml:lang="en">ANMN Queensland and Northern Australia (QLDandNA) Moorings Sub-Facility, Integrated Marine Observing System (IMOS)</skos:prefLabel>
	<skos:altLabel xml:lang="en">QLD and NA moorings</skos:altLabel>
	<skos:hiddenLabel xml:lang="en">QLDandNA</skos:hiddenLabel>
	<dc:source rdf:datatype="http://www.w3.org/2001/XMLSchema#string">Australian Ocean Data Network Organisation Register</dc:source>
	<dc:publisher rdf:datatype="http://www.w3.org/2001/XMLSchema#string">eMarine Information Infrastructure (eMII)</dc:publisher>
	<skos:inScheme rdf:resource="http://vocab.aodn.org.au/def/organisation/1"/>
	<skos:broader rdf:resource="http://vocab.aodn.org.au/def/organisation/entity/151"/>
</rdf:Description>

<rdf:Description rdf:about="http://vocab.aodn.org.au/def/organisation/entity/153">
	<rdf:type rdf:resource="http://www.w3.org/2000/01/rdf-schema#Resource"/>
	<rdf:type rdf:resource="http://www.w3.org/2004/02/skos/core#Concept"/>
	<dcterms:creator rdf:datatype="http://www.w3.org/2001/XMLSchema#string">Natalia Atkins</dcterms:creator>
	<dcterms:created rdf:datatype="http://www.w3.org/2001/XMLSchema#dateTime">2015-04-27T10:38:15Z</dcterms:created>
	<skos:prefLabel xml:lang="en">ANMN New South Wales (NSW) Moorings Sub-Facility, Integrated Marine Observing System (IMOS)</skos:prefLabel>
	<skos:altLabel xml:lang="en">NSW moorings</skos:altLabel>
	<skos:hiddenLabel xml:lang="en">NSW</skos:hiddenLabel>
	<dc:source rdf:datatype="http://www.w3.org/2001/XMLSchema#string">Australian Ocean Data Network Organisation Register</dc:source>
	<dc:publisher rdf:datatype="http://www.w3.org/2001/XMLSchema#string">eMarine Information Infrastructure (eMII)</dc:publisher>
	<skos:inScheme rdf:resource="http://vocab.aodn.org.au/def/organisation/1"/>
	<skos:broader rdf:resource="http://vocab.aodn.org.au/def/organisation/entity/151"/>
</rdf:Description>

<rdf:Description rdf:about="http://vocab.aodn.org.au/def/organisation/entity/154">
	<rdf:type rdf:resource="http://www.w3.org/2000/01/rdf-schema#Resource"/>
	<rdf:type rdf:resource="http://www.w3.org/2004/02/skos/core#Concept"/>
	<dcterms:creator rdf:datatype="http://www.w3.org/2001/XMLSchema#string">Natalia Atkins</dcterms:creator>
	<dcterms:created rdf:datatype="http://www.w3.org/2001/XMLSchema#dateTime">2015-04-27T10:38:15Z</dcterms:created>
	<skos:prefLabel xml:lang="en">ANMN South Australia (SA) Moorings Sub-Facility, Integrated Marine Observing System (IMOS)</skos:prefLabel>
	<skos:altLabel xml:lang="en">SA moorings</skos:altLabel>
	<skos:hiddenLabel xml:lang="en">SA</skos:hiddenLabel>
	<dc:source rdf:datatype="http://www.w3.org/2001/XMLSchema#string">Australian Ocean Data Network Organisation Register</dc:source>
	<dc:publisher rdf:datatype="http://www.w3.org/2001/XMLSchema#string">eMarine Information Infrastructure (eMII)</dc:publisher>
	<skos:inScheme rdf:resource="http://vocab.aodn.org.au/def/organisation/1"/>
	<skos:broader rdf:resource="http://vocab.aodn.org.au/def/organisation/entity/151"/>
</rdf:Description>

<rdf:Description rdf:about="http://vocab.aodn.org.au/def/organisation/entity/155">
	<rdf:type rdf:resource="http://www.w3.org/2000/01/rdf-schema#Resource"/>
	<rdf:type rdf:resource="http://www.w3.org/2004/02/skos/core#Concept"/>
	<dcterms:creator rdf:datatype="http://www.w3.org/2001/XMLSchema#string">Natalia Atkins</dcterms:creator>
	<dcterms:created rdf:datatype="http://www.w3.org/2001/XMLSchema#dateTime">2015-04-27T10:38:15Z</dcterms:created>
	<skos:prefLabel xml:lang="en">ANMN Western Australia (WA) Moorings Sub-Facility, Integrated Marine Observing System (IMOS)</skos:prefLabel>
	<skos:altLabel xml:lang="en">WA moorings</skos:altLabel>
	<skos:hiddenLabel xml:lang="en">WA</skos:hiddenLabel>
	<dc:source rdf:datatype="http://www.w3.org/2001/XMLSchema#string">Australian Ocean Data Network Organisation Register</dc:source>
	<dc:publisher rdf:datatype="http://www.w3.org/2001/XMLSchema#string">eMarine Information Infrastructure (eMII)</dc:publisher>
	<skos:inScheme rdf:resource="http://vocab.aodn.org.au/def/organisation/1"/>
	<skos:broader rdf:resource="http://vocab.aodn.org.au/def/organisation/entity/151"/>
</rdf:Description>

<rdf:Description rdf:about="http://vocab.aodn.org.au/def/organisation/entity/156">
	<rdf:type rdf:resource="http://www.w3.org/2000/01/rdf-schema#Resource"/>
	<rdf:type rdf:resource="http://www.w3.org/2004/02/skos/core#Concept"/>
	<dcterms:creator rdf:datatype="http://www.w3.org/2001/XMLSchema#string">Natalia Atkins</dcterms:creator>
	<dcterms:created rdf:datatype="http://www.w3.org/2001/XMLSchema#dateTime">2015-04-27T10:38:15Z</dcterms:created>
	<skos:prefLabel xml:lang="en">ANMN Passive Acoustic Observatories Sub-Facility, Integrated Marine Observing System (IMOS)</skos:prefLabel>
	<skos:altLabel xml:lang="en">Acoustic observations</skos:altLabel>
	<skos:hiddenLabel xml:lang="en">Acoustic</skos:hiddenLabel>
	<dc:source rdf:datatype="http://www.w3.org/2001/XMLSchema#string">Australian Ocean Data Network Organisation Register</dc:source>
	<dc:publisher rdf:datatype="http://www.w3.org/2001/XMLSchema#string">eMarine Information Infrastructure (eMII)</dc:publisher>
	<skos:inScheme rdf:resource="http://vocab.aodn.org.au/def/organisation/1"/>
	<skos:broader rdf:resource="http://vocab.aodn.org.au/def/organisation/entity/151"/>
</rdf:Description>

<rdf:Description rdf:about="http://vocab.aodn.org.au/def/organisation/entity/157">
	<rdf:type rdf:resource="http://www.w3.org/2000/01/rdf-schema#Resource"/>
	<rdf:type rdf:resource="http://www.w3.org/2004/02/skos/core#Concept"/>
	<dcterms:creator rdf:datatype="http://www.w3.org/2001/XMLSchema#string">Natalia Atkins</dcterms:creator>
	<dcterms:created rdf:datatype="http://www.w3.org/2001/XMLSchema#dateTime">2015-04-27T10:38:15Z</dcterms:created>
	<skos:prefLabel xml:lang="en">ANMN National Reference Stations (NRS) Sub-Facility, Integrated Marine Observing System (IMOS)</skos:prefLabel>
	<skos:altLabel xml:lang="en">National reference stations</skos:altLabel>
	<skos:hiddenLabel xml:lang="en">NRS</skos:hiddenLabel>
	<dc:source rdf:datatype="http://www.w3.org/2001/XMLSchema#string">Australian Ocean Data Network Organisation Register</dc:source>
	<dc:publisher rdf:datatype="http://www.w3.org/2001/XMLSchema#string">eMarine Information Infrastructure (eMII)</dc:publisher>
	<skos:inScheme rdf:resource="http://vocab.aodn.org.au/def/organisation/1"/>
	<skos:broader rdf:resource="http://vocab.aodn.org.au/def/organisation/entity/151"/>
</rdf:Description>

<rdf:Description rdf:about="http://vocab.aodn.org.au/def/organisation/entity/158">
	<rdf:type rdf:resource="http://www.w3.org/2000/01/rdf-schema#Resource"/>
	<rdf:type rdf:resource="http://www.w3.org/2004/02/skos/core#Concept"/>
	<dcterms:creator rdf:datatype="http://www.w3.org/2001/XMLSchema#string">Natalia Atkins</dcterms:creator>
	<dcterms:created rdf:datatype="http://www.w3.org/2001/XMLSchema#dateTime">2015-04-27T10:38:15Z</dcterms:created>
	<skos:prefLabel xml:lang="en">ANMN Acidification Moorings (AM) Sub-Facility, Integrated Marine Observing System (IMOS)</skos:prefLabel>
	<skos:altLabel xml:lang="en">Acidification moorings</skos:altLabel>
	<skos:hiddenLabel xml:lang="en">CO2</skos:hiddenLabel>
	<dc:source rdf:datatype="http://www.w3.org/2001/XMLSchema#string">Australian Ocean Data Network Organisation Register</dc:source>
	<dc:publisher rdf:datatype="http://www.w3.org/2001/XMLSchema#string">eMarine Information Infrastructure (eMII)</dc:publisher>
	<skos:inScheme rdf:resource="http://vocab.aodn.org.au/def/organisation/1"/>
	<skos:broader rdf:resource="http://vocab.aodn.org.au/def/organisation/entity/151"/>
</rdf:Description>

<rdf:Description rdf:about="http://vocab.aodn.org.au/def/organisation/entity/163">
	<rdf:type rdf:resource="http://www.w3.org/2000/01/rdf-schema#Resource"/>
	<rdf:type rdf:resource="http://www.w3.org/2004/02/skos/core#Concept"/>
	<dcterms:creator rdf:datatype="http://www.w3.org/2001/XMLSchema#string">Natalia Atkins</dcterms:creator>
	<dcterms:created rdf:datatype="http://www.w3.org/2001/XMLSchema#dateTime">2015-04-27T10:38:15Z</dcterms:created>
	<skos:prefLabel xml:lang="en">SRS Satellite Sea Surface Temperature (SST) Sub-Facility, Integrated Marine Observing System (IMOS)</skos:prefLabel>
	<skos:altLabel xml:lang="en">Satellite SST L2P</skos:altLabel>
	<skos:hiddenLabel xml:lang="en">SST L2P</skos:hiddenLabel>
	<dc:source rdf:datatype="http://www.w3.org/2001/XMLSchema#string">Australian Ocean Data Network Organisation Register</dc:source>
	<dc:publisher rdf:datatype="http://www.w3.org/2001/XMLSchema#string">eMarine Information Infrastructure (eMII)</dc:publisher>
	<skos:inScheme rdf:resource="http://vocab.aodn.org.au/def/organisation/1"/>
	<skos:broader rdf:resource="http://vocab.aodn.org.au/def/organisation/entity/162"/>
</rdf:Description>

<rdf:Description rdf:about="http://vocab.aodn.org.au/def/organisation/entity/164">
	<rdf:type rdf:resource="http://www.w3.org/2000/01/rdf-schema#Resource"/>
	<rdf:type rdf:resource="http://www.w3.org/2004/02/skos/core#Concept"/>
	<dcterms:creator rdf:datatype="http://www.w3.org/2001/XMLSchema#string">Natalia Atkins</dcterms:creator>
	<dcterms:created rdf:datatype="http://www.w3.org/2001/XMLSchema#dateTime">2015-04-27T10:38:15Z</dcterms:created>
	<skos:prefLabel xml:lang="en">SRS MODIS Aqua OC3 Chlorophyll-a - Ocean Colour, Integrated Marine Observing System (IMOS)</skos:prefLabel>
	<skos:altLabel xml:lang="en">Ocean colour</skos:altLabel>
	<skos:hiddenLabel xml:lang="en">OceanColour</skos:hiddenLabel>
	<dc:source rdf:datatype="http://www.w3.org/2001/XMLSchema#string">Australian Ocean Data Network Organisation Register</dc:source>
	<dc:publisher rdf:datatype="http://www.w3.org/2001/XMLSchema#string">eMarine Information Infrastructure (eMII)</dc:publisher>
	<skos:inScheme rdf:resource="http://vocab.aodn.org.au/def/organisation/1"/>
	<skos:broader rdf:resource="http://vocab.aodn.org.au/def/organisation/entity/162"/>
</rdf:Description>

<rdf:Description rdf:about="http://vocab.aodn.org.au/def/organisation/entity/165">
	<rdf:type rdf:resource="http://www.w3.org/2000/01/rdf-schema#Resource"/>
	<rdf:type rdf:resource="http://www.w3.org/2004/02/skos/core#Concept"/>
	<dcterms:creator rdf:datatype="http://www.w3.org/2001/XMLSchema#string">Natalia Atkins</dcterms:creator>
	<dcterms:created rdf:datatype="http://www.w3.org/2001/XMLSchema#dateTime">2015-04-27T10:38:15Z</dcterms:created>
	<skos:prefLabel xml:lang="en">SRS Satellite Altimetry Calibration and Validation Sub-Facility, Integrated Marine Observing System (IMOS)</skos:prefLabel>
	<skos:altLabel xml:lang="en">Satellite altimetry</skos:altLabel>
	<skos:hiddenLabel xml:lang="en">SatAltim</skos:hiddenLabel>
	<dc:source rdf:datatype="http://www.w3.org/2001/XMLSchema#string">Australian Ocean Data Network Organisation Register</dc:source>
	<dc:publisher rdf:datatype="http://www.w3.org/2001/XMLSchema#string">eMarine Information Infrastructure (eMII)</dc:publisher>
	<skos:inScheme rdf:resource="http://vocab.aodn.org.au/def/organisation/1"/>
	<skos:broader rdf:resource="http://vocab.aodn.org.au/def/organisation/entity/162"/>
</rdf:Description>

<rdf:Description rdf:about="http://vocab.aodn.org.au/def/organisation/entity/166">
	<rdf:type rdf:resource="http://www.w3.org/2000/01/rdf-schema#Resource"/>
	<rdf:type rdf:resource="http://www.w3.org/2004/02/skos/core#Concept"/>
	<dcterms:creator rdf:datatype="http://www.w3.org/2001/XMLSchema#string">Natalia Atkins</dcterms:creator>
	<dcterms:created rdf:datatype="http://www.w3.org/2001/XMLSchema#dateTime">2015-04-27T10:38:15Z</dcterms:created>
	<skos:prefLabel xml:lang="en">SRS Bio-Optical data base of Australian Waters (SRS-OC-BODBAW), Integrated Marine Observing System (IMOS)</skos:prefLabel>
	<skos:altLabel xml:lang="en">Bio-Optical</skos:altLabel>
	<skos:hiddenLabel xml:lang="en">BODBAW</skos:hiddenLabel>
	<dc:source rdf:datatype="http://www.w3.org/2001/XMLSchema#string">Australian Ocean Data Network Organisation Register</dc:source>
	<dc:publisher rdf:datatype="http://www.w3.org/2001/XMLSchema#string">eMarine Information Infrastructure (eMII)</dc:publisher>
	<skos:inScheme rdf:resource="http://vocab.aodn.org.au/def/organisation/1"/>
	<skos:broader rdf:resource="http://vocab.aodn.org.au/def/organisation/entity/162"/>
</rdf:Description>

<rdf:Description rdf:about="http://vocab.aodn.org.au/def/organisation/entity/167">
	<rdf:type rdf:resource="http://www.w3.org/2000/01/rdf-schema#Resource"/>
	<rdf:type rdf:resource="http://www.w3.org/2004/02/skos/core#Concept"/>
	<dcterms:creator rdf:datatype="http://www.w3.org/2001/XMLSchema#string">Natalia Atkins</dcterms:creator>
	<dcterms:created rdf:datatype="http://www.w3.org/2001/XMLSchema#dateTime">2015-04-27T10:38:15Z</dcterms:created>
	<skos:prefLabel xml:lang="en">SRS Satellite Ocean Colour Calibration (SOCC) Sub-Facility, Lucinda Jetty Coastal Observatory (LJCO), Integrated Marine Observing System (IMOS)</skos:prefLabel>
	<skos:altLabel xml:lang="en">Ocean colour calibration</skos:altLabel>
	<skos:hiddenLabel xml:lang="en">SOCC</skos:hiddenLabel>
	<dc:source rdf:datatype="http://www.w3.org/2001/XMLSchema#string">Australian Ocean Data Network Organisation Register</dc:source>
	<dc:publisher rdf:datatype="http://www.w3.org/2001/XMLSchema#string">eMarine Information Infrastructure (eMII)</dc:publisher>
	<skos:inScheme rdf:resource="http://vocab.aodn.org.au/def/organisation/1"/>
	<skos:broader rdf:resource="http://vocab.aodn.org.au/def/organisation/entity/162"/>
</rdf:Description>

<rdf:Description rdf:about="http://seadatanet.maris2.nl/v_edmo/print.asp?n_code=4187">
	<rdf:type rdf:resource="http://www.w3.org/2000/01/rdf-schema#Resource"/>
</rdf:Description>

<rdf:Description rdf:about="http://seadatanet.maris2.nl/v_edmo/print.asp?n_code=4188">
	<rdf:type rdf:resource="http://www.w3.org/2000/01/rdf-schema#Resource"/>
</rdf:Description>

<rdf:Description rdf:about="http://seadatanet.maris2.nl/v_edmo/print.asp?n_code=4189">
	<rdf:type rdf:resource="http://www.w3.org/2000/01/rdf-schema#Resource"/>
</rdf:Description>

<rdf:Description rdf:about="http://seadatanet.maris2.nl/v_edmo/print.asp?n_code=4190">
	<rdf:type rdf:resource="http://www.w3.org/2000/01/rdf-schema#Resource"/>
</rdf:Description>

<rdf:Description rdf:about="http://seadatanet.maris2.nl/v_edmo/print.asp?n_code=4191">
	<rdf:type rdf:resource="http://www.w3.org/2000/01/rdf-schema#Resource"/>
</rdf:Description>

<rdf:Description rdf:about="http://seadatanet.maris2.nl/v_edmo/print.asp?n_code=4186">
	<rdf:type rdf:resource="http://www.w3.org/2000/01/rdf-schema#Resource"/>
</rdf:Description>

<rdf:Description rdf:about="http://vocab.aodn.org.au/def/organisation/entity/180">
	<rdf:type rdf:resource="http://www.w3.org/2000/01/rdf-schema#Resource"/>
	<rdf:type rdf:resource="http://www.w3.org/2004/02/skos/core#Concept"/>
	<dcterms:modified rdf:datatype="http://www.w3.org/2001/XMLSchema#dateTime">2015-07-09T05:52:13Z</dcterms:modified>
	<dcterms:creator rdf:datatype="http://www.w3.org/2001/XMLSchema#string">Natalia Atkins</dcterms:creator>
	<dcterms:created rdf:datatype="http://www.w3.org/2001/XMLSchema#dateTime">2015-07-08T10:38:15Z</dcterms:created>
	<dcterms:contributor rdf:datatype="http://www.w3.org/2001/XMLSchema#string">Natalia_Atkins</dcterms:contributor>
	<skos:prefLabel xml:lang="en">School of Environmental Biology, Curtin University of Technology</skos:prefLabel>
	<skos:altLabel xml:lang="en"></skos:altLabel>
	<skos:altLabel xml:lang="en">School of Environmental Biology</skos:altLabel>
	<skos:hiddenLabel xml:lang="en"></skos:hiddenLabel>
	<skos:definition xml:lang="en">The School of Environmental Biology, existed between approximately 1995 and 2003. It changed its name to the Department of Environmental Biology.</skos:definition>
	<dc:source rdf:datatype="http://www.w3.org/2001/XMLSchema#string">Australian Ocean Data Network Organisation Register</dc:source>
	<dc:publisher rdf:datatype="http://www.w3.org/2001/XMLSchema#string">eMarine Information Infrastructure (eMII)</dc:publisher>
	<skos:inScheme rdf:resource="http://vocab.aodn.org.au/def/organisation/1"/>
	<skos:broader rdf:resource="http://vocab.aodn.org.au/def/organisation/entity/178"/>
	<skos:scopeNote xml:lang="en">Organisation no longer exists</skos:scopeNote>
	<skos:scopeNote xml:lang="en">Organisation no longer exists. Replaced by http://vocab.aodn.org.au/def/organisation/entity/181</skos:scopeNote>
	<dcterms:isReplacedBy rdf:resource="http://vocab.aodn.org.au/def/organisation/entity/181"/>
	<dcterms:isReplacedBy xml:lang="en">Department of Environmental Biology, Curtin University of Technology</dcterms:isReplacedBy>
</rdf:Description>

<rdf:Description rdf:about="http://vocab.aodn.org.au/def/organisation/entity/181">
	<rdf:type rdf:resource="http://www.w3.org/2000/01/rdf-schema#Resource"/>
	<rdf:type rdf:resource="http://www.w3.org/2004/02/skos/core#Concept"/>
	<dcterms:modified rdf:datatype="http://www.w3.org/2001/XMLSchema#dateTime">2015-07-09T05:51:29Z</dcterms:modified>
	<dcterms:creator rdf:datatype="http://www.w3.org/2001/XMLSchema#string">Natalia Atkins</dcterms:creator>
	<dcterms:created rdf:datatype="http://www.w3.org/2001/XMLSchema#dateTime">2015-07-08T10:38:15Z</dcterms:created>
	<dcterms:contributor rdf:datatype="http://www.w3.org/2001/XMLSchema#string">Natalia_Atkins</dcterms:contributor>
	<skos:prefLabel xml:lang="en">Department of Environmental Biology, Curtin University of Technology</skos:prefLabel>
	<skos:altLabel xml:lang="en"></skos:altLabel>
	<skos:altLabel xml:lang="en">Department of Environmental Biology</skos:altLabel>
	<skos:hiddenLabel xml:lang="en"></skos:hiddenLabel>
	<skos:definition xml:lang="en">The Department of Environmental Biology, existed between approximately 2005 and 2009. It is now known as the Department of Environment and Agriculture.</skos:definition>
	<dc:source rdf:datatype="http://www.w3.org/2001/XMLSchema#string">Australian Ocean Data Network Organisation Register</dc:source>
	<dc:publisher rdf:datatype="http://www.w3.org/2001/XMLSchema#string">eMarine Information Infrastructure (eMII)</dc:publisher>
	<skos:inScheme rdf:resource="http://vocab.aodn.org.au/def/organisation/1"/>
	<skos:broader rdf:resource="http://vocab.aodn.org.au/def/organisation/entity/178"/>
	<skos:scopeNote xml:lang="en">Organisation no longer exists</skos:scopeNote>
	<skos:scopeNote xml:lang="en">Organisation no longer exists. Replaced by http://vocab.aodn.org.au/def/organisation/entity/182. Replaces http://vocab.aodn.org.au/def/organisation/entity/180</skos:scopeNote>
	<dcterms:replaces rdf:resource="http://vocab.aodn.org.au/def/organisation/entity/180"/>
	<dcterms:replaces xml:lang="en">School of Environmental Biology, Curtin University of Technology</dcterms:replaces>
	<dcterms:isReplacedBy rdf:resource="http://vocab.aodn.org.au/def/organisation/entity/182"/>
	<dcterms:isReplacedBy xml:lang="en">Department of Environment and Agriculture, Curtin University</dcterms:isReplacedBy>
</rdf:Description>

<rdf:Description rdf:about="http://vocab.aodn.org.au/def/organisation/entity/182">
	<rdf:type rdf:resource="http://www.w3.org/2000/01/rdf-schema#Resource"/>
	<rdf:type rdf:resource="http://www.w3.org/2004/02/skos/core#Concept"/>
	<dcterms:modified rdf:datatype="http://www.w3.org/2001/XMLSchema#dateTime">2015-07-09T05:51:16Z</dcterms:modified>
	<dcterms:creator rdf:datatype="http://www.w3.org/2001/XMLSchema#string">Natalia Atkins</dcterms:creator>
	<dcterms:created rdf:datatype="http://www.w3.org/2001/XMLSchema#dateTime">2015-07-08T10:38:15Z</dcterms:created>
	<dcterms:contributor rdf:datatype="http://www.w3.org/2001/XMLSchema#string">Natalia_Atkins</dcterms:contributor>
	<skos:prefLabel xml:lang="en">Department of Environment and Agriculture, Curtin University</skos:prefLabel>
	<skos:altLabel xml:lang="en"></skos:altLabel>
	<skos:altLabel xml:lang="en">Department of Environment and Agriculture</skos:altLabel>
	<skos:hiddenLabel xml:lang="en"></skos:hiddenLabel>
	<skos:definition xml:lang="en">The Department of Environment and Agriculture caters for students who are interested in agriculture, biology, conserving biodiversity and the environment, or management of the coastal zone.</skos:definition>
	<dc:source rdf:datatype="http://www.w3.org/2001/XMLSchema#string">Australian Ocean Data Network Organisation Register</dc:source>
	<dc:publisher rdf:datatype="http://www.w3.org/2001/XMLSchema#string">eMarine Information Infrastructure (eMII)</dc:publisher>
	<skos:exactMatch rdf:resource="http://seadatanet.maris2.nl/v_edmo/print.asp?n_code=4255"/>
	<skos:inScheme rdf:resource="http://vocab.aodn.org.au/def/organisation/1"/>
	<skos:broader rdf:resource="http://vocab.aodn.org.au/def/organisation/entity/178"/>
	<skos:scopeNote xml:lang="en">Replaces http://vocab.aodn.org.au/def/organisation/entity/181</skos:scopeNote>
	<dcterms:replaces rdf:resource="http://vocab.aodn.org.au/def/organisation/entity/181"/>
	<dcterms:replaces xml:lang="en">Department of Environmental Biology, Curtin University of Technology</dcterms:replaces>
</rdf:Description>

<rdf:Description rdf:about="http://seadatanet.maris2.nl/v_edmo/print.asp?n_code=4255">
	<rdf:type rdf:resource="http://www.w3.org/2000/01/rdf-schema#Resource"/>
</rdf:Description>

<rdf:Description rdf:about="http://vocab.aodn.org.au/def/organisation/entity/183">
	<rdf:type rdf:resource="http://www.w3.org/2000/01/rdf-schema#Resource"/>
	<rdf:type rdf:resource="http://www.w3.org/2004/02/skos/core#Concept"/>
	<dcterms:modified rdf:datatype="http://www.w3.org/2001/XMLSchema#dateTime">2015-07-09T05:51:03Z</dcterms:modified>
	<dcterms:creator rdf:datatype="http://www.w3.org/2001/XMLSchema#string">Natalia Atkins</dcterms:creator>
	<dcterms:created rdf:datatype="http://www.w3.org/2001/XMLSchema#dateTime">2015-07-08T10:38:15Z</dcterms:created>
	<dcterms:contributor rdf:datatype="http://www.w3.org/2001/XMLSchema#string">Natalia_Atkins</dcterms:contributor>
	<skos:prefLabel xml:lang="en">Department of Applied Geology, Curtin University</skos:prefLabel>
	<skos:altLabel xml:lang="en"></skos:altLabel>
	<skos:altLabel xml:lang="en">Department of Applied Geology</skos:altLabel>
	<skos:hiddenLabel xml:lang="en"></skos:hiddenLabel>
	<skos:definition xml:lang="en">The Department of Applied Geology is part of the Western Australian School of Mines, one of six schools in Curtin's Faculty of Science and Engineering, and is one of Australia's leading providers of geoscience education and research. It is located at Curtin's metropolitan Bentley Campus and in Kalgoorlie at the heart of the West Australian goldfields. The present Department formed in 2006 when the Bentley-based Department of Applied Geology merged with the WA School of Mines.</skos:definition>
	<dc:source rdf:datatype="http://www.w3.org/2001/XMLSchema#string">Australian Ocean Data Network Organisation Register</dc:source>
	<dc:publisher rdf:datatype="http://www.w3.org/2001/XMLSchema#string">eMarine Information Infrastructure (eMII)</dc:publisher>
	<skos:exactMatch rdf:resource="http://seadatanet.maris2.nl/v_edmo/print.asp?n_code=4256"/>
	<skos:inScheme rdf:resource="http://vocab.aodn.org.au/def/organisation/1"/>
	<skos:broader rdf:resource="http://vocab.aodn.org.au/def/organisation/entity/178"/>
</rdf:Description>

<rdf:Description rdf:about="http://seadatanet.maris2.nl/v_edmo/print.asp?n_code=4256">
	<rdf:type rdf:resource="http://www.w3.org/2000/01/rdf-schema#Resource"/>
</rdf:Description>

<rdf:Description rdf:about="http://vocab.aodn.org.au/def/organisation/entity/184">
	<rdf:type rdf:resource="http://www.w3.org/2000/01/rdf-schema#Resource"/>
	<rdf:type rdf:resource="http://www.w3.org/2004/02/skos/core#Concept"/>
	<dcterms:modified rdf:datatype="http://www.w3.org/2001/XMLSchema#dateTime">2015-07-09T05:52:36Z</dcterms:modified>
	<dcterms:creator rdf:datatype="http://www.w3.org/2001/XMLSchema#string">Natalia Atkins</dcterms:creator>
	<dcterms:created rdf:datatype="http://www.w3.org/2001/XMLSchema#dateTime">2015-07-08T10:38:15Z</dcterms:created>
	<dcterms:contributor rdf:datatype="http://www.w3.org/2001/XMLSchema#string">Natalia_Atkins</dcterms:contributor>
	<skos:prefLabel xml:lang="en">School of Surveying and Land Information, Curtin University of Technology</skos:prefLabel>
	<skos:altLabel xml:lang="en"></skos:altLabel>
	<skos:altLabel xml:lang="en">School of Surveying and Land Information</skos:altLabel>
	<skos:hiddenLabel xml:lang="en"></skos:hiddenLabel>
	<skos:definition xml:lang="en">The School of Surveying and Land Information, changed its name to the School of Spatial Sciences, Curtin University of Technology in 1997. It is now known as the Department of Spatial Sciences, Curtin University.</skos:definition>
	<dc:source rdf:datatype="http://www.w3.org/2001/XMLSchema#string">Australian Ocean Data Network Organisation Register</dc:source>
	<dc:publisher rdf:datatype="http://www.w3.org/2001/XMLSchema#string">eMarine Information Infrastructure (eMII)</dc:publisher>
	<skos:inScheme rdf:resource="http://vocab.aodn.org.au/def/organisation/1"/>
	<skos:broader rdf:resource="http://vocab.aodn.org.au/def/organisation/entity/178"/>
	<skos:scopeNote xml:lang="en">Organisation no longer exists</skos:scopeNote>
	<skos:scopeNote xml:lang="en">Organisation no longer exists. Replaced by http://vocab.aodn.org.au/def/organisation/entity/185</skos:scopeNote>
	<dcterms:isReplacedBy rdf:resource="http://vocab.aodn.org.au/def/organisation/entity/185"/>
	<dcterms:isReplacedBy xml:lang="en">Department of Spatial Sciences, Curtin University</dcterms:isReplacedBy>
</rdf:Description>

<rdf:Description rdf:about="http://vocab.aodn.org.au/def/organisation/entity/185">
	<rdf:type rdf:resource="http://www.w3.org/2000/01/rdf-schema#Resource"/>
	<rdf:type rdf:resource="http://www.w3.org/2004/02/skos/core#Concept"/>
	<dcterms:modified rdf:datatype="http://www.w3.org/2001/XMLSchema#dateTime">2015-07-09T05:50:34Z</dcterms:modified>
	<dcterms:creator rdf:datatype="http://www.w3.org/2001/XMLSchema#string">Natalia Atkins</dcterms:creator>
	<dcterms:created rdf:datatype="http://www.w3.org/2001/XMLSchema#dateTime">2015-07-08T10:38:15Z</dcterms:created>
	<dcterms:contributor rdf:datatype="http://www.w3.org/2001/XMLSchema#string">Natalia_Atkins</dcterms:contributor>
	<skos:prefLabel xml:lang="en">Department of Spatial Sciences, Curtin University</skos:prefLabel>
	<skos:altLabel xml:lang="en"></skos:altLabel>
	<skos:altLabel xml:lang="en">Department of Spatial Sciences</skos:altLabel>
	<skos:hiddenLabel xml:lang="en"></skos:hiddenLabel>
	<skos:definition xml:lang="en">Spatial sciences involves a range of disciplines focussed around location on the Earth's (or moon's) surface including, but not limited to, surveying, geographic information science (GISc), global navigation and satellite systems (GNSS), geodesy, photogrammetry and laser scanning, and remote sensing.</skos:definition>
	<dc:source rdf:datatype="http://www.w3.org/2001/XMLSchema#string">Australian Ocean Data Network Organisation Register</dc:source>
	<dc:publisher rdf:datatype="http://www.w3.org/2001/XMLSchema#string">eMarine Information Infrastructure (eMII)</dc:publisher>
	<skos:exactMatch rdf:resource="http://seadatanet.maris2.nl/v_edmo/print.asp?n_code=4257"/>
	<skos:inScheme rdf:resource="http://vocab.aodn.org.au/def/organisation/1"/>
	<skos:broader rdf:resource="http://vocab.aodn.org.au/def/organisation/entity/178"/>
	<skos:scopeNote xml:lang="en">Replaces http://vocab.aodn.org.au/def/organisation/entity/184</skos:scopeNote>
	<dcterms:replaces rdf:resource="http://vocab.aodn.org.au/def/organisation/entity/184"/>
	<dcterms:replaces xml:lang="en">School of Surveying and Land Information, Curtin University of Technology</dcterms:replaces>
</rdf:Description>

<rdf:Description rdf:about="http://seadatanet.maris2.nl/v_edmo/print.asp?n_code=4257">
	<rdf:type rdf:resource="http://www.w3.org/2000/01/rdf-schema#Resource"/>
</rdf:Description>

<rdf:Description rdf:about="http://vocab.aodn.org.au/def/organisation/entity/186">
	<rdf:type rdf:resource="http://www.w3.org/2000/01/rdf-schema#Resource"/>
	<rdf:type rdf:resource="http://www.w3.org/2004/02/skos/core#Concept"/>
	<dcterms:modified rdf:datatype="http://www.w3.org/2001/XMLSchema#dateTime">2015-07-09T05:50:52Z</dcterms:modified>
	<dcterms:creator rdf:datatype="http://www.w3.org/2001/XMLSchema#string">Natalia Atkins</dcterms:creator>
	<dcterms:created rdf:datatype="http://www.w3.org/2001/XMLSchema#dateTime">2015-07-08T10:38:15Z</dcterms:created>
	<dcterms:contributor rdf:datatype="http://www.w3.org/2001/XMLSchema#string">Natalia_Atkins</dcterms:contributor>
	<skos:prefLabel xml:lang="en">Centre for Marine Science and Technology (CMST), Curtin University</skos:prefLabel>
	<skos:altLabel xml:lang="en"></skos:altLabel>
	<skos:altLabel xml:lang="en">Centre for Marine Science and Technology (CMST)</skos:altLabel>
	<skos:hiddenLabel xml:lang="en">CMST</skos:hiddenLabel>
	<skos:definition xml:lang="en">Founded in 1985, the Centre for Marine Science and Technology (CMST) comprises a multi-skilled group of scientists and engineers committed to the development of technical ocean-related skills in Australia. CMST’s expertise fits into four major categories: Hydrodynamics, Underwater Acoustics, Marine Ecology and Stereoscopic Imaging. The centre works in close cooperation with Curtin’s Department of Imaging and Applied Physics, Department of Applied Geology, Remote Sensing Group, Aquatic Science Group, and the Department of Environmental Biology, plus WA:ERA, IMOS, the Australian Maritime College, and many others.</skos:definition>
	<dc:source rdf:datatype="http://www.w3.org/2001/XMLSchema#string">Australian Ocean Data Network Organisation Register</dc:source>
	<dc:publisher rdf:datatype="http://www.w3.org/2001/XMLSchema#string">eMarine Information Infrastructure (eMII)</dc:publisher>
	<skos:exactMatch rdf:resource="http://seadatanet.maris2.nl/v_edmo/print.asp?n_code=4258"/>
	<skos:inScheme rdf:resource="http://vocab.aodn.org.au/def/organisation/1"/>
	<skos:broader rdf:resource="http://vocab.aodn.org.au/def/organisation/entity/178"/>
</rdf:Description>

<rdf:Description rdf:about="http://seadatanet.maris2.nl/v_edmo/print.asp?n_code=4258">
	<rdf:type rdf:resource="http://www.w3.org/2000/01/rdf-schema#Resource"/>
</rdf:Description>

<rdf:Description rdf:about="http://vocab.aodn.org.au/def/organisation/entity/187">
	<rdf:type rdf:resource="http://www.w3.org/2000/01/rdf-schema#Resource"/>
	<rdf:type rdf:resource="http://www.w3.org/2004/02/skos/core#Concept"/>
	<dcterms:modified rdf:datatype="http://www.w3.org/2001/XMLSchema#dateTime">2015-07-09T05:51:55Z</dcterms:modified>
	<dcterms:creator rdf:datatype="http://www.w3.org/2001/XMLSchema#string">Natalia Atkins</dcterms:creator>
	<dcterms:created rdf:datatype="http://www.w3.org/2001/XMLSchema#dateTime">2015-07-08T10:38:15Z</dcterms:created>
	<dcterms:contributor rdf:datatype="http://www.w3.org/2001/XMLSchema#string">Natalia_Atkins</dcterms:contributor>
	<skos:prefLabel xml:lang="en">Remote Sensing and Satellite Research Group (RSSRG), Curtin University</skos:prefLabel>
	<skos:altLabel xml:lang="en"></skos:altLabel>
	<skos:altLabel xml:lang="en">Remote Sensing and Satellite Research Group (RSSRG)</skos:altLabel>
	<skos:hiddenLabel xml:lang="en">RSSRG</skos:hiddenLabel>
	<skos:definition xml:lang="en">The Remote Sensing and Satellite Research Group (RSSRG), based at Curtin University in Bentley, Western Australia, is part of a national and international network of scientists that undertake quantitative research in the field of Earth observations from space.</skos:definition>
	<dc:source rdf:datatype="http://www.w3.org/2001/XMLSchema#string">Australian Ocean Data Network Organisation Register</dc:source>
	<dc:publisher rdf:datatype="http://www.w3.org/2001/XMLSchema#string">eMarine Information Infrastructure (eMII)</dc:publisher>
	<skos:exactMatch rdf:resource="http://seadatanet.maris2.nl/v_edmo/print.asp?n_code=4259"/>
	<skos:inScheme rdf:resource="http://vocab.aodn.org.au/def/organisation/1"/>
	<skos:broader rdf:resource="http://vocab.aodn.org.au/def/organisation/entity/178"/>
</rdf:Description>

<rdf:Description rdf:about="http://seadatanet.maris2.nl/v_edmo/print.asp?n_code=4259">
	<rdf:type rdf:resource="http://www.w3.org/2000/01/rdf-schema#Resource"/>
</rdf:Description>

<rdf:Description rdf:about="http://vocab.aodn.org.au/def/organisation/entity/188">
	<rdf:type rdf:resource="http://www.w3.org/2000/01/rdf-schema#Resource"/>
	<rdf:type rdf:resource="http://www.w3.org/2004/02/skos/core#Concept"/>
	<dcterms:modified rdf:datatype="http://www.w3.org/2001/XMLSchema#dateTime">2015-07-09T05:52:25Z</dcterms:modified>
	<dcterms:creator rdf:datatype="http://www.w3.org/2001/XMLSchema#string">Natalia Atkins</dcterms:creator>
	<dcterms:created rdf:datatype="http://www.w3.org/2001/XMLSchema#dateTime">2015-07-08T10:38:15Z</dcterms:created>
	<dcterms:contributor rdf:datatype="http://www.w3.org/2001/XMLSchema#string">Natalia_Atkins</dcterms:contributor>
	<skos:prefLabel xml:lang="en">School of Public Health (SoPH), Curtin University</skos:prefLabel>
	<skos:altLabel xml:lang="en"></skos:altLabel>
	<skos:altLabel xml:lang="en">School of Public Health (SoPH)</skos:altLabel>
	<skos:hiddenLabel xml:lang="en">SoPH</skos:hiddenLabel>
	<skos:definition xml:lang="en">The School of Public Health at Curtin University was established in 1979, and currently offers 11 disciplines, including all core public health disciplines. Many of the programs include an international component or perspective.</skos:definition>
	<dc:source rdf:datatype="http://www.w3.org/2001/XMLSchema#string">Australian Ocean Data Network Organisation Register</dc:source>
	<dc:publisher rdf:datatype="http://www.w3.org/2001/XMLSchema#string">eMarine Information Infrastructure (eMII)</dc:publisher>
	<skos:inScheme rdf:resource="http://vocab.aodn.org.au/def/organisation/1"/>
	<skos:broader rdf:resource="http://vocab.aodn.org.au/def/organisation/entity/178"/>
</rdf:Description>

<rdf:Description rdf:about="http://seadatanet.maris2.nl/v_edmo/print.asp?n_code=4027">
	<rdf:type rdf:resource="http://www.w3.org/2000/01/rdf-schema#Resource"/>
</rdf:Description>

<rdf:Description rdf:about="http://vocab.aodn.org.au/def/organisation/entity/179">
	<rdf:type rdf:resource="http://www.w3.org/2000/01/rdf-schema#Resource"/>
	<rdf:type rdf:resource="http://www.w3.org/2004/02/skos/core#Concept"/>
	<dcterms:modified rdf:datatype="http://www.w3.org/2001/XMLSchema#dateTime">2015-07-09T05:51:44Z</dcterms:modified>
	<dcterms:creator rdf:datatype="http://www.w3.org/2001/XMLSchema#string">Natalia Atkins</dcterms:creator>
	<dcterms:created rdf:datatype="http://www.w3.org/2001/XMLSchema#dateTime">2015-07-08T10:38:15Z</dcterms:created>
	<dcterms:contributor rdf:datatype="http://www.w3.org/2001/XMLSchema#string">Natalia_Atkins</dcterms:contributor>
	<skos:prefLabel xml:lang="en">Muresk Institute, Curtin University</skos:prefLabel>
	<skos:altLabel xml:lang="en"></skos:altLabel>
	<skos:altLabel xml:lang="en">Muresk Institute</skos:altLabel>
	<skos:hiddenLabel xml:lang="en"></skos:hiddenLabel>
	<skos:definition xml:lang="en">Muresk Institute is an education and training facility situated in the Wheatbelt (approximately 100km east of Perth). The Institute boasts modern education and training, conference and specialised research facilities. In 2012 the responsibility for Muresk’s operation was transferred from Curtin University to the State Government.</skos:definition>
	<dc:source rdf:datatype="http://www.w3.org/2001/XMLSchema#string">Australian Ocean Data Network Organisation Register</dc:source>
	<dc:publisher rdf:datatype="http://www.w3.org/2001/XMLSchema#string">eMarine Information Infrastructure (eMII)</dc:publisher>
	<skos:inScheme rdf:resource="http://vocab.aodn.org.au/def/organisation/1"/>
	<skos:broader rdf:resource="http://vocab.aodn.org.au/def/organisation/entity/178"/>
	<skos:scopeNote xml:lang="en">Organisation no longer exists</skos:scopeNote>
</rdf:Description>

<rdf:Description rdf:about="http://seadatanet.maris2.nl/v_edmo/print.asp?n_code=4266">
	<rdf:type rdf:resource="http://www.w3.org/2000/01/rdf-schema#Resource"/>
</rdf:Description>

<rdf:Description rdf:about="http://vocab.aodn.org.au/def/organisation/entity/190">
	<rdf:type rdf:resource="http://www.w3.org/2000/01/rdf-schema#Resource"/>
	<rdf:type rdf:resource="http://www.w3.org/2004/02/skos/core#Concept"/>
	<dcterms:creator rdf:datatype="http://www.w3.org/2001/XMLSchema#string">Natalia Atkins</dcterms:creator>
	<dcterms:created rdf:datatype="http://www.w3.org/2001/XMLSchema#dateTime">2015-07-08T10:38:15Z</dcterms:created>
	<skos:prefLabel xml:lang="en">Airborne Research Australia (ARA)</skos:prefLabel>
	<skos:altLabel xml:lang="en"></skos:altLabel>
	<skos:hiddenLabel xml:lang="en">ARA</skos:hiddenLabel>
	<skos:definition xml:lang="en">Airborne Research Australia (ARA) is a Research Centre at Flinders University and Australia's National Research Aircraft Facility located at Parafield Airport in Adelaide, South Australia. ARA was established in 1996 with funding from the Commonwealth Government's Major National Research Facilities Programme and Flinders University.</skos:definition>
	<dc:source rdf:datatype="http://www.w3.org/2001/XMLSchema#string">Australian Ocean Data Network Organisation Register</dc:source>
	<dc:publisher rdf:datatype="http://www.w3.org/2001/XMLSchema#string">eMarine Information Infrastructure (eMII)</dc:publisher>
	<skos:exactMatch rdf:resource="http://seadatanet.maris2.nl/v_edmo/print.asp?n_code=4267"/>
	<skos:inScheme rdf:resource="http://vocab.aodn.org.au/def/organisation/1"/>
	<skos:broader rdf:resource="http://vocab.aodn.org.au/def/organisation/entity/189"/>
</rdf:Description>

<rdf:Description rdf:about="http://vocab.aodn.org.au/def/organisation/entity/191">
	<rdf:type rdf:resource="http://www.w3.org/2000/01/rdf-schema#Resource"/>
	<rdf:type rdf:resource="http://www.w3.org/2004/02/skos/core#Concept"/>
	<dcterms:modified rdf:datatype="http://www.w3.org/2001/XMLSchema#dateTime">2015-07-09T05:53:18Z</dcterms:modified>
	<dcterms:creator rdf:datatype="http://www.w3.org/2001/XMLSchema#string">Natalia Atkins</dcterms:creator>
	<dcterms:created rdf:datatype="http://www.w3.org/2001/XMLSchema#dateTime">2015-07-08T10:38:15Z</dcterms:created>
	<dcterms:contributor rdf:datatype="http://www.w3.org/2001/XMLSchema#string">Natalia_Atkins</dcterms:contributor>
	<skos:prefLabel xml:lang="en">School of Earth Sciences, Flinders University</skos:prefLabel>
	<skos:altLabel xml:lang="en"></skos:altLabel>
	<skos:altLabel xml:lang="en">School of Earth Sciences</skos:altLabel>
	<skos:hiddenLabel xml:lang="en"></skos:hiddenLabel>
	<skos:definition xml:lang="en">This school became part of the School of Chemistry, Physics and Earth Sciences (SoCPES), which is now known as the School of the Environment.</skos:definition>
	<dc:source rdf:datatype="http://www.w3.org/2001/XMLSchema#string">Australian Ocean Data Network Organisation Register</dc:source>
	<dc:publisher rdf:datatype="http://www.w3.org/2001/XMLSchema#string">eMarine Information Infrastructure (eMII)</dc:publisher>
	<skos:inScheme rdf:resource="http://vocab.aodn.org.au/def/organisation/1"/>
	<skos:broader rdf:resource="http://vocab.aodn.org.au/def/organisation/entity/189"/>
	<skos:scopeNote xml:lang="en">Organisation no longer exists</skos:scopeNote>
	<skos:scopeNote xml:lang="en">Organisation no longer exists. Replaced by http://vocab.aodn.org.au/def/organisation/entity/193</skos:scopeNote>
	<dcterms:isReplacedBy rdf:resource="http://vocab.aodn.org.au/def/organisation/entity/193"/>
	<dcterms:isReplacedBy xml:lang="en">School of Chemistry, Physics and Earth Sciences (SoCPES), Flinders University</dcterms:isReplacedBy>
</rdf:Description>

<rdf:Description rdf:about="http://vocab.aodn.org.au/def/organisation/entity/192">
	<rdf:type rdf:resource="http://www.w3.org/2000/01/rdf-schema#Resource"/>
	<rdf:type rdf:resource="http://www.w3.org/2004/02/skos/core#Concept"/>
	<dcterms:modified rdf:datatype="http://www.w3.org/2001/XMLSchema#dateTime">2015-07-09T05:53:28Z</dcterms:modified>
	<dcterms:creator rdf:datatype="http://www.w3.org/2001/XMLSchema#string">Natalia Atkins</dcterms:creator>
	<dcterms:created rdf:datatype="http://www.w3.org/2001/XMLSchema#dateTime">2015-07-08T10:38:15Z</dcterms:created>
	<dcterms:contributor rdf:datatype="http://www.w3.org/2001/XMLSchema#string">Natalia_Atkins</dcterms:contributor>
	<skos:prefLabel xml:lang="en">School of the Environment, Flinders University</skos:prefLabel>
	<skos:altLabel xml:lang="en"></skos:altLabel>
	<skos:altLabel xml:lang="en">School of the Environment</skos:altLabel>
	<skos:hiddenLabel xml:lang="en"></skos:hiddenLabel>
	<skos:definition xml:lang="en">The School of the Environment is an interdisciplinary community delivering research in environmental, water, coastal and spatial sciences.</skos:definition>
	<dc:source rdf:datatype="http://www.w3.org/2001/XMLSchema#string">Australian Ocean Data Network Organisation Register</dc:source>
	<dc:publisher rdf:datatype="http://www.w3.org/2001/XMLSchema#string">eMarine Information Infrastructure (eMII)</dc:publisher>
	<skos:exactMatch rdf:resource="http://seadatanet.maris2.nl/v_edmo/print.asp?n_code=4268"/>
	<skos:inScheme rdf:resource="http://vocab.aodn.org.au/def/organisation/1"/>
	<skos:broader rdf:resource="http://vocab.aodn.org.au/def/organisation/entity/189"/>
	<skos:scopeNote xml:lang="en">Replaces http://vocab.aodn.org.au/def/organisation/entity/193</skos:scopeNote>
	<dcterms:replaces rdf:resource="http://vocab.aodn.org.au/def/organisation/entity/193"/>
	<dcterms:replaces xml:lang="en">School of Chemistry, Physics and Earth Sciences (SoCPES), Flinders University</dcterms:replaces>
</rdf:Description>

<rdf:Description rdf:about="http://vocab.aodn.org.au/def/organisation/entity/193">
	<rdf:type rdf:resource="http://www.w3.org/2000/01/rdf-schema#Resource"/>
	<rdf:type rdf:resource="http://www.w3.org/2004/02/skos/core#Concept"/>
	<dcterms:modified rdf:datatype="http://www.w3.org/2001/XMLSchema#dateTime">2015-07-09T05:53:07Z</dcterms:modified>
	<dcterms:creator rdf:datatype="http://www.w3.org/2001/XMLSchema#string">Natalia Atkins</dcterms:creator>
	<dcterms:created rdf:datatype="http://www.w3.org/2001/XMLSchema#dateTime">2015-07-08T10:38:15Z</dcterms:created>
	<dcterms:contributor rdf:datatype="http://www.w3.org/2001/XMLSchema#string">Natalia_Atkins</dcterms:contributor>
	<skos:prefLabel xml:lang="en">School of Chemistry, Physics and Earth Sciences (SoCPES), Flinders University</skos:prefLabel>
	<skos:altLabel xml:lang="en"></skos:altLabel>
	<skos:altLabel xml:lang="en">School of Chemistry, Physics and Earth Sciences (SoCPES)</skos:altLabel>
	<skos:hiddenLabel xml:lang="en">SoCPES</skos:hiddenLabel>
	<skos:definition xml:lang="en">University research and teaching department formed by the merger of the School of Earth Sciences with other departments.</skos:definition>
	<dc:source rdf:datatype="http://www.w3.org/2001/XMLSchema#string">Australian Ocean Data Network Organisation Register</dc:source>
	<dc:publisher rdf:datatype="http://www.w3.org/2001/XMLSchema#string">eMarine Information Infrastructure (eMII)</dc:publisher>
	<skos:exactMatch rdf:resource="http://seadatanet.maris2.nl/v_edmo/print.asp?n_code=2095"/>
	<skos:inScheme rdf:resource="http://vocab.aodn.org.au/def/organisation/1"/>
	<skos:broader rdf:resource="http://vocab.aodn.org.au/def/organisation/entity/189"/>
	<skos:scopeNote xml:lang="en">Organisation no longer exists</skos:scopeNote>
	<skos:scopeNote xml:lang="en">Organisation no longer exists. Replaced by http://vocab.aodn.org.au/def/organisation/entity/192. Replaces http://vocab.aodn.org.au/def/organisation/entity/191</skos:scopeNote>
	<dcterms:replaces xml:lang="en">School of Earth Sciences, Flinders University</dcterms:replaces>
	<dcterms:replaces xml:lang="en">http://vocab.aodn.org.au/def/organisation/entity/191</dcterms:replaces>
	<dcterms:isReplacedBy rdf:resource="http://vocab.aodn.org.au/def/organisation/entity/192"/>
	<dcterms:isReplacedBy xml:lang="en">School of the Environment, Flinders University</dcterms:isReplacedBy>
</rdf:Description>

<rdf:Description rdf:about="http://vocab.aodn.org.au/def/organisation/entity/410">
	<rdf:type rdf:resource="http://www.w3.org/2000/01/rdf-schema#Resource"/>
	<rdf:type rdf:resource="http://www.w3.org/2004/02/skos/core#Concept"/>
	<dcterms:modified rdf:datatype="http://www.w3.org/2001/XMLSchema#dateTime">2015-11-04T23:01:03Z</dcterms:modified>
	<dcterms:creator rdf:datatype="http://www.w3.org/2001/XMLSchema#string">Natalia Atkins</dcterms:creator>
	<dcterms:created rdf:datatype="http://www.w3.org/2001/XMLSchema#dateTime">2015-11-05T10:38:15Z</dcterms:created>
	<dcterms:contributor rdf:datatype="http://www.w3.org/2001/XMLSchema#string">eMII_Atkins.Natalia</dcterms:contributor>
	<skos:prefLabel xml:lang="en">School of Biological Sciences, Flinders University</skos:prefLabel>
	<skos:altLabel xml:lang="en">School of Biological Sciences</skos:altLabel>
	<skos:hiddenLabel xml:lang="en"></skos:hiddenLabel>
	<skos:definition xml:lang="en">The School of Biological Sciences is an integrated community researching and teaching biology. Our foundations are collaborative clusters in Biodiversity and Ecology, Marine Biology and Aquaculture (including the Lincoln Marine Science Centre), and Molecular Biology and Biotechnology.</skos:definition>
	<dc:source rdf:datatype="http://www.w3.org/2001/XMLSchema#string">Australian Ocean Data Network Organisation Register</dc:source>
	<dc:publisher rdf:datatype="http://www.w3.org/2001/XMLSchema#string">eMarine Information Infrastructure (eMII)</dc:publisher>
	<skos:exactMatch rdf:resource="http://seadatanet.maris2.nl/v_edmo/print.asp?n_code=4442"/>
	<skos:inScheme rdf:resource="http://vocab.aodn.org.au/def/organisation/1"/>
	<skos:broader rdf:resource="http://vocab.aodn.org.au/def/organisation/entity/189"/>
</rdf:Description>

<rdf:Description rdf:about="http://seadatanet.maris2.nl/v_edmo/print.asp?n_code=4267">
	<rdf:type rdf:resource="http://www.w3.org/2000/01/rdf-schema#Resource"/>
</rdf:Description>

<rdf:Description rdf:about="http://seadatanet.maris2.nl/v_edmo/print.asp?n_code=4268">
	<rdf:type rdf:resource="http://www.w3.org/2000/01/rdf-schema#Resource"/>
</rdf:Description>

<rdf:Description rdf:about="http://seadatanet.maris2.nl/v_edmo/print.asp?n_code=2095">
	<rdf:type rdf:resource="http://www.w3.org/2000/01/rdf-schema#Resource"/>
</rdf:Description>

<rdf:Description rdf:about="http://seadatanet.maris2.nl/v_edmo/print.asp?n_code=4287">
	<rdf:type rdf:resource="http://www.w3.org/2000/01/rdf-schema#Resource"/>
</rdf:Description>

<rdf:Description rdf:about="http://vocab.aodn.org.au/def/organisation/entity/195">
	<rdf:type rdf:resource="http://www.w3.org/2000/01/rdf-schema#Resource"/>
	<rdf:type rdf:resource="http://www.w3.org/2004/02/skos/core#Concept"/>
	<dcterms:modified rdf:datatype="http://www.w3.org/2001/XMLSchema#dateTime">2015-07-09T05:54:23Z</dcterms:modified>
	<dcterms:creator rdf:datatype="http://www.w3.org/2001/XMLSchema#string">Natalia Atkins</dcterms:creator>
	<dcterms:created rdf:datatype="http://www.w3.org/2001/XMLSchema#dateTime">2015-07-09T10:38:15Z</dcterms:created>
	<dcterms:contributor rdf:datatype="http://www.w3.org/2001/XMLSchema#string">Natalia_Atkins</dcterms:contributor>
	<skos:prefLabel xml:lang="en">Department of Earth and Marine Sciences (DEMS), The Australian National University (ANU)</skos:prefLabel>
	<skos:altLabel xml:lang="en"></skos:altLabel>
	<skos:altLabel xml:lang="en">Department of Earth and Marine Sciences (DEMS)</skos:altLabel>
	<skos:hiddenLabel xml:lang="en">DEMS</skos:hiddenLabel>
	<skos:definition xml:lang="en">The Australian National University (ANU) Department of Earth and Marine Sciences (previously Department of Geology) is a centre of excellence for teaching and research in areas of environmental, earth and marine science. It maintains a diverse range of interests, preparing students for careers in science, law and the humanities, offering both undergraduate and postgraduate studies. The primary focus is on both environmental science and earth processes. The Institute of Scientific Information (ISI) has ranked ANU geoscience the top university program in Australia, and amongst the top 10 universities worldwide. The Department is the only teaching department of Earth Sciences in Canberra, and its location provides a unique opportunity to collaborate with government departments such as Geoscience Australia and the Bureau of Rural Sciences. Thus, there is access to some of the most advanced equipment available for experimental work, and opportunities that no other university in Australia can offer. The Department is an active member of the Cooperative Research Centre for Landscape Environments and Mineral Exploration which sees some staff involved in teaching and research in hydrology, regolith geochemistry and biogeochemistry. The Department also holds the Office for the Consortium of Marine Geoscience Institutions for Australia and is the successor of the [now defunct] Australian Ocean Drilling Program with new aims for promoting marine geoscience in this country.</skos:definition>
	<dc:source rdf:datatype="http://www.w3.org/2001/XMLSchema#string">Australian Ocean Data Network Organisation Register</dc:source>
	<dc:publisher rdf:datatype="http://www.w3.org/2001/XMLSchema#string">eMarine Information Infrastructure (eMII)</dc:publisher>
	<skos:exactMatch rdf:resource="http://seadatanet.maris2.nl/v_edmo/print.asp?n_code=1492"/>
	<skos:inScheme rdf:resource="http://vocab.aodn.org.au/def/organisation/1"/>
	<skos:broader rdf:resource="http://vocab.aodn.org.au/def/organisation/entity/194"/>
	<skos:scopeNote xml:lang="en">Organisation no longer exists</skos:scopeNote>
	<skos:scopeNote xml:lang="en">Organisation no longer exists. Replaced by http://vocab.aodn.org.au/def/organisation/entity/196. Replaces http://vocab.aodn.org.au/def/organisation/entity/197</skos:scopeNote>
	<dcterms:replaces rdf:resource="http://vocab.aodn.org.au/def/organisation/entity/197"/>
	<dcterms:replaces xml:lang="en">Department of Geology, The Australian National University (ANU)</dcterms:replaces>
	<dcterms:isReplacedBy rdf:resource="http://vocab.aodn.org.au/def/organisation/entity/196"/>
	<dcterms:isReplacedBy xml:lang="en">Research School of Earth Sciences (RSES), The Australian National University (ANU)</dcterms:isReplacedBy>
</rdf:Description>

<rdf:Description rdf:about="http://vocab.aodn.org.au/def/organisation/entity/196">
	<rdf:type rdf:resource="http://www.w3.org/2000/01/rdf-schema#Resource"/>
	<rdf:type rdf:resource="http://www.w3.org/2004/02/skos/core#Concept"/>
	<dcterms:modified rdf:datatype="http://www.w3.org/2001/XMLSchema#dateTime">2015-07-09T05:56:10Z</dcterms:modified>
	<dcterms:creator rdf:datatype="http://www.w3.org/2001/XMLSchema#string">Natalia Atkins</dcterms:creator>
	<dcterms:created rdf:datatype="http://www.w3.org/2001/XMLSchema#dateTime">2015-07-09T10:38:15Z</dcterms:created>
	<dcterms:contributor rdf:datatype="http://www.w3.org/2001/XMLSchema#string">Natalia_Atkins</dcterms:contributor>
	<skos:prefLabel xml:lang="en">Research School of Earth Sciences (RSES), The Australian National University (ANU)</skos:prefLabel>
	<skos:altLabel xml:lang="en"></skos:altLabel>
	<skos:altLabel xml:lang="en">Research School of Earth Sciences (RSES)</skos:altLabel>
	<skos:hiddenLabel xml:lang="en">RSES</skos:hiddenLabel>
	<skos:definition xml:lang="en">Since January 2008 the Research School of Earth Sciences (RSES) incorporates the former Department of Earth and Marine Sciences of the Faculty of Science and now provides teaching at undergraduate and postgraduate levels, and higher degree research programs within a world-class institution. The Research School now has two locations. The main administration and much of the research facilities are housed in the Jaeger Building (Building 61), but teaching activities are concentrated at the D.A. Brown Building (Building 47) about 10 minutes away by foot.</skos:definition>
	<dc:source rdf:datatype="http://www.w3.org/2001/XMLSchema#string">Australian Ocean Data Network Organisation Register</dc:source>
	<dc:publisher rdf:datatype="http://www.w3.org/2001/XMLSchema#string">eMarine Information Infrastructure (eMII)</dc:publisher>
	<skos:exactMatch rdf:resource="http://seadatanet.maris2.nl/v_edmo/print.asp?n_code=1989"/>
	<skos:inScheme rdf:resource="http://vocab.aodn.org.au/def/organisation/1"/>
	<skos:broader rdf:resource="http://vocab.aodn.org.au/def/organisation/entity/194"/>
	<skos:scopeNote xml:lang="en">Replaces http://vocab.aodn.org.au/def/organisation/entity/195</skos:scopeNote>
	<dcterms:replaces rdf:resource="http://vocab.aodn.org.au/def/organisation/entity/195"/>
	<dcterms:replaces xml:lang="en">Department of Earth and Marine Sciences (DEMS), The Australian National University (ANU)</dcterms:replaces>
</rdf:Description>

<rdf:Description rdf:about="http://vocab.aodn.org.au/def/organisation/entity/197">
	<rdf:type rdf:resource="http://www.w3.org/2000/01/rdf-schema#Resource"/>
	<rdf:type rdf:resource="http://www.w3.org/2004/02/skos/core#Concept"/>
	<dcterms:modified rdf:datatype="http://www.w3.org/2001/XMLSchema#dateTime">2015-07-09T05:54:34Z</dcterms:modified>
	<dcterms:creator rdf:datatype="http://www.w3.org/2001/XMLSchema#string">Natalia Atkins</dcterms:creator>
	<dcterms:created rdf:datatype="http://www.w3.org/2001/XMLSchema#dateTime">2015-07-09T10:38:15Z</dcterms:created>
	<dcterms:contributor rdf:datatype="http://www.w3.org/2001/XMLSchema#string">Natalia_Atkins</dcterms:contributor>
	<skos:prefLabel xml:lang="en">Department of Geology, The Australian National University (ANU)</skos:prefLabel>
	<skos:altLabel xml:lang="en"></skos:altLabel>
	<skos:altLabel xml:lang="en">Department of Geology</skos:altLabel>
	<skos:hiddenLabel xml:lang="en"></skos:hiddenLabel>
	<skos:definition xml:lang="en">This former school became part of the Department of Earth and Marine Sciences (DEMS).</skos:definition>
	<dc:source rdf:datatype="http://www.w3.org/2001/XMLSchema#string">Australian Ocean Data Network Organisation Register</dc:source>
	<dc:publisher rdf:datatype="http://www.w3.org/2001/XMLSchema#string">eMarine Information Infrastructure (eMII)</dc:publisher>
	<skos:inScheme rdf:resource="http://vocab.aodn.org.au/def/organisation/1"/>
	<skos:broader rdf:resource="http://vocab.aodn.org.au/def/organisation/entity/194"/>
	<skos:scopeNote xml:lang="en">Organisation no longer exists</skos:scopeNote>
	<skos:scopeNote xml:lang="en">Organisation no longer exists. Replaced by http://vocab.aodn.org.au/def/organisation/entity/195</skos:scopeNote>
	<dcterms:isReplacedBy rdf:resource="http://vocab.aodn.org.au/def/organisation/entity/195"/>
	<dcterms:isReplacedBy xml:lang="en">Department of Earth and Marine Sciences (DEMS), The Australian National University (ANU)</dcterms:isReplacedBy>
</rdf:Description>

<rdf:Description rdf:about="http://vocab.aodn.org.au/def/organisation/entity/198">
	<rdf:type rdf:resource="http://www.w3.org/2000/01/rdf-schema#Resource"/>
	<rdf:type rdf:resource="http://www.w3.org/2004/02/skos/core#Concept"/>
	<dcterms:modified rdf:datatype="http://www.w3.org/2001/XMLSchema#dateTime">2015-07-09T05:56:45Z</dcterms:modified>
	<dcterms:creator rdf:datatype="http://www.w3.org/2001/XMLSchema#string">Natalia Atkins</dcterms:creator>
	<dcterms:created rdf:datatype="http://www.w3.org/2001/XMLSchema#dateTime">2015-07-09T10:38:15Z</dcterms:created>
	<dcterms:contributor rdf:datatype="http://www.w3.org/2001/XMLSchema#string">Natalia_Atkins</dcterms:contributor>
	<skos:prefLabel xml:lang="en">School of Botany and Zoology (BoZo), The Australian National University (ANU)</skos:prefLabel>
	<skos:altLabel xml:lang="en"></skos:altLabel>
	<skos:altLabel xml:lang="en">School of Botany and Zoology (BoZo)</skos:altLabel>
	<skos:hiddenLabel xml:lang="en">BoZo</skos:hiddenLabel>
	<skos:definition xml:lang="en">In 2009, the School of Botany and Zoology (BoZo) was merged with the Research School of Biological Sciences, and the School of Biochemistry and Molecular Biology to form the Research School of Biology. (Courtesy of Wikipedia)</skos:definition>
	<dc:source rdf:datatype="http://www.w3.org/2001/XMLSchema#string">Australian Ocean Data Network Organisation Register</dc:source>
	<dc:publisher rdf:datatype="http://www.w3.org/2001/XMLSchema#string">eMarine Information Infrastructure (eMII)</dc:publisher>
	<skos:inScheme rdf:resource="http://vocab.aodn.org.au/def/organisation/1"/>
	<skos:broader rdf:resource="http://vocab.aodn.org.au/def/organisation/entity/194"/>
	<skos:scopeNote xml:lang="en">Organisation no longer exists</skos:scopeNote>
	<skos:scopeNote xml:lang="en">Organisation no longer exists. Replaced by http://vocab.aodn.org.au/def/organisation/entity/200</skos:scopeNote>
	<dcterms:isReplacedBy rdf:resource="http://vocab.aodn.org.au/def/organisation/entity/200"/>
	<dcterms:isReplacedBy xml:lang="en">Research School of Biology (RSB), The Australian National University (ANU)</dcterms:isReplacedBy>
</rdf:Description>

<rdf:Description rdf:about="http://vocab.aodn.org.au/def/organisation/entity/199">
	<rdf:type rdf:resource="http://www.w3.org/2000/01/rdf-schema#Resource"/>
	<rdf:type rdf:resource="http://www.w3.org/2004/02/skos/core#Concept"/>
	<dcterms:modified rdf:datatype="http://www.w3.org/2001/XMLSchema#dateTime">2015-07-09T05:55:48Z</dcterms:modified>
	<dcterms:creator rdf:datatype="http://www.w3.org/2001/XMLSchema#string">Natalia Atkins</dcterms:creator>
	<dcterms:created rdf:datatype="http://www.w3.org/2001/XMLSchema#dateTime">2015-07-09T10:38:15Z</dcterms:created>
	<dcterms:contributor rdf:datatype="http://www.w3.org/2001/XMLSchema#string">Natalia_Atkins</dcterms:contributor>
	<skos:prefLabel xml:lang="en">Research School of Biological  Sciences (RSBS), The Australian National University (ANU)</skos:prefLabel>
	<skos:altLabel xml:lang="en"></skos:altLabel>
	<skos:altLabel xml:lang="en">Research School of Biological Sciences (RSBS)</skos:altLabel>
	<skos:hiddenLabel xml:lang="en">RSBS</skos:hiddenLabel>
	<skos:definition xml:lang="en">The Research School of Biological Sciences (RSBS) was formed in the 1960s at the The Australian National University. In 2009, RSBS was merged with the School of Botany and Zoology, and the School of Biochemistry and Molecular Biology to form the Research School of Biology. (Courtesy of Wikipedia)</skos:definition>
	<dc:source rdf:datatype="http://www.w3.org/2001/XMLSchema#string">Australian Ocean Data Network Organisation Register</dc:source>
	<dc:publisher rdf:datatype="http://www.w3.org/2001/XMLSchema#string">eMarine Information Infrastructure (eMII)</dc:publisher>
	<skos:inScheme rdf:resource="http://vocab.aodn.org.au/def/organisation/1"/>
	<skos:broader rdf:resource="http://vocab.aodn.org.au/def/organisation/entity/194"/>
	<skos:scopeNote xml:lang="en">Organisation no longer exists</skos:scopeNote>
	<skos:scopeNote xml:lang="en">Organisation no longer exists. Replaced by http://vocab.aodn.org.au/def/organisation/entity/200</skos:scopeNote>
	<dcterms:isReplacedBy rdf:resource="http://vocab.aodn.org.au/def/organisation/entity/200"/>
	<dcterms:isReplacedBy xml:lang="en">Research School of Biology (RSB), The Australian National University (ANU)</dcterms:isReplacedBy>
</rdf:Description>

<rdf:Description rdf:about="http://vocab.aodn.org.au/def/organisation/entity/200">
	<rdf:type rdf:resource="http://www.w3.org/2000/01/rdf-schema#Resource"/>
	<rdf:type rdf:resource="http://www.w3.org/2004/02/skos/core#Concept"/>
	<dcterms:modified rdf:datatype="http://www.w3.org/2001/XMLSchema#dateTime">2015-07-09T05:55:59Z</dcterms:modified>
	<dcterms:creator rdf:datatype="http://www.w3.org/2001/XMLSchema#string">Natalia Atkins</dcterms:creator>
	<dcterms:created rdf:datatype="http://www.w3.org/2001/XMLSchema#dateTime">2015-07-09T10:38:15Z</dcterms:created>
	<dcterms:contributor rdf:datatype="http://www.w3.org/2001/XMLSchema#string">Natalia_Atkins</dcterms:contributor>
	<skos:prefLabel xml:lang="en">Research School of Biology (RSB), The Australian National University (ANU)</skos:prefLabel>
	<skos:altLabel xml:lang="en"></skos:altLabel>
	<skos:altLabel xml:lang="en">Research School of Biology (RSB)</skos:altLabel>
	<skos:hiddenLabel xml:lang="en">RSB</skos:hiddenLabel>
	<skos:definition xml:lang="en">The ANU Research School of Biology carries out research, research training, undergraduate and coursework Masters teaching in a wide range of biological and biomedical sciences. The School comprises three divisions: Biomedical Science and Biochemistry; Evolution, Ecology and Genetics; and Plant Sciences.</skos:definition>
	<dc:source rdf:datatype="http://www.w3.org/2001/XMLSchema#string">Australian Ocean Data Network Organisation Register</dc:source>
	<dc:publisher rdf:datatype="http://www.w3.org/2001/XMLSchema#string">eMarine Information Infrastructure (eMII)</dc:publisher>
	<skos:exactMatch rdf:resource="http://seadatanet.maris2.nl/v_edmo/print.asp?n_code=4288"/>
	<skos:inScheme rdf:resource="http://vocab.aodn.org.au/def/organisation/1"/>
	<skos:broader rdf:resource="http://vocab.aodn.org.au/def/organisation/entity/194"/>
	<skos:scopeNote xml:lang="en">Replaces http://vocab.aodn.org.au/def/organisation/entity/198 and http://vocab.aodn.org.au/def/organisation/entity/199</skos:scopeNote>
	<dcterms:replaces rdf:resource="http://vocab.aodn.org.au/def/organisation/entity/198"/>
	<dcterms:replaces rdf:resource="http://vocab.aodn.org.au/def/organisation/entity/199"/>
	<dcterms:replaces xml:lang="en">School of Botany and Zoology (BoZo), The Australian National University (ANU)</dcterms:replaces>
	<dcterms:replaces xml:lang="en">Research School of Biological  Sciences (RSBS), The Australian National University (ANU)</dcterms:replaces>
</rdf:Description>

<rdf:Description rdf:about="http://vocab.aodn.org.au/def/organisation/entity/201">
	<rdf:type rdf:resource="http://www.w3.org/2000/01/rdf-schema#Resource"/>
	<rdf:type rdf:resource="http://www.w3.org/2004/02/skos/core#Concept"/>
	<dcterms:modified rdf:datatype="http://www.w3.org/2001/XMLSchema#dateTime">2015-07-09T05:56:34Z</dcterms:modified>
	<dcterms:creator rdf:datatype="http://www.w3.org/2001/XMLSchema#string">Natalia Atkins</dcterms:creator>
	<dcterms:created rdf:datatype="http://www.w3.org/2001/XMLSchema#dateTime">2015-07-09T10:38:15Z</dcterms:created>
	<dcterms:contributor rdf:datatype="http://www.w3.org/2001/XMLSchema#string">Natalia_Atkins</dcterms:contributor>
	<skos:prefLabel xml:lang="en">School of Archaeology and Anthropology, The Australian National University (ANU)</skos:prefLabel>
	<skos:altLabel xml:lang="en"></skos:altLabel>
	<skos:altLabel xml:lang="en">School of Archaeology and Anthropology</skos:altLabel>
	<skos:hiddenLabel xml:lang="en"></skos:hiddenLabel>
	<skos:definition xml:lang="en">The School of Archaeology and Anthropology combines five streams of social research and teaching — anthropology, archaeology, biological anthropology and the interdisciplinary fields of development studies and heritage and museum studies.</skos:definition>
	<dc:source rdf:datatype="http://www.w3.org/2001/XMLSchema#string">Australian Ocean Data Network Organisation Register</dc:source>
	<dc:publisher rdf:datatype="http://www.w3.org/2001/XMLSchema#string">eMarine Information Infrastructure (eMII)</dc:publisher>
	<skos:inScheme rdf:resource="http://vocab.aodn.org.au/def/organisation/1"/>
	<skos:broader rdf:resource="http://vocab.aodn.org.au/def/organisation/entity/194"/>
</rdf:Description>

<rdf:Description rdf:about="http://vocab.aodn.org.au/def/organisation/entity/202">
	<rdf:type rdf:resource="http://www.w3.org/2000/01/rdf-schema#Resource"/>
	<rdf:type rdf:resource="http://www.w3.org/2004/02/skos/core#Concept"/>
	<dcterms:modified rdf:datatype="http://www.w3.org/2001/XMLSchema#dateTime">2015-07-09T05:56:21Z</dcterms:modified>
	<dcterms:creator rdf:datatype="http://www.w3.org/2001/XMLSchema#string">Natalia Atkins</dcterms:creator>
	<dcterms:created rdf:datatype="http://www.w3.org/2001/XMLSchema#dateTime">2015-07-09T10:38:15Z</dcterms:created>
	<dcterms:contributor rdf:datatype="http://www.w3.org/2001/XMLSchema#string">Natalia_Atkins</dcterms:contributor>
	<skos:prefLabel xml:lang="en">Research School of Pacific and Asian Studies (RSPAS), The Australian National University (ANU)</skos:prefLabel>
	<skos:altLabel xml:lang="en"></skos:altLabel>
	<skos:altLabel xml:lang="en">Research School of Pacific and Asian Studies (RSPAS)</skos:altLabel>
	<skos:hiddenLabel xml:lang="en">RSPAS</skos:hiddenLabel>
	<skos:definition xml:lang="en">The Research School of Pacific and Asian Studies (RSPAS) was originally founded in 1946, in 2010,  the RSPAS was reduced in status in line with other changes to other research schools across the ANU. Shortly afterwards a new College of Asia and the Pacific was established, which took over much of the work of the former RSPAS. (Courtesy of Wikipedia)</skos:definition>
	<dc:source rdf:datatype="http://www.w3.org/2001/XMLSchema#string">Australian Ocean Data Network Organisation Register</dc:source>
	<dc:publisher rdf:datatype="http://www.w3.org/2001/XMLSchema#string">eMarine Information Infrastructure (eMII)</dc:publisher>
	<skos:inScheme rdf:resource="http://vocab.aodn.org.au/def/organisation/1"/>
	<skos:broader rdf:resource="http://vocab.aodn.org.au/def/organisation/entity/194"/>
	<skos:scopeNote xml:lang="en">Organisation no longer exists</skos:scopeNote>
	<skos:scopeNote xml:lang="en">Organisation no longer exists. http://vocab.aodn.org.au/def/organisation/entity/203</skos:scopeNote>
	<dcterms:isReplacedBy rdf:resource="http://vocab.aodn.org.au/def/organisation/entity/203"/>
	<dcterms:isReplacedBy xml:lang="en">Research School of Asia and the Pacific (RSAP), The Australian National University (ANU)</dcterms:isReplacedBy>
</rdf:Description>

<rdf:Description rdf:about="http://vocab.aodn.org.au/def/organisation/entity/203">
	<rdf:type rdf:resource="http://www.w3.org/2000/01/rdf-schema#Resource"/>
	<rdf:type rdf:resource="http://www.w3.org/2004/02/skos/core#Concept"/>
	<dcterms:modified rdf:datatype="http://www.w3.org/2001/XMLSchema#dateTime">2015-07-09T05:55:37Z</dcterms:modified>
	<dcterms:creator rdf:datatype="http://www.w3.org/2001/XMLSchema#string">Natalia Atkins</dcterms:creator>
	<dcterms:created rdf:datatype="http://www.w3.org/2001/XMLSchema#dateTime">2015-07-09T10:38:15Z</dcterms:created>
	<dcterms:contributor rdf:datatype="http://www.w3.org/2001/XMLSchema#string">Natalia_Atkins</dcterms:contributor>
	<skos:prefLabel xml:lang="en">Research School of Asia and the Pacific (RSAP), The Australian National University (ANU)</skos:prefLabel>
	<skos:altLabel xml:lang="en"></skos:altLabel>
	<skos:altLabel xml:lang="en">Research School of Asia and the Pacific (RSAP)</skos:altLabel>
	<skos:hiddenLabel xml:lang="en">RSAP</skos:hiddenLabel>
	<skos:definition xml:lang="en">The Research School of Asia and the Pacific (RSAP) is the institutional focus of the College of Asia and the Pacific's research efforts.</skos:definition>
	<dc:source rdf:datatype="http://www.w3.org/2001/XMLSchema#string">Australian Ocean Data Network Organisation Register</dc:source>
	<dc:publisher rdf:datatype="http://www.w3.org/2001/XMLSchema#string">eMarine Information Infrastructure (eMII)</dc:publisher>
	<skos:exactMatch rdf:resource="http://seadatanet.maris2.nl/v_edmo/print.asp?n_code=4289"/>
	<skos:inScheme rdf:resource="http://vocab.aodn.org.au/def/organisation/1"/>
	<skos:broader rdf:resource="http://vocab.aodn.org.au/def/organisation/entity/194"/>
	<skos:scopeNote xml:lang="en">Replaces http://vocab.aodn.org.au/def/organisation/entity/202</skos:scopeNote>
	<dcterms:replaces rdf:resource="http://vocab.aodn.org.au/def/organisation/entity/202"/>
	<dcterms:replaces xml:lang="en">Research School of Pacific and Asian Studies (RSPAS), The Australian National University (ANU)</dcterms:replaces>
</rdf:Description>

<rdf:Description rdf:about="http://vocab.aodn.org.au/def/organisation/entity/204">
	<rdf:type rdf:resource="http://www.w3.org/2000/01/rdf-schema#Resource"/>
	<rdf:type rdf:resource="http://www.w3.org/2004/02/skos/core#Concept"/>
	<dcterms:modified rdf:datatype="http://www.w3.org/2001/XMLSchema#dateTime">2015-07-09T05:54:01Z</dcterms:modified>
	<dcterms:creator rdf:datatype="http://www.w3.org/2001/XMLSchema#string">Natalia Atkins</dcterms:creator>
	<dcterms:created rdf:datatype="http://www.w3.org/2001/XMLSchema#dateTime">2015-07-09T10:38:15Z</dcterms:created>
	<dcterms:contributor rdf:datatype="http://www.w3.org/2001/XMLSchema#string">Natalia_Atkins</dcterms:contributor>
	<skos:prefLabel xml:lang="en">Centre for Resource and Environmental Studies (CRES), The Australian National University (ANU)</skos:prefLabel>
	<skos:altLabel xml:lang="en"></skos:altLabel>
	<skos:altLabel xml:lang="en">Centre for Resource and Environmental Studies (CRES)</skos:altLabel>
	<skos:hiddenLabel xml:lang="en">CRES</skos:hiddenLabel>
	<skos:definition xml:lang="en">The Centre for Resource and Environmental Studies (CRES), was founded in 1973. CRES was combined with the School of Resources, Environment and Society (SRES) to form The Fenner School of Environment and Society in 2007. (Courtesy of Wikipedia)</skos:definition>
	<dc:source rdf:datatype="http://www.w3.org/2001/XMLSchema#string">Australian Ocean Data Network Organisation Register</dc:source>
	<dc:publisher rdf:datatype="http://www.w3.org/2001/XMLSchema#string">eMarine Information Infrastructure (eMII)</dc:publisher>
	<skos:inScheme rdf:resource="http://vocab.aodn.org.au/def/organisation/1"/>
	<skos:broader rdf:resource="http://vocab.aodn.org.au/def/organisation/entity/194"/>
	<skos:scopeNote xml:lang="en">Organisation no longer exists</skos:scopeNote>
	<skos:scopeNote xml:lang="en">Organisation no longer exists. Replaced by http://vocab.aodn.org.au/def/organisation/entity/207</skos:scopeNote>
	<dcterms:isReplacedBy rdf:resource="http://vocab.aodn.org.au/def/organisation/entity/207"/>
	<dcterms:isReplacedBy xml:lang="en">Fenner School of Environment and Society, The Australian National University (ANU)</dcterms:isReplacedBy>
</rdf:Description>

<rdf:Description rdf:about="http://vocab.aodn.org.au/def/organisation/entity/205">
	<rdf:type rdf:resource="http://www.w3.org/2000/01/rdf-schema#Resource"/>
	<rdf:type rdf:resource="http://www.w3.org/2004/02/skos/core#Concept"/>
	<dcterms:modified rdf:datatype="http://www.w3.org/2001/XMLSchema#dateTime">2015-07-12T23:39:43Z</dcterms:modified>
	<dcterms:creator rdf:datatype="http://www.w3.org/2001/XMLSchema#string">Natalia Atkins</dcterms:creator>
	<dcterms:created rdf:datatype="http://www.w3.org/2001/XMLSchema#dateTime">2015-07-09T10:38:15Z</dcterms:created>
	<dcterms:contributor rdf:datatype="http://www.w3.org/2001/XMLSchema#string">Natalia_Atkins</dcterms:contributor>
	<skos:prefLabel xml:lang="en">Asia Pacific School of Economics and Government (APSEG), The Australian National University (ANU)</skos:prefLabel>
	<skos:altLabel xml:lang="en"></skos:altLabel>
	<skos:altLabel xml:lang="en">Asia Pacific School of Economics and Government (APSEG)</skos:altLabel>
	<skos:hiddenLabel xml:lang="en">APSEG</skos:hiddenLabel>
	<skos:definition xml:lang="en">The Asia Pacific School of Economics and Government, is now incorporated as part of the Crawford School of Public Policy (CSPP).</skos:definition>
	<dc:source rdf:datatype="http://www.w3.org/2001/XMLSchema#string">Australian Ocean Data Network Organisation Register</dc:source>
	<dc:publisher rdf:datatype="http://www.w3.org/2001/XMLSchema#string">eMarine Information Infrastructure (eMII)</dc:publisher>
	<skos:inScheme rdf:resource="http://vocab.aodn.org.au/def/organisation/1"/>
	<skos:broader rdf:resource="http://vocab.aodn.org.au/def/organisation/entity/194"/>
	<skos:scopeNote xml:lang="en">Organisation no longer exists</skos:scopeNote>
	<skos:scopeNote xml:lang="en">Organisation no longer exists. Replaced by http://vocab.aodn.org.au/def/organisation/entity/206</skos:scopeNote>
	<dcterms:isReplacedBy rdf:resource="http://vocab.aodn.org.au/def/organisation/entity/206"/>
	<dcterms:isReplacedBy xml:lang="en">Crawford School of Public Policy (CSPP), The Australian National University (ANU)</dcterms:isReplacedBy>
</rdf:Description>

<rdf:Description rdf:about="http://vocab.aodn.org.au/def/organisation/entity/206">
	<rdf:type rdf:resource="http://www.w3.org/2000/01/rdf-schema#Resource"/>
	<rdf:type rdf:resource="http://www.w3.org/2004/02/skos/core#Concept"/>
	<dcterms:modified rdf:datatype="http://www.w3.org/2001/XMLSchema#dateTime">2015-07-09T05:54:13Z</dcterms:modified>
	<dcterms:creator rdf:datatype="http://www.w3.org/2001/XMLSchema#string">Natalia Atkins</dcterms:creator>
	<dcterms:created rdf:datatype="http://www.w3.org/2001/XMLSchema#dateTime">2015-07-09T10:38:15Z</dcterms:created>
	<dcterms:contributor rdf:datatype="http://www.w3.org/2001/XMLSchema#string">Natalia_Atkins</dcterms:contributor>
	<skos:prefLabel xml:lang="en">Crawford School of Public Policy (CSPP), The Australian National University (ANU)</skos:prefLabel>
	<skos:altLabel xml:lang="en"></skos:altLabel>
	<skos:altLabel xml:lang="en">Crawford School of Public Policy (CSPP)</skos:altLabel>
	<skos:hiddenLabel xml:lang="en">CSPP</skos:hiddenLabel>
	<skos:definition xml:lang="en">The Crawford School of Public Policy is a graduate public policy school within the ANU College of Asia and the Pacific.</skos:definition>
	<dc:source rdf:datatype="http://www.w3.org/2001/XMLSchema#string">Australian Ocean Data Network Organisation Register</dc:source>
	<dc:publisher rdf:datatype="http://www.w3.org/2001/XMLSchema#string">eMarine Information Infrastructure (eMII)</dc:publisher>
	<skos:exactMatch rdf:resource="http://seadatanet.maris2.nl/v_edmo/print.asp?n_code=4290"/>
	<skos:inScheme rdf:resource="http://vocab.aodn.org.au/def/organisation/1"/>
	<skos:broader rdf:resource="http://vocab.aodn.org.au/def/organisation/entity/194"/>
	<skos:scopeNote xml:lang="en">Replaces http://vocab.aodn.org.au/def/organisation/entity/205</skos:scopeNote>
	<dcterms:replaces rdf:resource="http://vocab.aodn.org.au/def/organisation/entity/205"/>
	<dcterms:replaces xml:lang="en">Asia Pacific School of Economics and Government (APSEG), The Australian National University (ANU)</dcterms:replaces>
</rdf:Description>

<rdf:Description rdf:about="http://vocab.aodn.org.au/def/organisation/entity/207">
	<rdf:type rdf:resource="http://www.w3.org/2000/01/rdf-schema#Resource"/>
	<rdf:type rdf:resource="http://www.w3.org/2004/02/skos/core#Concept"/>
	<dcterms:modified rdf:datatype="http://www.w3.org/2001/XMLSchema#dateTime">2015-07-14T00:12:56Z</dcterms:modified>
	<dcterms:creator rdf:datatype="http://www.w3.org/2001/XMLSchema#string">Natalia Atkins</dcterms:creator>
	<dcterms:created rdf:datatype="http://www.w3.org/2001/XMLSchema#dateTime">2015-07-09T10:38:15Z</dcterms:created>
	<dcterms:contributor rdf:datatype="http://www.w3.org/2001/XMLSchema#string">Natalia_Atkins</dcterms:contributor>
	<skos:prefLabel xml:lang="en">Fenner School of Environment and Society, The Australian National University (ANU)</skos:prefLabel>
	<skos:altLabel xml:lang="en"></skos:altLabel>
	<skos:altLabel xml:lang="en">Fenner School of Environment and Society</skos:altLabel>
	<skos:hiddenLabel xml:lang="en"></skos:hiddenLabel>
	<skos:definition xml:lang="en">The Fenner School of Environment and Society brings together economists and hydrologists, historians and ecologists, foresters, geographers and climatologists to work together on the big environmental problems facing contemporary society.</skos:definition>
	<dc:source rdf:datatype="http://www.w3.org/2001/XMLSchema#string">Australian Ocean Data Network Organisation Register</dc:source>
	<dc:publisher rdf:datatype="http://www.w3.org/2001/XMLSchema#string">eMarine Information Infrastructure (eMII)</dc:publisher>
	<skos:exactMatch rdf:resource="http://seadatanet.maris2.nl/v_edmo/print.asp?n_code=4291"/>
	<skos:narrower rdf:resource="http://vocab.aodn.org.au/def/organisation/entity/208"/>
	<skos:inScheme rdf:resource="http://vocab.aodn.org.au/def/organisation/1"/>
	<skos:broader rdf:resource="http://vocab.aodn.org.au/def/organisation/entity/194"/>
	<skos:scopeNote xml:lang="en">Replaces http://vocab.aodn.org.au/def/organisation/entity/204</skos:scopeNote>
	<dcterms:replaces rdf:resource="http://vocab.aodn.org.au/def/organisation/entity/204"/>
	<dcterms:replaces xml:lang="en">Centre for Resource and Environmental Studies (CRES), The Australian National University (ANU)</dcterms:replaces>
</rdf:Description>

<rdf:Description rdf:about="http://vocab.aodn.org.au/def/organisation/entity/209">
	<rdf:type rdf:resource="http://www.w3.org/2000/01/rdf-schema#Resource"/>
	<rdf:type rdf:resource="http://www.w3.org/2004/02/skos/core#Concept"/>
	<dcterms:modified rdf:datatype="http://www.w3.org/2001/XMLSchema#dateTime">2015-07-09T05:55:27Z</dcterms:modified>
	<dcterms:creator rdf:datatype="http://www.w3.org/2001/XMLSchema#string">Natalia Atkins</dcterms:creator>
	<dcterms:created rdf:datatype="http://www.w3.org/2001/XMLSchema#dateTime">2015-07-09T10:38:15Z</dcterms:created>
	<dcterms:contributor rdf:datatype="http://www.w3.org/2001/XMLSchema#string">Natalia_Atkins</dcterms:contributor>
	<skos:prefLabel xml:lang="en">North Australia Research Unit (NARU), The Australian National University (ANU)</skos:prefLabel>
	<skos:altLabel xml:lang="en"></skos:altLabel>
	<skos:altLabel xml:lang="en">North Australia Research Unit (NARU)</skos:altLabel>
	<skos:hiddenLabel xml:lang="en">NARU</skos:hiddenLabel>
	<skos:definition xml:lang="en">The North Australia Research Unit (NARU) was established in 1973 to specialise in research in north Australia and to provide a base and logistic support for Canberra-based members of The Australian National University (ANU) and members of other Australian and overseas institutions undertaking research in North Australia.</skos:definition>
	<dc:source rdf:datatype="http://www.w3.org/2001/XMLSchema#string">Australian Ocean Data Network Organisation Register</dc:source>
	<dc:publisher rdf:datatype="http://www.w3.org/2001/XMLSchema#string">eMarine Information Infrastructure (eMII)</dc:publisher>
	<skos:exactMatch rdf:resource="http://seadatanet.maris2.nl/v_edmo/print.asp?n_code=4293"/>
	<skos:inScheme rdf:resource="http://vocab.aodn.org.au/def/organisation/1"/>
	<skos:broader rdf:resource="http://vocab.aodn.org.au/def/organisation/entity/194"/>
</rdf:Description>

<rdf:Description rdf:about="http://seadatanet.maris2.nl/v_edmo/print.asp?n_code=1492">
	<rdf:type rdf:resource="http://www.w3.org/2000/01/rdf-schema#Resource"/>
</rdf:Description>

<rdf:Description rdf:about="http://seadatanet.maris2.nl/v_edmo/print.asp?n_code=1989">
	<rdf:type rdf:resource="http://www.w3.org/2000/01/rdf-schema#Resource"/>
</rdf:Description>

<rdf:Description rdf:about="http://seadatanet.maris2.nl/v_edmo/print.asp?n_code=4288">
	<rdf:type rdf:resource="http://www.w3.org/2000/01/rdf-schema#Resource"/>
</rdf:Description>

<rdf:Description rdf:about="http://seadatanet.maris2.nl/v_edmo/print.asp?n_code=4289">
	<rdf:type rdf:resource="http://www.w3.org/2000/01/rdf-schema#Resource"/>
</rdf:Description>

<rdf:Description rdf:about="http://seadatanet.maris2.nl/v_edmo/print.asp?n_code=4290">
	<rdf:type rdf:resource="http://www.w3.org/2000/01/rdf-schema#Resource"/>
</rdf:Description>

<rdf:Description rdf:about="http://seadatanet.maris2.nl/v_edmo/print.asp?n_code=4291">
	<rdf:type rdf:resource="http://www.w3.org/2000/01/rdf-schema#Resource"/>
</rdf:Description>

<rdf:Description rdf:about="http://vocab.aodn.org.au/def/organisation/entity/208">
	<rdf:type rdf:resource="http://www.w3.org/2000/01/rdf-schema#Resource"/>
	<rdf:type rdf:resource="http://www.w3.org/2004/02/skos/core#Concept"/>
	<dcterms:modified rdf:datatype="http://www.w3.org/2001/XMLSchema#dateTime">2015-07-14T00:13:54Z</dcterms:modified>
	<dcterms:creator rdf:datatype="http://www.w3.org/2001/XMLSchema#string">Natalia Atkins</dcterms:creator>
	<dcterms:created rdf:datatype="http://www.w3.org/2001/XMLSchema#dateTime">2015-07-09T10:38:15Z</dcterms:created>
	<dcterms:contributor rdf:datatype="http://www.w3.org/2001/XMLSchema#string">Natalia_Atkins</dcterms:contributor>
	<skos:prefLabel xml:lang="en">Integrated Catchment Assessment and Management Centre (iCAM), Fenner School of Environment and Society, The Australian National University (ANU)</skos:prefLabel>
	<skos:altLabel xml:lang="en"></skos:altLabel>
	<skos:altLabel xml:lang="en">Integrated Catchment Assessment and Management Centre (iCAM)</skos:altLabel>
	<skos:hiddenLabel xml:lang="en">iCAM</skos:hiddenLabel>
	<skos:definition xml:lang="en">iCAM (the Integrated Catchment Assessment and Management Centre) is a highly interdisciplinary research group consisting of social scientists, economists, hydrologists and interdisciplinary modellers.  iCAM’s mission is to develop and integrate the knowledge required to clarify management and policy options for sustaining vital water and related resources.</skos:definition>
	<dc:source rdf:datatype="http://www.w3.org/2001/XMLSchema#string">Australian Ocean Data Network Organisation Register</dc:source>
	<dc:publisher rdf:datatype="http://www.w3.org/2001/XMLSchema#string">eMarine Information Infrastructure (eMII)</dc:publisher>
	<skos:exactMatch rdf:resource="http://seadatanet.maris2.nl/v_edmo/print.asp?n_code=4292"/>
	<skos:inScheme rdf:resource="http://vocab.aodn.org.au/def/organisation/1"/>
	<skos:broader rdf:resource="http://vocab.aodn.org.au/def/organisation/entity/207"/>
</rdf:Description>

<rdf:Description rdf:about="http://seadatanet.maris2.nl/v_edmo/print.asp?n_code=4292">
	<rdf:type rdf:resource="http://www.w3.org/2000/01/rdf-schema#Resource"/>
</rdf:Description>

<rdf:Description rdf:about="http://seadatanet.maris2.nl/v_edmo/print.asp?n_code=4293">
	<rdf:type rdf:resource="http://www.w3.org/2000/01/rdf-schema#Resource"/>
</rdf:Description>

<rdf:Description rdf:about="http://seadatanet.maris2.nl/v_edmo/print.asp?n_code=4294">
	<rdf:type rdf:resource="http://www.w3.org/2000/01/rdf-schema#Resource"/>
</rdf:Description>

<rdf:Description rdf:about="http://vocab.aodn.org.au/def/organisation/entity/211">
	<rdf:type rdf:resource="http://www.w3.org/2000/01/rdf-schema#Resource"/>
	<rdf:type rdf:resource="http://www.w3.org/2004/02/skos/core#Concept"/>
	<dcterms:creator rdf:datatype="http://www.w3.org/2001/XMLSchema#string">Natalia Atkins</dcterms:creator>
	<dcterms:created rdf:datatype="http://www.w3.org/2001/XMLSchema#dateTime">2015-07-09T10:38:15Z</dcterms:created>
	<skos:prefLabel xml:lang="en">School of Mathematics and Statistics (SMS), The University of New South Wales (UNSW)</skos:prefLabel>
	<skos:altLabel xml:lang="en">School of Mathematics and Statistics (SMS)</skos:altLabel>
	<skos:hiddenLabel xml:lang="en">SMS</skos:hiddenLabel>
	<skos:definition xml:lang="en">The School's program cover a wide spectrum of courses in Pure and Applied Mathematics and Statistics.</skos:definition>
	<dc:source rdf:datatype="http://www.w3.org/2001/XMLSchema#string">Australian Ocean Data Network Organisation Register</dc:source>
	<dc:publisher rdf:datatype="http://www.w3.org/2001/XMLSchema#string">eMarine Information Infrastructure (eMII)</dc:publisher>
	<skos:inScheme rdf:resource="http://vocab.aodn.org.au/def/organisation/1"/>
	<skos:broader rdf:resource="http://vocab.aodn.org.au/def/organisation/entity/210"/>
</rdf:Description>

<rdf:Description rdf:about="http://vocab.aodn.org.au/def/organisation/entity/212">
	<rdf:type rdf:resource="http://www.w3.org/2000/01/rdf-schema#Resource"/>
	<rdf:type rdf:resource="http://www.w3.org/2004/02/skos/core#Concept"/>
	<dcterms:creator rdf:datatype="http://www.w3.org/2001/XMLSchema#string">Natalia Atkins</dcterms:creator>
	<dcterms:created rdf:datatype="http://www.w3.org/2001/XMLSchema#dateTime">2015-07-09T10:38:15Z</dcterms:created>
	<skos:prefLabel xml:lang="en">School of Biotechnology and Biomolecular Sciences (BABS), The University of New South Wales (UNSW)</skos:prefLabel>
	<skos:altLabel xml:lang="en">School of Biotechnology and Biomolecular Sciences (BABS)</skos:altLabel>
	<skos:hiddenLabel xml:lang="en">BABS</skos:hiddenLabel>
	<skos:definition xml:lang="en">The School of BABS﻿ teaches undergraduates, mentors postgraduate research students and conducts research in the disciplines of biotechnology, biochemistry, genetics, molecular biology, microbiology, environmental microbiology, medical microbiology and immunology﻿. BABS hosts or is a major player in a number of innovative centres and research initiatives: Ramaciotti Centre for Genomics, NSW Systems Biology Initiative, Centre for Marine BioInnovation and the Environmental Microbiology Initiative.﻿</skos:definition>
	<dc:source rdf:datatype="http://www.w3.org/2001/XMLSchema#string">Australian Ocean Data Network Organisation Register</dc:source>
	<dc:publisher rdf:datatype="http://www.w3.org/2001/XMLSchema#string">eMarine Information Infrastructure (eMII)</dc:publisher>
	<skos:exactMatch rdf:resource="http://seadatanet.maris2.nl/v_edmo/print.asp?n_code=4295"/>
	<skos:inScheme rdf:resource="http://vocab.aodn.org.au/def/organisation/1"/>
	<skos:broader rdf:resource="http://vocab.aodn.org.au/def/organisation/entity/210"/>
</rdf:Description>

<rdf:Description rdf:about="http://vocab.aodn.org.au/def/organisation/entity/213">
	<rdf:type rdf:resource="http://www.w3.org/2000/01/rdf-schema#Resource"/>
	<rdf:type rdf:resource="http://www.w3.org/2004/02/skos/core#Concept"/>
	<dcterms:creator rdf:datatype="http://www.w3.org/2001/XMLSchema#string">Natalia Atkins</dcterms:creator>
	<dcterms:created rdf:datatype="http://www.w3.org/2001/XMLSchema#dateTime">2015-07-09T10:38:15Z</dcterms:created>
	<skos:prefLabel xml:lang="en">School of Physical, Environmental and Mathematical Science (PEMS), The University of New South Wales (UNSW)</skos:prefLabel>
	<skos:altLabel xml:lang="en">School of Physical, Environmental and Mathematical Science (PEMS)</skos:altLabel>
	<skos:hiddenLabel xml:lang="en">PEMS</skos:hiddenLabel>
	<skos:definition xml:lang="en">The School of Physical, Environmental and Mathematical Sciences encompasses the disciplines of Chemistry, Geography, Mathematics, Statistics, Oceanography and Physics. The School of PEMS is one of four Schools at UNSW Canberra, the academic component of the Australian Defence Force Academy located in Canberra.</skos:definition>
	<dc:source rdf:datatype="http://www.w3.org/2001/XMLSchema#string">Australian Ocean Data Network Organisation Register</dc:source>
	<dc:publisher rdf:datatype="http://www.w3.org/2001/XMLSchema#string">eMarine Information Infrastructure (eMII)</dc:publisher>
	<skos:exactMatch rdf:resource="http://seadatanet.maris2.nl/v_edmo/print.asp?n_code=4296"/>
	<skos:inScheme rdf:resource="http://vocab.aodn.org.au/def/organisation/1"/>
	<skos:broader rdf:resource="http://vocab.aodn.org.au/def/organisation/entity/210"/>
</rdf:Description>

<rdf:Description rdf:about="http://vocab.aodn.org.au/def/organisation/entity/214">
	<rdf:type rdf:resource="http://www.w3.org/2000/01/rdf-schema#Resource"/>
	<rdf:type rdf:resource="http://www.w3.org/2004/02/skos/core#Concept"/>
	<dcterms:creator rdf:datatype="http://www.w3.org/2001/XMLSchema#string">Natalia Atkins</dcterms:creator>
	<dcterms:created rdf:datatype="http://www.w3.org/2001/XMLSchema#dateTime">2015-07-09T10:38:15Z</dcterms:created>
	<skos:prefLabel xml:lang="en">School of Biological, Earth and Environmental Sciences (BEES), The University of New South Wales (UNSW)</skos:prefLabel>
	<skos:altLabel xml:lang="en">School of Biological, Earth and Environmental Sciences (BEES)</skos:altLabel>
	<skos:hiddenLabel xml:lang="en">BEES</skos:hiddenLabel>
	<skos:definition xml:lang="en">The University of New South Wales has a national and international reputation for quality education and research in many fields of biological, geographical and geological sciences. The School of Biological, Earth and Environmental Sciences (BEES) incorporates these environmentally relevant disciplines enabling the School to offer a comprehensive education in the traditional, mainstream disciplines of Biology, Geography and Geology. This also allows us to provide our students with opportunities for interdisciplinary and multidisciplinary studies, notably in the Marine and Environmental Sciences.</skos:definition>
	<dc:source rdf:datatype="http://www.w3.org/2001/XMLSchema#string">Australian Ocean Data Network Organisation Register</dc:source>
	<dc:publisher rdf:datatype="http://www.w3.org/2001/XMLSchema#string">eMarine Information Infrastructure (eMII)</dc:publisher>
	<skos:exactMatch rdf:resource="http://seadatanet.maris2.nl/v_edmo/print.asp?n_code=1487"/>
	<skos:inScheme rdf:resource="http://vocab.aodn.org.au/def/organisation/1"/>
	<skos:broader rdf:resource="http://vocab.aodn.org.au/def/organisation/entity/210"/>
</rdf:Description>

<rdf:Description rdf:about="http://seadatanet.maris2.nl/v_edmo/print.asp?n_code=4295">
	<rdf:type rdf:resource="http://www.w3.org/2000/01/rdf-schema#Resource"/>
</rdf:Description>

<rdf:Description rdf:about="http://seadatanet.maris2.nl/v_edmo/print.asp?n_code=4296">
	<rdf:type rdf:resource="http://www.w3.org/2000/01/rdf-schema#Resource"/>
</rdf:Description>

<rdf:Description rdf:about="http://seadatanet.maris2.nl/v_edmo/print.asp?n_code=1487">
	<rdf:type rdf:resource="http://www.w3.org/2000/01/rdf-schema#Resource"/>
</rdf:Description>

<rdf:Description rdf:about="http://seadatanet.maris2.nl/v_edmo/print.asp?n_code=1490">
	<rdf:type rdf:resource="http://www.w3.org/2000/01/rdf-schema#Resource"/>
</rdf:Description>

<rdf:Description rdf:about="http://vocab.aodn.org.au/def/organisation/entity/269">
	<rdf:type rdf:resource="http://www.w3.org/2000/01/rdf-schema#Resource"/>
	<rdf:type rdf:resource="http://www.w3.org/2004/02/skos/core#Concept"/>
	<dcterms:creator rdf:datatype="http://www.w3.org/2001/XMLSchema#string">Natalia Atkins</dcterms:creator>
	<dcterms:created rdf:datatype="http://www.w3.org/2001/XMLSchema#dateTime">2015-07-08T10:38:15Z</dcterms:created>
	<skos:prefLabel xml:lang="en">School of Environmental Sciences, Charles Sturt University (CSU)</skos:prefLabel>
	<skos:altLabel xml:lang="en">School of Environmental Sciences</skos:altLabel>
	<skos:hiddenLabel xml:lang="en"></skos:hiddenLabel>
	<skos:definition xml:lang="en">The School of Environmental Sciences, Charles Sturt University (CSU) is located at the Albury-Wodonga campus. It has courses in environmental science, park management, natural resource management, spatial science, and outdoor recreation and ecotourism.</skos:definition>
	<dc:source rdf:datatype="http://www.w3.org/2001/XMLSchema#string">Australian Ocean Data Network Organisation Register</dc:source>
	<dc:publisher rdf:datatype="http://www.w3.org/2001/XMLSchema#string">eMarine Information Infrastructure (eMII)</dc:publisher>
	<skos:exactMatch rdf:resource="http://seadatanet.maris2.nl/v_edmo/print.asp?n_code=4254"/>
	<skos:inScheme rdf:resource="http://vocab.aodn.org.au/def/organisation/1"/>
	<skos:broader rdf:resource="http://vocab.aodn.org.au/def/organisation/entity/268"/>
</rdf:Description>

<rdf:Description rdf:about="http://seadatanet.maris2.nl/v_edmo/print.asp?n_code=4253">
	<rdf:type rdf:resource="http://www.w3.org/2000/01/rdf-schema#Resource"/>
</rdf:Description>

<rdf:Description rdf:about="http://seadatanet.maris2.nl/v_edmo/print.asp?n_code=4254">
	<rdf:type rdf:resource="http://www.w3.org/2000/01/rdf-schema#Resource"/>
</rdf:Description>

<rdf:Description rdf:about="http://vocab.aodn.org.au/def/organisation/entity/271">
	<rdf:type rdf:resource="http://www.w3.org/2000/01/rdf-schema#Resource"/>
	<rdf:type rdf:resource="http://www.w3.org/2004/02/skos/core#Concept"/>
	<dcterms:creator rdf:datatype="http://www.w3.org/2001/XMLSchema#string">Natalia Atkins</dcterms:creator>
	<dcterms:created rdf:datatype="http://www.w3.org/2001/XMLSchema#dateTime">2015-07-16T10:38:15Z</dcterms:created>
	<skos:prefLabel xml:lang="en">School of Humanities and Social Sciences (SHSS), Deakin University</skos:prefLabel>
	<skos:altLabel xml:lang="en">School of Humanities and Social Sciences (SHSS)</skos:altLabel>
	<skos:hiddenLabel xml:lang="en">SHSS</skos:hiddenLabel>
	<skos:definition xml:lang="en">The School of Humanities and Social Sciences, provides for the study of Australian Studies, Anthropology, Criminology, History, International Relations, Politics, Sociology, Middle East Studies, and Philosophy. You can also learn Chinese, Arabic, Indonesian and Spanish.</skos:definition>
	<dc:source rdf:datatype="http://www.w3.org/2001/XMLSchema#string">Australian Ocean Data Network Organisation Register</dc:source>
	<dc:publisher rdf:datatype="http://www.w3.org/2001/XMLSchema#string">eMarine Information Infrastructure (eMII)</dc:publisher>
	<skos:inScheme rdf:resource="http://vocab.aodn.org.au/def/organisation/1"/>
	<skos:broader rdf:resource="http://vocab.aodn.org.au/def/organisation/entity/270"/>
</rdf:Description>

<rdf:Description rdf:about="http://vocab.aodn.org.au/def/organisation/entity/272">
	<rdf:type rdf:resource="http://www.w3.org/2000/01/rdf-schema#Resource"/>
	<rdf:type rdf:resource="http://www.w3.org/2004/02/skos/core#Concept"/>
	<dcterms:creator rdf:datatype="http://www.w3.org/2001/XMLSchema#string">Natalia Atkins</dcterms:creator>
	<dcterms:created rdf:datatype="http://www.w3.org/2001/XMLSchema#dateTime">2015-07-16T10:38:15Z</dcterms:created>
	<skos:prefLabel xml:lang="en">School of Ecology and Environment, Deakin University</skos:prefLabel>
	<skos:altLabel xml:lang="en">School of Ecology and Environment</skos:altLabel>
	<skos:hiddenLabel xml:lang="en"></skos:hiddenLabel>
	<skos:definition xml:lang="en">Deakin University's School of Ecology and Environment was part of the Faculty of Science and Technology. Areas the School specialised in included: Ecology, Earth science, Environmental Science and Management as well as Aquatic Sciences. The school no longer exists and was incorporated into the School of Life and Environmental Sciences, Faculty of Science and Technology. (Courtesy of Encyclopedia of Australian Science)</skos:definition>
	<dc:source rdf:datatype="http://www.w3.org/2001/XMLSchema#string">Australian Ocean Data Network Organisation Register</dc:source>
	<dc:publisher rdf:datatype="http://www.w3.org/2001/XMLSchema#string">eMarine Information Infrastructure (eMII)</dc:publisher>
	<skos:inScheme rdf:resource="http://vocab.aodn.org.au/def/organisation/1"/>
	<skos:broader rdf:resource="http://vocab.aodn.org.au/def/organisation/entity/270"/>
	<skos:scopeNote xml:lang="en">Organisation no longer exists</skos:scopeNote>
	<skos:scopeNote xml:lang="en">Organisation no longer exists. Replaced by http://vocab.aodn.org.au/def/organisation/entity/273</skos:scopeNote>
	<dcterms:isReplacedBy rdf:resource="http://vocab.aodn.org.au/def/organisation/entity/273"/>
	<dcterms:isReplacedBy xml:lang="en">School of Life and Environmental Sciences (LES), Deakin University</dcterms:isReplacedBy>
</rdf:Description>

<rdf:Description rdf:about="http://vocab.aodn.org.au/def/organisation/entity/273">
	<rdf:type rdf:resource="http://www.w3.org/2000/01/rdf-schema#Resource"/>
	<rdf:type rdf:resource="http://www.w3.org/2004/02/skos/core#Concept"/>
	<dcterms:creator rdf:datatype="http://www.w3.org/2001/XMLSchema#string">Natalia Atkins</dcterms:creator>
	<dcterms:created rdf:datatype="http://www.w3.org/2001/XMLSchema#dateTime">2015-07-16T10:38:15Z</dcterms:created>
	<skos:prefLabel xml:lang="en">School of Life and Environmental Sciences (LES), Deakin University</skos:prefLabel>
	<skos:altLabel xml:lang="en">School of Life and Environmental Sciences (LES)</skos:altLabel>
	<skos:hiddenLabel xml:lang="en">LES</skos:hiddenLabel>
	<skos:definition xml:lang="en">The School of Live and Environmental Sciences, has the following study areas: biological science, biomedical science, environmental management and sustainability, fisheries and agriculture, forensic science, marine biology, wildlfie and conservation biology, and zoology and animal science.</skos:definition>
	<dc:source rdf:datatype="http://www.w3.org/2001/XMLSchema#string">Australian Ocean Data Network Organisation Register</dc:source>
	<dc:publisher rdf:datatype="http://www.w3.org/2001/XMLSchema#string">eMarine Information Infrastructure (eMII)</dc:publisher>
	<skos:exactMatch rdf:resource="http://seadatanet.maris2.nl/v_edmo/print.asp?n_code=4261"/>
	<skos:inScheme rdf:resource="http://vocab.aodn.org.au/def/organisation/1"/>
	<skos:broader rdf:resource="http://vocab.aodn.org.au/def/organisation/entity/270"/>
	<skos:scopeNote xml:lang="en">Replaces http://vocab.aodn.org.au/def/organisation/entity/272</skos:scopeNote>
	<dcterms:replaces rdf:resource="http://vocab.aodn.org.au/def/organisation/entity/272"/>
	<dcterms:replaces xml:lang="en">School of Ecology and Environment, Deakin University</dcterms:replaces>
</rdf:Description>

<rdf:Description rdf:about="http://seadatanet.maris2.nl/v_edmo/print.asp?n_code=4260">
	<rdf:type rdf:resource="http://www.w3.org/2000/01/rdf-schema#Resource"/>
</rdf:Description>

<rdf:Description rdf:about="http://seadatanet.maris2.nl/v_edmo/print.asp?n_code=4261">
	<rdf:type rdf:resource="http://www.w3.org/2000/01/rdf-schema#Resource"/>
</rdf:Description>

<rdf:Description rdf:about="http://vocab.aodn.org.au/def/organisation/entity/275">
	<rdf:type rdf:resource="http://www.w3.org/2000/01/rdf-schema#Resource"/>
	<rdf:type rdf:resource="http://www.w3.org/2004/02/skos/core#Concept"/>
	<dcterms:modified rdf:datatype="http://www.w3.org/2001/XMLSchema#dateTime">2015-07-16T06:06:08Z</dcterms:modified>
	<dcterms:creator rdf:datatype="http://www.w3.org/2001/XMLSchema#string">Natalia Atkins</dcterms:creator>
	<dcterms:created rdf:datatype="http://www.w3.org/2001/XMLSchema#dateTime">2015-07-16T10:38:15Z</dcterms:created>
	<dcterms:contributor rdf:datatype="http://www.w3.org/2001/XMLSchema#string">Natalia_Atkins</dcterms:contributor>
	<skos:prefLabel xml:lang="en">School of Natural Sciences, Edith Cowan University (ECU)</skos:prefLabel>
	<skos:altLabel xml:lang="en">School of Natural Sciences</skos:altLabel>
	<skos:hiddenLabel xml:lang="en"></skos:hiddenLabel>
	<skos:definition xml:lang="en">The school is located at ECU’s Joondalup Campus. It includes laboratories as well as a host of research facilities including specialist laboratories for ecology, plant tissue culture, analytical and environmental chemistry, molecular biology, freshwater and marine science, and geographic information systems. We also provide constant temperature and aquarium rooms, outdoor experimental aquatic facilities, glasshouses, shade houses and operate two large surveyed boats for marine work, several dinghies and a fleet of 4WD and 2WD vehicles.</skos:definition>
	<dc:source rdf:datatype="http://www.w3.org/2001/XMLSchema#string">Australian Ocean Data Network Organisation Register</dc:source>
	<dc:publisher rdf:datatype="http://www.w3.org/2001/XMLSchema#string">eMarine Information Infrastructure (eMII)</dc:publisher>
	<skos:exactMatch rdf:resource="http://seadatanet.maris2.nl/v_edmo/print.asp?n_code=4263"/>
	<skos:narrower rdf:resource="http://vocab.aodn.org.au/def/organisation/entity/277"/>
	<skos:narrower rdf:resource="http://vocab.aodn.org.au/def/organisation/entity/276"/>
	<skos:inScheme rdf:resource="http://vocab.aodn.org.au/def/organisation/1"/>
	<skos:broader rdf:resource="http://vocab.aodn.org.au/def/organisation/entity/274"/>
</rdf:Description>

<rdf:Description rdf:about="http://seadatanet.maris2.nl/v_edmo/print.asp?n_code=4262">
	<rdf:type rdf:resource="http://www.w3.org/2000/01/rdf-schema#Resource"/>
</rdf:Description>

<rdf:Description rdf:about="http://seadatanet.maris2.nl/v_edmo/print.asp?n_code=4263">
	<rdf:type rdf:resource="http://www.w3.org/2000/01/rdf-schema#Resource"/>
</rdf:Description>

<rdf:Description rdf:about="http://vocab.aodn.org.au/def/organisation/entity/277">
	<rdf:type rdf:resource="http://www.w3.org/2000/01/rdf-schema#Resource"/>
	<rdf:type rdf:resource="http://www.w3.org/2004/02/skos/core#Concept"/>
	<dcterms:modified rdf:datatype="http://www.w3.org/2001/XMLSchema#dateTime">2015-07-16T06:05:54Z</dcterms:modified>
	<dcterms:creator rdf:datatype="http://www.w3.org/2001/XMLSchema#string">Natalia Atkins</dcterms:creator>
	<dcterms:created rdf:datatype="http://www.w3.org/2001/XMLSchema#dateTime">2015-07-16T10:38:15Z</dcterms:created>
	<dcterms:contributor rdf:datatype="http://www.w3.org/2001/XMLSchema#string">Natalia_Atkins</dcterms:contributor>
	<skos:prefLabel xml:lang="en">Centre for Ecosystem Management, School of Natural Sciences, Edith Cowan University (ECU)</skos:prefLabel>
	<skos:altLabel xml:lang="en">Centre for Ecosystem Management</skos:altLabel>
	<skos:hiddenLabel xml:lang="en"></skos:hiddenLabel>
	<skos:definition xml:lang="en">The Centre for Ecosystem Management's  researchers have diverse research interests that include freshwater ecosystems, ecological water requirements, conservation biology, ecophysiology, semi-arid environments, the ecology of forests and woodlands and the cultural ecology of wetlands and other landscapes.</skos:definition>
	<dc:source rdf:datatype="http://www.w3.org/2001/XMLSchema#string">Australian Ocean Data Network Organisation Register</dc:source>
	<dc:publisher rdf:datatype="http://www.w3.org/2001/XMLSchema#string">eMarine Information Infrastructure (eMII)</dc:publisher>
	<skos:exactMatch rdf:resource="http://seadatanet.maris2.nl/v_edmo/print.asp?n_code=4265"/>
	<skos:inScheme rdf:resource="http://vocab.aodn.org.au/def/organisation/1"/>
	<skos:broader rdf:resource="http://vocab.aodn.org.au/def/organisation/entity/275"/>
</rdf:Description>

<rdf:Description rdf:about="http://vocab.aodn.org.au/def/organisation/entity/276">
	<rdf:type rdf:resource="http://www.w3.org/2000/01/rdf-schema#Resource"/>
	<rdf:type rdf:resource="http://www.w3.org/2004/02/skos/core#Concept"/>
	<dcterms:modified rdf:datatype="http://www.w3.org/2001/XMLSchema#dateTime">2015-07-16T06:06:13Z</dcterms:modified>
	<dcterms:creator rdf:datatype="http://www.w3.org/2001/XMLSchema#string">Natalia Atkins</dcterms:creator>
	<dcterms:created rdf:datatype="http://www.w3.org/2001/XMLSchema#dateTime">2015-07-16T10:38:15Z</dcterms:created>
	<dcterms:contributor rdf:datatype="http://www.w3.org/2001/XMLSchema#string">Natalia_Atkins</dcterms:contributor>
	<skos:prefLabel xml:lang="en">Centre for Marine Ecosystems Research (CMER), School of Natural Sciences, Edith Cowan University (ECU)</skos:prefLabel>
	<skos:altLabel xml:lang="en">Centre for Marine Ecosystems Research (CMER)</skos:altLabel>
	<skos:hiddenLabel xml:lang="en">CMER</skos:hiddenLabel>
	<skos:definition xml:lang="en">The Centre for Marine Ecosystems Research (CMER) uses applied and fundamental research to improve understanding of the ecological processes of coastal marine systems, and how these respond to both natural and human induced pressures.</skos:definition>
	<dc:source rdf:datatype="http://www.w3.org/2001/XMLSchema#string">Australian Ocean Data Network Organisation Register</dc:source>
	<dc:publisher rdf:datatype="http://www.w3.org/2001/XMLSchema#string">eMarine Information Infrastructure (eMII)</dc:publisher>
	<skos:exactMatch rdf:resource="http://seadatanet.maris2.nl/v_edmo/print.asp?n_code=4264"/>
	<skos:inScheme rdf:resource="http://vocab.aodn.org.au/def/organisation/1"/>
	<skos:broader rdf:resource="http://vocab.aodn.org.au/def/organisation/entity/275"/>
</rdf:Description>

<rdf:Description rdf:about="http://seadatanet.maris2.nl/v_edmo/print.asp?n_code=4264">
	<rdf:type rdf:resource="http://www.w3.org/2000/01/rdf-schema#Resource"/>
</rdf:Description>

<rdf:Description rdf:about="http://seadatanet.maris2.nl/v_edmo/print.asp?n_code=4265">
	<rdf:type rdf:resource="http://www.w3.org/2000/01/rdf-schema#Resource"/>
</rdf:Description>

<rdf:Description rdf:about="http://seadatanet.maris2.nl/v_edmo/print.asp?n_code=4269">
	<rdf:type rdf:resource="http://www.w3.org/2000/01/rdf-schema#Resource"/>
</rdf:Description>

<rdf:Description rdf:about="http://vocab.aodn.org.au/def/organisation/entity/342">
	<rdf:type rdf:resource="http://www.w3.org/2000/01/rdf-schema#Resource"/>
	<rdf:type rdf:resource="http://www.w3.org/2004/02/skos/core#Concept"/>
	<dcterms:creator rdf:datatype="http://www.w3.org/2001/XMLSchema#string">Natalia Atkins</dcterms:creator>
	<dcterms:created rdf:datatype="http://www.w3.org/2001/XMLSchema#dateTime">2015-08-04T10:38:15Z</dcterms:created>
	<skos:prefLabel xml:lang="en">Australian Rivers Institute (ARI), Griffith University (GU)</skos:prefLabel>
	<skos:altLabel xml:lang="en">Australian Rivers Institute (ARI)</skos:altLabel>
	<skos:hiddenLabel xml:lang="en">ARI</skos:hiddenLabel>
	<skos:definition xml:lang="en">This is Australia’s largest university aquatic ecosystem research groups with globally recognised expertise in river, catchment and coastal ecosystems and the interaction with these systems in society. It brings together 130 staff and post-graduate students at the Nathan and Gold Coast campuses. Research focuses on a "source to sea" philosophy delivering six themes: Catchment and river ecosystem processes; Coastal and estuarine ecosystem processes; Integration, modelling and catchment management; Rehabilitation science and environmental flows; Aquatic biodiversity and conservation; and Aquatic ecosystem monitoring and assessment.</skos:definition>
	<dc:source rdf:datatype="http://www.w3.org/2001/XMLSchema#string">Australian Ocean Data Network Organisation Register</dc:source>
	<dc:publisher rdf:datatype="http://www.w3.org/2001/XMLSchema#string">eMarine Information Infrastructure (eMII)</dc:publisher>
	<skos:exactMatch rdf:resource="http://seadatanet.maris2.nl/v_edmo/print.asp?n_code=4367"/>
	<skos:inScheme rdf:resource="http://vocab.aodn.org.au/def/organisation/1"/>
	<skos:broader rdf:resource="http://vocab.aodn.org.au/def/organisation/entity/278"/>
</rdf:Description>

<rdf:Description rdf:about="http://vocab.aodn.org.au/def/organisation/entity/411">
	<rdf:type rdf:resource="http://www.w3.org/2000/01/rdf-schema#Resource"/>
	<rdf:type rdf:resource="http://www.w3.org/2004/02/skos/core#Concept"/>
	<dcterms:creator rdf:datatype="http://www.w3.org/2001/XMLSchema#string">Natalia Atkins</dcterms:creator>
	<dcterms:created rdf:datatype="http://www.w3.org/2001/XMLSchema#dateTime">2015-11-05T10:38:15Z</dcterms:created>
	<skos:prefLabel xml:lang="en">National Climate Change Adaptation Research Facility (NCCARF), Griffith University (GU)</skos:prefLabel>
	<skos:altLabel xml:lang="en">National Climate Change Adaptation Research Facility (NCCARF)</skos:altLabel>
	<skos:hiddenLabel xml:lang="en">NCCARF</skos:hiddenLabel>
	<skos:definition xml:lang="en">The National Climate Change Adaptation Research Facility (NCCARF) works to support decision makers throughout Australia as they prepare for and manage the risks of climate change and sea-level rise. Based at Griffith University on the Gold Coast, NCCARF has a national focus across Australia to build resilience to climate change in government, NGOs and the private sector.</skos:definition>
	<dc:source rdf:datatype="http://www.w3.org/2001/XMLSchema#string">Australian Ocean Data Network Organisation Register</dc:source>
	<dc:publisher rdf:datatype="http://www.w3.org/2001/XMLSchema#string">eMarine Information Infrastructure (eMII)</dc:publisher>
	<skos:exactMatch rdf:resource="http://seadatanet.maris2.nl/v_edmo/print.asp?n_code=4443"/>
	<skos:inScheme rdf:resource="http://vocab.aodn.org.au/def/organisation/1"/>
	<skos:broader rdf:resource="http://vocab.aodn.org.au/def/organisation/entity/278"/>
</rdf:Description>

<rdf:Description rdf:about="http://vocab.aodn.org.au/def/organisation/entity/288">
	<rdf:type rdf:resource="http://www.w3.org/2000/01/rdf-schema#Resource"/>
	<rdf:type rdf:resource="http://www.w3.org/2004/02/skos/core#Concept"/>
	<dcterms:creator rdf:datatype="http://www.w3.org/2001/XMLSchema#string">Natalia Atkins</dcterms:creator>
	<dcterms:created rdf:datatype="http://www.w3.org/2001/XMLSchema#dateTime">2015-07-17T10:38:15Z</dcterms:created>
	<skos:prefLabel xml:lang="en">Department of Biological Sciences, Macquarie University</skos:prefLabel>
	<skos:altLabel xml:lang="en">Department of Biological Sciences</skos:altLabel>
	<skos:hiddenLabel xml:lang="en"></skos:hiddenLabel>
	<skos:definition xml:lang="en">This department integrates research and teaching across all levels of biological organisation as well as across a diversity of taxa. It's work links structure with function and processes that influence the evolution and ecology of organisms, using models ranging from microbes through to fungi, plants and animals.</skos:definition>
	<dc:source rdf:datatype="http://www.w3.org/2001/XMLSchema#string">Australian Ocean Data Network Organisation Register</dc:source>
	<dc:publisher rdf:datatype="http://www.w3.org/2001/XMLSchema#string">eMarine Information Infrastructure (eMII)</dc:publisher>
	<skos:exactMatch rdf:resource="http://seadatanet.maris2.nl/v_edmo/print.asp?n_code=4277"/>
	<skos:inScheme rdf:resource="http://vocab.aodn.org.au/def/organisation/1"/>
	<skos:broader rdf:resource="http://vocab.aodn.org.au/def/organisation/entity/287"/>
</rdf:Description>

<rdf:Description rdf:about="http://seadatanet.maris2.nl/v_edmo/print.asp?n_code=4276">
	<rdf:type rdf:resource="http://www.w3.org/2000/01/rdf-schema#Resource"/>
</rdf:Description>

<rdf:Description rdf:about="http://seadatanet.maris2.nl/v_edmo/print.asp?n_code=4277">
	<rdf:type rdf:resource="http://www.w3.org/2000/01/rdf-schema#Resource"/>
</rdf:Description>

<rdf:Description rdf:about="http://vocab.aodn.org.au/def/organisation/entity/363">
	<rdf:type rdf:resource="http://www.w3.org/2000/01/rdf-schema#Resource"/>
	<rdf:type rdf:resource="http://www.w3.org/2004/02/skos/core#Concept"/>
	<dcterms:creator rdf:datatype="http://www.w3.org/2001/XMLSchema#string">Natalia Atkins</dcterms:creator>
	<dcterms:created rdf:datatype="http://www.w3.org/2001/XMLSchema#dateTime">2015-08-06T10:38:15Z</dcterms:created>
	<skos:prefLabel xml:lang="en">School of Management, University of Ottawa</skos:prefLabel>
	<skos:altLabel xml:lang="en">School of Management</skos:altLabel>
	<skos:hiddenLabel xml:lang="en"></skos:hiddenLabel>
	<skos:definition xml:lang="en">This school is now known as the Tefler School of Management.</skos:definition>
	<dc:source rdf:datatype="http://www.w3.org/2001/XMLSchema#string">Australian Ocean Data Network Organisation Register</dc:source>
	<dc:publisher rdf:datatype="http://www.w3.org/2001/XMLSchema#string">eMarine Information Infrastructure (eMMI)</dc:publisher>
	<skos:inScheme rdf:resource="http://vocab.aodn.org.au/def/organisation/1"/>
	<skos:broader rdf:resource="http://vocab.aodn.org.au/def/organisation/entity/327"/>
	<skos:scopeNote xml:lang="en">Organisation no longer exists</skos:scopeNote>
</rdf:Description>

<rdf:Description rdf:about="http://vocab.aodn.org.au/def/organisation/entity/304">
	<rdf:type rdf:resource="http://www.w3.org/2000/01/rdf-schema#Resource"/>
	<rdf:type rdf:resource="http://www.w3.org/2004/02/skos/core#Concept"/>
	<dcterms:creator rdf:datatype="http://www.w3.org/2001/XMLSchema#string">Natalia Atkins</dcterms:creator>
	<dcterms:created rdf:datatype="http://www.w3.org/2001/XMLSchema#dateTime">2015-07-22T10:38:15Z</dcterms:created>
	<skos:prefLabel xml:lang="en">School of Biological, Environmental and Chemical Sciences, Northern Territory University (NTU)</skos:prefLabel>
	<skos:altLabel xml:lang="en">School of Biological, Environmental and Chemical Sciences</skos:altLabel>
	<skos:hiddenLabel xml:lang="en"></skos:hiddenLabel>
	<skos:definition xml:lang="en">This school ceased to exist when the Northern Territory University became part of the new Charles Darwin University in 2004.</skos:definition>
	<dc:source rdf:datatype="http://www.w3.org/2001/XMLSchema#string">Australian Ocean Data Network Organisation Register</dc:source>
	<dc:publisher rdf:datatype="http://www.w3.org/2001/XMLSchema#string">eMarine Information Infrastructure (eMII)</dc:publisher>
	<skos:inScheme rdf:resource="http://vocab.aodn.org.au/def/organisation/1"/>
	<skos:broader rdf:resource="http://vocab.aodn.org.au/def/organisation/entity/303"/>
	<skos:scopeNote xml:lang="en">Organisation no longer exists</skos:scopeNote>
</rdf:Description>

<rdf:Description rdf:about="http://vocab.aodn.org.au/def/organisation/entity/306">
	<rdf:type rdf:resource="http://www.w3.org/2000/01/rdf-schema#Resource"/>
	<rdf:type rdf:resource="http://www.w3.org/2004/02/skos/core#Concept"/>
	<dcterms:creator rdf:datatype="http://www.w3.org/2001/XMLSchema#string">Natalia Atkins</dcterms:creator>
	<dcterms:created rdf:datatype="http://www.w3.org/2001/XMLSchema#dateTime">2015-07-22T10:38:15Z</dcterms:created>
	<skos:prefLabel xml:lang="en">School of Biological Sciences, The University of Adelaide</skos:prefLabel>
	<skos:altLabel xml:lang="en">School of Biological Sciences</skos:altLabel>
	<skos:hiddenLabel xml:lang="en"></skos:hiddenLabel>
	<skos:definition xml:lang="en">The School of Biological Sciences was formed in 2015, and brings together parts of the former schools of Earth and Environmental Sciences (EES), and Molecular and Biomedical Sciences (MBS). The School of Biological Sciences was formed to coordinate and consolidate the University's research and teaching in Ecology and Environmental Science; Genetics and Evolution; and Molecular and Cellular Biology.</skos:definition>
	<dc:source rdf:datatype="http://www.w3.org/2001/XMLSchema#string">Australian Ocean Data Network Organisation Register</dc:source>
	<dc:publisher rdf:datatype="http://www.w3.org/2001/XMLSchema#string">eMarine Information Infrastructure (eMII)</dc:publisher>
	<skos:exactMatch rdf:resource="http://seadatanet.maris2.nl/v_edmo/print.asp?n_code=4317"/>
	<skos:inScheme rdf:resource="http://vocab.aodn.org.au/def/organisation/1"/>
	<skos:broader rdf:resource="http://vocab.aodn.org.au/def/organisation/entity/305"/>
</rdf:Description>

<rdf:Description rdf:about="http://seadatanet.maris2.nl/v_edmo/print.asp?n_code=4028">
	<rdf:type rdf:resource="http://www.w3.org/2000/01/rdf-schema#Resource"/>
</rdf:Description>

<rdf:Description rdf:about="http://seadatanet.maris2.nl/v_edmo/print.asp?n_code=4317">
	<rdf:type rdf:resource="http://www.w3.org/2000/01/rdf-schema#Resource"/>
</rdf:Description>

<rdf:Description rdf:about="http://vocab.aodn.org.au/def/organisation/entity/308">
	<rdf:type rdf:resource="http://www.w3.org/2000/01/rdf-schema#Resource"/>
	<rdf:type rdf:resource="http://www.w3.org/2004/02/skos/core#Concept"/>
	<dcterms:creator rdf:datatype="http://www.w3.org/2001/XMLSchema#string">Natalia Atkins</dcterms:creator>
	<dcterms:created rdf:datatype="http://www.w3.org/2001/XMLSchema#dateTime">2015-07-22T10:38:15Z</dcterms:created>
	<skos:prefLabel xml:lang="en">Institute for Applied Ecology (IAE), University of Canberra (UC)</skos:prefLabel>
	<skos:altLabel xml:lang="en">Institute for Applied Ecology (IAE)</skos:altLabel>
	<skos:hiddenLabel xml:lang="en">IAE</skos:hiddenLabel>
	<skos:definition xml:lang="en">The Institute for Applied Ecology's core purpose is to undertake high quality research which improves our understanding of the environment to enhance decision-making for natural resource management and sustainable development. The Institute undertakes broadly based environmental research across four interrelated science programs: Conservation Ecology, Water Science, Ecochemistry and Toxicology, and Environmental Genetics and Genomics.</skos:definition>
	<dc:source rdf:datatype="http://www.w3.org/2001/XMLSchema#string">Australian Ocean Data Network Organisation Register</dc:source>
	<dc:publisher rdf:datatype="http://www.w3.org/2001/XMLSchema#string">eMarine Information Infrastructure (eMII)</dc:publisher>
	<skos:exactMatch rdf:resource="http://seadatanet.maris2.nl/v_edmo/print.asp?n_code=4319"/>
	<skos:inScheme rdf:resource="http://vocab.aodn.org.au/def/organisation/1"/>
	<skos:broader rdf:resource="http://vocab.aodn.org.au/def/organisation/entity/307"/>
</rdf:Description>

<rdf:Description rdf:about="http://seadatanet.maris2.nl/v_edmo/print.asp?n_code=4318">
	<rdf:type rdf:resource="http://www.w3.org/2000/01/rdf-schema#Resource"/>
</rdf:Description>

<rdf:Description rdf:about="http://seadatanet.maris2.nl/v_edmo/print.asp?n_code=4319">
	<rdf:type rdf:resource="http://www.w3.org/2000/01/rdf-schema#Resource"/>
</rdf:Description>

<rdf:Description rdf:about="http://vocab.aodn.org.au/def/organisation/entity/310">
	<rdf:type rdf:resource="http://www.w3.org/2000/01/rdf-schema#Resource"/>
	<rdf:type rdf:resource="http://www.w3.org/2004/02/skos/core#Concept"/>
	<dcterms:creator rdf:datatype="http://www.w3.org/2001/XMLSchema#string">Natalia Atkins</dcterms:creator>
	<dcterms:created rdf:datatype="http://www.w3.org/2001/XMLSchema#dateTime">2015-07-22T10:38:15Z</dcterms:created>
	<skos:prefLabel xml:lang="en">School of Botany, The University of Melbourne</skos:prefLabel>
	<skos:altLabel xml:lang="en">School of Botany</skos:altLabel>
	<skos:hiddenLabel xml:lang="en"></skos:hiddenLabel>
	<skos:definition xml:lang="en">The school offers training and research opportunities in the fields of: plant cell biology, molecular plant biology and biotechnology, plant diseases, plant physiology, ecology and environmental science, marine botany, plant systematics, and fossils and evolutionary biology. The school became part of the School of Biosciences in 2015.</skos:definition>
	<dc:source rdf:datatype="http://www.w3.org/2001/XMLSchema#string">Australian Ocean Data Network Organisation Register</dc:source>
	<dc:publisher rdf:datatype="http://www.w3.org/2001/XMLSchema#string">eMarine Information Infrastructure (eMII)</dc:publisher>
	<skos:inScheme rdf:resource="http://vocab.aodn.org.au/def/organisation/1"/>
	<skos:broader rdf:resource="http://vocab.aodn.org.au/def/organisation/entity/309"/>
	<skos:scopeNote xml:lang="en">Organisation no longer exists</skos:scopeNote>
	<skos:scopeNote xml:lang="en">Organisation no longer exists. Replaced by http://vocab.aodn.org.au/def/organisation/entity/312</skos:scopeNote>
	<dcterms:isReplacedBy rdf:resource="http://vocab.aodn.org.au/def/organisation/entity/312"/>
	<dcterms:isReplacedBy xml:lang="en">School of BioSciences, The University of Melbourne</dcterms:isReplacedBy>
</rdf:Description>

<rdf:Description rdf:about="http://vocab.aodn.org.au/def/organisation/entity/311">
	<rdf:type rdf:resource="http://www.w3.org/2000/01/rdf-schema#Resource"/>
	<rdf:type rdf:resource="http://www.w3.org/2004/02/skos/core#Concept"/>
	<dcterms:creator rdf:datatype="http://www.w3.org/2001/XMLSchema#string">Natalia Atkins</dcterms:creator>
	<dcterms:created rdf:datatype="http://www.w3.org/2001/XMLSchema#dateTime">2015-07-22T10:38:15Z</dcterms:created>
	<skos:prefLabel xml:lang="en">Department of Zoology, The University of Melbourne</skos:prefLabel>
	<skos:altLabel xml:lang="en">Department of Zoology</skos:altLabel>
	<skos:hiddenLabel xml:lang="en"></skos:hiddenLabel>
	<skos:definition xml:lang="en">The school's research program ranges from the structure and function of single cells through to the ecology, reproduction, development and evolution of animals. The school became part of the School of Biosciences in 2015.</skos:definition>
	<dc:source rdf:datatype="http://www.w3.org/2001/XMLSchema#string">Australian Ocean Data Network Organisation Register</dc:source>
	<dc:publisher rdf:datatype="http://www.w3.org/2001/XMLSchema#string">eMarine Information Infrastructure (eMII)</dc:publisher>
	<skos:inScheme rdf:resource="http://vocab.aodn.org.au/def/organisation/1"/>
	<skos:broader rdf:resource="http://vocab.aodn.org.au/def/organisation/entity/309"/>
	<skos:scopeNote xml:lang="en">Organisation no longer exists</skos:scopeNote>
	<skos:scopeNote xml:lang="en">Organisation no longer exists. Replaced by http://vocab.aodn.org.au/def/organisation/entity/312</skos:scopeNote>
	<dcterms:isReplacedBy rdf:resource="http://vocab.aodn.org.au/def/organisation/entity/312"/>
	<dcterms:isReplacedBy xml:lang="en">School of BioSciences, The University of Melbourne</dcterms:isReplacedBy>
</rdf:Description>

<rdf:Description rdf:about="http://vocab.aodn.org.au/def/organisation/entity/312">
	<rdf:type rdf:resource="http://www.w3.org/2000/01/rdf-schema#Resource"/>
	<rdf:type rdf:resource="http://www.w3.org/2004/02/skos/core#Concept"/>
	<dcterms:creator rdf:datatype="http://www.w3.org/2001/XMLSchema#string">Natalia Atkins</dcterms:creator>
	<dcterms:created rdf:datatype="http://www.w3.org/2001/XMLSchema#dateTime">2015-07-22T10:38:15Z</dcterms:created>
	<skos:prefLabel xml:lang="en">School of BioSciences, The University of Melbourne</skos:prefLabel>
	<skos:altLabel xml:lang="en">School of BioSciences</skos:altLabel>
	<skos:hiddenLabel xml:lang="en"></skos:hiddenLabel>
	<skos:definition xml:lang="en">The School of BioSciences came into existence in 2015, consolidating expertise from three disciplines - botany, genetics and zoology.</skos:definition>
	<dc:source rdf:datatype="http://www.w3.org/2001/XMLSchema#string">Australian Ocean Data Network Organisation Register</dc:source>
	<dc:publisher rdf:datatype="http://www.w3.org/2001/XMLSchema#string">eMarine Information Infrastructure (eMII)</dc:publisher>
	<skos:exactMatch rdf:resource="http://seadatanet.maris2.nl/v_edmo/print.asp?n_code=4321"/>
	<skos:inScheme rdf:resource="http://vocab.aodn.org.au/def/organisation/1"/>
	<skos:broader rdf:resource="http://vocab.aodn.org.au/def/organisation/entity/309"/>
	<skos:scopeNote xml:lang="en">Replaces http://vocab.aodn.org.au/def/organisation/entity/310 and http://vocab.aodn.org.au/def/organisation/entity/311</skos:scopeNote>
	<dcterms:replaces rdf:resource="http://vocab.aodn.org.au/def/organisation/entity/310"/>
	<dcterms:replaces rdf:resource="http://vocab.aodn.org.au/def/organisation/entity/311"/>
	<dcterms:replaces xml:lang="en">School of Botany, The University of Melbourne</dcterms:replaces>
	<dcterms:replaces xml:lang="en">Department of Zoology, The University of Melbourne</dcterms:replaces>
</rdf:Description>

<rdf:Description rdf:about="http://vocab.aodn.org.au/def/organisation/entity/313">
	<rdf:type rdf:resource="http://www.w3.org/2000/01/rdf-schema#Resource"/>
	<rdf:type rdf:resource="http://www.w3.org/2004/02/skos/core#Concept"/>
	<dcterms:creator rdf:datatype="http://www.w3.org/2001/XMLSchema#string">Natalia Atkins</dcterms:creator>
	<dcterms:created rdf:datatype="http://www.w3.org/2001/XMLSchema#dateTime">2015-07-22T10:38:15Z</dcterms:created>
	<skos:prefLabel xml:lang="en">Department of Infrastructure Engineering, The University of Melbourne</skos:prefLabel>
	<skos:altLabel xml:lang="en">Department of Infrastructure Engineering</skos:altLabel>
	<skos:hiddenLabel xml:lang="en"></skos:hiddenLabel>
	<skos:definition xml:lang="en">The Department of Infrastructure Engineering sits within the School of Engineering and houses the vital disciplines of Geomatics, Civil Engineering and Environmental Engineering.</skos:definition>
	<dc:source rdf:datatype="http://www.w3.org/2001/XMLSchema#string">Australian Ocean Data Network Organisation Register</dc:source>
	<dc:publisher rdf:datatype="http://www.w3.org/2001/XMLSchema#string">eMarine Information Infrastructure (eMII)</dc:publisher>
	<skos:exactMatch rdf:resource="http://seadatanet.maris2.nl/v_edmo/print.asp?n_code=4322"/>
	<skos:inScheme rdf:resource="http://vocab.aodn.org.au/def/organisation/1"/>
	<skos:broader rdf:resource="http://vocab.aodn.org.au/def/organisation/entity/309"/>
	<skos:scopeNote xml:lang="en">Replaces http://vocab.aodn.org.au/def/organisation/entity/314</skos:scopeNote>
	<dcterms:replaces rdf:resource="http://vocab.aodn.org.au/def/organisation/entity/314"/>
	<dcterms:replaces xml:lang="en">Department of Civil and Environmental Engineering, The University of Melbourne</dcterms:replaces>
</rdf:Description>

<rdf:Description rdf:about="http://vocab.aodn.org.au/def/organisation/entity/314">
	<rdf:type rdf:resource="http://www.w3.org/2000/01/rdf-schema#Resource"/>
	<rdf:type rdf:resource="http://www.w3.org/2004/02/skos/core#Concept"/>
	<dcterms:creator rdf:datatype="http://www.w3.org/2001/XMLSchema#string">Natalia Atkins</dcterms:creator>
	<dcterms:created rdf:datatype="http://www.w3.org/2001/XMLSchema#dateTime">2015-07-22T10:38:15Z</dcterms:created>
	<skos:prefLabel xml:lang="en">Department of Civil and Environmental Engineering, The University of Melbourne</skos:prefLabel>
	<skos:altLabel xml:lang="en">Department of Civil and Environmental Engineering</skos:altLabel>
	<skos:hiddenLabel xml:lang="en"></skos:hiddenLabel>
	<skos:definition xml:lang="en">This former department became part of the Department of Infrastructure Engineering.</skos:definition>
	<dc:source rdf:datatype="http://www.w3.org/2001/XMLSchema#string">Australian Ocean Data Network Organisation Register</dc:source>
	<dc:publisher rdf:datatype="http://www.w3.org/2001/XMLSchema#string">eMarine Information Infrastructure (eMII)</dc:publisher>
	<skos:inScheme rdf:resource="http://vocab.aodn.org.au/def/organisation/1"/>
	<skos:broader rdf:resource="http://vocab.aodn.org.au/def/organisation/entity/309"/>
	<skos:scopeNote xml:lang="en">Organisation no longer exists</skos:scopeNote>
	<skos:scopeNote xml:lang="en">Organisation no longer exists. Replaced by http://vocab.aodn.org.au/def/organisation/entity/313</skos:scopeNote>
	<dcterms:isReplacedBy rdf:resource="http://vocab.aodn.org.au/def/organisation/entity/313"/>
	<dcterms:isReplacedBy xml:lang="en">Department of Infrastructure Engineering, The University of Melbourne</dcterms:isReplacedBy>
</rdf:Description>

<rdf:Description rdf:about="http://vocab.aodn.org.au/def/organisation/entity/315">
	<rdf:type rdf:resource="http://www.w3.org/2000/01/rdf-schema#Resource"/>
	<rdf:type rdf:resource="http://www.w3.org/2004/02/skos/core#Concept"/>
	<dcterms:creator rdf:datatype="http://www.w3.org/2001/XMLSchema#string">Natalia Atkins</dcterms:creator>
	<dcterms:created rdf:datatype="http://www.w3.org/2001/XMLSchema#dateTime">2015-07-22T10:38:15Z</dcterms:created>
	<skos:prefLabel xml:lang="en">School of Anthropology, Geography and Environmental Studies (SAGES), The University of Melbourne</skos:prefLabel>
	<skos:altLabel xml:lang="en">School of Anthropology, Geography and Environmental Studies (SAGES)</skos:altLabel>
	<skos:hiddenLabel xml:lang="en">SAGES</skos:hiddenLabel>
	<skos:definition xml:lang="en">This school was part of The Univeristy of Melbourne in the 1990s, and ceased to exist in the mid 2000s.</skos:definition>
	<dc:source rdf:datatype="http://www.w3.org/2001/XMLSchema#string">Australian Ocean Data Network Organisation Register</dc:source>
	<dc:publisher rdf:datatype="http://www.w3.org/2001/XMLSchema#string">eMarine Information Infrastructure (eMII)</dc:publisher>
	<skos:inScheme rdf:resource="http://vocab.aodn.org.au/def/organisation/1"/>
	<skos:broader rdf:resource="http://vocab.aodn.org.au/def/organisation/entity/309"/>
	<skos:scopeNote xml:lang="en">Organisation no longer exists</skos:scopeNote>
</rdf:Description>

<rdf:Description rdf:about="http://seadatanet.maris2.nl/v_edmo/print.asp?n_code=4320">
	<rdf:type rdf:resource="http://www.w3.org/2000/01/rdf-schema#Resource"/>
</rdf:Description>

<rdf:Description rdf:about="http://seadatanet.maris2.nl/v_edmo/print.asp?n_code=4321">
	<rdf:type rdf:resource="http://www.w3.org/2000/01/rdf-schema#Resource"/>
</rdf:Description>

<rdf:Description rdf:about="http://seadatanet.maris2.nl/v_edmo/print.asp?n_code=4322">
	<rdf:type rdf:resource="http://www.w3.org/2000/01/rdf-schema#Resource"/>
</rdf:Description>

<rdf:Description rdf:about="http://vocab.aodn.org.au/def/organisation/entity/280">
	<rdf:type rdf:resource="http://www.w3.org/2000/01/rdf-schema#Resource"/>
	<rdf:type rdf:resource="http://www.w3.org/2004/02/skos/core#Concept"/>
	<dcterms:creator rdf:datatype="http://www.w3.org/2001/XMLSchema#string">Natalia Atkins</dcterms:creator>
	<dcterms:created rdf:datatype="http://www.w3.org/2001/XMLSchema#dateTime">2015-07-16T10:38:15Z</dcterms:created>
	<skos:prefLabel xml:lang="en">School of Tropical Environment Studies and Geography, James Cook University (JCU)</skos:prefLabel>
	<skos:altLabel xml:lang="en">School of Tropical Environment Studies and Geography</skos:altLabel>
	<skos:hiddenLabel xml:lang="en"></skos:hiddenLabel>
	<skos:definition xml:lang="en">This former school became part of the College of Marine and Environmental Sciences (CMES)</skos:definition>
	<dc:source rdf:datatype="http://www.w3.org/2001/XMLSchema#string">Australian Ocean Data Network Organisation Register</dc:source>
	<dc:publisher rdf:datatype="http://www.w3.org/2001/XMLSchema#string">eMarine Information Infrastructure (eMII)</dc:publisher>
	<skos:inScheme rdf:resource="http://vocab.aodn.org.au/def/organisation/1"/>
	<skos:broader rdf:resource="http://vocab.aodn.org.au/def/organisation/entity/279"/>
	<skos:scopeNote xml:lang="en">Organisation no longer exists</skos:scopeNote>
	<skos:scopeNote xml:lang="en">Organisation no longer exists. http://vocab.aodn.org.au/def/organisation/entity/281</skos:scopeNote>
	<dcterms:isReplacedBy rdf:resource="http://vocab.aodn.org.au/def/organisation/entity/281"/>
	<dcterms:isReplacedBy xml:lang="en">College of Marine And Environmental Sciences (CMES), James Cook University (JCU)</dcterms:isReplacedBy>
</rdf:Description>

<rdf:Description rdf:about="http://vocab.aodn.org.au/def/organisation/entity/281">
	<rdf:type rdf:resource="http://www.w3.org/2000/01/rdf-schema#Resource"/>
	<rdf:type rdf:resource="http://www.w3.org/2004/02/skos/core#Concept"/>
	<dcterms:creator rdf:datatype="http://www.w3.org/2001/XMLSchema#string">Natalia Atkins</dcterms:creator>
	<dcterms:created rdf:datatype="http://www.w3.org/2001/XMLSchema#dateTime">2015-07-16T10:38:15Z</dcterms:created>
	<skos:prefLabel xml:lang="en">College of Marine And Environmental Sciences (CMES), James Cook University (JCU)</skos:prefLabel>
	<skos:altLabel xml:lang="en">College of Marine And Environmental Sciences (CMES)</skos:altLabel>
	<skos:hiddenLabel xml:lang="en">CMES</skos:hiddenLabel>
	<skos:definition xml:lang="en">The College of Marine and Environmental Sciences includes four broad groups that reflect core areas of expertise as follows: Aquaculture and Fisheries; Marine Biology; Terrestrial Ecosystems; and Environment Geography and Sustainability.</skos:definition>
	<dc:source rdf:datatype="http://www.w3.org/2001/XMLSchema#string">Australian Ocean Data Network Organisation Register</dc:source>
	<dc:publisher rdf:datatype="http://www.w3.org/2001/XMLSchema#string">eMarine Information Infrastructure (eMII)</dc:publisher>
	<skos:exactMatch rdf:resource="http://seadatanet.maris2.nl/v_edmo/print.asp?n_code=4271"/>
	<skos:inScheme rdf:resource="http://vocab.aodn.org.au/def/organisation/1"/>
	<skos:broader rdf:resource="http://vocab.aodn.org.au/def/organisation/entity/279"/>
	<skos:scopeNote xml:lang="en">Replaces http://vocab.aodn.org.au/organisation/entity/280</skos:scopeNote>
	<dcterms:replaces rdf:resource="http://vocab.aodn.org.au/def/organisation/entity/280"/>
	<dcterms:replaces xml:lang="en">School of Tropical Environment Studies and Geography, James Cook University (JCU)</dcterms:replaces>
</rdf:Description>

<rdf:Description rdf:about="http://vocab.aodn.org.au/def/organisation/entity/282">
	<rdf:type rdf:resource="http://www.w3.org/2000/01/rdf-schema#Resource"/>
	<rdf:type rdf:resource="http://www.w3.org/2004/02/skos/core#Concept"/>
	<dcterms:creator rdf:datatype="http://www.w3.org/2001/XMLSchema#string">Natalia Atkins</dcterms:creator>
	<dcterms:created rdf:datatype="http://www.w3.org/2001/XMLSchema#dateTime">2015-07-16T10:38:15Z</dcterms:created>
	<skos:prefLabel xml:lang="en">Centre for Tropical Waters and Aquatic Research (TropWATER), James Cook University (JCU)</skos:prefLabel>
	<skos:altLabel xml:lang="en">Centre for Tropical Waters and Aquatic Research (TropWATER)</skos:altLabel>
	<skos:hiddenLabel xml:lang="en">TropWATER</skos:hiddenLabel>
	<skos:definition xml:lang="en">The Centre for Tropical Water and Aquatic Ecosystem Research, undertakes research in fields related to water science, resource management and the ecology of water ecosystems.</skos:definition>
	<dc:source rdf:datatype="http://www.w3.org/2001/XMLSchema#string">Australian Ocean Data Network Organisation Register</dc:source>
	<dc:publisher rdf:datatype="http://www.w3.org/2001/XMLSchema#string">eMarine Information Infrastructure (eMII)</dc:publisher>
	<skos:exactMatch rdf:resource="http://seadatanet.maris2.nl/v_edmo/print.asp?n_code=4272"/>
	<skos:inScheme rdf:resource="http://vocab.aodn.org.au/def/organisation/1"/>
	<skos:broader rdf:resource="http://vocab.aodn.org.au/def/organisation/entity/279"/>
</rdf:Description>

<rdf:Description rdf:about="http://vocab.aodn.org.au/def/organisation/entity/283">
	<rdf:type rdf:resource="http://www.w3.org/2000/01/rdf-schema#Resource"/>
	<rdf:type rdf:resource="http://www.w3.org/2004/02/skos/core#Concept"/>
	<dcterms:creator rdf:datatype="http://www.w3.org/2001/XMLSchema#string">Natalia Atkins</dcterms:creator>
	<dcterms:created rdf:datatype="http://www.w3.org/2001/XMLSchema#dateTime">2015-07-16T10:38:15Z</dcterms:created>
	<skos:prefLabel xml:lang="en">School of Mathematics, Physics and Information Technology, James Cook University (JCU)</skos:prefLabel>
	<skos:altLabel xml:lang="en">School of Mathematics, Physics and Information Technology</skos:altLabel>
	<skos:hiddenLabel xml:lang="en"></skos:hiddenLabel>
	<skos:definition xml:lang="en">The school was formed in 2006, when the School of Information Technology was merged with the School of Maths and Physical Sciences. In 2009, the school was dissolved when the school of Information Technology was detached, and merged with the School of Business. The former School of Maths and Physical Sciences, has now became part of the College of Science, Technology and Engineering.</skos:definition>
	<dc:source rdf:datatype="http://www.w3.org/2001/XMLSchema#string">Australian Ocean Data Network Organisation Register</dc:source>
	<dc:publisher rdf:datatype="http://www.w3.org/2001/XMLSchema#string">eMarine Information Infrastructure (eMII)</dc:publisher>
	<skos:inScheme rdf:resource="http://vocab.aodn.org.au/def/organisation/1"/>
	<skos:broader rdf:resource="http://vocab.aodn.org.au/def/organisation/entity/279"/>
	<skos:scopeNote xml:lang="en">Organisation no longer exists</skos:scopeNote>
	<skos:scopeNote xml:lang="en">Organisation no longer exists. http://vocab.aodn.org.au/def/organisation/entity/284</skos:scopeNote>
	<dcterms:isReplacedBy rdf:resource="http://vocab.aodn.org.au/def/organisation/entity/284"/>
	<dcterms:isReplacedBy xml:lang="en">College of Science, Technology and Engineering (CSTE), James Cook University (JCU)</dcterms:isReplacedBy>
</rdf:Description>

<rdf:Description rdf:about="http://vocab.aodn.org.au/def/organisation/entity/284">
	<rdf:type rdf:resource="http://www.w3.org/2000/01/rdf-schema#Resource"/>
	<rdf:type rdf:resource="http://www.w3.org/2004/02/skos/core#Concept"/>
	<dcterms:creator rdf:datatype="http://www.w3.org/2001/XMLSchema#string">Natalia Atkins</dcterms:creator>
	<dcterms:created rdf:datatype="http://www.w3.org/2001/XMLSchema#dateTime">2015-07-16T10:38:15Z</dcterms:created>
	<skos:prefLabel xml:lang="en">College of Science, Technology and Engineering (CSTE), James Cook University (JCU)</skos:prefLabel>
	<skos:altLabel xml:lang="en">College of Science, Technology and Engineering (CSTE)</skos:altLabel>
	<skos:hiddenLabel xml:lang="en">CSTE</skos:hiddenLabel>
	<skos:definition xml:lang="en">The college covers the fields of physical sciences, earth sciences and engineering. It is structured into four multidisciplinary groupings: Infrastructure and Design; Earth and Oceans; Matters and Materials; and Intelligent Systems, Information and Modelling.</skos:definition>
	<dc:source rdf:datatype="http://www.w3.org/2001/XMLSchema#string">Australian Ocean Data Network Organisation Register</dc:source>
	<dc:publisher rdf:datatype="http://www.w3.org/2001/XMLSchema#string">eMarine Information Infrastructure (eMII)</dc:publisher>
	<skos:exactMatch rdf:resource="http://seadatanet.maris2.nl/v_edmo/print.asp?n_code=4273"/>
	<skos:inScheme rdf:resource="http://vocab.aodn.org.au/def/organisation/1"/>
	<skos:broader rdf:resource="http://vocab.aodn.org.au/def/organisation/entity/279"/>
	<skos:scopeNote xml:lang="en">Replaces http://vocab.aodn.org.au/organisation/entity/283</skos:scopeNote>
	<dcterms:replaces rdf:resource="http://vocab.aodn.org.au/def/organisation/entity/283"/>
	<dcterms:replaces xml:lang="en">School of Mathematics, Physics and Information Technology, James Cook University (JCU)</dcterms:replaces>
</rdf:Description>

<rdf:Description rdf:about="http://vocab.aodn.org.au/def/organisation/entity/285">
	<rdf:type rdf:resource="http://www.w3.org/2000/01/rdf-schema#Resource"/>
	<rdf:type rdf:resource="http://www.w3.org/2004/02/skos/core#Concept"/>
	<dcterms:creator rdf:datatype="http://www.w3.org/2001/XMLSchema#string">Natalia Atkins</dcterms:creator>
	<dcterms:created rdf:datatype="http://www.w3.org/2001/XMLSchema#dateTime">2015-07-16T10:38:15Z</dcterms:created>
	<skos:prefLabel xml:lang="en">College of Business, Law and Governance, James Cook University (JCU)</skos:prefLabel>
	<skos:altLabel xml:lang="en">College of Business, Law and Governance</skos:altLabel>
	<skos:hiddenLabel xml:lang="en"></skos:hiddenLabel>
	<skos:definition xml:lang="en">The College of Business, Law and Governance was formed in 2014 to provide new opportunities and collaborations for both education and research. There is a focus on ethics, sustainability and governance, as well as an understanding of complex business systems. The college delivers a range of courses in Cairns, Singapore, Townsville and Brisbane.</skos:definition>
	<dc:source rdf:datatype="http://www.w3.org/2001/XMLSchema#string">Australian Ocean Data Network Organisation Register</dc:source>
	<dc:publisher rdf:datatype="http://www.w3.org/2001/XMLSchema#string">eMarine Information Infrastructure (eMII)</dc:publisher>
	<skos:exactMatch rdf:resource="http://seadatanet.maris2.nl/v_edmo/print.asp?n_code=4274"/>
	<skos:inScheme rdf:resource="http://vocab.aodn.org.au/def/organisation/1"/>
	<skos:broader rdf:resource="http://vocab.aodn.org.au/def/organisation/entity/279"/>
</rdf:Description>

<rdf:Description rdf:about="http://vocab.aodn.org.au/def/organisation/entity/286">
	<rdf:type rdf:resource="http://www.w3.org/2000/01/rdf-schema#Resource"/>
	<rdf:type rdf:resource="http://www.w3.org/2004/02/skos/core#Concept"/>
	<dcterms:creator rdf:datatype="http://www.w3.org/2001/XMLSchema#string">Natalia Atkins</dcterms:creator>
	<dcterms:created rdf:datatype="http://www.w3.org/2001/XMLSchema#dateTime">2015-07-16T10:38:15Z</dcterms:created>
	<skos:broadMatch rdf:resource="http://vocab.aodn.org.au/def/organisation_classes/category/6"/>
	<skos:prefLabel xml:lang="en">Seagrass-Watch</skos:prefLabel>
	<skos:altLabel xml:lang="en"></skos:altLabel>
	<skos:hiddenLabel xml:lang="en"></skos:hiddenLabel>
	<skos:definition xml:lang="en">Seagrass-Watch is a global scientific, non-destructive, seagrass assessment and monitoring program. Since it's genesis in 1998 in Australia, Seagrass-Watch has expanded internationally with participants in Micronesia, Papua New Guinea, Solomon Islands, Fiji, New Caledonia, Palau, Japan, China, Viet Nam, Philippines, Thailand, Malaysia, Indonesia, Myanmar, Bangladesh, India, Eritrea, Kuwait, France, Spain, Comoros Islands, Maldives, Carribbean, United States of America and Singapore. Monitoring is now occurring at approximately 259 sites across 17 countries and an additional 9 countries participate but are currently at resource identification stage.</skos:definition>
	<dc:source rdf:datatype="http://www.w3.org/2001/XMLSchema#string">Australian Ocean Data Network Organisation Register</dc:source>
	<dc:publisher rdf:datatype="http://www.w3.org/2001/XMLSchema#string">eMarine Information Infrastructure (eMII)</dc:publisher>
	<skos:exactMatch rdf:resource="http://seadatanet.maris2.nl/v_edmo/print.asp?n_code=4275"/>
	<skos:inScheme rdf:resource="http://vocab.aodn.org.au/def/organisation/1"/>
	<skos:broader rdf:resource="http://vocab.aodn.org.au/def/organisation/entity/279"/>
</rdf:Description>

<rdf:Description rdf:about="http://seadatanet.maris2.nl/v_edmo/print.asp?n_code=4270">
	<rdf:type rdf:resource="http://www.w3.org/2000/01/rdf-schema#Resource"/>
</rdf:Description>

<rdf:Description rdf:about="http://seadatanet.maris2.nl/v_edmo/print.asp?n_code=4271">
	<rdf:type rdf:resource="http://www.w3.org/2000/01/rdf-schema#Resource"/>
</rdf:Description>

<rdf:Description rdf:about="http://seadatanet.maris2.nl/v_edmo/print.asp?n_code=4272">
	<rdf:type rdf:resource="http://www.w3.org/2000/01/rdf-schema#Resource"/>
</rdf:Description>

<rdf:Description rdf:about="http://seadatanet.maris2.nl/v_edmo/print.asp?n_code=4273">
	<rdf:type rdf:resource="http://www.w3.org/2000/01/rdf-schema#Resource"/>
</rdf:Description>

<rdf:Description rdf:about="http://seadatanet.maris2.nl/v_edmo/print.asp?n_code=4274">
	<rdf:type rdf:resource="http://www.w3.org/2000/01/rdf-schema#Resource"/>
</rdf:Description>

<rdf:Description rdf:about="http://seadatanet.maris2.nl/v_edmo/print.asp?n_code=4275">
	<rdf:type rdf:resource="http://www.w3.org/2000/01/rdf-schema#Resource"/>
</rdf:Description>

<rdf:Description rdf:about="http://vocab.aodn.org.au/def/organisation/entity/290">
	<rdf:type rdf:resource="http://www.w3.org/2000/01/rdf-schema#Resource"/>
	<rdf:type rdf:resource="http://www.w3.org/2004/02/skos/core#Concept"/>
	<dcterms:creator rdf:datatype="http://www.w3.org/2001/XMLSchema#string">Natalia Atkins</dcterms:creator>
	<dcterms:created rdf:datatype="http://www.w3.org/2001/XMLSchema#dateTime">2015-07-17T10:38:15Z</dcterms:created>
	<skos:prefLabel xml:lang="en">Department of Ecology and Evolutionary Biology, Monash University</skos:prefLabel>
	<skos:altLabel xml:lang="en">Department of Ecology and Evolutionary Biology</skos:altLabel>
	<skos:hiddenLabel xml:lang="en"></skos:hiddenLabel>
	<skos:definition xml:lang="en">This former department became part of the School of Biological Sciences.</skos:definition>
	<dc:source rdf:datatype="http://www.w3.org/2001/XMLSchema#string">Australian Ocean Data Network Organisation Register</dc:source>
	<dc:publisher rdf:datatype="http://www.w3.org/2001/XMLSchema#string">eMarine Information Infrastructure (eMII)</dc:publisher>
	<skos:inScheme rdf:resource="http://vocab.aodn.org.au/def/organisation/1"/>
	<skos:broader rdf:resource="http://vocab.aodn.org.au/def/organisation/entity/289"/>
	<skos:scopeNote xml:lang="en">Organisation no longer exists</skos:scopeNote>
	<skos:scopeNote xml:lang="en">Organisation no longer exists. http://vocab.aodn.org.au/def/organisation/entity/291</skos:scopeNote>
	<dcterms:isReplacedBy rdf:resource="http://vocab.aodn.org.au/def/organisation/entity/291"/>
	<dcterms:isReplacedBy xml:lang="en">School of Biological Sciences, Monash University</dcterms:isReplacedBy>
</rdf:Description>

<rdf:Description rdf:about="http://vocab.aodn.org.au/def/organisation/entity/291">
	<rdf:type rdf:resource="http://www.w3.org/2000/01/rdf-schema#Resource"/>
	<rdf:type rdf:resource="http://www.w3.org/2004/02/skos/core#Concept"/>
	<dcterms:creator rdf:datatype="http://www.w3.org/2001/XMLSchema#string">Natalia Atkins</dcterms:creator>
	<dcterms:created rdf:datatype="http://www.w3.org/2001/XMLSchema#dateTime">2015-07-17T10:38:15Z</dcterms:created>
	<skos:prefLabel xml:lang="en">School of Biological Sciences, Monash University</skos:prefLabel>
	<skos:altLabel xml:lang="en">School of Biological Sciences</skos:altLabel>
	<skos:hiddenLabel xml:lang="en"></skos:hiddenLabel>
	<skos:definition xml:lang="en">The School of Biological Sciences is based at the Clayton campus. It has research strengths in four discipline areas: Evolution, Genetics, Ecology and Conservation Biology.</skos:definition>
	<dc:source rdf:datatype="http://www.w3.org/2001/XMLSchema#string">Australian Ocean Data Network Organisation Register</dc:source>
	<dc:publisher rdf:datatype="http://www.w3.org/2001/XMLSchema#string">eMarine Information Infrastructure (eMII)</dc:publisher>
	<skos:exactMatch rdf:resource="http://seadatanet.maris2.nl/v_edmo/print.asp?n_code=4279"/>
	<skos:inScheme rdf:resource="http://vocab.aodn.org.au/def/organisation/1"/>
	<skos:broader rdf:resource="http://vocab.aodn.org.au/def/organisation/entity/289"/>
	<skos:scopeNote xml:lang="en">Replaces http://vocab.aodn.org.au/def/organisation/entity/290</skos:scopeNote>
	<dcterms:replaces rdf:resource="http://vocab.aodn.org.au/def/organisation/entity/290"/>
	<dcterms:replaces xml:lang="en">Department of Ecology and Evolutionary Biology, Monash University</dcterms:replaces>
</rdf:Description>

<rdf:Description rdf:about="http://vocab.aodn.org.au/def/organisation/entity/292">
	<rdf:type rdf:resource="http://www.w3.org/2000/01/rdf-schema#Resource"/>
	<rdf:type rdf:resource="http://www.w3.org/2004/02/skos/core#Concept"/>
	<dcterms:creator rdf:datatype="http://www.w3.org/2001/XMLSchema#string">Natalia Atkins</dcterms:creator>
	<dcterms:created rdf:datatype="http://www.w3.org/2001/XMLSchema#dateTime">2015-07-17T10:38:15Z</dcterms:created>
	<skos:prefLabel xml:lang="en">Department of Civil Engineering, Monash University</skos:prefLabel>
	<skos:altLabel xml:lang="en">Department of Civil Engineering</skos:altLabel>
	<skos:hiddenLabel xml:lang="en"></skos:hiddenLabel>
	<skos:definition xml:lang="en">The Department of Civil Engineering is based at the Clayton campus, and was formed in 1961. It provides education and research outputs in the areas of: geomechanics, structures, transport, water and mining.</skos:definition>
	<dc:source rdf:datatype="http://www.w3.org/2001/XMLSchema#string">Australian Ocean Data Network Organisation Register</dc:source>
	<dc:publisher rdf:datatype="http://www.w3.org/2001/XMLSchema#string">eMarine Information Infrastructure (eMII)</dc:publisher>
	<skos:exactMatch rdf:resource="http://seadatanet.maris2.nl/v_edmo/print.asp?n_code=4280"/>
	<skos:inScheme rdf:resource="http://vocab.aodn.org.au/def/organisation/1"/>
	<skos:broader rdf:resource="http://vocab.aodn.org.au/def/organisation/entity/289"/>
</rdf:Description>

<rdf:Description rdf:about="http://vocab.aodn.org.au/def/organisation/entity/293">
	<rdf:type rdf:resource="http://www.w3.org/2000/01/rdf-schema#Resource"/>
	<rdf:type rdf:resource="http://www.w3.org/2004/02/skos/core#Concept"/>
	<dcterms:creator rdf:datatype="http://www.w3.org/2001/XMLSchema#string">Natalia Atkins</dcterms:creator>
	<dcterms:created rdf:datatype="http://www.w3.org/2001/XMLSchema#dateTime">2015-07-17T10:38:15Z</dcterms:created>
	<skos:prefLabel xml:lang="en">Water Studies Centre (WSC), School of Chemistry, Monash University</skos:prefLabel>
	<skos:altLabel xml:lang="en">Water Studies Centre (WSC)</skos:altLabel>
	<skos:hiddenLabel xml:lang="en">WSC</skos:hiddenLabel>
	<skos:definition xml:lang="en">The Water Studies Centre (WSC) was established at the Chisholm Institute of Technology in 1975 as the research and consultancy arm of the former Department of Chemistry and Biology. In 1990 Chisholm Institute merged with Monash University and the WSC became a research centre of the Faculty of Science with close links to the School of Chemistry. In late 1998, the Centre was relocated to new purpose-built premises on the Clayton campus.</skos:definition>
	<dc:source rdf:datatype="http://www.w3.org/2001/XMLSchema#string">Australian Ocean Data Network Organisation Register</dc:source>
	<dc:publisher rdf:datatype="http://www.w3.org/2001/XMLSchema#string">eMarine Information Infrastructure (eMII)</dc:publisher>
	<skos:exactMatch rdf:resource="http://seadatanet.maris2.nl/v_edmo/print.asp?n_code=4281"/>
	<skos:inScheme rdf:resource="http://vocab.aodn.org.au/def/organisation/1"/>
	<skos:broader rdf:resource="http://vocab.aodn.org.au/def/organisation/entity/289"/>
</rdf:Description>

<rdf:Description rdf:about="http://seadatanet.maris2.nl/v_edmo/print.asp?n_code=4278">
	<rdf:type rdf:resource="http://www.w3.org/2000/01/rdf-schema#Resource"/>
</rdf:Description>

<rdf:Description rdf:about="http://seadatanet.maris2.nl/v_edmo/print.asp?n_code=4279">
	<rdf:type rdf:resource="http://www.w3.org/2000/01/rdf-schema#Resource"/>
</rdf:Description>

<rdf:Description rdf:about="http://seadatanet.maris2.nl/v_edmo/print.asp?n_code=4280">
	<rdf:type rdf:resource="http://www.w3.org/2000/01/rdf-schema#Resource"/>
</rdf:Description>

<rdf:Description rdf:about="http://seadatanet.maris2.nl/v_edmo/print.asp?n_code=4281">
	<rdf:type rdf:resource="http://www.w3.org/2000/01/rdf-schema#Resource"/>
</rdf:Description>

<rdf:Description rdf:about="http://vocab.aodn.org.au/def/organisation/entity/295">
	<rdf:type rdf:resource="http://www.w3.org/2000/01/rdf-schema#Resource"/>
	<rdf:type rdf:resource="http://www.w3.org/2004/02/skos/core#Concept"/>
	<dcterms:creator rdf:datatype="http://www.w3.org/2001/XMLSchema#string">Natalia Atkins</dcterms:creator>
	<dcterms:created rdf:datatype="http://www.w3.org/2001/XMLSchema#dateTime">2015-07-17T10:38:15Z</dcterms:created>
	<skos:prefLabel xml:lang="en">School of Biological and Environmental Sciences, Murdoch University</skos:prefLabel>
	<skos:altLabel xml:lang="en">School of Biological and Environmental Sciences</skos:altLabel>
	<skos:hiddenLabel xml:lang="en"></skos:hiddenLabel>
	<skos:definition xml:lang="en">This former school was renamed the School of Biological Sciences.</skos:definition>
	<dc:source rdf:datatype="http://www.w3.org/2001/XMLSchema#string">Australian Ocean Data Network Organisation Register</dc:source>
	<dc:publisher rdf:datatype="http://www.w3.org/2001/XMLSchema#string">eMarine Information Infrastructure (eMII)</dc:publisher>
	<skos:inScheme rdf:resource="http://vocab.aodn.org.au/def/organisation/1"/>
	<skos:broader rdf:resource="http://vocab.aodn.org.au/def/organisation/entity/294"/>
	<skos:scopeNote xml:lang="en">Organisation no longer exists</skos:scopeNote>
	<skos:scopeNote xml:lang="en">Organisation no longer exists. Replaced by http://vocab.aodn.org.au/def/organisation/entity/296</skos:scopeNote>
	<dcterms:isReplacedBy rdf:resource="http://vocab.aodn.org.au/def/organisation/entity/296"/>
	<dcterms:isReplacedBy xml:lang="en">School of Biological Sciences, Murdoch University</dcterms:isReplacedBy>
</rdf:Description>

<rdf:Description rdf:about="http://vocab.aodn.org.au/def/organisation/entity/296">
	<rdf:type rdf:resource="http://www.w3.org/2000/01/rdf-schema#Resource"/>
	<rdf:type rdf:resource="http://www.w3.org/2004/02/skos/core#Concept"/>
	<dcterms:creator rdf:datatype="http://www.w3.org/2001/XMLSchema#string">Natalia Atkins</dcterms:creator>
	<dcterms:created rdf:datatype="http://www.w3.org/2001/XMLSchema#dateTime">2015-07-17T10:38:15Z</dcterms:created>
	<skos:prefLabel xml:lang="en">School of Biological Sciences, Murdoch University</skos:prefLabel>
	<skos:altLabel xml:lang="en">School of Biological Sciences</skos:altLabel>
	<skos:hiddenLabel xml:lang="en"></skos:hiddenLabel>
	<skos:definition xml:lang="en">This former school was renamed the School of Biological Sciences and Biotechnology.</skos:definition>
	<dc:source rdf:datatype="http://www.w3.org/2001/XMLSchema#string">Australian Ocean Data Network Organisation Register</dc:source>
	<dc:publisher rdf:datatype="http://www.w3.org/2001/XMLSchema#string">eMarine Information Infrastructure (eMII)</dc:publisher>
	<skos:inScheme rdf:resource="http://vocab.aodn.org.au/def/organisation/1"/>
	<skos:broader rdf:resource="http://vocab.aodn.org.au/def/organisation/entity/294"/>
	<skos:scopeNote xml:lang="en">Organisation no longer exists</skos:scopeNote>
	<skos:scopeNote xml:lang="en">Organisation no longer exists. Replaced by http://vocab.aodn.org.au/def/organisation/entity/298. Replaces http://vocab.aodn.org.au/def/organisation/entity/295</skos:scopeNote>
	<dcterms:replaces rdf:resource="http://vocab.aodn.org.au/def/organisation/entity/295"/>
	<dcterms:replaces xml:lang="en">School of Biological and Environmental Sciences, Murdoch University</dcterms:replaces>
	<dcterms:isReplacedBy rdf:resource="http://vocab.aodn.org.au/def/organisation/entity/298"/>
	<dcterms:isReplacedBy xml:lang="en">School of Biological Sciences and Biotechnology (BSB), Murdoch University</dcterms:isReplacedBy>
</rdf:Description>

<rdf:Description rdf:about="http://vocab.aodn.org.au/def/organisation/entity/297">
	<rdf:type rdf:resource="http://www.w3.org/2000/01/rdf-schema#Resource"/>
	<rdf:type rdf:resource="http://www.w3.org/2004/02/skos/core#Concept"/>
	<dcterms:creator rdf:datatype="http://www.w3.org/2001/XMLSchema#string">Natalia Atkins</dcterms:creator>
	<dcterms:created rdf:datatype="http://www.w3.org/2001/XMLSchema#dateTime">2015-07-17T10:38:15Z</dcterms:created>
	<skos:prefLabel xml:lang="en">School of Environmental Science, Murdoch University</skos:prefLabel>
	<skos:altLabel xml:lang="en">School of Environmental Science</skos:altLabel>
	<skos:hiddenLabel xml:lang="en"></skos:hiddenLabel>
	<skos:definition xml:lang="en">The school was dissolved in 2013, when it became part of the School of Veterinary and Life Sciences.</skos:definition>
	<dc:source rdf:datatype="http://www.w3.org/2001/XMLSchema#string">Australian Ocean Data Network Organisation Register</dc:source>
	<dc:publisher rdf:datatype="http://www.w3.org/2001/XMLSchema#string">eMarine Information Infrastructure (eMII)</dc:publisher>
	<skos:inScheme rdf:resource="http://vocab.aodn.org.au/def/organisation/1"/>
	<skos:broader rdf:resource="http://vocab.aodn.org.au/def/organisation/entity/294"/>
	<skos:scopeNote xml:lang="en">Organisation no longer exists</skos:scopeNote>
	<skos:scopeNote xml:lang="en">Organisation no longer exists. Replaced by http://vocab.aodn.org.au/def/organisation/entity/299</skos:scopeNote>
	<dcterms:isReplacedBy rdf:resource="http://vocab.aodn.org.au/def/organisation/entity/299"/>
	<dcterms:isReplacedBy xml:lang="en">School of Veterinary and Life Sciences (VLS), Murdoch University</dcterms:isReplacedBy>
</rdf:Description>

<rdf:Description rdf:about="http://vocab.aodn.org.au/def/organisation/entity/298">
	<rdf:type rdf:resource="http://www.w3.org/2000/01/rdf-schema#Resource"/>
	<rdf:type rdf:resource="http://www.w3.org/2004/02/skos/core#Concept"/>
	<dcterms:creator rdf:datatype="http://www.w3.org/2001/XMLSchema#string">Natalia Atkins</dcterms:creator>
	<dcterms:created rdf:datatype="http://www.w3.org/2001/XMLSchema#dateTime">2015-07-17T10:38:15Z</dcterms:created>
	<skos:prefLabel xml:lang="en">School of Biological Sciences and Biotechnology (BSB), Murdoch University</skos:prefLabel>
	<skos:altLabel xml:lang="en">School of Biological Sciences and Biotechnology (BSB)</skos:altLabel>
	<skos:hiddenLabel xml:lang="en">BSB</skos:hiddenLabel>
	<skos:definition xml:lang="en">The school was dissolved in 2013, when it became part of the School of Veterinary and Life Sciences.</skos:definition>
	<dc:source rdf:datatype="http://www.w3.org/2001/XMLSchema#string">Australian Ocean Data Network Organisation Register</dc:source>
	<dc:publisher rdf:datatype="http://www.w3.org/2001/XMLSchema#string">eMarine Information Infrastructure (eMII)</dc:publisher>
	<skos:inScheme rdf:resource="http://vocab.aodn.org.au/def/organisation/1"/>
	<skos:broader rdf:resource="http://vocab.aodn.org.au/def/organisation/entity/294"/>
	<skos:scopeNote xml:lang="en">Organisation no longer exists</skos:scopeNote>
	<skos:scopeNote xml:lang="en">Organisation no longer exists. Replaced by http://vocab.aodn.org.au/def/organisation/entity/299. Replaces http://vocab.aodn.org.au/def/organisation/entity/296</skos:scopeNote>
	<dcterms:replaces rdf:resource="http://vocab.aodn.org.au/def/organisation/entity/296"/>
	<dcterms:replaces xml:lang="en">School of Biological Sciences, Murdoch University</dcterms:replaces>
	<dcterms:isReplacedBy rdf:resource="http://vocab.aodn.org.au/def/organisation/entity/299"/>
	<dcterms:isReplacedBy xml:lang="en">School of Veterinary and Life Sciences (VLS), Murdoch University</dcterms:isReplacedBy>
</rdf:Description>

<rdf:Description rdf:about="http://vocab.aodn.org.au/def/organisation/entity/299">
	<rdf:type rdf:resource="http://www.w3.org/2000/01/rdf-schema#Resource"/>
	<rdf:type rdf:resource="http://www.w3.org/2004/02/skos/core#Concept"/>
	<dcterms:creator rdf:datatype="http://www.w3.org/2001/XMLSchema#string">Natalia Atkins</dcterms:creator>
	<dcterms:created rdf:datatype="http://www.w3.org/2001/XMLSchema#dateTime">2015-07-17T10:38:15Z</dcterms:created>
	<skos:prefLabel xml:lang="en">School of Veterinary and Life Sciences (VLS), Murdoch University</skos:prefLabel>
	<skos:altLabel xml:lang="en">School of Veterinary and Life Sciences (VLS)</skos:altLabel>
	<skos:hiddenLabel xml:lang="en">VLS</skos:hiddenLabel>
	<skos:definition xml:lang="en">The School of Veterinary and Life Sciences (“VLS”) was formed in January 2013 from an amalgamation of the Schools of Veterinary and Biomedical Science, Biological Sciences and Biotechnology and Environmental Science.</skos:definition>
	<dc:source rdf:datatype="http://www.w3.org/2001/XMLSchema#string">Australian Ocean Data Network Organisation Register</dc:source>
	<dc:publisher rdf:datatype="http://www.w3.org/2001/XMLSchema#string">eMarine Information Infrastructure (eMII)</dc:publisher>
	<skos:exactMatch rdf:resource="http://seadatanet.maris2.nl/v_edmo/print.asp?n_code=4283"/>
	<skos:inScheme rdf:resource="http://vocab.aodn.org.au/def/organisation/1"/>
	<skos:broader rdf:resource="http://vocab.aodn.org.au/def/organisation/entity/294"/>
	<skos:scopeNote xml:lang="en">Replaces http://vocab.aodn.org.au/def/organisation/entity/297 and http://vocab.aodn.org.au/def/organisation/entity/298</skos:scopeNote>
	<dcterms:replaces rdf:resource="http://vocab.aodn.org.au/def/organisation/entity/297"/>
	<dcterms:replaces rdf:resource="http://vocab.aodn.org.au/def/organisation/entity/298"/>
	<dcterms:replaces xml:lang="en">School of Environmental Science, Murdoch University</dcterms:replaces>
	<dcterms:replaces xml:lang="en">School of Biological Sciences and Biotechnology (BSB), Murdoch University</dcterms:replaces>
</rdf:Description>

<rdf:Description rdf:about="http://vocab.aodn.org.au/def/organisation/entity/300">
	<rdf:type rdf:resource="http://www.w3.org/2000/01/rdf-schema#Resource"/>
	<rdf:type rdf:resource="http://www.w3.org/2004/02/skos/core#Concept"/>
	<dcterms:creator rdf:datatype="http://www.w3.org/2001/XMLSchema#string">Natalia Atkins</dcterms:creator>
	<dcterms:created rdf:datatype="http://www.w3.org/2001/XMLSchema#dateTime">2015-07-17T10:38:15Z</dcterms:created>
	<skos:prefLabel xml:lang="en">Centre for Fish and Fisheries Research (CFFR), School of Veterinary and Life Sciences (VLS), Murdoch University</skos:prefLabel>
	<skos:altLabel xml:lang="en">Centre for Fish and Fisheries Research (CFFR)</skos:altLabel>
	<skos:hiddenLabel xml:lang="en">CFFR</skos:hiddenLabel>
	<skos:definition xml:lang="en">The Centre was established in 2000 in recognition of a history of sustained and internationally recognised excellence in research and postgraduate training in fish and fisheries biology. Its studies have focused on the faunas and ecosystems of Western Australia.</skos:definition>
	<dc:source rdf:datatype="http://www.w3.org/2001/XMLSchema#string">Australian Ocean Data Network Organisation Register</dc:source>
	<dc:publisher rdf:datatype="http://www.w3.org/2001/XMLSchema#string">eMarine Information Infrastructure (eMII)</dc:publisher>
	<skos:exactMatch rdf:resource="http://seadatanet.maris2.nl/v_edmo/print.asp?n_code=4284"/>
	<skos:inScheme rdf:resource="http://vocab.aodn.org.au/def/organisation/1"/>
	<skos:broader rdf:resource="http://vocab.aodn.org.au/def/organisation/entity/294"/>
</rdf:Description>

<rdf:Description rdf:about="http://vocab.aodn.org.au/def/organisation/entity/301">
	<rdf:type rdf:resource="http://www.w3.org/2000/01/rdf-schema#Resource"/>
	<rdf:type rdf:resource="http://www.w3.org/2004/02/skos/core#Concept"/>
	<dcterms:creator rdf:datatype="http://www.w3.org/2001/XMLSchema#string">Natalia Atkins</dcterms:creator>
	<dcterms:created rdf:datatype="http://www.w3.org/2001/XMLSchema#dateTime">2015-07-17T10:38:15Z</dcterms:created>
	<skos:prefLabel xml:lang="en">School of Management and Governance, Murdoch University</skos:prefLabel>
	<skos:altLabel xml:lang="en">School of Management and Governance</skos:altLabel>
	<skos:hiddenLabel xml:lang="en"></skos:hiddenLabel>
	<skos:definition xml:lang="en">The school has a strong research and a multi-disciplinary focus in management, marketing, economics, finance, accounting, sustainability and politics.</skos:definition>
	<dc:source rdf:datatype="http://www.w3.org/2001/XMLSchema#string">Australian Ocean Data Network Organisation Register</dc:source>
	<dc:publisher rdf:datatype="http://www.w3.org/2001/XMLSchema#string">eMarine Information Infrastructure (eMII)</dc:publisher>
	<skos:exactMatch rdf:resource="http://seadatanet.maris2.nl/v_edmo/print.asp?n_code=4285"/>
	<skos:inScheme rdf:resource="http://vocab.aodn.org.au/def/organisation/1"/>
	<skos:broader rdf:resource="http://vocab.aodn.org.au/def/organisation/entity/294"/>
</rdf:Description>

<rdf:Description rdf:about="http://vocab.aodn.org.au/def/organisation/entity/302">
	<rdf:type rdf:resource="http://www.w3.org/2000/01/rdf-schema#Resource"/>
	<rdf:type rdf:resource="http://www.w3.org/2004/02/skos/core#Concept"/>
	<dcterms:creator rdf:datatype="http://www.w3.org/2001/XMLSchema#string">Natalia Atkins</dcterms:creator>
	<dcterms:created rdf:datatype="http://www.w3.org/2001/XMLSchema#dateTime">2015-07-17T10:38:15Z</dcterms:created>
	<skos:prefLabel xml:lang="en">School of Engineering and Information Technology, Murdoch University</skos:prefLabel>
	<skos:altLabel xml:lang="en">School of Engineering and Information Technology</skos:altLabel>
	<skos:hiddenLabel xml:lang="en"></skos:hiddenLabel>
	<skos:definition xml:lang="en">The school covers the disciplines of: Engineering, Mathematics and Statistics, Physics, Information Technology, Energy Studies, Extractive Metallurgy and Chemistry.</skos:definition>
	<dc:source rdf:datatype="http://www.w3.org/2001/XMLSchema#string">Australian Ocean Data Network Organisation Register</dc:source>
	<dc:publisher rdf:datatype="http://www.w3.org/2001/XMLSchema#string">eMarine Information Infrastructure (eMII)</dc:publisher>
	<skos:exactMatch rdf:resource="http://seadatanet.maris2.nl/v_edmo/print.asp?n_code=4286"/>
	<skos:inScheme rdf:resource="http://vocab.aodn.org.au/def/organisation/1"/>
	<skos:broader rdf:resource="http://vocab.aodn.org.au/def/organisation/entity/294"/>
</rdf:Description>

<rdf:Description rdf:about="http://seadatanet.maris2.nl/v_edmo/print.asp?n_code=4282">
	<rdf:type rdf:resource="http://www.w3.org/2000/01/rdf-schema#Resource"/>
</rdf:Description>

<rdf:Description rdf:about="http://seadatanet.maris2.nl/v_edmo/print.asp?n_code=4283">
	<rdf:type rdf:resource="http://www.w3.org/2000/01/rdf-schema#Resource"/>
</rdf:Description>

<rdf:Description rdf:about="http://seadatanet.maris2.nl/v_edmo/print.asp?n_code=4284">
	<rdf:type rdf:resource="http://www.w3.org/2000/01/rdf-schema#Resource"/>
</rdf:Description>

<rdf:Description rdf:about="http://seadatanet.maris2.nl/v_edmo/print.asp?n_code=4285">
	<rdf:type rdf:resource="http://www.w3.org/2000/01/rdf-schema#Resource"/>
</rdf:Description>

<rdf:Description rdf:about="http://seadatanet.maris2.nl/v_edmo/print.asp?n_code=4286">
	<rdf:type rdf:resource="http://www.w3.org/2000/01/rdf-schema#Resource"/>
</rdf:Description>

<rdf:Description rdf:about="http://vocab.aodn.org.au/def/organisation/entity/317">
	<rdf:type rdf:resource="http://www.w3.org/2000/01/rdf-schema#Resource"/>
	<rdf:type rdf:resource="http://www.w3.org/2004/02/skos/core#Concept"/>
	<dcterms:creator rdf:datatype="http://www.w3.org/2001/XMLSchema#string">Natalia Atkins</dcterms:creator>
	<dcterms:created rdf:datatype="http://www.w3.org/2001/XMLSchema#dateTime">2015-07-22T10:38:15Z</dcterms:created>
	<skos:prefLabel xml:lang="en">School of Health and Sport Sciences, University of the Sunshine Coast (USC)</skos:prefLabel>
	<skos:altLabel xml:lang="en">School of Health and Sport Sciences</skos:altLabel>
	<skos:hiddenLabel xml:lang="en"></skos:hiddenLabel>
	<skos:definition xml:lang="en">The School’s teaching, research and outreach will focus on the prevention of disease and disability to improve quality of life by influencing the practices of the consumer and or the provider. Research will concentrate on the discovery of new knowledge and the application of new knowledge to programs, policies and practice. The School will focus on the improvement of activities in primary four areas, Research, teaching and learning, student experiences and community engagement and outreach.</skos:definition>
	<dc:source rdf:datatype="http://www.w3.org/2001/XMLSchema#string">Australian Ocean Data Network Organisation Register</dc:source>
	<dc:publisher rdf:datatype="http://www.w3.org/2001/XMLSchema#string">eMarine Information Infrastructure (eMII)</dc:publisher>
	<skos:inScheme rdf:resource="http://vocab.aodn.org.au/def/organisation/1"/>
	<skos:broader rdf:resource="http://vocab.aodn.org.au/def/organisation/entity/316"/>
</rdf:Description>

<rdf:Description rdf:about="http://seadatanet.maris2.nl/v_edmo/print.asp?n_code=4323">
	<rdf:type rdf:resource="http://www.w3.org/2000/01/rdf-schema#Resource"/>
</rdf:Description>

<rdf:Description rdf:about="http://seadatanet.maris2.nl/v_edmo/print.asp?n_code=4328">
	<rdf:type rdf:resource="http://www.w3.org/2000/01/rdf-schema#Resource"/>
</rdf:Description>

<rdf:Description rdf:about="http://vocab.aodn.org.au/def/organisation_classes/category/4">
	<rdf:type rdf:resource="http://www.w3.org/2000/01/rdf-schema#Resource"/>
</rdf:Description>

<rdf:Description rdf:about="http://seadatanet.maris2.nl/v_edmo/print.asp?n_code=992">
	<rdf:type rdf:resource="http://www.w3.org/2000/01/rdf-schema#Resource"/>
</rdf:Description>

<rdf:Description rdf:about="http://seadatanet.maris2.nl/v_edmo/print.asp?n_code=3807">
	<rdf:type rdf:resource="http://www.w3.org/2000/01/rdf-schema#Resource"/>
</rdf:Description>

<rdf:Description rdf:about="http://seadatanet.maris2.nl/v_edmo/print.asp?n_code=3790">
	<rdf:type rdf:resource="http://www.w3.org/2000/01/rdf-schema#Resource"/>
</rdf:Description>

<rdf:Description rdf:about="http://seadatanet.maris2.nl/v_edmo/print.asp?n_code=3829">
	<rdf:type rdf:resource="http://www.w3.org/2000/01/rdf-schema#Resource"/>
</rdf:Description>

<rdf:Description rdf:about="http://seadatanet.maris2.nl/v_edmo/print.asp?n_code=3840">
	<rdf:type rdf:resource="http://www.w3.org/2000/01/rdf-schema#Resource"/>
</rdf:Description>

<rdf:Description rdf:about="http://seadatanet.maris2.nl/v_edmo/print.asp?n_code=3533">
	<rdf:type rdf:resource="http://www.w3.org/2000/01/rdf-schema#Resource"/>
</rdf:Description>

<rdf:Description rdf:about="http://seadatanet.maris2.nl/v_edmo/print.asp?n_code=3839">
	<rdf:type rdf:resource="http://www.w3.org/2000/01/rdf-schema#Resource"/>
</rdf:Description>

<rdf:Description rdf:about="http://seadatanet.maris2.nl/v_edmo/print.asp?n_code=3633">
	<rdf:type rdf:resource="http://www.w3.org/2000/01/rdf-schema#Resource"/>
</rdf:Description>

<rdf:Description rdf:about="http://seadatanet.maris2.nl/v_edmo/print.asp?n_code=3721">
	<rdf:type rdf:resource="http://www.w3.org/2000/01/rdf-schema#Resource"/>
</rdf:Description>

<rdf:Description rdf:about="http://seadatanet.maris2.nl/v_edmo/print.asp?n_code=3646">
	<rdf:type rdf:resource="http://www.w3.org/2000/01/rdf-schema#Resource"/>
</rdf:Description>

<rdf:Description rdf:about="http://seadatanet.maris2.nl/v_edmo/print.asp?n_code=3810">
	<rdf:type rdf:resource="http://www.w3.org/2000/01/rdf-schema#Resource"/>
</rdf:Description>

<rdf:Description rdf:about="http://seadatanet.maris2.nl/v_edmo/print.asp?n_code=3649">
	<rdf:type rdf:resource="http://www.w3.org/2000/01/rdf-schema#Resource"/>
</rdf:Description>

<rdf:Description rdf:about="http://seadatanet.maris2.nl/v_edmo/print.asp?n_code=3597">
	<rdf:type rdf:resource="http://www.w3.org/2000/01/rdf-schema#Resource"/>
</rdf:Description>

<rdf:Description rdf:about="http://seadatanet.maris2.nl/v_edmo/print.asp?n_code=1801">
	<rdf:type rdf:resource="http://www.w3.org/2000/01/rdf-schema#Resource"/>
</rdf:Description>

<rdf:Description rdf:about="http://vocab.aodn.org.au/def/organisation/entity/357">
	<rdf:type rdf:resource="http://www.w3.org/2000/01/rdf-schema#Resource"/>
	<rdf:type rdf:resource="http://www.w3.org/2004/02/skos/core#Concept"/>
	<dcterms:creator rdf:datatype="http://www.w3.org/2001/XMLSchema#string">Natalia Atkins</dcterms:creator>
	<dcterms:created rdf:datatype="http://www.w3.org/2001/XMLSchema#dateTime">2015-08-06T10:38:15Z</dcterms:created>
	<skos:prefLabel xml:lang="en">Faculty of Mathematics and Natural Sciences, University of Groningen</skos:prefLabel>
	<skos:altLabel xml:lang="en">Faculty of Mathematics and Natural Sciences</skos:altLabel>
	<skos:hiddenLabel xml:lang="en"></skos:hiddenLabel>
	<skos:definition xml:lang="en">The Faculty of Mathematics and Natural Sciences harbours a kaleidoscope of disciplines and research strengths. Our programmes in research and education range from nanomaterials and biomachinery to astronomy, from mathematics to pharmacy, from neurosciences to computer science, and from molecular and evolutionary biology to marine biology. Our researchers pursue fundamental key questions while collaborating with partners from industry, the medical world and other realms of society. Frontline research groups explore new fields such as synthetic biologyand sustainable energy use.</skos:definition>
	<dc:source rdf:datatype="http://www.w3.org/2001/XMLSchema#string">Australian Ocean Data Network Organisation Register</dc:source>
	<dc:publisher rdf:datatype="http://www.w3.org/2001/XMLSchema#string">eMarine Information Infrastructure (eMMI)</dc:publisher>
	<skos:exactMatch rdf:resource="http://seadatanet.maris2.nl/v_edmo/print.asp?n_code=4369"/>
	<skos:inScheme rdf:resource="http://vocab.aodn.org.au/def/organisation/1"/>
	<skos:broader rdf:resource="http://vocab.aodn.org.au/def/organisation/entity/333"/>
</rdf:Description>

<rdf:Description rdf:about="http://seadatanet.maris2.nl/v_edmo/print.asp?n_code=1596">
	<rdf:type rdf:resource="http://www.w3.org/2000/01/rdf-schema#Resource"/>
</rdf:Description>

<rdf:Description rdf:about="http://seadatanet.maris2.nl/v_edmo/print.asp?n_code=2884">
	<rdf:type rdf:resource="http://www.w3.org/2000/01/rdf-schema#Resource"/>
</rdf:Description>

<rdf:Description rdf:about="http://vocab.aodn.org.au/def/organisation/entity/336">
	<rdf:type rdf:resource="http://www.w3.org/2000/01/rdf-schema#Resource"/>
	<rdf:type rdf:resource="http://www.w3.org/2004/02/skos/core#Concept"/>
	<dcterms:creator rdf:datatype="http://www.w3.org/2001/XMLSchema#string">Natalia Atkins</dcterms:creator>
	<dcterms:created rdf:datatype="http://www.w3.org/2001/XMLSchema#dateTime">2015-07-29T10:38:15Z</dcterms:created>
	<skos:prefLabel xml:lang="en">Institute of Arctic and Alpine Research (INSTAAR), University of Colorado</skos:prefLabel>
	<skos:altLabel xml:lang="en">Institute of Arctic and Alpine Research (INSTAAR)</skos:altLabel>
	<skos:hiddenLabel xml:lang="en">INSTAAR</skos:hiddenLabel>
	<skos:definition xml:lang="en">The Institute of Arctic and Alpine Research (INSTAAR) strives for excellence in research, education, and outreach related to Earth System Science and Global Change in high-latitude, alpine, and other environments. INSTAAR is located at the University of Colorado within the Graduate School and affiliated with departments of Anthropology, CEA Engineering, Environmental Studies, Ecology and Evolutionary Biology, Geography, Geological Sciences, and Atmospheric and Oceanic Sciences (ATOC). INSTAAR also participates in interdepartmental graduate education programs such as Hydrologic Sciences and Oceanography Certificate.</skos:definition>
	<dc:source rdf:datatype="http://www.w3.org/2001/XMLSchema#string">Australian Ocean Data Network Organisation Register</dc:source>
	<dc:publisher rdf:datatype="http://www.w3.org/2001/XMLSchema#string">eMarine Information Infrastructure (eMII)</dc:publisher>
	<skos:exactMatch rdf:resource="http://seadatanet.maris2.nl/v_edmo/print.asp?n_code=1976"/>
	<skos:inScheme rdf:resource="http://vocab.aodn.org.au/def/organisation/1"/>
	<skos:broader rdf:resource="http://vocab.aodn.org.au/def/organisation/entity/335"/>
</rdf:Description>

<rdf:Description rdf:about="http://seadatanet.maris2.nl/v_edmo/print.asp?n_code=3823">
	<rdf:type rdf:resource="http://www.w3.org/2000/01/rdf-schema#Resource"/>
</rdf:Description>

<rdf:Description rdf:about="http://seadatanet.maris2.nl/v_edmo/print.asp?n_code=1976">
	<rdf:type rdf:resource="http://www.w3.org/2000/01/rdf-schema#Resource"/>
</rdf:Description>

<rdf:Description rdf:about="http://vocab.aodn.org.au/def/organisation/entity/338">
	<rdf:type rdf:resource="http://www.w3.org/2000/01/rdf-schema#Resource"/>
	<rdf:type rdf:resource="http://www.w3.org/2004/02/skos/core#Concept"/>
	<dcterms:creator rdf:datatype="http://www.w3.org/2001/XMLSchema#string">Natalia Atkins</dcterms:creator>
	<dcterms:created rdf:datatype="http://www.w3.org/2001/XMLSchema#dateTime">2015-07-29T10:38:15Z</dcterms:created>
	<skos:prefLabel xml:lang="en">Hopkins Marine Station, Stanford University</skos:prefLabel>
	<skos:altLabel xml:lang="en">Hopkins Marine Station</skos:altLabel>
	<skos:hiddenLabel xml:lang="en"></skos:hiddenLabel>
	<skos:definition xml:lang="en">Marine research and teaching laboratory attached to Stanford University and located in Pacific Grove, California.</skos:definition>
	<dc:source rdf:datatype="http://www.w3.org/2001/XMLSchema#string">Australian Ocean Data Network Organisation Register</dc:source>
	<dc:publisher rdf:datatype="http://www.w3.org/2001/XMLSchema#string">eMarine Information Infrastructure (eMII)</dc:publisher>
	<skos:exactMatch rdf:resource="http://seadatanet.maris2.nl/v_edmo/print.asp?n_code=3163"/>
	<skos:inScheme rdf:resource="http://vocab.aodn.org.au/def/organisation/1"/>
	<skos:broader rdf:resource="http://vocab.aodn.org.au/def/organisation/entity/337"/>
</rdf:Description>

<rdf:Description rdf:about="http://seadatanet.maris2.nl/v_edmo/print.asp?n_code=3812">
	<rdf:type rdf:resource="http://www.w3.org/2000/01/rdf-schema#Resource"/>
</rdf:Description>

<rdf:Description rdf:about="http://seadatanet.maris2.nl/v_edmo/print.asp?n_code=3163">
	<rdf:type rdf:resource="http://www.w3.org/2000/01/rdf-schema#Resource"/>
</rdf:Description>

<rdf:Description rdf:about="http://vocab.aodn.org.au/def/organisation/entity/340">
	<rdf:type rdf:resource="http://www.w3.org/2000/01/rdf-schema#Resource"/>
	<rdf:type rdf:resource="http://www.w3.org/2004/02/skos/core#Concept"/>
	<dcterms:creator rdf:datatype="http://www.w3.org/2001/XMLSchema#string">Natalia Atkins</dcterms:creator>
	<dcterms:created rdf:datatype="http://www.w3.org/2001/XMLSchema#dateTime">2015-07-29T10:38:15Z</dcterms:created>
	<skos:prefLabel xml:lang="en">Centre for the Economics and Management of Aquatic Resources (CEMARE), University of Portsmouth</skos:prefLabel>
	<skos:altLabel xml:lang="en">Centre for the Economics and Management of Aquatic Resources (CEMARE)</skos:altLabel>
	<skos:hiddenLabel xml:lang="en">CEMARE</skos:hiddenLabel>
	<skos:definition xml:lang="en">The Centre for the Economics and Management of Aquatic Resources (CEMARE) is a specialised research centre within the Department of Economics at the University of Portsmouth. It was established in the early 1960s to promote multi-disciplinary research into marine resources, with an emphasis on the economic analysis of fisheries. Since then it has developed into an international centre for the multi-disciplinary research of aquatic resources and is actively involved in research, consultancy, training and advanced studies, particularly in fisheries economics. The areas of expertise have expanded to include aquaculture economics and management, recreational fisheries, freshwater fisheries and coastal zone management. In addition, the Centre provides economic, institutional and legal specialisations within the broad area of the management of aquatic resources. The results of research and consultancies are published in core scientific journals and Centre staff also produce a wide range of in-house publications, copies of which are available on request. CEMARE staff and students enjoy full access to the wide range of library, technical and computing services offered by the University, and the Centre keeps an extensive collection of books, reports and journals, maintained by experienced library and technical staff. CEMARE's collection includes material on fisheries economics, as well as material on related subjects. We also have access to various specialist databases such as ASFA (Aquatic Sciences and Fisheries Abstracts). The Centre has active collaborative links at national, regional and international level with a wide range of government, inter-governmental and non-governmental organisations, as well as with other universities and research organisations. Individual members of CEMARE are affiliated to and active participants of the European Association of Fisheries Economists (EAFE), the International Institute of Fisheries Economics and Trade (IIFET), the Institute of Fisheries Management (IFM), Eurocoast UK, the Royal Institution of Chartered Surveyors (RICS) and the International Association for the Study of Common Property (IASCP). CEMARE staff have substantial experience of research, consultancy and postgraduate training in many aspects of commercial and recreational fisheries, and have primary responsibility for running the Postgraduate Programme in Fisheries Economics and Management.</skos:definition>
	<dc:source rdf:datatype="http://www.w3.org/2001/XMLSchema#string">Australian Ocean Data Network Organisation Register</dc:source>
	<dc:publisher rdf:datatype="http://www.w3.org/2001/XMLSchema#string">eMarine Information Infrastructure (eMII)</dc:publisher>
	<skos:exactMatch rdf:resource="http://seadatanet.maris2.nl/v_edmo/print.asp?n_code=2925"/>
	<skos:inScheme rdf:resource="http://vocab.aodn.org.au/def/organisation/1"/>
	<skos:broader rdf:resource="http://vocab.aodn.org.au/def/organisation/entity/339"/>
</rdf:Description>

<rdf:Description rdf:about="http://seadatanet.maris2.nl/v_edmo/print.asp?n_code=2924">
	<rdf:type rdf:resource="http://www.w3.org/2000/01/rdf-schema#Resource"/>
</rdf:Description>

<rdf:Description rdf:about="http://seadatanet.maris2.nl/v_edmo/print.asp?n_code=2925">
	<rdf:type rdf:resource="http://www.w3.org/2000/01/rdf-schema#Resource"/>
</rdf:Description>

<rdf:Description rdf:about="http://seadatanet.maris2.nl/v_edmo/print.asp?n_code=1987">
	<rdf:type rdf:resource="http://www.w3.org/2000/01/rdf-schema#Resource"/>
</rdf:Description>

<rdf:Description rdf:about="http://seadatanet.maris2.nl/v_edmo/print.asp?n_code=4367">
	<rdf:type rdf:resource="http://www.w3.org/2000/01/rdf-schema#Resource"/>
</rdf:Description>

<rdf:Description rdf:about="http://seadatanet.maris2.nl/v_edmo/print.asp?n_code=4366">
	<rdf:type rdf:resource="http://www.w3.org/2000/01/rdf-schema#Resource"/>
</rdf:Description>

<rdf:Description rdf:about="http://seadatanet.maris2.nl/v_edmo/print.asp?n_code=4364">
	<rdf:type rdf:resource="http://www.w3.org/2000/01/rdf-schema#Resource"/>
</rdf:Description>

<rdf:Description rdf:about="http://seadatanet.maris2.nl/v_edmo/print.asp?n_code=4365">
	<rdf:type rdf:resource="http://www.w3.org/2000/01/rdf-schema#Resource"/>
</rdf:Description>

<rdf:Description rdf:about="http://seadatanet.maris2.nl/v_edmo/print.asp?n_code=4354">
	<rdf:type rdf:resource="http://www.w3.org/2000/01/rdf-schema#Resource"/>
</rdf:Description>

<rdf:Description rdf:about="http://seadatanet.maris2.nl/v_edmo/print.asp?n_code=4352">
	<rdf:type rdf:resource="http://www.w3.org/2000/01/rdf-schema#Resource"/>
</rdf:Description>

<rdf:Description rdf:about="http://seadatanet.maris2.nl/v_edmo/print.asp?n_code=4353">
	<rdf:type rdf:resource="http://www.w3.org/2000/01/rdf-schema#Resource"/>
</rdf:Description>

<rdf:Description rdf:about="http://seadatanet.maris2.nl/v_edmo/print.asp?n_code=4362">
	<rdf:type rdf:resource="http://www.w3.org/2000/01/rdf-schema#Resource"/>
</rdf:Description>

<rdf:Description rdf:about="http://vocab.aodn.org.au/def/organisation/entity/419">
	<rdf:type rdf:resource="http://www.w3.org/2000/01/rdf-schema#Resource"/>
	<rdf:type rdf:resource="http://www.w3.org/2004/02/skos/core#Concept"/>
	<dcterms:creator rdf:datatype="http://www.w3.org/2001/XMLSchema#string">Natalia Atkins</dcterms:creator>
	<dcterms:created rdf:datatype="http://www.w3.org/2001/XMLSchema#dateTime">2015-11-09T10:38:15Z</dcterms:created>
	<skos:prefLabel xml:lang="en">Ocean Biogeographic Information System USA (OBIS-USA)</skos:prefLabel>
	<skos:altLabel xml:lang="en"></skos:altLabel>
	<skos:hiddenLabel xml:lang="en">OBIS-USA</skos:hiddenLabel>
	<skos:definition xml:lang="en">OBIS-USA brings together marine biological occurrence data – recorded observations of identifiable marine species at a known time and place, collected primarily from U.S. Waters or with U.S. funding. Coordinated by the Core Science, Analytics, Synthesis, and Libraries (CSASandL) Program of the United States Geological Survey (USGS), OBIS-USA, strives to meet national needs for access to marine data about the organisms and ecosystems. OBIS-USA is part of an international data sharing network (Ocean Biogeographic Information System, OBIS) coordinated by the Intergovernmental Oceanographic Commission, of UNESCO (United Nations Educational, Science and Cultural Organization International Oceanographic Data and Information Exchange. Federal coordination is done in collaboration with the participants of the ad hoc Biodiversity working group organized under the Interagency Working Group on Ocean Partnerships Subcommittee on Ocean Science and Technology. The data contained in OBIS-USA may be used in two different ways. First, using the data dashboard, users can visually examine the full collection of data down to the record level. Second, the Biogeographic Analysis Tool provides an analysis or summary of the biodiversity for defined geographic regions.</skos:definition>
	<dc:source rdf:datatype="http://www.w3.org/2001/XMLSchema#string">Australian Ocean Data Network Organisation Register</dc:source>
	<dc:publisher rdf:datatype="http://www.w3.org/2001/XMLSchema#string">eMarine Information Infrastructure (eMMI)</dc:publisher>
	<skos:exactMatch rdf:resource="http://seadatanet.maris2.nl/webservices/edmo/ws_edmo_get_detail/n_code/4439"/>
	<skos:inScheme rdf:resource="http://vocab.aodn.org.au/def/organisation/1"/>
	<skos:broader rdf:resource="http://vocab.aodn.org.au/def/organisation/entity/350"/>
</rdf:Description>

<rdf:Description rdf:about="http://seadatanet.maris2.nl/v_edmo/print.asp?n_code=4357">
	<rdf:type rdf:resource="http://www.w3.org/2000/01/rdf-schema#Resource"/>
</rdf:Description>

<rdf:Description rdf:about="http://vocab.aodn.org.au/def/organisation/entity/399">
	<rdf:type rdf:resource="http://www.w3.org/2000/01/rdf-schema#Resource"/>
	<rdf:type rdf:resource="http://www.w3.org/2004/02/skos/core#Concept"/>
	<dcterms:creator rdf:datatype="http://www.w3.org/2001/XMLSchema#string">Natalia Atkins</dcterms:creator>
	<dcterms:created rdf:datatype="http://www.w3.org/2001/XMLSchema#dateTime">2015-09-23T10:38:15Z</dcterms:created>
	<skos:prefLabel xml:lang="en">SCAR Marine Biodiversity Information Network (SCAR-MarBIN)</skos:prefLabel>
	<skos:altLabel xml:lang="en"></skos:altLabel>
	<skos:hiddenLabel xml:lang="en">SCAR-MarBIN</skos:hiddenLabel>
	<skos:definition xml:lang="en">SCAR-MarBIN (SCAR Marine Biodiversity Information Network) establishes and supports a distributed system of interoperable databases, forming the Antarctic Regional OBIS Node, under the aegis of SCAR (Scientific Committee on Antarctic Research). SCAR-MarBIN compiles and manages existing and new information on Antarctic marine biodiversity by coordinating, supporting, completing and optimizing database networking. This information will in turn be sent to larger biodiversity initiatives such as OBIS - the information component of the Census of Marine Life (COML)- and GBIF (Global Biodiversity Information Facility). SCAR-MarBIN data policy protocols align with the Antarctic Treaty (Art. III.1) and IPY requirements, as well as data management protocols of GBIF and OBIS. SCAR-MarBIN integrates these efforts, giving a single and easy access to relevant marine biodiversity information and maximizing the exploitation of these resources. SCAR-MarBIN will leave a valuable legacy for future generations, in the form of an information tool that will provide a baseline reference for establishing a State of Antarctic Environment, and predicting the future for marine communities around Antarctica, which are currently facing global change.</skos:definition>
	<dc:source rdf:datatype="http://www.w3.org/2001/XMLSchema#string">Australian Ocean Data Network Organisation Register</dc:source>
	<dc:publisher rdf:datatype="http://www.w3.org/2001/XMLSchema#string">eMarine Information Infrastructure (eMMI)</dc:publisher>
	<skos:exactMatch rdf:resource="http://seadatanet.maris2.nl/v_edmerp/print.asp?n_code=12143"/>
	<skos:inScheme rdf:resource="http://vocab.aodn.org.au/def/organisation/1"/>
	<skos:broader rdf:resource="http://vocab.aodn.org.au/def/organisation/entity/351"/>
</rdf:Description>

<rdf:Description rdf:about="http://seadatanet.maris2.nl/v_edmo/print.asp?n_code=4355">
	<rdf:type rdf:resource="http://www.w3.org/2000/01/rdf-schema#Resource"/>
</rdf:Description>

<rdf:Description rdf:about="http://seadatanet.maris2.nl/v_edmo/print.asp?n_code=4351">
	<rdf:type rdf:resource="http://www.w3.org/2000/01/rdf-schema#Resource"/>
</rdf:Description>

<rdf:Description rdf:about="http://seadatanet.maris2.nl/v_edmo/print.asp?n_code=4356">
	<rdf:type rdf:resource="http://www.w3.org/2000/01/rdf-schema#Resource"/>
</rdf:Description>

<rdf:Description rdf:about="http://vocab.aodn.org.au/def/organisation/entity/361">
	<rdf:type rdf:resource="http://www.w3.org/2000/01/rdf-schema#Resource"/>
	<rdf:type rdf:resource="http://www.w3.org/2004/02/skos/core#Concept"/>
	<dcterms:creator rdf:datatype="http://www.w3.org/2001/XMLSchema#string">Natalia Atkins</dcterms:creator>
	<dcterms:created rdf:datatype="http://www.w3.org/2001/XMLSchema#dateTime">2015-08-05T10:38:15Z</dcterms:created>
	<skos:prefLabel xml:lang="en">Institute of Applied Science (IAS), The University of the South Pacific (USP)</skos:prefLabel>
	<skos:altLabel xml:lang="en">Institute of Applied Science (IAS)</skos:altLabel>
	<skos:hiddenLabel xml:lang="en">IAS</skos:hiddenLabel>
	<skos:definition xml:lang="en">The Institute of Applied Sciences (IAS) at The University of the South Pacific (USP), interfaces the University's expertise and facilities to the independent island countries of the South Pacific Region.  In particular, as a laboratory based institute, it makes these resources available to regional organisations, governments, business, and the people of the region. The Institute of Applied Sciences was established in 1977 (under the name of Institute of Natural Resources) at the Suva campus of The University of the South Pacific with a full time staff of one using the facilities and space provided by the science teaching departments at the University.  IAS has now grown to have 18 full time staff and its own laboratories and scientific equipment located in the Marine Science Building at the "lower" Laucala Bay Campus by the sea. The various units at IAS are the Analytical Unit, Environment Unit, Food Unit, Marine Natural Products Unit and the South Pacific Herbarium.</skos:definition>
	<dc:source rdf:datatype="http://www.w3.org/2001/XMLSchema#string">Australian Ocean Data Network Organisation Register</dc:source>
	<dc:publisher rdf:datatype="http://www.w3.org/2001/XMLSchema#string">eMarine Information Infrastructure (eMII)</dc:publisher>
	<skos:exactMatch rdf:resource="http://seadatanet.maris2.nl/v_edmo/print.asp?n_code=4359"/>
	<skos:inScheme rdf:resource="http://vocab.aodn.org.au/def/organisation/1"/>
	<skos:broader rdf:resource="http://vocab.aodn.org.au/def/organisation/entity/360"/>
</rdf:Description>

<rdf:Description rdf:about="http://seadatanet.maris2.nl/v_edmo/print.asp?n_code=4358">
	<rdf:type rdf:resource="http://www.w3.org/2000/01/rdf-schema#Resource"/>
</rdf:Description>

<rdf:Description rdf:about="http://seadatanet.maris2.nl/v_edmo/print.asp?n_code=4359">
	<rdf:type rdf:resource="http://www.w3.org/2000/01/rdf-schema#Resource"/>
</rdf:Description>

<rdf:Description rdf:about="http://vocab.aodn.org.au/def/organisation/entity/359">
	<rdf:type rdf:resource="http://www.w3.org/2000/01/rdf-schema#Resource"/>
	<rdf:type rdf:resource="http://www.w3.org/2004/02/skos/core#Concept"/>
	<dcterms:creator rdf:datatype="http://www.w3.org/2001/XMLSchema#string">Natalia Atkins</dcterms:creator>
	<dcterms:created rdf:datatype="http://www.w3.org/2001/XMLSchema#dateTime">2015-08-05T10:38:15Z</dcterms:created>
	<skos:prefLabel xml:lang="en">Centre for Biodiversity and Ecology Research (CBER), Department of Biological Sciences, University of Waikato</skos:prefLabel>
	<skos:altLabel xml:lang="en">Centre for Biodiversity and Ecology Research (CBER)</skos:altLabel>
	<skos:hiddenLabel xml:lang="en">CBER</skos:hiddenLabel>
	<skos:definition xml:lang="en">The centre's mssion statement is as follows: to promote sustainable management and habitat restoration through integrated research into biodiversity and ecology.</skos:definition>
	<dc:source rdf:datatype="http://www.w3.org/2001/XMLSchema#string">Australian Ocean Data Network Organisation Register</dc:source>
	<dc:publisher rdf:datatype="http://www.w3.org/2001/XMLSchema#string">eMarine Information Infrastructure (eMII)</dc:publisher>
	<skos:exactMatch rdf:resource="http://seadatanet.maris2.nl/v_edmo/print.asp?n_code=4361"/>
	<skos:inScheme rdf:resource="http://vocab.aodn.org.au/def/organisation/1"/>
	<skos:broader rdf:resource="http://vocab.aodn.org.au/def/organisation/entity/358"/>
</rdf:Description>

<rdf:Description rdf:about="http://seadatanet.maris2.nl/v_edmo/print.asp?n_code=4360">
	<rdf:type rdf:resource="http://www.w3.org/2000/01/rdf-schema#Resource"/>
</rdf:Description>

<rdf:Description rdf:about="http://seadatanet.maris2.nl/v_edmo/print.asp?n_code=4361">
	<rdf:type rdf:resource="http://www.w3.org/2000/01/rdf-schema#Resource"/>
</rdf:Description>

<rdf:Description rdf:about="http://vocab.aodn.org.au/def/organisation/entity/368">
	<rdf:type rdf:resource="http://www.w3.org/2000/01/rdf-schema#Resource"/>
	<rdf:type rdf:resource="http://www.w3.org/2004/02/skos/core#Concept"/>
	<dcterms:creator rdf:datatype="http://www.w3.org/2001/XMLSchema#string">Natalia Atkins</dcterms:creator>
	<dcterms:created rdf:datatype="http://www.w3.org/2001/XMLSchema#dateTime">2015-08-05T10:38:15Z</dcterms:created>
	<skos:prefLabel xml:lang="en">School of Biological Sciences, University of Wales Swansea</skos:prefLabel>
	<skos:altLabel xml:lang="en">School of Biological Sciences</skos:altLabel>
	<skos:hiddenLabel xml:lang="en"></skos:hiddenLabel>
	<skos:definition xml:lang="en">This school is now known as Department of Biosciences, Swansea University.</skos:definition>
	<dc:source rdf:datatype="http://www.w3.org/2001/XMLSchema#string">Australian Ocean Data Network Organisation Register</dc:source>
	<dc:publisher rdf:datatype="http://www.w3.org/2001/XMLSchema#string">eMarine Information Infrastructure (eMII)</dc:publisher>
	<skos:inScheme rdf:resource="http://vocab.aodn.org.au/def/organisation/1"/>
	<skos:broader rdf:resource="http://vocab.aodn.org.au/def/organisation/entity/367"/>
	<skos:scopeNote xml:lang="en">Organisation no longer exists</skos:scopeNote>
</rdf:Description>

<rdf:Description rdf:about="http://vocab.aodn.org.au/def/organisation/entity/356">
	<rdf:type rdf:resource="http://www.w3.org/2000/01/rdf-schema#Resource"/>
	<rdf:type rdf:resource="http://www.w3.org/2004/02/skos/core#Concept"/>
	<dcterms:creator rdf:datatype="http://www.w3.org/2001/XMLSchema#string">Natalia Atkins</dcterms:creator>
	<dcterms:created rdf:datatype="http://www.w3.org/2001/XMLSchema#dateTime">2015-08-05T10:38:15Z</dcterms:created>
	<skos:prefLabel xml:lang="en">Anthropological Institute and Museum (AIM), University of Zurich</skos:prefLabel>
	<skos:altLabel xml:lang="en">Anthropological Institute and Museum (AIM)</skos:altLabel>
	<skos:hiddenLabel xml:lang="en">AIM</skos:hiddenLabel>
	<skos:definition xml:lang="en">Work at the Anthropological Institute and Museum (AIM) is aimed at understanding the evolutionary origins of human morphology and behavior. For both research areas we follow a dual approach. The first is to identify the unique features of humans and reconstruct their evolutionary history. The second is to develop explanations for these novel features based on broad biological principles that emerge from studies of living and fossil primates and other animals.</skos:definition>
	<dc:source rdf:datatype="http://www.w3.org/2001/XMLSchema#string">Australian Ocean Data Network Organisation Register</dc:source>
	<dc:publisher rdf:datatype="http://www.w3.org/2001/XMLSchema#string">eMarine Information Infrastructure (eMII)</dc:publisher>
	<skos:exactMatch rdf:resource="http://seadatanet.maris2.nl/v_edmo/print.asp?n_code=4371"/>
	<skos:inScheme rdf:resource="http://vocab.aodn.org.au/def/organisation/1"/>
	<skos:broader rdf:resource="http://vocab.aodn.org.au/def/organisation/entity/355"/>
</rdf:Description>

<rdf:Description rdf:about="http://seadatanet.maris2.nl/v_edmo/print.asp?n_code=4370">
	<rdf:type rdf:resource="http://www.w3.org/2000/01/rdf-schema#Resource"/>
</rdf:Description>

<rdf:Description rdf:about="http://seadatanet.maris2.nl/v_edmo/print.asp?n_code=4371">
	<rdf:type rdf:resource="http://www.w3.org/2000/01/rdf-schema#Resource"/>
</rdf:Description>

<rdf:Description rdf:about="http://seadatanet.maris2.nl/v_edmo/print.asp?n_code=4369">
	<rdf:type rdf:resource="http://www.w3.org/2000/01/rdf-schema#Resource"/>
</rdf:Description>

<rdf:Description rdf:about="http://seadatanet.maris2.nl/v_edmerp/print.asp?n_code=12142">
	<rdf:type rdf:resource="http://www.w3.org/2000/01/rdf-schema#Resource"/>
</rdf:Description>

<rdf:Description rdf:about="http://seadatanet.maris2.nl/v_edmerp/print.asp?n_code=12143">
	<rdf:type rdf:resource="http://www.w3.org/2000/01/rdf-schema#Resource"/>
</rdf:Description>

<rdf:Description rdf:about="http://seadatanet.maris2.nl/v_edmo/print.asp?n_code=4380">
	<rdf:type rdf:resource="http://www.w3.org/2000/01/rdf-schema#Resource"/>
</rdf:Description>

<rdf:Description rdf:about="http://seadatanet.maris2.nl/v_edmo/print.asp?n_code=4379">
	<rdf:type rdf:resource="http://www.w3.org/2000/01/rdf-schema#Resource"/>
</rdf:Description>

<rdf:Description rdf:about="http://seadatanet.maris2.nl/v_edmo/print.asp?n_code=4381">
	<rdf:type rdf:resource="http://www.w3.org/2000/01/rdf-schema#Resource"/>
</rdf:Description>

<rdf:Description rdf:about="http://vocab.aodn.org.au/organisation/entity/395">
	<rdf:type rdf:resource="http://www.w3.org/2000/01/rdf-schema#Resource"/>
</rdf:Description>

<rdf:Description rdf:about="http://seadatanet.maris2.nl/v_edmo/print.asp?n_code=4368">
	<rdf:type rdf:resource="http://www.w3.org/2000/01/rdf-schema#Resource"/>
</rdf:Description>

<rdf:Description rdf:about="http://seadatanet.maris2.nl/v_edmo/print.asp?n_code=43">
	<rdf:type rdf:resource="http://www.w3.org/2000/01/rdf-schema#Resource"/>
</rdf:Description>

<rdf:Description rdf:about="http://seadatanet.maris2.nl/v_edmo/print.asp?n_code=1850">
	<rdf:type rdf:resource="http://www.w3.org/2000/01/rdf-schema#Resource"/>
</rdf:Description>

<rdf:Description rdf:about="http://seadatanet.maris2.nl/v_edmo/print.asp?n_code=3335">
	<rdf:type rdf:resource="http://www.w3.org/2000/01/rdf-schema#Resource"/>
</rdf:Description>

<rdf:Description rdf:about="http://seadatanet.maris2.nl/v_edmo/print.asp?n_code=2872">
	<rdf:type rdf:resource="http://www.w3.org/2000/01/rdf-schema#Resource"/>
</rdf:Description>

<rdf:Description rdf:about="http://seadatanet.maris2.nl/v_edmo/print.asp?n_code=1054">
	<rdf:type rdf:resource="http://www.w3.org/2000/01/rdf-schema#Resource"/>
</rdf:Description>

<rdf:Description rdf:about="http://seadatanet.maris2.nl/v_edmo/print.asp?n_code=1225">
	<rdf:type rdf:resource="http://www.w3.org/2000/01/rdf-schema#Resource"/>
</rdf:Description>

<rdf:Description rdf:about="http://seadatanet.maris2.nl/v_edmo/print.asp?n_code=3334">
	<rdf:type rdf:resource="http://www.w3.org/2000/01/rdf-schema#Resource"/>
</rdf:Description>

<rdf:Description rdf:about="http://seadatanet.maris2.nl/v_edmo/print.asp?n_code=1537">
	<rdf:type rdf:resource="http://www.w3.org/2000/01/rdf-schema#Resource"/>
</rdf:Description>

<rdf:Description rdf:about="http://seadatanet.maris2.nl/v_edmo/print.asp?n_code=1778">
	<rdf:type rdf:resource="http://www.w3.org/2000/01/rdf-schema#Resource"/>
</rdf:Description>

<rdf:Description rdf:about="http://seadatanet.maris2.nl/v_edmo/print.asp?n_code=3333">
	<rdf:type rdf:resource="http://www.w3.org/2000/01/rdf-schema#Resource"/>
</rdf:Description>

<rdf:Description rdf:about="http://seadatanet.maris2.nl/v_edmo/print.asp?n_code=3332">
	<rdf:type rdf:resource="http://www.w3.org/2000/01/rdf-schema#Resource"/>
</rdf:Description>

<rdf:Description rdf:about="http://vocab.aodn.org.au/organisation/entity/394">
	<rdf:type rdf:resource="http://www.w3.org/2000/01/rdf-schema#Resource"/>
</rdf:Description>

<rdf:Description rdf:about="http://seadatanet.maris2.nl/v_edmo/print.asp?n_code=2947">
	<rdf:type rdf:resource="http://www.w3.org/2000/01/rdf-schema#Resource"/>
</rdf:Description>

<rdf:Description rdf:about="http://vocab.aodn.org.au/organisation/entity/319">
	<rdf:type rdf:resource="http://www.w3.org/2000/01/rdf-schema#Resource"/>
</rdf:Description>

<rdf:Description rdf:about="http://seadatanet.maris2.nl/v_edmo/print.asp?n_code=3739">
	<rdf:type rdf:resource="http://www.w3.org/2000/01/rdf-schema#Resource"/>
</rdf:Description>

<rdf:Description rdf:about="http://vocab.aodn.org.au/def/organisation/entity/370">
	<rdf:type rdf:resource="http://www.w3.org/2000/01/rdf-schema#Resource"/>
	<rdf:type rdf:resource="http://www.w3.org/2004/02/skos/core#Concept"/>
	<dcterms:creator rdf:datatype="http://www.w3.org/2001/XMLSchema#string">Natalia Atkins</dcterms:creator>
	<dcterms:created rdf:datatype="http://www.w3.org/2001/XMLSchema#dateTime">2015-09-18T10:38:15Z</dcterms:created>
	<skos:prefLabel xml:lang="en">Atlantic Oceanographic and Meteorological Laboratory (AOML), National Oceanic and Atmospheric Administration (NOAA)</skos:prefLabel>
	<skos:altLabel xml:lang="en">Atlantic Oceanographic and Meteorological Laboratory (AOML)</skos:altLabel>
	<skos:hiddenLabel xml:lang="en">AOML</skos:hiddenLabel>
	<skos:definition xml:lang="en">NOAA laboratory located in Miami, Florida largely concerned with ocean-driven meteorology, especially hurricanes.</skos:definition>
	<dc:source rdf:datatype="http://www.w3.org/2001/XMLSchema#string">Australian Ocean Data Network Organisation Register</dc:source>
	<dc:publisher rdf:datatype="http://www.w3.org/2001/XMLSchema#string">eMarine Information Infrastructure (eMMI)</dc:publisher>
	<skos:exactMatch rdf:resource="http://seadatanet.maris2.nl/v_edmo/print.asp?n_code=1799"/>
	<skos:inScheme rdf:resource="http://vocab.aodn.org.au/def/organisation/1"/>
	<skos:broader rdf:resource="http://vocab.aodn.org.au/def/organisation/entity/384"/>
</rdf:Description>

<rdf:Description rdf:about="http://vocab.aodn.org.au/def/organisation/entity/392">
	<rdf:type rdf:resource="http://www.w3.org/2000/01/rdf-schema#Resource"/>
	<rdf:type rdf:resource="http://www.w3.org/2004/02/skos/core#Concept"/>
	<dcterms:modified rdf:datatype="http://www.w3.org/2001/XMLSchema#dateTime">2015-10-15T01:56:11Z</dcterms:modified>
	<dcterms:creator rdf:datatype="http://www.w3.org/2001/XMLSchema#string">Natalia Atkins</dcterms:creator>
	<dcterms:created rdf:datatype="http://www.w3.org/2001/XMLSchema#dateTime">2015-09-18T10:38:15Z</dcterms:created>
	<dcterms:contributor rdf:datatype="http://www.w3.org/2001/XMLSchema#string">eMII_Atkins.Natalia</dcterms:contributor>
	<skos:prefLabel xml:lang="en">NOAA National Marine Fisheries Service</skos:prefLabel>
	<skos:altLabel xml:lang="en"></skos:altLabel>
	<skos:hiddenLabel xml:lang="en"></skos:hiddenLabel>
	<skos:definition xml:lang="en">NOAA's National Marine Fisheries Service is the federal agency, a division of the Department of Commerce, responsible for the stewardship of the nation's living marine resources and their habitat. NOAA's National Marine Fisheries Service is responsible for the management, conservation and protection of living marine resources within the United States' Exclusive Economic Zone (water three to 200 mile offshore). Using the tools provided by the Magnuson-Stevens Act, NOAA's National Marine Fisheries Service assesses and predicts the status of fish stocks, ensures compliance with fisheries regulations and works to reduce wasteful fishing practices. Under the Marine Mammal Protection Act and the Endangered Species Act, NOAA's National Marine Fisheries Service recovers protected marine species (i.e. whales, turtles) without unnecessarily impeding economic and recreational opportunities. With the help of the six regional offices and eight councils, NOAA's National Marine Fisheries Service is able to work with communities on fishery management issues. NOAA's National Marine Fisheries Service works to promote sustainable fisheries and to prevent lost economic potential associated with overfishing, declining species and degraded habitats. NOAA's National Marine Fisheries Service strives to balance competing public needs.</skos:definition>
	<dc:source rdf:datatype="http://www.w3.org/2001/XMLSchema#string">Australian Ocean Data Network Organisation Register</dc:source>
	<dc:publisher rdf:datatype="http://www.w3.org/2001/XMLSchema#string">eMarine Information Infrastructure (eMMI)</dc:publisher>
	<skos:exactMatch rdf:resource="http://seadatanet.maris2.nl/v_edmo/print.asp?n_code=1558"/>
	<skos:inScheme rdf:resource="http://vocab.aodn.org.au/def/organisation/1"/>
	<skos:broader rdf:resource="http://vocab.aodn.org.au/def/organisation/entity/384"/>
</rdf:Description>

<rdf:Description rdf:about="http://seadatanet.maris2.nl/v_edmo/print.asp?n_code=1433">
	<rdf:type rdf:resource="http://www.w3.org/2000/01/rdf-schema#Resource"/>
</rdf:Description>

<rdf:Description rdf:about="http://seadatanet.maris2.nl/v_edmo/print.asp?n_code=1224">
	<rdf:type rdf:resource="http://www.w3.org/2000/01/rdf-schema#Resource"/>
</rdf:Description>

<rdf:Description rdf:about="http://seadatanet.maris2.nl/v_edmo/print.asp?n_code=3577">
	<rdf:type rdf:resource="http://www.w3.org/2000/01/rdf-schema#Resource"/>
</rdf:Description>

<rdf:Description rdf:about="http://seadatanet.maris2.nl/v_edmo/print.asp?n_code=17">
	<rdf:type rdf:resource="http://www.w3.org/2000/01/rdf-schema#Resource"/>
</rdf:Description>

<rdf:Description rdf:about="http://seadatanet.maris2.nl/v_edmo/print.asp?n_code=3234">
	<rdf:type rdf:resource="http://www.w3.org/2000/01/rdf-schema#Resource"/>
</rdf:Description>

<rdf:Description rdf:about="http://seadatanet.maris2.nl/v_edmo/print.asp?n_code=630">
	<rdf:type rdf:resource="http://www.w3.org/2000/01/rdf-schema#Resource"/>
</rdf:Description>

<rdf:Description rdf:about="http://seadatanet.maris2.nl/v_edmo/print.asp?n_code=3057">
	<rdf:type rdf:resource="http://www.w3.org/2000/01/rdf-schema#Resource"/>
</rdf:Description>

<rdf:Description rdf:about="http://seadatanet.maris2.nl/v_edmo/print.asp?n_code=1566">
	<rdf:type rdf:resource="http://www.w3.org/2000/01/rdf-schema#Resource"/>
</rdf:Description>

<rdf:Description rdf:about="http://seadatanet.maris2.nl/v_edmo/print.asp?n_code=3844">
	<rdf:type rdf:resource="http://www.w3.org/2000/01/rdf-schema#Resource"/>
</rdf:Description>

<rdf:Description rdf:about="http://vocab.aodn.org.au/organisation/entity/381">
	<rdf:type rdf:resource="http://www.w3.org/2000/01/rdf-schema#Resource"/>
</rdf:Description>

<rdf:Description rdf:about="http://seadatanet.maris2.nl/v_edmo/print.asp?n_code=1799">
	<rdf:type rdf:resource="http://www.w3.org/2000/01/rdf-schema#Resource"/>
</rdf:Description>

<rdf:Description rdf:about="http://seadatanet.maris2.nl/v_edmo/print.asp?n_code=1558">
	<rdf:type rdf:resource="http://www.w3.org/2000/01/rdf-schema#Resource"/>
</rdf:Description>

<rdf:Description rdf:about="http://seadatanet.maris2.nl/v_edmo/print.asp?n_code=4390">
	<rdf:type rdf:resource="http://www.w3.org/2000/01/rdf-schema#Resource"/>
</rdf:Description>

<rdf:Description rdf:about="http://seadatanet.maris2.nl/v_edmo/print.asp?n_code=4388">
	<rdf:type rdf:resource="http://www.w3.org/2000/01/rdf-schema#Resource"/>
</rdf:Description>

<rdf:Description rdf:about="http://vocab.aodn.org.au/def/organisation/entity/407">
	<rdf:type rdf:resource="http://www.w3.org/2000/01/rdf-schema#Resource"/>
	<rdf:type rdf:resource="http://www.w3.org/2004/02/skos/core#Concept"/>
	<dcterms:creator rdf:datatype="http://www.w3.org/2001/XMLSchema#string">Natalia Atkins</dcterms:creator>
	<dcterms:created rdf:datatype="http://www.w3.org/2001/XMLSchema#dateTime">2015-10-30T10:38:15Z</dcterms:created>
	<skos:prefLabel xml:lang="en">Maritime Division, Defence Science and Technology Group (DST Group), Department of Defence (DoD), Australian Government</skos:prefLabel>
	<skos:altLabel xml:lang="en">Maritime Division, Defence Science and Technology Group (DST Group)</skos:altLabel>
	<skos:hiddenLabel xml:lang="en"></skos:hiddenLabel>
	<skos:definition xml:lang="en">Defence Science and Technology Group's (DST Group) Maritime Division provides technologies and scientific and technical expertise to deliver the capability edge to the war fighter and enhance the operational performance and survivability of defence platforms in the maritime domain.</skos:definition>
	<dc:source rdf:datatype="http://www.w3.org/2001/XMLSchema#string">Australian Ocean Data Network Organisation Register</dc:source>
	<dc:publisher rdf:datatype="http://www.w3.org/2001/XMLSchema#string">eMarine Information Infrastructure (eMII)</dc:publisher>
	<skos:exactMatch rdf:resource="http://seadatanet.maris2.nl/v_edmo/print.asp?n_code=3934"/>
	<skos:inScheme rdf:resource="http://vocab.aodn.org.au/def/organisation/1"/>
	<skos:broader rdf:resource="http://vocab.aodn.org.au/def/organisation/entity/279"/>
	<skos:broader rdf:resource="http://vocab.aodn.org.au/def/organisation/entity/406"/>
	<skos:scopeNote xml:lang="en">Replaces http://vocab.aodn.org.au/def/organisation/entity/3</skos:scopeNote>
	<dcterms:replaces rdf:resource="http://vocab.aodn.org.au/def/organisation/entity/3"/>
	<dcterms:replaces xml:lang="en">Maritime Division, Defence Science and Technology Organisation (DSTO), Department of Defence (DoD), Australian Government</dcterms:replaces>
</rdf:Description>

<rdf:Description rdf:about="http://seadatanet.maris2.nl/v_edmo/print.asp?n_code=4442">
	<rdf:type rdf:resource="http://www.w3.org/2000/01/rdf-schema#Resource"/>
</rdf:Description>

<rdf:Description rdf:about="http://seadatanet.maris2.nl/v_edmo/print.asp?n_code=4443">
	<rdf:type rdf:resource="http://www.w3.org/2000/01/rdf-schema#Resource"/>
</rdf:Description>

<rdf:Description rdf:about="http://seadatanet.maris2.nl/v_edmo/print.asp?n_code=4433">
	<rdf:type rdf:resource="http://www.w3.org/2000/01/rdf-schema#Resource"/>
</rdf:Description>

<rdf:Description rdf:about="http://seadatanet.maris2.nl/v_edmo/print.asp?n_code=4434">
	<rdf:type rdf:resource="http://www.w3.org/2000/01/rdf-schema#Resource"/>
</rdf:Description>

<rdf:Description rdf:about="http://seadatanet.maris2.nl/v_edmo/print.asp?n_code=4435">
	<rdf:type rdf:resource="http://www.w3.org/2000/01/rdf-schema#Resource"/>
</rdf:Description>

<rdf:Description rdf:about="http://seadatanet.maris2.nl/v_edmo/print.asp?n_code=4436">
	<rdf:type rdf:resource="http://www.w3.org/2000/01/rdf-schema#Resource"/>
</rdf:Description>

<rdf:Description rdf:about="http://seadatanet.maris2.nl/v_edmo/print.asp?n_code=4437">
	<rdf:type rdf:resource="http://www.w3.org/2000/01/rdf-schema#Resource"/>
</rdf:Description>

<rdf:Description rdf:about="http://seadatanet.maris2.nl/v_edmo/print.asp?n_code=4438">
	<rdf:type rdf:resource="http://www.w3.org/2000/01/rdf-schema#Resource"/>
</rdf:Description>

<rdf:Description rdf:about="http://seadatanet.maris2.nl/v_edmo/print.asp?n_code=4440">
	<rdf:type rdf:resource="http://www.w3.org/2000/01/rdf-schema#Resource"/>
</rdf:Description>

<rdf:Description rdf:about="http://seadatanet.maris2.nl/webservices/edmo/ws_edmo_get_detail/n_code/4439">
	<rdf:type rdf:resource="http://www.w3.org/2000/01/rdf-schema#Resource"/>
</rdf:Description>

<rdf:Description rdf:about="http://purl.org/dc/terms/issued">
	<rdf:type rdf:resource="http://www.w3.org/1999/02/22-rdf-syntax-ns#Property"/>
	<rdf:type rdf:resource="http://www.w3.org/2000/01/rdf-schema#Resource"/>
	<rdfs:subPropertyOf rdf:resource="http://purl.org/dc/terms/issued"/>
</rdf:Description>

<rdf:Description rdf:about="http://www.w3.org/2002/07/owl#versionInfo">
	<rdf:type rdf:resource="http://www.w3.org/1999/02/22-rdf-syntax-ns#Property"/>
	<rdf:type rdf:resource="http://www.w3.org/2000/01/rdf-schema#Resource"/>
	<rdfs:subPropertyOf rdf:resource="http://www.w3.org/2002/07/owl#versionInfo"/>
</rdf:Description>

<rdf:Description rdf:about="http://vocab.aodn.org.au/def/organisation/entity/420">
	<rdf:type rdf:resource="http://www.w3.org/2000/01/rdf-schema#Resource"/>
	<rdf:type rdf:resource="http://www.w3.org/2004/02/skos/core#Concept"/>
	<dcterms:modified rdf:datatype="http://www.w3.org/2001/XMLSchema#dateTime">2016-01-04T04:54:19Z</dcterms:modified>
	<dcterms:creator rdf:datatype="http://www.w3.org/2001/XMLSchema#string">Natalia Atkins</dcterms:creator>
	<dcterms:created rdf:datatype="http://www.w3.org/2001/XMLSchema#dateTime">2016-01-04T10:38:15Z</dcterms:created>
	<dcterms:contributor rdf:datatype="http://www.w3.org/2001/XMLSchema#string">eMII_Atkins.Natalia</dcterms:contributor>
	<skos:broadMatch rdf:resource="http://vocab.aodn.org.au/def/organisation_classes/category/4"/>
	<skos:prefLabel xml:lang="en">The University of British Columbia (UBC)</skos:prefLabel>
	<skos:altLabel xml:lang="en"></skos:altLabel>
	<skos:hiddenLabel xml:lang="en">UBC</skos:hiddenLabel>
	<skos:definition xml:lang="en">Founded in 1908 as the McGill University College of British Columbia, the University became independent and adopted its current name in 1915. The University has two campuses: Vancouver and Okanagan Valley.</skos:definition>
	<dc:source rdf:datatype="http://www.w3.org/2001/XMLSchema#string">Australian Ocean Data Network Organisation Register</dc:source>
	<dc:publisher rdf:datatype="http://www.w3.org/2001/XMLSchema#string">eMarine Information Infrastructure (eMII)</dc:publisher>
	<skos:narrower rdf:resource="http://vocab.aodn.org.au/def/organisation/entity/421"/>
	<skos:narrower rdf:resource="http://vocab.aodn.org.au/def/organisation/entity/422"/>
	<skos:narrower rdf:resource="http://vocab.aodn.org.au/def/organisation/entity/362"/>
	<skos:narrower rdf:resource="http://vocab.aodn.org.au/def/organisation/entity/423"/>
	<skos:topConceptOf rdf:resource="http://vocab.aodn.org.au/def/organisation/1"/>
	<skos:inScheme rdf:resource="http://vocab.aodn.org.au/def/organisation/1"/>
</rdf:Description>

<rdf:Description rdf:about="http://vocab.aodn.org.au/def/organisation/entity/424">
	<rdf:type rdf:resource="http://www.w3.org/2000/01/rdf-schema#Resource"/>
	<rdf:type rdf:resource="http://www.w3.org/2004/02/skos/core#Concept"/>
	<dcterms:modified rdf:datatype="http://www.w3.org/2001/XMLSchema#dateTime">2016-01-04T04:54:04Z</dcterms:modified>
	<dcterms:creator rdf:datatype="http://www.w3.org/2001/XMLSchema#string">Natalia Atkins</dcterms:creator>
	<dcterms:created rdf:datatype="http://www.w3.org/2001/XMLSchema#dateTime">2016-01-04T10:38:15Z</dcterms:created>
	<dcterms:contributor rdf:datatype="http://www.w3.org/2001/XMLSchema#string">eMII_Atkins.Natalia</dcterms:contributor>
	<skos:broadMatch rdf:resource="http://vocab.aodn.org.au/def/organisation_classes/category/4"/>
	<skos:prefLabel xml:lang="en">Brock University</skos:prefLabel>
	<skos:altLabel xml:lang="en"></skos:altLabel>
	<skos:hiddenLabel xml:lang="en"></skos:hiddenLabel>
	<skos:definition xml:lang="en">Brock University was established in 1964, and is located in St Catharines, Ontario, Canada.</skos:definition>
	<dc:source rdf:datatype="http://www.w3.org/2001/XMLSchema#string">Australian Ocean Data Network Organisation Register</dc:source>
	<dc:publisher rdf:datatype="http://www.w3.org/2001/XMLSchema#string">eMarine Information Infrastructure (eMII)</dc:publisher>
	<skos:narrower rdf:resource="http://vocab.aodn.org.au/def/organisation/entity/425"/>
	<skos:topConceptOf rdf:resource="http://vocab.aodn.org.au/def/organisation/1"/>
	<skos:inScheme rdf:resource="http://vocab.aodn.org.au/def/organisation/1"/>
</rdf:Description>

<rdf:Description rdf:about="http://vocab.aodn.org.au/def/organisation/entity/431">
	<rdf:type rdf:resource="http://www.w3.org/2000/01/rdf-schema#Resource"/>
	<rdf:type rdf:resource="http://www.w3.org/2004/02/skos/core#Concept"/>
	<dcterms:modified rdf:datatype="http://www.w3.org/2001/XMLSchema#dateTime">2016-01-06T02:18:51Z</dcterms:modified>
	<dcterms:creator rdf:datatype="http://www.w3.org/2001/XMLSchema#string">Natalia Atkins</dcterms:creator>
	<dcterms:created rdf:datatype="http://www.w3.org/2001/XMLSchema#dateTime">2016-01-06T10:38:15Z</dcterms:created>
	<dcterms:contributor rdf:datatype="http://www.w3.org/2001/XMLSchema#string">eMII_Atkins.Natalia</dcterms:contributor>
	<skos:broadMatch rdf:resource="http://vocab.aodn.org.au/def/organisation_classes/category/4"/>
	<skos:prefLabel xml:lang="en">Iowa State University</skos:prefLabel>
	<skos:altLabel xml:lang="en"></skos:altLabel>
	<skos:hiddenLabel xml:lang="en"></skos:hiddenLabel>
	<skos:definition xml:lang="en">Iowa State is an international university with a friendly welcoming personality. Students from all 50 states and more than 100 countries come to Ames, Iowa, to choose from 100 majors, study with world-class scholars and hone their leadership skills in 800-plus student organizations. Iowa State offers a great environment where students can enjoy reaching their potential and discovering their passions.</skos:definition>
	<dc:source rdf:datatype="http://www.w3.org/2001/XMLSchema#string">Australian Ocean Data Network Organisation Register</dc:source>
	<dc:publisher rdf:datatype="http://www.w3.org/2001/XMLSchema#string">eMarine Information Infrastructure (eMII)</dc:publisher>
	<skos:exactMatch rdf:resource="http://seadatanet.maris2.nl/v_edmo/print.asp?n_code=4463"/>
	<skos:narrower rdf:resource="http://vocab.aodn.org.au/def/organisation/entity/432"/>
	<skos:topConceptOf rdf:resource="http://vocab.aodn.org.au/def/organisation/1"/>
	<skos:inScheme rdf:resource="http://vocab.aodn.org.au/def/organisation/1"/>
</rdf:Description>

<rdf:Description rdf:about="http://vocab.aodn.org.au/def/organisation/entity/436">
	<rdf:type rdf:resource="http://www.w3.org/2000/01/rdf-schema#Resource"/>
	<rdf:type rdf:resource="http://www.w3.org/2004/02/skos/core#Concept"/>
	<dcterms:modified rdf:datatype="http://www.w3.org/2001/XMLSchema#dateTime">2016-01-06T04:56:27Z</dcterms:modified>
	<dcterms:creator rdf:datatype="http://www.w3.org/2001/XMLSchema#string">Natalia Atkins</dcterms:creator>
	<dcterms:created rdf:datatype="http://www.w3.org/2001/XMLSchema#dateTime">2016-01-06T10:38:15Z</dcterms:created>
	<dcterms:contributor rdf:datatype="http://www.w3.org/2001/XMLSchema#string">eMII_Atkins.Natalia</dcterms:contributor>
	<skos:broadMatch rdf:resource="http://vocab.aodn.org.au/def/organisation_classes/category/4"/>
	<skos:prefLabel xml:lang="en">Florida International University (FIU)</skos:prefLabel>
	<skos:altLabel xml:lang="en"></skos:altLabel>
	<skos:hiddenLabel xml:lang="en">FIU</skos:hiddenLabel>
	<skos:definition xml:lang="en">FIU belongs to the 12-campus State University System of Florida and is one of Florida's primary graduate research universities, awarding over 3,400 graduate and professional degrees annually.[9] The university offers 191 programs of study with more than 280 majors in 23 colleges and schools. FIU offers many graduate programs, including architecture, business administration, engineering, law, and medicine, offering 81 master's degrees, 34 doctoral degrees, and 3 professional degrees.</skos:definition>
	<dc:source rdf:datatype="http://www.w3.org/2001/XMLSchema#string">Australian Ocean Data Network Organisation Register</dc:source>
	<dc:publisher rdf:datatype="http://www.w3.org/2001/XMLSchema#string">eMarine Information Infrastructure (eMII)</dc:publisher>
	<skos:exactMatch rdf:resource="http://seadatanet.maris2.nl/v_edmo/print.asp?n_code=4468"/>
	<skos:narrower rdf:resource="http://vocab.aodn.org.au/def/organisation/entity/437"/>
	<skos:narrower rdf:resource="http://vocab.aodn.org.au/def/organisation/entity/438"/>
	<skos:topConceptOf rdf:resource="http://vocab.aodn.org.au/def/organisation/1"/>
	<skos:inScheme rdf:resource="http://vocab.aodn.org.au/def/organisation/1"/>
</rdf:Description>

<rdf:Description rdf:about="http://vocab.aodn.org.au/def/organisation/entity/440">
	<rdf:type rdf:resource="http://www.w3.org/2000/01/rdf-schema#Resource"/>
	<rdf:type rdf:resource="http://www.w3.org/2004/02/skos/core#Concept"/>
	<dcterms:modified rdf:datatype="http://www.w3.org/2001/XMLSchema#dateTime">2016-01-06T05:02:27Z</dcterms:modified>
	<dcterms:creator rdf:datatype="http://www.w3.org/2001/XMLSchema#string">Natalia Atkins</dcterms:creator>
	<dcterms:created rdf:datatype="http://www.w3.org/2001/XMLSchema#dateTime">2016-01-06T10:38:15Z</dcterms:created>
	<dcterms:contributor rdf:datatype="http://www.w3.org/2001/XMLSchema#string">eMII_Atkins.Natalia</dcterms:contributor>
	<skos:broadMatch rdf:resource="http://vocab.aodn.org.au/def/organisation_classes/category/4"/>
	<skos:prefLabel xml:lang="en">Georgetown University (GU)</skos:prefLabel>
	<skos:altLabel xml:lang="en"></skos:altLabel>
	<skos:hiddenLabel xml:lang="en">GU</skos:hiddenLabel>
	<skos:definition xml:lang="en">Comprising 9 undergraduate and graduate schools, the university has about 7,000 undergraduate and over 10,000 post-graduate students from a wide variety of religious, ethnic, and geographic backgrounds, including 130 foreign countries.</skos:definition>
	<dc:source rdf:datatype="http://www.w3.org/2001/XMLSchema#string">Australian Ocean Data Network Organisation Register</dc:source>
	<dc:publisher rdf:datatype="http://www.w3.org/2001/XMLSchema#string">eMarine Information Infrastructure (eMII)</dc:publisher>
	<skos:exactMatch rdf:resource="http://seadatanet.maris2.nl/v_edmo/print.asp?n_code=4472"/>
	<skos:topConceptOf rdf:resource="http://vocab.aodn.org.au/def/organisation/1"/>
	<skos:inScheme rdf:resource="http://vocab.aodn.org.au/def/organisation/1"/>
</rdf:Description>

<rdf:Description rdf:about="http://vocab.aodn.org.au/def/organisation/entity/443">
	<rdf:type rdf:resource="http://www.w3.org/2000/01/rdf-schema#Resource"/>
	<rdf:type rdf:resource="http://www.w3.org/2004/02/skos/core#Concept"/>
	<dcterms:modified rdf:datatype="http://www.w3.org/2001/XMLSchema#dateTime">2016-01-06T05:57:47Z</dcterms:modified>
	<dcterms:creator rdf:datatype="http://www.w3.org/2001/XMLSchema#string">Natalia Atkins</dcterms:creator>
	<dcterms:created rdf:datatype="http://www.w3.org/2001/XMLSchema#dateTime">2016-01-06T10:38:15Z</dcterms:created>
	<dcterms:contributor rdf:datatype="http://www.w3.org/2001/XMLSchema#string">eMII_Atkins.Natalia</dcterms:contributor>
	<skos:broadMatch rdf:resource="http://vocab.aodn.org.au/def/organisation_classes/category/4"/>
	<skos:prefLabel xml:lang="en">The University of Texas at Austin</skos:prefLabel>
	<skos:altLabel xml:lang="en"></skos:altLabel>
	<skos:hiddenLabel xml:lang="en"></skos:hiddenLabel>
	<skos:definition xml:lang="en">UT Austin is home to more than 51,000 students and 3,000 teaching faculty. It is the flagship university of the UT system.</skos:definition>
	<dc:source rdf:datatype="http://www.w3.org/2001/XMLSchema#string">Australian Ocean Data Network Organisation Register</dc:source>
	<dc:publisher rdf:datatype="http://www.w3.org/2001/XMLSchema#string">eMarine Information Infrastructure (eMII)</dc:publisher>
	<skos:exactMatch rdf:resource="http://seadatanet.maris2.nl/v_edmo/print.asp?n_code=4475"/>
	<skos:topConceptOf rdf:resource="http://vocab.aodn.org.au/def/organisation/1"/>
	<skos:inScheme rdf:resource="http://vocab.aodn.org.au/def/organisation/1"/>
</rdf:Description>

<rdf:Description rdf:about="http://vocab.aodn.org.au/def/organisation/entity/444">
	<rdf:type rdf:resource="http://www.w3.org/2000/01/rdf-schema#Resource"/>
	<rdf:type rdf:resource="http://www.w3.org/2004/02/skos/core#Concept"/>
	<dcterms:modified rdf:datatype="http://www.w3.org/2001/XMLSchema#dateTime">2016-01-07T02:27:53Z</dcterms:modified>
	<dcterms:creator rdf:datatype="http://www.w3.org/2001/XMLSchema#string">Natalia Atkins</dcterms:creator>
	<dcterms:created rdf:datatype="http://www.w3.org/2001/XMLSchema#dateTime">2016-01-07T10:38:15Z</dcterms:created>
	<dcterms:contributor rdf:datatype="http://www.w3.org/2001/XMLSchema#string">eMII_Atkins.Natalia</dcterms:contributor>
	<skos:broadMatch rdf:resource="http://vocab.aodn.org.au/def/organisation_classes/category/4"/>
	<skos:prefLabel xml:lang="en">University of Potsdam</skos:prefLabel>
	<skos:altLabel xml:lang="en"></skos:altLabel>
	<skos:hiddenLabel xml:lang="en"></skos:hiddenLabel>
	<skos:definition xml:lang="en">The University of Potsdam promotes the dialogue between theory and practice by means of current research. The research profile of the University of Potsdam is shaped primarily by five faculties. Constantly increasing third-party funding volume testifies to the quality of the research conducted at the University today. The University of Potsdam also has successful, productive cooperative agreements with more than 20 non-university research institutions in the region.</skos:definition>
	<dc:source rdf:datatype="http://www.w3.org/2001/XMLSchema#string">Australian Ocean Data Network Organisation Register</dc:source>
	<dc:publisher rdf:datatype="http://www.w3.org/2001/XMLSchema#string">eMarine Information Infrastructure (eMII)</dc:publisher>
	<skos:exactMatch rdf:resource="http://seadatanet.maris2.nl/v_edmo/print.asp?n_code=4449"/>
	<skos:topConceptOf rdf:resource="http://vocab.aodn.org.au/def/organisation/1"/>
	<skos:inScheme rdf:resource="http://vocab.aodn.org.au/def/organisation/1"/>
</rdf:Description>

<rdf:Description rdf:about="http://vocab.aodn.org.au/def/organisation/entity/445">
	<rdf:type rdf:resource="http://www.w3.org/2000/01/rdf-schema#Resource"/>
	<rdf:type rdf:resource="http://www.w3.org/2004/02/skos/core#Concept"/>
	<dcterms:modified rdf:datatype="http://www.w3.org/2001/XMLSchema#dateTime">2016-01-07T02:27:46Z</dcterms:modified>
	<dcterms:creator rdf:datatype="http://www.w3.org/2001/XMLSchema#string">Natalia Atkins</dcterms:creator>
	<dcterms:created rdf:datatype="http://www.w3.org/2001/XMLSchema#dateTime">2016-01-07T10:38:15Z</dcterms:created>
	<dcterms:contributor rdf:datatype="http://www.w3.org/2001/XMLSchema#string">eMII_Atkins.Natalia</dcterms:contributor>
	<skos:broadMatch rdf:resource="http://vocab.aodn.org.au/def/organisation_classes/category/4"/>
	<skos:prefLabel xml:lang="en">University of Iceland</skos:prefLabel>
	<skos:altLabel xml:lang="en"></skos:altLabel>
	<skos:hiddenLabel xml:lang="en"></skos:hiddenLabel>
	<skos:definition xml:lang="en"></skos:definition>
	<dc:source rdf:datatype="http://www.w3.org/2001/XMLSchema#string">Australian Ocean Data Network Organisation Register</dc:source>
	<dc:publisher rdf:datatype="http://www.w3.org/2001/XMLSchema#string">eMarine Information Infrastructure (eMII)</dc:publisher>
	<skos:exactMatch rdf:resource="http://seadatanet.maris2.nl/v_edmo/print.asp?n_code=4447"/>
	<skos:narrower rdf:resource="http://vocab.aodn.org.au/def/organisation/entity/365"/>
	<skos:topConceptOf rdf:resource="http://vocab.aodn.org.au/def/organisation/1"/>
	<skos:inScheme rdf:resource="http://vocab.aodn.org.au/def/organisation/1"/>
</rdf:Description>

<rdf:Description rdf:about="http://vocab.aodn.org.au/def/organisation/entity/446">
	<rdf:type rdf:resource="http://www.w3.org/2000/01/rdf-schema#Resource"/>
	<rdf:type rdf:resource="http://www.w3.org/2004/02/skos/core#Concept"/>
	<dcterms:modified rdf:datatype="http://www.w3.org/2001/XMLSchema#dateTime">2016-01-07T02:40:02Z</dcterms:modified>
	<dcterms:creator rdf:datatype="http://www.w3.org/2001/XMLSchema#string">Natalia Atkins</dcterms:creator>
	<dcterms:created rdf:datatype="http://www.w3.org/2001/XMLSchema#dateTime">2016-01-07T10:38:15Z</dcterms:created>
	<dcterms:contributor rdf:datatype="http://www.w3.org/2001/XMLSchema#string">eMII_Atkins.Natalia</dcterms:contributor>
	<skos:broadMatch rdf:resource="http://vocab.aodn.org.au/def/organisation_classes/category/4"/>
	<skos:prefLabel xml:lang="en">Institute for Research in Economics and Business Administration (SNF)</skos:prefLabel>
	<skos:altLabel xml:lang="en"></skos:altLabel>
	<skos:hiddenLabel xml:lang="en">SNF</skos:hiddenLabel>
	<skos:definition xml:lang="en"></skos:definition>
	<dc:source rdf:datatype="http://www.w3.org/2001/XMLSchema#string">Australian Ocean Data Network Organisation Register</dc:source>
	<dc:publisher rdf:datatype="http://www.w3.org/2001/XMLSchema#string">eMarine Information Infrastructure (eMMI)</dc:publisher>
	<skos:exactMatch rdf:resource="http://seadatanet.maris2.nl/v_edmo/print.asp?n_code=4448"/>
	<skos:topConceptOf rdf:resource="http://vocab.aodn.org.au/def/organisation/1"/>
	<skos:inScheme rdf:resource="http://vocab.aodn.org.au/def/organisation/1"/>
</rdf:Description>

<rdf:Description rdf:about="http://vocab.aodn.org.au/def/organisation/entity/449">
	<rdf:type rdf:resource="http://www.w3.org/2000/01/rdf-schema#Resource"/>
	<rdf:type rdf:resource="http://www.w3.org/2004/02/skos/core#Concept"/>
	<dcterms:modified rdf:datatype="http://www.w3.org/2001/XMLSchema#dateTime">2016-01-07T02:39:16Z</dcterms:modified>
	<dcterms:creator rdf:datatype="http://www.w3.org/2001/XMLSchema#string">Natalia Atkins</dcterms:creator>
	<dcterms:created rdf:datatype="http://www.w3.org/2001/XMLSchema#dateTime">2016-01-07T10:38:15Z</dcterms:created>
	<dcterms:contributor rdf:datatype="http://www.w3.org/2001/XMLSchema#string">eMII_Atkins.Natalia</dcterms:contributor>
	<skos:broadMatch rdf:resource="http://vocab.aodn.org.au/def/organisation_classes/category/4"/>
	<skos:prefLabel xml:lang="en">University of Southampton</skos:prefLabel>
	<skos:altLabel xml:lang="en"></skos:altLabel>
	<skos:hiddenLabel xml:lang="en"></skos:hiddenLabel>
	<skos:definition xml:lang="en">The University of Southampton is a world-class university built on the quality and diversity of our community. Our staff place a high value on excellence and creativity, supporting independence of thought, and the freedom to challenge existing knowledge and beliefs through critical research and scholarship. Through our education and research we transform people’s lives and change the world for the better.</skos:definition>
	<dc:source rdf:datatype="http://www.w3.org/2001/XMLSchema#string">Australian Ocean Data Network Organisation Register</dc:source>
	<dc:publisher rdf:datatype="http://www.w3.org/2001/XMLSchema#string">eMarine Information Infrastructure (eMMI)</dc:publisher>
	<skos:exactMatch rdf:resource="http://seadatanet.maris2.nl/v_edmo/print.asp?n_code=4457"/>
	<skos:narrower rdf:resource="http://vocab.aodn.org.au/def/organisation/entity/332"/>
	<skos:topConceptOf rdf:resource="http://vocab.aodn.org.au/def/organisation/1"/>
	<skos:inScheme rdf:resource="http://vocab.aodn.org.au/def/organisation/1"/>
</rdf:Description>

<rdf:Description rdf:about="http://vocab.aodn.org.au/def/organisation/entity/447">
	<rdf:type rdf:resource="http://www.w3.org/2000/01/rdf-schema#Resource"/>
	<rdf:type rdf:resource="http://www.w3.org/2004/02/skos/core#Concept"/>
	<dcterms:modified rdf:datatype="http://www.w3.org/2001/XMLSchema#dateTime">2016-01-07T02:42:03Z</dcterms:modified>
	<dcterms:creator rdf:datatype="http://www.w3.org/2001/XMLSchema#string">Natalia Atkins</dcterms:creator>
	<dcterms:created rdf:datatype="http://www.w3.org/2001/XMLSchema#dateTime">2016-01-07T10:38:15Z</dcterms:created>
	<dcterms:contributor rdf:datatype="http://www.w3.org/2001/XMLSchema#string">eMII_Atkins.Natalia</dcterms:contributor>
	<skos:broadMatch rdf:resource="http://vocab.aodn.org.au/def/organisation_classes/category/4"/>
	<skos:prefLabel xml:lang="en">University of Hull</skos:prefLabel>
	<skos:altLabel xml:lang="en"></skos:altLabel>
	<skos:hiddenLabel xml:lang="en"></skos:hiddenLabel>
	<skos:definition xml:lang="en">At the University of Hull - an empowered and engaged institution - we're constantly 'going beyond' and investing in every facet of our culture in a bid to demonstrate our commitment to becoming the competitive, responsive and resilient community that will help you fulfil your potential during your time with us. Our quest for advanced knowledge has cultivated our renown for world-class, high-rated teaching, research provision, impressive facilities, and a strong support network on both Hull and Scarborough campuses. Our research, in particular, is of international acclaim in many fields, the quality of which informs our teaching at all levels.</skos:definition>
	<dc:source rdf:datatype="http://www.w3.org/2001/XMLSchema#string">Australian Ocean Data Network Organisation Register</dc:source>
	<dc:publisher rdf:datatype="http://www.w3.org/2001/XMLSchema#string">eMarine Information Infrastructure (eMII)</dc:publisher>
	<skos:exactMatch rdf:resource="http://seadatanet.maris2.nl/v_edmo/print.asp?n_code=4455"/>
	<skos:narrower rdf:resource="http://vocab.aodn.org.au/def/organisation/entity/448"/>
	<skos:topConceptOf rdf:resource="http://vocab.aodn.org.au/def/organisation/1"/>
	<skos:inScheme rdf:resource="http://vocab.aodn.org.au/def/organisation/1"/>
</rdf:Description>

<rdf:Description rdf:about="http://vocab.aodn.org.au/def/organisation/entity/451">
	<rdf:type rdf:resource="http://www.w3.org/2000/01/rdf-schema#Resource"/>
	<rdf:type rdf:resource="http://www.w3.org/2004/02/skos/core#Concept"/>
	<dcterms:modified rdf:datatype="http://www.w3.org/2001/XMLSchema#dateTime">2016-01-13T01:53:11Z</dcterms:modified>
	<dcterms:creator rdf:datatype="http://www.w3.org/2001/XMLSchema#string">Natalia Atkins</dcterms:creator>
	<dcterms:created rdf:datatype="http://www.w3.org/2001/XMLSchema#dateTime">2016-01-13T10:38:15Z</dcterms:created>
	<dcterms:contributor rdf:datatype="http://www.w3.org/2001/XMLSchema#string">eMII_Atkins.Natalia</dcterms:contributor>
	<skos:broadMatch rdf:resource="http://vocab.aodn.org.au/def/organisation_classes/category/4"/>
	<skos:prefLabel xml:lang="en">Schmidt Ocean Institute</skos:prefLabel>
	<skos:altLabel xml:lang="en"></skos:altLabel>
	<skos:hiddenLabel xml:lang="en">SOI</skos:hiddenLabel>
	<skos:definition xml:lang="en">Schmidt Ocean Institute was established to advance the frontiers of ocean research and exploration through innovative technologies, intelligent observation and analysis, and open sharing of information.</skos:definition>
	<dc:source rdf:datatype="http://www.w3.org/2001/XMLSchema#string">Australian Ocean Data Network Organisation Register</dc:source>
	<dc:publisher rdf:datatype="http://www.w3.org/2001/XMLSchema#string">eMarine Information Infrastructure (eMII)</dc:publisher>
	<skos:exactMatch rdf:resource="http://seadatanet.maris2.nl/v_edmo/print.asp?n_code=4378"/>
	<skos:topConceptOf rdf:resource="http://vocab.aodn.org.au/def/organisation/1"/>
	<skos:inScheme rdf:resource="http://vocab.aodn.org.au/def/organisation/1"/>
</rdf:Description>

<rdf:Description rdf:about="http://vocab.aodn.org.au/def/organisation/entity/452">
	<rdf:type rdf:resource="http://www.w3.org/2000/01/rdf-schema#Resource"/>
	<rdf:type rdf:resource="http://www.w3.org/2004/02/skos/core#Concept"/>
	<dcterms:modified rdf:datatype="http://www.w3.org/2001/XMLSchema#dateTime">2016-02-22T23:46:07Z</dcterms:modified>
	<dcterms:creator rdf:datatype="http://www.w3.org/2001/XMLSchema#string">Natalia Atkins</dcterms:creator>
	<dcterms:created rdf:datatype="http://www.w3.org/2001/XMLSchema#dateTime">2016-02-23T10:38:15Z</dcterms:created>
	<dcterms:contributor rdf:datatype="http://www.w3.org/2001/XMLSchema#string">eMII_Atkins.Natalia</dcterms:contributor>
	<skos:broadMatch rdf:resource="http://vocab.aodn.org.au/def/organisation_classes/category/2"/>
	<skos:prefLabel xml:lang="en">Department of Science, Information Technology and Innovation (DSITI), Queensland Government</skos:prefLabel>
	<skos:altLabel xml:lang="en">Department of Science, Information Technology and Innovation (DSITI)</skos:altLabel>
	<skos:hiddenLabel xml:lang="en">DSITI</skos:hiddenLabel>
	<skos:definition xml:lang="en">The Department aims to: develop and coordinate science and ICT policy across the Queensland Government; develop a whole-of-government approach on innovation as a key enabler of the knowledge economy; support and invest in research and development to meet the state's future challenges; build a strong relationship with key innovation and ICT industry stakeholders; improve government service delivery through efficient use of information and communications technology services and shared services; help Queensland businesses and consumers to benefit from current and emerging digital technologies and services; and, manage the state's intellectual property policy and assets.</skos:definition>
	<dc:source rdf:datatype="http://www.w3.org/2001/XMLSchema#string">Australian Ocean Data Network Organisation Register</dc:source>
	<dc:publisher rdf:datatype="http://www.w3.org/2001/XMLSchema#string">eMarine Information Infrastructure (eMII)</dc:publisher>
	<skos:exactMatch rdf:resource="http://seadatanet.maris2.nl/v_edmo/print.asp?n_code=4378"/>
	<skos:topConceptOf rdf:resource="http://vocab.aodn.org.au/def/organisation/1"/>
	<skos:inScheme rdf:resource="http://vocab.aodn.org.au/def/organisation/1"/>
</rdf:Description>

<rdf:Description rdf:about="http://vocab.aodn.org.au/def/organisation/entity/453">
	<rdf:type rdf:resource="http://www.w3.org/2000/01/rdf-schema#Resource"/>
	<rdf:type rdf:resource="http://www.w3.org/2004/02/skos/core#Concept"/>
	<dcterms:modified rdf:datatype="http://www.w3.org/2001/XMLSchema#dateTime">2016-04-18T01:14:49Z</dcterms:modified>
	<dcterms:creator rdf:datatype="http://www.w3.org/2001/XMLSchema#string">Natalia Atkins</dcterms:creator>
	<dcterms:created rdf:datatype="http://www.w3.org/2001/XMLSchema#dateTime">2016-04-18T10:38:15Z</dcterms:created>
	<dcterms:contributor rdf:datatype="http://www.w3.org/2001/XMLSchema#string">eMII_Atkins.Natalia</dcterms:contributor>
	<skos:broadMatch rdf:resource="http://vocab.aodn.org.au/def/organisation_classes/category/1"/>
	<skos:prefLabel xml:lang="en">Sydney Water</skos:prefLabel>
	<skos:altLabel xml:lang="en"></skos:altLabel>
	<skos:hiddenLabel xml:lang="en"></skos:hiddenLabel>
	<skos:definition xml:lang="en">Sydney Water is Australia's largest water utility. Their area of operations covers 12,700 km2  and includes Sydney, the Illawarra and the Blue Mountains regions. It is a statutory State Owned Corporation, wholly owned by the New South Wales Government.</skos:definition>
	<dc:source rdf:datatype="http://www.w3.org/2001/XMLSchema#string">Australian Ocean Data Network Organisation Register</dc:source>
	<dc:publisher rdf:datatype="http://www.w3.org/2001/XMLSchema#string">eMarine Information Infrastructure (eMII)</dc:publisher>
	<skos:exactMatch rdf:resource="http://seadatanet.maris2.nl/v_edmo/print.asp?n_code=4512"/>
	<skos:topConceptOf rdf:resource="http://vocab.aodn.org.au/def/organisation/1"/>
	<skos:inScheme rdf:resource="http://vocab.aodn.org.au/def/organisation/1"/>
</rdf:Description>

<rdf:Description rdf:about="http://vocab.aodn.org.au/def/organisation/entity/426">
	<rdf:type rdf:resource="http://www.w3.org/2000/01/rdf-schema#Resource"/>
	<rdf:type rdf:resource="http://www.w3.org/2004/02/skos/core#Concept"/>
	<dcterms:creator rdf:datatype="http://www.w3.org/2001/XMLSchema#string">Natalia Atkins</dcterms:creator>
	<dcterms:created rdf:datatype="http://www.w3.org/2001/XMLSchema#dateTime">2016-01-06T10:38:15Z</dcterms:created>
	<skos:prefLabel xml:lang="en">Cooperative Institute for Marine and Atmospheric Studies (CIMAS), University of Miami</skos:prefLabel>
	<skos:altLabel xml:lang="en">Cooperative Institute for Marine and Atmospheric Studies (CIMAS)</skos:altLabel>
	<skos:hiddenLabel xml:lang="en">CIMAS</skos:hiddenLabel>
	<skos:definition xml:lang="en">The Cooperative Institute for Marine and Atmospheric Studies (CIMAS) is a research institute of the University of Miami located in the Rosenstiel School of Marine and Atmospheric Science (RSMAS). CIMAS serves as a mechanism to bring together the research resources of the Partner Universities (including UM/RSMAS) with those of NOAA in order to develop a Center of Excellence that is relevant to understanding the Earth’s oceans and atmosphere within the context of NOAA’s mission. In 2010 CIMAS was restructured in light of its successful submission to a competitive award program to keep pace with changes in scientific and societal priorities as well as changes in both the NOAA and university regional context.</skos:definition>
	<dc:source rdf:datatype="http://www.w3.org/2001/XMLSchema#string">Australian Ocean Data Network Organisation Register</dc:source>
	<dc:publisher rdf:datatype="http://www.w3.org/2001/XMLSchema#string">eMarine Information Infrastructure (eMMI)</dc:publisher>
	<skos:exactMatch rdf:resource="http://seadatanet.maris2.nl/v_edmo/print.asp?n_code=4458"/>
	<skos:inScheme rdf:resource="http://vocab.aodn.org.au/def/organisation/1"/>
	<skos:broader rdf:resource="http://vocab.aodn.org.au/def/organisation/entity/322"/>
</rdf:Description>

<rdf:Description rdf:about="http://vocab.aodn.org.au/def/organisation/entity/427">
	<rdf:type rdf:resource="http://www.w3.org/2000/01/rdf-schema#Resource"/>
	<rdf:type rdf:resource="http://www.w3.org/2004/02/skos/core#Concept"/>
	<dcterms:creator rdf:datatype="http://www.w3.org/2001/XMLSchema#string">Natalia Atkins</dcterms:creator>
	<dcterms:created rdf:datatype="http://www.w3.org/2001/XMLSchema#dateTime">2016-01-06T10:38:15Z</dcterms:created>
	<skos:prefLabel xml:lang="en">Cooperative Institute for Meteorological Satellite Studies (CIMSS), University of Wisconsin-Madison</skos:prefLabel>
	<skos:altLabel xml:lang="en">Cooperative Institute for Meteorological Satellite Studies (CIMSS)</skos:altLabel>
	<skos:hiddenLabel xml:lang="en">CIMSSS</skos:hiddenLabel>
	<skos:definition xml:lang="en">CIMSS is a Cooperative Institute formed through a Memorandum of Understanding between the University of Wisconsin-Madison (UW-Madison), the National Oceanic and Atmospheric Administration (NOAA), and the National Aeronautics and Space Administration (NASA) in 1980. Directed by Dr. Steve Ackerman, CIMSS operates as an institute within the Space Science and Engineering Center (SSEC). CIMSS scientists conduct research using remote sensing systems for meteorological and surface-based applications.</skos:definition>
	<dc:source rdf:datatype="http://www.w3.org/2001/XMLSchema#string">Australian Ocean Data Network Organisation Register</dc:source>
	<dc:publisher rdf:datatype="http://www.w3.org/2001/XMLSchema#string">eMarine Information Infrastructure (eMMI)</dc:publisher>
	<skos:exactMatch rdf:resource="http://seadatanet.maris2.nl/v_edmo/print.asp?n_code=4459"/>
	<skos:inScheme rdf:resource="http://vocab.aodn.org.au/def/organisation/1"/>
	<skos:broader rdf:resource="http://vocab.aodn.org.au/def/organisation/entity/323"/>
</rdf:Description>

<rdf:Description rdf:about="http://vocab.aodn.org.au/def/organisation/entity/433">
	<rdf:type rdf:resource="http://www.w3.org/2000/01/rdf-schema#Resource"/>
	<rdf:type rdf:resource="http://www.w3.org/2004/02/skos/core#Concept"/>
	<dcterms:creator rdf:datatype="http://www.w3.org/2001/XMLSchema#string">Natalia Atkins</dcterms:creator>
	<dcterms:created rdf:datatype="http://www.w3.org/2001/XMLSchema#dateTime">2016-01-06T10:38:15Z</dcterms:created>
	<skos:prefLabel xml:lang="en">Department of Ecology, Evolution and Environmental Biology (E3B), Columbia University</skos:prefLabel>
	<skos:altLabel xml:lang="en">Department of Ecology, Evolution and Environmental Biology (E3B)</skos:altLabel>
	<skos:hiddenLabel xml:lang="en">E3B</skos:hiddenLabel>
	<skos:definition xml:lang="en">The Department of Ecology, Evolution, and Environmental Biology (E3B) at Columbia University was established in 2001. In creating E3B, the university recognized that the fields of ecology, evolutionary biology, and environmental biology constitute a distinct subdivision of the biological sciences with its own set of intellectual foci, theoretical foundations, scales of analysis, and methodologies.</skos:definition>
	<dc:source rdf:datatype="http://www.w3.org/2001/XMLSchema#string">Australian Ocean Data Network Organisation Register</dc:source>
	<dc:publisher rdf:datatype="http://www.w3.org/2001/XMLSchema#string">eMarine Information Infrastructure (eMMI)</dc:publisher>
	<skos:exactMatch rdf:resource="http://seadatanet.maris2.nl/v_edmo/print.asp?n_code=4465"/>
	<skos:inScheme rdf:resource="http://vocab.aodn.org.au/def/organisation/1"/>
	<skos:broader rdf:resource="http://vocab.aodn.org.au/def/organisation/entity/324"/>
</rdf:Description>

<rdf:Description rdf:about="http://vocab.aodn.org.au/def/organisation/entity/434">
	<rdf:type rdf:resource="http://www.w3.org/2000/01/rdf-schema#Resource"/>
	<rdf:type rdf:resource="http://www.w3.org/2004/02/skos/core#Concept"/>
	<dcterms:creator rdf:datatype="http://www.w3.org/2001/XMLSchema#string">Natalia Atkins</dcterms:creator>
	<dcterms:created rdf:datatype="http://www.w3.org/2001/XMLSchema#dateTime">2016-01-06T10:38:15Z</dcterms:created>
	<skos:prefLabel xml:lang="en">International Research Institute for Climate and Society (IRI)</skos:prefLabel>
	<skos:altLabel xml:lang="en"></skos:altLabel>
	<skos:hiddenLabel xml:lang="en">IRI</skos:hiddenLabel>
	<skos:definition xml:lang="en">The mission of the IRI is to enhance society’s capability to understand, anticipate and manage the impacts of climate in order to improve human welfare and the environment, especially in developing countries. The IRI conducts this mission through strategic and applied research, education, capacity building, and by providing forecasts and information products with an emphasis on practical and verifiable utility and partnership.</skos:definition>
	<dc:source rdf:datatype="http://www.w3.org/2001/XMLSchema#string">Australian Ocean Data Network Organisation Register</dc:source>
	<dc:publisher rdf:datatype="http://www.w3.org/2001/XMLSchema#string">eMarine Information Infrastructure (eMMI)</dc:publisher>
	<skos:exactMatch rdf:resource="http://seadatanet.maris2.nl/v_edmo/print.asp?n_code=4466"/>
	<skos:inScheme rdf:resource="http://vocab.aodn.org.au/def/organisation/1"/>
	<skos:broader rdf:resource="http://vocab.aodn.org.au/def/organisation/entity/324"/>
</rdf:Description>

<rdf:Description rdf:about="http://vocab.aodn.org.au/def/organisation/entity/428">
	<rdf:type rdf:resource="http://www.w3.org/2000/01/rdf-schema#Resource"/>
	<rdf:type rdf:resource="http://www.w3.org/2004/02/skos/core#Concept"/>
	<dcterms:creator rdf:datatype="http://www.w3.org/2001/XMLSchema#string">Natalia Atkins</dcterms:creator>
	<dcterms:created rdf:datatype="http://www.w3.org/2001/XMLSchema#dateTime">2016-01-06T10:38:15Z</dcterms:created>
	<skos:prefLabel xml:lang="en">School of Aquatic and Fishery Sciences (SAFS), University of Washington (UW)</skos:prefLabel>
	<skos:altLabel xml:lang="en">School of Aquatic and Fishery Sciences (SAFS)</skos:altLabel>
	<skos:hiddenLabel xml:lang="en">SAFS</skos:hiddenLabel>
	<skos:definition xml:lang="en">Founded in 1919, the School of Aquatic and Fishery Sciences (SAFS) is dedicated to sustaining healthy marine and freshwater environments. Our faculty conduct innovative research from the organism to the ecosystem scale and are recognized leaders in aquatic biology, sustainable fisheries management, aquatic resource conservation, and resource management. We study natural systems and species and present solutions to foster the sustainable use of aquatic resources.</skos:definition>
	<dc:source rdf:datatype="http://www.w3.org/2001/XMLSchema#string">Australian Ocean Data Network Organisation Register</dc:source>
	<dc:publisher rdf:datatype="http://www.w3.org/2001/XMLSchema#string">eMarine Information Infrastructure (eMMI)</dc:publisher>
	<skos:exactMatch rdf:resource="http://seadatanet.maris2.nl/v_edmo/print.asp?n_code=4460"/>
	<skos:inScheme rdf:resource="http://vocab.aodn.org.au/def/organisation/1"/>
	<skos:broader rdf:resource="http://vocab.aodn.org.au/def/organisation/entity/325"/>
</rdf:Description>

<rdf:Description rdf:about="http://vocab.aodn.org.au/def/organisation/entity/429">
	<rdf:type rdf:resource="http://www.w3.org/2000/01/rdf-schema#Resource"/>
	<rdf:type rdf:resource="http://www.w3.org/2004/02/skos/core#Concept"/>
	<dcterms:creator rdf:datatype="http://www.w3.org/2001/XMLSchema#string">Natalia Atkins</dcterms:creator>
	<dcterms:created rdf:datatype="http://www.w3.org/2001/XMLSchema#dateTime">2016-01-06T10:38:15Z</dcterms:created>
	<skos:prefLabel xml:lang="en">School of Environmental and Forest Sciences (SEFS), University of Washington (UW)</skos:prefLabel>
	<skos:altLabel xml:lang="en">School of Environmental and Forest Sciences (SEFS)</skos:altLabel>
	<skos:hiddenLabel xml:lang="en">SEFS</skos:hiddenLabel>
	<skos:definition xml:lang="en">The School of Environmental and Forest Sciences is dedicated to generating and disseminating knowledge for the stewardship of natural and managed environments and the sustainable use of their products and services through teaching, research and outreach.</skos:definition>
	<dc:source rdf:datatype="http://www.w3.org/2001/XMLSchema#string">Australian Ocean Data Network Organisation Register</dc:source>
	<dc:publisher rdf:datatype="http://www.w3.org/2001/XMLSchema#string">eMarine Information Infrastructure (eMMI)</dc:publisher>
	<skos:exactMatch rdf:resource="http://seadatanet.maris2.nl/v_edmo/print.asp?n_code=4461"/>
	<skos:inScheme rdf:resource="http://vocab.aodn.org.au/def/organisation/1"/>
	<skos:broader rdf:resource="http://vocab.aodn.org.au/def/organisation/entity/325"/>
</rdf:Description>

<rdf:Description rdf:about="http://vocab.aodn.org.au/def/organisation/entity/430">
	<rdf:type rdf:resource="http://www.w3.org/2000/01/rdf-schema#Resource"/>
	<rdf:type rdf:resource="http://www.w3.org/2004/02/skos/core#Concept"/>
	<dcterms:creator rdf:datatype="http://www.w3.org/2001/XMLSchema#string">Natalia Atkins</dcterms:creator>
	<dcterms:created rdf:datatype="http://www.w3.org/2001/XMLSchema#dateTime">2016-01-06T10:38:15Z</dcterms:created>
	<skos:prefLabel xml:lang="en">WM School of Marine Science at Virginia Institute of Marine Science (VIMS)</skos:prefLabel>
	<skos:altLabel xml:lang="en">School of Marine Science</skos:altLabel>
	<skos:hiddenLabel xml:lang="en"></skos:hiddenLabel>
	<skos:definition xml:lang="en">The School of Marine Science (SMS) at VIMS is the graduate school in marine science for the College of William and Mary. Chartered in 1940, VIMS is currently among the largest marine research and education centers in the United States.</skos:definition>
	<dc:source rdf:datatype="http://www.w3.org/2001/XMLSchema#string">Australian Ocean Data Network Organisation Register</dc:source>
	<dc:publisher rdf:datatype="http://www.w3.org/2001/XMLSchema#string">eMarine Information Infrastructure (eMMI)</dc:publisher>
	<skos:exactMatch rdf:resource="http://seadatanet.maris2.nl/v_edmo/print.asp?n_code=4462"/>
	<skos:inScheme rdf:resource="http://vocab.aodn.org.au/def/organisation/1"/>
	<skos:broader rdf:resource="http://vocab.aodn.org.au/def/organisation/entity/326"/>
</rdf:Description>

<rdf:Description rdf:about="http://vocab.aodn.org.au/def/organisation/entity/435">
	<rdf:type rdf:resource="http://www.w3.org/2000/01/rdf-schema#Resource"/>
	<rdf:type rdf:resource="http://www.w3.org/2004/02/skos/core#Concept"/>
	<dcterms:creator rdf:datatype="http://www.w3.org/2001/XMLSchema#string">Natalia Atkins</dcterms:creator>
	<dcterms:created rdf:datatype="http://www.w3.org/2001/XMLSchema#dateTime">2016-01-06T10:38:15Z</dcterms:created>
	<skos:prefLabel xml:lang="en">Department of Ecology and Evolutionary Biology (EEB), University of California, Los Angeles (UCLA)</skos:prefLabel>
	<skos:altLabel xml:lang="en">Department of Ecology and Evolutionary Biology (EEB)</skos:altLabel>
	<skos:hiddenLabel xml:lang="en">EEB</skos:hiddenLabel>
	<skos:definition xml:lang="en">Welcome to the Department of Ecology and Evolutionary Biology at UCLA, home of the Biology Major. Our mission is to provide new knowledge of the ecological and evolutionary processes that produce and sustain life on Earth and to educate the next generation of scholars, professionals, and citizens for the biological, environmental and biotechnological challenges of the future.</skos:definition>
	<dc:source rdf:datatype="http://www.w3.org/2001/XMLSchema#string">Australian Ocean Data Network Organisation Register</dc:source>
	<dc:publisher rdf:datatype="http://www.w3.org/2001/XMLSchema#string">eMarine Information Infrastructure (eMMI)</dc:publisher>
	<skos:exactMatch rdf:resource="http://seadatanet.maris2.nl/v_edmo/print.asp?n_code=4467"/>
	<skos:inScheme rdf:resource="http://vocab.aodn.org.au/def/organisation/1"/>
	<skos:broader rdf:resource="http://vocab.aodn.org.au/def/organisation/entity/328"/>
</rdf:Description>

<rdf:Description rdf:about="http://vocab.aodn.org.au/def/organisation/entity/439">
	<rdf:type rdf:resource="http://www.w3.org/2000/01/rdf-schema#Resource"/>
	<rdf:type rdf:resource="http://www.w3.org/2004/02/skos/core#Concept"/>
	<dcterms:creator rdf:datatype="http://www.w3.org/2001/XMLSchema#string">Natalia Atkins</dcterms:creator>
	<dcterms:created rdf:datatype="http://www.w3.org/2001/XMLSchema#dateTime">2016-01-06T10:38:15Z</dcterms:created>
	<skos:prefLabel xml:lang="en">Romberg Tiburon Center for Environmental Studies (RTC), San Francisco State University (SFSU)</skos:prefLabel>
	<skos:altLabel xml:lang="en">Romberg Tiburon Center for Environmental Studies (RTC)</skos:altLabel>
	<skos:hiddenLabel xml:lang="en">RTC</skos:hiddenLabel>
	<skos:definition xml:lang="en">The Center's location is an ideal setting for our scientists and students to conduct their research -- much of which focuses on understanding the natural forces at work in the San Francisco Bay and its surrounding wetland environments. RTC research scientists are also studying natural phenomena in the open ocean; along California's coastline and in remote locations such as the Ross Sea (Antarctica) and the Equatorial Pacific.</skos:definition>
	<dc:source rdf:datatype="http://www.w3.org/2001/XMLSchema#string">Australian Ocean Data Network Organisation Register</dc:source>
	<dc:publisher rdf:datatype="http://www.w3.org/2001/XMLSchema#string">eMarine Information Infrastructure (eMMI)</dc:publisher>
	<skos:exactMatch rdf:resource="http://seadatanet.maris2.nl/v_edmo/print.asp?n_code=4471"/>
	<skos:inScheme rdf:resource="http://vocab.aodn.org.au/def/organisation/1"/>
	<skos:broader rdf:resource="http://vocab.aodn.org.au/def/organisation/entity/329"/>
</rdf:Description>

<rdf:Description rdf:about="http://vocab.aodn.org.au/def/organisation/entity/441">
	<rdf:type rdf:resource="http://www.w3.org/2000/01/rdf-schema#Resource"/>
	<rdf:type rdf:resource="http://www.w3.org/2004/02/skos/core#Concept"/>
	<dcterms:creator rdf:datatype="http://www.w3.org/2001/XMLSchema#string">Natalia Atkins</dcterms:creator>
	<dcterms:created rdf:datatype="http://www.w3.org/2001/XMLSchema#dateTime">2016-01-06T10:38:15Z</dcterms:created>
	<skos:prefLabel xml:lang="en">Department of Biological Sciences, University of Illinois at Chicago (UIC)</skos:prefLabel>
	<skos:altLabel xml:lang="en">Department of Biological Sciences</skos:altLabel>
	<skos:hiddenLabel xml:lang="en"></skos:hiddenLabel>
	<skos:definition xml:lang="en">We offer undergraduate and graduate training opportunities in all major areas of biology, including molecular, cellular, and developmental biology, neuroscience, ecology, and evolution. We are currently composed of 32 tenure-track faculty, 6 non-tenure track faculty, 23 staff, 110 graduate students, and together we teach and mentor 2,000 biology majors, and 70 neuroscience majors.</skos:definition>
	<dc:source rdf:datatype="http://www.w3.org/2001/XMLSchema#string">Australian Ocean Data Network Organisation Register</dc:source>
	<dc:publisher rdf:datatype="http://www.w3.org/2001/XMLSchema#string">eMarine Information Infrastructure (eMMI)</dc:publisher>
	<skos:exactMatch rdf:resource="http://seadatanet.maris2.nl/v_edmo/print.asp?n_code=4473"/>
	<skos:inScheme rdf:resource="http://vocab.aodn.org.au/def/organisation/1"/>
	<skos:broader rdf:resource="http://vocab.aodn.org.au/def/organisation/entity/330"/>
</rdf:Description>

<rdf:Description rdf:about="http://vocab.aodn.org.au/def/organisation/entity/442">
	<rdf:type rdf:resource="http://www.w3.org/2000/01/rdf-schema#Resource"/>
	<rdf:type rdf:resource="http://www.w3.org/2004/02/skos/core#Concept"/>
	<dcterms:creator rdf:datatype="http://www.w3.org/2001/XMLSchema#string">Natalia Atkins</dcterms:creator>
	<dcterms:created rdf:datatype="http://www.w3.org/2001/XMLSchema#dateTime">2016-01-06T10:38:15Z</dcterms:created>
	<skos:prefLabel xml:lang="en">Halmos College of Natural Sciences and Oceanography, Nova Southeastern University (NSU)</skos:prefLabel>
	<skos:altLabel xml:lang="en">Halmos College of Natural Sciences and Oceanography</skos:altLabel>
	<skos:hiddenLabel xml:lang="en"></skos:hiddenLabel>
	<skos:definition xml:lang="en">Nova Southeastern University’s scientists are engaged in exciting interdisciplinary research projects to make discoveries and produce new knowledge in healthcare, biotechnology, life sciences, environment and social sciences. NSU faculty are using more than $76 million in externally provided funding to work on projects that advance the university’s mission of research, academic excellence and public service. They are working on more than 205 basic, applied and clinical research projects to improve patient care, make new drug discoveries, reduce mental health disorders, and examine the forces that impact our oceans. In the fall of 2012 NSU opened the Center for Excellence for Coral Reef Ecosystems Science Research Facility at its Oceanographic Center. Funded by the National Institute of Standards and Technology, America’s largest coral reef research center will be solely dedicated to coral reef ecosystem research.</skos:definition>
	<dc:source rdf:datatype="http://www.w3.org/2001/XMLSchema#string">Australian Ocean Data Network Organisation Register</dc:source>
	<dc:publisher rdf:datatype="http://www.w3.org/2001/XMLSchema#string">eMarine Information Infrastructure (eMMI)</dc:publisher>
	<skos:exactMatch rdf:resource="http://seadatanet.maris2.nl/v_edmo/print.asp?n_code=4474"/>
	<skos:inScheme rdf:resource="http://vocab.aodn.org.au/def/organisation/1"/>
	<skos:broader rdf:resource="http://vocab.aodn.org.au/def/organisation/entity/331"/>
</rdf:Description>

<rdf:Description rdf:about="http://vocab.aodn.org.au/def/organisation/entity/421">
	<rdf:type rdf:resource="http://www.w3.org/2000/01/rdf-schema#Resource"/>
	<rdf:type rdf:resource="http://www.w3.org/2004/02/skos/core#Concept"/>
	<dcterms:modified rdf:datatype="http://www.w3.org/2001/XMLSchema#dateTime">2016-01-05T01:51:58Z</dcterms:modified>
	<dcterms:creator rdf:datatype="http://www.w3.org/2001/XMLSchema#string">Natalia Atkins</dcterms:creator>
	<dcterms:created rdf:datatype="http://www.w3.org/2001/XMLSchema#dateTime">2016-01-04T10:38:15Z</dcterms:created>
	<dcterms:contributor rdf:datatype="http://www.w3.org/2001/XMLSchema#string">eMII_Atkins.Natalia</dcterms:contributor>
	<skos:prefLabel xml:lang="en">Department of Forest Resources Management, The University of British Columbia (UBC)</skos:prefLabel>
	<skos:altLabel xml:lang="en">Department of Forest Resources Management</skos:altLabel>
	<skos:hiddenLabel xml:lang="en"></skos:hiddenLabel>
	<skos:definition xml:lang="en"></skos:definition>
	<skos:definition xml:lang="en">The mission of the Forest Resources Management Department is to provide an outstanding education in forestry and conservation that is integrated, international, and experiential. We undertake significant, innovative research, and promote an interdisciplinary environment that attracts world-class scholars and graduate students. Research areas also include Hydrology. The Faculty of Forestry is host to the Watershed Hydrology Laboratory.</skos:definition>
	<dc:source rdf:datatype="http://www.w3.org/2001/XMLSchema#string">Australian Ocean Data Network Organisation Register</dc:source>
	<dc:publisher rdf:datatype="http://www.w3.org/2001/XMLSchema#string">eMarine Information Infrastructure (eMII)</dc:publisher>
	<skos:exactMatch rdf:resource="http://seadatanet.maris2.nl/v_edmo/print.asp?n_code=4452"/>
	<skos:inScheme rdf:resource="http://vocab.aodn.org.au/def/organisation/1"/>
	<skos:broader rdf:resource="http://vocab.aodn.org.au/def/organisation/entity/420"/>
</rdf:Description>

<rdf:Description rdf:about="http://seadatanet.maris2.nl/v_edmo/print.asp?n_code=4452">
	<rdf:type rdf:resource="http://www.w3.org/2000/01/rdf-schema#Resource"/>
</rdf:Description>

<rdf:Description rdf:about="http://vocab.aodn.org.au/def/organisation/entity/422">
	<rdf:type rdf:resource="http://www.w3.org/2000/01/rdf-schema#Resource"/>
	<rdf:type rdf:resource="http://www.w3.org/2004/02/skos/core#Concept"/>
	<dcterms:creator rdf:datatype="http://www.w3.org/2001/XMLSchema#string">Natalia Atkins</dcterms:creator>
	<dcterms:created rdf:datatype="http://www.w3.org/2001/XMLSchema#dateTime">2016-01-04T10:38:15Z</dcterms:created>
	<skos:prefLabel xml:lang="en">Department of Mathematics, The University of British Columbia (UBC)</skos:prefLabel>
	<skos:altLabel xml:lang="en">Department of Mathematics</skos:altLabel>
	<skos:hiddenLabel xml:lang="en"></skos:hiddenLabel>
	<skos:definition xml:lang="en"></skos:definition>
	<dc:source rdf:datatype="http://www.w3.org/2001/XMLSchema#string">Australian Ocean Data Network Organisation Register</dc:source>
	<dc:publisher rdf:datatype="http://www.w3.org/2001/XMLSchema#string">eMarine Information Infrastructure (eMII)</dc:publisher>
	<skos:exactMatch rdf:resource="http://seadatanet.maris2.nl/v_edmo/print.asp?n_code=4451"/>
	<skos:inScheme rdf:resource="http://vocab.aodn.org.au/def/organisation/1"/>
	<skos:broader rdf:resource="http://vocab.aodn.org.au/def/organisation/entity/420"/>
</rdf:Description>

<rdf:Description rdf:about="http://seadatanet.maris2.nl/v_edmo/print.asp?n_code=4451">
	<rdf:type rdf:resource="http://www.w3.org/2000/01/rdf-schema#Resource"/>
</rdf:Description>

<rdf:Description rdf:about="http://vocab.aodn.org.au/def/organisation/entity/362">
	<rdf:type rdf:resource="http://www.w3.org/2000/01/rdf-schema#Resource"/>
	<rdf:type rdf:resource="http://www.w3.org/2004/02/skos/core#Concept"/>
	<dcterms:creator rdf:datatype="http://www.w3.org/2001/XMLSchema#string">Natalia Atkins</dcterms:creator>
	<dcterms:created rdf:datatype="http://www.w3.org/2001/XMLSchema#dateTime">2016-01-04T10:38:15Z</dcterms:created>
	<skos:prefLabel xml:lang="en">Department of Economics and Fisheries Centre, The University of British Columbia (UBC)</skos:prefLabel>
	<skos:altLabel xml:lang="en">Department of Economics and Fisheries Centre</skos:altLabel>
	<skos:hiddenLabel xml:lang="en"></skos:hiddenLabel>
	<skos:definition xml:lang="en"></skos:definition>
	<dc:source rdf:datatype="http://www.w3.org/2001/XMLSchema#string">Australian Ocean Data Network Organisation Register</dc:source>
	<dc:publisher rdf:datatype="http://www.w3.org/2001/XMLSchema#string">eMarine Information Infrastructure (eMII)</dc:publisher>
	<skos:inScheme rdf:resource="http://vocab.aodn.org.au/def/organisation/1"/>
	<skos:broader rdf:resource="http://vocab.aodn.org.au/def/organisation/entity/420"/>
	<skos:scopeNote xml:lang="en">Organisation no longer exists</skos:scopeNote>
</rdf:Description>

<rdf:Description rdf:about="http://vocab.aodn.org.au/def/organisation/entity/423">
	<rdf:type rdf:resource="http://www.w3.org/2000/01/rdf-schema#Resource"/>
	<rdf:type rdf:resource="http://www.w3.org/2004/02/skos/core#Concept"/>
	<dcterms:modified rdf:datatype="http://www.w3.org/2001/XMLSchema#dateTime">2016-01-05T01:53:46Z</dcterms:modified>
	<dcterms:creator rdf:datatype="http://www.w3.org/2001/XMLSchema#string">Natalia Atkins</dcterms:creator>
	<dcterms:created rdf:datatype="http://www.w3.org/2001/XMLSchema#dateTime">2016-01-04T10:38:15Z</dcterms:created>
	<dcterms:contributor rdf:datatype="http://www.w3.org/2001/XMLSchema#string">eMII_Atkins.Natalia</dcterms:contributor>
	<skos:prefLabel xml:lang="en">Project Seahorse</skos:prefLabel>
	<skos:altLabel xml:lang="en"></skos:altLabel>
	<skos:hiddenLabel xml:lang="en"></skos:hiddenLabel>
	<skos:definition xml:lang="en"></skos:definition>
	<skos:definition xml:lang="en">Project Seahorse is a marine conservation group dedicated to securing a world where marine ecosystems are healthy and well-managed. Project Seahorse is a small team of scientists and conservationists with offices at the University of British Columbia in Vancouver, Canada and the Zoological Society of London in the United Kingdom. They work all over the world, with research and conservation projects in Asia, Europe, Africa, Australia, and the Americas. The Canadian office is located at the Institute for the Oceans and Fisheries of the University of British Columbia, Faculty of Science. The Institute, previously known as the Fisheries Centre (created in the 1950s as the Institute of Fisheries) is located in the University's Aquatic Ecosystem Research Laboratory. The Project started its activities in 1994.</skos:definition>
	<dc:source rdf:datatype="http://www.w3.org/2001/XMLSchema#string">Australian Ocean Data Network Organisation Register</dc:source>
	<dc:publisher rdf:datatype="http://www.w3.org/2001/XMLSchema#string">eMarine Information Infrastructure (eMII)</dc:publisher>
	<skos:exactMatch rdf:resource="http://seadatanet.maris2.nl/v_edmo/print.asp?n_code=4453"/>
	<skos:inScheme rdf:resource="http://vocab.aodn.org.au/def/organisation/1"/>
	<skos:broader rdf:resource="http://vocab.aodn.org.au/def/organisation/entity/420"/>
</rdf:Description>

<rdf:Description rdf:about="http://seadatanet.maris2.nl/v_edmo/print.asp?n_code=4453">
	<rdf:type rdf:resource="http://www.w3.org/2000/01/rdf-schema#Resource"/>
</rdf:Description>

<rdf:Description rdf:about="http://vocab.aodn.org.au/def/organisation/entity/425">
	<rdf:type rdf:resource="http://www.w3.org/2000/01/rdf-schema#Resource"/>
	<rdf:type rdf:resource="http://www.w3.org/2004/02/skos/core#Concept"/>
	<dcterms:creator rdf:datatype="http://www.w3.org/2001/XMLSchema#string">Natalia Atkins</dcterms:creator>
	<dcterms:created rdf:datatype="http://www.w3.org/2001/XMLSchema#dateTime">2016-01-04T10:38:15Z</dcterms:created>
	<skos:prefLabel xml:lang="en">Department of Economics, Brock University</skos:prefLabel>
	<skos:altLabel xml:lang="en">Department of Economics</skos:altLabel>
	<skos:hiddenLabel xml:lang="en"></skos:hiddenLabel>
	<skos:definition xml:lang="en"></skos:definition>
	<dc:source rdf:datatype="http://www.w3.org/2001/XMLSchema#string">Australian Ocean Data Network Organisation Register</dc:source>
	<dc:publisher rdf:datatype="http://www.w3.org/2001/XMLSchema#string">eMarine Information Infrastructure (eMII)</dc:publisher>
	<skos:exactMatch rdf:resource="http://seadatanet.maris2.nl/v_edmo/print.asp?n_code=4454"/>
	<skos:inScheme rdf:resource="http://vocab.aodn.org.au/def/organisation/1"/>
	<skos:broader rdf:resource="http://vocab.aodn.org.au/def/organisation/entity/424"/>
</rdf:Description>

<rdf:Description rdf:about="http://seadatanet.maris2.nl/v_edmo/print.asp?n_code=4454">
	<rdf:type rdf:resource="http://www.w3.org/2000/01/rdf-schema#Resource"/>
</rdf:Description>

<rdf:Description rdf:about="http://seadatanet.maris2.nl/v_edmo/print.asp?n_code=4458">
	<rdf:type rdf:resource="http://www.w3.org/2000/01/rdf-schema#Resource"/>
</rdf:Description>

<rdf:Description rdf:about="http://seadatanet.maris2.nl/v_edmo/print.asp?n_code=4459">
	<rdf:type rdf:resource="http://www.w3.org/2000/01/rdf-schema#Resource"/>
</rdf:Description>

<rdf:Description rdf:about="http://seadatanet.maris2.nl/v_edmo/print.asp?n_code=4460">
	<rdf:type rdf:resource="http://www.w3.org/2000/01/rdf-schema#Resource"/>
</rdf:Description>

<rdf:Description rdf:about="http://seadatanet.maris2.nl/v_edmo/print.asp?n_code=4461">
	<rdf:type rdf:resource="http://www.w3.org/2000/01/rdf-schema#Resource"/>
</rdf:Description>

<rdf:Description rdf:about="http://seadatanet.maris2.nl/v_edmo/print.asp?n_code=4462">
	<rdf:type rdf:resource="http://www.w3.org/2000/01/rdf-schema#Resource"/>
</rdf:Description>

<rdf:Description rdf:about="http://vocab.aodn.org.au/def/organisation/entity/432">
	<rdf:type rdf:resource="http://www.w3.org/2000/01/rdf-schema#Resource"/>
	<rdf:type rdf:resource="http://www.w3.org/2004/02/skos/core#Concept"/>
	<dcterms:creator rdf:datatype="http://www.w3.org/2001/XMLSchema#string">Natalia Atkins</dcterms:creator>
	<dcterms:created rdf:datatype="http://www.w3.org/2001/XMLSchema#dateTime">2016-01-06T10:38:15Z</dcterms:created>
	<skos:prefLabel xml:lang="en">Department of Economics, Iowa State University</skos:prefLabel>
	<skos:altLabel xml:lang="en">Department of Economics</skos:altLabel>
	<skos:hiddenLabel xml:lang="en"></skos:hiddenLabel>
	<skos:definition xml:lang="en">The Department of Economics is one of the oldest and most recognized units on the Iowa State University campus. It has a long and interesting history that is described further in some documents accessible from the panel on the right. The Department of Economics is currently jointly administered by the College of Agriculture and Life Sciences and by the College of Liberal Arts and Sciences.</skos:definition>
	<dc:source rdf:datatype="http://www.w3.org/2001/XMLSchema#string">Australian Ocean Data Network Organisation Register</dc:source>
	<dc:publisher rdf:datatype="http://www.w3.org/2001/XMLSchema#string">eMarine Information Infrastructure (eMII)</dc:publisher>
	<skos:exactMatch rdf:resource="http://seadatanet.maris2.nl/v_edmo/print.asp?n_code=4464"/>
	<skos:inScheme rdf:resource="http://vocab.aodn.org.au/def/organisation/1"/>
	<skos:broader rdf:resource="http://vocab.aodn.org.au/def/organisation/entity/431"/>
</rdf:Description>

<rdf:Description rdf:about="http://seadatanet.maris2.nl/v_edmo/print.asp?n_code=4463">
	<rdf:type rdf:resource="http://www.w3.org/2000/01/rdf-schema#Resource"/>
</rdf:Description>

<rdf:Description rdf:about="http://seadatanet.maris2.nl/v_edmo/print.asp?n_code=4464">
	<rdf:type rdf:resource="http://www.w3.org/2000/01/rdf-schema#Resource"/>
</rdf:Description>

<rdf:Description rdf:about="http://seadatanet.maris2.nl/v_edmo/print.asp?n_code=4465">
	<rdf:type rdf:resource="http://www.w3.org/2000/01/rdf-schema#Resource"/>
</rdf:Description>

<rdf:Description rdf:about="http://seadatanet.maris2.nl/v_edmo/print.asp?n_code=4466">
	<rdf:type rdf:resource="http://www.w3.org/2000/01/rdf-schema#Resource"/>
</rdf:Description>

<rdf:Description rdf:about="http://seadatanet.maris2.nl/v_edmo/print.asp?n_code=4467">
	<rdf:type rdf:resource="http://www.w3.org/2000/01/rdf-schema#Resource"/>
</rdf:Description>

<rdf:Description rdf:about="http://vocab.aodn.org.au/def/organisation/entity/437">
	<rdf:type rdf:resource="http://www.w3.org/2000/01/rdf-schema#Resource"/>
	<rdf:type rdf:resource="http://www.w3.org/2004/02/skos/core#Concept"/>
	<dcterms:creator rdf:datatype="http://www.w3.org/2001/XMLSchema#string">Natalia Atkins</dcterms:creator>
	<dcterms:created rdf:datatype="http://www.w3.org/2001/XMLSchema#dateTime">2016-01-06T10:38:15Z</dcterms:created>
	<skos:prefLabel xml:lang="en">Department of Biological Sciences, Florida International University (FIU)</skos:prefLabel>
	<skos:altLabel xml:lang="en">Department of Biological Sciences</skos:altLabel>
	<skos:hiddenLabel xml:lang="en"></skos:hiddenLabel>
	<skos:definition xml:lang="en">The research interests of our faculty span many levels of biological organization from molecules to ecosystems, and include both field- and laboratory-based studies in marine, terrestrial and freshwater environments. Faculty in the department address basic biological questions about how organisms work, how they develop, how they interact with other organisms and their environments, and how they have evolved over time. Active areas of research include cell and molecular biology, ecology, climate change, functional morphology, genetics, conservation biology and biodiversity, neurobiology and behavior, evolutionary biology and population genetics, phylogenetics and bioinformatics, physiology, virology, microbiology, and paleobiology. Many of our faculty specialize in tropical systems, including tropical ecosystems and tropical diseases.</skos:definition>
	<dc:source rdf:datatype="http://www.w3.org/2001/XMLSchema#string">Australian Ocean Data Network Organisation Register</dc:source>
	<dc:publisher rdf:datatype="http://www.w3.org/2001/XMLSchema#string">eMarine Information Infrastructure (eMII)</dc:publisher>
	<skos:exactMatch rdf:resource="http://seadatanet.maris2.nl/v_edmo/print.asp?n_code=4469"/>
	<skos:inScheme rdf:resource="http://vocab.aodn.org.au/def/organisation/1"/>
	<skos:broader rdf:resource="http://vocab.aodn.org.au/def/organisation/entity/436"/>
</rdf:Description>

<rdf:Description rdf:about="http://vocab.aodn.org.au/def/organisation/entity/438">
	<rdf:type rdf:resource="http://www.w3.org/2000/01/rdf-schema#Resource"/>
	<rdf:type rdf:resource="http://www.w3.org/2004/02/skos/core#Concept"/>
	<dcterms:creator rdf:datatype="http://www.w3.org/2001/XMLSchema#string">Natalia Atkins</dcterms:creator>
	<dcterms:created rdf:datatype="http://www.w3.org/2001/XMLSchema#dateTime">2016-01-06T10:38:15Z</dcterms:created>
	<skos:prefLabel xml:lang="en">School of Environment, Arts and Society (SEAS), Florida International University (FIU)</skos:prefLabel>
	<skos:altLabel xml:lang="en">School of Environment, Arts and Society (SEAS)</skos:altLabel>
	<skos:hiddenLabel xml:lang="en">SEAS</skos:hiddenLabel>
	<skos:definition xml:lang="en">Faculty in SEAS are invested in understanding how factors from both systems affect the environment, because long-term sustainability can only be achieved if human societies understand their impact in and responsibility toward these natural systems. The academic core of SEAS consists of the Departments of Biological Sciences, Earth and Environment, and English. Through research, education, and an interdisciplinary exchange of ideas, SEAS strives to bring about positive, tangible changes on local, national and international levels.</skos:definition>
	<dc:source rdf:datatype="http://www.w3.org/2001/XMLSchema#string">Australian Ocean Data Network Organisation Register</dc:source>
	<dc:publisher rdf:datatype="http://www.w3.org/2001/XMLSchema#string">eMarine Information Infrastructure (eMII)</dc:publisher>
	<skos:exactMatch rdf:resource="http://seadatanet.maris2.nl/v_edmo/print.asp?n_code=4470"/>
	<skos:inScheme rdf:resource="http://vocab.aodn.org.au/def/organisation/1"/>
	<skos:broader rdf:resource="http://vocab.aodn.org.au/def/organisation/entity/436"/>
</rdf:Description>

<rdf:Description rdf:about="http://seadatanet.maris2.nl/v_edmo/print.asp?n_code=4468">
	<rdf:type rdf:resource="http://www.w3.org/2000/01/rdf-schema#Resource"/>
</rdf:Description>

<rdf:Description rdf:about="http://seadatanet.maris2.nl/v_edmo/print.asp?n_code=4469">
	<rdf:type rdf:resource="http://www.w3.org/2000/01/rdf-schema#Resource"/>
</rdf:Description>

<rdf:Description rdf:about="http://seadatanet.maris2.nl/v_edmo/print.asp?n_code=4470">
	<rdf:type rdf:resource="http://www.w3.org/2000/01/rdf-schema#Resource"/>
</rdf:Description>

<rdf:Description rdf:about="http://seadatanet.maris2.nl/v_edmo/print.asp?n_code=4471">
	<rdf:type rdf:resource="http://www.w3.org/2000/01/rdf-schema#Resource"/>
</rdf:Description>

<rdf:Description rdf:about="http://seadatanet.maris2.nl/v_edmo/print.asp?n_code=4472">
	<rdf:type rdf:resource="http://www.w3.org/2000/01/rdf-schema#Resource"/>
</rdf:Description>

<rdf:Description rdf:about="http://seadatanet.maris2.nl/v_edmo/print.asp?n_code=4473">
	<rdf:type rdf:resource="http://www.w3.org/2000/01/rdf-schema#Resource"/>
</rdf:Description>

<rdf:Description rdf:about="http://seadatanet.maris2.nl/v_edmo/print.asp?n_code=4474">
	<rdf:type rdf:resource="http://www.w3.org/2000/01/rdf-schema#Resource"/>
</rdf:Description>

<rdf:Description rdf:about="http://seadatanet.maris2.nl/v_edmo/print.asp?n_code=4475">
	<rdf:type rdf:resource="http://www.w3.org/2000/01/rdf-schema#Resource"/>
</rdf:Description>

<rdf:Description rdf:about="http://seadatanet.maris2.nl/v_edmo/print.asp?n_code=4449">
	<rdf:type rdf:resource="http://www.w3.org/2000/01/rdf-schema#Resource"/>
</rdf:Description>

<rdf:Description rdf:about="http://vocab.aodn.org.au/def/organisation/entity/365">
	<rdf:type rdf:resource="http://www.w3.org/2000/01/rdf-schema#Resource"/>
	<rdf:type rdf:resource="http://www.w3.org/2004/02/skos/core#Concept"/>
	<dcterms:creator rdf:datatype="http://www.w3.org/2001/XMLSchema#string">Natalia Atkins</dcterms:creator>
	<dcterms:created rdf:datatype="http://www.w3.org/2001/XMLSchema#dateTime">2016-01-07T10:38:15Z</dcterms:created>
	<skos:prefLabel xml:lang="en">Department of Economics, University of Iceland</skos:prefLabel>
	<skos:altLabel xml:lang="en">Department of Economics</skos:altLabel>
	<skos:hiddenLabel xml:lang="en"></skos:hiddenLabel>
	<skos:definition xml:lang="en"></skos:definition>
	<dc:source rdf:datatype="http://www.w3.org/2001/XMLSchema#string">Australian Ocean Data Network Organisation Register</dc:source>
	<dc:publisher rdf:datatype="http://www.w3.org/2001/XMLSchema#string">eMarine Information Infrastructure (eMII)</dc:publisher>
	<skos:inScheme rdf:resource="http://vocab.aodn.org.au/def/organisation/1"/>
	<skos:broader rdf:resource="http://vocab.aodn.org.au/def/organisation/entity/445"/>
	<skos:scopeNote xml:lang="en">Organisation no longer exists</skos:scopeNote>
</rdf:Description>

<rdf:Description rdf:about="http://seadatanet.maris2.nl/v_edmo/print.asp?n_code=4447">
	<rdf:type rdf:resource="http://www.w3.org/2000/01/rdf-schema#Resource"/>
</rdf:Description>

<rdf:Description rdf:about="http://seadatanet.maris2.nl/v_edmo/print.asp?n_code=4448">
	<rdf:type rdf:resource="http://www.w3.org/2000/01/rdf-schema#Resource"/>
</rdf:Description>

<rdf:Description rdf:about="http://seadatanet.maris2.nl/v_edmo/print.asp?n_code=4457">
	<rdf:type rdf:resource="http://www.w3.org/2000/01/rdf-schema#Resource"/>
</rdf:Description>

<rdf:Description rdf:about="http://vocab.aodn.org.au/def/organisation/entity/448">
	<rdf:type rdf:resource="http://www.w3.org/2000/01/rdf-schema#Resource"/>
	<rdf:type rdf:resource="http://www.w3.org/2004/02/skos/core#Concept"/>
	<dcterms:creator rdf:datatype="http://www.w3.org/2001/XMLSchema#string">Natalia Atkins</dcterms:creator>
	<dcterms:created rdf:datatype="http://www.w3.org/2001/XMLSchema#dateTime">2016-01-07T10:38:15Z</dcterms:created>
	<skos:prefLabel xml:lang="en">School of Biological, Biomedical and Environmental Sciences, University of Hull</skos:prefLabel>
	<skos:altLabel xml:lang="en">School of Biological, Biomedical and Environmental Sciences</skos:altLabel>
	<skos:hiddenLabel xml:lang="en"></skos:hiddenLabel>
	<skos:definition xml:lang="en">In the latest UK-wide Research Excellence Framework (2014), our submitted research was assessed as having either ‘world-leading’ or ‘internationally excellent’ impact, while over half was of world-leading or internationally excellent standard. One of the University’s distinctive features is its strong research culture of collaboration and interdisciplinary working. The School and its researchers carry out true interdisciplinary research with scientists from Chemistry, Geography, the Hull York Medical School, academics from around the world, and clinicians and experts at local hospitals to become a centre of research excellence. The school’s research is structured around three major themes: Biomedical sciences: focusing on investigating the cellular processes involved in metabolism and energy transduction in health and disease. Ecology and Environment: includes physiological, behavioural and evolutionary studies as well as organism-level research. Evolutionary Biology: examining the varied processes which shape individual, population and species diversity.</skos:definition>
	<dc:source rdf:datatype="http://www.w3.org/2001/XMLSchema#string">Australian Ocean Data Network Organisation Register</dc:source>
	<dc:publisher rdf:datatype="http://www.w3.org/2001/XMLSchema#string">eMarine Information Infrastructure (eMII)</dc:publisher>
	<skos:exactMatch rdf:resource="http://seadatanet.maris2.nl/v_edmo/print.asp?n_code=4456"/>
	<skos:inScheme rdf:resource="http://vocab.aodn.org.au/def/organisation/1"/>
	<skos:broader rdf:resource="http://vocab.aodn.org.au/def/organisation/entity/447"/>
</rdf:Description>

<rdf:Description rdf:about="http://seadatanet.maris2.nl/v_edmo/print.asp?n_code=4455">
	<rdf:type rdf:resource="http://www.w3.org/2000/01/rdf-schema#Resource"/>
</rdf:Description>

<rdf:Description rdf:about="http://seadatanet.maris2.nl/v_edmo/print.asp?n_code=4456">
	<rdf:type rdf:resource="http://www.w3.org/2000/01/rdf-schema#Resource"/>
</rdf:Description>

<rdf:Description rdf:about="http://seadatanet.maris2.nl/v_edmo/print.asp?n_code=4378">
	<rdf:type rdf:resource="http://www.w3.org/2000/01/rdf-schema#Resource"/>
</rdf:Description>

<rdf:Description rdf:about="http://seadatanet.maris2.nl/v_edmo/print.asp?n_code=4512">
	<rdf:type rdf:resource="http://www.w3.org/2000/01/rdf-schema#Resource"/>
</rdf:Description>

</rdf:RDF>