<?xml version="1.0" encoding="UTF-8"?>
<rdf:RDF
	xmlns:rdf="http://www.w3.org/1999/02/22-rdf-syntax-ns#"
	xmlns:owl="http://www.w3.org/2002/07/owl#"
	xmlns:xsd="http://www.w3.org/2001/XMLSchema#"
	xmlns:fn="http://www.w3.org/2005/xpath-functions#"
	xmlns:dcterms="http://purl.org/dc/terms/"
	xmlns:rdfs="http://www.w3.org/2000/01/rdf-schema#"
	xmlns:sesame="http://www.openrdf.org/schema/sesame#"
	xmlns:foaf="http://xmlns.com/foaf/0.1/"
	xmlns:cycAnnot="http://sw.cyc.com/CycAnnotations_v1#"
	xmlns:csw="http://semantic-web.at/ontologies/csw.owl#"
	xmlns:freebase="http://rdf.freebase.com/ns/"
	xmlns:skos="http://www.w3.org/2004/02/skos/core#"
	xmlns:dbpedia="http://dbpedia.org/resource/"
	xmlns:cyc="http://sw.cyc.com/concept/"
	xmlns:tags="http://www.holygoat.co.uk/owl/redwood/0.1/tags/"
	xmlns:opencyc="http://sw.opencyc.org/concept/"
	xmlns:ctag="http://commontag.org/ns#"
	xmlns:dc="http://purl.org/dc/elements/1.1/">

<rdf:Description rdf:about="http://www.w3.org/1999/02/22-rdf-syntax-ns#type">
	<rdf:type rdf:resource="http://www.w3.org/1999/02/22-rdf-syntax-ns#Property"/>
	<rdf:type rdf:resource="http://www.w3.org/2000/01/rdf-schema#Resource"/>
	<rdfs:domain rdf:resource="http://www.w3.org/2000/01/rdf-schema#Resource"/>
	<rdfs:range rdf:resource="http://www.w3.org/2000/01/rdf-schema#Class"/>
	<rdfs:subPropertyOf rdf:resource="http://www.w3.org/1999/02/22-rdf-syntax-ns#type"/>
</rdf:Description>

<rdf:Description rdf:about="http://www.w3.org/1999/02/22-rdf-syntax-ns#Property">
	<rdf:type rdf:resource="http://www.w3.org/2000/01/rdf-schema#Resource"/>
	<rdf:type rdf:resource="http://www.w3.org/2000/01/rdf-schema#Class"/>
	<rdfs:subClassOf rdf:resource="http://www.w3.org/1999/02/22-rdf-syntax-ns#Property"/>
	<rdfs:subClassOf rdf:resource="http://www.w3.org/2000/01/rdf-schema#Resource"/>
</rdf:Description>

<rdf:Description rdf:about="http://www.w3.org/1999/02/22-rdf-syntax-ns#subject">
	<rdf:type rdf:resource="http://www.w3.org/1999/02/22-rdf-syntax-ns#Property"/>
	<rdf:type rdf:resource="http://www.w3.org/2000/01/rdf-schema#Resource"/>
	<rdfs:domain rdf:resource="http://www.w3.org/1999/02/22-rdf-syntax-ns#Statement"/>
	<rdfs:range rdf:resource="http://www.w3.org/2000/01/rdf-schema#Resource"/>
	<rdfs:subPropertyOf rdf:resource="http://www.w3.org/1999/02/22-rdf-syntax-ns#subject"/>
</rdf:Description>

<rdf:Description rdf:about="http://www.w3.org/1999/02/22-rdf-syntax-ns#predicate">
	<rdf:type rdf:resource="http://www.w3.org/1999/02/22-rdf-syntax-ns#Property"/>
	<rdf:type rdf:resource="http://www.w3.org/2000/01/rdf-schema#Resource"/>
	<rdfs:domain rdf:resource="http://www.w3.org/1999/02/22-rdf-syntax-ns#Statement"/>
	<rdfs:range rdf:resource="http://www.w3.org/2000/01/rdf-schema#Resource"/>
	<rdfs:subPropertyOf rdf:resource="http://www.w3.org/1999/02/22-rdf-syntax-ns#predicate"/>
</rdf:Description>

<rdf:Description rdf:about="http://www.w3.org/1999/02/22-rdf-syntax-ns#object">
	<rdf:type rdf:resource="http://www.w3.org/1999/02/22-rdf-syntax-ns#Property"/>
	<rdf:type rdf:resource="http://www.w3.org/2000/01/rdf-schema#Resource"/>
	<rdfs:domain rdf:resource="http://www.w3.org/1999/02/22-rdf-syntax-ns#Statement"/>
	<rdfs:range rdf:resource="http://www.w3.org/2000/01/rdf-schema#Resource"/>
	<rdfs:subPropertyOf rdf:resource="http://www.w3.org/1999/02/22-rdf-syntax-ns#object"/>
</rdf:Description>

<rdf:Description rdf:about="http://www.w3.org/1999/02/22-rdf-syntax-ns#first">
	<rdf:type rdf:resource="http://www.w3.org/1999/02/22-rdf-syntax-ns#Property"/>
	<rdf:type rdf:resource="http://www.w3.org/2000/01/rdf-schema#Resource"/>
	<rdfs:domain rdf:resource="http://www.w3.org/1999/02/22-rdf-syntax-ns#List"/>
	<rdfs:range rdf:resource="http://www.w3.org/2000/01/rdf-schema#Resource"/>
	<rdfs:subPropertyOf rdf:resource="http://www.w3.org/1999/02/22-rdf-syntax-ns#first"/>
</rdf:Description>

<rdf:Description rdf:about="http://www.w3.org/1999/02/22-rdf-syntax-ns#rest">
	<rdf:type rdf:resource="http://www.w3.org/1999/02/22-rdf-syntax-ns#Property"/>
	<rdf:type rdf:resource="http://www.w3.org/2000/01/rdf-schema#Resource"/>
	<rdfs:domain rdf:resource="http://www.w3.org/1999/02/22-rdf-syntax-ns#List"/>
	<rdfs:range rdf:resource="http://www.w3.org/1999/02/22-rdf-syntax-ns#List"/>
	<rdfs:subPropertyOf rdf:resource="http://www.w3.org/1999/02/22-rdf-syntax-ns#rest"/>
</rdf:Description>

<rdf:Description rdf:about="http://www.w3.org/1999/02/22-rdf-syntax-ns#value">
	<rdf:type rdf:resource="http://www.w3.org/1999/02/22-rdf-syntax-ns#Property"/>
	<rdf:type rdf:resource="http://www.w3.org/2000/01/rdf-schema#Resource"/>
	<rdfs:domain rdf:resource="http://www.w3.org/2000/01/rdf-schema#Resource"/>
	<rdfs:range rdf:resource="http://www.w3.org/2000/01/rdf-schema#Resource"/>
	<rdfs:subPropertyOf rdf:resource="http://www.w3.org/1999/02/22-rdf-syntax-ns#value"/>
</rdf:Description>

<rdf:Description rdf:about="http://www.w3.org/1999/02/22-rdf-syntax-ns#nil">
	<rdf:type rdf:resource="http://www.w3.org/1999/02/22-rdf-syntax-ns#List"/>
	<rdf:type rdf:resource="http://www.w3.org/2000/01/rdf-schema#Resource"/>
</rdf:Description>

<rdf:Description rdf:about="http://www.w3.org/1999/02/22-rdf-syntax-ns#List">
	<rdf:type rdf:resource="http://www.w3.org/2000/01/rdf-schema#Resource"/>
	<rdf:type rdf:resource="http://www.w3.org/2000/01/rdf-schema#Class"/>
	<rdfs:subClassOf rdf:resource="http://www.w3.org/1999/02/22-rdf-syntax-ns#List"/>
	<rdfs:subClassOf rdf:resource="http://www.w3.org/2000/01/rdf-schema#Resource"/>
</rdf:Description>

<rdf:Description rdf:about="http://www.w3.org/2000/01/rdf-schema#domain">
	<rdf:type rdf:resource="http://www.w3.org/1999/02/22-rdf-syntax-ns#Property"/>
	<rdf:type rdf:resource="http://www.w3.org/2000/01/rdf-schema#Resource"/>
	<rdfs:domain rdf:resource="http://www.w3.org/1999/02/22-rdf-syntax-ns#Property"/>
	<rdfs:range rdf:resource="http://www.w3.org/2000/01/rdf-schema#Class"/>
	<rdfs:subPropertyOf rdf:resource="http://www.w3.org/2000/01/rdf-schema#domain"/>
</rdf:Description>

<rdf:Description rdf:about="http://www.w3.org/2000/01/rdf-schema#Resource">
	<rdf:type rdf:resource="http://www.w3.org/2000/01/rdf-schema#Resource"/>
	<rdf:type rdf:resource="http://www.w3.org/2000/01/rdf-schema#Class"/>
	<rdfs:subClassOf rdf:resource="http://www.w3.org/2000/01/rdf-schema#Resource"/>
</rdf:Description>

<rdf:Description rdf:about="http://www.w3.org/2000/01/rdf-schema#range">
	<rdf:type rdf:resource="http://www.w3.org/1999/02/22-rdf-syntax-ns#Property"/>
	<rdf:type rdf:resource="http://www.w3.org/2000/01/rdf-schema#Resource"/>
	<rdfs:domain rdf:resource="http://www.w3.org/1999/02/22-rdf-syntax-ns#Property"/>
	<rdfs:range rdf:resource="http://www.w3.org/2000/01/rdf-schema#Class"/>
	<rdfs:subPropertyOf rdf:resource="http://www.w3.org/2000/01/rdf-schema#range"/>
</rdf:Description>

<rdf:Description rdf:about="http://www.w3.org/2000/01/rdf-schema#subPropertyOf">
	<rdf:type rdf:resource="http://www.w3.org/1999/02/22-rdf-syntax-ns#Property"/>
	<rdf:type rdf:resource="http://www.w3.org/2000/01/rdf-schema#Resource"/>
	<rdfs:domain rdf:resource="http://www.w3.org/1999/02/22-rdf-syntax-ns#Property"/>
	<rdfs:range rdf:resource="http://www.w3.org/1999/02/22-rdf-syntax-ns#Property"/>
	<rdfs:subPropertyOf rdf:resource="http://www.w3.org/2000/01/rdf-schema#subPropertyOf"/>
</rdf:Description>

<rdf:Description rdf:about="http://www.w3.org/2000/01/rdf-schema#subClassOf">
	<rdf:type rdf:resource="http://www.w3.org/1999/02/22-rdf-syntax-ns#Property"/>
	<rdf:type rdf:resource="http://www.w3.org/2000/01/rdf-schema#Resource"/>
	<rdfs:domain rdf:resource="http://www.w3.org/2000/01/rdf-schema#Class"/>
	<rdfs:range rdf:resource="http://www.w3.org/2000/01/rdf-schema#Class"/>
	<rdfs:subPropertyOf rdf:resource="http://www.w3.org/2000/01/rdf-schema#subClassOf"/>
</rdf:Description>

<rdf:Description rdf:about="http://www.w3.org/2000/01/rdf-schema#Class">
	<rdf:type rdf:resource="http://www.w3.org/2000/01/rdf-schema#Resource"/>
	<rdf:type rdf:resource="http://www.w3.org/2000/01/rdf-schema#Class"/>
	<rdfs:subClassOf rdf:resource="http://www.w3.org/2000/01/rdf-schema#Resource"/>
	<rdfs:subClassOf rdf:resource="http://www.w3.org/2000/01/rdf-schema#Class"/>
</rdf:Description>

<rdf:Description rdf:about="http://www.w3.org/1999/02/22-rdf-syntax-ns#Statement">
	<rdf:type rdf:resource="http://www.w3.org/2000/01/rdf-schema#Resource"/>
	<rdf:type rdf:resource="http://www.w3.org/2000/01/rdf-schema#Class"/>
	<rdfs:subClassOf rdf:resource="http://www.w3.org/2000/01/rdf-schema#Resource"/>
	<rdfs:subClassOf rdf:resource="http://www.w3.org/1999/02/22-rdf-syntax-ns#Statement"/>
</rdf:Description>

<rdf:Description rdf:about="http://www.w3.org/2000/01/rdf-schema#member">
	<rdf:type rdf:resource="http://www.w3.org/1999/02/22-rdf-syntax-ns#Property"/>
	<rdf:type rdf:resource="http://www.w3.org/2000/01/rdf-schema#Resource"/>
	<rdfs:domain rdf:resource="http://www.w3.org/2000/01/rdf-schema#Resource"/>
	<rdfs:range rdf:resource="http://www.w3.org/2000/01/rdf-schema#Resource"/>
	<rdfs:subPropertyOf rdf:resource="http://www.w3.org/2000/01/rdf-schema#member"/>
</rdf:Description>

<rdf:Description rdf:about="http://www.w3.org/2000/01/rdf-schema#seeAlso">
	<rdf:type rdf:resource="http://www.w3.org/1999/02/22-rdf-syntax-ns#Property"/>
	<rdf:type rdf:resource="http://www.w3.org/2000/01/rdf-schema#Resource"/>
	<rdfs:domain rdf:resource="http://www.w3.org/2000/01/rdf-schema#Resource"/>
	<rdfs:range rdf:resource="http://www.w3.org/2000/01/rdf-schema#Resource"/>
	<rdfs:subPropertyOf rdf:resource="http://www.w3.org/2000/01/rdf-schema#seeAlso"/>
</rdf:Description>

<rdf:Description rdf:about="http://www.w3.org/2000/01/rdf-schema#isDefinedBy">
	<rdf:type rdf:resource="http://www.w3.org/1999/02/22-rdf-syntax-ns#Property"/>
	<rdf:type rdf:resource="http://www.w3.org/2000/01/rdf-schema#Resource"/>
	<rdfs:domain rdf:resource="http://www.w3.org/2000/01/rdf-schema#Resource"/>
	<rdfs:range rdf:resource="http://www.w3.org/2000/01/rdf-schema#Resource"/>
	<rdfs:subPropertyOf rdf:resource="http://www.w3.org/2000/01/rdf-schema#seeAlso"/>
	<rdfs:subPropertyOf rdf:resource="http://www.w3.org/2000/01/rdf-schema#isDefinedBy"/>
</rdf:Description>

<rdf:Description rdf:about="http://www.w3.org/2000/01/rdf-schema#comment">
	<rdf:type rdf:resource="http://www.w3.org/1999/02/22-rdf-syntax-ns#Property"/>
	<rdf:type rdf:resource="http://www.w3.org/2000/01/rdf-schema#Resource"/>
	<rdfs:domain rdf:resource="http://www.w3.org/2000/01/rdf-schema#Resource"/>
	<rdfs:range rdf:resource="http://www.w3.org/2000/01/rdf-schema#Literal"/>
	<rdfs:subPropertyOf rdf:resource="http://www.w3.org/2000/01/rdf-schema#comment"/>
</rdf:Description>

<rdf:Description rdf:about="http://www.w3.org/2000/01/rdf-schema#label">
	<rdf:type rdf:resource="http://www.w3.org/1999/02/22-rdf-syntax-ns#Property"/>
	<rdf:type rdf:resource="http://www.w3.org/2000/01/rdf-schema#Resource"/>
	<rdfs:domain rdf:resource="http://www.w3.org/2000/01/rdf-schema#Resource"/>
	<rdfs:range rdf:resource="http://www.w3.org/2000/01/rdf-schema#Literal"/>
	<rdfs:subPropertyOf rdf:resource="http://www.w3.org/2000/01/rdf-schema#label"/>
</rdf:Description>

<rdf:Description rdf:about="http://www.w3.org/2000/01/rdf-schema#Literal">
	<rdf:type rdf:resource="http://www.w3.org/2000/01/rdf-schema#Resource"/>
	<rdf:type rdf:resource="http://www.w3.org/2000/01/rdf-schema#Class"/>
	<rdfs:subClassOf rdf:resource="http://www.w3.org/2000/01/rdf-schema#Resource"/>
	<rdfs:subClassOf rdf:resource="http://www.w3.org/2000/01/rdf-schema#Literal"/>
</rdf:Description>

<rdf:Description rdf:about="http://www.w3.org/1999/02/22-rdf-syntax-ns#Alt">
	<rdf:type rdf:resource="http://www.w3.org/2000/01/rdf-schema#Resource"/>
	<rdf:type rdf:resource="http://www.w3.org/2000/01/rdf-schema#Class"/>
	<rdfs:subClassOf rdf:resource="http://www.w3.org/2000/01/rdf-schema#Resource"/>
	<rdfs:subClassOf rdf:resource="http://www.w3.org/1999/02/22-rdf-syntax-ns#Alt"/>
	<rdfs:subClassOf rdf:resource="http://www.w3.org/2000/01/rdf-schema#Container"/>
</rdf:Description>

<rdf:Description rdf:about="http://www.w3.org/2000/01/rdf-schema#Container">
	<rdf:type rdf:resource="http://www.w3.org/2000/01/rdf-schema#Resource"/>
	<rdf:type rdf:resource="http://www.w3.org/2000/01/rdf-schema#Class"/>
	<rdfs:subClassOf rdf:resource="http://www.w3.org/2000/01/rdf-schema#Resource"/>
	<rdfs:subClassOf rdf:resource="http://www.w3.org/2000/01/rdf-schema#Container"/>
</rdf:Description>

<rdf:Description rdf:about="http://www.w3.org/1999/02/22-rdf-syntax-ns#Bag">
	<rdf:type rdf:resource="http://www.w3.org/2000/01/rdf-schema#Resource"/>
	<rdf:type rdf:resource="http://www.w3.org/2000/01/rdf-schema#Class"/>
	<rdfs:subClassOf rdf:resource="http://www.w3.org/2000/01/rdf-schema#Resource"/>
	<rdfs:subClassOf rdf:resource="http://www.w3.org/2000/01/rdf-schema#Container"/>
	<rdfs:subClassOf rdf:resource="http://www.w3.org/1999/02/22-rdf-syntax-ns#Bag"/>
</rdf:Description>

<rdf:Description rdf:about="http://www.w3.org/1999/02/22-rdf-syntax-ns#Seq">
	<rdf:type rdf:resource="http://www.w3.org/2000/01/rdf-schema#Resource"/>
	<rdf:type rdf:resource="http://www.w3.org/2000/01/rdf-schema#Class"/>
	<rdfs:subClassOf rdf:resource="http://www.w3.org/2000/01/rdf-schema#Resource"/>
	<rdfs:subClassOf rdf:resource="http://www.w3.org/2000/01/rdf-schema#Container"/>
	<rdfs:subClassOf rdf:resource="http://www.w3.org/1999/02/22-rdf-syntax-ns#Seq"/>
</rdf:Description>

<rdf:Description rdf:about="http://www.w3.org/2000/01/rdf-schema#ContainerMembershipProperty">
	<rdf:type rdf:resource="http://www.w3.org/2000/01/rdf-schema#Resource"/>
	<rdf:type rdf:resource="http://www.w3.org/2000/01/rdf-schema#Class"/>
	<rdfs:subClassOf rdf:resource="http://www.w3.org/1999/02/22-rdf-syntax-ns#Property"/>
	<rdfs:subClassOf rdf:resource="http://www.w3.org/2000/01/rdf-schema#Resource"/>
	<rdfs:subClassOf rdf:resource="http://www.w3.org/2000/01/rdf-schema#ContainerMembershipProperty"/>
</rdf:Description>

<rdf:Description rdf:about="http://www.w3.org/1999/02/22-rdf-syntax-ns#XMLLiteral">
	<rdf:type rdf:resource="http://www.w3.org/2000/01/rdf-schema#Resource"/>
	<rdf:type rdf:resource="http://www.w3.org/2000/01/rdf-schema#Class"/>
	<rdf:type rdf:resource="http://www.w3.org/2000/01/rdf-schema#Datatype"/>
	<rdfs:subClassOf rdf:resource="http://www.w3.org/2000/01/rdf-schema#Resource"/>
	<rdfs:subClassOf rdf:resource="http://www.w3.org/2000/01/rdf-schema#Literal"/>
	<rdfs:subClassOf rdf:resource="http://www.w3.org/1999/02/22-rdf-syntax-ns#XMLLiteral"/>
</rdf:Description>

<rdf:Description rdf:about="http://www.w3.org/2000/01/rdf-schema#Datatype">
	<rdf:type rdf:resource="http://www.w3.org/2000/01/rdf-schema#Resource"/>
	<rdf:type rdf:resource="http://www.w3.org/2000/01/rdf-schema#Class"/>
	<rdfs:subClassOf rdf:resource="http://www.w3.org/2000/01/rdf-schema#Resource"/>
	<rdfs:subClassOf rdf:resource="http://www.w3.org/2000/01/rdf-schema#Class"/>
	<rdfs:subClassOf rdf:resource="http://www.w3.org/2000/01/rdf-schema#Datatype"/>
</rdf:Description>

<rdf:Description rdf:about="http://editor.vocabs.ands.org.au/user/Natalia_Atkins">
	<rdf:type rdf:resource="http://www.w3.org/2000/01/rdf-schema#Resource"/>
	<rdf:type rdf:resource="http://purl.org/dc/terms/Agent"/>
	<foaf:name rdf:datatype="http://www.w3.org/2001/XMLSchema#string">Natalia_Atkins</foaf:name>
</rdf:Description>

<rdf:Description rdf:about="http://purl.org/dc/terms/Agent">
	<rdf:type rdf:resource="http://www.w3.org/2000/01/rdf-schema#Resource"/>
	<rdf:type rdf:resource="http://www.w3.org/2000/01/rdf-schema#Class"/>
	<rdfs:subClassOf rdf:resource="http://www.w3.org/2000/01/rdf-schema#Resource"/>
	<rdfs:subClassOf rdf:resource="http://purl.org/dc/terms/Agent"/>
</rdf:Description>

<rdf:Description rdf:about="http://xmlns.com/foaf/0.1/name">
	<rdf:type rdf:resource="http://www.w3.org/1999/02/22-rdf-syntax-ns#Property"/>
	<rdf:type rdf:resource="http://www.w3.org/2000/01/rdf-schema#Resource"/>
	<rdfs:subPropertyOf rdf:resource="http://xmlns.com/foaf/0.1/name"/>
</rdf:Description>

<rdf:Description rdf:about="http://editor.vocabs.ands.org.au/user/Sebastien-Mancini">
	<rdf:type rdf:resource="http://www.w3.org/2000/01/rdf-schema#Resource"/>
	<rdf:type rdf:resource="http://purl.org/dc/terms/Agent"/>
	<foaf:name rdf:datatype="http://www.w3.org/2001/XMLSchema#string">Sebastien-Mancini</foaf:name>
</rdf:Description>

<rdf:Description rdf:about="http://editor.vocabs.ands.org.au/user/Sebastien_Mancini">
	<rdf:type rdf:resource="http://www.w3.org/2000/01/rdf-schema#Resource"/>
	<rdf:type rdf:resource="http://purl.org/dc/terms/Agent"/>
	<foaf:name rdf:datatype="http://www.w3.org/2001/XMLSchema#string">Sebastien_Mancini</foaf:name>
</rdf:Description>

<rdf:Description rdf:about="http://editor.vocabs.ands.org.au/user/eMII_Atkins.Natalia">
	<rdf:type rdf:resource="http://www.w3.org/2000/01/rdf-schema#Resource"/>
	<rdf:type rdf:resource="http://purl.org/dc/terms/Agent"/>
	<foaf:name rdf:datatype="http://www.w3.org/2001/XMLSchema#string">eMII_Atkins.Natalia</foaf:name>
</rdf:Description>

<rdf:Description rdf:about="http://editor.vocabs.ands.org.au/user/eMII_Finney.Kim_Admin">
	<rdf:type rdf:resource="http://www.w3.org/2000/01/rdf-schema#Resource"/>
	<rdf:type rdf:resource="http://purl.org/dc/terms/Agent"/>
	<foaf:name rdf:datatype="http://www.w3.org/2001/XMLSchema#string">eMII_Finney.Kim_Admin</foaf:name>
</rdf:Description>

<rdf:Description rdf:about="http://editor.vocabs.ands.org.au/user/eMarine-Information-Infrastructure-eMII">
	<rdf:type rdf:resource="http://www.w3.org/2000/01/rdf-schema#Resource"/>
	<rdf:type rdf:resource="http://purl.org/dc/terms/Agent"/>
	<foaf:name rdf:datatype="http://www.w3.org/2001/XMLSchema#string">eMarine-Information-Infrastructure-eMII</foaf:name>
</rdf:Description>

<rdf:Description rdf:about="http://editor.vocabs.ands.org.au/user/eMII_Mancini.Sebastien">
	<rdf:type rdf:resource="http://www.w3.org/2000/01/rdf-schema#Resource"/>
	<rdf:type rdf:resource="http://purl.org/dc/terms/Agent"/>
	<foaf:name rdf:datatype="http://www.w3.org/2001/XMLSchema#string">eMII_Mancini.Sebastien</foaf:name>
</rdf:Description>

<rdf:Description rdf:about="http://vocab.aodn.org.au/def/instrument/2">
	<rdf:type rdf:resource="http://www.w3.org/2000/01/rdf-schema#Resource"/>
	<rdfs:label xml:lang="en">RBR TGR-2050 submersible tide gauge </rdfs:label>
	<owl:deprecated rdf:datatype="http://www.w3.org/2001/XMLSchema#boolean">true</owl:deprecated>
</rdf:Description>

<rdf:Description rdf:about="http://www.w3.org/2002/07/owl#deprecated">
	<rdf:type rdf:resource="http://www.w3.org/1999/02/22-rdf-syntax-ns#Property"/>
	<rdf:type rdf:resource="http://www.w3.org/2000/01/rdf-schema#Resource"/>
	<rdfs:subPropertyOf rdf:resource="http://www.w3.org/2002/07/owl#deprecated"/>
</rdf:Description>

<rdf:Description rdf:about="http://vocab.aodn.org.au/def/instrument/3">
	<rdf:type rdf:resource="http://www.w3.org/2000/01/rdf-schema#Resource"/>
	<rdfs:label xml:lang="en">Sea-Bird SBE 16plusV2 SeaCAT C-T Recorder</rdfs:label>
	<owl:deprecated rdf:datatype="http://www.w3.org/2001/XMLSchema#boolean">true</owl:deprecated>
</rdf:Description>

<rdf:Description rdf:about="http://vocab.aodn.org.au/def/instrument/entity/33">
	<rdf:type rdf:resource="http://www.w3.org/2000/01/rdf-schema#Resource"/>
	<rdfs:label xml:lang="en">Nortek Aquadopp Profiler</rdfs:label>
	<owl:deprecated rdf:datatype="http://www.w3.org/2001/XMLSchema#boolean">true</owl:deprecated>
</rdf:Description>

<rdf:Description rdf:about="http://vocab.aodn.org.au/def/instrument/entity/360">
	<rdf:type rdf:resource="http://www.w3.org/2000/01/rdf-schema#Resource"/>
	<rdfs:label xml:lang="en">water pressure sensor</rdfs:label>
	<owl:deprecated rdf:datatype="http://www.w3.org/2001/XMLSchema#boolean">true</owl:deprecated>
</rdf:Description>

<rdf:Description rdf:about="http://vocab.aodn.org.au/def/instrument/entity/37">
	<rdf:type rdf:resource="http://www.w3.org/2000/01/rdf-schema#Resource"/>
	<rdfs:label xml:lang="en">Nortek Continental</rdfs:label>
	<owl:deprecated rdf:datatype="http://www.w3.org/2001/XMLSchema#boolean">true</owl:deprecated>
</rdf:Description>

<rdf:Description rdf:about="http://vocab.aodn.org.au/def/instrument/entity/38">
	<rdf:type rdf:resource="http://www.w3.org/2000/01/rdf-schema#Resource"/>
	<rdfs:label xml:lang="en">Nortek AWAC</rdfs:label>
	<owl:deprecated rdf:datatype="http://www.w3.org/2001/XMLSchema#boolean">true</owl:deprecated>
</rdf:Description>

<rdf:Description rdf:about="http://vocab.aodn.org.au/def/instrument/entity/537">
	<rdf:type rdf:resource="http://www.w3.org/2000/01/rdf-schema#Resource"/>
	<rdfs:label xml:lang="en">Vaisala WAA15A cup anemometer</rdfs:label>
	<owl:deprecated rdf:datatype="http://www.w3.org/2001/XMLSchema#boolean">true</owl:deprecated>
</rdf:Description>

<rdf:Description rdf:about="http://vocab.aodn.org.au/def/instrument/entity/545">
	<rdf:type rdf:resource="http://www.w3.org/2000/01/rdf-schema#Resource"/>
	<rdfs:label xml:lang="en">Eppley Ultraviolet Radiometer (UVB)</rdfs:label>
	<owl:deprecated rdf:datatype="http://www.w3.org/2001/XMLSchema#boolean">true</owl:deprecated>
</rdf:Description>

<rdf:Description rdf:about="http://vocab.aodn.org.au/def/instrument/entity/553">
	<rdf:type rdf:resource="http://www.w3.org/2000/01/rdf-schema#Resource"/>
	<rdfs:label xml:lang="en">Everest Interscience 4000.4ZL Temperature Sensor</rdfs:label>
	<owl:deprecated rdf:datatype="http://www.w3.org/2001/XMLSchema#boolean">true</owl:deprecated>
</rdf:Description>

<rdf:Description rdf:about="http://vocab.nerc.ac.uk/collection/L05/current/302/">
	<rdf:type rdf:resource="http://www.w3.org/2000/01/rdf-schema#Resource"/>
	<rdfs:label xml:lang="en">water body temperature sensor</rdfs:label>
	<owl:deprecated rdf:datatype="http://www.w3.org/2001/XMLSchema#boolean">true</owl:deprecated>
	<dcterms:isReplacedBy rdf:resource="http://vocab.nerc.ac.uk/collection/L05/current/302"/>
</rdf:Description>

<rdf:Description rdf:about="http://purl.org/dc/terms/isReplacedBy">
	<rdf:type rdf:resource="http://www.w3.org/1999/02/22-rdf-syntax-ns#Property"/>
	<rdf:type rdf:resource="http://www.w3.org/2000/01/rdf-schema#Resource"/>
	<rdfs:subPropertyOf rdf:resource="http://purl.org/dc/terms/isReplacedBy"/>
</rdf:Description>

<rdf:Description rdf:about="http://vocab.nerc.ac.uk/collection/L05/current/302">
	<rdf:type rdf:resource="http://www.w3.org/2000/01/rdf-schema#Resource"/>
	<rdf:type rdf:resource="http://www.w3.org/2004/02/skos/core#Concept"/>
	<dcterms:created rdf:datatype="http://www.w3.org/2001/XMLSchema#dateTime">2015-08-07T00:00:00Z</dcterms:created>
	<dc:publisher rdf:datatype="http://www.w3.org/2001/XMLSchema#string">British Oceanographic Data Centre (BODC)</dc:publisher>
	<skos:definition xml:lang="en">Sensors that measure the intensity and nature of electromagnetic radiation emitted from the Earth in a manner optimised for the determination of water body surface temperature.</skos:definition>
	<skos:inScheme rdf:resource="http://vocab.aodn.org.au/def/instrument/1"/>
	<skos:narrower rdf:resource="http://vocab.nerc.ac.uk/collection/L22/current/TOOL0930"/>
	<skos:narrower rdf:resource="http://vocab.nerc.ac.uk/collection/L22/current/TOOL1016"/>
	<skos:prefLabel xml:lang="en">water body temperature sensor</skos:prefLabel>
	<skos:topConceptOf rdf:resource="http://vocab.aodn.org.au/def/instrument/1"/>
</rdf:Description>

<rdf:Description rdf:about="http://vocab.nerc.ac.uk/collection/L05/current/POS03/">
	<rdf:type rdf:resource="http://www.w3.org/2000/01/rdf-schema#Resource"/>
	<rdfs:label xml:lang="en">NAVSTAR Global Positioning System receivers</rdfs:label>
	<owl:deprecated rdf:datatype="http://www.w3.org/2001/XMLSchema#boolean">true</owl:deprecated>
</rdf:Description>

<rdf:Description rdf:about="http://vocab.nerc.ac.uk/collection/L05/current/TRTG/">
	<rdf:type rdf:resource="http://www.w3.org/2000/01/rdf-schema#Resource"/>
	<rdfs:label xml:lang="en">tracking tags</rdfs:label>
	<owl:deprecated rdf:datatype="http://www.w3.org/2001/XMLSchema#boolean">true</owl:deprecated>
	<dcterms:isReplacedBy rdf:resource="http://vocab.nerc.ac.uk/collection/L05/current/TRTG"/>
</rdf:Description>

<rdf:Description rdf:about="http://vocab.nerc.ac.uk/collection/L05/current/TRTG">
	<rdf:type rdf:resource="http://www.w3.org/2000/01/rdf-schema#Resource"/>
	<rdf:type rdf:resource="http://www.w3.org/2004/02/skos/core#Concept"/>
	<dcterms:created rdf:datatype="http://www.w3.org/2001/XMLSchema#dateTime">2015-08-07T00:00:00Z</dcterms:created>
	<dc:publisher rdf:datatype="http://www.w3.org/2001/XMLSchema#string">British Oceanographic Data Centre (BODC)</dc:publisher>
	<skos:definition xml:lang="en">Devices attached to living organisms with the purpose of determining the location of those organisms as a function of time after tagging and release.</skos:definition>
	<skos:inScheme rdf:resource="http://vocab.aodn.org.au/def/instrument/1"/>
	<skos:narrower rdf:resource="http://vocab.nerc.ac.uk/collection/L22/current/TOOL0929"/>
	<skos:narrower rdf:resource="http://vocab.nerc.ac.uk/collection/L22/current/TOOL1152"/>
	<skos:narrower rdf:resource="http://vocab.nerc.ac.uk/collection/L22/current/TOOL1153"/>
	<skos:narrower rdf:resource="http://vocab.nerc.ac.uk/collection/L22/current/TOOL1154"/>
	<skos:narrower rdf:resource="http://vocab.nerc.ac.uk/collection/L22/current/TOOL1155"/>
	<skos:narrower rdf:resource="http://vocab.nerc.ac.uk/collection/L22/current/TOOL1156"/>
	<skos:narrower rdf:resource="http://vocab.nerc.ac.uk/collection/L22/current/TOOL1157"/>
	<skos:prefLabel xml:lang="en">tracking tags</skos:prefLabel>
	<skos:topConceptOf rdf:resource="http://vocab.aodn.org.au/def/instrument/1"/>
</rdf:Description>

<rdf:Description rdf:about="http://vocab.nerc.ac.uk/collection/L22/current/TOOL007511">
	<rdf:type rdf:resource="http://www.w3.org/2000/01/rdf-schema#Resource"/>
	<rdfs:label xml:lang="en">Test Import Concept</rdfs:label>
	<owl:deprecated rdf:datatype="http://www.w3.org/2001/XMLSchema#boolean">true</owl:deprecated>
</rdf:Description>

<rdf:Description rdf:about="http://vocab.nerc.ac.uk/collection/L22/current/TOOL0869/">
	<rdf:type rdf:resource="http://www.w3.org/2000/01/rdf-schema#Resource"/>
	<rdfs:label xml:lang="en">Sea-Bird SBE 37-SMP-ODO MicroCAT C-...</rdfs:label>
	<owl:deprecated rdf:datatype="http://www.w3.org/2001/XMLSchema#boolean">true</owl:deprecated>
	<dcterms:isReplacedBy rdf:resource="http://vocab.nerc.ac.uk/collection/L22/current/TOOL0869"/>
</rdf:Description>

<rdf:Description rdf:about="http://vocab.nerc.ac.uk/collection/L22/current/TOOL0869">
	<rdf:type rdf:resource="http://www.w3.org/2000/01/rdf-schema#Resource"/>
	<rdf:type rdf:resource="http://www.w3.org/2004/02/skos/core#Concept"/>
	<dcterms:contributor rdf:resource="http://editor.vocabs.ands.org.au/user/eMII_Atkins.Natalia"/>
	<dcterms:created rdf:datatype="http://www.w3.org/2001/XMLSchema#dateTime">2015-06-03T00:00:00Z</dcterms:created>
	<dcterms:modified rdf:datatype="http://www.w3.org/2001/XMLSchema#dateTime">2015-08-28T00:06:17Z</dcterms:modified>
	<dc:publisher rdf:datatype="http://www.w3.org/2001/XMLSchema#string">British Oceanographic Data Centre (BODC)</dc:publisher>
	<dc:source rdf:datatype="http://www.w3.org/2001/XMLSchema#string">(L221) SeaVoX Device Catalogue</dc:source>
	<skos:definition xml:lang="en">The SBE 37 MicroCAT is a high accuracy conductivity and temperature recorder with an optional pressure sensor and an Optical Dissolved Oxygen (ODO) sensor designed for deployment on moorings. It is available with either a plastic (rated to 350m) or titanium (rated to 6000m) housing and has an internal pump to improve conductivity and oxygen response. Bio-fouling protection is provided by expendable anti-foulant devices, pump flow path and pumping regimen.</skos:definition>
	<skos:inScheme rdf:resource="http://vocab.aodn.org.au/def/instrument/1"/>
	<skos:prefLabel xml:lang="en">Sea-Bird SBE 37-SMP-ODO MicroCAT C-T-ODO</skos:prefLabel>
	<skos:broader rdf:resource="http://vocab.aodn.org.au/def/instrument/entity/365"/>
	<skos:broader rdf:resource="http://vocab.nerc.ac.uk/collection/L05/current/134"/>
	<skos:broader rdf:resource="http://vocab.nerc.ac.uk/collection/L05/current/350"/>
	<skos:broader rdf:resource="http://vocab.nerc.ac.uk/collection/L05/current/351"/>
	<skos:altLabel xml:lang="en">SBE 37-SMP-ODO MicroCAT</skos:altLabel>
</rdf:Description>

<rdf:Description rdf:about="http://vocab.nerc.ac.uk/collection/L22/current/TOOL0870/">
	<rdf:type rdf:resource="http://www.w3.org/2000/01/rdf-schema#Resource"/>
	<rdfs:label xml:lang="en">Sea-Bird SBE 16Plus V2 SEACAT C-T R...</rdfs:label>
	<owl:deprecated rdf:datatype="http://www.w3.org/2001/XMLSchema#boolean">true</owl:deprecated>
	<dcterms:isReplacedBy rdf:resource="http://vocab.nerc.ac.uk/collection/L22/current/TOOL0870"/>
</rdf:Description>

<rdf:Description rdf:about="http://vocab.nerc.ac.uk/collection/L22/current/TOOL0870">
	<rdf:type rdf:resource="http://www.w3.org/2000/01/rdf-schema#Resource"/>
	<rdf:type rdf:resource="http://www.w3.org/2004/02/skos/core#Concept"/>
	<dcterms:contributor rdf:resource="http://editor.vocabs.ands.org.au/user/eMII_Atkins.Natalia"/>
	<dcterms:created rdf:datatype="http://www.w3.org/2001/XMLSchema#dateTime">2015-06-03T00:00:00Z</dcterms:created>
	<dcterms:modified rdf:datatype="http://www.w3.org/2001/XMLSchema#dateTime">2015-08-28T00:04:45Z</dcterms:modified>
	<dc:publisher rdf:datatype="http://www.w3.org/2001/XMLSchema#string">British Oceanographic Data Centre (BODC)</dc:publisher>
	<dc:source rdf:datatype="http://www.w3.org/2001/XMLSchema#string">(L221) SeaVoX Device Catalogue</dc:source>
	<skos:definition xml:lang="en">The SBE 16plus V2 is a high accuracy conductivity and temperature recorder (pressure optional) with RS232 or RS485 interfaces. It is designed for moorings and other long-duration, fixed-site deployments. It has 6 amplified A/D input channels and conditioned power of 500 ma is available for auxiliary sensors, dissolved oxygen, turbidity, fluorescence, PAR etc. Compared to the previous 16plus, the V2 incorporates an electronics upgrade and additional features, with six differentially amplified A/D input channels, one RS-232 data input channel, and 64 MB FLASH memory. Data can be output in XML as well as ASCII and HEX formats. Firmware upgrades can be downloaded through the communications port, without opening the instrument.</skos:definition>
	<skos:inScheme rdf:resource="http://vocab.aodn.org.au/def/instrument/1"/>
	<skos:prefLabel xml:lang="en">Sea-Bird SBE 16Plus V2 SEACAT C-T Recorder</skos:prefLabel>
	<skos:broader rdf:resource="http://vocab.aodn.org.au/def/instrument/entity/365"/>
	<skos:broader rdf:resource="http://vocab.nerc.ac.uk/collection/L05/current/134"/>
	<skos:broader rdf:resource="http://vocab.nerc.ac.uk/collection/L05/current/350"/>
	<skos:altLabel xml:lang="en">SBE 16+ V2 SEACAT</skos:altLabel>
</rdf:Description>

<rdf:Description rdf:about="http://vocab.nerc.ac.uk/collection/L22/current/TOOL0871/">
	<rdf:type rdf:resource="http://www.w3.org/2000/01/rdf-schema#Resource"/>
	<rdfs:label xml:lang="en">Sea-Bird SBE 19plus V2 SEACAT CTD</rdfs:label>
	<owl:deprecated rdf:datatype="http://www.w3.org/2001/XMLSchema#boolean">true</owl:deprecated>
	<dcterms:isReplacedBy rdf:resource="http://vocab.nerc.ac.uk/collection/L22/current/TOOL0871"/>
</rdf:Description>

<rdf:Description rdf:about="http://vocab.nerc.ac.uk/collection/L22/current/TOOL0871">
	<rdf:type rdf:resource="http://www.w3.org/2000/01/rdf-schema#Resource"/>
	<rdf:type rdf:resource="http://www.w3.org/2004/02/skos/core#Concept"/>
	<dcterms:created rdf:datatype="http://www.w3.org/2001/XMLSchema#dateTime">2015-06-03T00:00:00Z</dcterms:created>
	<dcterms:modified rdf:datatype="http://www.w3.org/2001/XMLSchema#dateTime">2015-06-10T02:07:18Z</dcterms:modified>
	<dc:publisher rdf:datatype="http://www.w3.org/2001/XMLSchema#string">British Oceanographic Data Centre (BODC)</dc:publisher>
	<dc:source rdf:datatype="http://www.w3.org/2001/XMLSchema#string">(L221) SeaVoX Device Catalogue</dc:source>
	<skos:definition xml:lang="en">Self-contained self-powered CTD profiler. Measures conductivity, temperature and pressure (Digiquartz sensor) in both profiling (samples at 4 scans/sec) and moored (sample rates of once every 5 seconds to once every 9 hours) mode. Available in plastic or titanium housing with depth ranges of 600m and 7000m respectively. Miniature submersible pump provides water to the conductivity cell.  Compared to the previous 19plus, the V2 incorporates an electronics upgrade and additional features, with six differentially amplified A/D input channels, one RS-232 data input channel, and 64 MB FLASH memory.</skos:definition>
	<skos:inScheme rdf:resource="http://vocab.aodn.org.au/def/instrument/1"/>
	<skos:prefLabel xml:lang="en">Sea-Bird SBE 19plus V2 SEACAT CTD</skos:prefLabel>
	<skos:broader rdf:resource="http://vocab.nerc.ac.uk/collection/L05/current/130"/>
	<skos:broader rdf:resource="http://vocab.nerc.ac.uk/collection/L05/current/134"/>
	<skos:broader rdf:resource="http://vocab.nerc.ac.uk/collection/L05/current/350"/>
	<skos:altLabel xml:lang="en">SBE 19+ V2 SEACAT</skos:altLabel>
</rdf:Description>

<rdf:Description rdf:about="http://vocab.nerc.ac.uk/collection/L22/current/TOOL0872/">
	<rdf:type rdf:resource="http://www.w3.org/2000/01/rdf-schema#Resource"/>
	<rdfs:label xml:lang="en">Teledyne RDI Workhorse Navigator 12...</rdfs:label>
	<owl:deprecated rdf:datatype="http://www.w3.org/2001/XMLSchema#boolean">true</owl:deprecated>
	<dcterms:isReplacedBy rdf:resource="http://vocab.nerc.ac.uk/collection/L22/current/TOOL0872"/>
</rdf:Description>

<rdf:Description rdf:about="http://vocab.nerc.ac.uk/collection/L22/current/TOOL0872">
	<rdf:type rdf:resource="http://www.w3.org/2000/01/rdf-schema#Resource"/>
	<rdf:type rdf:resource="http://www.w3.org/2004/02/skos/core#Concept"/>
	<dcterms:contributor rdf:resource="http://editor.vocabs.ands.org.au/user/Natalia_Atkins"/>
	<dcterms:created rdf:datatype="http://www.w3.org/2001/XMLSchema#dateTime">2015-06-03T00:00:00Z</dcterms:created>
	<dcterms:modified rdf:datatype="http://www.w3.org/2001/XMLSchema#dateTime">2015-06-30T03:42:14Z</dcterms:modified>
	<dc:publisher rdf:datatype="http://www.w3.org/2001/XMLSchema#string">British Oceanographic Data Centre (BODC)</dc:publisher>
	<skos:definition xml:lang="en">A Doppler velocity log (DVL) measuring bottom track and water track velocities, altitude, heading, tilt, temperature and echo intensity. 1200kHz Broadband signal processing gives high data resolution and a four-beam solution gives an independent error velocity measurement as an indicator of data quality. It has a bottom track range of 30m and velocity accuracy for both bottom and water track modes is 0.2% of the velocity, ±0.1cm/s. The instrument operates effectively over a temperature range of -5°C to 45°C and with a tilt of up to ±15 deg.</skos:definition>
	<skos:inScheme rdf:resource="http://vocab.aodn.org.au/def/instrument/1"/>
	<skos:prefLabel xml:lang="en">Teledyne RDI Workhorse Navigator 1200kHz Doppler Velocity Log</skos:prefLabel>
	<skos:broader rdf:resource="http://vocab.nerc.ac.uk/collection/L05/current/134"/>
	<skos:broader rdf:resource="http://vocab.nerc.ac.uk/collection/L05/current/379"/>
	<skos:broader rdf:resource="http://vocab.nerc.ac.uk/collection/L05/current/385"/>
	<skos:altLabel xml:lang="en">RDI Workhorse Navigator 1200kHz DVL</skos:altLabel>
</rdf:Description>

<rdf:Description rdf:about="http://vocab.nerc.ac.uk/collection/L22/current/TOOL0873/">
	<rdf:type rdf:resource="http://www.w3.org/2000/01/rdf-schema#Resource"/>
	<rdfs:label xml:lang="en">SMRU GPS Satellite Relay Data Logge...</rdfs:label>
	<owl:deprecated rdf:datatype="http://www.w3.org/2001/XMLSchema#boolean">true</owl:deprecated>
	<dcterms:isReplacedBy rdf:resource="http://vocab.nerc.ac.uk/collection/L22/current/TOOL0873"/>
</rdf:Description>

<rdf:Description rdf:about="http://vocab.nerc.ac.uk/collection/L22/current/TOOL0873">
	<rdf:type rdf:resource="http://www.w3.org/2000/01/rdf-schema#Resource"/>
	<rdf:type rdf:resource="http://www.w3.org/2004/02/skos/core#Concept"/>
	<dcterms:contributor rdf:resource="http://editor.vocabs.ands.org.au/user/Natalia_Atkins"/>
	<dcterms:created rdf:datatype="http://www.w3.org/2001/XMLSchema#dateTime">2015-06-03T00:00:00Z</dcterms:created>
	<dcterms:modified rdf:datatype="http://www.w3.org/2001/XMLSchema#dateTime">2015-07-01T01:19:54Z</dcterms:modified>
	<dc:publisher rdf:datatype="http://www.w3.org/2001/XMLSchema#string">British Oceanographic Data Centre (BODC)</dc:publisher>
	<skos:definition xml:lang="en">A package comprising a wet/dry, pressure and temperature sensors with a GPS receiver for high accuracy position data and antenna suitable for transmission of data via the Argos satellite system. The unit contains an internal battery and a microprocessor that logs data and schedules the transfer of data.  GPS locations are acquired in less than a second so position may be transferred to the satellite on every surfacing. The package is designed for attachment to marine mammals and has an operational depth range of down to 2000 m. More information is available at http://www.smru.st-and.ac.uk/Instrumentation/GPSArgosTag/.</skos:definition>
	<skos:inScheme rdf:resource="http://vocab.aodn.org.au/def/instrument/1"/>
	<skos:prefLabel xml:lang="en">SMRU GPS Satellite Relay Data Logger (Argos)</skos:prefLabel>
	<skos:broader rdf:resource="http://vocab.nerc.ac.uk/collection/L05/current/134"/>
	<skos:broader rdf:resource="http://vocab.nerc.ac.uk/collection/L05/current/POS03"/>
	<skos:broader rdf:resource="http://vocab.nerc.ac.uk/collection/L05/current/WPS"/>
	<skos:altLabel xml:lang="en">SMRU GPS SRDL</skos:altLabel>
</rdf:Description>

<rdf:Description rdf:about="http://vocab.nerc.ac.uk/collection/L22/current/TOOL0877/">
	<rdf:type rdf:resource="http://www.w3.org/2000/01/rdf-schema#Resource"/>
	<rdfs:label xml:lang="en">Vaisala WAA15A cup anemometer</rdfs:label>
	<owl:deprecated rdf:datatype="http://www.w3.org/2001/XMLSchema#boolean">true</owl:deprecated>
	<dcterms:isReplacedBy rdf:resource="http://vocab.nerc.ac.uk/collection/L22/current/TOOL0877"/>
</rdf:Description>

<rdf:Description rdf:about="http://vocab.nerc.ac.uk/collection/L22/current/TOOL0877">
	<rdf:type rdf:resource="http://www.w3.org/2000/01/rdf-schema#Resource"/>
	<rdf:type rdf:resource="http://www.w3.org/2004/02/skos/core#Concept"/>
	<dcterms:created rdf:datatype="http://www.w3.org/2001/XMLSchema#dateTime">2015-06-03T00:00:00Z</dcterms:created>
	<dc:publisher rdf:datatype="http://www.w3.org/2001/XMLSchema#string">British Oceanographic Data Centre (BODC)</dc:publisher>
	<skos:definition xml:lang="en">Three lightweight, conical cups mounted on the cup wheel providing linearity with windspeeds up to 75m/s. Rotation speed is measured by a disk attached to the shaft cutting an infrared light beam 14 times per revolution producing pulses counted by a phototransistor. The output rate is directly proportional to wind speed. It was replaced by the WAA151 model which introduced a number of improvements such as plug-and-play design, an improved mechanical shaft attachment and addition of electrical lightning protection. Both models have the same output, mounting and wiring scheme and so are totally interchangeable.</skos:definition>
	<skos:inScheme rdf:resource="http://vocab.aodn.org.au/def/instrument/1"/>
	<skos:prefLabel xml:lang="en">Vaisala WAA15A cup anemometer</skos:prefLabel>
	<skos:broader rdf:resource="http://vocab.nerc.ac.uk/collection/L05/current/101"/>
	<skos:altLabel xml:lang="en">Vaisala WAA15A anemometer</skos:altLabel>
</rdf:Description>

<rdf:Description rdf:about="http://vocab.nerc.ac.uk/collection/L22/current/TOOL0878/">
	<rdf:type rdf:resource="http://www.w3.org/2000/01/rdf-schema#Resource"/>
	<rdfs:label xml:lang="en">Battele Seaology pCO2 monitoring sy...</rdfs:label>
	<owl:deprecated rdf:datatype="http://www.w3.org/2001/XMLSchema#boolean">true</owl:deprecated>
	<dcterms:isReplacedBy rdf:resource="http://vocab.nerc.ac.uk/collection/L22/current/TOOL0878"/>
</rdf:Description>

<rdf:Description rdf:about="http://vocab.nerc.ac.uk/collection/L22/current/TOOL0878">
	<rdf:type rdf:resource="http://www.w3.org/2000/01/rdf-schema#Resource"/>
	<rdf:type rdf:resource="http://www.w3.org/2004/02/skos/core#Concept"/>
	<dcterms:contributor rdf:resource="http://editor.vocabs.ands.org.au/user/eMII_Atkins.Natalia"/>
	<dcterms:created rdf:datatype="http://www.w3.org/2001/XMLSchema#dateTime">2015-06-03T00:00:00Z</dcterms:created>
	<dcterms:modified rdf:datatype="http://www.w3.org/2001/XMLSchema#dateTime">2017-10-01T22:56:40Z</dcterms:modified>
	<dc:publisher rdf:datatype="http://www.w3.org/2001/XMLSchema#string">British Oceanographic Data Centre (BODC)</dc:publisher>
	<skos:definition xml:lang="en">An autonomous air and water pCO2 monitoring device comprising an equilibrator to extract diffused gases from seawater, an air block that collects an air sample whilst excluding seawater and a non-dispersive infrared (NDIR) carbon dioxide detector. These are designed to be mounted in a surface buoy (moored or drifting) with a power source (battery and solar), a stock of calibration standard gas, a control system, satellite communications including GPS and data storage. It has a measurement range of 100 to 600 ppm and precision of about 1 ppm.More information at http://battelle.org/our-work/national-security/maritime-technologies/sensors/battelle-seaology/battelle-pco2-monitoring-system#sthash.qWbxMCsQ.dpuf.</skos:definition>
	<skos:inScheme rdf:resource="http://vocab.aodn.org.au/def/instrument/1"/>
	<skos:prefLabel xml:lang="en">Battele Seaology pCO2 monitoring system</skos:prefLabel>
	<skos:broader rdf:resource="http://vocab.nerc.ac.uk/collection/L05/current/351"/>
	<skos:broader rdf:resource="http://vocab.nerc.ac.uk/collection/L05/current/382"/>
	<skos:broader rdf:resource="http://vocab.nerc.ac.uk/collection/L05/current/POS03"/>
	<skos:altLabel xml:lang="en">Battele pCO2</skos:altLabel>
	<skos:hiddenLabel xml:lang="en">Battelle Seaology pCO2 monitoring system</skos:hiddenLabel>
</rdf:Description>

<rdf:Description rdf:about="http://vocab.nerc.ac.uk/collection/L22/current/TOOL0879/">
	<rdf:type rdf:resource="http://www.w3.org/2000/01/rdf-schema#Resource"/>
	<rdfs:label xml:lang="en">WETLabs ECO-NTU turbidity sensor</rdfs:label>
	<owl:deprecated rdf:datatype="http://www.w3.org/2001/XMLSchema#boolean">true</owl:deprecated>
	<dcterms:isReplacedBy rdf:resource="http://vocab.nerc.ac.uk/collection/L22/current/TOOL0879"/>
</rdf:Description>

<rdf:Description rdf:about="http://vocab.nerc.ac.uk/collection/L22/current/TOOL0879">
	<rdf:type rdf:resource="http://www.w3.org/2000/01/rdf-schema#Resource"/>
	<rdf:type rdf:resource="http://www.w3.org/2004/02/skos/core#Concept"/>
	<dcterms:created rdf:datatype="http://www.w3.org/2001/XMLSchema#dateTime">2015-06-03T00:00:00Z</dcterms:created>
	<dc:publisher rdf:datatype="http://www.w3.org/2001/XMLSchema#string">British Oceanographic Data Centre (BODC)</dc:publisher>
	<skos:definition xml:lang="en">The ECO-NTU uses optical scattering at 700m to measure turbidity over the range 0-125 NTU (nephelometric turbidity units), with a sensitivity of 0.02 NTU or a range of 0-1000 NTU at a sensitivity of 0.12 NTU. The instrument is stable over a temperature range of 0-30 degC.   It has an analog signal output and a depth ratting of 600 m (300 m if the optional bio-wiper is fitted).</skos:definition>
	<skos:inScheme rdf:resource="http://vocab.aodn.org.au/def/instrument/1"/>
	<skos:prefLabel xml:lang="en">WETLabs ECO-NTU turbidity sensor</skos:prefLabel>
	<skos:broader rdf:resource="http://vocab.nerc.ac.uk/collection/L05/current/123"/>
	<skos:altLabel xml:lang="en">WETLabs ECO-NTU turbidity</skos:altLabel>
</rdf:Description>

<rdf:Description rdf:about="http://vocab.nerc.ac.uk/collection/L22/current/TOOL0888/">
	<rdf:type rdf:resource="http://www.w3.org/2000/01/rdf-schema#Resource"/>
	<rdfs:label xml:lang="en">Nortek Aquadopp Doppler current pro...</rdfs:label>
	<owl:deprecated rdf:datatype="http://www.w3.org/2001/XMLSchema#boolean">true</owl:deprecated>
	<dcterms:isReplacedBy rdf:resource="http://vocab.nerc.ac.uk/collection/L22/current/TOOL0888"/>
</rdf:Description>

<rdf:Description rdf:about="http://vocab.nerc.ac.uk/collection/L22/current/TOOL0888">
	<rdf:type rdf:resource="http://www.w3.org/2000/01/rdf-schema#Resource"/>
	<rdf:type rdf:resource="http://www.w3.org/2004/02/skos/core#Concept"/>
	<dcterms:contributor rdf:resource="http://editor.vocabs.ands.org.au/user/Natalia_Atkins"/>
	<dcterms:created rdf:datatype="http://www.w3.org/2001/XMLSchema#dateTime">2015-06-03T00:00:00Z</dcterms:created>
	<dcterms:modified rdf:datatype="http://www.w3.org/2001/XMLSchema#dateTime">2015-07-01T02:07:35Z</dcterms:modified>
	<dc:publisher rdf:datatype="http://www.w3.org/2001/XMLSchema#string">British Oceanographic Data Centre (BODC)</dc:publisher>
	<skos:definition xml:lang="en">A family of self-contained Doppler current profilers designed for deployment on the seabed, moorings, buoys or fixed structures.  A range of transducers - 400 kHz (60-90m range: 2-8m cell size), 600 kHz (30-40m range: 1-4m cell size), Z-cell 600 kHz, 1 MHz (12-20m range: 0.3-4m cell size), Z-cell 1MHz, 2 MHz (4-10m range:0.1-2m cell size) and side-looking.  Each transducer has 3 beams and the instrument has a maximum of 128 cells. Current speeds up to 10 m/s may be measured at an accuracy of 1% of measured value ±0.5cm/s. The standard depth rating is 300 m with 3000 m or 600m versions available. Temperature (embedded thermistor with 0.1C accuracy and 0.01C resolution), compass (magnetometer with 2 degrees accuracy and 0.1 degree resolution providing tilt less than 20 degrees), tilt (liquid level with 0.2 degree accuracy and 0.1 degree resolution) and pressure (piezo resistive with accuracy of 0.5% full scale - usually 100m - and resolution of 0.005% full scale) sensors are provided as standard.</skos:definition>
	<skos:inScheme rdf:resource="http://vocab.aodn.org.au/def/instrument/1"/>
	<skos:prefLabel xml:lang="en">Nortek Aquadopp Doppler current profiler</skos:prefLabel>
	<skos:broader rdf:resource="http://vocab.nerc.ac.uk/collection/L05/current/115"/>
	<skos:broader rdf:resource="http://vocab.nerc.ac.uk/collection/L05/current/134"/>
	<skos:altLabel xml:lang="en">Aquadopp profiler</skos:altLabel>
</rdf:Description>

<rdf:Description rdf:about="http://vocab.nerc.ac.uk/collection/L22/current/TOOL0898/">
	<rdf:type rdf:resource="http://www.w3.org/2000/01/rdf-schema#Resource"/>
	<rdfs:label xml:lang="en">Nortek acoustic wave and current pr...</rdfs:label>
	<owl:deprecated rdf:datatype="http://www.w3.org/2001/XMLSchema#boolean">true</owl:deprecated>
	<dcterms:isReplacedBy rdf:resource="http://vocab.nerc.ac.uk/collection/L22/current/TOOL0898"/>
</rdf:Description>

<rdf:Description rdf:about="http://vocab.nerc.ac.uk/collection/L22/current/TOOL0898">
	<rdf:type rdf:resource="http://www.w3.org/2000/01/rdf-schema#Resource"/>
	<rdf:type rdf:resource="http://www.w3.org/2004/02/skos/core#Concept"/>
	<dcterms:contributor rdf:resource="http://editor.vocabs.ands.org.au/user/Natalia_Atkins"/>
	<dcterms:created rdf:datatype="http://www.w3.org/2001/XMLSchema#dateTime">2015-06-03T00:00:00Z</dcterms:created>
	<dcterms:modified rdf:datatype="http://www.w3.org/2001/XMLSchema#dateTime">2015-06-30T06:19:13Z</dcterms:modified>
	<dc:publisher rdf:datatype="http://www.w3.org/2001/XMLSchema#string">British Oceanographic Data Centre (BODC)</dc:publisher>
	<skos:definition xml:lang="en">A family of instruments that simultaneously measure current profiles and wave height and direction designed for coastal monitoring.  It is available in three transmit frequencies: 1 MHz (range 30 m, cell size 0.25-4 m); 600 kHz (range 50 m, cell size 0.5-8 m), 400 kHz (range 100 m, cell size 1-8 m) and has  four beams, one vertical and the other three 120 degrees apart slanted at 25 degrees. Maximum number of cells is 128. Current speeds up to 10 m/s may be measured at an accuracy of 1% of measured value ±0.5cm/s. Temperature (embedded thermistor with 0.1C accuracy and 0.01C resolution), compass (magnetometer with 2 degrees accuracy and 0.1 degree resolution providing tilt less than 15 degrees), tilt (liquid level) and pressure (piezo resistive with accuracy of 0.5% (optional 0.1%) full scale - usually 100m - and resolution of 0.005% full scale) sensors are provided as standard.</skos:definition>
	<skos:inScheme rdf:resource="http://vocab.aodn.org.au/def/instrument/1"/>
	<skos:prefLabel xml:lang="en">Nortek acoustic wave and current profiler</skos:prefLabel>
	<skos:broader rdf:resource="http://vocab.nerc.ac.uk/collection/L05/current/110"/>
	<skos:broader rdf:resource="http://vocab.nerc.ac.uk/collection/L05/current/115"/>
	<skos:broader rdf:resource="http://vocab.nerc.ac.uk/collection/L05/current/134"/>
	<skos:altLabel xml:lang="en">Nortek AWAC</skos:altLabel>
</rdf:Description>

<rdf:Description rdf:about="http://vocab.nerc.ac.uk/collection/L22/current/TOOL0903/">
	<rdf:type rdf:resource="http://www.w3.org/2000/01/rdf-schema#Resource"/>
	<rdfs:label xml:lang="en">Nortek Continental 470 kHz Doppler ...</rdfs:label>
	<owl:deprecated rdf:datatype="http://www.w3.org/2001/XMLSchema#boolean">true</owl:deprecated>
	<dcterms:isReplacedBy rdf:resource="http://vocab.nerc.ac.uk/collection/L22/current/TOOL0903"/>
</rdf:Description>

<rdf:Description rdf:about="http://vocab.nerc.ac.uk/collection/L22/current/TOOL0903">
	<rdf:type rdf:resource="http://www.w3.org/2000/01/rdf-schema#Resource"/>
	<rdf:type rdf:resource="http://www.w3.org/2004/02/skos/core#Concept"/>
	<dcterms:contributor rdf:resource="http://editor.vocabs.ands.org.au/user/eMII_Atkins.Natalia"/>
	<dcterms:created rdf:datatype="http://www.w3.org/2001/XMLSchema#dateTime">2015-07-31T00:00:00Z</dcterms:created>
	<dcterms:modified rdf:datatype="http://www.w3.org/2001/XMLSchema#dateTime">2017-03-23T04:59:20Z</dcterms:modified>
	<dc:publisher rdf:datatype="http://www.w3.org/2001/XMLSchema#string">British Oceanographic Data Centre (BODC)</dc:publisher>
	<skos:definition xml:lang="en">A self-contained 470 kHz Doppler current profiler designed for deployment on the seabed, moorings, buoys or fixed structures in applications where range beyond the Aquadopp's capability is required.  The transducer has 3 beams for vertical operation or 2 beams for horizontal operation. Range is 100m and cell sizes may be from 1 to 10m with a maximum of 128 cells. Current speeds up to 10 m/s may be measured at an accuracy of 1% of measured value. The standard depth rating is 500 m. Temperature (embedded thermistor with 0.1C accuracy and 0.01C resolution), compass (magnetometer with 2 degrees accuracy and 0.1 degree resolution providing tilt less than 20 degrees), tilt (liquid level with 0.2 degree accuracy and 0.1 degree resolution) and pressure (piezo resistive with accuracy of 0.5% full scale - usually 500m - and resolution of 0.005% full scale) sensors are provided as standard.</skos:definition>
	<skos:inScheme rdf:resource="http://vocab.aodn.org.au/def/instrument/1"/>
	<skos:prefLabel xml:lang="en">Nortek Continental 470 kHz Doppler current profiler</skos:prefLabel>
	<skos:broader rdf:resource="http://vocab.nerc.ac.uk/collection/L22/current/TOOL0905"/>
	<skos:altLabel xml:lang="en">Continental 470 kHz profiler</skos:altLabel>
</rdf:Description>

<rdf:Description rdf:about="http://vocab.nerc.ac.uk/collection/L22/current/TOOL0904/">
	<rdf:type rdf:resource="http://www.w3.org/2000/01/rdf-schema#Resource"/>
	<rdfs:label xml:lang="en">Nortek Continental 190 kHz Doppler ...</rdfs:label>
	<owl:deprecated rdf:datatype="http://www.w3.org/2001/XMLSchema#boolean">true</owl:deprecated>
	<dcterms:isReplacedBy rdf:resource="http://vocab.nerc.ac.uk/collection/L22/current/TOOL0904"/>
</rdf:Description>

<rdf:Description rdf:about="http://vocab.nerc.ac.uk/collection/L22/current/TOOL0904">
	<rdf:type rdf:resource="http://www.w3.org/2000/01/rdf-schema#Resource"/>
	<rdf:type rdf:resource="http://www.w3.org/2004/02/skos/core#Concept"/>
	<dcterms:contributor rdf:resource="http://editor.vocabs.ands.org.au/user/eMII_Atkins.Natalia"/>
	<dcterms:created rdf:datatype="http://www.w3.org/2001/XMLSchema#dateTime">2015-07-31T00:00:00Z</dcterms:created>
	<dcterms:modified rdf:datatype="http://www.w3.org/2001/XMLSchema#dateTime">2017-03-23T04:59:24Z</dcterms:modified>
	<dc:publisher rdf:datatype="http://www.w3.org/2001/XMLSchema#string">British Oceanographic Data Centre (BODC)</dc:publisher>
	<skos:definition xml:lang="en">A self-contained 190 kHz Doppler current profiler designed for deployment on the seabed, moorings, buoys or fixed structures in applications where range beyond the Aquadopp's capability is required.  The transducer has 3 beams for vertical operation or 2 beams for horizontal operation. Range is 200m and cell sizes may be from 2 to 20m with a maximum of 128 cells. Current speeds up to 10 m/s may be measured at an accuracy of 1 percent of measured value. The standard depth rating is 500 m. Temperature (embedded thermistor with 0.1C accuracy and 0.01C resolution), compass (magnetometer with 2 degrees accuracy and 0.1 degree resolution providing tilt less than 20 degrees), tilt (liquid level with 0.2 degree accuracy and 0.1 degree resolution) and pressure (piezo resistive with accuracy of 0.5 percent full scale - usually 500m - and resolution of 0.005 percent full scale) sensors are provided as standard.</skos:definition>
	<skos:inScheme rdf:resource="http://vocab.aodn.org.au/def/instrument/1"/>
	<skos:prefLabel xml:lang="en">Nortek Continental 190 kHz Doppler current profiler</skos:prefLabel>
	<skos:broader rdf:resource="http://vocab.nerc.ac.uk/collection/L22/current/TOOL0905"/>
	<skos:altLabel xml:lang="en">Continental 190 kHz profiler</skos:altLabel>
</rdf:Description>

<rdf:Description rdf:about="http://vocab.nerc.ac.uk/collection/L22/current/TOOL0905/">
	<rdf:type rdf:resource="http://www.w3.org/2000/01/rdf-schema#Resource"/>
	<rdfs:label xml:lang="en">Nortek Continental Doppler current ...</rdfs:label>
	<owl:deprecated rdf:datatype="http://www.w3.org/2001/XMLSchema#boolean">true</owl:deprecated>
	<dcterms:isReplacedBy rdf:resource="http://vocab.nerc.ac.uk/collection/L22/current/TOOL0905"/>
</rdf:Description>

<rdf:Description rdf:about="http://vocab.nerc.ac.uk/collection/L22/current/TOOL0905">
	<rdf:type rdf:resource="http://www.w3.org/2000/01/rdf-schema#Resource"/>
	<rdf:type rdf:resource="http://www.w3.org/2004/02/skos/core#Concept"/>
	<dcterms:contributor rdf:resource="http://editor.vocabs.ands.org.au/user/Natalia_Atkins"/>
	<dcterms:created rdf:datatype="http://www.w3.org/2001/XMLSchema#dateTime">2015-07-31T00:00:00Z</dcterms:created>
	<dcterms:modified rdf:datatype="http://www.w3.org/2001/XMLSchema#dateTime">2015-07-31T03:20:39Z</dcterms:modified>
	<dc:publisher rdf:datatype="http://www.w3.org/2001/XMLSchema#string">British Oceanographic Data Centre (BODC)</dc:publisher>
	<skos:definition xml:lang="en">A family of self-contained Doppler current profilers designed for deployment on the seabed, moorings, buoys or fixed structures in applications where range beyond the Aquadopp's capability is required.  There are two transducer options - 190 kHz (200m range: 2-20m cell size) and 470 kHz (100m range: 1-10m cell size).  Each transducer has 3 beams for vertical operation or 2 beams for horizontal operation and the instrument has a maximum of 128 cells. Current speeds up to 10 m/s may be measured at an accuracy of 1% of measured value. The standard depth rating is 500 m. Temperature (embedded thermistor with 0.1C accuracy and 0.01C resolution), compass (magnetometer with 2 degrees accuracy and 0.1 degree resolution providing tilt less than 20 degrees), tilt (liquid level with 0.2 degree accuracy and 0.1 degree resolution) and pressure (piezo resistive with accuracy of 0.5 percent full scale - usually 500m - and resolution of 0.005 percent] full scale) sensors are provided as standard.</skos:definition>
	<skos:inScheme rdf:resource="http://vocab.aodn.org.au/def/instrument/1"/>
	<skos:narrower rdf:resource="http://vocab.nerc.ac.uk/collection/L22/current/TOOL0903"/>
	<skos:narrower rdf:resource="http://vocab.nerc.ac.uk/collection/L22/current/TOOL0904"/>
	<skos:prefLabel xml:lang="en">Nortek Continental Doppler current profiler</skos:prefLabel>
	<skos:broader rdf:resource="http://vocab.nerc.ac.uk/collection/L05/current/115"/>
	<skos:broader rdf:resource="http://vocab.nerc.ac.uk/collection/L05/current/134"/>
	<skos:altLabel xml:lang="en">Continental profiler</skos:altLabel>
</rdf:Description>

<rdf:Description rdf:about="http://vocab.nerc.ac.uk/collection/L22/current/TOOL0906/">
	<rdf:type rdf:resource="http://www.w3.org/2000/01/rdf-schema#Resource"/>
	<rdfs:label xml:lang="en">Measurement Engineering Australia S...</rdfs:label>
	<owl:deprecated rdf:datatype="http://www.w3.org/2001/XMLSchema#boolean">true</owl:deprecated>
	<dcterms:isReplacedBy rdf:resource="http://vocab.nerc.ac.uk/collection/L22/current/TOOL0906"/>
</rdf:Description>

<rdf:Description rdf:about="http://vocab.nerc.ac.uk/collection/L22/current/TOOL0906">
	<rdf:type rdf:resource="http://www.w3.org/2000/01/rdf-schema#Resource"/>
	<rdf:type rdf:resource="http://www.w3.org/2004/02/skos/core#Concept"/>
	<dcterms:created rdf:datatype="http://www.w3.org/2001/XMLSchema#dateTime">2015-07-30T00:00:00Z</dcterms:created>
	<dc:publisher rdf:datatype="http://www.w3.org/2001/XMLSchema#string">British Oceanographic Data Centre (BODC)</dc:publisher>
	<skos:definition xml:lang="en">A CMOS chip containing a thermistor temperature sensor together with bias circuitry and an analogue to digital converter capable of delivering digital temperature measurements in engineering units down a single-wire bus. The sensors have a measurement range from -17 to +33 C, are accurate to 0.02 C, are matched to within 0.006 C and have a resolution of 0.001 C.  The sensors may be deployed singly or built into thermistor chains.</skos:definition>
	<skos:inScheme rdf:resource="http://vocab.aodn.org.au/def/instrument/1"/>
	<skos:prefLabel xml:lang="en">Measurement Engineering Australia SDI-12 temperature sensor</skos:prefLabel>
	<skos:broader rdf:resource="http://vocab.nerc.ac.uk/collection/L05/current/134"/>
	<skos:altLabel xml:lang="en">MEA SDI-12 TS</skos:altLabel>
</rdf:Description>

<rdf:Description rdf:about="http://vocab.nerc.ac.uk/collection/L22/current/TOOL0907/">
	<rdf:type rdf:resource="http://www.w3.org/2000/01/rdf-schema#Resource"/>
	<rdfs:label xml:lang="en">Omega ON-950 44005 thermistor</rdfs:label>
	<owl:deprecated rdf:datatype="http://www.w3.org/2001/XMLSchema#boolean">true</owl:deprecated>
	<dcterms:isReplacedBy rdf:resource="http://vocab.nerc.ac.uk/collection/L22/current/TOOL0907"/>
</rdf:Description>

<rdf:Description rdf:about="http://vocab.nerc.ac.uk/collection/L22/current/TOOL0907">
	<rdf:type rdf:resource="http://www.w3.org/2000/01/rdf-schema#Resource"/>
	<rdf:type rdf:resource="http://www.w3.org/2004/02/skos/core#Concept"/>
	<dcterms:created rdf:datatype="http://www.w3.org/2001/XMLSchema#dateTime">2015-07-30T00:00:00Z</dcterms:created>
	<dc:publisher rdf:datatype="http://www.w3.org/2001/XMLSchema#string">British Oceanographic Data Centre (BODC)</dc:publisher>
	<skos:definition xml:lang="en">A precision thermistor in a small SST housing with a #8-32 stud (ON-950 mounting). The bare thermistor (model 44005) has a base resistance of 3000 Ohms and a resistance change of 42 Ohms per 50 C.</skos:definition>
	<skos:inScheme rdf:resource="http://vocab.aodn.org.au/def/instrument/1"/>
	<skos:prefLabel xml:lang="en">Omega ON-950 44005 thermistor</skos:prefLabel>
	<skos:broader rdf:resource="http://vocab.nerc.ac.uk/collection/L05/current/134"/>
	<skos:altLabel xml:lang="en">ON-950 44005 thermistor</skos:altLabel>
</rdf:Description>

<rdf:Description rdf:about="http://vocab.nerc.ac.uk/collection/L22/current/TOOL0916/">
	<rdf:type rdf:resource="http://www.w3.org/2000/01/rdf-schema#Resource"/>
	<rdfs:label xml:lang="en">Imagenex 837B "Delta T" 1000m multi...</rdfs:label>
	<owl:deprecated rdf:datatype="http://www.w3.org/2001/XMLSchema#boolean">true</owl:deprecated>
	<dcterms:isReplacedBy rdf:resource="http://vocab.nerc.ac.uk/collection/L22/current/TOOL0916"/>
</rdf:Description>

<rdf:Description rdf:about="http://vocab.nerc.ac.uk/collection/L22/current/TOOL0916">
	<rdf:type rdf:resource="http://www.w3.org/2000/01/rdf-schema#Resource"/>
	<rdf:type rdf:resource="http://www.w3.org/2004/02/skos/core#Concept"/>
	<dcterms:created rdf:datatype="http://www.w3.org/2001/XMLSchema#dateTime">2015-07-30T00:00:00Z</dcterms:created>
	<dc:publisher rdf:datatype="http://www.w3.org/2001/XMLSchema#string">British Oceanographic Data Centre (BODC)</dc:publisher>
	<skos:definition xml:lang="en">This is a 260 kHz multibeam imaging sonar with an aluminium or stainless steel case capable of operating at depths down to 1000 metres.  Depending on mode selected there are 120, 240 or 480 beams. The transducer beam width is 120 by 3 degrees for both transmit and receive.  The effective horizontal beam with is 3 degrees (120 beams), 1.5 degrees (240 beams) or 0.75 degrees (480 beams). Minimum detectable range is 0.5m and the frame rate is up to 20 frames per second.</skos:definition>
	<skos:inScheme rdf:resource="http://vocab.aodn.org.au/def/instrument/1"/>
	<skos:prefLabel xml:lang="en">Imagenex 837B "Delta T" 1000m multibeam profiling sonar</skos:prefLabel>
	<skos:broader rdf:resource="http://vocab.nerc.ac.uk/collection/L05/current/157"/>
	<skos:altLabel xml:lang="en">Imagenex 837B "Delta T" sonar</skos:altLabel>
</rdf:Description>

<rdf:Description rdf:about="http://vocab.nerc.ac.uk/collection/L22/current/TOOL0917/">
	<rdf:type rdf:resource="http://www.w3.org/2000/01/rdf-schema#Resource"/>
	<rdfs:label xml:lang="en">Peterson Indented Rotating Sphere S...</rdfs:label>
	<owl:deprecated rdf:datatype="http://www.w3.org/2001/XMLSchema#boolean">true</owl:deprecated>
	<dcterms:isReplacedBy rdf:resource="http://vocab.nerc.ac.uk/collection/L22/current/TOOL0917"/>
</rdf:Description>

<rdf:Description rdf:about="http://vocab.nerc.ac.uk/collection/L22/current/TOOL0917">
	<rdf:type rdf:resource="http://www.w3.org/2000/01/rdf-schema#Resource"/>
	<rdf:type rdf:resource="http://www.w3.org/2004/02/skos/core#Concept"/>
	<dcterms:created rdf:datatype="http://www.w3.org/2001/XMLSchema#dateTime">2015-07-30T00:00:00Z</dcterms:created>
	<dc:publisher rdf:datatype="http://www.w3.org/2001/XMLSchema#string">British Oceanographic Data Centre (BODC)</dc:publisher>
	<skos:definition xml:lang="en">This is a sediment trap designed to eliminate sediment flux sample contamination by free-swimming organisms using an indented rotating sphere (IRS) valve within the trap. The trap has three components: a particle accumulator, the IRS valve and a sample accumulator. The particle collector is either cylindrical with a diameter of 15-17cm or conical with a 70cm mouth. The IRS valve comprises an acrylic outer cylinder, a slightly smaller diameter PVC sphere with small indentations over part of its surface and a sealing collar. The sphere is periodically (an hour to a day depending sedimentation rates) slowly (1 rpm) rotated on an axis perpendicular to the vertical axis of the cylinder transferring material accumulated in its surface indentations to the sample accumulator. The sample accumulator is either a central funnel feeding a single cup or a skewed funnel feeding multiple cups on a carousel. The trap is deployed closed with a buoyant lid held in place by a burn wire to prevent contamination.</skos:definition>
	<skos:inScheme rdf:resource="http://vocab.aodn.org.au/def/instrument/1"/>
	<skos:prefLabel xml:lang="en">Peterson Indented Rotating Sphere Sediment Trap</skos:prefLabel>
	<skos:broader rdf:resource="http://vocab.nerc.ac.uk/collection/L05/current/33"/>
	<skos:altLabel xml:lang="en">Peterson IRS Trap</skos:altLabel>
</rdf:Description>

<rdf:Description rdf:about="http://vocab.nerc.ac.uk/collection/L22/current/TOOL0918/">
	<rdf:type rdf:resource="http://www.w3.org/2000/01/rdf-schema#Resource"/>
	<rdfs:label xml:lang="en">Alec Electronics MDS-MkV/L light in...</rdfs:label>
	<owl:deprecated rdf:datatype="http://www.w3.org/2001/XMLSchema#boolean">true</owl:deprecated>
	<dcterms:isReplacedBy rdf:resource="http://vocab.nerc.ac.uk/collection/L22/current/TOOL0918"/>
</rdf:Description>

<rdf:Description rdf:about="http://vocab.nerc.ac.uk/collection/L22/current/TOOL0918">
	<rdf:type rdf:resource="http://www.w3.org/2000/01/rdf-schema#Resource"/>
	<rdf:type rdf:resource="http://www.w3.org/2004/02/skos/core#Concept"/>
	<dcterms:created rdf:datatype="http://www.w3.org/2001/XMLSchema#dateTime">2015-07-30T00:00:00Z</dcterms:created>
	<dc:publisher rdf:datatype="http://www.w3.org/2001/XMLSchema#string">British Oceanographic Data Centre (BODC)</dc:publisher>
	<skos:definition xml:lang="en">This is an ultra-miniature light meter less than 10cm long and 2cm in diameter with an approximately (due to a relatively large linkage to the body) spherical light collector and photodiode sensor. It can measure light intensities up to 2000 uMole/m2/s with an accuracy of 4% full-scale and a resolution of 1 uMole/m2/s.  No documentation can be found giving the spectral range of the sensor, but the approximate 4-pi geometry (measuring scalar irradiance) is usually associated with PAR wavelengths.</skos:definition>
	<skos:inScheme rdf:resource="http://vocab.aodn.org.au/def/instrument/1"/>
	<skos:prefLabel xml:lang="en">Alec Electronics MDS-MkV/L light intensity recorder</skos:prefLabel>
	<skos:broader rdf:resource="http://vocab.nerc.ac.uk/collection/L05/current/122"/>
	<skos:altLabel xml:lang="en">MDS-MkV/L light meter</skos:altLabel>
</rdf:Description>

<rdf:Description rdf:about="http://vocab.nerc.ac.uk/collection/L22/current/TOOL0929/">
	<rdf:type rdf:resource="http://www.w3.org/2000/01/rdf-schema#Resource"/>
	<rdfs:label xml:lang="en">Biotrack MK3 geolocator tags</rdfs:label>
	<owl:deprecated rdf:datatype="http://www.w3.org/2001/XMLSchema#boolean">true</owl:deprecated>
	<dcterms:isReplacedBy rdf:resource="http://vocab.nerc.ac.uk/collection/L22/current/TOOL0929"/>
</rdf:Description>

<rdf:Description rdf:about="http://vocab.nerc.ac.uk/collection/L22/current/TOOL0929">
	<rdf:type rdf:resource="http://www.w3.org/2000/01/rdf-schema#Resource"/>
	<rdf:type rdf:resource="http://www.w3.org/2004/02/skos/core#Concept"/>
	<dcterms:created rdf:datatype="http://www.w3.org/2001/XMLSchema#dateTime">2015-08-07T00:00:00Z</dcterms:created>
	<dc:publisher rdf:datatype="http://www.w3.org/2001/XMLSchema#string">British Oceanographic Data Centre (BODC)</dc:publisher>
	<skos:definition xml:lang="en">A family of tags designed for tracking animal movements over long periods based on measurement of light levels at dawn and dusk.  The tags also measure temperature and whether they are wet or dry. Geolocator accuracy is of the order of 150km. Tags must be recovered for data download. The MK3 family weigh 2.5 grams and are designed to be attached to deep-diving and larger water birds. Tags in this family were developed by British Antarctic Survey and are produced under licence by Biotrack: the BAS MK19 as the Biotrack MK3005 and the BAS MK16 as the Biotrack MK3006.</skos:definition>
	<skos:inScheme rdf:resource="http://vocab.aodn.org.au/def/instrument/1"/>
	<skos:prefLabel xml:lang="en">Biotrack MK3 geolocator tags</skos:prefLabel>
	<skos:broader rdf:resource="http://vocab.nerc.ac.uk/collection/L05/current/TRTG"/>
	<skos:altLabel xml:lang="en">MK3 GLS tags</skos:altLabel>
</rdf:Description>

<rdf:Description rdf:about="http://vocab.nerc.ac.uk/collection/L22/current/TOOL0930/">
	<rdf:type rdf:resource="http://www.w3.org/2000/01/rdf-schema#Resource"/>
	<rdfs:label xml:lang="en">Everest Interscience Sea-Therm 4000...</rdfs:label>
	<owl:deprecated rdf:datatype="http://www.w3.org/2001/XMLSchema#boolean">true</owl:deprecated>
	<dcterms:isReplacedBy rdf:resource="http://vocab.nerc.ac.uk/collection/L22/current/TOOL0930"/>
</rdf:Description>

<rdf:Description rdf:about="http://vocab.nerc.ac.uk/collection/L22/current/TOOL0930">
	<rdf:type rdf:resource="http://www.w3.org/2000/01/rdf-schema#Resource"/>
	<rdf:type rdf:resource="http://www.w3.org/2004/02/skos/core#Concept"/>
	<dcterms:created rdf:datatype="http://www.w3.org/2001/XMLSchema#dateTime">2015-08-07T00:00:00Z</dcterms:created>
	<dc:publisher rdf:datatype="http://www.w3.org/2001/XMLSchema#string">British Oceanographic Data Centre (BODC)</dc:publisher>
	<skos:definition xml:lang="en">A rugged temperature sensor designed to measure water surface temperature in harsh environments such as oil platforms. It is a non-contact system that measures infra-red radiation with a second senor - the Sky Spy - that provides input for sky radiation correction. It measures temperatures in the range -10-70C with an accuracy of 0.3C below 30C and 0.5C above 30C. The standard field of view is 10 degrees with 5 and 2 degrees available as options. The sensor is encased in a solid block of plastic hermetically sealed into a titanium case to provide waterproofing and resistance to salt spray.</skos:definition>
	<skos:inScheme rdf:resource="http://vocab.aodn.org.au/def/instrument/1"/>
	<skos:prefLabel xml:lang="en">Everest Interscience Sea-Therm 4000L temperature sensor</skos:prefLabel>
	<skos:broader rdf:resource="http://vocab.nerc.ac.uk/collection/L05/current/302"/>
	<skos:altLabel xml:lang="en">Sea-Therm 4000L TS</skos:altLabel>
</rdf:Description>

<rdf:Description rdf:about="http://vocab.nerc.ac.uk/collection/L22/current/TOOL0931/">
	<rdf:type rdf:resource="http://www.w3.org/2000/01/rdf-schema#Resource"/>
	<rdfs:label xml:lang="en">Paroscientific Digiquartz depth sen...</rdfs:label>
	<owl:deprecated rdf:datatype="http://www.w3.org/2001/XMLSchema#boolean">true</owl:deprecated>
	<dcterms:isReplacedBy rdf:resource="http://vocab.nerc.ac.uk/collection/L22/current/TOOL0931"/>
</rdf:Description>

<rdf:Description rdf:about="http://vocab.nerc.ac.uk/collection/L22/current/TOOL0931">
	<rdf:type rdf:resource="http://www.w3.org/2000/01/rdf-schema#Resource"/>
	<rdf:type rdf:resource="http://www.w3.org/2004/02/skos/core#Concept"/>
	<dcterms:created rdf:datatype="http://www.w3.org/2001/XMLSchema#dateTime">2015-08-07T00:00:00Z</dcterms:created>
	<dc:publisher rdf:datatype="http://www.w3.org/2001/XMLSchema#string">British Oceanographic Data Centre (BODC)</dc:publisher>
	<skos:definition xml:lang="en">A family of encapsulated pressure sensors based on Paroscientific patented technology that determines pressure by measuring the oscillating frequency of a quartz crystal resonator. They are available in depth ranges of 10-140m, 10-700m, 0-700m and 1400-7000m with accuracy of 0.01% full scale or 0.02% full scale for miniature sensors.</skos:definition>
	<skos:inScheme rdf:resource="http://vocab.aodn.org.au/def/instrument/1"/>
	<skos:prefLabel xml:lang="en">Paroscientific Digiquartz depth sensors</skos:prefLabel>
	<skos:broader rdf:resource="http://vocab.nerc.ac.uk/collection/L05/current/WPS"/>
	<skos:altLabel xml:lang="en">Digiquartz PS</skos:altLabel>
</rdf:Description>

<rdf:Description rdf:about="http://vocab.nerc.ac.uk/collection/L22/current/TOOL0932/">
	<rdf:type rdf:resource="http://www.w3.org/2000/01/rdf-schema#Resource"/>
	<rdfs:label xml:lang="en">Eppley UVB-1 pyranometer</rdfs:label>
	<owl:deprecated rdf:datatype="http://www.w3.org/2001/XMLSchema#boolean">true</owl:deprecated>
	<dcterms:isReplacedBy rdf:resource="http://vocab.nerc.ac.uk/collection/L22/current/TOOL0932"/>
</rdf:Description>

<rdf:Description rdf:about="http://vocab.nerc.ac.uk/collection/L22/current/TOOL0932">
	<rdf:type rdf:resource="http://www.w3.org/2000/01/rdf-schema#Resource"/>
	<rdf:type rdf:resource="http://www.w3.org/2004/02/skos/core#Concept"/>
	<dcterms:created rdf:datatype="http://www.w3.org/2001/XMLSchema#dateTime">2015-08-07T00:00:00Z</dcterms:created>
	<dc:publisher rdf:datatype="http://www.w3.org/2001/XMLSchema#string">British Oceanographic Data Centre (BODC)</dc:publisher>
	<skos:definition xml:lang="en">A precision radiometer that measures biologically effective solar UV radiation  with a spectral response of 280-320nm. Coloured filters and a UV-B phosphor convert incoming UV-B radiation into green light which is then measured by a calibrated solid-state photodetector. The UVB-1 measures global solar UV-B irradiance or the power per unit area of UV-B radiation received by a horizontal surface from the entire hemisphere of the sky. Global radiation includes both light transmitted directly through the atmosphere and light scattered by atmospheric gases and particulate matter in the atmosphere. The UVB-1 measures both the direct and diffuse components of global radiation.  Cosine response is ±5% for 0 - 60 degree solar zenith angle and sensitivity is 1.97 volt/(watt/m2) of total UV-B irradiance.</skos:definition>
	<skos:inScheme rdf:resource="http://vocab.aodn.org.au/def/instrument/1"/>
	<skos:prefLabel xml:lang="en">Eppley UVB-1 pyranometer</skos:prefLabel>
	<skos:broader rdf:resource="http://vocab.nerc.ac.uk/collection/L05/current/122"/>
	<skos:altLabel xml:lang="en">UVB-1 pyranometer</skos:altLabel>
</rdf:Description>

<rdf:Description rdf:about="http://vocab.nerc.ac.uk/collection/L22/current/TOOL0939/">
	<rdf:type rdf:resource="http://www.w3.org/2000/01/rdf-schema#Resource"/>
	<rdfs:label xml:lang="en">McLane RAS-500 remote-access sample...</rdfs:label>
	<owl:deprecated rdf:datatype="http://www.w3.org/2001/XMLSchema#boolean">true</owl:deprecated>
	<dcterms:isReplacedBy rdf:resource="http://vocab.nerc.ac.uk/collection/L22/current/TOOL0939"/>
</rdf:Description>

<rdf:Description rdf:about="http://vocab.nerc.ac.uk/collection/L22/current/TOOL0939">
	<rdf:type rdf:resource="http://www.w3.org/2000/01/rdf-schema#Resource"/>
	<rdf:type rdf:resource="http://www.w3.org/2004/02/skos/core#Concept"/>
	<dcterms:created rdf:datatype="http://www.w3.org/2001/XMLSchema#dateTime">2015-09-02T00:00:00Z</dcterms:created>
	<dc:publisher rdf:datatype="http://www.w3.org/2001/XMLSchema#string">British Oceanographic Data Centre (BODC)</dc:publisher>
	<skos:definition xml:lang="en">A deep water or coastal time series water sampler that collects samples for biological, dissolved major and minor nutrient, dissolved trace metal, or dissolved organic carbon analyses. It collects 48 500ml samples of ambient water and suspended material in Tedlar bags, isolating the samples for subsequent laboratory analysis following a user defined sampling schedule. RAS systems can optionally be fitted with in-line pre-filters and an external temperature sensor. Deployment data with a report of sample event conditions is stored to non-volatile EEPROM. Further information is available at http://www.mclanelabs.com/master_page/product-type/samplers/remote-access-sampler.</skos:definition>
	<skos:inScheme rdf:resource="http://vocab.aodn.org.au/def/instrument/1"/>
	<skos:prefLabel xml:lang="en">McLane RAS-500 remote-access sampler</skos:prefLabel>
	<skos:broader rdf:resource="http://vocab.nerc.ac.uk/collection/L05/current/30"/>
	<skos:altLabel xml:lang="en">McLane RAS-500 sampler</skos:altLabel>
</rdf:Description>

<rdf:Description rdf:about="http://vocab.aodn.org.au/def/instrument/1">
	<rdf:type rdf:resource="http://www.w3.org/2000/01/rdf-schema#Resource"/>
	<rdf:type rdf:resource="http://www.w3.org/2004/02/skos/core#ConceptScheme"/>
	<dc:rights rdf:datatype="http://www.w3.org/2001/XMLSchema#string">Freely Available For Reuse</dc:rights>
	<dcterms:contributor rdf:resource="http://editor.vocabs.ands.org.au/user/eMII_Finney.Kim_Admin"/>
	<dcterms:created rdf:datatype="http://www.w3.org/2001/XMLSchema#dateTime">2012-12-10T00:00:00Z</dcterms:created>
	<dcterms:creator rdf:resource="http://editor.vocabs.ands.org.au/user/Sebastien-Mancini"/>
	<dcterms:description xml:lang="en">A controlled vocabulary for instruments that can be used to populate Marine Community Profile metadata. The vocabulary will be used by the faceted search facility in the AODN/IMOS Portal 1-2-3.</dcterms:description>
	<dcterms:identifier xml:lang="en">entity</dcterms:identifier>
	<dcterms:modified rdf:datatype="http://www.w3.org/2001/XMLSchema#dateTime">2017-03-22T04:21:52Z</dcterms:modified>
	<dcterms:publisher rdf:resource="http://editor.vocabs.ands.org.au/user/eMarine-Information-Infrastructure-eMII"/>
	<dcterms:subject xml:lang="en">instrument</dcterms:subject>
	<dcterms:title xml:lang="en">AODN Instrument Vocabulary</dcterms:title>
	<identifier xmlns="http://schema.semantic-web.at/ppt/" rdf:datatype="http://www.w3.org/2001/XMLSchema#string">entity</identifier>
	<settingIdentifier xmlns="http://schema.semantic-web.at/ppt/urigen#" rdf:datatype="http://www.w3.org/2001/XMLSchema#string">instrument/entity</settingIdentifier>
	<skos:hasTopConcept rdf:resource="http://vocab.nerc.ac.uk/collection/L05/current/302"/>
	<skos:hasTopConcept rdf:resource="http://vocab.nerc.ac.uk/collection/L05/current/TRTG"/>
	<skos:hasTopConcept rdf:resource="http://vocab.aodn.org.au/def/instrument/entity/361"/>
	<skos:hasTopConcept rdf:resource="http://vocab.aodn.org.au/def/instrument/entity/363"/>
	<skos:hasTopConcept rdf:resource="http://vocab.aodn.org.au/def/instrument/entity/365"/>
	<skos:hasTopConcept rdf:resource="http://vocab.nerc.ac.uk/collection/L05/current/101"/>
	<skos:hasTopConcept rdf:resource="http://vocab.nerc.ac.uk/collection/L05/current/102"/>
	<skos:hasTopConcept rdf:resource="http://vocab.nerc.ac.uk/collection/L05/current/103"/>
	<skos:hasTopConcept rdf:resource="http://vocab.nerc.ac.uk/collection/L05/current/110"/>
	<skos:hasTopConcept rdf:resource="http://vocab.nerc.ac.uk/collection/L05/current/111"/>
	<skos:hasTopConcept rdf:resource="http://vocab.nerc.ac.uk/collection/L05/current/113"/>
	<skos:hasTopConcept rdf:resource="http://vocab.nerc.ac.uk/collection/L05/current/114"/>
	<skos:hasTopConcept rdf:resource="http://vocab.nerc.ac.uk/collection/L05/current/115"/>
	<skos:hasTopConcept rdf:resource="http://vocab.nerc.ac.uk/collection/L05/current/121"/>
	<skos:hasTopConcept rdf:resource="http://vocab.nerc.ac.uk/collection/L05/current/122"/>
	<skos:hasTopConcept rdf:resource="http://vocab.nerc.ac.uk/collection/L05/current/123"/>
	<skos:hasTopConcept rdf:resource="http://vocab.nerc.ac.uk/collection/L05/current/124"/>
	<skos:hasTopConcept rdf:resource="http://vocab.nerc.ac.uk/collection/L05/current/130"/>
	<skos:hasTopConcept rdf:resource="http://vocab.nerc.ac.uk/collection/L05/current/132"/>
	<skos:hasTopConcept rdf:resource="http://vocab.nerc.ac.uk/collection/L05/current/133"/>
	<skos:hasTopConcept rdf:resource="http://vocab.nerc.ac.uk/collection/L05/current/134"/>
	<skos:hasTopConcept rdf:resource="http://vocab.nerc.ac.uk/collection/L05/current/135"/>
	<skos:hasTopConcept rdf:resource="http://vocab.nerc.ac.uk/collection/L05/current/14"/>
	<skos:hasTopConcept rdf:resource="http://vocab.nerc.ac.uk/collection/L05/current/151"/>
	<skos:hasTopConcept rdf:resource="http://vocab.nerc.ac.uk/collection/L05/current/157"/>
	<skos:hasTopConcept rdf:resource="http://vocab.nerc.ac.uk/collection/L05/current/180"/>
	<skos:hasTopConcept rdf:resource="http://vocab.nerc.ac.uk/collection/L05/current/181"/>
	<skos:hasTopConcept rdf:resource="http://vocab.nerc.ac.uk/collection/L05/current/183"/>
	<skos:hasTopConcept rdf:resource="http://vocab.nerc.ac.uk/collection/L05/current/185"/>
	<skos:hasTopConcept rdf:resource="http://vocab.nerc.ac.uk/collection/L05/current/186"/>
	<skos:hasTopConcept rdf:resource="http://vocab.nerc.ac.uk/collection/L05/current/21"/>
	<skos:hasTopConcept rdf:resource="http://vocab.nerc.ac.uk/collection/L05/current/22"/>
	<skos:hasTopConcept rdf:resource="http://vocab.nerc.ac.uk/collection/L05/current/23"/>
	<skos:hasTopConcept rdf:resource="http://vocab.nerc.ac.uk/collection/L05/current/24"/>
	<skos:hasTopConcept rdf:resource="http://vocab.nerc.ac.uk/collection/L05/current/30"/>
	<skos:hasTopConcept rdf:resource="http://vocab.nerc.ac.uk/collection/L05/current/301"/>
	<skos:hasTopConcept rdf:resource="http://vocab.nerc.ac.uk/collection/L05/current/303"/>
	<skos:hasTopConcept rdf:resource="http://vocab.nerc.ac.uk/collection/L05/current/304"/>
	<skos:hasTopConcept rdf:resource="http://vocab.nerc.ac.uk/collection/L05/current/305"/>
	<skos:hasTopConcept rdf:resource="http://vocab.nerc.ac.uk/collection/L05/current/306"/>
	<skos:hasTopConcept rdf:resource="http://vocab.nerc.ac.uk/collection/L05/current/308"/>
	<skos:hasTopConcept rdf:resource="http://vocab.nerc.ac.uk/collection/L05/current/31"/>
	<skos:hasTopConcept rdf:resource="http://vocab.nerc.ac.uk/collection/L05/current/310"/>
	<skos:hasTopConcept rdf:resource="http://vocab.nerc.ac.uk/collection/L05/current/311"/>
	<skos:hasTopConcept rdf:resource="http://vocab.nerc.ac.uk/collection/L05/current/312"/>
	<skos:hasTopConcept rdf:resource="http://vocab.nerc.ac.uk/collection/L05/current/33"/>
	<skos:hasTopConcept rdf:resource="http://vocab.nerc.ac.uk/collection/L05/current/350"/>
	<skos:hasTopConcept rdf:resource="http://vocab.nerc.ac.uk/collection/L05/current/351"/>
	<skos:hasTopConcept rdf:resource="http://vocab.nerc.ac.uk/collection/L05/current/353"/>
	<skos:hasTopConcept rdf:resource="http://vocab.nerc.ac.uk/collection/L05/current/355"/>
	<skos:hasTopConcept rdf:resource="http://vocab.nerc.ac.uk/collection/L05/current/356"/>
	<skos:hasTopConcept rdf:resource="http://vocab.nerc.ac.uk/collection/L05/current/369"/>
	<skos:hasTopConcept rdf:resource="http://vocab.nerc.ac.uk/collection/L05/current/377"/>
	<skos:hasTopConcept rdf:resource="http://vocab.nerc.ac.uk/collection/L05/current/379"/>
	<skos:hasTopConcept rdf:resource="http://vocab.nerc.ac.uk/collection/L05/current/381"/>
	<skos:hasTopConcept rdf:resource="http://vocab.nerc.ac.uk/collection/L05/current/382"/>
	<skos:hasTopConcept rdf:resource="http://vocab.nerc.ac.uk/collection/L05/current/383"/>
	<skos:hasTopConcept rdf:resource="http://vocab.nerc.ac.uk/collection/L05/current/384"/>
	<skos:hasTopConcept rdf:resource="http://vocab.nerc.ac.uk/collection/L05/current/385"/>
	<skos:hasTopConcept rdf:resource="http://vocab.nerc.ac.uk/collection/L05/current/388"/>
	<skos:hasTopConcept rdf:resource="http://vocab.nerc.ac.uk/collection/L05/current/50"/>
	<skos:hasTopConcept rdf:resource="http://vocab.nerc.ac.uk/collection/L05/current/51"/>
	<skos:hasTopConcept rdf:resource="http://vocab.nerc.ac.uk/collection/L05/current/53"/>
	<skos:hasTopConcept rdf:resource="http://vocab.nerc.ac.uk/collection/L05/current/54"/>
	<skos:hasTopConcept rdf:resource="http://vocab.nerc.ac.uk/collection/L05/current/60"/>
	<skos:hasTopConcept rdf:resource="http://vocab.nerc.ac.uk/collection/L05/current/61"/>
	<skos:hasTopConcept rdf:resource="http://vocab.nerc.ac.uk/collection/L05/current/62"/>
	<skos:hasTopConcept rdf:resource="http://vocab.nerc.ac.uk/collection/L05/current/63"/>
	<skos:hasTopConcept rdf:resource="http://vocab.nerc.ac.uk/collection/L05/current/64"/>
	<skos:hasTopConcept rdf:resource="http://vocab.nerc.ac.uk/collection/L05/current/65"/>
	<skos:hasTopConcept rdf:resource="http://vocab.nerc.ac.uk/collection/L05/current/68"/>
	<skos:hasTopConcept rdf:resource="http://vocab.nerc.ac.uk/collection/L05/current/69"/>
	<skos:hasTopConcept rdf:resource="http://vocab.nerc.ac.uk/collection/L05/current/81"/>
	<skos:hasTopConcept rdf:resource="http://vocab.nerc.ac.uk/collection/L05/current/82"/>
	<skos:hasTopConcept rdf:resource="http://vocab.nerc.ac.uk/collection/L05/current/90"/>
	<skos:hasTopConcept rdf:resource="http://vocab.nerc.ac.uk/collection/L05/current/91"/>
	<skos:hasTopConcept rdf:resource="http://vocab.nerc.ac.uk/collection/L05/current/FFES"/>
	<skos:hasTopConcept rdf:resource="http://vocab.nerc.ac.uk/collection/L05/current/LAB02"/>
	<skos:hasTopConcept rdf:resource="http://vocab.nerc.ac.uk/collection/L05/current/LAB05"/>
	<skos:hasTopConcept rdf:resource="http://vocab.nerc.ac.uk/collection/L05/current/LAB06"/>
	<skos:hasTopConcept rdf:resource="http://vocab.nerc.ac.uk/collection/L05/current/LAB07"/>
	<skos:hasTopConcept rdf:resource="http://vocab.nerc.ac.uk/collection/L05/current/LAB08"/>
	<skos:hasTopConcept rdf:resource="http://vocab.nerc.ac.uk/collection/L05/current/LAB09"/>
	<skos:hasTopConcept rdf:resource="http://vocab.nerc.ac.uk/collection/L05/current/LAB10"/>
	<skos:hasTopConcept rdf:resource="http://vocab.nerc.ac.uk/collection/L05/current/LAB11"/>
	<skos:hasTopConcept rdf:resource="http://vocab.nerc.ac.uk/collection/L05/current/LAB15"/>
	<skos:hasTopConcept rdf:resource="http://vocab.nerc.ac.uk/collection/L05/current/LAB16"/>
	<skos:hasTopConcept rdf:resource="http://vocab.nerc.ac.uk/collection/L05/current/LAB17"/>
	<skos:hasTopConcept rdf:resource="http://vocab.nerc.ac.uk/collection/L05/current/LAB18"/>
	<skos:hasTopConcept rdf:resource="http://vocab.nerc.ac.uk/collection/L05/current/LAB19"/>
	<skos:hasTopConcept rdf:resource="http://vocab.nerc.ac.uk/collection/L05/current/LAB20"/>
	<skos:hasTopConcept rdf:resource="http://vocab.nerc.ac.uk/collection/L05/current/LAB21"/>
	<skos:hasTopConcept rdf:resource="http://vocab.nerc.ac.uk/collection/L05/current/LAB22"/>
	<skos:hasTopConcept rdf:resource="http://vocab.nerc.ac.uk/collection/L05/current/LAB25"/>
	<skos:hasTopConcept rdf:resource="http://vocab.nerc.ac.uk/collection/L05/current/LAB37"/>
	<skos:hasTopConcept rdf:resource="http://vocab.nerc.ac.uk/collection/L05/current/LAB39"/>
	<skos:hasTopConcept rdf:resource="http://vocab.nerc.ac.uk/collection/L05/current/LAB40"/>
	<skos:hasTopConcept rdf:resource="http://vocab.nerc.ac.uk/collection/L05/current/POS03"/>
	<skos:hasTopConcept rdf:resource="http://vocab.nerc.ac.uk/collection/L05/current/POS17"/>
	<skos:hasTopConcept rdf:resource="http://vocab.nerc.ac.uk/collection/L05/current/WPS"/>
	<dcterms:issued rdf:datatype="http://www.w3.org/2001/XMLSchema#string">2017-12-11</dcterms:issued>
	<owl:versionInfo rdf:datatype="http://www.w3.org/2001/XMLSchema#string">Version 2.1</owl:versionInfo>
</rdf:Description>

<rdf:Description rdf:about="http://purl.org/dc/elements/1.1/rights">
	<rdf:type rdf:resource="http://www.w3.org/1999/02/22-rdf-syntax-ns#Property"/>
	<rdf:type rdf:resource="http://www.w3.org/2000/01/rdf-schema#Resource"/>
	<rdfs:subPropertyOf rdf:resource="http://purl.org/dc/elements/1.1/rights"/>
</rdf:Description>

<rdf:Description rdf:about="http://purl.org/dc/terms/contributor">
	<rdf:type rdf:resource="http://www.w3.org/1999/02/22-rdf-syntax-ns#Property"/>
	<rdf:type rdf:resource="http://www.w3.org/2000/01/rdf-schema#Resource"/>
	<rdfs:subPropertyOf rdf:resource="http://purl.org/dc/terms/contributor"/>
</rdf:Description>

<rdf:Description rdf:about="http://purl.org/dc/terms/created">
	<rdf:type rdf:resource="http://www.w3.org/1999/02/22-rdf-syntax-ns#Property"/>
	<rdf:type rdf:resource="http://www.w3.org/2000/01/rdf-schema#Resource"/>
	<rdfs:subPropertyOf rdf:resource="http://purl.org/dc/terms/created"/>
</rdf:Description>

<rdf:Description rdf:about="http://purl.org/dc/terms/creator">
	<rdf:type rdf:resource="http://www.w3.org/1999/02/22-rdf-syntax-ns#Property"/>
	<rdf:type rdf:resource="http://www.w3.org/2000/01/rdf-schema#Resource"/>
	<rdfs:subPropertyOf rdf:resource="http://purl.org/dc/terms/creator"/>
</rdf:Description>

<rdf:Description rdf:about="http://purl.org/dc/terms/description">
	<rdf:type rdf:resource="http://www.w3.org/1999/02/22-rdf-syntax-ns#Property"/>
	<rdf:type rdf:resource="http://www.w3.org/2000/01/rdf-schema#Resource"/>
	<rdfs:subPropertyOf rdf:resource="http://purl.org/dc/terms/description"/>
</rdf:Description>

<rdf:Description rdf:about="http://purl.org/dc/terms/identifier">
	<rdf:type rdf:resource="http://www.w3.org/1999/02/22-rdf-syntax-ns#Property"/>
	<rdf:type rdf:resource="http://www.w3.org/2000/01/rdf-schema#Resource"/>
	<rdfs:subPropertyOf rdf:resource="http://purl.org/dc/terms/identifier"/>
</rdf:Description>

<rdf:Description rdf:about="http://purl.org/dc/terms/modified">
	<rdf:type rdf:resource="http://www.w3.org/1999/02/22-rdf-syntax-ns#Property"/>
	<rdf:type rdf:resource="http://www.w3.org/2000/01/rdf-schema#Resource"/>
	<rdfs:subPropertyOf rdf:resource="http://purl.org/dc/terms/modified"/>
</rdf:Description>

<rdf:Description rdf:about="http://purl.org/dc/terms/publisher">
	<rdf:type rdf:resource="http://www.w3.org/1999/02/22-rdf-syntax-ns#Property"/>
	<rdf:type rdf:resource="http://www.w3.org/2000/01/rdf-schema#Resource"/>
	<rdfs:subPropertyOf rdf:resource="http://purl.org/dc/terms/publisher"/>
</rdf:Description>

<rdf:Description rdf:about="http://purl.org/dc/terms/subject">
	<rdf:type rdf:resource="http://www.w3.org/1999/02/22-rdf-syntax-ns#Property"/>
	<rdf:type rdf:resource="http://www.w3.org/2000/01/rdf-schema#Resource"/>
	<rdfs:subPropertyOf rdf:resource="http://purl.org/dc/terms/subject"/>
</rdf:Description>

<rdf:Description rdf:about="http://purl.org/dc/terms/title">
	<rdf:type rdf:resource="http://www.w3.org/1999/02/22-rdf-syntax-ns#Property"/>
	<rdf:type rdf:resource="http://www.w3.org/2000/01/rdf-schema#Resource"/>
	<rdfs:subPropertyOf rdf:resource="http://purl.org/dc/terms/title"/>
</rdf:Description>

<rdf:Description rdf:about="http://schema.semantic-web.at/ppt/identifier">
	<rdf:type rdf:resource="http://www.w3.org/1999/02/22-rdf-syntax-ns#Property"/>
	<rdf:type rdf:resource="http://www.w3.org/2000/01/rdf-schema#Resource"/>
	<rdfs:subPropertyOf rdf:resource="http://schema.semantic-web.at/ppt/identifier"/>
</rdf:Description>

<rdf:Description rdf:about="http://schema.semantic-web.at/ppt/urigen#settingIdentifier">
	<rdf:type rdf:resource="http://www.w3.org/1999/02/22-rdf-syntax-ns#Property"/>
	<rdf:type rdf:resource="http://www.w3.org/2000/01/rdf-schema#Resource"/>
	<rdfs:subPropertyOf rdf:resource="http://schema.semantic-web.at/ppt/urigen#settingIdentifier"/>
</rdf:Description>

<rdf:Description rdf:about="http://www.w3.org/2004/02/skos/core#ConceptScheme">
	<rdf:type rdf:resource="http://www.w3.org/2000/01/rdf-schema#Resource"/>
	<rdf:type rdf:resource="http://www.w3.org/2000/01/rdf-schema#Class"/>
	<rdfs:subClassOf rdf:resource="http://www.w3.org/2000/01/rdf-schema#Resource"/>
	<rdfs:subClassOf rdf:resource="http://www.w3.org/2004/02/skos/core#ConceptScheme"/>
</rdf:Description>

<rdf:Description rdf:about="http://www.w3.org/2004/02/skos/core#hasTopConcept">
	<rdf:type rdf:resource="http://www.w3.org/1999/02/22-rdf-syntax-ns#Property"/>
	<rdf:type rdf:resource="http://www.w3.org/2000/01/rdf-schema#Resource"/>
	<rdfs:subPropertyOf rdf:resource="http://www.w3.org/2004/02/skos/core#hasTopConcept"/>
</rdf:Description>

<rdf:Description rdf:about="http://vocab.aodn.org.au/def/instrument/entity/361">
	<rdf:type rdf:resource="http://www.w3.org/2000/01/rdf-schema#Resource"/>
	<rdf:type rdf:resource="http://www.w3.org/2004/02/skos/core#Concept"/>
	<dcterms:created rdf:datatype="http://www.w3.org/2001/XMLSchema#dateTime">2013-07-18T00:00:00Z</dcterms:created>
	<dcterms:creator rdf:resource="http://editor.vocabs.ands.org.au/user/Sebastien-Mancini"/>
	<dc:publisher rdf:datatype="http://www.w3.org/2001/XMLSchema#string">eMarine Information Infrastructure (eMII)</dc:publisher>
	<dc:source rdf:datatype="http://www.w3.org/2001/XMLSchema#string">Australian Ocean Data Network instrument register</dc:source>
	<skos:definition xml:lang="en">A package of sensors that measure physical, chemical and biological properties in the water column. These typically include temperature, conductivity, pressure, dissolved oxygen, fluorescence and turbidity.</skos:definition>
	<skos:inScheme rdf:resource="http://vocab.aodn.org.au/def/instrument/1"/>
	<skos:narrower rdf:resource="http://vocab.nerc.ac.uk/collection/L22/current/TOOL0215"/>
	<skos:narrower rdf:resource="http://vocab.nerc.ac.uk/collection/L22/current/TOOL0673"/>
	<skos:narrower rdf:resource="http://vocab.nerc.ac.uk/collection/L22/current/TOOL0674"/>
	<skos:narrower rdf:resource="http://vocab.nerc.ac.uk/collection/L22/current/TOOL0675"/>
	<skos:prefLabel xml:lang="en">water biogeochemical sensor</skos:prefLabel>
	<skos:topConceptOf rdf:resource="http://vocab.aodn.org.au/def/instrument/1"/>
</rdf:Description>

<rdf:Description rdf:about="http://vocab.aodn.org.au/def/instrument/entity/363">
	<rdf:type rdf:resource="http://www.w3.org/2000/01/rdf-schema#Resource"/>
	<rdf:type rdf:resource="http://www.w3.org/2004/02/skos/core#Concept"/>
	<dcterms:created rdf:datatype="http://www.w3.org/2001/XMLSchema#dateTime">2013-07-18T00:00:00Z</dcterms:created>
	<dcterms:creator rdf:resource="http://editor.vocabs.ands.org.au/user/Sebastien-Mancini"/>
	<dc:publisher rdf:datatype="http://www.w3.org/2001/XMLSchema#string">eMarine Information Infrastructure (eMII)</dc:publisher>
	<dc:source rdf:datatype="http://www.w3.org/2001/XMLSchema#string">Australian Ocean Data Network instrument register</dc:source>
	<skos:definition xml:lang="en">A package lowered and raised vertically from a surface platform usually a ship. A CTD measures Conductivity, Temperature and Depth. Despite the name, all CTDs actually measure pressure. The CTD is attached to a frame fitted with a number of large water-collecting bottles called Niskins, the instrument together with the bottles is called the CTD rosette. The Niskin bottles are designed so that they have lids at both ends. They are sent down open, and triggered to close electronically at the depth that water needs to be collected. Additional optional sensors include ADCP, fluorometers, transmissometers and radiometers.</skos:definition>
	<skos:inScheme rdf:resource="http://vocab.aodn.org.au/def/instrument/1"/>
	<skos:prefLabel xml:lang="en">CTD Rosette</skos:prefLabel>
	<skos:topConceptOf rdf:resource="http://vocab.aodn.org.au/def/instrument/1"/>
</rdf:Description>

<rdf:Description rdf:about="http://vocab.aodn.org.au/def/instrument/entity/365">
	<rdf:type rdf:resource="http://www.w3.org/2000/01/rdf-schema#Resource"/>
	<rdf:type rdf:resource="http://www.w3.org/2004/02/skos/core#Concept"/>
	<dcterms:contributor rdf:resource="http://editor.vocabs.ands.org.au/user/eMII_Atkins.Natalia"/>
	<dcterms:created rdf:datatype="http://www.w3.org/2001/XMLSchema#dateTime">2013-07-18T00:00:00Z</dcterms:created>
	<dcterms:creator rdf:resource="http://editor.vocabs.ands.org.au/user/Sebastien-Mancini"/>
	<dcterms:modified rdf:datatype="http://www.w3.org/2001/XMLSchema#dateTime">2015-08-28T00:06:17Z</dcterms:modified>
	<dc:publisher rdf:datatype="http://www.w3.org/2001/XMLSchema#string">eMarine Information Infrastructure (eMII)</dc:publisher>
	<dc:source rdf:datatype="http://www.w3.org/2001/XMLSchema#string">Australian Ocean Data Network instrument register</dc:source>
	<skos:definition xml:lang="en">Instrument that simultaneously measures electrical conductivity and temperature in the water column. To reduce costs, the instrument may not include a pressure sensor, because the deployment depth is know (approximately).</skos:definition>
	<skos:inScheme rdf:resource="http://vocab.aodn.org.au/def/instrument/1"/>
	<skos:narrower rdf:resource="http://vocab.nerc.ac.uk/collection/L22/current/TOOL0869"/>
	<skos:narrower rdf:resource="http://vocab.nerc.ac.uk/collection/L22/current/TOOL0870"/>
	<skos:narrower rdf:resource="http://vocab.nerc.ac.uk/collection/L22/current/TOOL0017"/>
	<skos:narrower rdf:resource="http://vocab.nerc.ac.uk/collection/L22/current/TOOL0018"/>
	<skos:narrower rdf:resource="http://vocab.nerc.ac.uk/collection/L22/current/TOOL0019"/>
	<skos:narrower rdf:resource="http://vocab.nerc.ac.uk/collection/L22/current/TOOL0020"/>
	<skos:narrower rdf:resource="http://vocab.nerc.ac.uk/collection/L22/current/TOOL0023"/>
	<skos:narrower rdf:resource="http://vocab.nerc.ac.uk/collection/L22/current/TOOL0053"/>
	<skos:narrower rdf:resource="http://vocab.nerc.ac.uk/collection/L22/current/TOOL0100"/>
	<skos:prefLabel xml:lang="en">Conductivity-Temperature sensors</skos:prefLabel>
	<skos:topConceptOf rdf:resource="http://vocab.aodn.org.au/def/instrument/1"/>
</rdf:Description>

<rdf:Description rdf:about="http://vocab.nerc.ac.uk/collection/L05/current/101">
	<rdf:type rdf:resource="http://www.w3.org/2000/01/rdf-schema#Resource"/>
	<rdf:type rdf:resource="http://www.w3.org/2004/02/skos/core#Concept"/>
	<dcterms:contributor rdf:resource="http://editor.vocabs.ands.org.au/user/eMII_Atkins.Natalia"/>
	<dcterms:created rdf:datatype="http://www.w3.org/2001/XMLSchema#dateTime">2013-03-28T00:00:00Z</dcterms:created>
	<dcterms:modified rdf:datatype="http://www.w3.org/2001/XMLSchema#dateTime">2017-03-23T05:10:11Z</dcterms:modified>
	<dc:publisher rdf:datatype="http://www.w3.org/2001/XMLSchema#string">British Oceanographic Data Centre (BODC)</dc:publisher>
	<dc:source rdf:datatype="http://www.w3.org/2001/XMLSchema#string">(L051) SeaDataNet device categories</dc:source>
	<skos:definition xml:lang="en">Instrument that measures wind speed and direction at a single elevation</skos:definition>
	<skos:inScheme rdf:resource="http://vocab.aodn.org.au/def/instrument/1"/>
	<skos:narrower rdf:resource="http://vocab.nerc.ac.uk/collection/L22/current/TOOL0877"/>
	<skos:narrower rdf:resource="http://vocab.nerc.ac.uk/collection/L22/current/TOOL0126"/>
	<skos:narrower rdf:resource="http://vocab.nerc.ac.uk/collection/L22/current/TOOL0127"/>
	<skos:narrower rdf:resource="http://vocab.nerc.ac.uk/collection/L22/current/TOOL0195"/>
	<skos:narrower rdf:resource="http://vocab.nerc.ac.uk/collection/L22/current/TOOL0260"/>
	<skos:narrower rdf:resource="http://vocab.nerc.ac.uk/collection/L22/current/TOOL0704"/>
	<skos:narrower rdf:resource="http://vocab.nerc.ac.uk/collection/L22/current/TOOL1031"/>
	<skos:prefLabel xml:lang="en">anemometers</skos:prefLabel>
	<skos:topConceptOf rdf:resource="http://vocab.aodn.org.au/def/instrument/1"/>
</rdf:Description>

<rdf:Description rdf:about="http://vocab.nerc.ac.uk/collection/L05/current/102">
	<rdf:type rdf:resource="http://www.w3.org/2000/01/rdf-schema#Resource"/>
	<rdf:type rdf:resource="http://www.w3.org/2004/02/skos/core#Concept"/>
	<dcterms:contributor rdf:resource="http://editor.vocabs.ands.org.au/user/eMII_Atkins.Natalia"/>
	<dcterms:created rdf:datatype="http://www.w3.org/2001/XMLSchema#dateTime">2013-03-28T00:00:00Z</dcterms:created>
	<dcterms:modified rdf:datatype="http://www.w3.org/2001/XMLSchema#dateTime">2017-03-23T05:10:26Z</dcterms:modified>
	<dc:publisher rdf:datatype="http://www.w3.org/2001/XMLSchema#string">British Oceanographic Data Centre (BODC)</dc:publisher>
	<dc:source rdf:datatype="http://www.w3.org/2001/XMLSchema#string">(L051) SeaDataNet device categories</dc:source>
	<skos:definition xml:lang="en">Instrument that makes routine meteorological measurements on the atmosphere typically air pressure temperature and humidity</skos:definition>
	<skos:inScheme rdf:resource="http://vocab.aodn.org.au/def/instrument/1"/>
	<skos:narrower rdf:resource="http://vocab.nerc.ac.uk/collection/L22/current/TOOL1031"/>
	<skos:narrower rdf:resource="http://vocab.nerc.ac.uk/collection/L22/current/TOOL0081"/>
	<skos:narrower rdf:resource="http://vocab.nerc.ac.uk/collection/L22/current/TOOL0617"/>
	<skos:narrower rdf:resource="http://vocab.nerc.ac.uk/collection/L22/current/TOOL0672"/>
	<skos:narrower rdf:resource="http://vocab.nerc.ac.uk/collection/L22/current/TOOL0677"/>
	<skos:narrower rdf:resource="http://vocab.nerc.ac.uk/collection/L22/current/TOOL0680"/>
	<skos:narrower rdf:resource="http://vocab.nerc.ac.uk/collection/L22/current/TOOL0682"/>
	<skos:narrower rdf:resource="http://vocab.nerc.ac.uk/collection/L22/current/TOOL0683"/>
	<skos:narrower rdf:resource="http://vocab.nerc.ac.uk/collection/L22/current/TOOL0726"/>
	<skos:narrower rdf:resource="http://vocab.nerc.ac.uk/collection/L22/current/TOOL0727"/>
	<skos:narrower rdf:resource="http://vocab.nerc.ac.uk/collection/L22/current/TOOL0741"/>
	<skos:narrower rdf:resource="http://vocab.nerc.ac.uk/collection/L22/current/TOOL0779"/>
	<skos:narrower rdf:resource="http://vocab.nerc.ac.uk/collection/L22/current/TOOL0780"/>
	<skos:narrower rdf:resource="http://vocab.nerc.ac.uk/collection/L22/current/TOOL0808"/>
	<skos:narrower rdf:resource="http://vocab.nerc.ac.uk/collection/L22/current/TOOL1015"/>
	<skos:narrower rdf:resource="http://vocab.nerc.ac.uk/collection/L22/current/TOOL1180"/>
	<skos:prefLabel xml:lang="en">meteorological packages</skos:prefLabel>
	<skos:topConceptOf rdf:resource="http://vocab.aodn.org.au/def/instrument/1"/>
</rdf:Description>

<rdf:Description rdf:about="http://vocab.nerc.ac.uk/collection/L05/current/103">
	<rdf:type rdf:resource="http://www.w3.org/2000/01/rdf-schema#Resource"/>
	<rdf:type rdf:resource="http://www.w3.org/2004/02/skos/core#Concept"/>
	<dcterms:created rdf:datatype="http://www.w3.org/2001/XMLSchema#dateTime">2014-05-22T00:00:00Z</dcterms:created>
	<dc:publisher rdf:datatype="http://www.w3.org/2001/XMLSchema#string">British Oceanographic Data Centre (BODC)</dc:publisher>
	<dc:source rdf:datatype="http://www.w3.org/2001/XMLSchema#string">(L051) SeaDataNet device categories</dc:source>
	<skos:definition xml:lang="en">A balloon-borne package equipped with a radio transmitter and meteorological sensors typically measuring temperature pressure and humidity.</skos:definition>
	<skos:inScheme rdf:resource="http://vocab.aodn.org.au/def/instrument/1"/>
	<skos:prefLabel xml:lang="en">radiosondes</skos:prefLabel>
	<skos:topConceptOf rdf:resource="http://vocab.aodn.org.au/def/instrument/1"/>
</rdf:Description>

<rdf:Description rdf:about="http://vocab.nerc.ac.uk/collection/L05/current/110">
	<rdf:type rdf:resource="http://www.w3.org/2000/01/rdf-schema#Resource"/>
	<rdf:type rdf:resource="http://www.w3.org/2004/02/skos/core#Concept"/>
	<dcterms:contributor rdf:resource="http://editor.vocabs.ands.org.au/user/Natalia_Atkins"/>
	<dcterms:created rdf:datatype="http://www.w3.org/2001/XMLSchema#dateTime">2013-03-28T00:00:00Z</dcterms:created>
	<dcterms:modified rdf:datatype="http://www.w3.org/2001/XMLSchema#dateTime">2015-06-30T06:13:24Z</dcterms:modified>
	<dc:publisher rdf:datatype="http://www.w3.org/2001/XMLSchema#string">British Oceanographic Data Centre (BODC)</dc:publisher>
	<dc:source rdf:datatype="http://www.w3.org/2001/XMLSchema#string">(L051) SeaDataNet device categories</dc:source>
	<skos:definition xml:lang="en">Instrument that measures water column surface wave parameters including height period direction and energy spectra.</skos:definition>
	<skos:inScheme rdf:resource="http://vocab.aodn.org.au/def/instrument/1"/>
	<skos:narrower rdf:resource="http://vocab.nerc.ac.uk/collection/L22/current/TOOL0898"/>
	<skos:narrower rdf:resource="http://vocab.nerc.ac.uk/collection/L22/current/TOOL0268"/>
	<skos:narrower rdf:resource="http://vocab.nerc.ac.uk/collection/L22/current/TOOL0696"/>
	<skos:narrower rdf:resource="http://vocab.nerc.ac.uk/collection/L22/current/TOOL0710"/>
	<skos:narrower rdf:resource="http://vocab.nerc.ac.uk/collection/L22/current/TOOL0729"/>
	<skos:narrower rdf:resource="http://vocab.nerc.ac.uk/collection/L22/current/TOOL0733"/>
	<skos:narrower rdf:resource="http://vocab.nerc.ac.uk/collection/L22/current/TOOL0781"/>
	<skos:prefLabel xml:lang="en">wave recorders</skos:prefLabel>
	<skos:topConceptOf rdf:resource="http://vocab.aodn.org.au/def/instrument/1"/>
</rdf:Description>

<rdf:Description rdf:about="http://vocab.nerc.ac.uk/collection/L05/current/111">
	<rdf:type rdf:resource="http://www.w3.org/2000/01/rdf-schema#Resource"/>
	<rdf:type rdf:resource="http://www.w3.org/2004/02/skos/core#Concept"/>
	<dcterms:created rdf:datatype="http://www.w3.org/2001/XMLSchema#dateTime">2014-06-04T00:00:00Z</dcterms:created>
	<dcterms:modified rdf:datatype="http://www.w3.org/2001/XMLSchema#dateTime">2015-05-29T06:29:17Z</dcterms:modified>
	<dc:publisher rdf:datatype="http://www.w3.org/2001/XMLSchema#string">British Oceanographic Data Centre (BODC)</dc:publisher>
	<dc:source rdf:datatype="http://www.w3.org/2001/XMLSchema#string">(L051) SeaDataNet device categories</dc:source>
	<skos:definition xml:lang="en">Instrument that make smoothed measurements of the elevation of the sea surface relative to a fixed vertical datum</skos:definition>
	<skos:inScheme rdf:resource="http://vocab.aodn.org.au/def/instrument/1"/>
	<skos:narrower rdf:resource="http://vocab.nerc.ac.uk/collection/L22/current/TOOL0675"/>
	<skos:narrower rdf:resource="http://vocab.nerc.ac.uk/collection/L22/current/TOOL0680"/>
	<skos:narrower rdf:resource="http://vocab.nerc.ac.uk/collection/L22/current/TOOL0696"/>
	<skos:narrower rdf:resource="http://vocab.nerc.ac.uk/collection/L22/current/TOOL0729"/>
	<skos:narrower rdf:resource="http://vocab.nerc.ac.uk/collection/L22/current/TOOL0169"/>
	<skos:narrower rdf:resource="http://vocab.nerc.ac.uk/collection/L22/current/TOOL0685"/>
	<skos:narrower rdf:resource="http://vocab.nerc.ac.uk/collection/L22/current/TOOL0708"/>
	<skos:narrower rdf:resource="http://vocab.nerc.ac.uk/collection/L22/current/TOOL0731"/>
	<skos:narrower rdf:resource="http://vocab.nerc.ac.uk/collection/L22/current/TOOL0809"/>
	<skos:prefLabel xml:lang="en">sea level recorders</skos:prefLabel>
	<skos:topConceptOf rdf:resource="http://vocab.aodn.org.au/def/instrument/1"/>
</rdf:Description>

<rdf:Description rdf:about="http://vocab.nerc.ac.uk/collection/L05/current/113">
	<rdf:type rdf:resource="http://www.w3.org/2000/01/rdf-schema#Resource"/>
	<rdf:type rdf:resource="http://www.w3.org/2004/02/skos/core#Concept"/>
	<dcterms:contributor rdf:resource="http://editor.vocabs.ands.org.au/user/eMII_Atkins.Natalia"/>
	<dcterms:created rdf:datatype="http://www.w3.org/2001/XMLSchema#dateTime">2013-03-28T00:00:00Z</dcterms:created>
	<dcterms:modified rdf:datatype="http://www.w3.org/2001/XMLSchema#dateTime">2017-03-23T04:10:18Z</dcterms:modified>
	<dc:publisher rdf:datatype="http://www.w3.org/2001/XMLSchema#string">British Oceanographic Data Centre (BODC)</dc:publisher>
	<dc:source rdf:datatype="http://www.w3.org/2001/XMLSchema#string">(L051) SeaDataNet device categories</dc:source>
	<skos:definition xml:lang="en">Instrument that measures the amount of stimulated electromagnetic radiation produced by pulses of electromagnetic radiation emitted into the water column</skos:definition>
	<skos:inScheme rdf:resource="http://vocab.aodn.org.au/def/instrument/1"/>
	<skos:narrower rdf:resource="http://vocab.nerc.ac.uk/collection/L22/current/TOOL0215"/>
	<skos:narrower rdf:resource="http://vocab.nerc.ac.uk/collection/L22/current/TOOL0673"/>
	<skos:narrower rdf:resource="http://vocab.nerc.ac.uk/collection/L22/current/TOOL0674"/>
	<skos:narrower rdf:resource="http://vocab.nerc.ac.uk/collection/L22/current/TOOL0675"/>
	<skos:narrower rdf:resource="http://vocab.nerc.ac.uk/collection/L22/current/TOOL0075"/>
	<skos:narrower rdf:resource="http://vocab.nerc.ac.uk/collection/L22/current/TOOL0720"/>
	<skos:narrower rdf:resource="http://vocab.nerc.ac.uk/collection/L22/current/TOOL1141"/>
	<skos:prefLabel xml:lang="en">fluorometers</skos:prefLabel>
	<skos:topConceptOf rdf:resource="http://vocab.aodn.org.au/def/instrument/1"/>
</rdf:Description>

<rdf:Description rdf:about="http://vocab.nerc.ac.uk/collection/L05/current/114">
	<rdf:type rdf:resource="http://www.w3.org/2000/01/rdf-schema#Resource"/>
	<rdf:type rdf:resource="http://www.w3.org/2004/02/skos/core#Concept"/>
	<dcterms:created rdf:datatype="http://www.w3.org/2001/XMLSchema#dateTime">2013-03-28T00:00:00Z</dcterms:created>
	<dc:publisher rdf:datatype="http://www.w3.org/2001/XMLSchema#string">British Oceanographic Data Centre (BODC)</dc:publisher>
	<dc:source rdf:datatype="http://www.w3.org/2001/XMLSchema#string">(L051) SeaDataNet device categories</dc:source>
	<skos:definition xml:lang="en">Instrument that measures current speed and direction at a single depth</skos:definition>
	<skos:inScheme rdf:resource="http://vocab.aodn.org.au/def/instrument/1"/>
	<skos:narrower rdf:resource="http://vocab.nerc.ac.uk/collection/L22/current/TOOL0089"/>
	<skos:narrower rdf:resource="http://vocab.nerc.ac.uk/collection/L22/current/TOOL0121"/>
	<skos:narrower rdf:resource="http://vocab.nerc.ac.uk/collection/L22/current/TOOL0476"/>
	<skos:narrower rdf:resource="http://vocab.nerc.ac.uk/collection/L22/current/TOOL0477"/>
	<skos:narrower rdf:resource="http://vocab.nerc.ac.uk/collection/L22/current/TOOL0306"/>
	<skos:prefLabel xml:lang="en">current meters</skos:prefLabel>
	<skos:topConceptOf rdf:resource="http://vocab.aodn.org.au/def/instrument/1"/>
</rdf:Description>

<rdf:Description rdf:about="http://vocab.nerc.ac.uk/collection/L05/current/115">
	<rdf:type rdf:resource="http://www.w3.org/2000/01/rdf-schema#Resource"/>
	<rdf:type rdf:resource="http://www.w3.org/2004/02/skos/core#Concept"/>
	<dcterms:contributor rdf:resource="http://editor.vocabs.ands.org.au/user/eMII_Atkins.Natalia"/>
	<dcterms:created rdf:datatype="http://www.w3.org/2001/XMLSchema#dateTime">2012-12-19T00:00:00Z</dcterms:created>
	<dcterms:modified rdf:datatype="http://www.w3.org/2001/XMLSchema#dateTime">2017-03-23T04:51:48Z</dcterms:modified>
	<dc:publisher rdf:datatype="http://www.w3.org/2001/XMLSchema#string">British Oceanographic Data Centre (BODC)</dc:publisher>
	<dc:source rdf:datatype="http://www.w3.org/2001/XMLSchema#string">(L051) SeaDataNet device categories</dc:source>
	<skos:definition xml:lang="en">Instrument that measures current speed and direction at multiple predetermined depths simultaneously</skos:definition>
	<skos:inScheme rdf:resource="http://vocab.aodn.org.au/def/instrument/1"/>
	<skos:narrower rdf:resource="http://vocab.nerc.ac.uk/collection/L22/current/TOOL0888"/>
	<skos:narrower rdf:resource="http://vocab.nerc.ac.uk/collection/L22/current/TOOL0898"/>
	<skos:narrower rdf:resource="http://vocab.nerc.ac.uk/collection/L22/current/TOOL0905"/>
	<skos:narrower rdf:resource="http://vocab.nerc.ac.uk/collection/L22/current/TOOL0056"/>
	<skos:narrower rdf:resource="http://vocab.nerc.ac.uk/collection/L22/current/TOOL0293"/>
	<skos:narrower rdf:resource="http://vocab.nerc.ac.uk/collection/L22/current/TOOL0294"/>
	<skos:narrower rdf:resource="http://vocab.nerc.ac.uk/collection/L22/current/TOOL0295"/>
	<skos:narrower rdf:resource="http://vocab.nerc.ac.uk/collection/L22/current/TOOL0445"/>
	<skos:narrower rdf:resource="http://vocab.nerc.ac.uk/collection/L22/current/TOOL0732"/>
	<skos:narrower rdf:resource="http://vocab.nerc.ac.uk/collection/L22/current/TOOL1009"/>
	<skos:narrower rdf:resource="http://vocab.nerc.ac.uk/collection/L22/current/TOOL1010"/>
	<skos:prefLabel xml:lang="en">current profilers</skos:prefLabel>
	<skos:topConceptOf rdf:resource="http://vocab.aodn.org.au/def/instrument/1"/>
</rdf:Description>

<rdf:Description rdf:about="http://vocab.nerc.ac.uk/collection/L05/current/121">
	<rdf:type rdf:resource="http://www.w3.org/2000/01/rdf-schema#Resource"/>
	<rdf:type rdf:resource="http://www.w3.org/2004/02/skos/core#Concept"/>
	<dcterms:created rdf:datatype="http://www.w3.org/2001/XMLSchema#dateTime">2013-07-18T00:00:00Z</dcterms:created>
	<dc:publisher rdf:datatype="http://www.w3.org/2001/XMLSchema#string">British Oceanographic Data Centre (BODC)</dc:publisher>
	<dc:source rdf:datatype="http://www.w3.org/2001/XMLSchema#string">(L051) SeaDataNet device categories</dc:source>
	<skos:definition xml:lang="en">A network of statellites that determines the position of a transponder by triangulation such as Argos.  Generally used to track surface buoys for the determination of Lagrangian currents.</skos:definition>
	<skos:inScheme rdf:resource="http://vocab.aodn.org.au/def/instrument/1"/>
	<skos:prefLabel xml:lang="en">satellite tracking system</skos:prefLabel>
	<skos:topConceptOf rdf:resource="http://vocab.aodn.org.au/def/instrument/1"/>
</rdf:Description>

<rdf:Description rdf:about="http://vocab.nerc.ac.uk/collection/L05/current/122">
	<rdf:type rdf:resource="http://www.w3.org/2000/01/rdf-schema#Resource"/>
	<rdf:type rdf:resource="http://www.w3.org/2004/02/skos/core#Concept"/>
	<dcterms:contributor rdf:resource="http://editor.vocabs.ands.org.au/user/Natalia_Atkins"/>
	<dcterms:created rdf:datatype="http://www.w3.org/2001/XMLSchema#dateTime">2013-03-28T00:00:00Z</dcterms:created>
	<dcterms:modified rdf:datatype="http://www.w3.org/2001/XMLSchema#dateTime">2015-08-07T03:08:12Z</dcterms:modified>
	<dc:publisher rdf:datatype="http://www.w3.org/2001/XMLSchema#string">British Oceanographic Data Centre (BODC)</dc:publisher>
	<dc:source rdf:datatype="http://www.w3.org/2001/XMLSchema#string">(L051) SeaDataNet device categories</dc:source>
	<skos:definition xml:lang="en">Instrument that measures the intensity of electromagnetic radiation in either the atmosphere or the water column</skos:definition>
	<skos:inScheme rdf:resource="http://vocab.aodn.org.au/def/instrument/1"/>
	<skos:narrower rdf:resource="http://vocab.nerc.ac.uk/collection/L22/current/TOOL0918"/>
	<skos:narrower rdf:resource="http://vocab.nerc.ac.uk/collection/L22/current/TOOL0932"/>
	<skos:narrower rdf:resource="http://vocab.nerc.ac.uk/collection/L22/current/TOOL0083"/>
	<skos:narrower rdf:resource="http://vocab.nerc.ac.uk/collection/L22/current/TOOL0120"/>
	<skos:narrower rdf:resource="http://vocab.nerc.ac.uk/collection/L22/current/TOOL0193"/>
	<skos:narrower rdf:resource="http://vocab.nerc.ac.uk/collection/L22/current/TOOL0625"/>
	<skos:narrower rdf:resource="http://vocab.nerc.ac.uk/collection/L22/current/TOOL0666"/>
	<skos:narrower rdf:resource="http://vocab.nerc.ac.uk/collection/L22/current/TOOL0676"/>
	<skos:narrower rdf:resource="http://vocab.nerc.ac.uk/collection/L22/current/TOOL1117"/>
	<skos:narrower rdf:resource="http://vocab.nerc.ac.uk/collection/L22/current/TOOL1126"/>
	<skos:prefLabel xml:lang="en">radiometers</skos:prefLabel>
	<skos:topConceptOf rdf:resource="http://vocab.aodn.org.au/def/instrument/1"/>
</rdf:Description>

<rdf:Description rdf:about="http://vocab.nerc.ac.uk/collection/L05/current/123">
	<rdf:type rdf:resource="http://www.w3.org/2000/01/rdf-schema#Resource"/>
	<rdf:type rdf:resource="http://www.w3.org/2004/02/skos/core#Concept"/>
	<dcterms:created rdf:datatype="http://www.w3.org/2001/XMLSchema#dateTime">2013-07-18T00:00:00Z</dcterms:created>
	<dc:publisher rdf:datatype="http://www.w3.org/2001/XMLSchema#string">British Oceanographic Data Centre (BODC)</dc:publisher>
	<dc:source rdf:datatype="http://www.w3.org/2001/XMLSchema#string">(L051) SeaDataNet device categories</dc:source>
	<skos:definition xml:lang="en">Instrument that measures the amount of electromagnetic radiation emitted into the water column returned to the instrument.</skos:definition>
	<skos:inScheme rdf:resource="http://vocab.aodn.org.au/def/instrument/1"/>
	<skos:narrower rdf:resource="http://vocab.nerc.ac.uk/collection/L22/current/TOOL0879"/>
	<skos:narrower rdf:resource="http://vocab.nerc.ac.uk/collection/L22/current/TOOL0215"/>
	<skos:narrower rdf:resource="http://vocab.nerc.ac.uk/collection/L22/current/TOOL0673"/>
	<skos:narrower rdf:resource="http://vocab.nerc.ac.uk/collection/L22/current/TOOL0674"/>
	<skos:narrower rdf:resource="http://vocab.nerc.ac.uk/collection/L22/current/TOOL0675"/>
	<skos:narrower rdf:resource="http://vocab.nerc.ac.uk/collection/L22/current/TOOL1125"/>
	<skos:narrower rdf:resource="http://vocab.nerc.ac.uk/collection/L22/current/TOOL1141"/>
	<skos:prefLabel xml:lang="en">optical backscatter sensors</skos:prefLabel>
	<skos:topConceptOf rdf:resource="http://vocab.aodn.org.au/def/instrument/1"/>
</rdf:Description>

<rdf:Description rdf:about="http://vocab.nerc.ac.uk/collection/L05/current/124">
	<rdf:type rdf:resource="http://www.w3.org/2000/01/rdf-schema#Resource"/>
	<rdf:type rdf:resource="http://www.w3.org/2004/02/skos/core#Concept"/>
	<dcterms:created rdf:datatype="http://www.w3.org/2001/XMLSchema#dateTime">2013-07-18T00:00:00Z</dcterms:created>
	<dc:publisher rdf:datatype="http://www.w3.org/2001/XMLSchema#string">British Oceanographic Data Centre (BODC)</dc:publisher>
	<dc:source rdf:datatype="http://www.w3.org/2001/XMLSchema#string">(L051) SeaDataNet device categories</dc:source>
	<skos:definition xml:lang="en">Systems that measure the attenuation of electromagnetic radiation by the water column. Includes human observer plus Secchi Disk.</skos:definition>
	<skos:inScheme rdf:resource="http://vocab.aodn.org.au/def/instrument/1"/>
	<skos:narrower rdf:resource="http://vocab.nerc.ac.uk/collection/L22/current/TOOL0834"/>
	<skos:prefLabel xml:lang="en">transmissometers</skos:prefLabel>
	<skos:topConceptOf rdf:resource="http://vocab.aodn.org.au/def/instrument/1"/>
</rdf:Description>

<rdf:Description rdf:about="http://vocab.nerc.ac.uk/collection/L05/current/130">
	<rdf:type rdf:resource="http://www.w3.org/2000/01/rdf-schema#Resource"/>
	<rdf:type rdf:resource="http://www.w3.org/2004/02/skos/core#Concept"/>
	<dcterms:contributor rdf:resource="http://editor.vocabs.ands.org.au/user/eMII_Atkins.Natalia"/>
	<dcterms:created rdf:datatype="http://www.w3.org/2001/XMLSchema#dateTime">2013-07-18T00:00:00Z</dcterms:created>
	<dcterms:modified rdf:datatype="http://www.w3.org/2001/XMLSchema#dateTime">2017-03-23T04:09:03Z</dcterms:modified>
	<dc:publisher rdf:datatype="http://www.w3.org/2001/XMLSchema#string">British Oceanographic Data Centre (BODC)</dc:publisher>
	<dc:source rdf:datatype="http://www.w3.org/2001/XMLSchema#string">(L051) SeaDataNet device categories</dc:source>
	<skos:definition xml:lang="en">A CTD (acronym for Conductivity - Temperature - Depth) is a package carrying conductivity, temperature and pressure sensors. The package can be mounted on different platform like for examples Argo float, glider, marine mammals and moorings. Definal on the type of platform used, the measurements of the different parameters are collected through the vertical column of water or at fixed water depth.</skos:definition>
	<skos:inScheme rdf:resource="http://vocab.aodn.org.au/def/instrument/1"/>
	<skos:narrower rdf:resource="http://vocab.nerc.ac.uk/collection/L22/current/TOOL0871"/>
	<skos:narrower rdf:resource="http://vocab.nerc.ac.uk/collection/L22/current/TOOL0720"/>
	<skos:narrower rdf:resource="http://vocab.nerc.ac.uk/collection/L22/current/TOOL0040"/>
	<skos:narrower rdf:resource="http://vocab.nerc.ac.uk/collection/L22/current/TOOL0042"/>
	<skos:narrower rdf:resource="http://vocab.nerc.ac.uk/collection/L22/current/TOOL0047"/>
	<skos:narrower rdf:resource="http://vocab.nerc.ac.uk/collection/L22/current/TOOL0058"/>
	<skos:narrower rdf:resource="http://vocab.nerc.ac.uk/collection/L22/current/TOOL0173"/>
	<skos:narrower rdf:resource="http://vocab.nerc.ac.uk/collection/L22/current/TOOL0183"/>
	<skos:narrower rdf:resource="http://vocab.nerc.ac.uk/collection/L22/current/TOOL0446"/>
	<skos:narrower rdf:resource="http://vocab.nerc.ac.uk/collection/L22/current/TOOL0668"/>
	<skos:narrower rdf:resource="http://vocab.nerc.ac.uk/collection/L22/current/TOOL0669"/>
	<skos:narrower rdf:resource="http://vocab.nerc.ac.uk/collection/L22/current/TOOL0730"/>
	<skos:narrower rdf:resource="http://vocab.nerc.ac.uk/collection/L22/current/TOOL1162"/>
	<skos:narrower rdf:resource="http://vocab.nerc.ac.uk/collection/L22/current/TOOL1163"/>
	<skos:prefLabel xml:lang="en">CTD</skos:prefLabel>
	<skos:topConceptOf rdf:resource="http://vocab.aodn.org.au/def/instrument/1"/>
</rdf:Description>

<rdf:Description rdf:about="http://vocab.nerc.ac.uk/collection/L05/current/132">
	<rdf:type rdf:resource="http://www.w3.org/2000/01/rdf-schema#Resource"/>
	<rdf:type rdf:resource="http://www.w3.org/2004/02/skos/core#Concept"/>
	<dcterms:created rdf:datatype="http://www.w3.org/2001/XMLSchema#dateTime">2013-03-28T00:00:00Z</dcterms:created>
	<dc:publisher rdf:datatype="http://www.w3.org/2001/XMLSchema#string">British Oceanographic Data Centre (BODC)</dc:publisher>
	<dc:source rdf:datatype="http://www.w3.org/2001/XMLSchema#string">(L051) SeaDataNet device categories</dc:source>
	<skos:definition xml:lang="en">Instruments that measure vertical profiles of sea temperature by either lowering a pressure plus temperature senor package (MBT) or dropping a free falling disposable sensor (XBT).</skos:definition>
	<skos:inScheme rdf:resource="http://vocab.aodn.org.au/def/instrument/1"/>
	<skos:narrower rdf:resource="http://vocab.aodn.org.au/def/instrument/entity/39"/>
	<skos:narrower rdf:resource="http://vocab.nerc.ac.uk/collection/L22/current/TOOL0263"/>
	<skos:narrower rdf:resource="http://vocab.nerc.ac.uk/collection/L22/current/TOOL0435"/>
	<skos:prefLabel xml:lang="en">bathythermographs</skos:prefLabel>
	<skos:topConceptOf rdf:resource="http://vocab.aodn.org.au/def/instrument/1"/>
</rdf:Description>

<rdf:Description rdf:about="http://vocab.nerc.ac.uk/collection/L05/current/133">
	<rdf:type rdf:resource="http://www.w3.org/2000/01/rdf-schema#Resource"/>
	<rdf:type rdf:resource="http://www.w3.org/2004/02/skos/core#Concept"/>
	<dcterms:created rdf:datatype="http://www.w3.org/2001/XMLSchema#dateTime">2013-03-28T00:00:00Z</dcterms:created>
	<dc:publisher rdf:datatype="http://www.w3.org/2001/XMLSchema#string">British Oceanographic Data Centre (BODC)</dc:publisher>
	<dc:source rdf:datatype="http://www.w3.org/2001/XMLSchema#string">(L051) SeaDataNet device categories</dc:source>
	<skos:definition xml:lang="en">Temperature and conductivity sensors mounted on a sea-surface platform continuously measuring a surface water supply.</skos:definition>
	<skos:inScheme rdf:resource="http://vocab.aodn.org.au/def/instrument/1"/>
	<skos:narrower rdf:resource="http://vocab.nerc.ac.uk/collection/L22/current/TOOL0190"/>
	<skos:narrower rdf:resource="http://vocab.nerc.ac.uk/collection/L22/current/TOOL0667"/>
	<skos:prefLabel xml:lang="en">thermosalinographs</skos:prefLabel>
	<skos:topConceptOf rdf:resource="http://vocab.aodn.org.au/def/instrument/1"/>
</rdf:Description>

<rdf:Description rdf:about="http://vocab.nerc.ac.uk/collection/L05/current/134">
	<rdf:type rdf:resource="http://www.w3.org/2000/01/rdf-schema#Resource"/>
	<rdf:type rdf:resource="http://www.w3.org/2004/02/skos/core#Concept"/>
	<dcterms:contributor rdf:resource="http://editor.vocabs.ands.org.au/user/eMII_Atkins.Natalia"/>
	<dcterms:created rdf:datatype="http://www.w3.org/2001/XMLSchema#dateTime">2013-03-28T00:00:00Z</dcterms:created>
	<dcterms:modified rdf:datatype="http://www.w3.org/2001/XMLSchema#dateTime">2017-04-10T05:00:47Z</dcterms:modified>
	<dc:publisher rdf:datatype="http://www.w3.org/2001/XMLSchema#string">British Oceanographic Data Centre (BODC)</dc:publisher>
	<dc:source rdf:datatype="http://www.w3.org/2001/XMLSchema#string">(L051) SeaDataNet device categories</dc:source>
	<skos:definition xml:lang="en">An instrument that measures the temperature of the water with which it is in contact</skos:definition>
	<skos:inScheme rdf:resource="http://vocab.aodn.org.au/def/instrument/1"/>
	<skos:narrower rdf:resource="http://vocab.nerc.ac.uk/collection/L22/current/TOOL0869"/>
	<skos:narrower rdf:resource="http://vocab.nerc.ac.uk/collection/L22/current/TOOL0870"/>
	<skos:narrower rdf:resource="http://vocab.nerc.ac.uk/collection/L22/current/TOOL0871"/>
	<skos:narrower rdf:resource="http://vocab.nerc.ac.uk/collection/L22/current/TOOL0872"/>
	<skos:narrower rdf:resource="http://vocab.nerc.ac.uk/collection/L22/current/TOOL0873"/>
	<skos:narrower rdf:resource="http://vocab.nerc.ac.uk/collection/L22/current/TOOL0888"/>
	<skos:narrower rdf:resource="http://vocab.nerc.ac.uk/collection/L22/current/TOOL0898"/>
	<skos:narrower rdf:resource="http://vocab.nerc.ac.uk/collection/L22/current/TOOL0905"/>
	<skos:narrower rdf:resource="http://vocab.nerc.ac.uk/collection/L22/current/TOOL0906"/>
	<skos:narrower rdf:resource="http://vocab.nerc.ac.uk/collection/L22/current/TOOL0907"/>
	<skos:narrower rdf:resource="http://vocab.nerc.ac.uk/collection/L22/current/TOOL0675"/>
	<skos:narrower rdf:resource="http://vocab.nerc.ac.uk/collection/L22/current/TOOL0017"/>
	<skos:narrower rdf:resource="http://vocab.nerc.ac.uk/collection/L22/current/TOOL0018"/>
	<skos:narrower rdf:resource="http://vocab.nerc.ac.uk/collection/L22/current/TOOL0019"/>
	<skos:narrower rdf:resource="http://vocab.nerc.ac.uk/collection/L22/current/TOOL0020"/>
	<skos:narrower rdf:resource="http://vocab.nerc.ac.uk/collection/L22/current/TOOL0023"/>
	<skos:narrower rdf:resource="http://vocab.nerc.ac.uk/collection/L22/current/TOOL0053"/>
	<skos:narrower rdf:resource="http://vocab.nerc.ac.uk/collection/L22/current/TOOL0100"/>
	<skos:narrower rdf:resource="http://vocab.aodn.org.au/def/instrument/entity/39"/>
	<skos:narrower rdf:resource="http://vocab.nerc.ac.uk/collection/L22/current/TOOL0696"/>
	<skos:narrower rdf:resource="http://vocab.nerc.ac.uk/collection/L22/current/TOOL0729"/>
	<skos:narrower rdf:resource="http://vocab.nerc.ac.uk/collection/L22/current/TOOL0685"/>
	<skos:narrower rdf:resource="http://vocab.nerc.ac.uk/collection/L22/current/TOOL0731"/>
	<skos:narrower rdf:resource="http://vocab.nerc.ac.uk/collection/L22/current/TOOL0809"/>
	<skos:narrower rdf:resource="http://vocab.nerc.ac.uk/collection/L22/current/TOOL0720"/>
	<skos:narrower rdf:resource="http://vocab.nerc.ac.uk/collection/L22/current/TOOL1009"/>
	<skos:narrower rdf:resource="http://vocab.nerc.ac.uk/collection/L22/current/TOOL1010"/>
	<skos:narrower rdf:resource="http://vocab.nerc.ac.uk/collection/L22/current/TOOL1125"/>
	<skos:narrower rdf:resource="http://vocab.nerc.ac.uk/collection/L22/current/TOOL0040"/>
	<skos:narrower rdf:resource="http://vocab.nerc.ac.uk/collection/L22/current/TOOL0042"/>
	<skos:narrower rdf:resource="http://vocab.nerc.ac.uk/collection/L22/current/TOOL0047"/>
	<skos:narrower rdf:resource="http://vocab.nerc.ac.uk/collection/L22/current/TOOL0058"/>
	<skos:narrower rdf:resource="http://vocab.nerc.ac.uk/collection/L22/current/TOOL0173"/>
	<skos:narrower rdf:resource="http://vocab.nerc.ac.uk/collection/L22/current/TOOL0183"/>
	<skos:narrower rdf:resource="http://vocab.nerc.ac.uk/collection/L22/current/TOOL0446"/>
	<skos:narrower rdf:resource="http://vocab.nerc.ac.uk/collection/L22/current/TOOL0668"/>
	<skos:narrower rdf:resource="http://vocab.nerc.ac.uk/collection/L22/current/TOOL0669"/>
	<skos:narrower rdf:resource="http://vocab.nerc.ac.uk/collection/L22/current/TOOL0190"/>
	<skos:narrower rdf:resource="http://vocab.nerc.ac.uk/collection/L22/current/TOOL0667"/>
	<skos:narrower rdf:resource="http://vocab.nerc.ac.uk/collection/L22/current/TOOL0022"/>
	<skos:narrower rdf:resource="http://vocab.nerc.ac.uk/collection/L22/current/TOOL0054"/>
	<skos:narrower rdf:resource="http://vocab.nerc.ac.uk/collection/L22/current/TOOL0105"/>
	<skos:narrower rdf:resource="http://vocab.nerc.ac.uk/collection/L22/current/TOOL0181"/>
	<skos:narrower rdf:resource="http://vocab.nerc.ac.uk/collection/L22/current/TOOL0191"/>
	<skos:narrower rdf:resource="http://vocab.nerc.ac.uk/collection/L22/current/TOOL0266"/>
	<skos:narrower rdf:resource="http://vocab.nerc.ac.uk/collection/L22/current/TOOL0267"/>
	<skos:narrower rdf:resource="http://vocab.nerc.ac.uk/collection/L22/current/TOOL0416"/>
	<skos:narrower rdf:resource="http://vocab.nerc.ac.uk/collection/L22/current/TOOL0490"/>
	<skos:narrower rdf:resource="http://vocab.nerc.ac.uk/collection/L22/current/TOOL0640"/>
	<skos:narrower rdf:resource="http://vocab.nerc.ac.uk/collection/L22/current/TOOL0665"/>
	<skos:narrower rdf:resource="http://vocab.nerc.ac.uk/collection/L22/current/TOOL0670"/>
	<skos:narrower rdf:resource="http://vocab.nerc.ac.uk/collection/L22/current/TOOL0684"/>
	<skos:narrower rdf:resource="http://vocab.nerc.ac.uk/collection/L22/current/TOOL0687"/>
	<skos:narrower rdf:resource="http://vocab.nerc.ac.uk/collection/L22/current/TOOL0688"/>
	<skos:narrower rdf:resource="http://vocab.nerc.ac.uk/collection/L22/current/TOOL0706"/>
	<skos:narrower rdf:resource="http://vocab.nerc.ac.uk/collection/L22/current/TOOL0707"/>
	<skos:narrower rdf:resource="http://vocab.nerc.ac.uk/collection/L22/current/TOOL0712"/>
	<skos:narrower rdf:resource="http://vocab.nerc.ac.uk/collection/L22/current/TOOL0719"/>
	<skos:narrower rdf:resource="http://vocab.nerc.ac.uk/collection/L22/current/TOOL0728"/>
	<skos:narrower rdf:resource="http://vocab.nerc.ac.uk/collection/L22/current/TOOL1121"/>
	<skos:narrower rdf:resource="http://vocab.nerc.ac.uk/collection/L22/current/TOOL1122"/>
	<skos:narrower rdf:resource="http://vocab.nerc.ac.uk/collection/L22/current/TOOL1141"/>
	<skos:narrower rdf:resource="http://vocab.nerc.ac.uk/collection/L22/current/TOOL1162"/>
	<skos:narrower rdf:resource="http://vocab.nerc.ac.uk/collection/L22/current/TOOL1163"/>
	<skos:prefLabel xml:lang="en">water temperature sensor</skos:prefLabel>
	<skos:topConceptOf rdf:resource="http://vocab.aodn.org.au/def/instrument/1"/>
</rdf:Description>

<rdf:Description rdf:about="http://vocab.nerc.ac.uk/collection/L05/current/135">
	<rdf:type rdf:resource="http://www.w3.org/2000/01/rdf-schema#Resource"/>
	<rdf:type rdf:resource="http://www.w3.org/2004/02/skos/core#Concept"/>
	<dcterms:created rdf:datatype="http://www.w3.org/2001/XMLSchema#dateTime">2013-03-28T00:00:00Z</dcterms:created>
	<dc:publisher rdf:datatype="http://www.w3.org/2001/XMLSchema#string">British Oceanographic Data Centre (BODC)</dc:publisher>
	<dc:source rdf:datatype="http://www.w3.org/2001/XMLSchema#string">(L051) SeaDataNet device categories</dc:source>
	<skos:definition xml:lang="en">A group of rigidly-mounted temperature sensors sampled by a common data logger held at various depths in the water column.</skos:definition>
	<skos:inScheme rdf:resource="http://vocab.aodn.org.au/def/instrument/1"/>
	<skos:prefLabel xml:lang="en">thermistor chains</skos:prefLabel>
	<skos:topConceptOf rdf:resource="http://vocab.aodn.org.au/def/instrument/1"/>
</rdf:Description>

<rdf:Description rdf:about="http://vocab.nerc.ac.uk/collection/L05/current/14">
	<rdf:type rdf:resource="http://www.w3.org/2000/01/rdf-schema#Resource"/>
	<rdf:type rdf:resource="http://www.w3.org/2004/02/skos/core#Concept"/>
	<dcterms:created rdf:datatype="http://www.w3.org/2001/XMLSchema#dateTime">2013-03-28T00:00:00Z</dcterms:created>
	<dc:publisher rdf:datatype="http://www.w3.org/2001/XMLSchema#string">British Oceanographic Data Centre (BODC)</dc:publisher>
	<dc:source rdf:datatype="http://www.w3.org/2001/XMLSchema#string">(L051) SeaDataNet device categories</dc:source>
	<skos:definition xml:lang="en">A device that collects a sample of precipitation (rain hail or snow) as it falls</skos:definition>
	<skos:inScheme rdf:resource="http://vocab.aodn.org.au/def/instrument/1"/>
	<skos:prefLabel xml:lang="en">precipitation samplers</skos:prefLabel>
	<skos:topConceptOf rdf:resource="http://vocab.aodn.org.au/def/instrument/1"/>
</rdf:Description>

<rdf:Description rdf:about="http://vocab.nerc.ac.uk/collection/L05/current/151">
	<rdf:type rdf:resource="http://www.w3.org/2000/01/rdf-schema#Resource"/>
	<rdf:type rdf:resource="http://www.w3.org/2004/02/skos/core#Concept"/>
	<dcterms:created rdf:datatype="http://www.w3.org/2001/XMLSchema#dateTime">2014-05-22T00:00:00Z</dcterms:created>
	<dc:publisher rdf:datatype="http://www.w3.org/2001/XMLSchema#string">British Oceanographic Data Centre (BODC)</dc:publisher>
	<dc:source rdf:datatype="http://www.w3.org/2001/XMLSchema#string">(L051) SeaDataNet device categories</dc:source>
	<skos:definition xml:lang="en">A device that isolates a portion of seabed plus overlying water from its surroundings. Either returns the entire system to the surface or incorporates sampling devices and/or in-situ sensors.</skos:definition>
	<skos:inScheme rdf:resource="http://vocab.aodn.org.au/def/instrument/1"/>
	<skos:prefLabel xml:lang="en">benthic incubation chambers</skos:prefLabel>
	<skos:topConceptOf rdf:resource="http://vocab.aodn.org.au/def/instrument/1"/>
</rdf:Description>

<rdf:Description rdf:about="http://vocab.nerc.ac.uk/collection/L05/current/157">
	<rdf:type rdf:resource="http://www.w3.org/2000/01/rdf-schema#Resource"/>
	<rdf:type rdf:resource="http://www.w3.org/2004/02/skos/core#Concept"/>
	<dcterms:created rdf:datatype="http://www.w3.org/2001/XMLSchema#dateTime">2014-05-22T00:00:00Z</dcterms:created>
	<dc:publisher rdf:datatype="http://www.w3.org/2001/XMLSchema#string">British Oceanographic Data Centre (BODC)</dc:publisher>
	<dc:source rdf:datatype="http://www.w3.org/2001/XMLSchema#string">(L051) SeaDataNet device categories</dc:source>
	<skos:definition xml:lang="en">Instruments that measure water depth along several tracks parallel to the platform track by timing pulses of sound reflected on the seafloor</skos:definition>
	<skos:inScheme rdf:resource="http://vocab.aodn.org.au/def/instrument/1"/>
	<skos:narrower rdf:resource="http://vocab.nerc.ac.uk/collection/L22/current/TOOL0916"/>
	<skos:prefLabel xml:lang="en">multi-beam echosounders</skos:prefLabel>
	<skos:topConceptOf rdf:resource="http://vocab.aodn.org.au/def/instrument/1"/>
</rdf:Description>

<rdf:Description rdf:about="http://vocab.nerc.ac.uk/collection/L05/current/180">
	<rdf:type rdf:resource="http://www.w3.org/2000/01/rdf-schema#Resource"/>
	<rdf:type rdf:resource="http://www.w3.org/2004/02/skos/core#Concept"/>
	<dcterms:created rdf:datatype="http://www.w3.org/2001/XMLSchema#dateTime">2013-03-28T00:00:00Z</dcterms:created>
	<dc:publisher rdf:datatype="http://www.w3.org/2001/XMLSchema#string">British Oceanographic Data Centre (BODC)</dc:publisher>
	<dc:source rdf:datatype="http://www.w3.org/2001/XMLSchema#string">(L051) SeaDataNet device categories</dc:source>
	<skos:definition xml:lang="en">All types of photographic equipment that may be deployed underwater including stills video film and digital systems</skos:definition>
	<skos:inScheme rdf:resource="http://vocab.aodn.org.au/def/instrument/1"/>
	<skos:prefLabel xml:lang="en">underwater cameras</skos:prefLabel>
	<skos:topConceptOf rdf:resource="http://vocab.aodn.org.au/def/instrument/1"/>
</rdf:Description>

<rdf:Description rdf:about="http://vocab.nerc.ac.uk/collection/L05/current/181">
	<rdf:type rdf:resource="http://www.w3.org/2000/01/rdf-schema#Resource"/>
	<rdf:type rdf:resource="http://www.w3.org/2004/02/skos/core#Concept"/>
	<dcterms:created rdf:datatype="http://www.w3.org/2001/XMLSchema#dateTime">2013-07-18T00:00:00Z</dcterms:created>
	<dc:publisher rdf:datatype="http://www.w3.org/2001/XMLSchema#string">British Oceanographic Data Centre (BODC)</dc:publisher>
	<dc:source rdf:datatype="http://www.w3.org/2001/XMLSchema#string">(L051) SeaDataNet device categories</dc:source>
	<skos:definition xml:lang="en">Instrument that makes in-situ measurements of one or more of nitrate nitrite ammonium urea phosphate or silicate dissolved in the water column</skos:definition>
	<skos:inScheme rdf:resource="http://vocab.aodn.org.au/def/instrument/1"/>
	<skos:narrower rdf:resource="http://vocab.nerc.ac.uk/collection/L22/current/TOOL0528"/>
	<skos:prefLabel xml:lang="en">nutrient analysers</skos:prefLabel>
	<skos:topConceptOf rdf:resource="http://vocab.aodn.org.au/def/instrument/1"/>
</rdf:Description>

<rdf:Description rdf:about="http://vocab.nerc.ac.uk/collection/L05/current/183">
	<rdf:type rdf:resource="http://www.w3.org/2000/01/rdf-schema#Resource"/>
	<rdf:type rdf:resource="http://www.w3.org/2004/02/skos/core#Concept"/>
	<dcterms:created rdf:datatype="http://www.w3.org/2001/XMLSchema#dateTime">2013-03-28T00:00:00Z</dcterms:created>
	<dc:publisher rdf:datatype="http://www.w3.org/2001/XMLSchema#string">British Oceanographic Data Centre (BODC)</dc:publisher>
	<dc:source rdf:datatype="http://www.w3.org/2001/XMLSchema#string">(L051) SeaDataNet device categories</dc:source>
	<skos:definition xml:lang="en">Instrument that measures the amount of sound energy transmitted into the water column returned to the instrument.</skos:definition>
	<skos:inScheme rdf:resource="http://vocab.aodn.org.au/def/instrument/1"/>
	<skos:prefLabel xml:lang="en">acoustic backscatter sensors</skos:prefLabel>
	<skos:topConceptOf rdf:resource="http://vocab.aodn.org.au/def/instrument/1"/>
</rdf:Description>

<rdf:Description rdf:about="http://vocab.nerc.ac.uk/collection/L05/current/185">
	<rdf:type rdf:resource="http://www.w3.org/2000/01/rdf-schema#Resource"/>
	<rdf:type rdf:resource="http://www.w3.org/2004/02/skos/core#Concept"/>
	<dcterms:created rdf:datatype="http://www.w3.org/2001/XMLSchema#dateTime">2013-03-28T00:00:00Z</dcterms:created>
	<dc:publisher rdf:datatype="http://www.w3.org/2001/XMLSchema#string">British Oceanographic Data Centre (BODC)</dc:publisher>
	<dc:source rdf:datatype="http://www.w3.org/2001/XMLSchema#string">(L051) SeaDataNet device categories</dc:source>
	<skos:definition xml:lang="en">Instrument that measures the velocity of sound in seawater</skos:definition>
	<skos:inScheme rdf:resource="http://vocab.aodn.org.au/def/instrument/1"/>
	<skos:prefLabel xml:lang="en">sound velocity sensors</skos:prefLabel>
	<skos:topConceptOf rdf:resource="http://vocab.aodn.org.au/def/instrument/1"/>
</rdf:Description>

<rdf:Description rdf:about="http://vocab.nerc.ac.uk/collection/L05/current/186">
	<rdf:type rdf:resource="http://www.w3.org/2000/01/rdf-schema#Resource"/>
	<rdf:type rdf:resource="http://www.w3.org/2004/02/skos/core#Concept"/>
	<dcterms:created rdf:datatype="http://www.w3.org/2001/XMLSchema#dateTime">2013-07-18T00:00:00Z</dcterms:created>
	<dc:publisher rdf:datatype="http://www.w3.org/2001/XMLSchema#string">British Oceanographic Data Centre (BODC)</dc:publisher>
	<dc:source rdf:datatype="http://www.w3.org/2001/XMLSchema#string">(L051) SeaDataNet device categories</dc:source>
	<skos:definition xml:lang="en">Instruments that determine the distance between the platform and the Earth's surface by timing reflected electromagnetic radiation usually microwaves.</skos:definition>
	<skos:inScheme rdf:resource="http://vocab.aodn.org.au/def/instrument/1"/>
	<skos:prefLabel xml:lang="en">radar altimeters</skos:prefLabel>
	<skos:topConceptOf rdf:resource="http://vocab.aodn.org.au/def/instrument/1"/>
</rdf:Description>

<rdf:Description rdf:about="http://vocab.nerc.ac.uk/collection/L05/current/21">
	<rdf:type rdf:resource="http://www.w3.org/2000/01/rdf-schema#Resource"/>
	<rdf:type rdf:resource="http://www.w3.org/2004/02/skos/core#Concept"/>
	<dcterms:created rdf:datatype="http://www.w3.org/2001/XMLSchema#dateTime">2013-03-28T00:00:00Z</dcterms:created>
	<dc:publisher rdf:datatype="http://www.w3.org/2001/XMLSchema#string">British Oceanographic Data Centre (BODC)</dc:publisher>
	<dc:source rdf:datatype="http://www.w3.org/2001/XMLSchema#string">(L051) SeaDataNet device categories</dc:source>
	<skos:definition xml:lang="en">A device that continuously samples a flow of water separating and fixing plankton for subsequent identification and counting</skos:definition>
	<skos:inScheme rdf:resource="http://vocab.aodn.org.au/def/instrument/1"/>
	<skos:narrower rdf:resource="http://vocab.nerc.ac.uk/collection/L22/current/NETT0026"/>
	<skos:prefLabel xml:lang="en">plankton recorders</skos:prefLabel>
	<skos:topConceptOf rdf:resource="http://vocab.aodn.org.au/def/instrument/1"/>
</rdf:Description>

<rdf:Description rdf:about="http://vocab.nerc.ac.uk/collection/L05/current/22">
	<rdf:type rdf:resource="http://www.w3.org/2000/01/rdf-schema#Resource"/>
	<rdf:type rdf:resource="http://www.w3.org/2004/02/skos/core#Concept"/>
	<dcterms:created rdf:datatype="http://www.w3.org/2001/XMLSchema#dateTime">2013-07-18T00:00:00Z</dcterms:created>
	<dc:publisher rdf:datatype="http://www.w3.org/2001/XMLSchema#string">British Oceanographic Data Centre (BODC)</dc:publisher>
	<dc:source rdf:datatype="http://www.w3.org/2001/XMLSchema#string">(L051) SeaDataNet device categories</dc:source>
	<skos:definition xml:lang="en">A fine-meshed net designed for sampling microzooplankton mesozooplankton or nekton.</skos:definition>
	<skos:inScheme rdf:resource="http://vocab.aodn.org.au/def/instrument/1"/>
	<skos:narrower rdf:resource="http://vocab.nerc.ac.uk/collection/L22/current/NETT0044"/>
	<skos:prefLabel xml:lang="en">plankton nets</skos:prefLabel>
	<skos:topConceptOf rdf:resource="http://vocab.aodn.org.au/def/instrument/1"/>
</rdf:Description>

<rdf:Description rdf:about="http://vocab.nerc.ac.uk/collection/L05/current/23">
	<rdf:type rdf:resource="http://www.w3.org/2000/01/rdf-schema#Resource"/>
	<rdf:type rdf:resource="http://www.w3.org/2004/02/skos/core#Concept"/>
	<dcterms:created rdf:datatype="http://www.w3.org/2001/XMLSchema#dateTime">2014-05-22T00:00:00Z</dcterms:created>
	<dc:publisher rdf:datatype="http://www.w3.org/2001/XMLSchema#string">British Oceanographic Data Centre (BODC)</dc:publisher>
	<dc:source rdf:datatype="http://www.w3.org/2001/XMLSchema#string">(L051) SeaDataNet device categories</dc:source>
	<skos:definition xml:lang="en">A net towed through the water column designed to sample free-swimming nekton or fish.</skos:definition>
	<skos:inScheme rdf:resource="http://vocab.aodn.org.au/def/instrument/1"/>
	<skos:prefLabel xml:lang="en">pelagic trawl nets</skos:prefLabel>
	<skos:topConceptOf rdf:resource="http://vocab.aodn.org.au/def/instrument/1"/>
</rdf:Description>

<rdf:Description rdf:about="http://vocab.nerc.ac.uk/collection/L05/current/24">
	<rdf:type rdf:resource="http://www.w3.org/2000/01/rdf-schema#Resource"/>
	<rdf:type rdf:resource="http://www.w3.org/2004/02/skos/core#Concept"/>
	<dcterms:created rdf:datatype="http://www.w3.org/2001/XMLSchema#dateTime">2014-05-22T00:00:00Z</dcterms:created>
	<dc:publisher rdf:datatype="http://www.w3.org/2001/XMLSchema#string">British Oceanographic Data Centre (BODC)</dc:publisher>
	<dc:source rdf:datatype="http://www.w3.org/2001/XMLSchema#string">(L051) SeaDataNet device categories</dc:source>
	<skos:definition xml:lang="en">A net or sledge dragged across the seabed designed to sample benthic fauna.</skos:definition>
	<skos:inScheme rdf:resource="http://vocab.aodn.org.au/def/instrument/1"/>
	<skos:prefLabel xml:lang="en">benthos samplers</skos:prefLabel>
	<skos:topConceptOf rdf:resource="http://vocab.aodn.org.au/def/instrument/1"/>
</rdf:Description>

<rdf:Description rdf:about="http://vocab.nerc.ac.uk/collection/L05/current/30">
	<rdf:type rdf:resource="http://www.w3.org/2000/01/rdf-schema#Resource"/>
	<rdf:type rdf:resource="http://www.w3.org/2004/02/skos/core#Concept"/>
	<dcterms:contributor rdf:resource="http://editor.vocabs.ands.org.au/user/eMII_Atkins.Natalia"/>
	<dcterms:created rdf:datatype="http://www.w3.org/2001/XMLSchema#dateTime">2013-03-28T00:00:00Z</dcterms:created>
	<dcterms:modified rdf:datatype="http://www.w3.org/2001/XMLSchema#dateTime">2015-09-21T23:41:43Z</dcterms:modified>
	<dc:publisher rdf:datatype="http://www.w3.org/2001/XMLSchema#string">British Oceanographic Data Centre (BODC)</dc:publisher>
	<dc:source rdf:datatype="http://www.w3.org/2001/XMLSchema#string">(L051) SeaDataNet device categories</dc:source>
	<skos:definition xml:lang="en">A device that collects an in-situ discrete water sample from any depth and returns it to the surface without contamination by the waters through which it passes such as a water bottle</skos:definition>
	<skos:inScheme rdf:resource="http://vocab.aodn.org.au/def/instrument/1"/>
	<skos:narrower rdf:resource="http://vocab.nerc.ac.uk/collection/L22/current/TOOL0939"/>
	<skos:prefLabel xml:lang="en">discrete water samplers</skos:prefLabel>
	<skos:topConceptOf rdf:resource="http://vocab.aodn.org.au/def/instrument/1"/>
</rdf:Description>

<rdf:Description rdf:about="http://vocab.nerc.ac.uk/collection/L05/current/301">
	<rdf:type rdf:resource="http://www.w3.org/2000/01/rdf-schema#Resource"/>
	<rdf:type rdf:resource="http://www.w3.org/2004/02/skos/core#Concept"/>
	<dcterms:created rdf:datatype="http://www.w3.org/2001/XMLSchema#dateTime">2013-07-18T00:00:00Z</dcterms:created>
	<dc:publisher rdf:datatype="http://www.w3.org/2001/XMLSchema#string">British Oceanographic Data Centre (BODC)</dc:publisher>
	<dc:source rdf:datatype="http://www.w3.org/2001/XMLSchema#string">(L051) SeaDataNet device categories</dc:source>
	<skos:definition xml:lang="en">A network of statellites that generate signals that allow a receiver to determine its position such as GPS.</skos:definition>
	<skos:inScheme rdf:resource="http://vocab.aodn.org.au/def/instrument/1"/>
	<skos:prefLabel xml:lang="en">satellite positioning systems</skos:prefLabel>
	<skos:topConceptOf rdf:resource="http://vocab.aodn.org.au/def/instrument/1"/>
</rdf:Description>

<rdf:Description rdf:about="http://vocab.nerc.ac.uk/collection/L05/current/303">
	<rdf:type rdf:resource="http://www.w3.org/2000/01/rdf-schema#Resource"/>
	<rdf:type rdf:resource="http://www.w3.org/2004/02/skos/core#Concept"/>
	<dcterms:created rdf:datatype="http://www.w3.org/2001/XMLSchema#dateTime">2013-03-28T00:00:00Z</dcterms:created>
	<dc:publisher rdf:datatype="http://www.w3.org/2001/XMLSchema#string">British Oceanographic Data Centre (BODC)</dc:publisher>
	<dc:source rdf:datatype="http://www.w3.org/2001/XMLSchema#string">(L051) SeaDataNet device categories</dc:source>
	<skos:definition xml:lang="en">Instruments that measure the speed and direction of sea surface travel by timing reflected radio waves</skos:definition>
	<skos:inScheme rdf:resource="http://vocab.aodn.org.au/def/instrument/1"/>
	<skos:prefLabel xml:lang="en">surface current radars</skos:prefLabel>
	<skos:topConceptOf rdf:resource="http://vocab.aodn.org.au/def/instrument/1"/>
</rdf:Description>

<rdf:Description rdf:about="http://vocab.nerc.ac.uk/collection/L05/current/304">
	<rdf:type rdf:resource="http://www.w3.org/2000/01/rdf-schema#Resource"/>
	<rdf:type rdf:resource="http://www.w3.org/2004/02/skos/core#Concept"/>
	<dcterms:created rdf:datatype="http://www.w3.org/2001/XMLSchema#dateTime">2013-09-24T00:00:00Z</dcterms:created>
	<dc:publisher rdf:datatype="http://www.w3.org/2001/XMLSchema#string">British Oceanographic Data Centre (BODC)</dc:publisher>
	<dc:source rdf:datatype="http://www.w3.org/2001/XMLSchema#string">(L051) SeaDataNet device categories</dc:source>
	<skos:definition xml:lang="en">Sensors that measure the intensity and nature of electromagnetic radiation in a manner optimised for the determination of ocean chlorophyll concentration.</skos:definition>
	<skos:inScheme rdf:resource="http://vocab.aodn.org.au/def/instrument/1"/>
	<skos:narrower rdf:resource="http://vocab.nerc.ac.uk/collection/L22/current/TOOL1120"/>
	<skos:prefLabel xml:lang="en">ocean colour radiometers</skos:prefLabel>
	<skos:topConceptOf rdf:resource="http://vocab.aodn.org.au/def/instrument/1"/>
</rdf:Description>

<rdf:Description rdf:about="http://vocab.nerc.ac.uk/collection/L05/current/305">
	<rdf:type rdf:resource="http://www.w3.org/2000/01/rdf-schema#Resource"/>
	<rdf:type rdf:resource="http://www.w3.org/2004/02/skos/core#Concept"/>
	<dcterms:created rdf:datatype="http://www.w3.org/2001/XMLSchema#dateTime">2014-05-22T00:00:00Z</dcterms:created>
	<dc:publisher rdf:datatype="http://www.w3.org/2001/XMLSchema#string">British Oceanographic Data Centre (BODC)</dc:publisher>
	<dc:source rdf:datatype="http://www.w3.org/2001/XMLSchema#string">(L051) SeaDataNet device categories</dc:source>
	<skos:definition xml:lang="en">Sensors that measure the reflection or scattering effect produced while scanning the surface of the earth. Primarily used to measure near surface winds over the oceans.</skos:definition>
	<skos:inScheme rdf:resource="http://vocab.aodn.org.au/def/instrument/1"/>
	<skos:prefLabel xml:lang="en">scatterometers</skos:prefLabel>
	<skos:topConceptOf rdf:resource="http://vocab.aodn.org.au/def/instrument/1"/>
</rdf:Description>

<rdf:Description rdf:about="http://vocab.nerc.ac.uk/collection/L05/current/306">
	<rdf:type rdf:resource="http://www.w3.org/2000/01/rdf-schema#Resource"/>
	<rdf:type rdf:resource="http://www.w3.org/2004/02/skos/core#Concept"/>
	<dcterms:created rdf:datatype="http://www.w3.org/2001/XMLSchema#dateTime">2014-05-22T00:00:00Z</dcterms:created>
	<dc:publisher rdf:datatype="http://www.w3.org/2001/XMLSchema#string">British Oceanographic Data Centre (BODC)</dc:publisher>
	<dc:source rdf:datatype="http://www.w3.org/2001/XMLSchema#string">(L051) SeaDataNet device categories</dc:source>
	<skos:definition xml:lang="en">Instruments that generate maps of radar reflectivity through the synthesis of multiple pulses from a moving platform.</skos:definition>
	<skos:inScheme rdf:resource="http://vocab.aodn.org.au/def/instrument/1"/>
	<skos:prefLabel xml:lang="en">synthetic aperture radars</skos:prefLabel>
	<skos:topConceptOf rdf:resource="http://vocab.aodn.org.au/def/instrument/1"/>
</rdf:Description>

<rdf:Description rdf:about="http://vocab.nerc.ac.uk/collection/L05/current/308">
	<rdf:type rdf:resource="http://www.w3.org/2000/01/rdf-schema#Resource"/>
	<rdf:type rdf:resource="http://www.w3.org/2004/02/skos/core#Concept"/>
	<dcterms:created rdf:datatype="http://www.w3.org/2001/XMLSchema#dateTime">2014-07-11T00:00:00Z</dcterms:created>
	<dc:publisher rdf:datatype="http://www.w3.org/2001/XMLSchema#string">British Oceanographic Data Centre (BODC)</dc:publisher>
	<dc:source rdf:datatype="http://www.w3.org/2001/XMLSchema#string">(L051) SeaDataNet device categories</dc:source>
	<skos:definition xml:lang="en">Sensors that measure the intensity an nature of electromagnetic radiation in a manner optimised for the quantification of atmospheric phenomena.</skos:definition>
	<skos:inScheme rdf:resource="http://vocab.aodn.org.au/def/instrument/1"/>
	<skos:narrower rdf:resource="http://vocab.nerc.ac.uk/collection/L22/current/TOOL1120"/>
	<skos:narrower rdf:resource="http://vocab.nerc.ac.uk/collection/L22/current/TOOL0702"/>
	<skos:narrower rdf:resource="http://vocab.nerc.ac.uk/collection/L22/current/TOOL0703"/>
	<skos:narrower rdf:resource="http://vocab.nerc.ac.uk/collection/L22/current/TOOL0722"/>
	<skos:narrower rdf:resource="http://vocab.nerc.ac.uk/collection/L22/current/TOOL0723"/>
	<skos:prefLabel xml:lang="en">atmospheric radiometers</skos:prefLabel>
	<skos:topConceptOf rdf:resource="http://vocab.aodn.org.au/def/instrument/1"/>
</rdf:Description>

<rdf:Description rdf:about="http://vocab.nerc.ac.uk/collection/L05/current/31">
	<rdf:type rdf:resource="http://www.w3.org/2000/01/rdf-schema#Resource"/>
	<rdf:type rdf:resource="http://www.w3.org/2004/02/skos/core#Concept"/>
	<dcterms:created rdf:datatype="http://www.w3.org/2001/XMLSchema#dateTime">2013-03-28T00:00:00Z</dcterms:created>
	<dc:publisher rdf:datatype="http://www.w3.org/2001/XMLSchema#string">British Oceanographic Data Centre (BODC)</dc:publisher>
	<dc:source rdf:datatype="http://www.w3.org/2001/XMLSchema#string">(L051) SeaDataNet device categories</dc:source>
	<skos:definition xml:lang="en">A device that continuously supplies a flow of water either to an analytical instrument over a sensor or from which samples may be drawn</skos:definition>
	<skos:inScheme rdf:resource="http://vocab.aodn.org.au/def/instrument/1"/>
	<skos:prefLabel xml:lang="en">continuous water samplers</skos:prefLabel>
	<skos:topConceptOf rdf:resource="http://vocab.aodn.org.au/def/instrument/1"/>
</rdf:Description>

<rdf:Description rdf:about="http://vocab.nerc.ac.uk/collection/L05/current/310">
	<rdf:type rdf:resource="http://www.w3.org/2000/01/rdf-schema#Resource"/>
	<rdf:type rdf:resource="http://www.w3.org/2004/02/skos/core#Concept"/>
	<dcterms:created rdf:datatype="http://www.w3.org/2001/XMLSchema#dateTime">2014-05-22T00:00:00Z</dcterms:created>
	<dc:publisher rdf:datatype="http://www.w3.org/2001/XMLSchema#string">British Oceanographic Data Centre (BODC)</dc:publisher>
	<dc:source rdf:datatype="http://www.w3.org/2001/XMLSchema#string">(L051) SeaDataNet device categories</dc:source>
	<skos:definition xml:lang="en">Instruments that determine the distance between the platform and the Earth's surface by timing reflected pulses of laser light.</skos:definition>
	<skos:inScheme rdf:resource="http://vocab.aodn.org.au/def/instrument/1"/>
	<skos:prefLabel xml:lang="en">laser altimeters</skos:prefLabel>
	<skos:topConceptOf rdf:resource="http://vocab.aodn.org.au/def/instrument/1"/>
</rdf:Description>

<rdf:Description rdf:about="http://vocab.nerc.ac.uk/collection/L05/current/311">
	<rdf:type rdf:resource="http://www.w3.org/2000/01/rdf-schema#Resource"/>
	<rdf:type rdf:resource="http://www.w3.org/2004/02/skos/core#Concept"/>
	<dcterms:created rdf:datatype="http://www.w3.org/2001/XMLSchema#dateTime">2014-05-22T00:00:00Z</dcterms:created>
	<dc:publisher rdf:datatype="http://www.w3.org/2001/XMLSchema#string">British Oceanographic Data Centre (BODC)</dc:publisher>
	<dc:source rdf:datatype="http://www.w3.org/2001/XMLSchema#string">(L051) SeaDataNet device categories</dc:source>
	<skos:definition xml:lang="en">All types of photographic equipment that may be deployed in aircraft or satellites including stills video film and digital systems.</skos:definition>
	<skos:inScheme rdf:resource="http://vocab.aodn.org.au/def/instrument/1"/>
	<skos:prefLabel xml:lang="en">cameras</skos:prefLabel>
	<skos:topConceptOf rdf:resource="http://vocab.aodn.org.au/def/instrument/1"/>
</rdf:Description>

<rdf:Description rdf:about="http://vocab.nerc.ac.uk/collection/L05/current/312">
	<rdf:type rdf:resource="http://www.w3.org/2000/01/rdf-schema#Resource"/>
	<rdf:type rdf:resource="http://www.w3.org/2004/02/skos/core#Concept"/>
	<dcterms:created rdf:datatype="http://www.w3.org/2001/XMLSchema#dateTime">2014-05-22T00:00:00Z</dcterms:created>
	<dc:publisher rdf:datatype="http://www.w3.org/2001/XMLSchema#string">British Oceanographic Data Centre (BODC)</dc:publisher>
	<dc:source rdf:datatype="http://www.w3.org/2001/XMLSchema#string">(L051) SeaDataNet device categories</dc:source>
	<skos:definition xml:lang="en">Instruments that measure the depth of a water body by determining the distances from the platform to the surface and the bed by timing reflected pulses of laser light.</skos:definition>
	<skos:inScheme rdf:resource="http://vocab.aodn.org.au/def/instrument/1"/>
	<skos:prefLabel xml:lang="en">bathymetric LiDARs</skos:prefLabel>
	<skos:topConceptOf rdf:resource="http://vocab.aodn.org.au/def/instrument/1"/>
</rdf:Description>

<rdf:Description rdf:about="http://vocab.nerc.ac.uk/collection/L05/current/33">
	<rdf:type rdf:resource="http://www.w3.org/2000/01/rdf-schema#Resource"/>
	<rdf:type rdf:resource="http://www.w3.org/2004/02/skos/core#Concept"/>
	<dcterms:created rdf:datatype="http://www.w3.org/2001/XMLSchema#dateTime">2013-03-28T00:00:00Z</dcterms:created>
	<dc:publisher rdf:datatype="http://www.w3.org/2001/XMLSchema#string">British Oceanographic Data Centre (BODC)</dc:publisher>
	<dc:source rdf:datatype="http://www.w3.org/2001/XMLSchema#string">(L051) SeaDataNet device categories</dc:source>
	<skos:definition xml:lang="en">A collector of particulates as they sink through the water column</skos:definition>
	<skos:inScheme rdf:resource="http://vocab.aodn.org.au/def/instrument/1"/>
	<skos:narrower rdf:resource="http://vocab.nerc.ac.uk/collection/L22/current/TOOL0917"/>
	<skos:narrower rdf:resource="http://vocab.nerc.ac.uk/collection/L22/current/TOOL0785"/>
	<skos:narrower rdf:resource="http://vocab.nerc.ac.uk/collection/L22/current/TOOL0786"/>
	<skos:prefLabel xml:lang="en">sediment traps</skos:prefLabel>
	<skos:topConceptOf rdf:resource="http://vocab.aodn.org.au/def/instrument/1"/>
</rdf:Description>

<rdf:Description rdf:about="http://vocab.nerc.ac.uk/collection/L05/current/350">
	<rdf:type rdf:resource="http://www.w3.org/2000/01/rdf-schema#Resource"/>
	<rdf:type rdf:resource="http://www.w3.org/2004/02/skos/core#Concept"/>
	<dcterms:contributor rdf:resource="http://editor.vocabs.ands.org.au/user/eMII_Atkins.Natalia"/>
	<dcterms:created rdf:datatype="http://www.w3.org/2001/XMLSchema#dateTime">2013-10-10T00:00:00Z</dcterms:created>
	<dcterms:modified rdf:datatype="http://www.w3.org/2001/XMLSchema#dateTime">2017-03-23T04:09:32Z</dcterms:modified>
	<dc:publisher rdf:datatype="http://www.w3.org/2001/XMLSchema#string">British Oceanographic Data Centre (BODC)</dc:publisher>
	<dc:source rdf:datatype="http://www.w3.org/2001/XMLSchema#string">(L051) SeaDataNet device categories</dc:source>
	<skos:definition xml:lang="en">Instrument that simultaneously measures electrical conductivity and temperature in the water column to provide temperature and salinity data</skos:definition>
	<skos:inScheme rdf:resource="http://vocab.aodn.org.au/def/instrument/1"/>
	<skos:narrower rdf:resource="http://vocab.nerc.ac.uk/collection/L22/current/TOOL0869"/>
	<skos:narrower rdf:resource="http://vocab.nerc.ac.uk/collection/L22/current/TOOL0870"/>
	<skos:narrower rdf:resource="http://vocab.nerc.ac.uk/collection/L22/current/TOOL0871"/>
	<skos:narrower rdf:resource="http://vocab.nerc.ac.uk/collection/L22/current/TOOL0675"/>
	<skos:narrower rdf:resource="http://vocab.nerc.ac.uk/collection/L22/current/TOOL0017"/>
	<skos:narrower rdf:resource="http://vocab.nerc.ac.uk/collection/L22/current/TOOL0018"/>
	<skos:narrower rdf:resource="http://vocab.nerc.ac.uk/collection/L22/current/TOOL0019"/>
	<skos:narrower rdf:resource="http://vocab.nerc.ac.uk/collection/L22/current/TOOL0020"/>
	<skos:narrower rdf:resource="http://vocab.nerc.ac.uk/collection/L22/current/TOOL0023"/>
	<skos:narrower rdf:resource="http://vocab.nerc.ac.uk/collection/L22/current/TOOL0053"/>
	<skos:narrower rdf:resource="http://vocab.nerc.ac.uk/collection/L22/current/TOOL0100"/>
	<skos:narrower rdf:resource="http://vocab.nerc.ac.uk/collection/L22/current/TOOL0720"/>
	<skos:narrower rdf:resource="http://vocab.nerc.ac.uk/collection/L22/current/TOOL0040"/>
	<skos:narrower rdf:resource="http://vocab.nerc.ac.uk/collection/L22/current/TOOL0042"/>
	<skos:narrower rdf:resource="http://vocab.nerc.ac.uk/collection/L22/current/TOOL0047"/>
	<skos:narrower rdf:resource="http://vocab.nerc.ac.uk/collection/L22/current/TOOL0058"/>
	<skos:narrower rdf:resource="http://vocab.nerc.ac.uk/collection/L22/current/TOOL0173"/>
	<skos:narrower rdf:resource="http://vocab.nerc.ac.uk/collection/L22/current/TOOL0183"/>
	<skos:narrower rdf:resource="http://vocab.nerc.ac.uk/collection/L22/current/TOOL0446"/>
	<skos:narrower rdf:resource="http://vocab.nerc.ac.uk/collection/L22/current/TOOL0668"/>
	<skos:narrower rdf:resource="http://vocab.nerc.ac.uk/collection/L22/current/TOOL0669"/>
	<skos:narrower rdf:resource="http://vocab.nerc.ac.uk/collection/L22/current/TOOL0190"/>
	<skos:narrower rdf:resource="http://vocab.nerc.ac.uk/collection/L22/current/TOOL0667"/>
	<skos:narrower rdf:resource="http://vocab.nerc.ac.uk/collection/L22/current/TOOL0022"/>
	<skos:narrower rdf:resource="http://vocab.nerc.ac.uk/collection/L22/current/TOOL1162"/>
	<skos:narrower rdf:resource="http://vocab.nerc.ac.uk/collection/L22/current/TOOL1163"/>
	<skos:prefLabel xml:lang="en">salinity sensor</skos:prefLabel>
	<skos:topConceptOf rdf:resource="http://vocab.aodn.org.au/def/instrument/1"/>
</rdf:Description>

<rdf:Description rdf:about="http://vocab.nerc.ac.uk/collection/L05/current/351">
	<rdf:type rdf:resource="http://www.w3.org/2000/01/rdf-schema#Resource"/>
	<rdf:type rdf:resource="http://www.w3.org/2004/02/skos/core#Concept"/>
	<dcterms:contributor rdf:resource="http://editor.vocabs.ands.org.au/user/Natalia_Atkins"/>
	<dcterms:created rdf:datatype="http://www.w3.org/2001/XMLSchema#dateTime">2013-03-28T00:00:00Z</dcterms:created>
	<dcterms:modified rdf:datatype="http://www.w3.org/2001/XMLSchema#dateTime">2015-07-08T04:08:18Z</dcterms:modified>
	<dc:publisher rdf:datatype="http://www.w3.org/2001/XMLSchema#string">British Oceanographic Data Centre (BODC)</dc:publisher>
	<dc:source rdf:datatype="http://www.w3.org/2001/XMLSchema#string">(L051) SeaDataNet device categories</dc:source>
	<skos:definition xml:lang="en">Instrument that measures the concentration of gases generally oxygen dissolved in the water column</skos:definition>
	<skos:inScheme rdf:resource="http://vocab.aodn.org.au/def/instrument/1"/>
	<skos:narrower rdf:resource="http://vocab.nerc.ac.uk/collection/L22/current/TOOL0869"/>
	<skos:narrower rdf:resource="http://vocab.nerc.ac.uk/collection/L22/current/TOOL0878"/>
	<skos:narrower rdf:resource="http://vocab.nerc.ac.uk/collection/L22/current/TOOL0675"/>
	<skos:narrower rdf:resource="http://vocab.nerc.ac.uk/collection/L22/current/TOOL0036"/>
	<skos:narrower rdf:resource="http://vocab.nerc.ac.uk/collection/L22/current/TOOL0037"/>
	<skos:narrower rdf:resource="http://vocab.nerc.ac.uk/collection/L22/current/TOOL0369"/>
	<skos:narrower rdf:resource="http://vocab.nerc.ac.uk/collection/L22/current/TOOL0679"/>
	<skos:narrower rdf:resource="http://vocab.nerc.ac.uk/collection/L22/current/TOOL0724"/>
	<skos:narrower rdf:resource="http://vocab.nerc.ac.uk/collection/L22/current/TOOL0739"/>
	<skos:narrower rdf:resource="http://vocab.nerc.ac.uk/collection/L22/current/TOOL0805"/>
	<skos:narrower rdf:resource="http://vocab.nerc.ac.uk/collection/L22/current/TOOL0836"/>
	<skos:narrower rdf:resource="http://vocab.nerc.ac.uk/collection/L22/current/TOOL0103"/>
	<skos:narrower rdf:resource="http://vocab.nerc.ac.uk/collection/L22/current/TOOL0101"/>
	<skos:prefLabel xml:lang="en">dissolved gas sensors</skos:prefLabel>
	<skos:topConceptOf rdf:resource="http://vocab.aodn.org.au/def/instrument/1"/>
</rdf:Description>

<rdf:Description rdf:about="http://vocab.nerc.ac.uk/collection/L05/current/353">
	<rdf:type rdf:resource="http://www.w3.org/2000/01/rdf-schema#Resource"/>
	<rdf:type rdf:resource="http://www.w3.org/2004/02/skos/core#Concept"/>
	<dcterms:created rdf:datatype="http://www.w3.org/2001/XMLSchema#dateTime">2013-03-28T00:00:00Z</dcterms:created>
	<dc:publisher rdf:datatype="http://www.w3.org/2001/XMLSchema#string">British Oceanographic Data Centre (BODC)</dc:publisher>
	<dc:source rdf:datatype="http://www.w3.org/2001/XMLSchema#string">(L051) SeaDataNet device categories</dc:source>
	<skos:definition xml:lang="en">Fluorometers that measure photosynthetic parameters by taking measurements whilst manipulating the phytoplankton with controlled high-intensity illumination such as pump and probe and FRRF</skos:definition>
	<skos:inScheme rdf:resource="http://vocab.aodn.org.au/def/instrument/1"/>
	<skos:prefLabel xml:lang="en">active fluorometers</skos:prefLabel>
	<skos:topConceptOf rdf:resource="http://vocab.aodn.org.au/def/instrument/1"/>
</rdf:Description>

<rdf:Description rdf:about="http://vocab.nerc.ac.uk/collection/L05/current/355">
	<rdf:type rdf:resource="http://www.w3.org/2000/01/rdf-schema#Resource"/>
	<rdf:type rdf:resource="http://www.w3.org/2004/02/skos/core#Concept"/>
	<dcterms:created rdf:datatype="http://www.w3.org/2001/XMLSchema#dateTime">2013-07-18T00:00:00Z</dcterms:created>
	<dc:publisher rdf:datatype="http://www.w3.org/2001/XMLSchema#string">British Oceanographic Data Centre (BODC)</dc:publisher>
	<dc:source rdf:datatype="http://www.w3.org/2001/XMLSchema#string">(L051) SeaDataNet device categories</dc:source>
	<skos:definition xml:lang="en">Instruments that measure the hydrogen ion concentration in the water column</skos:definition>
	<skos:inScheme rdf:resource="http://vocab.aodn.org.au/def/instrument/1"/>
	<skos:prefLabel xml:lang="en">pH sensors</skos:prefLabel>
	<skos:topConceptOf rdf:resource="http://vocab.aodn.org.au/def/instrument/1"/>
</rdf:Description>

<rdf:Description rdf:about="http://vocab.nerc.ac.uk/collection/L05/current/356">
	<rdf:type rdf:resource="http://www.w3.org/2000/01/rdf-schema#Resource"/>
	<rdf:type rdf:resource="http://www.w3.org/2004/02/skos/core#Concept"/>
	<dcterms:created rdf:datatype="http://www.w3.org/2001/XMLSchema#dateTime">2013-07-18T00:00:00Z</dcterms:created>
	<dc:publisher rdf:datatype="http://www.w3.org/2001/XMLSchema#string">British Oceanographic Data Centre (BODC)</dc:publisher>
	<dc:source rdf:datatype="http://www.w3.org/2001/XMLSchema#string">(L051) SeaDataNet device categories</dc:source>
	<skos:definition xml:lang="en">Instruments that measure the tendency of the water column to either gain or lose electrons when it is subject to change by introduction of a new species</skos:definition>
	<skos:inScheme rdf:resource="http://vocab.aodn.org.au/def/instrument/1"/>
	<skos:prefLabel xml:lang="en">redox potential sensors</skos:prefLabel>
	<skos:topConceptOf rdf:resource="http://vocab.aodn.org.au/def/instrument/1"/>
</rdf:Description>

<rdf:Description rdf:about="http://vocab.nerc.ac.uk/collection/L05/current/369">
	<rdf:type rdf:resource="http://www.w3.org/2000/01/rdf-schema#Resource"/>
	<rdf:type rdf:resource="http://www.w3.org/2004/02/skos/core#Concept"/>
	<dcterms:created rdf:datatype="http://www.w3.org/2001/XMLSchema#dateTime">2013-03-28T00:00:00Z</dcterms:created>
	<dc:publisher rdf:datatype="http://www.w3.org/2001/XMLSchema#string">British Oceanographic Data Centre (BODC)</dc:publisher>
	<dc:source rdf:datatype="http://www.w3.org/2001/XMLSchema#string">(L051) SeaDataNet device categories</dc:source>
	<skos:definition xml:lang="en">Devices containing transducers that convert underwater sound waves into electrical signals.</skos:definition>
	<skos:inScheme rdf:resource="http://vocab.aodn.org.au/def/instrument/1"/>
	<skos:narrower rdf:resource="http://vocab.nerc.ac.uk/collection/L22/current/TOOL0663"/>
	<skos:narrower rdf:resource="http://vocab.nerc.ac.uk/collection/L22/current/TOOL1159"/>
	<skos:narrower rdf:resource="http://vocab.nerc.ac.uk/collection/L22/current/TOOL1160"/>
	<skos:narrower rdf:resource="http://vocab.nerc.ac.uk/collection/L22/current/TOOL1161"/>
	<skos:narrower rdf:resource="http://vocab.nerc.ac.uk/collection/L22/current/TOOL1164"/>
	<skos:prefLabel xml:lang="en">hydrophones</skos:prefLabel>
	<skos:topConceptOf rdf:resource="http://vocab.aodn.org.au/def/instrument/1"/>
</rdf:Description>

<rdf:Description rdf:about="http://vocab.nerc.ac.uk/collection/L05/current/377">
	<rdf:type rdf:resource="http://www.w3.org/2000/01/rdf-schema#Resource"/>
	<rdf:type rdf:resource="http://www.w3.org/2004/02/skos/core#Concept"/>
	<dcterms:created rdf:datatype="http://www.w3.org/2001/XMLSchema#dateTime">2014-05-22T00:00:00Z</dcterms:created>
	<dc:publisher rdf:datatype="http://www.w3.org/2001/XMLSchema#string">British Oceanographic Data Centre (BODC)</dc:publisher>
	<dc:source rdf:datatype="http://www.w3.org/2001/XMLSchema#string">(L051) SeaDataNet device categories</dc:source>
	<skos:definition xml:lang="en">Fixed physical markers that allow changes in the position of the boundary between a water body and the atmosphere by visible comparison against marked graduations in units of measurement of dimension length.</skos:definition>
	<skos:inScheme rdf:resource="http://vocab.aodn.org.au/def/instrument/1"/>
	<skos:prefLabel xml:lang="en">water level markers</skos:prefLabel>
	<skos:topConceptOf rdf:resource="http://vocab.aodn.org.au/def/instrument/1"/>
</rdf:Description>

<rdf:Description rdf:about="http://vocab.nerc.ac.uk/collection/L05/current/379">
	<rdf:type rdf:resource="http://www.w3.org/2000/01/rdf-schema#Resource"/>
	<rdf:type rdf:resource="http://www.w3.org/2004/02/skos/core#Concept"/>
	<dcterms:contributor rdf:resource="http://editor.vocabs.ands.org.au/user/eMII_Atkins.Natalia"/>
	<dcterms:created rdf:datatype="http://www.w3.org/2001/XMLSchema#dateTime">2013-07-18T00:00:00Z</dcterms:created>
	<dcterms:modified rdf:datatype="http://www.w3.org/2001/XMLSchema#dateTime">2016-10-21T02:27:06Z</dcterms:modified>
	<dc:publisher rdf:datatype="http://www.w3.org/2001/XMLSchema#string">British Oceanographic Data Centre (BODC)</dc:publisher>
	<dc:source rdf:datatype="http://www.w3.org/2001/XMLSchema#string">(L051) SeaDataNet device categories</dc:source>
	<skos:definition xml:lang="en">Instruments that measure their distance above a specified elevation such as the sea surface or the seabed. Classification includes acoustic and pressure-based instruments that are designed to provide platform z co-ordinate spatial coverage in the atmosphere or a water body. It excludes remote sensing instruments such as LIDAR and satellite radar altimeters designed to map surface elevation.</skos:definition>
	<skos:inScheme rdf:resource="http://vocab.aodn.org.au/def/instrument/1"/>
	<skos:narrower rdf:resource="http://vocab.nerc.ac.uk/collection/L22/current/TOOL0872"/>
	<skos:prefLabel xml:lang="en">altimeter</skos:prefLabel>
	<skos:topConceptOf rdf:resource="http://vocab.aodn.org.au/def/instrument/1"/>
</rdf:Description>

<rdf:Description rdf:about="http://vocab.nerc.ac.uk/collection/L05/current/381">
	<rdf:type rdf:resource="http://www.w3.org/2000/01/rdf-schema#Resource"/>
	<rdf:type rdf:resource="http://www.w3.org/2004/02/skos/core#Concept"/>
	<dcterms:created rdf:datatype="http://www.w3.org/2001/XMLSchema#dateTime">2013-03-28T00:00:00Z</dcterms:created>
	<dc:publisher rdf:datatype="http://www.w3.org/2001/XMLSchema#string">British Oceanographic Data Centre (BODC)</dc:publisher>
	<dc:source rdf:datatype="http://www.w3.org/2001/XMLSchema#string">(L051) SeaDataNet device categories</dc:source>
	<skos:definition xml:lang="en">Instruments that measure either the rate of fall or integrated amount of rain snow sleet hail or graupel.</skos:definition>
	<skos:inScheme rdf:resource="http://vocab.aodn.org.au/def/instrument/1"/>
	<skos:narrower rdf:resource="http://vocab.nerc.ac.uk/collection/L22/current/TOOL0671"/>
	<skos:narrower rdf:resource="http://vocab.nerc.ac.uk/collection/L22/current/TOOL0725"/>
	<skos:prefLabel xml:lang="en">precipitation gauges</skos:prefLabel>
	<skos:topConceptOf rdf:resource="http://vocab.aodn.org.au/def/instrument/1"/>
</rdf:Description>

<rdf:Description rdf:about="http://vocab.nerc.ac.uk/collection/L05/current/382">
	<rdf:type rdf:resource="http://www.w3.org/2000/01/rdf-schema#Resource"/>
	<rdf:type rdf:resource="http://www.w3.org/2004/02/skos/core#Concept"/>
	<dcterms:contributor rdf:resource="http://editor.vocabs.ands.org.au/user/Natalia_Atkins"/>
	<dcterms:created rdf:datatype="http://www.w3.org/2001/XMLSchema#dateTime">2013-10-08T00:00:00Z</dcterms:created>
	<dcterms:modified rdf:datatype="http://www.w3.org/2001/XMLSchema#dateTime">2015-07-08T04:07:58Z</dcterms:modified>
	<dc:publisher rdf:datatype="http://www.w3.org/2001/XMLSchema#string">British Oceanographic Data Centre (BODC)</dc:publisher>
	<dc:source rdf:datatype="http://www.w3.org/2001/XMLSchema#string">(L051) SeaDataNet device categories</dc:source>
	<skos:definition xml:lang="en">In-situ instruments that can determine the proportion of one or more gaseous components of the atmosphere.</skos:definition>
	<skos:inScheme rdf:resource="http://vocab.aodn.org.au/def/instrument/1"/>
	<skos:narrower rdf:resource="http://vocab.nerc.ac.uk/collection/L22/current/TOOL0878"/>
	<skos:narrower rdf:resource="http://vocab.nerc.ac.uk/collection/L22/current/TOOL0724"/>
	<skos:narrower rdf:resource="http://vocab.nerc.ac.uk/collection/L22/current/TOOL0705"/>
	<skos:narrower rdf:resource="http://vocab.nerc.ac.uk/collection/L22/current/TOOL1123"/>
	<skos:prefLabel xml:lang="en">atmospheric gas analysers</skos:prefLabel>
	<skos:topConceptOf rdf:resource="http://vocab.aodn.org.au/def/instrument/1"/>
</rdf:Description>

<rdf:Description rdf:about="http://vocab.nerc.ac.uk/collection/L05/current/383">
	<rdf:type rdf:resource="http://www.w3.org/2000/01/rdf-schema#Resource"/>
	<rdf:type rdf:resource="http://www.w3.org/2004/02/skos/core#Concept"/>
	<dcterms:created rdf:datatype="http://www.w3.org/2001/XMLSchema#dateTime">2013-03-28T00:00:00Z</dcterms:created>
	<dc:publisher rdf:datatype="http://www.w3.org/2001/XMLSchema#string">British Oceanographic Data Centre (BODC)</dc:publisher>
	<dc:source rdf:datatype="http://www.w3.org/2001/XMLSchema#string">(L051) SeaDataNet device categories</dc:source>
	<skos:definition xml:lang="en">In-situ instruments that can determine the total dissolved or particulate concentration of one or more metallic elements (including trace metalloids like arsenic) in a water body.</skos:definition>
	<skos:inScheme rdf:resource="http://vocab.aodn.org.au/def/instrument/1"/>
	<skos:prefLabel xml:lang="en">metal analysers</skos:prefLabel>
	<skos:topConceptOf rdf:resource="http://vocab.aodn.org.au/def/instrument/1"/>
</rdf:Description>

<rdf:Description rdf:about="http://vocab.nerc.ac.uk/collection/L05/current/384">
	<rdf:type rdf:resource="http://www.w3.org/2000/01/rdf-schema#Resource"/>
	<rdf:type rdf:resource="http://www.w3.org/2004/02/skos/core#Concept"/>
	<dcterms:created rdf:datatype="http://www.w3.org/2001/XMLSchema#dateTime">2014-05-22T00:00:00Z</dcterms:created>
	<dc:publisher rdf:datatype="http://www.w3.org/2001/XMLSchema#string">British Oceanographic Data Centre (BODC)</dc:publisher>
	<dc:source rdf:datatype="http://www.w3.org/2001/XMLSchema#string">(L051) SeaDataNet device categories</dc:source>
	<skos:definition xml:lang="en">ADV is the acronym for acoustic doppler velocimeter. The group includes all in-situ instruments that make high frequency measurements of three-dimensional current velocity in order to determine the extent of turbulence within a water body.</skos:definition>
	<skos:inScheme rdf:resource="http://vocab.aodn.org.au/def/instrument/1"/>
	<skos:prefLabel xml:lang="en">ADVs and turbulence probes</skos:prefLabel>
	<skos:topConceptOf rdf:resource="http://vocab.aodn.org.au/def/instrument/1"/>
</rdf:Description>

<rdf:Description rdf:about="http://vocab.nerc.ac.uk/collection/L05/current/385">
	<rdf:type rdf:resource="http://www.w3.org/2000/01/rdf-schema#Resource"/>
	<rdf:type rdf:resource="http://www.w3.org/2004/02/skos/core#Concept"/>
	<dcterms:contributor rdf:resource="http://editor.vocabs.ands.org.au/user/eMII_Atkins.Natalia"/>
	<dcterms:created rdf:datatype="http://www.w3.org/2001/XMLSchema#dateTime">2014-02-06T00:00:00Z</dcterms:created>
	<dcterms:modified rdf:datatype="http://www.w3.org/2001/XMLSchema#dateTime">2017-04-10T05:00:47Z</dcterms:modified>
	<dc:publisher rdf:datatype="http://www.w3.org/2001/XMLSchema#string">British Oceanographic Data Centre (BODC)</dc:publisher>
	<dc:source rdf:datatype="http://www.w3.org/2001/XMLSchema#string">(L051) SeaDataNet device categories</dc:source>
	<skos:definition xml:lang="en">Instruments that measure platform orientation or rates of platform motion or acceleration in any direction or along any axis. Excludes inertial navigation systems that are designed to determine platform location with respect to an external co-ordinate reference system.</skos:definition>
	<skos:inScheme rdf:resource="http://vocab.aodn.org.au/def/instrument/1"/>
	<skos:narrower rdf:resource="http://vocab.nerc.ac.uk/collection/L22/current/TOOL0872"/>
	<skos:narrower rdf:resource="http://vocab.nerc.ac.uk/collection/L22/current/TOOL0490"/>
	<skos:narrower rdf:resource="http://vocab.nerc.ac.uk/collection/L22/current/TOOL1121"/>
	<skos:narrower rdf:resource="http://vocab.nerc.ac.uk/collection/L22/current/TOOL0721"/>
	<skos:prefLabel xml:lang="en">platform altitude sensors</skos:prefLabel>
	<skos:topConceptOf rdf:resource="http://vocab.aodn.org.au/def/instrument/1"/>
</rdf:Description>

<rdf:Description rdf:about="http://vocab.nerc.ac.uk/collection/L05/current/388">
	<rdf:type rdf:resource="http://www.w3.org/2000/01/rdf-schema#Resource"/>
	<rdf:type rdf:resource="http://www.w3.org/2004/02/skos/core#Concept"/>
	<dcterms:created rdf:datatype="http://www.w3.org/2001/XMLSchema#dateTime">2013-03-28T00:00:00Z</dcterms:created>
	<dc:publisher rdf:datatype="http://www.w3.org/2001/XMLSchema#string">British Oceanographic Data Centre (BODC)</dc:publisher>
	<dc:source rdf:datatype="http://www.w3.org/2001/XMLSchema#string">(L051) SeaDataNet device categories</dc:source>
	<skos:definition xml:lang="en">Sensors that quantify the rate at which fluids (e.g. water or air) pass through sensor packages instruments or sampling devices.</skos:definition>
	<skos:inScheme rdf:resource="http://vocab.aodn.org.au/def/instrument/1"/>
	<skos:prefLabel xml:lang="en">flow meters</skos:prefLabel>
	<skos:topConceptOf rdf:resource="http://vocab.aodn.org.au/def/instrument/1"/>
</rdf:Description>

<rdf:Description rdf:about="http://vocab.nerc.ac.uk/collection/L05/current/50">
	<rdf:type rdf:resource="http://www.w3.org/2000/01/rdf-schema#Resource"/>
	<rdf:type rdf:resource="http://www.w3.org/2004/02/skos/core#Concept"/>
	<dcterms:created rdf:datatype="http://www.w3.org/2001/XMLSchema#dateTime">2014-05-22T00:00:00Z</dcterms:created>
	<dc:publisher rdf:datatype="http://www.w3.org/2001/XMLSchema#string">British Oceanographic Data Centre (BODC)</dc:publisher>
	<dc:source rdf:datatype="http://www.w3.org/2001/XMLSchema#string">(L051) SeaDataNet device categories</dc:source>
	<skos:definition xml:lang="en">A device that collects a sample of surface sediment including manually deployed equipment like a shovel or bucket.</skos:definition>
	<skos:inScheme rdf:resource="http://vocab.aodn.org.au/def/instrument/1"/>
	<skos:prefLabel xml:lang="en">sediment grabs</skos:prefLabel>
	<skos:topConceptOf rdf:resource="http://vocab.aodn.org.au/def/instrument/1"/>
</rdf:Description>

<rdf:Description rdf:about="http://vocab.nerc.ac.uk/collection/L05/current/51">
	<rdf:type rdf:resource="http://www.w3.org/2000/01/rdf-schema#Resource"/>
	<rdf:type rdf:resource="http://www.w3.org/2004/02/skos/core#Concept"/>
	<dcterms:created rdf:datatype="http://www.w3.org/2001/XMLSchema#dateTime">2014-05-22T00:00:00Z</dcterms:created>
	<dc:publisher rdf:datatype="http://www.w3.org/2001/XMLSchema#string">British Oceanographic Data Centre (BODC)</dc:publisher>
	<dc:source rdf:datatype="http://www.w3.org/2001/XMLSchema#string">(L051) SeaDataNet device categories</dc:source>
	<skos:definition xml:lang="en">Devices designed to collect samples of unconsolidated sediment from between the surface and depths from a metre to 10s of metres with minimal disturbance of the sediment structure.</skos:definition>
	<skos:inScheme rdf:resource="http://vocab.aodn.org.au/def/instrument/1"/>
	<skos:prefLabel xml:lang="en">unconsolidated sediment corers</skos:prefLabel>
	<skos:topConceptOf rdf:resource="http://vocab.aodn.org.au/def/instrument/1"/>
</rdf:Description>

<rdf:Description rdf:about="http://vocab.nerc.ac.uk/collection/L05/current/53">
	<rdf:type rdf:resource="http://www.w3.org/2000/01/rdf-schema#Resource"/>
	<rdf:type rdf:resource="http://www.w3.org/2004/02/skos/core#Concept"/>
	<dcterms:created rdf:datatype="http://www.w3.org/2001/XMLSchema#dateTime">2014-05-22T00:00:00Z</dcterms:created>
	<dc:publisher rdf:datatype="http://www.w3.org/2001/XMLSchema#string">British Oceanographic Data Centre (BODC)</dc:publisher>
	<dc:source rdf:datatype="http://www.w3.org/2001/XMLSchema#string">(L051) SeaDataNet device categories</dc:source>
	<skos:definition xml:lang="en">A device that drills into rock extracting a cylindrical sample</skos:definition>
	<skos:inScheme rdf:resource="http://vocab.aodn.org.au/def/instrument/1"/>
	<skos:prefLabel xml:lang="en">rock corers</skos:prefLabel>
	<skos:topConceptOf rdf:resource="http://vocab.aodn.org.au/def/instrument/1"/>
</rdf:Description>

<rdf:Description rdf:about="http://vocab.nerc.ac.uk/collection/L05/current/54">
	<rdf:type rdf:resource="http://www.w3.org/2000/01/rdf-schema#Resource"/>
	<rdf:type rdf:resource="http://www.w3.org/2004/02/skos/core#Concept"/>
	<dcterms:created rdf:datatype="http://www.w3.org/2001/XMLSchema#dateTime">2014-05-22T00:00:00Z</dcterms:created>
	<dc:publisher rdf:datatype="http://www.w3.org/2001/XMLSchema#string">British Oceanographic Data Centre (BODC)</dc:publisher>
	<dc:source rdf:datatype="http://www.w3.org/2001/XMLSchema#string">(L051) SeaDataNet device categories</dc:source>
	<skos:definition xml:lang="en">A device dragged across the seabed designed to collect loose rock samples.</skos:definition>
	<skos:inScheme rdf:resource="http://vocab.aodn.org.au/def/instrument/1"/>
	<skos:prefLabel xml:lang="en">rock dredges</skos:prefLabel>
	<skos:topConceptOf rdf:resource="http://vocab.aodn.org.au/def/instrument/1"/>
</rdf:Description>

<rdf:Description rdf:about="http://vocab.nerc.ac.uk/collection/L05/current/60">
	<rdf:type rdf:resource="http://www.w3.org/2000/01/rdf-schema#Resource"/>
	<rdf:type rdf:resource="http://www.w3.org/2004/02/skos/core#Concept"/>
	<dcterms:created rdf:datatype="http://www.w3.org/2001/XMLSchema#dateTime">2014-05-22T00:00:00Z</dcterms:created>
	<dc:publisher rdf:datatype="http://www.w3.org/2001/XMLSchema#string">British Oceanographic Data Centre (BODC)</dc:publisher>
	<dc:source rdf:datatype="http://www.w3.org/2001/XMLSchema#string">(L051) SeaDataNet device categories</dc:source>
	<skos:definition xml:lang="en">Bucket-like containers hauled over the sea bed collecting integrated samples of surface sediment along a segment of ship track.</skos:definition>
	<skos:inScheme rdf:resource="http://vocab.aodn.org.au/def/instrument/1"/>
	<skos:prefLabel xml:lang="en">sediment dredges</skos:prefLabel>
	<skos:topConceptOf rdf:resource="http://vocab.aodn.org.au/def/instrument/1"/>
</rdf:Description>

<rdf:Description rdf:about="http://vocab.nerc.ac.uk/collection/L05/current/61">
	<rdf:type rdf:resource="http://www.w3.org/2000/01/rdf-schema#Resource"/>
	<rdf:type rdf:resource="http://www.w3.org/2004/02/skos/core#Concept"/>
	<dcterms:created rdf:datatype="http://www.w3.org/2001/XMLSchema#dateTime">2014-05-22T00:00:00Z</dcterms:created>
	<dc:publisher rdf:datatype="http://www.w3.org/2001/XMLSchema#string">British Oceanographic Data Centre (BODC)</dc:publisher>
	<dc:source rdf:datatype="http://www.w3.org/2001/XMLSchema#string">(L051) SeaDataNet device categories</dc:source>
	<skos:definition xml:lang="en">Nets towed over the sea floor designed to sample species living on or near the bottom.</skos:definition>
	<skos:inScheme rdf:resource="http://vocab.aodn.org.au/def/instrument/1"/>
	<skos:prefLabel xml:lang="en">demersal trawl nets</skos:prefLabel>
	<skos:topConceptOf rdf:resource="http://vocab.aodn.org.au/def/instrument/1"/>
</rdf:Description>

<rdf:Description rdf:about="http://vocab.nerc.ac.uk/collection/L05/current/62">
	<rdf:type rdf:resource="http://www.w3.org/2000/01/rdf-schema#Resource"/>
	<rdf:type rdf:resource="http://www.w3.org/2004/02/skos/core#Concept"/>
	<dcterms:created rdf:datatype="http://www.w3.org/2001/XMLSchema#dateTime">2014-05-22T00:00:00Z</dcterms:created>
	<dc:publisher rdf:datatype="http://www.w3.org/2001/XMLSchema#string">British Oceanographic Data Centre (BODC)</dc:publisher>
	<dc:source rdf:datatype="http://www.w3.org/2001/XMLSchema#string">(L051) SeaDataNet device categories</dc:source>
	<skos:definition xml:lang="en">Nets towed over the sea floor having the horizontal net opening provided by a wooden or metal beam that disrupts the surface of the bed.</skos:definition>
	<skos:inScheme rdf:resource="http://vocab.aodn.org.au/def/instrument/1"/>
	<skos:prefLabel xml:lang="en">beam trawls</skos:prefLabel>
	<skos:topConceptOf rdf:resource="http://vocab.aodn.org.au/def/instrument/1"/>
</rdf:Description>

<rdf:Description rdf:about="http://vocab.nerc.ac.uk/collection/L05/current/63">
	<rdf:type rdf:resource="http://www.w3.org/2000/01/rdf-schema#Resource"/>
	<rdf:type rdf:resource="http://www.w3.org/2004/02/skos/core#Concept"/>
	<dcterms:created rdf:datatype="http://www.w3.org/2001/XMLSchema#dateTime">2014-05-22T00:00:00Z</dcterms:created>
	<dc:publisher rdf:datatype="http://www.w3.org/2001/XMLSchema#string">British Oceanographic Data Centre (BODC)</dc:publisher>
	<dc:source rdf:datatype="http://www.w3.org/2001/XMLSchema#string">(L051) SeaDataNet device categories</dc:source>
	<skos:definition xml:lang="en">Apparatus where capture is based on the movement of the target species towards the gear (e.g. creels and fish traps).</skos:definition>
	<skos:inScheme rdf:resource="http://vocab.aodn.org.au/def/instrument/1"/>
	<skos:prefLabel xml:lang="en">passive fishing gear</skos:prefLabel>
	<skos:topConceptOf rdf:resource="http://vocab.aodn.org.au/def/instrument/1"/>
</rdf:Description>

<rdf:Description rdf:about="http://vocab.nerc.ac.uk/collection/L05/current/64">
	<rdf:type rdf:resource="http://www.w3.org/2000/01/rdf-schema#Resource"/>
	<rdf:type rdf:resource="http://www.w3.org/2004/02/skos/core#Concept"/>
	<dcterms:created rdf:datatype="http://www.w3.org/2001/XMLSchema#dateTime">2014-05-22T00:00:00Z</dcterms:created>
	<dc:publisher rdf:datatype="http://www.w3.org/2001/XMLSchema#string">British Oceanographic Data Centre (BODC)</dc:publisher>
	<dc:source rdf:datatype="http://www.w3.org/2001/XMLSchema#string">(L051) SeaDataNet device categories</dc:source>
	<skos:definition xml:lang="en">Apparatus where capture is based on chasing the target species (e.g. a trawl).</skos:definition>
	<skos:inScheme rdf:resource="http://vocab.aodn.org.au/def/instrument/1"/>
	<skos:prefLabel xml:lang="en">active fishing gear</skos:prefLabel>
	<skos:topConceptOf rdf:resource="http://vocab.aodn.org.au/def/instrument/1"/>
</rdf:Description>

<rdf:Description rdf:about="http://vocab.nerc.ac.uk/collection/L05/current/65">
	<rdf:type rdf:resource="http://www.w3.org/2000/01/rdf-schema#Resource"/>
	<rdf:type rdf:resource="http://www.w3.org/2004/02/skos/core#Concept"/>
	<dcterms:created rdf:datatype="http://www.w3.org/2001/XMLSchema#dateTime">2014-05-22T00:00:00Z</dcterms:created>
	<dc:publisher rdf:datatype="http://www.w3.org/2001/XMLSchema#string">British Oceanographic Data Centre (BODC)</dc:publisher>
	<dc:source rdf:datatype="http://www.w3.org/2001/XMLSchema#string">(L051) SeaDataNet device categories</dc:source>
	<skos:definition xml:lang="en">Nets drifting in the sea or standing on the sea floor in which fish become entangled usually through their gill covers.</skos:definition>
	<skos:inScheme rdf:resource="http://vocab.aodn.org.au/def/instrument/1"/>
	<skos:prefLabel xml:lang="en">gill nets</skos:prefLabel>
	<skos:topConceptOf rdf:resource="http://vocab.aodn.org.au/def/instrument/1"/>
</rdf:Description>

<rdf:Description rdf:about="http://vocab.nerc.ac.uk/collection/L05/current/68">
	<rdf:type rdf:resource="http://www.w3.org/2000/01/rdf-schema#Resource"/>
	<rdf:type rdf:resource="http://www.w3.org/2004/02/skos/core#Concept"/>
	<dcterms:created rdf:datatype="http://www.w3.org/2001/XMLSchema#dateTime">2014-05-22T00:00:00Z</dcterms:created>
	<dc:publisher rdf:datatype="http://www.w3.org/2001/XMLSchema#string">British Oceanographic Data Centre (BODC)</dc:publisher>
	<dc:source rdf:datatype="http://www.w3.org/2001/XMLSchema#string">(L051) SeaDataNet device categories</dc:source>
	<skos:definition xml:lang="en">A system comprising several nets that can be opened and closed sequentially to collect a series of samples during a tow or haul. Samples microzooplankton mesozooplankton and nekton.</skos:definition>
	<skos:inScheme rdf:resource="http://vocab.aodn.org.au/def/instrument/1"/>
	<skos:prefLabel xml:lang="en">multinet</skos:prefLabel>
	<skos:topConceptOf rdf:resource="http://vocab.aodn.org.au/def/instrument/1"/>
</rdf:Description>

<rdf:Description rdf:about="http://vocab.nerc.ac.uk/collection/L05/current/69">
	<rdf:type rdf:resource="http://www.w3.org/2000/01/rdf-schema#Resource"/>
	<rdf:type rdf:resource="http://www.w3.org/2004/02/skos/core#Concept"/>
	<dcterms:created rdf:datatype="http://www.w3.org/2001/XMLSchema#dateTime">2014-05-22T00:00:00Z</dcterms:created>
	<dc:publisher rdf:datatype="http://www.w3.org/2001/XMLSchema#string">British Oceanographic Data Centre (BODC)</dc:publisher>
	<dc:source rdf:datatype="http://www.w3.org/2001/XMLSchema#string">(L051) SeaDataNet device categories</dc:source>
	<skos:definition xml:lang="en">A fine-meshed net designed to collect samples living within a few centimetres of the sea surface. Samples microzooplankton mesozooplankton and nekton.</skos:definition>
	<skos:inScheme rdf:resource="http://vocab.aodn.org.au/def/instrument/1"/>
	<skos:prefLabel xml:lang="en">neuston net</skos:prefLabel>
	<skos:topConceptOf rdf:resource="http://vocab.aodn.org.au/def/instrument/1"/>
</rdf:Description>

<rdf:Description rdf:about="http://vocab.nerc.ac.uk/collection/L05/current/81">
	<rdf:type rdf:resource="http://www.w3.org/2000/01/rdf-schema#Resource"/>
	<rdf:type rdf:resource="http://www.w3.org/2004/02/skos/core#Concept"/>
	<dcterms:created rdf:datatype="http://www.w3.org/2001/XMLSchema#dateTime">2014-05-22T00:00:00Z</dcterms:created>
	<dc:publisher rdf:datatype="http://www.w3.org/2001/XMLSchema#string">British Oceanographic Data Centre (BODC)</dc:publisher>
	<dc:source rdf:datatype="http://www.w3.org/2001/XMLSchema#string">(L051) SeaDataNet device categories</dc:source>
	<skos:definition xml:lang="en">A device mounted on a ship that holds water samples under conditions of controlled temperature or controlled temperature and illumination.</skos:definition>
	<skos:inScheme rdf:resource="http://vocab.aodn.org.au/def/instrument/1"/>
	<skos:prefLabel xml:lang="en">shipboard incubators</skos:prefLabel>
	<skos:topConceptOf rdf:resource="http://vocab.aodn.org.au/def/instrument/1"/>
</rdf:Description>

<rdf:Description rdf:about="http://vocab.nerc.ac.uk/collection/L05/current/82">
	<rdf:type rdf:resource="http://www.w3.org/2000/01/rdf-schema#Resource"/>
	<rdf:type rdf:resource="http://www.w3.org/2004/02/skos/core#Concept"/>
	<dcterms:created rdf:datatype="http://www.w3.org/2001/XMLSchema#dateTime">2014-05-22T00:00:00Z</dcterms:created>
	<dc:publisher rdf:datatype="http://www.w3.org/2001/XMLSchema#string">British Oceanographic Data Centre (BODC)</dc:publisher>
	<dc:source rdf:datatype="http://www.w3.org/2001/XMLSchema#string">(L051) SeaDataNet device categories</dc:source>
	<skos:definition xml:lang="en">A rig that allows water samples to be retained from where they were collected whilst physically separated from their surroundings.  Includes small-scale incubation rigs and mesocosms.</skos:definition>
	<skos:inScheme rdf:resource="http://vocab.aodn.org.au/def/instrument/1"/>
	<skos:prefLabel xml:lang="en">in-situ incubators</skos:prefLabel>
	<skos:topConceptOf rdf:resource="http://vocab.aodn.org.au/def/instrument/1"/>
</rdf:Description>

<rdf:Description rdf:about="http://vocab.nerc.ac.uk/collection/L05/current/90">
	<rdf:type rdf:resource="http://www.w3.org/2000/01/rdf-schema#Resource"/>
	<rdf:type rdf:resource="http://www.w3.org/2004/02/skos/core#Concept"/>
	<dcterms:created rdf:datatype="http://www.w3.org/2001/XMLSchema#dateTime">2014-05-22T00:00:00Z</dcterms:created>
	<dc:publisher rdf:datatype="http://www.w3.org/2001/XMLSchema#string">British Oceanographic Data Centre (BODC)</dc:publisher>
	<dc:source rdf:datatype="http://www.w3.org/2001/XMLSchema#string">(L051) SeaDataNet device categories</dc:source>
	<skos:definition xml:lang="en">A simple tool like a hammer saw or even just a hand for the collection of biota samples</skos:definition>
	<skos:inScheme rdf:resource="http://vocab.aodn.org.au/def/instrument/1"/>
	<skos:prefLabel xml:lang="en">manual biota samplers</skos:prefLabel>
	<skos:topConceptOf rdf:resource="http://vocab.aodn.org.au/def/instrument/1"/>
</rdf:Description>

<rdf:Description rdf:about="http://vocab.nerc.ac.uk/collection/L05/current/91">
	<rdf:type rdf:resource="http://www.w3.org/2000/01/rdf-schema#Resource"/>
	<rdf:type rdf:resource="http://www.w3.org/2004/02/skos/core#Concept"/>
	<dcterms:created rdf:datatype="http://www.w3.org/2001/XMLSchema#dateTime">2014-05-22T00:00:00Z</dcterms:created>
	<dc:publisher rdf:datatype="http://www.w3.org/2001/XMLSchema#string">British Oceanographic Data Centre (BODC)</dc:publisher>
	<dc:source rdf:datatype="http://www.w3.org/2001/XMLSchema#string">(L051) SeaDataNet device categories</dc:source>
	<skos:definition xml:lang="en">Humans who estimate a parameter through observation of a phenomenon such as bird counts and visual wave observations</skos:definition>
	<skos:inScheme rdf:resource="http://vocab.aodn.org.au/def/instrument/1"/>
	<skos:prefLabel xml:lang="en">observers</skos:prefLabel>
	<skos:topConceptOf rdf:resource="http://vocab.aodn.org.au/def/instrument/1"/>
</rdf:Description>

<rdf:Description rdf:about="http://vocab.nerc.ac.uk/collection/L05/current/FFES">
	<rdf:type rdf:resource="http://www.w3.org/2000/01/rdf-schema#Resource"/>
	<rdf:type rdf:resource="http://www.w3.org/2004/02/skos/core#Concept"/>
	<dcterms:created rdf:datatype="http://www.w3.org/2001/XMLSchema#dateTime">2013-10-09T00:00:00Z</dcterms:created>
	<dc:publisher rdf:datatype="http://www.w3.org/2001/XMLSchema#string">British Oceanographic Data Centre (BODC)</dc:publisher>
	<dc:source rdf:datatype="http://www.w3.org/2001/XMLSchema#string">(L051) SeaDataNet device categories</dc:source>
	<skos:definition xml:lang="en">Instruments primarily designed to detect shoals of fish through transmission and reception of acoustic signals.  They are often optimised for this purpose through the use of multiple frequencies.</skos:definition>
	<skos:inScheme rdf:resource="http://vocab.aodn.org.au/def/instrument/1"/>
	<skos:narrower rdf:resource="http://vocab.nerc.ac.uk/collection/L22/current/TOOL0198"/>
	<skos:narrower rdf:resource="http://vocab.nerc.ac.uk/collection/L22/current/TOOL0689"/>
	<skos:narrower rdf:resource="http://vocab.nerc.ac.uk/collection/L22/current/TOOL1151"/>
	<skos:prefLabel xml:lang="en">Fish-finder echosounders</skos:prefLabel>
	<skos:topConceptOf rdf:resource="http://vocab.aodn.org.au/def/instrument/1"/>
</rdf:Description>

<rdf:Description rdf:about="http://vocab.nerc.ac.uk/collection/L05/current/LAB02">
	<rdf:type rdf:resource="http://www.w3.org/2000/01/rdf-schema#Resource"/>
	<rdf:type rdf:resource="http://www.w3.org/2004/02/skos/core#Concept"/>
	<dcterms:created rdf:datatype="http://www.w3.org/2001/XMLSchema#dateTime">2014-05-22T00:00:00Z</dcterms:created>
	<dc:publisher rdf:datatype="http://www.w3.org/2001/XMLSchema#string">British Oceanographic Data Centre (BODC)</dc:publisher>
	<dc:source rdf:datatype="http://www.w3.org/2001/XMLSchema#string">(L051) SeaDataNet device categories</dc:source>
	<skos:definition xml:lang="en">Instruments separating gases volatile substances or substances dissolved in a volatile solvent by transporting an inert gas through a column packed with a sorbent to a detector for assay.</skos:definition>
	<skos:inScheme rdf:resource="http://vocab.aodn.org.au/def/instrument/1"/>
	<skos:prefLabel xml:lang="en">gas chromatographs</skos:prefLabel>
	<skos:topConceptOf rdf:resource="http://vocab.aodn.org.au/def/instrument/1"/>
</rdf:Description>

<rdf:Description rdf:about="http://vocab.nerc.ac.uk/collection/L05/current/LAB05">
	<rdf:type rdf:resource="http://www.w3.org/2000/01/rdf-schema#Resource"/>
	<rdf:type rdf:resource="http://www.w3.org/2004/02/skos/core#Concept"/>
	<dcterms:created rdf:datatype="http://www.w3.org/2001/XMLSchema#dateTime">2014-05-22T00:00:00Z</dcterms:created>
	<dc:publisher rdf:datatype="http://www.w3.org/2001/XMLSchema#string">British Oceanographic Data Centre (BODC)</dc:publisher>
	<dc:source rdf:datatype="http://www.w3.org/2001/XMLSchema#string">(L051) SeaDataNet device categories</dc:source>
	<skos:definition xml:lang="en">Instruments that generate enlarged images of samples using the phenomena of reflection and absorption of visible light. Includes conventional and inverted instruments.</skos:definition>
	<skos:inScheme rdf:resource="http://vocab.aodn.org.au/def/instrument/1"/>
	<skos:prefLabel xml:lang="en">optical microscopes</skos:prefLabel>
	<skos:topConceptOf rdf:resource="http://vocab.aodn.org.au/def/instrument/1"/>
</rdf:Description>

<rdf:Description rdf:about="http://vocab.nerc.ac.uk/collection/L05/current/LAB06">
	<rdf:type rdf:resource="http://www.w3.org/2000/01/rdf-schema#Resource"/>
	<rdf:type rdf:resource="http://www.w3.org/2004/02/skos/core#Concept"/>
	<dcterms:created rdf:datatype="http://www.w3.org/2001/XMLSchema#dateTime">2014-05-22T00:00:00Z</dcterms:created>
	<dc:publisher rdf:datatype="http://www.w3.org/2001/XMLSchema#string">British Oceanographic Data Centre (BODC)</dc:publisher>
	<dc:source rdf:datatype="http://www.w3.org/2001/XMLSchema#string">(L051) SeaDataNet device categories</dc:source>
	<skos:definition xml:lang="en">Instruments that generate enlarged images of samples using the phenomena of fluorescence and phosphorescence instead of or in addition to reflection and absorption of visible light. Includes conventional and inverted instruments.</skos:definition>
	<skos:inScheme rdf:resource="http://vocab.aodn.org.au/def/instrument/1"/>
	<skos:prefLabel xml:lang="en">fluorescence microscopes</skos:prefLabel>
	<skos:topConceptOf rdf:resource="http://vocab.aodn.org.au/def/instrument/1"/>
</rdf:Description>

<rdf:Description rdf:about="http://vocab.nerc.ac.uk/collection/L05/current/LAB07">
	<rdf:type rdf:resource="http://www.w3.org/2000/01/rdf-schema#Resource"/>
	<rdf:type rdf:resource="http://www.w3.org/2004/02/skos/core#Concept"/>
	<dcterms:created rdf:datatype="http://www.w3.org/2001/XMLSchema#dateTime">2014-05-22T00:00:00Z</dcterms:created>
	<dc:publisher rdf:datatype="http://www.w3.org/2001/XMLSchema#string">British Oceanographic Data Centre (BODC)</dc:publisher>
	<dc:source rdf:datatype="http://www.w3.org/2001/XMLSchema#string">(L051) SeaDataNet device categories</dc:source>
	<skos:definition xml:lang="en">Instruments that generate enlarged images of samples using the phenomena of reflection and absorption of electrons behaving as waves.</skos:definition>
	<skos:inScheme rdf:resource="http://vocab.aodn.org.au/def/instrument/1"/>
	<skos:prefLabel xml:lang="en">electron microscopes</skos:prefLabel>
	<skos:topConceptOf rdf:resource="http://vocab.aodn.org.au/def/instrument/1"/>
</rdf:Description>

<rdf:Description rdf:about="http://vocab.nerc.ac.uk/collection/L05/current/LAB08">
	<rdf:type rdf:resource="http://www.w3.org/2000/01/rdf-schema#Resource"/>
	<rdf:type rdf:resource="http://www.w3.org/2004/02/skos/core#Concept"/>
	<dcterms:created rdf:datatype="http://www.w3.org/2001/XMLSchema#dateTime">2014-05-22T00:00:00Z</dcterms:created>
	<dc:publisher rdf:datatype="http://www.w3.org/2001/XMLSchema#string">British Oceanographic Data Centre (BODC)</dc:publisher>
	<dc:source rdf:datatype="http://www.w3.org/2001/XMLSchema#string">(L051) SeaDataNet device categories</dc:source>
	<skos:definition xml:lang="en">Instruments that chemically analyse a small area of a sample by bombarding it with electrons and spectroscopically assaying the resulting X-Ray emissions.</skos:definition>
	<skos:inScheme rdf:resource="http://vocab.aodn.org.au/def/instrument/1"/>
	<skos:prefLabel xml:lang="en">electron microprobes</skos:prefLabel>
	<skos:topConceptOf rdf:resource="http://vocab.aodn.org.au/def/instrument/1"/>
</rdf:Description>

<rdf:Description rdf:about="http://vocab.nerc.ac.uk/collection/L05/current/LAB09">
	<rdf:type rdf:resource="http://www.w3.org/2000/01/rdf-schema#Resource"/>
	<rdf:type rdf:resource="http://www.w3.org/2004/02/skos/core#Concept"/>
	<dcterms:created rdf:datatype="http://www.w3.org/2001/XMLSchema#dateTime">2014-05-22T00:00:00Z</dcterms:created>
	<dc:publisher rdf:datatype="http://www.w3.org/2001/XMLSchema#string">British Oceanographic Data Centre (BODC)</dc:publisher>
	<dc:source rdf:datatype="http://www.w3.org/2001/XMLSchema#string">(L051) SeaDataNet device categories</dc:source>
	<skos:definition xml:lang="en">Instruments that isotopically analyse a small area of sample by bombarding it with ions to form a plasma that is analysed in a mass spectrometer.</skos:definition>
	<skos:inScheme rdf:resource="http://vocab.aodn.org.au/def/instrument/1"/>
	<skos:prefLabel xml:lang="en">ion microprobes</skos:prefLabel>
	<skos:topConceptOf rdf:resource="http://vocab.aodn.org.au/def/instrument/1"/>
</rdf:Description>

<rdf:Description rdf:about="http://vocab.nerc.ac.uk/collection/L05/current/LAB10">
	<rdf:type rdf:resource="http://www.w3.org/2000/01/rdf-schema#Resource"/>
	<rdf:type rdf:resource="http://www.w3.org/2004/02/skos/core#Concept"/>
	<dcterms:created rdf:datatype="http://www.w3.org/2001/XMLSchema#dateTime">2014-05-22T00:00:00Z</dcterms:created>
	<dc:publisher rdf:datatype="http://www.w3.org/2001/XMLSchema#string">British Oceanographic Data Centre (BODC)</dc:publisher>
	<dc:source rdf:datatype="http://www.w3.org/2001/XMLSchema#string">(L051) SeaDataNet device categories</dc:source>
	<skos:definition xml:lang="en">Instruments that volatilise the sample illuminate the resultant vapour with light wavelengths matched to the analyte of interest and quantify the radiation absorbed which is proportional to concentration.</skos:definition>
	<skos:inScheme rdf:resource="http://vocab.aodn.org.au/def/instrument/1"/>
	<skos:prefLabel xml:lang="en">atomic absorption spectrometers</skos:prefLabel>
	<skos:topConceptOf rdf:resource="http://vocab.aodn.org.au/def/instrument/1"/>
</rdf:Description>

<rdf:Description rdf:about="http://vocab.nerc.ac.uk/collection/L05/current/LAB11">
	<rdf:type rdf:resource="http://www.w3.org/2000/01/rdf-schema#Resource"/>
	<rdf:type rdf:resource="http://www.w3.org/2004/02/skos/core#Concept"/>
	<dcterms:created rdf:datatype="http://www.w3.org/2001/XMLSchema#dateTime">2013-03-28T00:00:00Z</dcterms:created>
	<dc:publisher rdf:datatype="http://www.w3.org/2001/XMLSchema#string">British Oceanographic Data Centre (BODC)</dc:publisher>
	<dc:source rdf:datatype="http://www.w3.org/2001/XMLSchema#string">(L051) SeaDataNet device categories</dc:source>
	<skos:definition xml:lang="en">Instruments that separate and analyse mixtures of substances by high pressure pumping the sample through a column packed with microspheres coated with the stationary phase.</skos:definition>
	<skos:inScheme rdf:resource="http://vocab.aodn.org.au/def/instrument/1"/>
	<skos:prefLabel xml:lang="en">high performance liquid chromatographs</skos:prefLabel>
	<skos:topConceptOf rdf:resource="http://vocab.aodn.org.au/def/instrument/1"/>
</rdf:Description>

<rdf:Description rdf:about="http://vocab.nerc.ac.uk/collection/L05/current/LAB15">
	<rdf:type rdf:resource="http://www.w3.org/2000/01/rdf-schema#Resource"/>
	<rdf:type rdf:resource="http://www.w3.org/2004/02/skos/core#Concept"/>
	<dcterms:created rdf:datatype="http://www.w3.org/2001/XMLSchema#dateTime">2014-05-22T00:00:00Z</dcterms:created>
	<dc:publisher rdf:datatype="http://www.w3.org/2001/XMLSchema#string">British Oceanographic Data Centre (BODC)</dc:publisher>
	<dc:source rdf:datatype="http://www.w3.org/2001/XMLSchema#string">(L051) SeaDataNet device categories</dc:source>
	<skos:definition xml:lang="en">Instruments that pass nebulised samples into an inductively-coupled gas plasma (8-10000 K) where they are atomised and ionised. Ions of specific mass-to-charge ratios are quantified in a quadrupole mass spectrometer.</skos:definition>
	<skos:inScheme rdf:resource="http://vocab.aodn.org.au/def/instrument/1"/>
	<skos:prefLabel xml:lang="en">inductively-coupled plasma mass spectrometers</skos:prefLabel>
	<skos:topConceptOf rdf:resource="http://vocab.aodn.org.au/def/instrument/1"/>
</rdf:Description>

<rdf:Description rdf:about="http://vocab.nerc.ac.uk/collection/L05/current/LAB16">
	<rdf:type rdf:resource="http://www.w3.org/2000/01/rdf-schema#Resource"/>
	<rdf:type rdf:resource="http://www.w3.org/2004/02/skos/core#Concept"/>
	<dcterms:created rdf:datatype="http://www.w3.org/2001/XMLSchema#dateTime">2014-05-22T00:00:00Z</dcterms:created>
	<dc:publisher rdf:datatype="http://www.w3.org/2001/XMLSchema#string">British Oceanographic Data Centre (BODC)</dc:publisher>
	<dc:source rdf:datatype="http://www.w3.org/2001/XMLSchema#string">(L051) SeaDataNet device categories</dc:source>
	<skos:definition xml:lang="en">Instruments used to measure the mass-to-charge ratio of ions most generally used to find the composition of a sample by generating a mass spectrum representing the masses of sample components.</skos:definition>
	<skos:inScheme rdf:resource="http://vocab.aodn.org.au/def/instrument/1"/>
	<skos:prefLabel xml:lang="en">mass spectrometers</skos:prefLabel>
	<skos:topConceptOf rdf:resource="http://vocab.aodn.org.au/def/instrument/1"/>
</rdf:Description>

<rdf:Description rdf:about="http://vocab.nerc.ac.uk/collection/L05/current/LAB17">
	<rdf:type rdf:resource="http://www.w3.org/2000/01/rdf-schema#Resource"/>
	<rdf:type rdf:resource="http://www.w3.org/2004/02/skos/core#Concept"/>
	<dcterms:created rdf:datatype="http://www.w3.org/2001/XMLSchema#dateTime">2014-05-22T00:00:00Z</dcterms:created>
	<dc:publisher rdf:datatype="http://www.w3.org/2001/XMLSchema#string">British Oceanographic Data Centre (BODC)</dc:publisher>
	<dc:source rdf:datatype="http://www.w3.org/2001/XMLSchema#string">(L051) SeaDataNet device categories</dc:source>
	<skos:definition xml:lang="en">Instruments measuring the mass-to-charge ratio of the products of sample molecule disassociation atom ionisation and ion acceleration in a particle accelerator.</skos:definition>
	<skos:inScheme rdf:resource="http://vocab.aodn.org.au/def/instrument/1"/>
	<skos:prefLabel xml:lang="en">accelerator mass spectrometers</skos:prefLabel>
	<skos:topConceptOf rdf:resource="http://vocab.aodn.org.au/def/instrument/1"/>
</rdf:Description>

<rdf:Description rdf:about="http://vocab.nerc.ac.uk/collection/L05/current/LAB18">
	<rdf:type rdf:resource="http://www.w3.org/2000/01/rdf-schema#Resource"/>
	<rdf:type rdf:resource="http://www.w3.org/2004/02/skos/core#Concept"/>
	<dcterms:created rdf:datatype="http://www.w3.org/2001/XMLSchema#dateTime">2014-05-22T00:00:00Z</dcterms:created>
	<dc:publisher rdf:datatype="http://www.w3.org/2001/XMLSchema#string">British Oceanographic Data Centre (BODC)</dc:publisher>
	<dc:source rdf:datatype="http://www.w3.org/2001/XMLSchema#string">(L051) SeaDataNet device categories</dc:source>
	<skos:definition xml:lang="en">Instruments that identify and quantify magnetically active chemical entities by subjecting a sample to orthogonal magnetic and electrical fields.</skos:definition>
	<skos:inScheme rdf:resource="http://vocab.aodn.org.au/def/instrument/1"/>
	<skos:prefLabel xml:lang="en">nuclear magnetic resonance spectrometers</skos:prefLabel>
	<skos:topConceptOf rdf:resource="http://vocab.aodn.org.au/def/instrument/1"/>
</rdf:Description>

<rdf:Description rdf:about="http://vocab.nerc.ac.uk/collection/L05/current/LAB19">
	<rdf:type rdf:resource="http://www.w3.org/2000/01/rdf-schema#Resource"/>
	<rdf:type rdf:resource="http://www.w3.org/2004/02/skos/core#Concept"/>
	<dcterms:created rdf:datatype="http://www.w3.org/2001/XMLSchema#dateTime">2014-05-22T00:00:00Z</dcterms:created>
	<dc:publisher rdf:datatype="http://www.w3.org/2001/XMLSchema#string">British Oceanographic Data Centre (BODC)</dc:publisher>
	<dc:source rdf:datatype="http://www.w3.org/2001/XMLSchema#string">(L051) SeaDataNet device categories</dc:source>
	<skos:definition xml:lang="en">Instruments separating gases volatile substances or substances dissolved in a volatile solvent by transporting an inert gas through a column packed with a sorbent to a detector for assay by a mass spectrometer.</skos:definition>
	<skos:inScheme rdf:resource="http://vocab.aodn.org.au/def/instrument/1"/>
	<skos:prefLabel xml:lang="en">gas chromatograph mass spectrometers</skos:prefLabel>
	<skos:topConceptOf rdf:resource="http://vocab.aodn.org.au/def/instrument/1"/>
</rdf:Description>

<rdf:Description rdf:about="http://vocab.nerc.ac.uk/collection/L05/current/LAB20">
	<rdf:type rdf:resource="http://www.w3.org/2000/01/rdf-schema#Resource"/>
	<rdf:type rdf:resource="http://www.w3.org/2004/02/skos/core#Concept"/>
	<dcterms:created rdf:datatype="http://www.w3.org/2001/XMLSchema#dateTime">2014-05-22T00:00:00Z</dcterms:created>
	<dc:publisher rdf:datatype="http://www.w3.org/2001/XMLSchema#string">British Oceanographic Data Centre (BODC)</dc:publisher>
	<dc:source rdf:datatype="http://www.w3.org/2001/XMLSchema#string">(L051) SeaDataNet device categories</dc:source>
	<skos:definition xml:lang="en">Instruments measuring the relative absorption of electromagnetic radiation of different wavelengths in the near infra-red visible and ultraviolet wavebands by samples.</skos:definition>
	<skos:inScheme rdf:resource="http://vocab.aodn.org.au/def/instrument/1"/>
	<skos:prefLabel xml:lang="en">spectrophotometers</skos:prefLabel>
	<skos:topConceptOf rdf:resource="http://vocab.aodn.org.au/def/instrument/1"/>
</rdf:Description>

<rdf:Description rdf:about="http://vocab.nerc.ac.uk/collection/L05/current/LAB21">
	<rdf:type rdf:resource="http://www.w3.org/2000/01/rdf-schema#Resource"/>
	<rdf:type rdf:resource="http://www.w3.org/2004/02/skos/core#Concept"/>
	<dcterms:created rdf:datatype="http://www.w3.org/2001/XMLSchema#dateTime">2014-05-22T00:00:00Z</dcterms:created>
	<dc:publisher rdf:datatype="http://www.w3.org/2001/XMLSchema#string">British Oceanographic Data Centre (BODC)</dc:publisher>
	<dc:source rdf:datatype="http://www.w3.org/2001/XMLSchema#string">(L051) SeaDataNet device categories</dc:source>
	<skos:definition xml:lang="en">Instruments assaying beta radiation by quantitative detection of visible light produced by the passage of rays or particles through a suitable scintillant incorporated into the sample.</skos:definition>
	<skos:inScheme rdf:resource="http://vocab.aodn.org.au/def/instrument/1"/>
	<skos:prefLabel xml:lang="en">liquid scintillation counters</skos:prefLabel>
	<skos:topConceptOf rdf:resource="http://vocab.aodn.org.au/def/instrument/1"/>
</rdf:Description>

<rdf:Description rdf:about="http://vocab.nerc.ac.uk/collection/L05/current/LAB22">
	<rdf:type rdf:resource="http://www.w3.org/2000/01/rdf-schema#Resource"/>
	<rdf:type rdf:resource="http://www.w3.org/2004/02/skos/core#Concept"/>
	<dcterms:created rdf:datatype="http://www.w3.org/2001/XMLSchema#dateTime">2014-05-22T00:00:00Z</dcterms:created>
	<dc:publisher rdf:datatype="http://www.w3.org/2001/XMLSchema#string">British Oceanographic Data Centre (BODC)</dc:publisher>
	<dc:source rdf:datatype="http://www.w3.org/2001/XMLSchema#string">(L051) SeaDataNet device categories</dc:source>
	<skos:definition xml:lang="en">Instruments measuring the relative levels of electromagnetic radiation of different wavelengths in the gamma-ray waveband.</skos:definition>
	<skos:inScheme rdf:resource="http://vocab.aodn.org.au/def/instrument/1"/>
	<skos:prefLabel xml:lang="en">gamma-ray spectrometers</skos:prefLabel>
	<skos:topConceptOf rdf:resource="http://vocab.aodn.org.au/def/instrument/1"/>
</rdf:Description>

<rdf:Description rdf:about="http://vocab.nerc.ac.uk/collection/L05/current/LAB25">
	<rdf:type rdf:resource="http://www.w3.org/2000/01/rdf-schema#Resource"/>
	<rdf:type rdf:resource="http://www.w3.org/2004/02/skos/core#Concept"/>
	<dcterms:created rdf:datatype="http://www.w3.org/2001/XMLSchema#dateTime">2014-05-22T00:00:00Z</dcterms:created>
	<dc:publisher rdf:datatype="http://www.w3.org/2001/XMLSchema#string">British Oceanographic Data Centre (BODC)</dc:publisher>
	<dc:source rdf:datatype="http://www.w3.org/2001/XMLSchema#string">(L051) SeaDataNet device categories</dc:source>
	<skos:definition xml:lang="en">Instruments that identify and quantify the elemental constituents of a sample from the spectrum of electromagnetic radiation emitted by the atoms in the sample when excited by X-ray radiation.</skos:definition>
	<skos:inScheme rdf:resource="http://vocab.aodn.org.au/def/instrument/1"/>
	<skos:prefLabel xml:lang="en">X-ray fluorescence analysers</skos:prefLabel>
	<skos:topConceptOf rdf:resource="http://vocab.aodn.org.au/def/instrument/1"/>
</rdf:Description>

<rdf:Description rdf:about="http://vocab.nerc.ac.uk/collection/L05/current/LAB37">
	<rdf:type rdf:resource="http://www.w3.org/2000/01/rdf-schema#Resource"/>
	<rdf:type rdf:resource="http://www.w3.org/2004/02/skos/core#Concept"/>
	<dcterms:created rdf:datatype="http://www.w3.org/2001/XMLSchema#dateTime">2013-03-28T00:00:00Z</dcterms:created>
	<dc:publisher rdf:datatype="http://www.w3.org/2001/XMLSchema#string">British Oceanographic Data Centre (BODC)</dc:publisher>
	<dc:source rdf:datatype="http://www.w3.org/2001/XMLSchema#string">(L051) SeaDataNet device categories</dc:source>
	<skos:definition xml:lang="en">Instruments that suspend cells in a stream of fluid past detection sensors whilst illuminating them with laser light. Used for cell counting sorting biomarker detection and protein engineering.</skos:definition>
	<skos:inScheme rdf:resource="http://vocab.aodn.org.au/def/instrument/1"/>
	<skos:prefLabel xml:lang="en">flow cytometers</skos:prefLabel>
	<skos:topConceptOf rdf:resource="http://vocab.aodn.org.au/def/instrument/1"/>
</rdf:Description>

<rdf:Description rdf:about="http://vocab.nerc.ac.uk/collection/L05/current/LAB39">
	<rdf:type rdf:resource="http://www.w3.org/2000/01/rdf-schema#Resource"/>
	<rdf:type rdf:resource="http://www.w3.org/2004/02/skos/core#Concept"/>
	<dcterms:contributor rdf:resource="http://editor.vocabs.ands.org.au/user/eMII_Atkins.Natalia"/>
	<dcterms:created rdf:datatype="http://www.w3.org/2001/XMLSchema#dateTime">2014-05-29T00:00:00Z</dcterms:created>
	<dcterms:modified rdf:datatype="http://www.w3.org/2001/XMLSchema#dateTime">2016-10-21T02:29:03Z</dcterms:modified>
	<dc:publisher rdf:datatype="http://www.w3.org/2001/XMLSchema#string">British Oceanographic Data Centre (BODC)</dc:publisher>
	<dc:source rdf:datatype="http://www.w3.org/2001/XMLSchema#string">(L051) SeaDataNet device categories</dc:source>
	<skos:definition xml:lang="en">Instruments that measure the amount of alpha, beta or gamma radiation through quantification of the ionization of a low-pressure gas contained in a tube. Sometimes referred to as Geiger-Müller counters.</skos:definition>
	<skos:inScheme rdf:resource="http://vocab.aodn.org.au/def/instrument/1"/>
	<skos:prefLabel xml:lang="en">Geiger counters</skos:prefLabel>
	<skos:topConceptOf rdf:resource="http://vocab.aodn.org.au/def/instrument/1"/>
</rdf:Description>

<rdf:Description rdf:about="http://vocab.nerc.ac.uk/collection/L05/current/LAB40">
	<rdf:type rdf:resource="http://www.w3.org/2000/01/rdf-schema#Resource"/>
	<rdf:type rdf:resource="http://www.w3.org/2004/02/skos/core#Concept"/>
	<dcterms:created rdf:datatype="http://www.w3.org/2001/XMLSchema#dateTime">2013-07-18T00:00:00Z</dcterms:created>
	<dc:publisher rdf:datatype="http://www.w3.org/2001/XMLSchema#string">British Oceanographic Data Centre (BODC)</dc:publisher>
	<dc:source rdf:datatype="http://www.w3.org/2001/XMLSchema#string">(L051) SeaDataNet device categories</dc:source>
	<skos:definition xml:lang="en">Pieces of apparatus that determine the volume of a liquid sample or dispense measured volumes of liquid. Includes devices covering a wide range of sophistication from measuring cylinders syringes and manual pipettes through to programmable electronic instruments.</skos:definition>
	<skos:inScheme rdf:resource="http://vocab.aodn.org.au/def/instrument/1"/>
	<skos:prefLabel xml:lang="en">Volume measures</skos:prefLabel>
	<skos:topConceptOf rdf:resource="http://vocab.aodn.org.au/def/instrument/1"/>
</rdf:Description>

<rdf:Description rdf:about="http://vocab.nerc.ac.uk/collection/L05/current/POS03">
	<rdf:type rdf:resource="http://www.w3.org/2000/01/rdf-schema#Resource"/>
	<rdf:type rdf:resource="http://www.w3.org/2004/02/skos/core#Concept"/>
	<dcterms:contributor rdf:resource="http://editor.vocabs.ands.org.au/user/Natalia_Atkins"/>
	<dcterms:created rdf:datatype="http://www.w3.org/2001/XMLSchema#dateTime">2015-06-03T00:00:00Z</dcterms:created>
	<dcterms:modified rdf:datatype="http://www.w3.org/2001/XMLSchema#dateTime">2015-07-08T04:07:04Z</dcterms:modified>
	<dc:publisher rdf:datatype="http://www.w3.org/2001/XMLSchema#string">British Oceanographic Data Centre (BODC)</dc:publisher>
	<skos:definition xml:lang="en">Accuracy better than 100m, Global navigation based on a network of satellites deployed and maintained by the USA.</skos:definition>
	<skos:inScheme rdf:resource="http://vocab.aodn.org.au/def/instrument/1"/>
	<skos:narrower rdf:resource="http://vocab.nerc.ac.uk/collection/L22/current/TOOL0873"/>
	<skos:narrower rdf:resource="http://vocab.nerc.ac.uk/collection/L22/current/TOOL0878"/>
	<skos:prefLabel xml:lang="en">NAVSTAR Global Positioning System receivers</skos:prefLabel>
	<skos:topConceptOf rdf:resource="http://vocab.aodn.org.au/def/instrument/1"/>
	<skos:altLabel xml:lang="en">GPS</skos:altLabel>
</rdf:Description>

<rdf:Description rdf:about="http://vocab.nerc.ac.uk/collection/L05/current/POS17">
	<rdf:type rdf:resource="http://www.w3.org/2000/01/rdf-schema#Resource"/>
	<rdf:type rdf:resource="http://www.w3.org/2004/02/skos/core#Concept"/>
	<dcterms:contributor rdf:resource="http://editor.vocabs.ands.org.au/user/Natalia_Atkins"/>
	<dcterms:created rdf:datatype="http://www.w3.org/2001/XMLSchema#dateTime">2013-07-18T00:00:00Z</dcterms:created>
	<dcterms:modified rdf:datatype="http://www.w3.org/2001/XMLSchema#dateTime">2015-07-17T01:38:50Z</dcterms:modified>
	<dc:publisher rdf:datatype="http://www.w3.org/2001/XMLSchema#string">British Oceanographic Data Centre (BODC)</dc:publisher>
	<dc:source rdf:datatype="http://www.w3.org/2001/XMLSchema#string">(L051) SeaDataNet device categories</dc:source>
	<skos:definition xml:lang="en">&lt;mode&gt;Doppler-derived Argos localisation&lt;/mode&gt;&lt;accuracy&gt;better than 250m (class 3) to worse than 1500m (class 0)&lt;/accuracy&gt;</skos:definition>
	<skos:inScheme rdf:resource="http://vocab.aodn.org.au/def/instrument/1"/>
	<skos:narrower rdf:resource="http://vocab.nerc.ac.uk/collection/L22/current/TOOL0720"/>
	<skos:narrower rdf:resource="http://vocab.nerc.ac.uk/collection/L22/current/TOOL0446"/>
	<skos:narrower rdf:resource="http://vocab.nerc.ac.uk/collection/L22/current/TOOL0719"/>
	<skos:prefLabel xml:lang="en">Argos doppler-localised transmitters</skos:prefLabel>
	<skos:topConceptOf rdf:resource="http://vocab.aodn.org.au/def/instrument/1"/>
</rdf:Description>

<rdf:Description rdf:about="http://vocab.nerc.ac.uk/collection/L05/current/WPS">
	<rdf:type rdf:resource="http://www.w3.org/2000/01/rdf-schema#Resource"/>
	<rdf:type rdf:resource="http://www.w3.org/2004/02/skos/core#Concept"/>
	<dcterms:contributor rdf:resource="http://editor.vocabs.ands.org.au/user/eMII_Atkins.Natalia"/>
	<dcterms:created rdf:datatype="http://www.w3.org/2001/XMLSchema#dateTime">2015-06-03T00:00:00Z</dcterms:created>
	<dcterms:modified rdf:datatype="http://www.w3.org/2001/XMLSchema#dateTime">2017-04-10T05:00:47Z</dcterms:modified>
	<dc:publisher rdf:datatype="http://www.w3.org/2001/XMLSchema#string">British Oceanographic Data Centre (BODC)</dc:publisher>
	<skos:definition xml:lang="en">Sensors measuring hydrostatic pressure that are capable of withstanding the physical demands made by in-situ measurements in water bodies. Depending upon the mode of deployment they may measure sea level, waves, mooring performance or the depth of a profiling instrument.</skos:definition>
	<skos:inScheme rdf:resource="http://vocab.aodn.org.au/def/instrument/1"/>
	<skos:narrower rdf:resource="http://vocab.nerc.ac.uk/collection/L22/current/TOOL0873"/>
	<skos:narrower rdf:resource="http://vocab.nerc.ac.uk/collection/L22/current/TOOL0931"/>
	<skos:narrower rdf:resource="http://vocab.nerc.ac.uk/collection/L22/current/TOOL1009"/>
	<skos:narrower rdf:resource="http://vocab.nerc.ac.uk/collection/L22/current/TOOL1010"/>
	<skos:narrower rdf:resource="http://vocab.nerc.ac.uk/collection/L22/current/TOOL1125"/>
	<skos:narrower rdf:resource="http://vocab.nerc.ac.uk/collection/L22/current/TOOL1121"/>
	<skos:narrower rdf:resource="http://vocab.nerc.ac.uk/collection/L22/current/TOOL1122"/>
	<skos:narrower rdf:resource="http://vocab.nerc.ac.uk/collection/L22/current/TOOL1124"/>
	<skos:narrower rdf:resource="http://vocab.nerc.ac.uk/collection/L22/current/TOOL1141"/>
	<skos:prefLabel xml:lang="en">water pressure sensors</skos:prefLabel>
	<skos:topConceptOf rdf:resource="http://vocab.aodn.org.au/def/instrument/1"/>
</rdf:Description>

<rdf:Description rdf:about="http://purl.org/dc/elements/1.1/publisher">
	<rdf:type rdf:resource="http://www.w3.org/1999/02/22-rdf-syntax-ns#Property"/>
	<rdf:type rdf:resource="http://www.w3.org/2000/01/rdf-schema#Resource"/>
	<rdfs:subPropertyOf rdf:resource="http://purl.org/dc/elements/1.1/publisher"/>
</rdf:Description>

<rdf:Description rdf:about="http://purl.org/dc/elements/1.1/source">
	<rdf:type rdf:resource="http://www.w3.org/1999/02/22-rdf-syntax-ns#Property"/>
	<rdf:type rdf:resource="http://www.w3.org/2000/01/rdf-schema#Resource"/>
	<rdfs:subPropertyOf rdf:resource="http://purl.org/dc/elements/1.1/source"/>
</rdf:Description>

<rdf:Description rdf:about="http://www.w3.org/2004/02/skos/core#Concept">
	<rdf:type rdf:resource="http://www.w3.org/2000/01/rdf-schema#Resource"/>
	<rdf:type rdf:resource="http://www.w3.org/2000/01/rdf-schema#Class"/>
	<rdfs:subClassOf rdf:resource="http://www.w3.org/2000/01/rdf-schema#Resource"/>
	<rdfs:subClassOf rdf:resource="http://www.w3.org/2004/02/skos/core#Concept"/>
</rdf:Description>

<rdf:Description rdf:about="http://www.w3.org/2004/02/skos/core#definition">
	<rdf:type rdf:resource="http://www.w3.org/1999/02/22-rdf-syntax-ns#Property"/>
	<rdf:type rdf:resource="http://www.w3.org/2000/01/rdf-schema#Resource"/>
	<rdfs:subPropertyOf rdf:resource="http://www.w3.org/2004/02/skos/core#definition"/>
</rdf:Description>

<rdf:Description rdf:about="http://www.w3.org/2004/02/skos/core#inScheme">
	<rdf:type rdf:resource="http://www.w3.org/1999/02/22-rdf-syntax-ns#Property"/>
	<rdf:type rdf:resource="http://www.w3.org/2000/01/rdf-schema#Resource"/>
	<rdfs:subPropertyOf rdf:resource="http://www.w3.org/2004/02/skos/core#inScheme"/>
</rdf:Description>

<rdf:Description rdf:about="http://www.w3.org/2004/02/skos/core#narrower">
	<rdf:type rdf:resource="http://www.w3.org/1999/02/22-rdf-syntax-ns#Property"/>
	<rdf:type rdf:resource="http://www.w3.org/2000/01/rdf-schema#Resource"/>
	<rdfs:subPropertyOf rdf:resource="http://www.w3.org/2004/02/skos/core#narrower"/>
</rdf:Description>

<rdf:Description rdf:about="http://vocab.nerc.ac.uk/collection/L22/current/TOOL0215">
	<rdf:type rdf:resource="http://www.w3.org/2000/01/rdf-schema#Resource"/>
	<rdf:type rdf:resource="http://www.w3.org/2004/02/skos/core#Concept"/>
	<dcterms:created rdf:datatype="http://www.w3.org/2001/XMLSchema#dateTime">2013-12-16T00:00:00Z</dcterms:created>
	<dc:publisher rdf:datatype="http://www.w3.org/2001/XMLSchema#string">British Oceanographic Data Centre (BODC)</dc:publisher>
	<dc:source rdf:datatype="http://www.w3.org/2001/XMLSchema#string">(L221) SeaVoX Device Catalogue</dc:source>
	<skos:definition xml:lang="en">The ECO-FLNTU combines the ECO fluorometer with an optical scattering measurement at 700nm for simultaneous determination of turbidity. The fluorometer can typically measure phytoplankton concentrations in the range 0.01-50 ug/l, with a sensitivity of 0.01 ug/l. The turbidity sensor can measure within the range 0.01-25 NTU, with a sensitivity of 0.01 NTU. The instrument is stable over a temperature range of 0-20 degC and is rated to a depth of 600 m as standard, with the option of a 'deep' instrument rated to 6000m.</skos:definition>
	<skos:inScheme rdf:resource="http://vocab.aodn.org.au/def/instrument/1"/>
	<skos:prefLabel xml:lang="en">WETLabs ECO-FLNTU combined fluorometer and turbidity sensor</skos:prefLabel>
	<skos:broader rdf:resource="http://vocab.aodn.org.au/def/instrument/entity/361"/>
	<skos:broader rdf:resource="http://vocab.nerc.ac.uk/collection/L05/current/113"/>
	<skos:broader rdf:resource="http://vocab.nerc.ac.uk/collection/L05/current/123"/>
	<skos:scopeNote xml:lang="en">manufacture:WETLabs Inc.</skos:scopeNote>
</rdf:Description>

<rdf:Description rdf:about="http://vocab.nerc.ac.uk/collection/L22/current/TOOL0673">
	<rdf:type rdf:resource="http://www.w3.org/2000/01/rdf-schema#Resource"/>
	<rdf:type rdf:resource="http://www.w3.org/2004/02/skos/core#Concept"/>
	<dcterms:created rdf:datatype="http://www.w3.org/2001/XMLSchema#dateTime">2013-09-11T00:00:00Z</dcterms:created>
	<dc:publisher rdf:datatype="http://www.w3.org/2001/XMLSchema#string">British Oceanographic Data Centre (BODC)</dc:publisher>
	<dc:source rdf:datatype="http://www.w3.org/2001/XMLSchema#string">(L221) SeaVoX Device Catalogue</dc:source>
	<skos:definition xml:lang="en">A miniature version of the Environmental Characterisation Optics (ECO) sensors built for OEM applications, with the design specifically targeted at AUVs, gliders and profiling floats. The triplet version carries a fluorometer plus two other sensors that may be additional fluorometers, single-wavelength scattering meters (BB) or a volume scattering function meter (VSF). The fluorometers are single wavelength sensors that can be configured for chlorophyll-a, CDOM, phycocyanin, phycoerythrin, fluorescein or rhodamine. BB measures optical scattering at 117 degrees at 470, 532 or 650 nm wavelengths. VSF measures optical scattering at 100, 125 and 150 degrees. More information may be found at http://www.wetlabs.com/eco-puck.</skos:definition>
	<skos:inScheme rdf:resource="http://vocab.aodn.org.au/def/instrument/1"/>
	<skos:prefLabel xml:lang="en">WETLabs ECO Puck Triple-Measurement Meter</skos:prefLabel>
	<skos:broader rdf:resource="http://vocab.aodn.org.au/def/instrument/entity/361"/>
	<skos:broader rdf:resource="http://vocab.nerc.ac.uk/collection/L05/current/113"/>
	<skos:broader rdf:resource="http://vocab.nerc.ac.uk/collection/L05/current/123"/>
	<skos:scopeNote xml:lang="en">manufacture:WETLabs Inc.</skos:scopeNote>
</rdf:Description>

<rdf:Description rdf:about="http://vocab.nerc.ac.uk/collection/L22/current/TOOL0674">
	<rdf:type rdf:resource="http://www.w3.org/2000/01/rdf-schema#Resource"/>
	<rdf:type rdf:resource="http://www.w3.org/2004/02/skos/core#Concept"/>
	<dcterms:created rdf:datatype="http://www.w3.org/2001/XMLSchema#dateTime">2013-09-10T00:00:00Z</dcterms:created>
	<dc:publisher rdf:datatype="http://www.w3.org/2001/XMLSchema#string">British Oceanographic Data Centre (BODC)</dc:publisher>
	<dc:source rdf:datatype="http://www.w3.org/2001/XMLSchema#string">(L221) SeaVoX Device Catalogue</dc:source>
	<skos:definition xml:lang="en">A three-optical-sensor instrument that may carry any combination of fluorometers or single-wavelength scattering meters. The fluorometers are single wavelength sensors that can be configured for chlorophyll-a, CDOM, phycocyanin, phycoerythrin, fluorescein or rhodamine. Scattering meters measure optical scattering at blue, green or red wavelengths. More information may be found at http://www.wetlabs.com/eco-triplet.</skos:definition>
	<skos:inScheme rdf:resource="http://vocab.aodn.org.au/def/instrument/1"/>
	<skos:prefLabel xml:lang="en">WETLabs ECO Triplet</skos:prefLabel>
	<skos:broader rdf:resource="http://vocab.aodn.org.au/def/instrument/entity/361"/>
	<skos:broader rdf:resource="http://vocab.nerc.ac.uk/collection/L05/current/113"/>
	<skos:broader rdf:resource="http://vocab.nerc.ac.uk/collection/L05/current/123"/>
	<skos:scopeNote xml:lang="en">manufacture:WETLabs Inc.</skos:scopeNote>
</rdf:Description>

<rdf:Description rdf:about="http://vocab.nerc.ac.uk/collection/L22/current/TOOL0675">
	<rdf:type rdf:resource="http://www.w3.org/2000/01/rdf-schema#Resource"/>
	<rdf:type rdf:resource="http://www.w3.org/2004/02/skos/core#Concept"/>
	<dcterms:created rdf:datatype="http://www.w3.org/2001/XMLSchema#dateTime">2014-04-01T00:00:00Z</dcterms:created>
	<dc:publisher rdf:datatype="http://www.w3.org/2001/XMLSchema#string">British Oceanographic Data Centre (BODC)</dc:publisher>
	<dc:source rdf:datatype="http://www.w3.org/2001/XMLSchema#string">(L221) SeaVoX Device Catalogue</dc:source>
	<skos:definition xml:lang="en">An instrument that incorporates WET Labs fluorometer-turbidity and Sea-Bird's CTD sensors, providing temperature, salinity, depth, dissolved oxygen, chlorophyll fluorescence, turbidity and backscattering data. It is designed for long-term deployment in coastal waters with protection against biofouling and fouling by sediment loads. More information is available at http://www.wetlabs.com/wqm.</skos:definition>
	<skos:inScheme rdf:resource="http://vocab.aodn.org.au/def/instrument/1"/>
	<skos:prefLabel xml:lang="en">WETLabs Water Quality Monitor</skos:prefLabel>
	<skos:broader rdf:resource="http://vocab.aodn.org.au/def/instrument/entity/361"/>
	<skos:broader rdf:resource="http://vocab.nerc.ac.uk/collection/L05/current/111"/>
	<skos:broader rdf:resource="http://vocab.nerc.ac.uk/collection/L05/current/113"/>
	<skos:broader rdf:resource="http://vocab.nerc.ac.uk/collection/L05/current/123"/>
	<skos:broader rdf:resource="http://vocab.nerc.ac.uk/collection/L05/current/134"/>
	<skos:broader rdf:resource="http://vocab.nerc.ac.uk/collection/L05/current/350"/>
	<skos:broader rdf:resource="http://vocab.nerc.ac.uk/collection/L05/current/351"/>
	<skos:scopeNote xml:lang="en">manufacture:WETLabs Inc.</skos:scopeNote>
</rdf:Description>

<rdf:Description rdf:about="http://www.w3.org/2004/02/skos/core#prefLabel">
	<rdf:type rdf:resource="http://www.w3.org/1999/02/22-rdf-syntax-ns#Property"/>
	<rdf:type rdf:resource="http://www.w3.org/2000/01/rdf-schema#Resource"/>
	<rdfs:subPropertyOf rdf:resource="http://www.w3.org/2004/02/skos/core#prefLabel"/>
</rdf:Description>

<rdf:Description rdf:about="http://www.w3.org/2004/02/skos/core#topConceptOf">
	<rdf:type rdf:resource="http://www.w3.org/1999/02/22-rdf-syntax-ns#Property"/>
	<rdf:type rdf:resource="http://www.w3.org/2000/01/rdf-schema#Resource"/>
	<rdfs:subPropertyOf rdf:resource="http://www.w3.org/2004/02/skos/core#topConceptOf"/>
</rdf:Description>

<rdf:Description rdf:about="http://vocab.nerc.ac.uk/collection/L22/current/TOOL0017">
	<rdf:type rdf:resource="http://www.w3.org/2000/01/rdf-schema#Resource"/>
	<rdf:type rdf:resource="http://www.w3.org/2004/02/skos/core#Concept"/>
	<dcterms:created rdf:datatype="http://www.w3.org/2001/XMLSchema#dateTime">2014-02-06T00:00:00Z</dcterms:created>
	<dc:publisher rdf:datatype="http://www.w3.org/2001/XMLSchema#string">British Oceanographic Data Centre (BODC)</dc:publisher>
	<dc:source rdf:datatype="http://www.w3.org/2001/XMLSchema#string">(L221) SeaVoX Device Catalogue</dc:source>
	<skos:definition xml:lang="en">The SBE 37 MicroCAT is a high accuracy conductivity and temperature recorder with an optional pressure sensor designed for depolyment on moorings. The SM model has a serial interface plus internal flash memory data storage. Further information may be found on the BODC document server at URL http://www.bodc.ac.uk/data/documents/nodb/108613/.</skos:definition>
	<skos:inScheme rdf:resource="http://vocab.aodn.org.au/def/instrument/1"/>
	<skos:prefLabel xml:lang="en">Sea-Bird SBE 37-SM MicroCAT C-T Sensor</skos:prefLabel>
	<skos:broader rdf:resource="http://vocab.aodn.org.au/def/instrument/entity/365"/>
	<skos:broader rdf:resource="http://vocab.nerc.ac.uk/collection/L05/current/134"/>
	<skos:broader rdf:resource="http://vocab.nerc.ac.uk/collection/L05/current/350"/>
	<skos:scopeNote xml:lang="en">manufacturer:Sea-Bird Electronics Inc.</skos:scopeNote>
</rdf:Description>

<rdf:Description rdf:about="http://vocab.nerc.ac.uk/collection/L22/current/TOOL0018">
	<rdf:type rdf:resource="http://www.w3.org/2000/01/rdf-schema#Resource"/>
	<rdf:type rdf:resource="http://www.w3.org/2004/02/skos/core#Concept"/>
	<dcterms:created rdf:datatype="http://www.w3.org/2001/XMLSchema#dateTime">2014-02-06T00:00:00Z</dcterms:created>
	<dc:publisher rdf:datatype="http://www.w3.org/2001/XMLSchema#string">British Oceanographic Data Centre (BODC)</dc:publisher>
	<dc:source rdf:datatype="http://www.w3.org/2001/XMLSchema#string">(L221) SeaVoX Device Catalogue</dc:source>
	<skos:definition xml:lang="en">The SBE 37 MicroCAT is a high accuracy conductivity and temperature recorder with an optional pressure sensor designed for depolyment on moorings. The SMP model has a serial interface plus internal flash memory data storage with an internal pump to improve conductivity response and protection against fouling.</skos:definition>
	<skos:inScheme rdf:resource="http://vocab.aodn.org.au/def/instrument/1"/>
	<skos:prefLabel xml:lang="en">Sea-Bird SBE 37-SMP MicroCAT C-T Sensor</skos:prefLabel>
	<skos:broader rdf:resource="http://vocab.aodn.org.au/def/instrument/entity/365"/>
	<skos:broader rdf:resource="http://vocab.nerc.ac.uk/collection/L05/current/134"/>
	<skos:broader rdf:resource="http://vocab.nerc.ac.uk/collection/L05/current/350"/>
	<skos:scopeNote xml:lang="en">manufacturer:Sea-Bird Electronics Inc.</skos:scopeNote>
</rdf:Description>

<rdf:Description rdf:about="http://vocab.nerc.ac.uk/collection/L22/current/TOOL0019">
	<rdf:type rdf:resource="http://www.w3.org/2000/01/rdf-schema#Resource"/>
	<rdf:type rdf:resource="http://www.w3.org/2004/02/skos/core#Concept"/>
	<dcterms:created rdf:datatype="http://www.w3.org/2001/XMLSchema#dateTime">2014-02-17T00:00:00Z</dcterms:created>
	<dc:publisher rdf:datatype="http://www.w3.org/2001/XMLSchema#string">British Oceanographic Data Centre (BODC)</dc:publisher>
	<dc:source rdf:datatype="http://www.w3.org/2001/XMLSchema#string">(L221) SeaVoX Device Catalogue</dc:source>
	<skos:definition xml:lang="en">The SBE 37 MicroCAT is a high accuracy conductivity and temperature recorder with an optional pressure sensor designed for depolyment on moorings. The IMP model has an inductive modem for real-time data transmission plus internal flash memory data storage with an internal pump to improve conductivity response and protection against fouling.</skos:definition>
	<skos:inScheme rdf:resource="http://vocab.aodn.org.au/def/instrument/1"/>
	<skos:prefLabel xml:lang="en">Sea-Bird SBE 37-IMP MicroCAT C-T Sensor</skos:prefLabel>
	<skos:broader rdf:resource="http://vocab.aodn.org.au/def/instrument/entity/365"/>
	<skos:broader rdf:resource="http://vocab.nerc.ac.uk/collection/L05/current/134"/>
	<skos:broader rdf:resource="http://vocab.nerc.ac.uk/collection/L05/current/350"/>
	<skos:scopeNote xml:lang="en">manufacturer:Sea-Bird Electronics Inc.</skos:scopeNote>
</rdf:Description>

<rdf:Description rdf:about="http://vocab.nerc.ac.uk/collection/L22/current/TOOL0020">
	<rdf:type rdf:resource="http://www.w3.org/2000/01/rdf-schema#Resource"/>
	<rdf:type rdf:resource="http://www.w3.org/2004/02/skos/core#Concept"/>
	<dcterms:created rdf:datatype="http://www.w3.org/2001/XMLSchema#dateTime">2014-02-26T00:00:00Z</dcterms:created>
	<dc:publisher rdf:datatype="http://www.w3.org/2001/XMLSchema#string">British Oceanographic Data Centre (BODC)</dc:publisher>
	<dc:source rdf:datatype="http://www.w3.org/2001/XMLSchema#string">(L221) SeaVoX Device Catalogue</dc:source>
	<skos:definition xml:lang="en">The SBE 37 MicroCAT is a high accuracy conductivity and temperature recorder with an optional pressure sensor designed for depolyment on moorings. The SIP model has a serial interface with an internal pump to improve conductivity response and protection against fouling.</skos:definition>
	<skos:inScheme rdf:resource="http://vocab.aodn.org.au/def/instrument/1"/>
	<skos:prefLabel xml:lang="en">Sea-Bird SBE 37-SIP MicroCAT C-T Sensor</skos:prefLabel>
	<skos:broader rdf:resource="http://vocab.aodn.org.au/def/instrument/entity/365"/>
	<skos:broader rdf:resource="http://vocab.nerc.ac.uk/collection/L05/current/134"/>
	<skos:broader rdf:resource="http://vocab.nerc.ac.uk/collection/L05/current/350"/>
	<skos:scopeNote xml:lang="en">manufacturer:Sea-Bird Electronics Inc.</skos:scopeNote>
</rdf:Description>

<rdf:Description rdf:about="http://vocab.nerc.ac.uk/collection/L22/current/TOOL0023">
	<rdf:type rdf:resource="http://www.w3.org/2000/01/rdf-schema#Resource"/>
	<rdf:type rdf:resource="http://www.w3.org/2004/02/skos/core#Concept"/>
	<dcterms:created rdf:datatype="http://www.w3.org/2001/XMLSchema#dateTime">2014-02-17T00:00:00Z</dcterms:created>
	<dc:publisher rdf:datatype="http://www.w3.org/2001/XMLSchema#string">British Oceanographic Data Centre (BODC)</dc:publisher>
	<dc:source rdf:datatype="http://www.w3.org/2001/XMLSchema#string">(L221) SeaVoX Device Catalogue</dc:source>
	<skos:definition xml:lang="en">The SBE 16 SEACAT is a conductivity and temperature recorder with an optional pressure sensor designed for depolyment on moorings. Further information may be found on the BODC document server at URL http://www.bodc.ac.uk/data/documents/nodb/117180/. Replaced by the SBE 16plus range in 2001.</skos:definition>
	<skos:inScheme rdf:resource="http://vocab.aodn.org.au/def/instrument/1"/>
	<skos:prefLabel xml:lang="en">Sea-Bird SBE 16 SEACAT C-T Recorder</skos:prefLabel>
	<skos:broader rdf:resource="http://vocab.aodn.org.au/def/instrument/entity/365"/>
	<skos:broader rdf:resource="http://vocab.nerc.ac.uk/collection/L05/current/134"/>
	<skos:broader rdf:resource="http://vocab.nerc.ac.uk/collection/L05/current/350"/>
	<skos:scopeNote xml:lang="en">manufacturer:Sea-Bird Electronics Inc.</skos:scopeNote>
</rdf:Description>

<rdf:Description rdf:about="http://vocab.nerc.ac.uk/collection/L22/current/TOOL0053">
	<rdf:type rdf:resource="http://www.w3.org/2000/01/rdf-schema#Resource"/>
	<rdf:type rdf:resource="http://www.w3.org/2004/02/skos/core#Concept"/>
	<dcterms:created rdf:datatype="http://www.w3.org/2001/XMLSchema#dateTime">2014-02-17T00:00:00Z</dcterms:created>
	<dc:publisher rdf:datatype="http://www.w3.org/2001/XMLSchema#string">British Oceanographic Data Centre (BODC)</dc:publisher>
	<dc:source rdf:datatype="http://www.w3.org/2001/XMLSchema#string">(L221) SeaVoX Device Catalogue</dc:source>
	<skos:definition xml:lang="en">A small autonomous data logger designed to monitor conductivity, temperature and depth. Conductivity (accuracy ± 0.003 mS/cm) is measured using a 3-coil closed loop feedback inductive cell for superior temperature compensation. The thermistor (Themometrics) used to record temperature (accuracy ± 0.002°C) is aged and hermetically sealed in the tip of a shock resistant solid glass rod. Pressure (accuracy 0.05% full scale) sensors use reliable semiconductor technology and 316 stainless steel housing developed for long-term stability in harsh environments.</skos:definition>
	<skos:inScheme rdf:resource="http://vocab.aodn.org.au/def/instrument/1"/>
	<skos:prefLabel xml:lang="en">RBR XR-420 CTD Marine</skos:prefLabel>
	<skos:broader rdf:resource="http://vocab.aodn.org.au/def/instrument/entity/365"/>
	<skos:broader rdf:resource="http://vocab.nerc.ac.uk/collection/L05/current/134"/>
	<skos:broader rdf:resource="http://vocab.nerc.ac.uk/collection/L05/current/350"/>
	<skos:scopeNote xml:lang="en">manufacturer: RBR</skos:scopeNote>
</rdf:Description>

<rdf:Description rdf:about="http://vocab.nerc.ac.uk/collection/L22/current/TOOL0100">
	<rdf:type rdf:resource="http://www.w3.org/2000/01/rdf-schema#Resource"/>
	<rdf:type rdf:resource="http://www.w3.org/2004/02/skos/core#Concept"/>
	<dcterms:created rdf:datatype="http://www.w3.org/2001/XMLSchema#dateTime">2014-02-07T00:00:00Z</dcterms:created>
	<dc:publisher rdf:datatype="http://www.w3.org/2001/XMLSchema#string">British Oceanographic Data Centre (BODC)</dc:publisher>
	<dc:source rdf:datatype="http://www.w3.org/2001/XMLSchema#string">(L221) SeaVoX Device Catalogue</dc:source>
	<skos:definition xml:lang="en">The SBE 16plus is a high accuracy conductivity and temperature recorder (pressure optional) with RS232 or RS485 interfaces. It is designed for moorings and other long-duration, fixed-site deployments. The SBE 16plus has 6 amplified A/D input channels and conditioned power of 500 ma is avaliable for auxiliary sensors, dissolved oxygen, turbidity, fluorescence, PAR etc. Further information may be found on the BODC document server at URL: http://www.bodc.ac.uk/data/documents/nodb/153217/ (RS485) or http://www.bodc.ac.uk/data/documents/nodb/158981/ (RS232).</skos:definition>
	<skos:inScheme rdf:resource="http://vocab.aodn.org.au/def/instrument/1"/>
	<skos:prefLabel xml:lang="en">Sea-Bird SBE 16Plus SEACAT C-T Recorder</skos:prefLabel>
	<skos:broader rdf:resource="http://vocab.aodn.org.au/def/instrument/entity/365"/>
	<skos:broader rdf:resource="http://vocab.nerc.ac.uk/collection/L05/current/134"/>
	<skos:broader rdf:resource="http://vocab.nerc.ac.uk/collection/L05/current/350"/>
	<skos:scopeNote xml:lang="en">manufacturer:Sea-Bird Electronics Inc.</skos:scopeNote>
</rdf:Description>

<rdf:Description rdf:about="http://vocab.aodn.org.au/def/instrument/entity/39">
	<rdf:type rdf:resource="http://www.w3.org/2000/01/rdf-schema#Resource"/>
	<rdf:type rdf:resource="http://www.w3.org/2004/02/skos/core#Concept"/>
	<dcterms:contributor rdf:resource="http://editor.vocabs.ands.org.au/user/Natalia_Atkins"/>
	<dcterms:created rdf:datatype="http://www.w3.org/2001/XMLSchema#dateTime">2013-03-28T00:00:00Z</dcterms:created>
	<dcterms:creator rdf:resource="http://editor.vocabs.ands.org.au/user/Sebastien-Mancini"/>
	<dcterms:modified rdf:datatype="http://www.w3.org/2001/XMLSchema#dateTime">2015-06-30T05:43:15Z</dcterms:modified>
	<dc:publisher rdf:datatype="http://www.w3.org/2001/XMLSchema#string">eMarine Information Infrastructure (eMII)</dc:publisher>
	<dc:source rdf:datatype="http://www.w3.org/2001/XMLSchema#string">Australian Ocean Data Network instrument register</dc:source>
	<skos:definition xml:lang="en">An expendable free-fall temperature probe that provides a profile of measured temperature against depth calculated from a fall-rate model. The Deep Blue XBT Probe (sometimes referred to as the T-7DB) can be used to a maximum depth of 460m, may be deployed at a ship speed of up to 20 knots and has a vertical resolution of 65cm.</skos:definition>
	<skos:inScheme rdf:resource="http://vocab.aodn.org.au/def/instrument/1"/>
	<skos:prefLabel xml:lang="en">Lockheed Martin Sippican Deep Blue XBT probe</skos:prefLabel>
	<skos:broader rdf:resource="http://vocab.nerc.ac.uk/collection/L05/current/132"/>
	<skos:broader rdf:resource="http://vocab.nerc.ac.uk/collection/L05/current/134"/>
	<skos:scopeNote xml:lang="en">manufacturer: Lockheed Martin</skos:scopeNote>
</rdf:Description>

<rdf:Description rdf:about="http://www.w3.org/2004/02/skos/core#broader">
	<rdf:type rdf:resource="http://www.w3.org/1999/02/22-rdf-syntax-ns#Property"/>
	<rdf:type rdf:resource="http://www.w3.org/2000/01/rdf-schema#Resource"/>
	<rdfs:subPropertyOf rdf:resource="http://www.w3.org/2004/02/skos/core#broader"/>
</rdf:Description>

<rdf:Description rdf:about="http://www.w3.org/2004/02/skos/core#scopeNote">
	<rdf:type rdf:resource="http://www.w3.org/1999/02/22-rdf-syntax-ns#Property"/>
	<rdf:type rdf:resource="http://www.w3.org/2000/01/rdf-schema#Resource"/>
	<rdfs:subPropertyOf rdf:resource="http://www.w3.org/2004/02/skos/core#scopeNote"/>
</rdf:Description>

<rdf:Description rdf:about="http://vocab.nerc.ac.uk/collection/L22/current/TOOL0126">
	<rdf:type rdf:resource="http://www.w3.org/2000/01/rdf-schema#Resource"/>
	<rdf:type rdf:resource="http://www.w3.org/2004/02/skos/core#Concept"/>
	<dcterms:created rdf:datatype="http://www.w3.org/2001/XMLSchema#dateTime">2013-10-11T00:00:00Z</dcterms:created>
	<dc:publisher rdf:datatype="http://www.w3.org/2001/XMLSchema#string">British Oceanographic Data Centre (BODC)</dc:publisher>
	<dc:source rdf:datatype="http://www.w3.org/2001/XMLSchema#string">(L221) SeaVoX Device Catalogue</dc:source>
	<skos:definition xml:lang="en">Three lightweight, conical cups mounted on the cup wheel providing linearity with windspeeds up to 75m/s. Rotation speed is measured by a disk attached to the shaft cutting an infrared light beam 14 times per revolution producing pulses counted by a phototransistor. The output rate is directly proportional to wind speed.</skos:definition>
	<skos:inScheme rdf:resource="http://vocab.aodn.org.au/def/instrument/1"/>
	<skos:prefLabel xml:lang="en">Vaisala WAA151 cup anemometer</skos:prefLabel>
	<skos:broader rdf:resource="http://vocab.nerc.ac.uk/collection/L05/current/101"/>
	<skos:scopeNote xml:lang="en">manufacturer:Vaisala</skos:scopeNote>
</rdf:Description>

<rdf:Description rdf:about="http://vocab.nerc.ac.uk/collection/L22/current/TOOL0127">
	<rdf:type rdf:resource="http://www.w3.org/2000/01/rdf-schema#Resource"/>
	<rdf:type rdf:resource="http://www.w3.org/2004/02/skos/core#Concept"/>
	<dcterms:created rdf:datatype="http://www.w3.org/2001/XMLSchema#dateTime">2013-10-11T00:00:00Z</dcterms:created>
	<dc:publisher rdf:datatype="http://www.w3.org/2001/XMLSchema#string">British Oceanographic Data Centre (BODC)</dc:publisher>
	<dc:source rdf:datatype="http://www.w3.org/2001/XMLSchema#string">(L221) SeaVoX Device Catalogue</dc:source>
	<skos:definition xml:lang="en">A counter-balanced, low-threshold, optoelectic wind-vane. Infrared LEDs and phototransistors are mounted on six orbits on each side of a 6-bit GRAY-coded disc. Turning the vane causes the disc to change the code received by the phototransistors.</skos:definition>
	<skos:inScheme rdf:resource="http://vocab.aodn.org.au/def/instrument/1"/>
	<skos:prefLabel xml:lang="en">Vaisala WAV151 wind vane</skos:prefLabel>
	<skos:broader rdf:resource="http://vocab.nerc.ac.uk/collection/L05/current/101"/>
	<skos:scopeNote xml:lang="en">manufacturer:Vaisala</skos:scopeNote>
</rdf:Description>

<rdf:Description rdf:about="http://vocab.nerc.ac.uk/collection/L22/current/TOOL0195">
	<rdf:type rdf:resource="http://www.w3.org/2000/01/rdf-schema#Resource"/>
	<rdf:type rdf:resource="http://www.w3.org/2004/02/skos/core#Concept"/>
	<dcterms:created rdf:datatype="http://www.w3.org/2001/XMLSchema#dateTime">2013-10-11T00:00:00Z</dcterms:created>
	<dc:publisher rdf:datatype="http://www.w3.org/2001/XMLSchema#string">British Oceanographic Data Centre (BODC)</dc:publisher>
	<dc:source rdf:datatype="http://www.w3.org/2001/XMLSchema#string">(L221) SeaVoX Device Catalogue</dc:source>
	<skos:definition xml:lang="en">A lightweight anemometer with a helicoid propellor speed sensor attached to a vane. The instrument is designed to withstand the marine environment.</skos:definition>
	<skos:inScheme rdf:resource="http://vocab.aodn.org.au/def/instrument/1"/>
	<skos:prefLabel xml:lang="en">Young MA05106 Wind Monitor anemometer</skos:prefLabel>
	<skos:broader rdf:resource="http://vocab.nerc.ac.uk/collection/L05/current/101"/>
	<skos:scopeNote xml:lang="en">manufacturer:R.M. Young Company</skos:scopeNote>
</rdf:Description>

<rdf:Description rdf:about="http://vocab.nerc.ac.uk/collection/L22/current/TOOL0260">
	<rdf:type rdf:resource="http://www.w3.org/2000/01/rdf-schema#Resource"/>
	<rdf:type rdf:resource="http://www.w3.org/2004/02/skos/core#Concept"/>
	<dcterms:created rdf:datatype="http://www.w3.org/2001/XMLSchema#dateTime">2013-10-11T00:00:00Z</dcterms:created>
	<dc:publisher rdf:datatype="http://www.w3.org/2001/XMLSchema#string">British Oceanographic Data Centre (BODC)</dc:publisher>
	<dc:source rdf:datatype="http://www.w3.org/2001/XMLSchema#string">(L221) SeaVoX Device Catalogue</dc:source>
	<skos:definition xml:lang="en">An anemometer with a four blade helicoid propeller and lightweight direction vane. Vane angle is sensed by a precision potentiometer. The instrument body is UV stabilized plastic with stainless steel and anodized aluminum fittings. The instrument mounts on standard 1 inch pipe. Windspeed accuracy is +-0.3m/s and wind direction accuracy is 3 degrees.</skos:definition>
	<skos:inScheme rdf:resource="http://vocab.aodn.org.au/def/instrument/1"/>
	<skos:prefLabel xml:lang="en">Young MA05103 Wind Monitor anemometer</skos:prefLabel>
	<skos:broader rdf:resource="http://vocab.nerc.ac.uk/collection/L05/current/101"/>
	<skos:scopeNote xml:lang="en">manufacturer:R.M. Young Company</skos:scopeNote>
</rdf:Description>

<rdf:Description rdf:about="http://vocab.nerc.ac.uk/collection/L22/current/TOOL0704">
	<rdf:type rdf:resource="http://www.w3.org/2000/01/rdf-schema#Resource"/>
	<rdf:type rdf:resource="http://www.w3.org/2004/02/skos/core#Concept"/>
	<dcterms:created rdf:datatype="http://www.w3.org/2001/XMLSchema#dateTime">2013-10-11T00:00:00Z</dcterms:created>
	<dc:publisher rdf:datatype="http://www.w3.org/2001/XMLSchema#string">British Oceanographic Data Centre (BODC)</dc:publisher>
	<dc:source rdf:datatype="http://www.w3.org/2001/XMLSchema#string">(L221) SeaVoX Device Catalogue</dc:source>
	<skos:definition xml:lang="en">The WindObserver II is a solid state ultrasonic anemometer, with a stainless steel housing suitable for marine and offshore applications. It measures wind speed and direction over ranges of 0-65 m/s and 0-359 degrees respectively.</skos:definition>
	<skos:inScheme rdf:resource="http://vocab.aodn.org.au/def/instrument/1"/>
	<skos:prefLabel xml:lang="en">Gill Instruments WindObserver II Anemometer</skos:prefLabel>
	<skos:broader rdf:resource="http://vocab.nerc.ac.uk/collection/L05/current/101"/>
	<skos:scopeNote xml:lang="en">manufacturer:Gill Instruments</skos:scopeNote>
</rdf:Description>

<rdf:Description rdf:about="http://vocab.nerc.ac.uk/collection/L22/current/TOOL1031">
	<rdf:type rdf:resource="http://www.w3.org/2000/01/rdf-schema#Resource"/>
	<rdf:type rdf:resource="http://www.w3.org/2004/02/skos/core#Concept"/>
	<dcterms:contributor rdf:resource="http://editor.vocabs.ands.org.au/user/eMII_Atkins.Natalia"/>
	<dcterms:created rdf:datatype="http://www.w3.org/2001/XMLSchema#dateTime">2017-03-15T00:00:00Z</dcterms:created>
	<dcterms:modified rdf:datatype="http://www.w3.org/2001/XMLSchema#dateTime">2017-03-23T05:10:26Z</dcterms:modified>
	<dc:publisher rdf:datatype="http://www.w3.org/2001/XMLSchema#string">British Oceanographic Data Centre (BODC)</dc:publisher>
	<skos:definition xml:lang="en">Airmar Ultrasonic WeatherStation 150WX is a compact meteorological station designed to provide real-time, site-specific weather information on moving platforms. The instrument combines up to seven sensors to measure apparent and true wind speed and direction, barometric pressure, air temperature, relative humidity, dew point and wind chill temperature. Ultrasonic readings of true and apparent wind speed and direction are taken for wind speeds up to 40 m/s. This model includes: optional heater and upper ring; field-serviceable relative humidity calculated dew point and heat index; a 10 Hz GPS; a two-axis solid-state compass; a three-axis accelerometer. Output options include RS422/CAN BUS and RS232/CAN BUS.</skos:definition>
	<skos:inScheme rdf:resource="http://vocab.aodn.org.au/def/instrument/1"/>
	<skos:prefLabel xml:lang="en">Airmar Ultrasonic WeatherStation 150WX</skos:prefLabel>
	<skos:broader rdf:resource="http://vocab.nerc.ac.uk/collection/L05/current/101"/>
	<skos:broader rdf:resource="http://vocab.nerc.ac.uk/collection/L05/current/102"/>
	<skos:altLabel xml:lang="en">Airmar 150WX</skos:altLabel>
</rdf:Description>

<rdf:Description rdf:about="http://vocab.nerc.ac.uk/collection/L22/current/TOOL0081">
	<rdf:type rdf:resource="http://www.w3.org/2000/01/rdf-schema#Resource"/>
	<rdf:type rdf:resource="http://www.w3.org/2004/02/skos/core#Concept"/>
	<dcterms:created rdf:datatype="http://www.w3.org/2001/XMLSchema#dateTime">2013-10-11T00:00:00Z</dcterms:created>
	<dc:publisher rdf:datatype="http://www.w3.org/2001/XMLSchema#string">British Oceanographic Data Centre (BODC)</dc:publisher>
	<dc:source rdf:datatype="http://www.w3.org/2001/XMLSchema#string">(L221) SeaVoX Device Catalogue</dc:source>
	<skos:definition xml:lang="en">A family of sensors and instruments (sensors plus integral displays or loggers) for the measurement of air temperature and relative humidity. All are based on a probe containing a patent (HUMICAP) capacitive thin film polymer humidity sensor and a Pt100 platinum resistance thermometer. The probes are available with a wide range of packaging, cabling and interface options all of which have designations of the form HMPnn such as HMP45 and HMP75. Vaisala sensors are incorporated into weather stations and marketed by Campbell Scientific.</skos:definition>
	<skos:inScheme rdf:resource="http://vocab.aodn.org.au/def/instrument/1"/>
	<skos:prefLabel xml:lang="en">Vaisala HMP temperature and humidity sensor</skos:prefLabel>
	<skos:broader rdf:resource="http://vocab.nerc.ac.uk/collection/L05/current/102"/>
	<skos:scopeNote xml:lang="en">manufacturer:Vaisala</skos:scopeNote>
</rdf:Description>

<rdf:Description rdf:about="http://vocab.nerc.ac.uk/collection/L22/current/TOOL0617">
	<rdf:type rdf:resource="http://www.w3.org/2000/01/rdf-schema#Resource"/>
	<rdf:type rdf:resource="http://www.w3.org/2004/02/skos/core#Concept"/>
	<dcterms:created rdf:datatype="http://www.w3.org/2001/XMLSchema#dateTime">2014-02-07T00:00:00Z</dcterms:created>
	<dc:publisher rdf:datatype="http://www.w3.org/2001/XMLSchema#string">British Oceanographic Data Centre (BODC)</dc:publisher>
	<dc:source rdf:datatype="http://www.w3.org/2001/XMLSchema#string">(L221) SeaVoX Device Catalogue</dc:source>
	<skos:definition xml:lang="en">An analogue, linear response atmospheric humidity and temperature probe. The instrument operates within 0-100 percent relative humidity (0 to 1 volts), with an accuracy of +/-1 percent. The temperature range varies between -40 to 60 degC (-0.4 to 0.6 volts) definal on the specific model and has an accuracy of +/-0.3 degC.</skos:definition>
	<skos:inScheme rdf:resource="http://vocab.aodn.org.au/def/instrument/1"/>
	<skos:prefLabel xml:lang="en">Rotronic Instruments MP1xxA humidity and temperature probe series</skos:prefLabel>
	<skos:broader rdf:resource="http://vocab.nerc.ac.uk/collection/L05/current/102"/>
	<skos:scopeNote xml:lang="en">manufacturer:Rotronic Instrument Corp.</skos:scopeNote>
</rdf:Description>

<rdf:Description rdf:about="http://vocab.nerc.ac.uk/collection/L22/current/TOOL0672">
	<rdf:type rdf:resource="http://www.w3.org/2000/01/rdf-schema#Resource"/>
	<rdf:type rdf:resource="http://www.w3.org/2004/02/skos/core#Concept"/>
	<dcterms:created rdf:datatype="http://www.w3.org/2001/XMLSchema#dateTime">2013-10-11T00:00:00Z</dcterms:created>
	<dc:publisher rdf:datatype="http://www.w3.org/2001/XMLSchema#string">British Oceanographic Data Centre (BODC)</dc:publisher>
	<dc:source rdf:datatype="http://www.w3.org/2001/XMLSchema#string">(L221) SeaVoX Device Catalogue</dc:source>
	<skos:definition xml:lang="en">Fully compensated digital barometer using a silicon capacitive absolute pressure sensor designed to cover a wide range of environmental pressure and temperature. The pressure and temperature adjustment in the PTB220 consists of seven temperature levels over the operating temperature range of the barometer and of six to eleven pressure levels over the operating pressure range of the barometer at each temperature level. The instrument can operate over a pressure range of 50 to 1100 hPa and a temperature range of -40 to 60 degC with an accuracy better than 0.1%. More information may be found at http://www.vaisala.com/Vaisala%20Documents/User%20Guides%20and%20Quick%20Ref%20Guides/PTB220_User_Guide_in_English.pdf.</skos:definition>
	<skos:inScheme rdf:resource="http://vocab.aodn.org.au/def/instrument/1"/>
	<skos:prefLabel xml:lang="en">Vaisala PTB220 Digital Barometer</skos:prefLabel>
	<skos:broader rdf:resource="http://vocab.nerc.ac.uk/collection/L05/current/102"/>
	<skos:scopeNote xml:lang="en">manufacturer:Vaisala</skos:scopeNote>
</rdf:Description>

<rdf:Description rdf:about="http://vocab.nerc.ac.uk/collection/L22/current/TOOL0677">
	<rdf:type rdf:resource="http://www.w3.org/2000/01/rdf-schema#Resource"/>
	<rdf:type rdf:resource="http://www.w3.org/2004/02/skos/core#Concept"/>
	<dcterms:created rdf:datatype="http://www.w3.org/2001/XMLSchema#dateTime">2013-10-14T00:00:00Z</dcterms:created>
	<dc:publisher rdf:datatype="http://www.w3.org/2001/XMLSchema#string">British Oceanographic Data Centre (BODC)</dc:publisher>
	<dc:source rdf:datatype="http://www.w3.org/2001/XMLSchema#string">(L221) SeaVoX Device Catalogue</dc:source>
	<skos:definition xml:lang="en">The Vaisala HMT330 is a series of humidity and temperature transmitters comprising a base station and sensors that may be attached directly or on a remote probe suited to the application. The probes are designed for installation in various environments: HMT331 for wall mounting, HMT333 for duct mounting and tight spaces, HMT334 for high pressures up to 100 bar and vacuum conditions, HMT335 for high temperature, HMT337 for high humidity and meteorological applications and HMT338 for pressurized pipelines up to 40 bar. All incorporate a thermistor and the Vaisala HUMICAP humidity sensor giving temperature accurate to 0.2C and humidity accurate to 1%. The base station includes a graphical display giving continuous digital readout and keypad for operation control. Definal upon the options selected data may be logged internally (up 4 years) or transmitted via wired LAN, wireless LAN, USB, RS232 or RS485. More information is available at http://www.vaisala.com/en/products/humidity/Pages/HMT330.aspx.</skos:definition>
	<skos:inScheme rdf:resource="http://vocab.aodn.org.au/def/instrument/1"/>
	<skos:prefLabel xml:lang="en">Vaisala HMT330 temperature and humidity transmitter</skos:prefLabel>
	<skos:broader rdf:resource="http://vocab.nerc.ac.uk/collection/L05/current/102"/>
	<skos:scopeNote xml:lang="en">manufacturer:Vaisala</skos:scopeNote>
</rdf:Description>

<rdf:Description rdf:about="http://vocab.nerc.ac.uk/collection/L22/current/TOOL0680">
	<rdf:type rdf:resource="http://www.w3.org/2000/01/rdf-schema#Resource"/>
	<rdf:type rdf:resource="http://www.w3.org/2004/02/skos/core#Concept"/>
	<dcterms:created rdf:datatype="http://www.w3.org/2001/XMLSchema#dateTime">2013-10-15T00:00:00Z</dcterms:created>
	<dc:publisher rdf:datatype="http://www.w3.org/2001/XMLSchema#string">British Oceanographic Data Centre (BODC)</dc:publisher>
	<dc:source rdf:datatype="http://www.w3.org/2001/XMLSchema#string">(L221) SeaVoX Device Catalogue</dc:source>
	<skos:definition xml:lang="en">The GE Druck RPT350 Resonant Pressure Transducer, uses silicon technology to give high accuracy and stability with low manufacturing costs. It ranges from 35 to 3500 mbar abs.</skos:definition>
	<skos:inScheme rdf:resource="http://vocab.aodn.org.au/def/instrument/1"/>
	<skos:prefLabel xml:lang="en">GE Druck RPT 350 Resonant Pressure Transducer</skos:prefLabel>
	<skos:broader rdf:resource="http://vocab.nerc.ac.uk/collection/L05/current/102"/>
	<skos:broader rdf:resource="http://vocab.nerc.ac.uk/collection/L05/current/111"/>
	<skos:scopeNote xml:lang="en">manufacturer:General Electric Company</skos:scopeNote>
</rdf:Description>

<rdf:Description rdf:about="http://vocab.nerc.ac.uk/collection/L22/current/TOOL0682">
	<rdf:type rdf:resource="http://www.w3.org/2000/01/rdf-schema#Resource"/>
	<rdf:type rdf:resource="http://www.w3.org/2004/02/skos/core#Concept"/>
	<dcterms:created rdf:datatype="http://www.w3.org/2001/XMLSchema#dateTime">2014-06-05T00:00:00Z</dcterms:created>
	<dc:publisher rdf:datatype="http://www.w3.org/2001/XMLSchema#string">British Oceanographic Data Centre (BODC)</dc:publisher>
	<dc:source rdf:datatype="http://www.w3.org/2001/XMLSchema#string">(L221) SeaVoX Device Catalogue</dc:source>
	<skos:definition xml:lang="en">This is a a self-contained weather station measuring wind speed and direction, precipitation , air temperature, humidity and barometric pressure. The station has the following sensors: Vaisala WINDCAP ultrasonic wind sensor measuring average, maximum and minimum windspeed  accurate to the greater of 0.3 m/s or 3% (0-35 m/s range) or 5% (36-60 m/s) range and average, maximum and minimum wind direction to an accuracy of 3 degrees. Default averaging interval is 60 minutes. Vaisala RAINCAP sensor-2 - a piezoelectrical sensor that measures rainfall amount and intensity (rate) to an accuracy of 5% by counting raindrop impacts. Capacitive silicon BAROCAP air pressure sensor. Capacitive ceramic THERMOCAP air temperature sensor. Capacitive thin film polymer HUMICAP 180 humidity sensor. The precipitation and wind sensors may be optionally heated to keep them free from snow and ice. Output is via an RS232 connection. More information may be found at http://www.vaisala.com/Vaisala%20Documents/User%20Guides%20and%20Quick%20Ref%20Guides/WXT510_User_Guide_in_English.pdf.</skos:definition>
	<skos:inScheme rdf:resource="http://vocab.aodn.org.au/def/instrument/1"/>
	<skos:prefLabel xml:lang="en">Vaisala WXT510 weather transmitter</skos:prefLabel>
	<skos:broader rdf:resource="http://vocab.nerc.ac.uk/collection/L05/current/102"/>
</rdf:Description>

<rdf:Description rdf:about="http://vocab.nerc.ac.uk/collection/L22/current/TOOL0683">
	<rdf:type rdf:resource="http://www.w3.org/2000/01/rdf-schema#Resource"/>
	<rdf:type rdf:resource="http://www.w3.org/2004/02/skos/core#Concept"/>
	<dcterms:created rdf:datatype="http://www.w3.org/2001/XMLSchema#dateTime">2014-06-05T00:00:00Z</dcterms:created>
	<dc:publisher rdf:datatype="http://www.w3.org/2001/XMLSchema#string">British Oceanographic Data Centre (BODC)</dc:publisher>
	<dc:source rdf:datatype="http://www.w3.org/2001/XMLSchema#string">(L221) SeaVoX Device Catalogue</dc:source>
	<skos:definition xml:lang="en">This is a a self-contained weather station measuring wind speed and direction, precipitation , air temperature, humidity and barometric pressure. The station has the following sensors: Vaisala WINDCAP ultrasonic wind sensor measuring average, maximum and minimum windspeed  accurate to the 3% at 10 m/s and average, maximum and minimum wind direction to an accuracy of 3 degrees. Default averaging interval is 60 minutes. Vaisala RAINCAP sensor-2 - a piezoelectrical sensor that measures rainfall amount and intensity (rate) to an accuracy of 5% by counting raindrop impacts. Capacitive silicon BAROCAP air pressure sensor giving an accuracy of 0.5 hPa at 0-30C  or 1 hPa at -52-60C. Capacitive ceramic THERMOCAP air temperature sensor giving an accuracy of 0.3C at 20C. Capacitive thin film polymer HUMICAP 180 humidity sensor giving an accuracy of 3% below 90% humidity or 5% above 90% humidity. The precipitation and wind sensors may be optionally heated to keep them free from snow and ice. Output is via USB connection. This is an upgrade of the WXT510 weather transmitter that may be applied to existing units during service by Vaisala. More information may be found at http://www.vaisala.com/en/products/multiweathersensors/Pages/WXT520.aspx.</skos:definition>
	<skos:inScheme rdf:resource="http://vocab.aodn.org.au/def/instrument/1"/>
	<skos:prefLabel xml:lang="en">Vaisala WXT520 weather transmitter</skos:prefLabel>
	<skos:broader rdf:resource="http://vocab.nerc.ac.uk/collection/L05/current/102"/>
</rdf:Description>

<rdf:Description rdf:about="http://vocab.nerc.ac.uk/collection/L22/current/TOOL0726">
	<rdf:type rdf:resource="http://www.w3.org/2000/01/rdf-schema#Resource"/>
	<rdf:type rdf:resource="http://www.w3.org/2004/02/skos/core#Concept"/>
	<dcterms:created rdf:datatype="http://www.w3.org/2001/XMLSchema#dateTime">2013-10-14T00:00:00Z</dcterms:created>
	<dc:publisher rdf:datatype="http://www.w3.org/2001/XMLSchema#string">British Oceanographic Data Centre (BODC)</dc:publisher>
	<dc:source rdf:datatype="http://www.w3.org/2001/XMLSchema#string">(L221) SeaVoX Device Catalogue</dc:source>
	<skos:definition xml:lang="en">The Osi OWI-430 WIVIS is an optical weather and visibility sensor that measures visibility, rain, snow, drizzle, freezing and mixed precipitation conditions. It measures rain in dynamic range 0.1 to 3000 mm/hr; snow in dynamic range 0.01 to 300 mm/hr; visibility in dynamic range 0.001 to 10 km. It is designed to operate in temperatures from -40 to 50 degC, and humidity from 0 to 100 percent.</skos:definition>
	<skos:inScheme rdf:resource="http://vocab.aodn.org.au/def/instrument/1"/>
	<skos:prefLabel xml:lang="en">OSi OWI-430 DSP-WIVIS Present Weather and Visibility Sensor</skos:prefLabel>
	<skos:broader rdf:resource="http://vocab.nerc.ac.uk/collection/L05/current/102"/>
	<skos:scopeNote xml:lang="en">manufacturer:Optical Scientific Inc.</skos:scopeNote>
</rdf:Description>

<rdf:Description rdf:about="http://vocab.nerc.ac.uk/collection/L22/current/TOOL0727">
	<rdf:type rdf:resource="http://www.w3.org/2000/01/rdf-schema#Resource"/>
	<rdf:type rdf:resource="http://www.w3.org/2004/02/skos/core#Concept"/>
	<dcterms:created rdf:datatype="http://www.w3.org/2001/XMLSchema#dateTime">2013-10-15T00:00:00Z</dcterms:created>
	<dc:publisher rdf:datatype="http://www.w3.org/2001/XMLSchema#string">British Oceanographic Data Centre (BODC)</dc:publisher>
	<dc:source rdf:datatype="http://www.w3.org/2001/XMLSchema#string">(L221) SeaVoX Device Catalogue</dc:source>
	<skos:definition xml:lang="en">The Pico Technologies Pt104 is a four-channel temperature measuring data logger. It measures temperatures in the range -200 to 800 degC, with accuracy of 0.015degC plus 0.01% of reading, and resolution of 0.001 degC.</skos:definition>
	<skos:inScheme rdf:resource="http://vocab.aodn.org.au/def/instrument/1"/>
	<skos:prefLabel xml:lang="en">Pico Technologies PT-104 Platinum Resistance Data Logger</skos:prefLabel>
	<skos:broader rdf:resource="http://vocab.nerc.ac.uk/collection/L05/current/102"/>
	<skos:scopeNote xml:lang="en">manufacturer:Pico Technology</skos:scopeNote>
</rdf:Description>

<rdf:Description rdf:about="http://vocab.nerc.ac.uk/collection/L22/current/TOOL0741">
	<rdf:type rdf:resource="http://www.w3.org/2000/01/rdf-schema#Resource"/>
	<rdf:type rdf:resource="http://www.w3.org/2004/02/skos/core#Concept"/>
	<dcterms:created rdf:datatype="http://www.w3.org/2001/XMLSchema#dateTime">2013-10-11T00:00:00Z</dcterms:created>
	<dc:publisher rdf:datatype="http://www.w3.org/2001/XMLSchema#string">British Oceanographic Data Centre (BODC)</dc:publisher>
	<dc:source rdf:datatype="http://www.w3.org/2001/XMLSchema#string">(L221) SeaVoX Device Catalogue</dc:source>
	<skos:definition xml:lang="en">The Vaisala PTU300 is a series of air pressure, humidity and temperature transmitters comprising a base station and sensors that may be attached directly or on a remote probe suited to the application. The probes are designed for installation in various environments: PTU301 for laboratories, PTU303 for general use and PTU307 for outdoor and meteorological applications (warmed probe). All incorporate the Vaisala BAROCAP pressure sensor, a thermistor and the Vaisala HUMICAP humidity sensor giving pressure accurate to 0.1-0.3 hPa (depends upon sensor class), temperature accurate to 0.2C and humidity accurate to 1%. The base station includes a graphical display giving continuous digital readout and keypad for operation control. Depending upon the options selected data may be logged internally (up 4 years) or transmitted via wired LAN, wireless LAN, USB, RS232 or RS485. More information is available at http://www.vaisala.com/Vaisala%20Documents/Brochures%20and%20Datasheets/CEN-TIA-G-PTU300-Combined-Brochure-B210954EN-E-LOW-v6.pdf.</skos:definition>
	<skos:inScheme rdf:resource="http://vocab.aodn.org.au/def/instrument/1"/>
	<skos:prefLabel xml:lang="en">Vaisala PTU300 Pressure, Humidity and Temperature Transmitter</skos:prefLabel>
	<skos:broader rdf:resource="http://vocab.nerc.ac.uk/collection/L05/current/102"/>
	<skos:scopeNote xml:lang="en">manufacturer:Vaisala</skos:scopeNote>
</rdf:Description>

<rdf:Description rdf:about="http://vocab.nerc.ac.uk/collection/L22/current/TOOL0779">
	<rdf:type rdf:resource="http://www.w3.org/2000/01/rdf-schema#Resource"/>
	<rdf:type rdf:resource="http://www.w3.org/2004/02/skos/core#Concept"/>
	<dcterms:created rdf:datatype="http://www.w3.org/2001/XMLSchema#dateTime">2013-10-11T00:00:00Z</dcterms:created>
	<dcterms:modified rdf:datatype="http://www.w3.org/2001/XMLSchema#dateTime">2015-06-02T03:00:09Z</dcterms:modified>
	<dc:publisher rdf:datatype="http://www.w3.org/2001/XMLSchema#string">British Oceanographic Data Centre (BODC)</dc:publisher>
	<dc:source rdf:datatype="http://www.w3.org/2001/XMLSchema#string">(L221) SeaVoX Device Catalogue</dc:source>
	<skos:definition xml:lang="en"></skos:definition>
	<skos:definition xml:lang="en">A digital aneroid barometer with serial communication in use since the late 1980s.</skos:definition>
	<skos:inScheme rdf:resource="http://vocab.aodn.org.au/def/instrument/1"/>
	<skos:prefLabel xml:lang="en">Vaisala DPA21 digital barometer</skos:prefLabel>
	<skos:broader rdf:resource="http://vocab.nerc.ac.uk/collection/L05/current/102"/>
	<skos:scopeNote xml:lang="en">manufacturer:Vaisala</skos:scopeNote>
</rdf:Description>

<rdf:Description rdf:about="http://vocab.nerc.ac.uk/collection/L22/current/TOOL0780">
	<rdf:type rdf:resource="http://www.w3.org/2000/01/rdf-schema#Resource"/>
	<rdf:type rdf:resource="http://www.w3.org/2004/02/skos/core#Concept"/>
	<dcterms:created rdf:datatype="http://www.w3.org/2001/XMLSchema#dateTime">2013-10-11T00:00:00Z</dcterms:created>
	<dc:publisher rdf:datatype="http://www.w3.org/2001/XMLSchema#string">British Oceanographic Data Centre (BODC)</dc:publisher>
	<dc:source rdf:datatype="http://www.w3.org/2001/XMLSchema#string">(L221) SeaVoX Device Catalogue</dc:source>
	<skos:definition xml:lang="en">An aviation quality digital barometer providing accurate and reliable pressure measurement over the range of 800 to 1050 mb.It had a unique construction consisting of three independently operating sensors controlled by a microprocessor. Triple redundancy ensured excellent long-term stability and measurement accuracy. Short term accuracy was determined by WMO as about 0.2 hPa and long-term accuracy (over approximately a year) was determined as approximately 0.35 hPa or 0.45 hPa if subjected to temperature variations in excess of 20C.</skos:definition>
	<skos:inScheme rdf:resource="http://vocab.aodn.org.au/def/instrument/1"/>
	<skos:prefLabel xml:lang="en">Vaisala PA 11 digital barometer</skos:prefLabel>
	<skos:broader rdf:resource="http://vocab.nerc.ac.uk/collection/L05/current/102"/>
	<skos:scopeNote xml:lang="en">manufacturer:Vaisala</skos:scopeNote>
</rdf:Description>

<rdf:Description rdf:about="http://vocab.nerc.ac.uk/collection/L22/current/TOOL0808">
	<rdf:type rdf:resource="http://www.w3.org/2000/01/rdf-schema#Resource"/>
	<rdf:type rdf:resource="http://www.w3.org/2004/02/skos/core#Concept"/>
	<dcterms:created rdf:datatype="http://www.w3.org/2001/XMLSchema#dateTime">2013-10-11T00:00:00Z</dcterms:created>
	<dc:publisher rdf:datatype="http://www.w3.org/2001/XMLSchema#string">British Oceanographic Data Centre (BODC)</dc:publisher>
	<dc:source rdf:datatype="http://www.w3.org/2001/XMLSchema#string">(L221) SeaVoX Device Catalogue</dc:source>
	<skos:definition xml:lang="en">A platinum resistor thermometer with a serial interface primarily used for air temperature measurements in meteorological packages but also used as a shipboard hull thermometer.</skos:definition>
	<skos:inScheme rdf:resource="http://vocab.aodn.org.au/def/instrument/1"/>
	<skos:prefLabel xml:lang="en">Rosemount ST2401 temperature probe</skos:prefLabel>
	<skos:broader rdf:resource="http://vocab.nerc.ac.uk/collection/L05/current/102"/>
	<skos:scopeNote xml:lang="en">manufacturer:Emerson Electric Co.</skos:scopeNote>
</rdf:Description>

<rdf:Description rdf:about="http://vocab.nerc.ac.uk/collection/L22/current/TOOL1015">
	<rdf:type rdf:resource="http://www.w3.org/2000/01/rdf-schema#Resource"/>
	<rdf:type rdf:resource="http://www.w3.org/2004/02/skos/core#Concept"/>
	<dcterms:created rdf:datatype="http://www.w3.org/2001/XMLSchema#dateTime">2017-03-13T00:00:00Z</dcterms:created>
	<dc:publisher rdf:datatype="http://www.w3.org/2001/XMLSchema#string">British Oceanographic Data Centre (BODC)</dc:publisher>
	<skos:definition xml:lang="en">A series of class A and B barometers designed for meteorology, aviation, laboratories and demanding industrial applications. It uses a BAROCAP silicon capacitive absolute pressure sensor developed by Vaisala. The measurement is based on an advanced RC oscillator and reference capacitors against which the capacitive pressure sensor is continuously measured. The microprocessor of the barometer performs compensation for pressure linearity and temperature dependence. It is available with one, two or three modules. Each module has its own adjustment coefficients for different reference pressures across the entire temperature range. It is available with digital (RS-232 or RS-422/485) or analogue output (voltage or current). The instrument can operate over a pressure range of 50 to 1100 hPa or 500 to 1100 hPa and a temperature range of -40 to 60 degC. The best accuracy achieved is +/-0.1 hPa at 20 degC using a class A sensor and +/-0.2 using a class B sensor.</skos:definition>
	<skos:inScheme rdf:resource="http://vocab.aodn.org.au/def/instrument/1"/>
	<skos:prefLabel xml:lang="en">Vaisala PTB330 digital barometer</skos:prefLabel>
	<skos:broader rdf:resource="http://vocab.nerc.ac.uk/collection/L05/current/102"/>
	<skos:altLabel xml:lang="en">PTB 330 barometer</skos:altLabel>
</rdf:Description>

<rdf:Description rdf:about="http://vocab.nerc.ac.uk/collection/L22/current/TOOL0268">
	<rdf:type rdf:resource="http://www.w3.org/2000/01/rdf-schema#Resource"/>
	<rdf:type rdf:resource="http://www.w3.org/2004/02/skos/core#Concept"/>
	<dcterms:created rdf:datatype="http://www.w3.org/2001/XMLSchema#dateTime">2014-02-17T00:00:00Z</dcterms:created>
	<dc:publisher rdf:datatype="http://www.w3.org/2001/XMLSchema#string">British Oceanographic Data Centre (BODC)</dc:publisher>
	<dc:source rdf:datatype="http://www.w3.org/2001/XMLSchema#string">(L221) SeaVoX Device Catalogue</dc:source>
	<skos:definition xml:lang="en">A directional waverider buoy comprising a heave-pitch-roll sensor, two accelerometers and a 3-axis fluxgate compass in a 90cm diameter spherical buoy that measures waves using a translational principle so that horizontal motions rather than wave slopes are measured making the measurement independent of buoy roll motions. A single point rubber cord vertical mooring ensures adequate symmetrical horizontal buoy response to resolve small motions at low frequencies. Data are transmitted to a shore based station and/or an Argos satellite. Three versions of the buoy designated MkI, MkII and MkIII have been produced with evolving internal electronics but fundamentally the same design. More information may be found at http://www.bodc.ac.uk/data/documents/nodb/65329/</skos:definition>
	<skos:inScheme rdf:resource="http://vocab.aodn.org.au/def/instrument/1"/>
	<skos:prefLabel xml:lang="en">Datawell directional waverider buoy</skos:prefLabel>
	<skos:broader rdf:resource="http://vocab.nerc.ac.uk/collection/L05/current/110"/>
	<skos:scopeNote xml:lang="en">manufacturer:Datawell</skos:scopeNote>
</rdf:Description>

<rdf:Description rdf:about="http://vocab.nerc.ac.uk/collection/L22/current/TOOL0696">
	<rdf:type rdf:resource="http://www.w3.org/2000/01/rdf-schema#Resource"/>
	<rdf:type rdf:resource="http://www.w3.org/2004/02/skos/core#Concept"/>
	<dcterms:created rdf:datatype="http://www.w3.org/2001/XMLSchema#dateTime">2013-09-25T00:00:00Z</dcterms:created>
	<dc:publisher rdf:datatype="http://www.w3.org/2001/XMLSchema#string">British Oceanographic Data Centre (BODC)</dc:publisher>
	<dc:source rdf:datatype="http://www.w3.org/2001/XMLSchema#string">(L221) SeaVoX Device Catalogue</dc:source>
	<skos:definition xml:lang="en">The SBE 26 SEAGAUGE is a water level recorder with a Digiquartz pressure sensor, accurate clock, precision thermometer and optional conductivity sensor in a casing able to operate down to 600m. Pressure data are integrated to give sea level or are burst recorded at rates up to 4 Hz to measure characterise waves. The instrument offers improved temperature sensor accuracy (0.01C with 0.001C resolution or optionally 0.001C with 0.0001C resolution), data storage and operational functionality over the SBE-26. More information at http://www.seabird.com/products/spec_sheets/26plusdata.htm.</skos:definition>
	<skos:inScheme rdf:resource="http://vocab.aodn.org.au/def/instrument/1"/>
	<skos:prefLabel xml:lang="en">Sea-Bird SBE 26plus SEAGAUGE Wave and Tide Recorder</skos:prefLabel>
	<skos:broader rdf:resource="http://vocab.nerc.ac.uk/collection/L05/current/110"/>
	<skos:broader rdf:resource="http://vocab.nerc.ac.uk/collection/L05/current/111"/>
	<skos:broader rdf:resource="http://vocab.nerc.ac.uk/collection/L05/current/134"/>
	<skos:scopeNote xml:lang="en">manufacturer:Sea-Bird Electronics Inc.</skos:scopeNote>
</rdf:Description>

<rdf:Description rdf:about="http://vocab.nerc.ac.uk/collection/L22/current/TOOL0710">
	<rdf:type rdf:resource="http://www.w3.org/2000/01/rdf-schema#Resource"/>
	<rdf:type rdf:resource="http://www.w3.org/2004/02/skos/core#Concept"/>
	<dcterms:created rdf:datatype="http://www.w3.org/2001/XMLSchema#dateTime">2014-07-14T00:00:00Z</dcterms:created>
	<dc:publisher rdf:datatype="http://www.w3.org/2001/XMLSchema#string">British Oceanographic Data Centre (BODC)</dc:publisher>
	<dc:source rdf:datatype="http://www.w3.org/2001/XMLSchema#string">(L221) SeaVoX Device Catalogue</dc:source>
	<skos:definition xml:lang="en">A sensor packaged in a small stainless steel box with a single connector for power and data that outputs fully processed wave data. Sampling is in bursts from 1-34 minutes with a sampling interval from 5-1440 minutes. It may be located anywhere on a floating platform and comprises three accelerometers and three rate sensors that measure displacement along the three orthogonal axes of the platform. Direction is measured using a gimballed fluxgate compass. Resolution is 0.01m for height, 0.1 second for period and one degree for direction. Accuracy is better than 2% for height and period and 3 degrees for direction. More information is available in http://axystechnologies.com/wp-content/uploads/2014/01/TRIAXYS-NW-Sensors-Digital-Layout.pdf.</skos:definition>
	<skos:inScheme rdf:resource="http://vocab.aodn.org.au/def/instrument/1"/>
	<skos:prefLabel xml:lang="en">TRIAXYS directional wave sensor</skos:prefLabel>
	<skos:broader rdf:resource="http://vocab.nerc.ac.uk/collection/L05/current/110"/>
</rdf:Description>

<rdf:Description rdf:about="http://vocab.nerc.ac.uk/collection/L22/current/TOOL0729">
	<rdf:type rdf:resource="http://www.w3.org/2000/01/rdf-schema#Resource"/>
	<rdf:type rdf:resource="http://www.w3.org/2004/02/skos/core#Concept"/>
	<dcterms:created rdf:datatype="http://www.w3.org/2001/XMLSchema#dateTime">2014-07-14T00:00:00Z</dcterms:created>
	<dc:publisher rdf:datatype="http://www.w3.org/2001/XMLSchema#string">British Oceanographic Data Centre (BODC)</dc:publisher>
	<dc:source rdf:datatype="http://www.w3.org/2001/XMLSchema#string">(L221) SeaVoX Device Catalogue</dc:source>
	<skos:definition xml:lang="en">The TWR-2050P is a small, self-contained, submersible temperature, wave and depth recorder (sensors and data logger). It can be deployed for a period of up to three years and can collect more than 1,200,000 sets of samples. Data can be retained in memory for 20 years (even without batteries). Available in two casings, plastic and titanium, with depth ratings of 740m and 6600m respectively. The temperature channel of the TWR-2050 is calibrated to an accuracy of ± 0.002°C (ITS-90) over the range -5 to +35°C.  Typical drift has been measured to be 0.002°C per year. The thermistor may be external (&lt;3sec time constant) or internal (&lt;20sec time constant). A fast thermistor probe (0.095sec) is also available. The depth channel is calibrated to an accuracy of 0.05%fs  Ranges from 10m to 6,600m are available. Temperature and depth only sensors (TDR) and surface-mounted sensors (HT) are also available.</skos:definition>
	<skos:inScheme rdf:resource="http://vocab.aodn.org.au/def/instrument/1"/>
	<skos:prefLabel xml:lang="en">RBR TWR-2050 Submersible Tide and Wave Recorder</skos:prefLabel>
	<skos:broader rdf:resource="http://vocab.nerc.ac.uk/collection/L05/current/110"/>
	<skos:broader rdf:resource="http://vocab.nerc.ac.uk/collection/L05/current/111"/>
	<skos:broader rdf:resource="http://vocab.nerc.ac.uk/collection/L05/current/134"/>
</rdf:Description>

<rdf:Description rdf:about="http://vocab.nerc.ac.uk/collection/L22/current/TOOL0733">
	<rdf:type rdf:resource="http://www.w3.org/2000/01/rdf-schema#Resource"/>
	<rdf:type rdf:resource="http://www.w3.org/2004/02/skos/core#Concept"/>
	<dcterms:created rdf:datatype="http://www.w3.org/2001/XMLSchema#dateTime">2014-07-16T00:00:00Z</dcterms:created>
	<dc:publisher rdf:datatype="http://www.w3.org/2001/XMLSchema#string">British Oceanographic Data Centre (BODC)</dc:publisher>
	<dc:source rdf:datatype="http://www.w3.org/2001/XMLSchema#string">(L221) SeaVoX Device Catalogue</dc:source>
	<skos:definition xml:lang="en">A module that may be attached to the Workhorse ADCP Waves Array to process the data and reduce it to a volume that can be transmitted in near real-time. The maximum working depth is 200m.  More information may be found in http://www.rdinstruments.com/datasheets/nemo_ds.pdf.</skos:definition>
	<skos:inScheme rdf:resource="http://vocab.aodn.org.au/def/instrument/1"/>
	<skos:prefLabel xml:lang="en">Teledyne RDI Workhorse NEMO-WHSW600 Waves Processing Array</skos:prefLabel>
	<skos:broader rdf:resource="http://vocab.nerc.ac.uk/collection/L05/current/110"/>
</rdf:Description>

<rdf:Description rdf:about="http://vocab.nerc.ac.uk/collection/L22/current/TOOL0781">
	<rdf:type rdf:resource="http://www.w3.org/2000/01/rdf-schema#Resource"/>
	<rdf:type rdf:resource="http://www.w3.org/2004/02/skos/core#Concept"/>
	<dcterms:created rdf:datatype="http://www.w3.org/2001/XMLSchema#dateTime">2013-03-28T00:00:00Z</dcterms:created>
	<dc:publisher rdf:datatype="http://www.w3.org/2001/XMLSchema#string">British Oceanographic Data Centre (BODC)</dc:publisher>
	<dc:source rdf:datatype="http://www.w3.org/2001/XMLSchema#string">(L221) SeaVoX Device Catalogue</dc:source>
	<skos:definition xml:lang="en">A non-directional waverider system with an accelerometer mounted in a loose tethered buoy (0.7 or 0.9m in diameter) that measures the vertical accelerations of the buoy as it moves with the water surface.  The accelerations are integrated twice within the buoy and the displacement signal so obtained is then transmitted to a shore station where it is processed to provide wave data statistics.</skos:definition>
	<skos:inScheme rdf:resource="http://vocab.aodn.org.au/def/instrument/1"/>
	<skos:prefLabel xml:lang="en">Datawell waverider buoy</skos:prefLabel>
	<skos:broader rdf:resource="http://vocab.nerc.ac.uk/collection/L05/current/110"/>
	<skos:altLabel xml:lang="en">Datawell waverider</skos:altLabel>
</rdf:Description>

<rdf:Description rdf:about="http://vocab.nerc.ac.uk/collection/L22/current/TOOL0169">
	<rdf:type rdf:resource="http://www.w3.org/2000/01/rdf-schema#Resource"/>
	<rdf:type rdf:resource="http://www.w3.org/2004/02/skos/core#Concept"/>
	<dcterms:created rdf:datatype="http://www.w3.org/2001/XMLSchema#dateTime">2013-03-28T00:00:00Z</dcterms:created>
	<dc:publisher rdf:datatype="http://www.w3.org/2001/XMLSchema#string">British Oceanographic Data Centre (BODC)</dc:publisher>
	<dc:source rdf:datatype="http://www.w3.org/2001/XMLSchema#string">(L221) SeaVoX Device Catalogue</dc:source>
	<skos:definition xml:lang="en">The DR-1050 is a pressure recorder with possible ranges of 10, 20, 50, 100, 200, 500, 740, 1000, 2000, 4000, 6000 and 10000 dbar; an accuracy of 0.05% full scale; a resolution of &lt;0.001% full scale; and a time constant of &lt;10 msec.</skos:definition>
	<skos:inScheme rdf:resource="http://vocab.aodn.org.au/def/instrument/1"/>
	<skos:prefLabel xml:lang="en">RBR DR-1050 Depth recorder</skos:prefLabel>
	<skos:broader rdf:resource="http://vocab.nerc.ac.uk/collection/L05/current/111"/>
	<skos:scopeNote xml:lang="en">manufacturer: RBR</skos:scopeNote>
</rdf:Description>

<rdf:Description rdf:about="http://vocab.nerc.ac.uk/collection/L22/current/TOOL0685">
	<rdf:type rdf:resource="http://www.w3.org/2000/01/rdf-schema#Resource"/>
	<rdf:type rdf:resource="http://www.w3.org/2004/02/skos/core#Concept"/>
	<dcterms:created rdf:datatype="http://www.w3.org/2001/XMLSchema#dateTime">2014-06-04T00:00:00Z</dcterms:created>
	<dc:publisher rdf:datatype="http://www.w3.org/2001/XMLSchema#string">British Oceanographic Data Centre (BODC)</dc:publisher>
	<dc:source rdf:datatype="http://www.w3.org/2001/XMLSchema#string">(L221) SeaVoX Device Catalogue</dc:source>
	<skos:definition xml:lang="en">A miniature (200mm long, 32mm diameter) self-contained data logger incorporating a thermistor temperature sensor (resolution better that 0.007C, accuracy 0.05C) and a pressure sensor in a housing designed to operate at depths down to 1000m.  The type of pressure sensor fitted depends upon the maximum operating depth required with resolution and accuracy a function of the full-scale reading. The logger may be programmed to provide a wide variety of sampling regimes, including burst recording. More information may be found in http://www.aquatecgroup.com/images/manual_guides/bg%20-%20520.pdf.</skos:definition>
	<skos:inScheme rdf:resource="http://vocab.aodn.org.au/def/instrument/1"/>
	<skos:prefLabel xml:lang="en">Aquatech AQUAlogger 520PT mini temperature and pressure logger</skos:prefLabel>
	<skos:broader rdf:resource="http://vocab.nerc.ac.uk/collection/L05/current/111"/>
	<skos:broader rdf:resource="http://vocab.nerc.ac.uk/collection/L05/current/134"/>
</rdf:Description>

<rdf:Description rdf:about="http://vocab.nerc.ac.uk/collection/L22/current/TOOL0708">
	<rdf:type rdf:resource="http://www.w3.org/2000/01/rdf-schema#Resource"/>
	<rdf:type rdf:resource="http://www.w3.org/2004/02/skos/core#Concept"/>
	<dcterms:created rdf:datatype="http://www.w3.org/2001/XMLSchema#dateTime">2014-07-11T00:00:00Z</dcterms:created>
	<dc:publisher rdf:datatype="http://www.w3.org/2001/XMLSchema#string">British Oceanographic Data Centre (BODC)</dc:publisher>
	<dc:source rdf:datatype="http://www.w3.org/2001/XMLSchema#string">(L221) SeaVoX Device Catalogue</dc:source>
	<skos:definition xml:lang="en">This is digital pressure transducer with an RS232 or RS485 interface in a stainless steel housing with an accuracy of 0.02% full scale. More information is available at http://www.heise.com/Products/pressure_transducers/upload/Heise-Bul-HTR-4-08-3.pdf.</skos:definition>
	<skos:inScheme rdf:resource="http://vocab.aodn.org.au/def/instrument/1"/>
	<skos:prefLabel xml:lang="en">Heise Model DXD Digital Output Pressure Transducer</skos:prefLabel>
	<skos:broader rdf:resource="http://vocab.nerc.ac.uk/collection/L05/current/111"/>
</rdf:Description>

<rdf:Description rdf:about="http://vocab.nerc.ac.uk/collection/L22/current/TOOL0731">
	<rdf:type rdf:resource="http://www.w3.org/2000/01/rdf-schema#Resource"/>
	<rdf:type rdf:resource="http://www.w3.org/2004/02/skos/core#Concept"/>
	<dcterms:created rdf:datatype="http://www.w3.org/2001/XMLSchema#dateTime">2014-07-14T00:00:00Z</dcterms:created>
	<dc:publisher rdf:datatype="http://www.w3.org/2001/XMLSchema#string">British Oceanographic Data Centre (BODC)</dc:publisher>
	<dc:source rdf:datatype="http://www.w3.org/2001/XMLSchema#string">(L221) SeaVoX Device Catalogue</dc:source>
	<skos:definition xml:lang="en">The ReefNet Sensus Ultra is a compact temperature and depth logging sensor designed for use as a dive computer. Depths between 0 and 500 feet are measured with precision better than 0.5 inches of water, and accuracy of +/-12 inches. Temperature is measured between -20 degC and + 40 degC, with precision of 0.01 degC, and accuracy of +/-0.8 degC. Sampling interval is configurable from 1 second to over 18 hours, with storage capacity of one year at 60 second sampling resolution.</skos:definition>
	<skos:inScheme rdf:resource="http://vocab.aodn.org.au/def/instrument/1"/>
	<skos:prefLabel xml:lang="en">ReefNet Sensus Ultra</skos:prefLabel>
	<skos:broader rdf:resource="http://vocab.nerc.ac.uk/collection/L05/current/111"/>
	<skos:broader rdf:resource="http://vocab.nerc.ac.uk/collection/L05/current/134"/>
</rdf:Description>

<rdf:Description rdf:about="http://vocab.nerc.ac.uk/collection/L22/current/TOOL0809">
	<rdf:type rdf:resource="http://www.w3.org/2000/01/rdf-schema#Resource"/>
	<rdf:type rdf:resource="http://www.w3.org/2004/02/skos/core#Concept"/>
	<dcterms:contributor rdf:resource="http://editor.vocabs.ands.org.au/user/Natalia_Atkins"/>
	<dcterms:created rdf:datatype="http://www.w3.org/2001/XMLSchema#dateTime">2013-03-28T00:00:00Z</dcterms:created>
	<dcterms:modified rdf:datatype="http://www.w3.org/2001/XMLSchema#dateTime">2015-07-07T04:49:53Z</dcterms:modified>
	<dc:publisher rdf:datatype="http://www.w3.org/2001/XMLSchema#string">British Oceanographic Data Centre (BODC)</dc:publisher>
	<dc:source rdf:datatype="http://www.w3.org/2001/XMLSchema#string">(L221) SeaVoX Device Catalogue</dc:source>
	<skos:definition xml:lang="en">A small (265mm x 38mm OD) self-contained, submersible temperature and pressure logger designed to monitor tide levels without interference from wave action by averaging pressure data sampled at 4 Hz. This operating mode differentiates it from the similar TDR-2050. Temperature channel is calibrated to ±0.002C. Depth channel is calibrated to an accuracy of ±0.05% full scale.</skos:definition>
	<skos:inScheme rdf:resource="http://vocab.aodn.org.au/def/instrument/1"/>
	<skos:prefLabel xml:lang="en">RBR TGR-2050 submersible tide gauge</skos:prefLabel>
	<skos:broader rdf:resource="http://vocab.nerc.ac.uk/collection/L05/current/111"/>
	<skos:broader rdf:resource="http://vocab.nerc.ac.uk/collection/L05/current/134"/>
	<skos:altLabel xml:lang="en">RBR TGR-2050 TG</skos:altLabel>
</rdf:Description>

<rdf:Description rdf:about="http://vocab.nerc.ac.uk/collection/L22/current/TOOL0075">
	<rdf:type rdf:resource="http://www.w3.org/2000/01/rdf-schema#Resource"/>
	<rdf:type rdf:resource="http://www.w3.org/2004/02/skos/core#Concept"/>
	<dcterms:created rdf:datatype="http://www.w3.org/2001/XMLSchema#dateTime">2017-03-13T00:00:00Z</dcterms:created>
	<dc:publisher rdf:datatype="http://www.w3.org/2001/XMLSchema#string">British Oceanographic Data Centre (BODC)</dc:publisher>
	<skos:definition xml:lang="en">Submersible fluorometer designed for through-flow or pumped CTD applications manufactured by WetLabs and which can be configured for various types of fluorescence. The probe has a temperature range of 0-30°C and a depth rating of 600m.</skos:definition>
	<skos:inScheme rdf:resource="http://vocab.aodn.org.au/def/instrument/1"/>
	<skos:prefLabel xml:lang="en">WETLabs WETStar fluorometer</skos:prefLabel>
	<skos:broader rdf:resource="http://vocab.nerc.ac.uk/collection/L05/current/113"/>
	<skos:altLabel xml:lang="en">WETStar fluorometer</skos:altLabel>
</rdf:Description>

<rdf:Description rdf:about="http://vocab.nerc.ac.uk/collection/L22/current/TOOL0720">
	<rdf:type rdf:resource="http://www.w3.org/2000/01/rdf-schema#Resource"/>
	<rdf:type rdf:resource="http://www.w3.org/2004/02/skos/core#Concept"/>
	<dcterms:created rdf:datatype="http://www.w3.org/2001/XMLSchema#dateTime">2013-10-10T00:00:00Z</dcterms:created>
	<dc:publisher rdf:datatype="http://www.w3.org/2001/XMLSchema#string">British Oceanographic Data Centre (BODC)</dc:publisher>
	<dc:source rdf:datatype="http://www.w3.org/2001/XMLSchema#string">(L221) SeaVoX Device Catalogue</dc:source>
	<skos:definition xml:lang="en">A package comprising a Valeport CTD sensor head plus a customised Turner Cyclops-7 fluorometer combined with an RF unit and antenna suitable for transmission of data via the Argos satellite system. The unit contains an internal battery and a microprocessor that logs data and schedules the transfer of data. The package is designed for attachment to marine mammals and has an operational depth range of down to 2000 m. CTD accuracy is 0.005 C (temperature), 0.01 mS/cm (conductivity) and 2 dBar (pressure).  It is built and calibrated at Valeport Ltd, while SMRU Ltd, the commercial arm of the Sea Mammal Research Unit of the University of St Andrews, is responsible for its distribution, and for streaming and processing the data. More information is available at http://www.smru.st-and.ac.uk/Instrumentation/FluorometryTag/.</skos:definition>
	<skos:inScheme rdf:resource="http://vocab.aodn.org.au/def/instrument/1"/>
	<skos:prefLabel xml:lang="en">SMRU Ltd CTD/Fluorometer Satellite Relay Data Logger</skos:prefLabel>
	<skos:broader rdf:resource="http://vocab.nerc.ac.uk/collection/L05/current/113"/>
	<skos:broader rdf:resource="http://vocab.nerc.ac.uk/collection/L05/current/130"/>
	<skos:broader rdf:resource="http://vocab.nerc.ac.uk/collection/L05/current/134"/>
	<skos:broader rdf:resource="http://vocab.nerc.ac.uk/collection/L05/current/350"/>
	<skos:broader rdf:resource="http://vocab.nerc.ac.uk/collection/L05/current/POS17"/>
	<skos:scopeNote xml:lang="en">manufacturer:SMRU Instrumentation</skos:scopeNote>
</rdf:Description>

<rdf:Description rdf:about="http://vocab.nerc.ac.uk/collection/L22/current/TOOL0089">
	<rdf:type rdf:resource="http://www.w3.org/2000/01/rdf-schema#Resource"/>
	<rdf:type rdf:resource="http://www.w3.org/2004/02/skos/core#Concept"/>
	<dcterms:created rdf:datatype="http://www.w3.org/2001/XMLSchema#dateTime">2013-03-28T00:00:00Z</dcterms:created>
	<dc:publisher rdf:datatype="http://www.w3.org/2001/XMLSchema#string">British Oceanographic Data Centre (BODC)</dc:publisher>
	<dc:source rdf:datatype="http://www.w3.org/2001/XMLSchema#string">(L221) SeaVoX Device Catalogue</dc:source>
	<skos:definition xml:lang="en">The Aquadopp is a single-depth doppler current meter designed both for real time data collection and self contained deployments logging internally. It comes with compass, tilt, pressure and temperature sensors. It can also be configured to measure surface wave height, period and direction concurrently. It has the unique feature of being run in diagnostic mode when set to collect data at 1 Hz frequency in user specified intervals. This allows studies of mooring motion and the performance of other current meters to be conducted. It can be set in various configurations with titanium housings for deployment at greater depths.</skos:definition>
	<skos:inScheme rdf:resource="http://vocab.aodn.org.au/def/instrument/1"/>
	<skos:prefLabel xml:lang="en">Nortek Aquadopp 3D doppler current meter</skos:prefLabel>
	<skos:broader rdf:resource="http://vocab.nerc.ac.uk/collection/L05/current/114"/>
	<skos:scopeNote xml:lang="en">manufacturer:Nortek</skos:scopeNote>
</rdf:Description>

<rdf:Description rdf:about="http://vocab.nerc.ac.uk/collection/L22/current/TOOL0121">
	<rdf:type rdf:resource="http://www.w3.org/2000/01/rdf-schema#Resource"/>
	<rdf:type rdf:resource="http://www.w3.org/2004/02/skos/core#Concept"/>
	<dcterms:created rdf:datatype="http://www.w3.org/2001/XMLSchema#dateTime">2014-04-01T00:00:00Z</dcterms:created>
	<dc:publisher rdf:datatype="http://www.w3.org/2001/XMLSchema#string">British Oceanographic Data Centre (BODC)</dc:publisher>
	<dc:source rdf:datatype="http://www.w3.org/2001/XMLSchema#string">(L221) SeaVoX Device Catalogue</dc:source>
	<skos:definition xml:lang="en">Family of self-recording paddle wheel current meters with different pressure cases that record the vector averaged speed and direction over a sampling interval. The paddle wheel rotor is magnetically coupled to an electronic counter. The meter has a balanced weight vane which aligns it with the current flow. For more details see http://www.bodc.ac.uk/data/documents/nodb/65611/.</skos:definition>
	<skos:inScheme rdf:resource="http://vocab.aodn.org.au/def/instrument/1"/>
	<skos:prefLabel xml:lang="en">Aanderaa RCM 7/8 Recording Current Meter</skos:prefLabel>
	<skos:broader rdf:resource="http://vocab.nerc.ac.uk/collection/L05/current/114"/>
	<skos:scopeNote xml:lang="en">manufacturer:Aanderaa Data Instruments</skos:scopeNote>
</rdf:Description>

<rdf:Description rdf:about="http://vocab.nerc.ac.uk/collection/L22/current/TOOL0476">
	<rdf:type rdf:resource="http://www.w3.org/2000/01/rdf-schema#Resource"/>
	<rdf:type rdf:resource="http://www.w3.org/2004/02/skos/core#Concept"/>
	<dcterms:created rdf:datatype="http://www.w3.org/2001/XMLSchema#dateTime">2013-03-28T00:00:00Z</dcterms:created>
	<dc:publisher rdf:datatype="http://www.w3.org/2001/XMLSchema#string">British Oceanographic Data Centre (BODC)</dc:publisher>
	<dc:source rdf:datatype="http://www.w3.org/2001/XMLSchema#string">(L221) SeaVoX Device Catalogue</dc:source>
	<skos:definition xml:lang="en">The Nortek Aquadopp 3000 is a single-depth doppler current meter designed for deployment in intermediate water depths down to 3000 m. It is suitable for use on moorings or fixed structures. It features higher power and an increased signal-to-noise ratio compared with the standard (300 m depth rated) Aquadopp so that it can provide accurate current measurements in water with low concentrations of suspended particulate matter. Current velocity is derived from the Doppler shift measured by two or three 2MHz acoustic beams. It comes with compass, tilt, pressure and temperature sensors. Data are stored on an internal data logger. It can be run in diagnostic mode when set to collect data at 1 Hz frequency in user specified intervals, which allows studies of mooring motion and the performance of other current meters to be conducted.</skos:definition>
	<skos:inScheme rdf:resource="http://vocab.aodn.org.au/def/instrument/1"/>
	<skos:prefLabel xml:lang="en">Nortek Aquadopp 3000 3D doppler current meter</skos:prefLabel>
	<skos:broader rdf:resource="http://vocab.nerc.ac.uk/collection/L05/current/114"/>
	<skos:scopeNote xml:lang="en">manufacturer:Nortek</skos:scopeNote>
</rdf:Description>

<rdf:Description rdf:about="http://vocab.nerc.ac.uk/collection/L22/current/TOOL0477">
	<rdf:type rdf:resource="http://www.w3.org/2000/01/rdf-schema#Resource"/>
	<rdf:type rdf:resource="http://www.w3.org/2004/02/skos/core#Concept"/>
	<dcterms:created rdf:datatype="http://www.w3.org/2001/XMLSchema#dateTime">2013-03-28T00:00:00Z</dcterms:created>
	<dc:publisher rdf:datatype="http://www.w3.org/2001/XMLSchema#string">British Oceanographic Data Centre (BODC)</dc:publisher>
	<dc:source rdf:datatype="http://www.w3.org/2001/XMLSchema#string">(L221) SeaVoX Device Catalogue</dc:source>
	<skos:definition xml:lang="en">The Nortek Aquadopp 6000 is a single-depth doppler current meter designed for deployment on deep water moorings, although it is also suitable for attachment to fixed structures. It features higher power and an increased signal-to-noise ratio compared with the standard (300 m depth rated) Aquadopp so that it can provide accurate current measurements in water with low concentrations of suspended particulate matter. Current velocity is derived from the Doppler shift measured by two or three 2MHz acoustic beams. It comes with compass, tilt, pressure and temperature sensors. It has a titanium casing rated to 6000 m and data are stored on an internal logger. It can be run in diagnostic mode when set to collect data at 1 Hz frequency in user specified intervals, which allows studies of mooring motion and the performance of other current meters to be conducted.</skos:definition>
	<skos:inScheme rdf:resource="http://vocab.aodn.org.au/def/instrument/1"/>
	<skos:prefLabel xml:lang="en">Nortek Aquadopp 6000 3D doppler current meter</skos:prefLabel>
	<skos:broader rdf:resource="http://vocab.nerc.ac.uk/collection/L05/current/114"/>
	<skos:scopeNote xml:lang="en">manufacturer:Nortek</skos:scopeNote>
</rdf:Description>

<rdf:Description rdf:about="http://vocab.nerc.ac.uk/collection/L22/current/TOOL0056">
	<rdf:type rdf:resource="http://www.w3.org/2000/01/rdf-schema#Resource"/>
	<rdf:type rdf:resource="http://www.w3.org/2004/02/skos/core#Concept"/>
	<dcterms:created rdf:datatype="http://www.w3.org/2001/XMLSchema#dateTime">2013-03-28T00:00:00Z</dcterms:created>
	<dc:publisher rdf:datatype="http://www.w3.org/2001/XMLSchema#string">British Oceanographic Data Centre (BODC)</dc:publisher>
	<dc:source rdf:datatype="http://www.w3.org/2001/XMLSchema#string">(L221) SeaVoX Device Catalogue</dc:source>
	<skos:definition xml:lang="en">The Teledyne RDI Workhorse Long-Ranger acoustic doppler current profiler is a long-range and long-term self contained ADCP. It has a patented broadband signal (75 kHz) and a standard depth rating of 1500m. It operates effectively between temperatures of -5 DegC and 45 DegC and has a velocity accuracy of plus or minus 1%; plus or minus 5 mm per s</skos:definition>
	<skos:inScheme rdf:resource="http://vocab.aodn.org.au/def/instrument/1"/>
	<skos:prefLabel xml:lang="en">Teledyne RDI Workhorse Long-Ranger ADCP</skos:prefLabel>
	<skos:broader rdf:resource="http://vocab.nerc.ac.uk/collection/L05/current/115"/>
	<skos:scopeNote xml:lang="en">manufacturer:Teledyne RD Instruments</skos:scopeNote>
</rdf:Description>

<rdf:Description rdf:about="http://vocab.nerc.ac.uk/collection/L22/current/TOOL0293">
	<rdf:type rdf:resource="http://www.w3.org/2000/01/rdf-schema#Resource"/>
	<rdf:type rdf:resource="http://www.w3.org/2004/02/skos/core#Concept"/>
	<dcterms:created rdf:datatype="http://www.w3.org/2001/XMLSchema#dateTime">2013-03-28T00:00:00Z</dcterms:created>
	<dc:publisher rdf:datatype="http://www.w3.org/2001/XMLSchema#string">British Oceanographic Data Centre (BODC)</dc:publisher>
	<dc:source rdf:datatype="http://www.w3.org/2001/XMLSchema#string">(L221) SeaVoX Device Catalogue</dc:source>
	<skos:definition xml:lang="en">An ADCP designed for self-contained use on moorings or vessel mounting. It has a patented 1200 kHz broadband signal and a standard depth rating of 200 metres. It operates effectively between temperatures of -5 to 45 DegC and a range of up to 20m with a depth cell size of 2m. Velocity accuracy is plus or minus  0.3% or 0.3 cm/sec.</skos:definition>
	<skos:inScheme rdf:resource="http://vocab.aodn.org.au/def/instrument/1"/>
	<skos:prefLabel xml:lang="en">Teledyne RDI Workhorse Sentinel-1200 ADCP</skos:prefLabel>
	<skos:broader rdf:resource="http://vocab.nerc.ac.uk/collection/L05/current/115"/>
	<skos:scopeNote xml:lang="en">manufacturer:Teledyne RD Instruments</skos:scopeNote>
</rdf:Description>

<rdf:Description rdf:about="http://vocab.nerc.ac.uk/collection/L22/current/TOOL0294">
	<rdf:type rdf:resource="http://www.w3.org/2000/01/rdf-schema#Resource"/>
	<rdf:type rdf:resource="http://www.w3.org/2004/02/skos/core#Concept"/>
	<dcterms:created rdf:datatype="http://www.w3.org/2001/XMLSchema#dateTime">2013-03-28T00:00:00Z</dcterms:created>
	<dc:publisher rdf:datatype="http://www.w3.org/2001/XMLSchema#string">British Oceanographic Data Centre (BODC)</dc:publisher>
	<dc:source rdf:datatype="http://www.w3.org/2001/XMLSchema#string">(L221) SeaVoX Device Catalogue</dc:source>
	<skos:definition xml:lang="en">An ADCP designed for self-contained use on moorings or vessel mounting. It has a patented 600 kHz broadband signal and a standard depth rating of 200 metres. It operates effectively between temperatures of -5 to 45 DegC and a range of up to 70m with a depth cell size of 4m.Velocity accuracy is plus or minus 0.3% or 0.3 cm/sec.</skos:definition>
	<skos:inScheme rdf:resource="http://vocab.aodn.org.au/def/instrument/1"/>
	<skos:prefLabel xml:lang="en">Teledyne RDI Workhorse Sentinel-600 ADCP</skos:prefLabel>
	<skos:broader rdf:resource="http://vocab.nerc.ac.uk/collection/L05/current/115"/>
	<skos:scopeNote xml:lang="en">manufacturer:Teledyne RD Instruments</skos:scopeNote>
</rdf:Description>

<rdf:Description rdf:about="http://vocab.nerc.ac.uk/collection/L22/current/TOOL0295">
	<rdf:type rdf:resource="http://www.w3.org/2000/01/rdf-schema#Resource"/>
	<rdf:type rdf:resource="http://www.w3.org/2004/02/skos/core#Concept"/>
	<dcterms:created rdf:datatype="http://www.w3.org/2001/XMLSchema#dateTime">2013-03-28T00:00:00Z</dcterms:created>
	<dc:publisher rdf:datatype="http://www.w3.org/2001/XMLSchema#string">British Oceanographic Data Centre (BODC)</dc:publisher>
	<dc:source rdf:datatype="http://www.w3.org/2001/XMLSchema#string">(L221) SeaVoX Device Catalogue</dc:source>
	<skos:definition xml:lang="en">An ADCP designed for self-contained use on moorings or vessel mounting. It has a patented 300 kHz broadband signal and a standard depth rating of 200 metres. It operates effectively between temperatures of -5 to 45 DegC and a range of up to 165m with a depth cell size of 8m. Velocity accuracy is plus or minus 0.5% or 0.5 cm/sec.</skos:definition>
	<skos:inScheme rdf:resource="http://vocab.aodn.org.au/def/instrument/1"/>
	<skos:prefLabel xml:lang="en">Teledyne RDI Workhorse Sentinel-300 ADCP</skos:prefLabel>
	<skos:broader rdf:resource="http://vocab.nerc.ac.uk/collection/L05/current/115"/>
	<skos:scopeNote xml:lang="en">manufacturer:Teledyne RD Instruments</skos:scopeNote>
</rdf:Description>

<rdf:Description rdf:about="http://vocab.nerc.ac.uk/collection/L22/current/TOOL0445">
	<rdf:type rdf:resource="http://www.w3.org/2000/01/rdf-schema#Resource"/>
	<rdf:type rdf:resource="http://www.w3.org/2004/02/skos/core#Concept"/>
	<dcterms:created rdf:datatype="http://www.w3.org/2001/XMLSchema#dateTime">2014-02-06T00:00:00Z</dcterms:created>
	<dc:publisher rdf:datatype="http://www.w3.org/2001/XMLSchema#string">British Oceanographic Data Centre (BODC)</dc:publisher>
	<dc:source rdf:datatype="http://www.w3.org/2001/XMLSchema#string">(L221) SeaVoX Device Catalogue</dc:source>
	<skos:definition xml:lang="en">The RDI Broadband ADCP is designed for mooring deployment and has an operating frequency of 150 kHz. The instrument uses Doppler-technology to achieve accurate and non-intrusive measurements and it can come with pressure and temperature sensors. It can be used in real time measurement situations or can log to an internal recorder powered by internal batteries.</skos:definition>
	<skos:inScheme rdf:resource="http://vocab.aodn.org.au/def/instrument/1"/>
	<skos:prefLabel xml:lang="en">Teledyne RDI Broadband 150kHz ADCP</skos:prefLabel>
	<skos:broader rdf:resource="http://vocab.nerc.ac.uk/collection/L05/current/115"/>
	<skos:scopeNote xml:lang="en">manufacturer:Teledyne RD Instruments</skos:scopeNote>
</rdf:Description>

<rdf:Description rdf:about="http://vocab.nerc.ac.uk/collection/L22/current/TOOL0732">
	<rdf:type rdf:resource="http://www.w3.org/2000/01/rdf-schema#Resource"/>
	<rdf:type rdf:resource="http://www.w3.org/2004/02/skos/core#Concept"/>
	<dcterms:created rdf:datatype="http://www.w3.org/2001/XMLSchema#dateTime">2014-07-16T00:00:00Z</dcterms:created>
	<dc:publisher rdf:datatype="http://www.w3.org/2001/XMLSchema#string">British Oceanographic Data Centre (BODC)</dc:publisher>
	<dc:source rdf:datatype="http://www.w3.org/2001/XMLSchema#string">(L221) SeaVoX Device Catalogue</dc:source>
	<skos:definition xml:lang="en">A 4-beam 150 KHz instrument designed for moored instrument applications at depths down to 1500m as standard or 3000m and 600m as options. Effective measurement range is 300m with up to 255 bins each 2-24m deep. Velocity accuracy is the greater of 1% or 0.5 cm/s.  More information is available at http://www.rdinstruments.com/datasheets/quartermaster_ds.pdf.</skos:definition>
	<skos:inScheme rdf:resource="http://vocab.aodn.org.au/def/instrument/1"/>
	<skos:prefLabel xml:lang="en">Teledyne RDI Workhorse Quartermaster 150kHz ADCP</skos:prefLabel>
	<skos:broader rdf:resource="http://vocab.nerc.ac.uk/collection/L05/current/115"/>
</rdf:Description>

<rdf:Description rdf:about="http://vocab.nerc.ac.uk/collection/L22/current/TOOL1009">
	<rdf:type rdf:resource="http://www.w3.org/2000/01/rdf-schema#Resource"/>
	<rdf:type rdf:resource="http://www.w3.org/2004/02/skos/core#Concept"/>
	<dcterms:contributor rdf:resource="http://editor.vocabs.ands.org.au/user/eMII_Atkins.Natalia"/>
	<dcterms:created rdf:datatype="http://www.w3.org/2001/XMLSchema#dateTime">2017-03-13T00:00:00Z</dcterms:created>
	<dcterms:modified rdf:datatype="http://www.w3.org/2001/XMLSchema#dateTime">2017-03-23T04:40:23Z</dcterms:modified>
	<dc:publisher rdf:datatype="http://www.w3.org/2001/XMLSchema#string">British Oceanographic Data Centre (BODC)</dc:publisher>
	<skos:definition xml:lang="en">An Acoustic Doppler Current Profiler (ADCP) for use in turbulence studies. It consists of five acoustic transducers, four slanted at 25 degrees from vertical, and a fifth vertical beam. All beams operate at the same frequency of 1 MHz. The instrument has integrated pressure and temperature sensors.</skos:definition>
	<skos:inScheme rdf:resource="http://vocab.aodn.org.au/def/instrument/1"/>
	<skos:prefLabel xml:lang="en">Nortek Signature1000 Acoustic Doppler Current Profiler</skos:prefLabel>
	<skos:broader rdf:resource="http://vocab.nerc.ac.uk/collection/L05/current/115"/>
	<skos:broader rdf:resource="http://vocab.nerc.ac.uk/collection/L05/current/134"/>
	<skos:broader rdf:resource="http://vocab.nerc.ac.uk/collection/L05/current/WPS"/>
	<skos:altLabel xml:lang="en">Nortek Signature1000 ADCP</skos:altLabel>
</rdf:Description>

<rdf:Description rdf:about="http://vocab.nerc.ac.uk/collection/L22/current/TOOL1010">
	<rdf:type rdf:resource="http://www.w3.org/2000/01/rdf-schema#Resource"/>
	<rdf:type rdf:resource="http://www.w3.org/2004/02/skos/core#Concept"/>
	<dcterms:contributor rdf:resource="http://editor.vocabs.ands.org.au/user/eMII_Atkins.Natalia"/>
	<dcterms:created rdf:datatype="http://www.w3.org/2001/XMLSchema#dateTime">2017-03-13T00:00:00Z</dcterms:created>
	<dcterms:modified rdf:datatype="http://www.w3.org/2001/XMLSchema#dateTime">2017-03-22T04:32:54Z</dcterms:modified>
	<dc:publisher rdf:datatype="http://www.w3.org/2001/XMLSchema#string">British Oceanographic Data Centre (BODC)</dc:publisher>
	<skos:definition xml:lang="en">An Acoustic Doppler Current Profiler (ADCP) for use in turbulence studies. It consists of five acoustic transducers, four slanted at 25 degrees from vertical, and a fifth vertical beam. All beams operate at the same frequency of 500 kHz. The instrument has integrated pressure and temperature sensors.</skos:definition>
	<skos:inScheme rdf:resource="http://vocab.aodn.org.au/def/instrument/1"/>
	<skos:prefLabel xml:lang="en">Nortek Signature500 Acoustic Doppler Current Profiler</skos:prefLabel>
	<skos:broader rdf:resource="http://vocab.nerc.ac.uk/collection/L05/current/115"/>
	<skos:broader rdf:resource="http://vocab.nerc.ac.uk/collection/L05/current/134"/>
	<skos:broader rdf:resource="http://vocab.nerc.ac.uk/collection/L05/current/WPS"/>
	<skos:altLabel xml:lang="en">Nortek Signature500 ADCP</skos:altLabel>
</rdf:Description>

<rdf:Description rdf:about="http://vocab.nerc.ac.uk/collection/L22/current/TOOL0083">
	<rdf:type rdf:resource="http://www.w3.org/2000/01/rdf-schema#Resource"/>
	<rdf:type rdf:resource="http://www.w3.org/2004/02/skos/core#Concept"/>
	<dcterms:created rdf:datatype="http://www.w3.org/2001/XMLSchema#dateTime">2013-10-15T00:00:00Z</dcterms:created>
	<dc:publisher rdf:datatype="http://www.w3.org/2001/XMLSchema#string">British Oceanographic Data Centre (BODC)</dc:publisher>
	<dc:source rdf:datatype="http://www.w3.org/2001/XMLSchema#string">(L221) SeaVoX Device Catalogue</dc:source>
	<skos:definition xml:lang="en">The Eppley Precision Infrared Radiometer (PIR) pyrgyometer measures longwave (infrared) radiation. It is housed in a weatherproof titanium canister that has been painted with a very flat black paint that absorbs radiation. A small glass dome at the top of the instrument is covered with an 'interference coating' which allows only infrared radiation to come through. Light levels are detected as temperature changes creating voltages in fine wire coil detectors.</skos:definition>
	<skos:inScheme rdf:resource="http://vocab.aodn.org.au/def/instrument/1"/>
	<skos:prefLabel xml:lang="en">Eppley Precision Infrared Radiometer Pyrgyometer</skos:prefLabel>
	<skos:broader rdf:resource="http://vocab.nerc.ac.uk/collection/L05/current/122"/>
	<skos:scopeNote xml:lang="en">manufacturer:The Eppley Laboratory Inc.</skos:scopeNote>
</rdf:Description>

<rdf:Description rdf:about="http://vocab.nerc.ac.uk/collection/L22/current/TOOL0120">
	<rdf:type rdf:resource="http://www.w3.org/2000/01/rdf-schema#Resource"/>
	<rdf:type rdf:resource="http://www.w3.org/2004/02/skos/core#Concept"/>
	<dcterms:created rdf:datatype="http://www.w3.org/2001/XMLSchema#dateTime">2013-10-15T00:00:00Z</dcterms:created>
	<dc:publisher rdf:datatype="http://www.w3.org/2001/XMLSchema#string">British Oceanographic Data Centre (BODC)</dc:publisher>
	<dc:source rdf:datatype="http://www.w3.org/2001/XMLSchema#string">(L221) SeaVoX Device Catalogue</dc:source>
	<skos:definition xml:lang="en">An underwater or atmospheric quantum sensor with cosine correction that can operate down to 560m. Fitted with a blue-enhanced silicon photovoltaic detector.</skos:definition>
	<skos:inScheme rdf:resource="http://vocab.aodn.org.au/def/instrument/1"/>
	<skos:prefLabel xml:lang="en">LI-COR LI-192 PAR sensor</skos:prefLabel>
	<skos:broader rdf:resource="http://vocab.nerc.ac.uk/collection/L05/current/122"/>
	<skos:scopeNote xml:lang="en">manufacturer:LI-COR Incorporated</skos:scopeNote>
</rdf:Description>

<rdf:Description rdf:about="http://vocab.nerc.ac.uk/collection/L22/current/TOOL0193">
	<rdf:type rdf:resource="http://www.w3.org/2000/01/rdf-schema#Resource"/>
	<rdf:type rdf:resource="http://www.w3.org/2004/02/skos/core#Concept"/>
	<dcterms:created rdf:datatype="http://www.w3.org/2001/XMLSchema#dateTime">2013-10-15T00:00:00Z</dcterms:created>
	<dc:publisher rdf:datatype="http://www.w3.org/2001/XMLSchema#string">British Oceanographic Data Centre (BODC)</dc:publisher>
	<dc:source rdf:datatype="http://www.w3.org/2001/XMLSchema#string">(L221) SeaVoX Device Catalogue</dc:source>
	<skos:definition xml:lang="en">A non-submersible cosine-corrected PAR sensor sensitive wavelengths from 400-700nm with sharp cut-off due to an interference filter. It may be used as a reference sensor for LI-192 and LI-193 Underwater Quantum Sensor.</skos:definition>
	<skos:inScheme rdf:resource="http://vocab.aodn.org.au/def/instrument/1"/>
	<skos:prefLabel xml:lang="en">LI-COR LI-190 PAR sensor</skos:prefLabel>
	<skos:broader rdf:resource="http://vocab.nerc.ac.uk/collection/L05/current/122"/>
	<skos:scopeNote xml:lang="en">manufacturer:LI-COR Incorporated</skos:scopeNote>
</rdf:Description>

<rdf:Description rdf:about="http://vocab.nerc.ac.uk/collection/L22/current/TOOL0625">
	<rdf:type rdf:resource="http://www.w3.org/2000/01/rdf-schema#Resource"/>
	<rdf:type rdf:resource="http://www.w3.org/2004/02/skos/core#Concept"/>
	<dcterms:created rdf:datatype="http://www.w3.org/2001/XMLSchema#dateTime">2013-09-09T00:00:00Z</dcterms:created>
	<dc:publisher rdf:datatype="http://www.w3.org/2001/XMLSchema#string">British Oceanographic Data Centre (BODC)</dc:publisher>
	<dc:source rdf:datatype="http://www.w3.org/2001/XMLSchema#string">(L221) SeaVoX Device Catalogue</dc:source>
	<skos:definition xml:lang="en">In 2010, Satlantic joined Sea-Bird Electronics and WET Labs Inc. to form Sea-Bird Scientific. Within Sea-Bird Scientific, Satlantic works closely with Sea-Bird and WET Labs to design integrated physical and biogeochemical sensors for the global scientific community. The OCR-500 Series Radiometers are fully digital optical sensors that combine precision optics and high performance microelectronics.  The radiometers may be operated as a stand-alone device or in a networked environment as part of a larger system.  These units are available in four (this model) or seven channel discrete wavelengths.     Features: Irradiance and Radiance sensors for in-water and in-air applications, Standard wavelengths from 400 - 865 nm, UV wavelengths available 305, 325, 340 &amp; 380 nm, Fully characterized cosine response, Custom low fluorescence filters,  Networking capability, Data logging and processing software included, Fast sampling rate (7 - 24 Hz optional), and Compatible with the Bioshutter anti-biofouling solution.</skos:definition>
	<skos:inScheme rdf:resource="http://vocab.aodn.org.au/def/instrument/1"/>
	<skos:prefLabel xml:lang="en">Satlantic OCR-504 multispectral radiometer</skos:prefLabel>
	<skos:broader rdf:resource="http://vocab.nerc.ac.uk/collection/L05/current/122"/>
	<skos:scopeNote xml:lang="en">manufacturer:Satlantic</skos:scopeNote>
</rdf:Description>

<rdf:Description rdf:about="http://vocab.nerc.ac.uk/collection/L22/current/TOOL0666">
	<rdf:type rdf:resource="http://www.w3.org/2000/01/rdf-schema#Resource"/>
	<rdf:type rdf:resource="http://www.w3.org/2004/02/skos/core#Concept"/>
	<dcterms:created rdf:datatype="http://www.w3.org/2001/XMLSchema#dateTime">2013-10-15T00:00:00Z</dcterms:created>
	<dc:publisher rdf:datatype="http://www.w3.org/2001/XMLSchema#string">British Oceanographic Data Centre (BODC)</dc:publisher>
	<dc:source rdf:datatype="http://www.w3.org/2001/XMLSchema#string">(L221) SeaVoX Device Catalogue</dc:source>
	<skos:definition xml:lang="en">A discontinued instrument that measured sun and sky irradiance in the range of wavelengths 0.285 to 2.8 microns, including most of the solar spectrum.  It had a "hemispheric receiver" intended to approximate the cosine response for oblique rays. More information may be found at http://www.yale.edu/ceo/Documentation/Eppley%20Precision%20Spectral%20Pyranometer.pdf.</skos:definition>
	<skos:inScheme rdf:resource="http://vocab.aodn.org.au/def/instrument/1"/>
	<skos:prefLabel xml:lang="en">Eppley Precision Spectral Pyranometer</skos:prefLabel>
	<skos:broader rdf:resource="http://vocab.nerc.ac.uk/collection/L05/current/122"/>
	<skos:scopeNote xml:lang="en">manufacturer:The Eppley Laboratory Inc.</skos:scopeNote>
</rdf:Description>

<rdf:Description rdf:about="http://vocab.nerc.ac.uk/collection/L22/current/TOOL0676">
	<rdf:type rdf:resource="http://www.w3.org/2000/01/rdf-schema#Resource"/>
	<rdf:type rdf:resource="http://www.w3.org/2004/02/skos/core#Concept"/>
	<dcterms:created rdf:datatype="http://www.w3.org/2001/XMLSchema#dateTime">2014-04-01T00:00:00Z</dcterms:created>
	<dc:publisher rdf:datatype="http://www.w3.org/2001/XMLSchema#string">British Oceanographic Data Centre (BODC)</dc:publisher>
	<dc:source rdf:datatype="http://www.w3.org/2001/XMLSchema#string">(L221) SeaVoX Device Catalogue</dc:source>
	<skos:definition xml:lang="en">A cosine-collector underwater light meter in an acetal co-polymer housing sensitive to photosynthetically-active (400-700nm) radiation (PAR).  It is equipped with 'Bio-wiper' technology to prevent biofouling and so is capable of long-term deployments on buoys and moorings. For more information see http://www.wetlabs.com/eco-par.</skos:definition>
	<skos:inScheme rdf:resource="http://vocab.aodn.org.au/def/instrument/1"/>
	<skos:prefLabel xml:lang="en">WETLabs ECO-PAR</skos:prefLabel>
	<skos:broader rdf:resource="http://vocab.nerc.ac.uk/collection/L05/current/122"/>
	<skos:scopeNote xml:lang="en">manufacture:WETLabs Inc.</skos:scopeNote>
</rdf:Description>

<rdf:Description rdf:about="http://vocab.nerc.ac.uk/collection/L22/current/TOOL1117">
	<rdf:type rdf:resource="http://www.w3.org/2000/01/rdf-schema#Resource"/>
	<rdf:type rdf:resource="http://www.w3.org/2004/02/skos/core#Concept"/>
	<dcterms:contributor rdf:resource="http://editor.vocabs.ands.org.au/user/eMII_Atkins.Natalia"/>
	<dcterms:created rdf:datatype="http://www.w3.org/2001/XMLSchema#dateTime">2017-03-21T00:00:00Z</dcterms:created>
	<dcterms:modified rdf:datatype="http://www.w3.org/2001/XMLSchema#dateTime">2017-04-10T04:59:14Z</dcterms:modified>
	<dc:publisher rdf:datatype="http://www.w3.org/2001/XMLSchema#string">British Oceanographic Data Centre (BODC)</dc:publisher>
	<skos:definition xml:lang="en">A series of cosine-response radiometers for in-water and in-air applications. Each sensor contains a 256 channel silicon photodiode array. They have a sampling rate of up to 3 Hz and a spectral range of 300-1200 nm (350-800 nm calibrated range). Spectral accuracy is 0.3 nm and spectral resolution is 10 nm.</skos:definition>
	<skos:inScheme rdf:resource="http://vocab.aodn.org.au/def/instrument/1"/>
	<skos:prefLabel xml:lang="en">Satlantic HyperOCR spectroradiometer series</skos:prefLabel>
	<skos:broader rdf:resource="http://vocab.nerc.ac.uk/collection/L05/current/122"/>
</rdf:Description>

<rdf:Description rdf:about="http://vocab.nerc.ac.uk/collection/L22/current/TOOL1126">
	<rdf:type rdf:resource="http://www.w3.org/2000/01/rdf-schema#Resource"/>
	<rdf:type rdf:resource="http://www.w3.org/2004/02/skos/core#Concept"/>
	<dcterms:created rdf:datatype="http://www.w3.org/2001/XMLSchema#dateTime">2017-04-10T00:00:00Z</dcterms:created>
	<dc:publisher rdf:datatype="http://www.w3.org/2001/XMLSchema#string">British Oceanographic Data Centre (BODC)</dc:publisher>
	<skos:definition xml:lang="en">A pocket-sized PAR logger. It measures photon flux density using a photodiode. It has non-opening infrared communication. It has a titanium body and polycarbonate window. It has a measurement range of 0-5000 micromole per metre sq. per second. Accuracy is +/- 4.0% F.S. (0-2000 micromole per metre sq. per s) and it is depth-rated to 500 m (depth equivalent).</skos:definition>
	<skos:inScheme rdf:resource="http://vocab.aodn.org.au/def/instrument/1"/>
	<skos:prefLabel xml:lang="en">JFE Advantech DEFI2-L PAR sensor</skos:prefLabel>
	<skos:broader rdf:resource="http://vocab.nerc.ac.uk/collection/L05/current/122"/>
	<skos:altLabel xml:lang="en">JFE Advantech DEF12-L</skos:altLabel>
</rdf:Description>

<rdf:Description rdf:about="http://vocab.nerc.ac.uk/collection/L22/current/TOOL1125">
	<rdf:type rdf:resource="http://www.w3.org/2000/01/rdf-schema#Resource"/>
	<rdf:type rdf:resource="http://www.w3.org/2004/02/skos/core#Concept"/>
	<dcterms:created rdf:datatype="http://www.w3.org/2001/XMLSchema#dateTime">2017-04-10T00:00:00Z</dcterms:created>
	<dc:publisher rdf:datatype="http://www.w3.org/2001/XMLSchema#string">British Oceanographic Data Centre (BODC)</dc:publisher>
	<skos:definition xml:lang="en">A sensor system for measuring optical backscattering at 9 wavelengths between 412 - 715 nm. It uses nine LEDs (modulated at 1 kHz) for source light. The source light enters the water volume and scattered material is detected by a detector positioned where the acceptance angle forms a 117-degree intersection with the source beam. It contains three BB3 instruments and one data multiplexer (ECO Mux), all contained within a single pressure housing. Each BB3 instrument provides a backscatter measurement for three different wavelengths. It can include auxiliary sensors. Older versions could be fitted with an optional temperature and pressure sensor. Optical range is approx. 0.0024 - 5 m-1.</skos:definition>
	<skos:inScheme rdf:resource="http://vocab.aodn.org.au/def/instrument/1"/>
	<skos:prefLabel xml:lang="en">WETLabs ECO BB9 backscattering sensor</skos:prefLabel>
	<skos:broader rdf:resource="http://vocab.nerc.ac.uk/collection/L05/current/123"/>
	<skos:broader rdf:resource="http://vocab.nerc.ac.uk/collection/L05/current/134"/>
	<skos:broader rdf:resource="http://vocab.nerc.ac.uk/collection/L05/current/WPS"/>
	<skos:altLabel xml:lang="en">WETLabs ECO BB9</skos:altLabel>
</rdf:Description>

<rdf:Description rdf:about="http://vocab.nerc.ac.uk/collection/L22/current/TOOL0834">
	<rdf:type rdf:resource="http://www.w3.org/2000/01/rdf-schema#Resource"/>
	<rdf:type rdf:resource="http://www.w3.org/2004/02/skos/core#Concept"/>
	<dcterms:created rdf:datatype="http://www.w3.org/2001/XMLSchema#dateTime">2017-03-13T00:00:00Z</dcterms:created>
	<dc:publisher rdf:datatype="http://www.w3.org/2001/XMLSchema#string">British Oceanographic Data Centre (BODC)</dc:publisher>
	<skos:definition xml:lang="en">The WETLabs ac-s in-situ spectrophotometer is based on the ac-9 flow through sensor offering increased spectral resolution of in-situ absorption and beam attenuation. The ac-s can have 80 (+/- 5) wavelength outputs with a range of 400-730 nm. The ac-s consists of a 10 or 25 cm pathlength, a 4nm resolution, an accuracy of 0.001 - 10 m-1, an operational temperature range of 0 - 30 deg C and an operational depth rating of 500 m.</skos:definition>
	<skos:inScheme rdf:resource="http://vocab.aodn.org.au/def/instrument/1"/>
	<skos:prefLabel xml:lang="en">WETLabs ac-s in-situ spectrophotometer</skos:prefLabel>
	<skos:broader rdf:resource="http://vocab.nerc.ac.uk/collection/L05/current/124"/>
	<skos:altLabel xml:lang="en">WETLabs ACS</skos:altLabel>
</rdf:Description>

<rdf:Description rdf:about="http://vocab.nerc.ac.uk/collection/L22/current/TOOL0040">
	<rdf:type rdf:resource="http://www.w3.org/2000/01/rdf-schema#Resource"/>
	<rdf:type rdf:resource="http://www.w3.org/2004/02/skos/core#Concept"/>
	<dcterms:created rdf:datatype="http://www.w3.org/2001/XMLSchema#dateTime">2014-02-07T00:00:00Z</dcterms:created>
	<dc:publisher rdf:datatype="http://www.w3.org/2001/XMLSchema#string">British Oceanographic Data Centre (BODC)</dc:publisher>
	<dc:source rdf:datatype="http://www.w3.org/2001/XMLSchema#string">(L221) SeaVoX Device Catalogue</dc:source>
	<skos:definition xml:lang="en">A compact self-contained CTD comprising a conductivity sensor plumbed into a pumped water supply and separate pressure and temperature sensor modules. The whole unit is mounted in a stainless steel cage with a battery pack, data logger and memory. A dissolved oxygen sensor may be plumbed into the pumped water supply and other sensor modules such as fluorometers and transmissometers may be mounted in the cage and interfaced to the data logger. The instrument may also be used with external power and data logging through an RS-232 interface.</skos:definition>
	<skos:inScheme rdf:resource="http://vocab.aodn.org.au/def/instrument/1"/>
	<skos:prefLabel xml:lang="en">Sea-Bird SBE 25 Sealogger CTD</skos:prefLabel>
	<skos:broader rdf:resource="http://vocab.nerc.ac.uk/collection/L05/current/130"/>
	<skos:broader rdf:resource="http://vocab.nerc.ac.uk/collection/L05/current/134"/>
	<skos:broader rdf:resource="http://vocab.nerc.ac.uk/collection/L05/current/350"/>
	<skos:scopeNote xml:lang="en">manufacturer:Sea-Bird Electronics Inc.</skos:scopeNote>
</rdf:Description>

<rdf:Description rdf:about="http://vocab.nerc.ac.uk/collection/L22/current/TOOL0042">
	<rdf:type rdf:resource="http://www.w3.org/2000/01/rdf-schema#Resource"/>
	<rdf:type rdf:resource="http://www.w3.org/2004/02/skos/core#Concept"/>
	<dcterms:created rdf:datatype="http://www.w3.org/2001/XMLSchema#dateTime">2014-02-17T00:00:00Z</dcterms:created>
	<dc:publisher rdf:datatype="http://www.w3.org/2001/XMLSchema#string">British Oceanographic Data Centre (BODC)</dc:publisher>
	<dc:source rdf:datatype="http://www.w3.org/2001/XMLSchema#string">(L221) SeaVoX Device Catalogue</dc:source>
	<skos:definition xml:lang="en">A self-contained battery powered CTD with precision semiconductor strain gauge pressure sensor. Water was supplied to the conductivity sensor by a pump. Housing was plastic (up to 600m depth), aluminium (up to 6800m depth) or titanium (up to 10500m depth). Optional oxygen, pH, fluorescence, PAR, light transmission and turbidity sensors could be fitted. Primarily designed for profiling applications but may be used on a short (less than 2 weeks) duration mooring. Replaced by the SBE19plus model in 2001.</skos:definition>
	<skos:inScheme rdf:resource="http://vocab.aodn.org.au/def/instrument/1"/>
	<skos:prefLabel xml:lang="en">Sea-Bird SBE 19 SEACAT CTD</skos:prefLabel>
	<skos:broader rdf:resource="http://vocab.nerc.ac.uk/collection/L05/current/130"/>
	<skos:broader rdf:resource="http://vocab.nerc.ac.uk/collection/L05/current/134"/>
	<skos:broader rdf:resource="http://vocab.nerc.ac.uk/collection/L05/current/350"/>
	<skos:scopeNote xml:lang="en">manufacturer:Sea-Bird Electronics Inc.</skos:scopeNote>
</rdf:Description>

<rdf:Description rdf:about="http://vocab.nerc.ac.uk/collection/L22/current/TOOL0047">
	<rdf:type rdf:resource="http://www.w3.org/2000/01/rdf-schema#Resource"/>
	<rdf:type rdf:resource="http://www.w3.org/2004/02/skos/core#Concept"/>
	<dcterms:created rdf:datatype="http://www.w3.org/2001/XMLSchema#dateTime">2014-02-07T00:00:00Z</dcterms:created>
	<dc:publisher rdf:datatype="http://www.w3.org/2001/XMLSchema#string">British Oceanographic Data Centre (BODC)</dc:publisher>
	<dc:source rdf:datatype="http://www.w3.org/2001/XMLSchema#string">(L221) SeaVoX Device Catalogue</dc:source>
	<skos:definition xml:lang="en">Self contained self powered CTD profiler. Measures conductivity, temperature and pressure in both profiling (samples at 4 scans/sec) and moored (sample rates of once every 5 seconds to once every 9 hours) mode. Available in plastic or titanium housing with depth ranges of 600m and 7000m respectively. Minature submersible pump provides water to conductivity cell.</skos:definition>
	<skos:inScheme rdf:resource="http://vocab.aodn.org.au/def/instrument/1"/>
	<skos:prefLabel xml:lang="en">Sea-Bird SBE 19plus SEACAT CTD</skos:prefLabel>
	<skos:broader rdf:resource="http://vocab.nerc.ac.uk/collection/L05/current/130"/>
	<skos:broader rdf:resource="http://vocab.nerc.ac.uk/collection/L05/current/134"/>
	<skos:broader rdf:resource="http://vocab.nerc.ac.uk/collection/L05/current/350"/>
	<skos:scopeNote xml:lang="en">manufacturer:Sea-Bird Electronics Inc.</skos:scopeNote>
</rdf:Description>

<rdf:Description rdf:about="http://vocab.nerc.ac.uk/collection/L22/current/TOOL0058">
	<rdf:type rdf:resource="http://www.w3.org/2000/01/rdf-schema#Resource"/>
	<rdf:type rdf:resource="http://www.w3.org/2004/02/skos/core#Concept"/>
	<dcterms:created rdf:datatype="http://www.w3.org/2001/XMLSchema#dateTime">2014-07-14T00:00:00Z</dcterms:created>
	<dc:publisher rdf:datatype="http://www.w3.org/2001/XMLSchema#string">British Oceanographic Data Centre (BODC)</dc:publisher>
	<dc:source rdf:datatype="http://www.w3.org/2001/XMLSchema#string">(L221) SeaVoX Device Catalogue</dc:source>
	<skos:definition xml:lang="en">High precision and accuracy CTD comprising an SBE 9plus underwater unit (SBE 3 temperature and SBE 4 conductivity sensors) and an SBE 11plus deck unit. Sensors may be connected to a pump-fed plastic tubing circuit (usually temperature, salinity and oxygen) or stand-alone. All instruments (8 channels available) on the package are logged by the SBE 11. The unit is the production off the shelf version of the SBE 911 (each 911 was custom built to individual specification).</skos:definition>
	<skos:inScheme rdf:resource="http://vocab.aodn.org.au/def/instrument/1"/>
	<skos:prefLabel xml:lang="en">Sea-Bird SBE 911plus CTD</skos:prefLabel>
	<skos:broader rdf:resource="http://vocab.nerc.ac.uk/collection/L05/current/130"/>
	<skos:broader rdf:resource="http://vocab.nerc.ac.uk/collection/L05/current/134"/>
	<skos:broader rdf:resource="http://vocab.nerc.ac.uk/collection/L05/current/350"/>
</rdf:Description>

<rdf:Description rdf:about="http://vocab.nerc.ac.uk/collection/L22/current/TOOL0173">
	<rdf:type rdf:resource="http://www.w3.org/2000/01/rdf-schema#Resource"/>
	<rdf:type rdf:resource="http://www.w3.org/2004/02/skos/core#Concept"/>
	<dcterms:contributor rdf:resource="http://editor.vocabs.ands.org.au/user/eMII_Atkins.Natalia"/>
	<dcterms:created rdf:datatype="http://www.w3.org/2001/XMLSchema#dateTime">2014-02-07T00:00:00Z</dcterms:created>
	<dcterms:modified rdf:datatype="http://www.w3.org/2001/XMLSchema#dateTime">2017-11-08T04:57:26Z</dcterms:modified>
	<dc:publisher rdf:datatype="http://www.w3.org/2001/XMLSchema#string">British Oceanographic Data Centre (BODC)</dc:publisher>
	<dc:source rdf:datatype="http://www.w3.org/2001/XMLSchema#string">(L221) SeaVoX Device Catalogue</dc:source>
	<skos:definition xml:lang="en">	A collection of conductivity, temperature and depth (CTD) sensors which are generally linked to a common data logger that samples at up to 15Hz. The CTD sensors utilise the patented Non-eXternal Inductive Cell (NXIC) conductivity sensor, originally developed by FSI for the US Navy DT-705 Sound Velocity/Salinity sensor. Models in the collection include the NXIC CT Bio Direct Read-500M, NXIC CTD Bio Direct Read-500M, NXIC CTD Bio Auto-500M, NXIC CTD Direct Read-500M, NXIC CTD Direct Read-700M, NXIC CTD Auto-500M, NXIC CTD Auto-700M, NXIC CTD-ADC with external sensors, and the NXIC ETSG Thermosalinograph. Parameters are measured to an accuracy ranging from 0.002-0.010 mS/cm for conductivity, 0.005 degC for temperature and 0.08% for full scale pressure. Now marketed by Teledyne RD Instruments.</skos:definition>
	<skos:inScheme rdf:resource="http://vocab.aodn.org.au/def/instrument/1"/>
	<skos:prefLabel xml:lang="en">Falmouth Scientific Instruments NXIC CTD</skos:prefLabel>
	<skos:broader rdf:resource="http://vocab.nerc.ac.uk/collection/L05/current/130"/>
	<skos:broader rdf:resource="http://vocab.nerc.ac.uk/collection/L05/current/134"/>
	<skos:broader rdf:resource="http://vocab.nerc.ac.uk/collection/L05/current/350"/>
	<skos:scopeNote xml:lang="en">manufacturer:Falmouth Scientific Inc.</skos:scopeNote>
</rdf:Description>

<rdf:Description rdf:about="http://vocab.nerc.ac.uk/collection/L22/current/TOOL0183">
	<rdf:type rdf:resource="http://www.w3.org/2000/01/rdf-schema#Resource"/>
	<rdf:type rdf:resource="http://www.w3.org/2004/02/skos/core#Concept"/>
	<dcterms:contributor rdf:resource="http://editor.vocabs.ands.org.au/user/eMII_Mancini.Sebastien"/>
	<dcterms:created rdf:datatype="http://www.w3.org/2001/XMLSchema#dateTime">2017-03-13T00:00:00Z</dcterms:created>
	<dcterms:modified rdf:datatype="http://www.w3.org/2001/XMLSchema#dateTime">2017-11-21T01:30:10Z</dcterms:modified>
	<dc:publisher rdf:datatype="http://www.w3.org/2001/XMLSchema#string">British Oceanographic Data Centre (BODC)</dc:publisher>
	<skos:definition xml:lang="en">A miniature self-contained CTD primarily designed for mounting on fish, birds or marine mammals. Salinity resolution is 0.02 PSU and accuracy +-0.75 PSU. Temperature resolution is 0.032C and accuracy +-0.1C.</skos:definition>
	<skos:inScheme rdf:resource="http://vocab.aodn.org.au/def/instrument/1"/>
	<skos:prefLabel xml:lang="en">Star-Oddi DST CTD</skos:prefLabel>
	<skos:broader rdf:resource="http://vocab.nerc.ac.uk/collection/L05/current/130"/>
	<skos:broader rdf:resource="http://vocab.nerc.ac.uk/collection/L05/current/134"/>
	<skos:broader rdf:resource="http://vocab.nerc.ac.uk/collection/L05/current/350"/>
</rdf:Description>

<rdf:Description rdf:about="http://vocab.nerc.ac.uk/collection/L22/current/TOOL0446">
	<rdf:type rdf:resource="http://www.w3.org/2000/01/rdf-schema#Resource"/>
	<rdf:type rdf:resource="http://www.w3.org/2004/02/skos/core#Concept"/>
	<dcterms:created rdf:datatype="http://www.w3.org/2001/XMLSchema#dateTime">2013-10-10T00:00:00Z</dcterms:created>
	<dc:publisher rdf:datatype="http://www.w3.org/2001/XMLSchema#string">British Oceanographic Data Centre (BODC)</dc:publisher>
	<dc:source rdf:datatype="http://www.w3.org/2001/XMLSchema#string">(L221) SeaVoX Device Catalogue</dc:source>
	<skos:definition xml:lang="en">This tag provides oceanographic quality Conductivity/Temperature/Depth casts. Oceanographic quality temperature &amp; salinity profiles (4 - 12 profiles per day), CTD data automatically submitted to the GTS in near real-time. Up to 50,000 full length Argos data transmissions and pressure-proof to 2000m.  Retains a continuous record of depth readings (4 sec sample rate), which can be retrieved by bluetooth link if the tag is recovered. Also records all individual temperature and salinity measurements (1 Hz) made during profiling. Longevity: up to one year. Size: 10.5 x 7 x 4 cm. Weight: 545 g.</skos:definition>
	<skos:inScheme rdf:resource="http://vocab.aodn.org.au/def/instrument/1"/>
	<skos:prefLabel xml:lang="en">SMRU CTD Satellite Relay Data Logger</skos:prefLabel>
	<skos:broader rdf:resource="http://vocab.nerc.ac.uk/collection/L05/current/130"/>
	<skos:broader rdf:resource="http://vocab.nerc.ac.uk/collection/L05/current/134"/>
	<skos:broader rdf:resource="http://vocab.nerc.ac.uk/collection/L05/current/350"/>
	<skos:broader rdf:resource="http://vocab.nerc.ac.uk/collection/L05/current/POS17"/>
	<skos:scopeNote xml:lang="en">manufacturer:SMRU Instrumentation</skos:scopeNote>
</rdf:Description>

<rdf:Description rdf:about="http://vocab.nerc.ac.uk/collection/L22/current/TOOL0668">
	<rdf:type rdf:resource="http://www.w3.org/2000/01/rdf-schema#Resource"/>
	<rdf:type rdf:resource="http://www.w3.org/2004/02/skos/core#Concept"/>
	<dcterms:created rdf:datatype="http://www.w3.org/2001/XMLSchema#dateTime">2013-09-09T00:00:00Z</dcterms:created>
	<dc:publisher rdf:datatype="http://www.w3.org/2001/XMLSchema#string">British Oceanographic Data Centre (BODC)</dc:publisher>
	<dc:source rdf:datatype="http://www.w3.org/2001/XMLSchema#string">(L221) SeaVoX Device Catalogue</dc:source>
	<skos:definition xml:lang="en">A self-contained unit comprising the MicroCAT temperature, conductivity and pressure sensors and a pump that is designed specifically for deployment on profiling floats, particularly Argo.  The unit is designed to provide stable salinity data accurate to 0.005 PSU for periods in excess of three years without any form of maintenance. Temperature is within 0.002 C (stability 0.0002 C/year) and pressure within 2 dbar (stability 0.8 dbar/year).  During float ascent spot samples are taken and transmitted to the float controller.  More information is given in http://www.seabird.com/products/spec_sheets/41data.htm.</skos:definition>
	<skos:inScheme rdf:resource="http://vocab.aodn.org.au/def/instrument/1"/>
	<skos:prefLabel xml:lang="en">Sea-Bird SBE 41 CTD</skos:prefLabel>
	<skos:broader rdf:resource="http://vocab.nerc.ac.uk/collection/L05/current/130"/>
	<skos:broader rdf:resource="http://vocab.nerc.ac.uk/collection/L05/current/134"/>
	<skos:broader rdf:resource="http://vocab.nerc.ac.uk/collection/L05/current/350"/>
	<skos:scopeNote xml:lang="en">manufacturer:Sea-Bird Electronics Inc.</skos:scopeNote>
</rdf:Description>

<rdf:Description rdf:about="http://vocab.nerc.ac.uk/collection/L22/current/TOOL0669">
	<rdf:type rdf:resource="http://www.w3.org/2000/01/rdf-schema#Resource"/>
	<rdf:type rdf:resource="http://www.w3.org/2004/02/skos/core#Concept"/>
	<dcterms:created rdf:datatype="http://www.w3.org/2001/XMLSchema#dateTime">2014-04-02T00:00:00Z</dcterms:created>
	<dc:publisher rdf:datatype="http://www.w3.org/2001/XMLSchema#string">British Oceanographic Data Centre (BODC)</dc:publisher>
	<dc:source rdf:datatype="http://www.w3.org/2001/XMLSchema#string">(L221) SeaVoX Device Catalogue</dc:source>
	<skos:definition xml:lang="en">A self-contained unit comprising the MicroCAT temperature, conductivity and pressure sensors and a pump that is designed specifically for deployment on profiling floats, particularly Argo.  The unit is designed to provide stable salinity data accurate to 0.005 PSU for periods in excess of three years without any form of maintenance. Temperature is within 0.002 C (stability 0.0002 C/year) and pressure within 2 dbar (stability 0.8 dbar/year).  During float ascent samples are collected at 1 Hz and logged to internal storage to provide a continuous profile passed to the float controller at the surface.  More information is given in http://www.seabird.com/products/spec_sheets/41data.htm.</skos:definition>
	<skos:inScheme rdf:resource="http://vocab.aodn.org.au/def/instrument/1"/>
	<skos:prefLabel xml:lang="en">Sea-Bird SBE 41CP CTD</skos:prefLabel>
	<skos:broader rdf:resource="http://vocab.nerc.ac.uk/collection/L05/current/130"/>
	<skos:broader rdf:resource="http://vocab.nerc.ac.uk/collection/L05/current/134"/>
	<skos:broader rdf:resource="http://vocab.nerc.ac.uk/collection/L05/current/350"/>
	<skos:scopeNote xml:lang="en">manufacturer:Sea-Bird Electronics Inc.</skos:scopeNote>
</rdf:Description>

<rdf:Description rdf:about="http://vocab.nerc.ac.uk/collection/L22/current/TOOL0730">
	<rdf:type rdf:resource="http://www.w3.org/2000/01/rdf-schema#Resource"/>
	<rdf:type rdf:resource="http://www.w3.org/2004/02/skos/core#Concept"/>
	<dcterms:created rdf:datatype="http://www.w3.org/2001/XMLSchema#dateTime">2014-07-14T00:00:00Z</dcterms:created>
	<dc:publisher rdf:datatype="http://www.w3.org/2001/XMLSchema#string">British Oceanographic Data Centre (BODC)</dc:publisher>
	<dc:source rdf:datatype="http://www.w3.org/2001/XMLSchema#string">(L221) SeaVoX Device Catalogue</dc:source>
	<skos:definition xml:lang="en">A small profiling data logger designed to monitor conductivity, temperature and depth. Conductivity (accuracy ± 0.003 mS/cm) is measured using a 3-coil closed loop feedback inductive cell for superior temperature compensation. The thermistor (Themometrics) used to record temperature (accuracy ± 0.002°C) is aged and hermetically sealed in the tip of a shock resistant solid glass rod. Pressure (accuracy 0.05% full scale) sensors use reliable semiconductor technology and 316 stainless steel housing developed for long-term stability in harsh environments. The XR-620 is a profiling version of the XR-420.</skos:definition>
	<skos:inScheme rdf:resource="http://vocab.aodn.org.au/def/instrument/1"/>
	<skos:prefLabel xml:lang="en">RBR XR-620 CTD Profiler</skos:prefLabel>
	<skos:broader rdf:resource="http://vocab.nerc.ac.uk/collection/L05/current/130"/>
</rdf:Description>

<rdf:Description rdf:about="http://vocab.nerc.ac.uk/collection/L22/current/TOOL0263">
	<rdf:type rdf:resource="http://www.w3.org/2000/01/rdf-schema#Resource"/>
	<rdf:type rdf:resource="http://www.w3.org/2004/02/skos/core#Concept"/>
	<dcterms:created rdf:datatype="http://www.w3.org/2001/XMLSchema#dateTime">2013-03-28T00:00:00Z</dcterms:created>
	<dc:publisher rdf:datatype="http://www.w3.org/2001/XMLSchema#string">British Oceanographic Data Centre (BODC)</dc:publisher>
	<dc:source rdf:datatype="http://www.w3.org/2001/XMLSchema#string">(L221) SeaVoX Device Catalogue</dc:source>
	<skos:definition xml:lang="en">An expendable free-fall temperature probe that provides a profile of measured temperature against depth calculated from a fall-rate model. The T-7 XBT Probe can be used within a maximum depth of 760m, may be deployed at a ship speed of up to 15 knots and has a vertical resolution of 65cm.</skos:definition>
	<skos:inScheme rdf:resource="http://vocab.aodn.org.au/def/instrument/1"/>
	<skos:prefLabel xml:lang="en">Lockheed Martin Sippican T-7 XBT probe</skos:prefLabel>
	<skos:broader rdf:resource="http://vocab.nerc.ac.uk/collection/L05/current/132"/>
	<skos:scopeNote xml:lang="en">manufacturer: Lockheed Martin</skos:scopeNote>
</rdf:Description>

<rdf:Description rdf:about="http://vocab.nerc.ac.uk/collection/L22/current/TOOL0435">
	<rdf:type rdf:resource="http://www.w3.org/2000/01/rdf-schema#Resource"/>
	<rdf:type rdf:resource="http://www.w3.org/2004/02/skos/core#Concept"/>
	<dcterms:created rdf:datatype="http://www.w3.org/2001/XMLSchema#dateTime">2013-03-28T00:00:00Z</dcterms:created>
	<dc:publisher rdf:datatype="http://www.w3.org/2001/XMLSchema#string">British Oceanographic Data Centre (BODC)</dc:publisher>
	<dc:source rdf:datatype="http://www.w3.org/2001/XMLSchema#string">(L221) SeaVoX Device Catalogue</dc:source>
	<skos:definition xml:lang="en">An expendable free-fall temperature probe that provides a profile of measured temperature against depth calculated from a fall-rate model. The T-4 XBT Probe can be used within a maximum depth of 460m, may be deployed at a ship speed of up to 30 knots and has a vertical resolution of 65cm.</skos:definition>
	<skos:inScheme rdf:resource="http://vocab.aodn.org.au/def/instrument/1"/>
	<skos:prefLabel xml:lang="en">Lockheed Martin Sippican T-4 XBT probe</skos:prefLabel>
	<skos:broader rdf:resource="http://vocab.nerc.ac.uk/collection/L05/current/132"/>
	<skos:scopeNote xml:lang="en">manufacturer: Lockheed Martin</skos:scopeNote>
</rdf:Description>

<rdf:Description rdf:about="http://vocab.nerc.ac.uk/collection/L22/current/TOOL0190">
	<rdf:type rdf:resource="http://www.w3.org/2000/01/rdf-schema#Resource"/>
	<rdf:type rdf:resource="http://www.w3.org/2004/02/skos/core#Concept"/>
	<dcterms:created rdf:datatype="http://www.w3.org/2001/XMLSchema#dateTime">2013-10-08T00:00:00Z</dcterms:created>
	<dc:publisher rdf:datatype="http://www.w3.org/2001/XMLSchema#string">British Oceanographic Data Centre (BODC)</dc:publisher>
	<dc:source rdf:datatype="http://www.w3.org/2001/XMLSchema#string">(L221) SeaVoX Device Catalogue</dc:source>
	<skos:definition xml:lang="en">A small externally powered, high-accuracy instrument, designed for shipboard determination of sea surface (pumped-water) conductivity and temperature. It is constructed of plastic and titanium to ensure long life with minimum maintenance. It may optionally be interfaced to an external SBE 38 hull temperature sensor.</skos:definition>
	<skos:inScheme rdf:resource="http://vocab.aodn.org.au/def/instrument/1"/>
	<skos:prefLabel xml:lang="en">Sea-Bird SBE 45 MicroTSG thermosalinograph</skos:prefLabel>
	<skos:broader rdf:resource="http://vocab.nerc.ac.uk/collection/L05/current/133"/>
	<skos:broader rdf:resource="http://vocab.nerc.ac.uk/collection/L05/current/134"/>
	<skos:broader rdf:resource="http://vocab.nerc.ac.uk/collection/L05/current/350"/>
	<skos:scopeNote xml:lang="en">manufacturer:Sea-Bird Electronics Inc.</skos:scopeNote>
</rdf:Description>

<rdf:Description rdf:about="http://vocab.nerc.ac.uk/collection/L22/current/TOOL0667">
	<rdf:type rdf:resource="http://www.w3.org/2000/01/rdf-schema#Resource"/>
	<rdf:type rdf:resource="http://www.w3.org/2004/02/skos/core#Concept"/>
	<dcterms:created rdf:datatype="http://www.w3.org/2001/XMLSchema#dateTime">2013-10-08T00:00:00Z</dcterms:created>
	<dc:publisher rdf:datatype="http://www.w3.org/2001/XMLSchema#string">British Oceanographic Data Centre (BODC)</dc:publisher>
	<dc:source rdf:datatype="http://www.w3.org/2001/XMLSchema#string">(L221) SeaVoX Device Catalogue</dc:source>
	<skos:definition xml:lang="en">A platinum-electrode conductivity sensor and a thermistor mounted in a corrosion-resistant plastic and titanium housing designed to be continuously plumbed into a vessel's pumped seawater supply. The instrument may be interfaced to a remote SBE 38 temperature sensor mounted either on the hull or in the seawater inlet. Data are both stored in internal memory and output to a serial port for external logging.  Conductivity is measured in the range 0-7 S/m with an accuracy of 0.001 S/m and a resolution  of 0.0001 S/m. Housing temperature is measured in the range -5-35C with an accuracy of 0.01 C and a resolution  of 0.001 C. Remote temperature is measured in the range -5-35C  with an accuracy of 0.001 C and a resolution  of 0.0003 C. More information at http://www.seabird.com/products/spec_sheets/21data.htm.</skos:definition>
	<skos:inScheme rdf:resource="http://vocab.aodn.org.au/def/instrument/1"/>
	<skos:prefLabel xml:lang="en">Sea-Bird SBE 21 Thermosalinograph</skos:prefLabel>
	<skos:broader rdf:resource="http://vocab.nerc.ac.uk/collection/L05/current/133"/>
	<skos:broader rdf:resource="http://vocab.nerc.ac.uk/collection/L05/current/134"/>
	<skos:broader rdf:resource="http://vocab.nerc.ac.uk/collection/L05/current/350"/>
	<skos:scopeNote xml:lang="en">manufacturer:Sea-Bird Electronics Inc.</skos:scopeNote>
</rdf:Description>

<rdf:Description rdf:about="http://vocab.nerc.ac.uk/collection/L22/current/TOOL0022">
	<rdf:type rdf:resource="http://www.w3.org/2000/01/rdf-schema#Resource"/>
	<rdf:type rdf:resource="http://www.w3.org/2004/02/skos/core#Concept"/>
	<dcterms:contributor rdf:resource="http://editor.vocabs.ands.org.au/user/eMII_Atkins.Natalia"/>
	<dcterms:created rdf:datatype="http://www.w3.org/2001/XMLSchema#dateTime">2013-03-28T00:00:00Z</dcterms:created>
	<dcterms:modified rdf:datatype="http://www.w3.org/2001/XMLSchema#dateTime">2017-03-23T05:02:07Z</dcterms:modified>
	<dc:publisher rdf:datatype="http://www.w3.org/2001/XMLSchema#string">British Oceanographic Data Centre (BODC)</dc:publisher>
	<dc:source rdf:datatype="http://www.w3.org/2001/XMLSchema#string">(L221) SeaVoX Device Catalogue</dc:source>
	<skos:definition xml:lang="en">The SBE 37 MicroCAT is a high accuracy conductivity and temperature recorder with an optional pressure sensor designed for depolyment on moorings. The IM model has an inductive modem for real-time data transmission plus internal flash memory data storage. Further information may be found on the BODC document server at URL http://www.bodc.ac.uk/data/documents/nodb/113079/.</skos:definition>
	<skos:inScheme rdf:resource="http://vocab.aodn.org.au/def/instrument/1"/>
	<skos:prefLabel xml:lang="en">Sea-Bird SBE 37-IM MicroCAT C-T Sensor</skos:prefLabel>
	<skos:broader rdf:resource="http://vocab.nerc.ac.uk/collection/L05/current/134"/>
	<skos:broader rdf:resource="http://vocab.nerc.ac.uk/collection/L05/current/350"/>
	<skos:altLabel xml:lang="en">SBE 37-IM MicroCAT</skos:altLabel>
</rdf:Description>

<rdf:Description rdf:about="http://vocab.nerc.ac.uk/collection/L22/current/TOOL0054">
	<rdf:type rdf:resource="http://www.w3.org/2000/01/rdf-schema#Resource"/>
	<rdf:type rdf:resource="http://www.w3.org/2004/02/skos/core#Concept"/>
	<dcterms:created rdf:datatype="http://www.w3.org/2001/XMLSchema#dateTime">2014-02-06T00:00:00Z</dcterms:created>
	<dc:publisher rdf:datatype="http://www.w3.org/2001/XMLSchema#string">British Oceanographic Data Centre (BODC)</dc:publisher>
	<dc:source rdf:datatype="http://www.w3.org/2001/XMLSchema#string">(L221) SeaVoX Device Catalogue</dc:source>
	<skos:definition xml:lang="en">The TDR-2050 is a small (235mm x 38mm OD), self-contained, submersible temperature and depth recorder (sensors and data logger). It can be deployed for a period of up to three years and can collect more than 1,200,000 sets of samples. Data can be retained in memory for 20 years (even without batteries). Available in two casings, plastic and titanium, with depth ratings of 740m and 6600m respectively. The temperature channel of the TDR-2050 is calibrated to an accuracy of ± 0.002°C (ITS-90) over the range -5 to +35°C.  Typical drift has been measured to be 0.002°C per year. The thermistor may be external (&lt;3sec time constant) or internal (&lt;20sec time constant). A fast thermistor probe (0.095sec) is also available. The depth channel is calibrated to an accuracy of 0.05%fs  Ranges from 10m to 6,600m are available.</skos:definition>
	<skos:inScheme rdf:resource="http://vocab.aodn.org.au/def/instrument/1"/>
	<skos:prefLabel xml:lang="en">RBR TDR-2050 underwater temperature logger</skos:prefLabel>
	<skos:broader rdf:resource="http://vocab.nerc.ac.uk/collection/L05/current/134"/>
	<skos:scopeNote xml:lang="en">manufacturer:RBR Ltd.</skos:scopeNote>
</rdf:Description>

<rdf:Description rdf:about="http://vocab.nerc.ac.uk/collection/L22/current/TOOL0105">
	<rdf:type rdf:resource="http://www.w3.org/2000/01/rdf-schema#Resource"/>
	<rdf:type rdf:resource="http://www.w3.org/2004/02/skos/core#Concept"/>
	<dcterms:created rdf:datatype="http://www.w3.org/2001/XMLSchema#dateTime">2014-08-06T00:00:00Z</dcterms:created>
	<dc:publisher rdf:datatype="http://www.w3.org/2001/XMLSchema#string">British Oceanographic Data Centre (BODC)</dc:publisher>
	<dc:source rdf:datatype="http://www.w3.org/2001/XMLSchema#string">(L221) SeaVoX Device Catalogue</dc:source>
	<skos:definition xml:lang="en">A miniature data logger that records temperature at a user programmed time interval. 12-bit version gives a resolution of 0.015C and an accuracy of +-0.1C. It is housed in a waterproof cylinder and the temperature sensor is mounted on a protruding stainless steel probe. Further information may be found on the BODC document server at URL: http://www.bodc.ac.uk/data/documents/nodb/108661/</skos:definition>
	<skos:inScheme rdf:resource="http://vocab.aodn.org.au/def/instrument/1"/>
	<skos:prefLabel xml:lang="en">Vemco Minilog12 temperature recorder</skos:prefLabel>
	<skos:broader rdf:resource="http://vocab.nerc.ac.uk/collection/L05/current/134"/>
</rdf:Description>

<rdf:Description rdf:about="http://vocab.nerc.ac.uk/collection/L22/current/TOOL0181">
	<rdf:type rdf:resource="http://www.w3.org/2000/01/rdf-schema#Resource"/>
	<rdf:type rdf:resource="http://www.w3.org/2004/02/skos/core#Concept"/>
	<dcterms:created rdf:datatype="http://www.w3.org/2001/XMLSchema#dateTime">2014-08-06T00:00:00Z</dcterms:created>
	<dc:publisher rdf:datatype="http://www.w3.org/2001/XMLSchema#string">British Oceanographic Data Centre (BODC)</dc:publisher>
	<dc:source rdf:datatype="http://www.w3.org/2001/XMLSchema#string">(L221) SeaVoX Device Catalogue</dc:source>
	<skos:definition xml:lang="en">A miniature data logger that records temperature at a user programmed time interval. 8-bit version gives a resolution of 0.1C and an accuracy of between +-0.2C to +-0.3C depending on range specified. It is housed in a waterproof cylinder and the temperature sensor is mounted on a protruding stainless steel probe.</skos:definition>
	<skos:inScheme rdf:resource="http://vocab.aodn.org.au/def/instrument/1"/>
	<skos:prefLabel xml:lang="en">Vemco Minilog8 temperature recorder</skos:prefLabel>
	<skos:broader rdf:resource="http://vocab.nerc.ac.uk/collection/L05/current/134"/>
</rdf:Description>

<rdf:Description rdf:about="http://vocab.nerc.ac.uk/collection/L22/current/TOOL0191">
	<rdf:type rdf:resource="http://www.w3.org/2000/01/rdf-schema#Resource"/>
	<rdf:type rdf:resource="http://www.w3.org/2004/02/skos/core#Concept"/>
	<dcterms:created rdf:datatype="http://www.w3.org/2001/XMLSchema#dateTime">2013-10-08T00:00:00Z</dcterms:created>
	<dc:publisher rdf:datatype="http://www.w3.org/2001/XMLSchema#string">British Oceanographic Data Centre (BODC)</dc:publisher>
	<dc:source rdf:datatype="http://www.w3.org/2001/XMLSchema#string">(L221) SeaVoX Device Catalogue</dc:source>
	<skos:definition xml:lang="en">An oceanographic thermometer with a measurement range of -5 to +35C; absolute accuracy better than 0.001C and resolution of approximately 0.00025C. The sensor is an ultra-stable aged thermistor with a drift rate of less than 0.002C per year. The reference resistor is a hermetically sealed VISHAY. It may be fitted in a 10,500m titanium pressure housing.</skos:definition>
	<skos:inScheme rdf:resource="http://vocab.aodn.org.au/def/instrument/1"/>
	<skos:prefLabel xml:lang="en">Sea-Bird SBE 38 thermometer</skos:prefLabel>
	<skos:broader rdf:resource="http://vocab.nerc.ac.uk/collection/L05/current/134"/>
	<skos:scopeNote xml:lang="en">manufacturer:Sea-Bird Electronics Inc.</skos:scopeNote>
</rdf:Description>

<rdf:Description rdf:about="http://vocab.nerc.ac.uk/collection/L22/current/TOOL0266">
	<rdf:type rdf:resource="http://www.w3.org/2000/01/rdf-schema#Resource"/>
	<rdf:type rdf:resource="http://www.w3.org/2004/02/skos/core#Concept"/>
	<dcterms:created rdf:datatype="http://www.w3.org/2001/XMLSchema#dateTime">2014-02-06T00:00:00Z</dcterms:created>
	<dc:publisher rdf:datatype="http://www.w3.org/2001/XMLSchema#string">British Oceanographic Data Centre (BODC)</dc:publisher>
	<dc:source rdf:datatype="http://www.w3.org/2001/XMLSchema#string">(L221) SeaVoX Device Catalogue</dc:source>
	<skos:definition xml:lang="en">A high-accuracy temperature recorder (pressure optional) with internal battery and non-volatile memory for deployment at depths up to 10500 meters. It is intended for moorings or other long-term, fixed-site applications, as well as shorter-term deployments on nets, towed vehicles or ROVs. Calibration coefficients stored in EEPROM allow the SBE 39 to transmit data in engineering units. The SBE 39 thermistor has a long history of exceptional accuracy and stability (typical drift is less than 0.002C per year). The SBE 39 communicates directly with a computer via a standard RA-232 interface. For more information see http://www.bodc.ac.uk/data/documents/nodb/108627/</skos:definition>
	<skos:inScheme rdf:resource="http://vocab.aodn.org.au/def/instrument/1"/>
	<skos:prefLabel xml:lang="en">Sea-Bird SBE 39 temperature recorder</skos:prefLabel>
	<skos:broader rdf:resource="http://vocab.nerc.ac.uk/collection/L05/current/134"/>
	<skos:scopeNote xml:lang="en">manufacturer:Sea-Bird Electronics Inc.</skos:scopeNote>
</rdf:Description>

<rdf:Description rdf:about="http://vocab.nerc.ac.uk/collection/L22/current/TOOL0267">
	<rdf:type rdf:resource="http://www.w3.org/2000/01/rdf-schema#Resource"/>
	<rdf:type rdf:resource="http://www.w3.org/2004/02/skos/core#Concept"/>
	<dcterms:created rdf:datatype="http://www.w3.org/2001/XMLSchema#dateTime">2014-02-06T00:00:00Z</dcterms:created>
	<dc:publisher rdf:datatype="http://www.w3.org/2001/XMLSchema#string">British Oceanographic Data Centre (BODC)</dc:publisher>
	<dc:source rdf:datatype="http://www.w3.org/2001/XMLSchema#string">(L221) SeaVoX Device Catalogue</dc:source>
	<skos:definition xml:lang="en">An underwater temperature recorder in either a plastic (400m) or titanium (11000m) casing.  Temperature average resolution is 0.013C and accuracy is +-0.05C over a range -2C to 40C: clock accuray better than 1 minute per month. Temperature equilibration: 63% 18 seconds (plastic case) or 6 seconds (titanium case); 100% 3 minutes (plastic case) or 1 minute (titanium case).</skos:definition>
	<skos:inScheme rdf:resource="http://vocab.aodn.org.au/def/instrument/1"/>
	<skos:prefLabel xml:lang="en">Star-Oddi Starmon mini temperature recorder</skos:prefLabel>
	<skos:broader rdf:resource="http://vocab.nerc.ac.uk/collection/L05/current/134"/>
	<skos:scopeNote xml:lang="en">manufacturer:Star-Oddi</skos:scopeNote>
</rdf:Description>

<rdf:Description rdf:about="http://vocab.nerc.ac.uk/collection/L22/current/TOOL0416">
	<rdf:type rdf:resource="http://www.w3.org/2000/01/rdf-schema#Resource"/>
	<rdf:type rdf:resource="http://www.w3.org/2004/02/skos/core#Concept"/>
	<dcterms:created rdf:datatype="http://www.w3.org/2001/XMLSchema#dateTime">2014-07-21T00:00:00Z</dcterms:created>
	<dc:publisher rdf:datatype="http://www.w3.org/2001/XMLSchema#string">British Oceanographic Data Centre (BODC)</dc:publisher>
	<dc:source rdf:datatype="http://www.w3.org/2001/XMLSchema#string">(L221) SeaVoX Device Catalogue</dc:source>
	<skos:definition xml:lang="en">Water temperature sensor designed for use on the SBE 9plus CTD system. The sensor operates over the range -5 to +35 °C, a resolution of 0.0003 °C at 24 Hz and an initial accuracy of ± 0.001 °C. The typical sampling rate is 24 Hz, and the sensor has a depth rating of 6800 meters (aluminum housing) or 10500 meters (titanium housing).</skos:definition>
	<skos:inScheme rdf:resource="http://vocab.aodn.org.au/def/instrument/1"/>
	<skos:prefLabel xml:lang="en">Sea-Bird SBE 3plus (SBE 3P) temperature sensor</skos:prefLabel>
	<skos:broader rdf:resource="http://vocab.nerc.ac.uk/collection/L05/current/134"/>
</rdf:Description>

<rdf:Description rdf:about="http://vocab.nerc.ac.uk/collection/L22/current/TOOL0490">
	<rdf:type rdf:resource="http://www.w3.org/2000/01/rdf-schema#Resource"/>
	<rdf:type rdf:resource="http://www.w3.org/2004/02/skos/core#Concept"/>
	<dcterms:created rdf:datatype="http://www.w3.org/2001/XMLSchema#dateTime">2014-02-06T00:00:00Z</dcterms:created>
	<dc:publisher rdf:datatype="http://www.w3.org/2001/XMLSchema#string">British Oceanographic Data Centre (BODC)</dc:publisher>
	<dc:source rdf:datatype="http://www.w3.org/2001/XMLSchema#string">(L221) SeaVoX Device Catalogue</dc:source>
	<skos:definition xml:lang="en">A miniature underwater data logger which measures temperature, pressure and pitch and roll (tilt angle) relative to the earth gravity. It has a range of depth ratings from 30 m to 3000 m and a temperature range of -1 degC to 40 degC with an accuracy of +/- 0.1 degC and a resolution of 0.032 degC. The tilt range is 160 deg (+/- 80 deg) with an accuracy of +/- 5deg and a resolution of 0.3 deg.</skos:definition>
	<skos:inScheme rdf:resource="http://vocab.aodn.org.au/def/instrument/1"/>
	<skos:prefLabel xml:lang="en">Star-Oddi DST Pitch and Roll Recorder</skos:prefLabel>
	<skos:broader rdf:resource="http://vocab.nerc.ac.uk/collection/L05/current/134"/>
	<skos:broader rdf:resource="http://vocab.nerc.ac.uk/collection/L05/current/385"/>
	<skos:scopeNote xml:lang="en">manufacturer:Star-Oddi</skos:scopeNote>
</rdf:Description>

<rdf:Description rdf:about="http://vocab.nerc.ac.uk/collection/L22/current/TOOL0640">
	<rdf:type rdf:resource="http://www.w3.org/2000/01/rdf-schema#Resource"/>
	<rdf:type rdf:resource="http://www.w3.org/2004/02/skos/core#Concept"/>
	<dcterms:created rdf:datatype="http://www.w3.org/2001/XMLSchema#dateTime">2013-10-31T00:00:00Z</dcterms:created>
	<dc:publisher rdf:datatype="http://www.w3.org/2001/XMLSchema#string">British Oceanographic Data Centre (BODC)</dc:publisher>
	<dc:source rdf:datatype="http://www.w3.org/2001/XMLSchema#string">(L221) SeaVoX Device Catalogue</dc:source>
	<skos:definition xml:lang="en">Water temperature sensor primarily designed for use on the SBE 25 and 25plus Sealogger CTD systems but can be used as a component in custom oceanographic profiling systems or high-accuracy temperature-monitoring applications. The sensor operates over the range -5 to +35 degC and has an initial accuracy of +/-0.001 degC. The sensor has a depth rating of 6800 m (aluminum housing) or 10500 m (titanium housing). The SBE 3F is an enhanced version of the SBE 3 temperature sensor.</skos:definition>
	<skos:inScheme rdf:resource="http://vocab.aodn.org.au/def/instrument/1"/>
	<skos:prefLabel xml:lang="en">Sea-Bird SBE 3F temperature sensor</skos:prefLabel>
	<skos:broader rdf:resource="http://vocab.nerc.ac.uk/collection/L05/current/134"/>
	<skos:scopeNote xml:lang="en">manufacturer:Sea-Bird Electronics Inc.</skos:scopeNote>
</rdf:Description>

<rdf:Description rdf:about="http://vocab.nerc.ac.uk/collection/L22/current/TOOL0665">
	<rdf:type rdf:resource="http://www.w3.org/2000/01/rdf-schema#Resource"/>
	<rdf:type rdf:resource="http://www.w3.org/2004/02/skos/core#Concept"/>
	<dcterms:created rdf:datatype="http://www.w3.org/2001/XMLSchema#dateTime">2014-08-06T00:00:00Z</dcterms:created>
	<dc:publisher rdf:datatype="http://www.w3.org/2001/XMLSchema#string">British Oceanographic Data Centre (BODC)</dc:publisher>
	<dc:source rdf:datatype="http://www.w3.org/2001/XMLSchema#string">(L221) SeaVoX Device Catalogue</dc:source>
	<skos:definition xml:lang="en">A miniature data logger that records temperature and depth at a user programmed time interval. 12-bit version gives a resolution of 0.015 degC and an accuracy of +/-0.1 degC. It is housed in a waterproof cylinder and the temperature sensor is mounted on a protruding stainless steel probe.</skos:definition>
	<skos:inScheme rdf:resource="http://vocab.aodn.org.au/def/instrument/1"/>
	<skos:prefLabel xml:lang="en">Vemco Minilog12 temperature-pressure recorder</skos:prefLabel>
	<skos:broader rdf:resource="http://vocab.nerc.ac.uk/collection/L05/current/134"/>
</rdf:Description>

<rdf:Description rdf:about="http://vocab.nerc.ac.uk/collection/L22/current/TOOL0670">
	<rdf:type rdf:resource="http://www.w3.org/2000/01/rdf-schema#Resource"/>
	<rdf:type rdf:resource="http://www.w3.org/2004/02/skos/core#Concept"/>
	<dcterms:created rdf:datatype="http://www.w3.org/2001/XMLSchema#dateTime">2013-10-15T00:00:00Z</dcterms:created>
	<dc:publisher rdf:datatype="http://www.w3.org/2001/XMLSchema#string">British Oceanographic Data Centre (BODC)</dc:publisher>
	<dc:source rdf:datatype="http://www.w3.org/2001/XMLSchema#string">(L221) SeaVoX Device Catalogue</dc:source>
	<skos:definition xml:lang="en">A high-accuracy temperature recorder with non-volatile memory and RS-232 port, designed for shipboard determination of sea surface temperature. It is magnetically fixed just below the water line with the temperature sensor in contact with the inside of the ship's hull. The thermistor is the same as the SBE 39 which has an accuracy of 0.002C, stability of 0.0002 C/month and resolution of 0.0001 C .  A real-time clock accurate within 1 minute/year is included for self-contained operation. More information is given in http://www.seabird.com/pdf_documents/manuals/48_004.pdf.</skos:definition>
	<skos:inScheme rdf:resource="http://vocab.aodn.org.au/def/instrument/1"/>
	<skos:prefLabel xml:lang="en">Sea-Bird SBE 48 Hull Temperature Sensor</skos:prefLabel>
	<skos:broader rdf:resource="http://vocab.nerc.ac.uk/collection/L05/current/134"/>
	<skos:scopeNote xml:lang="en">manufacturer:Sea-Bird Electronics Inc.</skos:scopeNote>
</rdf:Description>

<rdf:Description rdf:about="http://vocab.nerc.ac.uk/collection/L22/current/TOOL0684">
	<rdf:type rdf:resource="http://www.w3.org/2000/01/rdf-schema#Resource"/>
	<rdf:type rdf:resource="http://www.w3.org/2004/02/skos/core#Concept"/>
	<dcterms:created rdf:datatype="http://www.w3.org/2001/XMLSchema#dateTime">2014-06-04T00:00:00Z</dcterms:created>
	<dc:publisher rdf:datatype="http://www.w3.org/2001/XMLSchema#string">British Oceanographic Data Centre (BODC)</dc:publisher>
	<dc:source rdf:datatype="http://www.w3.org/2001/XMLSchema#string">(L221) SeaVoX Device Catalogue</dc:source>
	<skos:definition xml:lang="en">A miniature (200mm long, 32mm diameter) self-contained data logger incorporating a thermistor temperature sensor (resolution better that 0.007C, accuracy 0.05C) in a housing designed to operate at depths down to 1000m.  The logger may be programmed to provide a wide variety of sampling regimes, including burst recording. More information may be found in http://www.aquatecgroup.com/images/manual_guides/bg%20-%20520.pdf.</skos:definition>
	<skos:inScheme rdf:resource="http://vocab.aodn.org.au/def/instrument/1"/>
	<skos:prefLabel xml:lang="en">Aquatech AQUAlogger 520T mini temperature logger</skos:prefLabel>
	<skos:broader rdf:resource="http://vocab.nerc.ac.uk/collection/L05/current/134"/>
</rdf:Description>

<rdf:Description rdf:about="http://vocab.nerc.ac.uk/collection/L22/current/TOOL0687">
	<rdf:type rdf:resource="http://www.w3.org/2000/01/rdf-schema#Resource"/>
	<rdf:type rdf:resource="http://www.w3.org/2004/02/skos/core#Concept"/>
	<dcterms:created rdf:datatype="http://www.w3.org/2001/XMLSchema#dateTime">2014-06-05T00:00:00Z</dcterms:created>
	<dc:publisher rdf:datatype="http://www.w3.org/2001/XMLSchema#string">British Oceanographic Data Centre (BODC)</dc:publisher>
	<dc:source rdf:datatype="http://www.w3.org/2001/XMLSchema#string">(L221) SeaVoX Device Catalogue</dc:source>
	<skos:definition xml:lang="en">This is a small (30cm by 2.54cm diameter) high-accuracy battery-powered temperature and time logger capable of sampling intervals from 0.5 seconds to 9 hours. Battery life with a sampling rate of 15 seconds is almost two years and the memory can store over 15 million samples. Temperature is measured by a pressure-protected (1500m depth) thermistor. Initial accuracy is 0.002C and drift is typically less than 0.002C per year. More information may be found at http://www.seabird.com/products/spec_sheets/39imdata.htm.</skos:definition>
	<skos:inScheme rdf:resource="http://vocab.aodn.org.au/def/instrument/1"/>
	<skos:prefLabel xml:lang="en">Sea-Bird SBE 56 temperature recorder</skos:prefLabel>
	<skos:broader rdf:resource="http://vocab.nerc.ac.uk/collection/L05/current/134"/>
</rdf:Description>

<rdf:Description rdf:about="http://vocab.nerc.ac.uk/collection/L22/current/TOOL0688">
	<rdf:type rdf:resource="http://www.w3.org/2000/01/rdf-schema#Resource"/>
	<rdf:type rdf:resource="http://www.w3.org/2004/02/skos/core#Concept"/>
	<dcterms:created rdf:datatype="http://www.w3.org/2001/XMLSchema#dateTime">2014-06-05T00:00:00Z</dcterms:created>
	<dc:publisher rdf:datatype="http://www.w3.org/2001/XMLSchema#string">British Oceanographic Data Centre (BODC)</dc:publisher>
	<dc:source rdf:datatype="http://www.w3.org/2001/XMLSchema#string">(L221) SeaVoX Device Catalogue</dc:source>
	<skos:definition xml:lang="en">A high-accuracy temperature recorder (pressure optional) with internal battery and a built-in inductive modem intended for moorings with either real-time telemetry or a surface data logger.  Data are also stored in internal non-volatile memory as insurance against data loss.  Calibration coefficients stored in EEPROM allow the SBE 39 to transmit data in engineering units. The SBE 39 thermistor has a long history of exceptional initial accuracy (0.002C) and stability (typical drift is 0.0002C per month).  The standard plastic housing is for depths down to 600m, but an optional titanium housing can withstand depths of 10500m.  For more information see http://www.seabird.com/products/spec_sheets/39imdata.htm.</skos:definition>
	<skos:inScheme rdf:resource="http://vocab.aodn.org.au/def/instrument/1"/>
	<skos:prefLabel xml:lang="en">Sea-Bird SBE 39-IM temperature recorder</skos:prefLabel>
	<skos:broader rdf:resource="http://vocab.nerc.ac.uk/collection/L05/current/134"/>
</rdf:Description>

<rdf:Description rdf:about="http://vocab.nerc.ac.uk/collection/L22/current/TOOL0706">
	<rdf:type rdf:resource="http://www.w3.org/2000/01/rdf-schema#Resource"/>
	<rdf:type rdf:resource="http://www.w3.org/2004/02/skos/core#Concept"/>
	<dcterms:created rdf:datatype="http://www.w3.org/2001/XMLSchema#dateTime">2014-06-16T00:00:00Z</dcterms:created>
	<dc:publisher rdf:datatype="http://www.w3.org/2001/XMLSchema#string">British Oceanographic Data Centre (BODC)</dc:publisher>
	<dc:source rdf:datatype="http://www.w3.org/2001/XMLSchema#string">(L221) SeaVoX Device Catalogue</dc:source>
	<skos:definition xml:lang="en">The VEMCO Minilog II T is a fully submersible, 10-year temperature data logger measures and stores temperature at specified sampling intervals. The Minilog- II-T data logger is manufactured to withstand both fresh and saltwater environments.</skos:definition>
	<skos:inScheme rdf:resource="http://vocab.aodn.org.au/def/instrument/1"/>
	<skos:prefLabel xml:lang="en">Vemco Minilog II T 16-bit Temperature Logger</skos:prefLabel>
	<skos:broader rdf:resource="http://vocab.nerc.ac.uk/collection/L05/current/134"/>
</rdf:Description>

<rdf:Description rdf:about="http://vocab.nerc.ac.uk/collection/L22/current/TOOL0707">
	<rdf:type rdf:resource="http://www.w3.org/2000/01/rdf-schema#Resource"/>
	<rdf:type rdf:resource="http://www.w3.org/2004/02/skos/core#Concept"/>
	<dcterms:created rdf:datatype="http://www.w3.org/2001/XMLSchema#dateTime">2013-10-15T00:00:00Z</dcterms:created>
	<dc:publisher rdf:datatype="http://www.w3.org/2001/XMLSchema#string">British Oceanographic Data Centre (BODC)</dc:publisher>
	<dc:source rdf:datatype="http://www.w3.org/2001/XMLSchema#string">(L221) SeaVoX Device Catalogue</dc:source>
	<skos:definition xml:lang="en">This is a 2-terminal integrated circuit temperature transducer that produces an output current proportional to absolute temperature (one microAmp per Kelvin). It is calibrated by laser trimming of the resistors on the chip to produce an output of 298.2 microAmps at 298.2K. It is supplied in a range of standard electronic component packages for inclusion on circuit boards. It can operate from -55-150C, is linear to 0.3C over full range and has an accuracy of 0.5C. Further details may be found at http://www.analog.com/en/mems-sensors/digital-temperature-sensors/ad590/products/product.html.</skos:definition>
	<skos:inScheme rdf:resource="http://vocab.aodn.org.au/def/instrument/1"/>
	<skos:prefLabel xml:lang="en">Analog Devices AD590 Temperature Transducer</skos:prefLabel>
	<skos:broader rdf:resource="http://vocab.nerc.ac.uk/collection/L05/current/134"/>
	<skos:scopeNote xml:lang="en">manufacturer:Analog Devices</skos:scopeNote>
</rdf:Description>

<rdf:Description rdf:about="http://vocab.nerc.ac.uk/collection/L22/current/TOOL0712">
	<rdf:type rdf:resource="http://www.w3.org/2000/01/rdf-schema#Resource"/>
	<rdf:type rdf:resource="http://www.w3.org/2004/02/skos/core#Concept"/>
	<dcterms:created rdf:datatype="http://www.w3.org/2001/XMLSchema#dateTime">2013-10-15T00:00:00Z</dcterms:created>
	<dc:publisher rdf:datatype="http://www.w3.org/2001/XMLSchema#string">British Oceanographic Data Centre (BODC)</dc:publisher>
	<dc:source rdf:datatype="http://www.w3.org/2001/XMLSchema#string">(L221) SeaVoX Device Catalogue</dc:source>
	<skos:definition xml:lang="en">A compact fully integrated sensor for measuring the water temperature. The sensor is designed to be mounted on Aanderaa recording instruments (e.g. RCM 9/11 doppler current meter) and data loggers. The sensor can also be used as stand alone, and is easily integrated in other measurement systems with third party data loggers. Resolution is 0.001 C and accuracy is 0.03 C. Further development of the 4050 has been suspended in favour of the replacement 4060 model. More information may be found in http://www.aanderaa.com/productsdetail.php?Temperature-Sensor-12.</skos:definition>
	<skos:inScheme rdf:resource="http://vocab.aodn.org.au/def/instrument/1"/>
	<skos:prefLabel xml:lang="en">Aanderaa temperature sensor 4050</skos:prefLabel>
	<skos:broader rdf:resource="http://vocab.nerc.ac.uk/collection/L05/current/134"/>
	<skos:scopeNote xml:lang="en">manufacturer:Aanderaa Data Instruments</skos:scopeNote>
</rdf:Description>

<rdf:Description rdf:about="http://vocab.nerc.ac.uk/collection/L22/current/TOOL0719">
	<rdf:type rdf:resource="http://www.w3.org/2000/01/rdf-schema#Resource"/>
	<rdf:type rdf:resource="http://www.w3.org/2004/02/skos/core#Concept"/>
	<dcterms:contributor rdf:resource="http://editor.vocabs.ands.org.au/user/Natalia_Atkins"/>
	<dcterms:created rdf:datatype="http://www.w3.org/2001/XMLSchema#dateTime">2015-07-08T00:00:00Z</dcterms:created>
	<dcterms:modified rdf:datatype="http://www.w3.org/2001/XMLSchema#dateTime">2015-07-17T01:39:47Z</dcterms:modified>
	<dc:publisher rdf:datatype="http://www.w3.org/2001/XMLSchema#string">British Oceanographic Data Centre (BODC)</dc:publisher>
	<dc:source rdf:datatype="http://www.w3.org/2001/XMLSchema#string">(L221) SeaVoX Device Catalogue</dc:source>
	<skos:definition xml:lang="en">A depth and temperature sensor package combined with an RF unit and antenna suitable for transmission of data via the Argos satellite system. The unit contains an internal battery and a microprocessor that logs data and schedules the transfer of data. The package is designed for attachment to marine mammals and has an operational depth range of down to 2000 m. It is built and calibrated at Valeport Ltd, while SMRU Ltd, the commercial arm of the Sea Mammal Research Unit of the University of St Andrews, is responsible for its distribution, and for streaming and processing the data. More information is available at http://www.smru.st-and.ac.uk/Instrumentation/SRDL/.</skos:definition>
	<skos:inScheme rdf:resource="http://vocab.aodn.org.au/instrument/1"/>
	<skos:prefLabel xml:lang="en">SMRU Ltd Satellite Relay Data Logger 9000x</skos:prefLabel>
	<skos:broader rdf:resource="http://vocab.nerc.ac.uk/collection/L05/current/134"/>
	<skos:broader rdf:resource="http://vocab.nerc.ac.uk/collection/L05/current/POS17"/>
	<skos:altLabel xml:lang="en">SMRU Ltd SRDL 9000x</skos:altLabel>
</rdf:Description>

<rdf:Description rdf:about="http://vocab.nerc.ac.uk/collection/L22/current/TOOL0728">
	<rdf:type rdf:resource="http://www.w3.org/2000/01/rdf-schema#Resource"/>
	<rdf:type rdf:resource="http://www.w3.org/2004/02/skos/core#Concept"/>
	<dcterms:created rdf:datatype="http://www.w3.org/2001/XMLSchema#dateTime">2014-07-14T00:00:00Z</dcterms:created>
	<dc:publisher rdf:datatype="http://www.w3.org/2001/XMLSchema#string">British Oceanographic Data Centre (BODC)</dc:publisher>
	<dc:source rdf:datatype="http://www.w3.org/2001/XMLSchema#string">(L221) SeaVoX Device Catalogue</dc:source>
	<skos:definition xml:lang="en">The TR-1060P is a small, self-contained, submersible temperature logger calibrated to +/-0.002 degC, with a typical calibration drift of less than 0.002 degC per year. It is a 25mm diameter version of the TR-1050, but has the same or better performance with a 24 bit a/d. It can be deployed for a period of up to three years and can collect more than 2,400,000 samples. Data are retained in memory for 20 years (even without batteries).  It has a depth rating of 1200 m, download speed ~115000 samples per minute, clock accuracy +/- 32 seconds per year, 8 Mb flash memory, and 240mm x 25 mm casing. Measures temperature from -5 to 35 degC, but can be calibrated to a wider range on request. Accuracy is +/-0.002 degC, resolution better than 0.00005 degC.</skos:definition>
	<skos:inScheme rdf:resource="http://vocab.aodn.org.au/def/instrument/1"/>
	<skos:prefLabel xml:lang="en">RBR TR-1060P Temperature Logger</skos:prefLabel>
	<skos:broader rdf:resource="http://vocab.nerc.ac.uk/collection/L05/current/134"/>
</rdf:Description>

<rdf:Description rdf:about="http://vocab.nerc.ac.uk/collection/L22/current/TOOL1121">
	<rdf:type rdf:resource="http://www.w3.org/2000/01/rdf-schema#Resource"/>
	<rdf:type rdf:resource="http://www.w3.org/2004/02/skos/core#Concept"/>
	<dcterms:created rdf:datatype="http://www.w3.org/2001/XMLSchema#dateTime">2017-04-10T00:00:00Z</dcterms:created>
	<dc:publisher rdf:datatype="http://www.w3.org/2001/XMLSchema#string">British Oceanographic Data Centre (BODC)</dc:publisher>
	<skos:definition xml:lang="en">A miniature data logger that measures and records temperature, depth (pressure) and tilt (in three directions) in relation to earth's gravity field. It is mainly used for monitoring orientation of underwater gear or movements of marine animals. Recorded data is stored in the logger‘s internal memory with a real-time clock reference for each measurement. Tilt measuring range is +/-90 degrees for each of the axis X, Y and Z.</skos:definition>
	<skos:inScheme rdf:resource="http://vocab.aodn.org.au/def/instrument/1"/>
	<skos:prefLabel xml:lang="en">Star-Oddi DST Tilt platform orientation sensor</skos:prefLabel>
	<skos:broader rdf:resource="http://vocab.nerc.ac.uk/collection/L05/current/134"/>
	<skos:broader rdf:resource="http://vocab.nerc.ac.uk/collection/L05/current/385"/>
	<skos:broader rdf:resource="http://vocab.nerc.ac.uk/collection/L05/current/WPS"/>
	<skos:altLabel xml:lang="en">Star-Oddi Tilt</skos:altLabel>
</rdf:Description>

<rdf:Description rdf:about="http://vocab.nerc.ac.uk/collection/L22/current/TOOL1122">
	<rdf:type rdf:resource="http://www.w3.org/2000/01/rdf-schema#Resource"/>
	<rdf:type rdf:resource="http://www.w3.org/2004/02/skos/core#Concept"/>
	<dcterms:created rdf:datatype="http://www.w3.org/2001/XMLSchema#dateTime">2017-04-10T00:00:00Z</dcterms:created>
	<dc:publisher rdf:datatype="http://www.w3.org/2001/XMLSchema#string">British Oceanographic Data Centre (BODC)</dc:publisher>
	<skos:definition xml:lang="en">A water body temperature sensor. It is designed for moorings or other long-duration, fixed-site deployments, as well as deployments on nets, towed vehicles, or ROVs. It uses an aged and pressure-protected thermistor that is available in two configurations: embedded in titanium endcap (25-sec time constant) for rugged conditions, or external thermistor in pressure-protected sheath (0.5-sec time constant) for fast sampling. It can be fitted with an optional strain-gauge pressure sensor with temperature compensation available in eight ranges (maximum depth 7000 m). Sensor housing is either PET plastic or titanium. The temperature sensor has a measurement range of -5 to +45 deg C, an accuracy of +/- 0.002 (-5 to +35 deg C) or +/- 0.01 (+35 to +45 deg C) and a depth rating of 600 m (plastic) or 10,500 m (titanium).</skos:definition>
	<skos:inScheme rdf:resource="http://vocab.aodn.org.au/def/instrument/1"/>
	<skos:prefLabel xml:lang="en">Sea-Bird SBE 39plus temperature sensor</skos:prefLabel>
	<skos:broader rdf:resource="http://vocab.nerc.ac.uk/collection/L05/current/134"/>
	<skos:broader rdf:resource="http://vocab.nerc.ac.uk/collection/L05/current/WPS"/>
	<skos:altLabel xml:lang="en">SBE 39plus</skos:altLabel>
</rdf:Description>

<rdf:Description rdf:about="http://vocab.nerc.ac.uk/collection/L22/current/TOOL0528">
	<rdf:type rdf:resource="http://www.w3.org/2000/01/rdf-schema#Resource"/>
	<rdf:type rdf:resource="http://www.w3.org/2004/02/skos/core#Concept"/>
	<dcterms:created rdf:datatype="http://www.w3.org/2001/XMLSchema#dateTime">2014-02-07T00:00:00Z</dcterms:created>
	<dc:publisher rdf:datatype="http://www.w3.org/2001/XMLSchema#string">British Oceanographic Data Centre (BODC)</dc:publisher>
	<dc:source rdf:datatype="http://www.w3.org/2001/XMLSchema#string">(L221) SeaVoX Device Catalogue</dc:source>
	<skos:definition xml:lang="en">An active optical instrument with an internal UV light source and spectrometer used to measure in-situ dissolved nitrate. It is a chemical-free method that allows real-time and continuous nitrate concentration measurements in a variety of environments. It uses a Deuterium lamp as a light source and has a 1cm path length and 200-400 nm wavelength range. It has a depth rating of 1000 m and a detection range of  0.5 to 2000 uM *(0.007 to 28 mg/l-N)  and accuracy of +/- 0.2 uM (0.028 mg/l) or ± 10% of reading, whichever is greater. The V3 has USB data transfer ability and window based software.</skos:definition>
	<skos:inScheme rdf:resource="http://vocab.aodn.org.au/def/instrument/1"/>
	<skos:prefLabel xml:lang="en">Satlantic ISUS V3 Nitrate Sensor</skos:prefLabel>
	<skos:broader rdf:resource="http://vocab.nerc.ac.uk/collection/L05/current/181"/>
	<skos:scopeNote xml:lang="en">manufacturer:Satlantic</skos:scopeNote>
</rdf:Description>

<rdf:Description rdf:about="http://vocab.nerc.ac.uk/collection/L22/current/NETT0026">
	<rdf:type rdf:resource="http://www.w3.org/2000/01/rdf-schema#Resource"/>
	<rdf:type rdf:resource="http://www.w3.org/2004/02/skos/core#Concept"/>
	<dcterms:created rdf:datatype="http://www.w3.org/2001/XMLSchema#dateTime">2014-02-26T00:00:00Z</dcterms:created>
	<dc:publisher rdf:datatype="http://www.w3.org/2001/XMLSchema#string">British Oceanographic Data Centre (BODC)</dc:publisher>
	<dc:source rdf:datatype="http://www.w3.org/2001/XMLSchema#string">(L221) SeaVoX Device Catalogue</dc:source>
	<skos:definition xml:lang="en">Construction is a 1.27 cm on side square mouth opening (originally 10.1 cm diameter) high-speed (12 to 17 knots) towed body collecting plankton on gauze (22.9 cm wide and 23.6 meshes per cm) rolls. The body is 50 cm wide x 50 cm tall x 100 cm long.  A propellor drives the rollers winding up the gauze.  The system is normally towed at 10 m depth at speeds up to 20 ktnos [Wiebe and Benfield 2003 Plate 19 A, B].</skos:definition>
	<skos:inScheme rdf:resource="http://vocab.aodn.org.au/def/instrument/1"/>
	<skos:prefLabel xml:lang="en">Continuous Plankton Recorder - Hardy (1926, 1936); Glover (1962)</skos:prefLabel>
	<skos:broader rdf:resource="http://vocab.nerc.ac.uk/collection/L05/current/21"/>
</rdf:Description>

<rdf:Description rdf:about="http://vocab.nerc.ac.uk/collection/L22/current/NETT0044">
	<rdf:type rdf:resource="http://www.w3.org/2000/01/rdf-schema#Resource"/>
	<rdf:type rdf:resource="http://www.w3.org/2004/02/skos/core#Concept"/>
	<dcterms:created rdf:datatype="http://www.w3.org/2001/XMLSchema#dateTime">2014-02-03T00:00:00Z</dcterms:created>
	<dc:publisher rdf:datatype="http://www.w3.org/2001/XMLSchema#string">British Oceanographic Data Centre (BODC)</dc:publisher>
	<dc:source rdf:datatype="http://www.w3.org/2001/XMLSchema#string">(L221) SeaVoX Device Catalogue</dc:source>
	<skos:definition xml:lang="en">A modified WP2 cylinder-cone closing net (mesh not specified) which is allowed to free-fall and then is strangled shut and retrieved.  [Wiebe and Benfield 2003 Plate 10C]</skos:definition>
	<skos:inScheme rdf:resource="http://vocab.aodn.org.au/def/instrument/1"/>
	<skos:prefLabel xml:lang="en">Free-fall plankton net - Heron (1982)</skos:prefLabel>
	<skos:broader rdf:resource="http://vocab.nerc.ac.uk/collection/L05/current/22"/>
</rdf:Description>

<rdf:Description rdf:about="http://vocab.nerc.ac.uk/collection/L22/current/TOOL1016">
	<rdf:type rdf:resource="http://www.w3.org/2000/01/rdf-schema#Resource"/>
	<rdf:type rdf:resource="http://www.w3.org/2004/02/skos/core#Concept"/>
	<dcterms:created rdf:datatype="http://www.w3.org/2001/XMLSchema#dateTime">2017-03-13T00:00:00Z</dcterms:created>
	<dc:publisher rdf:datatype="http://www.w3.org/2001/XMLSchema#string">British Oceanographic Data Centre (BODC)</dc:publisher>
	<skos:definition xml:lang="en">An autonomous radiometer developed by the University of Southampton (UK) and Brookhaven National Laboratories (US) for satellite Sea Surface Temperature (SST) validation and other scientific programs. It detects infrared temperature using a single channel with a spectral bandpass of 9.6–11.5 um. It is compact (570 mm × 220 mm cylinder) and employs two reference blackbody cavities to maintain the radiance calibration of a special Heitronics KT15.85D radiometer to an accuracy of +/-0.1K. It has a temperature range of 173–373 K. It can be deployed continuously on voluntary observing ships (VOS) without any service requirement or operator intervention for periods of up to 3 months. http://dx.doi.org/10.1175/2007JTECHO505.1</skos:definition>
	<skos:inScheme rdf:resource="http://vocab.aodn.org.au/def/instrument/1"/>
	<skos:prefLabel xml:lang="en">University of Southampton ISAR SST radiometer</skos:prefLabel>
	<skos:broader rdf:resource="http://vocab.nerc.ac.uk/collection/L05/current/302"/>
	<skos:altLabel xml:lang="en">UOS ISAR SST</skos:altLabel>
</rdf:Description>

<rdf:Description rdf:about="http://vocab.nerc.ac.uk/collection/L22/current/TOOL1120">
	<rdf:type rdf:resource="http://www.w3.org/2000/01/rdf-schema#Resource"/>
	<rdf:type rdf:resource="http://www.w3.org/2004/02/skos/core#Concept"/>
	<dcterms:created rdf:datatype="http://www.w3.org/2001/XMLSchema#dateTime">2017-04-10T00:00:00Z</dcterms:created>
	<dc:publisher rdf:datatype="http://www.w3.org/2001/XMLSchema#string">British Oceanographic Data Centre (BODC)</dc:publisher>
	<skos:definition xml:lang="en">A CIMEL CE 318 Sun Photometer that has been modified to validate satellite ocean colour measurements in the AERONET-OC network. It autonomously performs sky and sea radiance observations at programmable viewing and azimuth angles at centre wavelengths in the 412-1020 nanometre spectral range.</skos:definition>
	<skos:inScheme rdf:resource="http://vocab.aodn.org.au/def/instrument/1"/>
	<skos:prefLabel xml:lang="en">AERONET SeaWIFS SeaPRISM radiometer</skos:prefLabel>
	<skos:broader rdf:resource="http://vocab.nerc.ac.uk/collection/L05/current/304"/>
	<skos:broader rdf:resource="http://vocab.nerc.ac.uk/collection/L05/current/308"/>
	<skos:altLabel xml:lang="en">AERONET SeaPRISM</skos:altLabel>
</rdf:Description>

<rdf:Description rdf:about="http://vocab.nerc.ac.uk/collection/L22/current/TOOL0702">
	<rdf:type rdf:resource="http://www.w3.org/2000/01/rdf-schema#Resource"/>
	<rdf:type rdf:resource="http://www.w3.org/2004/02/skos/core#Concept"/>
	<dcterms:created rdf:datatype="http://www.w3.org/2001/XMLSchema#dateTime">2014-07-11T00:00:00Z</dcterms:created>
	<dc:publisher rdf:datatype="http://www.w3.org/2001/XMLSchema#string">British Oceanographic Data Centre (BODC)</dc:publisher>
	<dc:source rdf:datatype="http://www.w3.org/2001/XMLSchema#string">(L221) SeaVoX Device Catalogue</dc:source>
	<skos:definition xml:lang="en">The CNR4 is a net radiometer that measures the energy balance between incoming and shortwave IR radiation versus surface reflected shortwave and outgoing longwave IR radiation. The instrument comprises an upward-facing pyranometer/pyrgeometer pair, and a downward facing pair. There is an internal thermisor, an internal Pt-100 RTD, and a solar shield. There is an optional ventilation unit with heater to minimise condensation.</skos:definition>
	<skos:inScheme rdf:resource="http://vocab.aodn.org.au/def/instrument/1"/>
	<skos:prefLabel xml:lang="en">Kipp and Zonen CNR4 Net Radiometer</skos:prefLabel>
	<skos:broader rdf:resource="http://vocab.nerc.ac.uk/collection/L05/current/308"/>
</rdf:Description>

<rdf:Description rdf:about="http://vocab.nerc.ac.uk/collection/L22/current/TOOL0703">
	<rdf:type rdf:resource="http://www.w3.org/2000/01/rdf-schema#Resource"/>
	<rdf:type rdf:resource="http://www.w3.org/2004/02/skos/core#Concept"/>
	<dcterms:created rdf:datatype="http://www.w3.org/2001/XMLSchema#dateTime">2014-07-11T00:00:00Z</dcterms:created>
	<dc:publisher rdf:datatype="http://www.w3.org/2001/XMLSchema#string">British Oceanographic Data Centre (BODC)</dc:publisher>
	<dc:source rdf:datatype="http://www.w3.org/2001/XMLSchema#string">(L221) SeaVoX Device Catalogue</dc:source>
	<skos:definition xml:lang="en">The CNR4 is a net radiometer that measures the energy balance between incoming and shortwave IR radiation versus surface reflected shortwave and outgoing longwave IR radiation. The instrument comprises an upward-facing pyranometer/pyrgeometer pair, and a downward facing pair. There is an internal RTD, and a heater to prevent condensation.</skos:definition>
	<skos:inScheme rdf:resource="http://vocab.aodn.org.au/def/instrument/1"/>
	<skos:prefLabel xml:lang="en">Kipp and Zonen CNR1 Net Radiometer</skos:prefLabel>
	<skos:broader rdf:resource="http://vocab.nerc.ac.uk/collection/L05/current/308"/>
</rdf:Description>

<rdf:Description rdf:about="http://vocab.nerc.ac.uk/collection/L22/current/TOOL0722">
	<rdf:type rdf:resource="http://www.w3.org/2000/01/rdf-schema#Resource"/>
	<rdf:type rdf:resource="http://www.w3.org/2004/02/skos/core#Concept"/>
	<dcterms:created rdf:datatype="http://www.w3.org/2001/XMLSchema#dateTime">2013-10-15T00:00:00Z</dcterms:created>
	<dc:publisher rdf:datatype="http://www.w3.org/2001/XMLSchema#string">British Oceanographic Data Centre (BODC)</dc:publisher>
	<dc:source rdf:datatype="http://www.w3.org/2001/XMLSchema#string">(L221) SeaVoX Device Catalogue</dc:source>
	<skos:definition xml:lang="en">The Middleton EQ08 Solar Pyranometer is designed for the measurement of global solar irradiance on a plane surface. It has a response time (to 95%) of less than 11 seconds; zero offset at 200 W/m2 of less than 3 W/m2 and at 5K/h of less than 2W/m2; non-linearity of less than 0.5 percent; directional response with respect to 1000 W/m2 of less than 15 W/m2, Spectral selectivity (0.35 to 1.5 um) of less than 3 percent; temperature response (for 50K interval) of less than 2 percent; and tilt response (0-90 degrees) of less than 0.35 percent.</skos:definition>
	<skos:inScheme rdf:resource="http://vocab.aodn.org.au/def/instrument/1"/>
	<skos:prefLabel xml:lang="en">Middleton Solar EQ08 Pyranometer</skos:prefLabel>
	<skos:broader rdf:resource="http://vocab.nerc.ac.uk/collection/L05/current/308"/>
	<skos:scopeNote xml:lang="en">manufacturer:Middleton Solar</skos:scopeNote>
</rdf:Description>

<rdf:Description rdf:about="http://vocab.nerc.ac.uk/collection/L22/current/TOOL0723">
	<rdf:type rdf:resource="http://www.w3.org/2000/01/rdf-schema#Resource"/>
	<rdf:type rdf:resource="http://www.w3.org/2004/02/skos/core#Concept"/>
	<dcterms:created rdf:datatype="http://www.w3.org/2001/XMLSchema#dateTime">2013-10-15T00:00:00Z</dcterms:created>
	<dc:publisher rdf:datatype="http://www.w3.org/2001/XMLSchema#string">British Oceanographic Data Centre (BODC)</dc:publisher>
	<dc:source rdf:datatype="http://www.w3.org/2001/XMLSchema#string">(L221) SeaVoX Device Catalogue</dc:source>
	<skos:definition xml:lang="en">The Middleton SK01-DP2 PAR Sensor (or Quantum Sensor) is for measuring electromagnetic radiation  at Photosynthetically Active wavelengths. It uses a silicon photodiode detector, shielded by a cosine-corrected diffuser and an interference reflector, to measure PAR on a horizontal surface. The detector is boosted by a low noise amplifier that is drift stabilised. The SK01-DP2 features: viewing angle 2*pi steradians; spectral range of 400-700nm; irradiance of 0-3000 umol/s/m2; sensitivity of 0.5 mV/umol/s/m2; response time (to 95 percent) of 30 ms; operating temperature of -35 to 60 degreesC; non-linearity of less than 1 percent; spectral response of +/- 5 percent.</skos:definition>
	<skos:inScheme rdf:resource="http://vocab.aodn.org.au/def/instrument/1"/>
	<skos:prefLabel xml:lang="en">Middleton Solar SK01-DP2 Pyranometer</skos:prefLabel>
	<skos:broader rdf:resource="http://vocab.nerc.ac.uk/collection/L05/current/308"/>
	<skos:scopeNote xml:lang="en">manufacturer:Middleton Solar</skos:scopeNote>
</rdf:Description>

<rdf:Description rdf:about="http://vocab.nerc.ac.uk/collection/L22/current/TOOL0785">
	<rdf:type rdf:resource="http://www.w3.org/2000/01/rdf-schema#Resource"/>
	<rdf:type rdf:resource="http://www.w3.org/2004/02/skos/core#Concept"/>
	<dcterms:created rdf:datatype="http://www.w3.org/2001/XMLSchema#dateTime">2013-03-28T00:00:00Z</dcterms:created>
	<dc:publisher rdf:datatype="http://www.w3.org/2001/XMLSchema#string">British Oceanographic Data Centre (BODC)</dc:publisher>
	<dc:source rdf:datatype="http://www.w3.org/2001/XMLSchema#string">(L221) SeaVoX Device Catalogue</dc:source>
	<skos:definition xml:lang="en">A sediment trap designed for mid-water mooring deployment (maximum depth 6500m) with a conical collector passing settled particles into one of a set of bottles mounted in a carousel. The bottles are changed after a user-selected period of time.  An optional wet sample particle divider may be fitted to divide wet specimens into 5-10 equal parts. Compass/tilt and pressure sensors may also be fitted.  This model carries 21 bottles (250 or 500 ml) and is 1.64m tall and 0.91m diameter.</skos:definition>
	<skos:inScheme rdf:resource="http://vocab.aodn.org.au/def/instrument/1"/>
	<skos:prefLabel xml:lang="en">McLane PARFLUX Mark78H-21 Sediment Traps</skos:prefLabel>
	<skos:broader rdf:resource="http://vocab.nerc.ac.uk/collection/L05/current/33"/>
	<skos:altLabel xml:lang="en">PARFLUX Mark78H-21</skos:altLabel>
</rdf:Description>

<rdf:Description rdf:about="http://vocab.nerc.ac.uk/collection/L22/current/TOOL0786">
	<rdf:type rdf:resource="http://www.w3.org/2000/01/rdf-schema#Resource"/>
	<rdf:type rdf:resource="http://www.w3.org/2004/02/skos/core#Concept"/>
	<dcterms:created rdf:datatype="http://www.w3.org/2001/XMLSchema#dateTime">2013-03-28T00:00:00Z</dcterms:created>
	<dc:publisher rdf:datatype="http://www.w3.org/2001/XMLSchema#string">British Oceanographic Data Centre (BODC)</dc:publisher>
	<dc:source rdf:datatype="http://www.w3.org/2001/XMLSchema#string">(L221) SeaVoX Device Catalogue</dc:source>
	<skos:definition xml:lang="en">A sediment trap designed for mid-water mooring deployment (maximum depth 6500m) with a conical collector passing settled particles into one of a set of bottles mounted in a carousel. The bottles are changed after a user-selected period of time.  An optional wet sample particle divider may be fitted to divide wet specimens into 5-10 equal parts. Compass/tilt and pressure sensors may also be fitted. This model carries 13 wide bottles (250 or 500 ml) and is 1.64m tall and 0.91m diameter.</skos:definition>
	<skos:inScheme rdf:resource="http://vocab.aodn.org.au/def/instrument/1"/>
	<skos:prefLabel xml:lang="en">McLane PARFLUX Mark78HW-13 Sediment Traps</skos:prefLabel>
	<skos:broader rdf:resource="http://vocab.nerc.ac.uk/collection/L05/current/33"/>
	<skos:altLabel xml:lang="en">PARFLUX Mark78HW-13</skos:altLabel>
</rdf:Description>

<rdf:Description rdf:about="http://vocab.nerc.ac.uk/collection/L22/current/TOOL0036">
	<rdf:type rdf:resource="http://www.w3.org/2000/01/rdf-schema#Resource"/>
	<rdf:type rdf:resource="http://www.w3.org/2004/02/skos/core#Concept"/>
	<dcterms:created rdf:datatype="http://www.w3.org/2001/XMLSchema#dateTime">2013-09-09T00:00:00Z</dcterms:created>
	<dc:publisher rdf:datatype="http://www.w3.org/2001/XMLSchema#string">British Oceanographic Data Centre (BODC)</dc:publisher>
	<dc:source rdf:datatype="http://www.w3.org/2001/XMLSchema#string">(L221) SeaVoX Device Catalogue</dc:source>
	<skos:definition xml:lang="en">High performance through-flow Clark polarographic membrane sensor designed to be plumbed in to a Sea-Bird underwater unit pumped water supply on a profiling CTD package. Designed specifically to give rapid temperature response and minimal pressure hysteresis. Signal output is voltage based to interface to a CTD deck unit.</skos:definition>
	<skos:inScheme rdf:resource="http://vocab.aodn.org.au/def/instrument/1"/>
	<skos:prefLabel xml:lang="en">Sea-Bird SBE 43 Dissolved Oxygen sensor</skos:prefLabel>
	<skos:broader rdf:resource="http://vocab.nerc.ac.uk/collection/L05/current/351"/>
	<skos:scopeNote xml:lang="en">manufacturer:Sea-Bird Electronics Inc.</skos:scopeNote>
</rdf:Description>

<rdf:Description rdf:about="http://vocab.nerc.ac.uk/collection/L22/current/TOOL0037">
	<rdf:type rdf:resource="http://www.w3.org/2000/01/rdf-schema#Resource"/>
	<rdf:type rdf:resource="http://www.w3.org/2004/02/skos/core#Concept"/>
	<dcterms:created rdf:datatype="http://www.w3.org/2001/XMLSchema#dateTime">2014-02-26T00:00:00Z</dcterms:created>
	<dc:publisher rdf:datatype="http://www.w3.org/2001/XMLSchema#string">British Oceanographic Data Centre (BODC)</dc:publisher>
	<dc:source rdf:datatype="http://www.w3.org/2001/XMLSchema#string">(L221) SeaVoX Device Catalogue</dc:source>
	<skos:definition xml:lang="en">High performance through-flow Clark polarographic membrane sensor designed to be interfaced to an SBE 52-MP profiling moored CTD or integrated into OEM moorings. Designed specifically to give rapid temperature response and minimal pressure hysteresis. Signal output is frequency based.</skos:definition>
	<skos:inScheme rdf:resource="http://vocab.aodn.org.au/def/instrument/1"/>
	<skos:prefLabel xml:lang="en">Sea-Bird SBE 43F Dissolved Oxygen Sensor</skos:prefLabel>
	<skos:broader rdf:resource="http://vocab.nerc.ac.uk/collection/L05/current/351"/>
	<skos:scopeNote xml:lang="en">manufacturer:Sea-Bird Electronics Inc.</skos:scopeNote>
</rdf:Description>

<rdf:Description rdf:about="http://vocab.nerc.ac.uk/collection/L22/current/TOOL0369">
	<rdf:type rdf:resource="http://www.w3.org/2000/01/rdf-schema#Resource"/>
	<rdf:type rdf:resource="http://www.w3.org/2004/02/skos/core#Concept"/>
	<dcterms:created rdf:datatype="http://www.w3.org/2001/XMLSchema#dateTime">2014-02-06T00:00:00Z</dcterms:created>
	<dc:publisher rdf:datatype="http://www.w3.org/2001/XMLSchema#string">British Oceanographic Data Centre (BODC)</dc:publisher>
	<dc:source rdf:datatype="http://www.w3.org/2001/XMLSchema#string">(L221) SeaVoX Device Catalogue</dc:source>
	<skos:definition xml:lang="en">A dissolved oxygen sensor which provides analogue output to third party data loggers. Measurement is based on the ability of selected substances to act as dynamic fluorescence quenchers. The fluorescent indicator is a special platinum porphyrin complex embedded in a gas permeable foil that is exposed to the surrounding water. A black optical isolation coating protects the complex from sunlight and fluorescent particles in the water. This sensing foil is attached to a window providing optical access for the measuring system from inside a watertight titanium housing.The foil is excited by modulated blue light, and the phase of a returned red light is measured. By linearizing and temperature compensating, with an incorporated temperature sensor, the absolute O2 concentration can be determined.</skos:definition>
	<skos:inScheme rdf:resource="http://vocab.aodn.org.au/def/instrument/1"/>
	<skos:prefLabel xml:lang="en">Aanderaa Oxygen Optode 3975</skos:prefLabel>
	<skos:broader rdf:resource="http://vocab.nerc.ac.uk/collection/L05/current/351"/>
	<skos:scopeNote xml:lang="en">manufacturer:Aanderaa Data Instruments</skos:scopeNote>
</rdf:Description>

<rdf:Description rdf:about="http://vocab.nerc.ac.uk/collection/L22/current/TOOL0679">
	<rdf:type rdf:resource="http://www.w3.org/2000/01/rdf-schema#Resource"/>
	<rdf:type rdf:resource="http://www.w3.org/2004/02/skos/core#Concept"/>
	<dcterms:created rdf:datatype="http://www.w3.org/2001/XMLSchema#dateTime">2014-06-04T00:00:00Z</dcterms:created>
	<dc:publisher rdf:datatype="http://www.w3.org/2001/XMLSchema#string">British Oceanographic Data Centre (BODC)</dc:publisher>
	<dc:source rdf:datatype="http://www.w3.org/2001/XMLSchema#string">(L221) SeaVoX Device Catalogue</dc:source>
	<skos:definition xml:lang="en">In-situ dissolved gas sensor measuring the sum of the partial pressures of all dissolved gases, i.e. gas tension.</skos:definition>
	<skos:inScheme rdf:resource="http://vocab.aodn.org.au/def/instrument/1"/>
	<skos:prefLabel xml:lang="en">Pro Oceanus GTD-Pro dissolved gas sensor</skos:prefLabel>
	<skos:broader rdf:resource="http://vocab.nerc.ac.uk/collection/L05/current/351"/>
</rdf:Description>

<rdf:Description rdf:about="http://vocab.nerc.ac.uk/collection/L22/current/TOOL0724">
	<rdf:type rdf:resource="http://www.w3.org/2000/01/rdf-schema#Resource"/>
	<rdf:type rdf:resource="http://www.w3.org/2004/02/skos/core#Concept"/>
	<dcterms:created rdf:datatype="http://www.w3.org/2001/XMLSchema#dateTime">2013-10-08T00:00:00Z</dcterms:created>
	<dc:publisher rdf:datatype="http://www.w3.org/2001/XMLSchema#string">British Oceanographic Data Centre (BODC)</dc:publisher>
	<dc:source rdf:datatype="http://www.w3.org/2001/XMLSchema#string">(L221) SeaVoX Device Catalogue</dc:source>
	<skos:definition xml:lang="en">The General Oceanics model 8050 pCO2 Measuring System is an autonomous analytical system for measuring carbon dioxide in surface water. It includes a headspace equilibrator, an infrared CO2 analyser, and computer-controlled and -monitored pumps. It measures: pressure (flow) in range 0 to 10 dbar, with accuracy of 0.2 percent and resolution of 0.03 percent; temperature in range -3 to 50 degC, with accuracy of 0.003 percent and resolution of 0.0005 degC; conductivity in range 0 to 64 mS/cm, with accuracy of 0.003 mS/cm and resolution of 0.001 mS/cm; Oxygen in range 0 to 25ppm (250 percent saturation), with accuracy of 0.1ppm (1 percent saturation) and 0.01ppm (0.1 percent saturation); pH in range 0 to 0.14 pH, with accuracy of 0.01 pH and resolution of 0.001 pH; Redox in range -1000 to 1000 mV, with accuracy of 1 mV and resolution of 0.1 mV.</skos:definition>
	<skos:inScheme rdf:resource="http://vocab.aodn.org.au/def/instrument/1"/>
	<skos:prefLabel xml:lang="en">General Oceanics model 8050 pCO2 measuring system</skos:prefLabel>
	<skos:broader rdf:resource="http://vocab.nerc.ac.uk/collection/L05/current/351"/>
	<skos:broader rdf:resource="http://vocab.nerc.ac.uk/collection/L05/current/382"/>
	<skos:scopeNote xml:lang="en">manufacturer:General Oceanics</skos:scopeNote>
</rdf:Description>

<rdf:Description rdf:about="http://vocab.nerc.ac.uk/collection/L22/current/TOOL0739">
	<rdf:type rdf:resource="http://www.w3.org/2000/01/rdf-schema#Resource"/>
	<rdf:type rdf:resource="http://www.w3.org/2004/02/skos/core#Concept"/>
	<dcterms:created rdf:datatype="http://www.w3.org/2001/XMLSchema#dateTime">2013-03-28T00:00:00Z</dcterms:created>
	<dc:publisher rdf:datatype="http://www.w3.org/2001/XMLSchema#string">British Oceanographic Data Centre (BODC)</dc:publisher>
	<dc:source rdf:datatype="http://www.w3.org/2001/XMLSchema#string">(L221) SeaVoX Device Catalogue</dc:source>
	<skos:definition xml:lang="en">An optode dissolved oxygen sensor mounted in plastic (600m operating depth) or titanium (7000m operating depth) housing that interfaces through an RS-232 connection to SeaCAT  or MicroCAT CTDs or Navis Argo float. Accuracy is the greater of 3 micromole/kg or 2%. More information is available at http://www.seabird.com/products/spec_sheets/63data.htm.</skos:definition>
	<skos:inScheme rdf:resource="http://vocab.aodn.org.au/def/instrument/1"/>
	<skos:prefLabel xml:lang="en">Sea-Bird SBE 63 dissolved oxygen sensor</skos:prefLabel>
	<skos:broader rdf:resource="http://vocab.nerc.ac.uk/collection/L05/current/351"/>
	<skos:altLabel xml:lang="en">Sea-Bird SBE 63 DO</skos:altLabel>
</rdf:Description>

<rdf:Description rdf:about="http://vocab.nerc.ac.uk/collection/L22/current/TOOL0805">
	<rdf:type rdf:resource="http://www.w3.org/2000/01/rdf-schema#Resource"/>
	<rdf:type rdf:resource="http://www.w3.org/2004/02/skos/core#Concept"/>
	<dcterms:created rdf:datatype="http://www.w3.org/2001/XMLSchema#dateTime">2013-09-09T00:00:00Z</dcterms:created>
	<dc:publisher rdf:datatype="http://www.w3.org/2001/XMLSchema#string">British Oceanographic Data Centre (BODC)</dc:publisher>
	<dc:source rdf:datatype="http://www.w3.org/2001/XMLSchema#string">(L221) SeaVoX Device Catalogue</dc:source>
	<skos:definition xml:lang="en">A generic label for a range of dissolved oxygen sensors produced by Aanderaa covering various mounting options. Each has a specific model number but in this case it is not known. All make measurements based on the ability of selected substances to act as dynamic fluorescence quenchers. The fluorescent indicator is a special platinum porphyrin complex embedded in a gas permeable foil that is exposed to the surrounding water. A black optical isolation coating protects the complex from sunlight and fluorescent particles in the water. This sensing foil is attached to a window providing optical access for the measuring system from inside a watertight titanium housing.The foil is excited by modulated blue light, and the phase of a returned red light is measured. By linearizing and temperature compensating, with an incorporated temperature sensor, the absolute O2 concentration can be determined.</skos:definition>
	<skos:inScheme rdf:resource="http://vocab.aodn.org.au/def/instrument/1"/>
	<skos:prefLabel xml:lang="en">Aanderaa optode</skos:prefLabel>
	<skos:broader rdf:resource="http://vocab.nerc.ac.uk/collection/L05/current/351"/>
	<skos:scopeNote xml:lang="en">manufacturer:Aanderaa Data Instruments</skos:scopeNote>
</rdf:Description>

<rdf:Description rdf:about="http://vocab.nerc.ac.uk/collection/L22/current/TOOL0663">
	<rdf:type rdf:resource="http://www.w3.org/2000/01/rdf-schema#Resource"/>
	<rdf:type rdf:resource="http://www.w3.org/2004/02/skos/core#Concept"/>
	<dcterms:created rdf:datatype="http://www.w3.org/2001/XMLSchema#dateTime">2014-02-11T00:00:00Z</dcterms:created>
	<dc:publisher rdf:datatype="http://www.w3.org/2001/XMLSchema#string">British Oceanographic Data Centre (BODC)</dc:publisher>
	<dc:source rdf:datatype="http://www.w3.org/2001/XMLSchema#string">(L221) SeaVoX Device Catalogue</dc:source>
	<skos:definition xml:lang="en">Instrument that contains a hydrophone plus a data logger in a deep-water housing designed for long-term monitoring of underwater noise. It can be deployed for periods of up to two years. Sampling frequency and schedule (including burst recording) may be programmed. More information at http://cmst.curtin.edu.au/products/usr.cfm.</skos:definition>
	<skos:inScheme rdf:resource="http://vocab.aodn.org.au/def/instrument/1"/>
	<skos:prefLabel xml:lang="en">CMST-DSTO underwater sound recorder</skos:prefLabel>
	<skos:broader rdf:resource="http://vocab.nerc.ac.uk/collection/L05/current/369"/>
	<skos:scopeNote xml:lang="en">manufacturer:CMST</skos:scopeNote>
</rdf:Description>

<rdf:Description rdf:about="http://vocab.nerc.ac.uk/collection/L22/current/TOOL0671">
	<rdf:type rdf:resource="http://www.w3.org/2000/01/rdf-schema#Resource"/>
	<rdf:type rdf:resource="http://www.w3.org/2004/02/skos/core#Concept"/>
	<dcterms:created rdf:datatype="http://www.w3.org/2001/XMLSchema#dateTime">2013-10-14T00:00:00Z</dcterms:created>
	<dc:publisher rdf:datatype="http://www.w3.org/2001/XMLSchema#string">British Oceanographic Data Centre (BODC)</dc:publisher>
	<dc:source rdf:datatype="http://www.w3.org/2001/XMLSchema#string">(L221) SeaVoX Device Catalogue</dc:source>
	<skos:definition xml:lang="en">An instrument that accurately measures rain or snow precipitation without moving parts, making it ideal for use on moving platforms such as buoys and ships. Insulated housings and thermostatically controlled heaters permit operation at temperatures below freezing. Precipitation measurement is made with a capacitive transducer and electronic circuit that produce a voltage output. Total precipitation can be tracked by a data logger or recorder. It has an accuracy and threshold of 1mm. More information may be found at http://www.youngusa.com/products/3/17.html.</skos:definition>
	<skos:inScheme rdf:resource="http://vocab.aodn.org.au/def/instrument/1"/>
	<skos:prefLabel xml:lang="en">Young 50202 Precipitation Gauge</skos:prefLabel>
	<skos:broader rdf:resource="http://vocab.nerc.ac.uk/collection/L05/current/381"/>
	<skos:scopeNote xml:lang="en">manufacturer:R.M. Young Company</skos:scopeNote>
</rdf:Description>

<rdf:Description rdf:about="http://vocab.nerc.ac.uk/collection/L22/current/TOOL0725">
	<rdf:type rdf:resource="http://www.w3.org/2000/01/rdf-schema#Resource"/>
	<rdf:type rdf:resource="http://www.w3.org/2004/02/skos/core#Concept"/>
	<dcterms:created rdf:datatype="http://www.w3.org/2001/XMLSchema#dateTime">2013-10-14T00:00:00Z</dcterms:created>
	<dc:publisher rdf:datatype="http://www.w3.org/2001/XMLSchema#string">British Oceanographic Data Centre (BODC)</dc:publisher>
	<dc:source rdf:datatype="http://www.w3.org/2001/XMLSchema#string">(L221) SeaVoX Device Catalogue</dc:source>
	<skos:definition xml:lang="en">The OSi ORG-815-DR is an optical scintillation rain gauge that measures rain rate in the range 0.1 to 500 mm/hr; rain accumulation in the range 0.001 to 999.999 mm with accuracy of 5% accumulation and resolution of 0.001 mm. It features RS-232 serial input/output, and operates in temperatures from -40 to 50 degrees C.</skos:definition>
	<skos:inScheme rdf:resource="http://vocab.aodn.org.au/def/instrument/1"/>
	<skos:prefLabel xml:lang="en">OSi ORG-815-DR Optical Rain Gauge</skos:prefLabel>
	<skos:broader rdf:resource="http://vocab.nerc.ac.uk/collection/L05/current/381"/>
	<skos:scopeNote xml:lang="en">manufacturer:Optical Scientific Inc.</skos:scopeNote>
</rdf:Description>

<rdf:Description rdf:about="http://vocab.nerc.ac.uk/collection/L22/current/TOOL0705">
	<rdf:type rdf:resource="http://www.w3.org/2000/01/rdf-schema#Resource"/>
	<rdf:type rdf:resource="http://www.w3.org/2004/02/skos/core#Concept"/>
	<dcterms:created rdf:datatype="http://www.w3.org/2001/XMLSchema#dateTime">2013-10-08T00:00:00Z</dcterms:created>
	<dc:publisher rdf:datatype="http://www.w3.org/2001/XMLSchema#string">British Oceanographic Data Centre (BODC)</dc:publisher>
	<dc:source rdf:datatype="http://www.w3.org/2001/XMLSchema#string">(L221) SeaVoX Device Catalogue</dc:source>
	<skos:definition xml:lang="en">The LI-7000 is a differential, single source, non-dispersive, infrared gas analyser. Two solid state detectors, one each for CO2 and H2O, filter at 4.255 microns and 2.595 microns respectively. CO2 is measured in the range 0-3000ppm, with accuracy of 1 percent nominally. H2O is measured in the range 0-60 mmol per mol, with accuracy of one 1 percent.</skos:definition>
	<skos:inScheme rdf:resource="http://vocab.aodn.org.au/def/instrument/1"/>
	<skos:prefLabel xml:lang="en">LI-COR LI-7000 CO2/H20 Gas Analyser</skos:prefLabel>
	<skos:broader rdf:resource="http://vocab.nerc.ac.uk/collection/L05/current/382"/>
	<skos:scopeNote xml:lang="en">manufacturer:LI-COR Incorporated</skos:scopeNote>
</rdf:Description>

<rdf:Description rdf:about="http://vocab.nerc.ac.uk/collection/L22/current/TOOL1123">
	<rdf:type rdf:resource="http://www.w3.org/2000/01/rdf-schema#Resource"/>
	<rdf:type rdf:resource="http://www.w3.org/2004/02/skos/core#Concept"/>
	<dcterms:created rdf:datatype="http://www.w3.org/2001/XMLSchema#dateTime">2017-04-10T00:00:00Z</dcterms:created>
	<dc:publisher rdf:datatype="http://www.w3.org/2001/XMLSchema#string">British Oceanographic Data Centre (BODC)</dc:publisher>
	<skos:definition xml:lang="en">A differential, non-dispersive, infrared (NDIR) gas analyser that measures CO2 and H2O gas concentration. Measurements are based on the difference in absorption of infrared (IR) radiation passing through two gas sampling cells. The reference cell is used for a gas of known CO2 or H2O concentration, and the sample cell is used for a gas of unknown concentration. Infrared radiation is transmitted through both cell paths, and the output of the analyser is proportional to the difference in absorption between the two. It contains two solid state lead selenide detectors; one each for CO2 and H2O, filtered at 4.26 and 2.59 microns, respectively.The analyser has a measurement range of 0 to + 7.5 kPa or 40 degrees C dewpoint (H2O); 0 to 3000 ppm (CO2). Accuracy is less than 1% of the reading (H2O); +/- 1 ppm (CO2).</skos:definition>
	<skos:inScheme rdf:resource="http://vocab.aodn.org.au/def/instrument/1"/>
	<skos:prefLabel xml:lang="en">LI-COR LI-6262 CO2/H2O infrared gas analyser</skos:prefLabel>
	<skos:broader rdf:resource="http://vocab.nerc.ac.uk/collection/L05/current/382"/>
	<skos:altLabel xml:lang="en">LI-COR LI-6262 gas analyser</skos:altLabel>
</rdf:Description>

<rdf:Description rdf:about="http://vocab.nerc.ac.uk/collection/L22/current/TOOL0721">
	<rdf:type rdf:resource="http://www.w3.org/2000/01/rdf-schema#Resource"/>
	<rdf:type rdf:resource="http://www.w3.org/2004/02/skos/core#Concept"/>
	<dcterms:created rdf:datatype="http://www.w3.org/2001/XMLSchema#dateTime">2014-07-11T00:00:00Z</dcterms:created>
	<dc:publisher rdf:datatype="http://www.w3.org/2001/XMLSchema#string">British Oceanographic Data Centre (BODC)</dc:publisher>
	<dc:source rdf:datatype="http://www.w3.org/2001/XMLSchema#string">(L221) SeaVoX Device Catalogue</dc:source>
	<skos:definition xml:lang="en">The MicroStrain 3DM-GX3 is a triaxial accelerometer designed to measure 360 degrees of angular motion on three orthogonal axes. The 3DM-GX1 has now been retired in favour of later MicroStrain products. The 3DM-GX1 featured on-board processing/filtering of accelerometer, gyro and magnetometer channels, with standard RS-232 and RS-485 outputs, and optional analog output. It offers 16 bit A/D resolution, accuracy of +/-0.5 degrees for static test conditions or +/-2 degrees for dynamic test conditions, 100 Hz digital output rate for Euler, Matrix and Quaternion, and operates in temperatures of -40 to 70 degrees C with enclosure (or +85 degrees C without enclosure).</skos:definition>
	<skos:inScheme rdf:resource="http://vocab.aodn.org.au/def/instrument/1"/>
	<skos:prefLabel xml:lang="en">Microstrain 3DM-GX1 Gyro Enhanced Orientation Sensor</skos:prefLabel>
	<skos:broader rdf:resource="http://vocab.nerc.ac.uk/collection/L05/current/385"/>
</rdf:Description>

<rdf:Description rdf:about="http://vocab.nerc.ac.uk/collection/L22/current/TOOL0198">
	<rdf:type rdf:resource="http://www.w3.org/2000/01/rdf-schema#Resource"/>
	<rdf:type rdf:resource="http://www.w3.org/2004/02/skos/core#Concept"/>
	<dcterms:created rdf:datatype="http://www.w3.org/2001/XMLSchema#dateTime">2013-10-09T00:00:00Z</dcterms:created>
	<dc:publisher rdf:datatype="http://www.w3.org/2001/XMLSchema#string">British Oceanographic Data Centre (BODC)</dc:publisher>
	<dc:source rdf:datatype="http://www.w3.org/2001/XMLSchema#string">(L221) SeaVoX Device Catalogue</dc:source>
	<skos:definition xml:lang="en">A split-beam scientific echosounder primarily designed for fisheries research. It can operate seven frequencies simultaneously ranging from 18 to 710 kHz. Real time echo integration and target strength analysis in an unlimited number of layers is provided as well as storage of raw data for replay or analysis in one of several post-processing software packages such as Simrad's BI60.</skos:definition>
	<skos:inScheme rdf:resource="http://vocab.aodn.org.au/def/instrument/1"/>
	<skos:prefLabel xml:lang="en">Simrad EK-60 echosounder</skos:prefLabel>
	<skos:broader rdf:resource="http://vocab.nerc.ac.uk/collection/L05/current/FFES"/>
	<skos:scopeNote xml:lang="en">manufacturer:Kongsberg Maritime AS</skos:scopeNote>
</rdf:Description>

<rdf:Description rdf:about="http://vocab.nerc.ac.uk/collection/L22/current/TOOL0689">
	<rdf:type rdf:resource="http://www.w3.org/2000/01/rdf-schema#Resource"/>
	<rdf:type rdf:resource="http://www.w3.org/2004/02/skos/core#Concept"/>
	<dcterms:created rdf:datatype="http://www.w3.org/2001/XMLSchema#dateTime">2013-10-09T00:00:00Z</dcterms:created>
	<dc:publisher rdf:datatype="http://www.w3.org/2001/XMLSchema#string">British Oceanographic Data Centre (BODC)</dc:publisher>
	<dc:source rdf:datatype="http://www.w3.org/2001/XMLSchema#string">(L221) SeaVoX Device Catalogue</dc:source>
	<skos:definition xml:lang="en">A third generation single-beam or split-beam multi-frequncy echosounder primarily designed for fish-finding but may also be used in fisheries research. More information may be found in http://www.simrad.com/www/01/NOKBG0397.nsf/AllWeb/1C1B8782314422F9C12570F300270EAC/$file/Simrad_ES60_Brochure_English.pdf?OpenElement.This instrument is now (April 2014) flagged as discontinues on the Simrad web site.</skos:definition>
	<skos:inScheme rdf:resource="http://vocab.aodn.org.au/def/instrument/1"/>
	<skos:prefLabel xml:lang="en">Simrad ES60 echosounder</skos:prefLabel>
	<skos:broader rdf:resource="http://vocab.nerc.ac.uk/collection/L05/current/FFES"/>
	<skos:scopeNote xml:lang="en">manufacturer:Kongsberg Maritime AS</skos:scopeNote>
</rdf:Description>

<rdf:Description rdf:about="http://www.w3.org/2004/02/skos/core#altLabel">
	<rdf:type rdf:resource="http://www.w3.org/1999/02/22-rdf-syntax-ns#Property"/>
	<rdf:type rdf:resource="http://www.w3.org/2000/01/rdf-schema#Resource"/>
	<rdfs:subPropertyOf rdf:resource="http://www.w3.org/2004/02/skos/core#altLabel"/>
</rdf:Description>

<rdf:Description rdf:about="http://vocab.nerc.ac.uk/collection/L22/current/TOOL1124">
	<rdf:type rdf:resource="http://www.w3.org/2000/01/rdf-schema#Resource"/>
	<rdf:type rdf:resource="http://www.w3.org/2004/02/skos/core#Concept"/>
	<dcterms:created rdf:datatype="http://www.w3.org/2001/XMLSchema#dateTime">2017-04-10T00:00:00Z</dcterms:created>
	<dc:publisher rdf:datatype="http://www.w3.org/2001/XMLSchema#string">British Oceanographic Data Centre (BODC)</dc:publisher>
	<skos:definition xml:lang="en">A submersible pressure transducer. Its applications are for long-term deployments such as water-level measurements in canals, wells, ponds, harbours, lakes, streams and tanks. It has a titanium case and outputs either a digital SDI-12 or RS-232 signal to indicate observed pressure and temperature. The CS456 replaces the CS455 transducer. It has a smaller gap between the water ports and the diaphragm so that less air is trapped that the user must remove during deployment. It is available in 6 pressure depth range options (0-2.9, 0-7.25, 0-14.5, 0-29, 0-72.5, 0-145 psig) and two accuracy options. The standard accuracy option provides +/-0.1% full-scale range TEB over the 0 - 60 degrees C temperature range. The high accuracy option provides +/-0.05% full scale range TEB over the 0 - 60 degrees C temperature range.</skos:definition>
	<skos:inScheme rdf:resource="http://vocab.aodn.org.au/def/instrument/1"/>
	<skos:prefLabel xml:lang="en">Campbell Scientific CS456 pressure transducer</skos:prefLabel>
	<skos:broader rdf:resource="http://vocab.nerc.ac.uk/collection/L05/current/WPS"/>
	<skos:altLabel xml:lang="en">Campbell Scientific CS456</skos:altLabel>
</rdf:Description>

<rdf:Description rdf:about="http://vocab.nerc.ac.uk/collection/L22/current/TOOL1141">
	<rdf:type rdf:resource="http://www.w3.org/2000/01/rdf-schema#Resource"/>
	<rdf:type rdf:resource="http://www.w3.org/2004/02/skos/core#Concept"/>
	<dcterms:created rdf:datatype="http://www.w3.org/2001/XMLSchema#dateTime">2017-11-21T00:00:00Z</dcterms:created>
	<dc:publisher rdf:datatype="http://www.w3.org/2001/XMLSchema#string">British Oceanographic Data Centre (BODC)</dc:publisher>
	<skos:definition xml:lang="en">A combined three channel ECO back scatter sensor for floats. It measures proxies of phytoplankton abundance (chlorophyll fluorescence), total particle concentration (backscattering, 700 nm), and dissolved organic matter (CDOM fluorescence) in a single data stream. It has an in-water centroid angle of 124 degrees and is housed in aluminium. The sensor can be fitted with optional temperature and pressure sensor. It has an operating temperature range of 0-30 degrees Celsius and operating depth range of 2000 m.</skos:definition>
	<skos:inScheme rdf:resource="http://vocab.aodn.org.au/def/instrument/1"/>
	<skos:prefLabel xml:lang="en">WETLabs ECO FLBBCD backscattering sensor</skos:prefLabel>
	<skos:broader rdf:resource="http://vocab.nerc.ac.uk/collection/L05/current/113"/>
	<skos:broader rdf:resource="http://vocab.nerc.ac.uk/collection/L05/current/123"/>
	<skos:broader rdf:resource="http://vocab.nerc.ac.uk/collection/L05/current/134"/>
	<skos:broader rdf:resource="http://vocab.nerc.ac.uk/collection/L05/current/WPS"/>
	<skos:altLabel xml:lang="en">WETLabs ECO FLBBCD</skos:altLabel>
</rdf:Description>

<rdf:Description rdf:about="http://vocab.aodn.org.au/instrument/1">
	<rdf:type rdf:resource="http://www.w3.org/2000/01/rdf-schema#Resource"/>
</rdf:Description>

<rdf:Description rdf:about="http://www.w3.org/2004/02/skos/core#hiddenLabel">
	<rdf:type rdf:resource="http://www.w3.org/1999/02/22-rdf-syntax-ns#Property"/>
	<rdf:type rdf:resource="http://www.w3.org/2000/01/rdf-schema#Resource"/>
	<rdfs:subPropertyOf rdf:resource="http://www.w3.org/2004/02/skos/core#hiddenLabel"/>
</rdf:Description>

<rdf:Description rdf:about="http://vocab.nerc.ac.uk/collection/L22/current/TOOL1151">
	<rdf:type rdf:resource="http://www.w3.org/2000/01/rdf-schema#Resource"/>
	<rdf:type rdf:resource="http://www.w3.org/2004/02/skos/core#Concept"/>
	<dcterms:created rdf:datatype="http://www.w3.org/2001/XMLSchema#dateTime">2017-11-09T00:00:00Z</dcterms:created>
	<dc:publisher rdf:datatype="http://www.w3.org/2001/XMLSchema#string">British Oceanographic Data Centre (BODC)</dc:publisher>
	<skos:definition xml:lang="en">An autonomous scientific echosounder for the measurement and monitoring of environmental conditions in oceans, lakes and rivers. Abundance of zooplankton, fish, bubbles and suspended sediments in the water column are common targets, via the measurement of acoustic backscatter returns at multiple ultrasonic frequencies. Using onboard data storage, the AZFP can collect data continuously for periods of up to one year at high temporal and spatial resolution. The AZFP is available with up to four frequencies in a single transducer housing. It can be operated in bottom-mounted, upward looking mode or in downward looking mode from a buoy, and is ideally suited for taut-line mooring operation. It has a configurable ping rate up to 1 Hz, 16 Gb Compact Flash storage with up to 32 Gb available, and weighs 50 kg in its ruggedised shipping case.</skos:definition>
	<skos:inScheme rdf:resource="http://vocab.aodn.org.au/def/instrument/1"/>
	<skos:prefLabel xml:lang="en">ASL AZFP Acoustic Zooplankton Fish Profiler</skos:prefLabel>
	<skos:broader rdf:resource="http://vocab.nerc.ac.uk/collection/L05/current/FFES"/>
	<skos:altLabel xml:lang="en">ASL AZFP</skos:altLabel>
</rdf:Description>

<rdf:Description rdf:about="http://vocab.nerc.ac.uk/collection/L22/current/TOOL1152">
	<rdf:type rdf:resource="http://www.w3.org/2000/01/rdf-schema#Resource"/>
	<rdf:type rdf:resource="http://www.w3.org/2004/02/skos/core#Concept"/>
	<dcterms:contributor rdf:resource="http://editor.vocabs.ands.org.au/user/eMII_Atkins.Natalia"/>
	<dcterms:created rdf:datatype="http://www.w3.org/2001/XMLSchema#dateTime">2017-11-20T00:00:00Z</dcterms:created>
	<dcterms:modified rdf:datatype="http://www.w3.org/2001/XMLSchema#dateTime">2017-11-20T06:02:08Z</dcterms:modified>
	<dc:publisher rdf:datatype="http://www.w3.org/2001/XMLSchema#string">British Oceanographic Data Centre (BODC)</dc:publisher>
	<skos:definition xml:lang="en">A small (13 mm diameter) acoustic transmitter used to track and determine the behavioural patterns of small and juvenile fish, for applications such as site residency studies and automated monitoring of migrations. Coded transmitters send acoustic pings at 69 kHz that are infrequent and random about an average delay. This ping train includes an ID number which permits identification of the specific tag along with the sensor telemetry data. The V13 can function as a simple pinger for location only, or it can be equipped with additional sensors to include depth (V13P) and temperature (V13T) data. When used with the VR2 and or VR3 receiver, they can be used to track large numbers of fish over large areas. The V13 can also be tracked using the VR28, the VR100, or VR60 (with Option 07 version 2.01) receivers, or the VRAP system.</skos:definition>
	<skos:inScheme rdf:resource="http://vocab.aodn.org.au/def/instrument/1"/>
	<skos:prefLabel xml:lang="en">Vemco V13 Coded Transmitter Tag</skos:prefLabel>
	<skos:broader rdf:resource="http://vocab.nerc.ac.uk/collection/L05/current/TRTG"/>
	<skos:altLabel xml:lang="en">Vemco V13</skos:altLabel>
</rdf:Description>

<rdf:Description rdf:about="http://vocab.nerc.ac.uk/collection/L22/current/TOOL1153">
	<rdf:type rdf:resource="http://www.w3.org/2000/01/rdf-schema#Resource"/>
	<rdf:type rdf:resource="http://www.w3.org/2004/02/skos/core#Concept"/>
	<dcterms:created rdf:datatype="http://www.w3.org/2001/XMLSchema#dateTime">2017-11-20T00:00:00Z</dcterms:created>
	<dc:publisher rdf:datatype="http://www.w3.org/2001/XMLSchema#string">British Oceanographic Data Centre (BODC)</dc:publisher>
	<skos:definition xml:lang="en">A coded acoustic transmitter used to measure the activity of free-ranging marine fauna, most commonly fish. The transmitter measures the 3D acceleration with depth of fauna moving within a reciever array as a vector quantity, i.e. it measures acceleration on 3 axes X, Y and Z, in metres per second squared. Other applications may include determination of swimming speed via tail beat acceleration, activity responses to changing oxygen, temperature and salinity, and detecting mortality through predation, seismic blasting, toxic spills, feeding events, spawning activity, nocturnal/diurnal activity or wave action. One of two modes of operation can be specified; an activity alogorithm or tailbeat algorithm. Coded transmitters send acoustic pings at 69 kHz that are infrequent and random about an average delay. This ping train includes an ID number which permits identification of the specific tag and sensor data. For dual sensor tags, there are two tag IDs.</skos:definition>
	<skos:inScheme rdf:resource="http://vocab.aodn.org.au/def/instrument/1"/>
	<skos:prefLabel xml:lang="en">Vemco V13AP Coded Accelerometer Pressure Transmitter Tag</skos:prefLabel>
	<skos:broader rdf:resource="http://vocab.nerc.ac.uk/collection/L05/current/TRTG"/>
	<skos:altLabel xml:lang="en">Vemco V13AP</skos:altLabel>
</rdf:Description>

<rdf:Description rdf:about="http://vocab.nerc.ac.uk/collection/L22/current/TOOL1154">
	<rdf:type rdf:resource="http://www.w3.org/2000/01/rdf-schema#Resource"/>
	<rdf:type rdf:resource="http://www.w3.org/2004/02/skos/core#Concept"/>
	<dcterms:created rdf:datatype="http://www.w3.org/2001/XMLSchema#dateTime">2017-11-20T00:00:00Z</dcterms:created>
	<dc:publisher rdf:datatype="http://www.w3.org/2001/XMLSchema#string">British Oceanographic Data Centre (BODC)</dc:publisher>
	<skos:definition xml:lang="en">A 16 mm diamter acoustic transmitter used to track and determine the behavioural patterns of medium to large marine species. Coded transmitters send acoustic pings at 69 kHz that are infrequent and random about an average delay. This ping train includes an ID number which permits identification of the specific tag along with the sensor telemetry data. The V16 can function as a simple pinger for location only, or it can be equipped with additional sensors to include depth (V16P) and temperature (V16T) data, or both (V16TP). When used with the VR2W or VR4-UWM receiver, they can be used to track large numbers of fish over large areas. The V16 can also be manually tracked using the VR100 acoustic tracking receiver. The V16 tag will last anywhere between one month and several years depending on the chosen battery size, and will give a transmission range in excess of several hundered metres.</skos:definition>
	<skos:inScheme rdf:resource="http://vocab.aodn.org.au/def/instrument/1"/>
	<skos:prefLabel xml:lang="en">Vemco V16 Coded Transmitter Tag</skos:prefLabel>
	<skos:broader rdf:resource="http://vocab.nerc.ac.uk/collection/L05/current/TRTG"/>
	<skos:altLabel xml:lang="en">Vemco V16</skos:altLabel>
</rdf:Description>

<rdf:Description rdf:about="http://vocab.nerc.ac.uk/collection/L22/current/TOOL1155">
	<rdf:type rdf:resource="http://www.w3.org/2000/01/rdf-schema#Resource"/>
	<rdf:type rdf:resource="http://www.w3.org/2004/02/skos/core#Concept"/>
	<dcterms:created rdf:datatype="http://www.w3.org/2001/XMLSchema#dateTime">2017-11-20T00:00:00Z</dcterms:created>
	<dc:publisher rdf:datatype="http://www.w3.org/2001/XMLSchema#string">British Oceanographic Data Centre (BODC)</dc:publisher>
	<skos:definition xml:lang="en">A small (7 mm diamter) acoustic transmitter used to track and determine the behavioural patterns of small and juvenile fish. The V7 tag is particularly suited for monitoring of salmon smolt migrations, and can be used to track large numbers of fish over large areas. V7 coded transmitters send acoustic pings at 69 kHz that are infrequent and random about an average delay. This ping train includes an ID number which permits identification of the specific tag. The V7 can be detected by all VEMCO 69 kHz receivers. There are two battery options, the 2L or 4L. To control the characteristics of the tags, users can choose from one to four programming steps: Status (ON/OFF), time interval, acoustic power level (L/H) and nominal delay.</skos:definition>
	<skos:inScheme rdf:resource="http://vocab.aodn.org.au/def/instrument/1"/>
	<skos:prefLabel xml:lang="en">Vemco V7 Coded Transmitter Tag</skos:prefLabel>
	<skos:broader rdf:resource="http://vocab.nerc.ac.uk/collection/L05/current/TRTG"/>
	<skos:altLabel xml:lang="en">Vemco V7</skos:altLabel>
</rdf:Description>

<rdf:Description rdf:about="http://vocab.nerc.ac.uk/collection/L22/current/TOOL1156">
	<rdf:type rdf:resource="http://www.w3.org/2000/01/rdf-schema#Resource"/>
	<rdf:type rdf:resource="http://www.w3.org/2004/02/skos/core#Concept"/>
	<dcterms:created rdf:datatype="http://www.w3.org/2001/XMLSchema#dateTime">2017-11-20T00:00:00Z</dcterms:created>
	<dc:publisher rdf:datatype="http://www.w3.org/2001/XMLSchema#string">British Oceanographic Data Centre (BODC)</dc:publisher>
	<skos:definition xml:lang="en">A small (8 mm diamter) acoustic transmitter used to track and determine the behavioural patterns of small and juvenile fish. The V8 tag is particularly suited for monitoring of salmon smolt migrations, and can be used to track large numbers of fish over large areas. The V8 offers an alternative between the V7 and V9 tags due to its higher output power and greater detection range. V8 coded transmitters send acoustic pings at 69 kHz that are infrequent and random about an average delay. This ping train includes an ID number which permits identification of the specific tag. The V8 can be detected by all VEMCO 69 kHz receivers. There are two battery options, the 4L or 4H. To control the characteristics of the tags, users can choose from one to four programming steps: Status (ON/OFF), time interval, acoustic power level (L/H) and nominal delay.</skos:definition>
	<skos:inScheme rdf:resource="http://vocab.aodn.org.au/def/instrument/1"/>
	<skos:prefLabel xml:lang="en">Vemco V8 Coded Transmitter Tag</skos:prefLabel>
	<skos:broader rdf:resource="http://vocab.nerc.ac.uk/collection/L05/current/TRTG"/>
	<skos:altLabel xml:lang="en">Vemco V8</skos:altLabel>
</rdf:Description>

<rdf:Description rdf:about="http://vocab.nerc.ac.uk/collection/L22/current/TOOL1157">
	<rdf:type rdf:resource="http://www.w3.org/2000/01/rdf-schema#Resource"/>
	<rdf:type rdf:resource="http://www.w3.org/2004/02/skos/core#Concept"/>
	<dcterms:created rdf:datatype="http://www.w3.org/2001/XMLSchema#dateTime">2017-11-20T00:00:00Z</dcterms:created>
	<dc:publisher rdf:datatype="http://www.w3.org/2001/XMLSchema#string">British Oceanographic Data Centre (BODC)</dc:publisher>
	<skos:definition xml:lang="en">A small (9 mm diamter) acoustic transmitter used to track and determine the behavioural patterns of small and juvenile fish. The V9 tag is particularly suited for monitoring of salmon smolt migrations, and can be used to track large numbers of fish over large areas. V9 coded transmitters send acoustic pings at 69 kHz that are infrequent and random about an average delay. This ping train includes an ID number which permits identification of the specific tag. The V9 tag can function as a simple pinger giving location only, or it can be equipped with depth (V9P) and temperature (V9T) sensors, or both (V9TP). The V9 can be used with the VR2W monitoring receiver, and can also be actively tracked using the VR100 acoustic tracking receiver.</skos:definition>
	<skos:inScheme rdf:resource="http://vocab.aodn.org.au/def/instrument/1"/>
	<skos:prefLabel xml:lang="en">Vemco V9 Coded Transmitter Tag</skos:prefLabel>
	<skos:broader rdf:resource="http://vocab.nerc.ac.uk/collection/L05/current/TRTG"/>
	<skos:altLabel xml:lang="en">Vemco V9</skos:altLabel>
</rdf:Description>

<rdf:Description rdf:about="http://vocab.nerc.ac.uk/collection/L22/current/TOOL1159">
	<rdf:type rdf:resource="http://www.w3.org/2000/01/rdf-schema#Resource"/>
	<rdf:type rdf:resource="http://www.w3.org/2004/02/skos/core#Concept"/>
	<dcterms:created rdf:datatype="http://www.w3.org/2001/XMLSchema#dateTime">2017-11-20T00:00:00Z</dcterms:created>
	<dc:publisher rdf:datatype="http://www.w3.org/2001/XMLSchema#string">British Oceanographic Data Centre (BODC)</dc:publisher>
	<skos:definition xml:lang="en">The VR2AR is a submersible acoustic receiver, combining an acoustic release with a VR2Tx (a VR2W receiver with a built in V16-like transmitter). It is used with Vemco coded transmitter tags placed on marine fauna to track their movements or behaviour. These detections are then received and stored by Vemco receivers, whose content are monitored by the VR2AR. The unit allows remote communication with all Vemco 69 kHz receivers while still deployed, and it can be retrieved via the built-in acoustic release. Deployed receivers can also be retrieved via the VR2AR, and their status monitored on demand via communication with a surface VR100 tracking receiver and transponding hydrophone. Receiver health, tilt angle, range, temperature, battery life and memory can be monitored in this way. The total number of detections stored by different receivers and specific transmitter tag IDs can also be monitored. An optional flotation collar is available to assist in location and retrieval of the VR2AR. It attaches below the receiver hydrophone ensuring there are no shadowing effects on the receiver. It has a maximum depth rating of 500m, battery life of approximately 14 months and 16 MB internal storage.</skos:definition>
	<skos:inScheme rdf:resource="http://vocab.aodn.org.au/def/instrument/1"/>
	<skos:prefLabel xml:lang="en">Vemco VR2AR Acoustic Release, Receiver and Transmitter</skos:prefLabel>
	<skos:broader rdf:resource="http://vocab.nerc.ac.uk/collection/L05/current/369"/>
	<skos:altLabel xml:lang="en">Vemco VR2AR</skos:altLabel>
</rdf:Description>

<rdf:Description rdf:about="http://vocab.nerc.ac.uk/collection/L22/current/TOOL1160">
	<rdf:type rdf:resource="http://www.w3.org/2000/01/rdf-schema#Resource"/>
	<rdf:type rdf:resource="http://www.w3.org/2004/02/skos/core#Concept"/>
	<dcterms:created rdf:datatype="http://www.w3.org/2001/XMLSchema#dateTime">2017-11-20T00:00:00Z</dcterms:created>
	<dc:publisher rdf:datatype="http://www.w3.org/2001/XMLSchema#string">British Oceanographic Data Centre (BODC)</dc:publisher>
	<skos:definition xml:lang="en">A single channel acoustic receiver comprising hydrophone, receiver, ID detector, data logging memory and battery all within submersible housing. It is used to remotely retrieve ID numbers and time stamps from all Vemco 69 and 180 kHz acoustic transmitter tags deployed on marine fauna travelling within the VR2W's receiver range. The VR2W is ideal for use in river monitoring or freshwater lake studies, as well as large tracking operations in oceanic systems. Depth, temperature and other data can also be downloaded, and uploaded to a PC via Bluetooth wireless technology at a rate of approximately 8 seconds per 10000 detections. The VR2W features 16 MB internal storage, enabling storage of approximately 1.6 million detections.</skos:definition>
	<skos:inScheme rdf:resource="http://vocab.aodn.org.au/def/instrument/1"/>
	<skos:prefLabel xml:lang="en">Vemco VR2W Single Channel Receiver</skos:prefLabel>
	<skos:broader rdf:resource="http://vocab.nerc.ac.uk/collection/L05/current/369"/>
	<skos:altLabel xml:lang="en">Vemco VR2W</skos:altLabel>
</rdf:Description>

<rdf:Description rdf:about="http://vocab.nerc.ac.uk/collection/L22/current/TOOL1161">
	<rdf:type rdf:resource="http://www.w3.org/2000/01/rdf-schema#Resource"/>
	<rdf:type rdf:resource="http://www.w3.org/2004/02/skos/core#Concept"/>
	<dcterms:created rdf:datatype="http://www.w3.org/2001/XMLSchema#dateTime">2017-11-20T00:00:00Z</dcterms:created>
	<dc:publisher rdf:datatype="http://www.w3.org/2001/XMLSchema#string">British Oceanographic Data Centre (BODC)</dc:publisher>
	<skos:definition xml:lang="en">A submersible acoustic receiver capable of detecting all Vemco coded transmitter tags (both 69 kHz and 180 kHz tags) and communicating remotely to a surface modem. The instrument is ideally suited to site residency and migratory studies of marine fauna over an extended period, and is suitable in offshore deployments. The VR4-UWM records the ID and time stamp from coded transmitter tags deployed on marine fauna that enter the receiver's range. Temperature, depth and acceleration data can also be collected. The instrument subsequently transmits this data to a surface unit, which can be loaded to a PC in the field without the need to retrieve the instrument. The VR4-UWM has a maximum depth rating of 500 m. It can store more than 800000 detections and be deployed undisturbed for more than six years.</skos:definition>
	<skos:inScheme rdf:resource="http://vocab.aodn.org.au/def/instrument/1"/>
	<skos:prefLabel xml:lang="en">Vemco VR4-UWM Underwater Modem Receiver</skos:prefLabel>
	<skos:broader rdf:resource="http://vocab.nerc.ac.uk/collection/L05/current/369"/>
	<skos:altLabel xml:lang="en">Vemco VR4-UWM</skos:altLabel>
</rdf:Description>

<rdf:Description rdf:about="http://vocab.nerc.ac.uk/collection/L22/current/TOOL1162">
	<rdf:type rdf:resource="http://www.w3.org/2000/01/rdf-schema#Resource"/>
	<rdf:type rdf:resource="http://www.w3.org/2004/02/skos/core#Concept"/>
	<dcterms:created rdf:datatype="http://www.w3.org/2001/XMLSchema#dateTime">2017-11-09T00:00:00Z</dcterms:created>
	<dc:publisher rdf:datatype="http://www.w3.org/2001/XMLSchema#string">British Oceanographic Data Centre (BODC)</dc:publisher>
	<skos:definition xml:lang="en">A compact and self-contained battery-powered CTD for use in coastal, estuarine and deep-water deployments to measure temperature and conductivity with depth. The whole unit is mounted in a stainless steel cage with battery pack, data logger and internal memory. The 25plus comprises an SBE 3F temperature sensor, SBE 4C conductivity sensor, and a strain-gauge pressure sensor. It utilises pump-controlled T-C ducted flow to minimise salinity spiking. The instrument may also be used with external power and data logging through an RS-232 interface, and offers channels for up to ten auxiliary sensors such as oxygen, pH, fluorescence, PAR, turbidity, light transmission and nitrates. The 25plus samples at 16 Hz and is suitable for use in water depths ranging from 600-6800 m. The SBE 25plus replaces the SBE 25 which was discontinued in 2012.</skos:definition>
	<skos:inScheme rdf:resource="http://vocab.aodn.org.au/def/instrument/1"/>
	<skos:prefLabel xml:lang="en">Sea-Bird SBE 25plus Sealogger CTD</skos:prefLabel>
	<skos:broader rdf:resource="http://vocab.nerc.ac.uk/collection/L05/current/130"/>
	<skos:broader rdf:resource="http://vocab.nerc.ac.uk/collection/L05/current/134"/>
	<skos:broader rdf:resource="http://vocab.nerc.ac.uk/collection/L05/current/350"/>
	<skos:altLabel xml:lang="en">SBE 25+ Sealogger</skos:altLabel>
</rdf:Description>

<rdf:Description rdf:about="http://vocab.nerc.ac.uk/collection/L22/current/TOOL0306">
	<rdf:type rdf:resource="http://www.w3.org/2000/01/rdf-schema#Resource"/>
	<rdf:type rdf:resource="http://www.w3.org/2004/02/skos/core#Concept"/>
	<dcterms:created rdf:datatype="http://www.w3.org/2001/XMLSchema#dateTime">2017-11-21T00:00:00Z</dcterms:created>
	<dc:publisher rdf:datatype="http://www.w3.org/2001/XMLSchema#string">British Oceanographic Data Centre (BODC)</dc:publisher>
	<skos:definition xml:lang="en">A multi-frequency Doppler current sensor for measuring horizontal current speed and direction. The shallow water (SW), intermediate water (IW) and deep water (DW) models can be deployed to 300 m, 2000 m and 6000 m, respectively. The instrument has a maximum sampling rate of 0.5 Hz, a velocity range of 0 - 300 cm s-1, and incorporates an electronic compass and a tilt sensor. A number of additional oceanographic sensors may also be attached. Further details can be found at http://www.bodc.ac.uk/data/documents/nodb/pdf/Aanderaa_Seaguard_RCM.pdf</skos:definition>
	<skos:inScheme rdf:resource="http://vocab.aodn.org.au/def/instrument/1"/>
	<skos:prefLabel xml:lang="en">Aanderaa Seaguard Recording Current Meter</skos:prefLabel>
	<skos:broader rdf:resource="http://vocab.nerc.ac.uk/collection/L05/current/114"/>
	<skos:altLabel xml:lang="en">Aanderaa Seaguard RCM</skos:altLabel>
</rdf:Description>

<rdf:Description rdf:about="http://vocab.nerc.ac.uk/collection/L22/current/TOOL0836">
	<rdf:type rdf:resource="http://www.w3.org/2000/01/rdf-schema#Resource"/>
	<rdf:type rdf:resource="http://www.w3.org/2004/02/skos/core#Concept"/>
	<dcterms:created rdf:datatype="http://www.w3.org/2001/XMLSchema#dateTime">2017-11-21T00:00:00Z</dcterms:created>
	<dc:publisher rdf:datatype="http://www.w3.org/2001/XMLSchema#string">British Oceanographic Data Centre (BODC)</dc:publisher>
	<skos:definition xml:lang="en">A dissolved oxygen sensor designed to mount on RCM 9 or RDCP 600 or similar OEM applications. Measurement based on the ability of selected substances to act as dynamic fluorescence quenchers. The fluorescent indicator is a special platinum porphyrin complex embedded in a gas permeable foil that is exposed to the surrounding water. A black optical isolation coating protects the complex from sunlight and fluorescent particles in the water. This sensing foil is attached to a window providing optical access for the measuring system from inside a watertight titanium housing (depth rating 6000m).The foil is excited by modulated blue light, and the phase of a returned red light is measured. By linearizing and temperature compensating, with an incorporated temperature sensor, the absolute O2 concentration can be determined. Accuracy +/- 5% or 8uM; precision +/- 0.4 uM.</skos:definition>
	<skos:inScheme rdf:resource="http://vocab.aodn.org.au/def/instrument/1"/>
	<skos:prefLabel xml:lang="en">Aanderaa Oxygen Optode 3830</skos:prefLabel>
	<skos:broader rdf:resource="http://vocab.nerc.ac.uk/collection/L05/current/351"/>
	<skos:altLabel xml:lang="en">AA Optode 3830</skos:altLabel>
</rdf:Description>

<rdf:Description rdf:about="http://vocab.nerc.ac.uk/collection/L22/current/TOOL0103">
	<rdf:type rdf:resource="http://www.w3.org/2000/01/rdf-schema#Resource"/>
	<rdf:type rdf:resource="http://www.w3.org/2004/02/skos/core#Concept"/>
	<dcterms:created rdf:datatype="http://www.w3.org/2001/XMLSchema#dateTime">2017-11-21T00:00:00Z</dcterms:created>
	<dc:publisher rdf:datatype="http://www.w3.org/2001/XMLSchema#string">British Oceanographic Data Centre (BODC)</dc:publisher>
	<skos:definition xml:lang="en">A dissolved oxygen sensor designed to mount on RCM 9 or RDCP 600 or similar OEM applications. Measurement based on the ability of selected substances to act as dynamic fluorescence quenchers. The fluorescent indicator is a special platinum porphyrin complex embedded in a gas permeable foil that is exposed to the surrounding water. A black optical isolation coating protects the complex from sunlight and fluorescent particles in the water. This sensing foil is attached to a window providing optical access for the measuring system from inside a watertight plastic and titanium housing (depth rating 300m).The foil is excited by modulated blue light, and the phase of a returned red light is measured. By linearizing and temperature compensating, with an incorporated temperature sensor, the absolute O2 concentration can be determined. Accuracy +/- 5% or 8uM; precision +/- 0.4 uM.</skos:definition>
	<skos:inScheme rdf:resource="http://vocab.aodn.org.au/def/instrument/1"/>
	<skos:prefLabel xml:lang="en">Aanderaa Oxygen Optode 3835</skos:prefLabel>
	<skos:broader rdf:resource="http://vocab.nerc.ac.uk/collection/L05/current/351"/>
	<skos:altLabel xml:lang="en">AA Optode 3835</skos:altLabel>
</rdf:Description>

<rdf:Description rdf:about="http://vocab.nerc.ac.uk/collection/L22/current/TOOL0101">
	<rdf:type rdf:resource="http://www.w3.org/2000/01/rdf-schema#Resource"/>
	<rdf:type rdf:resource="http://www.w3.org/2004/02/skos/core#Concept"/>
	<dcterms:created rdf:datatype="http://www.w3.org/2001/XMLSchema#dateTime">2017-11-21T00:00:00Z</dcterms:created>
	<dc:publisher rdf:datatype="http://www.w3.org/2001/XMLSchema#string">British Oceanographic Data Centre (BODC)</dc:publisher>
	<skos:definition xml:lang="en">A dissolved oxygen sensor for OEM applications. Measurement based on the ability of selected substances to act as dynamic fluorescence quenchers. The fluorescent indicator is a special platinum porphyrin complex embedded in a gas permeable foil that is exposed to the surrounding water. A black optical isolation coating protects the complex from sunlight and fluorescent particles in the water. This sensing foil is attached to a window providing optical access for the measuring system from inside a watertight titanium housing.The foil is excited by modulated blue light, and the phase of a returned red light is measured. By linearizing and temperature compensating, with an incorporated temperature sensor, the absolute O2 concentration can be determined. Further information may be found on the BODC document server at URL: http://www.bodc.ac.uk/data/documents/nodb/119483/.</skos:definition>
	<skos:inScheme rdf:resource="http://vocab.aodn.org.au/def/instrument/1"/>
	<skos:prefLabel xml:lang="en">Aanderaa Oxygen Optode 4175</skos:prefLabel>
	<skos:broader rdf:resource="http://vocab.nerc.ac.uk/collection/L05/current/351"/>
	<skos:altLabel xml:lang="en">AA Optode 4175</skos:altLabel>
</rdf:Description>

<rdf:Description rdf:about="http://vocab.nerc.ac.uk/collection/L22/current/TOOL1164">
	<rdf:type rdf:resource="http://www.w3.org/2000/01/rdf-schema#Resource"/>
	<rdf:type rdf:resource="http://www.w3.org/2004/02/skos/core#Concept"/>
	<dcterms:created rdf:datatype="http://www.w3.org/2001/XMLSchema#dateTime">2017-11-21T00:00:00Z</dcterms:created>
	<dc:publisher rdf:datatype="http://www.w3.org/2001/XMLSchema#string">British Oceanographic Data Centre (BODC)</dc:publisher>
	<skos:definition xml:lang="en">An acoustic receiver comprising hydrophone, receiver, ID detector, data logging memory and battery housed within a submersible corrosion-resistant case. It is used to remotely retrieve ID numbers and time stamps from VEMCO coded transmitter tags deployed on marine fauna travelling within the VR2's receiver range. The VR2 is ideal for use in river monitoring or freshwater lake studies, as well as large tracking operations in oceanic systems. It features a Smart LED (light emitting diode), two megabytes of data storage (approx. 300000 detections), a resume study feature, and a replaceable battery (single Lithium cell). Detections are stored in the VR2's memory for later retrieval using a VR PC interface and a PC computer running VUE software. The VR2 is now discontinued and has been replaced by the Vemco VR2W receivers.</skos:definition>
	<skos:inScheme rdf:resource="http://vocab.aodn.org.au/def/instrument/1"/>
	<skos:prefLabel xml:lang="en">Vemco VR2 Receiver</skos:prefLabel>
	<skos:broader rdf:resource="http://vocab.nerc.ac.uk/collection/L05/current/369"/>
	<skos:altLabel xml:lang="en">Vemco VR2</skos:altLabel>
</rdf:Description>

<rdf:Description rdf:about="http://vocab.nerc.ac.uk/collection/L22/current/TOOL1163">
	<rdf:type rdf:resource="http://www.w3.org/2000/01/rdf-schema#Resource"/>
	<rdf:type rdf:resource="http://www.w3.org/2004/02/skos/core#Concept"/>
	<dcterms:created rdf:datatype="http://www.w3.org/2001/XMLSchema#dateTime">2017-11-21T00:00:00Z</dcterms:created>
	<dc:publisher rdf:datatype="http://www.w3.org/2001/XMLSchema#string">British Oceanographic Data Centre (BODC)</dc:publisher>
	<skos:definition xml:lang="en">A fast-sampling, fully integrated CTD package for use in environmental monitoring, fisheries, ocean observing networks and other marine applications. It measures condutivity and temperature with depth and utilises the patented Non-eXternal Inductive Cell (NXIC) conductivity sensor. The CTD-NH exhibits a bio-fouling resistant design, and the NXIC internal conductivity cells do not suffer from proximity effects, allowing it to be mounted in any orientation close to other instruments. The CTD-NH offers optional datalogging and external analog sensor input, and can run for 400 hours on its internal 3V battery pack. It is depth rated to 500 m.</skos:definition>
	<skos:inScheme rdf:resource="http://vocab.aodn.org.au/def/instrument/1"/>
	<skos:prefLabel xml:lang="en">Teledyne RDI Citadel CTD-NH</skos:prefLabel>
	<skos:broader rdf:resource="http://vocab.nerc.ac.uk/collection/L05/current/130"/>
	<skos:broader rdf:resource="http://vocab.nerc.ac.uk/collection/L05/current/134"/>
	<skos:broader rdf:resource="http://vocab.nerc.ac.uk/collection/L05/current/350"/>
	<skos:altLabel xml:lang="en">RDI Citadel CTD-NH</skos:altLabel>
</rdf:Description>

<rdf:Description rdf:about="http://vocab.nerc.ac.uk/collection/L22/current/TOOL1180">
	<rdf:type rdf:resource="http://www.w3.org/2000/01/rdf-schema#Resource"/>
	<rdf:type rdf:resource="http://www.w3.org/2004/02/skos/core#Concept"/>
	<dcterms:created rdf:datatype="http://www.w3.org/2001/XMLSchema#dateTime">2017-11-28T00:00:00Z</dcterms:created>
	<dc:publisher rdf:datatype="http://www.w3.org/2001/XMLSchema#string">British Oceanographic Data Centre (BODC)</dc:publisher>
	<skos:definition xml:lang="en">A combined thermistor component and resistor set. It is used for applications requiring linear electrical response to temperature change. The sensor can be operated in voltage or resistance mode and comprises YSI 44018 thermistor components and YSI 44303 resistor sets. It has a linear temperature range of -30 to +50 degrees C and linearity deviation of +/- 0.16 degrees C.</skos:definition>
	<skos:inScheme rdf:resource="http://vocab.aodn.org.au/def/instrument/1"/>
	<skos:prefLabel xml:lang="en">YSI 44203 (thermilinear network) temperature sensor</skos:prefLabel>
	<skos:broader rdf:resource="http://vocab.nerc.ac.uk/collection/L05/current/102"/>
	<skos:altLabel xml:lang="en">YSI 44203 temp</skos:altLabel>
</rdf:Description>

<rdf:Description rdf:about="http://purl.org/dc/terms/issued">
	<rdf:type rdf:resource="http://www.w3.org/1999/02/22-rdf-syntax-ns#Property"/>
	<rdf:type rdf:resource="http://www.w3.org/2000/01/rdf-schema#Resource"/>
	<rdfs:subPropertyOf rdf:resource="http://purl.org/dc/terms/issued"/>
</rdf:Description>

<rdf:Description rdf:about="http://www.w3.org/2002/07/owl#versionInfo">
	<rdf:type rdf:resource="http://www.w3.org/1999/02/22-rdf-syntax-ns#Property"/>
	<rdf:type rdf:resource="http://www.w3.org/2000/01/rdf-schema#Resource"/>
	<rdfs:subPropertyOf rdf:resource="http://www.w3.org/2002/07/owl#versionInfo"/>
</rdf:Description>

</rdf:RDF>